Based on the initial state provided:

- `t` is an integer between 1 and \(10^4\).
- `i` is 1.
- `m` is at least 6.
- `n` is an input integer.
- `count` is `m + 1`.
- `ans` is calculated as follows: `ans = n + (2 - 1) / 3 + 1 + (n / 4 - 3) / 5 + 1 + (n / 5 - 7) / 6 + 1 + ... + (n / (m-1) - (m-5)) / m + 1`.
- `countmins` is `m - 1`.
- `g` is `n / m - (m - 1)`.

The `print(int(ans))` statement will print the integer value of `ans`.

To break down the calculation of `ans`:
- The formula for `ans` involves adding terms where each term is structured as \(\frac{n / k - (k - 5)}{k} + 1\) for \(k\) ranging from 3 to \(m\).

Given this, let's consider the general form of the term in the summation:
- For \(k = 3\): \(\frac{n / 3 - (3 - 5)}{3} + 1 = \frac{n / 3 + 2}{3} + 1 = \frac{n + 6}{9} + 1 = \frac{n + 15}{9}\)
- For \(k = 4\): \(\frac{n / 4 - (4 - 5)}{4} + 1 = \frac{n / 4 + 1}{4} + 1 = \frac{n + 4}{16} + 1 = \frac{n + 20}{16}\)
- For \(k = 5\): \(\frac{n / 5 - (5 - 5)}{5} + 1 = \frac{n / 5}{5} + 1 = \frac{n}{25} + 1 = \frac{n + 25}{25}\)
- And so on, until \(k = m\): \(\frac{n / (m-1) - (m-5)}{(m-1)} + 1 = \frac{n - (m-5)(m-1)}{(m-1)} + 1 = \frac{n - (m^2 - 6m + 5)}{(m-1)} + 1 = \frac{n - m^2 + 6m - 5}{(m-1)} + 1 = \frac{n - m^2 + 6m - 4}{(m-1)}\)

Summing these terms along with the base value `n` gives us the total value of `ans`.

Therefore, the output will be the integer value of `ans`, which is the sum of `n` and the series of terms described above.

Output: **int(ans) (where ans is the sum of n and the series of terms as described)**