To determine the output state, let's analyze the given code snippet and its effect on the variables.

The code snippet is:
```python
b += b[-2] + v ** (v > x - w), b[-1] + v ** (v > z - y)
```

Given the initial state:
- `t` is an integer read from input such that 0 ≤ t ≤ 10^4
- `n` is an integer such that 2 ≤ n ≤ 10^5
- `a` is a list of `n+2` integers where -1000000000.0 ≤ a_1 < a_2 < ... < a_n ≤ 2000000000.0
- `m` is an integer such that 1 ≤ m ≤ 10^5
- `r` is a lambda function that reads a line of input, splits it into components, and maps each component to an integer
- `b` is a list containing `[0, 0, v]`
- `v` is `y - x`

Let's break down the code snippet:
- `b[-2]` refers to the second last element of `b`, which is `0` (since `b` is `[0, 0, v]`).
- `b[-1]` refers to the last element of `b`, which is `v`.
- `v ** (v > x - w)` evaluates to `v` if `v > x - w`, otherwise `1`. However, since the exact values of `x`, `w`, and `z` are not specified, we can only express this conditionally.
- Similarly, `v ** (v > z - y)` evaluates to `v` if `v > z - y`, otherwise `1`.

Thus, the new elements added to `b` are:
- `b[-2] + v ** (v > x - w)` → `0 + v ** (v > x - w)` → `v ** (v > x - w)`
- `b[-1] + v ** (v > z - y)` → `v + v ** (v > z - y)`

Therefore, the updated list `b` will be:
- `[0, 0, v, v ** (v > x - w), v + v ** (v > z - y)]`

Since the exact values of `x`, `w`, and `z` are not provided, we cannot simplify `v ** (v > x - w)` and `v + v ** (v > z - y)` further. We can only express them conditionally based on the comparison results.

Output State: **`t` is an integer read from input such that 0 ≤ t ≤ 10^4; `n` is an integer such that 2 ≤ n ≤ 10^5; `a` is a list of `n+2` integers where -1000000000.0 ≤ a_1 < a_2 < ... < a_n ≤ 2000000000.0; `m` is an integer such that 1 ≤ m ≤ 10^5; `r` is a lambda function that reads a line of input, splits it into components, and maps each component to an integer; `b` is a list containing `[0, 0, v, v ** (v > x - w), v + v ** (v > z - y)]`; `v` is `y - x`.**