The code snippet `d = not d` changes the value of `d` to its logical negation. Given the initial state, let's determine the output state:

- `d` was previously some boolean value (`True` or `False`). After executing `d = not d`, `d` will be the opposite of its previous value.
- All other variables (`n`, `i`, `k`, `b`, `a`, `s`, `c`) remain unchanged.

Therefore, the Output State is:

**`n` is `vals[0]` and must be greater than 1, `i` is 2, 1 ≤ k ≤ `vals[0]` ≤ 105, `k` is `vals[1]`, `b` is `vals[3] - 1` (or possibly updated), `a` is either `vals[2] - 2` or `vals[2] - 1` (or possibly updated), `s` is either 'GGB' or 'BGB', `c` is 1, `a < 0 or b < 0` is the termination condition. If `c == k`, `d` is the opposite of its previous value. Otherwise, the state remains unchanged.** 

However, since `d` is explicitly updated in this code snippet, the specific update to `d` should be noted:

**`n` is `vals[0]` and must be greater than 1, `i` is 2, 1 ≤ k ≤ `vals[0]` ≤ 105, `k` is `vals[1]`, `b` is `vals[3] - 1` (or possibly updated), `a` is either `vals[2] - 2` or `vals[2] - 1` (or possibly updated), `s` is either 'GGB' or 'BGB', `c` is 1, `a < 0 or b < 0` is the termination condition, `d` is the opposite of its previous value.**