Let's break down the problem step by step to determine what will be printed by the given `print` statement.

### Initial State:
- `a` is a list with at least 7 elements:
  - The first element is `-1000000000.0`.
  - Followed by at least five elements returned by `r()`.
  - The last element is `2000000000.0`.

- `w` is the fourth element of `a`.
- `x` is the fifth element of `a`.
- `y` is the sixth element of `a`.
- `z` is the seventh element of `a`.
- `u` is now a falsy value (since it was initially truthy and is decremented by 1).
- `c` is the new value returned by `r()`.
- `d` is the new value returned by `r()`.
- `v` is `y - x`.
- `b` is `[0, 0, v, 1, 2*v, 2, 3*v, 2 + v, 4*v, 2 + 2*v]`.
- `t` is `False`.
- `c` is less than `d`.

### Step-by-Step Analysis:
1. **List `a`**:
   - `a = [-1000000000.0, r(), r(), r(), r(), r(), 2000000000.0]`
   - Let's denote the elements returned by `r()` as `r1, r2, r3, r4, r5`.

2. **Variables from `a`**:
   - `w = a[3] = r3`
   - `x = a[4] = r4`
   - `y = a[5] = r5`
   - `z = a[6] = 2000000000.0`

3. **Variable `v`**:
   - `v = y - x = r5 - r4`

4. **List `b`**:
   - `b = [0, 0, v, 1, 2*v, 2, 3*v, 2 + v, 4*v, 2 + 2*v]`

5. **Variables `c` and `d`**:
   - `c` and `d` are new values returned by `r()`, and `c < d`.

6. **Expression in the `print` statement**:
   - `print(b[(d - 1) * 2] - b[(c - 1) * 2])`

### Calculation:
- `b` is indexed by `(d - 1) * 2` and `(c - 1) * 2`.
- Since `c < d`, let's assume `c = 1` and `d = 2` for simplicity (the exact values of `c` and `d` are not specified, but they must be positive integers where `c < d`).

- For `c = 1`:
  - `(c - 1) * 2 = (1 - 1) * 2 = 0`
  - `b[0] = 0`

- For `d = 2`:
  - `(d - 1) * 2 = (2 - 1) * 2 = 2`
  - `b[2] = v`

- Therefore, the expression becomes:
  - `b[(d - 1) * 2] - b[(c - 1) * 2] = v - 0 = v`

### Final Output:
- `v` is `y - x`, which is `r5 - r4`.

Output: **r5 - r4 (where r5 and r4 are the fifth and fourth elements of the list `a` respectively)**