The code `a, b = b, a % b` swaps the values of `a` and `b` and assigns the remainder of `a` divided by `b` to `b`. Since `a % b` must be non-zero, `b` will take the value of `a % b`, and `a` will take the value of the original `b`.

Given the initial conditions:
- `a` is not zero
- `b` must be non-zero (`a % b` must be non-zero)
- `k` is an integer such that 1 ≤ k ≤ 1500 (unchanged by the code)

After executing the code, the updated values are:
- `a` is the original value of `b`
- `b` is the original value of `a % b`

Therefore, the output state is:
Output State: **`a` is the original value of `b`, `b` is the original value of `a % b`, `k` is an integer such that 1 ≤ k ≤ 1500**