Let's break down the problem step by step:

1. **Initial States at the End of Previous Iteration:**
   - \( n \) is greater than or equal to 3.
   - \( ways \) is either 1 or 2.
   - \( a \) is less than or equal to \( n // 2 \).
   - \( a \) is not equal to \( b \).
   - Twice the sum of \( a \) and \( b \) equals \( n \), i.e., \( 2 * (a + b) == n \).

2. **For Loop:**
   ```python
   for b in range(a, (n - a) // 2 + 1):
       # the loop body is omitted
   ```

3. **Loop Execution Analysis:**
   - The loop iterates over values of \( b \) starting from \( a \) up to \( \frac{n - a}{2} \).
   - For each value of \( b \), the condition \( 2 * (a + b) == n \) must hold true.

4. **Determine the Next Value of \( b \):**
   - Since the loop starts from \( a \) and goes up to \( \frac{n - a}{2} \), we need to find the next possible value of \( b \) that satisfies the condition \( 2 * (a + b) == n \).

5. **Next Value of \( b \):**
   - The current \( b \) value is such that \( 2 * (a + b) == n \).
   - The next value of \( b \) would be \( b + 1 \) (since the loop increments \( b \) by 1 each iteration).
   - We need to check if \( 2 * (a + (b + 1)) == n \). This simplifies to \( 2 * (a + b + 1) == n \), which means \( 2 * a + 2 * b + 2 == n \). Given \( 2 * (a + b) == n \), this becomes \( n + 2 == n \), which is not possible unless \( b + 1 \leq \frac{n - a}{2} \).

6. **Adjusting the States:**
   - \( n \) remains the same as it does not change within the loop.
   - \( ways \) remains the same as it is incremented only when the condition is met, and we are checking the next possible value of \( b \).
   - \( a \) remains the same as it is the starting point for the range.
   - \( b \) increases by 1, so the new value of \( b \) is \( b + 1 \).

7. **New Conditions:**
   - The new value of \( b \) must satisfy \( b + 1 \leq \frac{n - a}{2} \).

Therefore, the states need to be adjusted as follows:

**State: **`n` is greater than or equal to 3, `ways` is either 1 or 2, `a` is less than or equal to `n // 2`, `a` is not equal to `b`, and twice the sum of `a` and `b + 1` equals `n`.**