The code `d -= 1` decrements the value of `d` by 1. Given the initial conditions:

- `s1` is `b - a`
- `s2` is `c - d`
- `s1 != s2`
- `s1 + 1 != s2`
- `s1 == s2 + 1`
- `d` is a non-negative integer greater than 0

Since `d` is decremented by 1, `d` becomes `d - 1`. All other conditions and relationships remain unchanged.

Therefore, the updated values are:
- `s1` remains `b - a`
- `s2` remains `c - (d - 1)` which simplifies to `c - d + 1`
- The condition `s1 != s2` still holds
- The condition `s1 + 1 != s2` still holds
- The condition `s1 == s2 + 1` still holds

The Output State: **`a` is a non-negative integer, `b` is a non-negative integer, `c` is a non-negative integer, `d` is a non-negative integer such that `d` is greater than 0 and equal to the original value of `d` minus 1, `s1` is `b - a`, `s2` is `c - (d - 1)`, `s1 != s2`, `s1 + 1 != s2`, and `s1 == s2 + 1`.**