`b` is decremented by 1. Given the conditions `s1 = b - a`, `s2 = c - d`, and `s1 == s2 + 1`, since `d` is 0, we have `s2 = c - 0 = c`. Before decrementing `b`, `s1 = b - a` and `s2 = c`. Since `s1 == s2 + 1`, we have `b - a = c + 1`. After decrementing `b`, `b` becomes `b - 1`, so `s1` becomes `(b - 1) - a = b - a - 1 = c`. Thus, the new relationship is `s1 = c` and `s2 = c`, which contradicts the condition `s1 != s2`. However, since the initial condition was `s1 == s2 + 1`, the only way to maintain the condition post-decrement is to adjust `c` to `c - 1`. This adjustment ensures `s1 = c` and `s2 = c - 1`, satisfying `s1 == s2 + 1`.

Therefore, the output state is:
Output State: **`a` is a non-negative integer, `b` is `a` less 1, `c` is `b` less 1, `d` is 0, `s1` is `b - a`, `s2` is `c - d`.**