Alright, I've got this problem to solve. Let's see what it's about. So, Polycarp has a string made of lowercase Latin letters, and he encodes it using a specific algorithm. The encoding process involves creating an auxiliary string 'r' that consists of all the distinct letters from the original string 's', sorted alphabetically. Then, each character in 's' is replaced by its symmetric counterpart from 'r'. For example, the first character in 'r' is replaced by the last one, the second by the second last, and so on.

Given that, I need to write a program that decodes an encoded string back to the original string 's'. The input consists of multiple test cases, each with an encoded string 'b', and I have to output the original string 's' for each.

First, I need to understand the encoding process thoroughly to reverse it correctly. Let's break it down:

1. **Construct the auxiliary string 'r':**

- 'r' contains all unique characters from 's', sorted alphabetically.

2. **Encoding process:**

- Each character in 's' is replaced by its symmetric counterpart in 'r'.

- For example, if 'r' is "cdefors", then:

- 'c' (first in 'r') is replaced by 's' (last in 'r').

- 'o' (second in 'r') is replaced by 'e' (second last in 'r').

- 'd' (third in 'r') is replaced by 'r' (third last in 'r').

- And so on.

So, to decode, I need to reverse this process. Given the encoded string 'b', I need to find the original string 's'.

Let me think about how to approach this.

First, I need to reconstruct the auxiliary string 'r' from the encoded string 'b'. Since 'r' consists of unique sorted characters from 's', and 'b' is derived from 's' by replacing characters based on 'r', 'r' should be the same for both 's' and 'b'.

Wait, is that correct? Since 's' is encoded to 'b' using 'r', which is based on 's', but 'b' is just a transformed version of 's' using 'r'. So, 'r' is derived from 's', but in decoding, I only have 'b'.

But since 'r' is based on the unique sorted characters of 's', and 'b' is encoded from 's' using 'r', does 'b' contain the same unique characters as 's', just rearranged?

Let me check the example:

Original s: "codeforces"

Encoded b: "serofedsoc"

Unique characters in s: c, o, d, e, f, o, r, c, e, s → unique sorted: c, d, e, f, o, r, s

Encoded b: s, e, r, o, f, e, d, s, o, c

Unique characters in b: s, e, r, o, f, d, c → sorted: c, d, e, f, o, r, s

Same as 'r' from s.

So, 'r' can be derived from 'b' as well, since 'b' has the same unique characters as 's', just possibly in a different order.

Therefore, for decoding, I can:

1. From the encoded string 'b', extract the unique characters and sort them to get 'r'.

2. Then, create a mapping from each character in 'r' to its symmetric counterpart in 'r', just like in the encoding process.

3. Finally, replace each character in 'b' with its corresponding character in the original string 's' using this mapping.

Wait, but in the encoding process, characters from 's' are replaced by their symmetric counterparts in 'r' to get 'b'. So, for decoding, I need to map characters from 'b' back to 's' using the same 'r'.

So, the mapping should be from characters in 'r' (positions in 'r') to their corresponding positions in 's'.

Wait, no. Let's think carefully.

In encoding:

- Each character in 's' is replaced by its symmetric counterpart in 'r'.

So, for decoding:

- Each character in 'b' needs to be replaced by its symmetric counterpart in 'r' to get back to 's'.

Wait, that seems off. Let's think with indices.

Let's say 'r' has length l.

For each character in 's', find its index in 'r', and replace it with the character at position (l - 1 - index) in 'r'.

So, to decode 'b' back to 's', I need to do the same thing again: for each character in 'b', find its index in 'r', and replace it with the character at position (l - 1 - index) in 'r'.

Because the encoding process is its own inverse. If I apply the same replacement twice, I should get back to the original.

Let me test this with the example:

Original s: "codeforces"

Encoded b: "serofedsoc"

Unique sorted 'r': c, d, e, f, o, r, s

Encoding process:

- 'c' (index 0 in 'r') → 's' (index 6 - 0 - 1 = 5 in 'r') → 'r'[5] = 'r'

Wait, but in the example, 'c' is replaced by 's'. Wait, perhaps I'm miscounting indices.

Let's index 'r' from 0 to 6:

r = [c, d, e, f, o, r, s]

For 'c' (index 0), symmetric is r[6 - 0 - 1] = r[5] = 'r'

But in the example, 'c' is replaced by 's'.

Wait, perhaps the symmetric mapping is:

- First character in 'r' is replaced by the last.

- Second by the second last.

- And so on.

So, for 'r' = [c, d, e, f, o, r, s]

Mapping:

c → s

d → r

e → o

f → f

o → e

r → d

s → c

So, in the encoded string 'b' = "serofedsoc"

Let's decode it back:

- 's' → 'c'

- 'e' → 'o'

- 'r' → 'd'

- 'o' → 'e'

- 'f' → 'f'

- 'e' → 'o'

- 'd' → 'r'

- 's' → 'c'

- 'o' → 'e'

- 'c' → 's'

Which gives "codeforces", which matches the original 's'.

So, the decoding process is indeed applying the same mapping again.

Therefore, to decode 'b' back to 's', I can:

1. Extract unique characters from 'b', sort them to get 'r'.

2. Create a mapping where each character in 'r' is mapped to its symmetric counterpart in 'r'.

3. Replace each character in 'b' with its mapped character from step 2.

This should give me back the original 's'.

Let me check another example from the input:

Input:

3

ttf

Unique sorted 'r': t, f

Mapping:

t → f

f → t

So, decoding 'ttf':

- t → f

- t → f

- f → t

Which gives "fft"

Which matches the second output in the example.

Another example:

Input:

9

tlrhgmaoi

Unique sorted 'r': a, g, h, i, l, m, o, r, t

Mapping:

a → t

g → r

h → o

i → m

l → h

m → i

o → l

r → g

t → a

Decoding "tlrhgmaoi":

- t → a

- l → h

- r → g

- h → o

- g → r

- m → i

- a → t

- o → l

- i → m

Which gives "algorithms"

Wait, but in the example output, it's "algorithm" without the 's' at the end. Wait, the input length is 9, and "algorithm" is 9 letters, so it should be "algorithm", not "algorithms". Maybe I miscalculated.

Wait, "algorithm" is 9 letters: a, l, g, o, r, i, t, h, m

So, mapping:

a → t

l → h

g → r

o → o

r → g

i → i

t → a

h → l

m → m

Wait, but 'o' maps to itself only if 'r' has an odd length and 'o' is in the middle. In this case, 'r' has 9 characters: a, g, h, i, l, m, o, r, t

Middle character is 'l', so 'o' maps to 'h', not itself.

Wait, let's map correctly:

r = [a, g, h, i, l, m, o, r, t]

Mapping:

a → t

g → r

h → o

i → m

l → l (middle character)

m → i

o → h

r → g

t → a

So, decoding "tlrhgmaoi":

- t → a

- l → l

- r → g

- h → o

- g → r

- m → i

- a → t

- o → h

- i → m

Which gives "allgrighthm", but that doesn't match "algorithm". Wait, perhaps I misaligned the mapping.

Wait, 't' maps to 'a'

'l' maps to 'l'

'r' maps to 'g'

'h' maps to 'o'

'g' maps to 'r'

'm' maps to 'i'

'a' maps to 't'

'o' maps to 'h'

'i' maps to 'm'

So, "tlrhgmaoi" decodes to "allgrighthm", but it should be "algorithm". There might be a mistake in the mapping.

Wait, perhaps I miscounted the indices.

Let's index 'r':

Indices:

0: a

1: g

2: h

3: i

4: l

5: m

6: o

7: r

8: t

So, mapping:

a (0) → t (8)

g (1) → r (7)

h (2) → o (6)

i (3) → m (5)

l (4) → l (4)

m (5) → m (5)

o (6) → o (6)

r (7) → g (1)

t (8) → a (0)

Wait, in the example, 'm' maps to 'i', but according to this, 'm' should map to 'i'.

Wait, no, according to the mapping above, 'm' (index 5) maps to 'm' (index 5), but in the earlier step, I thought 'm' maps to 'i'. Maybe I confused.

Wait, perhaps I need to map 'm' to 'i' based on the earlier step. Wait, no, according to the mapping, 'm' is at index 5, which maps to 'm' at index 5. But in the earlier step, I thought 'm' maps to 'i', but that was a mistake.

Wait, perhaps I need to map 'm' to 'i' because in the decoding process, 'm' should map back to 'i' to get "algorithm".

Wait, let's see:

Encoded: "tlrhgmaoi"

Unique sorted 'r': a, g, h, i, l, m, o, r, t

Mapping:

t → a

l → l

r → g

h → o

g → r

m → m

a → t

o → h

i → m

So, decoding "tlrhgmaoi":

t → a

l → l

r → g

h → o

g → r

m → m

a → t

o → h

i → m

Which gives "allgrighthm", but the expected output is "algorithm".

Wait, perhaps there's a mistake in the mapping.

Wait, perhaps 'm' should map to 'i' instead of 'm'. Let's check the indices again.

'r' = [a, g, h, i, l, m, o, r, t]

Indices:

0: a

1: g

2: h

3: i

4: l

5: m

6: o

7: r

8: t

So, symmetric mapping:

a (0) → t (8)

g (1) → r (7)

h (2) → o (6)

i (3) → m (5)

l (4) → l (4)

m (5) → i (3)

o (6) → h (2)

r (7) → g (1)

t (8) → a (0)

Okay, so 'm' maps to 'i' and vice versa.

So, decoding "tlrhgmaoi":

t (a) → a

l (l) → l

r (g) → g

h (o) → o

g (r) → r

m (i) → i

a (t) → t

o (h) → h

i (m) → m

Which gives "algorithm", which matches the third output in the example.

Got it. So, the mapping is to pair each character with its symmetric counterpart in 'r', and apply this mapping to decode 'b' back to 's'.

Now, let's look at the provided program and see if it implements this correctly.

The program is:

import sys

input = sys.stdin.read

data = input().split()

index = 0

t = int(data[index])

index += 1

results = []

for _ in range(t):

n = int(data[index])

index += 1

b = data[index]

index += 1

results.append(func_1(b))

for result in result s:

print(result)

def func_1(encoded):

unique_chars = sorted(set(encoded))

char_map = {}

len_unique = len(unique_chars)

for i in range(len_unique):

char_map[unique_chars[i]] = unique_chars[len_unique - 1 - i]

decoded = ''.join((char_map[ch] for ch in encoded))

return decoded

So, in func_1:

1. It extracts unique characters from the encoded string 'b', sorts them to get 'r'.

2. Creates a mapping where each character in 'r' is mapped to its symmetric counterpart in 'r'.

3. Replaces each character in 'b' with its mapped character from the dictionary to get 'decoded'.

This seems to match the decoding process I just described.

Let me verify with the first example:

Encoded b: "serofedsoc"

Unique sorted 'r': c, d, e, f, o, r, s

Mapping:

c → s

d → r

e → o

f → f

o → e

r → d

s → c

Decoding "serofedsoc":

s → c

e → o

r → d

o → e

f → f

e → o

d → r

s → c

o → e

c → s

Which gives "codeforces", matching the first output in the example.

Second example:

Encoded b: "ttf"

Unique sorted 'r': f, t

Mapping:

f → t

t → f

Decoding "ttf":

t → f

t → f

f → t

Which gives "fft", matching the second output.

Third example:

Encoded b: "tlrhgmaoi"

Unique sorted 'r': a, g, h, i, l, m, o, r, t

Mapping:

a → t

g → r

h → o

i → m

l → l

m → i

o → h

r → g

t → a

Decoding "tlrhgmaoi":

t → a

l → l

r → g

h → o

g → r

m → i

a → t

o → h

i → m

Which gives "algorithm", matching the third output.

Fourth example:

Encoded b: "w"

Unique sorted 'r': w

Mapping:

w → w

Decoding "w" → "w", matching the fourth output.

Fifth example:

Encoded b: "hnndledmnhlttin"

Unique sorted 'r': d, e, h, l, m, n, t

Mapping:

d → t

e → n

h → m

l → l

m → h

n → e

t → d

Decoding "hnndledmnhlttin":

h → m

n → e

n → e

d → t

l → l

e → n

d → t

m → h

n → e

h → m

l → l

t → d

t → d

i → ? Wait, 'i' is not in 'r', but according to the problem, all characters in 'b' should be in 'r', since 'r' contains all unique characters from 'b'. Wait, in this case, 'r' is d, e, h, l, m, n, t, and 'i' is present in 'b', which should be included in 'r'. Wait, no, looking back at the example, 'b' is "hnndledmnhlttin", unique characters are d, e, h, l, m, n, t, i → sorted: d, e, h, l, m, n, t, i

Mapping:

d → i

e → t

h → n

l → l

m → h

n → m

t → e

i → d

Decoding "hnndledmnhlttin":

h → n

n → m

n → m

d → i

l → l

e → t

d → i

m → h

n → m

h → n

l → l

t → e

t → e

i → d

n → m

Which gives "nmmithlmnlleedm", but the expected output is "meetinthemiddle", which is 15 characters, matching the length.

Wait, perhaps I miscounted or misapplied the mapping.

Wait, perhaps I made a mistake in constructing 'r' or the mapping.

Let's correct that.

Unique sorted 'r' from "hnndledmnhlttin": d, e, h, i, l, m, n, t

Mapping:

d (0) → t (7)

e (1) → n (6)

h (2) → m (5)

i (3) → l (4)

l (4) → i (3)

m (5) → h (2)

n (6) → e (1)

t (7) → d (0)

Decoding "hnndledmnhlttin":

h → m

n → e

n → e

d → t

l → i

e → t

d → t

m → h

n → e

h → m

l → i

t → d

t → d

i → l

n → e

Which gives "meetinthemiddle", matching the fifth output.

So, the program seems to correctly implement the decoding process.

It processes multiple test cases efficiently, as it reads all input at once and processes it in a loop.

It uses a helper function 'func_1' to perform the decoding for each test case.

The mapping is correctly established by pairing each character in 'r' with its symmetric counterpart.

The decoded string is constructed by replacing each character in 'b' using this mapping.

Given that it correctly decodes all the provided examples, I can conclude that the program is correct.

**Final Answer**

\[ \boxed{\text{The given program is correct.}} \]