To determine the output state after the loop has finished executing, we need to analyze the given code and the initial state provided. However, the variable `n` and the string `s` are not defined in the initial state. Since these are crucial for the loop's execution, let's assume some values for `n` and `s` to proceed with the analysis. 

Let's assume:
- `n` is 5 (the length of string `s`).
- `s` is ">>><<".

With these assumptions, we can go through the loop and see how the variables change.

### Initial State:
- A is [0, 2, 6, 9, 13]
- idx_A is [0, 2, 4, 5, 6]
- B is [0, 1, 5]
- idx_B is [4, 3, 1]
- `l` is 0
- `r` is 3
- `n` is 5
- `s` is ">>><<"

### Loop Execution:
1. **Iteration 1 (i=0, s[0]='>')**:
   - `l < r` (0 < 3) is true.
   - `a = A[l] = A[0] = 0`
   - `x = r - (l + 2) = 3 - (0 + 2) = 1`
   - `b = B[r - 1] = B[2] = 5`
   - `x >= 0` (1 >= 0) is true.
     - `b = b - B[x] = 5 - B[1] = 5 - 1 = 4`
     - `b = b - (idx_B[x] - idx_B[r - 1]) * (x + 1) = 4 - (idx_B[1] - idx_B[2]) * (1 + 1) = 4 - (3 - 1) * 2 = 4 - 4 = 0`
   - `b = b + (idx_B[r - 1] - i) * (l + 1) = 0 + (idx_B[2] - 0) * (0 + 1) = 0 + (1 - 0) * 1 = 1`
   - `print(a * 2 + b * 2 + i + 1, end=' ')` prints `0 * 2 + 1 * 2 + 0 + 1 = 3`
   - `l += 1` → `l` becomes 1

2. **Iteration 2 (i=1, s[1]='>')**:
   - `l < r` (1 < 3) is true.
   - `a = A[l] = A[1] = 2`
   - `x = r - (l + 2) = 3 - (1 + 2) = 0`
   - `b = B[r - 1] = B[2] = 5`
   - `x >= 0` (0 >= 0) is true.
     - `b = b - B[x] = 5 - B[0] = 5 - 0 = 5`
     - `b = b - (idx_B[x] - idx_B[r - 1]) * (x + 1) = 5 - (idx_B[0] - idx_B[2]) * (0 + 1) = 5 - (4 - 1) * 1 = 5 - 3 = 2`
   - `b = b + (idx_B[r - 1] - i) * (l + 1) = 2 + (idx_B[2] - 1) * (1 + 1) = 2 + (1 - 1) * 2 = 2`
   - `print(a * 2 + b * 2 + i + 1, end=' ')` prints `2 * 2 + 2 * 2 + 1 + 1 = 9`
   - `l += 1` → `l` becomes 2

3. **Iteration 3 (i=2, s[2]='>')**:
   - `l < r` (2 < 3) is true.
   - `a = A[l] = A[2] = 6`
   - `x = r - (l + 2) = 3 - (2 + 2) = -1`
   - `b = B[r - 1] = B[2] = 5`
   - `x >= 0` (-1 >= 0) is false.
   - `b = b + (idx_B[r - 1] - i) * (l + 1) = 5 + (idx_B[2] - 2) * (2 + 1) = 5 + (1 - 2) * 3 = 5 - 3 = 2`
   - `print(a * 2 + b * 2 + i + 1, end=' ')` prints `6 * 2 + 2 * 2 + 2 + 1 = 17`
   - `l += 1` → `l` becomes 3

4. **Iteration 4 (i=3, s[3]='<')**:
   - `r -= 1` → `r` becomes 2
   - `l <= r` (3 <= 2) is false.
   - `r == 0` (2 == 0) is false.
   - `a = B[r] = B[2] = 5`
   - `b = A[l - 1] = A[2] = 6`
   - `l - r - 1 > 0` (3 - 2 - 1 > 0) is false.
   - `b = b + (i - idx_A[l - 1]) * (r + 1) = 6 + (3 - idx_A[2]) * (2 + 1) = 6 + (3 - 4) * 3 = 6 - 3 = 3`
   - `print(a * 2 + b * 2 + (n - i), end=' ')` prints `5 * 2 + 3 * 2 + (5 - 3) = 10 + 6 + 2 = 18`

5. **Iteration 5 (i=4, s[4]='<')**:
   - `r -= 1` → `r` becomes 1
   - `l <= r` (3 <= 1) is false.
   - `r == 0` (1 == 0) is false.
   - `a = B[r] = B[1] = 1`
   - `b = A[l - 1] = A[2] = 6`
   - `l - r - 1 > 0` (3 - 1 - 1 > 0) is true.
     - `b = b - A[l - r - 2] = 6 - A[0] = 6 - 0 = 6`
     - `b = b - (idx_A[l - 1] - idx_A[l - r - 2]) * (l - r - 1) = 6 - (idx_A[2] - idx_A[0]) * (3 - 1 - 1) = 6 - (4 - 0) * 1 = 6 - 4 = 2`
   - `b = b + (i - idx_A[l - 1]) * (r + 1) = 2 + (4 - idx_A[2]) * (1 + 1) = 2 + (4 - 4) * 2 = 2`
   - `print(a * 2 + b * 2 + (n - i), end=' ')` prints `1 * 2 + 2 * 2 + (5 - 4) = 2 + 4 + 1 = 7`

### Output:
The printed values are `3 9 17 18 7`.

### Output State:
The variables `A`, `idx_A`, `B`, `idx_B` remain unchanged, and `l` and `r` have new values after the loop execution.

Output State: **A is [0, 2, 6, 9, 13] and idx_A is [0, 2, 4, 5, 6]; B is [0, 1, 5]; idx_B is [4, 3, 1]; `l` is 3; `r` is 1.**