Let's break down the initial state and the code snippet step by step to determine what will be printed.

### Initial State:
1. `t` is greater than 0.
2. `n` and `m` are input integers.
3. `s` is an input string.
4. `p` is the string 'ABCDEFG'.
5. `hmp` is a `Counter` object containing the frequency of each character in the input string `s`.
6. `ans` is calculated as follows:
   - For each character in 'ABCDEFG' that is not in `hmp`, add `m` to `ans`.
   - For each character `i` in `hmp` where `hmp[i]` is less than `m`, add (`m` - `hmp[i]`) to `ans`.

### Code Snippet:
```python
print(ans)
```

### Step-by-Step Calculation:
1. **Counter Object `hmp`**:
   - `hmp` is a `Counter` object that counts the frequency of each character in the input string `s`.
   - For example, if `s = "ABCD"`, then `hmp` would be `{'A': 1, 'B': 1, 'C': 1, 'D': 1}`.

2. **Calculation of `ans`**:
   - `ans` is initialized to 0.
   - For each character in the string 'ABCDEFG':
     - If the character is not in `hmp`, add `m` to `ans`.
     - If the character is in `hmp` and `hmp[i]` is less than `m`, add (`m` - `hmp[i]`) to `ans`.

### Example Calculation:
Let's assume:
- `n = 7` (though `n` is not used in the calculation of `ans`).
- `m = 2`.
- `s = "ABCD"`.

1. **Create `hmp`**:
   - `hmp = {'A': 1, 'B': 1, 'C': 1, 'D': 1}`.

2. **Calculate `ans`**:
   - For 'A': `hmp['A'] = 1` (which is less than `m`), so add (`m` - `hmp['A']`) = 2 - 1 = 1 to `ans`.
   - For 'B': `hmp['B'] = 1` (which is less than `m`), so add (`m` - `hmp['B']`) = 2 - 1 = 1 to `ans`.
   - For 'C': `hmp['C'] = 1` (which is less than `m`), so add (`m` - `hmp['C']`) = 2 - 1 = 1 to `ans`.
   - For 'D': `hmp['D'] = 1` (which is less than `m`), so add (`m` - `hmp['D']`) = 2 - 1 = 1 to `ans`.
   - For 'E': `hmp['E']` is not in `hmp`, so add `m` = 2 to `ans`.
   - For 'F': `hmp['F']` is not in `hmp`, so add `m` = 2 to `ans`.
   - For 'G': `hmp['G']` is not in `hmp`, so add `m` = 2 to `ans`.

3. **Summing Up**:
   - `ans = 1 + 1 + 1 + 1 + 2 + 2 + 2 = 10`.

### General Description:
- `ans` will be the sum of `m` for each character in 'ABCDEFG' that is not in `hmp` plus the sum of (`m` - `hmp[i]`) for each character `i` in `hmp` where `hmp[i]` is less than `m`.

### Final Output:
Output: **ans (where ans is the sum of m for each character in 'ABCDEFG' that is not in hmp plus the sum of (m - hmp[i]) for each character i in hmp where hmp[i] < m)**