To determine the output state, let's analyze the given code snippet:

```
b += b[-2] + v ** (v > x - w), b[-1] + v ** (v > z - y)
```

Given the initial state:
- `t` is `t - 1`
- `n` is an integer such that 2 ≤ n ≤ 10^5
- `a` is a list starting with `-1000000000.0`, followed by at least 2 elements from `r()`, and ending with `2000000000.0`
- `m` is an integer such that 1 ≤ m ≤ 10^5
- `b` is `[0, 0]`
- `v` is `y - x`

Let's break down the code snippet:

1. `b[-2]` refers to the second last element of `b`, which is `0` since `b` is initially `[0, 0]`.
2. `b[-1]` refers to the last element of `b`, which is also `0` since `b` is initially `[0, 0]`.

The expression `v ** (v > x - w)` evaluates to `v ** True` if `v > x - w` and `v ** False` if `v <= x - w`. Since `True` is equivalent to `1` and `False` is equivalent to `0`, this simplifies to:
- `v` if `v > x - w`
- `1` if `v <= x - w`

Similarly, `v ** (v > z - y)` evaluates to:
- `v` if `v > z - y`
- `1` if `v <= z - y`

Thus, the code appends two new elements to `b`:
- The first new element is `b[-2] + v ** (v > x - w)`, which is `0 + v` if `v > x - w` or `0 + 1` if `v <= x - w`.
- The second new element is `b[-1] + v ** (v > z - y)`, which is `0 + v` if `v > z - y` or `0 + 1` if `v <= z - y`.

Therefore, the new elements appended to `b` depend on the conditions `v > x - w` and `v > z - y`.

Output State: **`t` is `t - 1`, `n` is an integer such that 2 ≤ n ≤ 10^5, `a` is a list starting with `-1000000000.0`, followed by at least 2 elements from `r()`, and ending with `2000000000.0`, `m` is an integer such that 1 ≤ m ≤ 10^5, `b` is `[0, 0, v if v > x - w else 1, v if v > z - y else 1]`, `v` is `y - x`**

This means that the list `b` now contains four elements: the original two zeros, and two new elements that are either `v` or `1` depending on the conditions `v > x - w` and `v > z - y`.