To determine the output of the given print statement, let's break down the initial state and the code snippet step by step:

### Initial State Breakdown

1. **Variable `u`**: 
   - `u` is described as "a non-zero value minus 1". This means if the non-zero value is `n`, then `u = n - 1`. However, `u` is not directly used in the print statement, so its exact value is not critical for this calculation.

2. **List `b`**:
   - The list `b` is defined as `[0, 0, y - x, y - x, y - x + v, y - x + v, y - x + v]`.
   - This list contains seven elements, where the first two elements are `0`, and the next five elements are variations of `y - x` and `y - x + v`.

3. **Variables `c` and `d`**:
   - `c` and `d` are the values returned by a function `r()`.
   - It is mentioned that the current value of `c` is less than `d`.

### Code Snippet Analysis

The print statement is:
```python
print(b[(d - 1) * 2] - b[(c - 1) * 2])
```

Let's analyze the indices used in the list `b`:

- `(d - 1) * 2`: Since `d` is a value returned by `r()` and `c < d`, `d` must be at least 2 (because `c` is at least 1). Therefore, `(d - 1) * 2` will be an even number starting from 2.
- `(c - 1) * 2`: Similarly, since `c` is at least 1, `(c - 1) * 2` will be 0 when `c` is 1, and an even number greater than 0 for higher values of `c`.

### List Index Mapping

Given the list `b = [0, 0, y - x, y - x, y - x + v, y - x + v, y - x + v]`, let's map the indices:

- `b[0] = 0`
- `b[1] = 0`
- `b[2] = y - x`
- `b[3] = y - x`
- `b[4] = y - x + v`
- `b[5] = y - x + v`
- `b[6] = y - x + v`

### Calculation

- If `c = 1`, then `(c - 1) * 2 = 0`, so `b[(c - 1) * 2] = b[0] = 0`.
- If `d = 2`, then `(d - 1) * 2 = 2`, so `b[(d - 1) * 2] = b[2] = y - x`.
- If `d = 3`, then `(d - 1) * 2 = 4`, so `b[(d - 1) * 2] = b[4] = y - x + v`.
- If `d = 4`, then `(d - 1) * 2 = 6`, so `b[(d - 1) * 2] = b[6] = y - x + v`.

### Example Calculation

Let's assume `c = 1` and `d = 3` for concreteness:

- `b[(c - 1) * 2] = b[0] = 0`
- `b[(d - 1) * 2] = b[4] = y - x + v`

Thus, the expression becomes:
```python
print((y - x + v) - 0)
```

Which simplifies to:
```python
print(y - x + v)
```

### General Case

For any valid `c` and `d` where `c < d`, the expression `b[(d - 1) * 2] - b[(c - 1) * 2]` will always result in a difference between two elements of the list `b` at even indices. Given the structure of `b`, the result will be either `y - x` or `y - x + v` depending on the specific values of `c` and `d`.

### Final Output

Since the exact values of `c` and `d` are not specified, the output will depend on these values. However, based on the structure of the list and the given conditions, the output will be either `y - x` or `y - x + v`.

Output: **y - x or y - x + v (depending on the values of c and d)**