To determine what will be printed, let's break down the given information and the code snippet step by step:

### Initial State Breakdown:
- `u` is a non-zero value minus 1. This doesn't directly affect the print statement, so we can ignore it for now.
- The list `b` is defined as `[0, 0, y - x, y - x, y - x + v, y - x + v, y - x + v]`.
- `c` and `d` are values returned by a function `r()`, with the condition that `c` is greater than or equal to `d`.

### Code Snippet Analysis:
The print statement is:
```python
print(b[c * 2 - 1] - b[d * 2 - 1])
```

### Step-by-Step Calculation:
1. **List Indexing**: The list `b` has 7 elements, indexed from 0 to 6.
2. **Index Calculation**:
   - For `b[c * 2 - 1]`: The index is `c * 2 - 1`.
   - For `b[d * 2 - 1]`: The index is `d * 2 - 1`.
3. **Value Extraction**:
   - Since `c` and `d` are indices that are doubled and then decremented by 1, they must be such that `c * 2 - 1` and `d * 2 - 1` fall within the range of valid indices for the list `b` (0 to 6).
   - Given `c >= d`, the possible valid values for `c` and `d` are integers such that `c * 2 - 1` and `d * 2 - 1` are between 0 and 6.
4. **Possible Values**:
   - Let's consider the possible pairs `(c, d)`:
     - If `c = 1`, then `c * 2 - 1 = 1` (valid).
     - If `c = 2`, then `c * 2 - 1 = 3` (valid).
     - If `c = 3`, then `c * 2 - 1 = 5` (valid).
     - If `c = 4`, then `c * 2 - 1 = 7` (invalid, out of bounds).

   Similarly, for `d`:
     - If `d = 1`, then `d * 2 - 1 = 1` (valid).
     - If `d = 2`, then `d * 2 - 1 = 3` (valid).
     - If `d = 3`, then `d * 2 - 1 = 5` (valid).

5. **Element Values**:
   - `b[1] = 0`
   - `b[3] = y - x`
   - `b[5] = y - x + v`

6. **Subtraction**:
   - If `c = 1` and `d = 1`, then `b[1] - b[1] = 0 - 0 = 0`.
   - If `c = 2` and `d = 1`, then `b[3] - b[1] = (y - x) - 0 = y - x`.
   - If `c = 2` and `d = 2`, then `b[3] - b[3] = (y - x) - (y - x) = 0`.
   - If `c = 3` and `d = 1`, then `b[5] - b[1] = (y - x + v) - 0 = y - x + v`.
   - If `c = 3` and `d = 2`, then `b[5] - b[3] = (y - x + v) - (y - x) = v`.
   - If `c = 3` and `d = 3`, then `b[5] - b[5] = (y - x + v) - (y - x + v) = 0`.

### Conclusion:
Given the possible valid pairs `(c, d)` and their corresponding index calculations, the printed value depends on the specific values of `c` and `d`. However, the most precise description we can provide is based on the possible outcomes.

Output: **the difference between `b[c * 2 - 1]` and `b[d * 2 - 1]` (where `b` is the list `[0, 0, y - x, y - x, y - x + v, y - x + v, y - x + v]`, and `c` and `d` are integers such that `c >= d` and both `c * 2 - 1` and `d * 2 - 1` are valid indices for the list `b`)**

This description covers all possible valid scenarios based on the given initial state.