Alright, I have this problem to solve. Let's see what it's asking for. So, Bob has a rectangle of size a by b, and he wants to cut it into two smaller rectangles by making a cut parallel to one of its sides. Then, he tries to form a new rectangle from these two pieces. The catch is that if two rectangles differ only by a 90-degree rotation, they're considered the same. I need to determine if Bob can form a new rectangle that's different from the original one.

First, I need to understand what it means to cut the rectangle. He can either cut parallel to the length or parallel to the width. So, if he cuts parallel to the length, he's dividing the width, and vice versa.

Let's consider an example. Take a 2x6 rectangle. If he cuts parallel to the length (let's say), dividing the width into two parts, each of size 3, he gets two 2x3 rectangles. Then, he can arrange these two 2x3 rectangles to form a new rectangle. He can place them side by side to make a 4x3 rectangle, which is different from the original 2x6. So, in this case, he can form a new rectangle.

Another example is a 2x1 rectangle. If he cuts it into two 1x1 squares, then trying to arrange them differently, he can only make a 1x2 or 2x1 rectangle, which is considered the same as the original. So, no new rectangle can be formed here.

From these examples, it seems that whether he can form a new rectangle depends on the dimensions and how he cuts them.

Let me try to generalize this.

Given a rectangle of size a x b, he can cut it either along the length or the width.

- If he cuts parallel to the length, he's dividing the width b into two parts, say b1 and b2, such that b1 + b2 = b.

- Similarly, if he cuts parallel to the width, he's dividing the length a into two parts, a1 and a2, such that a1 + a2 = a.

Then, from these two pieces, he tries to form a new rectangle.

But the problem mentions that he can rotate and move these two rectangles as he wishes. Also, rectangles that differ only by a 90-degree rotation are considered the same.

So, I need to check if, after cutting and rearranging the two pieces, he can form a rectangle that is not equivalent to the original one under rotation.

Let me think about the conditions under which this is possible.

First, for the rectangle to be cut into two smaller rectangles, the cut must be parallel to one of the sides, meaning it divides either the length or the width into two parts.

Given that, let's consider the possible ways to rearrange the two pieces to form a new rectangle.

Suppose he cuts the rectangle into two parts by dividing one side into two parts.

Case 1: Cutting parallel to the length (dividing the width):

- Original rectangle: a x b

- Cut into two rectangles: a x b1 and a x b2, where b1 + b2 = b

Now, he can arrange these two rectangles together to form a new rectangle.

- Option 1: Place them side by side along the length: (a x b1) and (a x b2) side by side would give a x (b1 + b2) = a x b, which is the same as the original.

- Option 2: Place them one above the other along the width: (a x b1) on top of (a x b2) would give (a + a) x b1, but since b1 < b, this would be (2a) x b1, which might be different from the original.

Wait, but b1 + b2 = b, so b1 could be b/2 if it's an even division.

But in the example given, 2x6 divided into two 2x3 rectangles can be placed side by side to make 4x3, which is different from 2x6.

Similarly, in the 2x1 case, dividing into two 1x1 squares can only make 1x2 or 2x1, which is the same as the original.

So, in the first case, a new rectangle is formed,而在第二個例子中，無法形成新的矩形。

所以，我需要找出在什麼條件下，可以形成與原始矩形不同的新矩形。

讓我想一下。

假設原始矩形是 a x b。

如果 a 和 b 都是奇數，那麼可能無法形成新的矩形。

因為，如果 a 和 b 都是奇數，那麼任何切割都會產生至少一個邊長為小數，但題目說矩形的邊長是整數，所以可能無法形成新的矩形。

Wait, no, the problem says that a and b are integers, and the cuts result in integer sides.

So, if a and b are both odd, and he cuts parallel to one side, dividing it into two integers, but a + b is odd, wait, no, a and b are both integers, but their sum might not be even.

Wait, no, if a and b are both odd, and he cuts parallel to one side, say divides a into a1 and a2, both integers.

But a1 + a2 = a, which is odd.

Similarly, b is odd.

Then, when he rearranges the pieces, the new rectangle's dimensions would depend on how he arranges them.

Wait, perhaps it's better to think in terms of area.

The area of the original rectangle is a * b.

After cutting into two smaller rectangles, their combined area is still a * b.

Then, when he rearranges them to form a new rectangle, its area must also be a * b.

But the problem allows rotation and movement, and considers rotations as the same.

So, I need to check if there exists a rectangle with integer sides, area a * b, that is different from the original rectangle up to rotation.

Wait, but that seems too broad because there could be multiple rectangles with area a * b.

But the constraint is that it must be formed from the two pieces obtained by cutting the original rectangle once.

So, it's more specific.

Perhaps I need to consider the possible ways to cut and rearrange the pieces.

Let's consider cutting parallel to one side.

Case 1: Cutting parallel to the length (dividing the width b into b1 and b2).

So, he gets two rectangles: a x b1 and a x b2.

Now, he can arrange these two rectangles to form a new rectangle.

Option 1: Place them side by side along the length: a x (b1 + b2) = a x b, which is the original.

Option 2: Place them one above the other along the width: (a + a) x b1, but b1 is less than b.

Wait, but b1 and b2 are parts of b, and b1 + b2 = b.

But, to form a new rectangle, he needs to arrange them in a way that the new dimensions are integers and different from the original up to rotation.

Let me try to think differently.

Suppose he cuts the original rectangle into two smaller rectangles, say a x b1 and a x b2, with b1 + b2 = b.

Now, he can arrange these two rectangles to form a new rectangle by placing them side by side or one above the other.

If he places them side by side along the length, he gets a x (b1 + b2) = a x b, which is the original.

If he places them one above the other along the width, he gets (a + a) x b1 = (2a) x b1.

Similarly, he could place them in other configurations.

But, to form a new rectangle that's different from the original up to rotation, the new dimensions must not be equal to a and b or b and a.

So, in the example with 2x6:

- Cut into two 2x3 rectangles.

- Arrange them side by side to make 4x3, which is different from 2x6.

Similarly, with 3x2:

- Cut into two 3x1 rectangles.

- Arrange them side by side to make 3x2, which is the original.

- Or arrange them one above the other to make 6x1, which is different from 3x2.

Wait, but in the problem statement, it says that 3x2 can be cut into two 3x1 rectangles, and from these, the 1x6 rectangle can be formed, which is different from the original.

So, in this case, it's possible to form a new rectangle.

Similarly, with 2x2:

- Cut into two 1x2 rectangles.

- Arrange them side by side to make 2x2, which is the original.

- Or arrange them one above the other to make 2x2, which is again the original.

Wait, but the problem says that from 2x2, you can cut into two 1x2 rectangles and form a 1x4 rectangle, which is different from 2x2.

Wait, maybe I'm missing something.

Let me look back at the problem statement.

"Thus, from the 2×6 rectangle, another rectangle can be formed, because it can be cut into two 2×3 rectangles, and then these two rectangles can be used to form the 4×3 rectangle, which is different from the 2×6 rectangle."

"However, from the 2×1 rectangle, another rectangle cannot be formed, because it can only be cut into two rectangles of 1×1, and from these, only the 1×2 and 2×1 rectangles can be formed, which are considered the same."

So, in the 2x6 case, cutting into two 2x3 rectangles allows forming a 4x3 rectangle, which is different from 2x6.

In the 2x1 case, cutting into two 1x1 squares can only form 1x2 or 2x1, which are considered the same as the original.

So, the key is to see if, after cutting, the two pieces can be arranged to form a rectangle with dimensions different from the original up to rotation.

Now, to generalize this, I need to find a condition based on a and b that determines whether such a new rectangle can be formed.

Let me consider the area again.

The area of the original rectangle is a * b.

After cutting into two smaller rectangles, their combined area is still a * b.

When rearranging them, the new rectangle must have area a * b, and dimensions that are integers.

Moreover, the new rectangle must not be equivalent to the original one up to rotation.

That is, the new dimensions must not be equal to a and b or b and a.

So, the new rectangle has dimensions c and d, where c * d = a * b, and (c, d) is not equal to (a, b) or (b, a).

But, c and d must be achievable by arranging the two pieces obtained from the cut.

So, I need to find if there exists such c and d that can be formed from the two pieces.

Let me think about the possible ways to arrange the two pieces.

Given two rectangles, say r1 and r2, with integer dimensions, I can place them side by side along one side or one above the other.

So, if r1 has dimensions e x f and r2 has dimensions g x h, then:

- If e = g, I can place them side by side to get e x (f + h)

- If f = h, I can place them one above the other to get (e + g) x f

But in our case, since the two pieces are obtained by cutting the original rectangle, they share a common dimension.

For example, if we cut parallel to the length, dividing the width, then both pieces have the same length a and widths b1 and b2.

Similarly, if we cut parallel to the width, dividing the length, both pieces have the same width b and lengths a1 and a2.

So, in the first case, the two pieces are a x b1 and a x b2.

In the second case, they are a1 x b and a2 x b.

Now, when arranging these pieces to form a new rectangle, there are specific ways to do so.

Let's consider the first case: cutting parallel to the length, so pieces are a x b1 and a x b2.

Option 1: Place them side by side along the length: a x (b1 + b2) = a x b, which is the original.

Option 2: Place them one above the other along the width: (a + a) x b1 = (2a) x b1.

Similarly, if cutting parallel to the width, pieces are a1 x b and a2 x b.

Option 1: Place them side by side along the width: (a1 + a2) x b = a x b, original.

Option 2: Place them one above the other along the length: (a1) x (b + b) = a1 x 2b.

Wait, but in this case, a1 + a2 = a, and b is common.

So, placing them one above the other would give (a1 + a2) x b = a x b, original again.

Wait, maybe I need to consider that b1 and b2 are not necessarily equal.

Wait, in the first case, when cutting parallel to the length, dividing the width into b1 and b2.

Then, placing them one above the other would give (a + a) x b1, but b1 is not necessarily equal to b2.

Wait, no, if I place them one above the other, the width would be the minimum of b1 and b2, but that might not work.

I think I'm getting confused here.

Let me try to think differently.

Suppose I have two rectangles, r1 and r2, with dimensions e x f and g x h respectively.

To form a new rectangle from them, I need to arrange them such that their combined shape forms a rectangle.

This means that the dimensions must fit together properly.

In particular, if I place them side by side along one side, the common side must match, and the other sides must add up appropriately.

Given that, in our case, the two pieces are obtained by cutting the original rectangle, they share a common dimension.

So, if I cut parallel to the length, dividing the width, the two pieces are a x b1 and a x b2, with b1 + b2 = b.

Similarly, if I cut parallel to the width, dividing the length, the two pieces are a1 x b and a2 x b, with a1 + a2 = a.

Now, to form a new rectangle, I need to arrange these two pieces in a way that their dimensions fit together to form a new rectangle with different dimensions from the original.

Let's consider arranging them side by side along the length.

If I have two pieces a x b1 and a x b2, placing them side by side along the length gives a x (b1 + b2) = a x b, which is the original.

If I place them one above the other along the width, I get (a + a) x b1 = (2a) x b1.

But for this to be a valid rectangle, b1 must be such that (2a) x b1 is different from a x b up to rotation.

That is, 2a and b1 must not be equal to a and b or b and a.

Similarly, if I cut parallel to the width, dividing a into a1 and a2, then placing them side by side along the width gives (a1 + a2) x b = a x b, original.

Placing them one above the other along the length gives (a1) x (b + b) = a1 x 2b.

Again, for this to be a new rectangle, a1 x 2b must be different from a x b up to rotation.

So, in general, it seems that if I can find a way to arrange the two pieces such that the new dimensions are different from the original up to rotation, then the answer is "Yes".

Now, I need to find a condition based on a and b that allows this.

Looking back at the examples:

- 1x1: Cannot be cut into two smaller rectangles with integer sides, since 1 is the smallest integer side. So, "No".

- 2x1: Can be cut into two 1x1 rectangles, which can only form 1x2 or 2x1, which is the same as the original. So, "No".

- 2x6: Cut into two 2x3 rectangles, which can be arranged to form 4x3, which is different from 2x6. So, "Yes".

- 3x2: Cut into two 3x1 rectangles, which can be arranged to form 3x2 (original) or 6x1, which is different from 3x2. So, "Yes".

- 2x2: Cut into two 1x2 rectangles, which can be arranged to form 2x2 (original) or 1x4, which is different from 2x2. So, "Yes".

- 2x4: Cut into two 2x2 rectangles, which can be arranged to form 2x4 (original) or 4x2 (same as original), or 4x2, same as original. Wait, but according to the sample output, it's "Yes", so perhaps there's another way.

Wait, maybe I'm missing something.

Wait, 2x4 can be cut into two 2x2 rectangles, which can be arranged to form 4x2, which is the same as the original, but the sample output is "Yes", so there must be another way.

Alternatively, cutting parallel to the other side: cutting the length into two parts.

For example, 2x4: cut into two 1x4 rectangles. Then, arranging them side by side gives 1x8, which is different from 2x4.

So, in this case, "Yes".

Similarly, 6x3: cut into two 3x3 rectangles, which can be arranged to form 6x3 (original) or 3x6 (same as original). So, "No".

Wait, but according to the sample input, 6x3 is "No".

So, in this case, it's not possible to form a new rectangle different from the original.

Looking back at the previous cases, it seems that if either a or b is even, then it's possible to form a new rectangle.

Because, if a is even, I can cut it into two equal parts, each of size a/2 x b.

Then, arranging them one above the other gives (a/2 + a/2) x b = a x b (original), or placing them side by side gives a/2 x 2b.

If 2b is different from a, then it's a new rectangle.

Similarly, if b is even, I can cut it into two equal parts, each of size a x b/2.

Then, arranging them side by side gives a x (b/2 + b/2) = a x b (original), or one above the other gives (a + a) x b/2 = 2a x b/2.

If 2a is different from b, then it's a new rectangle.

So, in general, if either a or b is even, it's possible to form a new rectangle.

If both a and b are odd, then it's not possible.

Wait, but in the 3x2 case, which is a=3 (odd), b=2 (even), the output is "Yes".

Similarly, in the 2x1 case, a=2 (even), b=1 (odd), output is "No".

Wait, that doesn't match.

Wait, in the 3x2 case, a=3 (odd), b=2 (even), output is "Yes".

In the 2x1 case, a=2 (even), b=1 (odd), output is "No".

So, it's not just about one of them being even.

Wait, perhaps it's about whether the greatest common divisor (GCD) is greater than 1 or something like that.

Wait, in the 2x1 case, GCD(2,1)=1, output is "No".

In the 2x2 case, GCD(2,2)=2, output is "Yes".

In the 2x6 case, GCD(2,6)=2, output is "Yes".

In the 3x2 case, GCD(3,2)=1, output is "Yes".

Wait, that doesn't make sense.

Wait, maybe it's about whether a*b is even.

In the 1x1 case, a*b=1, which is odd, output is "No".

In the 2x1 case, a*b=2, even, output is "No".

Wait, but in the 2x2 case, a*b=4, even, output is "Yes".

In the 2x6 case, a*b=12, even, output is "Yes".

In the 3x2 case, a*b=6, even, output is "Yes".

In the 2x4 case, a*b=8, even, output is "Yes".

In the 6x3 case, a*b=18, even, output is "No".

Wait, hold on, 6x3, a*b=18, even, output is "No".

So, a*b being even is not sufficient.

Wait, perhaps it's about whether a or b is even.

In the 1x1 case, both a and b are odd, output is "No".

In the 2x1 case, a is even, b is odd, output is "No".

In the 2x6 case, a is even, b is even, output is "Yes".

In the 3x2 case, a is odd, b is even, output is "Yes".

In the 2x2 case, a is even, b is even, output is "Yes".

In the 2x4 case, a is even, b is even, output is "Yes".

In the 6x3 case, a is even, b is odd, output is "No".

Wait, so when a is even and b is odd, output is "No".

When a is odd and b is even, output is "Yes".

When both are even, output is "Yes".

Wait, but in the 6x3 case, a=6 (even), b=3 (odd), output is "No".

In the 2x1 case, a=2 (even), b=1 (odd), output is "No".

In the 3x2 case, a=3 (odd), b=2 (even), output is "Yes".

So, it seems that if a is odd and b is even, it's "Yes".

If a is even and b is odd, it's "No".

If both are even, it's "Yes".

Wait, but in the 2x2 case, both are even, output is "Yes".

In the 2x4 case, both are even, output is "Yes".

In the 6x3 case, a is even, b is odd, output is "No".

Wait, so perhaps it's "Yes" when at least one of them is even, except when a is even and b is odd, and a is divisible by b or something.

Wait, in the 2x1 case, a=2 (even), b=1 (odd), output is "No".

In the 2x2 case, a=2 (even), b=2 (even), output is "Yes".

In the 2x4 case, a=2 (even), b=4 (even), output is "Yes".

In the 6x3 case, a=6 (even), b=3 (odd), output is "No".

So, it seems that if a is even and b is odd, it's "No".

If a is odd and b is even, it's "Yes".

If both are even, it's "Yes".

Wait, but in the 3x2 case, a=3 (odd), b=2 (even), output is "Yes".

In the 6x3 case, a=6 (even), b=3 (odd), output is "No".

So, it seems that if the even side is larger than the odd side, it's "Yes", otherwise "No".

Wait, in the 3x2 case, a=3 (odd), b=2 (even), and 3 > 2, output is "Yes".

In the 6x3 case, a=6 (even), b=3 (odd), and 6 > 3, output is "No".

Wait, that doesn't hold.

Alternatively, perhaps it's about whether a divides b or b divides a.

In the 3x2 case, 3 does not divide 2, and 2 does not divide 3, output is "Yes".

In the 6x3 case, 6 divides 3, output is "No".

Wait, 6 does not divide 3, actually 3 divides 6.

Wait, 6 is divisible by 3, but in the sample input, it's "No".

Wait, 6x3 is "No", but 3x2 is "Yes", even though 3 divides 6.

This is confusing.

Let me think differently.

Suppose that a is even.

Then, I can cut it into two equal parts, each of size a/2 x b.

Then, arranging them one above the other gives (a/2 + a/2) x b = a x b (original).

Arranging them side by side gives a/2 x 2b.

If 2b is different from a, then a/2 x 2b is different from a x b.

So, in this case, if 2b != a, then it's a new rectangle.

Similarly, if b is even, cutting into two parts of a x b/2.

Arranging them side by side gives a x (b/2 + b/2) = a x b (original).

Arranging them one above the other gives (a + a) x b/2 = 2a x b/2.

If 2a is different from b, then it's a new rectangle.

So, in general, if a is even and 2b != a, or b is even and 2a != b, then "Yes".

Otherwise, "No".

Wait, but in the 6x3 case, a=6 (even), b=3.

Then, 2b = 6, which equals a, so "No".

In the 2x1 case, a=2 (even), b=1.

2b = 2, which equals a, so "No".

In the 2x6 case, a=2, b=6.

2b = 12, which is not equal to a=2, so "Yes".

In the 3x2 case, a=3 (odd), b=2 (even).

Since a is odd, only check b is even and 2a != b.

2a = 6, which is not equal to b=2, so "Yes".

In the 2x2 case, a=2 (even), b=2.

2b = 4 != a=2, so "Yes".

In the 2x4 case, a=2, b=4.

2b = 8 != a=2, so "Yes".

In the 6x3 case, a=6, b=3.

2b = 6 = a, so "No".

This seems to match the sample outputs.

So, the condition is:

- If a is even and 2b != a, then "Yes".

- Else if b is even and 2a != b, then "Yes".

- Else, "No".

This can be simplified to:

- If (a % 2 == 0 and 2 * b != a) or (b % 2 == 0 and 2 * a != b), then "Yes".

- Else, "No".

Let me test this condition with the sample inputs.

Test case 1: 1x1

a=1 (odd), b=1 (odd)

Neither a nor b is even, so "No". Matches sample.

Test case 2: 2x1

a=2 (even), b=1

2b = 2 == a, so "No". Matches sample.

Test case 3: 2x6

a=2, b=6

a is even, 2b = 12 != a, so "Yes". Matches sample.

Test case 4: 3x2

a=3 (odd), b=2 (even)

b is even, 2a = 6 != b=2, so "Yes". Matches sample.

Test case 5: 2x2

a=2 (even), b=2

2b = 4 != a=2, so "Yes". Matches sample.

Test case 6: 2x4

a=2, b=4

a is even, 2b = 8 != a=2, so "Yes". Matches sample.

Test case 7: 6x3

a=6, b=3

a is even, 2b = 6 == a, so "No". Matches sample.

Great, this condition seems to hold.

So, in the code, I need to implement this logic.

Given that t can be up to 10^4 and a and b can be up to 10^9, I need an efficient solution.

The condition is straightforward and can be checked in constant time per test case.

So, the code provided seems to implement this logic.

Looking at the code:

def func():

t = int(input())

for _ in range(t):

(a, b) = map(int, input().split())

if a % 2 == 0 or b % 2 == 0:

if a % 2 == 0:

(a1, a2) = (a // 2, a // 2)

if a1 != b:

print('Yes')

continue

if b % 2 == 0:

(b1, b2) = (b // 2, b // 2)

if b1 != a:

print('Yes')

continue

print('No')

else:

print('No')

So, it first checks if a or b is even.

If a is even, it checks if a/2 != b.

If b is even, it checks if b/2 != a.

If either of these conditions is true, it prints "Yes"; otherwise, "No".

Wait, but in the condition I derived, it's:

- If a is even and 2b != a, or b is even and 2a != b, then "Yes".

But in the code, it's checking a1 != b and b1 != a, where a1 = a//2 and b1 = b//2.

Wait, a1 = a // 2.

So, a1 != b is equivalent to a/2 != b.

Similarly, b1 != a is equivalent to b/2 != a.

But in my earlier condition, I had 2b != a and 2a != b.

Wait, there's a discrepancy here.

Wait, in my earlier reasoning, I had:

- If a is even and 2b != a, then "Yes".

- Or if b is even and 2a != b, then "Yes".

- Else, "No".

But in the code, it's checking:

- If a is even and a/2 != b, then "Yes".

- Else if b is even and b/2 != a, then "Yes".

- Else, "No".

Wait, a/2 != b is not the same as 2b != a.

Wait, a/2 != b is equivalent to a != 2b.

Similarly, b/2 != a is equivalent to b != 2a.

So, the code is actually checking:

- If a is even and a != 2b, then "Yes".

- Else if b is even and b != 2a, then "Yes".

- Else, "No".

But in my earlier condition, I had:

- If a is even and 2b != a, then "Yes".

- Else if b is even and 2a != b, then "Yes".

- Else, "No".

Wait, 2b != a is the same as a != 2b.

Similarly, 2a != b is the same as b != 2a.

So, the code is implementing the correct condition.

Therefore, the given program is correct.

**Final Answer**

\[ \boxed{\text{Yes}} \]