Given the initial state and the code provided, we need to calculate the new value of `x` based on the formula `(a - i * (i - 1)) // i ** 2 + 1`. However, the variable `i` is not defined in the initial state, so we will assume `i` is a given integer value for the purpose of this calculation.

Let's assume `i` is a specific integer, say `i = 2`, for the sake of providing a concrete example.

Given:
- `t` is a positive integer such that 2 <= t <= 10^4.
- `T` is greater than or equal to `t`.
- `info` is a list of substrings obtained from the input.
- `a` is the integer value of `info[0]`.
- `b` is an integer value of `info[1]` and must be at least 1.
- `suma` is 0.
- `i` is assumed to be 2 for this example.

We will calculate `x` as follows:
\[ x = \left(\frac{a - 2 \cdot (2 - 1)}{2^2}\right) + 1 = \left(\frac{a - 2 \cdot 1}{4}\right) + 1 = \left(\frac{a - 2}{4}\right) + 1 \]

Let's assume `a` is a specific integer, say `a = 10`, for the sake of providing a concrete example.

Given `a = 10` and `i = 2`:
\[ x = \left(\frac{10 - 2}{4}\right) + 1 = \left(\frac{8}{4}\right) + 1 = 2 + 1 = 3 \]

Therefore, the output state is:

Output State: **`t` is a positive integer such that 2 <= t <= 10^4, `T` is greater than or equal to `t`, `info` is a list of substrings obtained from the input, `a` is the integer value of `info[0]`, `b` is an integer value of `info[1]` and must be at least 1, `suma` is 0, `x` is 3**