Example Answer:
After entering the if statement, the condition (x * (x + 1) > n) is true. Therefore, the value of `answr` is calculated as (x + x + 1) * 2. Since x is the square root of n, the value of x varies based on the input integer n. The output state is: N is a positive integer such that 1 ≤ N ≤ 10^6, n is an input integer, x is the square root of n, and answr is calculated based on x.
Output State: **N is a positive integer such that 1 ≤ N ≤ 10^6, n is an input integer, x is the square root of n, and answr is calculated based on x**