First, let's analyze the given code snippet:

```python
curr += a[i + 1] + (c[i] - b[i + 1] + 1)
```

Given the initial state:
- `best` is updated to `max(best, curr + a[4] + (c[3] - b[4] + 1))`
- `i` is 4
- `curr` is updated to `curr + a[4] + (c[3] - b[4] + 1)` if `a[4] != b[4]`, otherwise `curr` remains 1.

Since `i` is 4, the code snippet will access `a[5]`, `c[4]`, and `b[5]`.

Let's assume the following values for clarity (since actual values are not provided):
- Let `a[4] = 2`, `b[4] = 3`, `a[5] = 4`, `c[4] = 5`, and `b[5] = 6`.

Given these values:
- If `a[4] != b[4]`, which is true (`2 != 3`), then `curr` is updated to `curr + a[4] + (c[3] - b[4] + 1)`.
- Since `a[4]` is 2 and `b[4]` is 3, `curr` becomes `curr + 2 + (c[3] - 3 + 1)`.
- If `c[3]` is not specified, let's assume `c[3] = 4` for calculation purposes.

So, `curr` becomes `curr + 2 + (4 - 3 + 1) = curr + 2 + 2 = curr + 4`.

After the operation, the updated value of `curr` is `curr + 4`.

The other variables remain unchanged: `best` and `n` are still in their original state because they are not directly modified by the code snippet.

Therefore, the Output State is:
Output State: **`best` is updated to max(`best`, `curr + a[4] + (c[3] - b[4] + 1))`, `i` is 4, `n` remains the same, `curr` is `curr + 4`.**