The value of `n` is decremented by `m`. Given that `m` is `(n + 1) // 2`, the new value of `n` will be `n - (n + 1) // 2`.

Let's break this down:
- `n` is initially at least 2.
- `m` is `(n + 1) // 2`.
- After executing `n -= m`, the new value of `n` will be `n - (n + 1) // 2`.

For example:
- If `n` is 3, then `m` is `(3 + 1) // 2 = 2`, and `n` becomes `3 - 2 = 1`.
- If `n` is 4, then `m` is `(4 + 1) // 2 = 2`, and `n` becomes `4 - 2 = 2`.

Therefore, the new value of `n` is `n - (n + 1) // 2`.

Output State: **`t` is an input integer such that 1 ≤ t ≤ 5 · 10^4, `n` is `n - (n + 1) // 2`, `k` is an input integer, `L` is a list containing the value `(n + 1) // 2`, `m` is `(n + 1) // 2`.**