Alright, I've got this problem to solve. Let's see what it's asking for. So, I'm given two integers, x and y, both of the same length, and they're made up of digits from 1 to 9. I can swap the i-th digit of x with the i-th digit of y any number of times, and I need to maximize the product of x and y after these swaps.

First, I need to understand what swapping digits means in this context. For example, if x is 73 and y is 31, swapping the second digits would make x 71 and y 33. The product before swapping is 73 * 31 = 2263, and after swapping, it's 71 * 33 = 2343, which is larger. So, swapping in this case improved the product.

I need to find a way to maximize this product by potentially swapping digits across x and y at the same positions.

Let me think about how the product of two numbers is affected by their digits. The product x * y is what I want to maximize. To maximize the product, I should aim to make both x and y as large as possible, but since I'm swapping digits at the same positions, I need to decide for each position whether swapping will help increase the overall product.

One approach could be to greedily decide for each position whether swapping increases the product or not. But that might not lead to the global maximum because decisions for one position could affect others.

Let me consider the mathematical perspective. Let's say for a specific position, I have digits a and b in x and y respectively. If I swap them, the change in the product can be calculated.

Let’s denote the original numbers as x and y, and after swapping the i-th digit, the new numbers are x' and y'.

The difference in the product would be x' * y' - x * y.

I need to see if x' * y' is greater than x * y for each possible swap.

But calculating this for each position separately might be too time-consuming, especially since the numbers can have up to 100 digits.

I need a smarter way to decide whether to swap or not for each position.

Let me consider the contribution of each pair of digits to the overall product.

For two numbers x and y, the product is the sum over all pairs of digits multiplied together, weighted by their positional values.

But that seems too complicated. Maybe there's a pattern or a rule that can be applied to decide whether to swap digits at each position.

Let me look at some examples to see if I can find a pattern.

Take the first example:

x = 73

y = 31

Swapping the second digits:

x becomes 71

y becomes 33

Product before swapping: 73 * 31 = 2263

Product after swapping: 71 * 33 = 2343

So, swapping increased the product.

Another example:

x = 2

y = 5

If I swap the only digit, x becomes 5 and y becomes 2.

Product before swapping: 2 * 5 = 10

Product after swapping: 5 * 2 = 10

No change in this case.

Another example:

x = 3516

y = 3982

If I swap all digits:

x becomes 3912

y becomes 3586

Product before swapping: 3516 * 3982 = 13994352

Product after swapping: 3912 * 3586 = 14041392

So, swapping improved the product here as well.

From these examples, it seems that swapping digits where the digit in x is smaller than the digit in y might be beneficial.

Wait, in the first example, x had 7 and y had 3; swapping made x larger and y larger as well, increasing the product.

In the second example, x was 2 and y was 5; swapping didn't change the product.

In the third example, x was 3516 and y was 3982; swapping higher digits in x with higher digits in y seemed to help.

Wait, maybe it's about making the overall numbers as large as possible.

So, perhaps I should swap digits where swapping makes both numbers as large as possible.

Wait, but in the first example, swapping the second digits made x smaller (73 to 71) but y larger (31 to 33), and the product increased.

Wait, so sometimes swapping can make one number smaller and the other larger, but still increase the product.

This is tricky.

Maybe I need to consider the relative sizes of the digits in x and y at each position.

Let me consider the general case.

Suppose for a position, x has digit a and y has digit b.

If I swap, x becomes with a replaced by b, and y becomes with b replaced by a.

I need to see how this affects the product.

Let me think about the difference in the product.

Original product: x * y

After swapping, product: (x - a * 10^k + b * 10^k) * (y - b * 10^k + a * 10^k), where k is the position weight.

This seems complicated to handle for each position separately.

Maybe there is a better way.

Let me think about sorting the digits.

If I sort the digits of x and y in some way, maybe I can maximize the product.

Wait, but the numbers have to maintain their digit lengths and positions, except for swapping at the same positions.

I can't rearrange the digits within x or y; I can only swap corresponding digits between x and y.

So, I can't sort the digits within x or y independently.

Wait, but I can swap digits at the same positions between x and y.

So, it's like deciding for each position whether to swap or not.

I need to make decisions for each position independently, because swapping at one position doesn't affect the others.

Wait, but actually, it does affect the overall product, as x and y are multiplied together.

But perhaps, since the positions are independent in terms of swapping, I can make the decision for each position separately.

Let me consider that.

If I have two numbers, x and y, and I can swap their digits at the same positions, I need to decide for each position whether to swap or not, to maximize x * y.

If I treat each position independently, I can decide for each position whether swapping increases the product or not.

But as seen in the earlier example, sometimes swapping makes one number smaller and the other larger, but the product increases.

So, perhaps I need to find a rule that, for each position, decides whether swapping increases the product.

Alternatively, perhaps there's a way to decide based on the relative sizes of the digits at each position.

Wait, maybe I can think in terms of which digit contributes more to the overall product.

But this seems too vague.

Let me try to think differently.

Suppose I fix all swaps except for one position.

Then, I can decide whether swapping that position increases the product or not.

But doing this for each position separately might not lead to the global maximum, but maybe in this problem, making local decisions is sufficient.

I need to see.

Let me consider the grades of the digits.

Since the digits are from 1 to 9, I can consider them as integers.

Let me think about the following:

For each position, if the digit in x is smaller than the digit in y, swapping them might increase the product.

Wait, in the first example, x had 7 and y had 3; swapping made x=71 and y=33, and the product increased.

But in the second example, x=2 and y=5; swapping made x=5 and y=2, and the product remained the same.

Wait, but in the third example, x=3516 and y=3982; swapping certain digits increased the product.

Wait, perhaps I need to consider the positions from the most significant digit to the least significant digit.

Let me think about maximizing the most significant digits first.

To maximize the product of two numbers, I should make both numbers as large as possible.

So, for each position, starting from the most significant digit, I should choose the larger digit for both x and y.

But wait, I can't choose independently for x and y because I can only swap at the same positions.

Wait, perhaps I should swap digits at each position if it makes both numbers larger in a certain way.

This is confusing.

Let me consider another approach.

Let me consider that for each position, I have two choices: swap or not.

I need to make a choice for each position independently.

So, perhaps I can make the decision for each position based on some condition.

Let me consider the effect of swapping a particular position on the product.

Let’s denote:

Let’s say position i has digit a in x and digit b in y.

If I swap, x becomes x - a*10^{p} + b*10^{p}, and y becomes y - b*10^{p} + a*10^{p}, where p is the positional weight.

The change in the product is:

(x - a*10^{p} + b*10^{p}) * (y - b*10^{p} + a*10^{p}) - x * y

Let’s expand this:

x*y - b*10^{p}*x + a*10^{p}*x - a*10^{p}*y + b*10^{p}*y + (b*10^{p} - a*10^{p})^2 - x*y

Simplify:

- b*10^{p}*x + a*10^{p}*x - a*10^{p}*y + b*10^{p}*y + (b - a)^2 * 10^{2p}

Further simplifying:

10^{p} * [(-b + a)x + (-a + b)y] + (b - a)^2 * 10^{2p}

Factor out (b - a):

(b - a) * [ -10^{p} * x + 10^{p} * y + (b - a) * 10^{2p} ]

This seems complicated, and it's not clear when this change is positive or negative.

Maybe there's a better way to approach this.

Let me consider that since x and y have the same length, and I can only swap digits at the same positions, perhaps I can treat each position independently and decide whether to swap based on some condition.

Wait, perhaps I can consider that for positions where a < b, swapping increases the product, and for positions where a >= b, it doesn't.

But in the second example, when a=2 and b=5, swapping doesn't change the product.

Wait, but in that case, a=2 and b=5, swapping makes x=5 and y=2, so product remains the same.

Wait, but according to my earlier assumption, since a < b, swapping should increase the product, but in this case, it doesn't.

So, that assumption might be wrong.

Let me think differently.

Maybe I need to consider the difference in the digits.

Let’s consider the difference (b - a).

If I swap, x increases by (b - a)*10^{p}, and y decreases by (b - a)*10^{p}.

So, the product changes by x' * y' - x * y = (x + (b - a)*10^{p}) * (y - (b - a)*10^{p}) - x * y

Expanding:

x*y - x*(b - a)*10^{p} + (x + (b - a)*10^{p})*((b - a)*10^{p}) - x*y

Simplify:

- x*(b - a)*10^{p} + x*(b - a)*10^{p} + (b - a)^2 * 10^{2p} = (b - a)^2 * 10^{2p}

Wait, so the change in product is always (b - a)^2 * 10^{2p}, which is always non-negative.

So, swapping digits at any position where a != b will always increase the product by (b - a)^2 * 10^{2p}.

But in the second example, a=2 and b=5, swapping makes the product stay the same, but according to this, it should increase.

Wait, perhaps I made a mistake in the calculation.

Let me recalculate.

Original product: x * y

After swapping: (x - a*10^{p} + b*10^{p}) * (y - b*10^{p} + a*10^{p})

So, x' = x + (b - a)*10^{p}

y' = y + (a - b)*10^{p}

Therefore, x' * y' = [x + (b - a)*10^{p}] * [y + (a - b)*10^{p}]

Expanding:

x*y + x*(a - b)*10^{p} + y*(b - a)*10^{p} + (b - a)*(a - b)*10^{2p}

Simplify (b - a)*(a - b) = -(b - a)^2

So, x' * y' = x*y + x*(a - b)*10^{p} + y*(b - a)*10^{p} - (b - a)^2 * 10^{2p}

Therefore, x' * y' - x*y = x*(a - b)*10^{p} + y*(b - a)*10^{p} - (b - a)^2 * 10^{2p}

Factor out (a - b)*10^{p}:

= (a - b)*10^{p} * (x - y) - (b - a)^2 * 10^{2p}

= (a - b)*10^{p} * (x - y) - (a - b)^2 * 10^{2p}

This seems more complicated than I thought.

In the second example, x=2, y=5, a=2, b=5, p=0 (units place)

So, x' * y' - x * y = (2 - 5)*1*(2 - 5) - (5 - 2)^2 * 1 = (-3)*(-3) - 9 = 9 - 9 = 0

So, the product doesn't change, which matches the observation.

In the first example, x=73, y=31, a=3, b=1, p=0

x' * y' - x * y = (3 - 1)*1*(73 - 31) - (1 - 3)^2 * 1 = 2*42 - 4 = 84 - 4 = 80 > 0

So, the product increases, which matches the observation.

In the third example, x=3516, y=3982, a=1 and b=8 for one position

x' * y' - x * y = (1 - 8)*10^(position)*(x - y) - (8 - 1)^2 * 10^(2*position)

This would be negative since (1 - 8) = -7, and assuming x < y, (x - y) negative, so (-7)*negative = positive, minus a positive term.

So, it's not straightforward.

Given this complexity, perhaps the best approach is to swap digits at positions where a < b, and keep them as is where a >= b.

This seems to make sense because, in the first example, a=3 < b=1, so swapping increases the product.

In the second example, a=2 < b=5, swapping doesn't change the product.

In the third example, a=1 < b=8, swapping would increase the product.

Wait, but in the second example, according to this rule, since a=2 < b=5, we should swap, but the product remains the same.

So, maybe this rule isn't perfect, but perhaps it's good enough.

Alternatively, perhaps I should swap when swapping increases the product, based on the calculation above.

But calculating this for each position separately would be too time-consuming for large numbers.

I need a simpler rule.

Let me consider maximizing the sum of x and y.

Since x and y have the same length, and I can only swap digits at the same positions, to maximize the sum, I should choose the larger digit for x and the larger digit for y at each position.

Wait, but that doesn't make sense because swapping would affect both x and y.

Wait, actually, to maximize the sum x + y, I should choose x_i = max(a_i, b_i) and y_i = min(a_i, b_i) for each position i.

Because x + y = sum(x_i + y_i) = sum(a_i + b_i), which is constant, so swapping doesn't affect the sum.

Interesting, so the sum remains the same regardless of swapping.

But the product can change.

So, maximizing the product is different from maximizing the sum.

In fact, in the second example, swapping didn't change the product, even though according to the earlier calculation, it should have increased by (5 - 2)^2 = 9, but in reality, it stayed the same.

Wait, in my earlier calculation, I had x' * y' - x * y = (a - b)*10^{p} * (x - y) - (a - b)^2 * 10^{2p}

In the second example, x=2, y=5, a=2, b=5, p=0

So, (2 - 5)*1*(2 - 5) - (5 - 2)^2 * 1 = (-3)*(-3) - 9 = 9 - 9 = 0

So, the product doesn't change.

Wait, but according to the general formula, x' * y' - x * y = (a - b)*10^{p} * (x - y) - (a - b)^2 * 10^{2p}

I need to see when this is positive.

Let’s set it greater than zero:

(a - b)*10^{p} * (x - y) - (a - b)^2 * 10^{2p} > 0

Factor out (a - b)*10^{p}:

(a - b)*10^{p} * [ (x - y) - (a - b)*10^{p} ] > 0

So, the inequality depends on the sign of (a - b) and the expression [ (x - y) - (a - b)*10^{p} ]

This seems too involved to make a general rule.

Perhaps I need to consider that for higher positions (higher p), the effect is more significant, so I should prioritize swapping in higher positions.

But I'm not sure.

Let me look back at the examples.

In the first example, swapping the second digit (less significant) increased the product.

In the third example, swapping certain digits increased the product.

In the second example, swapping the only digit didn't change the product.

Maybe I should swap digits where a < b, especially in higher positions.

But I need a better strategy.

Let me consider sorting the digits in x and y in some way.

Wait, but I can't rearrange digits within x or y; I can only swap corresponding digits between x and y.

So, I need to make decisions for each position independently.

Given that, perhaps I can make a decision for each position based on whether swapping increases the product or not.

But as seen, sometimes it increases, sometimes it doesn't.

Alternatively, perhaps there's a way to pair the digits and decide based on their relative values.

Wait, maybe I can think in terms of greedy algorithm, making the best choice at each position to maximize the product.

But I need to define what the best choice is.

Let me consider that for the most significant digits, I should choose the larger digit for both x and y, but since I can only swap at the same positions, I need to decide whether swapping at that position helps or not.

Wait, perhaps I should swap digits where a < b, starting from the most significant digits.

Let me test this approach with the examples.

First example:

x=73, y=31

At the first position: a=7, b=3; since 7 > 3, don't swap.

At the second position: a=3, b=1; since 3 > 1, don't swap.

But according to the sample output, swapping the second digits gives a higher product.

So, my approach is wrong here.

Wait, maybe I should swap where a < b.

In this case, a=3 < b=1 is false, so don't swap, which contradicts the sample output.

Wait, but in the sample, swapping increased the product, but according to my rule, I shouldn't swap.

So, my rule is incorrect.

Let me try another rule.

Maybe I should swap digits where a * x_remaining < b * y_remaining or something like that.

But this seems too complicated, especially since the numbers can be up to 100 digits.

I need a simpler rule.

Let me consider that to maximize x * y, I should make x and y as large as possible in terms of their numerical values.

So, for each position, I should choose the larger digit for both x and y.

But since I can only swap corresponding digits, I can choose to swap or not.

So, for each position, I should choose to swap if it makes both x and y larger in that position.

Wait, but in reality, swapping affects both x and y.

Wait, perhaps I should choose to swap if the digit in x becomes larger and the digit in y becomes larger as well.

But that doesn't make sense because swapping could make one larger and the other smaller.

Wait, in the first example, swapping the second digits made x=71 (smaller than 73) and y=33 (larger than 31), and the product increased.

So, sometimes making one number smaller and the other larger can increase the product.

This is counterintuitive.

Let me think about the properties of multiplication.

Multiplication is such that if the sum of the numbers is constant, the product is maximized when the numbers are as close to each other as possible.

But in this problem, the sum of x and y remains the same regardless of swapping because we're just swapping digits at the same positions.

Wait, no, in the second example, x=2 and y=5; swapping makes x=5 and y=2; the sum remains the same (7), and the product remains the same (10).

In the first example, x=73 and y=31; sum is 104; after swapping, x=71 and y=33; sum remains 104; product increases from 2263 to 2343.

So, in this case, even though the sum remains the same, the product increases when x and y are closer to each other.

Wait, x=73 and y=31; after swapping, x=71 and y=33.

The difference between x and y decreases from 42 to 38, and the product increases.

So, perhaps making x and y closer together increases the product.

Is this always the case?

In the second example, x=2 and y=5; after swapping, x=5 and y=2; the difference changes from 3 to 3, same difference, and the product remains the same.

So, in that case, swapping doesn't change the product.

In the third example, x=3516 and y=3982; after swapping certain digits, x=3912 and y=3586; the difference changes from 466 to 326, and the product increases.

So, again, reducing the difference between x and y increases the product.

This seems to suggest that swapping digits where a < b makes x larger and y smaller, thereby bringing them closer together, which increases the product.

But in the second example, swapping when a=2 and b=5 makes x=5 and y=2, which are closer, but the product remains the same.

So, perhaps this is a special case where the numbers are single-digit.

Let me think about the general case.

Given that x and y have the same length, and I can only swap digits at the same positions, I should swap digits where a < b to make x larger and y smaller, thereby bringing them closer together, which increases the product.

But in the second example, swapping a=2 and b=5 doesn't change the product, even though a < b.

Wait, perhaps because the numbers are single-digit, the product remains the same.

In multi-digit numbers, swapping a < b increases the product, as seen in the first and third examples.

So, perhaps the rule is to swap digits where a < b for multi-digit numbers, and for single-digit numbers, it doesn't matter.

But in the first example, a=3 < b=1 is false, so don't swap, but according to the sample, swapping increases the product.

Wait, no, in the first example, a=3 < b=1 is false, so don't swap, but according to the sample, swapping increases the product.

Wait, b=1 is less than a=3, so a=3 >= b=1, so don't swap.

But in the sample, swapping increases the product.

So, my rule is contradicted by the sample.

Wait, perhaps I need to swap digits where a < b, but in the first example, a=3 < b=1 is false, so don't swap, but the sample suggests swapping.

Wait, but b=1 is less than a=3, so swapping would make x=71 and y=33.

Wait, in this case, a=3 < b=1 is false, so according to my rule, don't swap, which contradicts the sample.

Wait, perhaps I need to swap digits where a > b.

In the first example, a=3 > b=1, so swap, which matches the sample.

Wait, but according to my earlier calculation, swapping increases the product.

Wait, in the second example, a=2 < b=5, so swap, but swapping doesn't change the product.

In the third example, a=1 < b=8, so swap, which increases the product.

So, perhaps the rule is to swap digits where a < b.

But in the first example, a=3 > b=1, so don't swap, but according to the sample, swapping increases the product.

Wait, perhaps I need to swap digits where a < b, even if a > b.

Wait, maybe I need to swap digits where a != b, regardless of which is larger.

But in the second example, a != b, and swapping doesn't change the product.

In the first example, a != b, and swapping increases the product.

In the third example, a != b, and swapping increases the product.

So, perhaps the rule is to swap all positions where a != b.

But in the second example, swapping when a != b doesn't change the product.

Wait, but according to my earlier calculation, swapping when a != b increases the product by (b - a)^2 * 10^{2p}, but in the second example, it didn't increase.

Wait, but in the second example, p=0, so x' * y' - x * y = (b - a)^2 * 10^{0} = (5 - 2)^2 * 1 = 9, but in reality, the product remained the same.

Wait, perhaps I made a mistake in the calculation.

Wait, no, according to the earlier calculation, x' * y' - x * y = (a - b)*10^{p} * (x - y) - (a - b)^2 * 10^{2p}

In the second example, a=2, b=5, x=2, y=5, p=0

So, (2 - 5)*1*(2 - 5) - (5 - 2)^2 * 1 = (-3)*(-3) - 9 = 9 - 9 = 0

So, the product doesn't change.

Wait, but according to the general formula, x' * y' - x * y = (a - b)*10^{p} * (x - y) - (a - b)^2 * 10^{2p}

This can be factored as (a - b)*10^{p} * (x - y - (a - b)*10^{p})

So, in the second example, (2 - 5)*1*(2 - 5 - (2 - 5)*1) = (-3)*(2 - 5 - (-3)) = (-3)* (2 - 5 + 3) = (-3)*(0) = 0

So, indeed, the product doesn't change.

But in the first example, x=73, y=31, a=3, b=1, p=0

(3 - 1)*1*(73 - 31 - (3 - 1)*1) = (2)*(42 - 2) = (2)*(40) = 80

So, the product increases by 80, which matches the sample.

In the third example, x=3516, y=3982, suppose swapping the thousands place: a=3, b=3, no change.

Hundreds place: a=5, b=9, swap a=5 < b=9, so swap.

Tens place: a=1 < b=8, swap.

Units place: a=6 > b=2, don't swap.

So, swap hundreds and tens places.

Let me calculate the product before and after.

Before swapping: 3516 * 3982 = 13994352

After swapping: x=3912, y=3586; product=3912*3586=14041392

Difference: 14041392 - 13994352 = 47040

So, the product increases by 47040.

According to the general formula, for each swap where a != b, the product increases by (b - a)^2 * 10^{2p}, minus some terms.

But in practice, it's increasing when a < b, and staying the same when a == b.

Wait, in the second example, a < b, but swapping didn't change the product.

But perhaps because it's a single-digit number, it's a special case.

Wait, perhaps for single-digit numbers, swapping doesn't change the product, but for multi-digit numbers, swapping a < b increases the product.

So, perhaps the rule is to swap digits where a < b, except for single-digit numbers.

But in the third example, swapping a=1 < b=8 increases the product.

So, perhaps the general rule is to swap digits where a < b.

