Output State: `total` is 0, `l` is `n - 3 - (n - 4)`, `r` is `n - 2 - (n - 4)`, `a` is a list of integers where `a[1] == a[2]` and `a[2] == a[3]` and so on until `a[n-4] == a[n-3]`, `le` is the length of list `a`, `st` is `-2`, `end` is `n - 3`, `ans` is `-1`.

Explanation: After each iteration of the loop, `l` is incremented by 1 and `r` is decremented by 1, while `end` is incremented by 1. The loop continues as long as `r > l`. Given that the initial values were `l = n - 3` and `r = n - 2`, after `n - 3` iterations (since `l` increases by 1 and `r` decreases by 1 with each iteration, they will meet when `l` becomes `0` and `r` becomes `-1`), `l` will be `0` and `r` will be `-1`. Therefore, `l` is `n - 3 - (n - 4)` which simplifies to `1`, and `r` is `n - 2 - (n - 4)` which simplifies to `-1`. The variable `end` will be `n - 3` after `n - 3` iterations. The other variables (`total`, `a`, `le`, `st`, `ans`) remain unchanged as per the problem statement.