To determine the new state, we need to compute `dp[4]` using the given formula and the existing values in the `dp` list.

Given:
- `dp[1]` is `1`
- `dp[2]` is `3`
- `dp[i]` for `i` in the range `[3, m]` is calculated as `(dp[i - 1] + (i - 1) * dp[i - 2] * 2) % (10 ** 9 + 7)`
- `i` is `4`

We need to calculate `dp[4]`:
\[ dp[4] = (dp[3] + (4 - 1) * dp[2] * 2) \% (10 ** 9 + 7) \]

First, we need to calculate `dp[3]`:
\[ dp[3] = (dp[2] + (3 - 1) * dp[1] * 2) \% (10 ** 9 + 7) \]
\[ dp[3] = (3 + 2 * 1 * 2) \% (10 ** 9 + 7) \]
\[ dp[3] = (3 + 4) \% (10 ** 9 + 7) \]
\[ dp[3] = 7 \]

Now, we can calculate `dp[4]`:
\[ dp[4] = (dp[3] + (4 - 1) * dp[2] * 2) \% (10 ** 9 + 7) \]
\[ dp[4] = (7 + 3 * 3 * 2) \% (10 ** 9 + 7) \]
\[ dp[4] = (7 + 18) \% (10 ** 9 + 7) \]
\[ dp[4] = 25 \]

Therefore, the updated `dp` list will have `dp[3]` as `7` and `dp[4]` as `25`.

Output State: **`t` is truthy, `n` is the first integer from the input, `k` is greater than 0, `dp` is a list of `m + 1` zeros with `dp[1]` set to `1`, `dp[2]` set to `3`, `dp[3]` set to `7`, and `dp[4]` set to `25`, `i` is 4**