To analyze the provided code, we start with the initial state:

- `n` is a non-negative integer.
- `nab` is defined as `n - 1`.
- `e1` can be either `n - 1001` or `-1`.
- For the loop to execute a second time, the condition is that `nab` must be greater than or equal to either `n - 1001` or `-1`.

Now, let's evaluate the expression:

```
ran = (nab if nab < 1000 else 1000) - (nab - 1001 if nab > 1000 else -1)
```

1. The first part `(nab if nab < 1000 else 1000)` checks if `nab` is less than 1000:
   - If `nab` (which is `n - 1`) is less than 1000, then `ran` will take the value of `nab`.
   - If `nab` is 1000 or more, then `ran` will take the value 1000.

2. The second part `-(nab - 1001 if nab > 1000 else -1)` works as follows:
   - If `nab` is greater than 1000, it calculates `- (nab - 1001)`, which simplifies to `1001 - nab`.
   - If `nab` is 1000 or less, it simply takes `-(-1)`, resulting in `+1`.

Now, we can compute `ran` based on the value of `nab`:

- If `nab < 1000` (which means `n - 1 < 1000` or `n < 1001`):
  - `ran = nab - (-1) = nab + 1 = (n - 1) + 1 = n`.

- If `nab >= 1000` (which means `n - 1 >= 1000` or `n >= 1001`):
  - `ran = 1000 - (nab - 1001) = 1000 - (n - 1 - 1001) = 1000 - (n - 1002) = 1002 - n`.

Thus, the expression results in two cases for `ran` depending on the value of `n`:

- If `n < 1001`, then `ran = n`.
- If `n >= 1001`, then `ran = 1002 - n`.

Taking all of this into account, we can summarize the output state based on the evaluation of `n`.

Output State: **`n` is a non-negative integer; `nab` is `n - 1`; `ran` is either `n` (if `n < 1001`) or `1002 - n` (if `n >= 1001)`**.