Output State: **`list` is a list of non-negative integers of length `n` (3 <= n <= 2 * 10^5), `i` is 1, `list[0]` is greater than 0, `list[1]` is `list[1] - 2 * list[0]`, `list[2]` is `list[2] - 2 * list[0]`**

Explanation:
- The initial state specifies that `list` is a list of non-negative integers of length `n` (3 <= n <= 2 * 10^5).
- `i` is 1.
- `list[0]` is greater than 0.
- `list[1]` is already `list[1] - 2 * list[0]`.
- `list[2]` is already `list[2] - list[0]`.

The code snippet `list[i + 1] -= 1 * list[i - 1]` updates `list[2]` by subtracting `list[0]` from it again. Therefore, `list[2]` becomes `list[2] - 2 * list[0]`. The other variables and conditions remain unchanged.