To determine the output, we need to carefully analyze the given initial state and the calculations leading up to the `print` statement.

### Initial State Recap:
- `t` is an input integer where \(1 \leq t \leq 10^4\).
- `i` is initialized to 2.
- `n` and `m` are the first and second integers from a new input, respectively.
- `count` is initialized to `m + 1`.
- `countmins` is initialized to `m`.
- `g` is calculated as `n / (m + 1) - m`.
- `ans` is the accumulated sum of `g / count + 1` for each iteration from `count = 2` to `count = m`.

### Calculation Breakdown:
1. **Initialization**:
   - `count` starts at `m + 1`.
   - `g` is calculated as `n / (m + 1) - m`.

2. **Accumulated Sum Calculation (`ans`)**:
   - `ans` is the sum of `g / count + 1` for each `count` from 2 to `m`.
   - This means `ans` is the sum of:
     \[
     \left(\frac{g}{2} + 1\right) + \left(\frac{g}{3} + 1\right) + \ldots + \left(\frac{g}{m} + 1\right)
     \]
   - This can be rewritten as:
     \[
     \sum_{k=2}^{m} \left(\frac{g}{k} + 1\right) = \sum_{k=2}^{m} \frac{g}{k} + \sum_{k=2}^{m} 1 = g \sum_{k=2}^{m} \frac{1}{k} + (m - 1)
     \]
   - Here, `g = n / (m + 1) - m`.

3. **Final Calculation**:
   - `ans` is computed as:
     \[
     \left(n / (m + 1) - m\right) \sum_{k=2}^{m} \frac{1}{k} + (m - 1)
     \]
   - The `print(int(ans))` statement will print the integer part of `ans`.

### Output Description:
Given the above calculations, the output will be the integer part of the accumulated sum `ans` which is calculated based on the formula above.

Output: **int(ans) (where ans is the accumulated sum of (g / count + 1) for count from 2 to m, and g is n / (m + 1) - m)**