To determine what will be printed, let's break down the code snippet and the initial state provided.

### Initial State:
1. `t` must be greater than 0 (though `t` is not used in the provided code snippet, it's part of the precondition).
2. `n` is an input integer.
3. `mat` is a list of `n` lists, where each inner list contains integers from 1 to `n`. (Note: `mat` is not used in the provided code snippet, so it's irrelevant for the output.)
4. `res` is the sum of `(i + 1) * (2 * i + 1)` for `i` from 0 to `n-1`.

### Code Snippet:
```python
print(res, n << 1)
```

### Analysis:
1. **`res` Calculation**:
   - `res` is calculated as the sum of `(i + 1) * (2 * i + 1)` for `i` from 0 to `n-1`.
   - This can be expanded as:
     \[
     \text{res} = \sum_{i=0}^{n-1} (i + 1) \cdot (2i + 1)
     \]
   - Simplifying the expression inside the sum:
     \[
     (i + 1) \cdot (2i + 1) = 2i^2 + i + 2i + 1 = 2i^2 + 3i + 1
     \]
   - Therefore:
     \[
     \text{res} = \sum_{i=0}^{n-1} (2i^2 + 3i + 1)
     \]
   - This sum can be further broken down into three separate sums:
     \[
     \text{res} = 2 \sum_{i=0}^{n-1} i^2 + 3 \sum_{i=0}^{n-1} i + \sum_{i=0}^{n-1} 1
     \]
   - Using the formulas for the sums of squares and the sum of the first `n` integers:
     \[
     \sum_{i=0}^{n-1} i^2 = \frac{(n-1)n(2n-1)}{6}
     \]
     \[
     \sum_{i=0}^{n-1} i = \frac{(n-1)n}{2}
     \]
     \[
     \sum_{i=0}^{n-1} 1 = n
     \]
   - Substituting these into the expression for `res`:
     \[
     \text{res} = 2 \left(\frac{(n-1)n(2n-1)}{6}\right) + 3 \left(\frac{(n-1)n}{2}\right) + n
     \]
     \[
     \text{res} = \frac{(n-1)n(2n-1)}{3} + \frac{3(n-1)n}{2} + n
     \]
     \[
     \text{res} = \frac{2(n-1)n(2n-1) + 9(n-1)n + 6n}{6}
     \]
     \[
     \text{res} = \frac{(n-1)n(4n-2+9) + 6n}{6}
     \]
     \[
     \text{res} = \frac{(n-1)n(4n+7) + 6n}{6}
     \]
     \[
     \text{res} = \frac{4n^3 + 7n^2 - 4n^2 - 7n + 6n}{6}
     \]
     \[
     \text{res} = \frac{4n^3 + 3n^2 - n}{6}
     \]

2. **`n << 1` Calculation**:
   - The expression `n << 1` is a bitwise left shift operation, which is equivalent to multiplying `n` by 2.
   - Therefore, `n << 1` is `2 * n`.

### Final Output:
The `print` statement will output the calculated value of `res` and the value of `n << 1` (which is `2 * n`).

Output: **res (where res is the sum of (i + 1) * (2 * i + 1) for i from 0 to n-1), 2 * n**