To determine the output state after the loop has completed all its iterations, we need to understand the behavior of the loop and compute the value of `res` based on the given formula: `res += (i + 1) * (2 * i + 1)`.

Here's a step-by-step breakdown of the computation for `res`:

1. **Initialization:**
   - `n` is the input integer.
   - `mat` is a list of lists where each sublist contains integers from 1 to `n`.
   - `res` is initialized to 0.
   - `i` is initialized to 0.

2. **Loop Execution:**
   - The loop runs for `i` from 0 to `n-1`.
   - In each iteration, `res` is updated by adding `(i + 1) * (2 * i + 1)`.

Let's compute `res` for a general `n` using the formula.

For each iteration `i`, the value added to `res` is:
\[ \text{value added} = (i + 1) \times (2i + 1) \]

We need to sum this value for all `i` from 0 to `n-1`.

\[ \text{res} = \sum_{i=0}^{n-1} (i + 1) \times (2i + 1) \]

Expanding the expression inside the summation:
\[ (i + 1) \times (2i + 1) = 2i^2 + 3i + 1 \]

So,
\[ \text{res} = \sum_{i=0}^{n-1} (2i^2 + 3i + 1) \]

This can be broken down into three separate summations:
\[ \text{res} = 2 \sum_{i=0}^{n-1} i^2 + 3 \sum_{i=0}^{n-1} i + \sum_{i=0}^{n-1} 1 \]

Using the formulas for the summations of squares and integers:
\[ \sum_{i=0}^{n-1} i^2 = \frac{(n-1)n(2n-1)}{6} \]
\[ \sum_{i=0}^{n-1} i = \frac{(n-1)n}{2} \]
\[ \sum_{i=0}^{n-1} 1 = n \]

Substituting these into the expression for `res`:
\[ \text{res} = 2 \left( \frac{(n-1)n(2n-1)}{6} \right) + 3 \left( \frac{(n-1)n}{2} \right) + n \]
\[ \text{res} = \frac{(n-1)n(2n-1)}{3} + \frac{3(n-1)n}{2} + n \]

Combining these terms:
\[ \text{res} = \frac{2(n-1)n(2n-1) + 9(n-1)n + 6n}{6} \]
\[ \text{res} = \frac{(n-1)n(4n-2 + 9) + 6n}{6} \]
\[ \text{res} = \frac{(n-1)n(4n + 7) + 6n}{6} \]
\[ \text{res} = \frac{4n^3 + 7n^2 - 4n^2 - 7n + 6n}{6} \]
\[ \text{res} = \frac{4n^3 + 3n^2 - n}{6} \]
\[ \text{res} = \frac{n(4n^2 + 3n - 1)}{6} \]

Given the pattern from the first few iterations, we can confirm this formula is correct.

Finally, after the loop completes all `n` iterations, the output state is:

Output State: **`n` is the input integer, `mat` is a list of lists where each sublist contains integers from 1 to `n`, `res` is \(\frac{n(4n^2 + 3n - 1)}{6}\), and `i` is \(n-1\)**

In natural language: After all iterations, `res` holds the value \(\frac{n(4n^2 + 3n - 1)}{6}\), `i` is \(n-1\), and `mat` remains unchanged as a list of lists where each sublist contains integers from 1 to `n`.