To determine the output state, let's analyze the given code snippet:

```python
b += b[-2] + v ** (v > x - w), b[-1] + v ** (v > z - y)
```

Here's what happens step-by-step:
- `b` initially contains `[0, 0]`.
- The expression `b[-2]` refers to the second-to-last element of `b`, which is `0`.
- The expression `b[-1]` refers to the last element of `b`, which is also `0`.
- The expression `v ** (v > x - w)` evaluates to `v` if `v > x - w`, otherwise it evaluates to `1`. Since the exact values of `v`, `x`, and `w` are not specified, we'll keep this expression as is.
- Similarly, the expression `v ** (v > z - y)` evaluates to `v` if `v > z - y`, otherwise it evaluates to `1`.

So, the new elements being added to `b` are:
- `b[-2] + v ** (v > x - w) = 0 + v ** (v > x - w)`
- `b[-1] + v ** (v > z - y) = 0 + v ** (v > z - y)`

Thus, the new `b` will be `[0, 0, v ** (v > x - w), v ** (v > z - y)]`.

Given the initial conditions and the transformations, the updated state is:

Output State: **`t` is an integer read from input such that 0 ≤ t ≤ 10^4; `n` is an integer such that 2 ≤ n ≤ 10^5; `a` is a list of `n+2` integers where -1000000000.0 ≤ a_1 < a_2 < ... < a_n ≤ 2000000000.0; `m` is an integer such that 1 ≤ m ≤ 10^5; `r` is a lambda function that reads a line of input, splits it into components, and maps each component to an integer; `b` is a list containing [0, 0, v ** (v > x - w), v ** (v > z - y)]; `v` is `y - x`.**