The code snippet modifies the value of `s` by adding `s // (k - 1) + 1` to it. The values of `k`, `x`, and `a` are not altered by this code snippet. The initial state of `s` is 3, and `i` remains unchanged at 2.

Given the initial state, the new value of `s` can be calculated as:
\[ s = 3 + \left(\frac{3}{k - 1}\right) + 1 \]
\[ s = 4 + \left(\frac{3}{k - 1}\right) \]

Since `k` is an integer between 2 and 30, the value of `s` will vary based on `k`. However, the expression for `s` remains as calculated.

Output State: **`k`, `x`, and `a` are integers read from the input with the constraints 2 ≤ k ≤ 30, 1 ≤ x ≤ 100, and 1 ≤ a ≤ 10^9; `s` is 4 + (3 / (k - 1)); `i` is 2**.