To determine what will be printed, let's break down the initial state and the conditions for `res`.

Given:
- `a > 0`
- `i = 2`
- `x1` and `y1` are input integers
- `x2` and `y2` are the first and second integers from the input split
- `x3` and `y3` are the first and second integers from the input split
- `x4` and `y4` are the third and fourth integers from the input split

The value of `res` depends on several conditions:

1. If `x1 == x3` and `x2 == x4` and `y1 < y3`, then `res` is the absolute difference between `y3` and `y1`.
2. If `x1 == x3` and `x2 == x4` and `y1 >= y3`, then `res` is the absolute difference between `y1` and `y3`.
3. If `x1 == x2` and `x3 == x4`, then `res` is the absolute difference between `y1` and `y2` if `y1 < y2`, otherwise `res` is the absolute difference between `y2` and `y1`.
4. If `x1 == x4` and `x3 == x2`, then `res` is the absolute difference between `y1` and `y2` if `y1 < y2`, otherwise `res` is the absolute difference between `y2` and `y1`.

Since the exact values of `x1, y1, x2, y2, x3, y3, x4, y4` are not provided, we need to consider the possible outcomes based on the conditions. However, the key point is that `res` will always be the absolute difference between two specific `y` values under one of the conditions.

Let's assume the following for simplicity (since the exact values are not given):
- `x1 == x3` and `x2 == x4` and `y1 < y3`

In this case:
- `res` would be `abs(y3 - y1)`

When we square `res`, we get:
- `res ** 2` would be `(abs(y3 - y1)) ** 2`

Therefore, the output will be the squared absolute difference between `y3` and `y1`.

Output: **(abs(y3 - y1)) ** 2**