To determine the output of the `print(p1 - cur + p3)` statement, we need to analyze the given initial state and conditions step by step.

### Initial State Recap:
- `t` is an integer greater than or equal to 1.
- `p1`, `p2`, and `p3` are integers such that \(0 \leq p1 \leq p2 \leq p3 \leq 30\).
- The sum of `p1`, `p2`, and `p3` is odd.
- `p3` is less than the sum of `p1` and `p2` (\(p3 < p1 + p2\)).
- `low` is defined as `p3 - p2`.
- `high` is defined as `p3 - p1` and must be at least `cur`.
- `cur` is determined by the condition:
  - If `p1 - cur` is less than or equal to `p2 - (p3 - cur)`, then `cur` remains `low`.
  - Otherwise, `cur` is `low + 1` and `p1 - cur` is greater than `p2 - (p3 - cur)`.

### Step-by-Step Analysis:
1. **Determine `low` and `high`:**
   - `low = p3 - p2`
   - `high = p3 - p1`

2. **Determine `cur`:**
   - The condition for `cur` is based on the comparison `p1 - cur` and `p2 - (p3 - cur)`:
     - If `p1 - cur <= p2 - (p3 - cur)`, then `cur = low`.
     - Otherwise, `cur = low + 1`.

3. **Expression to Evaluate:**
   - We need to evaluate `p1 - cur + p3`.

### Simplifying the Expression:
- Let's rewrite the expression `p1 - cur + p3`:
  - If `cur = low` (i.e., `p1 - low <= p2 - (p3 - low)`):
    - `p1 - cur + p3 = p1 - (p3 - p2) + p3 = p1 - p3 + p2 + p3 = p1 + p2`.
  - If `cur = low + 1` (i.e., `p1 - (low + 1) > p2 - (p3 - (low + 1))`):
    - `p1 - cur + p3 = p1 - (p3 - p2 + 1) + p3 = p1 - p3 + p2 + p3 - 1 = p1 + p2 - 1`.

### Conclusion:
Given the conditions, the expression `p1 - cur + p3` simplifies to either `p1 + p2` or `p1 + p2 - 1`. However, we need to ensure that `p1 + p2` is odd because the sum of `p1`, `p2`, and `p3` is odd and `p3` is less than `p1 + p2`.

Since `p1 + p2` must be even (because `p1 + p2 + p3` is odd and `p3` is an integer), the only valid expression is `p1 + p2 - 1` to maintain the odd sum condition.

### Final Output:
Output: **p1 + p2 - 1 (where p1, p2, and p3 are integers such that 0 ≤ p1 ≤ p2 ≤ p3 ≤ 30, the sum of p1, p2, and p3 is odd, and p3 < p1 + p2)**