Let's break down the given initial state and the code to determine what will be printed by the `print` statement.

### Initial State:
- `t`: An integer greater than or equal to 2.
- `p1`, `p2`, and `p3`: Integers read from the input such that \(0 \leq p1 \leq p2 \leq p3 \leq 30\).
- The sum of `p1`, `p2`, and `p3` is odd.
- `low`: The minimum of `p3 - p1` and `p3 - p2`.
- `high`: The maximum of `p3 - p1` and `p3 - p2`, with the condition that `high` must be at least `low + 1`.
- `cur`: Initially set based on the condition:
  - If `p1 - cur <= p2 - (p3 - cur)`, `cur` remains `low`.
  - Otherwise, `cur` is updated to `low + 1`.

### Code to Analyze:
```
print(p1 - cur + p3)
```

### Step-by-Step Analysis:
1. **Determine `low` and `high`**:
   - `low = min(p3 - p1, p3 - p2)`
   - `high = max(p3 - p1, p3 - p2)`

2. **Determine `cur`**:
   - The condition `p1 - cur <= p2 - (p3 - cur)` simplifies to:
     \[
     p1 - cur \leq p2 - p3 + cur \implies p1 + p3 \leq p2 + 2 \cdot cur \implies cur \geq \frac{p1 + p3 - p2}{2}
     \]
   - If the above inequality holds, `cur` is set to `low`.
   - Otherwise, `cur` is set to `low + 1`.

3. **Evaluate the Print Statement**:
   - The expression `p1 - cur + p3` is what gets printed.
   - Given the value of `cur` depends on the condition, let's consider both cases:
     - **Case 1**: If `cur = low`, then the expression becomes:
       \[
       p1 - low + p3
       \]
     - **Case 2**: If `cur = low + 1`, then the expression becomes:
       \[
       p1 - (low + 1) + p3 = p1 - low + p3 - 1
       \]

### Output Description:
The printed value depends on whether `cur` is `low` or `low + 1`.

- If `cur = low`, the output is `p1 - low + p3`.
- If `cur = low + 1`, the output is `p1 - low + p3 - 1`.

Since `low` is defined as `min(p3 - p1, p3 - p2)`, we can express the final output in terms of `p1`, `p2`, and `p3`.

### Final Output:
Output: **p1 - low + p3 (where low is min(p3 - p1, p3 - p2) and cur is either low or low + 1 depending on the condition p1 - cur <= p2 - (p3 - cur))**