To determine the output state, we need to understand how the loop modifies the variables `tem` and `ans` based on the initial state of `arr`.

Given:
- `arr` is a list of integers.
- `ans` is an empty list.
- `tem` is initialized to 1.

The loop iterates over the indices of `arr` in reverse order (from the last index to the first index). In each iteration:
- `tem` is multiplied by the current element of `arr`.
- The updated value of `tem` is appended to `ans`.

Let's illustrate this with an example. Suppose `arr = [2, 3, 4]`.

1. **Initial State:**
   - `arr = [2, 3, 4]`
   - `ans = []`
   - `tem = 1`

2. **First Iteration (i = 2):**
   - `tem = tem * arr[2] = 1 * 4 = 4`
   - `ans = [4]`

3. **Second Iteration (i = 1):**
   - `tem = tem * arr[1] = 4 * 3 = 12`
   - `ans = [4, 12]`

4. **Third Iteration (i = 0):**
   - `tem = tem * arr[0] = 12 * 2 = 24`
   - `ans = [4, 12, 24]`

After the loop completes, the final state is:
- `arr` remains `[2, 3, 4]` (unchanged).
- `ans` is `[4, 12, 24]`.
- `tem` is `24`.

In general, the `ans` list will contain the cumulative products of the elements of `arr` in reverse order, starting from the last element of `arr` to the first element.

Output State: **arr is a list of integers; ans is a list of cumulative products of arr in reverse order; tem is the product of all elements in arr.**