In the given code snippet, `numerator` is updated by multiplying it with `total_days - i`. 

- `total_days` is equal to \(2^n\).
- `i` is equal to 2.
- Thus, the expression `total_days - i` becomes \(2^n - 2\).

Now, let's update the `numerator`:

- The previous value of `numerator` is \(2^n \times (2^n - 1)\).
- Therefore, after executing the statement `numerator *= total_days - i`, we have:
  
\[
numerator = numerator \times (total_days - i) = (2^n \times (2^n - 1)) \times (2^n - 2)
\]

The other variables remain unaffected by this operation.

Output State: **`n` is an integer such that 1 ≤ `n` ≤ 10^18; `k` is an integer such that 3 ≤ `k` ≤ 10^18; `total_days` is equal to \(2^n\); `numerator` is equal to \(2^n \times (2^n - 1) \times (2^n - 2)\); `denominator` is equal to \(2^{2n}\); `i` is 2.**