To determine the output of the `print(p1 - cur + p3)` statement, let's break down the given initial state and the variables involved:

1. **Variables and Conditions:**
   - `p1`, `p2`, and `p3` are integers.
   - The sum of `p1`, `p2`, and `p3` is odd.
   - `p3` is less than `p1 + p2`.
   - `low` is the minimum of `p3 - p1` and `p3 - p2`.
   - `high` is the maximum of `p3 - p1` and `p3 - p2`.
   - `cur` is either `low` or `low + 1`.
   - `high` must be at least `cur`.

2. **Understanding `low` and `high`:**
   - `low` is the smaller of the two differences `p3 - p1` and `p3 - p2`.
   - `high` is the larger of the two differences `p3 - p1` and `p3 - p2`.

3. **Understanding `cur`:**
   - `cur` can be either `low` or `low + 1`.
   - Since `high` must be at least `cur`, `cur` cannot be greater than `high`.

4. **Expression to Evaluate:**
   - The expression to be printed is `p1 - cur + p3`.

Given the conditions, let's determine the value of `cur`:
- If `p3 < p1 + p2`, then both `p3 - p1` and `p3 - p2` can be negative, zero, or positive.
- `low` will be the smaller of these two differences.
- `cur` will be either `low` or `low + 1`.

To understand the specific value of `p1 - cur + p3`, let's consider the possible scenarios for `cur`:

- **Scenario 1:** `cur = low`
  - In this case, the expression becomes `p1 - low + p3`.
  - Since `low` is the minimum of `p3 - p1` and `p3 - p2`, the expression simplifies to:
    - If `low = p3 - p1`, then `p1 - low + p3 = p1 - (p3 - p1) + p3 = p1 - p3 + p1 + p3 = 2 * p1`.
    - If `low = p3 - p2`, then `p1 - low + p3 = p1 - (p3 - p2) + p3 = p1 - p3 + p2 + p3 = p1 + p2`.

- **Scenario 2:** `cur = low + 1`
  - In this case, the expression becomes `p1 - (low + 1) + p3`.
  - Simplifying, we get:
    - If `low = p3 - p1`, then `p1 - (low + 1) + p3 = p1 - (p3 - p1 + 1) + p3 = p1 - p3 + p1 - 1 + p3 = 2 * p1 - 1`.
    - If `low = p3 - p2`, then `p1 - (low + 1) + p3 = p1 - (p3 - p2 + 1) + p3 = p1 - p3 + p2 - 1 + p3 = p1 + p2 - 1`.

Given the constraints and the need for the sum `p1 + p2 + p3` to be odd, the most precise and general answer is based on the possible values of `cur`:

Output: **p1 - cur + p3 (where cur is either the minimum of p3 - p1 and p3 - p2, or one more than that minimum)**