Given the initial state where:
- `W` is a positive integer such that \(1 \leq W \leq 100000\),
- `a` is an integer such that \(1 \leq a \leq 100000\),
- `c` is assigned a value from `raw_input`,
- `b` is updated to \(a + W\),
- `d` is assigned the value of \(c + W\),
- `b` is greater than or equal to `c`,
- `d` is less than `a`.

Now, analyzing the code:
```
ans = a - d
```
Here, `d` is calculated as \(c + W\), therefore `ans` becomes \(a - (c + W)\).

From the conditions provided:
- Since \(d < a\), we can derive that \(c + W < a\).
- This means \(a - d = a - (c + W)\) will certainly yield a positive result since \(a\) is greater than \(c + W\).

Thus, the output state based on these calculations is:
- `W` is a positive integer where \(1 \leq W \leq 100000\),
- `a` is an integer where \(1 \leq a \leq 100000\),
- `c` is the input value,
- `b` is \(a + W\),
- `d` is \(c + W\),
- `b` is greater than or equal to `c`,
- `d` is less than `a`,
- `ans` is calculated as \(a - d\).

Output State: **`W` is a positive integer such that 1 ≤ `W` ≤ 100000, `a` is an integer such that 1 ≤ `a` ≤ 100000, `c` is the input value, `b` is `a + W`, `d` is `c + W`, `b` is greater than or equal to `c`, `d` is less than `a`, `ans` is `a - d`.**