Let's break down the initial state and the code step by step:

1. **Initial State**:
   - `t` is a positive integer such that \(1 \leq t \leq 10^4\).
   - `n` is the first integer input split from `t`.
   - `m` is the second integer input split from `t`.
   - `k` is the absolute difference between `n` and `m`: \( k = |n - m| \).
   - `l` is the binary string representation of `k` without the '0b' prefix.
   - `p` is the length of `l`.
   - `q` is \(2^{(p - 1)}\).

2. **Code Snippet**:
   ```python
   print(k - q)
   ```

3. **Determine Values**:
   - Since `k` is the absolute difference between `n` and `m`, it can be any non-negative integer.
   - `l` is the binary string representation of `k` without the '0b' prefix. For example, if `k = 5`, then `l = "101"`.
   - `p` is the length of `l`. If `k = 5`, then `p = 3`.
   - `q` is \(2^{(p - 1)}\). If `p = 3`, then \(q = 2^{(3 - 1)} = 2^2 = 4\).

4. **Final Calculation**:
   - The expression `k - q` will be evaluated as `k - 2^(p - 1)`.
   - Given that `p` is the length of the binary string `l`, and `q` is \(2^{(p - 1)}\), the value of `k - q` will depend on the specific values of `n` and `m`.

Since the exact values of `n` and `m` are not provided, we can express the final result in terms of `k` and `q`:
- `k` is the absolute difference between `n` and `m`.
- `q` is \(2^{(p - 1)}\), where `p` is the length of the binary string representation of `k`.

Therefore, the output will be:
Output: **k - 2^(p - 1)**