Let's break down the initial state and the code snippet step by step:

1. **Initial State:**
   - `i` is `m`
   - `k` is equal to `m`
   - `s` is `m * (c * i * c * m + c * a)`

2. **Code Snippet:**
   ```python
   print(s % M)
   ```

From the initial state:
- `i = m`
- `k = m`
- `s = m * (c * i * c * m + c * a)`

Substituting `i = m` into the expression for `s`:
\[ s = m \times (c \times m \times c \times m + c \times a) \]
\[ s = m \times (c^2 \times m^2 + c \times a) \]
\[ s = m \times c^2 \times m^2 + m \times c \times a \]
\[ s = m^3 \times c^2 + m \times c \times a \]

So, `s` is expressed as:
\[ s = m^3 \times c^2 + m \times c \times a \]

The code snippet `print(s % M)` will print the result of `s` modulo `M`.

Therefore, the output will be:
Output: **(m^3 * c^2 + m * c * a) % M**