The value of `ans` is updated to the value of `t`. The calculation for `t` depends on whether `b % 2 == 0` or `b % 2 == 1`.

- If `b % 2 == 0`, then `t` is calculated as `a * a - 2 * (b // 2) * (b // 2)`.
- If `b % 2 == 1`, then `t` is calculated as `a * a - (b // 2 + 1) * (b // 2 + 1) - (b // 2) * (b // 2)`.

Since the current value of `ans` is less than `t`, `ans` will be updated to `t`.

Output State: **`a` and `b` are non-negative integers such that 0 ≤ a, b ≤ 105 and a + b ≥ 1, both `a` and `b` are non-zero, `ans` is `a * a - 2 * (b // 2) * (b // 2)` if `b % 2 == 0` or `a * a - (b // 2 + 1) * (b // 2 + 1) - (b // 2) * (b // 2)` if `b % 2 == 1`, `v` is 0, `i` is 1, `x` is `b // 2`, `y` is `b % 2`, `t` is `a * a - 2 * (b // 2) * (b // 2)` if `b % 2 == 0` or `a * a - (b // 2 + 1) * (b // 2 + 1) - (b // 2) * (b // 2)` if `b % 2 == 1`.**