To determine the output state, let's analyze the given code snippet step by step:

### Initial State:
- `a` and `b` are non-negative integers such that 0 ≤ a, b ≤ 105 and a + b ≥ 1, both `a` and `b` are non-zero.
- `ans` is -10000000000000000000.
- `v` is 1.
- `i` is 2.
- `x` is `b // 3`.
- `y` is `b % 3`.
- `a` is ≥ 2.

### Code Snippet:
```python
t = i - 1 + (a - i + 1) * (a - i + 1) - y * (x + 1) * (x + 1) - (i + 1 - y) * x * x
```

### Step-by-Step Analysis:
1. **Calculate `i - 1`**:
   - `i` is 2.
   - `i - 1` is `2 - 1` which equals `1`.

2. **Calculate `(a - i + 1) * (a - i + 1)`**:
   - `i` is 2.
   - `a - i + 1` is `a - 2 + 1` which simplifies to `a - 1`.
   - `(a - 1) * (a - 1)` is `(a - 1)^2`.

3. **Calculate `y * (x + 1) * (x + 1)`**:
   - `y` is `b % 3`.
   - `x` is `b // 3`.
   - `x + 1` is `b // 3 + 1`.
   - `(x + 1) * (x + 1)` is `(b // 3 + 1)^2`.
   - `y * (x + 1) * (x + 1)` is `y * (b // 3 + 1)^2`.

4. **Calculate `(i + 1 - y) * x * x`**:
   - `i` is 2.
   - `i + 1` is `2 + 1` which equals `3`.
   - `i + 1 - y` is `3 - y`.
   - `x` is `b // 3`.
   - `x * x` is `(b // 3)^2`.
   - `(i + 1 - y) * x * x` is `(3 - y) * (b // 3)^2`.

5. **Combine all parts to form `t`**:
   - `t = 1 + (a - 1)^2 - y * (b // 3 + 1)^2 - (3 - y) * (b // 3)^2`.

### Final Calculation:
- `t = 1 + (a - 1)^2 - y * (b // 3 + 1)^2 - (3 - y) * (b // 3)^2`.

### Output State:
- `a` and `b` are non-negative integers such that 0 ≤ a, b ≤ 105 and a + b ≥ 1, both `a` and `b` are non-zero.
- `ans` is -10000000000000000000.
- `v` is 1.
- `i` is 2.
- `x` is `b // 3`.
- `y` is `b % 3`.
- `a` is ≥ 2.
- `t` is `1 + (a - 1)^2 - y * (b // 3 + 1)^2 - (3 - y) * (b // 3)^2`.

Output State: **`a` and `b` are non-negative integers such that 0 ≤ a, b ≤ 105 and a + b ≥ 1, both `a` and `b` are non-zero, `ans` is -10000000000000000000, `v` is 1, `i` is 2, `x` is `b // 3`, `y` is `b % 3`, `a` is ≥ 2, `t` is `1 + (a - 1)^2 - y * (b // 3 + 1)^2 - (3 - y) * (b // 3)^2`.**