The value of `ans` is updated to the value of `t`. The value of `t` is calculated as `1 + (a - 1)^2 - y * (b // 3 + 1)^2 - (3 - y) * (b // 3)^2`. The other variables remain unchanged.

Output State: **`a` and `b` are non-negative integers such that 0 ≤ a, b ≤ 105 and a + b ≥ 1, both `a` and `b` are non-zero, `ans` is `1 + (a - 1)^2 - y * (b // 3 + 1)^2 - (3 - y) * (b // 3)^2`, `v` is 1, `i` is 2, `x` is `b // 3`, `y` is `b % 3`, `a` is ≥ 2, `t` is `1 + (a - 1)^2 - y * (b // 3 + 1)^2 - (3 - y) * (b // 3)^2`.**