The provided code snippet updates the value of `t` based on the current values of `a`, `b`, `i`, `x`, and `y`. Let's break down the calculation step by step:

1. **Initial Values:**
   - `a` and `b` are non-negative integers such that \(0 \leq a, b \leq 105\) and \(a + b \geq 1\).
   - Both `a` and `b` are non-zero.
   - `v` is 1.
   - `i` is 3.
   - `x` is \(b // 4\).
   - `y` is \(b \% 4\).
   - `a` is \(\geq 2\).
   - `t` is \(1 + (a - 1)^2 - y \cdot (b // 3 + 1)^2 - (3 - y) \cdot (b // 3)^2\).
   - `ans` is \(-10000000000000000000\) if `ans` < `t`, otherwise `ans` remains \(-10000000000000000000\) and `v` remains 1.

2. **New Calculation for `t`:**
   - `t = i - 1 + (a - i + 1) * (a - i + 1) - y * (x + 1) * (x + 1) - (i + 1 - y) * x * x`
   - Substituting the known values:
     - `i` is 3.
     - `i - 1` is 2.
     - `a - i + 1` is \(a - 3 + 1 = a - 2\).
     - \((a - i + 1) * (a - i + 1)\) is \((a - 2) * (a - 2) = (a - 2)^2\).
     - `y * (x + 1) * (x + 1)` is \(y * (x + 1)^2\).
     - \((i + 1 - y) * x * x\) is \((3 + 1 - y) * x^2 = (4 - y) * x^2\).

   Therefore, the new value of `t` is:
   \[
   t = 2 + (a - 2)^2 - y * (x + 1)^2 - (4 - y) * x^2
   \]

3. **Update the Output State:**
   - The values of `a`, `b`, `v`, `i`, `x`, and `y` remain unchanged.
   - The new value of `t` is calculated as above.
   - `ans` remains \(-10000000000000000000\) because the condition `ans < t` is not checked in this snippet.

Output State: **`a` and `b` are non-negative integers such that \(0 \leq a, b \leq 105\) and \(a + b \geq 1\), both `a` and `b` are non-zero, `v` is 1, `i` is 3, `x` is \(b // 4\), `y` is \(b \% 4\), `a` is \(\geq 2\), `t` is \(2 + (a - 2)^2 - y * (x + 1)^2 - (4 - y) * x^2\), `ans` is \(-10000000000000000000\)**.