### Reasoning:

1. **Problem Understanding:**
   - The task is to find the number of ordered pairs \((a, b)\) such that:
     - \(1 \le a \le n\)
     - \(1 \le b \le m\)
     - \(a + b\) is a multiple of \(b \cdot \gcd(a, b)\).

2. **Key Insight:**
   - The condition \(a + b\) being a multiple of \(b \cdot \gcd(a, b)\) can be rewritten using the property of gcd. If \(d = \gcd(a, b)\), then \(a = d \cdot a'\) and \(b = d \cdot b'\) where \(\gcd(a', b') = 1\).
   - Substituting these into the condition, we get:
     \[
     d \cdot a' + d \cdot b' = d \cdot (a' + b')
     \]
     This must be a multiple of \(b \cdot d = d^2 \cdot b'\).
   - Simplifying, we get:
     \[
     a' + b' \text{ must be a multiple of } b'
     \]
   - Since \(\gcd(a', b') = 1\), \(a' + b'\) must be a multiple of \(b'\). This implies \(a' \equiv 0 \pmod{b'}\), which means \(a'\) must be a multiple of \(b'\).

3. **Algorithm Analysis:**
   - The program iterates over all possible values of \(b\) from 1 to \(m\).
   - For each \(b\), it calculates the number of valid \(a\) values using the formula:
     \[
     x = \left\lfloor \frac{a - i \cdot (i - 1)}{i^2} \right\rfloor + 1
     \]
   - This formula is derived from the condition \(a + b\) being a multiple of \(b \cdot \gcd(a, b)\). However, it does not correctly account for the gcd condition and the multiple condition.

4. **Issues in the Program:**
   - The formula used to calculate \(x\) is not correct. It should be based on the gcd and the multiple condition.
   - The additional check:
     \[
     \text{if } (a - i \cdot (i - 1)) \% i^2 == 0 \text{ and } i \cdot (i - 1) \% i^2 == 0:
     \]
     This check is also incorrect and unnecessary. It does not align with the problem's requirements.
   - The final result is calculated as `suma - 2`, which is not justified and seems arbitrary.

5. **Correct Approach:**
   - For each \(b\), we need to count the number of \(a\) such that \(a + b\) is a multiple of \(b \cdot \gcd(a, b)\).
   - This can be done by iterating over all possible \(a\) and checking the condition directly. Specifically, for each \(b\), we need to find all \(a\) such that:
     \[
     a + b \equiv 0 \pmod{b \cdot \gcd(a, b)}
     \]
   - This can be simplified to:
     \[
     a \equiv -b \pmod{b \cdot \gcd(a, b)}
     \]
   - We can use the fact that \(\gcd(a, b)\) must divide \(b\) and \(a\), and thus \(a\) must be of the form \(k \cdot \gcd(a, b)\) for some integer \(k\).

6. **Conclusion:**
   - The given program does not correctly implement the logic to solve the problem. The formula and the additional checks are flawed and do not align with the problem's requirements.

### Final Evaluation:
Final: **False**