The code snippet `ans[-1] = ans[-2] + arr[-1]` updates the last element of the list `ans` to be the sum of the second-to-last element of `ans` and the last element of `arr`.

Initial State:
- `ans` is a list of `n` integers where `ans[0] = arr[0] + 1`, and for each `1 <= i < n`, `ans[i]` is the smallest integer such that `ans[i] >= arr[i]` and `ans[i]` is a multiple of `ans[i-1]`.

After executing the code:
- The last element of `ans` is updated to `ans[-2] + arr[-1]`.

Output State: **`ans` is a list of `n` integers where `ans[0] = arr[0] + 1`, and for each `1 <= i < n-1`, `ans[i]` is the smallest integer such that `ans[i] >= arr[i]` and `ans[i]` is a multiple of `ans[i-1]`. The last element `ans[-1]` is now equal to `ans[-2] + arr[-1]`.**