Reasoning:

1. **Problem Understanding**:
   - The problem requires maximizing the sum of all elements in an \( n \times n \) matrix using at most \( 2n \) operations.
   - The operations involve setting a row or a column to a permutation of integers from 1 to \( n \).

2. **Solution Analysis**:
   - The program initializes the sum to 1 and then iterates from 2 to \( n \) to calculate the sum using the formula \( \sum_{i=2}^{n} (i^2 - (i-1)^2) \cdot i \).
   - This formula is derived from the sum of the first \( n \) natural numbers squared, which is \( \sum_{i=1}^{n} i^2 = \frac{n(n+1)(2n+1)}{6} \). However, the formula used in the program is not directly derived from this, and it seems to be a specific calculation for the problem.
   - The program then prints the sum and \( 2n \) operations.
   - For each row \( j \) from 1 to \( n \), it prints two operations: one for the row and one for the column, both using the same permutation \( [1, 2, \ldots, n] \).

3. **Correctness of the Sum Calculation**:
   - The sum calculation in the program is \( 1 + \sum_{i=2}^{n} (i^2 - (i-1)^2) \cdot i \).
   - Simplifying \( i^2 - (i-1)^2 \):
     \[
     i^2 - (i-1)^2 = i^2 - (i^2 - 2i + 1) = 2i - 1
     \]
   - Therefore, the sum becomes:
     \[
     1 + \sum_{i=2}^{n} (2i - 1) \cdot i = 1 + \sum_{i=2}^{n} (2i^2 - i)
     \]
   - This can be further simplified to:
     \[
     1 + 2 \sum_{i=2}^{n} i^2 - \sum_{i=2}^{n} i
     \]
   - The sum of squares from 2 to \( n \) is:
     \[
     \sum_{i=2}^{n} i^2 = \sum_{i=1}^{n} i^2 - 1^2 = \frac{n(n+1)(2n+1)}{6} - 1
     \]
   - The sum of integers from 2 to \( n \) is:
     \[
     \sum_{i=2}^{n} i = \sum_{i=1}^{n} i - 1 = \frac{n(n+1)}{2} - 1
     \]
   - Substituting these into the sum formula:
     \[
     1 + 2 \left( \frac{n(n+1)(2n+1)}{6} - 1 \right) - \left( \frac{n(n+1)}{2} - 1 \right)
     \]
     \[
     = 1 + \frac{n(n+1)(2n+1)}{3} - 2 - \frac{n(n+1)}{2} + 1
     \]
     \[
     = \frac{n(n+1)(2n+1)}{3} - \frac{n(n+1)}{2}
     \]
     \[
     = \frac{2n(n+1)(2n+1) - 3n(n+1)}{6}
     \]
     \[
     = \frac{n(n+1)(4n + 2 - 3)}{6}
     \]
     \[
     = \frac{n(n+1)(4n - 1)}{6}
     \]
   - This formula matches the sum of all elements in the matrix when each row and each column is set to the permutation \( [1, 2, \ldots, n] \).

4. **Correctness of the Operations**:
   - The program prints \( 2n \) operations, which is within the allowed limit.
   - Each operation sets a row or a column to the permutation \( [1, 2, \ldots, n] \).
   - This ensures that each element in the matrix is set to a value from 1 to \( n \), and the sum of all elements is maximized.

5. **Edge Cases**:
   - For \( n = 1 \), the sum is 1, and the program correctly prints 1 operation.
   - For \( n = 2 \), the sum is 7, and the program correctly prints 4 operations.

Given the above reasoning, the program correctly calculates the maximum sum and provides a valid sequence of operations to achieve it.

Correctness: **True**