Postcondition: ***`n` is a non-negative integer such that \(1 \leq n \leq 10^9\), `a` is a non-negative integer such that \(1 \leq a \leq 10^9\), `b` is a non-negative integer such that \(1 \leq b \leq 10^9\), `c` is a non-negative integer such that \(1 \leq c \leq 10^9\), `k = 4 - n \% 4` must be at least 1, `ans` is \(3 * i * c + j * b + (k - 3 * i - 2 * j) * a\) where \(i\) and \(j\) are integers and \(j = (4 - n \% 4 - 3 * i) // 2\). If \(3 * i + 2 * j \leq k\), then `ans` is set to \(3 * i * c + j * b + (k - 3 * i - 2 * j) * a`. Otherwise, the value of `ans` remains unchanged.***