`j` is assigned the value of `(k - 3 * i) // 2`. The value of `i` is updated to `i_prev + 1` but the exact value of `i_prev` is not given. Therefore, the value of `i` is `i_prev + 1`. The other variables remain unchanged.

Output State: **`n` is a non-negative integer such that \(1 \leq n \leq 10^9\), `a` is a non-negative integer such that \(1 \leq a \leq 10^9\), `b` is a non-negative integer such that \(1 \leq b \leq 10^9\), `c` is a non-negative integer such that \(1 \leq c \leq 10^9\), `k` is at least 1, `i` is `i_prev + 1`, `j` is \((k - 3 * (i_prev + 1)) // 2**