The given code snippet updates the variable `ans` with the minimum value between its current value and a new value calculated using the formula `3 * i * c + j * b + (k - 3 * i - 2 * j) * a`. However, the initial values of `i` and `j` are defined in terms of `i_prev` and `k`:

- `i = i_prev + 1`
- `j = (k - 3 * (i_prev + 1)) // 2`

Since these values are not provided initially, we cannot determine the exact values of `i` and `j`. But we know they are derived from `i_prev` and `k`.

The other variables (`n`, `a`, `b`, `c`, `k`) remain unchanged.

Therefore, the output state will include the updated values of `i` and `j` in terms of `i_prev` and `k`, and the updated formula for `ans`.

Output State: **`i` is `i_prev + 1`, `j` is \((k - 3 * (i_prev + 1)) // 2\), `ans` is updated to be the minimum of its current value and the expression `3 * (i_prev + 1) * c + ((k - 3 * (i_prev + 1)) // 2) * b + (k - 3 * (i_prev + 1) - 2 * ((k - 3 * (i_prev + 1)) // 2)) * a`, `n` is a non-negative integer such that \(1 \leq n \leq 10^9\), `a` is a non-negative integer such that \(1 \leq a \leq 10^9\), `b` is a non-negative integer such that \(1 \leq b \leq 10^9\), `c` is a non-negative integer such that \(1 \leq c \leq 10^9\), `k` is at least 1.**