Postcondition: **`i` is `i_prev + 1`, `j` is \((k - 3 * (i_prev + 1)) // 2\), `ans` is updated to be the minimum of its current value and the expression `3 * (i_prev + 1) * c + ((k - 3 * (i_prev + 1)) // 2) * b + (k - 3 * (i_prev + 1) - 2 * ((k - 3 * (i_prev + 1)) // 2)) * a`, `n` is a non-negative integer such that \(1 \leq n \leq 10^9\), `a` is a non-negative integer such that \(1 \leq a \leq 10^9\), `b` is a non-negative integer such that \(1 \leq b \leq 10^9\), `c` is a non-negative integer such that \(1 \leq c \leq 10^9\), `k` is at least 1. Since there is no else part, the values of `i`, `j`, and `ans` remain as described above regardless of the condition of the if statement.**