Let's break down the problem step by step:

1. **Identify the Variables in the Loop Head**: The variables in the loop head are `i`.
2. **Understand the Loop Condition**: The loop runs from `i = 0` to `i = k // 3`.

Given the current state:
- `i` is `i_prev + 1`
- `j` is \((k - 3 * (i_prev + 1)) // 2\)
- `ans` is updated to be the minimum of its current value and the expression \(3 * (i_prev + 1) * c + ((k - 3 * (i_prev + 1)) // 2) * b + (k - 3 * (i - 1) - 2 * ((k - 3 * (i - 1)) // 2)) * a\)
- `n` is a non-negative integer such that \(1 \leq n \leq 10^9\)
- `a` is a non-negative integer such that \(1 \leq a \leq 10^9\)
- `b` is a non-negative integer such that \(1 \leq b \leq 10^9\)
- `c` is a non-negative integer such that \(1 \leq c \leq 10^9\)
- `k` is at least 1.

For the loop to execute one more time, `i` must be less than or equal to `k // 3`. Given that `i` is currently `i_prev + 1`, it means that `i` needs to be incremented by 1.

Let's denote the new value of `i` as `i_new`:
- `i_new = i_prev + 2`

Now, let's calculate the new value of `j`:
- `j_new = (k - 3 * (i_new - 1)) // 2`
- Substituting `i_new = i_prev + 2`:
  - `j_new = (k - 3 * (i_prev + 1)) // 2`
  - This is the same as the previous value of `j`.

Finally, the value of `ans` remains the same as it is updated based on the loop body but does not change unless the loop body modifies it.

Therefore, the only variable that changes is `i`.

**Final State:**
State: **`i` is `i_prev + 2`, `j` is \((k - 3 * (i_prev + 1)) // 2\), `ans` is updated to be the minimum of its current value and the expression \(3 * (i_prev + 1) * c + ((k - 3 * (i_prev + 1)) // 2) * b + (k - 3 * (i_prev + 1) - 2 * ((k - 3 * (i_prev + 1)) // 2)) * a\), `n` is a non-negative integer such that \(1 \leq n \leq 10^9\), `a` is a non-negative integer such that \(1 \leq a \leq 10^9\), `b` is a non-negative integer such that \(1 \leq b \leq 10^9\), `c` is a non-negative integer such that \(1 \leq c \leq 10^9\), `k` is at least 1.**