To determine what will be printed, let's break down the given initial state and the operations performed within the loop.

### Initial State Recap:
- `t` is the cumulative sum of `s` over all iterations.
- `c` is the cumulative sum of `s * (l[i] + t)` over all iterations.
- `k` is reduced by the cumulative sum of `s` over all iterations.
- `i` will be `n` after the loop runs `n` times.
- `m`, `n`, `l` remain unchanged.

### Loop Analysis:
Assume there is a loop that runs `n` times, and in each iteration:
- `t` is updated by adding `s` to it.
- `c` is updated by adding `s * (l[i] + t)` to it.
- `k` is updated by subtracting `s` from it.

### Final State:
After `n` iterations:
- `t` will be the sum of `s` added `n` times, i.e., `t = n * s`.
- `c` will be the sum of `s * (l[i] + t)` for `i` from 0 to `n-1`.

Let's denote the cumulative sum of `l[i]` over `n` iterations as `L_sum = l[0] + l[1] + ... + l[n-1]`.

Then, the expression for `c` can be expanded as follows:
\[ c = \sum_{i=0}^{n-1} s * (l[i] + t) \]
\[ c = \sum_{i=0}^{n-1} s * l[i] + \sum_{i=0}^{n-1} s * t \]
\[ c = s * L_sum + s * \sum_{i=0}^{n-1} t \]

Since `t` changes in each iteration, we need to consider the value of `t` at each step:
- In iteration 0, `t = 0`.
- In iteration 1, `t = s`.
- In iteration 2, `t = 2s`.
- ...
- In iteration `i`, `t = i * s`.

Thus, the sum of `t` over `n` iterations is:
\[ \sum_{i=0}^{n-1} t = 0 + s + 2s + ... + (n-1)s = s * \frac{(n-1)n}{2} \]

So, the expression for `c` becomes:
\[ c = s * L_sum + s * s * \frac{(n-1)n}{2} \]
\[ c = s * L_sum + s^2 * \frac{(n-1)n}{2} \]

### Print Statement:
The print statement is:
```python
print(int(c))
```

### Output:
The value of `c` is determined by the above formula. Since `m`, `n`, `l`, and `s` are not explicitly given, we express the output in terms of these variables.

Output: **int(s * L_sum + s^2 * (n-1)*n / 2) (where L_sum is the sum of all elements in the list `l`, s is a given integer, and n is the number of iterations)**