Alright, I've got this problem to solve. Let's see what it's asking for. So, I'm given two positive integers, n and m, and I need to find the number of ordered pairs (a, b) where 1 ≤ a ≤ n and 1 ≤ b ≤ m, with the condition that a + b is a multiple of b times the greatest common divisor (GCD) of a and b. That condition sounds a bit tricky, so I need to understand it better.

First, let's rephrase the condition: a + b should be divisible by b * gcd(a, b). In mathematical terms, that means (a + b) mod (b * gcd(a, b)) = 0.

I know that gcd(a, b) is the greatest common divisor of a and b, which divides both a and b. Let's think about how a and b relate through their GCD.

Let me denote d = gcd(a, b). Then, a = d * x and b = d * y, where x and y are coprime integers (since d is the greatest common divisor).

Substituting into the condition:

a + b = d*x + d*y = d*(x + y)

And b * gcd(a, b) = d*y * d = d^2 * y

So, the condition becomes:

d*(x + y) must be divisible by d^2 * y

Simplifying, x + y must be divisible by d * y

But since x and y are coprime, and d divides both a and b (which are d*x and d*y), I need to see how this simplifies further.

Wait, maybe there's a better way to approach this. Let's consider the ratio (a + b)/(b * gcd(a, b)). For this to be an integer, (a + b) must be divisible by b * gcd(a, b).

Given that, perhaps I can find a relationship or a formula to count the number of such pairs (a, b) efficiently.

Looking at the sample inputs and outputs might help. For example, when n = 1 and m = 1, the only pair is (1,1), and it satisfies the condition. Similarly, for n = 2 and m = 3, there are 3 valid pairs, and so on.

I need to find a way to compute this efficiently, especially since n and m can be up to 2*10^6, and there can be up to 10^4 test cases, with the sum of n and m not exceeding 2*10^6 in total.

That means I need an algorithm that's linear or near-linear in terms of n and m.

Looking at the provided program, it seems to be attempting to solve the problem by iterating over possible values of b and calculating some expression involving n and b.

Let's look at the code step by step.

First, it reads the number of test cases, t.

Then, for each test case, it reads n and m.

It initializes the answer, ans, to n. That's interesting; why start with n?

Then, it loops over b from 2 to the minimum of n and m plus one.

In each iteration, it adds (n + b) // (b * b) to the answer.

Finally, it prints the answer.

I need to understand why it's doing this.

Starting with ans = n: perhaps it's accounting for some base cases.

Then, for b from 2 to min(n, m), it's adding some expression involving floor division.

I need to see if this aligns with the mathematical condition given in the problem.

Let me consider small values to see if this makes sense.

Take n = 2, m = 3.

According to the code:

ans = 2

For b = 2:

(n + b) // (b * b) = (2 + 2) // (4) = 4 // 4 = 1

ans = 2 + 1 = 3

Then, b = 3 is not considered since min(n, m) = 2.

So, ans = 3, which matches the sample output for n=2, m=3.

Another sample: n=1, m=1.

ans = 1

b from 2 to 1 (since min(n, m) + 1 = 2, but range(2, 2) is empty).

So, ans = 1, which matches the sample.

Another sample: n=3, m=5.

ans = 3

b=2: (3 + 2) // (4) = 5 // 4 = 1

b=3: (3 + 3) // (9) = 6 // 9 = 0

ans = 3 + 1 + 0 = 4, which matches the sample.

Seems correct so far.

But why is this the correct approach?

Let me try to derive this.

Recall that we have a + b divisible by b * gcd(a, b).

Expressed differently: b * gcd(a, b) divides a + b.

Let’s consider gcd(a, b) = d.

Then, a = d * a1, b = d * b1, where gcd(a1, b1) = 1.

Substituting:

b * d divides a + b => d * b1 * d divides d * a1 + d * b1 = d(a1 + b1).

So, d^2 * b1 divides d(a1 + b1) => d * b1 divides a1 + b1.

But a1 and b1 are coprime.

So, d * b1 divides a1 + b1.

Since b1 and a1 are coprime, b1 divides a1 + b1 implies b1 divides a1.

But a1 and b1 are coprime, and b1 divides a1 only if b1 = 1.

Therefore, for b1 > 1, the only way is if a1 is a multiple of b1, but since they are coprime, that's only possible if b1 = 1.

Wait, that seems conflicting.

Wait, if b1 > 1 and b1 divides a1 + b1, and a1 and b1 are coprime, then b1 divides a1.

But since b1 divides a1 and gcd(a1, b1) = 1, b1 must be 1.

Therefore, the only solution is b1 = 1, which means b = d.

So, b = d, which is gcd(a, b).

Therefore, b = gcd(a, b).

Given that, a is a multiple of b, since b divides a.

So, a is a multiple of b.

Wait, but a is d * a1, and b is d * b1, with b1 = 1.

So, b = d, and a = d * a1.

Thus, a is a multiple of b.

Given that, the condition simplifies to a + b divisible by b * b.

Since a is a multiple of b, let’s say a = k * b.

Then, a + b = k*b + b = b*(k + 1)

And b * b = b^2.

So, b*(k + 1) must be divisible by b^2, which implies that k + 1 is divisible by b.

Since a = k*b and a ≤ n, k ≤ n / b.

So, for each b, k can range from 1 to floor(n / b), and k + 1 must be divisible by b.

Let’s set k + 1 = m * b, where m is an integer ≥ 1.

Then, k = m*b - 1.

Since k ≥ 1, m*b - 1 ≥ 1 => m*b ≥ 2 => m ≥ ceil(2 / b).

But m must be integers, so m ≥ 1.

Also, k ≤ floor(n / b), so m*b - 1 ≤ floor(n / b).

Solving for m: m ≤ floor((floor(n / b) + 1)/b)

Wait, this seems messy.

Alternatively, since k = m*b - 1, and k ≤ floor(n / b), then m*b - 1 ≤ floor(n / b).

So, m ≤ floor((floor(n / b) + 1)/b)

This seems complicated.

Maybe there's a better way to count the number of valid k for each b.

Given that k + 1 must be divisible by b, i.e., k ≡ -1 mod b.

Since k starts from 1, we need to find the number of k in [1, floor(n / b)] such that k ≡ -1 mod b.

This is equivalent to k ≡ b - 1 mod b.

So, k can be b - 1, 2b - 1, 3b - 1, ..., up to the largest m where m*b - 1 ≤ floor(n / b).

Let’s set m*b - 1 ≤ floor(n / b)

Then, m*b ≤ floor(n / b) + 1

So, m ≤ floor( (floor(n / b) + 1)/ b )

Therefore, the number of valid k for each b is floor( (floor(n / b) + 1)/ b )

But floor(n / b) can be computed as (n + b - 1) // b

So, floor(n / b) = (n + b - 1) // b

Then, floor( (floor(n / b) + 1)/ b ) = floor( ((n + b - 1) // b) + 1 ) / b )

This seems a bit convoluted.

But in the code, it's simply (n + b) // (b * b)

Let’s check if this matches.

(n + b) // (b * b) = floor( (n + b) / (b^2) )

Compare this to floor( (floor(n / b) + 1)/ b )

We have floor( (floor(n / b) + 1)/ b ) = floor( (floor(n / b) + 1) / b )

And floor(n / b) = floor(n / b), which is equal to (n + b - 1) // b

So, floor( (floor(n / b) + 1)/ b ) = floor( ((n + b - 1)//b + 1)/ b )

This seems to match (n + b) // (b * b), because:

(n + b - 1)//b + 1 = (n + b - 1 + b)//b = (n + 2b - 1)//b

But that doesn't directly match (n + b)//(b^2)

Wait, perhaps I'm overcomplicating this.

Let’s consider that for each b, the number of valid a is floor( (floor(n / b) + 1)/ b )

And floor(n / b) is (n + b - 1)//b

So, floor( (floor(n / b) + 1)/ b ) = floor( ((n + b - 1)//b + 1)/ b )

But (n + b - 1)//b is equal to ceil(n / b)

So, ceil(n / b) + 1 is ceil(n / b) + 1

Then, floor( (ceil(n / b) + 1)/ b )

This seems difficult to simplify further.

Alternatively, perhaps there's a better mathematical approach.

Let’s consider that for each b, a must be a multiple of b, and a + b must be divisible by b * gcd(a, b)

But since b divides a, gcd(a, b) = b

So, a + b must be divisible by b * b = b^2

Therefore, a + b ≡ 0 mod b^2

But a is a multiple of b, so a = k * b

Thus, k * b + b = b(k + 1) ≡ 0 mod b^2

Which implies that k + 1 ≡ 0 mod b

So, k ≡ -1 mod b

Therefore, k = m * b - 1 for some integer m ≥ 1

Given that a = k * b = (m * b - 1) * b = m * b^2 - b

And a must be ≤ n, so m * b^2 - b ≤ n

Solving for m: m ≤ floor( (n + b)/ (b^2) )

Therefore, for each b, the number of valid m is floor( (n + b)/ (b^2) )

Which is exactly (n + b) // (b * b)

This matches the expression in the code.

Therefore, for each b ≥ 2, the number of valid a is (n + b) // (b * b)

Additionally, the code starts with ans = n, which likely accounts for b = 1.

Let’s check for b = 1.

When b = 1, a can be from 1 to n, since b = 1 divides a, and a + 1 must be divisible by b * gcd(a, b) = 1 * gcd(a, 1) = 1, which is always true, since any integer is divisible by 1.

Therefore, for b = 1, all a from 1 to n are valid, hence ans starts with n.

Then, for b from 2 to min(n, m), it adds (n + b) // (b * b) to ans.

Moreover, since b can be from 1 to m, but in the loop, b starts from 2, so m must be at least 1.

But in the code, it loops from 2 to min(n, m) + 1.

Wait, but in the sample input where n=1 and m=1, it only considers b=1, which is already included in ans = n.

For b ≥ 2, (n + b) // (b * b) would be zero or more, but in that case, min(n, m) + 1 = 2, and b=2 is not considered since range(2, 2) is empty.

Hence, ans remains n = 1, which is correct.

Another sample: n=2, m=3.

ans = 2

b=2: (2 + 2)//4 = 1

ans = 2 + 1 = 3, which matches the sample.

n=3, m=5.

ans=3

b=2: (3+2)//4 = 1

b=3: (3+3)//9 = 0

ans = 3 + 1 + 0 = 4, matches the sample.

Seems consistent.

Therefore, the code correctly calculates the number of valid pairs (a, b) by considering b from 1 to m, with b=1 contributing n pairs, and b from 2 to min(n, m) contributing (n + b)//(b * b) pairs each.

Hence, the program is correct.

**Final Answer**

\[ \boxed{\text{True}} \]