To determine the output state after the loop finishes executing, we need to understand the behavior of the loop based on the provided code and initial state. However, the variable `n` and the string `s` are not defined in the initial state, which are crucial for the loop to execute. Assuming `n` is the length of the string `s`, we need to know `s` to proceed.

Since `s` is not given, let's assume a simple example for `s` to illustrate the process. Let's assume `s = "><>"` and `n = 3`.

### Iteration 1 (i = 0, s[0] = '>')
- Since `s[0]` is '>', we check the conditions:
  - `l < r` (0 < 2) is true.
  - `a = A[l] = A[0] = 0`
  - `x = r - (l + 2) = 2 - (0 + 2) = 0`
  - `b = B[r - 1] = B[1] = 1`
  - Since `x >= 0` (0 >= 0) is true:
    - `b = b - B[x] = 1 - B[0] = 1 - 0 = 1`
    - `b = b - (idx_B[x] - idx_B[r - 1]) * (x + 1) = 1 - (idx_B[0] - idx_B[1]) * (0 + 1) = 1 - (1 - 0) * 1 = 0`
  - `b = (idx_B[r - 1] - i) * (l + 1) = (0 - 0) * (0 + 1) = 0`
  - `print(a * 2 + b * 2 + i + 1, end=' ')` results in `print(0 * 2 + 0 * 2 + 0 + 1, end=' ')` which is `print(1, end=' ')`
  - `l += 1` results in `l = 1`

### Iteration 2 (i = 1, s[1] = '<')
- Since `s[1]` is '<', we check the conditions:
  - `r -= 1` results in `r = 1`
  - `l <= r` (1 <= 1) is true.
  - `a = A[l - 1] = A[0] = 0`
  - `a = a + (i - idx_A[l - 1]) * l = 0 + (1 - 0) * 1 = 1`
  - `b = B[r] = B[1] = 1`
  - Since `r - l >= 0` (1 - 1 >= 0) is true:
    - `b = b - B[r - l] = 1 - B[0] = 1 - 0 = 1`
    - `b = b - (idx_B[r - l] - i) * (r - l) = 1 - (idx_B[0] - 1) * (1 - 1) = 1 - (1 - 1) * 0 = 1`
  - `b = b + (idx_B[r] - i) * l = 1 + (0 - 1) * 1 = 0`
  - `print(a * 2 + b * 2 + i + 1, end=' ')` results in `print(1 * 2 + 0 * 2 + 1 + 1, end=' ')` which is `print(4, end=' ')`

### Iteration 3 (i = 2, s[2] = '>')
- Since `s[2]` is '>', we check the conditions:
  - `l < r` (1 < 1) is false.
  - `r == 0` (1 == 0) is false.
  - `a = B[r - 1] + (idx_B[r - 1] - i) * r = B[0] + (1 - 2) * 1 = 0 + (-1) * 1 = -1`
  - `b = A[l - 1] = A[0] = 0`
  - Since `l - r > 0` (1 - 1 > 0) is false.
  - `b = b + (i - idx_A[l - 1]) * r = 0 + (2 - 0) * 1 = 2`
  - `print(a * 2 + b * 2 + (n - i), end=' ')` results in `print((-1) * 2 + 2 * 2 + (3 - 2), end=' ')` which is `print(-2 + 4 + 1, end=' ')` which is `print(3, end=' ')`
  - `l += 1` results in `l = 2`

### Final Output
The output of the loop is `1 4 3`.

### Final State
The final state of the variables after the loop finishes is:
- `A` remains `[0, 1, 3, 12]`
- `idx_A` remains `[0, 1, 2, 5]`
- `B` remains `[0, 1]`
- `idx_B` remains `[1, 0]`
- `l` is `2`
- `r` is `1`

Output State: **A is [0, 1, 3, 12]; idx_A is [0, 1, 2, 5]; B is [0, 1]; idx_B is [1, 0]; l is 2; r is 1.**