Let's analyze the loop and determine how the variables change with each iteration.

The loop iterates over the elements in the `costs` list, which is `[n - k + 1, 1]`. The loop performs the following operations for each element `i` in `costs`:
1. `curr = n // i`: Calculates the integer division of `n` by `i`.
2. `h += curr`: Adds `curr` to `h`.
3. `n -= i * curr`: Subtracts `i * curr` from `n`.

Let's break down the iterations:

**First Iteration (i = n - k + 1):**
- `curr = n // (n - k + 1)`: This will be 1 if `n` is greater than or equal to `n - k + 1`, which is always true given the constraints.
- `h += curr`: `h` becomes 1.
- `n -= (n - k + 1) * 1`: `n` becomes `k - 1`.

**Second Iteration (i = 1):**
- `curr = n // 1`: This will be `n` itself, which is `k - 1` after the first iteration.
- `h += curr`: `h` becomes `1 + (k - 1) = k`.
- `n -= 1 * (k - 1)`: `n` becomes `0`.

After the loop, `n` becomes `0` and `h` becomes `k`.

Output State: **n is 0, k is unchanged, costs is [n - k + 1, 1], h is k.**