The code snippet `mn = min(mn, cur)` updates `mn` to be the minimum value between its current value and `cur`. Given the initial conditions:

- `cur` is either 3, -1, 1, or -3.
- `mn` is either -1, -2.

We need to consider both cases of the condition `(cur % 2 == 0) == (c == '1')` which affects the value of `cur`.

**Case 1:** If `(cur % 2 == 0) == (c == '1')` is true:
- `cur` is set to either 3 or -1.

**Case 2:** If `(cur % 2 == 0) == (c == '1')` is false:
- `cur` is set to either 1 or -3.

Let's analyze each case:

### Case 1: `(cur % 2 == 0) == (c == '1')` is true
- If `cur` is initially 3, it remains 3 because 3 is odd and thus does not satisfy `(cur % 2 == 0)`.
- If `cur` is initially -1, it remains -1 because -1 is odd and thus does not satisfy `(cur % 2 == 0)`.
- If `cur` is initially 1, it changes to -1 because 1 is odd and satisfies `(cur % 2 == 0) == (c == '1')`.
- If `cur` is initially -3, it changes to 3 because -3 is odd and satisfies `(cur % 2 == 0) == (c == '1')`.

### Case 2: `(cur % 2 == 0) == (c == '1')` is false
- If `cur` is initially 3, it changes to -3 because 3 is odd and does not satisfy `(cur % 2 == 0) == (c == '1')`.
- If `cur` is initially -1, it changes to 1 because -1 is odd and does not satisfy `(cur % 2 == 0) == (c == '1')`.
- If `cur` is initially 1, it remains 1 because 1 is odd and does not satisfy `(cur % 2 == 0) == (c == '1')`.
- If `cur` is initially -3, it remains -3 because -3 is odd and does not satisfy `(cur % 2 == 0) == (c == '1')`.

After updating `cur` based on the condition, `mn` is updated to be the minimum of its current value and the new value of `cur`.

### Updated Values Based on Cases
Given the above analysis, we have four sub-cases for `cur` and `mn`:

1. **Case 1a: Initial `cur` is 3**
   - New `cur` is 3.
   - If `mn` is -1, `mn` remains -1.
   - If `mn` is -2, `mn` remains -2.

2. **Case 1b: Initial `cur` is -1**
   - New `cur` is -1.
   - If `mn` is -1, `mn` remains -1.
   - If `mn` is -2, `mn` remains -2.

3. **Case 1c: Initial `cur` is 1**
   - New `cur` is -1.
   - If `mn` is -1, `mn` remains -1.
   - If `mn` is -2, `mn` remains -2.

4. **Case 1d: Initial `cur` is -3**
   - New `cur` is 3.
   - If `mn` is -1, `mn` changes to -1.
   - If `mn` is -2, `mn` remains -2.

5. **Case 2a: Initial `cur` is 3**
   - New `cur` is -3.
   - If `mn` is -1, `mn` changes to -3.
   - If `mn` is -2, `mn` remains -2.

6. **Case 2b: Initial `cur` is -1**
   - New `cur` is 1.
   - If `mn` is -1, `mn` remains -1.
   - If `mn` is -2, `mn` remains -2.

7. **Case 2c: Initial `cur` is 1**
   - New `cur` is 1.
   - If `mn` is -1, `mn` remains -1.
   - If `mn` is -2, `mn` remains -2.

8. **Case 2d: Initial `cur` is -3**
   - New `cur` is -3.
   - If `mn` is -1, `mn` remains -1.
   - If `mn` is -2, `mn` remains -2.

### Conclusion
The final output state will depend on the initial values of `cur` and `mn`:

- If `cur` is initially 3 and `mn` is -1 or -2, `cur` remains 3 and `mn` remains -1 or -2.
- If `cur` is initially 3 and `mn` is -1, `mn` changes to -1.
- If `cur` is initially -1 and `mn` is -1 or -2, `cur` remains -1 and `mn` remains -1 or -2.
- If `cur` is initially 1 and `mn` is -1 or -2, `cur` remains 1 and `mn` remains -1 or -2.
- If `cur` is initially -3 and `mn` is -1, `mn` changes to -1.
- All other combinations keep their values unchanged.

Thus, the output state is:

Output State: **`s` is a non-empty string with at least one character remaining, `cur` is either 3, -1, 1, or -3, depending on the condition `(cur % 2 == 0) == (c == '1')`, `mn` is either -1 or -2.**