The code `cur = cur + 1` increments the value of `cur` by 1. The initial state is such that `s` is not an empty string, `t` must be greater than 0, and the current value of `cur` modulo 2 is equal to the boolean value represented by `c == '1'`. Since the code only changes the value of `cur`, we need to update `cur` while keeping the other variables unchanged.

Given the initial condition that the current value of `cur` modulo 2 is equal to the boolean value of `c == '1'`, we can deduce that if `c == '1'` is `True`, then `cur % 2 == 1`, and if `c == '1'` is `False`, then `cur % 2 == 0`.

After executing `cur = cur + 1`, the new value of `cur` will be its original value plus 1. This means:

- If the original `cur % 2 == 1`, then the new `cur % 2` will be `0`.
- If the original `cur % 2 == 0`, then the new `cur % 2` will be `1`.

Therefore, the updated value of `cur` will be `cur + 1`.

Output State: **`s` is not an empty string, `t` must be greater than 0, the current value of `cur` is `cur + 1`, and the boolean value of `c == '1'` determines whether `(cur + 1) % 2` is 0 or 1.**