The code `cur = cur - 1` decrements the value of `cur` by 1. Based on the initial state, `cur` is updated based on the condition `(cur % 2 == 0) == (c == '1')` where `c` is the first character of the original string, and `mx` is the maximum of its current value and `cur`.

Since the exact initial value of `cur` is not specified, we will keep it in terms of the condition. However, regardless of the condition, `cur` will be decremented by 1.

The output state will be:
- `s` is a non-empty substring of the original string starting from the second character.
- `t` is greater than 1.
- `cur` is the previous value of `cur` minus 1.
- `mx` remains the maximum of its current value and the new value of `cur`.

Therefore, the Output State is:
**`s` is a non-empty substring of the original string starting from the second character, `t` is greater than 1, `cur` is the previous value of `cur` - 1, `mx` is the maximum of its current value and the new value of `cur`.**