To determine the output of the `print` statement, let's break down the code and the given initial state.

Initial State:
- `s` is a string containing the first `k` lowercase letters of the alphabet.
- `i` is `i + 1` (This does not affect the print statement, so we can ignore it for this task).
- `t` remains unchanged (This also does not affect the print statement, so we can ignore it for this task).
- `n` is the first input integer.
- `k` is the second input integer, and `k` is not equal to 1.

The print statement is:
```python
print((2 - (n == 1)) * s)
```

Let's analyze this step by step:
1. **Expression `n == 1`**:
   - This is a comparison that evaluates to `True` if `n` is 1, and `False` otherwise.
   - In Python, `True` is equivalent to `1` and `False` is equivalent to `0`.

2. **Expression `2 - (n == 1)`**:
   - If `n == 1` is `True` (which means `n` is 1), then `2 - 1` is `1`.
   - If `n == 1` is `False` (which means `n` is not 1), then `2 - 0` is `2`.

3. **Expression `(2 - (n == 1)) * s`**:
   - If `n` is 1, then the expression becomes `1 * s`, which is simply `s`.
   - If `n` is not 1, then the expression becomes `2 * s`, which means the string `s` is repeated twice.

Since `s` is the string containing the first `k` lowercase letters of the alphabet, the output will depend on the value of `n`.

- If `n` is 1, the output will be the string `s`.
- If `n` is not 1, the output will be the string `s` repeated twice.

Therefore, the final output can be described as:

Output: **s (if n is 1) or s repeated twice (if n is not 1) (where s is the string containing the first k lowercase letters of the alphabet)**