The code snippet `k -= (i + 1) * (a[i + 1] - a[i])` modifies the value of `k` by subtracting `(i + 1) * (a[i + 1] - a[i])` from it. Given the initial state, `i` is 4, so the expression becomes `k -= 5 * (a[5] - a[4])`. This means `k` is updated to `k - 5 * (a[5] - a[4])`.

The values of other variables (`t`, `ii`, `n`, `a`, `i`) are not changed by this operation.

Output State: **`t` is an integer such that 1 <= `t` <= 100, `ii` is 2, `n` is greater than 1, `a` is a sorted list of integers, `i` is 4, `k` is `k - 5 * (a[5] - a[4])`.**