To determine what will be printed by the `print` statement, let's break down the problem step-by-step based on the initial state provided.

### Initial State Breakdown:
- `b` is a list with elements: `[-1000000000.0, r1, r2, 2000000000.0, 2000000000.0, 2000000000.0 if 2000000000.0 - r2 > r2 - r1 else r2 + 1, 4000000000.0 - r2 if 2000000000.0 - r2 > 2000000000.0 - (2000000000.0 - r2) else 2000000000.0 + 1, (4000000000.0 - r2) + (2000000000.0 - r2) if 2000000000.0 - r2 > r2 - r1 else (4000000000.0 - r2) + 1, (2000000000.0 if 2000000000.0 - r2 > r2 - r1 else r2 + 1) + (2000000000.0 - r2)]`
- `u` is 0.
- `c` and `d` are the values returned by `r()`, and `c < d`.

### Key Points to Consider:
1. The list `b` contains several elements, including `r1` and `r2`, and some conditional expressions.
2. The indices used in the print statement are `(d - 1) * 2` and `(c - 1) * 2`.
3. Since `c < d`, both `(d - 1) * 2` and `(c - 1) * 2` will be even numbers, and they will refer to the even-indexed elements in the list `b`.

### Analyzing the List `b`:
Let's denote the elements of `b` as follows for clarity:
- `b[0] = -1000000000.0`
- `b[1] = r1`
- `b[2] = r2`
- `b[3] = 2000000000.0`
- `b[4] = 2000000000.0`
- `b[5] = 2000000000.0 if 2000000000.0 - r2 > r2 - r1 else r2 + 1`
- `b[6] = 4000000000.0 - r2 if 2000000000.0 - r2 > 2000000000.0 - (2000000000.0 - r2) else 2000000000.0 + 1`
- `b[7] = (4000000000.0 - r2) + (2000000000.0 - r2) if 2000000000.0 - r2 > r2 - r1 else (4000000000.0 - r2) + 1`
- `b[8] = (2000000000.0 if 2000000000.0 - r2 > r2 - r1 else r2 + 1) + (2000000000.0 - r2)`

### Determining the Values:
Given that `c` and `d` are indices such that `c < d`, the expression `(d - 1) * 2` and `(c - 1) * 2` will refer to even indices in the list `b`. The even indices in `b` are `0`, `2`, `4`, `6`, and `8`.

Let's assume `c = 1` and `d = 2` for simplicity (since `c < d`), then:
- `(c - 1) * 2 = (1 - 1) * 2 = 0`
- `(d - 1) * 2 = (2 - 1) * 2 = 2`

Thus, the print statement will evaluate to:
```python
print(b[0] - b[2])
```
Substituting the known values:
- `b[0] = -1000000000.0`
- `b[2] = r2`

So the expression becomes:
```python
print(-1000000000.0 - r2)
```

### Final Output:
The final output will be:
Output: **-1000000000.0 - r2 (where r2 is the value of the second element in the list b)**