Output State: **`t` is the absolute value of `y2 - y1`, `r` is a list containing six integers, `n` is the second element of `r`, `m` is the second element of `r`, `x1` is increased by `a`, `y1` is 1, `x2` is the fifth element of `r`, `y2` is the sixth element of `r` minus `a`, `b` is the difference between `x2` and `x1`, `(x2 - x1)` is even, `y1` is not equal to `y2`, `a` is `m - y1`, `x2` is decreased by `a`, `x2 > x1`, `x1 >= 1`, `x2 <= n`, and `abs(y1 - 1) < abs(y1 - m)`**

Explanation:
- `y2 -= a` decreases `y2` by the value of `a`.
- Since `a = m - y1` and `y1 = 1`, `a = m - 1`.
- Therefore, `y2` becomes `y2 - (m - 1)`, which simplifies to `y2 - m + 1`.

All other conditions and values remain unchanged.