To analyze the given code snippet, we determine the impact on the existing variables based on the initial state:

Initial State: `n` is a positive integer (1 ≤ `n` ≤ 2·10^9, and `n` must be greater than or equal to 6), `count` is 0, `a` is 1, `b` is 1
```
rem = n - 2 * (a + b)
```

Step-by-step analysis:
1. The code calculates `rem` using the formula `n - 2 * (a + b)`.
2. Since `a` and `b` are both equal to 1, we first compute `a + b`, which equals `1 + 1 = 2`.
3. Next, we multiply this sum by 2: `2 * (a + b) = 2 * 2 = 4`.
4. Finally, we calculate `rem` as `n - 4`.

The states of the other variables (`n`, `count`, `a`, `b`) remain unchanged, but we have determined the value of `rem` based on the given expression.

Output State: **`n` is a positive integer (1 ≤ `n` ≤ 2·10^9, and `n` must be greater than or equal to 6); `count` is 0; `a` is 1; `b` is 1; `rem` is `n - 4`.**