The code prints two expressions: `n * n / 4 - 1` and `n * n / 4 + 1`. 

First, we calculate `n * n / 4`. Since `n` is an even positive integer larger than 2, we can denote `n` as `2k`, where `k` is a positive integer. Thus:

1. `n * n` = `n^2` = `(2k)^2` = `4k^2`
2. Therefore, `n * n / 4` = `4k^2 / 4` = `k^2`

Now, we can calculate both expressions:
- `n * n / 4 - 1` = `k^2 - 1`
- `n * n / 4 + 1` = `k^2 + 1`

After substituting back, we can say:
- For the first expression: `n * n / 4 - 1` can be any integer value that is `k^2 - 1` depending on `n`.
- For the second expression: `n * n / 4 + 1` can be any integer value that is `k^2 + 1` depending on `n`.

Thus, the output states based on the calculations are:
Output State: **`n` is a positive integer such that 1 ≤ `n` ≤ 10^9, `n` is larger than 2, and `n` is an even number; the expressions result in `k^2 - 1` and `k^2 + 1`.**