
Given a Python loop, an initial execution state, and the output states after the first 3 iterations of the loop, determine the output state after all the executions of the loop have finished. 

You must adhere to the text format: Output State: **output state.**

Initial State: `t` is an integer such that 0 ≤ t-1 ≤ 10^4; `n`, `k`, `x` are integers read from the input where 1 ≤ n ≤ 2 · 10^5, 1 ≤ k ≤ n, and 1 ≤ x ≤ n; `a` is a list of `n` integers sorted in descending order as read from the input; `i` is `k + x - 1`; `ans1` is `sum(a) - 2 * (a[k-1] + a[k] + ... + a[k + x - 2])`; `ans2` is `sum(a) - 2 * (a[k-1] + a[k] + ... + a[k + x - 2])`; `ans` is the maximum of `ans1` and `ans2` observed during the loop.
Code of the loop:
for i in range(k):
    ans1 += a[i]
    if i + x < n:
        ans1 -= a[i + x] * 2
    ans = max(ans1, ans2)


The output state after the loop executes the first 3 of times includes what needed to be true for the loop to execute at least that number of times:

Output State after the loop executes 1 time: `t` is an integer such that 0 ≤ t-1 ≤ 10^4; `n`, `k`, `x` are integers read from the input where 1 ≤ n ≤ 2 · 10^5, 1 ≤ k ≤ n, and 1 ≤ x ≤ n; `a` is a list of `n` integers sorted in descending order as read from the input; `i` is `k + x - 1`; if `i + x` is less than `n`, then `ans1` is `sum(a) - 2 * (a[k-1] + a[k] + ... + a[k + x - 2]) + a[i] - a[i + x] * 2` and `ans2` is `sum(a) - 2 * (a[k-1] + a[k] + ... + a[k + x - 2])`; otherwise, `ans1` is `sum(a) - 2 * (a[k-1] + a[k] + ... + a[k + x - 2]) + a[i]` and `ans2` is `sum(a) - 2 * (a[k-1] + a[k] + ... + a[k + x - 2])`; `ans` is the maximum of `ans1` and `ans2` observed during the loop.

**Output State after the loop executes 2 times**: `t` is an integer such that 0 ≤ t-1 ≤ 10^4; `n`, `k`, `x` are integers read from the input where 1 ≤ n ≤ 2 · 10^5, 1 ≤ k ≤ n, and 1 ≤ x ≤ n; `a` is a list of `n` integers sorted in descending order as read from the input; `i` is `k + x - 2`. If `i + x` is less than `n`, then `ans1` is `sum(a) - 2 * (a[k-1] + a[k] + ... + a[k + x - 2]) + 2 * a[i] - a[i + x] * 4` and `ans2` is `sum(a) - 2 * (a[k-1] + a[k] + ... + a[k + x - 2])`. Otherwise, `ans1` is `sum(a) - 2 * (a[k-1] + a[k] + ... + a[k + x - 2]) + 2 * a[i] - a[i + x] * 2` and `ans2` is `sum(a) - 2 * (a[k-1] + a[k] + ... + a[k + x - 2])`. `ans` is the maximum of `ans1` and `ans2` observed during the loop. The value of `ans` has been updated to the maximum of `ans1` and `ans2`.

**Output State after the loop executes 3 times**: `t` is an integer such that 0 ≤ t-1 ≤ 10^4; `n`, `k`, `x` are integers read from the input where 1 ≤ n ≤ 2 · 10^5, 1 ≤ k ≤ n, and 1 ≤ x ≤ n; `a` is a list of `n` integers sorted in descending order as read from the input; `i` is `i + 1` (where `i` is the value at the end of the previous iteration, adjusted to be within the range of the loop); `ans` is the maximum of `ans1` and `ans2` observed during the loop. If `i + x < n`, then `ans1` is the previous value of `ans1` plus `a[i]` minus `a[i + x] * 2`. Otherwise, `ans1` remains unchanged.




What is the ouput state after the loop executes all the iterations? Change the values of only the variables in the loop head and body.The state of the other variables in the precondition that are not affected by the loop head and body must remain unchanged.
In your response strictly use the format: Output State: **the output state you calculate.**, and describe this output state in Natural language easily understandable by humans.

