To determine the output of the given `print` statement, we need to analyze the values of the variables `j % n` and `j` based on the provided initial state.

Here's the breakdown of the variables:

1. **`t`**: An integer read from the input and is greater than or equal to 0. However, `t` is not used in the provided code snippet.
2. **`n`**: A non-negative integer input.
3. **`r`**: The last `i` for which `n * (n + 1) // 2 > i * n` is true and is non-negative. This variable is not used in the provided code snippet.
4. **`sum`**: The total accumulated sum based on the condition. This variable is not used in the provided code snippet.
5. **`j`**: Defined as `n + (n + 1) // 2 + 1` and is greater than `n`.

Let's focus on the calculation of `j` and `j % n`:

- `j` is calculated as `n + (n + 1) // 2 + 1`.
- To find `j % n`, we need to compute the remainder when `j` is divided by `n`.

Let's simplify the expression for `j`:
\[ j = n + \left\lfloor \frac{n + 1}{2} \right\rfloor + 1 \]

Now, let's consider the two cases for `n`:

**Case 1: `n` is even**
- Let `n = 2k` for some integer `k`.
- Then, `j = 2k + \left\lfloor \frac{2k + 1}{2} \right\rfloor + 1 = 2k + k + 1 + 1 = 3k + 2`.
- Now, `j % n = (3k + 2) % 2k`.
- Since `3k + 2 = 2k + k + 2`, we get `j % n = (2k + k + 2) % 2k = (k + 2) % 2k`.
- Because `k + 2` is less than `2k` for `k >= 0`, `j % n = k + 2`.

**Case 2: `n` is odd**
- Let `n = 2k + 1` for some integer `k`.
- Then, `j = 2k + 1 + \left\lfloor \frac{2k + 2}{2} \right\rfloor + 1 = 2k + 1 + k + 1 + 1 = 3k + 3`.
- Now, `j % n = (3k + 3) % (2k + 1)`.
- Since `3k + 3 = 2k + 1 + k + 2`, we get `j % n = (2k + 1 + k + 2) % (2k + 1) = (k + 2) % (2k + 1)`.
- Because `k + 2` is less than `2k + 1` for `k >= 0`, `j % n = k + 2`.

In both cases, `j % n = (n // 2) + 2`.

Now, let's put this into the `print` statement:
```python
print(2, j % n, end=' ')
```

Given `j % n = (n // 2) + 2`, the output will be:
Output: **2, (n // 2) + 2**