Let's break down the code snippet step by step to determine what will be printed.

### Initial State:
- `t` is an integer such that \(1 \leq t \leq 10^4\).
- Each of the four integers \(p_i\) in the sequence is an integer such that \(0 \leq p_i \leq 200\).

### Code Breakdown:
1. **Reading Input:**
   - The code reads an integer `t` from the input, which represents the number of test cases.
   - For each test case, it reads a sequence of four integers \(p_0, p_1, p_2, p_3\) from the input.

2. **Processing Each Test Case:**
   - For each test case, the code processes the sequence of four integers using the following formula:
     \[
     \text{result} = \sum_{i=0}^{3} \left(3 \left(\left\lfloor \frac{x}{2} \right\rfloor \right) + (x \mod 2) \cdot (i < 3)\right) // 3
     \]
     where \(x\) is each integer in the sequence.

3. **Explanation of the Formula:**
   - For each integer \(x\) in the sequence:
     - `x // 2` gives the integer division of \(x\) by 2.
     - `3 * (x // 2)` multiplies the integer division result by 3.
     - `x % 2` gives the remainder of \(x\) when divided by 2 (0 if \(x\) is even, 1 if \(x\) is odd).
     - `(x % 2) * (i < 3)` adds 1 to the sum if \(x\) is odd and \(i < 3\), otherwise it adds 0.
     - The sum of these values is then divided by 3 using integer division (`// 3`).

4. **Output:**
   - The result of the formula for each test case is printed on a new line.

### Detailed Calculation:
- For each integer \(x\) in the sequence:
  - If \(x\) is even, `x % 2` is 0, so the formula simplifies to:
    \[
    3 \left(\left\lfloor \frac{x}{2} \right\rfloor \right)
    \]
  - If \(x\) is odd, `x % 2` is 1, so the formula becomes:
    \[
    3 \left(\left\lfloor \frac{x}{2} \right\rfloor \right) + 1 \cdot (i < 3)
    \]
    - This means for \(i < 3\), an additional 1 is added to the sum if \(x\) is odd.
    - For \(i = 3\), no additional 1 is added.

- The sum of these values for all four integers in the sequence is then divided by 3 using integer division.

### Example Calculation:
- Suppose the input is:
  - `t = 2`
  - For the first test case: `p_0 = 4, p_1 = 5, p_2 = 6, p_3 = 7`
  - For the second test case: `p_0 = 0, p_1 = 1, p_2 = 2, p_3 = 3`

- For the first test case:
  - \(p_0 = 4\): \(3 \left(\left\lfloor \frac{4}{2} \right\rfloor \right) + 0 = 3 \cdot 2 + 0 = 6\)
  - \(p_1 = 5\): \(3 \left(\left\lfloor \frac{5}{2} \right\rfloor \right) + 1 = 3 \cdot 2 + 1 = 7\)
  - \(p_2 = 6\): \(3 \left(\left\lfloor \frac{6}{2} \right\rfloor \right) + 0 = 3 \cdot 3 + 0 = 9\)
  - \(p_3 = 7\): \(3 \left(\left\lfloor \frac{7}{2} \right\rfloor \right) + 0 = 3 \cdot 3 + 0 = 9\)
  - Sum: \(6 + 7 + 9 + 9 = 31\)
  - Result: \(31 // 3 = 10\)

- For the second test case:
  - \(p_0 = 0\): \(3 \left(\left\lfloor \frac{0}{2} \right\rfloor \right) + 0 = 3 \cdot 0 + 0 = 0\)
  - \(p_1 = 1\): \(3 \left(\left\lfloor \frac{1}{2} \right\rfloor \right) + 1 = 3 \cdot 0 + 1 = 1\)
  - \(p_2 = 2\): \(3 \left(\left\lfloor \frac{2}{2} \right\rfloor \right) + 0 = 3 \cdot 1 + 0 = 3\)
  - \(p_3 = 3\): \(3 \left(\left\lfloor \frac{3}{2} \right\rfloor \right) + 0 = 3 \cdot 1 + 0 = 3\)
  - Sum: \(0 + 1 + 3 + 3 = 7\)
  - Result: \(7 // 3 = 2\)

### Final Output:
- The code will print the results of the formula for each test case, one result per line.

Output: **10
2** (where the first line is the result for the first test case and the second line is the result for the second test case)