The code snippet `su += c[i]` updates the value of `su` by adding the value of `c[i]` to it. Given the initial state:

- `n`, `m`, and `d` are integers read from input, 1 ≤ `n`, `m`, `d` ≤ 1000, `m` ≤ `n`, and `m` > 0.
- `c` is a list of `m` integers where each `c_i` satisfies 1 ≤ `c_i` ≤ `n` and the sum of all `c_i` is less than or equal to `n`.
- `ans` is a list of zeros of length `n`.
- `pos` is a list containing two elements: `n + 1 - c[m - 1]` and `n + 1 - c[m - 1] - c[m - 2]`.
- `su` is `c[m - 1]`.
- `i` is `m - 2`.

The value of `su` is initially `c[m - 1]`. After executing `su += c[i]`, `su` becomes `c[m - 1] + c[i]`. Since `i` is `m - 2`, the updated value of `su` is `c[m - 1] + c[m - 2]`.

Therefore, the output state is:
**`n`, `m`, and `d` are integers read from input, 1 ≤ `n`, `m`, `d` ≤ 1000, `m` ≤ `n`, and `m` > 0; `c` is a list of `m` integers where each `c_i` satisfies 1 ≤ `c_i` ≤ `n` and the sum of all `c_i` is less than or equal to `n`; `ans` is a list of zeros of length `n`; `pos` is a list containing two elements: `n + 1 - c[m - 1]` and `n + 1 - c[m - 1] - c[m - 2]`; `su` is `c[m - 1] + c[m - 2]`; `i` is `m - 2`.**