The code snippet `pos.reverse()` reverses the order of the elements in the list `pos`. This means that the first element becomes the last, the second element becomes the second-to-last, and so on. 

Given the initial state:
- `n`, `m`, and `d` are integers read from input, with constraints 1 ≤ `n`, `m`, `d` ≤ 1000, `m` ≤ `n`.
- `c` is a list of `m` integers where each `c_i` satisfies 1 ≤ `c_i` ≤ `n` and the sum of all `c_i` is less than or equal to `n`.
- `ans` is a list of zeros of length `n`.
- `pos` is a list containing `m + 1` elements, where the first `m` elements are `n + 1 - su - c[i]` for `i` from `m - 1` to `0`, and the last element is `0`.
- `su` is the sum of all elements in `c`, i.e., `su = sum(c)`.
- `i` is `-1`.

After reversing `pos`, the new state of `pos` will have its elements in reverse order. The last element (which was `0`) will now be the first element, and the first element (which was `n + 1 - su - c[m-1]`) will now be the last element.

Therefore, the output state is:
- `n`, `m`, and `d` are integers read from input, with constraints 1 ≤ `n`, `m`, `d` ≤ 1000, `m` ≤ `n`.
- `c` is a list of `m` integers where each `c_i` satisfies 1 ≤ `c_i` ≤ `n` and the sum of all `c_i` is less than or equal to `n`.
- `ans` is a list of zeros of length `n`.
- `pos` is a list containing `m + 1` elements, where the first element is `0`, and the subsequent elements are `n + 1 - su - c[i]` for `i` from `0` to `m - 1` in reverse order.
- `su` is the sum of all elements in `c`, i.e., `su = sum(c)`.
- `i` is `-1`.

Output State: **`n`, `m`, and `d` are integers read from input, with constraints 1 ≤ `n`, `m`, `d` ≤ 1000, `m` ≤ `n`; `c` is a list of `m` integers where each `c_i` satisfies 1 ≤ `c_i` ≤ `n` and the sum of all `c_i` is less than or equal to `n`; `ans` is a list of zeros of length `n`; `pos` is a list containing `m + 1` elements, where the first element is `0`, and the subsequent elements are `n + 1 - su - c[i]` for `i` from `0` to `m - 1` in reverse order; `su` is the sum of all elements in `c`, i.e., `su = sum(c)`; `i` is `-1`.**