The code snippet `ans[j - 1] = i + 1` updates the value of the element at index `j - 1` in the list `ans` to `i + 1`. Given the initial state:

- `n`, `m`, and `d` are integers with constraints 1 ≤ `n`, `m`, `d` ≤ 1000, `m` ≤ `n`, `m` > 0.
- `c` is a list of `m` integers where each `c_i` satisfies 1 ≤ `c_i` ≤ `n` and the sum of all `c_i` is less than or equal to `n`.
- `ans` is a list of length `n` where the element at index `j - 1` is set to `i + 2`.
- `pos` is a list containing `m + 1` elements, where the first element is `0`, and the subsequent elements are `n + 1 - su - c[i]` for `i` from `0` to `m - 1` in reverse order.
- `su` is the sum of all elements in `c`.
- `i` is an integer in the range `[2, m]`.

After executing the code snippet:

- The element at index `j - 1` in the list `ans` is updated from `i + 2` to `i + 1`.
- All other variables and their values remain unchanged.

Therefore, the output state is:

Output State: **`n`, `m`, and `d` are integers with constraints 1 ≤ `n`, `m`, `d` ≤ 1000, `m` ≤ `n`, `m` > 0; `c` is a list of `m` integers where each `c_i` satisfies 1 ≤ `c_i` ≤ `n` and the sum of all `c_i` is less than or equal to `n`; `ans` is a list of length `n` where the element at index `j - 1` is set to `i + 1` and all other elements remain as they were; `pos` is a list containing `m + 1` elements, where the first element is `0`, and the subsequent elements are `n + 1 - su - c[i]` for `i` from `0` to `m - 1` in reverse order; `su` is the sum of all elements in `c`; `i` is an integer in the range `[2, m]`**.