`ans` is incremented by `n // 2 - 1`. Given that `n` is even, let's denote `n` as `2k` where `k` is an integer. So, `n // 2` is `k`, and `n // 2 - 1` is `k - 1`. Therefore, `ans` is incremented by `k - 1`.

Since `n` is even and within the range of 1 to \(2^h\) (where `1 ≤ h ≤ 50`), and given that `n` is greater than 1, the value of `k` (which is `n // 2`) is an integer between 1 and \(2^{h-1}\). 

Given the initial state where `ans` is 0, the new value of `ans` will be `0 + (k - 1)`, which simplifies to `k - 1`.

Thus, the updated state is:

Output State: **`h` is an input integer such that 1 ≤ h ≤ 50; `n` is an input integer such that 1 ≤ n ≤ 2^`h` and `n` is greater than 1; `ans` is `n // 2 - 1`, and the current value of `n` is even.**