# Test 1
**Input**: 
```
1
10
```
**Output**: 
```
5
```
*Explanation*: For \( x = 10 \), the value of \( y = 5 \) maximizes \( \gcd(10, 5) + 5 = 5 + 5 = 10 \).

# Test 2
**Input**: 
```
1
7
```
**Output**: 
```
6
```
*Explanation*: For \( x = 7 \), the value of \( y = 6 \) maximizes \( \gcd(7, 6) + 6 = 1 + 6 = 7 \).

# Test 3
**Input**: 
```
1
21
```
**Output**: 
```
18
```
*Explanation*: For \( x = 21 \), the value of \( y = 18 \) maximizes \( \gcd(21, 18) + 18 = 3 + 18 = 21 \).

# Test 4
**Input**: 
```
1
100
```
**Output**: 
```
98
```
*Explanation*: For \( x = 100 \), the value of \( y = 98 \) maximizes \( \gcd(100, 98) + 98 = 2 + 98 = 100 \).

# Test 5
**Input**: 
```
1
2
```
**Output**: 
```
1
```
*Explanation*: For \( x = 2 \), the value of \( y = 1 \) maximizes \( \gcd(2, 1) + 1 = 1 + 1 = 2 \).

# Test 6
**Input**: 
```
1
1000
```
**Output**: 
```
750
```
*Explanation*: For \( x = 1000 \), the value of \( y = 750 \) maximizes \( \gcd(1000, 750) + 750 = 250 + 750 = 1000 \).

# Test 7
**Input**: 
```
1
6
```
**Output**: 
```
3
```
*Explanation*: For \( x = 6 \), the value of \( y = 3 \) maximizes \( \gcd(6, 3) + 3 = 3 + 3 = 6 \).

# Test 8
**Input**: 
```
3
11
13
17
```
**Output**: 
```
6
6
8
```
*Explanation*: For \( x = 11 \), the value of \( y = 6 \) maximizes \( \gcd(11, 6) + 6 = 1 + 6 = 7 \).
For \( x = 13 \), the value of \( y = 6 \) maximizes \( \gcd(13, 6) + 6 = 1 + 6 = 7 \).
For \( x = 17 \), the value of \( y = 8 \) maximizes \( \gcd(17, 8) + 8 = 1 + 8 = 9 \).

# Test 9
**Input**: 
```
3
1001
1002
1003
```
**Output**: 
```
501
501
502
```
*Explanation*: For \( x = 1001 \), the value of \( y = 501 \) maximizes \( \gcd(1001, 501) + 501 = 1 + 501 = 502 \).
For \( x = 1002 \), the value of \( y = 501 \) maximizes \( \gcd(1002, 501) + 501 = 3 + 501 = 504 \).
For \( x = 1003 \), the value of \( y = 502 \) maximizes \( \gcd(1003, 502) + 502 = 1 + 502 = 503 \).

# Test 10
**Input**: 
```
3
4
8
12
```
**Output**: 
```
2
4
6
```
*Explanation*: For \( x = 4 \), the value of \( y = 2 \) maximizes \( \gcd(4, 2) + 2 = 2 + 2 = 4 \).
For \( x = 8 \), the value of \( y = 4 \) maximizes \( \gcd(8, 4) + 4 = 4 + 4 = 8 \).
For \( x = 12 \), the value of \( y = 6 \) maximizes \( \gcd(12, 6) + 6 = 6 + 6 = 12 \).

# Test 11
**Input**: 
```
3
10000
10001
10002
```
**Output**: 
```
5000
5001
5001
```
*Explanation*: For \( x = 10000 \), the value of \( y = 5000 \) maximizes \( \gcd(10000, 5000) + 5000 = 5000 + 5000 = 10000 \).
For \( x = 10001 \), the value of \( y = 5001 \) maximizes \( \gcd(10001, 5001) + 5001 = 1 + 5001 = 5002 \).
For \( x = 10002 \), the value of \( y = 5001 \) maximizes \( \gcd(10002, 5001) + 5001 = 3 + 5001 = 5004 \).

# Test 12
**Input**: 
```
3
111
112
113
```
**Output**: 
```
56
56
57
```
*Explanation*: For \( x = 111 \), the value of \( y = 56 \) maximizes \( \gcd(111, 56) + 56 = 1 + 56 = 57 \).
For \( x = 112 \), the value of \( y = 56 \) maximizes \( \gcd(112, 56) + 56 = 56 + 56 = 112 \).
For \( x = 113 \), the value of \( y = 57 \) maximizes \( \gcd(113, 57) + 57 = 1 + 57 = 58 \).