The value of `b` is updated to be `a` raised to the power of `x`. Given that `a` is equal to `b` raised to the power of `x`, we can substitute this into the equation for `b`. Thus, `b` becomes `(b ^ x) ^ x`, which is equivalent to `b ^ (x * x)` or `b ^ (x ^ 2)`. 

The states of the other variables, `s` and `x`, are not affected by this operation. Therefore, `s` remains an integer such that 2 ≤ `s` ≤ 10^12, and `x` remains an integer such that 0 ≤ `x` ≤ 10^12.

Output State: **`s` is an integer such that 2 ≤ `s` ≤ 10^12, `x` is an integer such that 0 ≤ `x` ≤ 10^12, `a` is equal to `b` ^ `x`, `b` is equal to `b` ^ (`x` ^ 2)**