Alright, I've got this problem to solve. Let's see what it's asking for. So, there's this concept of a "good" array, and I need to determine whether certain subarrays are good based on some conditions.

First, let's understand what makes an array "good." According to the problem, an array \( a \) of length \( m \) is considered good if there exists another integer array \( b \) of the same length such that three conditions are met:

1. The sum of elements in \( a \) is equal to the sum of elements in \( b \): \( \sum_{i=1}^{m} a_i = \sum_{i=1}^{m} b_i \).

2. For every index \( i \), \( a_i \) is not equal to \( b_i \): \( a_i \neq b_i \).

3. Every element in \( b \) is positive: \( b_i > 0 \) for all \( i \).

So, essentially, for the array \( a \) to be good, I need to be able to find another array \( b \) where each \( b_i \) is different from \( a_i \), all \( b_i \) are positive, and the total sum remains the same.

Let me try to rephrase this to understand it better. I need to transform the array \( a \) into another array \( b \) where:

- No element remains the same.

- All elements in \( b \) are positive.

- The sum of \( b \) is equal to the sum of \( a \).

My task is to check if such a transformation is possible for given subarrays of \( c \).

Given that, I need to process multiple queries, each asking whether a particular subarray \( c_{l_i} \) to \( c_{r_i} \) is good based on the above conditions.

Looking at the constraints:

- \( t \) (number of test cases) can be up to \( 10^4 \).

- \( n \) and \( q \) (length of array \( c \) and number of queries) can be up to \( 3 \times 10^5 \).

- The sum of \( n \) over all test cases doesn't exceed \( 3 \times 10^5 \), and the same for \( q \).

This suggests that the solution needs to be efficient, probably with a time complexity of around \( O(n + q) \).

Now, let's think about how to approach this.

First, for a subarray to be good, I need to find a way to adjust each element so that it's different from its original value, positive, and the total sum remains the same.

Let me consider what changes I can make to each \( a_i \) to get \( b_i \):

- \( b_i \) must be positive and not equal to \( a_i \).

- To keep the sum the same, the adjustments must balance out.

I need to ensure that for each \( a_i \), I can choose a \( b_i \) that is positive, not equal to \( a_i \), and such that the sum over all \( b_i \) equals the sum of all \( a_i \).

Let me consider the minimal possible \( b_i \). Since \( b_i > 0 \) and \( b_i \neq a_i \), the smallest \( b_i \) can be is:

- If \( a_i > 1 \), then \( b_i \) can be \( a_i - 1 \) or \( a_i + 1 \), but to minimize, choose \( a_i - 1 \).

- If \( a_i = 1 \), since \( b_i \) must be positive and different, the smallest \( b_i \) can be is 2.

Wait, no. If \( a_i = 1 \), \( b_i \) must be greater than 1 because it has to be different and positive. So, the smallest \( b_i \) can be is 2.

Similarly, for \( a_i > 1 \), the smallest \( b_i \) can be is \( a_i - 1 \), as long as it's positive and different from \( a_i \).

But wait, \( a_i - 1 \) could be less than or equal to zero if \( a_i \) is 1, but since \( a_i \) is at least 1, \( a_i - 1 \) is at least 0. But \( b_i \) must be positive, so if \( a_i = 1 \), \( b_i \) cannot be 0; it has to be at least 2.

So, in general:

- If \( a_i > 1 \), the minimal \( b_i \) is \( a_i - 1 \).

- If \( a_i = 1 \), the minimal \( b_i \) is 2.

So, for each element in the subarray, I can define a minimal possible \( b_i \) that satisfies \( b_i > 0 \) and \( b_i \neq a_i \).

Then, the minimal sum of \( b \) is the sum of these minimal \( b_i \) for each element in the subarray.

For the subarray to be good, the sum of \( a \) should be at least this minimal sum of \( b \).

But wait, the sum of \( b \) needs to be equal to the sum of \( a \), not just at least.

So, if the sum of \( a \) is less than the minimal sum of \( b \), it's impossible to find such a \( b \), so the subarray is not good.

Moreover, I need to ensure that the sum of \( a \) is exactly equal to the sum of \( b \), and that each \( b_i \) is at least its minimal value.

But, since I can choose \( b_i \) to be greater than its minimal value, as long as the total sum remains the same, I need to check if the sum of \( a \) is at least the minimal sum of \( b \), and that the difference between the sum of \( a \) and the minimal sum of \( b \) can be distributed among the elements to make up the required sum.

Wait, but since I need the sum to be exactly the same, and I can adjust \( b_i \) to be either \( a_i - 1 \) (if \( a_i > 1 \)) or 2 (if \( a_i = 1 \)), and possibly higher, but ensuring that \( b_i \neq a_i \), I need to make sure that the sum of these minimal \( b_i \) is less than or equal to the sum of \( a_i \), and that there's a way to adjust the \( b_i \) to match the sum of \( a_i \).

But actually, since I can set \( b_i \) to be greater than its minimal value, as long as it's different from \( a_i \), and positive, I need to ensure that the sum of \( a \) is at least the minimal sum of \( b \), and that the difference can be distributed in a way that doesn't violate the conditions.

But perhaps there's a simpler way to look at it.

Let me consider the minimal sum of \( b \):

- For each \( a_i \), if \( a_i > 1 \), minimal \( b_i = a_i - 1 \).

- If \( a_i = 1 \), minimal \( b_i = 2 \).

So, I can precompute for each position in the array \( c \), the minimal \( b_i \) based on \( c_i \).

Then, for each query, I can compute the sum of \( c \) from \( l_i \) to \( r_i \), and the sum of the minimal \( b_i \) from \( l_i \) to \( r_i \), and check if the sum of \( c \) is at least the sum of minimal \( b_i \).

But actually, I need the sum to be exactly equal to the sum of \( b_i \), not just at least.

Wait, but in the code provided, it seems to check if the sum of the subarray is greater than or equal to the sum of some values computed in array \( b \), which seems to be the sum of minimal \( b_i \).

But according to the problem, the sum needs to be exactly equal.

Wait, in the code, it's checking if \( a[y] - a[x-1] < b[y] - b[x-1] \), and printing 'NO' in that case, else 'YES', unless \( x == y \), in which case it always prints 'NO'.

Wait, let's look at the code more carefully.

In the code:

- It reads the number of test cases \( t \).

- For each test case, it defines function \( func_1() \), which reads \( n \) and \( q \), then reads array \( a \), which is padded with a 0 at the beginning.

- It computes array \( b \), where for each position \( i \), if \( a[i] > 1 \), \( b[i] = b[i-1] + 1 \), else \( b[i] = b[i-1] + 2 \). It seems like it's accumulating the minimal \( b_i \).

- Then it computes the prefix sums of \( a \), using the accumulate function.

- For each query, it computes the sum of \( a \) from \( l_i \) to \( r_i \), and the sum of \( b \) from \( l_i \) to \( r_i \), and checks if the sum of \( a \) is less than the sum of \( b \), or if \( x == y \), in which case it prints 'NO', else 'YES'.

So, it's using prefix sums to compute the sum of \( a \) and the sum of \( b \) for each subarray defined by the query.

Now, is this correct?

Let me think about it.

First, the way \( b \) is computed:

- For each \( i \), if \( a[i] > 1 \), add 1 to the previous \( b \), else add 2.

This seems to be calculating the minimal sum of \( b_i \) for each position.

Because:

- If \( a_i > 1 \), minimal \( b_i = a_i - 1 \), which is \( a_i \) minus 1.

- If \( a_i = 1 \), minimal \( b_i = 2 \), which is \( a_i + 1 \).

Wait, no, for \( a_i = 1 \), minimal \( b_i = 2 \), which is \( a_i + 1 \).

But for \( a_i > 1 \), minimal \( b_i = a_i - 1 \), which is \( a_i \) minus 1.

So, the difference between \( b_i \) and \( a_i \) is:

- If \( a_i > 1 \), \( b_i - a_i = -1 \).

- If \( a_i = 1 \), \( b_i - a_i = 1 \).

So, the difference is either -1 or +1, depending on whether \( a_i > 1 \) or \( a_i = 1 \).

Now, the sum of \( b \) would be the sum of \( a \) plus the sum of these differences.

Wait, no. Sum of \( b \) is sum of \( a \) plus the sum of \( (b_i - a_i) \).

So, sum of \( b \) = sum of \( a \) + sum of \( (b_i - a_i) \).

In the minimal case:

- For \( a_i > 1 \), \( b_i - a_i = -1 \).

- For \( a_i = 1 \), \( b_i - a_i = 1 \).

So, sum of \( b \) in minimal case is sum of \( a \) plus the sum of these differences.

Wait, but in the code, \( b[i] = b[i-1] + x \), where \( x = 1 \) if \( a_i > 1 \), else 2.

Wait, no, in the code, \( x = 1 \) if \( a_i > 1 \), else 2, and \( b[i] = b[i-1] + x \).

So, \( b[i] \) is accumulating these \( x \) values, which are 1 or 2, depending on \( a_i \).

But what does this \( b[i] \) represent?

Wait, perhaps it's a misunderstanding on my part.

Let me think differently.

Suppose I define for each \( a_i \):

- If \( a_i > 1 \), then \( b_i = a_i - 1 \).

- If \( a_i = 1 \), then \( b_i = 2 \).

Then, the minimal sum of \( b \) for a subarray is the sum of these \( b_i \) over that subarray.

Now, for the subarray to be good, the sum of \( a \) over that subarray must be equal to the sum of \( b \) over that subarray.

Wait, but according to the above definitions:

- If \( a_i > 1 \), \( b_i = a_i - 1 \), so \( b_i = a_i - 1 \).

- If \( a_i = 1 \), \( b_i = 2 \), so \( b_i = a_i + 1 \).

Therefore, the difference \( b_i - a_i \) is:

- \( -1 \) if \( a_i > 1 \).

- \( +1 \) if \( a_i = 1 \).

So, the total sum of \( b \) would be the sum of \( a \) plus the sum of these differences.

Therefore, sum of \( b \) = sum of \( a \) + number of \( a_i = 1 \) - number of \( a_i > 1 \).

Wait, no.

Wait, sum of \( b \) = sum of \( a \) + sum of \( (b_i - a_i) \).

And \( b_i - a_i \) is:

- \( -1 \) if \( a_i > 1 \).

- \( +1 \) if \( a_i = 1 \).

Therefore, sum of \( b \) = sum of \( a \) + (number of \( a_i = 1 \)) - (number of \( a_i > 1 \)).

But in the code, \( b[i] \) is accumulating 1 for each \( a_i > 1 \) and 2 for each \( a_i = 1 \).

Wait, no, in the code, \( x = 1 \) if \( a_i > 1 \), else 2, and \( b[i] = b[i-1] + x \).

So, \( b[i] \) is the sum of \( x \) from 1 to \( i \), where \( x = 1 \) if \( a_i > 1 \), else 2.

Therefore, \( b[i] \) is the sum of 1's and 2's based on the values of \( a_i \).

But what does this sum represent?

Wait, perhaps it represents the minimal sum of \( b_i \) minus the sum of \( a_i \).

Wait, let's see:

If \( a_i > 1 \), \( b_i = a_i - 1 \), so \( b_i - a_i = -1 \).

If \( a_i = 1 \), \( b_i = 2 \), so \( b_i - a_i = +1 \).

Therefore, sum of \( b_i - a_i \) over the subarray is (number of \( a_i = 1 \)) - (number of \( a_i > 1 \)).

But in the code, \( b[i] \) is sum of 1's and 2's based on \( a_i \).

Wait, perhaps I need to relate this differently.

Let me consider that the sum of minimal \( b_i \) is sum of \( (a_i - 1) \) for \( a_i > 1 \) and \( 2 \) for \( a_i = 1 \).

So, sum of minimal \( b \) = sum over \( i \) of:

\( a_i - 1 \) if \( a_i > 1 \), else \( 2 \).

Which is equal to sum of \( a_i \) for all \( i \) minus the number of \( a_i > 1 \) plus the number of \( a_i = 1 \).

Because for \( a_i > 1 \), we subtract 1, and for \( a_i = 1 \), we add 1 (since \( 2 = 1 + 1 \)).

Wait, no:

sum of minimal \( b_i \) = sum_{a_i > 1} (a_i - 1) + sum_{a_i = 1} (2)

= sum_{a_i > 1} a_i - sum_{a_i > 1} 1 + sum_{a_i = 1} 2

= sum_{a_i > 1} a_i + sum_{a_i = 1} 2 - number of \( a_i > 1 \)

But I'm getting confused.

Let me compute sum of minimal \( b_i \):

sum_{i=1 to m} b_i = sum_{a_i > 1} (a_i - 1) + sum_{a_i = 1} 2

= sum_{i=1 to m} a_i - number of \( a_i > 1 \) + 2 * number of \( a_i = 1 \)

So, sum of minimal \( b_i \) = sum of \( a_i \) - number of \( a_i > 1 \) + 2 * number of \( a_i = 1 \)

But in the code, \( b[i] \) is sum of 1's and 2's based on \( a_i \):

\( b[i] = b[i-1] + x \), where \( x = 1 \) if \( a_i > 1 \), else 2.

So, \( b[i] \) is the cumulative sum of these \( x \)'s.

Therefore, \( b[y] - b[x-1] \) is the sum of \( x \)'s from \( x \) to \( y \), which is:

sum_{i=x to y} x_i = sum_{a_i > 1} 1 + sum_{a_i = 1} 2

But according to the earlier equation:

sum of minimal \( b_i \) = sum of \( a_i \) - number of \( a_i > 1 \) + 2 * number of \( a_i = 1 \)

Wait, but in the code, it's checking if sum of \( a \) from \( x \) to \( y \) is less than \( b[y] - b[x-1] \), and if so, prints 'NO', else prints 'YES', unless \( x == y \), in which case it always prints 'NO'.

Wait, but according to the earlier equation:

sum of minimal \( b_i \) = sum of \( a_i \) - number of \( a_i > 1 \) + 2 * number of \( a_i = 1 \)

But sum of minimal \( b_i \) should be less than or equal to sum of \( a_i \), and for the subarray to be good, sum of \( b_i \) should be equal to sum of \( a_i \).

Wait, no, actually, in the minimal case, sum of \( b_i \) is sum of \( a_i \) minus number of \( a_i > 1 \) plus 2 * number of \( a_i = 1 \).

But I need sum of \( b_i \) to be equal to sum of \( a_i \).

So, for the subarray to be good, sum of \( a_i \) should be equal to sum of minimal \( b_i \), which is sum of \( a_i \) - number of \( a_i > 1 \) + 2 * number of \( a_i = 1 \).

Wait, that would imply:

sum of \( a_i \) = sum of \( a_i \) - number of \( a_i > 1 \) + 2 * number of \( a_i = 1 \)

Simplifying:

0 = - number of \( a_i > 1 \) + 2 * number of \( a_i = 1 \)

Which implies:

number of \( a_i > 1 \) = 2 * number of \( a_i = 1 \)

Wait, that doesn't make sense.

Wait, perhaps I made a mistake in defining the minimal sum of \( b_i \).

Let me think again.

If \( a_i > 1 \), minimal \( b_i = a_i - 1 \).

If \( a_i = 1 \), minimal \( b_i = 2 \).

Therefore, sum of minimal \( b_i \) = sum_{i=1 to m} (a_i - 1 if a_i > 1 else 2)

= sum_{i=1 to m} a_i - number of \( a_i > 1 \) + number of \( a_i = 1 \)

Because for \( a_i > 1 \), we subtract 1, and for \( a_i = 1 \), we add 1 (since 2 = 1 + 1).

Wait, no:

sum of minimal \( b_i \) = sum_{a_i > 1} (a_i - 1) + sum_{a_i = 1} 2

= sum_{a_i > 1} a_i - sum_{a_i > 1} 1 + sum_{a_i = 1} 2

= sum_{a_i > 1} a_i + sum_{a_i = 1} 2 - number of \( a_i > 1 \)

But sum of all \( a_i \) is sum_{a_i > 1} a_i + sum_{a_i = 1} 1

So, sum of minimal \( b_i \) = sum of all \( a_i \) - sum_{a_i = 1} 1 - number of \( a_i > 1 \) + 2 * number of \( a_i = 1 \)

= sum of all \( a_i \) - number of \( a_i > 1 \) + number of \( a_i = 1 \)

But number of \( a_i > 1 \) = total elements - number of \( a_i = 1 \)

So, number of \( a_i > 1 \) = m - number of \( a_i = 1 \)

Substituting:

sum of minimal \( b_i \) = sum of all \( a_i \) - (m - number of \( a_i = 1 \)) + number of \( a_i = 1 \)

= sum of all \( a_i \) - m + 2 * number of \( a_i = 1 \)

Wait, this seems off.

Let me try with an example.

Take the example from the problem:

n = 5, q = 4

c = [1, 2, 1, 4, 5]

Queries:

1. 1 to 5

2. 4 to 4

3. 3 to 4

4. 1 to 3

Compute sum of minimal \( b_i \):

For c = [1,2,1,4,5]

Minimal b:

- c[1] = 1 -> b[1] = 2

- c[2] = 2 -> b[2] = 1

- c[3] = 1 -> b[3] = 2

- c[4] = 4 -> b[4] = 3

- c[5] = 5 -> b[5] = 4

Sum of minimal b:

2 + 1 + 2 + 3 + 4 = 12

Sum of c: 1 + 2 + 1 + 4 + 5 = 13

So, 13 >= 12, and 13 - 12 = 1, which is the difference.

But according to the problem, for the subarray to be good, sum of a should be equal to sum of b.

But in this case, sum of c is 13 and sum of minimal b is 12, so sum of c is greater than sum of minimal b by 1.

But in the example, for query 1 (1 to 5), it's 'YES', which suggests that it's possible to adjust b to make sum equal to sum of c.

Wait, but according to the code, it prints 'NO' if sum of a is less than sum of b, else 'YES'.

In this case, sum of a is greater than sum of b, so it would print 'YES'.

But how can I make sum of b equal to sum of a?

I need to adjust b_i to be greater than or equal to their minimal values, while keeping sum of b equal to sum of a.

In this example:

c: [1,2,1,4,5]

minimal b: [2,1,2,3,4], sum = 12

sum of c = 13

I need to increase the sum of b by 1 to make it equal to sum of c.

I can do this by increasing one of the b_i by 1.

For example, increase b[2] from 1 to 2.

Now, b = [2,2,2,3,4], sum = 13, which matches sum of c.

And all b_i are positive and not equal to a_i.

So, it's possible.

Hence, 'YES'.

Similarly, for query 2: 4 to 4, c[4] = 4

minimal b[4] = 3

sum of c = 4

sum of minimal b = 3

difference = 1

But subarray length is 1, which is handled separately in the code.

The code prints 'NO' if x == y.

Why is that?

Because for a single element, it's impossible to have b_i != a_i and sum of b equal to sum of a.

Because b_i != a_i, so b_i must be different from a_i, but sum of b must equal sum of a, which is only possible if b_i = a_i, which violates the condition.

Hence, for single element subarrays, it's always 'NO'.

In the example, query 2 is 'NO'.

Query 3: 3 to 4, c[3]=1, c[4]=4

sum of c = 5

minimal b: [2,3], sum = 5

difference = 0

So, sum of b equals sum of a, so 'YES'.

Query 4: 1 to 3, c[1]=1, c[2]=2, c[3]=1

sum of c = 4

minimal b: [2,1,2], sum = 5

sum of a = 4 < sum of minimal b = 5, so 'NO'.

Wait, but according to the code, it prints 'NO' if sum of a < sum of b, else 'YES', unless x == y, in which case always 'NO'.

In query 4, sum of a = 4 < sum of b = 5, so 'NO'.

Hence, the code seems to be correct based on this example.

But let's verify the logic.

The logic seems to be:

- Compute sum of a for the subarray.

- Compute sum of minimal b for the subarray.

- If sum of a < sum of minimal b, it's impossible to make sum of b equal to sum of a, so 'NO'.

- If sum of a >= sum of minimal b, then it's possible to adjust b_i to make sum of b equal to sum of a, by increasing some b_i by the necessary amount, as long as b_i remains positive and not equal to a_i.

- For subarrays of length 1, it's always 'NO', because b_i cannot be equal to a_i, but sum of b must equal sum of a, which is impossible.

Hence, the code seems correct.

Therefore, Correctness: **True**