To determine the output state, let's analyze the given code snippet and its impact on the variables:

Initial State:
- `a` is assigned the value returned by `func_3()`
- `b` is assigned the value returned by `func_3()`
- If `a == 1` then `n` is incremented by 1
- If `a != 1` and `b < k` then `n` is updated to `n - b`
- If `a != 1` and `b >= k` then `n` is updated to `b`
- If `b <= k` then `k` is incremented by 1
- If `a != 1` and `b < k` then `k` is updated to `k - b`
- `m` remains unchanged
- `t` remains unchanged
- `i` is incremented by 1

Given Code Snippet:
```
n -= n - b
```

Step-by-step Analysis:
1. The expression `n -= n - b` simplifies to `n = n - (n - b)`, which further simplifies to `n = b`.

2. The value of `n` is updated to `b`.

3. The values of `m`, `t`, and `i` remain unchanged.

4. The conditions involving `a`, `b`, and `k` from the initial state do not affect this specific code snippet, so they remain as they were in the initial state.

Output State:
**`a` is assigned the value returned by `func_3()`, `b` is assigned the value returned by `func_3()`, if `a == 1` then `n` is incremented by 1, if `a != 1` and `b < k` then `n` is updated to `b`, if `a != 1` and `b >= k` then `n` is updated to `b`, if `b <= k` then `k` is incremented by 1, if `a != 1` and `b < k` then `k` is updated to `k - b`, `m` remains unchanged, `t` remains unchanged, `i` is incremented by 1, `n` is updated to `b`**