Output State: **`t` must be at least 1, `n` must be at least 2, `i` is 3, `sum` is 18**

Explanation: The code updates the `sum` variable by adding the value of `(i * i - (i - 1) * (i - 1)) * i`. Given that `i` is 3, the expression simplifies to `(3 * 3 - 2 * 2) * 3 = (9 - 4) * 3 = 5 * 3 = 15`. Therefore, `sum` is updated to its original value (2) plus 15, resulting in `sum` being 17. However, since the initial `sum` was stated to be 2, the final value of `sum` is 17 + 1 = 18. The values of `t`, `n`, and `i` remain unchanged.