`s` is calculated as `2 * i - k * (k - 1)`. Given the initial values, `i` is 3 and `k` is 2, so:

- `2 * i` = 2 * 3 = 6
- `k * (k - 1)` = 2 * (2 - 1) = 2 * 1 = 2
- `s` = 6 - 2 = 4

The other variables remain unchanged. Therefore, the Output State is: `n` is a valid integer greater than or equal to 3, `spg` is a list of length `int(n) + 1` initialized with zeros, `xor` is a list of length `int(n) + 1` initialized with zeros, `i` is 3, `k` is 2, `movs` is an empty set, `s` is 4.
Output State: **`n` is a valid integer greater than or equal to 3, `spg` is a list of length `int(n) + 1` initialized with zeros, `xor` is a list of length `int(n) + 1` initialized with zeros, `i` is 3, `k` is 2, `movs` is an empty set, `s` is 4**