The value of `s` is updated by the expression `2 * i - k * (k - 1)`. Given the initial values `i` is 5 and `k` is 4, the calculation is as follows:

- `2 * i` = 2 * 5 = 10
- `k * (k - 1)` = 4 * (4 - 1) = 4 * 3 = 12
- `s` = 10 - 12 = -2

Thus, the new value of `s` is -2. All other variables remain unchanged.

Output State: **`n` is a valid integer greater than or equal to 3, `spg` is a list of length `int(n) + 1` initialized with zeros except `spg[3]` which is 0 and `spg[4]` which is 1, `xor` is a list of length `int(n) + 1` initialized with zeros except `xor[3]` which is 0 and `xor[4]` which is 1, `i` is 5, `k` is 4, `movs` is a set containing 0, `mex` is 1, `s` is -2, and `a` is 2**