The code snippet updates `total_sum` to `(total_sum + num) % MOD`. Given the initial state:
- `l` is a non-negative integer such that \(1 \leq l \leq r < 10^{18}\)
- `r` is a non-negative integer such that \(1 \leq l \leq r < 10^{18}\)
- `k` is an integer such that \(1 \leq k \leq 10\)
- `total_sum` is `l % MOD`
- `num` is equal to `l + 1`

The variable `total_sum` is updated as follows:
\[ \text{total\_sum} = (\text{total\_sum} + \text{num}) \% \text{MOD} \]
Since `num` is `l + 1`, we substitute this into the equation:
\[ \text{total\_sum} = ((l \% \text{MOD}) + (l + 1)) \% \text{MOD} \]
This simplifies to:
\[ \text{total\_sum} = (l \% \text{MOD} + l + 1) \% \text{MOD} \]

Therefore, the updated state of the variables is:
- `l` is a non-negative integer such that \(1 \leq l \leq r < 10^{18}\)
- `r` is a non-negative integer such that \(1 \leq l \leq r < 10^{18}\)
- `k` is an integer such that \(1 \leq k \leq 10\)
- `total_sum` is \((l \% \text{MOD} + l + 1) \% \text{MOD}\)
- `num` is equal to `l + 1`

Output State: **`l` is a non-negative integer such that \(1 \leq l \leq r < 10^{18}\); `r` is a non-negative integer such that \(1 \leq l \leq r < 10^{18}\); `k` is an integer such that \(1 \leq k \leq 10\); `total_sum` is \((l \% \text{MOD} + l + 1) \% \text{MOD}\); `num` is equal to `l + 1`**