`total_sum` is initially assigned the value \((l \% \text{MOD} + l + 1) \% \text{MOD}\). The code updates `total_sum` by adding `num` (which is `l + 2`) to it and taking the modulus with `MOD`. Therefore, the new value of `total_sum` will be \(((l \% \text{MOD} + l + 1) \% \text{MOD} + (l + 2)) \% \text{MOD}\).

The other variables remain unchanged.

Output State: **`l` is a non-negative integer such that \(1 \leq l \leq r < 10^{18}\), `r` is a non-negative integer such that \(1 \leq l \leq r < 10^{18}\), `k` is an integer such that \(1 \leq k \leq 10\), `num` is equal to `l + 2`, `total_sum` is \(((l \% \text{MOD} + l + 1) \% \text{MOD} + (l + 2)) \% \text{MOD}\)**