The code `ans += l - pos` updates the value of `ans` by adding the difference between `l` and `pos` to its current value. Given that `ans` is initially 0, the new value of `ans` will be `l - pos`.

Therefore, the Output State is: `n`, `pos`, `l`, `r` are integers such that 1 ≤ `n` ≤ 100, 1 ≤ `pos` ≤ `n`, 1 ≤ `l` ≤ `r` ≤ `n`, `ans` is `l - pos`, and `pos` is less than `l`.

Output State: **`n`, `pos`, `l`, `r` are integers such that 1 ≤ `n` ≤ 100, 1 ≤ `pos` ≤ `n`, 1 ≤ `l` ≤ `r` ≤ `n`, `ans` is `l - pos`, and `pos` is less than `l`.**