The code snippet `ans += pos - r` adds the difference between `pos` and `r` to the current value of `ans`.

Given the initial state:
- `n`, `pos`, `l`, `r` are integers such that 1 ≤ `n` ≤ 100, 1 ≤ `pos` ≤ `n`, 1 ≤ `l` ≤ `r` ≤ `n`.
- If `pos` < `l`, `ans` is set to `l - pos`. Otherwise, `ans` remains 0.
- The current value of `pos` is greater than `r`.

Since `pos` is greater than `r`, the condition `pos < l` does not affect the value of `ans` (as it only applies if `pos` is less than `l`). Therefore, the initial value of `ans` is 0.

After executing the code:
- `ans` is updated to `ans + (pos - r)`, which simplifies to `0 + (pos - r)` or simply `pos - r`.

Thus, the output state is:
Output State: **`n` is an integer such that 1 ≤ `n` ≤ 100, `pos` is an integer such that 1 ≤ `pos` ≤ `n`, `l` is an integer such that 1 ≤ `l` ≤ `n`, `r` is an integer such that 1 ≤ `r` ≤ `n`, `pos` is greater than `r`, `ans` is `pos - r`**.