First, let's break down the initial state:
- `n` is a positive integer such that \(1 \leq n \leq 2 \cdot 10^9\) and \(n \geq 6\).
- `count` is either 0 or 1.
- `rem` is \(n - 2 \cdot (a + b)\) with `rem` greater than 0 and even.
- `a` is \(n // 4 + 1\).
- `b` is \(n // 4 + 1\).
- `rem` is recalculated as \(n - 2 \cdot (n // 2 + 2)\).

Next, let's look at the code snippet:
```python
count += 1
```

This line increments the value of `count` by 1. Since the initial state does not specify the exact value of `count` (it is either 0 or 1), we will consider both cases.

### Case 1: `count` is initially 0
If `count` is initially 0, then after executing `count += 1`, `count` becomes 1.

### Case 2: `count` is initially 1
If `count` is initially 1, then after executing `count += 1`, `count` becomes 2.

The values of `n`, `rem`, `a`, and `b` remain unchanged because the code does not affect these variables.

Therefore, the output state is:

Output State: **`n` is a positive integer such that \(1 \leq n \leq 2 \cdot 10^9\) and \(n \geq 6\); `count` is either 1 or 2; `rem` is \(n - 2 \cdot (a + b)\) with `rem` greater than 0 and even; `a` is \(n // 4 + 1\); `b` is \(n // 4 + 1\); `rem` is recalculated as \(n - 2 \cdot (n // 2 + 2)\)**.