`y_max` is assigned the value of `math.floor(math.sqrt(y_max_sq))`. Given that `y_max_sq` is defined as \(4r - 1\), we substitute this into the equation to get:

\[ y_max = \math.floor(\sqrt{4r - 1}) \]

Since \(y_max\) was previously defined as \(\text{math.floor}(\sqrt{2r})\), and we now reassign it based on `y_max_sq`, we need to determine the relationship between these two expressions. For \(1 \leq r \leq 10^5\):

- If \(r = 1\), then \(y_max = \math.floor(\sqrt{2 \cdot 1}) = 1\) and \(y_max = \math.floor(\sqrt{4 \cdot 1 - 1}) = 1\).
- For larger values of \(r\), \(\sqrt{4r - 1}\) is slightly less than \(\sqrt{4r}\), which is \(2\sqrt{r}\), and since \(\sqrt{2r}\) is approximately \(\sqrt{2}\sqrt{r}\) (which is less than \(2\sqrt{r}\)), the floor function will keep them aligned.

Thus, for all valid \(r\), the new value of `y_max` remains consistent with the original definition of `y_max` as \(\text{math.floor}(\sqrt{2r})\).

The states of the other variables are not affected. Therefore, the Output State is: `r` is an integer such that \(1 \leq r \leq 10^5\); `r_squared` is \(r \times r\); `r_plus_1_squared` is \((r + 1) \times (r + 1)\); `x` is \(-r + 1\); `x_squared` is \((r - 1)^2\); `y_max` is \(\text{math.floor}(\sqrt{2r})\); `y_max_sq` is \(4r - 1\); `y_min_sq` is \(2r - 1\); `y_min` is `math.ceil(math.sqrt(2r - 1))`.

Output State: **`r` is an integer such that \(1 \leq r \leq 10^5\); `r_squared` is \(r \times r\); `r_plus_1_squared` is \((r + 1) \times (r + 1)\); `x` is \(-r + 1\); `x_squared` is \((r - 1)^2\); `y_max` is \(\text{math.floor}(\sqrt{2r})\); `y_max_sq` is \(4r - 1\); `y_min_sq` is \(2r - 1\); `y_min` is `math.ceil(math.sqrt(2r - 1))`**.