Alright, I've got this problem to solve. Let's see what it's asking for. So, I'm given two positive integers, n and m, and I need to find the number of ordered pairs (a, b) where 1 ≤ a ≤ n and 1 ≤ b ≤ m, with the condition that a + b is a multiple of b multiplied by the greatest common divisor of a and b. That is, a + b should be divisible by b * gcd(a, b).

First, I need to understand what this condition means. Let's break it down. Gcd(a, b) is the greatest common divisor of a and b. So, b * gcd(a, b) is b multiplied by that gcd. The condition is that a + b is divisible by this product.

Let me try to rephrase this condition to see if I can find a pattern or a way to simplify it. So, a + b should be divisible by b * gcd(a, b). That means (a + b) mod (b * gcd(a, b)) = 0.

Let me see if I can express a and b in terms of their gcd. Let’s denote d = gcd(a, b). Then, a = d * a' and b = d * b', where a' and b' are coprime integers (gcd(a', b') = 1).

Substituting these into the condition:

(a + b) should be divisible by b * d

Which is d * a' + d * b' should be divisible by d * b' * d

Simplify the numerator: d * (a' + b')

Denominator: d * b' * d = d^2 * b'

So, d * (a' + b') should be divisible by d^2 * b'

Simplify by dividing numerator and denominator by d:

(a' + b') should be divisible by d * b'

Wait, but d = gcd(a, b), and since a' and b' are coprime, d * b' = d * b', which is d * (b / d) = b.

Wait, that seems off. Let me double-check.

Given that a = d * a' and b = d * b', with gcd(a', b') = 1.

Then, a + b = d * a' + d * b' = d * (a' + b')

And b * gcd(a, b) = b * d = d * b'

So, the condition is that d * (a' + b') is divisible by d * b', which simplifies to a' + b' being divisible by b'.

But a' and b' are coprime, so what does this imply?

If a' + b' is divisible by b', then a' must be divisible by b', because b' divides b' and a' + b'. Therefore, b' divides a'.

But a' and b' are coprime, so the only way b' divides a' is if b' = 1.

Because if b' > 1, and b' divides a', but a' and b' are coprime, that would imply b' divides a', which can only happen if b' = 1.

Therefore, b' must be 1.

So, b = d * b' = d * 1 = d.

Therefore, b = d, which is gcd(a, b).

So, the condition simplifies to b = gcd(a, b).

But b = gcd(a, b) implies that a is a multiple of b.

Because gcd(a, b) is b, which means b divides a.

So, a is a multiple of b.

Therefore, the condition a + b is divisible by b * gcd(a, b) = b * b = b^2, when b = gcd(a, b).

Wait, but earlier I concluded that b = gcd(a, b), which implies that b divides a.

So, a is a multiple of b.

Let me see if this holds.

Assume b = gcd(a, b). Then, since gcd(a, b) divides b, and b divides a, this is consistent.

So, the condition seems to be that b divides a.

But is that the only condition? Wait, in the earlier steps, I think I might have missed something.

Let me try to verify with some examples.

Take n = 1, m = 1.

Possible pair: (1,1)

Check: a + b = 2, b * gcd(a,b) = 1 * 1 = 1, and 2 is divisible by 1. So, valid.

Total pairs: 1.

Which matches the first example.

Second example: n = 2, m = 3.

Possible pairs: (1,1), (1,2), (1,3), (2,1), (2,2), (2,3).

Check each:

(1,1): 1+1=2, 1*1=1, 2%1=0 → valid

(1,2): 1+2=3, 2*1=2, 3%2 ≠0 → invalid

(1,3): 1+3=4, 3*1=3, 4%3 ≠0 → invalid

(2,1): 2+1=3, 1*1=1, 3%1=0 → valid

(2,2): 2+2=4, 2*2=4, 4%4=0 → valid

(2,3): 2+3=5, 3*1=3, 5%3 ≠0 → invalid

Total valid pairs: 3, which matches the example.

Third example: n=3, m=5.

Possible pairs: (1,1), (1,2), (1,3), (1,4), (1,5), (2,1), (2,2), (2,3), (2,4), (2,5), (3,1), (3,2), (3,3), (3,4), (3,5).

Check each:

(1,1): valid

(1,2): invalid

(1,3): invalid

(1,4): invalid

(1,5): invalid

(2,1): valid

(2,2): valid

(2,3): invalid

(2,4): invalid

(2,5): invalid

(3,1): valid

(3,2): invalid

(3,3): 3+3=6, 3*3=9, 6%9 ≠0 → invalid

(3,4): invalid

(3,5): invalid

Total valid pairs: 4, matches the example.

From these examples, it seems that when b divides a, the condition holds.

Wait, in the third example, (3,3) is invalid, even though 3 divides 3.

Wait, 3 + 3 = 6, and b * gcd(a,b) = 3 * 3 = 9, and 6 is not divisible by 9. So, it's invalid.

So, my earlier assumption that b divides a is necessary but not sufficient.

Wait, in the earlier steps, I thought that b = gcd(a,b), which implies b divides a.

But in this case, (3,3) has b=3, a=3, gcd(a,b)=3, so b = gcd(a,b), but the condition fails.

Wait, no, 3 + 3 = 6, and b * gcd(a,b) = 9, and 6 is not divisible by 9.

So, my earlier conclusion that b = gcd(a,b) is not sufficient.

Wait, perhaps I need to revisit the condition.

Given that b = gcd(a,b), which implies that b divides a, and a is a multiple of b.

Let’s say a = k * b, where k is a positive integer.

Then, a + b = k*b + b = (k+1)*b

And b * gcd(a,b) = b * b = b^2

So, the condition is that (k+1)*b is divisible by b^2.

Which simplifies to (k+1)*b / b^2 = (k+1)/b is an integer.

Therefore, b divides (k+1).

Since k = a / b, and a is a multiple of b.

So, k is an integer, and b divides (k+1).

Therefore, k ≡ -1 mod b.

But k is a positive integer.

Wait, perhaps I'm overcomplicating this.

Let me consider that a = k*b, where k is a positive integer.

Then, a + b = b*(k + 1)

And b * gcd(a, b) = b * b, since gcd(a, b) = b.

So, the condition is that b*(k + 1) is divisible by b*b, which simplifies to (k + 1) is divisible by b.

Therefore, b divides (k + 1).

But k = a / b, and k is an integer.

So, b divides (a / b + 1).

Wait, that seems messy.

Let me think differently.

Given that a = k*b, then a / b = k.

So, the condition is that b divides (k + 1).

Meaning, k ≡ -1 mod b.

Since k is a positive integer, we can find the number of k's that satisfy k ≡ -1 mod b, and a = k*b ≤ n.

So, k ≤ n / b

And k ≡ -1 mod b

Which means k = m*b - 1, for some integer m ≥ 1.

Wait, let's see.

If k ≡ -1 mod b, then k = m*b - 1, for integer m ≥ 1.

Then, a = k*b = (m*b - 1)*b = m*b^2 - b

We need a ≤ n, so m*b^2 - b ≤ n

=> m*b^2 ≤ n + b

=> m ≤ (n + b) / b^2

Since m must be an integer ≥1, the number of valid m's is floor((n + b)/b^2)

But we need to ensure that m ≥1.

So, for each b from 1 to m, and for each m from 1 to floor((n + b)/b^2), we have one valid a.

Therefore, the total number of valid pairs is sum over b from 1 to m of floor((n + b)/b^2)

Wait, but in the examples, for n=1, m=1, this would be floor((1 + 1)/1^2) = floor(2/1) =2, but the correct answer is 1.

Hmm, that doesn't match.

Wait, perhaps I made a mistake.

Let me recast this.

Given a = k*b, and k ≡ -1 mod b.

Wait, k ≡ -1 mod b means k = m*b -1 for some integer m ≥1.

Then a = k*b = (m*b -1)*b = m*b^2 - b

We need a ≤ n, so m*b^2 - b ≤ n

=> m*b^2 ≤ n + b

=> m ≤ (n + b)/b^2

So, for each b from 1 to m, the number of valid m's is floor((n + b)/b^2)

But in the first example, n=1, m=1.

floor((1 +1)/1^2) = floor(2/1) =2

But only (1,1) is valid, so it's counting (1,1) and perhaps another pair that isn't valid.

Wait, what's happening here.

Wait, for b=1, m ≤ (1 +1)/1^2 =2, so m=1 and m=2.

For m=1, a=1*1^2 -1 =0, but a must be ≥1, so invalid.

For m=2, a=2*1^2 -1=1, which is valid.

So, only one valid pair, which matches the example.

So, in this case, although floor((n+b)/b^2)=2, only m=2 gives a valid a=1.

m=1 gives a=0, which is invalid.

So, perhaps we need to adjust the lower limit of m to ensure a ≥1.

So, a = m*b^2 - b ≥1

=> m*b^2 - b ≥1

=> m*b^2 ≥ b +1

=> m ≥ (b +1)/b^2

But b is ≥1, so (b +1)/b^2 can be less than 1, so m starts from 1.

But in practice, for b=1, m needs to be at least 2 to have a ≥1.

For b=2, m*b^2 -b =4m -2 ≥1 =>4m ≥3=>m ≥1

For b=3,9m -3 ≥1 =>9m ≥4=>m ≥1

So, for b ≥2, m starts from 1, but for b=1, m starts from 2.

So, perhaps we need to handle b=1 separately.

For b=1, a = m*1^2 -1 =m -1

We need a ≤n, so m -1 ≤n =>m ≤n +1

But a ≥1, so m -1 ≥1 =>m ≥2

So, for b=1, the number of valid m's is from 2 to n+1, which is n elements.

But in the first example, n=1, so m from 2 to 2, giving a=1, which is valid.

For b ≥2, m starts from 1.

So, total pairs:

For b=1: floor((n +1)/1^2) -1 = (n +1) -1 =n

For b ≥2: sum over b from 2 to m of floor((n +b)/b^2)

Wait, but in the first example, n=1, m=1, so only b=1 contributes n=1, which matches.

In the second example, n=2, m=3.

b=1: n=2 pairs

b=2: floor((2 +2)/4)=floor(4/4)=1

b=3: floor((2 +3)/9)=floor(5/9)=0

Total: 2 +1 +0=3, which matches the example.

In the third example, n=3, m=5.

b=1:3 pairs

b=2: floor((3 +2)/4)=floor(5/4)=1

b=3: floor((3 +3)/9)=floor(6/9)=0

b=4: floor((3 +4)/16)=floor(7/16)=0

b=5: floor((3 +5)/25)=floor(8/25)=0

Total:3 +1 +0 +0 +0=4, which matches.

Fourth example: n=10, m=8.

b=1:10 pairs

b=2: floor((10 +2)/4)=3

b=3: floor((10 +3)/9)=1

b=4: floor((10 +4)/16)=1

b=5: floor((10 +5)/25)=1

b=6: floor((10 +6)/36)=0

b=7: floor((10 +7)/49)=0

b=8: floor((10 +8)/64)=0

Total:10 +3 +1 +1 +1 +0 +0 +0=16, but the example shows 14.

Wait, discrepancy here.

Wait, in the note, it shows 14 pairs, but according to this, it's 16.

Hmm, perhaps I'm miscounting.

Wait, in b=1, a can be from 1 to 10, but we need to ensure that a + b is divisible by b * gcd(a,b).

For b=1, gcd(a,1)=1, so a +1 should be divisible by 1, which is always true.

So, all a from 1 to 10 are valid, that's 10 pairs.

b=2: floor((10 +2)/4)=3, so m=1,2,3

m=1: a=1*4 -2=2, which is valid.

m=2: a=2*4 -2=6, valid.

m=3: a=3*4 -2=10, valid.

So, 3 pairs.

b=3: floor((10 +3)/9)=1

m=1: a=1*9 -3=6, which is valid.

b=4: floor((10 +4)/16)=1

m=1: a=1*16 -4=12, but 12 >10, so invalid.

So, no pair for b=4.

Similarly for higher b, no pairs.

So, total pairs:10 +3 +1 +0 +0 +0 +0 +0=14, which matches the example.

So, perhaps I miscounted earlier.

Therefore, the total number of pairs is n (for b=1) plus sum over b=2 to m of floor((n +b)/b^2)

But we need to ensure that for b ≥2, floor((n +b)/b^2) counts only valid a's, i.e., a ≤n.

In the case of b=4, floor((10 +4)/16)=1, but a=12>10, so it's invalid.

So, perhaps we need to adjust the formula to take into account that a ≤n.

Therefore, for each b, the number of valid m's is floor(min(n +b -1)/b^2 )

But in the case of b=4, n=10, floor((10 +4)/16)=1, but a=12>10, so we need to exclude it.

Wait, perhaps it's better to compute floor((n +b)/b^2 ), but then check if a ≤n.

Wait, but in the earlier step, a = m*b^2 - b ≤n

m ≤ floor((n +b)/b^2 )

But for b=4, n=10, m ≤ floor((10 +4)/16)=1

a=1*16 -4=12>10, so invalid.

So, in this case, we need to set floor((n +b -1)/b^2 )

Wait, perhaps floor((n +b -1)/b^2 )

Let's check:

For b=4, n=10, floor((10 +4 -1)/16)=floor(13/16)=0

Which would correctly give no pairs for b=4.

Similarly, for b=2, floor((10 +2 -1)/4)=floor(11/4)=2

m=1: a=4 -2=2 ≤10

m=2:8 -2=6 ≤10

m=3:12 -2=10 ≤10

Wait, but floor(11/4)=2, which would miss m=3.

Wait, 11/4=2.75, floor is 2, but m=3 is allowed because 3*4 -2=10 ≤10.

Wait, so m=3 is allowed, but floor(11/4)=2 doesn't account for it.

Wait, perhaps I need to use ceiling instead.

Wait, no.

Wait, m ≤ (n +b -1)/b^2

For m=3, 3*16 -4=48 -4=44 >10, which is invalid.

Wait, no, for b=2, m=3: a=3*4 -2=10 ≤10, which is valid.

Wait, b=4: m=1: a=16 -4=12 >10, invalid.

So, for b=4, no valid m.

For b=2, m=1: a=2 ≤10

m=2:6 ≤10

m=3:10 ≤10

So, m=1,2,3 are valid for b=2.

But floor((10 +2 -1)/4)=floor(11/4)=2, which would miss m=3.

So, perhaps floor((n +b -1)/b^2 ) is not sufficient.

Wait, perhaps it's floor((n +b -1)/(b^2 )) is the correct formula, but in this case, it gives floor(11/4)=2, but m=3 is also valid because a=10 ≤n.

Wait, but 3*4 -2=10 ≤10.

So, m=3 is valid.

Wait, but (n +b -1)/b^2 =11/4=2.75, floor is 2.

But m=3 is still valid because a=10 ≤n.

Wait, perhaps the correct formula is floor((n +b -1)/(b^2 -1)), but I need to think differently.

Wait, perhaps it's better to express m ≤ (n +b)/b^2

But in the case of b=2, n=10, (10 +2)/4=12/4=3, floor is 3, which matches m=1,2,3.

For b=4, (10 +4)/16=14/16=0.875, floor is 0, but a=12 >10, which is invalid.

Wait, but m=1: a=16 -4=12 >10, invalid.

So, perhaps it's floor((n +b)/b^2 ) -1, but then for b=2, floor(12/4)=3 -1=2, but we have m=1,2,3 as valid.

Wait, confusing.

Perhaps it's better to iterate over b from 1 to m, and for each b, compute floor((n +b)/b^2 ), but then check if a ≤n.

In practice, for b=1, a from 1 to n.

For b ≥2, m from 1 to floor((n +b)/b^2 ), and a = m*b^2 - b ≤n.

So, in code, for b from 2 to m:

max_m = floor((n +b)/b^2 )

for m from 1 to max_m:

a = m*b^2 - b

if a ≤n, count it.

But in the fourth example, n=10, m=8.

b=2: floor(12/4)=3, a=2,6,10 ≤10, all valid.

b=3: floor(13/9)=1, a=9 -3=6 ≤10, valid.

b=4: floor(14/16)=0, no a.

b=5: floor(15/25)=0, no a.

b=6: floor(16/36)=0, no a.

b=7: floor(17/49)=0, no a.

b=8: floor(18/64)=0, no a.

Total:10 +3 +1=14, which matches.

So, in code, it's feasible to iterate over b from 2 to m, compute floor((n +b)/b^2 ), and add that to the total.

But for large n and m, this could be slow, as t can be up to 10^4, and n and m up to 2*10^6, with the sum of n and m over all test cases up to 2*10^6.

So, we need an efficient way to compute this.

Let’s see if we can optimize the calculation.

For b=1, it's simply n.

For b ≥2, we need to sum floor((n +b)/b^2 ) over b from 2 to m.

But floor((n +b)/b^2 ) can be rewritten as floor(n/b^2 + 1/b).

But since b ≥2, 1/b <1, so floor(n/b^2 + 1/b) = floor(n/b^2 ) or floor(n/b^2 ) +1 depending on the fractional part.

Wait, but n/b^2 +1/b could be such that the fractional part of n/b^2 plus 1/b is less than 1 or equal to or greater than 1.

This seems messy.

Alternatively, perhaps we can consider that floor((n +b)/b^2 ) = floor(n/b^2 + 1/b) = floor(n/b^2 ) + floor fractional part.

But again, it's complicated.

Let me think about the number of operations required.

For each test case, if we iterate over b from 2 to m, and compute floor((n +b)/b^2 ), it's O(m) per test case.

But m can be up to 2*10^6, and t up to 10^4, but the sum of m over all test cases is up to 2*10^6, so overall time complexity is O(2*10^6), which should be acceptable.

But perhaps we can optimize it further.

Let’s see.

For b from 2 to m, floor((n +b)/b^2 ) can be considered as floor(n/b^2 + b/b^2 ) = floor(n/b^2 + 1/b).

Since b ≥2, 1/b <1, so floor(n/b^2 + 1/b) = floor(n/b^2 ) + floor(1/b) = floor(n/b^2 ) +0 = floor(n/b^2 )

Because 1/b <1, so adding it to n/b^2 doesn't increase the floor value unless n/b^2 +1/b ≥ ceiling(n/b^2 ), but since 1/b <1, it's complex.

Wait, perhaps it's safer to compute floor((n +b)/b^2 ) directly.

In code, this would be (n +b) // b**2

So, in Python, it's straightforward.

So, the total number of pairs is n (for b=1) plus sum over b=2 to m of (n +b) // b**2

Now, implementing this directly in code would be acceptable, given the constraints.

But let's look at the provided code to see if it matches this logic.

Looking at the provided code:

import math

"""

~~~~~~~~~~~~~~~~~~~~~~~~~~~~~~~~~~~~~~~~~~~~~~~~~~~~~~~~~~~~~~~~~~~~~~~~~~**

*                      BISMILLAHIR RAHMANIR RAHEEM                         *                                                    *

**~~~~~~~~~~~~~~~~~~~~~~~~~~~~~~~~~~~~~~~~~~~~~~~~~~~~~~~~~~~~~~~~~~~~~~~~~~

"""

t = int(input())

for _ in range(t):

func_1()

def func_1():

(n, k) = map(int, input().split())

ans = n

root = int(math.sqrt(n)) + 1

for i in range(2, root + 1):

cnt = i * i

ans += (n + i) // cnt

print(ans)

So, it defines a function func_1() that reads n and k (which should be m), then initializes ans = n, which accounts for b=1.

Then, it computes root = sqrt(n) +1, and iterates i from 2 to root +1.

For each i, cnt = i*i, which is b^2.

Then, ans += (n + i) // cnt, which is floor((n +b)/b^2 )

Wait, but b is i, and b^2 is cnt.

So, it's summing floor((n +b)/b^2 ) for b from 2 to sqrt(n) +1.

Wait, but in our earlier reasoning, we need to sum over b from 2 to m.

But in the code, it's summing over b from 2 to sqrt(n) +1.

Wait, that's a discrepancy.

In the code, it's only iterating b up to sqrt(n) +1, but m can be up to 2*10^6.

So, it's missing b's from sqrt(n)+1 to m.

But in the examples, it seems to give the correct answer.

Wait, in the fourth example, n=10, m=8.

sqrt(10)+1 ≈3+1=4.

So, it iterates b=2,3,4.

In our earlier calculation, b=2,3,4,5,6,7,8.

But in this case, b=5,6,7,8 don't contribute because floor((10 +b)/b^2 )=0.

So, in this case, it's okay.

But is this always the case?

Let’s check for n=100, m=1233.

sqrt(100)+1=10+1=11.

So, it iterates b=2 to 11.

But m=1233, which is much larger.

Do b from 12 to 1233 contribute anything?

Let’s see.

For b=12, floor((100 +12)/144)=floor(112/144)=0

Similarly, higher b's will have floor((n +b)/b^2 )=0.

So, in this case, summing up to b=sqrt(n)+1 is sufficient.

Is this always true that for b > sqrt(n)+1, floor((n +b)/b^2 )=0?

Let’s see.

Suppose b > sqrt(n) +1.

Then, b^2 > (sqrt(n) +1)^2 = n +2*sqrt(n) +1.

So, (n +b)/b^2 < (n +b)/(n +2*sqrt(n) +1)

Since b > sqrt(n)+1, n +b > n + sqrt(n)+1.

So, (n +b)/b^2 < (n + sqrt(n)+1)/(n +2*sqrt(n)+1)

For large n, this ratio approaches 1, but since b^2 grows faster than n +b, for sufficiently large b, (n +b)/b^2 <1, hence floor((n +b)/b^2 )=0.

Therefore, for b > sqrt(n)+1, floor((n +b)/b^2 )=0.

Hence, summing up to b=sqrt(n)+1 is sufficient.

Therefore, the code is correct in iterating b from 2 to sqrt(n)+1.

Thus, the provided code correctly calculates the number of valid pairs as per the derived formula.

Hence, the program is correct.

**Final Answer**

\boxed{\text{The program is correct.}}