Let's analyze the initial state and the provided code snippet step by step:

### Initial State:
- `t` is an integer such that \(1 \leq t \leq 1000\).
- `n` is an input integer such that \(1 \leq n \leq 10^{18}\).
- `k` is an input integer such that \(1 \leq k \leq 10^{18}\).
- `n` is greater than or equal to `k`.
- `n` is not equal to `k`.
- The condition \((k - 1 < n - k + 1)\) holds true.

### Analysis:
1. **Condition Analysis**:
   - The condition \((k - 1 < n - k + 1)\) simplifies to:
     \[
     k - 1 < n - k + 1
     \]
     Simplifying further:
     \[
     k - 1 < n - k + 1 \implies k - 1 < n - k + 1 \implies k - 1 < n - k + 1 \implies 2k - 2 < n \implies 2k < n + 2 \implies k < \frac{n + 2}{2}
     \]
   - This condition must hold true for the given values of `n` and `k`.

2. **Print Statement**:
   - The code snippet contains a simple `print` statement:
     ```python
     print('YES')
     ```

### Conclusion:
- The condition \((k - 1 < n - k + 1)\) is given to be true.
- Since the condition is true, the `print` statement will execute and print the string `'YES'`.

### Final Output:
Output: **YES**