The code snippet `r -= 1` decrements the value of `r` by 1. The other variables remain unchanged. Given the initial state, `r` was initially `n`. After the decrement, `r` becomes `n - 1`. 

Here is the updated output state:

Output State: **`t` is an integer such that \(1 \leq t \leq 10^4\); `n` is an integer such that `n <= le`; `a` is a list of integers derived from the input; `le` is the length of the list `a`; `l` is `n - 1`; `r` is `n - 1`; `st` is `n`; `end` is `1`; `a[n]` equals `a[n - 1]`; if `a[0] == a[-1]`, then `ans` is `max(0, le - (st + end))`; otherwise, `ans` is `le - max(st, end)`**.