The code snippet provided is `r -= 1`, which means the value of `r` is decremented by 1.

Given the initial state:
- `t` is an integer such that \(1 \leq t \leq 10^4\)
- `n` is an integer such that `n <= le`
- `a` is a list of integers derived from the input
- `le` is the length of the list `a`
- `l` is `n - 1`
- `r` is `n`
- `st` is `n`
- `end` is `3`
- `a[n]` equals `a[n - 1]`
- If `a[0] == a[-1]`, then `ans` is `max(0, le - (st + end))`; otherwise, `ans` is `le - max(st, end)`

The only variable affected by the code snippet is `r`. Since `r` was initially equal to `n`, after executing `r -= 1`, `r` will be equal to `n - 1`.

The other variables remain unchanged.

Output State: **`t` is an integer such that \(1 \leq t \leq 10^4\); `n` is an integer such that `n <= le`; `a` is a list of integers derived from the input; `le` is the length of the list `a`; `l` is `n - 1`; `r` is `n - 1`; `st` is `n`; `end` is `3`; `a[n]` equals `a[n - 1]`; if `a[0] == a[-1]`, then `ans` is `max(0, le - (st + end))`; otherwise, `ans` is `le - max(st, end)`**.