To execute the provided code and determine the output state:

1. We have the variables already defined:
   - `m`: a positive integer such that 1 <= `m` <= 10^9
   - `a`: a positive integer such that 1 <= `a` <= 10^5
   - `b`: a positive integer such that 1 <= `b` <= 10^5
   - `g` = 1
   - `k` = `a + b - 1`
   - `sum_k` = `(a + b - 1) * (a + b) // 2`

2. The code computes `sum_m` as follows:
   - `sum_m` = `m * (m + 1) // 2` - `k * (k - 1) // 2`
   - Here, `k` has already been defined as `a + b - 1`, so its value is retained in the calculation of `sum_m`.

3. Since all other variable states remain unchanged, we summarize them into the output state.

Output State: **`m` is a positive integer such that 1 <= `m` <= 10^9; `a` is a positive integer such that 1 <= `a` <= 10^5; `b` is a positive integer such that 1 <= `b` <= 10^5; `g` is equal to 1; `k` is equal to `a + b - 1`; `sum_k` is equal to `(a + b - 1) * (a + b) // 2`; `sum_m` is equal to `m * (m + 1) // 2 - (a + b - 1) * (a + b - 2) // 2`.**