Let's break down the given initial state and the code snippet to determine what will be printed.

1. **Variables and Conditions:**
   - `t` is an integer such that \(0 \leq t \leq 499\).
   - `p1`, `p2`, and `p3` are integers.
   - The sum of `p1`, `p2`, and `p3` is odd.
   - `low` is the minimum of `p3 - p1` and `p3 - p2`.
   - `high` is the maximum of `p3 - p1` and `p3 - p2`.
   - `cur` is equal to `low`.
   - `p1 - cur` is less than or equal to `p2 - (p3 - cur)`.

2. **Expression to Evaluate:**
   - The expression to be printed is `p1 - cur + p3`.

3. **Analysis:**
   - Since `cur` is set to `low`, which is the minimum of `p3 - p1` and `p3 - p2`, we need to consider the values of `p3 - p1` and `p3 - p2`.
   - Let's denote `p3 - p1` as `diff1` and `p3 - p2` as `diff2`.
   - Therefore, `low` is `min(diff1, diff2)`.
   - `cur` is `low`, so `cur` is either `diff1` or `diff2`, whichever is smaller.

4. **Expression Substitution:**
   - The expression `p1 - cur + p3` can be rewritten using the definition of `cur`.
   - If `cur` is `diff1`, then `cur = p3 - p1`.
     - Substituting `cur = p3 - p1` into the expression, we get:
       \[
       p1 - (p3 - p1) + p3 = p1 - p3 + p1 + p3 = 2p1
       \]
   - If `cur` is `diff2`, then `cur = p3 - p2`.
     - Substituting `cur = p3 - p2` into the expression, we get:
       \[
       p1 - (p3 - p2) + p3 = p1 - p3 + p2 + p3 = p1 + p2
       \]

5. **Condition Analysis:**
   - The condition `p1 - cur` is less than or equal to `p2 - (p3 - cur)` needs to be satisfied.
   - If `cur` is `diff1` (i.e., `cur = p3 - p1`), the condition becomes:
     \[
     p1 - (p3 - p1) \leq p2 - (p3 - (p3 - p1)) \implies 2p1 - p3 \leq p2 - p1 \implies 3p1 - p3 \leq p2
     \]
   - If `cur` is `diff2` (i.e., `cur = p3 - p2`), the condition becomes:
     \[
     p1 - (p3 - p2) \leq p2 - (p3 - (p3 - p2)) \implies p1 - p3 + p2 \leq p2 - p2 \implies p1 - p3 \leq 0 \implies p1 \leq p3
     \]
   - Given that `low` is the minimum of `p3 - p1` and `p3 - p2`, and the condition `p1 - cur` is less than or equal to `p2 - (p3 - cur)`, it is more likely that `cur` is `diff2` (i.e., `cur = p3 - p2`), because this condition is generally easier to satisfy.

6. **Conclusion:**
   - Based on the analysis, the expression `p1 - cur + p3` simplifies to `p1 + p2` when `cur` is `p3 - p2`.

Therefore, the output of the `print` statement is `p1 + p2`.

Output: **p1 + p2**