Let's break down the initial state and the logic step by step:

1. **Initial Values:**
   - `a` is the integer value of the first input split by space.
   - `b` is the integer value of the second input split by space.
   - `t1` is calculated as `b * 28 - (b * 2 // 5) * 15 + b * 4`.
   - `t2` is calculated as `a - t1`.

2. **Updating `t`:**
   - `t1` is updated to `t * 15 - b * 4`.
   - If `t1 >= a`, then `t` remains unchanged.
   - Otherwise, if `t2 % 15 == 0`, then `t` is updated to `t + (a - t1) // 15`.
   - Otherwise, `t` is updated to `t + t2 // 15 + 1`.

3. **Final Calculation:**
   - We need to determine the value of `t` after the updates.

Let's go through the steps with a concrete example. Suppose the inputs are `a = 100` and `b = 5`.

- Calculate `t1`:
  \[
  t1 = 5 \times 28 - (5 \times 2 // 5) \times 15 + 5 \times 4 = 140 - 0 + 20 = 160
  \]

- Calculate `t2`:
  \[
  t2 = 100 - 160 = -60
  \]

- Update `t1`:
  \[
  t1 = t \times 15 - 5 \times 4 = t \times 15 - 20
  \]

- Since `t2` is negative, it doesn't affect the calculation directly, but we need to consider the conditions for updating `t`.

Given the conditions:
- If `t1 >= a`, `t` remains unchanged.
- If `t2 % 15 == 0`, `t` is updated to `t + (a - t1) // 15`.
- Otherwise, `t` is updated to `t + t2 // 15 + 1`.

Since `t2` is negative, let's assume `t` starts as 0 for simplicity (since the exact initial value of `t` isn't specified).

- `t1` becomes:
  \[
  t1 = 0 \times 15 - 20 = -20
  \]

- Since `-20 < 100`, we check the conditions:
  - `t2 % 15 != 0` because `-60 % 15 = 0` is false.
  - Therefore, `t` is updated to `t + (-60 // 15 + 1) = 0 + (-4 + 1) = -3`.

However, since `t` cannot be negative in this context, we should interpret it as 0.

Thus, the final value of `t` is 0.

Output: **0**