Let's break down the given initial state and the print statement step by step:

1. **Initial State:**
   - `i` is `n - 2`, where `n` is the length of the string `s`.
   - The character at index `i` in `s` is not `'>`'.
   - `l` is greater than `r`.
   - The current value of `r` is `0`.

2. **Print Statement:**
   ```python
   print(n - i + (i - idx_A[l - 1]) * 2, end=' ')
   ```

3. **Analysis:**
   - We know `i = n - 2`.
   - Since `r = 0`, the expression `idx_A[l - 1]` simplifies to `idx_A[0]` because `l - 1` is `0` (since `l > r` and `r = 0`).
   - Therefore, the expression inside the print statement becomes `n - (n - 2) + (i - idx_A[0]) * 2`.

4. **Substitute Known Values:**
   - Substitute `i = n - 2` into the expression:
     \[
     n - (n - 2) + ((n - 2) - idx_A[0]) * 2
     \]
   - Simplify the expression:
     \[
     n - n + 2 + (n - 2 - idx_A[0]) * 2 = 2 + (n - 2 - idx_A[0]) * 2
     \]
     \[
     = 2 + 2(n - 2 - idx_A[0]) = 2 + 2n - 4 - 2idx_A[0] = 2n - 2 - 2idx_A[0]
     \]

5. **Final Expression:**
   - The final expression to be printed is `2n - 2 - 2idx_A[0]`.

Given the above steps, the output of the print statement is:

Output: **2n - 2 - 2idx_A[0]**