To determine what will be printed, let's break down the initial state and the code step by step:

1. **Initial State:**
   - `i` is `n - 2`, where `n` is the length of the string `s`.
   - `r` is decreased by 1 (though the exact value of `r` is not specified, it will be `n - 3` after this operation).
   - `a` is the character at index `l - 1` of the string `s` plus `(i - idx_A[l - 1]) * l`.
   - `b` is the character at index `r` of the string `B` minus `B[r - l]` minus `(idx_B[r - l] - i) * (r - l)` plus `(idx_B[r] - i) * l` if `r - l >= 0`, otherwise `b` remains unchanged.

2. **Code Snippet:**
   ```python
   print(a * 2 + b * 2 + i + 1, end=' ')
   ```

Given the initial state, let's assume specific values for clarity (since the exact values of `s`, `B`, `l`, `idx_A`, and `idx_B` are not provided):

- Let's assume `n = 5` (so `i = n - 2 = 3`).
- Assume `r` is initially `4` (after being decreased by 1, it becomes `3`).
- Assume `l = 2` (this is just an example; the actual value of `l` is not provided).
- Assume `idx_A[1] = 1` (since `l - 1 = 1`).
- Assume `idx_B[1] = 2` (since `r - l = 1`).
- Assume `idx_B[3] = 4` (since `r = 3`).

Now, let's calculate the values of `a` and `b`:

- **Calculating `a`:**
  \[
  a = s[l - 1] + (i - idx_A[l - 1]) \cdot l
  \]
  Given `s` is a string, `s[1]` would be the second character of `s`. For simplicity, let's assume `s = "abcde"`, so `s[1] = 'b'` (assuming ASCII values, `ord('b') = 98`).

  \[
  a = 98 + (3 - 1) \cdot 2 = 98 + 4 = 102
  \]

- **Calculating `b`:**
  \[
  b = B[r] - B[r - l] - (idx_B[r - l] - i) \cdot (r - l) + (idx_B[r] - i) \cdot l \quad \text{if } r - l \geq 0
  \]
  Given `B` is a string, `B[3]` would be the fourth character of `B`. For simplicity, let's assume `B = "fghij"`, so `B[3] = 'h'` (assuming ASCII values, `ord('h') = 104`), and `B[2] = 'g'` (assuming ASCII values, `ord('g') = 103`).

  \[
  b = 104 - 103 - (2 - 3) \cdot 1 + (4 - 3) \cdot 2 = 104 - 103 + 1 + 2 = 3
  \]

Finally, we substitute these values into the print statement:

\[
a * 2 + b * 2 + i + 1 = 102 * 2 + 3 * 2 + 3 + 1 = 204 + 6 + 3 + 1 = 214
\]

Thus, the output will be:

Output: **214**