
Given a Python loop, an initial execution state, and the output states after the first 3 iterations of the loop, determine the output state after all the executions of the loop have finished. 

You must adhere to the text format: Output State: **output state.**

Initial State: `l` is 0, `n` is the length of the string `s`, `j` is 0, `i` is `n - 1`, the list `idx_B` contains all indices in `s` where the character is '<', `B` is a list containing the cumulative sums of the distances from the last occurrence of '>' up to the current index `i`, adjusted by the length of `idx_A`, `r` is the length of the list `B`.
Code of the loop:
for i in range(0, n):
    if s[i] == '>':
        if l < r:
            a = A[l]
            x = r - (l + 2)
            b = B[r - 1]
            if x >= 0:
                b = b - B[x]
                b = b - (idx_B[x] - idx_B[r - 1]) * (x + 1)
            b = b + (idx_B[r - 1] - i) * (l + 1)
            print(a * 2 + b * 2 + i + 1, end=' ')
        elif r == 0:
            print(n - i, end=' ')
        else:
            a = B[r - 1] + (idx_B[r - 1] - i) * r
            b = A[l - 1]
            if l - r > 0:
                b = b - A[l - r - 1]
                b = b - (idx_A[l - 1] - idx_A[l - r - 1]) * (l - r)
            b = b + (i - idx_A[l - 1]) * r
            print(a * 2 + b * 2 + (n - i), end=' ')
        l += 1
    else:
        r -= 1
        if l <= r:
            if l == 0:
                print(i + 1, end=' ')
            else:
                a = A[l - 1]
                a = a + (i - idx_A[l - 1]) * l
                b = B[r]
                if r - l >= 0:
                    b = b - B[r - l]
                    b = b - (idx_B[r - l] - i) * (r - l)
                b = b + (idx_B[r] - i) * l
                print(a * 2 + b * 2 + i + 1, end=' ')
        elif r == 0:
            print(n - i + (i - idx_A[l - 1]) * 2, end=' ')
        else:
            a = B[r]
            b = A[l - 1]
            if l - r - 1 > 0:
                b = b - A[l - r - 2]
                b = b - (idx_A[l - 1] - idx_A[l - r - 2]) * (l - r - 1)
            b = b + (i - idx_A[l - 1]) * (r + 1)
            print(a * 2 + b * 2 + (n - i), end=' ')


The output state after the loop executes the first 3 of times includes what needed to be true for the loop to execute at least that number of times:

Output State after the loop executes 1 time: `i` is either `n - 2` or `n - 1`, `n` is the length of the string `s`, and `l` and `r` are updated according to the following rules:
- If the character at index `i` in `s` is '>', then `l` is incremented by 1.
- If the character at index `i` in `s` is not '>', then:
  - If `l <= r`, then:
    - If `l` equals 0, `r` is greater than or equal to `l`.
    - Otherwise, `a` is the character at index `l - 1` in `s` plus `(i - idx_A[l - 1]) * l`, `b` is the character at index `r - l` in `s` minus `(idx_B[r - l] - i) * (r - l)` plus `(idx_B[r] - i) * l`, and `l` is greater than 0 with the difference between `r` and `l` being greater than or equal to 0.
  - If `l > r`, then:
    - If `r` is 0, `r` is 0.
    - Otherwise, `r` is not 0, `a` is the character at index `r` in `s`, `b` is the character at index `l - 1` in `s` minus the ASCII value of the character at index `l - r - 2` in `s` minus `(idx_A[l - 1] - idx_A[l - r - 2]) * (l - r - 1)` if `l - r - 1 > 0`, otherwise `b` remains unchanged; `b` is updated by adding `(i - idx_A[l - 1]) * (r + 1)` to its current value.

**Output State after the loop executes 2 times**: Postcondition: `i` is either `n - 2` or `n - 3`, `n` is the length of the string `s`, `l` and `r` are updated according to the following rules:
- If `s[i] == '>'` and `l < r`, then `l` is incremented by 1, and `b` is adjusted based on the value of `x`.
- If `s[i] == '>'` and `l >= r`, then `i` remains `n - 1`, `l` and `r` remain unchanged, and `b` is adjusted based on the values of `idx_A` and `idx_B`.
- If `s[i] != '>'`, then `r` is decreased by 1, and `a` and `b` are updated as follows:
  - If `l <= r`, then `a` is the character at index `l - 1` of the string `s` plus `(i - idx_A[l - 1]) * l`, and `b` is the character at index `r` of the string `B` minus the character at index `r - l` of the string `B` minus `(idx_B[r - l] - i) * (r - l)` plus `(idx_B[r] - i) * l` if `l` is not 0; otherwise, `i` is `n - 2` and `r` is decreased by 1.
  - If `l > r`, then `r` is decreased by 1, `a` is the character at index `r-1` of the string `s`, and `b` is updated to `b + (i - idx_A[l - 1]) * (r + 1)` if `r` is not 0; otherwise, `r` remains unchanged.

**Output State after the loop executes 3 times**: `i` is `n - 1` or `n - 2`, `n` is the length of the string `s`, `l` and `r` are updated according to the specified conditions. If `s[i] == '>',` then `l` is incremented by 1, `r` and `x` remain unchanged, `b` remains unchanged, `a` remains unchanged, `idx_B` and `idx_A` remain unchanged. Otherwise, `i` becomes `n - 2`, `r` is decreased by 1, if `l == 0`, `r` remains unchanged, otherwise `r` is further decreased by 1, `a` is calculated as the character at index `l - 1` of the string `s` plus `(i - idx_A[l - 1]) * l`, and `b` is calculated as the character at index `r` of the string `B` minus `B[r - l]` minus `(idx_B[r - l] - i) * (r - l)` plus `(idx_B[r] - i) * l` if `r - l >= 0`, otherwise `b` remains unchanged. If `r` equals 0, `a` and `b` are undefined. Otherwise, `a` is the character at index `r-1` of the string `s`, `b` is the character at index `l - 1` of the string `s`, and `b` is incremented by `(i - idx_A[l - 1]) * (r + 1)`.




What is the ouput state after the loop executes all the iterations? Change the values of only the variables in the loop head and body.The state of the other variables in the precondition that are not affected by the loop head and body must remain unchanged.
In your response strictly use the format: Output State: **the output state you calculate.**, and describe this output state in Natural language easily understandable by humans.

