Let's break down the initial state and the print statement step by step:

1. **Initial State:**
   - `n` and `k` are positive integers provided by the user such that 1 <= `n` <= 26 and 1 <= `k` <= 26.
   - `t` is greater than 0 (though `t` is not used in the print statement).
   - `i` is 1 (though `i` is not used in the print statement).
   - `s` is the string containing the first `k` lowercase letters of the English alphabet.
   - `j` is `k` + 96 (though `j` is not used in the print statement).
   - `k` is greater than 1.

2. **Print Statement:**
   ```
   print((2 - (n == 1)) * s)
   ```

3. **Explanation:**
   - The expression `(n == 1)` evaluates to `True` if `n` is 1, and `False` otherwise.
   - In Python, `True` is equivalent to 1 and `False` is equivalent to 0.
   - Therefore, `(2 - (n == 1))` will be:
     - `2 - 1 = 1` if `n` is 1.
     - `2 - 0 = 2` if `n` is not 1.
   - The string `s` is the first `k` lowercase letters of the English alphabet. For example, if `k` is 3, `s` will be "abc".

4. **Output Calculation:**
   - If `n` is 1, the expression `(2 - (n == 1))` evaluates to 1, so the print statement will output `1 * s`, which is just `s`.
   - If `n` is not 1, the expression `(2 - (n == 1))` evaluates to 2, so the print statement will output `2 * s`, which is `s` repeated twice.

5. **Final Output:**
   - If `n` is 1, the output will be the string `s`.
   - If `n` is not 1, the output will be the string `s` repeated twice.

Given the initial state, `k` is greater than 1, so `s` will always contain at least two letters.

Output: **s (if n is 1) or s + s (if n is not 1), where s is the string containing the first k lowercase letters of the English alphabet and k > 1**