Let's break down the given code snippet and the initial state to determine what will be printed.

### Initial State Recap
- `p_1`, `p_2`, and `p_3` are integers with the constraint \(0 \leq p_1 \leq p_2 \leq p_3 \leq 30\).
- `t` is a variable (though its value is not specified in the precondition, it is not used in the `print` statement, so we can ignore it).
- `v` is a list of integers, but the specific values are not provided.
- `result` is calculated using the formula: \((v[0] + v[1] + v[2] - \max(0, v[2] - v[0] - v[1])) // 2\).

### Calculation of `result`
The formula for `result` is:
\[ \text{result} = \frac{v[0] + v[1] + v[2] - \max(0, v[2] - v[0] - v[1])}{2} \]

Let's analyze the term \(\max(0, v[2] - v[0] - v[1])\):
- If \(v[2] \leq v[0] + v[1]\), then \(v[2] - v[0] - v[1] \leq 0\), so \(\max(0, v[2] - v[0] - v[1]) = 0\).
- If \(v[2] > v[0] + v[1]\), then \(v[2] - v[0] - v[1] > 0\), so \(\max(0, v[2] - v[0] - v[1]) = v[2] - v[0] - v[1]\).

So, the formula simplifies to:
\[ \text{result} = \begin{cases} 
\frac{v[0] + v[1] + v[2]}{2} & \text{if } v[2] \leq v[0] + v[1] \\
\frac{v[0] + v[1] + v[2] - (v[2] - v[0] - v[1])}{2} = \frac{2(v[0] + v[1])}{2} = v[0] + v[1] & \text{if } v[2] > v[0] + v[1]
\end{cases} \]

### Output
The output of the `print(result)` statement will depend on the values of `v[0]`, `v[1]`, and `v[2]`.

- If \(v[2] \leq v[0] + v[1]\), the result is \(\frac{v[0] + v[1] + v[2]}{2}\).
- If \(v[2] > v[0] + v[1]\), the result is \(v[0] + v[1]\).

Since the specific values of `v[0]`, `v[1]`, and `v[2]` are not provided, we can't compute the exact numerical value of `result`. However, based on the structure of the problem, the print statement will output the calculated result.

Output: **result (where result is \(\frac{v[0] + v[1] + v[2]}{2}\) if \(v[2] \leq v[0] + v[1]\), otherwise \(v[0] + v[1]\))**