### Reasoning:

Let's re-evaluate the problem and the provided solution step-by-step, using the annotations and the original assessment as references.

#### Problem Analysis:
The goal is to maximize the sum of all numbers in an n x n matrix using no more than 2n operations. We can perform two types of operations:
1. Assign a row with a permutation of numbers from 1 to n.
2. Assign a column with a permutation of numbers from 1 to n.

The optimal strategy to maximize the sum of the matrix involves filling the matrix with the highest possible values. The highest sum can be achieved by filling the matrix with numbers from 1 to n in a way that maximizes the sum of all elements.

#### Theoretical Maximum Sum:
For an n x n matrix, the maximum sum is achieved by filling the matrix with the numbers from 1 to n in a way that maximizes the sum of all elements. The sum of the first n natural numbers is given by the formula:
\[ \text{Sum of first n natural numbers} = \frac{n(n + 1)}{2} \]

Since each row and column can be filled with a permutation of these numbers, the maximum sum of the matrix is:
\[ \text{Maximum sum} = n \times \left(\frac{n(n + 1)}{2}\right) = \frac{n^2(n + 1)}{2} \]

#### Program's Calculation of Sum:
The provided program calculates the sum differently:
\[ \text{Sum} = 1 + \sum_{i=2}^{n} (i^2 - (i-1)^2) \times i \]

Let's simplify this expression:
\[ \text{Sum} = 1 + \sum_{i=2}^{n} (i^2 - (i^2 - 2i + 1)) \times i \]
\[ \text{Sum} = 1 + \sum_{i=2}^{n} (2i - 1) \times i \]
\[ \text{Sum} = 1 + \sum_{i=2}^{n} (2i^2 - i) \]
\[ \text{Sum} = 1 + 2\sum_{i=2}^{n} i^2 - \sum_{i=2}^{n} i \]

Using the formulas for the sum of squares and the sum of the first n natural numbers:
\[ \sum_{i=1}^{n} i^2 = \frac{n(n + 1)(2n + 1)}{6} \]
\[ \sum_{i=1}^{n} i = \frac{n(n + 1)}{2} \]

We can rewrite the sums starting from i=2:
\[ \sum_{i=2}^{n} i^2 = \sum_{i=1}^{n} i^2 - 1 = \frac{n(n + 1)(2n + 1)}{6} - 1 \]
\[ \sum_{i=2}^{n} i = \sum_{i=1}^{n} i - 1 = \frac{n(n + 1)}{2} - 1 \]

Substituting these into the expression for the sum:
\[ \text{Sum} = 1 + 2\left(\frac{n(n + 1)(2n + 1)}{6} - 1\right) - \left(\frac{n(n + 1)}{2} - 1\right) \]
\[ \text{Sum} = 1 + \frac{2n(n + 1)(2n + 1)}{6} - 2 - \frac{n(n + 1)}{2} + 1 \]
\[ \text{Sum} = \frac{2n(n + 1)(2n + 1)}{6} - \frac{3n(n + 1)}{6} \]
\[ \text{Sum} = \frac{2n(n + 1)(2n + 1) - 3n(n + 1)}{6} \]
\[ \text{Sum} = \frac{n(n + 1)(4n + 2 - 3)}{6} \]
\[ \text{Sum} = \frac{n(n + 1)(4n - 1)}{6} \]

This expression does not match the theoretical maximum sum of \(\frac{n^2(n + 1)}{2}\).

#### Operations:
The provided program performs 2n operations, which is within the allowed limit. Each operation fills a row and a column with a permutation of numbers from 1 to n. However, the way the operations are performed does not necessarily maximize the sum of the matrix.

### Re-evaluation with Annotations:
The annotated code shows that the program calculates the sum and prints the operations. However, the sum is calculated differently from the theoretical maximum sum. The operations described in the code do not guarantee that the matrix will be filled in a way that maximizes the sum.

The operations in the code are:
- For each row `n - j + 1`, it assigns the permutation `1, 2, ..., n` to the row.
- For each column `n - j + 1`, it assigns the permutation `1, 2, ..., n` to the column.

This approach does not ensure that the matrix will be filled with the highest possible values in a way that maximizes the sum.

### Conclusion:
The program does not correctly calculate the maximum sum of the matrix. Therefore, the correctness of the program is **False**.

Final: **False**