The variable `r` is assigned the value of `r * p`. Previously, `r` is defined as `n * (n - 1)` and `p` is defined as `n - 2`. Thus, we will compute the new value of `r` based on the existing values of `n` and `p`. However, since `n` can take on any integer value from 5 to 100, we can express the new value of `r` in terms of `n`.

Calculating:
- `p = n - 2`
- `r = n * (n - 1)`

So,
```
r = (n * (n - 1)) * (n - 2)
```

The states of the other variables (`n`, `p`, `s`, `g`, `i`) remain unchanged. Therefore, the Output State is: `n` is an integer such that 5 ≤ `n` ≤ 100; `p` is `n - 2`; `r` is `n * (n - 1) * (n - 2)`; `s` is 2; `g` is 3; `i` is 2.

Output State: **`n` is an integer such that 5 ≤ `n` ≤ 100; `p` is `n - 2`; `r` is `n * (n - 1) * (n - 2)`; `s` is 2; `g` is 3; `i` is 2**