Output State: **`n` and `m` are positive integers such that 1 <= n, m <= 2 * 10^6, `i` is `m`, `cnt` is `sum(math.ceil((n - (j * j - j)) / (j * j)) + ((n - (j * j - j)) % (j * j) == 0) for j in range(1, m + 1)) - 1`, `x` is `n - (m * m - m)`, `y` is `m * m`.**

### Natural Language Explanation:
- **`n` and `m`**: These remain positive integers within the range 1 to 2 * 10^6, as they are not modified by the loop.
- **`i`**: After the loop completes, `i` will be equal to `m`, because the loop runs from 1 to `m` inclusive.
- **`cnt`**: This variable accumulates the sum of `math.ceil((n - (j * j - j)) / (j * j)) + ((n - (j * j - j)) % (j * j) == 0)` for each iteration `j` from 1 to `m`, starting from an initial value of -1.
- **`x`**: After the loop completes, `x` will be `n - (m * m - m)`, which is the value of `n` minus the expression `(i * i - i)` evaluated at the final iteration `i = m`.
- **`y`**: After the loop completes, `y` will be `m * m`, which is the value of `i * i` evaluated at the final iteration `i = m`.