Output State: **`total` is 0, `l` is 1, `r` is -1, `a` is a list of integers where `a[1] == a[2]` and `a[2] == a[3]` and so on until `a[n-4] == a[n-3]`, `le` is the length of list `a`, `st` is -2, `end` is n - 3, `ans` is le - max(-2, n - 3)**

Explanation: 
- The variable `l` is updated to 1 and `r` is updated to -1 after the loop.
- The variable `end` remains `n - 3`.
- The variable `ans` is calculated as `le - max(st, end)`, which is `le - max(-2, n - 3)`. Since `n - 3` is always greater than -2 for positive `n`, `max(-2, n - 3)` simplifies to `n - 3`. Therefore, `ans` is `le - (n - 3)`.