In the initial state, we have the following variables:
- `n` is an integer such that \(3 \leq n \leq 10^6\)
- `mod` is a positive integer
- `result` is \(2 \mod \text{mod}\)
- `i` is \(3\)

The code snippet modifies the value of `result` by performing the operation:
```
result = result * i % mod
```
Now, we will calculate the new value of `result`:
- The previous value of `result` is \(2 \mod \text{mod}\).
- The value of `i` is \(3\).

Thus, the new value of `result` is calculated as:
\[
result = (2 \mod \text{mod}) * 3 \mod \text{mod}
\]
Since \(2 < \text{mod}\), \(2 \mod \text{mod} = 2\). Therefore:
\[
result = 2 * 3 \mod \text{mod} = 6 \mod \text{mod}
\]
Since \(6\) is less than `mod` (because `mod` is a positive integer greater than \(2\)), the value of `result` now becomes \(6\).

The values of `n`, `mod`, and `i` remain unchanged.

Output State: **`n` is an integer such that 3 <= n <= 10^6, `mod` is a positive integer, `result` is 6, `i` is 3**