Step-by-step analysis:
- Initial State: `n` is a positive integer such that \(1 \leq n \leq 2 \times 10^9\) and \(n \geq 6\), `count` is 1, `b` is \(n // 4 + 1\), `rem` is undefined, and `a` is \(n // 4 + 1\).
- Code: `rem = n - 2 * (a + b)`

Breaking down the code:
1. Calculate `a`: `a = n // 4 + 1`.
2. Calculate `b`: `b = n // 4 + 1`.
3. Substitute `a` and `b` into the expression for `rem`: 
   \[
   rem = n - 2 \times ((n // 4 + 1) + (n // 4 + 1)) = n - 2 \times (2 \times (n // 4) + 2) = n - (n // 2 + 2)
   \]
   Simplifying further:
   \[
   rem = n - \frac{n}{2} - 2 = \frac{2n - n}{2} - 2 = \frac{n}{2} - 2
   \]

Output State: **`n` is a positive integer such that \(1 \leq n \leq 2 \times 10^9\) and \(n \geq 6\), `count` is 1, `b` is \(n // 4 + 1\), `rem` is \(\frac{n}{2} - 2\), and `a` is \(n // 4 + 1\)**.