The code snippet `a[i], a[j] = a[j], a[i]` swaps the values of `a[i]` and `a[j]`.

Given the initial state:
- `n` is an integer such that \(1 \leq n \leq 1000\)
- `a` is a list of integers where \(1 \leq a_i \leq 10^9\) for all \(1 \leq i \leq \text{len}(a)\)
- `d` is a list of `n` lists, where each `d[i]` contains the indices `j` (where \(i + 1 \leq j < n\)) such that `a[i] > a[j]`
- `ans` includes the tuples `(1, j + 1)` for each `j` in `d[0]` and now includes the tuples `(2, j + 1)`, `(3, j + 1)`, and `(2, j + 1)`
- `i` is 1
- The elements of `a` at indices 1 and `j` are swapped
- `d[1]` is sorted in descending order based on the values of `a[x]` and `x`
- `d[1]` must contain at least one element
- `j` is the next element in `d[1]`

After executing the code snippet:
- The value of `a[i]` (which is `a[1]`) is swapped with the value of `a[j]` (where `j` is the next element in `d[1]`).

Output State: **`n` is an integer such that \(1 \leq n \leq 1000\), `a` is a list of integers where \(1 \leq a_i \leq 10^9\) for all \(1 \leq i \leq \text{len}(a)\), `d` is a list of `n` lists, where each `d[i]` contains the indices `j` (where \(i + 1 \leq j < n\)) such that `a[i] > a[j]`, `ans` includes the tuples `(1, j + 1)` for each `j` in `d[0]` and now includes the tuples `(2, j + 1)`, `(3, j + 1)`, and `(2, j + 1)`, `i` is 1, `a[1]` and `a[j]` are swapped, `d[1]` is sorted in descending order based on the values of `a[x]` and `x`, `d[1]` must contain at least one element, `j` is the next element in `d[1]`.**