To determine what will be printed by the `print(suma - 2)` statement, let's break down the initial state and the conditions step by step:

1. **Initial State**:
   - `n` and `m` are positive integers such that \(1 \leq n, m \leq 2 \times 10^6\).
   - `T` is greater than 0.
   - `t` is 0.
   - `a` is the integer value of the first string in `info`.
   - `b` is the integer value of the second string in `info`.
   - `suma` is the sum of all valid `x` values calculated in the loop, where `x` is \(\left(\frac{a - i \cdot (i - 1)}{i^2} + 1\right)\) for \(i\) from 1 to `b`.
   - An additional 1 is added to `suma` for each `i` where \((a - i \cdot (i - 1)) \% i^2 == 0\) and \(i \cdot (i - 1) \% i^2 == 0\).

2. **Understanding the Loop**:
   - The loop iterates from \(i = 1\) to \(i = b\).
   - For each \(i\), the value of `x` is calculated as \(\left(\frac{a - i \cdot (i - 1)}{i^2} + 1\right)\).
   - An additional 1 is added to `suma` if both conditions \((a - i \cdot (i - 1)) \% i^2 == 0\) and \(i \cdot (i - 1) \% i^2 == 0\) are true.

3. **Conditions Analysis**:
   - The condition \(i \cdot (i - 1) \% i^2 == 0\) is only true when \(i = 1\) because for \(i > 1\), \(i \cdot (i - 1)\) is not divisible by \(i^2\).
   - The condition \((a - i \cdot (i - 1)) \% i^2 == 0\) needs to be checked for each \(i\) from 1 to `b`.

4. **Calculating `suma`**:
   - For \(i = 1\):
     - \(x = \left(\frac{a - 1 \cdot (1 - 1)}{1^2} + 1\right) = \left(\frac{a - 0}{1} + 1\right) = a + 1\).
     - The condition \((a - 1 \cdot (1 - 1)) \% 1^2 == 0\) is always true.
     - The condition \(1 \cdot (1 - 1) \% 1^2 == 0\) is also always true.
     - Therefore, an additional 1 is added to `suma`.
     - `suma` after \(i = 1\) is \(a + 1 + 1 = a + 2\).

   - For \(i > 1\):
     - \(x = \left(\frac{a - i \cdot (i - 1)}{i^2} + 1\right)\).
     - The condition \((a - i \cdot (i - 1)) \% i^2 == 0\) and \(i \cdot (i - 1) \% i^2 == 0\) are both false for \(i > 1\).
     - Therefore, no additional 1 is added to `suma` for \(i > 1\).

5. **Final Calculation**:
   - `suma` is the sum of all valid `x` values plus the additional 1 for \(i = 1\).
   - Since the only valid \(i\) is 1, `suma` is \(a + 2\).
   - The print statement `print(suma - 2)` will print \(a + 2 - 2 = a\).

Output: **a (where a is the integer value of the first string in `info`)**