Postcondition: **`n` and `m` are positive integers such that \(1 \leq n, m \leq 2 \times 10^6\), `T` is greater than 0, `t` is 1, `info` is a list of strings from the input, `a` is the integer value of the first string in `info`, `b` is the integer value of the second string in `info` and must be greater than or equal to 2, `x` is \((a - 1 \times (1 - 1)) // 1^2 + 1\). If \((a - i \times (i - 1)) \% i^2 == 0\) and \((i \times (i - 1)) \% i^2 == 0\), then `suma` is \(a + 1 + x + 1\). Otherwise, `suma` remains \(a + 1 + x\).**