Postcondition: **`n` and `m` are positive integers such that \(1 \leq n, m \leq 2 \times 10^6\), `T` is greater than 1, `t` is 2, `info` is a list of strings from the new input, `a` is the integer value of the first string in `info`, `b` is the integer value of the second string in `info` and must be greater than or equal to 2, `i` is 2, and `x` is \((a - 2 \times 1) // 4 + 1\). If \((a - i \times (i - 1)) // i^2 + 1 > 0\), then `suma` is increased by 1 if \((a - i \times (i - 1)) \% i^2 == 0\) and \(i \times (i - 1) \% i^2 == 0\). Otherwise, `suma` is increased by \((a - 2) // 4 + 1\). If the condition \((a - i \times (i - 1)) // i^2 + 1 > 0\) is not met, `suma` remains unchanged.**