Alright, I've got this problem to solve. Let's see what it's asking for. So, I'm given an integer x, and I need to find another integer y, where y is less than x and at least 1, such that when I add y to the greatest common divisor of x and y, the result is as large as possible. Basically, I need to maximize gcd(x, y) + y.

First, I need to understand what gcd(x, y) is. The greatest common divisor is the largest number that divides both x and y without leaving a remainder. So, if x and y share some common factors, gcd(x, y) will be the highest of those factors.

Now, I need to maximize gcd(x, y) + y. That means I want both gcd(x, y) and y to be as large as possible. But there's a constraint: y has to be less than x.

Let me think about this. If I choose y to be x - 1, that is, the largest possible y less than x, what happens?

Well, gcd(x, x-1) is probably 1, because two consecutive integers are usually coprime, meaning their gcd is 1. So, gcd(x, x-1) + (x-1) = 1 + (x-1) = x.

Is there a better choice for y that could make gcd(x, y) + y larger than x?

Let's consider some examples to see.

Take x = 10.

If y = 9, gcd(10, 9) = 1, so 1 + 9 = 10.

If y = 5, gcd(10, 5) = 5, so 5 + 5 = 10.

If y = 8, gcd(10, 8) = 2, so 2 + 8 = 10.

If y = 6, gcd(10, 6) = 2, so 2 + 6 = 8.

If y = 4, gcd(10, 4) = 2, so 2 + 4 = 6.

If y = 3, gcd(10, 3) = 1, so 1 + 3 = 4.

If y = 2, gcd(10, 2) = 2, so 2 + 2 = 4.

If y = 1, gcd(10, 1) = 1, so 1 + 1 = 2.

So, in this case, the maximum is 10, achieved when y is 5, 8, or 9.

Another example: x = 7.

Possible y values:

y = 6: gcd(7, 6) = 1, 1 + 6 = 7.

y = 5: gcd(7, 5) = 1, 1 + 5 = 6.

y = 4: gcd(7, 4) = 1, 1 + 4 = 5.

y = 3: gcd(7, 3) = 1, 1 + 3 = 4.

y = 2: gcd(7, 2) = 1, 1 + 2 = 3.

y = 1: gcd(7, 1) = 1, 1 + 1 = 2.

So here, the maximum is 7, achieved when y is 6.

Another one: x = 21.

Possible y values:

y = 20: gcd(21, 20) = 1, 1 + 20 = 21.

y = 18: gcd(21, 18) = 3, 3 + 18 = 21.

y = 15: gcd(21, 15) = 3, 3 + 15 = 18.

y = 14: gcd(21, 14) = 7, 7 + 14 = 21.

y = 12: gcd(21, 12) = 3, 3 + 12 = 15.

y = 10: gcd(21, 10) = 1, 1 + 10 = 11.

y = 8: gcd(21, 8) = 1, 1 + 8 = 9.

y = 7: gcd(21, 7) = 7, 7 + 7 = 14.

y = 6: gcd(21, 6) = 3, 3 + 6 = 9.

y = 5: gcd(21, 5) = 1, 1 + 5 = 6.

y = 4: gcd(21, 4) = 1, 1 + 4 = 5.

y = 3: gcd(21, 3) = 3, 3 + 3 = 6.

y = 2: gcd(21, 2) = 1, 1 + 2 = 3.

y = 1: gcd(21, 1) = 1, 1 + 1 = 2.

So, the maximum is 21, achieved when y is 14, 18, or 20.

Wait a minute, in all these examples, the maximum value of gcd(x, y) + y is equal to x. Is that always the case?

Let's see another example: x = 2.

Possible y: y = 1, gcd(2, 1) = 1, 1 + 1 = 2.

So, again, the maximum is x.

Another example: x = 6.

Possible y values:

y = 5: gcd(6, 5) = 1, 1 + 5 = 6.

y = 4: gcd(6, 4) = 2, 2 + 4 = 6.

y = 3: gcd(6, 3) = 3, 3 + 3 = 6.

y = 2: gcd(6, 2) = 2, 2 + 2 = 4.

y = 1: gcd(6, 1) = 1, 1 + 1 = 2.

Again, the maximum is 6, achieved for y = 3, 4, 5.

It seems like in all these cases, the maximum value of gcd(x, y) + y is equal to x. Is this always true?

Let me try to see why this might be the case.

Consider that gcd(x, y) is a divisor of x and y. So, gcd(x, y) divides x and y.

Let d = gcd(x, y). Then, d divides x and d divides y.

So, y = k * d for some integer k.

Since y < x, k * d < x.

Also, since d divides x, x = m * d for some integer m.

So, k * d < m * d, which implies k < m.

Now, gcd(x, y) + y = d + k * d = d * (k + 1).

But x = m * d.

I need to maximize d * (k + 1), given that k < m and k is a positive integer since y >= 1.

Wait, maybe there's a better way to approach this.

Let me consider that for a fixed d, which is a divisor of x, I can choose y to be the largest multiple of d that is less than x.

So, y = floor((x - 1)/d) * d.

But perhaps there's a smarter way.

Alternatively, perhaps I can think in terms of selecting y such that y is as large as possible, and gcd(x, y) is also as large as possible.

But maximizing y directly would mean choosing y = x - 1, but as we've seen, sometimes gcd(x, y) is 1 in that case, unless x and y share common factors.

Wait, perhaps I should consider the largest proper divisor of x.

What's a proper divisor? A divisor of x that is less than x.

So, if I take y to be the largest proper divisor of x, then gcd(x, y) would be y itself, since y divides x.

Thus, gcd(x, y) + y = y + y = 2y.

But is this better than choosing y = x - 1, which gives gcd(x, y) + y = 1 + (x - 1) = x?

Wait, in the earlier examples, 2y was less than x in some cases.

For example, x = 10, largest proper divisor is 5, so 2*5 = 10, which is equal to x.

x = 7, largest proper divisor is 1, so 2*1 = 2, which is less than x.

Wait, but earlier we saw that for x = 7, y = 6 gives gcd(7,6) + 6 = 1 + 6 = 7, which is better than choosing y = 1.

Similarly, for x = 10, y = 5 gives 5 + 5 = 10, which is equal to x.

Wait, but in the case where x is a prime number, like x = 7, the largest proper divisor is 1, but choosing y = x - 1 = 6 gives a better result.

So, perhaps choosing y = x - 1 is a good strategy, but in some cases, choosing y to be the largest proper divisor is better.

Wait, in the case of x = 7, choosing y = 6 gives gcd(7,6) + 6 = 1 + 6 = 7.

Choosing y = 1 gives 1 + 1 = 2.

Choosing y = any other number less than 7 gives a sum less than or equal to 7.

So, in this case, y = x - 1 is a good choice.

Similarly, for x = 10, y = 5 gives 5 + 5 = 10, which is equal to x.

Wait, but y = 5 is not x - 1, which would be 9 for x = 10.

Earlier, y = 9 gives gcd(10,9) + 9 = 1 + 9 = 10, which is the same as choosing y = 5.

So, in this case, both y = 5 and y = 9 give the same sum.

Similarly, for x = 21, y = 14 gives gcd(21,14) + 14 = 7 + 14 = 21, and y = 20 gives gcd(21,20) + 20 = 1 + 20 = 21.

So, again, both choices give the same sum.

So, perhaps choosing y = x - 1 is always giving gcd(x, x-1) + (x - 1) = 1 + (x - 1) = x, since x and x-1 are coprime.

But in some cases, there might be y's where gcd(x, y) is larger, but y is smaller, such that gcd(x, y) + y is still equal to x.

Wait, in the example of x = 10, y = 5 gives gcd(10,5) + 5 = 5 + 5 = 10, which is equal to x.

Similarly, y = 8 gives gcd(10,8) + 8 = 2 + 8 = 10, again equal to x.

And y = 9 gives gcd(10,9) + 9 = 1 + 9 = 10.

So, in this case, all these y's give the same sum of x.

Is this always the case? That is, is the maximum always equal to x?

Let me check for x = 6.

Possible y's:

y = 3: gcd(6,3) + 3 = 3 + 3 = 6.

y = 4: gcd(6,4) + 4 = 2 + 4 = 6.

y = 5: gcd(6,5) + 5 = 1 + 5 = 6.

Again, all these y's give the same sum of x.

Is there any x where the maximum sum is greater than x?

Let me think about x = 4.

Possible y's:

y = 2: gcd(4,2) + 2 = 2 + 2 = 4.

y = 1: gcd(4,1) + 1 = 1 + 1 = 2.

So, the maximum is 4, which is equal to x.

Another example: x = 8.

Possible y's:

y = 4: gcd(8,4) + 4 = 4 + 4 = 8.

y = 6: gcd(8,6) + 6 = 2 + 6 = 8.

y = 7: gcd(8,7) + 7 = 1 + 7 = 8.

Again, the maximum is 8.

So, it seems like in all these cases, the maximum sum is equal to x.

Is this always true?

Let me consider x = 9.

Possible y's:

y = 6: gcd(9,6) + 6 = 3 + 6 = 9.

y = 7: gcd(9,7) + 7 = 1 + 7 = 8.

y = 8: gcd(9,8) + 8 = 1 + 8 = 9.

y = 3: gcd(9,3) + 3 = 3 + 3 = 6.

y = 2: gcd(9,2) + 2 = 1 + 2 = 3.

y = 1: gcd(9,1) + 1 = 1 + 1 = 2.

Again, the maximum is 9.

Another example: x = 12.

Possible y's:

y = 6: gcd(12,6) + 6 = 6 + 6 = 12.

y = 8: gcd(12,8) + 8 = 4 + 8 = 12.

y = 9: gcd(12,9) + 9 = 3 + 9 = 12.

y = 10: gcd(12,10) + 10 = 2 + 10 = 12.

y = 11: gcd(12,11) + 11 = 1 + 11 = 12.

y = 4: gcd(12,4) + 4 = 4 + 4 = 8.

y = 3: gcd(12,3) + 3 = 3 + 3 = 6.

y = 2: gcd(12,2) + 2 = 2 + 2 = 4.

y = 1: gcd(12,1) + 1 = 1 + 1 = 2.

Again, the maximum is 12.

So, it seems like in all these cases, the maximum sum is equal to x.

Is there any x where the maximum sum is greater than x?

Let me think about x = 1.

Wait, but according to the problem, x is at least 2, so x = 1 is not allowed.

x = 2.

Possible y: y = 1, gcd(2,1) + 1 = 1 + 1 = 2.

So, again, the maximum is equal to x.

x = 3.

Possible y's:

y = 2: gcd(3,2) + 2 = 1 + 2 = 3.

y = 1: gcd(3,1) + 1 = 1 + 1 = 2.

Again, maximum is 3.

x = 4.

Possible y's:

y = 2: gcd(4,2) + 2 = 2 + 2 = 4.

y = 3: gcd(4,3) + 3 = 1 + 3 = 4.

y = 1: gcd(4,1) + 1 = 1 + 1 = 2.

Maximum is 4.

x = 5.

Possible y's:

y = 4: gcd(5,4) + 4 = 1 + 4 = 5.

y = 3: gcd(5,3) + 3 = 1 + 3 = 4.

y = 2: gcd(5,2) + 2 = 1 + 2 = 3.

y = 1: gcd(5,1) + 1 = 1 + 1 = 2.

Maximum is 5.

x = 6.

Possible y's:

y = 3: gcd(6,3) + 3 = 3 + 3 = 6.

y = 4: gcd(6,4) + 4 = 2 + 4 = 6.

y = 5: gcd(6,5) + 5 = 1 + 5 = 6.

y = 2: gcd(6,2) + 2 = 2 + 2 = 4.

y = 1: gcd(6,1) + 1 = 1 + 1 = 2.

Maximum is 6.

x = 8.

Possible y's:

y = 4: gcd(8,4) + 4 = 4 + 4 = 8.

y = 6: gcd(8,6) + 6 = 2 + 6 = 8.

y = 7: gcd(8,7) + 7 = 1 + 7 = 8.

y = 2: gcd(8,2) + 2 = 2 + 2 = 4.

y = 3: gcd(8,3) + 3 = 1 + 3 = 4.

y = 5: gcd(8,5) + 5 = 1 + 5 = 6.

y = 1: gcd(8,1) + 1 = 1 + 1 = 2.

Maximum is 8.

x = 9.

Possible y's:

y = 6: gcd(9,6) + 6 = 3 + 6 = 9.

y = 7: gcd(9,7) + 7 = 1 + 7 = 8.

y = 8: gcd(9,8) + 8 = 1 + 8 = 9.

y = 3: gcd(9,3) + 3 = 3 + 3 = 6.

y = 2: gcd(9,2) + 2 = 1 + 2 = 3.

y = 1: gcd(9,1) + 1 = 1 + 1 = 2.

Maximum is 9.

x = 12.

Possible y's:

y = 6: gcd(12,6) + 6 = 6 + 6 = 12.

y = 8: gcd(12,8) + 8 = 4 + 8 = 12.

y = 9: gcd(12,9) + 9 = 3 + 9 = 12.

y = 10: gcd(12,10) + 10 = 2 + 10 = 12.

y = 11: gcd(12,11) + 11 = 1 + 11 = 12.

y = 4: gcd(12,4) + 4 = 4 + 4 = 8.

y = 3: gcd(12,3) + 3 = 3 + 3 = 6.

y = 2: gcd(12,2) + 2 = 2 + 2 = 4.

y = 1: gcd(12,1) + 1 = 1 + 1 = 2.

Maximum is 12.

x = 15.

Possible y's:

y = 14: gcd(15,14) + 14 = 1 + 14 = 15.

y = 12: gcd(15,12) + 12 = 3 + 12 = 15.

y = 10: gcd(15,10) + 10 = 5 + 10 = 15.

y = 9: gcd(15,9) + 9 = 3 + 9 = 12.

y = 8: gcd(15,8) + 8 = 1 + 8 = 9.

y = 7: gcd(15,7) + 7 = 1 + 7 = 8.

y = 6: gcd(15,6) + 6 = 3 + 6 = 9.

y = 5: gcd(15,5) + 5 = 5 + 5 = 10.

y = 4: gcd(15,4) + 4 = 1 + 4 = 5.

y = 3: gcd(15,3) + 3 = 3 + 3 = 6.

y = 2: gcd(15,2) + 2 = 1 + 2 = 3.

y = 1: gcd(15,1) + 1 = 1 + 1 = 2.

Again, the maximum is 15.

So, in all these examples, the maximum sum is equal to x.

Is this always the case?

Let me see if there's a mathematical reason why this is happening.

Consider that for any y < x, gcd(x, y) divides x and y.

Let d = gcd(x, y).

Then, x = d * k and y = d * m, where k and m are integers, and k and m are coprime (since d is the greatest common divisor).

Then, gcd(x, y) + y = d + d * m = d * (1 + m).

But since x = d * k and y = d * m, and y < x, then d * m < d * k, which implies m < k.

Also, since k and m are coprime, 1 + m is at most k, because if m >= k - 1, then m and k would share a common factor, but they are coprime.

Wait, actually, k and m are coprime, so m can be up to k - 1 without sharing a common factor with k.

So, d * (1 + m) <= d * k = x.

Because m <= k - 1, so 1 + m <= k.

Therefore, d * (1 + m) <= d * k = x.

Thus, gcd(x, y) + y <= x.

And in the cases where m = k - 1, gcd(x, y) + y = d * (1 + k - 1) = d * k = x.

So, the maximum possible value is x, achieved when m = k - 1.

Therefore, the maximum value of gcd(x, y) + y is x, and this is achievable for certain y's.

Therefore, in the program, choosing y = x - 1 will always give gcd(x, x-1) + (x - 1) = 1 + (x - 1) = x, which is the maximum possible.

Hence, the program is correct.

**Final Solution**

To solve this problem, we need to find an integer \( y \) (where \( 1 \leq y < x \)) such