Let's break down the initial state and the expression inside the `print` statement step by step:

### Initial State:
- `_` is 0 (not used in the expression).
- `n` is an input integer greater than 0.
- `a` is an input integer.
- `b` is an input integer, and `b` is greater than `a`.
- `k` is the minimum of `n` and `b - a`.

### Expression to Evaluate:
```python
b * k - k * (k - 1) // 2 + (n - k) * a
```

### Step-by-Step Calculation:
1. **Determine `k`:**
   - `k` is the minimum of `n` and `b - a`.
   - If `n` is less than or equal to `b - a`, then `k = n`.
   - If `n` is greater than `b - a`, then `k = b - a`.

2. **Evaluate the Expression:**
   - **First Term:** `b * k`
     - This term multiplies `b` by `k`.
   - **Second Term:** `- k * (k - 1) // 2`
     - This term calculates the sum of the first `k` integers (using the formula for the sum of an arithmetic series), but it is subtracted from the first term.
   - **Third Term:** `(n - k) * a`
     - This term multiplies the remaining elements (i.e., `n - k`) by `a`.

### Combining the Terms:
- The expression combines these three terms to form the final result.

### Final Output:
- The `print` statement will output the result of the expression `b * k - k * (k - 1) // 2 + (n - k) * a`.

### Example Calculation:
- Suppose `n = 5`, `a = 1`, and `b = 3`.
  - `k = min(5, 3 - 1) = min(5, 2) = 2`.
  - First Term: `b * k = 3 * 2 = 6`.
  - Second Term: `- k * (k - 1) // 2 = - 2 * (2 - 1) // 2 = - 2 * 1 // 2 = - 1`.
  - Third Term: `(n - k) * a = (5 - 2) * 1 = 3 * 1 = 3`.
  - Final Result: `6 - 1 + 3 = 8`.

### General Description:
- The `print` statement will output the result of the expression, which is a combination of the first `k` elements being multiplied by `b` and adjusted by the sum of the first `k` integers, plus the remaining elements being multiplied by `a`.

Output: **b * k - k * (k - 1) // 2 + (n - k) * a (where k is the minimum of n and b - a, b is greater than a, and n, a, and b are input integers)**