Let's break down the initial state and the print statement step by step:

### Initial State:
- `_` is 1 (This variable is not used in the print statement, so we can ignore it).
- `n` is an input integer greater than 0.
- `a` is an input integer.
- `b` is an input integer.
- `k` is the minimum of `n` and `b - a`.

### Print Statement:
```python
print(b * k - k * (k - 1) // 2 + (n - k) * a)
```

### Step-by-Step Calculation:
1. **Determine `k`:**
   - `k` is the minimum of `n` and `b - a`.
   - This means `k` will be the smaller of the two values: `n` or `b - a`.

2. **Calculate the expression inside the print statement:**
   - The expression is `b * k - k * (k - 1) // 2 + (n - k) * a`.
   - Let's break it down further:
     - `b * k`: This is simply `b` multiplied by `k`.
     - `k * (k - 1) // 2`: This is the sum of the first `k-1` integers, which is a common formula for the sum of an arithmetic series.
     - `(n - k) * a`: This is the product of `n - k` and `a`.

3. **Combine the parts:**
   - The expression `b * k - k * (k - 1) // 2 + (n - k) * a` combines these three parts.

### Final Output:
- The output will be the result of the expression `b * k - k * (k - 1) // 2 + (n - k) * a`.
- Since `k` is the minimum of `n` and `b - a`, the exact numerical value depends on the specific values of `n`, `a`, and `b`.

### Example Calculation:
- Suppose `n = 5`, `a = 2`, and `b = 7`.
  - `k = min(5, 7 - 2) = min(5, 5) = 5`.
  - `b * k = 7 * 5 = 35`.
  - `k * (k - 1) // 2 = 5 * 4 // 2 = 10`.
  - `(n - k) * a = (5 - 5) * 2 = 0`.
  - The expression becomes `35 - 10 + 0 = 25`.

### General Description:
- The output will be the result of the expression `b * k - k * (k - 1) // 2 + (n - k) * a`, where `k` is the minimum of `n` and `b - a`.

Output: **b * k - k * (k - 1) // 2 + (n - k) * a (where k is the minimum of n and b - a)**