Output State: **`n` and `m` are positive integers such that \(1 \leq n, m \leq 2 \times 10^6\), `T` is greater than 0, `t` is 1, `info` is a list of strings obtained from the input, `a` is the integer value of `info[0]`, `b` is the integer value of `info[1]` and must be at least 1, `suma` is 0, `i` is 1, `x` is \((a - 1) // 1 + 1\) which simplifies to \((a - 1) + 1\) or `a`.**

Explanation:
- The code calculates the value of `x` using the formula: `x = (a - i * (i - 1)) // i ** 2 + 1`.
- Given `i` is 1, the expression simplifies to: `x = (a - 1 * (1 - 1)) // 1 ** 2 + 1`.
- This further simplifies to: `x = (a - 0) // 1 + 1`.
- Since `//` is integer division, `(a - 0) // 1` is simply `a`.
- Adding 1 to `a` gives `x = a + 1 - 1`, which simplifies to `x = a`.

Therefore, the value of `x` is `a`. All other variables remain unchanged.