The code `per = n - 2` assigns the value of `n - 2` to the variable `per`. Since the initial state includes the condition `(n - 1) % 4 != 2` and the new value of `per` is derived from `n - 2`, we can deduce that the new condition for `per` would be `(per - 1) % 4 != 2`. Given that `(n - 1) % 4 != 2`, it follows that `(n - 2 - 1) % 4 = (n - 3) % 4 != 2`.

Therefore, the updated values are:
- `per` is now `n - 2`
- The condition for `per` is `(per - 1) % 4 != 2`, which simplifies to `(n - 3) % 4 != 2`

Output State: **`ost` contains all integers from `pos + 1` to `n` inclusive that satisfy the condition `(i % 2 != 0 or i % 4 == 0) and i > n // 2`, `pos` is unspecified, `n` is unspecified, `per` is `n - 2`, and `(n - 3) % 4 != 2`**