Postcondition: ***`n` and `m` are positive integers such that \(1 \leq n, m \leq 2 \times 10^6\), `T` is greater than 1, `t` is 2, `info` is a list of strings from the new input, `a` is the integer value of the first string in `info`, `b` is the integer value of the second string in `info` and must be greater than or equal to 1, `i` is 1, and `x` is \((a - 1) // 1 + 1\). If \((a - i * (i - 1)) // i ** 2 + 1 > 0\), then: if \((a - i * (i - 1)) \% i^2 == 0\) and \(i * (i - 1) \% i^2 == 0\), `suma` is `a + 1` and `x` is `a`. Otherwise, `suma` remains \((a - 1) // 1 + 1\). If \((a - i * (i - 1)) // i ** 2 + 1 \leq 0\), `suma` remains 0 and `x` remains \((a - 1) // 1 + 1\).***