To determine what will be printed by the `print(suma - 2)` statement, let's break down the initial state and the logic of the code step by step.

### Initial State:
- `n` and `m` are positive integers such that \(1 \leq n, m \leq 2 \times 10^6\).
- `T` is greater than 1.
- `t` is 2.
- `info` is a list of strings from the new input.
- `a` is the integer value of the first string in `info`.
- `b` is the integer value of the second string in `info` and must be greater than or equal to 1.
- `i` is initialized to `b`.
- `suma` is the sum of all valid `x` values calculated in the loop, where `x` is \((a - i \times (i - 1)) // i^2 + 1\) for each `i` from 1 to `b`.
- `suma` is incremented by 1 if \((a - i \times (i - 1)) \% i^2 == 0\) and \(i \times (i - 1) \% i^2 == 0\) for each `i` from 1 to `b`.

### Code Execution:
The `print(suma - 2)` statement will print the value of `suma` minus 2. To understand what `suma` is, we need to analyze the loop that calculates it.

### Loop Analysis:
1. **Initialization**:
   - `i` starts at `b`.
   - `suma` is initially 0.

2. **Loop Execution**:
   - The loop runs for each `i` from 1 to `b`.
   - For each `i`, the value of `x` is calculated as \((a - i \times (i - 1)) // i^2 + 1\).
   - `suma` is incremented by `x`.
   - Additionally, `suma` is incremented by 1 if both \((a - i \times (i - 1)) \% i^2 == 0\) and \(i \times (i - 1) \% i^2 == 0\).

### Simplifying the Conditions:
- The condition \(i \times (i - 1) \% i^2 == 0\) simplifies to checking if \(i \times (i - 1)\) is divisible by \(i^2\). This is true only if \(i - 1\) is divisible by \(i\), which is never true for any integer \(i > 1\). Therefore, this condition is always false for \(i > 1\).

### Simplifying the Calculation:
- The value of `x` is \((a - i \times (i - 1)) // i^2 + 1\).
- The condition \((a - i \times (i - 1)) \% i^2 == 0\) checks if \(a - i \times (i - 1)\) is divisible by \(i^2\).

### Final Calculation:
- For each `i` from 1 to `b`, `suma` is incremented by \((a - i \times (i - 1)) // i^2 + 1\).
- The additional increment by 1 is never applied because \(i \times (i - 1) \% i^2 == 0\) is always false for \(i > 1\).

### Example Calculation:
Let's assume `a` and `b` are given as specific values. For instance, let `a = 10` and `b = 3`.

- For \(i = 1\):
  - \(x = (10 - 1 \times (1 - 1)) // 1^2 + 1 = (10 - 0) // 1 + 1 = 10 + 1 = 11\).
  - `suma` is incremented by 11.
  - The condition \((10 - 1 \times (1 - 1)) \% 1^2 == 0\) is true, but the second condition is false, so no additional increment.

- For \(i = 2\):
  - \(x = (10 - 2 \times (2 - 1)) // 2^2 + 1 = (10 - 2) // 4 + 1 = 8 // 4 + 1 = 2 + 1 = 3\).
  - `suma` is incremented by 3.
  - The condition \((10 - 2 \times (2 - 1)) \% 2^2 == 0\) is true, but the second condition is false, so no additional increment.

- For \(i = 3\):
  - \(x = (10 - 3 \times (3 - 1)) // 3^2 + 1 = (10 - 6) // 9 + 1 = 4 // 9 + 1 = 0 + 1 = 1\).
  - `suma` is incremented by 1.
  - The condition \((10 - 3 \times (3 - 1)) \% 3^2 == 0\) is false, so no additional increment.

- Final `suma` value: \(11 + 3 + 1 = 15\).

- The `print(suma - 2)` statement will print \(15 - 2 = 13\).

### General Output:
Since the exact values of `a` and `b` are not provided, we can only describe the output in terms of the variables and the loop logic.

Output: **suma - 2 (where suma is the sum of all valid x values calculated in the loop, and x is (a - i * (i - 1)) // i^2 + 1 for each i from 1 to b, with no additional increments because the conditions are never met for i > 1)**