To determine the final output state after the loop has executed all its iterations, we need to understand how the loop modifies the variables `cnt`, `x`, and `y` with each iteration. Let's break down the loop and see how the state evolves.

### Loop Analysis:
The loop runs from `i = 1` to `i = m-1`. For each iteration, it performs the following operations:
1. Calculate `x = n - (i * i - i)`.
2. Calculate `y = i * i`.
3. Update `cnt = cnt + (x // y) + (i > 1)`.

### Iteration Details:
- **First Iteration (i=1)**:
  - `x = n - (1*1 - 1) = n`
  - `y = 1*1 = 1`
  - `cnt = cnt + (n // 1) + (1 > 1) = cnt + n + 0 = cnt + n`

- **Second Iteration (i=2)**:
  - `x = n - (2*2 - 2) = n - 2`
  - `y = 2*2 = 4`
  - `cnt = cnt + ((n - 2) // 4) + (2 > 1) = cnt + (n - 2) // 4 + 1`

- **Third Iteration (i=3)**:
  - `x = n - (3*3 - 3) = n - 6`
  - `y = 3*3 = 9`
  - `cnt = cnt + ((n - 6) // 9) + (3 > 1) = cnt + (n - 6) // 9 + 1`

### General Iteration (i=k):
- `x = n - (k*k - k)`
- `y = k*k`
- `cnt = cnt + ((n - (k*k - k)) // (k*k)) + (k > 1)`

### Final State:
The loop will run for `i` from 1 to `m-1`. Therefore, the final value of `cnt` will be the sum of all these individual contributions.

The final state of `cnt` can be expressed as:
\[ \text{cnt} = n + \sum_{k=2}^{m-1} \left( \left( \frac{n - (k^2 - k)}{k^2} \right) + 1 \right) \]

### Simplifying the Final State:
- The first term `n` comes from the first iteration.
- For each subsequent iteration `k` from 2 to `m-1`, we add `1` and the integer division result.

Thus, the final state of `cnt` can be described as:
\[ \text{cnt} = n + (m - 2) + \sum_{k=2}^{m-1} \left( \frac{n - (k^2 - k)}{k^2} \right) \]

### Final Output State:
Given the loop structure and the provided initial state, the final output state after all iterations is:

Output State: **cnt is `n + (m - 2) + sum((n - (k^2 - k)) // (k^2) for k in range(2, m))`**

In natural language, this means that `cnt` will be the initial value of `n` plus `m-2` (since we add 1 for each iteration from 2 to `m-1`), plus the sum of integer divisions `(n - (k^2 - k)) // (k^2)` for each `k` from 2 to `m-1`.