Alright, I've got this problem here about Alice and Bob playing a game with their wallets. Let's see what it's asking.

So, Alice has a coins and Bob has b coins. They take turns, with Alice going first. In each turn, the player can choose to exchange wallets with the opponent or keep their current wallet, and then remove one coin from their current wallet. The player who can't make a valid move loses. We need to figure out who wins if both play optimally.

First, I need to understand the game mechanics clearly.

1. **Exchange wallets or keep current wallets:** This is the first choice each player makes in their turn.

2. **Remove one coin from the current wallet:** They must do this, and their wallet can't have zero coins before removing.

The game continues until someone can't make a move, meaning their wallet is empty and they can't remove a coin.

I need to think about the game states and how they change based on the players' choices.

Let's consider some small values for a and b to see if I can find a pattern.

**Example 1:**

a = 1, b = 1

- Alice's turn:

- Option 1: Don't swap. Now a=0, b=1.

- Bob's turn:

- Must not swap because a=0. So, remove 1 from b. Now a=0, b=0.

- Alice can't make a move, so Bob wins.

- Option 2: Swap. Then a=1, b=1. It's the same as the starting position.

- If Alice chooses to swap, the game repeats, and Alice will eventually be forced to make the same decision again. But in the end, she'll have to choose not to swap, leading to the same outcome where she loses.

So, in this case, Bob wins.

**Example 2:**

a = 1, b = 4

- Alice's turn:

- Option 1: Don't swap. a=0, b=4.

- Bob's turn:

- Must not swap. a=0, b=3.

- Alice's turn:

- Can only swap. a=0, b=3.

- Bob's turn:

- Must not swap. a=0, b=2.

- Alice's turn:

- Swap. a=0, b=2.

- Bob's turn:

- Must not swap. a=0, b=1.

- Alice's turn:

- Swap. a=0, b=1.

- Bob's turn:

- Must not swap. a=0, b=0.

- Alice can't make a move, so Bob wins.

Wait, but the sample output says Alice wins for a=1, b=4. Hmm, maybe I made a mistake in this simulation.

Let me try again.

- Alice's turn:

- Option 1: Swap. a=4, b=1.

- Now, a=4, b=1.

- Bob's turn:

- Option 1: Swap. a=1, b=4.

- Back to the original position.

- Alice's turn:

- Swap again. a=4, b=1.

- This seems like it's cycling.

Wait, perhaps there's a better strategy.

Let me look at the sample output again.

In the second test case, a=1, b=4, and the output is Alice.

But in my simulation, it seems like Bob wins. Maybe I'm missing something.

Let me read the note again.

In the second test case:

- Alice swaps: a=4, b=1.

- Bob swaps: a=1, b=4.

- Alice doesn't swap: a=0, b=4.

- Bob doesn't swap: a=0, b=3.

- Alice swaps: a=0, b=3.

- Bob can't make a move, so Alice wins.

Wait, in my earlier simulation, I thought Bob would continue to decrease b, but according to the note, after Alice swaps, Bob is forced to not swap because a=0.

So, perhaps I need to consider that when a player's wallet is empty, they can't choose to swap.

Wait, no, the rule is that after choosing to swap or not, they must remove one coin from their current wallet, and the wallet can't have zero coins before removing.

So, if a player's wallet is empty, they can't choose to swap because after swapping, they still need to remove a coin, but if their wallet is empty, they can't do that.

Wait, no. The rules are:

1. Choose to exchange wallets with the opponent or keep their current wallets.

2. Remove 1 coin from the player's current wallet. The current wallet cannot have 0 coins before performing this step.

So, if a player's wallet is empty, they cannot perform step 2, hence they lose.

In the note, it shows:

- Alice chooses to swap: a=4, b=1.

- Bob chooses to swap: a=1, b=4.

- Alice chooses not to swap: a=0, b=4.

- Bob must not swap: a=0, b=3.

- Alice chooses to swap: a=0, b=3.

- Bob cannot make a move, so Alice wins.

So, in this sequence, Alice wins.

But in my earlier simulation, I had Alice choosing not to swap initially, leading to Bob winning.

So, perhaps the key is in the choice of swapping or not.

I need to think about the game in terms of game theory, specifically the concept of winning and losing positions.

A position is a losing position if any move from that position leads to a winning position for the opponent.

Conversely, a position is a winning position if there exists at least one move that leads to a losing position for the opponent.

Given that, I need to find a general rule for any a and b.

But considering the large constraints (a and b can be up to 10^9), I need an efficient way to determine the winner.

Looking at the sample input and output:

1 1 -> Bob

1 4 -> Alice

5 3 -> Bob

4 5 -> Alice

11 9 -> Bob

83 91 -> Bob

1032 9307 -> Alice

839204 7281 -> Alice

1000000000 1000000000 -> Bob

53110 2024 -> Bob

Looking for patterns:

- When a and b are both odd or both even, it seems Bob wins in some cases, but not always.

- For a=1, b=1: Bob wins.

- a=1, b=4: Alice wins.

- a=5, b=3: Bob wins.

- a=4, b=5: Alice wins.

- a=11, b=9: Bob wins.

- a=83, b=91: Bob wins.

- a=1032, b=9307: Alice wins.

- a=839204, b=7281: Alice wins.

- a=1000000000, b=1000000000: Bob wins.

- a=53110, b=2024: Bob wins.

Hmm, it's not immediately obvious.

Let me consider the sum of a and b.

- a + b = 2: Bob wins.

- a + b = 5: Alice wins.

- a + b = 8: Bob wins.

- a + b = 9: Alice wins.

- a + b = 20: Bob wins.

- a + b = 174: Bob wins.

- a + b = 1032 + 9307 = 1032 + 9307 = 1032 + 9307 = 1032 + 9307 = 1032 + 9307 = Bob wins.

Wait, 1032 + 9307 = 1032 + 9307 = 1032 + 9307 = 1032 + 9307 = 1032 + 9307 = Alice wins.

Wait, perhaps it's about the parity of a + b.

Looking back:

- a + b = 2: even, Bob wins.

- a + b = 5: odd, Alice wins.

- a + b = 8: even, Bob wins.

- a + b = 9: odd, Alice wins.

- a + b = 20: even, Bob wins.

- a + b = 174: even, Bob wins.

- a + b = 1032 + 9307 = 1032 + 9307 = 1032 + 9307 = 1032 + 9307 = 1032 + 9307 = odd, Alice wins.

- a + b = 839204 + 7281 = even, Alice wins.

- a + b = 1000000000 + 1000000000 = even, Bob wins.

- a + b = 53110 + 2024 = even, Bob wins.

Wait, now I'm getting confused.

Wait, 1032 + 9307 = 1032 + 9307 = 1032 + 9307 = 1032 + 9307 = 1032 + 9307 = 10334.

10334 is even, but output is Alice.

Wait, perhaps it's not just about the sum being even or odd.

Wait, 1032 + 9307 = 1032 + 9307 = 1032 + 9307 = 1032 + 9307 = 1032 + 9307 = 10334, which is even, but Alice wins.

Similarly, 839204 + 7281 = 846485, which is odd, and Alice wins.

Wait, but in the first test case, a=1, b=1: sum=2, even, Bob wins.

Second test case, a=1, b=4: sum=5, odd, Alice wins.

Third test case, a=5, b=3: sum=8, even, Bob wins.

Fourth test case, a=4, b=5: sum=9, odd, Alice wins.

Fifth test case, a=11, b=9: sum=20, even, Bob wins.

Sixth test case, a=83, b=91: sum=174, even, Bob wins.

Seventh test case, a=1032, b=9307: sum=10334, even, Alice wins.

Eighth test case, a=839204, b=7281: sum=846485, odd, Alice wins.

Ninth test case, a=1000000000, b=1000000000: sum=2000000000, even, Bob wins.

Tenth test case, a=53110, b=2024: sum=55134, even, Bob wins.

Looking at this:

- When sum is even:

- Test cases 1,3,5,6,9,10: Bob wins.

- Test case 7: Alice wins.

- When sum is odd:

- Test cases 2,4,8: Alice wins.

Wait, but test case 7 has sum even, and Alice wins.

So, perhaps there's another factor at play.

Alternatively, maybe it's about the difference between a and b.

Looking at the differences:

- Test case 1: diff=0, Bob wins.

- Test case 2: diff=3, Alice wins.

- Test case 3: diff=2, Bob wins.

- Test case 4: diff=1, Alice wins.

- Test case 5: diff=2, Bob wins.

- Test case 6: diff=8, Bob wins.

- Test case 7: diff=8275, Alice wins.

- Test case 8: diff=831923, Alice wins.

- Test case 9: diff=0, Bob wins.

- Test case 10: diff=51086, Bob wins.

Not seeing a clear pattern here.

Maybe I should think in terms of who can force the game to end in an even or odd number of moves.

Each move reduces the total number of coins by one, because one coin is removed each turn.

The game ends when a player can't make a move, which happens when their wallet is empty and they can't swap.

Wait, but swapping can change the wallets, so it's not just about the total number of coins.

I need to think differently.

Perhaps I should consider the game as a Nim game or some other impartial game.

But in this game, the moves are not straightforward like removing objects from heaps.

Let me consider the possible game states.

A game state can be represented by the pair (a, b), where a and b are the number of coins in Alice's and Bob's wallets, respectively.

Each player, on their turn, can choose to swap or not swap, and then remove one coin from their current wallet.

So, from state (a, b), if the player chooses not to swap, they remove one coin from a, resulting in (a-1, b).

If they choose to swap, they swap wallets to get (b, a), and then remove one coin from b, resulting in (b, a-1).

Wait, no.

If they choose to swap, they exchange wallets, so their wallets become (b, a), and then they remove one coin from their current wallet, which is now b, so it becomes (b-1, a).

So, from (a, b):

- Option 1: Don't swap. Then remove one from a: (a-1, b).

- Option 2: Swap. Then remove one from b: (b-1, a).

So, the possible next states are (a-1, b) and (b-1, a).

Now, this is starting to look like a standard impartial game where we can find the Grundy numbers for each position.

But with a and b up to 10^9, calculating Grundy numbers directly is impossible due to time and space constraints.

I need a smarter way to determine the winner.

Let me consider the parity of a and b.

Looking back at the sample outputs:

- When a and b are both odd or both even, Bob wins.

- When one is odd and the other is even, Alice wins.

Wait, let's check:

Test case 1: a=1, b=1 (both odd), Bob wins.

Test case 2: a=1, b=4 (one odd, one even), Alice wins.

Test case 3: a=5, b=3 (both odd), Bob wins.

Test case 4: a=4, b=5 (one even, one odd), Alice wins.

Test case 5: a=11, b=9 (both odd), Bob wins.

Test case 6: a=83, b=91 (both odd), Bob wins.

Test case 7: a=1032, b=9307 (one even, one odd), Alice wins.

Test case 8: a=839204, b=7281 (one even, one odd), Alice wins.

Test case 9: a=1000000000, b=1000000000 (both even), Bob wins.

Test case 10: a=53110, b=2024 (both even), Bob wins.

So, it seems that:

- If a and b have the same parity (both even or both odd), Bob wins.

- If a and b have different parities, Alice wins.

Wait, but test case 7: a=1032 (even), b=9307 (odd), Alice wins.

Test case 8: a=839204 (even), b=7281 (odd), Alice wins.

Test case 9: a=1000000000 (even), b=1000000000 (even), Bob wins.

Test case 10: a=53110 (even), b=2024 (even), Bob wins.

Yes, this seems consistent.

So, the winning condition could be:

- If a and b have the same parity, Bob wins.

- If a and b have different parities, Alice wins.

But why is that?

Let me try to find a logical explanation.

Suppose a and b have the same parity.

Then, the sum a + b is even.

In each turn, one coin is removed, so the parity of the sum changes each turn.

The game ends when one player can't make a move, which happens when both a and b are zero.

Wait, no. The game ends when a player cannot remove a coin from their current wallet.

That is, when their current wallet has zero coins, and they can't swap to the other wallet if it's also zero.

Wait, but if a player has a > 0, they can choose not to swap and remove a coin.

If a = 0, they must swap if b > 0, and remove a coin from b.

If both a and b are zero, the player can't make a move and loses.

So, the game continues until both a and b are zero.

But in reality, the game ends when a player is unable to make a move, which is when a = 0 and b = 0.

Wait, no. If a > 0, the player can choose not to swap and remove a coin.

If a = 0, the player must swap if b > 0 and remove a coin from b.

If both a and b are zero, the player can't make a move.

So, the game ends when a player is faced with a = 0 and b = 0.

But in practice, the game can't reach a = 0 and b = 0 because the previous player would have to make the move that leaves a = 0 and b = 0.

Wait, no. Let's think about it step by step.

Suppose a = 1, b = 1.

- Alice's turn: choose not to swap, a = 0, b = 1.

- Bob's turn: must not swap (since a = 0), remove 1 from b, b = 0.

- Alice's turn: a = 0, b = 0. Can't make a move. Bob wins.

If Alice chooses to swap initially:

- a = 1, b = 1.

- Bob's turn: choose to swap, a = 1, b = 1.

- Alice's turn: choose not to swap, a = 0, b = 1.

- Bob's turn: must not swap, b = 0.

- Alice's turn: a = 0, b = 0. Can't make a move. Bob wins.

So, in this case, Bob wins.

Now, a = 1, b = 4.

- Alice's turn: choose to swap, a = 4, b = 1.

- Bob's turn: choose to swap, a = 1, b = 4.

- Alice's turn: choose not to swap, a = 0, b = 4.

- Bob's turn: must not swap, b = 3.

- Alice's turn: choose to swap, a = 0, b = 3.

- Bob's turn: must not swap, b = 2.

- Alice's turn: choose to swap, a = 0, b = 2.

- Bob's turn: must not swap, b = 1.

- Alice's turn: choose to swap, a = 0, b = 1.

- Bob's turn: must not swap, b = 0.

- Alice's turn: a = 0, b = 0. Can't make a move. Bob loses.

Wait, but according to the note, Alice wins.

Wait, in the note, it says Bob cannot make a move, so Alice wins.

But in my simulation, it seems like Bob loses when a=0 and b=0.

Wait, perhaps I need to think differently.

Maybe the player who is faced with a=0 and b=0 loses, because they can't make a move.

So, if a + b is even, Bob wins; otherwise, Alice wins.

But test case 7: a=1032, b=9307. Sum is even, but Alice wins.

Wait, 1032 + 9307 = 10339, which is odd. Wait, 1032 is even, 9307 is odd, sum is odd. Alice wins.

Wait, in my earlier assumption, if sum is odd, Alice wins; if sum is even, Bob wins.

But test case 1: sum=2, even, Bob wins.

Test case 2: sum=5, odd, Alice wins.

Test case 3: sum=8, even, Bob wins.

Test case 4: sum=9, odd, Alice wins.

Test case 5: sum=20, even, Bob wins.

Test case 6: sum=174, even, Bob wins.

Test case 7: sum=10339, odd, Alice wins.

Test case 8: sum=846485, odd, Alice wins.

Test case 9: sum=2000000000, even, Bob wins.

Test case 10: sum=55134, even, Bob wins.

Yes, so it seems that if a + b is even, Bob wins; if a + b is odd, Alice wins.

But in test case 7, a=1032, b=9307: 1032 + 9307 = 10339, which is odd, Alice wins.

So, the rule seems to hold.

Wait, but earlier I thought that if a and b have the same parity, Bob wins; otherwise, Alice wins.

But a + b is even if and only if a and b have the same parity.

So, yes, same parity: Bob wins; different parity: Alice wins.

Hence, the winning condition is based on the parity of a + b.

So, the program provided:

def func():

t = int(input())

for i in range(t):

s = input()

a = int(list(s.split())[0])

b = int(list(s.split())[1])

if (a + b) % 2 == 0:

print('Bob')

else:

print('Alice')

This seems correct based on the analysis.

Therefore, the program is correct.

**Final Answer**

\boxed{\text{The given program is correct.}}