Alright, I've got this problem to solve. Let's see what it's asking for. So, Nikita has some cubes, and he wants to build a tower by adding or removing one cube at a time in each move. The tower starts with no cubes, and after a certain number of moves, n, I need to figure out if it's possible to have exactly m cubes on the tower.

First, I need to understand the operations he can perform. In each move, he can either add one cube to the top or remove one cube from the top. So, it's always one cube at a time, and he can't remove a cube if there isn't one there.

Okay, so let's think about this. If he has n moves, and each move is either adding or removing a cube, I need to find out if there's a sequence of these adds and removes that results in exactly m cubes on the tower.

Let me try to model this mathematically. Let's say he adds a cube x times and removes a cube y times. Then, the total number of moves is n = x + y. The net effect on the number of cubes in the tower is x - y, because each add increases the count by one and each remove decreases it by one. So, the final number of cubes is x - y.

But wait, the tower can't have a negative number of cubes. If he tries to remove a cube when there are none, maybe that's not allowed. So, I have to consider that he can't remove a cube if there aren't any cubes on the tower.

Hmm, that complicates things. So, the sequence of adds and removes has to be such that he never tries to remove a cube when there are zero cubes.

But maybe there's a simpler way to look at it. Let's consider that the final number of cubes is x - y, and n = x + y. I can solve these equations.

From n = x + y and m = x - y, I can add these two equations to get n + m = 2x, so x = (n + m)/2. Similarly, subtracting the second equation from the first gives n - m = 2y, so y = (n - m)/2.

So, for x and y to be integers (since you can't have half a move), both (n + m) and (n - m) must be even numbers. Because x and y must be integers.

Wait, but actually, since x and y are counts of actions, they have to be non-negative integers.

So, not only do (n + m) and (n - m) need to be even, but also y = (n - m)/2 must be non-negative, meaning n - m >= 0.

Wait, but m could be greater than n, right? For example, if n=3 and m=4, is that possible?

Let me see: if n=3 and m=4, then x = (3+4)/2 = 3.5, which is not an integer, so it's impossible. So, in this case, the answer should be "No".

In the example provided, for n=3 and m=3, the answer is "Yes", which makes sense because he can add three times: +1, +1, +1, to get 3 cubes.

For n=2 and m=4, it's "No", which aligns with what I just thought about n=3 and m=4.

For n=5 and m=3, it's "Yes". Let's see: x = (5+3)/2 = 4, y = (5-3)/2 = 1. So, he adds 4 times and removes 1 time. One possible sequence could be: +1, +1, +1, +1, -1, resulting in 3 cubes.

But wait, the sequence matters because you can't remove a cube if there isn't one. In this sequence, he adds four times to get to 4, then removes one to get to 3. That's fine.

But what if he tries to remove before having enough cubes? For example, sequence: +1, -1, +1, +1, +1. That would also end up with 3 cubes, but he removes one after adding one, which is allowed.

Another sequence: -1, +1, +1, +1, +1. But removing one when there are zero cubes isn't allowed. So, this sequence is invalid because he can't remove a cube when there are none.

So, to ensure the sequence is valid, I need to make sure that at no point does the number of removes exceed the number of adds up to that point.

But checking all possible sequences sounds complicated. Is there a simpler way?

Well, from the earlier equations, x = (n + m)/2 and y = (n - m)/2, and both x and y must be integers and y >= 0.

Additionally, since he can't remove more cubes than he has at any point, the sequence must maintain a certain order.

But in the condition I have so far, if x and y are integers and y >= 0, that seems to cover it.

Wait, but in the case where n=2 and m=4, x = (2+4)/2=3, y=(2-4)/2=-1, which is invalid because y < 0. So, correctly, it's "No".

In the case where n=5 and m=3, x=4, y=1, which is valid.

But what about n=4 and m=0? x=(4+0)/2=2, y=(4-0)/2=2. So, he adds twice and removes twice, in some order, ending up with zero cubes.

A possible sequence: +1, +1, -1, -1. That's fine.

Another sequence: +1, -1, +1, -1. Also fine.

What about n=1 and m=0? x=(1+0)/2=0.5, which is not an integer, so "No".

n=1 and m=1: x=1, y=0. That's fine; he just adds one cube.

So, based on this, it seems that the condition is:

- (n + m) is even

- (n - m) is even

- (n - m)/2 >= 0

Because y must be non-negative.

Wait, but (n - m)/2 >= 0 is equivalent to n >= m.

So, combining these, the condition simplifies to:

- n >= m

- (n - m) is even

Wait, but in the earlier example, for n=5 and m=3, (n - m)=2, which is even, and n >= m.

For n=3 and m=3, (n - m)=0, which is even, and n >= m.

For n=2 and m=4, (n - m)=-2, which is less than zero, so y would be negative, invalid.

So, seems like the conditions are n >= m and (n - m) is even.

But wait, in the earlier case where n=4 and m=0, (n - m)=4, which is even, and n >= m, which is valid.

n=1 and m=1, (n - m)=0, which is even, and n >= m, valid.

n=1 and m=0, (n - m)=1, which is odd, so invalid.

Wait, but earlier I thought n=1 and m=0 should be invalid because x and y aren't integers, and indeed, (n - m)=1 is odd.

Wait, no, (n - m)=1 is odd, but in my earlier condition, I said (n - m) is even.

Wait, perhaps I need to rethink this.

Wait, from x = (n + m)/2 and y = (n - m)/2, both x and y need to be integers.

So, (n + m) and (n - m) must both be even, or both must be odd, but since their sum is 2n, which is always even, they must both be even.

Wait, no, if n and m are both integers, then (n + m) and (n - m) are both even only if n and m are both even or both odd.

But in the condition, both (n + m) and (n - m) being even is equivalent to n and m being both even or both odd.

Wait, but in the earlier example, n=3, m=3: both odd, (n - m)=0, which is even, valid.

n=5, m=3: both odd, (n - m)=2, even, valid.

n=2, m=4: both even, (n - m)= -2, which is invalid because y would be negative.

n=1, m=1: both odd, (n - m)=0, even, valid.

n=1, m=0: one odd, one even, (n - m)=1, odd, invalid.

So, seems like the condition is:

- n >= m

- n and m are both even or both odd

Which is equivalent to (n - m) is even and n >= m.

So, in the program, it's checking if (n - m) % 2 == 0 and n - m >= 0.

Which aligns with my condition.

Wait, but in the program, it's checking if (n - m) % 2 == 0 and n - m >= 0.

Which is exactly what I derived.

So, in the example:

3 3: (3 - 3) = 0, which is even, and 3 >= 3, so "Yes"

2 4: (2 - 4) = -2, which is even, but 2 < 4, so invalid, "No"

5 3: (5 - 3) = 2, which is even, and 5 >= 3, so "Yes"

Perfect, matches the expected output.

Let me think about another test case.

n=4, m=0: (4 - 0)=4, even, 4 >= 0, "Yes"

n=3, m=2: (3 - 2)=1, odd, "No"

n=4, m=2: (4 - 2)=2, even, 4 >= 2, "Yes"

n=5, m=5: (5 - 5)=0, even, 5 >= 5, "Yes"

n=6, m=1: (6 - 1)=5, odd, "No"

Seems consistent.

But wait, is there any case where n and m are both even, (n - m) is even, n >= m, but it's actually impossible due to the sequence constraints?

For example, n=4, m=2: x=3, y=1. Sequence: +1, +1, +1, -1, ending with 2 cubes.

Another sequence: +1, -1, +1, +1. Still ends with 2.

In both cases, it's valid.

What about n=4, m=0: x=2, y=2. Sequence: +1, +1, -1, -1.

Or +1, -1, +1, -1.

Both are valid.

What about n=3, m=1: x=2, y=1. Sequence: +1, +1, -1, ending with 1.

Or +1, -1, +1, ending with 1.

Both valid.

Seems like the condition holds.

But what about n=1, m=0: x=0.5, y=0.5, which are not integers, so invalid.

But according to my earlier condition, (1 - 0)=1, which is odd, so "No", which is correct.

Another case: n=2, m=0: x=1, y=1. Sequence: +1, -1, ending with 0.

Or -1, +1, but -1 when there are zero cubes is invalid.

Wait a minute, in the sequence -1, +1, he tries to remove a cube when there are zero cubes, which is invalid.

But according to my condition, (2 - 0)=2, even, 2 >= 0, so "Yes".

But the sequence -1, +1 is invalid.

Wait, but the sequence +1, -1 is valid, so as long as there's at least one valid sequence, it should be "Yes".

Hence, even though one invalid sequence exists, there's at least one valid sequence, so it's "Yes".

So, the condition seems sufficient.

Another way to think about it is that the number of adds must always be at least the number of removes up to any point in the sequence.

This is similar to the concept of Catalan numbers in combinatorics, where you have sequences of plus and minus ones with certain constraints.

But I don't need to go into that much detail for this problem.

Given that, it seems that the condition in the program is correct.

Let me look at the program again.

The program reads t, the number of test cases, then for each test case, it calls func_1().

In func_1(), it reads n and m, then checks if (n - m) % 2 == 0 and n - m >= 0.

If yes, prints "Yes"; else, "No".

This aligns with my reasoning.

Hence, the program is correct.

**Final Answer**

\[\boxed{\text{Yes}}\]

**Correctness: True**