Let's break down the problem step by step:

1. **Initial State:**
   - `a` is explicitly given as 2.
   - `L` is a list `[2, 1, 1, 1, 1, 1]`.
   - `tot` is less than `k`.
   - `k` is less than or equal to the sum of `tot` plus the value of `a`.

2. **Expression to Evaluate:**
   - The expression inside the `print` statement is `pow * (2 * (k - tot) - 1)`.

3. **Identify Variables and Their Values:**
   - `a = 2`.
   - `L = [2, 1, 1, 1, 1, 1]`.
   - Since `tot < k` and `k <= tot + a`, let's denote `tot` as some value less than `k`. For simplicity, let's assume `tot = 1` and `k = 2` (since `k` must be greater than `tot` but less than or equal to `tot + a`).

4. **Evaluate the Expression:**
   - Substitute `k = 2` and `tot = 1` into the expression:
     \[
     \text{Expression} = \text{pow} \times (2 \times (2 - 1) - 1)
     \]
   - Simplify the expression:
     \[
     \text{Expression} = \text{pow} \times (2 \times 1 - 1) = \text{pow} \times (2 - 1) = \text{pow} \times 1 = \text{pow}
     \]

5. **Determine the Value of `pow`:**
   - The variable `pow` is not explicitly defined in the initial state. Given the context, it is likely a typo or placeholder for a power operation. If we assume `pow` is meant to be a power operation, it would typically be something like `2**n` where `n` is an integer. Without further context, let's assume `pow` is `2` (a common base for such operations).

6. **Final Calculation:**
   - If `pow = 2`, then the expression evaluates to:
     \[
     2
     \]

Therefore, the output of the print statement is:

Output: **2**