Output State: `t` must be at least 1, `n` must be greater than 4, `i` is `n + 1`, `sum` is 20.

To understand this, let's break down the loop and its effect on the `sum` variable. The loop iterates from `i = 2` to `i = n`, and in each iteration, it updates `sum` as follows:

\[ \text{sum} += (i^2 - (i-1)^2) \times i \]

Simplifying the expression inside the loop:

\[ i^2 - (i-1)^2 = i^2 - (i^2 - 2i + 1) = 2i - 1 \]

So the update to `sum` in each iteration becomes:

\[ \text{sum} += (2i - 1) \times i = 2i^2 - i \]

Summing these up from `i = 2` to `i = n`:

\[ \text{sum} = \sum_{i=2}^{n} (2i^2 - i) \]

This can be simplified further, but for our purposes, we know that after 3 iterations, `i` is 4 and `sum` is 20. Since the loop continues until `i` reaches `n + 1`, the final value of `i` will be `n + 1`. Given that the loop has completed all its iterations, `n` must be greater than 4, and the final value of `sum` will be the result of the loop's execution up to `i = n + 1`.