Given the initial state and the loop described, let's break down the problem step-by-step:

1. **Initial State:**
   - `t` must be at least 1.
   - `n` must be greater than 4.
   - `i` is set to `n + 1`.
   - `sum` is initially 20.

2. **Loop Execution:**
   - The loop runs from `i = 2` to `i = n`.
   - In each iteration, `sum` is updated by the formula: `sum += (2i^2 - i)`.
   - After 3 iterations, `i` is 4 and `sum` is 20.

3. **Final Iteration Analysis:**
   - The loop continues until `i` reaches `n + 1`.
   - Since `i` starts at `n + 1` and the loop increments `i` from 2 to `n`, the loop must have completed all iterations up to `i = n + 1`.

4. **Calculating the Final Value of `sum`:**
   - We need to determine the value of `sum` after the loop completes.
   - The loop updates `sum` as follows:
     \[
     \text{sum} += (2i^2 - i)
     \]
   - For `i = 2` to `i = n`, the loop updates `sum` accordingly.
   - Given that after 3 iterations (`i = 4`), `sum` is 20, we need to find the value of `sum` when `i = n + 1`.

5. **Determining `n`:**
   - Since the loop runs from `i = 2` to `i = n` and `i` is set to `n + 1` initially, `n` must be such that the loop completes all iterations up to `i = n + 1`.
   - If `i` is 4 after 3 iterations, then `n` must be 3, but since `n` must be greater than 4, we need to consider the next value.
   - Let's assume `n = 5` (the smallest value greater than 4 that fits the pattern).
   - When `i = 6` (which is `n + 1`), the loop would have completed all iterations from `i = 2` to `i = 5`.

6. **Final Calculation:**
   - We need to calculate the sum for `i = 2` to `i = 5`:
     \[
     \text{sum} = \sum_{i=2}^{5} (2i^2 - i)
     \]
   - Calculate each term:
     \[
     \begin{align*}
     i = 2: & \quad 2(2^2) - 2 = 8 - 2 = 6 \\
     i = 3: & \quad 2(3^2) - 3 = 18 - 3 = 15 \\
     i = 4: & \quad 2(4^2) - 4 = 32 - 4 = 28 \\
     i = 5: & \quad 2(5^2) - 5 = 50 - 5 = 45 \\
     \end{align*}
     \]
   - Sum these values:
     \[
     \text{sum} = 6 + 15 + 28 + 45 = 94
     \]

7. **Final Output:**
   - The loop completes, and the final value of `sum` is 94.
   - `n + n` is `5 + 5 = 10`.

Therefore, the output will be:
Output: **94, 10**