Let's break down the initial state and the print statement step by step:

1. **Initial State:**
   - `j` is defined as `k + 1`.
   - `n` must be the same as before, but no specific value for `n` is provided in the initial state. We need to assume a value for `n` since it's not explicitly given.

2. **Print Statement:**
   - The print statement is `print(1, n - j + 1, *range(1, n + 1))`.

Given these details, let's assume a value for `n` and `k` to proceed with the calculation. Since `n` is not specified, let's assume `n = 5` and `k = 3` for demonstration purposes.

- If `k = 3`, then `j = k + 1 = 3 + 1 = 4`.
- Now, substituting `n = 5` and `j = 4` into the print statement:
  - `1` is directly printed.
  - `n - j + 1 = 5 - 4 + 1 = 2`.
  - `*range(1, n + 1)` will print the range from 1 to `n` inclusive, which is `1, 2, 3, 4, 5`.

Therefore, the output of the print statement will be:
Output: **1 2 1 2 3 4 5**