Output State: **The loop has executed from \( j = 1 \) to \( j = n \), updating the sum according to the formula \( \text{sum} += 2i^2 - i \) for each \( i \) from 2 to \( n + 1 \). The final value of `sum` is the result of this summation.**

Given that the loop has completed all its iterations, the final value of `sum` will be the sum of the series \( \sum_{i=2}^{n+1} (2i^2 - i) \). Since the initial state provided does not give specific values for `n` and `sum` after the first three iterations, we can infer that after all iterations, `i` will be `n + 1`, and the `sum` will be the result of the loop's execution from `i = 2` to `i = n + 1`.

Since the exact value of `n` is not provided, the output state will be the final value of `sum` after the loop has completed all its iterations, which is the sum of the series as described.