The value of `dp[j]` is increased by `dp[j - 1]`. Given that `j` is `f_max_n - 1` and `dp[i]` = 0 for `i` from 1 to `f_max_n`, we can deduce that initially `dp[f_max_n - 1]` = 0 and `dp[f_max_n - 2]` = 0. However, `dp[0]` = 1 and we are adding `dp[j - 1]` to `dp[j]`, which means we now have `dp[f_max_n - 1]` = `dp[f_max_n - 2]`. But since `dp[f_max_n - 2]` = 0, we get `dp[f_max_n - 1]` = 0. The value of `n` is still greater than 0, `f_max_n` is a positive integer greater than or equal to 1, `MOD` is still `1000000007`, `dp` is still a list of size `f_max_n + 1` but now `dp[f_max_n - 1]` = `dp[f_max_n - 2]` = 0. The variable `i` is 1 and `j` is `f_max_n - 1`. 

Output State: **`n` is greater than 0, `f_max_n` is a positive integer greater than or equal to 1, `MOD` is `1000000007`, `dp` is a list of size `f_max_n + 1` where `dp[0]` = 1 and `dp[i]` = 0 for `i` from 1 to `f_max_n`, `dp[f_max_n - 1]` = `dp[f_max_n - 2]` = 0, `i` is 1, `j` is `f_max_n - 1**