The code `x, y = y, x % y` assigns the current value of `y` to `x` and the remainder of `x` divided by `y` to `y`. Given the initial state where `x` is the original value of `y` and `y` is `x % y` (with `y` being non-zero), we can determine the new values of `x` and `y`.

1. Initially, `x = y` and `y = x % y`.
2. After executing the code, `x` becomes `y` and `y` becomes `x % y`.

Since `y = x % y`, substituting `x` with `y` in the second part gives us `y = y % y`. The remainder of any number divided by itself is 0. However, since `y` is non-zero, the condition holds, and the value remains unchanged.

Therefore, after the code execution:
- `x` is now `y`.
- `y` is still `x % y`, which simplifies to `y % y = 0` but remains `y` because `y` is non-zero.

Output State: **`x` is `y`, `y` is `x % y`**