The code calculates the sum of the first `k` positive integers using the formula `sum_k = k * (k + 1) // 2`. Here, `k` is defined as `a + b - 1`. Since the values of `a` and `b` are positive integers, `k` is also a positive integer. The formula `k * (k + 1) // 2` computes the sum of the first `k` positive integers.

Given the initial state:
- `m` is a non-negative integer such that \(1 \leq m \leq 10^9\)
- `a` is a positive integer such that \(1 \leq a \leq 10^5\)
- `b` is a positive integer such that \(1 \leq b \leq 10^5\)
- `g` is equal to 1
- `k` is `a + b - 1`
- \(m \geq k\)

After executing the code, the value of `sum_k` is calculated as follows:
- `k = a + b - 1`
- `sum_k = k * (k + 1) // 2`

Therefore, the Output State is:
Output State: **`m` is a non-negative integer such that \(1 \leq m \leq 10^9\), `a` is a positive integer such that \(1 \leq a \leq 10^5\), `b` is a positive integer such that \(1 \leq b \leq 10^5\), `g` is equal to 1, `k` is `a + b - 1`, \(m \geq k\), and `sum_k` is \(k * (k + 1) // 2**.