To determine what the `print` statement will output, let's break down the code and the initial state provided.

### Initial State Recap:
- `t` is at least 1 (though `t` is not used in the print statement, it's part of the initial state).
- `s` is the first line of input starting from the second line.
- `n` is the first integer from the split of `s`.
- `k` is the second integer from the split of `s`.

### Code Breakdown:
The print statement is:
```python
print((k // 2 + k % 2) * (k < 4 * n - 3) + 2 * n * (k >= 4 * n - 3) + (k == 4 * n - 2))
```

Let's break this down into parts:
1. **`(k // 2 + k % 2)`**: This expression calculates the ceiling of `k/2`. If `k` is even, `k // 2 + k % 2` is `k // 2`. If `k` is odd, `k // 2 + k % 2` is `k // 2 + 1`.
2. **`(k < 4 * n - 3)`**: This is a boolean expression that evaluates to `1` if `k` is less than `4 * n - 3`, and `0` otherwise.
3. **`(k >= 4 * n - 3)`**: This is a boolean expression that evaluates to `1` if `k` is greater than or equal to `4 * n - 3`, and `0` otherwise.
4. **`(k == 4 * n - 2)`**: This is a boolean expression that evaluates to `1` if `k` is equal to `4 * n - 2`, and `0` otherwise.

### Combining the Expressions:
- The term `(k // 2 + k % 2) * (k < 4 * n - 3)` will contribute its value only if `k < 4 * n - 3`. Otherwise, it will contribute `0`.
- The term `2 * n * (k >= 4 * n - 3)` will contribute its value only if `k >= 4 * n - 3`. Otherwise, it will contribute `0`.
- The term `(k == 4 * n - 2)` will contribute `1` if `k` is exactly `4 * n - 2`, otherwise, it will contribute `0`.

### Possible Scenarios:
1. **If `k < 4 * n - 3`**:
   - The first term `(k // 2 + k % 2) * (k < 4 * n - 3)` will be `(k // 2 + k % 2)`.
   - The second term `2 * n * (k >= 4 * n - 3)` will be `0`.
   - The third term `(k == 4 * n - 2)` will be `0` unless `k` is exactly `4 * n - 2`, but since `k < 4 * n - 3`, it will be `0`.
   - **Output**: `(k // 2 + k % 2)`

2. **If `k == 4 * n - 3`**:
   - The first term `(k // 2 + k % 2) * (k < 4 * n - 3)` will be `0`.
   - The second term `2 * n * (k >= 4 * n - 3)` will be `2 * n`.
   - The third term `(k == 4 * n - 2)` will be `0`.
   - **Output**: `2 * n`

3. **If `k == 4 * n - 2`**:
   - The first term `(k // 2 + k % 2) * (k < 4 * n - 3)` will be `0`.
   - The second term `2 * n * (k >= 4 * n - 3)` will be `2 * n`.
   - The third term `(k == 4 * n - 2)` will be `1`.
   - **Output**: `2 * n + 1`

4. **If `k > 4 * n - 2`**:
   - The first term `(k // 2 + k % 2) * (k < 4 * n - 3)` will be `0`.
   - The second term `2 * n * (k >= 4 * n - 3)` will be `2 * n`.
   - The third term `(k == 4 * n - 2)` will be `0`.
   - **Output**: `2 * n`

### Conclusion:
The output depends on the value of `k` relative to `4 * n - 3` and `4 * n - 2`.

- If `k < 4 * n - 3`, the output is `(k // 2 + k % 2)`.
- If `k == 4 * n - 3`, the output is `2 * n`.
- If `k == 4 * n - 2`, the output is `2 * n + 1`.
- If `k > 4 * n - 2`, the output is `2 * n`.

### Final Output:
Output: **(k // 2 + k % 2) if k < 4 * n - 3, 2 * n if k == 4 * n - 3, 2 * n + 1 if k == 4 * n - 2, 2 * n if k > 4 * n - 2**