The expression `dp[n, k] += 9 * 10 ** (i - 1) * (10 ** (k - i) - 10 ** (i - 1))` modifies the value of `dp[n, k]`. 

1. The current value of `dp[n, k]` is 9.
2. The variable `i` is 1, so `i - 1` equals 0.
3. The expression `10 ** (i - 1)` evaluates to `10 ** 0`, which is 1.
4. The expression `k - i` is `k - 1`, and `10 ** (k - i)` evaluates to `10 ** (k - 1)`.
5. Therefore, the term `(10 ** (k - i) - 10 ** (i - 1))` simplifies to `(10 ** (k - 1) - 1)`.
6. The complete expression becomes: `dp[n, k] += 9 * 1 * (10 ** (k - 1) - 1)`, which simplifies to `dp[n, k] += 9 * (10 ** (k - 1) - 1)`.

The value of `dp[n, k]` is updated based on the calculation above. 

Output State: **`l` is an integer such that 1 <= `l` <= `r` < 10^18, `r` is an integer such that 1 <= `l` <= `r` < 10^18, `k` is greater than 1 and less than or equal to 10, `n` is greater than or equal to 10 raised to the power of `k`, `dp[n, k]` is updated, and `i` is 1**.