Alright, I've got this problem to solve. Let me read it carefully.

So, I'm given two positive integers, n and m, and I need to find the number of ordered pairs (a, b) where 1 ≤ a ≤ n and 1 ≤ b ≤ m, with the condition that a + b is a multiple of b multiplied by the greatest common divisor of a and b. In mathematical terms, a + b is a multiple of b * gcd(a, b).

First, I need to understand what this condition means. Let's denote gcd(a, b) as g. Then, b * g divides a + b. So, b * g | a + b.

I know that g divides both a and b, since g is the greatest common divisor of a and b. So, a = g * a' and b = g * b', where a' and b' are positive integers that are coprime (their gcd is 1).

Substituting these into the condition:

b * g | a + b ⇒ g * b' * g | (g * a' + g * b') ⇒ g^2 * b' | g(a' + b') ⇒ g * b' | a' + b'

Since a' and b' are coprime, and b' divides a' + b', then b' divides a' + b'. But b' divides itself, so b' divides a'.

Wait, but a' and b' are coprime, and b' divides a', which implies that b' must be 1.

So, b' = 1.

This means that b = g * 1 = g.

And since b = g, and a = g * a', and a' and b' are coprime, but b' = 1, then a' and 1 are coprime, which is always true.

So, b = gcd(a, b).

Therefore, the condition simplifies to b = gcd(a, b).

Now, I need to find the number of pairs (a, b) where 1 ≤ a ≤ n, 1 ≤ b ≤ m, and b = gcd(a, b).

This seems more manageable.

Given that b = gcd(a, b), it means that b divides a, because gcd(a, b) divides both a and b.

So, b divides a.

Moreover, since gcd(a, b) = b, and b divides a, we can write a = k * b, where k is a positive integer.

So, a is a multiple of b.

Therefore, for each b from 1 to m, I need to find the number of a in the range 1 to n such that a is a multiple of b.

In other words, for each b in [1, m], count the number of multiples of b that are ≤ n.

This is equivalent to floor(n / b) for each b.

So, the total number of valid pairs is the sum over b from 1 to m of floor(n / b).

Wait, but is that all?

Let me verify with the sample input.

First sample input:

6

1 1

2 3

3 5

10 8

100 1233

1000000 1145141

Corresponding outputs:

1

3

4

14

153

1643498

Let's check the first one: n=1, m=1.

floor(1/1) = 1, which matches the output.

Second one: n=2, m=3.

floor(2/1) + floor(2/2) + floor(2/3) = 2 + 1 + 0 = 3, which matches.

Third one: n=3, m=5.

floor(3/1) + floor(3/2) + floor(3/3) + floor(3/4) + floor(3/5) = 3 + 1 + 1 + 0 + 0 = 5, but the output is 4. Hmm, that doesn't match.

Wait, perhaps I missed something.

Wait, perhaps the condition is more restrictive.

Let me go back.

I had b = gcd(a, b), and a = k * b.

But in this case, gcd(a, b) = b, which is correct.

Wait, maybe I need to consider that a and b are positive integers within their respective ranges.

Wait, perhaps I need to consider that for each b, a must be a multiple of b, and a <= n.

So, for b=1, a can be 1,2,3 in the third sample.

For b=2, a can be 2.

For b=3, a can be 3.

For b=4, a can be 4, but 4 > 3, so no.

For b=5, a can be 5, but 5 > 3, so no.

So, only b=1,2,3 are valid, with a=1,2,3 respectively.

Wait, but the output is 4, which suggests that there are 4 valid pairs.

But according to my calculation, it should be 3.

Wait, perhaps I'm missing some pairs.

Wait, let's list all possible pairs:

(1,1): 1+1=2, b*gcd(1,1)=1*1=1, and 2 is a multiple of 1. Yes.

(1,2): 1+2=3, b*gcd(1,2)=2*1=2, and 3 is not a multiple of 2. No.

(1,3): 1+3=4, b*gcd(1,3)=3*1=3, and 4 is not a multiple of 3. No.

(2,1): 2+1=3, b*gcd(2,1)=1*1=1, and 3 is a multiple of 1. Yes.

(2,2): 2+2=4, b*gcd(2,2)=2*2=4, and 4 is a multiple of 4. Yes.

(2,3): 2+3=5, b*gcd(2,3)=3*1=3, and 5 is not a multiple of 3. No.

(3,1): 3+1=4, b*gcd(3,1)=1*1=1, and 4 is a multiple of 1. Yes.

(3,2): 3+2=5, b*gcd(3,2)=2*1=2, and 5 is not a multiple of 2. No.

(3,3): 3+3=6, b*gcd(3,3)=3*3=9, and 6 is not a multiple of 9. No.

So, the valid pairs are (1,1), (2,1), (2,2), (3,1), which is 4 pairs. That matches the sample output.

But according to my earlier reasoning, I had only considered b dividing a, which for b=1,2,3 gives a=1,2,3 respectively, totaling 3 pairs, but the correct count is 4.

So, I must have missed something.

Wait, in the pair (2,2), b=2 and a=2. b divides a, which is fine, and gcd(2,2)=2, so b*gcd(a,b)=2*2=4, and a+b=4, which is a multiple of 4. So, it's valid.

Similarly, for (2,1), b=1, gcd(2,1)=1, b*gcd=1, a+b=3, which is a multiple of 1. So, it's valid.

And for (3,1), b=1, gcd(3,1)=1, b*gcd=1, a+b=4, which is a multiple of 1.

And for (1,1), b=1, gcd(1,1)=1, b*gcd=1, a+b=2, which is a multiple of 1.

So, all pairs where b divides a are valid, but in the earlier calculation, I thought that for b=1, a can be 1,2,3; for b=2, a can be 2; for b=3, a can be 3. That's 3 + 1 + 1 = 5, but in reality, (2,2) is also valid, which is an additional pair.

Wait, no, in the earlier enumeration, (2,2) is included because b=2 divides a=2.

Wait, perhaps my mistake was in calculating floor(n / b) for each b.

For n=3, m=5:

b=1: floor(3/1)=3 (a=1,2,3)

b=2: floor(3/2)=1 (a=2)

b=3: floor(3/3)=1 (a=3)

b=4: floor(3/4)=0

b=5: floor(3/5)=0

Total: 3 + 1 + 1 + 0 + 0 = 5, but the correct answer is 4.

Wait, but according to the sample, it's 4. So, I must be overcounting.

Looking back at the valid pairs: (1,1), (2,1), (3,1), (2,2). So, 4 pairs.

But according to floor(n / b), for b=1:3; b=2:1; b=3:1; total 5, but only 4 are valid.

Wait, perhaps there's an overlap or some pairs are being double-counted, but that doesn't make sense because each a and b are unique pairs.

Wait, perhaps the condition is not solely b divides a.

Wait, going back to the original condition: a + b is a multiple of b * gcd(a, b).

I had simplified it to b = gcd(a, b), which implies b divides a.

But perhaps there are cases where b divides a, but the original condition isn't satisfied.

Wait, in the sample with n=3 and m=5, according to the sample, only 4 pairs are valid, but floor(n / b) sums to 5.

So, perhaps not all pairs where b divides a satisfy the original condition.

Wait, in the pair (2,2): b=2, a=2, a+b=4, b*gcd(a,b)=2*2=4, and 4 is a multiple of 4. So, it's valid.

Similarly, (1,1):1+1=2,1*1=1,2 is a multiple of 1.

(2,1):2+1=3,1*1=1,3 is a multiple of 1.

(3,1):3+1=4,1*1=1,4 is a multiple of 1.

So, all pairs where b divides a seem to satisfy the condition.

Wait, but according to the sample, only 4 pairs are valid, but there are 5 such pairs where b divides a.

Wait, what's going on?

Wait, perhaps I miscounted the valid pairs.

Wait, in n=3, m=5:

Possible a:1,2,3; b:1,2,3,4,5

Pairs where b divides a:

(1,1)

(2,1),(2,2)

(3,1),(3,3)

That's 5 pairs, but the sample output is 4.

Wait, perhaps one of these doesn't satisfy the original condition.

Looking back:

(1,1):1+1=2, b*gcd(1,1)=1*1=1, 2 is a multiple of 1. Valid.

(2,1):2+1=3, b*gcd(2,1)=1*1=1, 3 is a multiple of 1. Valid.

(2,2):2+2=4, b*gcd(2,2)=2*2=4, 4 is a multiple of 4. Valid.

(3,1):3+1=4, b*gcd(3,1)=1*1=1, 4 is a multiple of 1. Valid.

(3,3):3+3=6, b*gcd(3,3)=3*3=9, 6 is not a multiple of 9. Invalid.

Ah! So, (3,3) is invalid.

Wait, but according to my earlier reasoning, b divides a, which is 3 divides 3, so a=3 is a multiple of b=3.

But in this case, a + b = 6, and b * gcd(a,b) = 3 * 3 = 9, and 6 is not a multiple of 9.

So, this pair doesn't satisfy the original condition.

Therefore, my earlier assumption that b divides a is necessary but not sufficient.

Wait, in this case, b divides a, but a + b is not necessarily a multiple of b * gcd(a,b).

Wait, but in the earlier steps, I thought that b = gcd(a,b), which implies b divides a.

But in this pair (3,3), b=3 and gcd(a,b)=3, so b = gcd(a,b), but a + b =6 is not a multiple of b * gcd(a,b)=9.

Wait, that seems contradictory to my earlier conclusion.

Wait, perhaps there's a mistake in concluding that b = gcd(a,b).

Let me revisit that.

I had:

b * g | a + b, where g = gcd(a,b).

And since g divides both a and b, a = g * a', b = g * b', with gcd(a', b')=1.

Substituting:

b * g | a + b ⇒ (g * b') * g | (g * a' + g * b') ⇒ g^2 * b' | g(a' + b') ⇒ g * b' | a' + b'

Now, since a' and b' are coprime, and b' divides a' + b', then b' divides a'.

But a' and b' are coprime, so b' must be 1.

Therefore, b' = 1.

Thus, b = g * 1 = g, so b = g.

Therefore, b = gcd(a,b).

But in the pair (3,3), b=3 and gcd(a,b)=3, which satisfies b = gcd(a,b), but a + b =6 is not a multiple of b * g =9.

Wait, but according to the condition, b * g = b * b = b^2, and a + b =2b.

So, 2b must be a multiple of b^2 ⇒ b^2 | 2b ⇒ b | 2.

So, in the pair (3,3), 3 does not divide 2, hence it's invalid.

Wait, so even though b = gcd(a,b), if b does not divide 2, it's invalid.

Wait, perhaps I need to consider that a + b =2b, and b * g =b^2.

So, b^2 divides 2b ⇒ b divides 2.

Hence, for b >2, it's invalid.

Wait, but in the pair (2,2): b=2, a=2, a+b=4, b*g=4, 4 divides 4, which is valid.

For b=1: b*g=1, a+b=2, 1 divides 2, valid.

For b=3: b*g=9, a+b=6, 9 does not divide 6, invalid.

So, in addition to b dividing a, we need b dividing a + b.

But a is a multiple of b, so a = k*b, then a + b = (k+1)*b.

So, b divides a + b ⇒ b divides (k+1)*b ⇒ b divides k*b + b ⇒ b divides b(k+1), which is always true.

Wait, that seems always true.

But in the earlier example, for b=3, a=3, a + b=6, and b*g=9, which is 9 does not divide 6.

Wait, so perhaps there's another condition.

Wait, perhaps I need to consider that b * g divides a + b, where g = gcd(a,b)=b.

So, b * b | a + b ⇒ b^2 | a + b.

Given that a = k * b, then a + b = k*b + b = b(k +1).

So, b^2 | b(k +1) ⇒ b | (k +1).

Therefore, b divides (k +1).

So, in the pair (2,2): b=2, k=1 (since a=2, b=2, k=1), so b=2 divides k+1=2, which is true.

In the pair (3,3): b=3, k=1, b=3 divides k+1=2, which is false.

Hence, for b > k +1, it's invalid.

Therefore, the condition is that b divides a and b divides (a + b), which simplifies to b divides (k +1).

Given that a = k*b, and b divides (k +1).

So, for each b, k can be such that k +1 is a multiple of b.

So, k = m*b -1, for some integer m.

Wait, perhaps I need to think differently.

Given that b divides (k +1), and k is a positive integer such that a = k*b ≤ n.

So, k ≤ n / b.

And k +1 is a multiple of b.

So, k +1 ≡ 0 mod b ⇒ k ≡ -1 mod b.

So, k = t*b -1, for some integer t ≥1.

And k ≥1, since a = k*b ≥1.

So, t*b -1 ≥1 ⇒ t*b ≥2 ⇒ t ≥ ceil(2/b).

But b is at least 1, so t ≥1.

Therefore, for each b, the possible k are of the form t*b -1, where t is an integer ≥1, and k ≤ n / b.

So, a = (t*b -1)*b = t*b^2 - b.

And since a ≤n, t*b^2 - b ≤n ⇒ t ≤ (n +b)/b^2.

So, for each b, the number of valid t is floor((n +b)/b^2).

Therefore, the total number of valid pairs is the sum over b from 1 to m of floor((n +b)/b^2).

Wait, but in the sample input where n=3 and m=5, sum floor((3 +b)/b^2) for b=1 to 5:

b=1: (3+1)/1 =4/1=4

b=2: (3+2)/4=5/4=1

b=3: (3+3)/9=6/9=0

b=4: (3+4)/16=7/16=0

b=5: (3+5)/25=8/25=0

Total:4+1+0+0+0=5, but the sample output is 4.

Hmm, discrepancy again.

Wait, perhaps I need to adjust the formula.

Wait, in the pair (3,3), which should be invalid, but according to floor((3+3)/9)=0, which is counted as 0.

Wait, but in the sum, it's floor((3+1)/1)=4, which includes t=1,2,3,4.

For t=1: a=1*1^2 -1=0, which is invalid since a ≥1.

So, perhaps t starts from 1, but a must be ≥1.

So, for b=1, t*b^2 - b = t*1 -1 = t -1.

For t=1: a=0, invalid.

For t=2: a=1, valid.

For t=3: a=2, valid.

For t=4: a=3, valid.

So, only t=2,3,4 are valid for b=1.

Hence, floor((n+b)/b^2) -1, since t starts from 2 when b=1.

Wait, but for b=1, floor((n+b)/b^2)=floor((3+1)/1)=4, but t starts from t=1, but t=1 gives a=0, which is invalid.

So, for b=1, the valid t are from t=1 to floor((n+b)/b^2), but t=1 is invalid.

Hence, for b=1, the number of valid t is floor((n+b)/b^2) -1.

For b ≥2, t starts from t=1.

Wait, but in the earlier example, for b=1, floor((3+1)/1)=4, but t=1 gives a=0, which is invalid, so only t=2,3,4 are valid, which is 3 pairs.

For b=2: floor((3+2)/4)=1, t=1: a=2*4 -2=6, which is greater than n=3, so invalid.

Wait, hold on.

Wait, perhaps my formula is incorrect.

Wait, I need to double-check the formula for a.

Given a = t*b^2 - b.

For b=2, t=1: a=4 -2=2, which is ≤3, valid.

t=2: a=8 -2=6, which is >3, invalid.

So, only t=1 is valid for b=2.

Similarly, for b=1, t=1: a=1-1=0, invalid.

t=2: a=1-1=0, wait, no.

Wait, a = t*b^2 - b.

For b=1, t=1: a=1*1 -1=0, invalid.

t=2: a=2*1 -1=1, valid.

t=3: a=3*1 -1=2, valid.

t=4: a=4*1 -1=3, valid.

So, for b=1, 3 valid pairs.

For b=2, 1 valid pair.

For b=3, floor((3+3)/9)=0, no pairs.

For b=4, floor((3+4)/16)=0.

For b=5, floor((3+5)/25)=0.

Total: 3 +1 +0 +0 +0 =4, which matches the sample.

So, the correct formula is sum over b from 1 to m of floor((n +b)/b^2) minus 1 for b=1 if n >=1.

Wait, but in the sample, n=3, m=5, and the sum is floor((3+1)/1)=4, but t=1 gives a=0, which is invalid, so subtract 1.

Similarly, for b=2, floor((3+2)/4)=1, t=1 gives a=2, valid.

For b>=3, floor((3+b)/b^2)=0.

So, total is (4-1) +1 +0 +0 +0 =4, which matches.

Hence, for b=1, need to adjust the count by subtracting 1 if n >=1.

Similarly, for other b, no adjustment needed.

Wait, but in general, for b=1, t starts from t=1, but a=t*1 -1=t-1, which is >=1 only if t >=2.

Hence, for b=1, the number of valid t is floor((n +1)/1) -1 = n.

But in the sample, n=3, so floor((3+1)/1)=4, subtract 1 for t=1, giving 3 valid pairs for b=1.

Wait, but n=3, floor((3+1)/1)=4, subtract 1, gives 3, which matches.

For b=2, floor((3+2)/4)=1, no need to subtract, as t=1 gives a=2, which is valid.

For b=3, floor((3+3)/9)=0, nothing to subtract.

So, perhaps the general formula is sum over b from 1 to m of floor((n +b)/b^2), but for b=1, subtract 1 if n >=1.

Wait, but in the sample, it's floor((n +b)/b^2), and for b=1, subtract 1.

So, perhaps it's sum over b from 1 to m of floor((n +b)/b^2) - [b ==1 and n >=1].

Wait, but in the sample, n=3, m=5, sum is floor((3+1)/1)=4, floor((3+2)/4)=1, floor((3+3)/9)=0, etc., total 4+1+0+0+0=5, then subtract 1 for b=1, giving 4, which matches.

Similarly, for n=2, m=3:

b=1: floor((2+1)/1)=3, subtract 1 ⇒ 2

b=2: floor((2+2)/4)=1 ⇒1

b=3: floor((2+3)/9)=0 ⇒0

Total:2+1+0=3, which matches the sample.

For n=1, m=1:

b=1: floor((1+1)/1)=2, subtract 1 ⇒1

Total:1, which matches.

So, the formula seems correct.

Hence, the total number of valid pairs is sum over b from 1 to m of floor((n +b)/b^2) minus 1 if b=1 and n >=1.

Now, I need to implement this efficiently, considering the constraints.

Constraints:

- t ≤10^4

- 1 ≤n,m ≤2*10^6

- Sum of n and m over all test cases does not exceed 2*10^6.

So, per test case, n and m can be up to 2*10^6, but the total sum over all test cases is limited to 2*10^6.

Hence, the time complexity should be O(t * something), where something is efficient.

Given that t can be up to 10^4, and something is up to 2*10^6 total over all test cases, I need an efficient solution.

Let me think about how to compute sum over b from 1 to m of floor((n +b)/b^2).

Let me denote k = b^2.

Then, floor((n +b)/k) = floor((n +b)/b^2).

But I'm not sure if that helps.

Alternatively, let's consider that for each b, floor((n +b)/b^2) can be computed directly.

But iterating over b from 1 to m for each test case would be too slow for t=10^4 and m=2*10^6.

Hence, I need a way to compute this sum efficiently.

Let me see if I can find some patterns or find a way to group terms.

Let me consider the expression floor((n +b)/b^2).

Let me denote it as floor(n/b^2 + 1/b).

Since b is positive integer, 1/b is less than or equal to 1.

Hence, floor(n/b^2 + 1/b) = floor(n/b^2) + 1 if 1/b >= {n/b^2}, where {x} is the fractional part of x.

But this seems complicated.

Alternatively, let's consider that for b >=1, b^2 >= b, so (n +b)/b^2 = n/b^2 + 1/b.

Now, n/b^2 decreases as b increases, and 1/b also decreases.

I need to find a way to group b's where floor(n/b^2 + 1/b) is constant.

But this seems tricky.

Alternatively, perhaps I can iterate over b in a smarter way, similar to how we optimize the calculation of sum of floor(n/i) over i.

In number theory, sum of floor(n/i) for i from 1 to m can be computed efficiently using number theory techniques or by iterating up to sqrt(n) and handling blocks.

But in this case, it's floor((n +b)/b^2), which is not exactly floor(n/i).

Let me see if I can transform it.

Let me set k = b^2.

Then, floor((n +b)/k) = floor((n +b)/b^2).

But k = b^2, so b = sqrt(k).

But b is integer, so k is perfect squares.

Wait, perhaps I can iterate over b such that b^2 <= n +b, which is always true for b <= sqrt(n +b), but this seems circular.

Alternatively, I can iterate b up to floor(sqrt(n +m)), since b^2 <= n +b.

Wait, b^2 <= n +b ⇒ b^2 - b -n <=0.

Solving quadratic inequality: b = [1 +- sqrt(1 +4n)] / 2.

So, b <= [1 + sqrt(1 +4n)] / 2.

Hence, the maximum b for which b^2 <=n +b is floor([1 + sqrt(1 +4n)] / 2).

Let me denote this as b_max.

So, for b from 1 to min(m, b_max), I can compute floor((n +b)/b^2).

Beyond b_max, b^2 > n +b, so floor((n +b)/b^2)=0.

Hence, I only need to iterate b from 1 to min(m, b_max).

Now, b_max is approximately sqrt(n), since sqrt(1 +4n)/2 ≈ sqrt(n).

Hence, b_max is up to O(sqrt(n)).

Given that n can be up to 2*10^6, b_max is up to around 1414.

Hence, for each test case, I can iterate b from 1 to min(m, b_max), compute floor((n +b)/b^2), and sum them up, subtracting 1 if b=1 and n >=1.

This should be efficient enough, since b_max is up to around 1414, and t is up to 10^4.

Total time complexity would be O(t * b_max), which is around 10^4 * 1414 = 1.4*10^7 operations, which should be acceptable.

Now, let's confirm this with the sample input.

Sample input:

6

1 1

2 3

3 5

10 8

100 1233

1000000 1145141

Compute for each:

1. n=1, m=1:

b_max = floor((1 + sqrt(1 +4*1))/2) = floor((1 + sqrt(5))/2) ≈ floor(1.618) =1

So, b from 1 to 1:

floor((1+1)/1)=2, subtract 1 (since b=1 and n=1 >=1), so 1.

Total:1.

2. n=2, m=3:

b_max = floor((1 + sqrt(1 +8))/2) = floor((1 +3)/2)=2

So, b from 1 to 2:

b=1: floor((2+1)/1)=3, subtract 1 ⇒2

b=2: floor((2+2)/4)=1 ⇒1

Total:2+1=3.

3. n=3, m=5:

b_max = floor((1 + sqrt(1 +12))/2) = floor((1 + sqrt(13))/2) ≈ floor(2.302)=2

So, b from 1 to 2:

b=1: floor((3+1)/1)=4, subtract 1 ⇒3

b=2: floor((3+2)/4)=1 ⇒1

Total:3+1=4.

4. n=10, m=8:

b_max = floor((1 + sqrt(1 +40))/2) = floor((1 + sqrt(41))/2) ≈ floor(3.702)/2=1

Wait, sqrt(41) ≈6.403, so 1 +6.403=7.403, floor(7.403/2)=3.

So, b from 1 to 3 (since m=8, but b_max=3):

b=1: floor((10+1)/1)=11, subtract 1 ⇒10

b=2: floor((10+2)/4)=3 ⇒3

b=3: floor((10+3)/9)=1 ⇒1

Total:10+3+1=14.

5. n=100, m=1233:

b_max = floor((1 + sqrt(1 +400))/2) = floor((1 +21)/2)=11

So, b from 1 to 11 (since m=1233, but b_max=11):

Compute floor((100 +b)/b^2) for b=1 to11, subtract 1 for b=1.

Let's compute:

b=1: floor(101/1)=101, subtract 1 ⇒100

b=2: floor(102/4)=25 ⇒25

b=3: floor(103/9)=11 ⇒11

b=4: floor(104/16)=6 ⇒6

b=5: floor(105/25)=4 ⇒4

b=6: floor(106/36)=2 ⇒2

b=7: floor(107/49)=2 ⇒2

b=8: floor(108/64)=1 ⇒1

b=9: floor(109/81)=1 ⇒1

b=10: floor(110/100)=1 ⇒1

b=11: floor(111/121)=0 ⇒0

Total:100+25+11+6+4+2+2+1+1+1+0=153.

6. n=1000000, m=1145141:

b_max = floor((1 + sqrt(1 +4*1000000))/2) = floor((1 + sqrt(4000001))/2) ≈ floor((1 +2000)/2)=1000.5 ⇒1000

So, b from1 to1000 (since m=1145141, but b_max=1000):

Compute floor((1000000 +b)/b^2) for b=1 to1000, subtract 1 for b=1.

This would be time-consuming to compute manually, but the code should handle it efficiently.

Hence, this approach seems correct.

Now, let's look at the given program and see if it implements this logic.

Looking at the code:

There are multiple functions defined, but the main function is func_16(), which calls func_15() for each test case.

func_15():

(n, m) = func_7()

i =1

ans =0

while i *i <=n +i:

ans += (n +i) // (i *i)

i +=1

return ans -1

Wait, this seems similar to what I derived.

It iterates i from1 up to floor(sqrt(n +i)), which is similar to b_max.

In each iteration, it adds floor((n +i)/i^2) to ans.

Finally, it returns ans -1.

Comparing to my earlier logic, for b from1 to b_max, sum floor((n +b)/b^2), and subtract1 if b=1 and n >=1.

Wait, but in this code, it's subtracting1 unconditionally.

But in my earlier analysis, I conditionally subtract1 only if b=1 and n >=1.

Wait, but in the sample input where n=1, m=1, it subtracts1, giving the correct answer of1.

In n=2, m=3, it subtracts1, giving3, which is correct.

In n=3, m=5, it subtracts1, giving4, which is correct.

Wait, but for n=10, m=8, sum is floor((10+1)/1)=11, floor((10+2)/4)=3, floor((10+3)/9)=1, total11+3+1=15, then subtract1 to get14, which matches the sample.

For n=100, m=1233, sum is101+25+11+6+4+2+2+1+1+1+0=154, then subtract1 to get153, which matches.

For n=1000000, m=1145141, sum floor((1000000 +i)/i^2) for i=1 to1000, then subtract1.

Seems consistent.

Hence, the program is correct.

Therefore, Correctness: **True**