Let's break down the problem step by step:

1. **Initial State**:
   - `t` is an integer such that \(1 \leq t \leq 10^4\).
   - `ap` is an input integer greater than 1.
   - `k` is 1.
   - `x` is defined as `x - bxsfory * 15 + y * 4`.
   - `y` is an input integer from the second input split.
   - `bxsfory` is the ceiling value of `y / 2`.
   - `bxsfory1` is 0 if `x - bxsfory * 15 + y * 4 <= 0` else the ceiling value of `(x - bxsfory * 15 + y * 4) / 15`.

2. **Calculating `bxsfory`**:
   - `bxsfory` is the ceiling value of `y / 2`. This means if `y` is even, `bxsfory = y / 2`, and if `y` is odd, `bxsfory = (y + 1) / 2`.

3. **Calculating `x`**:
   - `x = x - bxsfory * 15 + y * 4`. Since `x` is initially undefined, let's assume it is some integer value `x0` for now.

4. **Calculating `bxsfory1`**:
   - `bxsfory1` is determined by the condition `x - bxsfory * 15 + y * 4 <= 0`.
     - If `x - bxsfory * 15 + y * 4 <= 0`, then `bxsfory1 = 0`.
     - Otherwise, `bxsfory1 = ceil((x - bxsfory * 15 + y * 4) / 15)`.

5. **Final Expression to Print**:
   - We need to print `bxsfory1 + bxsfory`.

Given the complexity and the lack of specific values for `x0` and `y`, let's consider a general case where `y` is an arbitrary integer and `x0` is also an arbitrary integer.

### Step-by-Step Calculation:

1. **Calculate `bxsfory`**:
   - Suppose `y = 6` (an example value). Then `bxsfory = ceil(6 / 2) = 3`.

2. **Calculate `x`**:
   - Suppose `x0 = 100` (an example value). Then `x = 100 - 3 * 15 + 6 * 4 = 100 - 45 + 24 = 79`.

3. **Calculate `bxsfory1`**:
   - Check the condition: `79 - 3 * 15 + 6 * 4 = 79 - 45 + 24 = 58 > 0`. Therefore, `bxsfory1 = ceil(58 / 15) = 4`.

4. **Final Value to Print**:
   - `bxsfory1 + bxsfory = 4 + 3 = 7`.

Thus, the output will be the sum of `bxsfory1` and `bxsfory`.

Output: **7**