Let's break down the given code and initial state to determine what will be printed.

### Initial State:
- `s` is a string of the first `k` letters of the alphabet.
- `k` is not equal to 1.
- The variable `n` is not mentioned in the initial state, so we need to assume it is defined elsewhere in the code. However, since it's not provided, we can infer its role from the expression.

### Code:
```python
print((2 - (n == 1)) * s)
```

### Analysis:
1. **Expression Breakdown**:
   - `(n == 1)` evaluates to `True` if `n` is 1, and `False` otherwise.
   - In Python, `True` is equivalent to `1` and `False` is equivalent to `0`.
   - Therefore, `(2 - (n == 1))` will be:
     - `2 - 1 = 1` if `n == 1`
     - `2 - 0 = 2` if `n != 1`
   
2. **String Multiplication**:
   - The expression `(2 - (n == 1)) * s` multiplies the string `s` by the result of the expression.
   - If `n == 1`, the result is `1 * s`, which is just `s`.
   - If `n != 1`, the result is `2 * s`, which is `s` concatenated with itself.

### Given Information:
- `k` is not equal to 1, but this does not directly affect the expression involving `n`.

### Final Output:
- If `n == 1`, the output will be the string `s`.
- If `n != 1`, the output will be the string `s` concatenated with itself.

Since the value of `n` is not provided, we cannot determine the exact output. However, we can describe the output based on the possible values of `n`.

### Conclusion:
Output: **(s if n == 1 else s + s) (where s is a string of the first k letters of the alphabet and k is not equal to 1)**