Let's break down the problem step by step:

1. **Identify the loop condition**: The loop condition is `k >= reachable_count - 1 and k > 0`.

2. **Determine the current values**:
   - `k` is `n - reachable_count`.
   - `reachable_count` is `n - 2`.

3. **Substitute the current values into the loop condition**:
   - First, express `k` in terms of `n`:
     \[
     k = n - (n - 2) = 2
     \]
   - Now, substitute `k = 2` and `reachable_count = n - 2` into the loop condition:
     \[
     2 \geq (n - 2) - 1 \quad \text{and} \quad 2 > 0
     \]
   - Simplify the inequality:
     \[
     2 \geq n - 3 \quad \text{and} \quad 2 > 0
     \]
   - Since `2 > 0` is always true, we only need to focus on:
     \[
     2 \geq n - 3
     \]
   - Rearrange the inequality:
     \[
     n \leq 5
     \]

4. **Adjust the states for the loop to execute one more time**:
   - For the loop to execute one more time, `k` must satisfy the condition `k >= reachable_count - 1 and k > 0`.
   - Given `k = 2`, we need to ensure that the condition holds for the next iteration.
   - The condition `k >= reachable_count - 1` simplifies to `2 >= (n - 2) - 1`, which means `n <= 5`.
   - The condition `k > 0` is already satisfied since `k = 2`.

5. **Conclusion**:
   - To ensure the loop executes one more time, `n` must be such that `k` remains valid for the next iteration.
   - Therefore, `n` must be less than or equal to 5.

So, the final state to be adjusted is:
State: **`k` is `n - reachable_count`, `reachable_count` is `n - 2`, and `n` must be less than or equal to 5**.