
Given a Python loop, an initial execution state, and the output states after the first 3 iterations of the loop, determine the output state after all the executions of the loop have finished. 

You must adhere to the text format: Output State: **output state.**

Initial State: `T` is an integer read from standard input and stripped of any trailing whitespace, and it is between 1 and 10^4 inclusive; `MOD` remains 1000000007.
Code of the loop:
for _ in range(T):
    n, k = map(int, sys.stdin.readline().strip().split())
    a = list(map(int, sys.stdin.readline().strip().split()))
    s = sum(a)
    t, tmp = 0, 0
    for x in a:
        tmp += x
        if tmp < 0:
            tmp = 0
        t = max(tmp, t)
    ans = ((s + t) % MOD + MOD) % MOD
    for i in range(k - 1):
        t *= 2
        t %= MOD
        ans += t
        ans %= MOD
    print(ans)


The output state after the loop executes the first 3 of times includes what needed to be true for the loop to execute at least that number of times:

Output State after the loop executes 1 time: Output State: After all iterations of the loop, `ans` will be the sum of `t` (which starts at 0 and doubles each iteration until it reaches \(2^{k-1} - 1\)) modulo `MOD`, and `t` will be `2^{k-1} - 1` modulo `MOD`. The variable `i` will be equal to `k-1`, and `k` will remain the same as its initial value. All other variables (`t`, `tmp`, `T`, `n`, `a`, `s`) will retain their values from the final iteration of the loop.

To break it down further:
- `t` will be \(2^{k-1} - 1\) because it doubles each time until just before it would exceed the limit, then stops.
- `ans` will be the cumulative sum of all these values of `t` taken modulo `MOD`.
- `i` will be `k-1` because the loop runs `k-1` times.
- `k` remains unchanged.
- `tmp` is not used in the loop and thus remains 0.
- `T`, `n`, `a`, and `s` are not affected by the loop and retain their initial or final values from the last iteration.

**Output State after the loop executes 2 times**: Output State: `i` is `k-1`, `k` must be greater than `k-1`, `t` is \(2^{k-1} \mod \text{MOD}\), `ans` is the cumulative sum of terms \(t\) from \(2^0 \mod \text{MOD}\) to \(2^{k-1} \mod \text{MOD}\) modulo `MOD`.

In simpler terms, after the loop has executed all its iterations, `i` will be `k-1`, `k` must be greater than `k-1` (which is always true since `k` does not change within the loop), `t` will be \(2^{k-1} \mod \text{MOD}\) because it doubles in each iteration starting from 2, and `ans` will be the sum of all `t` values from the start of the loop up to the final value of `t`, all taken modulo `MOD`.

**Output State after the loop executes 3 times**: Output State: `i` is 3, `t` is 8 % MOD, `ans` is 12 % MOD.

To understand this output state, let's break down the loop execution:

- Initially, `i` is 0, `t` is 2 % MOD (which is 2), and `ans` is 2 % MOD (which is 2).
- After the first iteration (`i` becomes 1):
  - `t` is updated to `2 * 2` % MOD = 4 % MOD = 4.
  - `ans` is updated to `2 + 4` % MOD = 6 % MOD = 6.
- After the second iteration (`i` becomes 2):
  - `t` is updated to `4 * 2` % MOD = 8 % MOD = 0.
  - `ans` is updated to `6 + 0` % MOD = 6 % MOD = 6.
- After the third iteration (`i` becomes 3):
  - `t` is updated to `0 * 2` % MOD = 0 % MOD = 0.
  - `ans` is updated to `6 + 0` % MOD = 6 % MOD = 6.

Since the loop condition `i < k - 1` will no longer be satisfied when `i` reaches 3 (assuming `k` is 4 or more), the loop terminates. Therefore, after all iterations, `i` is 3, `t` is 0, and `ans` is 6. However, based on the provided output states, it seems `t` should be 8 % MOD after 3 iterations, which implies `k` might be 5. Let's re-evaluate with `k` as 5:

- After the third iteration (`i` becomes 2):
  - `t` is updated to `0 * 2` % MOD = 0 % MOD = 0.
  - `ans` is updated to `6 + 0` % MOD = 6 % MOD = 6.
- After the fourth iteration (`i` becomes 3):
  - `t` is updated to `0 * 2` % MOD = 0 % MOD = 0.
  - `ans` is updated to `6 + 0` % MOD = 6 % MOD = 6.
- After the fifth iteration (`i` becomes 4):
  - `t` is updated to `0 * 2` % MOD = 0 % MOD = 0.
  - `ans` is updated to `6 + 0` % MOD = 6 % MOD = 6.

But since the problem specifies the output state after 3 iterations, we can infer that `k` is 4, and the final state after all iterations would be:

- `i` is 3.
- `t` is 0 * 2 % MOD = 0 % MOD = 0.
- `ans` is 6 + 0 % MOD = 6 % MOD = 6.

However, given the pattern and the provided output states, it seems there might be a slight misalignment. Assuming the pattern continues correctly, the correct state after 4 iterations (if `k` were 5) would be:

- `i` is 4.
- `t` is 0 * 2 % MOD = 0 % MOD = 0.
- `ans` is 6 + 0 % MOD = 6 % MOD = 6.

But following the exact provided states, the correct interpretation for 3 iterations with `k` being 4 is:

- `i` is 3.
- `t` is 0.
- `ans` is 6.

Given the provided states, the most accurate answer considering the pattern is:

Output State: `i` is 3, `t` is 8 % MOD, `ans` is 12 % MOD.




What is the ouput state after the loop executes all the iterations? Change the values of only the variables in the loop head and body.The state of the other variables in the precondition that are not affected by the loop head and body must remain unchanged.
In your response strictly use the format: Output State: **the output state you calculate.**, and describe this output state in Natural language easily understandable by humans.

