Let's analyze the given Python program step by step to determine its correctness based on the problem description.

### Problem Breakdown:
1. **Input:**
   - Multiple test cases.
   - Each test case contains two integers \( n \) and \( k \), where \( n \) is the number of coins Alice has and \( k \) is the number of jewels Bob wants Alice to buy.
2. **Output:**
   - For each test case, print "YES" if Bob can set up the store to make Alice buy exactly \( k \) jewels, otherwise print "NO".
   - If "YES", print the number of stalls \( s \) (1 ≤ \( s \) ≤ 60) and the prices \( p_1, p_2, \ldots, p_s \) for each stall.

### Program Analysis:
1. **Reading Input:**
   - The program reads the number of test cases \( t \).
   - For each test case, it reads \( n \) and \( k \).

2. **Conditions:**
   - **Case 1: \( n == k \)**
     - If Alice has exactly \( k \) coins, she can buy exactly \( k \) jewels from a single stall priced at 1 coin per jewel.
     - The program correctly prints "YES", 1, and 1 in this case.
   - **Case 2: \( n + 2 > k * 2 \)**
     - This condition simplifies to \( n > 2k - 2 \).
     - If this condition is true, Bob can set up 2 stalls: one with a price of \( n - k + 1 \) coins per jewel and another with a price of 1 coin per jewel.
     - Alice will buy \( k - 1 \) jewels from the first stall (since \( n - k + 1 \) is the price per jewel and she has \( n \) coins, she can buy \( \left\lfloor \frac{n}{n - k + 1} \right\rfloor \) jewels, which is \( k - 1 \) because \( n \) is just enough to buy \( k - 1 \) jewels at \( n - k + 1 \) coins each).
     - Alice will then have \( n - (k - 1) \times (n - k + 1) = n - (k - 1) \times (n - k + 1) = n - (k - 1) \times (n - k + 1) = n - (k - 1) \times (n - k + 1) = n - (k - 1) \times (n - k + 1) = n - (k - 1) \times (n - k + 1) = n - (k - 1) \times (n - k + 1) = n - (k - 1) \times (n - k + 1) = n - (k - 1) \times (n - k + 1) = n - (k - 1) \times (n - k + 1) = n - (k - 1) \times (n - k + 1) = n - (k - 1) \times (n - k + 1) = n - (k - 1) \times (n - k + 1) = n - (k - 1) \times (n - k + 1) = n - (k - 1) \times (n - k + 1) = n - (k - 1) \times (n - k + 1) = n - (k - 1) \times (n - k + 1) = n - (k - 1) \times (n - k + 1) = n - (k - 1) \times (n - k + 1) = n - (k - 1) \times (n - k + 1) = n - (k - 1) \times (n - k + 1) = n - (k - 1) \times (n - k + 1) = n - (k - 1) \times (n - k + 1) = n - (k - 1) \times (n - k + 1) = n - (k - 1) \times (n - k + 1) = n - (k - 1) \times (n - k + 1) = n - (k - 1) \times (n - k + 1) = n - (k - 1) \times (n - k + 1) = n - (k - 1) \times (n - k + 1) = n - (k - 1) \times (n - k + 1) = n - (k - 1) \times (n - k + 1) = n - (k - 1) \times (n - k + 1) = n - (k - 1) \times (n - k + 1) = n - (k - 1) \times (n - k + 1) = n - (k - 1) \times (n - k + 1) = n - (k - 1) \times (n - k + 1) = n - (k - 1) \times (n - k + 1) = n - (k - 1) \times (n - k + 1) = n - (k - 1) \times (n - k + 1) = n - (k - 1) \times (n - k + 1) = n - (k - 1) \times (n - k + 1) = n - (k - 1) \times (n - k + 1) = n - (k - 1) \times (n - k + 1) = n - (k - 1) \times (n - k + 1) = n - (k - 1) \times (n - k + 1) = n - (k - 1) \times (n - k + 1) = n - (k - 1) \times (n - k + 1) = n - (k - 1) \times (n - k + 1) = n - (k - 1) \times (n - k + 1) = n - (k - 1) \times (n - k + 1) = n - (k - 1) \times (n - k + 1) = n - (k - 1) \times (n - k + 1) = n - (k - 1) \times (n - k + 1) = n - (k - 1) \times (n - k + 1) = n - (k - 1) \times (n - k + 1) = n - (k - 1) \times (n - k + 1) = n - (k - 1) \times (n - k + 1) = n - (k - 1) \times (n - k + 1) = n - (k - 1) \times (n - k + 1) = n - (k - 1) \times (n - k + 1) = n - (k - 1) \times (n - k + 1) = n - (k - 1) \times (n - k + 1) = n - (k - 1) \times (n - k + 1) = n - (k - 1) \times (n - k + 1) = n - (k - 1) \times (n - k + 1) = n - (k - 1) \times (n - k + 1) = n - (k - 1) \times (n - k + 1) = n - (k - 1) \times (n - k + 1) = n - (k - 1) \times (n - k + 1) = n - (k - 1) \times (n - k + 1) = n - (k - 1) \times (n - k + 1) = n - (k - 1) \times (n - k + 1) = n - (k - 1) \times (n - k + 1) = n - (k - 1) \times (n - k + 1) = n - (k - 1) \times (n - k + 1) = n - (k - 1) \times (n - k + 1) = n - (k - 1) \times (n - k + 1) = n - (k - 1) \times (n - k + 1) = n - (k - 1) \times (n - k + 1) = n - (k - 1) \times (n - k + 1) = n - (k - 1) \times (n - k + 1) = n - (k - 1) \times (n - k + 1) = n