Alright, I have this problem to solve. Let's understand what's being asked here. So, Polycarp has a string `s` consisting of lowercase Latin letters. He encodes this string using a specific algorithm, and my task is to write a program that decodes it back to the original string `s`.

First, I need to understand the encoding algorithm clearly. It has two main steps:

1. **Constructing the auxiliary string `r`**:
   - `r` consists of all distinct letters from `s`, sorted in alphabetical order.
   
2. **Encoding the string `s`**:
   - Each character in `s` is replaced by its symmetric character from `r`. That means the first character of `r` is replaced by the last character of `r`, the second by the second last, and so on.

For example, given `s = "codeforces"`, the auxiliary string `r` is "cdefors". Now, encoding replaces each character in `s` with its symmetric character from `r`:

- 'c' (first in `r`) is replaced by 's' (last in `r`)

- 'o' (second in `r`) is replaced by 'e' (second last in `r`)

- 'd' (third in `r`) is replaced by 'r' (third last in `r`)

- and so on.

The encoded string is "serofedsoc".

Now, my task is to decode the encoded string back to the original string `s`. So, given the encoded string, I need to find out what the original string was.

Looking at the encoding process, it seems that there's a one-to-one mapping between characters in `r` and their replacements. Since `r` consists of unique sorted characters from `s`, and the mapping is symmetric, I need to reverse this mapping to decode the string.

But there's a catch: I don't know what `r` was, because `r` is derived from the original string `s`, which is what I'm trying to find. So, I need to figure out `r` from the encoded string.

Looking at the example:

Encoded string: "serofedsoc"

Original string: "codeforces"

Auxiliary string `r`: "cdefors"

From the encoded string, I can see that each character in the encoded string corresponds to a character in the original string based on the mapping defined by `r`.

To decode, I need to map each character in the encoded string back to its original character using the same symmetric mapping.

But since I don't know `r`, I need to deduce `r` from the encoded string and the properties of the encoding algorithm.

Wait, in the problem statement, it says: "Write a program that performs decoding â€” that is, restores the original string `s` from the encoding result."

Given that, I need to write a function that, given the encoded string, outputs the original string `s`.

Looking at the provided program, there's a function `func_1` that seems to attempt this decoding.

Let's look at the code:

```python
def func_1(encoded: str) -> str:
    mapping = {}
    decoded = []
    for char in encoded:
        if char in mapping:
            decoded.append(mapping[char])
        else:
            for c in range(ord('a'), ord('z') + 1):
                if chr(c) not in mapping.values():
                    mapping[chr(c)] = char
                    break
            decoded.append(chr(c))
    return ''.join(decoded)
```

This function creates a mapping dictionary and iterates through each character in the encoded string. If the character is already in the mapping, it appends the corresponding decoded character to the list. If not, it finds the first available lowercase letter that hasn't been used in the mapping yet and maps it to the current encoded character.

Wait, this doesn't seem right. This approach seems to be creating a mapping from decoded characters to encoded characters, but it's not considering the symmetric property based on the auxiliary string `r`.

I think this is incorrect because it doesn't take into account the symmetric replacement based on `r`. It's just creating a new mapping without considering the sorted unique characters and their symmetric positions.

Let me think about how to correctly decode the string.

First, I need to determine what the auxiliary string `r` was, based on the encoded string.

Given that `r` is the sorted unique characters from the original string `s`, and the encoding replaces each character in `s` with its symmetric counterpart in `r`, I need to reverse this process.

One way to approach this is:

1. Identify the unique characters in the encoded string, since they correspond to the unique characters in `r`, but in symmetric positions.

2. Determine the mapping from encoded characters back to the original characters based on the symmetric positions in `r`.

Wait, that seems confusing. Let's think differently.

Suppose I can find out what `r` was. Since `r` is the sorted unique characters from `s`, and the encoding replaces each character in `s` with its symmetric counterpart in `r`, then to decode, I need to map each character in the encoded string back to its original character in `s` based on the symmetric positions in `r`.

But the problem is that `r` is derived from `s`, which is unknown. However, the encoded string is derived from `s` using `r`, so there must be a way to reverse the process.

Let's consider that `r` is a sorted list of unique characters from `s`, and the encoding maps each character in `s` to its symmetric counterpart in `r`.

So, if I can find out `r`, then I can create a mapping from encoded characters back to the original characters.

But how do I find `r` from the encoded string?

Wait, here's an idea:

- Since `r` is the sorted unique characters from `s`, and each character in `s` is replaced by its symmetric counterpart in `r`, then in the encoded string, the unique characters correspond to the unique characters in `r`, but in reverse order.

Wait, no. Not necessarily in reverse order, but in symmetric positions.

Let me think with an example.

Given `s = "codeforces"`, `r = "cdefors"`, encoded string is "serofedsoc".

Unique characters in encoded string: 's', 'e', 'r', 'o', 'f', 'd', 'c'

Sorted unique characters in encoded string: 'c', 'd', 'e', 'f', 'o', 'r', 's'

Comparing this to `r = "cdefors"`, which is sorted unique characters from `s`.

Wait, in this case, the sorted unique characters in encoded string match `r`, but the mapping is symmetric.

Wait, no. In `r = "cdefors"`, 'c' maps to 's', 'd' maps to 'r', 'e' maps to 'o', 'f' maps to 'f', 'o' maps to 'e', 'r' maps to 'd', 's' maps to 'c'.

So, in the encoded string "serofedsoc", the unique characters are 's', 'e', 'r', 'o', 'f', 'd', 'c', sorted as 'c', 'd', 'e', 'f', 'o', 'r', 's', which matches `r`.

But in general, the unique characters in the encoded string will be the same as `r`, since the encoding replaces each character in `s` with a character from `r` based on the symmetric mapping.

Therefore, `r` can be obtained by sorting the unique characters in the encoded string.

Wait, is that correct?

In the example, yes. But let's consider another example.

Take the second test case:

Encoded string: "ttf"

Original string: "fft"

What is `r` in this case?

Unique characters in `s = "fft"` are 'f' and 't', sorted as "ft".

Encoding replaces 'f' with 't' and 't' with 'f'.

So, encoded string is "ttf", unique characters are 'f' and 't', sorted as "ft", which matches `r`.

Another test case:

Encoded string: "tlrhgmaoi"

Original string: "algorithm"

Unique characters in `s = "algorithm"` are "a", "l", "g", "o", "r", "i", "t", "h", "m", sorted as "aeghilmoqrt".

Encoding replaces each character in `s` with its symmetric counterpart in `r`.

Wait, but in this case, the encoded string is "tlrhgmaoi", unique characters are 't', 'l', 'r', 'h', 'g', 'm', 'a', 'o', 'i', sorted as "aghilmort".

Wait, this seems consistent.

So, in general, `r` can be obtained by sorting the unique characters in the encoded string, because the encoding replaces each character in `s` with a character from `r`, and `r` is the sorted unique characters from `s`.

But since `s` and the encoded string have the same unique characters (because the encoding is a mapping within `r`), sorting the unique characters of the encoded string gives us `r`.

Therefore, to decode, I can:

1. Obtain `r` by sorting the unique characters in the encoded string.

2. Create a mapping from each character in `r` to its symmetric counterpart in `r`.

3. Then, for each character in the encoded string, map it back to the original character using the inverse mapping.

Wait, more precisely:

- The encoding maps each character in `s` to its symmetric counterpart in `r`.

- Therefore, to decode, I need to map each character in the encoded string back to the original character in `s`, which is its symmetric counterpart in `r`.

So, the decoding mapping is the same as the encoding mapping.

Wait, no. Let's think carefully.

If encoding maps character `c` in `s` to `r[::-1][r.index(c)]`, then decoding should map character `c` in the encoded string back to `r[r.index(c[::-1])]`.

Wait, perhaps it's better to think in terms of indices.

Let me denote:

- `r = sorted(unique(s))`

- For each character `c` in `s`, find its index `i` in `r`, and replace it with `r[-(i+1)]`.

So, encoding: `encoded[c] = r[r.index(c) from the end]`

Decoding should be the reverse: for each character `c` in the encoded string, find its index `i` in `r`, and map it back to `r[-(i+1)]`.

Wait, actually, since the mapping is symmetric, decoding should use the same mapping as encoding.

Wait, no. Let's consider:

- In encoding, each character `c` in `s` is replaced by `r[-(r.index(c)+1)]`.

- Therefore, to decode, each character `c` in the encoded string should be replaced by `r[-(r.index(c)+1)]`.

Wait, but in the example:

`r = "cdefors"`

Encoding:

- 'c' -> 's'

- 'o' -> 'e'

- 'd' -> 'r'

- 'e' -> 'o'

- 'f' -> 'f'

- 'o' -> 'e'

- 'r' -> 'd'

- 'c' -> 's'

- 'e' -> 'o'

- 's' -> 'c'

So, to decode "serofedsoc":

- 's' -> 'c'

- 'e' -> 'o'

- 'r' -> 'd'

- 'o' -> 'e'

- 'f' -> 'f'

- 'e' -> 'o'

- 'd' -> 'r'

- 's' -> 'c'

- 'o' -> 'e'

- 'c' -> 's'

Which would give "codedeforscos", which is not the original string "codeforces".

Wait, that's not matching. What's wrong here?

Wait, perhaps I made a mistake in the decoding mapping.

Let me think again.

Given that encoding maps `c` to `s`, `o` to `e`, `d` to `r`, etc., then decoding should map `s` back to `c`, `e` back to `o`, `r` back to `d`, etc.

So, the decoding mapping is the inverse of the encoding mapping.

But in this case, since the mapping is symmetric, the inverse mapping is the same as the original mapping.

Wait, but in the above example, decoding "serofedsoc" using the same mapping gives "codedeforscos", which is not "codeforces". So, something is wrong.

Wait, perhaps I need to consider that `r` is determined from the unique sorted characters of the encoded string.

In this case, unique sorted characters of "serofedsoc" are "cdefors", which matches `r`.

So, to decode, I should:

- Have `r = "cdefors"`

- For each character in the encoded string, map it to its symmetric counterpart in `r`.

- So, 's' -> 'c', 'e' -> 'o', 'r' -> 'd', 'o' -> 'e', 'f' -> 'f', 'e' -> 'o', 'd' -> 'r', 's' -> 'c', 'o' -> 'e', 'c' -> 's'

- Concatenating these gives "codedeforscos", which is not "codeforces".

Wait, that's incorrect. So, my understanding is flawed.

Looking back at the problem, perhaps I need to consider that the mapping is based on the positions in `r`, and that `r` is known from the sorted unique characters of the encoded string.

Wait, perhaps I need to pair the characters in `r` with their symmetric counterparts and create a mapping accordingly.

Let me try to create a mapping for `r = "cdefors"`:

- 'c' (position 0) maps to 's' (position 6)

- 'd' (position 1) maps to 'r' (position 5)

- 'e' (position 2) maps to 'o' (position 4)

- 'f' (position 3) maps to 'f' (position 3)

So, the mapping is:

Encoded: 's' -> 'c'

 'r' -> 'd'

 'o' -> 'e'

 'f' -> 'f'

 'e' -> 'o'

 'd' -> 'r'

 'c' -> 's'

So, to decode "serofedsoc":

- 's' -> 'c'

- 'e' -> 'o'

- 'r' -> 'd'

- 'o' -> 'e'

- 'f' -> 'f'

- 'e' -> 'o'

- 'd' -> 'r'

- 's' -> 'c'

- 'o' -> 'e'

- 'c' -> 's'

Which gives "codedeforscos", but the original string is "codeforces".

This doesn't match. So, my approach is incorrect.

What's the mistake here?

Wait, perhaps I need to consider that the mapping is between the positions in `r`, not the characters themselves.

Let me try to think differently.

Suppose `r` has length `k`. Then, each character in `s` is replaced by the character in `r` at position `k - 1 - index`.

So, to decode, I need to map each character in the encoded string to the character in `r` at position `k - 1 - index`.

Wait, no. Wait, in encoding, each character in `s` is replaced by `r[k - 1 - index]`, where `index` is the position of the character in `r`.

Therefore, to decode, I need to map each character in the encoded string back to `r[index]`, where `index` is `k - 1 - position` in `r`.

This is getting confusing. Maybe I should think in terms of a dictionary.

Let me try to create a mapping for encoding and decoding.

Given `r = "cdefors"`, length `k = 7`.

Create a mapping for encoding:

- 'c' (position 0) -> 's' (position 6)

- 'd' (position 1) -> 'r' (position 5)

- 'e' (position 2) -> 'o' (position 4)

- 'f' (position 3) -> 'f' (position 3)

- 'o' (position 4) -> 'e' (position 2)

- 'r' (position 5) -> 'd' (position 1)

- 's' (position 6) -> 'c' (position 0)

So, the encoding mapping is:

{'c': 's', 'd': 'r', 'e': 'o', 'f': 'f', 'o': 'e', 'r': 'd', 's': 'c'}

Then, the decoding mapping should be the inverse:

{'s': 'c', 'r': 'd', 'o': 'e', 'f': 'f', 'e': 'o', 'd': 'r', 'c': 's'}

So, to decode, I need to use the inverse mapping.

But in the first approach, when I tried to decode "serofedsoc" using the inverse mapping, I got "codedeforscos", which is incorrect.

Wait, perhaps I made a mistake in applying the mapping.

Let's apply the inverse mapping step by step:

- 's' -> 'c'

- 'e' -> 'o'

- 'r' -> 'd'

- 'o' -> 'e'

- 'f' -> 'f'

- 'e' -> 'o'

- 'd' -> 'r'

- 's' -> 'c'

- 'o' -> 'e'

- 'c' -> 's'

Concatenating these gives "codedeforscos", but the original string is "codeforces".

This doesn't match. So, perhaps my assumption is wrong.

Wait, maybe I need to consider that the original string `s` can have duplicate characters, but `r` has unique sorted characters.

Perhaps I need to consider the frequency of characters.

Wait, in the encoding process, characters are replaced based on their position in `r`, but `r` is determined by the unique sorted characters of `s`.

So, in "codeforces", `r` is "cdefors", and the mapping is as above.

But when decoding, I need to make sure that the frequencies of characters match.

Wait, perhaps just mapping the characters as above isn't sufficient because the original string `s` might have characters in a specific order that needs to be preserved.

Wait, perhaps I need to consider the positions in the encoded string and map them back using the symmetric mapping based on `r`.

But I'm getting stuck here.

Let me look at another test case to see if that helps.

Take the second test case:

Encoded string: "ttf"

Original string: "fft"

Unique characters in encoded string: 't' and 'f', sorted as "ft"

So, `r = "ft"`

Mapping for encoding:

- 'f' (position 0) -> 't' (position 1)

- 't' (position 1) -> 'f' (position 0)

So, encoding mapping: {'f': 't', 't': 'f'}

Decoding mapping: {'t': 'f', 'f': 't'}

Decoding "ttf":

- 't' -> 'f'

- 't' -> 'f'

- 'f' -> 't'

Which gives "fft", matching the original string.

So, in this case, it works.

Wait, but in the first test case, it didn't work. Why is that?

Wait, perhaps because in the first test case, there are multiple characters, and the mapping needs to be applied correctly based on `r`.

Wait, perhaps I need to think of `r` as a list, and for each character in the encoded string, find its position in `r` and map it to the character in `r` at the symmetric position.

Wait, perhaps I need to create a mapping where for each character in `r`, its encoding is `r[::-1][r.index(c)]`.

Wait, no, I think I need to map each character in the encoded string to its symmetric counterpart in `r`.

Wait, perhaps I need to map each character in the encoded string to `r[k - 1 - r.index(c)]`.

Wait, let's try that with the first test case.

`r = "cdefors"`, k = 7

For each character in the encoded string "serofedsoc":

- 's' is at position 6 in `r`, so map to `r[6 - 6] = r[0] = 'c'`

- 'e' is at position 2 in `r`, so map to `r[6 - 2] = r[4] = 'o'`

- 'r' is at position 5 in `r`, so map to `r[6 - 5] = r[1] = 'd'`

- 'o' is at position 4 in `r`, so map to `r[6 - 4] = r[2] = 'e'`

- 'f' is at position 3 in `r`, so map to `r[6 - 3] = r[3] = 'f'`

- 'e' is at position 2 in `r`, so map to `r[6 - 2] = r[4] = 'o'`

- 'd' is at position 1 in `r`, so map to `r[6 - 1] = r[5] = 'r'`

- 's' is at position 6 in `r`, so map to `r[6 - 6] = r[0] = 'c'`

- 'o' is at position 4 in `r`, so map to `r[6 - 4] = r[2] = 'e'`

- 'c' is at position 0 in `r`, so map to `r[6 - 0] = r[6] = 's'`

So, concatenating these gives "codedeforscos", which is not "codeforces".

Wait, that's the same result as before. So, it seems like my mapping is incorrect.

Wait, perhaps the formula for decoding is different.

Let me think differently.

Since encoding maps `s[i]` to `r[k - 1 - r.index(s[i])]`, then to decode, I need to map `encoded[i]` back to `r[k - 1 - r.index(encoded[i])]`.

Wait, but in the first test case, this gives "codedeforscos", which is incorrect.

So, perhaps I need to consider that the mapping is unique and that some characters might map to the same character in the encoded string.

Wait, perhaps there's a better way to approach this.

Let me consider that `r` is a sorted list of unique characters from `s`, and the encoding replaces each character in `s` with its symmetric counterpart in `r`.

To decode, I need to replace each character in the encoded string with its symmetric counterpart in `r`.

Wait, but in the first test case, applying this gives "codedeforscos", which is not "codeforces".

So, perhaps my understanding is incomplete.

Wait, maybe I need to consider that the original string `s` can have duplicate characters, but `r` has unique characters.

So, in "codeforces", 'c' and 's' appear once, 'o' appears twice, etc.

But in the encoding, each character is replaced based on its position in `r`, regardless of its frequency.

So, perhaps I need to count the frequency of each character in the encoded string and arrange them according to the symmetric positions in `r`.

Wait, perhaps I need to sort the encoded string based on the symmetric positions in `r`.

Wait, I'm getting confused.

Let me try to think about it differently.

Suppose I have `r` and the encoding mapping. Then, to decode, I need to apply the inverse mapping.

But in the first test case, applying the inverse mapping gives "codedeforscos", which is incorrect.

So, perhaps there's a mistake in assuming that `r` is obtained by sorting the unique characters of the encoded string.

Wait, perhaps `r` is obtained by sorting the unique characters of the original string `s`, but in the encoding process, `s` is transformed to the encoded string based on `r`.

But since I don't know `s`, I need another way to find `r`.

Wait, perhaps I can find `r` by analyzing the encoded string and considering the symmetric mapping.

Let me consider that `r` is a sorted list of unique characters from `s`, and the encoding maps each character in `s` to its symmetric counterpart in `r`.

Therefore, in the encoded string, characters appear in positions corresponding to their symmetric counterparts in `s`.

Wait, perhaps I need to find a permutation of characters in `r` such that applying the symmetric mapping twice returns to the original string.

Wait, that sounds like an involution.

In any case, I'm getting stuck here.

Let me look at another test case.

Take the third test case:

Encoded string: "tlrhgmaoi"

Original string: "algorithm"

Unique sorted characters in original string: "aeghilmoqrt"

Wait, but in the encoded string, unique sorted characters are "aghilmort".

Wait, "tlrhgmaoi" unique characters: 'a', 'g', 'h', 'i', 'l', 'm', 'o', 'r', 't', sorted as "aghilmort".

But the original `r` is "aeghilmoqrt".

Wait, they are different.

So, in this case, sorting the unique characters of the encoded string does not give the same `r` as the sorted unique characters of `s`.

Wait, this contradicts my earlier assumption.

So, perhaps my assumption that `r` can be obtained by sorting the unique characters of the encoded string is incorrect.

Wait, but in the second test case, it worked.

Wait, in the second test case, encoded string "ttf", unique sorted characters "ft", which matches `r = "ft"`.

In the first test case, encoded string "serofedsoc", unique sorted characters "cdefors", which matches `r = "cdefors"`.

In the third test case, encoded string "tlrhgmaoi", unique sorted characters "aghilmort", but original `r` is "aeghilmoqrt".

These are different.

So, my assumption is wrong.

Therefore, I cannot obtain `r` by sorting the unique characters of the encoded string.

Wait, why is this the case?

Wait, perhaps because the encoding process replaces characters based on their positions in `r`, and the encoded string may not contain all characters from `r` in the same frequencies.

Wait, no. In the encoding, each character in `s` is replaced by its symmetric counterpart in `r`, so the unique characters in the encoded string should match the unique characters in `r`.

Wait, but in the third test case, "tlrhgmaoi" has unique characters "aghilmort", but original `r` is "aeghilmoqrt".

Wait, "aeghilmoqrt" has 'e' and 'q' which are not in the encoded string.

Wait, no, the original string is "algorithm", unique characters "a", "l", "g", "o", "r", "i", "t", "h", "m", sorted as "aeghilmoqrt".

But in the encoded string "tlrhgmaoi", unique characters are "a", "g", "h", "i", "l", "m", "o", "r", "t", sorted as "aghilmort".

Wait, "aeghilmoqrt" vs "aghilmort", so 'e' and 'q' are missing in the encoded string's unique characters.

Wait, but 'e' is in "algorithm", but in the encoded string, 'e' might not be present.

Wait, no, "algorithm" has 'a', 'l', 'g', 'o', 'r', 'i', 't', 'h', 'm', no 'e' or 'q'.

Wait, perhaps I made a mistake.

Wait, "algorithm" has characters 'a', 'l', 'g', 'o', 'r', 'i', 't', 'h', 'm', sorted as "aghilmort".

Wait, but in the encoded string "tlrhgmaoi", unique sorted characters are "aghilmort", which matches the sorted unique characters of "algorithm".

Wait, perhaps I misread earlier.

So, in this case, `r` is "aghilmort".

Then, encoding mapping would be:

- 'a' (pos 0) -> 't' (pos 8)

- 'g' (pos 1) -> 'm' (pos 7)

- 'h' (pos 2) -> 'o' (pos 6)

- 'i' (pos 3) -> 'r' (pos 5)

- 'l' (pos 4) -> 'l' (pos 4)

- 'm' (pos 5) -> 'i' (pos 3)

- 'o' (pos 6) -> 'h' (pos 2)

- 'r' (pos 7) -> 'g' (pos 1)

- 't' (pos 8) -> 'a' (pos 0)

So, encoding mapping: {'a': 't', 'g': 'm', 'h': 'o', 'i': 'r', 'l': 'l', 'm': 'i', 'o': 'h', 'r': 'g', 't': 'a'}

Decoding mapping: inverse of above: {'t': 'a', 'm': 'g', 'o': 'h', 'r': 'i', 'l': 'l', 'i': 'm', 'h': 'o', 'g': 'r', 'a': 't'}

Decoding "tlrhgmaoi":

- 't' -> 'a'

- 'l' -> 'l'

- 'r' -> 'i'

- 'h' -> 'o'

- 'g' -> 'r'

- 'm' -> 'g'

- 'a' -> 't'

- 'o' -> 'h'

- 'i' -> 'm'

Which gives "allirogrtmh", which is not "algorithm".

Wait, that's not matching. So, perhaps my approach is still incorrect.

Wait, perhaps I need to consider that the positions are zero-based, and the symmetric position is `k - 1 - index`.

In the third test case:

`r = "aghilmort"`, k = 9

- 'a' at pos 0 -> 't' at pos 8

- 'g' at pos 1 -> 'm' at pos 7

- 'h' at pos 2 -> 'o' at pos 6

- 'i' at pos 3 -> 'r' at pos 5

- 'l' at pos 4 -> 'l' at pos 4

- 'm' at pos 5 -> 'i' at pos 3

- 'o' at pos 6 -> 'h' at pos 2

- 'r' at pos 7 -> 'g' at pos 1

- 't' at pos 8 -> 'a' at pos 0

So, encoding mapping is as above.

Decoding mapping is the inverse.

Decoding "tlrhgmaoi":

- 't' -> 'a'

- 'l' -> 'l'

- 'r' -> 'i'

- 'h' -> 'o'

- 'g' -> 'r'

- 'm' -> 'g'

- 'a' -> 't'

- 'o' -> 'h'

- 'i' -> 'm'

Which gives "allirogrtmh", but the original string is "algorithm".

This doesn't match. So, perhaps there's a mistake in my understanding.

Wait, perhaps the positions are one-based or zero-based differently.

Let me try considering one-based indexing.

So, for `r = "aghilmort"`, k = 9

- 'a' at pos 0 -> 't' at pos 8

- 'g' at pos 1 -> 'm' at pos 7

- 'h' at pos 2 -> 'o' at pos 6

- 'i' at pos 3 -> 'r' at pos 5

- 'l' at pos 4 -> 'l' at pos 4

- 'm' at pos 5 -> 'i' at pos 3

- 'o' at pos 6 -> 'h' at pos 2

- 'r' at pos 7 -> 'g' at pos 1

- 't' at pos 8 -> 'a' at pos 0

Same as before.

Decoding "tlrhgmaoi" gives "allirogrtmh", which is incorrect.

Wait, maybe the positions are based on the one-based index.

So, positions start from 1 to 9.

Then, symmetric position of character at position `i` is `k - i + 1`.

So, for `r = "aghilmort"`, k = 9

- 'a' at pos 1 -> 't' at pos 9

- 'g' at pos 2 -> 'm' at pos 8

- 'h' at pos 3 -> 'o' at pos 7

- 'i' at pos 4 -> 'r' at pos 6

- 'l' at pos 5 -> 'l' at pos 5

- 'm' at pos 6 -> 'i' at pos 4

- 'o' at pos 7 -> 'h' at pos 3

- 'r' at pos 8 -> 'g' at pos 2

- 't' at pos 9 -> 'a' at pos 1

So, encoding mapping is same as before.

Decoding "tlrhgmaoi":

- 't' -> 'a'

- 'l' -> 'l'

- 'r' -> 'i'

- 'h' -> 'o'

- 'g' -> 'r'

- 'm' -> 'g'

- 'a' -> 't'

- 'o' -> 'h'

- 'i' -> 'm'

Which gives "allirogrtmh", still not "algorithm".

So, my approach is flawed.

Perhaps I need to consider that the original string `s` can have characters in any order, and the encoding replaces each character based on its position in `r`.

But in decoding, I need to map each character in the encoded string back to its original character in `s`, which requires knowing the symmetric mapping based on `r`.

Wait, perhaps I need to create a mapping from encoded characters to original characters based on their positions in `r`.

Let me try to think of `r` as a list, and create a mapping where each character in `r` is mapped to its symmetric counterpart.

Then, to decode, I need to map each character in the encoded string to its symmetric counterpart in `r`.

Wait, but in the first test case, this doesn't give the correct result.

Alternatively, perhaps I need to consider that the encoding is a permutation, and to decode, I need to apply the inverse permutation.

In the first test case, the mapping is:

{'c': 's', 'd': 'r', 'e': 'o', 'f': 'f', 'o': 'e', 'r': 'd', 's': 'c'}

The inverse mapping is:

{'s': 'c', 'r': 'd', 'o': 'e', 'f': 'f', 'e': 'o', 'd': 'r', 'c': 's'}

Applying this to "serofedsoc" gives "codedeforscos", which is incorrect.

So, perhaps this approach is wrong.

Wait, maybe I need to consider that the original string `s` can have duplicate characters, and the mapping needs to preserve those frequencies.

Wait, but in the first test case, "codeforces" has two 'o's, and "serofedsoc" also has two 'o's.

But when decoding "serofedsoc", I get "codedeforscos", which has two 'o's as well.

But the arrangement is incorrect.

So, perhaps I need to consider the positions in the encoded string and map them back according to the symmetric positions in `r`.

Wait, perhaps I need to map each character in the encoded string to its symmetric counterpart in `r`, but considering the frequency of characters.

Wait, I'm stuck.

Let me look at the fourth test case:

Encoded string: "w"

Original string: "w"

Unique sorted characters in `s` is "w", so `r = "w"`

Encoding mapping: 'w' -> 'w'

Decoding is the same: 'w' -> 'w'

So, it works.

Fifth test case:

Encoded string: "hnndledmnhlttin"

Original string: "meetinthemiddle"

Unique sorted characters in `s` are "demhilt", so `r = "demhilt"`

Encoding mapping:

- 'd' (pos 0) -> 't' (pos 6)

- 'e' (pos 1) -> 'l' (pos 5)

- 'm' (pos 2) -> 'h' (pos 4)

- 'h' (pos 3) -> 'm' (pos 3)

- 'i' (pos 4) -> 'h' (pos 2)

- 'l' (pos 5) -> 'e' (pos 1)

- 't' (pos 6) -> 'd' (pos 0)

Decoding mapping:

- 't' -> 'd'

- 'l' -> 'e'

- 'h' -> 'm'

- 'm' -> 'h'

- 'e' -> 'l'

- 'i' -> 'i'

- 'd' -> 't'

Decoding "hnndledmnhlttin":

- 'h' -> 'm'

- 'n' -> ?

Wait, 'n' is not in the mapping. Hmm.

Wait, in the encoded string "hnndledmnhlttin", unique sorted characters are "demhilt", so 'n' is not in `r`.

Wait, that can't be.

Wait, "meetinthemiddle" has unique characters 'd', 'e', 'h', 'i', 'l', 'm', 't', sorted as "dehilmt".

So, `r = "dehilmt"`, k = 7

Encoding mapping:

- 'd' (pos 0) -> 't' (pos 6)

- 'e' (pos 1) -> 'l' (pos 5)

- 'h' (pos 2) -> 'm' (pos 4)

- 'i' (pos 3) -> 'i' (pos 3)

- 'l' (pos 4) -> 'h' (pos 2)

- 'm' (pos 5) -> 'e' (pos 1)

- 't' (pos 6) -> 'd' (pos 0)

Decoding mapping:

- 't' -> 'd'

- 'l' -> 'e'

- 'm' -> 'h'

- 'i' -> 'i'

- 'h' -> 'l'

- 'e' -> 'm'

- 'd' -> 't'

Decoding "hnndledmnhlttin":

- 'h' -> 'l'

- 'n' -> ?

Again, 'n' is not in the mapping.

Wait, perhaps there's a mistake in assuming that `r` is obtained by sorting the unique characters of the encoded string.

In this case, "hnndledmnhlttin" has unique sorted characters "dehilmt", which matches `r`.

But 'n' appears in the encoded string, which is not in `r`. So, how is that possible?

Wait, no, "hnndledmnhlttin" has unique characters 'd', 'e', 'h', 'l', 'm', 'n', 't', sorted as "dehlmnt".

Original `r` is "dehilmt".

So, in this case, 'n' is present in the encoded string but not in `r`.

Wait, but according to the encoding process, all characters in the encoded string should be in `r`, since `r` contains all unique characters from `s`.

Wait, but in this test case, 'n' appears in the encoded string, but 'n' is not in `r`.

Wait, perhaps I'm misunderstanding something.

Looking back at the problem statement:

"It is guaranteed that the sum of the values of n over all test cases in the test does not exceed 2â‹…10^5."

Wait, no, that's about the input constraints.

Wait, perhaps the problem allows for characters in the encoded string that are not in `r`. But according to the encoding process, all characters in the encoded string should be in `r`, since they are replacements from `r`.

So, perhaps there's a mistake in my earlier assumption.

Wait, perhaps I need to consider that `r` contains all unique characters from `s`, and the encoded string only contains characters from `r`.

But in the fifth test case, 'n' appears in the encoded string, but 'n' is not in `r`.

Wait, perhaps I misread the test case.

Looking back at the test cases:

Input:

5

10

serofedsoc

3

ttf

9

tlrhgmaoi

1

w

15

hnndledmnhlttin

Output:

codeforces

fft

algorithm

w

meetinthemiddle

Wait, in the fifth test case, encoded string is "hnndledmnhlttin", original string is "meetinthemiddle".

Unique sorted characters in "meetinthemiddle" are 'd', 'e', 'h', 'i', 'l', 'm', 't', sorted as "dehilmt", so `r = "dehilmt"`, k = 7

Encoding mapping:

- 'd' -> 't'

- 'e' -> 'l'

- 'h' -> 'm'

- 'i' -> 'i'

- 'l' -> 'h'

- 'm' -> 'e'

- 't' -> 'd'

Encoding "meetinthemiddle":

- 'm' -> 'e'

- 'e' -> 'l'

- 'e' -> 'l'

- 't' -> 'd'

- 'i' -> 'i'

- 'n' -> ?

Wait, 'n' is not in `r`, so how is it encoded?

Wait, that's the issue. The original string "meetinthemiddle" contains 'n', which is not in `r`. But according to the encoding process, all characters in `s` should be in `r`, since `r` contains all unique characters from `s`.

Wait, no, `r` contains all unique characters from `s`, sorted. So, if 'n' is in `s`, it should be in `r`.

Wait, but "meetinthemiddle" has 'n' in it.

Wait, no, "meetinthemiddle" consists of 'm', 'e', 't', 'i', 'n', 'h', 'l', 'd', 'i', 'l', 'l', 'e'.

Unique characters: 'd', 'e', 'h', 'i', 'l', 'm', 'n', 't', sorted as "dehilmt".

Wait, 'n' is present in `r`.

Wait, no, "dehilmt" does not have 'n'.

Wait, no, "meetinthemiddle" has 'n', so unique sorted characters should be "dehilmt".

Wait, no, "meetinthemiddle" has 'm', 'e', 'e', 't', 'i', 'n', 't', 'h', 'e', 'm', 'i', 'd', 'd', 'l', 'e'.

Unique characters: 'd', 'e', 'h', 'i', 'l', 'm', 'n', 't', sorted as "dehilmnt".

So, `r = "dehilmnt"`, k = 8

Encoding mapping:

- 'd' (pos 0) -> 't' (pos 7)

- 'e' (pos 1) -> 'n' (pos 6)

- 'h' (pos 2) -> 'm' (pos 5)

- 'i' (pos 3) -> 'l' (pos 4)

- 'l' (pos 4) -> 'i' (pos 3)

- 'm' (pos 5) -> 'h' (pos 2)

- 'n' (pos 6) -> 'e' (pos 1)

- 't' (pos 7) -> 'd' (pos 0)

So, encoding mapping: {'d': 't', 'e': 'n', 'h': 'm', 'i': 'l', 'l': 'i', 'm': 'h', 'n': 'e', 't': 'd'}

Encoding "meetinthemiddle":

- 'm' -> 'h'

- 'e' -> 'n'

- 'e' -> 'n'

- 't' -> 'd'

- 'i'