The code snippet `r = mid - 1` updates the value of `r` to `mid - 1`. The values of `l`, `mid`, `array`, `find`, and `n` remain unchanged. 

Given that `mid` is calculated as `(l + r) // 2`, and `l` is initially 0 and `r` is initially `n - 1`, the new value of `r` after the assignment will be `((0 + (n - 1)) // 2) - 1`, which simplifies to `(n - 1) // 2 - 1`.

Output State: **`array` is a list of integers representing a permutation of length `n` (1 ≤ `n` ≤ 2·10^5), `find` is an integer (1 ≤ `find` ≤ `n`) that exists in the array, `n` is the length of `array`, `l` is 0, `r` is `(n - 1) // 2 - 1`, `mid` is `(l + r) // 2`**.