First, let's analyze the given code snippet and the initial state:

- `i` is 1.
- `k` is a valid integer within the range 1 ≤ k ≤ 45.
- `M` must be at least 1.
- `t` is a sorted list of integers.
- `dp` is a 2D list with dimensions `(k+1) x (M+1)`. For `dp[1][j]`, it is 2 if `j >= t[0]` and 1 otherwise, for `1 ≤ j ≤ M`, and all other elements of `dp` are 0.
- `j` is 3.
- `dp[1][3]` is equal to `dp[1][2]`.

The code snippet is:
```python
dp[i][j] = max(dp[i][j], dp[i - 1][j - t[i - 1]] + 1)
```

Given that `i` is 1, the equation simplifies to:
```python
dp[1][j] = max(dp[1][j], dp[0][j - t[0]] + 1)
```

Since `dp[0][...]` is undefined, this equation is effectively:
```python
dp[1][j] = max(dp[1][j], 0 + 1) = max(dp[1][j], 1)
```

Given the initial state, we know:
- `dp[1][3]` is already set to `dp[1][2]`, which is 1 because `j < t[0]` initially.

Therefore, when `i` is 1 and `j` is 3:
- `dp[1][3]` remains unchanged because `max(dp[1][3], 1)` is just `dp[1][3]` since `dp[1][3]` is already 1.

Output State: **`i` is 1; `k` is a valid integer within the range 1 ≤ k ≤ 45; `M` must be at least 1; `t` is a sorted list of integers; `dp` is a 2D list with dimensions `(k+1) x (M+1)`, where `dp[1][3]` is 1, and all other elements remain 0; `j` is 3.**