Alright, I have this problem to solve. Let's see what it's asking for. So, Nikita has a word consisting of exactly 3 lowercase Latin letters. Each letter has a position in the alphabet from 1 to 26, where 'a' is 1, 'b' is 2, up to 'z' is 26. He encodes the word by summing up the positions of its letters. For example, "cat" is 3 + 1 + 20 = 24.

But the problem is that this encoding can be ambiguous because different words can have the same sum. For example, "ava" also sums to 24. So, given the sum, I need to find the lexicographically smallest word that could have been encoded to that sum.

First, I need to understand what "lexicographically smallest" means. It means that among all possible words that sum to the given number, I have to find the one that would come first in a dictionary. So, for example, "aav" would be smaller than "ava" because 'a' is smaller than 'v' at the second position.

Okay, so the task is to, for each test case, given an integer n (which is the sum of the positions of the three letters), output the smallest possible word consisting of three lowercase letters that sums to n.

The constraints are that t, the number of test cases, is between 1 and 100, and n is between 3 and 78. Since each letter is at least 1 ('a') and at most 26 ('z'), the minimum sum is 1+1+1=3 and the maximum sum is 26+26+26=78, which matches the constraints.

Now, I need to think about how to find the smallest word for a given sum n.

One approach is to start with the smallest possible letters and maximize the last letter. Wait, no. To get the lexicographically smallest word, I should minimize the first letter, then the second, and maximize the third.

Wait, actually, to minimize the word lexicographically, I should choose the smallest possible first letter, then the smallest possible second letter given the first, and then the third letter is determined by the remaining sum.

So, for example, if n=24, I start with 'a' (1), then the remaining sum is 23 for the last two letters. Then, for the second letter, I choose the smallest possible, which is 'a' again (1), leaving 22 for the third letter, which is 'v' (22). So, "aav" is one possible word. But "ava" is also possible, but "aav" is smaller than "ava" because 'a' is smaller than 'v' at the second position.

Wait, but in the example, for n=24, the output is "aav", which matches what I just thought.

Another example in the input is 70, and the output is "rzz". Let's see: 'r' is 18, 'z' is 26, so 18 + 26 + 26 = 70. Is there a smaller word than "rzz"? Let's see: starting with 'q' (17), then the remaining sum is 53 for the last two letters. 'z' and 'z' would be 26 + 27 = 53, but 'z' is only 26, so that's not possible. Wait, no: 17 + 26 + 27 = 70, but 'z' is 26, so it's 17 + 26 + 27 = 70, but since 'z' is 26, it's the maximum. So, 'qaz' would be 17 + 1 + 26 = 44, which is less than 70. So, 'q' is too small. Need to start with a larger first letter.

Wait, perhaps it's better to work backwards. To minimize the word, fix the first letter as small as possible, then fix the second letter as small as possible given the first, and then set the third letter to be as large as possible given the first two.

So, for n=24, start with 'a' (1), then second letter 'a' (1), third letter 'v' (22), sum=24.

Is there any smaller word than "aav"? No, because any word starting with 'a' and second letter smaller than 'a' isn't possible, and 'a' is already the smallest. So, "aav" is the smallest.

Another example: n=3. The smallest word is "aaa", which makes sense because 1+1+1=3.

n=55: "czz", which is 'c' (3) + 'z' (26) + 'z' (26) = 55.

n=48: "auz", which is 'a' (1) + 'u' (21) + 'z' (26) = 48.

So, the strategy seems to be: minimize the first letter, then minimize the second letter given the first, and maximize the third letter given the first two.

Wait, but in the code provided, it seems to handle different cases based on the value of n.

Let me look at the provided program:

```python

import string

def func():

    alphabet = string.ascii_lowercase

    for _ in range(int(input())):

        n = int(input())

        word = ''

        if n > 52:

            word += alphabet[n - 53] + 'zz'

        elif n > 26:

            word += 'a' + alphabet[n - 28] + 'z'

        else:

            word += 'aa' + alphabet[n - 3]

        print(word)

```

So, it's handling three cases:

1. If n > 52, it does alphabet[n - 53] + 'zz'

2. If n > 26, it does 'a' + alphabet[n - 28] + 'z'

3. Otherwise, it does 'aa' + alphabet[n - 3]

I need to verify if this logic is correct.

Let's test it with n=24.

Since 24 > 26 is False, it goes to the else clause: 'aa' + alphabet[24 - 3] = 'aa' + alphabet[21] = 'aa' + 'u' = 'aau'

But in the sample input, for n=24, the output is "aav", which is 1 + 1 + 22 = 24.

Wait, that's different from what the code is producing.

Wait, maybe I misread the code.

Wait, let's see:

For n=24:

n > 52: 24 > 52 is False

n > 26: 24 > 26 is False

So, it goes to the else clause: 'aa' + alphabet[24 - 3] = 'aa' + alphabet[21] = 'aa' + 'u' = 'aau'

But in the sample output, it's "aav" for n=24.

So, there's a discrepancy here.

Wait, maybe I'm misreading the conditions.

Let me look again:

if n > 52:

word += alphabet[n - 53] + 'zz'

elif n > 26:

word += 'a' + alphabet[n - 28] + 'z'

else:

word += 'aa' + alphabet[n - 3]

For n=24:

n > 52: False

n > 26: 24 > 26 is False

So, it goes to 'aa' + alphabet[21] = 'aau'

But sample output is "aav" for n=24.

So, the code is producing "aau", but the correct output is "aav".

Wait, but "aau" sums to 1 + 1 + 21 = 23, which is not 24.

Wait, alphabet[21] is 'u', which is 21, so 1 + 1 + 21 = 23, which is less than 24.

So, the code is wrong here.

Wait, maybe I'm misunderstanding the indexing.

In Python, string.ascii_lowercase is 'abcdefghijklmnopqrstuvwxyz', and alphabet[0] is 'a', alphabet[1] is 'b', up to alphabet[25] is 'z'.

So, alphabet[n - 53] would be for n=24, 24 - 53 = -29, which is invalid.

Wait, no, for n=24, it doesn't enter the first condition because 24 <= 52.

Then, n > 26: 24 > 26 is False, so it goes to 'aa' + alphabet[21] = 'aau'

But 'aau' sums to 1 + 1 + 21 = 23, which is less than 24.

So, it's incorrect.

Wait, perhaps the logic is to make sure that the sum is exactly n.

Wait, maybe I need to understand the logic behind the code.

Let me try to understand the three cases:

1. If n > 52: It uses alphabet[n - 53] + 'zz'

So, for n=78: 78 > 52, so alphabet[78 - 53] = alphabet[25] = 'z' + 'zz' = 'zzz', which sums to 26 + 26 + 26 = 78. Correct.

n=53: alphabet[53 - 53] = alphabet[0] = 'a' + 'zz' = 'azz', which sums to 1 + 26 + 26 = 53. Correct.

n=52: 52 > 52 is False, so it goes to the next condition.

Wait, n=52: 52 > 52 is False, so it goes to n > 26: 52 > 26 is True, so 'a' + alphabet[52 - 28] + 'z' = 'a' + alphabet[24] + 'z' = 'a' + 'x' + 'z' = 'axz', which sums to 1 + 24 + 26 = 51, which is less than 52. So, incorrect.

Wait, that's a problem.

Wait, maybe there's an off-by-one error in the indexing.

Wait, alphabet is 0-indexed, with alphabet[0] = 'a', alphabet[1] = 'b', ..., alphabet[25] = 'z'.

So, for n=52, 'axz' sums to 1 + 24 + 26 = 51, which is less than 52.

So, it's incorrect.

Wait, perhaps it should be 'ayz': 1 + 25 + 26 = 52. That's correct.

So, for n=52, it should be 'ayz'.

But according to the code, it's 'a' + alphabet[52 - 28] + 'z' = 'a' + alphabet[24] + 'z' = 'a' + 'x' + 'z' = 'axz', which is incorrect.

So, there's an error in the code.

Wait, perhaps it's off by one.

Let me check n=52: 52 - 28 = 24, alphabet[24] = 'x', but should be 'y' for 25.

Wait, 'y' is alphabet[24], actually.

Wait, no: alphabet[24] is 'y', not 'x'. Wait, no, 'y' is 25, 'x' is 24.

Wait, letters are numbered from 1 to 26, so 'a' is 1, 'b' is 2, ..., 'z' is 26.

But in the code, alphabet is 0-indexed, so alphabet[0] = 'a', alphabet[1] = 'b', ..., alphabet[25] = 'z'.

So, for n=52, it should be 'a' + 'y' + 'z' = 1 + 25 + 26 = 52.

But according to the code, alphabet[24] is 'y', because alphabet[24] = 'y'.

Wait, but in the code, for n=52, it's 'a' + alphabet[24] + 'z' = 'ayz', which is correct.

Wait, but earlier I thought it was 'axz', but that was a mistake.

Wait, no, for n=52, it's 'a' + alphabet[52 - 28] + 'z' = 'a' + alphabet[24] + 'z' = 'ayz', which is correct.

Wait, perhaps I miscalculated earlier.

So, for n=52, it's 'ayz', which is correct.

Earlier, I mistakenly thought alphabet[24] was 'x', but actually it's 'y'.

So, 'y' is 25, 'z' is 26, so 1 + 25 + 26 = 52. Correct.

Wait, but earlier for n=24, it was 'aau', which is 1 + 1 + 21 = 23, which is less than 24.

So, it's incorrect.

Wait, perhaps there's a mistake in how the letters are being selected.

Let me think differently.

Maybe a better approach is to minimize the first letter, then minimize the second letter given the first, and set the third letter to be the remaining value.

So, for n=24, start with 'a' (1), then minimize the second letter, say 'a' (1), then the third letter is 24 - 1 - 1 = 22, which is 'v'. So, "aav".

But the code is producing 'aau' for n=24, which is 1 + 1 + 21 = 23, which is incorrect.

So, the code is wrong here.

Wait, perhaps I need to understand the logic behind the code's conditions.

Let me see:

if n > 52:

word += alphabet[n - 53] + 'zz'

So, for n > 52, it sets the first letter to alphabet[n - 53], and the next two letters to 'z'.

For example, n=78: alphabet[78 - 53] = alphabet[25] = 'z' + 'zz' = 'zzz', which is correct.

n=53: alphabet[53 - 53] = alphabet[0] = 'a' + 'zz' = 'azz', which is 1 + 26 + 26 = 53. Correct.

n=52: 'a' + alphabet[52 - 28] + 'z' = 'a' + alphabet[24] + 'z' = 'a' + 'y' + 'z' = 'ayz', which is 1 + 25 + 26 = 52. Correct.

n=24: since 24 <= 52 and 24 <= 26, it goes to 'aa' + alphabet[24 - 3] = 'aa' + alphabet[21] = 'aa' + 'v' = 'aav', which is 1 + 1 + 22 = 24. Correct.

Wait, in the earlier step, I thought it would be 'aau', but actually, 24 - 3 = 21, which is 'v', so 'aav' is correct.

Wait, perhaps I made a mistake earlier.

So, for n=24:

n > 52: False

n > 26: 24 > 26 is False

So, it goes to 'aa' + alphabet[21] = 'aav', which is correct.

Wait, but earlier I thought it would be 'aau', but 24 - 3 = 21, which is 'v', so 'aav' is correct.

So, perhaps I misread the code initially.

Let me check n=70:

n > 52: 70 > 52 is True, so alphabet[70 - 53] + 'zz' = alphabet[17] + 'zz' = 'rzz', which is 18 + 26 + 26 = 70. Correct.

n=3:

n > 52: False

n > 26: 3 > 26 is False

So, 'aa' + alphabet[0] = 'aaa', which is 1 + 1 + 1 = 3. Correct.

n=55:

n > 52: 55 > 52 is True, so alphabet[55 - 53] + 'zz' = alphabet[2] + 'zz' = 'czz', which is 3 + 26 + 26 = 55. Correct.

n=48:

n > 52: False

n > 26: 48 > 26 is True, so 'a' + alphabet[48 - 28] + 'z' = 'a' + alphabet[20] + 'z' = 'a' + 'u' + 'z' = 'auz', which is 1 + 21 + 26 = 48. Correct.

So, it seems that the code is correct for these cases.

Wait, but earlier I thought for n=24 it was producing 'aau', but actually it's producing 'aav', which is correct.

So, perhaps I misread the code initially.

Therefore, the code seems to be correct.

Hence, Correctness: **True**

## Final Solution
To solve this problem, we need to find the lexicographically smallest three-letter word that sums up to a given value \( n \), where each letter's position in the alphabet corresponds to its value (a=1, b=2, ..., z=26).

### Approach
1. **Minimizing the Word Lexicographically**:
    - To get the smallest word lexicographically, we should make the first letter as small as possible, then the second letter as small as possible given the first letter, and finally set the third letter to make the sum equal to \( n \).

2. **Handling Different Ranges of \( n \)**:
    - If \( n \) is greater than 52, the first letter must be such that the remaining sum for two 'z's (each worth 26) is accounted for.
    - If \( n \) is greater than 26 but less than or equal to 52, set the first letter to 'a' and adjust the second and third letters accordingly.
    - If \( n \) is 26 or less, set the first two letters to 'a' and determine the third letter based on the remaining sum.

### Solution Code
```python
import string

def main():
    alphabet = string.ascii_lowercase
    t = int(input())
    for _ in range(t):
        n = int(input())
        word = ''
        if n > 52:
            # Set first letter to the letter that allows 'zz' to reach the sum
            first_letter_index = n - 53  # Because 'z' is 26, so two 'z's are 52, hence n - 53
            word += alphabet[first_letter_index] + 'zz'
        elif n > 26:
            # Set first letter to 'a', and find the second letter accordingly
            second_letter_index = n - 28  # Because 'a' is 1 and 'z' is 26, so 1 + x + 26 = n => x = n - 27
            word += 'a' + alphabet[second_letter_index] + 'z'
        else:
            # Set first two letters to 'a', and find the third letter
            third_letter_index = n - 3  # Because 'a' + 'a' + x = n => x = n - 2
            word += 'aa' + alphabet[third_letter_index]
        print(word)

if __name__ == "__main__":
    main()
```

### Explanation
1. **Reading Input**:
    - Read the number of test cases \( t \).
    - For each test case, read the integer \( n \).

2. **Generating the Word**:
    - **Case 1**: If \( n > 52 \):
        - Calculate the index for the first letter such that the remaining sum for 'zz' is correct.
        - Append the corresponding letter and 'zz'.
    - **Case 2**: If \( 26 < n \leq 52 \):
        - Set the first letter to 'a'.
        - Calculate the index for the second letter based on the remaining sum after assigning 'a' and 'z' to the third letter.
        - Append 'a', the second letter, and 'z'.
    - **Case 3**: If \( n \leq 26 \):
        - Set the first two letters to 'a'.
        - Calculate the index for the third letter based on the remaining sum.
        - Append 'aa' and the third letter.

3. **Output the Word**:
    - Print the generated word for each test case.

This approach ensures that we always get the lexicographically smallest word for the given sum \( n \).