`rem` is assigned the value of `n - 2 * (a + b)`. Given that `a` is 1 and `b` is 1, the expression simplifies to `n - 2 * (1 + 1)` which further simplifies to `n - 4`. The value of `n` is a positive integer such that 1 ≤ n ≤ 2·10^9 and n is greater than or equal to 6. Therefore, `rem` is calculated as `n - 4`. The states of the other variables (`n`, `count`, `a`, `b`) remain unchanged.

Output State: **`n` is a positive integer such that 1 ≤ n ≤ 2·10^9 and n is greater than or equal to 6, `count` is 0, `a` is 1, `b` is 1, `rem` is `n - 4`**