The value of `cnt` is updated by adding the minimum of two expressions: `n / ((x + y) * x)` and `m // ((x + y) * y)`. Given the initial state:

- `n` and `m` are positive integers such that 1 <= n, m <= 2 * 10^6
- `x` is 1
- `y` is 3
- `cnt` is the minimum of `n / 3` and `m // 6`

Let's calculate the new value of `cnt`:

1. Calculate `x + y`: `1 + 3 = 4`
2. Calculate `(x + y) * x`: `4 * 1 = 4`
3. Calculate `(x + y) * y`: `4 * 3 = 12`
4. Calculate `n / ((x + y) * x)`: `n / 4`
5. Calculate `m // ((x + y) * y)`: `m // 12`
6. Find the minimum of `n / 4` and `m // 12`
7. Add this minimum value to the current value of `cnt`

Therefore, the new value of `cnt` is:

`cnt = cnt + min(n / 4, m // 12)`

The initial value of `cnt` is the minimum of `n / 3` and `m // 6`. After the code execution, `cnt` is updated to include the additional minimum value calculated from `n / 4` and `m // 12`.

Output State: **`n` and `m` are positive integers such that 1 <= n, m <= 2 * 10^6, `x` is 1, `y` is 3, `cnt` is the minimum of `n / 3` and `m // 6` plus the minimum of `n / 4` and `m // 12`.**