Let's break down the problem step by step:

1. **Identify the Variables in the Loop Head:**
   - The loop variable is `i`.
   - The list being iterated over is `a`.

2. **Understand the Condition for Loop Execution:**
   - The loop runs from `1` to `len(a) - 1` (since `i` starts at `1`).
   - For each iteration, the loop checks the condition `(a[i] - a[i - 1]) % 2 == 0 and y > (a[i] - a[i - 1]) // 2 - 1`.
   - If the condition is met, `tmp` is updated with `(a[i] - a[i - 1]) // 2`.
   - `ans` is incremented by `1` if `a[i] - a[i - 1] == 2`, otherwise, it is updated by adding `(a[1] - a[0]) // 2` to its current value.

3. **Current State at the End of the Previous Iteration:**
   - `a` is a sorted list of integers with at least 2 elements.
   - `i` is either `2` or remains `1`.
   - `tmp` contains one element which is the integer `(a[1] - a[0]) // 2` if the condition is met.
   - `ans` is incremented by `1` if `a[i] - a[i - 1] == 2`, otherwise, it is the original value of `ans` plus `(a[1] - a[0]) // 2`.

4. **Determine the Next State:**
   - Since `i` is either `2` or remains `1`, the next iteration will increment `i` to `2` if it was `1`.
   - We need to check the condition for `i = 2`:
     - Calculate `a[2] - a[1]`.
     - Check if `(a[2] - a[1]) % 2 == 0` and `y > (a[2] - a[1]) // 2 - 1`.
     - If the condition is met, update `tmp` with `(a[2] - a[1]) // 2`.
     - Update `ans` based on the condition `a[2] - a[1] == 2`.

5. **Adjust the States:**
   - `i` will be `2`.
   - `tmp` will be updated based on the condition.
   - `ans` will be updated based on the condition.

Given the above steps, the state at the start of the next iteration should be:

**State: **`a` is a sorted list of integers with at least 2 elements, `i` is 2, `tmp` is a list containing one element which is the integer `(a[2] - a[1]) // 2` if the condition `(a[2] - a[1]) % 2 == 0 and y > (a[2] - a[1]) // 2 - 1` is met, `ans` is incremented by `1` if `a[2] - a[1] == 2`, otherwise, it is the original value of `ans` plus `(a[1] - a[0]) // 2`**.