Let's break down the code snippet and its impact on the variables.

Given:
- `t` is an integer such that \( 1 \leq t \leq 1000 \)
- `k` and `x` are integers such that \( x > k - 3 \)
- `a` is an integer
- If `k = 2` then `z` is 1, else `z` is `k - 1`
- `i` is incremented by 1

The code snippet is:
```
z += z // (k - 1) + 1
```

Impact of the code:
- The value of `z` is updated based on the expression `z += z // (k - 1) + 1`.

Let's consider the two cases for `z`:

1. **If `k = 2`:**
   - `z` is initially 1.
   - The expression becomes `z += 1 // (2 - 1) + 1`, which simplifies to `z += 1 // 1 + 1` or `z += 1 + 1`, so `z += 2`.
   - Therefore, `z` becomes `1 + 2 = 3`.

2. **If `k > 2`:**
   - `z` is initially `k - 1`.
   - The expression becomes `z += (k - 1) // (k - 1) + 1`, which simplifies to `z += 1 + 1`, so `z += 2`.
   - Therefore, `z` becomes `(k - 1) + 2 = k + 1`.

The values of `t`, `k`, `x`, `a`, and `i` remain unchanged. `i` is incremented by 1 but since the increment operation is not shown in the provided code snippet, we will assume `i` was incremented before or after this operation, and we will just note the state of `i` as incremented.

Output State: **`t` is an integer such that \( 1 \leq t \leq 1000 \), `k` and `x` are integers such that \( x > k - 3 \), `a` is an integer, if `k = 2` then `z` is 3, else `z` is `k + 1`, `i` is incremented by 1.**