Functionality: ** The function `func_1` accepts a non-negative integer `n` and returns the value `(n * (n + 1) // 2) ** 2 - (n * (n + 1) // 2)`. This expression simplifies to `((n * (n + 1) // 2) ** 2) - (n * (n + 1) // 2)`, which is not necessarily 0. For example, when `n = 1`, the function returns `1 - 1 = 0`, but for `n = 2`, it returns `36 - 3 = 33`. The function does not always return 0; it returns a value that depends on `n`. **

**Edge Cases:**
- If `n = 0`, the function returns `0 - 0 = 0`.
- If `n = 1`, the function returns `1 - 1 = 0`.
- For any other non-negative integer `n > 1`, the function returns a non-zero value.

**Missing Functionality:**
- The annotation incorrectly states that the function always returns 0, which is not true for all values of `n`. The actual behavior is more complex and depends on the value of `n`.