Let's break down the code step by step to understand what will be printed:

1. **Input Handling**:
   - The code first reads an integer from the user input, which represents the number of test cases.
   - For each test case, it reads four non-negative integers \( p_1, p_2, p_3, p_4 \) from the user input. These integers represent the number of ones, twos, threes, and fours in the sequence, respectively.

2. **Processing Each Test Case**:
   - For each test case, the code processes the four integers using a list comprehension.
   - The list comprehension iterates over the four integers using `enumerate(map(int, input().split()))`, which pairs each integer with its index \( i \) (0 for \( p_1 \), 1 for \( p_2 \), 2 for \( p_3 \), and 3 for \( p_4 \)).
   - For each integer \( x \) at index \( i \), it calculates the expression `3 * (x // 2) + x % 2 * (i < 3)`.
     - `x // 2` gives the integer division of \( x \) by 2.
     - `3 * (x // 2)` multiplies this result by 3.
     - `x % 2` gives the remainder of \( x \) divided by 2 (0 if \( x \) is even, 1 if \( x \) is odd).
     - `x % 2 * (i < 3)` multiplies the remainder by 1 if \( i \) is less than 3 (i.e., for \( p_1, p_2, p_3 \)), and by 0 if \( i \) is 3 (i.e., for \( p_4 \)).
   - The results of these calculations are summed up.
   - The sum is then divided by 3 and converted to an integer using `// 3`.

3. **Output**:
   - The results for each test case are joined into a single string with each result on a new line using `'\n'.join(...)`.
   - This string is printed.

Given the initial state and the structure of the code, the output will be a series of integers, one for each test case, where each integer is the result of the described calculation.

Output: **[result_1]
[result_2]
...
[result_n] (where each result_i is the integer result of the calculation for the i-th test case, and n is the number of test cases)**

To provide a more precise example, let's assume the user inputs:
- Number of test cases: 2
- Test case 1: \( p_1 = 4, p_2 = 3, p_3 = 2, p_4 = 1 \)
- Test case 2: \( p_1 = 5, p_2 = 0, p_3 = 3, p_4 = 2 \)

For Test Case 1:
- \( p_1 = 4 \): \( 3 * (4 // 2) + 4 % 2 * (0 < 3) = 3 * 2 + 0 * 1 = 6 \)
- \( p_2 = 3 \): \( 3 * (3 // 2) + 3 % 2 * (1 < 3) = 3 * 1 + 1 * 1 = 4 \)
- \( p_3 = 2 \): \( 3 * (2 // 2) + 2 % 2 * (2 < 3) = 3 * 1 + 0 * 1 = 3 \)
- \( p_4 = 1 \): \( 3 * (1 // 2) + 1 % 2 * (3 < 3) = 3 * 0 + 1 * 0 = 0 \)
- Sum: \( 6 + 4 + 3 + 0 = 13 \)
- Result: \( 13 // 3 = 4 \)

For Test Case 2:
- \( p_1 = 5 \): \( 3 * (5 // 2) + 5 % 2 * (0 < 3) = 3 * 2 + 1 * 1 = 7 \)
- \( p_2 = 0 \): \( 3 * (0 // 2) + 0 % 2 * (1 < 3) = 3 * 0 + 0 * 1 = 0 \)
- \( p_3 = 3 \): \( 3 * (3 // 2) + 3 % 2 * (2 < 3) = 3 * 1 + 1 * 1 = 4 \)
- \( p_4 = 2 \): \( 3 * (2 // 2) + 2 % 2 * (3 < 3) = 3 * 1 + 0 * 0 = 3 \)
- Sum: \( 7 + 0 + 4 + 3 = 14 \)
- Result: \( 14 // 3 = 4 \)

So, the output for the given example inputs would be:
Output: **4
4**