To determine what will be printed by the `print(suma - 1)` statement, let's break down the initial state and the logic step by step:

### Initial State:
- `n` and `m` are positive integers such that \(1 \leq n, m \leq 2 \times 10^6\).
- `T` is greater than 0.
- `t` is 1.
- `info` is a list of strings obtained from splitting the new input.
- `a` is the integer value of `info[0]`.
- `b` is the integer value of `info[1]` and must be at least 1.
- `i` is `b + 1`.
- `suma` is the sum of all valid `x` values calculated during the loop where `x` is \((a - i \cdot (i - 1)) // i^2 + 1\) for each `i` from 1 to `b` inclusive, provided that `a - i * (i - 1) > 0` for each iteration.

### Step-by-Step Calculation:
1. **Initialization:**
   - `a` and `b` are derived from the `info` list.
   - `i` starts at `b + 1`.

2. **Loop Calculation:**
   - The loop iterates from `i = 1` to `i = b`.
   - For each `i`, the value of `x` is calculated as:
     \[
     x = \left( \frac{a - i \cdot (i - 1)}{i^2} \right) + 1
     \]
   - This calculation is only valid if \(a - i \cdot (i - 1) > 0\).

3. **Sum Calculation:**
   - `suma` is the sum of all valid `x` values calculated during the loop.

4. **Final Output:**
   - The `print(suma - 1)` statement will print the value of `suma` minus 1.

### Example Calculation:
Let's assume `info` is `["10", "3"]`:
- `a = 10`
- `b = 3`

For `i = 1`:
\[
x = \left( \frac{10 - 1 \cdot (1 - 1)}{1^2} \right) + 1 = \left( \frac{10 - 0}{1} \right) + 1 = 10 + 1 = 11
\]

For `i = 2`:
\[
x = \left( \frac{10 - 2 \cdot (2 - 1)}{2^2} \right) + 1 = \left( \frac{10 - 2}{4} \right) + 1 = \left( \frac{8}{4} \right) + 1 = 2 + 1 = 3
\]

For `i = 3`:
\[
x = \left( \frac{10 - 3 \cdot (3 - 1)}{3^2} \right) + 1 = \left( \frac{10 - 6}{9} \right) + 1 = \left( \frac{4}{9} \right) + 1 = 0 + 1 = 1
\]

Summing these valid `x` values:
\[
suma = 11 + 3 + 1 = 15
\]

Finally, the output of `print(suma - 1)` will be:
\[
15 - 1 = 14
\]

### Final Output:
Output: **suma - 1 (where suma is the sum of all valid x values calculated during the loop for each i from 1 to b inclusive, provided that a - i * (i - 1) > 0 for each iteration)**

In the example provided, the output would be:
Output: **14**