The code appends the tuple `(i + 1, j + 1)` to the list `ops`. Given the initial state, the values of `i` and `j` are known, so we can calculate the new tuple. 

- `i` is 1
- `j` is `m - 2`

Therefore, the new tuple becomes `(1 + 1, m - 2 + 1)` which simplifies to `(2, m - 1)`. Since the original tuple `(2, m - 1)` was already in `ops`, appending this tuple again does not change the set of elements in `ops`. 

The other variables remain unchanged.

Output State: **`i` is 1, `j` is `m - 2`, `n` is greater than or equal to 2, `m` is greater than 0, the matrix `A` has the first row and first column containing at least one '1', the list `ops` now includes the tuples `(2, m - 1)` and `(2, m - 1)`, and the condition `A[i][j] == 1 and A[i + 1][j] == 1 and (A[i][j + 1] == 1) and (A[i + 1][j + 1] == 1)` remains true.**