Let's break down the problem step by step:

1. **Initial State at the End of the Previous Iteration:**
   - `j` is 0.
   - `A` contains at least one element such that \(A[i][j] == 1\), \(A[i + 1][j] == 1\), \(A[i][j + 1] == 1\), and \(A[i + 1][j + 1] == 1\).
   - The condition for the if part is met, i.e., \(A[i][j] == 1\) or \(A[i + 1][j] == 1\) or \(A[i][j + 1] == 1\) or \(A[i + 1][j + 1] == 1\).
   - `ops` now includes the tuple \((i + 1, 1)\).

2. **For Loop Statement:**
   ```python
   for j in range(m - 1):
       # the loop body is omitted
   ```

3. **Step-by-Step Analysis:**
   - The loop iterates over `j` from 0 to \(m - 2\) (since `range(m - 1)` generates values from 0 to \(m - 2\)).
   - At the end of the previous iteration, `j` was 0.
   - For the loop to execute one more time, `j` needs to be incremented by 1.

4. **Adjusted States:**
   - `j` will be incremented from 0 to 1.
   - The conditions in the for loop statement depend on `j` being within the range \(0 \leq j < m - 1\). Since `j` is now 1, it still satisfies this condition as long as \(m > 2\).

5. **Summary of Adjusted States:**
   - `j` will be 1.
   - The conditions involving `A` and `ops` remain the same because they do not depend on `j`.

**Final State:**
State: **`j` is 1; `A` contains at least one element such that \(A[i][j] == 1\), \(A[i + 1][j] == 1\), \(A[i][j + 1] == 1\), and \(A[i + 1][j + 1] == 1\); the condition for the if part is met, i.e., \(A[i][j] == 1\) or \(A[i + 1][j] == 1\) or \(A[i][j + 1] == 1\) or \(A[i + 1][j + 1] == 1\); and `ops` now includes the tuple \((i + 1, 1)\).**