The code snippet updates the value of `cnt` based on the minimum of two expressions involving `n`, `m`, `x`, and `y`. Let's break down the calculation:

- `x` is 1
- `y` is 2
- `(x + y) * x` is `(1 + 2) * 1 = 3`
- `(x + y) * y` is `(1 + 2) * 2 = 6`
- `n / ((x + y) * x)` is `n / 3`
- `m // ((x + y) * y)` is `m // 6`

The value of `cnt` is incremented by the minimum of these two results.

Given the initial state:
- `n` and `m` are positive integers such that 1 <= n, m <= 2 * 10^6
- `x` is 1
- `y` is 2
- `cnt` is 0

The new value of `cnt` is:
- `cnt += min(n / 3, m // 6)`

Since `n` and `m` are positive integers, `n / 3` will be a floating-point number, and `m // 6` will be an integer. The `min` function will choose the smaller of these two values.

Output State: **`n` and `m` are positive integers such that 1 <= n, m <= 2 * 10^6, `x` is 1, `y` is 2, `cnt` is `min(n / 3, m // 6)`**