To solve this, let's break down the given code and its impact on the variables:

- Initial State: `n` must be at least 6, `m` must be at least 3, `x` is 2, `y` is 1, `cnt` is the sum of the minimum of `n / ((x + y) * x)` and `m // ((x + y) * y)` for all pairs `(x, y)` where `gcd(x, y) == 1` and `(x + y) * x <= n` and `(x + y) * y <= m`.

Given the current values:
- `x` is 2
- `y` is 1
- `x + y` is 3
- `(x + y) * x` is 6
- `(x + y) * y` is 3

We need to calculate the minimum of:
- `n / ((x + y) * x)` which is `n / 6`
- `m // ((x + y) * y)` which is `m // 3`

Since `n` is at least 6 and `m` is at least 3, these expressions are valid.

Let's compute the new value of `cnt`:
- `cnt` is initially the sum of the minimum of `n / 6` and `m // 3` for all valid pairs `(x, y)`.
- The new value of `cnt` is the old value plus the minimum of `n / 6` and `m // 3`.

Thus, the new value of `cnt` is:
- `cnt += min(n / 6, m // 3)`

The other variables (`n`, `m`, `x`, `y`) remain unchanged.

Output State: **`n` must be at least 6, `m` must be at least 3, `x` is 2, `y` is 1, `cnt` is the sum of the minimum of `n / 6` and `m // 3` for all pairs `(x, y)` where `gcd(x, y) == 1` and `(x + y) * x <= n` and `(x + y) * y <= m`, plus `min(n / 6, m // 3)`.**