To determine what will be printed by the `print(d2[y] - d2[x])` statement, let's break down the initial state and the relevant parts of the code:

### Initial State:
- `t` is an integer where 1 ≤ t ≤ 10^4.
- `i` is 1.
- `n` is greater than or equal to 2.
- `l` is a list of integers provided by the user input.
- `d1` is a defaultdict initialized with default factory `int` and `d1[2]` is 1.
- `d2` is a defaultdict initialized with default factory `int` and `d2[n - 1]` is 1.
- `m` is a new input integer and must be greater than 1.
- `j` is 1.
- `x` and `y` are a new pair of integers provided by the user input.
- If `y` > `x`, the condition `y` > `x` holds true.
- If `y` ≤ `x`, the condition `y` ≤ `x` holds true.

### Analysis:
- `d2` is a defaultdict with a default factory of `int`, meaning any key that is not explicitly set will have a default value of 0.
- `d2[n - 1]` is explicitly set to 1, so `d2[n - 1] = 1`.

### Print Statement:
```python
print(d2[y] - d2[x])
```

### Step-by-Step Calculation:
1. **Determine `d2[y]`**:
   - If `y == n - 1`, then `d2[y] = 1`.
   - If `y != n - 1`, then `d2[y] = 0` (since `d2` defaults to 0 for any key not explicitly set).

2. **Determine `d2[x]`**:
   - If `x == n - 1`, then `d2[x] = 1`.
   - If `x != n - 1`, then `d2[x] = 0` (since `d2` defaults to 0 for any key not explicitly set).

3. **Calculate `d2[y] - d2[x]`**:
   - If `y == n - 1` and `x == n - 1`, then `d2[y] - d2[x] = 1 - 1 = 0`.
   - If `y == n - 1` and `x != n - 1`, then `d2[y] - d2[x] = 1 - 0 = 1`.
   - If `y != n - 1` and `x == n - 1`, then `d2[y] - d2[x] = 0 - 1 = -1`.
   - If `y != n - 1` and `x != n - 1`, then `d2[y] - d2[x] = 0 - 0 = 0`.

### Conclusion:
The value printed by the `print(d2[y] - d2[x])` statement depends on the values of `y` and `x` relative to `n - 1`:
- If both `y` and `x` are equal to `n - 1`, the output is 0.
- If `y` is `n - 1` and `x` is not `n - 1`, the output is 1.
- If `y` is not `n - 1` and `x` is `n - 1`, the output is -1.
- If neither `y` nor `x` is `n - 1`, the output is 0.

Output: **d2[y] - d2[x] (where d2[y] and d2[x] are determined based on whether y and x are equal to n - 1)**