The code prints the absolute difference between `x` and `y`. Given the initial state where `x` is an input integer such that \(3 < y < x \leq 100,000\) and `y` is an input integer such that \(3 \leq y < x \leq 100,000\), we can determine that \(x\) is greater than \(y\).

Thus, the absolute difference \(abs(x - y)\) simplifies to \(x - y\). The specific values of `x` and `y` are not provided, but we know that \(x > y\).

Therefore, the output state reflects the relationship between `x` and `y` and the printed result as the absolute difference.

Output State: **`x` is an input integer such that \(3 < y < x \leq 100,000\); `y` is an input integer such that \(3 \leq y < x \leq 100,000\); printed value is \(x - y\)**