To determine what will be printed, let's break down the initial state and the print statement step by step:

### Initial State:
1. `wins` is less than `k`.
2. `win_with_swap` is defined as `wins + (k - win_with_swap)`.
3. `i` is `k - 2`.
4. If `a[i] > a[k - 1]`, the loop breaks. Otherwise, the loop completes all iterations.

### Print Statement:
```
print(max(wins - 1, win_with_swap - wins - 1 + (wins != 0)))
```

### Step-by-Step Analysis:
1. **Understanding `win_with_swap`**:
   - The formula `win_with_swap = wins + (k - win_with_swap)` is a bit tricky. Let's solve it for `win_with_swap`.
   - Rearrange the equation: `win_with_swap + win_with_swap = wins + k`
   - Simplify: `2 * win_with_swap = wins + k`
   - Therefore: `win_with_swap = (wins + k) / 2`

2. **Substitute `win_with_swap` in the print statement**:
   - The print statement is: `max(wins - 1, win_with_swap - wins - 1 + (wins != 0))`
   - Substitute `win_with_swap` with `(wins + k) / 2`:
     - `win_with_swap - wins - 1 + (wins != 0) = ((wins + k) / 2) - wins - 1 + (wins != 0)`
     - Simplify the expression:
       - `((wins + k) / 2) - wins - 1 + (wins != 0) = (wins + k - 2 * wins - 2) / 2 + (wins != 0)`
       - `= (k - wins - 2) / 2 + (wins != 0)`

3. **Evaluate the expression**:
   - The expression inside the `max` function is:
     - `wins - 1`
     - `(k - wins - 2) / 2 + (wins != 0)`
   - We need to compare these two values to determine which one is larger.

4. **Consider the condition `wins != 0`**:
   - If `wins` is 0, then `(wins != 0)` evaluates to 0.
   - If `wins` is not 0, then `(wins != 0)` evaluates to 1.

5. **Evaluate the two expressions**:
   - If `wins` is 0:
     - `wins - 1 = 0 - 1 = -1`
     - `(k - wins - 2) / 2 + (wins != 0) = (k - 0 - 2) / 2 + 0 = (k - 2) / 2`
     - The `max` function will compare `-1` and `(k - 2) / 2`.
     - Since `k` is greater than `wins` (which is 0), `(k - 2) / 2` is always greater than or equal to 0, and thus greater than `-1`.
     - Therefore, the output will be `(k - 2) / 2`.

   - If `wins` is not 0:
     - `wins - 1` is a positive integer or 0.
     - `(k - wins - 2) / 2 + 1` is the value of the second expression.
     - The `max` function will compare `wins - 1` and `(k - wins - 2) / 2 + 1`.
     - Since `k` is greater than `wins`, `(k - wins - 2) / 2` is a non-negative integer.
     - Adding 1 to `(k - wins - 2) / 2` makes it at least 1, which is always greater than or equal to `wins - 1` (since `wins` is at least 1).

### Conclusion:
- If `wins` is 0, the output will be `(k - 2) / 2`.
- If `wins` is not 0, the output will be `(k - wins - 2) / 2 + 1`.

### Final Output:
Output: **(k - wins - 2) / 2 + (wins != 0)** (where `wins` is less than `k` and `win_with_swap` is \((wins + k) / 2\))