Let's analyze the given code snippet and the initial state to determine the output state.

The code snippet is:
```python
(p2 if p1[-1] == v2 else p1).append(v1)
```

Given the initial state:
- `vx` contains 1 or 2 elements.
- `ops` contains at least two tuples with two elements.
- If `p1[-1] == v2`, then `p1` contains the same elements as `vx` and `p2` contains `v1`.
- Otherwise, `p1` contains the same elements as `vx` with `v1` appended and `p2` is an empty list.
- `v1` is the first element of the next tuple in `ops` when iterating in reverse.
- `v2` is the second element of the next tuple in `ops` when iterating in reverse.

Let's consider the two possible scenarios based on the condition `p1[-1] == v2`:

1. **If `p1[-1] == v2`:**
   - `p1` contains the same elements as `vx`.
   - `p2` contains `v1`.
   - The code will execute `p2.append(v1)`.
   - Since `p2` already contains `v1`, appending `v1` again will result in `p2` having `v1` repeated.

2. **If `p1[-1] != v2`:**
   - `p1` contains the same elements as `vx` with `v1` appended.
   - `p2` is an empty list.
   - The code will execute `p1.append(v1)`.
   - Since `p1` already contains `vx` with `v1` appended, appending `v1` again will result in `p1` having `v1` repeated at the end.

Let's formulate the output state in both scenarios:

1. **If `p1[-1] == v2`:**
   - `p1` remains the same as `vx`.
   - `p2` becomes `[v1, v1]`.

2. **If `p1[-1] != v2`:**
   - `p1` becomes `vx + [v1, v1]`.
   - `p2` remains an empty list.

Since the exact values of `vx`, `v1`, and `v2` are not provided, we'll express the output state in terms of these variables.

Output State: **If `p1[-1] == v2`, then `p1` contains the same elements as `vx` and `p2` is `[v1, v1]`. If `p1[-1] != v2`, then `p1` contains `vx + [v1, v1]` and `p2` is an empty list.**