The code assigns `next_elem - a[i] - 1` to `gap`. Given the initial state, if `i == x - 1`, `next_elem` is `a[0] + n`, otherwise, `next_elem` is `a[i + 1]`. Therefore, the value of `gap` will be:

- If `i == x - 1`, then `gap = (a[0] + n) - a[i] - 1`
- If `i != x - 1`, then `gap = a[i + 1] - a[i] - 1`

In both cases, the values of `i`, `x`, and `a` remain unchanged. Therefore, the Output State is:

Output State: **if `i == x - 1`, `next_elem` is `a[0] + n`, `gap` is `(a[0] + n) - a[i] - 1`; if `i != x - 1`, `next_elem` is `a[i + 1]`, `gap` is `a[i + 1] - a[i] - 1`; `i` is in its initial state, `x` is in its initial state, `a` is in its initial state.**