The code snippet updates the value of `next_elem` based on the condition `if i == x - 1`. However, the current state does not provide a specific value for `x`, and the value of `next_elem` depends on the value of `a` and the conditions specified. Since `x` is in its initial state and no specific value for `x` is provided, the condition `i == x - 1` cannot be evaluated directly. 

Given the initial state where `i` is 1, let's consider two cases:

1. If `x` is 1, then `i == x - 1` is `1 == 0`, which is `False`. So, `next_elem = a[i + 1] = a[2]`.
2. If `x` is not 1, then `i == x - 1` is `1 == (x - 1)`, which is `True` only if `x` is 2. In this case, `next_elem = a[0] + n`.

Since `x` is in its initial state and no specific value for `x` is given, we can't determine the exact value of `next_elem`. But we know that if `x` is 2, then `next_elem` will be `a[0] + n`, otherwise, `next_elem` will be `a[2]`.

Therefore, the output state is:
- `i` is 1,
- `x` is in its initial state (no specific value),
- `a` is in its initial state (no specific value),
- `next_elem` is either `a[0] + n` if `x` is 2, or `a[2]` if `x` is not 2.

Output State: **`i` is 1, `x` is in its initial state, `a` is in its initial state, `next_elem` is either `a[0] + n` if `x` is 2, or `a[2]` if `x` is not 2.**