The code `ans += gap` increments the value of `ans` by the current value of `gap`. Given the initial state, `ans` was already increased by `(ans + gap)` and `gap` was updated to `(gap + 2)`. The new value of `ans` will be the previous value of `ans` plus the current value of `gap`. However, the condition `if y < gap // 2` may cause a break, but since the break is not directly affecting the assignment of `ans += gap`, we can proceed with the calculation.

Let's denote the initial value of `ans` as `A` and the initial value of `gap` as `G`.

1. Initially, `ans = A` and `gap = G`.
2. After the first operation `ans += gap`, `ans` becomes `A + G`.
3. Now, `ans = A + G` and `gap = G + 2`.
4. The next line `ans += gap` means `ans` is updated to `(A + G) + (G + 2)`, which simplifies to `A + 2G + 2`.

The states of the other variables are not affected, and the condition `if y < gap // 2` does not change the value of `ans` or `gap`.

Output State: **`y` is an integer, `ans` is `A + 2G + 2`, `gap` is `G + 2`, and we do not break out of the most internal loop or if statement.**