The code snippet `ans += gap` updates the value of `ans` by adding the current value of `gap` to it. Let's analyze the possible values of `gap` and `ans` based on the initial conditions.

From the initial state:
- If `y < (G + 3) / 2`, then `y = 0` and `ans = A + G - 2`.
- Otherwise, the values of `y`, `ans`, and `gap` remain as in the precondition.

Since the value of `gap` is given as `G + 3`, it remains unchanged. Now, we need to consider both cases for `ans`:

1. If `y < (G + 3) / 2`:
   - `y = 0`
   - `ans = A + G - 2`
   - After executing `ans += gap`, `ans` becomes `(A + G - 2) + (G + 3) = A + 2G + 1`

2. Otherwise:
   - `y` remains its original value
   - `ans` remains its original value
   - After executing `ans += gap`, `ans` becomes `ans + (G + 3)`

Therefore, the output state depends on the condition `y < (G + 3) / 2`:

- If `y < (G + 3) / 2`, then `ans` is updated to `A + 2G + 1`, and `gap` is `G + 3`.
- If `y >= (G + 3) / 2`, then `ans` is updated to `ans + (G + 3)`, and `gap` is `G + 3`.

Output State: **If `y < (G + 3) / 2`, then `ans` is `A + 2G + 1` and `gap` is `G + 3`; otherwise, `ans` is `ans + (G + 3)` and `gap` is `G + 3`.**