To determine the new value of `z` after the given code snippet is executed, we need to consider the initial conditions and the operation performed on `z`.

Initial State:
- `t` is an integer such that \( 1 \leq t \leq 1000 \)
- `k` and `x` are integers such that \( x > k - 3 \)
- `a` is an integer
- If `k = 2` then `z` is 3, else `z` is `k + 1`
- `i` is incremented by 1

The code snippet is:
```python
z += z // (k - 1) + 1
```

Let's break down the operation:
- `z // (k - 1)` performs integer division of `z` by `k - 1`
- The result of this division is added to `z` along with 1

Now, let's consider the two cases for `k`:

### Case 1: `k = 2`
- If `k = 2`, then `z = 3` initially.
- The operation becomes: `z += 3 // (2 - 1) + 1`
- Simplifying: `z += 3 // 1 + 1`
- Further simplifying: `z += 3 + 1`
- Therefore, `z = 3 + 4 = 7`

### Case 2: `k \neq 2`
- If `k \neq 2`, then `z = k + 1` initially.
- The operation becomes: `z += (k + 1) // (k - 1) + 1`
- Simplifying: `z += (k + 1) // (k - 1) + 1`
- The value of `(k + 1) // (k - 1)` depends on the value of `k`:
  - For `k = 3`, `(k + 1) // (k - 1) = 4 // 2 = 2`
  - For `k > 3`, `(k + 1) // (k - 1) = 1` (since `k + 1` is just 2 more than `k - 1`, integer division will be 1)
- Therefore, for `k = 3`, `z = (3 + 1) + 2 + 1 = 7`
- For `k > 3`, `z = (k + 1) + 1 + 1 = k + 3`

Combining both cases, we can summarize the final value of `z`:
- If `k = 2`, `z` becomes 7.
- If `k > 2`, `z` becomes `k + 3`.

The other variables (`t`, `k`, `x`, `a`, `i`) remain unchanged.

Output State: **`t` is an integer such that \( 1 \leq t \leq 1000 \), `k` and `x` are integers such that \( x > k - 3 \), `a` is an integer, if `k = 2` then `z` is 7, else `z` is `k + 3`, `i` is incremented by 1.**