Let's break down the problem step by step:

1. **Identify the loop head variables**: The loop head variables are `i` and `b`.

2. **Determine the conditions for the loop to continue**:
   - The loop starts with `i = 2` and increments `i` by 1 each iteration.
   - The loop continues as long as `i <= b`.

3. **Current state at the end of the previous iteration**:
   - `t` is 0 (not relevant for the loop).
   - `info` is a list of strings obtained from splitting the input string (not directly relevant for the loop).
   - `a` is an integer equal to the first element of `info`.
   - `b` must be a positive integer.
   - `suma` is `x + 1` (not directly relevant for the loop).
   - `i` is 2.
   - `x` is \((a - 1) // 2\).
   - `x` satisfies \(((a - 1) \% 4 == 0 \text{ and } 1 \% 4 == 0)\).

4. **Adjust the state for the next iteration**:
   - Since `i` is currently 2, for the loop to continue, `i` must be incremented to 3.
   - For the loop to continue, `b` must still be a positive integer.

Given these points, the states that need to be adjusted are `i` and `b`.

**State:**
- `t` remains 0.
- `info` remains a list of strings obtained from splitting the input string.
- `a` remains an integer equal to the first element of `info`.
- `b` must still be a positive integer.
- `suma` remains `x + 1`.
- `i` is now 3.
- `x` remains \((a - 1) // 2\) and satisfies \(((a - 1) \% 4 == 0 \text{ and } 1 \% 4 == 0)\).

So, the final state is:
**`t` is 0, `info` is a list of strings obtained from splitting the input string, `a` is an integer equal to the first element of `info`, `b` must be a positive integer, `suma` is `x + 1`, `i` is 3, `x` is \((a - 1) // 2\), and `x` satisfies \(((a - 1) \% 4 == 0 \text{ and } 1 \% 4 == 0)\).**