To determine the necessary adjustments for the loop to execute, let's analyze the given code and the initial state step by step.

1. **Initial State:**
   - `n` is an integer where \(1 \leq n \leq 1000\).
   - `k` is an integer where \(0 \leq k \leq 1000\).
   - `l` is defined as \((n + k - 1) // (k * 2 + 1)\), and it is calculated before the loop.
   - `res` is an empty list.

2. **For Loop:**
   - The loop iterates over `i` using `range(l)`, meaning `i` will take values from `0` to `l-1`.

3. **Condition for Loop Execution:**
   - The loop will execute if `l` is greater than 0.
   - Therefore, we need to ensure that `l` is greater than 0 for the loop to execute.

4. **Expression for `l`:**
   - \( l = \frac{n + k - 1}{k * 2 + 1} \)
   - For \( l \) to be greater than 0, the numerator \((n + k - 1)\) must be greater than the denominator \((k * 2 + 1)\).

5. **Possible Values:**
   - Given \(1 \leq n \leq 1000\) and \(0 \leq k \leq 1000\), the minimum value for \(n + k - 1\) is 0 (when \(n = 1\) and \(k = 0\)), but since \(k * 2 + 1\) would be 1, \(l\) would be 0.
   - To ensure \(l > 0\), both \(n\) and \(k\) must be such that \(n + k - 1 > k * 2 + 1\).

6. **Simplifying the Condition:**
   - Simplify the inequality \(n + k - 1 > k * 2 + 1\):
     \[
     n + k - 1 > 2k + 1 \implies n - 1 > k + 1 \implies n > k + 2
     \]

7. **Conclusion:**
   - For the loop to execute, \(n\) must be greater than \(k + 2\).
   - Additionally, `i` will start from 0 and increment up to `l-1`, but the loop will only run if \(l > 0\).

Therefore, the states that need to be adjusted for the loop to execute are:

State: **`n` is an integer where \(1 \leq n \leq 1000\) and \(n > k + 2\), `k` is an integer where \(0 \leq k \leq 1000\), `l` is \(\frac{n + k - 1}{k * 2 + 1}\) and \(l > 0\), `res` is an empty list**.