The code snippet `tmp = asum[i + k] - asum[i]` calculates the difference between the cumulative sums at indices `i + k` and `i` in the `asum` list. Given the initial conditions, let's analyze the impact:

- `n` is an integer such that 1 ≤ n ≤ 10^5.
- `k` is an integer such that 1 ≤ k ≤ n.
- `a` is a list of integers with length `n`.
- `total` is a list of length `n + 1` where `total[i]` is the sum of all positive integers in `a[:i]` for 0 ≤ i ≤ n.
- `asum` is a list of length `n + 1` where `asum[i]` is the cumulative sum of the first `i` elements of `a` for 0 ≤ i ≤ n.
- `ans` is 0.
- `i` is 0.
- `n` must be greater than or equal to `k`.

Given `i` is 0, the expression `tmp = asum[i + k] - asum[i]` simplifies to `tmp = asum[k] - asum[0]`. Since `asum[0]` is the cumulative sum of the first 0 elements (which is 0), the expression further simplifies to `tmp = asum[k]`.

Therefore, the value of `tmp` is the cumulative sum of the first `k` elements of the list `a`.

Output State: **`n` is an integer such that 1 ≤ n ≤ 10^5, `k` is an integer such that 1 ≤ k ≤ n, `a` is a list of integers with length `n`, `total` is a list of length `n + 1` where `total[i]` is the sum of all positive integers in `a[:i]` for 0 ≤ i ≤ n, `asum` is a list of length `n + 1` where `asum[i]` is the cumulative sum of the first `i` elements of `a` for 0 ≤ i ≤ n, `ans` is 0, `i` is 0, `n` must be greater than or equal to `k`, `tmp` is `asum[k]`**.