The code snippet provided is `y = i * i`. This line updates the value of `y` to be the square of the current value of `i`. The other variables remain unchanged.

Given the initial state:
- `n` is a positive integer such that 1 <= n <= 2 * 10^6
- `m` is greater than 1
- `cnt` is `cnt + x // y + (i > 1)`
- `x` is `n - (i * i - i)`
- `y` is `i * i`
- `i` is `i + 1`

After executing `y = i * i`, the value of `y` is updated to `i * i` (which is the square of the new value of `i` since `i` was incremented by 1 in the initial state).

Output State: **`n` is a positive integer such that 1 <= n <= 2 * 10^6, `m` is greater than 1, `cnt` is `cnt + x // y + (i > 1)`, `x` is `n - (i * i - i)`, `y` is `i * i`, `i` is `i + 1`**. The value of `y` has been updated to the square of the new value of `i`.