The code snippet `n -= i * curr` modifies the value of `n`. Given the initial state, `n` is initially `n - i * (n // k)`, `i` is `1`, and `curr` is `n`. Substituting these values into the expression, we get:

\[ n_{\text{new}} = n - 1 \times n = n - n = 0 \]

Therefore, after executing the code, `n` becomes `0`. The other variables (`k`, `costs`, `h`, and `i`) remain unchanged.

Output State: **`n` is 0, `k` is a positive integer such that \(1 \leq k \leq 10^{18}\), `costs` is a list containing `[n - k + 1, 1]`, `h` is `n // k + n`, `curr` is `n`, `i` is `1`**.