Output State: **`t` is a positive integer such that 1 ≤ t ≤ 10^4; `n` is a positive integer such that 1 ≤ n ≤ 2⋅10^5; `k` is a non-negative integer such that 1 ≤ k ≤ 10^15 and its current value is `k - 2*a[l]`; `a` is a list of positive integers such that 1 ≤ a_i ≤ 10^9 for all i, and the length of `a` is equal to `n`; `l` is 0; `r` is n - 1; `sumk` is 0; the current value of `l` is equal to `r`; `a[r]` is decreased by `a[l]` (i.e., `a[r] = a[r] - a[l]`).**

Explanation: The value of `a[r]` is decreased by the value of `a[l]`. Since `l` is 0 and `r` is `n - 1`, the operation `a[r] -= a[l]` modifies `a[r]` to be `a[r] - a[l]`. All other variables remain unchanged according to the initial state and the given constraints.