The code snippet `k -= (i + 1) * (a[i + 1] - a[i])` modifies the value of `k` by subtracting `(i + 1) * (a[i + 1] - a[i])` from it. Given the initial state, `i` is 2, so the expression becomes `k -= (2 + 1) * (a[3] - a[2])` or `k -= 3 * (a[3] - a[2])`.

The other variables (`t`, `ii`, `n`, `a`, `rem`, `y`, `r`) are not modified by this line of code.

Output State: **`t` is an integer such that 1 <= t <= 100, `ii` is 0, `n` is the first integer from the input and must be greater than 1, `a` is a sorted list of integers obtained from the input, `rem` is 0, `y` is either 0 or `n - 2`, `i` is 2, and `k` is decreased by `3 * (a[3] - a[2])`.**