To determine the output state, we need to evaluate the expression `k -= (i + 1) * (a[i + 1] - a[i])` based on the given initial state.

Given:
- `t` is an integer such that 1 <= t <= 100
- `ii` is 1
- `n` is at least 4
- `a` is a sorted list of integers
- `i` is 3

The expression `k -= (i + 1) * (a[i + 1] - a[i])` modifies the value of `k` by subtracting `(i + 1) * (a[i + 1] - a[i])` from it. Since `i` is 3, the expression becomes `k -= 4 * (a[4] - a[3])`.

Let's denote the value of `k` before the operation as `k_initial`. After the operation, the value of `k` will be `k_initial - 4 * (a[4] - a[3])`.

The values of `t`, `ii`, `n`, `a`, and `i` remain unchanged.

Therefore, the Output State is:
Output State: **`t` is an integer such that 1 <= t <= 100, `ii` is 1, `n` is at least 4, `a` is a sorted list of integers, `i` is 3, `k` is `k_initial - 4 * (a[4] - a[3])`**.