The code snippet appends the value `i * (k * 2 + 1) + 1` to the list `res`. From the initial state, we know:

- `n` is an integer where \(1 \leq n \leq 1000\) and \(n > k + 2\).
- `k` is an integer where \(0 \leq k \leq 1000\).
- \(l = \frac{n + k - 1}{k * 2 + 1}\) and \(l > 0\).
- `res` is a list containing \([i * (k * 2 + 1) + 1, n + k]\).
- `i` is \(i_max + 1\).

After executing the line `res.append(i * (k * 2 + 1) + 1)`:

- The list `res` will now contain three elements: the original first element, the second element, and the new element `i * (k * 2 + 1) + 1`.
- The value of `i` remains unchanged.

Therefore, the updated state of the variables is:

- `n` is an integer where \(1 \leq n \leq 1000\) and \(n > k + 2\).
- `k` is an integer where \(0 \leq k \leq 1000\).
- \(l = \frac{n + k - 1}{k * 2 + 1}\) and \(l > 0\).
- `res` is a list containing \([i * (k * 2 + 1) + 1, n + k, i * (k * 2 + 1) + 1]\).
- `i` is \(i_max + 1\).

Output State: **`n` is an integer where \(1 \leq n \leq 1000\) and \(n > k + 2\); `k` is an integer where \(0 \leq k \leq 1000\); \(l = \frac{n + k - 1}{k * 2 + 1}\) and \(l > 0\); `res` is a list containing \([i * (k * 2 + 1) + 1, n + k, i * (k * 2 + 1) + 1]\); `i` is \(i_max + 1\)**.