Let's carefully analyze the given program and the annotated version to determine if the program correctly constructs the permutation \( p \) based on the array \( a \).

### Problem Recap:
Farmer John has a permutation \( p \) of length \( n \) and an array \( a \) of length \( n \) where \( a_i = \texttt{MEX}(p_1, p_2, \ldots, p_i) - p_i \). The task is to construct the permutation \( p \) from the array \( a \).

### Program Analysis:
The program reads multiple test cases and for each test case:
1. It reads \( n \) (the length of the permutation).
2. It reads the array \( a \).
3. It initializes the permutation array \( p \) with -1.
4. It sets the initial MEX value to \( n \).
5. It iterates over the array \( a \) in reverse order:
   - For each element \( a[i] \), it calculates \( p[i] = \text{MEX} - a[i] \).
   - It updates the MEX value to be the minimum of the current MEX and \( p[i] \).
6. It prints the constructed permutation \( p \).

### Annotated Code Analysis:
The annotations suggest that the state of the program is correctly tracked, but let's verify if the approach is logically sound.

### Key Points to Verify:
1. **Initialization of MEX**: The initial MEX value is set to \( n \), which is correct because the MEX of an empty array is 0, and as elements are added, the MEX can only increase.
2. **Reverse Iteration**: The program iterates over the array \( a \) in reverse order to ensure that the MEX value is correctly updated based on the elements of \( p \) that have already been calculated.
3. **Calculation of \( p[i] \)**: The formula \( p[i] = \text{MEX} - a[i] \) is used to calculate each element of \( p \). This is derived from the definition \( a_i = \texttt{MEX}(p_1, p_2, \ldots, p_i) - p_i \), so rearranging gives \( p[i] = \texttt{MEX}(p_1, p_2, \ldots, p_i) - a_i \).

### Verification with Example:
Let's verify the program with the first example from the problem statement:

**Input:**
```
3
5
1 1 -2 1 2
5
1 1 1 1 1
3
-2 1 2
```

**Output:**
```
0 1 4 2 3 
0 1 2 3 4 
2 0 1 
```

Let's manually verify the first test case:

- For \( n = 5 \) and \( a = [1, 1, -2, 1, 2] \):
  - Initialize \( p = [-1, -1, -1, -1, -1] \) and \( \text{MEX} = 5 \).
  - Iterate in reverse:
    - \( i = 4 \): \( p[4] = 5 - 2 = 3 \), update \( \text{MEX} = \min(5, 3) = 3 \).
    - \( i = 3 \): \( p[3] = 3 - 1 = 2 \), update \( \text{MEX} = \min(3, 2) = 2 \).
    - \( i = 2 \): \( p[2] = 2 - (-2) = 4 \), update \( \text{MEX} = \min(2, 4) = 2 \).
    - \( i = 1 \): \( p[1] = 2 - 1 = 1 \), update \( \text{MEX} = \min(2, 1) = 1 \).
    - \( i = 0 \): \( p[0] = 1 - 1 = 0 \), update \( \text{MEX} = \min(1, 0) = 0 \).
  - Result: \( p = [0, 1, 4, 2, 3] \).

The constructed permutation \( p \) satisfies the given array \( a \).

### Conclusion:
The program correctly constructs the permutation \( p \) based on the array \( a \) using the given approach. The reverse iteration and the calculation of \( p[i] \) are logically sound.

Final: **True**