### Reasoning

The original assessment correctly identifies that the provided code does not accurately implement the logic required to solve the problem. Let's analyze the code step-by-step to understand why it fails and how we can improve it.

#### Analysis of the Given Code

1. **Input Handling**:
   - The code reads the number of test cases `T` and processes each test case individually.
   - For each test case, it reads two integers `a` and `b`.

2. **Formula Used**:
   - The code uses the formula `x = (a - i * (i - 1)) // i ** 2 + 1` to calculate `x`.
   - This formula is intended to count the number of valid pairs `(a, b)` but seems to be incorrect based on the problem statement and manual checks.

3. **Loop Logic**:
   - The outer loop runs from `1` to `b`.
   - The inner logic calculates `x` and adds it to `suma` if `a - i * (i - 1) > 0`.

#### Manual Check Example

Let's manually check the pairs for `n = 10` and `m = 8`:

1. **Valid Pairs**:
   - For \(a = 1\) and \(b = 1\):
     - \(a + b = 2\)
     - \(b \cdot \gcd(a, b) = 1 \cdot 1 = 1\)
     - \(2 \mod 1 = 0\), so \((1, 1)\) is valid.
   
   - For \(a = 2\) and \(b = 1\):
     - \(a + b = 3\)
     - \(b \cdot \gcd(a, b) = 1 \cdot 1 = 1\)
     - \(3 \mod 1 = 0\), so \((2, 1)\) is valid.
   
   - For \(a = 2\) and \(b = 2\):
     - \(a + b = 4\)
     - \(b \cdot \gcd(a, b) = 2 \cdot 2 = 4\)
     - \(4 \mod 4 = 0\), so \((2, 2)\) is valid.
   
   - For \(a = 3\) and \(b = 1\):
     - \(a + b = 4\)
     - \(b \cdot \gcd(a, b) = 1 \cdot 1 = 1\)
     - \(4 \mod 1 = 0\), so \((3, 1)\) is valid.
   
   - For \(a = 4\) and \(b = 1\):
     - \(a + b = 5\)
     - \(b \cdot \gcd(a, b) = 1 \cdot 1 = 1\)
     - \(5 \mod 1 = 0\), so \((4, 1)\) is valid.
   
   - For \(a = 5\) and \(b = 1\):
     - \(a + b = 6\)
     - \(b \cdot \gcd(a, b) = 1 \cdot 1 = 1\)
     - \(6 \mod 1 = 0\), so \((5, 1)\) is valid.
   
   - For \(a = 6\) and \(b = 1\):
     - \(a + b = 7\)
     - \(b \cdot \gcd(a, b) = 1 \cdot 1 = 1\)
     - \(7 \mod 1 = 0\), so \((6, 1)\) is valid.
   
   - For \(a = 6\) and \(b = 2\):
     - \(a + b = 8\)
     - \(b \cdot \gcd(a, b) = 2 \cdot 2 = 4\)
     - \(8 \mod 4 = 0\), so \((6, 2)\) is valid.
   
   - For \(a = 6\) and \(b = 3\):
     - \(a + b = 9\)
     - \(b \cdot \gcd(a, b) = 3 \cdot 3 = 9\)
     - \(9 \mod 9 = 0\), so \((6, 3)\) is valid.
   
   - For \(a = 7\) and \(b = 1\):
     - \(a + b = 8\)
     - \(b \cdot \gcd(a, b) = 1 \cdot 1 = 1\)
     - \(8 \mod 1 = 0\), so \((7, 1)\) is valid.
   
   - For \(a = 8\) and \(b = 1\):
     - \(a + b = 9\)
     - \(b \cdot \gcd(a, b) = 1 \cdot 1 = 1\)
     - \(9 \mod 1 = 0\), so \((8, 1)\) is valid.
   
   - For \(a = 9\) and \(b = 1\):
     - \(a + b = 10\)
     - \(b \cdot \gcd(a, b) = 1 \cdot 1 = 1\)
     - \(10 \mod 1 = 0\), so \((9, 1)\) is valid.
   
   - For \(a = 10\) and \(b = 1\):
     - \(a + b = 11\)
     - \(b \cdot \gcd(a, b) = 1 \cdot 1 = 1\)
     - \(11 \mod 1 = 0\), so \((10, 1)\) is valid.
   
   - For \(a = 10\) and \(b = 2\):
     - \(a + b = 12\)
     - \(b \cdot \gcd(a, b) = 2 \cdot 2 = 4\)
     - \(12 \mod 4 = 0\), so \((10, 2)\) is valid.

This results in 14 valid pairs, which matches the expected output.

#### Correct Implementation

The formula used in the original code is incorrect. Instead, we should iterate over all possible pairs \((a, b)\) and check if they satisfy the condition directly.

Here is the corrected implementation:

```python
import math

def func():
    T = int(input())
    for t in range(T):
        info = input().split()
        a, b = int(info[0]), int(info[1])
        suma = 0
        for i in range(1, a + 1):
            for j in range(1, b + 1):
                if (i + j) % (j * math.gcd(i, j)) == 0:
                    suma += 1
        print(suma)

func()
```

### Final Evaluation

The original assessment was accurate. The provided code does not correctly implement the logic required to solve the problem. The corrected implementation iterates over all possible pairs and checks the condition directly, ensuring correctness.

**Final: False**