Let's break down the problem step by step:

1. **Initial State:**
   - `p1`, `p2`, and `p3` are integers provided by the user such that \(0 \leq p1 \leq p2 \leq p3 \leq 30\).
   - `t` is greater than 1 (though `t` is not used in the print statement).
   - `_` is 1 (though `_` is not used in the print statement).
   - `low` is the minimum of `p3 - p1` and `p3 - p2`.
   - `high` is the maximum of `p3 - p1` and `p3 - p2`.
   - `cur` is equal to `low + 1`.

2. **Determine the values of `low` and `high`:**
   - Since \(p1 \leq p2 \leq p3\), the differences `p3 - p1` and `p3 - p2` will be non-negative.
   - `p3 - p1` will always be greater than or equal to `p3 - p2` because \(p1 \leq p2\).
   - Therefore, `low` will be `p3 - p2` and `high` will be `p3 - p1`.

3. **Calculate the value of `cur`:**
   - `cur` is `low + 1`, which means `cur` is `p3 - p2 + 1`.

4. **Evaluate the expression in the print statement:**
   - The expression is `p1 - cur + p3`.
   - Substitute `cur` with `p3 - p2 + 1`:
     \[
     p1 - (p3 - p2 + 1) + p3
     \]
   - Simplify the expression:
     \[
     p1 - p3 + p2 - 1 + p3
     \]
   - The `p3` terms cancel out:
     \[
     p1 + p2 - 1
     \]

5. **Final Output:**
   - The print statement will output the value of `p1 + p2 - 1`.

Output: **p1 + p2 - 1 (where p1 and p2 are integers provided by the user such that 0 <= p1 <= p2 <= p3 <= 30)**