In the provided code snippet, the statement `dp[i][j] = dp[i][j - 1]` assigns the value of `dp[i][j - 1]` to `dp[i][j]`. 

The initial state indicates:
- `n` is an integer (1 ≤ n ≤ 45)
- `k` is greater than or equal to 2
- `M` is at least 1
- `t` is a sorted list of `k` integers
- `j` is 1
- `i` is k + 1

The update will result in the variable `j` remaining 1, while `i` is `k + 1`. Hence, `dp[i][j]` will be updated based on `dp[i][j - 1]`, which refers to `dp[i][0]` because `j - 1` is 0.

Therefore, the updated value will be `dp[k + 1][1] = dp[k + 1][0]`.

The states of the other variables remain unchanged.

Output State: **`n` is an integer (1 ≤ n ≤ 45), `k` is greater than or equal to 2, `M` is at least 1, `t` is a sorted list of `k` integers, `j` is 1, `i` is k + 1, `dp[k + 1][1] = dp[k + 1][0]`**.