The code `a, b = b, a % b` simultaneously updates the values of `a` and `b`. 
Initially, `a` is the original `b`, and `b` is the remainder of the original `a` divided by the original `b`. 
After execution, `a` becomes the original `b` (which is the new value of `a`), and `b` becomes the remainder of the new `a` (which is the original `b`) divided by the new `b` (which is the original `a` modulo the original `b`).

Let's denote the original `a` as `orig_a` and the original `b` as `orig_b`. 
Initially, `a = orig_b` and `b = orig_a % orig_b`.

After the update, `a = b = orig_b` and `b = a % b = orig_b % (orig_a % orig_b)`.

So, `a` becomes `orig_b` and `b` becomes `orig_b % (orig_a % orig_b)`.

Output State: **`a` is the original `b`, `b` is the remainder of the original `b` divided by the remainder of the original `a` divided by the original `b`**.