To determine the output state after the loop executes all the iterations, we need to carefully analyze the given initial state and the loop code. Let's break down the steps to understand how the variables evolve during the loop execution.

### Initial State Recap:
- `s`: remains unchanged (not specified, so we assume it's a string)
- `n`: remains unchanged (not specified, so we assume it's the length of `s`)
- `A`: contains cumulative values based on the positions of '>' characters
- `idx_A`: contains the indices of '>' characters
- `B = [0, 2]`
- `idx_B = [4, 2]`
- `l = 0`
- `r = 2`

### Loop Analysis:
The loop iterates over the string `s` from index `0` to `n-1`. Depending on whether the current character is `'>'` or not, different calculations are performed, and `l` and `r` are adjusted accordingly.

### Steps to Determine the Output State:
1. **Initialization**:
   - `l = 0`
   - `r = 2`
   
2. **Loop Execution**:
   - We need to simulate the loop for each character in `s` and update `l` and `r` based on the conditions.
   - We need to track the values of `A` and `B` as they are used in the calculations.

### Example Simulation (Assuming `s = ">>><<>"` and `n = 6`):

#### Iteration 1 (i = 0, s[0] = '>'):
- `l < r` (0 < 2)
- Calculate `a`, `x`, `b`:
  - `a = A[0]`
  - `x = 2 - (0 + 2) = 0`
  - `b = B[1] = 2`
  - Since `x >= 0`:
    - `b = 2 - B[0] = 2 - 0 = 2`
    - `b = 2 - (idx_B[0] - idx_B[1]) * (0 + 1) = 2 - (4 - 2) * 1 = 0`
  - `b = 0 + (idx_B[1] - 0) * (0 + 1) = 2`
  - Print `a * 2 + b * 2 + 0 + 1 = 2 * 2 + 2 * 2 + 1 = 9`
- `l += 1` (l = 1)

#### Iteration 2 (i = 1, s[1] = '>'):
- `l < r` (1 < 2)
- Calculate `a`, `x`, `b`:
  - `a = A[1]`
  - `x = 2 - (1 + 2) = -1`
  - `b = B[1] = 2`
  - Since `x < 0`:
    - `b = 2 + (idx_B[1] - 1) * (1 + 1) = 2 + (2 - 1) * 2 = 4`
  - Print `a * 2 + b * 2 + 1 + 1 = 2 * 2 + 4 * 2 + 2 = 14`
- `l += 1` (l = 2)

#### Iteration 3 (i = 2, s[2] = '>'):
- `l == r` (2 == 2)
- Calculate `a`, `b`:
  - `a = B[1] + (idx_B[1] - 2) * 2 = 2 + (2 - 2) * 2 = 2`
  - `b = A[1]`
  - Since `l - r == 0`:
    - `b = b + (2 - idx_A[1]) * 2`
  - Print `a * 2 + b * 2 + (6 - 2) = 2 * 2 + 2 * 2 + 4 = 16`
- `l += 1` (l = 3)

#### Iteration 4 (i = 3, s[3] = '<'):
- `r -= 1` (r = 1)
- `l > r` (3 > 1)
- Calculate `a`, `b`:
  - `a = B[0] + (idx_B[0] - 3) * 1 = 0 + (4 - 3) * 1 = 1`
  - `b = A[2]`
  - Since `l - r - 1 > 0`:
    - `b = b - A[0] - (idx_A[2] - idx_A[0]) * (l - r - 1)`
  - Print `a * 2 + b * 2 + (6 - 3) = 1 * 2 + 2 * 2 + 3 = 9`
- `r -= 1` (r = 0)

#### Iteration 5 (i = 4, s[4] = '<'):
- `r == 0`
- Print `6 - 4 = 2`

#### Iteration 6 (i = 5, s[5] = '>'):
- `l < r` (3 < 0) is false, so we check `l == r` (3 == 0) is false, so we check `l > r` (3 > 0) is true
- Calculate `a`, `b`:
  - `a = B[0] + (idx_B[0] - 5) * 0 = 0 + (4 - 5) * 0 = 0`
  - `b = A[2]`
  - Since `l - r - 1 > 0`:
    - `b = b - A[0] - (idx_A[2] - idx_A[0]) * (l - r - 1)`
  - Print `a * 2 + b * 2 + (6 - 5) = 0 * 2 + 2 * 2 + 1 = 5`

### Output State:
After the loop completes, the values of `l` and `r` will be:
- `l = 3`
- `r = 0`

The other variables (`s`, `n`, `A`, `idx_A`, `B`, `idx_B`) remain unchanged.

Output State: **`s` remains unchanged; `n` remains unchanged; `A` contains the cumulative values calculated based on the positions of '>' characters; `idx_A` contains the indices of '>' characters; `B = [0, 2]`; `idx_B = [4, 2]`; `l = 3`; `r = 0`.**