Let's break down the problem step by step:

1. **Initial Values:**
   - `m = 16`
   - `_ = 1`
   - `n = 0`
   - `k > 1`
   - `n_back = 1`
   - `s = 1`

2. **Loop Condition:**
   - The loop continues as long as `s < k`.

3. **Loop Execution:**
   - Each iteration of the loop updates `m` to `2 * m` and `n` to `n / 2`.
   - After 4 iterations, `m` becomes 16 and `n` becomes 0.
   - The loop terminates because `n` becomes 0, making `s` no longer less than `k`.

4. **Final Values:**
   - `m = 16`
   - `_ = 1`
   - `n = 0`
   - `k > 1`
   - `n_back = 1`
   - `s = 1`

5. **Expression to Evaluate:**
   - The expression to evaluate is `(2 * (k - (s - n)) - 1) * m`.

6. **Substitute Known Values:**
   - Since `n = 0`, the expression simplifies to `(2 * (k - (1 - 0)) - 1) * 16`.
   - This further simplifies to `(2 * (k - 1) - 1) * 16`.

7. **Evaluate the Expression:**
   - Let's denote `k - 1` as `k_prime` (since `k > 1`, `k_prime` is a positive integer).
   - The expression then becomes `(2 * k_prime - 1) * 16`.
   - Since `k` is greater than 1 but we don't know the exact value, we can represent it as `k_prime + 1`.

8. **Final Output:**
   - The expression evaluates to `(2 * (k - 1) - 1) * 16 = (2 * k_prime - 1) * 16`.
   - Since `k` is greater than 1, let's assume the smallest possible value for `k` which is 2 (since `k > 1` and we need a concrete example):
     - If `k = 2`, then `k - 1 = 1`, so the expression becomes `(2 * 1 - 1) * 16 = 1 * 16 = 16`.

Therefore, the output of the print statement is:

Output: **16**