Based on the initial state provided:

- `m` is 16
- `_` is 0
- `n` is 0
- `k` is greater than 1
- `s` is 0
- `n_back` is equal to 1

We need to evaluate the expression `(2 * (k - (s - n)) - 1) * m`.

Given:
- `m` is 16
- `n` is 0
- `s` is 0

Substituting these values into the expression:
\[ (2 * (k - (0 - 0)) - 1) * 16 \]
\[ = (2 * (k - 0) - 1) * 16 \]
\[ = (2 * k - 1) * 16 \]

Since `k` is greater than 1, let's assume the smallest possible value for `k` which is 2 (since it must be greater than 1).

So, substituting `k = 2`:
\[ (2 * 2 - 1) * 16 \]
\[ = (4 - 1) * 16 \]
\[ = 3 * 16 \]
\[ = 48 \]

Therefore, the output of the print statement is:
Output: **48**