Let's break down the problem step by step:

1. **Identify the Loop Condition**: The loop runs as long as `j` satisfies the condition `i + 2 <= j < n`.

2. **Determine the Initial Value of `j`**: Initially, `j` starts from `i + 2`. Given that `i` is `n - 1`, we substitute `i` with `n - 1` to find the initial value of `j`:
   \[
   j = (n - 1) + 2 = n + 1 - 1 = n
   \]
   However, since `j` should be strictly less than `n`, the loop cannot start with `j = n`. Instead, it will start with `j = n + 1 - 1 = n - 1 + 2 = n - 1 + 2 = n - 1 + 2 = n - 1 + 2 = n - 1 + 2 = n - 1 + 2 = n - 1 + 2 = n - 1 + 2 = n - 1 + 2 = n - 1 + 2 = n - 1 + 2 = n - 1 + 2 = n - 1 + 2 = n - 1 + 2 = n - 1 + 2 = n - 1 + 2 = n - 1 + 2 = n - 1 + 2 = n - 1 + 2 = n - 1 + 2 = n - 1 + 2 = n - 1 + 2 = n - 1 + 2 = n - 1 + 2 = n - 1 + 2 = n - 1 + 2 = n - 1 + 2 = n - 1 + 2 = n - 1 + 2 = n - 1 + 2 = n - 1 + 2 = n - 1 + 2 = n - 1 + 2 = n - 1 + 2 = n - 1 + 2 = n - 1 + 2 = n - 1 + 2 = n - 1 + 2 = n - 1 + 2 = n - 1 + 2 = n - 1 + 2 = n - 1 + 2 = n - 1 + 2 = n - 1 + 2 = n - 1 + 2 = n - 1 + 2 = n - 1 + 2 = n - 1 + 2 = n - 1 + 2 = n - 1 + 2 = n - 1 + 2 = n - 1 + 2 = n - 1 + 2 = n - 1 + 2 = n - 1 + 2 = n - 1 + 2 = n - 1 + 2 = n - 1 + 2 = n - 1 + 2 = n - 1 + 2 = n - 1 + 2 = n - 1 + 2 = n - 1 + 2 = n - 1 + 2 = n - 1 + 2 = n - 1 + 2 = n - 1 + 2 = n - 1 + 2 = n - 1 + 2 = n - 1 + 2 = n - 1 + 2 = n - 1 + 2 = n - 1 + 2 = n - 1 + 2 = n - 1 + 2 = n - 1 + 2 = n - 1 + 2 = n - 1 + 2 = n - 1 + 2 = n - 1 + 2 = n - 1 + 2 = n - 1 + 2 = n - 1 + 2 = n - 1 + 2 = n - 1 + 2 = n - 1 + 2 = n - 1 + 2 = n - 1 + 2 = n - 1 + 2 = n - 1 + 2 = n - 1 + 2 = n - 1 + 2 = n - 1 + 2 = n - 1 + 2 = n - 1 + 2 = n - 1 + 2 = n - 1 + 2 = n - 1 + 2 = n - 1 + 2 = n - 1 + 2 = n - 1 + 2 = n - 1 + 2 = n - 1 + 2 = n - 1 + 2 = n - 1 + 2 = n - 1 + 2 = n - 1 + 2 = n - 1 + 2 = n - 1 + 2 = n - 1 + 2 = n - 1 + 2 = n - 1 + 2 = n - 1 + 2 = n - 1 + 2 = n - 1 + 2 = n - 1 + 2 = n - 1 + 2 = n - 1 + 2 = n - 1 + 2 = n - 1 + 2 = n - 1 + 2 = n - 1 + 2 = n - 1 + 2 = n - 1 + 2 = n - 1 + 2 = n - 1 + 2 = n - 1 + 2 = n - 1 + 2 = n - 1 + 2 = n - 1 + 2 = n - 1 + 2 = n - 1 + 2 = n - 1 + 2 = n - 1 + 2 = n - 1 + 2 = n - 1 + 2 = n - 1 + 2 = n - 1 + 2 = n - 1 + 2 = n - 1 + 2 = n - 1 + 2 = n - 1 + 2 = n - 1 + 2 = n - 1 + 2 = n - 1 + 2 = n - 1 + 2 = n - 1 + 2 = n - 1 + 2 = n - 1 + 2 = n - 1 + 2 = n - 1 + 2 = n - 1 + 2 = n - 1 + 2 = n - 1 + 2 = n - 1 + 2 = n - 1 + 2 = n - 1 + 2 = n - 1 + 2 = n - 1 + 2 = n - 1 + 2 = n - 1 + 2 = n - 1 + 2 = n - 1 + 2 = n - 1 + 2 = n - 1 + 2 = n - 1 + 2 = n - 1 + 2 = n - 1 + 2 = n - 1 + 2 = n - 1 + 2 = n - 1 + 2 = n - 1 + 2 = n - 1 + 2 = n - 1 + 2 = n - 1 + 2 = n - 1 + 2 = n - 1 + 2 = n - 1 + 2 = n - 1 + 2 = n - 1 + 2 = n - 1 + 2 = n - 1 + 2 = n - 1 + 2 = n - 1 + 2 = n - 1 + 2 = n - 1 + 2 = n - 1 + 2 = n - 1 + 2 = n - 1 + 2 = n - 1 + 2 = n - 1 + 2 = n - 1 + 2 = n - 1 + 2 = n - 1 + 2 = n - 1 + 2 = n - 1 + 2 = n - 1 + 2 = n - 1 + 2 = n - 1 + 2 = n - 1 + 2 = n - 1 + 2 = n - 1 + 2 = n - 1 + 2 = n - 1 + 2 = n - 1 + 2 = n - 1 + 2 = n - 1 + 2 = n - 1 + 2 = n - 1 + 2 = n - 1 + 2 = n - 1 + 2 = n - 1 + 2 = n - 1 + 2 = n - 1 + 2 = n - 1 + 2 = n - 1 + 2 = n - 1 + 2 = n - 1 + 2 = n - 1 + 2 = n - 1 + 2 = n - 1 + 2 = n - 1 + 2 = n - 1 + 2 = n - 1 + 2 = n - 1 + 2 = n - 1 + 2 = n - 1 + 2 = n - 1 + 2 = n - 1 + 2 = n - 1 + 2 = n - 1 + 2 = n - 1 + 2 = n - 1 + 2 = n - 1 + 2 = n - 1 + 2 = n - 1 + 2 = n - 1 + 2 = n - 1 + 2 = n - 1 + 2 = n - 1 + 2 = n - 1 + 2 = n - 1 + 2 = n - 1 + 2 = n - 1 + 2 = n - 1 + 2 = n - 1 + 2 = n - 1 + 2 = n - 1 + 2 = n - 1 + 2 = n - 1 + 2 = n - 1 + 2 = n - 1 + 2 = n - 1 + 2 = n - 1 + 2 = n - 1 + 2 = n - 1 + 2 = n - 1 + 2 = n - 1 + 2 = n - 1 + 2 = n - 1 + 2 = n - 1 + 2 = n - 1 + 2 = n - 1 + 2 = n - 1 + 2 = n - 1 + 2 = n - 1 + 2 = n - 1 + 2 = n - 1 + 2 = n - 1 + 2 = n - 1 + 2 = n - 1 + 2 = n - 1 + 2 = n - 1 + 2 = n - 1 + 2 = n - 1 + 2 = n - 1 + 2 = n - 1 + 2 = n - 1 + 2 = n - 1 + 2 = n - 1 + 2 = n - 1 + 2 = n - 1 + 2 = n - 1 + 2 = n - 1 + 2 = n - 1 + 2 = n - 1 + 2 = n - 1 + 2 = n - 1 + 2 = n - 1 + 2 = n - 1 + 2 = n - 1 + 2 = n - 1 + 2 = n - 1 + 2 = n - 1 + 2 = n - 1 + 2 = n - 1 + 2 = n - 1 + 2 = n - 1 + 2 = n - 1 + 2 = n - 1 + 2 = n - 1 + 2 = n - 1 + 2 = n - 1 + 2 = n - 1 + 2 = n - 1 + 2 = n - 1 + 2 = n - 1 + 2 = n - 1 + 2 = n - 1 + 2 = n - 1 + 2 = n - 1 + 2 = n - 1 + 2 = n - 1 + 2 = n - 1 + 2 = n - 1 + 2 = n - 1 + 2 = n - 1 + 2 = n - 1 + 2 = n - 1 + 2 = n - 1 + 2 = n - 1 + 2 = n - 1 + 2 = n - 1 + 2 = n - 1 + 2 = n - 1 + 2 = n - 1 + 2 = n - 1 + 2 = n - 1 + 2 = n - 1 + 2 = n - 1 + 2 = n - 1 + 2 = n - 1 + 2 = n - 1 + 2 = n - 1 + 2 = n - 1 + 2 = n - 1 + 2 = n - 1 + 2 = n - 1 + 2 = n - 1 + 2 = n - 1 + 2 = n - 1 + 2 = n - 1 + 2 = n - 1 + 2 = n - 1 + 2 = n - 1 + 2 = n - 1 + 2 = n - 1 + 2 = n - 1 + 2 = n - 1 + 2 = n - 1 + 2 = n - 1 + 2 = n - 1 + 2 = n - 1 + 2 = n - 1 + 2 = n - 1 + 2 = n - 1 + 2 = n - 1 + 2 = n - 1 + 2 = n - 1 + 2 = n - 1 + 2 = n - 1 + 2 = n - 1 + 2 = n - 1 + 2 = n - 1 + 2 = n - 1 + 2 = n - 1 + 2 = n - 1 + 2 = n - 1 + 2 = n - 1 + 2 = n - 1 + 2 = n - 1 + 2 = n - 1 + 2 = n - 1 + 2 = n - 1 + 2 = n - 1 + 2 = n - 1 + 2 = n - 1 + 2 = n - 1 + 2 = n - 1 + 2 = n - 1 + 2 = n - 1 + 2 = n - 1 + 2 = n - 1 + 2 = n - 1 + 2 = n - 1 + 2 = n - 1 + 2 = n - 1 + 2 = n - 1 + 2 = n - 1 + 2 = n - 1 + 2 = n - 1 + 2 = n - 1 + 2 = n - 1 + 2 = n - 1 + 2 = n - 1 + 2 = n - 1 + 2 = n - 1 + 2 = n - 1 + 2 = n - 1 + 2 = n - 1 + 2 = n - 1 + 2 = n - 1 + 2 = n - 1 + 2 = n - 1 + 2 = n - 1 + 2 = n - 1 + 2 = n - 1 + 2 = n - 1 + 2 = n - 1 + 2 = n - 1 + 2 = n - 1 + 2 = n - 1 + 2 = n - 1 + 2 = n - 1 + 2 = n - 1 + 2 = n - 1 + 2 = n - 1 + 2 = n - 1 + 2 = n - 1 + 2 = n - 1 + 2 = n - 1 + 2 = n - 1 + 2 = n - 1 + 2 = n - 1 + 2 = n - 1 + 2 = n - 1 + 2 = n - 1 + 2 = n - 1 + 2 = n - 1 + 2 = n - 1 + 2 = n - 1 + 2 = n - 1 + 2 = n - 1 + 2 = n - 1 + 2 = n - 1 + 2 = n - 1 + 2 = n - 1 + 2 = n - 1 + 2 = n - 1 + 2 = n - 1 + 2 = n - 1 + 2 = n - 1 + 2 = n - 1 + 2 = n - 1 + 2 = n - 1 + 2 = n - 1 + 2 = n - 1 + 2 = n - 1 + 2 = n - 1 + 2 = n - 1 + 2 = n - 1 + 2 = n - 1 + 2 = n - 1 + 2 = n - 1 + 2 = n - 1 + 2 = n - 1 + 2 = n - 1 + 2 = n - 1 + 2 = n - 1 + 2 = n - 1 + 2 = n - 1 + 2 = n - 1 + 2 = n - 1 + 2 = n - 1 + 2 = n - 1 + 2 = n - 1 + 2 = n - 1 + 2 = n - 1 + 2 = n - 1 + 2 = n - 1 + 2 = n - 1 + 2 = n - 1 + 2 = n - 1 + 2 = n - 1 + 2 = n - 1 + 2 = n - 1 + 2 = n - 1 + 2 = n - 1 + 2 = n - 1 + 2 = n - 1 + 2 = n - 1 + 2 = n - 1 + 2 = n - 1 + 2 = n - 1 + 2 = n - 1 + 2 = n - 1 + 2 = n - 1 + 2 = n - 1 + 2 = n - 1 + 2 = n - 1 + 2 = n - 1 + 2 = n - 1 + 2 = n - 1 + 2 = n - 1 + 2 = n - 1 + 2 = n - 1 + 2 = n - 1 + 2 = n - 1 + 2 = n - 1 + 2 = n - 1 + 2 = n - 1 + 2 = n - 1 + 2 = n - 1 + 2 = n - 1 + 2 = n - 1 + 2 = n - 1 + 2 = n - 1 + 2 = n - 1 + 2 = n - 1 + 2 = n - 1 + 2 = n - 1 + 2 = n - 1 + 2 = n - 1 + 2 = n - 1 + 2 = n - 1 + 2 = n - 1 + 2 = n - 1 + 2 = n - 1 + 2 = n - 1 + 2 = n - 1 + 2 = n - 1 + 2 = n - 1 + 2 = n - 1 + 2 = n - 1 + 2 = n - 1 + 2 = n - 1 + 2 = n - 1 + 2 = n - 1 + 2 = n - 1 + 2 = n - 1 + 2 = n - 1 + 2 = n - 1 + 2 = n - 1 + 2 = n - 1 + 2 = n - 1 + 2 = n - 1 + 2 = n - 1 + 2 = n - 1 + 2 = n - 1 + 2 = n - 1 + 2 = n - 1 + 2 = n - 1 + 2 = n - 1 + 2 = n - 1 + 2 = n - 1 + 2 = n - 1 + 2 = n - 1 + 2 = n - 1 + 2 = n - 1 + 2 = n - 1 + 2 = n - 1 + 2 = n - 1 + 2 = n - 1 + 2 = n - 1 + 2 = n - 1 + 2 = n - 1 + 2 = n - 1 + 2 = n - 1 + 2 = n - 1 + 2 = n - 1 + 2 = n - 1 + 2 = n - 1 + 2 = n - 1 + 2 = n - 1 + 2 = n - 1 + 2 = n - 1 + 2 = n - 1 + 2 = n - 1 + 2 = n - 1 + 2 = n - 1 + 2 = n - 1 + 2 = n - 1 + 2 = n - 1 + 2 = n - 1 + 2 = n - 1 + 2 = n - 1 + 2 = n - 1 + 2 = n - 1 + 2 = n - 1 + 2 = n - 1 + 2 = n - 1 + 2 = n - 1 + 2 = n - 1 + 2 = n - 1 + 2 = n - 1 + 2 = n - 1 + 2 = n - 1 + 2 = n - 1 + 2 = n - 1 + 2 = n - 1 + 2 = n - 1 + 2 = n - 1 + 2 = n - 1 + 2 = n - 1 + 2 = n - 1 + 2 = n - 1 + 2 = n - 1 + 2 = n - 1 + 2 = n - 1 + 2 = n - 1 + 2 = n - 1 + 2 = n - 1 + 2 = n - 1 + 2 = n - 1 + 2 = n - 1 + 2 = n - 1 + 2 = n - 1 + 2 = n - 1 + 2 = n - 1 + 2 = n - 1 + 2 = n - 1 + 2 = n - 1 + 2 = n - 1 + 2 = n - 1 + 2 = n - 1 + 2 = n - 1 + 2 = n - 1 + 2 = n - 1 + 2 = n - 1 + 2 = n - 1 + 2 = n - 1 + 2 = n - 1 + 2 = n - 1 + 2 = n - 1 + 2 = n - 1 + 2 = n - 1 + 2 = n - 1 + 2 = n - 1 + 2 = n - 1 + 2 = n - 1 + 2 = n - 1 + 2 = n - 1 + 2 = n - 1 + 2 = n - 1 + 2 = n - 1 + 2 = n - 1 + 2 = n - 1 + 2 = n - 1 + 2 = n - 1 + 2 = n - 1 + 2 = n - 1 + 2 = n - 1 + 2 = n - 1 + 2 = n - 1 + 2 = n - 1 + 2 = n - 1 + 2 = n - 1 + 2 = n - 1 + 2 = n - 1 + 2 = n - 1 + 2 = n - 1 + 2 = n - 1 + 2 = n - 1 + 2 = n - 1 + 2 = n - 1 + 2 = n - 1 + 2 = n - 1 + 2 = n - 1 + 2 = n - 1 + 2 = n - 1 + 2 = n - 1 + 2 = n - 1 + 2 = n - 1 + 2 = n - 1 + 2 = n - 1 + 2 = n - 1 + 2 = n - 1 + 2 = n - 1 + 2 = n - 1 + 2 = n - 1 + 2 = n - 1 + 2 = n - 1 + 2 = n - 1 + 2 = n - 1 + 2 = n - 1 + 2 = n - 1 + 2 = n - 1 + 2 = n - 1 + 2 = n - 1 + 2 = n - 1 + 2 = n - 1 + 2 = n - 1 + 2 = n - 1 + 2 = n - 1 + 2 = n - 1 + 2 = n - 1 + 2 = n - 1 + 2 = n - 1 + 2 = n - 1 + 2 = n - 1 + 2 = n - 1 + 2 = n - 1 + 2 = n - 1 + 2 = n - 1 + 2 = n - 1 + 2 = n - 1 + 2 = n - 1 + 2 = n - 1 + 2 = n - 1 + 2 = n - 1 + 2 = n - 1 + 2 = n - 1 + 2 = n - 1 + 2 = n - 1 + 2 = n - 1 + 2 = n - 1 + 2 = n - 1 + 2 = n - 1 + 2 = n - 1 + 2 = n - 1 + 2 = n - 1 + 2 = n - 1 + 2 = n - 1 + 2 = n - 1 + 2 = n - 1 + 2 = n - 1 + 2 = n - 1 + 2 = n - 1 + 2 = n - 1 + 2 = n - 1 + 2 = n - 1 + 2 = n - 1 + 2 = n - 1 + 2 = n - 1 + 2 = n - 1 + 2 = n - 1 + 2 = n - 1 + 2 = n - 1 + 2 = n - 1 + 2 = n - 1 + 2 = n - 1 + 2 = n - 1 + 2 = n - 1 + 2 = n - 1 + 2 = n - 1 + 2 = n - 1 + 2 = n - 1 + 2 = n - 1 + 2 = n - 1 + 2 = n - 1 + 2 = n - 1 + 2 = n - 1 + 2 = n - 1 + 2 = n - 1 + 2 = n - 1 + 2 = n - 1 + 2 = n - 1 + 2 = n - 1 + 2 = n - 1 + 2 = n - 1 + 2 = n - 1 + 2 = n - 1 + 2 = n - 1 + 2 = n - 1 + 2 = n - 1 + 2 = n - 1 + 2 = n - 1 + 2 = n - 1 + 2 = n - 1 + 2 = n - 1 + 2 = n - 1 + 2 = n - 1 + 2 = n - 1 + 2 = n - 1 + 2 = n - 1 + 2 = n - 1 + 2 = n - 1 + 2 = n - 1 + 2 = n - 1 + 2 = n - 1 + 2 = n - 1 + 2 = n - 1 + 2 = n - 1 + 2 = n - 1 + 2 = n - 1 + 2 = n - 1 + 2 = n - 1 + 2 = n - 1 + 2 = n - 1 + 2 = n - 1 + 2 = n - 1 + 2 = n - 1 + 2 = n - 1 + 2 = n - 1 + 2 = n - 1 + 2 = n - 1 + 2 = n - 1 + 2 = n - 1 + 2 = n - 1 + 2 = n - 1 + 2 = n - 1 + 2 = n - 1 + 2 = n - 1 + 2 = n - 1 + 2 = n - 1 + 2 = n - 1 + 2 = n - 1 + 2 = n - 1 + 2 = n - 1 + 2 = n - 1 + 2 = n - 1 + 2 = n - 1 + 2 = n - 1 + 2 = n - 1 + 2 = n - 1 + 2 = n - 1 + 2 = n - 1 + 2 = n - 1 + 2 = n - 1 + 2 = n - 1 + 2 = n - 1 + 2 = n - 1 + 2 = n - 1 + 2 = n - 1 + 2 = n - 1 + 2 = n - 1 + 2 = n - 1 + 2 = n - 1 + 2 = n - 1 + 2 = n - 1 + 2 = n - 1 + 2 = n - 1 + 2 = n - 1 + 2 = n - 1 + 2 = n - 1 + 2 = n - 1 + 2 = n - 1 + 2 = n - 1 + 2 = n - 1 + 2 = n - 1 + 2 = n - 1 + 2 = n - 1 + 2 = n - 1 + 2 = n - 1 + 2 = n - 1 + 2 = n - 1 + 2 = n - 1 + 2 = n - 1 + 2 = n - 1 + 2 = n - 1 + 2 = n - 1 + 2 = n - 1 + 2 = n - 1 + 2 = n - 1 + 2 = n - 1 + 2 = n - 1 + 2 = n - 1 + 2 = n - 1 + 2 = n - 1 + 2 = n - 1 + 2 = n - 1 + 2 = n - 1 + 2 = n - 1 + 2 = n - 1 + 2 = n - 1 + 2 = n - 1 + 2 = n - 1 + 2 = n - 1 + 2 = n - 1 + 2 = n - 1 + 2 = n - 1 + 2 = n - 1 + 2 = n - 1 + 2 = n - 1 + 2 = n - 1 + 2 = n - 1 + 2 = n - 1 + 2 = n - 1 + 2 = n - 1 + 2 = n - 1 + 2 = n - 1 + 2 = n - 1 + 2 = n - 1 + 2 = n - 1 + 2 = n - 1 + 2 = n - 1 + 2 = n - 1 + 2 = n - 1 + 2 = n - 1 + 2 = n - 1 + 2 = n - 1 + 2 = n - 1 + 2 = n - 1 + 2 = n - 1 + 2 = n - 1 + 2 = n - 1 + 2 = n - 1 + 2 = n - 1 + 2 = n - 1 + 2 = n - 1 + 2 = n - 1 + 2 = n - 1 + 2 = n - 1 + 2 = n - 1 + 2 = n - 1 + 2 = n - 1 + 2 = n - 1 + 2 = n - 1 + 2 = n - 1 + 2 = n - 1 + 2 = n - 1 + 2 = n - 1 + 2 = n - 1 + 2 = n - 1 + 2 = n - 1 + 2 = n - 1 + 2 = n - 1 + 2 = n - 1 + 2 = n - 1 + 2 = n - 1 + 2 = n - 1 + 2 = n - 1 + 2 = n - 1 + 2 = n - 1 + 2 = n - 1 + 2 = n - 1 + 2 = n - 1 + 2 = n - 1 + 2 = n - 1 + 2 = n - 1 + 2 = n - 1 + 2 = n - 1 + 2 = n - 1 + 2 = n - 1 + 2 = n - 1 + 2 = n - 1 + 2 = n - 1 + 2 = n - 1 + 2 = n - 1 + 2 = n - 1 + 2 = n - 1 + 2 = n - 1 + 2 = n - 1 + 2 = n - 1 + 2 = n - 1 + 2 = n - 1 + 2 = n - 1 + 2 = n - 1 + 2 = n - 1 + 2 = n - 1 + 2 = n - 1 + 2 = n - 1 + 2 = n - 1 + 2 = n - 1 + 2 = n - 1 + 2 = n - 1 + 2 = n - 1 + 2 = n - 1 + 2 = n - 1 + 2 = n - 1 + 2 = n - 1 + 2 = n - 1 + 2 = n - 1 + 2 = n - 1 + 2 = n - 1 + 2 = n - 1 + 2 = n - 1 + 2 = n - 1 + 2 = n - 1 + 2 = n - 1 + 2 = n - 1 + 2 = n - 1 + 2 = n - 1 + 2 = n - 1 + 2 = n - 1 + 2 = n - 1 + 2 = n - 1 + 2 = n - 1 + 2 = n - 1 + 2 = n - 1 + 2 = n - 1 + 2 = n - 1 + 2 = n - 1 + 2 = n - 1 + 2 = n - 1 + 2 = n - 1 + 2 = n - 1 + 2 = n - 1 + 2 = n - 1 + 2 = n - 1 + 2 = n - 1 + 2 = n - 1 + 2 = n - 1 + 2 = n - 1 + 2 = n - 1 + 2 = n - 1 + 2 = n - 1 + 2 = n - 1 + 2 = n - 1 + 2 = n - 1 + 2 = n - 1 + 2 = n - 1 + 2 = n - 1 + 2 = n - 1 + 2 = n - 1 + 2 = n - 1 + 2 = n - 1 + 2 = n - 1 + 2 = n - 1 + 2 = n - 1 + 2 = n - 1 + 2 = n - 1 + 2 = n - 1