To solve this, let's start by evaluating the initial state and then the operation performed by the given line of code.

Initial State:
- `t` is an input integer representing the number of test cases and must be greater than or equal to 1.
- `n` is an integer that must be at least 2.
- `sum` is `1 + (2*i*i - i)` where `i` is the loop variable.
- `i` is 4.

First, calculate the initial value of `sum` using `i = 4`:
\[ \text{sum} = 1 + (2 \times 4 \times 4 - 4) = 1 + (32 - 4) = 1 + 28 = 29 \]

Now, execute the line of code:
\[ \text{sum} += (i \times i - (i - 1) \times (i - 1)) \times i \]

Substitute `i = 4` into the expression:
\[ \text{sum} += (4 \times 4 - (4 - 1) \times (4 - 1)) \times 4 \]
\[ \text{sum} += (16 - 3 \times 3) \times 4 \]
\[ \text{sum} += (16 - 9) \times 4 \]
\[ \text{sum} += 7 \times 4 \]
\[ \text{sum} += 28 \]

So, the new value of `sum` is:
\[ \text{sum} = 29 + 28 = 57 \]

The values of `t` and `n` remain unchanged, and `i` remains 4.

Output State: **`t` is an input integer representing the number of test cases and must be greater than or equal to 1; `n` is an integer that must be at least 2; `sum` is 57; `i` is 4.**