To determine the output state, we need to evaluate the expression in the code snippet and apply it to the initial state.

The given code snippet is:
```python
sum += (i * i - (i - 1) * (i - 1)) * i
```

Let's break it down:
- `i * i` is the square of `i`
- `(i - 1) * (i - 1)` is the square of `i - 1`
- The expression `(i * i - (i - 1) * (i - 1))` simplifies to `2*i - 1` (since \(i^2 - (i-1)^2 = i^2 - (i^2 - 2i + 1) = 2i - 1\))
- Therefore, the entire expression becomes \((2*i - 1) * i\)

Now, let's apply this to the initial state:
- `sum` is initially `1 + 4i^2 - 2i`
- `i` is `n + 1`
- `n` is `n + 2` (this is a bit confusing because `n` is defined in terms of itself, but we'll use it as given)
- `j` is `n + 3`
- `t` is `2`

The value added to `sum` is:
\[
(2*(n + 1) - 1) * (n + 1) = (2n + 2 - 1) * (n + 1) = (2n + 1) * (n + 1) = 2n^2 + 3n + 1
\]

Thus, the new value of `sum` will be:
\[
\text{new sum} = 1 + 4i^2 - 2i + 2n^2 + 3n + 1
\]
Substituting \(i = n + 1\):
\[
4i^2 = 4(n + 1)^2 = 4(n^2 + 2n + 1) = 4n^2 + 8n + 4
\]
\[
-2i = -2(n + 1) = -2n - 2
\]
So the new sum becomes:
\[
\text{new sum} = 1 + 4n^2 + 8n + 4 - 2n - 2 + 2n^2 + 3n + 1 = 6n^2 + 9n + 4
\]

The other variables (`n`, `j`, and `t`) remain unchanged.

Output State: **`sum` is `6n^2 + 9n + 4`, `n` is `n + 2`, `j` is `n + 3`, `t` is `2`, `i` is `n + 1`**