To determine the final state after all iterations of the loop, we need to understand the pattern in how the `sum` variable is updated. The loop iterates from `i = 2` to `i = n`, and in each iteration, it adds `(i * i - (i - 1) * (i - 1)) * i` to `sum`.

Let's simplify the expression inside the loop:
- `(i * i - (i - 1) * (i - 1))` simplifies to `(i^2 - (i^2 - 2i + 1))` which further simplifies to `2i - 1`.
- Therefore, the expression being added to `sum` in each iteration is `(2i - 1) * i = 2i^2 - i`.

So, the loop effectively adds `2i^2 - i` to `sum` for each `i` from 2 to `n`.

The initial value of `sum` is 1. After the loop completes, `sum` will be:
\[ \text{sum} = 1 + \sum_{i=2}^{n} (2i^2 - i) \]

We can split this summation into two separate summations:
\[ \text{sum} = 1 + 2\sum_{i=2}^{n} i^2 - \sum_{i=2}^{n} i \]

The formulas for these summations are:
\[ \sum_{i=1}^{n} i^2 = \frac{n(n + 1)(2n + 1)}{6} \]
\[ \sum_{i=1}^{n} i = \frac{n(n + 1)}{2} \]

Therefore:
\[ \sum_{i=2}^{n} i^2 = \sum_{i=1}^{n} i^2 - 1^2 = \frac{n(n + 1)(2n + 1)}{6} - 1 \]
\[ \sum_{i=2}^{n} i = \sum_{i=1}^{n} i - 1 = \frac{n(n + 1)}{2} - 1 \]

Substituting these into our expression for `sum`:
\[ \text{sum} = 1 + 2\left(\frac{n(n + 1)(2n + 1)}{6} - 1\right) - \left(\frac{n(n + 1)}{2} - 1\right) \]
\[ \text{sum} = 1 + \frac{n(n + 1)(2n + 1)}{3} - 2 - \frac{n(n + 1)}{2} + 1 \]
\[ \text{sum} = \frac{n(n + 1)(2n + 1)}{3} - \frac{n(n + 1)}{2} \]

Finding a common denominator:
\[ \text{sum} = \frac{2n(n + 1)(2n + 1) - 3n(n + 1)}{6} \]
\[ \text{sum} = \frac{n(n + 1)(4n + 2 - 3)}{6} \]
\[ \text{sum} = \frac{n(n + 1)(4n - 1)}{6} \]

After all iterations, `n`, `j`, and `t` remain unchanged from their initial values. The final output state is:

Output State: **sum is \(\frac{n(n + 1)(4n - 1)}{6}\), n is the input integer, j is \(n + 1\), t is 2.**

In natural language: After the loop completes, the value of `sum` will be \(\frac{n(n + 1)(4n - 1)}{6}\), while `n`, `j`, and `t` will remain as the input integer, \(n + 1\), and 2, respectively.