To determine the output state after all the iterations of the loop have finished, we need to analyze the behavior of the loop and how the variables evolve with each iteration.

### Loop Analysis
1. **Outer Loop**: The outer loop runs `t` times, where `t` is the number of test cases.
2. **Inner Loop**: For each test case, the inner loop calculates `sum` and prints specific patterns.

### Key Variables:
- `t`: Number of test cases.
- `n`: Size of the `n√ón` matrix for each test case.
- `sum`: Accumulated sum calculated in the inner loop.
- `j`: Loop variable used in printing patterns.

### Calculation of `sum`:
The `sum` is calculated as:
\[ \text{sum} = 1 + \sum_{i=2}^{n} (i^2 - (i-1)^2) \cdot i \]

Simplifying the expression inside the summation:
\[ i^2 - (i-1)^2 = i^2 - (i^2 - 2i + 1) = 2i - 1 \]

Thus, the `sum` becomes:
\[ \text{sum} = 1 + \sum_{i=2}^{n} (2i - 1) \cdot i = 1 + \sum_{i=2}^{n} (2i^2 - i) \]

This can be further simplified to:
\[ \text{sum} = 1 + 2 \sum_{i=2}^{n} i^2 - \sum_{i=2}^{n} i \]

Using the formulas for the sum of squares and the sum of integers:
\[ \sum_{i=1}^{n} i^2 = \frac{n(n + 1)(2n + 1)}{6} \]
\[ \sum_{i=1}^{n} i = \frac{n(n + 1)}{2} \]

Therefore:
\[ \sum_{i=2}^{n} i^2 = \frac{n(n + 1)(2n + 1)}{6} - 1 \]
\[ \sum_{i=2}^{n} i = \frac{n(n + 1)}{2} - 1 \]

Substituting these into the `sum` equation:
\[ \text{sum} = 1 + 2 \left( \frac{n(n + 1)(2n + 1)}{6} - 1 \right) - \left( \frac{n(n + 1)}{2} - 1 \right) \]
\[ \text{sum} = 1 + \frac{n(n + 1)(2n + 1)}{3} - 2 - \frac{n(n + 1)}{2} + 1 \]
\[ \text{sum} = \frac{n(n + 1)(2n + 1)}{3} - \frac{n(n + 1)}{2} \]
\[ \text{sum} = \frac{2n(n + 1)(2n + 1) - 3n(n + 1)}{6} \]
\[ \text{sum} = \frac{n(n + 1)(4n + 2 - 3)}{6} \]
\[ \text{sum} = \frac{n(n + 1)(4n - 1)}{6} \]

### Final Output State:
After all iterations, the output state will be:
- `t` will be 0 (since all test cases have been processed).
- `n` will be the last input integer from the test cases.
- `sum` will be the value calculated for the last test case using the formula \(\frac{n(n + 1)(4n - 1)}{6}\).
- `j` will be \(n + 1\) for the last test case.

### Final Output State in the Required Format:
Output State: **t is 0, n is the last input integer, sum is \(\frac{n(n + 1)(4n - 1)}{6}\), j is \(n + 1\)**.

In natural language: After all the test cases have been processed, `t` becomes 0, `n` is the size of the matrix from the last test case, `sum` is calculated using the formula \(\frac{n(n + 1)(4n - 1)}{6}\) for the last test case, and `j` is \(n + 1\).