Alright, I have this problem to solve. Let's read it carefully.

We have t test cases, and for each test case, we're given n sticks with lengths that are powers of 2, specifically 2 raised to the power of a_i for each stick i. We need to choose exactly 3 sticks that can form a non-degenerate triangle. A non-degenerate triangle has an area greater than 0, which means the three sides must satisfy the triangle inequality: the sum of any two sides must be greater than the third side.

So, the task is to count the number of ways to choose such triples of sticks for each test case.

First, I need to understand the input and output format. The input starts with an integer t, the number of test cases. Then, for each test case, there's an integer n, followed by a list of n integers a_i, where each a_i represents the exponent in the length of the stick, which is 2^{a_i}.

Constraints:

- 1 ≤ t ≤ 10^4

- For each test case:

- 1 ≤ n ≤ 3⋅10^5

- 0 ≤ a_i ≤ n

- The sum of n over all test cases does not exceed 3⋅10^5.

Output:

For each test case, print one integer — the number of ways to choose exactly 3 sticks so that a triangle can be formed out of them.

Example:

Input:

4

7

1 1 1 1 1 1 1

4

3 2 1 3

3

1 2 3

1

1

Output:

35

2

0

0

In the first test case, all sticks have the same length 2^1 = 2. So, any three sticks will form an equilateral triangle, and the number of ways to choose 3 sticks out of 7 is C(7,3) = 35.

In the second test case, the lengths are 2^3=8, 2^2=4, 2^1=2, and 2^3=8. The possible triangles are:

- 8, 8, 4: This satisfies the triangle inequality because 8 + 4 > 8, 8 + 8 > 4, and 4 + 8 > 8.

- 8, 8, 8: But in the input, there are only two sticks of length 8, so we can't choose three of them.

Wait, but in the input, there are two sticks of length 8 (a_i=3 appears twice), and one stick of length 4 (a_i=2), and one stick of length 2 (a_i=1). So, we can choose:

- Stick 1 (8), stick 3 (4), stick 4 (8): 8, 4, 8.

- Stick 1 (8), stick 2 (4), stick 4 (8): 8, 4, 8.

But stick 2 is length 4, and stick 3 is length 2. Wait, no, stick 2 is a_i=2, which is length 4, stick 3 is a_i=1, which is length 2, and stick 4 is a_i=3, which is length 8.

So, the possible triangles are:

- Sticks 1,2,4: 8,4,8

- Sticks 1,3,4: 8,2,8

But in the note, it says only choosing the 1st, 2nd, and 4th stick, or the 1st, 3rd, and 4th stick. But in the output, it's 2, which matches.

In the third test case, lengths are 2, 4, 8, which cannot form a triangle because 2 + 4 = 6, which is not greater than 8.

In the fourth test case, only one stick, so no way to choose 3 sticks.

Alright, now to think about how to solve this in general.

First, since the lengths are powers of 2, which are distinct except when a_i are equal, that simplifies things because powers of 2 are distinct and can be ordered easily.

To form a triangle, we need to choose three sticks such that the sum of the two smaller ones is greater than the largest one.

Given that, perhaps we can sort the list of a_i, compute the corresponding lengths, and then look for triplets where the sum of the two smaller lengths is greater than the largest length.

However, since n can be up to 3*10^5 and t up to 10^4, with the sum of n over all test cases not exceeding 3*10^5, we need an efficient algorithm, probably O(n log n) per test case.

First, sort the list of a_i for each test case, then compute the lengths as 2^{a_i}.

But computing 2^{a_i} for large a_i could be time-consuming, but since a_i <= n and n <= 3*10^5, 2^{a_i} could be up to 2^{3*10^5}, which is way too big to handle directly. But perhaps we can work with the exponents directly.

Let's think about the properties of the powers of 2.

Given three lengths 2^x, 2^y, 2^z, where x <= y <= z, the triangle inequality requires that 2^x + 2^y > 2^z.

Given that 2^x + 2^y <= 2^{y+1} (since 2^x + 2^y <= 2^y + 2^y = 2^{y+1}), so for 2^x + 2^y > 2^z to hold, we need z < y + 1.

Since x <= y <= z and z < y + 1, the only possibilities are z = y or z = y + 1 - but wait, z < y + 1, so z <= y.

But z >= y, so z = y.

Therefore, the only way for 2^x + 2^y > 2^z is when z = y.

So, 2^x + 2^y > 2^y, which simplifies to 2^x > 0, which is always true since x >= 0.

Wait, that can't be right. Because in the third test case, with a_i = 1,2,3, which correspond to lengths 2,4,8, we have z = 3, y = 2, x = 1, and 2 + 4 = 6 > 8 is false, which matches the output of 0.

But according to the above, z = y would mean z = y, so z = y implies 2^x + 2^y > 2^y, which is 2^x > 0, always true, but in the example, it's not forming a triangle when z = y.

Wait, maybe I made a mistake.

Wait, in the third test case, a_i = 1,2,3, so lengths are 2,4,8.

Here, x=1, y=2, z=3, and z = 3 > y = 2, so z > y, but earlier I thought z <= y, but that's not the case here.

Wait, perhaps I need to think differently.

Let me consider that for 2^x + 2^y > 2^z to hold, given x <= y <= z.

Case 1: z > y

Then, 2^x + 2^y <= 2^y + 2^y = 2^{y+1}

So, 2^{y+1} > 2^z only if y + 1 > z.

But since z > y, and z is an integer, z >= y + 1.

So, 2^{y+1} > 2^z only if y + 1 > z, which can't happen since z >= y + 1.

Therefore, when z > y, 2^x + 2^y <= 2^{y+1} <= 2^z, so 2^x + 2^y <= 2^z, which doesn't satisfy the triangle inequality.

Case 2: z = y

Then, 2^x + 2^y = 2^x + 2^y.

If x < y, then 2^x + 2^y = 2^x + 2^y = 2^y + 2^x < 2^y + 2^y = 2^{y+1}

But since z = y, 2^z = 2^y.

So, 2^x + 2^y > 2^y implies 2^x > 0, which is always true.

Therefore, as long as z = y, the triangle inequality holds.

Wait, but in the third test case, z = y = 3, but 2^1 + 2^3 = 2 + 8 = 10 > 8, which should form a triangle, but according to the output, it's 0, meaning no triangle can be formed.

Wait, perhaps I'm misunderstanding something.

Wait, in the third test case, a_i = 1,2,3, which correspond to lengths 2,4,8.

Choosing x=1, y=2, z=3: 2 + 4 = 6 > 8? No, 6 < 8, so no triangle.

Wait, but according to earlier reasoning, if z = y, then 2^x + 2^y > 2^z.

But in this case, z = 3, y = 3, x = 2: 4 + 8 > 8, which is true.

Wait, but in the test case, a_i = 1,2,3, so possible triplets are (1,2,3): 2,4,8 -> 2 + 4 = 6 < 8, so no triangle.

Wait, perhaps I need to consider all possible triplets.

In this test case, n=3, a_i=[1,2,3], which correspond to lengths [2,4,8].

Only one possible triplet: (1,2,3): 2,4,8, which doesn't satisfy the triangle inequality, hence output is 0.

Wait, but according to my earlier reasoning, if z = y, then 2^x + 2^y > 2^z.

But in this case, z = 3, y = 3, x = 2: 4 + 8 > 8, which is true.

But in the triplet (1,2,3), x=1, y=2, z=3: 2 + 4 = 6 > 8? No, 6 < 8, so no triangle.

Wait, perhaps I need to ensure that for any permutation of x,y,z where x <= y <= z, the condition holds.

So, in the triplet (1,2,3), sorted as 2,4,8, 2 + 4 <= 8, so no triangle.

In another scenario, if we have multiple sticks of the same length, but in this test case, all a_i are distinct.

Wait, perhaps I need to consider that for z = y, the sum of the two smaller sides is greater than the largest side.

Wait, perhaps I need to think in terms of the exponents.

Let me consider that for three sticks with exponents a, b, c where a <= b <= c, the condition 2^a + 2^b > 2^c must hold.

Given that 2^a + 2^b > 2^c, and a <= b <= c, let's see what this implies.

We can consider the exponents.

If c > b, then 2^a + 2^b <= 2^b + 2^b = 2^{b+1}.

If c < b + 1, then 2^{b+1} > 2^c, so 2^a + 2^b > 2^c.

But since c >= b, and c < b + 1, the only possibility is c = b.

If c = b, then 2^a + 2^b > 2^c = 2^b, which simplifies to 2^a > 0, which is always true.

If c = b + 1, then 2^a + 2^b > 2^{b+1}.

This would require 2^a > 2^{b+1} - 2^b = 2^b, which implies a > b, but a <= b, so this is impossible.

If c > b + 1, then 2^a + 2^b <= 2^{b+1} < 2^c, so the condition fails.

Therefore, the only way to satisfy the triangle inequality is when c = b.

Meaning, the largest exponent must be equal to the middle exponent.

In other words, the three exponents must be such that the largest is equal to the middle one.

So, in sorted order, a <= b <= c, and c = b.

Therefore, in terms of exponents, for three sticks with exponents a, b, c where a <= b <= c, they can form a triangle if and only if c = b.

This simplifies things a lot.

So, in each test case, I need to count the number of triplets (a,b,c) where a <= b <= c and c = b.

Given that, I can proceed to count such triplets.

First, I can sort the list of a_i in non-decreasing order.

Then, I need to count the number of triplets where the largest exponent is equal to the middle one.

This can be done by iterating through the sorted list and for each pair of equal exponents, count the number of exponents less than or equal to that value.

Wait, more carefully:

Let's sort the list of a_i in non-decreasing order.

Let's say the sorted list is a[1] <= a[2] <= ... <= a[n].

We need to count the number of triplets (i,j,k) such that i < j < k and a[k] = a[j].

Because in the sorted order, a[i] <= a[j] <= a[k], and we need a[k] = a[j].

So, for each pair (j,k) where a[j] = a[k], and for each i < j such that a[i] <= a[j], we have a valid triplet.

So, for each pair (j,k) where a[j] = a[k], the number of i < j such that a[i] <= a[j].

But since the list is sorted, a[i] <= a[j] for all i < j.

Therefore, for each pair (j,k) where a[j] = a[k], there are j-1 possible i's.

So, the total number of triplets is the sum over all pairs (j,k) where a[j] = a[k], of (j-1).

Wait, but this seems inefficient for n up to 3*10^5.

I need a better way to compute this.

An optimized approach would be to group the exponents into their frequency counts.

Let freq[x] be the number of sticks with exponent x.

Then, for each group with freq[x] >= 2, we can choose two sticks from this group and pair them with any stick with exponent <= x.

Wait, but we need to choose three sticks, with the largest two having the same exponent.

Wait, perhaps it's better to think in terms of combinations.

For each group with freq[x], the number of ways to choose two sticks with exponent x is C(freq[x], 2).

Then, for each y < x, we can choose one stick with exponent y and pair it with the two sticks with exponent x.

Additionally, we can choose all three sticks from the same group if freq[x] >= 3.

So, the total number of triplets is:

Sum over x:

If freq[x] >= 3, add C(freq[x], 3)

Sum over x:

If freq[x] >= 2, add C(freq[x], 2) * (number of sticks with exponent < x)

Wait, more precisely:

For each x, if freq[x] >= 2, we can choose two sticks with exponent x and pair them with any stick with exponent <= x.

But in sorted order, the sticks with exponent <= x are all sticks up to that group.

Wait, perhaps it's better to sort the exponents and compute prefix sums.

Let me think differently.

Let's sort the exponents in non-decreasing order.

Compute the prefix sum of the frequency, prefix[x] = number of sticks with exponent <= x.

Then, for each pair of sticks with exponent x, the number of sticks with exponent <= x minus one (since we've already chosen two sticks with exponent x).

Wait, I'm getting confused.

Let me think about it differently.

Given that in the sorted list, for any triplet where the largest two exponents are equal, the number of such triplets is equal to the number of pairs with equal exponents multiplied by the number of sticks with exponents less than or equal to that exponent, minus the number of sticks with exponents equal to that exponent.

Wait, perhaps it's better to group the exponents and compute combinations.

Let me try to implement this step by step.

First, sort the exponents.

Then, group the exponents into their frequency counts.

For each group with frequency freq[x], the number of ways to choose two sticks with exponent x is C(freq[x], 2).

Then, for each such pair, we can choose the third stick from any stick with exponent <= x, excluding the two sticks already chosen.

Wait, but in the sorted list, the sticks with exponent <= x are all previous sticks.

Wait, perhaps it's better to iterate through the sorted exponents and for each exponent x, keep track of the number of sticks with exponent < x.

Then, for each group with freq[x], if freq[x] >= 2, add C(freq[x], 2) * (prefix[x-1]).

Also, if freq[x] >= 3, add C(freq[x], 3).

Wait, but exponents are not necessarily consecutive, so I need to handle that properly.

Alternatively, I can sort the exponents, compute the prefix sums, and for each group with freq[x], add C(freq[x], 2) * prefix[x].

But prefix[x] would be the number of sticks with exponent <= x.

Wait, but in the triplet, we need a[i] <= a[j] = a[k].

So, for each pair of sticks with exponent x, we can choose the third stick from any stick with exponent <= x.

But since we are choosing three distinct sticks, we need to subtract the cases where all three sticks have exponent x.

Wait, perhaps it's better to consider that for each pair of sticks with exponent x, we can choose the third stick from any stick with exponent <= x, but not both of the sticks with exponent x.

Wait, this is getting messy.

Let me look at the code provided and see if it implements this logic correctly.

Given the code:

t = int(input())

func_1(t)

def func_1(test_cases):

results = []

for _ in range(test_cases):

n = int(input())

num_list = list(map(int, input().split()))

num_of_lens = {}

for x in num_list:

if x in num_of_lens:

num_of_lens[x] += 1

else:

num_of_lens[x] = 1

res = 0

total_count = 0

for cnt in num_of_lens.values():

if cnt >= 3:

res += cnt * (cnt - 1) * (cnt - 2) // 6

if cnt >= 2:

res += cnt * (cnt - 1) // 2 * total_count

total_count += cnt

results.append(res)

for result in results:

print(result)

So, the code does the following:

- Reads t test cases.

- For each test case:

- Reads n and the list of a_i.

- Counts the frequency of each a_i in num_of_lens.

- Initializes res and total_count to 0.

- Iterates through the frequencies:

- If cnt >= 3, adds C(cnt, 3) to res.

- If cnt >= 2, adds C(cnt, 2) * total_count to res.

- Adds cnt to total_count.

- Appends res to results.

- After processing all test cases, prints each result in results.

Now, let's see if this logic matches what we need.

Recall that we need to count triplets where in the sorted triplet, the largest two exponents are equal.

The code counts:

- For each group with freq[x] >= 3, it adds C(freq[x], 3), which counts the triplets where all three exponents are x.

- For each group with freq[x] >= 2, it adds C(freq[x], 2) * total_count, where total_count is the total number of sticks encountered so far.

Wait, but total_count includes all sticks from previous groups, i.e., sticks with exponents less than or equal to x.

Wait, no, in the code, total_count is incremented by cnt after processing cnt.

Wait, let's see:

- num_of_lens is a dictionary with exponents as keys and their frequencies as values.

- The loop is over num_of_lens.values(), which are the frequencies, but not necessarily in sorted order.

This is a problem because the order of iteration over num_of_lens.values() is not guaranteed.

We need to process the exponents in sorted order to correctly accumulate total_count.

Wait, perhaps the code sorts the exponents before processing.

Wait, no, the code doesn't sort the exponents; it iterates over num_of_lens.values() directly, which is not sorted.

This could lead to incorrect total_count values.

Wait, perhaps in Python 3.7+, dictionaries maintain insertion order, but that doesn't help here because we need sorted order by exponent.

This might be an issue.

Assuming that num_of_lens is iterated in sorted order of exponents, let's proceed.

So, if we assume that num_of_lens is iterated in sorted order of exponents, then total_count would be the total number of sticks with exponents less than or equal to the current x.

Then, for each group with freq[x] >= 3, it adds C(freq[x], 3) to res.

This accounts for triplets where all three sticks have exponent x.

Then, for each group with freq[x] >= 2, it adds C(freq[x], 2) * total_count to res.

This seems to account for choosing two sticks with exponent x and one stick with exponent less than or equal to x.

However, in our earlier reasoning, for triplets where the largest two exponents are equal, the third exponent can be anything less than or equal to x.

So, this seems correct.

Wait, but in the first test case, all a_i are 1, so freq[1] = 7.

Then, res += C(7,3) = 35, and since total_count = 7, but in the loop, total_count is incremented after processing cnt.

Wait, let's see:

Initialize total_count = 0

For cnt = 7 (assuming only one group with x=1):

if cnt >= 3: res += C(7,3) = 35

if cnt >= 2: res += C(7,2) * 0 = 21 * 0 = 0

total_count += 7 => total_count = 7

So, res = 35 + 0 = 35, which matches the first test case.

In the second test case, a_i = [3,2,1,3], so num_of_lens = {1:1, 2:1, 3:2}

Assuming iteration in order of exponents: x=1, then x=2, then x=3.

For x=1, cnt=1: no addition to res, total_count +=1 => total_count=1

For x=2, cnt=1: no addition to res, total_count +=1 => total_count=2

For x=3, cnt=2: res += C(2,2) * 2 = 1 * 2 = 2

So, res = 0 + 0 + 2 = 2, which matches the second test case