Correctness: **False**

### Explanation:
The provided solution has a logical flaw in how it constructs the array `ans`. The goal is to find an array `a` such that `x_i = a_i \bmod a_{i-1}` for all `2 \le i \le n`. However, the current implementation does not correctly satisfy this condition.

Let's analyze the current logic:
1. `ans[0] = arr[0] + 1`: This sets the first element of `ans` to be one more than the first element of `arr`.
2. For subsequent elements, it tries to construct `ans[i+1]` based on `arr[i]` and `ans[i]`, but it doesn't ensure that `x_i = a_i \bmod a_{i-1}`.

To fix this, we need to ensure that each `a_i` is chosen such that `x_i = a_i \bmod a_{i-1}`. Hereâ€™s a corrected approach:

1. Start with `a_1` as any value greater than or equal to `x_2` (since `x_2 = a_2 \bmod a_1`).
2. For each subsequent `a_i`, choose `a_i` such that `a_i = x_i + k * a_{i-1}` for some integer `k` that makes `a_i \geq a_{i-1}`.

Here is the corrected code:

```python
t = int(input())
while t:
    n = int(input())
    arr = [int(x) for x in input().split(' ')]
    ans = func_1(arr, n)
    for i in ans:
        print(i, end=' ')
    print()
    t -= 1

def func_1(arr, n):
    ans = [0] * n
    # Initialize a_1 arbitrarily, but must be at least arr[1]
    ans[0] = max(1, arr[0])
    for i in range(1, n-1):
        # Ensure a_i > a_{i-1}
        ans[i] = arr[i] + ans[i-1]
    # Set a_n such that x_n = a_n % a_{n-1}
    ans[n-1] = arr[n-2] + ans[n-2]
    return ans
```

This corrected function ensures that each `a_i` is chosen appropriately to satisfy the modulo condition.