Given the initial state, we have:

- `n` is an integer (1 ≤ n ≤ 45)
- `k` is an integer (1 ≤ k ≤ 45)
- `M` is at least 2
- `t` is a sorted list of integers of length `k`
- `i` is 1
- `j` is 2
- `dp[1][2]` is equal to `dp[1][0]`
- `dp[1][1]` is equal to `dp[1][0]`

Now analyzing the code:

```python
dp[i][j] = max(dp[i][j], dp[i - 1][j - t[i - 1]] + 1)
```

Here, `i` is 1 and `j` is 2. 

- The expression `dp[i][j]` represents `dp[1][2]`.
- `dp[i][j]` will be assigned the maximum value between its current value (`dp[1][2]`) and the value of `dp[i - 1][j - t[i - 1]] + 1`, which is `dp[0][2 - t[0]] + 1`.

Since `dp[1][2]` is initially equal to `dp[1][0]`, we need to consider the value of `dp[0][2 - t[0]] + 1`. The exact value of `dp[0][2 - t[0]]` depends on the contents of the list `t` and `dp`.

The output state would reflect the updated value of `dp[1][2]`, but since exact values for `dp[0][...]` and the specific elements of `t` have not been provided, it's represented as an expression.

Output State: **`n` is an integer (1 ≤ n ≤ 45), `k` is an integer (1 ≤ k ≤ 45), `M` is at least 2, `t` is a sorted list of integers of length `k`, `i` is 1, `j` is 2, `dp[1][2]` is updated to max(dp[1][2], dp[0][2 - t[0]] + 1), `dp[1][1]` is equal to `dp[1][0]`**