The code `s = s - spend + back` modifies the value of `s`. Let's break down the impact:

- `s` is initially a positive integer within the range 1 ≤ s ≤ 10^9.
- `spend` is defined as `int(ss[0]) * 10`.
- `back` is defined as `int(ss[0])`.

The new value of `s` is calculated as:
- `s = s - (int(ss[0]) * 10) + int(ss[0])`

This simplifies to:
- `s = s - 9 * int(ss[0])`

The other variables (`t`, `i`, `total`, `ss`, `spend`, `back`) remain unchanged.

Therefore, the Output State is:
**`t` is an integer within the range 1 ≤ t ≤ 10^4, `i` is 0, `s` is `s - 9 * int(ss[0])`, `total` is `int(ss[0]) * 10`, `ss` is the string representation of `s`, `spend` is `int(ss[0]) * 10`, `back` is `int(ss[0])`**