Let's break down the problem step by step to determine what will be printed by the `print` statement.

### Initial State:
1. `t` must be greater than 0.
2. `n` must be greater than or equal to 2.
3. `sum` is calculated as:
   \[
   \text{sum} = 1 + (2 \times 2 - 1 \times 1) \times 2 + (3 \times 3 - 2 \times 2) \times 3 + \ldots + (n \times n - (n - 1) \times (n - 1)) \times n
   \]
4. `i` is `n + 1`.

### Understanding the Formula for `sum`:
The formula for `sum` can be broken down as follows:
- The first term is `1`.
- Each subsequent term is of the form \((k \times k - (k - 1) \times (k - 1)) \times k\) for \(k\) from 2 to \(n\).

Let's simplify the term \((k \times k - (k - 1) \times (k - 1)) \times k\):
\[
k \times k - (k - 1) \times (k - 1) = k^2 - (k - 1)^2 = k^2 - (k^2 - 2k + 1) = 2k - 1
\]
So, the term simplifies to:
\[
(2k - 1) \times k = 2k^2 - k
\]

Therefore, the formula for `sum` becomes:
\[
\text{sum} = 1 + \sum_{k=2}^{n} (2k^2 - k)
\]

### Calculating `sum`:
To find the exact value of `sum`, we need to sum the series:
\[
\text{sum} = 1 + \sum_{k=2}^{n} (2k^2 - k)
\]

This can be further broken down into:
\[
\text{sum} = 1 + 2 \sum_{k=2}^{n} k^2 - \sum_{k=2}^{n} k
\]

Using the formulas for the sum of squares and the sum of integers:
\[
\sum_{k=1}^{n} k^2 = \frac{n(n + 1)(2n + 1)}{6}
\]
\[
\sum_{k=1}^{n} k = \frac{n(n + 1)}{2}
\]

We can adjust these formulas to start from \(k = 2\):
\[
\sum_{k=2}^{n} k^2 = \sum_{k=1}^{n} k^2 - 1^2 = \frac{n(n + 1)(2n + 1)}{6} - 1
\]
\[
\sum_{k=2}^{n} k = \sum_{k=1}^{n} k - 1 = \frac{n(n + 1)}{2} - 1
\]

Substituting these into the formula for `sum`:
\[
\text{sum} = 1 + 2 \left( \frac{n(n + 1)(2n + 1)}{6} - 1 \right) - \left( \frac{n(n + 1)}{2} - 1 \right)
\]
\[
\text{sum} = 1 + \frac{2n(n + 1)(2n + 1)}{6} - 2 - \frac{n(n + 1)}{2} + 1
\]
\[
\text{sum} = \frac{2n(n + 1)(2n + 1)}{6} - \frac{n(n + 1)}{2}
\]
\[
\text{sum} = \frac{n(n + 1)(2n + 1)}{3} - \frac{n(n + 1)}{2}
\]
\[
\text{sum} = \frac{2n(n + 1)(2n + 1) - 3n(n + 1)}{6}
\]
\[
\text{sum} = \frac{n(n + 1)(4n + 2 - 3)}{6}
\]
\[
\text{sum} = \frac{n(n + 1)(4n - 1)}{6}
\]

### Calculating `n + n`:
\[
n + n = 2n
\]

### Final Output:
The `print` statement will print the value of `sum` and `2n`.

Output: **\(\frac{n(n + 1)(4n - 1)}{6}\), 2n (where \(n\) is the value of \(n\))**