Output State: **`t` must be greater than 0, `sum` is 19, `i` is 3, `j` is `n`, `n` must be at least 3, `t` is `t` - 1**

Explanation:
- The value of `sum` is updated to `sum += (i * i - (i - 1) * (i - 1)) * i`.
- Given `i` is 3, the expression `(i * i - (i - 1) * (i - 1)) * i` evaluates to `(3 * 3 - (3 - 1) * (3 - 1)) * 3 = (9 - 4) * 3 = 5 * 3 = 15`.
- Therefore, `sum` is updated from 7 to 7 + 15 = 19.
- The values of `i`, `j`, and `n` remain unchanged.
- The value of `t` is decremented by 1, but it must still be greater than 0.