The code `res += (b[i] + c) * m` increments `res` by the value of `(b[i] + c) * m`. Given the conditions in the initial state, if the condition `b[i] == mx and i == mx_ind_lt` is met, then `c` is increased by `(k % m)` and `res` is increased by `(b[i] + c) * (k % m)`. Otherwise, `c` is increased by `m` and `res` is increased by `(b[i] + c) * m`.

Since the condition `b[i] == mx and i == mx_ind_lt` is not specified to be true in the initial state, we assume it is false. Thus, `c` is increased by `m` and `res` is increased by `(b[i] + c) * m`.

Therefore, the updated values are:
- `c` is increased by `m`
- `res` is increased by `(b[i] + c) * m`

Output State: **`i` is increased by 1, `c` is increased by `m`, `res` is increased by `(b[i] + c) * m`, `b[i] == mx and i == mx_ind_lt` is false**