Let's break down the problem step by step.

### Initial States:
- `i` is increased by 1.
- `c` is increased by either `(k % m)` or `2m`.
- `res` is increased by either `(b[i] + c) * (k % m)` or `(b[i] + c) * m`.
- Specifically, if the condition `b[i] == mx and i == mx_ind_lt` is met, then `c` is increased by `(k % m)`, `res` is increased by `(b[i] + c) * (k % m)`, and `res` is updated by adding `(b[i] + c) * (k % m)` to its current value. Otherwise, `c` is increased by `2m`, `res` is increased by `(b[i] + c) * m`, and `b[i] == mx and i == mx_ind_lt` is false.

### Step-by-Step Analysis:

1. **Increment `i`:**
   - At the end of the previous iteration, `i` is increased by 1. So, for the next iteration, `i` will be incremented from its current value by 1.

2. **Determine the increment of `c`:**
   - The value of `c` depends on the condition `b[i] == mx and i == mx_ind_lt`.
     - If this condition is true, `c` is increased by `(k % m)`.
     - If this condition is false, `c` is increased by `2m`.

3. **Determine the increment of `res`:**
   - Similarly, the value of `res` depends on the same condition `b[i] == mx and i == mx_ind_lt`.
     - If this condition is true, `res` is increased by `(b[i] + c) * (k % m)`.
     - If this condition is false, `res` is increased by `(b[i] + c) * m`.

### Final Adjustments:

Given that we need to determine the state at the start of the next iteration, we adjust the following:

- `i` will be `i + 1`.
- `c` will be `c + (k % m)` if `b[i] == mx and i == mx_ind_lt`, otherwise `c` will be `c + 2m`.
- `res` will be `res + (b[i] + c) * (k % m)` if `b[i] == mx and i == mx_ind_lt`, otherwise `res` will be `res + (b[i] + c) * m`.

Thus, the state at the start of the next iteration should reflect these changes.

### Final State:

State: **`i` is i + 1, `c` is increased by either `(k % m)` or `2m` based on the condition `b[i] == mx and i == mx_ind_lt`, and `res` is increased by either `(b[i] + c) * (k % m)` or `(b[i] + c) * m` based on the same condition.**