The line of code `ans += b - before[1]` updates the variable `ans` by adding the difference between `b` and the second element of the tuple `before`. 

Given the initial state, we know:
- `arr` is a list of `n` integers where `arr[x-1] = 1` and all other elements are 0.
- `pairs` is a list of `m` tuples `(l_i, r_i)` such that `1 ≤ l_i ≤ r_i ≤ n`.
- `n`, `x`, and `m` are positive integers such that `1 ≤ x ≤ n` and `1 ≤ m ≤ 100`.
- `a` and `b` are the next tuple in the `pairs` list.
- `ans` and `before` are updated based on the conditions provided in the loop body.

After executing the code:
- `ans` is updated to `ans + (b - before[1])`.

The values of `arr`, `pairs`, `n`, `x`, `m`, `a`, and `b` remain unchanged. The value of `before` is not modified by this specific line of code.

Therefore, the output state is:
**`arr` is a list of `n` integers where `arr[x-1] = 1` and all other elements are 0, `pairs` is a list of `m` tuples `(l_i, r_i)` such that `1 ≤ l_i ≤ r_i ≤ n`, `n`, `x`, and `m` are positive integers such that `1 ≤ x ≤ n` and `1 ≤ m ≤ 100`, `a` and `b` are the next tuple in the `pairs` list, `ans` is `ans + (b - before[1])`, `before` remains unchanged.**