The code snippet `ans += b - before[1]` updates the value of `ans` by adding the difference between `b` and `before[1]`. Let's analyze the impact of this code:

- `ans` is updated to `ans + (b - before[1])`.
- `b` is the second element of the current tuple `(a, b)` from the `pairs` list.
- `before` is a list that remains unchanged, so `before[1]` retains its original value.

The rest of the initial state remains unchanged. Therefore, the output state is:

Output State: **`arr` is a list of `n` integers where `arr[x-1] = 1` and all other elements are 0, `pairs` is a list of `m` tuples `(l_i, r_i)` such that `1 ≤ l_i ≤ r_i ≤ n`, `n`, `x`, and `m` are positive integers such that `1 ≤ x ≤ n` and `1 ≤ m ≤ 100`, `a` and `b` are the next tuple in the `pairs` list, `ans` is updated to `ans + (b - before[1])`, `before` remains unchanged.**