To calculate the output state, we first need to understand the initial state and how the given code snippet affects it.

Given:
- `a` is 3 times its initial value, which we can denote as `a_init`. So, `a = 3 * a_init`.
- `b` is 2 times its initial value, denoted as `b_init`. So, `b = 2 * b_init`.
- `years` is 1.
- The condition `3 * a_init <= 2 * b_init` holds.

The code snippet is:
```python
a *= 3
```
This operation multiplies the current value of `a` by 3.

Given that `a = 3 * a_init`, after the operation, `a` becomes:
```python
a = 3 * (3 * a_init) = 9 * a_init
```

The values of `b` and `years` and the condition `3 * a_init <= 2 * b_init` are not affected by this operation.

Therefore, the output state, considering the changes and the initial conditions, is:
- `a` is `9 * a_init`.
- `b` is `2 * b_init`.
- `years` is 1.
- The condition `3 * a_init <= 2 * b_init` still holds, as the relationship between `a_init` and `b_init` hasn't changed, only the value of `a` has been updated.

Output State: **`a` is `9 * a_init`, `b` is `2 * b_init`, `years` is 1, and `3 * a_init <= 2 * b_init`**