The value of `a` is multiplied by 3, so the new value of `a` is `3 * 9 * a_init` = `27 * a_init`. The states of the other variables are not affected. The condition `9 * a_init <= 4 * b_init` is still valid, and since `a` is now `27 * a_init`, we can infer that `27 * a_init` = `3 * 9 * a_init` and `9 * a_init <= 4 * b_init`. Therefore, the Output State is: `a` is `27 * a_init`, `b` is `4 * b_init`, `years` is 2, and `27 * a_init` = `3 * (9 * a_init)` <= `3 * (4 * b_init)` which is `27 * a_init` <= `12 * b_init`.
Output State: **`a` is `27 * a_init`, `b` is `4 * b_init`, `years` is 2, and `27 * a_init` <= `12 * b_init`**