The code `y_min_sq = r_squared - x_squared` calculates the difference between `r_squared` and `x_squared`. Given that `r_squared = r * r` and `x_squared = (-r + 1) * (-r + 1)`, we can substitute these into the equation.

So, `y_min_sq` becomes:
\[ y_min_sq = r * r - (-r + 1) * (-r + 1) \]
\[ y_min_sq = r^2 - ((-r)^2 - 2*r + 1) \]
\[ y_min_sq = r^2 - (r^2 - 2*r + 1) \]
\[ y_min_sq = r^2 - r^2 + 2*r - 1 \]
\[ y_min_sq = 2*r - 1 \]

Therefore, the value of `y_min_sq` is `2*r - 1`.

The other variables remain unchanged from their initial states:
- `r` is an integer such that \(1 \leq r \leq 10^5\),
- `count` is updated according to the given rules,
- `r_squared` is \(r \times r\),
- `r_plus_1_squared` is \((r + 1) \times (r + 1)\),
- `x` is \(-r + 1\),
- `x_squared` is \((-r + 1) * (-r + 1)\).

Output State: **`r` is an integer such that \(1 \leq r \leq 10^5\), `count` is updated according to the given rules, `r_squared` is \(r \times r\), `r_plus_1_squared` is \((r + 1) \times (r + 1)\), `x` is \(-r + 1\), `x_squared` is \((-r + 1) * (-r + 1)\), `y_min_sq` is \(2*r - 1\)**