The code updates the value of `y_max_sq` based on the formula `y_max_sq = r_plus_1_squared - x_squared - 1`. Let's break this down step-by-step:

1. `r_squared` is \(r \times r\).
2. `r_plus_1_squared` is \((r + 1) \times (r + 1)\).
3. `x` is \(-r + 1\).
4. `x_squared` is \((-r + 1) * (-r + 1)\).

From the given code snippet, `y_max_sq` is updated as follows:
\[ y_max_sq = r_plus_1_squared - x_squared - 1 \]

Substituting the expressions for `r_plus_1_squared` and `x_squared`:
\[ y_max_sq = (r + 1)^2 - (-r + 1)^2 - 1 \]
\[ y_max_sq = (r^2 + 2r + 1) - (r^2 - 2r + 1) - 1 \]
\[ y_max_sq = r^2 + 2r + 1 - r^2 + 2r - 1 - 1 \]
\[ y_max_sq = 4r - 1 \]

So, `y_max_sq` is now equal to \(4r - 1\).

The other variables remain unchanged.

Output State: **`r` is an integer such that \(1 \leq r \leq 10^5\), `count` is updated according to the given rules, `r_squared` is \(r \times r\), `r_plus_1_squared` is \((r + 1) \times (r + 1)\), `x` is \(-r + 1\), `x_squared` is \((-r + 1) * (-r + 1)\), `y_min_sq` is \(2*r - 1\), `y_max_sq` is \(4r - 1\)**