The code snippet calculates `y_max_sq` using the formula `r_plus_1_squared - x_squared - 1`. Let's break down the calculation:

1. `r_plus_1_squared` is \((r + 1) \times (r + 1)\).
2. `x_squared` is \((-r + 1) \times (-r + 1)\).

So, `y_max_sq` is:
\[ y_max_sq = (r + 1)^2 - (-r + 1)^2 - 1 \]

Expanding the squares:
\[ (r + 1)^2 = r^2 + 2r + 1 \]
\[ (-r + 1)^2 = r^2 - 2r + 1 \]

Substitute these into the equation for `y_max_sq`:
\[ y_max_sq = (r^2 + 2r + 1) - (r^2 - 2r + 1) - 1 \]
\[ y_max_sq = r^2 + 2r + 1 - r^2 + 2r - 1 - 1 \]
\[ y_max_sq = 4r - 1 \]

Therefore, after executing the code, the value of `y_max_sq` is `4r - 1`. The states of the other variables are not affected.

Output State: **`r` is an integer such that \(1 \leq r \leq 10^5\), `count` is updated according to the given rules, `r_squared` is \(r \times r\), `r_plus_1_squared` is \((r + 1) \times (r + 1)\), `x` is \(-r + 1\), `x_squared` is \((-r + 1) * (-r + 1), `y_max_sq` is \(4r - 1\)**.