Based on the initial state provided:

- `i` is 0
- `n` is a positive integer
- `l` is a list where the element at index `a[i] - 1` is equal to 2

We need to determine the value of `a[i]`.

Given that `i` is 0, we substitute `i` into the expression `a[i] - 1`:

\[ a[0] - 1 = \text{index in list } l \]

From the postcondition, we know that the element at this index in list `l` is 2. Therefore:

\[ l[a[0] - 1] = 2 \]

This implies:

\[ a[0] - 1 = \text{index of 2 in list } l \]

Since `l` contains the element 2 at the specified index, and knowing that list indices start from 0, if `l` has 2 at index 1 (since `a[0] - 1 = 1`), then `a[0]` must be 2.

Thus, `a[i]` (which is `a[0]`) is 2.

The print statement is:

```python
print(a[i], a[i], end=' ')
```

Substituting the value of `a[i]`:

\[ \text{print(2, 2, end=' ')} \]

This will print `2 2` followed by a space due to the `end=' '` parameter.

Output: **2 2**