To determine the output of the given print statement, let's break down the initial state and the operations step by step.

### Initial State:
- `[*open(0)][1:]` is a list that must have at least 2 elements. This list is created by reading the contents of the file descriptor `0` (which is typically standard input), converting each line to a list, and then slicing to remove the first element.
- `s` is the second element in this list.
- `n` is the integer value of the first part of `s` split by whitespace.
- `k` is the integer value of the second part of `s` split by whitespace.

### Code Snippet:
```python
print((k // 2 + k % 2) * (k < 4 * n - 3) + 2 * n * (k >= 4 * n - 3) + (k == 4 * n - 2))
```

### Step-by-Step Analysis:
1. **Extracting `s` from the list:**
   - `s` is the second element in the list `[*open(0)][1:]`.

2. **Splitting `s` by whitespace:**
   - `s.split()` will split `s` into a list of two strings, where the first string is the value of `n` and the second string is the value of `k`.

3. **Converting `n` and `k` to integers:**
   - `n = int(s.split()[0])`
   - `k = int(s.split()[1])`

4. **Evaluating the expression:**
   - The expression inside the `print` statement is:
     ```python
     (k // 2 + k % 2) * (k < 4 * n - 3) + 2 * n * (k >= 4 * n - 3) + (k == 4 * n - 2)
     ```

5. **Breaking down the expression:**
   - `k // 2 + k % 2`: This is the ceiling of `k / 2`. If `k` is even, `k % 2` is 0, so the result is `k // 2`. If `k` is odd, `k % 2` is 1, so the result is `k // 2 + 1`.
   - `(k < 4 * n - 3)`: This is a boolean condition that evaluates to 1 if true and 0 if false.
   - `2 * n * (k >= 4 * n - 3)`: This is `2 * n` if `k >= 4 * n - 3` and 0 otherwise.
   - `(k == 4 * n - 2)`: This is a boolean condition that evaluates to 1 if true and 0 if false.

6. **Combining the results:**
   - The expression can be broken down into three parts:
     - `(k // 2 + k % 2) * (k < 4 * n - 3)`: This part contributes `k // 2 + k % 2` if `k < 4 * n - 3` and 0 otherwise.
     - `2 * n * (k >= 4 * n - 3)`: This part contributes `2 * n` if `k >= 4 * n - 3` and 0 otherwise.
     - `(k == 4 * n - 2)`: This part contributes 1 if `k == 4 * n - 2` and 0 otherwise.

7. **Final Calculation:**
   - The final value printed is the sum of these three parts.

### Example Calculation:
Let's assume `s = "5 17"`, so:
- `n = 5`
- `k = 17`

Now, evaluate the expression:
- `k // 2 + k % 2 = 17 // 2 + 17 % 2 = 8 + 1 = 9`
- `k < 4 * n - 3 = 17 < 4 * 5 - 3 = 17 < 17 = False` (0)
- `2 * n * (k >= 4 * n - 3) = 2 * 5 * (17 >= 17) = 10 * 1 = 10`
- `k == 4 * n - 2 = 17 == 4 * 5 - 2 = 17 == 18 = False` (0)

So, the expression becomes:
```python
9 * 0 + 10 * 1 + 0 = 0 + 10 + 0 = 10
```

### General Output:
Since the exact values of `n` and `k` are not provided, we can describe the output based on the given conditions.

Output: **(k // 2 + k % 2) * (k < 4 * n - 3) + 2 * n * (k >= 4 * n - 3) + (k == 4 * n - 2) (where n is the integer value of the first part of s split by whitespace, and k is the integer value of the second part of s split by whitespace)**

This output will be a single integer value based on the values of `n` and `k` derived from `s`.