`k` is decremented by `n - 1`. Given the initial conditions, `k` is an integer such that \(0 \leq k < nm\) and \(k \geq n - 1\). After decrementing `k` by `n - 1`, the new value of `k` will be \(k - (n - 1)\). Since `n` is an even positive integer, `n - 1` is an odd positive integer. The new value of `k` will still satisfy the condition \(0 \leq k < nm\), but now \(k\) could be less than \(n - 1\) if it was exactly \(n - 1\) initially. However, since \(k \geq n - 1\), the new value of `k` will be in the range \(n - 1 - (n - 1) \leq k < nm - (n - 1)\), which simplifies to \(0 \leq k < nm - (n - 1)\).

Therefore, the updated conditions are:
- `n` is an even positive integer such that \(2 \leq n \leq 10^9\)
- `m` is an odd positive integer such that \(2 \leq m \leq 10^9\)
- `k` is an integer such that \(0 \leq k < nm - (n - 1)\) and \(k \geq n - 1\)

Output State: **`n` is an even positive integer such that \(2 \leq n \leq 10^9\); `m` is an odd positive integer such that \(2 \leq m \leq 10^9\); `k` is an integer such that \(0 \leq k < nm - (n - 1)\) and \(k \geq n - 1\)**