Let's break down the initial state and the expression in the print statement step by step:

1. **Initial State Values:**
   - `a` is 8
   - `L` is `[8, 3, 1]`
   - `tot` is 15
   - `k` is 15
   - `pow` is 2
   - `m` is 1
   - `n` is 0

2. **Expression in Print Statement:**
   The expression is `pow * (2 * (k - tot) - 1)`

3. **Step-by-Step Calculation:**
   - Calculate `k - tot`: 
     \[
     k - tot = 15 - 15 = 0
     \]
   - Multiply by 2:
     \[
     2 * (k - tot) = 2 * 0 = 0
     \]
   - Subtract 1:
     \[
     2 * (k - tot) - 1 = 0 - 1 = -1
     \]
   - Multiply by `pow`:
     \[
     pow * (2 * (k - tot) - 1) = 2 * (-1) = -2
     \]

4. **Final Value:**
   The value that will be printed is `-2`.

Output: **-2**