The code snippet `a[l] -= a[r]` subtracts the value of `a[r]` from `a[l]`. Given that `a[r]` is less than `a[l]`, the new value of `a[l]` will be `a[l] - a[r]`.

All other variables (`t`, `n`, `a`, `l`, `r`, `sunks`, and `k`) remain unchanged except for `a[l]`. The condition `k` is greater than or equal to `a[r] * 2` and `k` being updated to `k - a[r] * 2` are not affected by the current operation.

Output State: **`t` is an integer such that 1 ≤ t ≤ 10^4, `n` is an integer such that 1 ≤ n ≤ 2 · 10^5, `a[r]` is less than `a[l]`, `a[l]` is now `a[l] - a[r]`, `l`, `r`, and `sunks` remain unchanged, `k` is greater than or equal to `a[r] * 2` and `k` is now `k - a[r] * 2`.**