Let's break down the initial state and the code snippet step by step:

1. **Initial State**:
   - `t` is an integer between 1 and \(10^4\).
   - `i` is 0.
   - `a` is an input integer.
   - `b` is an input integer.
   - `m` is an input integer.
   - `mn` is the sum of `min(a, b)` and `m`.

2. **Condition**:
   - The condition \((m \% a \neq 0 \text{ or } m \% b \neq 0 \text{ or } (a == 1) \text{ or } (b == 1))\) holds true.

3. **Code Snippet**:
   ```python
   print(mn // a + mn // b)
   ```

Given the condition, let's analyze the expression `mn // a + mn // b`:

- `mn` is defined as `min(a, b) + m`.
- Since the condition \((m \% a \neq 0 \text{ or } m \% b \neq 0 \text{ or } (a == 1) \text{ or } (b == 1))\) holds true, it implies that either `a` or `b` is 1, or `m` is not divisible by both `a` and `b`.

To simplify the expression `mn // a + mn // b`:

- If `a == 1`, then `mn // a = (min(a, b) + m) // 1 = min(a, b) + m`.
- If `b == 1`, then `mn // b = (min(a, b) + m) // 1 = min(a, b) + m`.

In both cases, the expression simplifies to:
\[ mn // a + mn // b = (min(a, b) + m) + (min(a, b) + m) = 2 \times (min(a, b) + m) \]

Therefore, the output of the print statement is:
Output: **2 \* (min(a, b) + m)**