Correctness: **True**

### Explanation:
The provided solution correctly implements the logic to maximize Bob's profit based on the given conditions. Let's break down the logic:

1. **Case 1:** If `b <= a`, it means there is no benefit in reducing the price for any buns. Therefore, Bob should sell all buns at the usual price `a`. The total profit would be `n * a`.

2. **Case 2:** If `b - a < n`, it means the reduction in price (`b - a`) is less than the number of buns. In this case, it's beneficial to reduce the price for the first `k` buns where `k = b - a`. The price of the `i-th` bun (for `1 <= i <= k`) is `(b - i + 1)` coins. The remaining buns `(n - k)` are sold at the usual price `a`.

   The total profit in this case is calculated as:
   \[
   \text{Profit} = \sum_{i=1}^{k} (b - i + 1) + (n - k) \times a
   \]
   Simplifying the summation part:
   \[
   \sum_{i=1}^{k} (b - i + 1) = \sum_{i=1}^{k} (b + 1 - i) = \sum_{i=1}^{k} (b + 1) - \sum_{i=1}^{k} i = k(b + 1) - \frac{k(k + 1)}{2}
   \]
   So the total profit becomes:
   \[
   \text{Profit} = k(b + 1) - \frac{k(k + 1)}{2} + (n - k) \times a
   \]

3. **Case 3:** If `b - a >= n`, it means the reduction in price is sufficient to cover all buns. In this case, Bob should reduce the price for all `n` buns. The total profit is the sum of the reduced prices:
   \[
   \text{Profit} = \sum_{i=1}^{n} (b - i + 1) = \sum_{i=1}^{n} (b + 1 - i) = \sum_{i=1}^{n} (b + 1) - \sum_{i=1}^{n} i = n(b + 1) - \frac{n(n + 1)}{2}
   \]

The provided code correctly handles these cases and calculates the profit accordingly. Thus, the solution is correct.