Reasoning:  
The problem statement asks for the difference between the sum of cubes of the first n natural numbers and the sum of the first n natural numbers. The formula for the sum of the first n natural numbers is \( \text{sum\_n} = \frac{n(n + 1)}{2} \). The formula for the sum of the cubes of the first n natural numbers is \( (\text{sum\_n})^2 \). 

The program correctly calculates `sum_n` and then calculates `sum_cubes_n` as `sum_n ** 2`. However, the comment at the end of the program is incorrect. It states that the program returns \( (n * (n + 1) // 2) - (n * (n + 1) // 2) \), which would indeed simplify to 0. But this is not what the program does; it correctly returns \( (\text{sum\_n})^2 - \text{sum\_n} \).

To verify the correctness, we can check the test cases:
- For \( n = 3 \):
  - \( \text{sum\_n} = \frac{3 \times 4}{2} = 6 \)
  - \( \text{sum\_cubes\_n} = 6^2 = 36 \)
  - Difference: \( 36 - 6 = 30 \)

- For \( n = 5 \):
  - \( \text{sum\_n} = \frac{5 \times 6}{2} = 15 \)
  - \( \text{sum\_cubes\_n} = 15^2 = 225 \)
  - Difference: \( 225 - 15 = 210 \)

- For \( n = 2 \):
  - \( \text{sum\_n} = \frac{2 \times 3}{2} = 3 \)
  - \( \text{sum\_cubes\_n} = 3^2 = 9 \)
  - Difference: \( 9 - 3 = 6 \)

All test cases match the expected results, confirming that the program is correct.

Correctness: **True**