Let's break down the given Python code step by step:

1. **Initial State:**
   - `n` is an even and positive integer within the range [2, \(10^9\)]
   - `m` is an even and positive integer within the range [2, \(10^9\)]
   - `k` is an integer such that \(0 \leq k < n \cdot m\)
   - `k` has been updated to be `k % (n * 2 - 2)`, and its current value is less than `n * 2 - 2`
   - `k` is greater than or equal to `n - 1`

2. **Code Execution:**
   - The code prints the following expression:
     \[
     n - (k - n + 1) \% (n - 1) - 1, \quad (k - n + 1) // (n - 1) + 1
     \]

3. **Step-by-Step Calculation:**
   - First, let's focus on the first part of the print statement: \( n - (k - n + 1) \% (n - 1) - 1 \).
     - Since \( k \) is already updated to be `k % (n * 2 - 2)`, and it is less than `n * 2 - 2`, the modulo operation will not change the value of \( k \) in the context of `(n - 1)`.
     - Let's denote \( k' = k \% (n - 1) \), which is the remainder when \( k \) is divided by \( n - 1 \). Given the constraint \( n - 1 \leq k < n * 2 - 2 \), \( k' \) can range from \( n - 1 \) to \( n * 2 - 3 \).
     - Simplifying the expression:
       \[
       n - (k - n + 1) \% (n - 1) - 1 = n - k' - 1 = n - k - 1 + n - 1 = 2n - k - 2
       \]
   - Next, let's look at the second part of the print statement: \( (k - n + 1) // (n - 1) + 1 \).
     - Again, using \( k' \):
       \[
       (k - n + 1) // (n - 1) + 1 = k' // (n - 1) + 1
       \]
     - Given \( k' \) ranges from \( n - 1 \) to \( n * 2 - 3 \):
       - For \( k' = n - 1 \), \( k' // (n - 1) = 1 \), so the result is \( 1 + 1 = 2 \).
       - For \( k' = n \), \( k' // (n - 1) = 1 \), so the result is \( 1 + 1 = 2 \).
       - For \( k' = n + 1 \), \( k' // (n - 1) = 2 \), so the result is \( 2 + 1 = 3 \).
       - And so on up to \( k' = n * 2 - 3 \), \( k' // (n - 1) = 2 \), so the result is \( 2 + 1 = 3 \).

4. **Final Output State:**
   - From the above analysis, the output will be two numbers.
   - The first number will be \( 2n - k - 2 \).
   - The second number will be \( (k - n + 1) // (n - 1) + 1 \), which depends on the exact value of \( k \).

Since we know \( n \) and \( k \) but not their specific values, we can't simplify further without knowing \( n \) and \( k \). However, we can express the final output state as:

Output State: **`2n - k - 2`, `(k - n + 1) // (n - 1) + 1`**