The given code snippet updates the value of `dp[i]` using the formula `(dp[i - 1] + (i - 1) * dp[i - 2] * 2) % (10 ** 9 + 7)`. Given the initial state, `i` is 4, so we need to calculate `dp[4]`.

From the initial state:
- `dp[1]` is 1
- `dp[2]` is 3
- `dp[3]` can be calculated as `(dp[2] + (2) * dp[1] * 2) % (10 ** 9 + 7) = (3 + 2 * 1 * 2) % (10 ** 9 + 7) = 7`

Now, we calculate `dp[4]`:
- `dp[4] = (dp[3] + (3) * dp[2] * 2) % (10 ** 9 + 7) = (7 + 3 * 3 * 2) % (10 ** 9 + 7) = (7 + 18) % (10 ** 9 + 7) = 25`

The values of `t`, `n`, `k`, `num`, `m`, and the rest of the `dp` list remain unchanged except for `dp[4]` which is now 25.

Output State: **`t` is an integer such that 0 ≤ `t` ≤ 10^4, `n` is the first integer read from the input, 1 ≤ `n` ≤ 3 · 10^5, `k` is the second integer read from the input and must be greater than 0, `num` is the sum of 1 for each iteration where `c` equals `r` and 2 for each iteration where `c` does not equal `r` such that `n - num` is at least 2, `m` is `n - num` and `m` is not equal to 0 and `m` is not equal to 1, `dp` is a list of length `m + 1` with all elements initialized to 0 except `dp[1]` which is 1, `dp[2]` which is 3, `dp[3]` which is 7, and `dp[4]` which is 25, `i` is 4**