To calculate the new value of `dp[i]`, we use the given formula:

\[ dp[i] = (dp[i - 1] + (i - 1) * dp[i - 2] * 2) \% (10^9 + 7) \]

Given:
- `i` is 5
- `dp[1]` is 1
- `dp[2]` is 3
- `dp[3]` is 7
- `dp[4]` is 25

Substitute `i = 5` into the formula:

\[ dp[5] = (dp[4] + (5 - 1) * dp[3] * 2) \% (10^9 + 7) \]

\[ dp[5] = (25 + 4 * 7 * 2) \% (10^9 + 7) \]

\[ dp[5] = (25 + 56) \% (10^9 + 7) \]

\[ dp[5] = 81 \% (10^9 + 7) \]

\[ dp[5] = 81 \]

The other variables (`t`, `n`, `k`, `num`, `m`) remain unchanged.

Output State: **`t` is `t - 1` and is still greater than 0, `n` is the first integer read from the input, `k` is the second integer read from the input, `num` is the sum of 1s and 2s based on whether `c == r` or not across all `k` iterations, `m` is at least 3, `dp` is a list of length `m + 1` with `dp[1]` as 1, `dp[2]` as 3, `dp[3]` as 7, `dp[4]` as 25, and `dp[5]` as 81, `i` is 5**