The value of `sum_k` is calculated as `k * (k + 1) // 2`. The variable `k` is defined as `a + b - 1`. Therefore, `sum_k` will be equal to `(a + b - 1) * (a + b) // 2`.

The precondition states that `m` is a positive integer such that 1 <= `m` <= 10^9; `a` is a positive integer such that 1 <= `a` <= 10^5; `b` is a positive integer such that 1 <= `b` <= 10^5; `g` is equal to 1; `k` is equal to `a + b - 1`; and `m` is greater than or equal to `k`. The values of `m`, `g`, and the conditions on `a`, `b`, and `k` remain unchanged.

After executing the code, we introduce a new variable `sum_k`, and the other variables retain their original values. 

Output State: **`m` is a positive integer such that 1 <= `m` <= 10^9; `a` is a positive integer such that 1 <= `a` <= 10^5; `b` is a positive integer such that 1 <= `b` <= 10^5; `g` is equal to 1; `k` is equal to `a + b - 1`; `sum_k` is equal to `(a + b - 1) * (a + b) // 2`**.