Reasoning:  
To solve the problem, we need to compute two things:
1. The sum of the first `n` natural numbers.
2. The sum of the cubes of the first `n` natural numbers.

The formula for the sum of the first `n` natural numbers is:
\[ \text{sum\_n} = \frac{n \times (n + 1)}{2} \]

The formula for the sum of the cubes of the first `n` natural numbers is:
\[ \text{sum\_cubes\_n} = \left( \frac{n \times (n + 1)}{2} \right)^2 \]

The function `func_1` correctly calculates these values and returns the difference between the sum of the cubes and the sum of the first `n` natural numbers.

Let's verify the test cases:
- For \( n = 3 \):
  \[ \text{sum\_n} = \frac{3 \times 4}{2} = 6 \]
  \[ \text{sum\_cubes\_n} = 6^2 = 36 \]
  \[ \text{result} = 36 - 6 = 30 \]
  This matches the expected output.

- For \( n = 5 \):
  \[ \text{sum\_n} = \frac{5 \times 6}{2} = 15 \]
  \[ \text{sum\_cubes\_n} = 15^2 = 225 \]
  \[ \text{result} = 225 - 15 = 210 \]
  This matches the expected output.

- For \( n = 2 \):
  \[ \text{sum\_n} = \frac{2 \times 3}{2} = 3 \]
  \[ \text{sum\_cubes\_n} = 3^2 = 9 \]
  \[ \text{result} = 9 - 3 = 6 \]
  This matches the expected output.

Since all the test cases are correct and the logic of the function is sound, the program is correct.

Correctness: **True**