First, let's analyze the initial state and the code snippet:

Initial State: 
- \( j = \frac{n}{2} \)
- \(\text{max\_size} = \frac{n}{2} + 1 \)
- \( h = [] \)
- \(\text{output} = (h[0], 1) \text{ if } h[0] \geq \left( \left( \frac{n}{2} - 1 \right) \times \text{smallest element in } h \right), \text{ otherwise } \text{output} = \left( \left( \frac{n}{2} - 1 \right) \times \text{smallest element in } h, \frac{n}{2} - 1 \right)\)

Code Snippet:
```python
print(output[0], output[1])
```

Step-by-step analysis:
1. The code simply prints the values of `output[0]` and `output[1]`.
2. Since `h` is initially an empty list, `h[0]` does not exist, meaning that the condition for the assignment of `output` cannot be evaluated as `True`. Thus, the default value of `output` is used.

Therefore, the value of `output` remains as specified in the initial state:
- \(\text{output} = \left( \left( \frac{n}{2} - 1 \right) \times \text{smallest element in } h, \frac{n}{2} - 1 \right)\)

Since `h` is empty, the smallest element in `h` does not exist, which implies that the second part of the ternary operator is used:
- \(\text{output} = \left( \left( \frac{n}{2} - 1 \right) \times 0, \frac{n}{2} - 1 \right) = \left( 0, \frac{n}{2} - 1 \right)\)

Thus, when the code is executed, it will print `0` and \(\frac{n}{2} - 1\).

Output State: **`j = \frac{n}{2}`, `max_size` = \(\frac{n}{2} + 1\), `h` = [], `output` = (0, \(\frac{n}{2} - 1\))**