The code sets `low` to `mid + 1`. From the initial state, we know that `mid` is `(low + high) // 2`. Since `low = mid + 1`, we can substitute the expression for `mid` into this equation.

Given:
- `low` must be 0 or `(0 + high) // 2 + 1`.
- `high` must be such that `low <= high` holds true.
- `mid` is `(low + high) // 2`.

Let's substitute `mid` in the equation `low = mid + 1`:
\[ \text{low} = \left(\frac{\text{low} + \text{high}}{2}\right) + 1 \]

Since `low` is initially set to 0 or `(0 + high) // 2 + 1`, let's consider both cases:

1. If `low` is 0:
   \[ 0 = \left(\frac{0 + \text{high}}{2}\right) + 1 \]
   This simplifies to:
   \[ 0 = \frac{\text{high}}{2} + 1 \]
   Which implies:
   \[ \text{high} = -2 \]
   But since `high` must be non-negative and `low <= high`, this case is invalid.

2. If `low` is `(0 + high) // 2 + 1`:
   \[ (0 + \text{high}) // 2 + 1 = \left(\frac{(0 + \text{high}) // 2 + 1 + \text{high}}{2}\right) + 1 \]
   Simplifying the right side:
   \[ (0 + \text{high}) // 2 + 1 = \left(\frac{(0 + \text{high}) // 2 + \text{high} + 1}{2}\right) + 1 \]
   Let \( \text{high} = 2k \) (since high must be even for the division to work correctly):
   \[ k + 1 = \left(\frac{k + 2k + 1}{2}\right) + 1 \]
   \[ k + 1 = \left(\frac{3k + 1}{2}\right) + 1 \]
   \[ k + 1 = \frac{3k + 3}{2} \]
   Multiplying both sides by 2:
   \[ 2k + 2 = 3k + 3 \]
   \[ 2k + 2 = 3k + 3 \]
   \[ k = -1 \]
   Again, this implies an invalid value for `high`.

Given these considerations, we conclude that the only valid scenario is where `low` is set to a value that satisfies the condition and updates correctly after setting `low = mid + 1`.

Therefore, the output state is:
Output State: **`data` is a list with at least 3 elements, `idx` is `idx + 3`, `low` is `mid + 1`, `high` is unchanged, `mid` is unchanged.**