Given the initial state and the code snippet, we need to determine the new state after the code is executed. The key is to calculate the value of `mid` based on the provided initial conditions.

Initial State: 
- `n` must be greater than 3
- `low` is either 0 or `(n - 1) // 2`
- `high` is either `(n - 1) // 2` or `n - 1`

The code snippet:
```python
mid = (low + high) // 2
```

Let's consider the possible values of `low` and `high`:

1. If `low` is 0 and `high` is `(n - 1) // 2`, then:
   \[
   mid = (0 + (n - 1) // 2) // 2 = (n - 1) // 4
   \]

2. If `low` is `(n - 1) // 2` and `high` is `n - 1`, then:
   \[
   mid = ((n - 1) // 2 + (n - 1)) // 2 = ((n - 1) // 2 + (n - 1)) // 2
   \]
   Simplifying the above expression:
   \[
   mid = (2 \cdot (n - 1) // 2 + (n - 1) % 2) // 2 = (n - 1 + (n - 1) % 2) // 2
   \]
   If `n - 1` is even, then `(n - 1) % 2` is 0, so:
   \[
   mid = (n - 1) // 2
   \]
   If `n - 1` is odd, then `(n - 1) % 2` is 1, so:
   \[
   mid = (n - 1 + 1) // 2 = n // 2
   \]

Thus, `mid` can be either `(n - 1) // 4` or `(n - 1) // 2` or `n // 2` depending on the values of `low` and `high`.

Output State: **`n` must be greater than 3, `low` is either 0 or `(n - 1) // 2`, `high` is either `(n - 1) // 2` or `n - 1`, `mid` is either `(n - 1) // 4` or `(n - 1) // 2` or `n // 2`**.