The value of `cnt` is incremented by the minimum of two expressions: `n // ((x + y) * x)` and `m // ((x + y) * y)`. Given the initial state:

- `n` must be at least 15
- `m` must be at least 10
- `x` is 3
- `y` is 2
- `cnt` remains unchanged (let's assume `cnt` is initially 0, as no specific value is given)

First, calculate `(x + y) * x` and `(x + y) * y`:
- `(x + y) * x = (3 + 2) * 3 = 5 * 3 = 15`
- `(x + y) * y = (3 + 2) * 2 = 5 * 2 = 10`

Next, calculate `n // 15` and `m // 10`:
- Since `n` is at least 15, `n // 15` is at least 1.
- Since `m` is at least 10, `m // 10` is at least 1.

The minimum of these two values is 1. Therefore, `cnt` is incremented by 1.

Output State: **`n` must be at least 15, `m` must be at least 10, `x` is 3, `y` is 2, `cnt` is 1**.