Output State: **`ls` is 0, `t` is a positive integer such that \(1 \leq t \leq 10^4\), `N` is an input integer, `n` is a positive integer such that \(1 \leq n \leq 2 \cdot 10^5\), `a_1, a_2, ..., a_n` is a list of \(n\) integers where \(1 \leq a_i \leq 10^9\), `nums` is a sorted list of integers, `i` is 3, and `nums[i]` is now equal to `nums[i] - ls`.**

Explanation: The code `nums[i] -= ls` subtracts the value of `ls` from `nums[i]`. Given that `ls` is defined as `nums[0] + nums[i]` and `i` is 3, the expression `nums[i]` initially is `nums[3]`. Thus, `nums[3]` is decreased by `nums[0] + nums[3]`, making `nums[3]` equal to `nums[3] - (nums[0] + nums[3])`, which simplifies to `-nums[0]`. However, since `ls` is defined as `nums[0] + nums[3]`, when `ls` is subtracted from `nums[3]`, `nums[3]` becomes 0. All other variables remain unchanged.