To determine what will be printed by the given `print` statement, let's break down the initial state and the operations step by step:

### Initial State:
- `s` is a string of length `n` (1 ≤ n ≤ 5 · 10^5) consisting of characters '<' and '>'.
- `n` is the length of `s` and must be greater than 2.
- `A` contains the cumulative counts of '>' characters encountered, adjusted by their positions and the number of previous '>' characters.
- `idx_A` contains the indices of all '>' characters in `s`.
- `B` contains the cumulative counts of '<' characters encountered from the end of the string, adjusted by their positions and the number of previous '<' characters.
- `idx_B` contains the indices of all '<' characters in `s` in reverse order.
- `j` is `n`.
- `i` is `2`.
- `l - r - 1 > 0` if initially true, `r` is one less than its original value.
- `a` is `B[r]`.
- `b` is updated to `A[l - 1] - A[l - r - 2] - (idx_A[l - 1] - idx_A[l - r - 2]) * (l - r - 1)`.
- `b` is further updated to `b + (i - idx_A[l - 1]) * (r + 1)`.
- If `l - r - 1 <= 0`, `r`, `a`, and `b` remain unchanged, and `b` is updated to `b + (i - idx_A[l - 1]) * (r + 1)`.

### Step-by-Step Calculation:
1. **Determine `l` and `r`:**
   - `l` is the length of `idx_A` (number of '>' characters).
   - `r` is the length of `idx_B` (number of '<' characters).

2. **Check the condition `l - r - 1 > 0`:**
   - If true, `r` is decremented by 1.
   - If false, `r` remains unchanged.

3. **Calculate `a` and `b`:**
   - `a` is `B[r]`.
   - `b` is initially `A[l - 1] - A[l - r - 2] - (idx_A[l - 1] - idx_A[l - r - 2]) * (l - r - 1)`.
   - `b` is then updated to `b + (i - idx_A[l - 1]) * (r + 1)`.

4. **Final Calculation:**
   - The expression `a * 2 + b * 2 + (n - i)` is evaluated.

### Example Calculation:
Let's assume a specific example to illustrate the calculation:
- `s = "><><"`
- `n = 4`
- `A = [0, 1, 1, 2]` (cumulative counts of '>' characters)
- `idx_A = [1, 3]` (indices of '>' characters)
- `B = [0, 1, 1, 2]` (cumulative counts of '<' characters from the end)
- `idx_B = [2, 0]` (indices of '<' characters in reverse order)

1. **Determine `l` and `r`:**
   - `l = 2` (length of `idx_A`)
   - `r = 2` (length of `idx_B`)

2. **Check the condition `l - r - 1 > 0`:**
   - `l - r - 1 = 2 - 2 - 1 = -1` (false)
   - `r` remains `2`.

3. **Calculate `a` and `b`:**
   - `a = B[r] = B[2] = 1`
   - `b = A[l - 1] - A[l - r - 2] - (idx_A[l - 1] - idx_A[l - r - 2]) * (l - r - 1)`
     - `A[l - 1] = A[1] = 1`
     - `A[l - r - 2] = A[1 - 2 - 2] = A[-3]` (out of bounds, so we need to handle this case carefully)
     - Since `l - r - 1 <= 0`, we skip the subtraction part and directly update `b`:
     - `b = 1 + (i - idx_A[l - 1]) * (r + 1)`
     - `i = 2`
     - `idx_A[l - 1] = idx_A[1] = 3`
     - `b = 1 + (2 - 3) * (2 + 1) = 1 + (-1) * 3 = 1 - 3 = -2`

4. **Final Calculation:**
   - `a * 2 + b * 2 + (n - i) = 1 * 2 + (-2) * 2 + (4 - 2) = 2 - 4 + 2 = 0`

### Final Output:
Output: **0**