To analyze the code, we have the following variables:

- `n` is a positive integer (1 <= n <= 1000)
- `a` is a list of `n` integers (1 <= `a_i` <= 100)
- `min_cost` is float('inf')
- `best_t` is -1
- `t` is 1
- `current_cost` is 0
- `length` is greater than or equal to `t - 1` (0) and currently, `length` is greater than `t + 1` (2)

Now, looking at the code:
```
current_cost += length - (t + 1)
```

We can simplify the expression:
- Since `t` is 1, then `t + 1` is 2.
- Therefore, the expression becomes `current_cost += length - 2`.

Given that `length` is greater than 2, we know that `(length - 2)` is a positive value.

After executing the code:
- The value of `current_cost` will increase by a positive amount, which results from `length - 2`.

Since the other variables haven't changed, the output state will be:
Output State: **`n` is a positive integer (1 <= n <= 1000), `a` is a list of `n` integers (1 <= `a_i` <= 100), `min_cost` is float('inf'), `best_t` is -1, `t` is 1, `current_cost` is a positive value greater than 0, and `length` is greater than or equal to 2.**