Let's break down the initial state and the print statement step by step:

1. **Initial State:**
   - `p1`, `p2`, and `p3` are integers where \(0 \leq p1 \leq p2 \leq p3 \leq 30\).
   - `t` is greater than 0 (though `t` is not used in the print statement).
   - `_` is 0 (though `_` is not used in the print statement).
   - `x` is 0.
   - `y` is equal to `p3`.
   - The current value of `p1 - x` is less than or equal to `p2 - y`.

2. **Print Statement:**
   ```
   print(p1 - x + p3)
   ```

3. **Variable Values:**
   - `x` is 0.
   - `y` is equal to `p3`.
   - `p1 - x` simplifies to `p1` because `x` is 0.
   - `p2 - y` simplifies to `p2 - p3`.

4. **Condition:**
   - The condition `p1 - x <= p2 - y` simplifies to `p1 <= p2 - p3`.

5. **Expression to Print:**
   - The expression `p1 - x + p3` simplifies to `p1 + p3` because `x` is 0.

6. **Final Output:**
   - The print statement will output the value of `p1 + p3`.

Given the initial state and the conditions, the value of `p1 + p3` will be printed. Since `p1` and `p3` are integers within the specified range and `p1 + p3` is a straightforward sum of these two integers, the output will be the sum of `p1` and `p3`.

Output: **p1 + p3 (where p1 and p3 are integers such that 0 ≤ p1 ≤ p2 ≤ p3 ≤ 30 and p1 ≤ p2 - p3)**