Let's break down the given initial state and the print statement to determine what will be printed:

1. **Variables and their values:**
   - `p1`, `p2`, and `p3` are integers such that \(0 \leq p1 \leq p2 \leq p3 \leq 30\).
   - `t` is greater than 1 (though it's not used in the print statement).
   - `_` is 1 (though it's not used in the print statement).
   - The sum of `p1`, `p2`, and `p3` is even.
   - `y` is `p3`.
   - `x` is 0.
   - The current value of `p1 - x` is less than or equal to `p2 - y`.

2. **Understanding the conditions:**
   - Since `x` is 0, `p1 - x` simplifies to `p1`.
   - Since `y` is `p3`, `p2 - y` simplifies to `p2 - p3`.
   - The condition `p1 - x <= p2 - y` becomes `p1 <= p2 - p3`.

3. **Print statement:**
   - The print statement is `print(p1 - x + p3)`.
   - Substituting the values, this becomes `print(p1 + p3)`.

4. **Determining the output:**
   - Given that `p1` and `p3` are integers and `p1 <= p2 - p3`, we need to consider the possible values of `p1` and `p3`.
   - Since `p1` and `p3` are part of the list of integers where \(0 \leq p1 \leq p2 \leq p3 \leq 30\) and the sum of `p1`, `p2`, and `p3` is even, the value of `p1 + p3` will also be an integer.
   - The condition `p1 <= p2 - p3` ensures that `p1` is not greater than the difference between `p2` and `p3`.

Therefore, the print statement will output the sum of `p1` and `p3`.

Output: **p1 + p3 (where p1 and p3 are integers such that 0 ≤ p1 ≤ p2 ≤ p3 ≤ 30, the sum of p1, p2, and p3 is even, and p1 ≤ p2 - p3)**