The code snippet `s -= 1 if b[j] else 0` means that if `b[j]` is `True` (or non-zero), `s` is decremented by 1; otherwise, `s` remains unchanged. The other variables `j` and `i` are not affected.

Given the initial state:
- \( j \geq i \)
- \( s < j - i + 1 \)

After executing the code, the value of `s` will be:
- If `b[j]` is `True` (or non-zero), then \( s = s - 1 \).
- If `b[j]` is `False` (or zero), then \( s \) remains unchanged.

Therefore, the output state is:
Output State: **\( j \geq i \); \( s \leq j - i \)**