Output State: **`n` is a positive integer (1 ≤ n ≤ 3 · 10^5), `i` is 3, `ones[1]` is `ones[0] + (1 if nums[0] == 1 else 0)`, `sum[1]` is `sum[0] + nums[0] - 1`, `ones[2]` is `ones[1] + (1 if nums[1] == 1 else 0)`, `sum[2]` is `sum[1] + nums[1] - 1`, `ones[3]` is `ones[2] + (1 if nums[2] == 1 else 0)`, `sum[3]` is `sum[2] + nums[2] - 1`.**

Explanation: The code snippet updates the value of `sum[3]` based on the previous value of `sum[2]` and the value of `nums[2]`. The value of `sum[3]` is calculated as `sum[2] + nums[2] - 1`. All other variables and conditions remain unchanged.