To determine the output state after the loop has executed, let's break down the given information and the loop logic:

### Initial State:
- `main_ar` and `sec_arr` remain unchanged.
- `sub_summ` is the sum of the first integers of all tuples in `sec_arr`.

### Loop Code:
```python
for val_b in main_ar:
    if val_b[0] + val_b[1] >= 0:
        sub_summ += val_b[0] + val_b[1]
```

### Analysis:
1. **Initial `sub_summ` Calculation:**
   - `sub_summ` starts as the sum of the first integers of all tuples in `sec_arr`.

2. **Loop Execution:**
   - The loop iterates over each tuple `val_b` in `main_ar`.
   - For each tuple `val_b`, it checks if the sum of the first and second elements (`val_b[0] + val_b[1]`) is greater than or equal to 0.
   - If the condition is true, it adds the sum of the first and second elements to `sub_summ`.

### Output State:
- `main_ar` and `sec_arr` remain unchanged.
- `sub_summ` will be the sum of the first integers of all tuples in `sec_arr` plus the sum of the first and second elements of all tuples in `main_ar` where the sum is greater than or equal to 0.

### Example:
Suppose:
- `main_ar = [(1, 2), (-3, 4), (5, -6), (0, 0)]`
- `sec_arr = [(10, 20), (30, 40)]`

**Initial `sub_summ` Calculation:**
- `sub_summ = 10 + 30 = 40`

**Loop Execution:**
- For `val_b = (1, 2)`: `1 + 2 = 3` (>= 0), so `sub_summ += 3` → `sub_summ = 43`
- For `val_b = (-3, 4)`: `-3 + 4 = 1` (>= 0), so `sub_summ += 1` → `sub_summ = 44`
- For `val_b = (5, -6)`: `5 + (-6) = -1` (< 0), so no change → `sub_summ = 44`
- For `val_b = (0, 0)`: `0 + 0 = 0` (>= 0), so `sub_summ += 0` → `sub_summ = 44`

### Final Output State:
- `main_ar` remains `[(1, 2), (-3, 4), (5, -6), (0, 0)]`
- `sec_arr` remains `[(10, 20), (30, 40)]`
- `sub_summ` is `44`

Output State: **`main_ar` and `sec_arr` remain unchanged, and `sub_summ` is the sum of the first integers of all tuples in `sec_arr` plus the sum of the first and second elements of all tuples in `main_ar` where the sum is greater than or equal to 0.**