The code snippet `a[l] -= a[r]` modifies the value of `a[l]` by subtracting the value of `a[r]` from it. Let's break down the changes:

- `a[l]` is updated to `a[l] - a[r]`.
- All other variables (`n`, `k`, `a`, `l`, `r`, `sunks`) remain unchanged.

Given the initial state:
- `n` and `k` are positive integers where 1 ≤ `n` ≤ 2 · 10^5 and 1 ≤ `k` ≤ 10^15.
- `a` is a list of `n` positive integers where 1 ≤ `a_i` ≤ 10^9.
- `l` is 0, 1, or 2.
- `r` is `n - 1`, `n - 2`, or `n - 3`.
- `sunks` is 0, 1, 2, or 3.
- `k` is now `k - (a[r] * 2)`.

After executing the code snippet:
- `a[l]` is now `a[l] - a[r]`.

Output State: **`n` and `k` are positive integers where 1 ≤ `n` ≤ 2 · 10^5 and 1 ≤ `k` ≤ 10^15, `a` is a list of `n` positive integers where 1 ≤ `a_i` ≤ 10^9, `l` is 0, 1, or 2, `r` is `n - 1`, `n - 2`, or `n - 3`, `sunks` is 0, 1, 2, or 3, `k` is `k - (a[r] * 2)`, and `a[l]` is `a[l] - a[r]`.**