Let's break down the initial state and the code snippet step by step:

1. **Initial State:**
   - `n = 0`
   - `h = (n - k + 1) // (n - k + 1) + (n - k + 1) // 1`
   - `costs = [n - k + 1, 1]`
   - `h` is greater than or equal to `k`

2. **Calculate `h`:**
   - Given `n = 0`, the expression for `h` becomes:
     \[
     h = (0 - k + 1) // (0 - k + 1) + (0 - k + 1) // 1
     \]
   - Simplify the expression:
     \[
     h = (1 - k) // (1 - k) + (1 - k) // 1
     \]
   - Since `(1 - k) // (1 - k)` is 1 (assuming `k` is not 1, because division by zero is undefined):
     \[
     h = 1 + (1 - k) // 1
     \]
   - `(1 - k) // 1` is simply `1 - k`:
     \[
     h = 1 + (1 - k)
     \]
   - Simplify further:
     \[
     h = 2 - k
     \]

3. **Check the condition `h >= k`:**
   - We need to ensure that `2 - k >= k`:
     \[
     2 - k \ge k
     \]
   - Rearrange the inequality:
     \[
     2 \ge 2k
     \]
   - Simplify:
     \[
     1 \ge k
     \]
   - This implies that `k` must be 1 or less. However, if `k` were 1, the division by zero would occur in the initial calculation of `h`. Therefore, `k` must be 0.

4. **Substitute `k = 0` into the expression for `h`:**
   - If `k = 0`:
     \[
     h = 2 - 0 = 2
     \]

5. **Verify the condition `h >= k`:**
   - With `k = 0` and `h = 2`, the condition `h >= k` is satisfied (`2 >= 0`).

6. **Output:**
   - The code snippet `print('YES')` will execute because the condition `h >= k` is true.

Output: **YES**