Let's break down the initial state and the provided code snippet to determine what will be printed.

### Initial State:
- `t` is an input integer such that \(0 \leq t \leq 10^4 - 1\).
- `n` is an integer where \(1 \leq n \leq 3 \cdot 10^5\).
- `k` is an integer where \(1 \leq k \leq n\).
- `i` is defined as \(k - 1\).
- `num` is the sum of 1 for each move where `c` equals `r` and 2 for each move where `c` does not equal `r`.
- `m` is defined as \(n - num\).
- `m` is explicitly stated to be 1.

### Analysis:
1. **`m` is explicitly stated to be 1**:
   - This means that the value of `m` is 1, regardless of the values of `n` and `num`.

2. **`m` is defined as \(n - num\)**:
   - Given that `m` is 1, we can write the equation:
     \[
     n - num = 1
     \]
   - Rearranging this equation, we get:
     \[
     num = n - 1
     \]

3. **`num` is the sum of 1 for each move where `c` equals `r` and 2 for each move where `c` does not equal `r`**:
   - Let's denote the number of moves where `c` equals `r` as \(x\) and the number of moves where `c` does not equal `r` as \(y\).
   - The total number of moves is \(x + y = n\).
   - The value of `num` can be expressed as:
     \[
     num = x \cdot 1 + y \cdot 2
     \]
   - Substituting \(num = n - 1\) into the equation, we get:
     \[
     n - 1 = x + 2y
     \]
   - Since \(x + y = n\), we can substitute \(x = n - y\) into the equation:
     \[
     n - 1 = (n - y) + 2y
     \]
     \[
     n - 1 = n + y
     \]
     \[
     y = -1
     \]
   - This result is not possible because \(y\) must be a non-negative integer. Therefore, the only feasible solution is that \(y = 0\) and \(x = n - 1\).

4. **Conclusion**:
   - `num` is \(n - 1\).
   - `m` is 1.
   - The `print` statement will print the value 1.

### Final Output:
Output: **1**