The code snippet `h -= (h + 1) // 2` updates the value of `h` by subtracting the result of `(h + 1) // 2` from the current value of `h`. Let's break down the impact:

- `h` is initially set to `n`.
- The expression `(h + 1) // 2` calculates the integer division of `h + 1` by 2.
- This result is then subtracted from `h`.

Given the initial state:
- `h` is `n`.
- `n` is an integer such that 1 ≤ k ≤ n ≤ 10^9.
- `k` is greater than `(n + 1) // 2`.

Let's calculate the new value of `h`:
- `h` is initially `n`.
- `(h + 1) // 2` is equivalent to `(n + 1) // 2`.
- Therefore, `h -= (h + 1) // 2` becomes `h -= (n + 1) // 2`.

So, the new value of `h` is:
- `h = n - (n + 1) // 2`.

Since `n` is an integer, `(n + 1) // 2` is the integer division of `n + 1` by 2, which is approximately half of `n` (rounded down).

Thus, the new value of `h` is:
- `h = n - (n + 1) // 2`.

For example, if `n` is 7:
- `(n + 1) // 2` is `(7 + 1) // 2` which is 4.
- `h` becomes `7 - 4` which is 3.

Therefore, the updated value of `h` is `n - (n + 1) // 2`.

Output State: **`t` is an integer such that 1 ≤ t ≤ 5 · 10^4, `n` and `k` are integers such that 1 ≤ k ≤ n ≤ 10^9, `s` is `k`, `i` is at least 2, `d` is 0, `h` is `n - (n + 1) // 2`, `p` is 1, `g` is `(n + 1) // 2`, and `k` is greater than `(n + 1) // 2`.**