The code snippet `s += (d + 1) // 2` updates the value of `s` by adding the result of `(d + 1) // 2` to its current value. Let's break down the impact of this code:

1. **Initial Value of `s`:** `s` is initially defined as `(d + 1) // 2 + (d + 1) // 2`.
2. **Expression `(d + 1) // 2`:** This expression calculates the integer division of `(d + 1)` by 2.
3. **Update `s`:** The new value of `s` is the sum of its initial value and the result of `(d + 1) // 2`.

Let's calculate the new value of `s`:

- Initial `s` = `(d + 1) // 2 + (d + 1) // 2`
- New `s` = `(d + 1) // 2 + (d + 1) // 2 + (d + 1) // 2`

Simplifying the expression:
- New `s` = `3 * ((d + 1) // 2)`

Therefore, the output state is:

Output State: **`t` is an integer such that 1 ≤ t ≤ 5 · 10^4, `n` and `k` are integers such that 1 ≤ k ≤ n ≤ 10^9, `n` and `k` are the values read from the input, `s` is `3 * ((d + 1) // 2)`, `i` is 2, `d` is an integer such that 0 < d < k - 1, `h` is `n`, `p` is 1, `g` is 0, `f` is undefined, `y` is undefined.**