Output State: The value of `sum` will be the sum calculated by the loop for the given `n`. Since the loop runs from `i = 2` to `i = n`, the final value of `sum` will be the result of the expression \((i * i - (i - 1) * (i - 1)) * i\) for each `i` from 2 to `n`, summed up. The variable `j` remains `n+1` as it is not affected by the loop. The variable `i` will be `n+1` after the loop completes, and `n` will remain unchanged as it is an input parameter.

For example, if `n` is 5, the loop will run 4 times (for `i = 2, 3, 4, 5`), and the final `sum` will be calculated as follows:
- For `i = 2`: \(2^2 - 1^2) * 2 = 6\)
- For `i = 3`: \(3^2 - 2^2) * 3 = 15\)
- For `i = 4`: \(4^2 - 3^2) * 4 = 28\)
- For `i = 5`: \(5^2 - 4^2) * 5 = 45\)

So, `sum` will be \(6 + 15 + 28 + 45 = 94\).

Therefore, the output state after the loop executes all the iterations is: `sum` is 94, `j` is `n+1`, `i` is `n+1`, `n` is the original input integer.