Reasoning:

The provided solution aims to reconstruct the permutation `p` from the array `a` using the relationship \( a_i = \texttt{MEX}(p_1, p_2, \ldots, p_i) - p_i \). The key idea is to work backwards from the last element of `a` to the first, maintaining the current value of `mex` (the minimum excluded value).

Here's a step-by-step breakdown of the logic:

1. **Initialization**: 
   - `mex` is initialized to `n`, which is the maximum possible value for the MEX of the entire permutation.
   - `res` is initialized as a list of `None` values with length `n`.

2. **Backward Iteration**:
   - The loop iterates from the last element of `ar` to the first.
   - For each index `i`, the value `res[i]` is set to `mex - ar[i]`.
   - `mex` is then updated to `mex - ar[i]` if this new value is smaller than the current `mex`.

3. **Output**:
   - After constructing the `res` list, it is printed as a space-separated string.

### Verification of Logic:

- **MEX Calculation**: The MEX of a sequence is the smallest non-negative integer not present in the sequence. By starting `mex` at `n` and decrementing it based on the values in `ar`, the algorithm ensures that `mex` is always the correct MEX for the subsequence up to the current index.
- **Permutation Construction**: The value `res[i]` is calculated as `mex - ar[i]`, which correctly reconstructs the permutation `p` because it aligns with the given relationship \( a_i = \texttt{MEX}(p_1, p_2, \ldots, p_i) - p_i \).
- **Update of `mex`**: The update `mex = mex - ar[i]` ensures that `mex` is always the smallest non-negative integer not yet used in the permutation.

### Edge Cases:

- **Single Element Permutation**: For `n = 1`, the algorithm works correctly as `mex` starts at 1 and `res[0]` is set to `1 - ar[0]`.
- **Multiple Test Cases**: The function handles multiple test cases by iterating over the number of test cases and processing each one independently.

### Example Verification:

- **Test Case 1**: 
  - Input: `5\n1 1 -2 1 2`
  - Output: `0 1 4 2 3`
  - Explanation: 
    - `a_5 = 2` implies `p_5 = 3` (since `mex = 5` initially and `5 - 2 = 3`).
    - `a_4 = 1` implies `p_4 = 2` (since `mex = 3` now and `3 - 1 = 2`).
    - `a_3 = -2` implies `p_3 = 4` (since `mex = 2` now and `2 - (-2) = 4`).
    - `a_2 = 1` implies `p_2 = 1` (since `mex = 0` now and `0 - 1 = 1`).
    - `a_1 = 1` implies `p_1 = 0` (since `mex = 1` now and `1 - 1 = 0`).

- **Test Case 2**:
  - Input: `5\n1 1 1 1 1`
  - Output: `0 1 2 3 4`
  - Explanation: 
    - `a_5 = 1` implies `p_5 = 4` (since `mex = 5` initially and `5 - 1 = 4`).
    - `a_4 = 1` implies `p_4 = 3` (since `mex = 4` now and `4 - 1 = 3`).
    - `a_3 = 1` implies `p_3 = 2` (since `mex = 3` now and `3 - 1 = 2`).
    - `a_2 = 1` implies `p_2 = 1` (since `mex = 2` now and `2 - 1 = 1`).
    - `a_1 = 1` implies `p_1 = 0` (since `mex = 1` now and `1 - 1 = 0`).

- **Test Case 3**:
  - Input: `3\n-2 1 2`
  - Output: `2 0 1`
  - Explanation: 
    - `a_3 = 2` implies `p_3 = 1` (since `mex = 3` initially and `3 - 2 = 1`).
    - `a_2 = 1` implies `p_2 = 0` (since `mex = 2` now and `2 - 1 = 0`).
    - `a_1 = -2` implies `p_1 = 2` (since `mex = 1` now and `1 - (-2) = 2`).

### Conclusion:

The provided solution correctly reconstructs the permutation `p` from the array `a` based on the given problem constraints and examples. Therefore, the program is correct.

Correctness: **True**