Alright, I've got this problem to solve. Let's see what it's asking for. So, I'm given an array of integers, and I need to find the number of tuples (x, y, z) where 1 ≤ x ≤ y ≤ z ≤ n, and f(x, y) XOR f(y, z) is greater than f(x, z). Here, f(l, r) is the XOR of all elements from a_l to a_r.

First, I need to understand what f(x, y) represents. It's the XOR of elements from a_x to a_y. Similarly, f(y, z) is the XOR from a_y to a_z, and f(x, z) is the XOR from a_x to a_z.

So, the condition is f(x, y) XOR f(y, z) > f(x, z).

I need to find all tuples (x, y, z) with x ≤ y ≤ z that satisfy this condition.

Let me think about the properties of XOR. XOR is associative and commutative, which might help simplify the expression.

Let's see:

f(x, y) = a_x to a_y XOR

f(y, z) = a_y to a_z XOR

So, f(x, y) XOR f(y, z) = (a_x to a_y) XOR (a_y to a_z)

Since XOR is associative, this is equal to a_x to a_z, which is f(x, z).

Wait, that can't be right because then f(x, y) XOR f(y, z) would be equal to f(x, z), and the condition is that it's greater than f(x, z). But if they are equal, then how can one be greater than the other?

Hmm, maybe I'm missing something here.

Let me recall that XOR compares each bit and returns 1 if the bits are different and 0 if they are the same. So, when I say A XOR B > A, it means that the numerical value of A XOR B is greater than A.

Wait, but in this case, f(x, y) XOR f(y, z) is being compared to f(x, z).

Given that f(x, y) XOR f(y, z) equals f(x, z), as per the earlier thought, but according to the problem, we need f(x, y) XOR f(y, z) > f(x, z), which would never be true if they are equal.

But looking back at the example, there are cases where the condition holds. So, maybe my assumption is wrong.

Let me check the example provided:

For the array [6, 2, 4]:

- Tuple (1,2,2): f(1,2) = 6 XOR 2 = 4, f(2,2) = 2, f(1,2) XOR f(2,2) = 4 XOR 2 = 6, which is greater than f(1,2) = 4.

- Tuple (1,1,3): f(1,1) = 6, f(1,3) = 6 XOR 2 XOR 4 = 0, f(1,1) XOR f(1,3) = 6 XOR 0 = 6, which is greater than f(1,3) = 0.

- Tuple (1,2,3): f(1,2) = 4, f(2,3) = 2 XOR 4 = 6, f(1,2) XOR f(2,3) = 4 XOR 6 = 2, which is greater than f(1,3) = 0.

- Tuple (1,3,3): f(1,3) = 0, f(3,3) = 4, f(1,3) XOR f(3,3) = 0 XOR 4 = 4, which is greater than f(1,3) = 0.

So, in these cases, f(x, y) XOR f(y, z) is indeed greater than f(x, z). But according to my earlier thought, f(x, y) XOR f(y, z) should be equal to f(x, z), but in the example, it's greater in some cases. So, perhaps my understanding is incorrect.

Let me double-check the XOR properties.

Given that f(x, y) is a XOR b XOR ... up to y, and f(y, z) is b XOR c XOR ... up to z, then f(x, y) XOR f(y, z) should be a XOR c XOR ... depending on the overlap.

Wait, perhaps I need to think differently.

Let me consider that f(x, y) XOR f(y, z) = f(x, z), as per the properties of XOR on overlapping ranges.

But according to the problem, we need f(x, y) XOR f(y, z) > f(x, z), which would imply f(x, z) > f(x, z), which is impossible unless f(x, y) XOR f(y, z) is not equal to f(x, z). But according to XOR properties, it should be equal.

This confusion suggests that maybe I'm misunderstanding the definition or the properties.

Wait, perhaps f(x, y) XOR f(y, z) is not necessarily equal to f(x, z). Let me verify with the example.

Take the first tuple: f(1,2) = 4, f(2,2) = 2, f(1,2) XOR f(2,2) = 4 XOR 2 = 6, and f(1,2) = 4. So, 6 > 4 holds.

But according to my earlier assumption, f(x, y) XOR f(y, z) should be equal to f(x, z), but in this case, f(1,2) XOR f(2,2) is 6, and f(1,2) is 4, which are not equal. So, my assumption was wrong.

Let me think again.

Actually, f(x, y) XOR f(y, z) = (a_x to a_y) XOR (a_y to a_z).

In terms of XOR, this would be a_x to a_{y-1} XOR a_y to a_z, which simplifies to a_x to a_z, assuming y starts from 1.

Wait, no. XOR is associative and commutative, but let's think carefully.

f(x, y) = a_x to a_y XOR

f(y, z) = a_y to a_z XOR

So, f(x, y) XOR f(y, z) = (a_x to a_y) XOR (a_y to a_z)

Since XOR cancels out duplicate terms, this should be a_x to a_z, which is f(x, z).

But in the example, f(1,2) XOR f(2,2) is 4 XOR 2 = 6, while f(1,2) is 4, and f(1,3) is 0.

Wait, perhaps I need to consider that f(x, z) is a_x to a_z, and f(x, y) XOR f(y, z) is also a_x to a_z, but in the example, they are different.

Wait, in the first tuple, f(1,2) XOR f(2,2) is 4 XOR 2 = 6, and f(1,3) is 0.

So, 6 > 0 holds.

But according to my earlier thought, f(x, y) XOR f(y, z) should be equal to f(x, z), but in this case, it's not.

Wait, maybe I need to recall that f(x, y) XOR f(y, z) is actually f(x, z), based on XOR properties.

But in the example, it's showing that f(x, y) XOR f(y, z) can be different from f(x, z), and in some cases, greater.

This suggests that perhaps my understanding of XOR properties is incomplete.

Let me look up the properties of XOR.

XOR is indeed associative and commutative, and for ranges, f(x, y) XOR f(y, z) should be equal to f(x, z).

But in the example, it's showing that f(x, y) XOR f(y, z) can be greater than f(x, z), which suggests they are not always equal.

This inconsistency is confusing.

Wait, perhaps there's a mistake in my calculation.

Let me calculate f(x, y) XOR f(y, z):

f(x, y) = a_x to a_y XOR

f(y, z) = a_y to a_z XOR

So, f(x, y) XOR f(y, z) = (a_x to a_{y-1} XOR a_y to a_z) = a_x to a_z, assuming y starts from x.

Wait, in the first tuple (1,2,2):

f(1,2) = a1 XOR a2 = 6 XOR 2 = 4

f(2,2) = a2 = 2

f(1,2) XOR f(2,2) = 4 XOR 2 = 6

f(1,3) = a1 XOR a2 XOR a3 = 6 XOR 2 XOR 4 = 0

So, 6 > 0 holds.

But according to XOR properties, f(x, y) XOR f(y, z) should be f(x, z), but in this case, 6 ≠ 0.

This suggests that my understanding is incorrect.

Wait, perhaps f(x, y) XOR f(y, z) is not equal to f(x, z). Maybe I'm misapplying the properties.

Let me consider another example.

Suppose array [1, 2, 3]:

Compute f(1,2) = 1 XOR 2 = 3

f(2,2) = 2

f(1,2) XOR f(2,2) = 3 XOR 2 = 1

f(1,3) = 1 XOR 2 XOR 3 = 0

So, 1 > 0 holds.

Again, f(x, y) XOR f(y, z) = 1, and f(x, z) = 0, which are different.

So, perhaps f(x, y) XOR f(y, z) is not equal to f(x, z). Maybe I have a misunderstanding.

Wait, perhaps f(x, y) XOR f(y, z) = f(x, z).

Wait, in the first example, f(x, y) XOR f(y, z) was 6, and f(x, z) was 0, which are not equal.

So, perhaps my assumption that f(x, y) XOR f(y, z) = f(x, z) is wrong.

Let me see:

f(x, y) XOR f(y, z) = (a_x to a_y) XOR (a_y to a_z)

If y > x, then a_x to a_{y-1} XOR a_y to a_z = a_x to a_z

But in the example, it's giving a different value.

Wait, perhaps when y = z, or other specific cases, it behaves differently.

This confusion suggests that perhaps f(x, y) XOR f(y, z) is not always equal to f(x, z). Maybe there are cases where it's different.

Given that, perhaps the condition f(x, y) XOR f(y, z) > f(x, z) can hold true in some cases.

Now, moving forward, I need to find an efficient way to count the number of such tuples, given the constraints on n and t.

Given that t can be up to 10^4 and n up to 10^5, with the sum of n over all test cases up to 10^5, I need an algorithm that is linear or linearithmic in n for each test case.

Brute-force enumeration of all possible (x, y, z) tuples would be O(n^3), which is too slow.

Hence, I need a smarter approach.

Let me try to simplify the condition:

We have f(x, y) XOR f(y, z) > f(x, z)

Let me denote a = f(x, y), b = f(y, z), c = f(x, z)

So, a XOR b > c

I need to find the number of tuples where this holds.

Is there a way to exploit the properties of XOR to compute this efficiently?

Perhaps I can precompute prefix XOR values and then use some data structure to count the number of valid (x, y, z) tuples.

Let me define prefix[i] = a1 XOR a2 XOR ... XOR a_i

Then, f(x, y) = prefix[y] XOR prefix[x-1]

Similarly, f(y, z) = prefix[z] XOR prefix[y-1]

And f(x, z) = prefix[z] XOR prefix[x-1]

So, the condition becomes:

(prefix[y] XOR prefix[x-1]) XOR (prefix[z] XOR prefix[y-1]) > prefix[z] XOR prefix[x-1]

Simplify the left side:

(prefix[y] XOR prefix[x-1]) XOR (prefix[z] XOR prefix[y-1]) = prefix[y] XOR prefix[x-1] XOR prefix[z] XOR prefix[y-1]

So, the condition is:

prefix[y] XOR prefix[x-1] XOR prefix[z] XOR prefix[y-1] > prefix[z] XOR prefix[x-1]

Let me see if I can rearrange this.

Note that XOR is commutative and associative, so:

prefix[y] XOR prefix[x-1] XOR prefix[z] XOR prefix[y-1] = prefix[z] XOR prefix[x-1] XOR prefix[y] XOR prefix[y-1]

So, the condition is:

prefix[z] XOR prefix[x-1] XOR prefix[y] XOR prefix[y-1] > prefix[z] XOR prefix[x-1]

Let me denote temp = prefix[z] XOR prefix[x-1]

Then, the condition becomes:

temp XOR prefix[y] XOR prefix[y-1] > temp

This seems a bit messy. Maybe there's another way to approach this.

Let me consider fixing y and then finding suitable x and z.

Given that x ≤ y ≤ z, for each y, I can iterate over x from 1 to y and z from y to n, and check the condition.

But this is still O(n^3), which is too slow.

I need a better way.

Perhaps I can consider the binary representation of the XOR values and find a way to count the number of tuples based on bit manipulation.

Alternatively, maybe I can find a way to count the number of tuples where f(x, y) XOR f(y, z) > f(x, z) by considering the most significant bit where they differ.

This seems complicated.

Let me think differently.

I recall that XOR can be treated like addition in a vector space over GF(2). Maybe I can use linear algebra properties here.

But I'm not sure how to apply that directly to this problem.

Another idea: since XOR is involved, perhaps I can consider the problem in terms of bit independence. That is, for each bit position, I can consider the bits independently.

Wait, perhaps I can consider each bit position from 0 to 31 (since a_i can be up to 10^9, which is within 32 bits), and for each bit, analyze the condition separately.

Let me try that.

Suppose I look at the k-th bit for all involved XORs.

Let me denote the k-th bit of a number x as x_k.

Then, the condition f(x, y) XOR f(y, z) > f(x, z) implies that there exists at least one bit position where f(x, y)_k XOR f(y, z)_k > f(x, z)_k.

Wait, but bits are either 0 or 1, so a > b only if a=1 and b=0.

Hence, for the overall condition to hold, there must be at least one bit position k where:

(f(x, y)_k XOR f(y, z)_k) > f(x, z)_k

Which only happens when f(x, y)_k XOR f(y, z)_k = 1 and f(x, z)_k = 0.

So, for each bit position k, I can count the number of tuples where f(x, y)_k XOR f(y, z)_k = 1 and f(x, z)_k = 0.

Then, the total number of tuples is the sum over all bit positions k of these counts.

Wait, but since the bits are independent, perhaps I can compute the total number of tuples where the condition holds for at least one bit position.

But I need to be careful with overlapping bit positions.

Wait, perhaps inclusion-exclusion could be applied here, but that might not be efficient.

Alternatively, since the bits are independent, maybe I can compute for each bit position separately and sum up the counts.

But I need to make sure that I'm not double-counting tuples that satisfy the condition in multiple bit positions.

Wait, actually, since the condition is that f(x, y) XOR f(y, z) > f(x, z), which translates to the bitwise condition that for at least one bit position k, f(x, y)_k XOR f(y, z)_k = 1 and f(x, z)_k = 0, and for all higher bit positions j > k, f(x, y)_j XOR f(y, z)_j = f(x, z)_j.

But this seems complicated to implement.

Let me consider a different approach.

I recall that for XOR operations, prefix XOR arrays are often useful.

Let me define prefix[i] = a1 XOR a2 XOR ... XOR a_i

Then, f(x, y) = prefix[y] XOR prefix[x-1]

Similarly, f(y, z) = prefix[z] XOR prefix[y-1]

And f(x, z) = prefix[z] XOR prefix[x-1]

So, the condition is:

(prefix[y] XOR prefix[x-1]) XOR (prefix[z] XOR prefix[y-1]) > prefix[z] XOR prefix[x-1]

Simplify the left side:

prefix[y] XOR prefix[x-1] XOR prefix[z] XOR prefix[y-1] > prefix[z] XOR prefix[x-1]

Let me denote a = prefix[x-1], b = prefix[y-1], c = prefix[y], d = prefix[z]

Then, the condition is:

(c XOR a) XOR (d XOR b) > d XOR a

Which simplifies to:

c XOR a XOR d XOR b > d XOR a

Which is:

c XOR b XOR d XOR d XOR a XOR a XOR b > d XOR a

Wait, that seems messy.

Alternatively, perhaps I can rearrange the terms.

Note that XOR is associative and commutative, so I can rearrange the terms.

Let me see:

c XOR a XOR d XOR b = c XOR b XOR d XOR a

So, c XOR b XOR d XOR a > d XOR a

Let me denote e = d XOR a

Then, c XOR b XOR e > e

Since e is a number, and c XOR b is another number, I need to find when c XOR b XOR e > e

But c XOR b XOR e = c XOR b XOR (d XOR a)

Wait, this seems too convoluted.

Maybe I need to think differently.

Let me consider that for the condition to hold, c XOR b > e, where c = prefix[y], b = prefix[y-1], e = prefix[z] XOR prefix[x-1]

But this still seems complicated.

Perhaps I need to find a way to iterate over y and for each y, find the suitable x and z.

Given that x ≤ y ≤ z, perhaps I can fix y and then find x and z such that the condition holds.

But I need a way to count the number of such x and z efficiently for each y.

Let me think about the properties of XOR and how it affects the comparison.

I recall that for two numbers A and B, A XOR B > A if and only if the most significant bit where A and B differ is set to 1 in B.

But I'm not sure how to apply this here directly.

Another idea: perhaps I can consider the binary representations of the involved XORs and find a way to count the tuples based on the bit positions where the condition holds.

This seems promising, but I need to formalize it.

Let me consider that for the condition f(x, y) XOR f(y, z) > f(x, z), it must be the case that there exists at least one bit position k where:

- The k-th bit of f(x, y) XOR f(y, z) is 1

- The k-th bit of f(x, z) is 0

- And for all higher bit positions j > k, the j-th bits of f(x, y) XOR f(y, z) and f(x, z) are equal.

This is similar to how numerical comparison works bit by bit.

But this seems too involved for an efficient implementation.

Let me look for a different approach.

I found that directly manipulating the condition is too complicated. Maybe I can look for patterns or properties that can simplify the problem.

Let me consider that f(x, y) XOR f(y, z) = f(x, z), based on the earlier thought, but the example shows that it's not always the case. So, perhaps I need to accept that f(x, y) XOR f(y, z) can be different from f(x, z).

Wait, but according to XOR properties, f(x, y) XOR f(y, z) should be equal to f(x, z). Let me verify this with the example.

In the first test case:

Array: [6, 2, 4]

prefix = [0, 6, 4, 0]

For tuple (1,2,2):

f(1,2) = 6 XOR 2 = 4

f(2,2) = 2

f(1,2) XOR f(2,2) = 4 XOR 2 = 6

f(1,3) = 0

So, 6 > 0 holds.

But according to the prefix array, f(x, z) = prefix[z] XOR prefix[x-1] = prefix[2] XOR prefix[0] = 4 XOR 0 = 4 for (1,2,2), but wait, in the note, it says f(1,3) = 0, which is correct.

Wait, for tuple (1,2,2), z=2, so f(1,2) XOR f(2,2) = 4 XOR 2 = 6, and f(1,2) = 4, but in the note, it says f(1,z) where z=2, which is 4, but in the tuple (1,2,2), z=2, but in the note, it