To calculate the output state, we need to understand the impact of the given code snippet on the variables. 

The provided code snippet is:
```
x = (a - i * (i - 1)) // i ** 2 + 1
```

Given the initial state:
- `t` is a positive integer such that 1 <= t <= 10^4
- `T` must be greater than 0
- `info` is a list of strings from the input
- `a` is the integer value of `info[0]`
- `b` must be greater than or equal to 1
- `suma` is 0
- `i` is 1

Let's evaluate the expression for `x` using the initial values of the variables:

- `a` is the integer value of `info[0]` (specific value unknown, but it is an integer)
- `i` is 1

Substituting `i = 1` into the expression:
```
x = (a - 1 * (1 - 1)) // 1 ** 2 + 1
x = (a - 1 * 0) // 1 + 1
x = (a - 0) // 1 + 1
x = a // 1 + 1
x = a + 1
```

Thus, `x` is assigned the value `a + 1`.

The values of the other variables (`t`, `T`, `info`, `b`, `suma`, `i`) remain unchanged.

Output State: **`t` is a positive integer such that 1 <= t <= 10^4, `T` must be greater than 0, `info` is a list of strings from the input, `a` is the integer value of `info[0]`, `b` must be greater than or equal to 1, `suma` is 0, `i` is 1, `x` is `a + 1`**.