Let's break down the given code snippet and the initial state step by step:

### Initial State
- `t` is a positive integer such that \(1 \leq t \leq 10^4\).
- For each test case, there are four non-negative integers \(p_i\) (where \(0 \leq p_i \leq 200\)) representing the counts of 1s, 2s, 3s, and 4s in the initial sequence.

### Code Snippet
```python
print('\n'.join([str(sum(3 * (x // 2) + x % 2 * (i < 3) for i, x in
    enumerate(map(int, input().split()))) // 3) for _ in range(int(input()))]))
```

### Step-by-Step Analysis

1. **Input Reading**:
   - The code reads an integer \(t\) from the input, which represents the number of test cases.
   - For each test case, it reads a line of input, splits it into four integers, and converts them to integers.

2. **Processing Each Test Case**:
   - For each test case, the code processes the four integers \(p_0, p_1, p_2, p_3\) (counts of 1s, 2s, 3s, and 4s respectively).
   - It calculates a value for each test case using the formula inside the `sum` function:
     - `3 * (x // 2) + x % 2 * (i < 3)` where \(i\) is the index (0-based) and \(x\) is the count of the corresponding number (1, 2, 3, or 4).

3. **Formula Breakdown**:
   - For \(i = 0\) (count of 1s):
     - If \(x = 1\), then \(3 * (1 // 2) + 1 % 2 * (0 < 3) = 0 + 1 = 1\).
     - If \(x = 2\), then \(3 * (2 // 2) + 2 % 2 * (0 < 3) = 3 + 0 = 3\).
     - If \(x = 3\), then \(3 * (3 // 2) + 3 % 2 * (0 < 3) = 4 + 0 = 4\).
     - If \(x = 4\), then \(3 * (4 // 2) + 4 % 2 * (0 < 3) = 6 + 0 = 6\).
   - For \(i = 1\) (count of 2s):
     - If \(x = 1\), then \(3 * (1 // 2) + 1 % 2 * (1 < 3) = 0 + 1 = 1\).
     - If \(x = 2\), then \(3 * (2 // 2) + 2 % 2 * (1 < 3) = 3 + 0 = 3\).
     - If \(x = 3\), then \(3 * (3 // 2) + 3 % 2 * (1 < 3) = 4 + 0 = 4\).
     - If \(x = 4\), then \(3 * (4 // 2) + 4 % 2 * (1 < 3) = 6 + 0 = 6\).
   - For \(i = 2\) (count of 3s):
     - If \(x = 1\), then \(3 * (1 // 2) + 1 % 2 * (2 < 3) = 0 + 1 = 1\).
     - If \(x = 2\), then \(3 * (2 // 2) + 2 % 2 * (2 < 3) = 3 + 0 = 3\).
     - If \(x = 3\), then \(3 * (3 // 2) + 3 % 2 * (2 < 3) = 4 + 0 = 4\).
     - If \(x = 4\), then \(3 * (4 // 2) + 4 % 2 * (2 < 3) = 6 + 0 = 6\).
   - For \(i = 3\) (count of 4s):
     - If \(x = 1\), then \(3 * (1 // 2) + 1 % 2 * (3 < 3) = 0 + 0 = 0\).
     - If \(x = 2\), then \(3 * (2 // 2) + 2 % 2 * (3 < 3) = 3 + 0 = 3\).
     - If \(x = 3\), then \(3 * (3 // 2) + 3 % 2 * (3 < 3) = 4 + 0 = 4\).
     - If \(x = 4\), then \(3 * (4 // 2) + 4 % 2 * (3 < 3) = 6 + 0 = 6\).

4. **Summation and Division**:
   - The result of the summation is then divided by 3.

5. **Output**:
   - The result of the division is converted to a string and joined with newlines for each test case.

### Final Output
Given the nature of the problem, the exact output depends on the input provided. However, based on the formula and the constraints, the output will be a series of lines, each containing the result of the division of the summation by 3 for each test case.

Output: **the result of the division of the summation by 3 for each test case, separated by newlines**