To determine what will be printed, let's break down the initial state and the calculation of `kq`.

Given:
- `kq` is the sum of differences between elements symmetrically placed around the center of the list `a`.

The formula for `kq` is:
\[ kq = \sum_{i=0}^{len(a)//2-1} \left( a[len(a) - (len(a) // 2 - 1) - 1 - i] - a[len(a) // 2 - 1 - i] \right) + \left( a[len(a) - len(a) // 2 - 1 - i] - a[len(a) // 2 - 1 - i] \right) + \left( a[len(a) - (len(a) // 2 + 1) - 1 - i] - a[len(a) // 2 + 1 - 1 - i] \right) \]

This means for each `i` from `0` to `len(a) // 2 - 1`, we calculate three differences and sum them up.

Let's denote the length of the list `a` as `n`. The formula simplifies to:
\[ kq = \sum_{i=0}^{n//2-1} \left( a[n - (n // 2 - 1) - 1 - i] - a[n // 2 - 1 - i] \right) + \left( a[n - n // 2 - 1 - i] - a[n // 2 - 1 - i] \right) + \left( a[n - (n // 2 + 1) - 1 - i] - a[n // 2 + 1 - 1 - i] \right) \]

For simplicity, let's assume `a` is a list with an even number of elements, say `a = [1, 2, 3, 4, 5, 6]` (the length `n = 6`).

1. For `i = 0`:
   - First term: \( a[6 - (6 // 2 - 1) - 1 - 0] - a[6 // 2 - 1 - 0] = a[6 - 2 - 1] - a[2] = a[3] - a[2] = 4 - 3 = 1 \)
   - Second term: \( a[6 - 6 // 2 - 1 - 0] - a[6 // 2 - 1 - 0] = a[6 - 3 - 1] - a[2] = a[2] - a[2] = 3 - 3 = 0 \)
   - Third term: \( a[6 - (6 // 2 + 1) - 1 - 0] - a[6 // 2 + 1 - 1 - 0] = a[6 - 4 - 1] - a[2] = a[1] - a[2] = 2 - 3 = -1 \)

2. Summing these up for `i = 0`: \( 1 + 0 - 1 = 0 \)

3. Since there is only one iteration (`i = 0`), the final value of `kq` is `0`.

Therefore, the print statement will output:
Output: **0**