Alright, I have this problem to solve. Let's see what it's asking for. So, Nikita has some cubes and he wants to build a tower using these cubes. He can perform two types of moves: either add one cube to the top of the tower or remove one cube from the top. He can do this for a total of n moves, and I need to figure out if it's possible that after these n moves, the tower has exactly m cubes.

First, I need to understand the initial state. The problem says that initially, the tower doesn't have any cubes. So, starting from zero cubes, Nikita will perform n moves, each move either adding or removing one cube.

So, each move can be thought of as either +1 (adding a cube) or -1 (removing a cube). I need to see if after n such operations, starting from zero, I can end up with m cubes in the tower.

Let me try to model this mathematically. Let’s say Nikita adds a cube x times and removes a cube y times. Then, the total number of moves is x + y = n. And the final number of cubes in the tower would be x - y, since he adds x cubes and removes y cubes.

So, x - y = m and x + y = n.

I can solve these two equations. Adding them up: 2x = m + n, so x = (m + n)/2.

Similarly, subtracting them: 2y = n - m, so y = (n - m)/2.

Now, since x and y have to be non-negative integers (because you can't perform a negative number of moves), this gives me some conditions.

First, (m + n) must be even, because x must be an integer. So, (m + n) % 2 == 0.

Second, (n - m) must be even, for y to be an integer. But actually, since m and n are both integers, if (m + n) is even, then (n - m) is also even, because (n - m) = (n + m) - 2m.

So, the first condition is that (m + n) is even.

Also, x and y must be non-negative. So, x = (m + n)/2 >= 0 and y = (n - m)/2 >= 0.

Since n and m are both positive integers, and n >= 1 and m >= 1, I need to make sure that x and y are non-negative.

Let me consider x = (m + n)/2 >= 0, which is always true since m and n are positive.

And y = (n - m)/2 >= 0, which implies that n - m >= 0, so n >= m.

Wait, that's an important condition. n must be greater than or equal to m.

But hold on, what if m is greater than n? For example, if n = 3 and m = 4, can I have 4 cubes after 3 moves starting from 0? Let's see.

If I add a cube three times: 0 -> 1 -> 2 -> 3. So, I have 3 cubes, not 4.

Alternatively, if I add and remove cubes in some sequence, like add, remove, add: 0->1->0->1. After 3 moves, I have 1 cube, not 4.

So, it's impossible to have m > n, because the maximum number of cubes I can have is n, by adding a cube in every move.

Wait, but according to my earlier equation, x = (m + n)/2, and y = (n - m)/2.

If m > n, then y would be negative, which doesn't make sense, because y can't be negative.

So, n must be greater than or equal to m.

Also, (m + n) must be even.

So, the conditions are:

1. n >= m

2. (m + n) is even

If both these conditions are satisfied, then it's possible to have m cubes after n moves.

Let me test this with the example given.

First test case: n=3, m=3.

Condition 1: 3 >= 3, which is true.

Condition 2: (3 + 3) = 6, which is even.

So, output should be "Yes", which matches the sample output.

Second test case: n=2, m=4.

Condition 1: 2 >= 4? No, 2 < 4. So, condition 1 fails.

Hence, "No", which matches the sample output.

Third test case: n=5, m=3.

Condition 1: 5 >= 3, which is true.

Condition 2: (5 + 3) = 8, which is even.

So, "Yes", matching the sample output.

Seems correct.

Wait, but is there any other scenario I'm missing?

Let's consider n=1, m=1.

Condition 1: 1 >= 1, true.

Condition 2: (1 + 1) = 2, even.

So, "Yes".

n=1, m=0.

Condition 1: 1 >= 0, true.

But condition 2: (0 + 1) = 1, which is odd.

So, "No".

Is that correct?

If n=1, m=0.

Possible sequences:

- Add: 0->1

- Remove: 0->-1

Wait, but removing a cube from zero is not allowed, as per the problem statement. It says "remove exactly 1 cube from the top of the tower", assuming that the tower has at least one cube.

So, in reality, you can't remove a cube if there are zero cubes.

Hence, with n=1, m=0 is impossible.

Hence, "No", which aligns with my earlier conclusion.

Another test case: n=4, m=2.

Condition 1: 4 >= 2, true.

Condition 2: (4 + 2) = 6, even.

So, "Yes".

Possible sequence: add, add, remove, add: 0->1->2->1->2.

After 4 moves, m=2.

Another test case: n=4, m=4.

Condition 1: 4 >= 4, true.

Condition 2: (4 + 4) = 8, even.

"yes".

Sequence: add, add, add, add: 0->1->2->3->4.

Another test case: n=4, m=0.

Condition 1: 4 >= 0, true.

Condition 2: (0 + 4) = 4, even.

"yes".

Sequence: add, remove, add, remove: 0->1->0->1->0.

So, it works.

Another test case: n=3, m=2.

Condition 1: 3 >= 2, true.

Condition 2: (3 + 2) = 5, odd.

"no".

Sequence: add, add, add: 0->1->2->3.

Or add, add, remove: 0->1->2->1.

Cannot get m=2 in 3 moves.

Hence, "No".

Seems consistent.

Wait, but in the earlier reasoning, I assumed that y = (n - m)/2 >= 0, which implies n >= m.

But what if n < m?

In that case, y would be negative, which is invalid.

Hence, n must be >= m.

And (m + n) must be even.

Seems comprehensive.

Hence, the solution should be to check if n >= m and (m + n) % 2 == 0.

If both are true, print "Yes"; else, "No".

Looking back at the provided program:

def func():

for _ in range(int(input())):

(n, m) = map(int, input().split())

if n >= m and (n - m) % 2 == 0:

print('YES')

else:

print('NO')

Wait a minute, in my reasoning, the condition is (m + n) % 2 == 0.

But in the code, it's (n - m) % 2 == 0.

Is that a mistake?

Wait, let's see.

Earlier, I derived that x = (m + n)/2 and y = (n - m)/2.

But in the condition, I said (m + n) % 2 == 0.

But in the code, it's (n - m) % 2 == 0.

Are these equivalent?

Let me check.

Suppose (m + n) is even, then (n - m) = (n + m) - 2m, which is even minus even, since m is integer.

Wait, 2m is even, so (n + m) - 2m = (n - m), which is even.

Hence, (m + n) % 2 == (n - m) % 2.

So, checking either (m + n) % 2 == 0 or (n - m) % 2 == 0 is the same.

Hence, the code is correct.

So, the code checks if n >= m and (n - m) % 2 == 0, which is equivalent to my conditions.

Hence, the program is correct.

**Final Solution**

To solve this problem, we need to determine if Nikita can achieve a tower of exactly `m` cubes after performing `n` moves, where each move consists of either adding one cube to the top of the tower or removing one cube from the top.

### Approach

1. **Initial Analysis**:
   - We start with zero cubes.
   - Each move can either add or remove one cube.
   
2. **Mathematical Modeling**:
   - Let `x` be the number of times we add a cube.
   - Let `y` be the number of times we remove a cube.
   - We have two equations:
     - `x + y = n` (total moves)
     - `x - y = m` (final number of cubes)
   
3. **Solving Equations**:
   - Adding the equations: `2x = m + n` ⇒ `x = (m + n)/2`
   - Subtracting the equations: `2y = n - m` ⇒ `y = (n - m)/2`
   
4. **Conditions for Feasibility**:
   - `x` and `y` must be non-negative integers.
   - Therefore:
     - `n >= m` to ensure `y` is non-negative.
     - `(m + n)` must be even to ensure `x` is an integer.
     - `(n - m)` must be even to ensure `y` is an integer.

5. **Simplified Condition**:
   - Since `(m + n)` and `(n - m)` are both even if one of them is even (because they differ by `2m`, which is even), we only need to check one of them.

### Solution Code

```python
def func():
    for _ in range(int(input())):
        (n, m) = map(int, input().split())
        if n >= m and (n - m) % 2 == 0:
            print('YES')
        else:
            print('NO')

func()
```

### Explanation

- **Input Handling**:
  - Read the number of test cases `t`.
  - For each test case, read `n` and `m`.

- **Logic**:
  - Check if `n >= m` and `(n - m)` is even.
  - If both conditions are satisfied, print "YES"; otherwise, print "NO".

- **Efficiency**:
  - The solution runs in O(1) per test case, making it efficient for the input constraints.

This approach ensures that we correctly determine whether it is possible to achieve the desired number of cubes after the given number of moves, adhering to the problem constraints.