The code snippet `tem = x[i] - x[i + 1]` updates the value of `tem` to the difference between the first and second elements of the list `x`. Given the initial conditions, `tem` was 0, and now it is updated to `x[0] - x[1]`.

The rest of the variables and conditions remain unchanged.

Output State: **`n` and `c` are integers where 2 ≤ `n` ≤ 100 and 0 ≤ `c` ≤ 100, `x` is a list with at least 2 elements, `N` is a non-negative integer, `C` is an integer, `tem` is `x[0] - x[1]`, `i` is 0, and `x[i] - x[i + 1] - C` is greater than 0**