The code snippet `tem = tem - C` updates the value of `tem` by subtracting `C` from its current value. Given the initial conditions:

- `n` and `c` are integers where 2 ≤ `n` ≤ 100 and 0 ≤ `c` ≤ 100
- `x` is a list with at least 2 elements
- `N` is a non-negative integer
- `C` is an integer
- `i` is `len(x) - 2`
- `tem` is the maximum value of `x[j] - x[j + 1]` for all `j` in the range `[0, len(x) - 2]` such that `x[j] - x[j + 1] - C > 0`
- The current value of `tem` is greater than 0

After executing the code snippet:

- `tem` is now `tem - C`

Therefore, the updated state is:

Output State: **`n` and `c` are integers where 2 ≤ `n` ≤ 100 and 0 ≤ `c` ≤ 100, `x` is a list with at least 2 elements, `N` is a non-negative integer, `C` is an integer, `i` is `len(x) - 2`, `tem` is `tem - C` (where `tem` was the maximum value of `x[j] - x[j + 1]` for all `j` in the range `[0, len(x) - 2]` such that `x[j] - x[j + 1] - C > 0` and was greater than 0)**