To determine the final output state after all iterations of the loop, we need to understand how the loop modifies the variable `suma` based on the given conditions and the range of the loop.

Here's a step-by-step breakdown of the loop's behavior:

- The loop runs from `i = 1` to `i = b`.
- For each iteration, `x` is calculated as `(a - i * (i - 1)) // i ** 2 + 1`.
- The condition `if a - i * (i - 1) > 0` determines whether `suma` is incremented by `x`.

Let's analyze the loop's effect on `suma`:

1. For `i = 1`: 
   - `x = (a - 1 * 0) // 1 ** 2 + 1 = a + 1`
   - If `a > 0`, then `suma` becomes `a + 1`.

2. For `i = 2`:
   - `x = (a - 2 * 1) // 2 ** 2 + 1 = (a - 2) // 4 + 1`
   - If `a - 2 > 0`, then `suma` is incremented by `x`.

3. For `i = 3`:
   - `x = (a - 3 * 2) // 3 ** 2 + 1 = (a - 6) // 9 + 1`
   - If `a - 6 > 0`, then `suma` is incremented by `x`.

This pattern continues up to `i = b`. Therefore, `suma` accumulates the values of `x` for each `i` where `a - i * (i - 1) > 0`.

After all iterations, `suma` will be the sum of all valid `x` values calculated during the loop.

Thus, the final output state after all iterations of the loop is:

Output State: **`suma` is the accumulated sum of all `x` values where `a - i * (i - 1) > 0` for `i` from 1 to `b`. `t` is incremented by 1, `info` remains the list of strings obtained from the input, `a` is the integer value of `info[0]`, and `b` remains the same.**

In simpler terms, `suma` will be the total of all computed `x` values that meet the condition `a - i * (i - 1) > 0` across all iterations from `i = 1` to `i = b`.