The code snippet `b[i] = b[i - 1] + x` updates the list `b` based on the value of `x`, which is determined by the condition `x = 1 if a[i] > 1 else 2`. This means that for each index `i` from 1 to `n`, the value of `b[i]` is calculated by adding `x` to the previous value `b[i - 1]`.

Since `b` is initially a list of `n + 1` integers all set to 0, the first element `b[0]` remains 0. For each subsequent element `b[i]`, the value depends on whether `a[i]` is greater than 1 or not.

Given the initial state, the values of `t`, `n`, `q`, `c`, and the queries `l_i` and `r_i` do not change. The only change is in the list `b` after the execution of the code snippet.

Output State: **`t` is an integer such that 1 ≤ t ≤ 10^4; `n` is an integer such that 1 ≤ n ≤ 3 · 10^5; `q` is an integer such that 1 ≤ q ≤ 3 · 10^5; `c` is a list of `n` integers where each element `c_i` satisfies 1 ≤ `c_i` ≤ 10^9; `a` is a list where `a[0]` is 0 and `a[1]` to `a[n]` are the integers read from the input; For each query, `l_i` and `r_i` are integers such that 1 ≤ `l_i` ≤ `r_i` ≤ `n`; `b` is a list of `n + 1` integers where `b[0]` is 0 and `b[i]` for `i` from 1 to `n` is `b[i - 1] + x`, with `x` being 1 if `a[i] > 1` else 2; `x` is 1 if `a[i] > 1` else 2.**