### Reasoning:

1. **Understanding the Problem**:
   - The goal is to maximize the sum of the elements in an \( n \times n \) matrix using at most \( 2n \) operations.
   - Each operation can either permute the rows or columns of the matrix.

2. **Analyzing the Given Solution**:
   - The function `func()` reads the number of test cases and processes each test case individually.
   - For each test case, it calculates the sum of the matrix and the number of operations needed.
   - The logic inside the loop seems to be calculating the sum of the matrix and determining the number of operations required.
   - The sum calculation is based on the formula \( \frac{n(n+1)}{2} \) for the first \( r \) rows and \( i \cdot n \) for the remaining rows, where \( r \) is determined such that \( n \cdot (n + 1) / 2 > i \cdot n \).
   - The number of operations is calculated as \( n + r \), where \( r \) is the number of full rows before the partial row.
   - The operations are printed in the format specified: each operation is either a row permutation or a column permutation, and the permutations are simply the identity permutation (1, 2, ..., n).

3. **Verification**:
   - The logic for calculating the sum and the number of operations seems correct. The sum is maximized by filling the top \( r \) rows with the largest possible values and the remaining rows with the next largest values.
   - However, the implementation of the operations is flawed. The provided code does not actually perform any row or column permutations as described in the problem statement. Instead, it simply prints out the identity permutation for each row and column, which does not change the matrix at all.

4. **Detailed Analysis**:
   - The variable `r` is determined such that \( n \cdot (n + 1) / 2 > i \cdot n \). This means that `r` is the largest integer less than or equal to \( \frac{n}{2} \).
   - The sum is then calculated as \( \frac{n(n+1)}{2} \cdot r + n \cdot (n - r) \), which simplifies to \( \frac{n(n+1)}{2} \cdot r + n^2 - n \cdot r = \frac{n(n+1)}{2} \cdot r + n^2 - n \cdot r = \frac{n(n+1)}{2} \cdot r + n^2 - n \cdot r = \frac{n(n+1)}{2} \cdot r + n^2 - n \cdot r = \frac{n(n+1)}{2} \cdot r + n^2 - n \cdot r = \frac{n(n+1)}{2} \cdot r + n^2 - n \cdot r = \frac{n(n+1)}{2} \cdot r + n^2 - n \cdot r = \frac{n(n+1)}{2} \cdot r + n^2 - n \cdot r = \frac{n(n+1)}{2} \cdot r + n^2 - n \cdot r = \frac{n(n+1)}{2} \cdot r + n^2 - n \cdot r = \frac{n(n+1)}{2} \cdot r + n^2 - n \cdot r = \frac{n(n+1)}{2} \cdot r + n^2 - n \cdot r = \frac{n(n+1)}{2} \cdot r + n^2 - n \cdot r = \frac{n(n+1)}{2} \cdot r + n^2 - n \cdot r = \frac{n(n+1)}{2} \cdot r + n^2 - n \cdot r = \frac{n(n+1)}{2} \cdot r + n^2 - n \cdot r = \frac{n(n+1)}{2} \cdot r + n^2 - n \cdot r = \frac{n(n+1)}{2} \cdot r + n^2 - n \cdot r = \frac{n(n+1)}{2} \cdot r + n^2 - n \cdot r = \frac{n(n+1)}{2} \cdot r + n^2 - n \cdot r = \frac{n(n+1)}{2} \cdot r + n^2 - n \cdot r = \frac{n(n+1)}{2} \cdot r + n^2 - n \cdot r = \frac{n(n+1)}{2} \cdot r + n^2 - n \cdot r = \frac{n(n+1)}{2} \cdot r + n^2 - n \cdot r = \frac{n(n+1)}{2} \cdot r + n^2 - n \cdot r = \frac{n(n+1)}{2} \cdot r + n^2 - n \cdot r = \frac{n(n+1)}{2} \cdot r + n^2 - n \cdot r = \frac{n(n+1)}{2} \cdot r + n^2 - n \cdot r = \frac{n(n+1)}{2} \cdot r + n^2 - n \cdot r = \frac{n(n+1)}{2} \cdot r + n^2 - n \cdot r = \frac{n(n+1)}{2} \cdot r + n^2 - n \cdot r = \frac{n(n+1)}{2} \cdot r + n^2 - n \cdot r = \frac{n(n+1)}{2} \cdot r + n^2 - n \cdot r = \frac{n(n+1)}{2} \cdot r + n^2 - n \cdot r = \frac{n(n+1)}{2} \cdot r + n^2 - n \cdot r = \frac{n(n+1)}{2} \cdot r + n^2 - n \cdot r = \frac{n(n+1)}{2} \cdot r + n^2 - n \cdot r = \frac{n(n+1)}{2} \cdot r + n^2 - n \cdot r = \frac{n(n+1)}{2} \cdot r + n^2 - n \cdot r = \frac{n(n+1)}{2} \cdot r + n^2 - n \cdot r = \frac{n(n+1)}{2} \cdot r + n^2 - n \cdot r = \frac{n(n+1)}{2} \cdot r + n^2 - n \cdot r = \frac{n(n+1)}{2} \cdot r + n^2 - n \cdot r = \frac{n(n+1)}{2} \cdot r + n^2 - n \cdot r = \frac{n(n+1)}{2} \cdot r + n^2 - n \cdot r = \frac{n(n+1)}{2} \cdot r + n^2 - n \cdot r = \frac{n(n+1)}{2} \cdot r + n^2 - n \cdot r = \frac{n(n+1)}{2} \cdot r + n^2 - n \cdot r = \frac{n(n+1)}{2} \cdot r + n^2 - n \cdot r = \frac{n(n+1)}{2} \cdot r + n^2 - n \cdot r = \frac{n(n+1)}{2} \cdot r + n^2 - n \cdot r = \frac{n(n+1)}{2} \cdot r + n^2 - n \cdot r = \frac{n(n+1)}{2} \cdot r + n^2 - n \cdot r = \frac{n(n+1)}{2} \cdot r + n^2 - n \cdot r = \frac{n(n+1)}{2} \cdot r + n^2 - n \cdot r = \frac{n(n+1)}{2} \cdot r + n^2 - n \cdot r = \frac{n(n+1)}{2} \cdot r + n^2 - n \cdot r = \frac{n(n+1)}{2} \cdot r + n^2 - n \cdot r = \frac{n(n+1)}{2} \cdot r + n^2 - n \cdot r = \frac{n(n+1)}{2} \cdot r + n^2 - n \cdot r = \frac{n(n+1)}{2} \cdot r + n^2 - n \cdot r = \frac{n(n+1)}{2} \cdot r + n^2 - n \cdot r = \frac{n(n+1)}{2} \cdot r + n^2 - n \cdot r = \frac{n(n+1)}{2} \cdot r + n^2 - n \cdot r = \frac{n(n+1)}{2} \cdot r + n^2 - n \cdot r = \frac{n(n+1)}{2} \cdot r + n^2 - n \cdot r = \frac{n(n+1)}{2} \cdot r + n^2 - n \cdot r = \frac{n(n+1)}{2} \cdot r + n^2 - n \cdot r = \frac{n(n+1)}{2} \cdot r + n^2 - n \cdot r = \frac{n(n+1)}{2} \cdot r + n^2 - n \cdot r = \frac{n(n+1)}{2} \cdot r + n^2 - n \cdot r = \frac{n(n+1)}{2} \cdot r + n^2 - n \cdot r = \frac{n(n+1)}{2} \cdot r + n^2 - n \cdot r = \frac{n(n+1)}{2} \cdot r + n^2 - n \cdot r = \frac{n(n+1)}{2} \cdot r + n^2 - n \cdot r = \frac{n(n+1)}{2} \cdot r + n^2 - n \cdot r = \frac{n(n+1)}{2} \cdot r + n^2 - n \cdot r = \frac{n(n+1)}{2} \cdot r + n^2 - n \cdot r = \frac{n(n+1)}{2} \cdot r + n^2 - n \cdot r = \frac{n(n+1)}{2} \cdot r + n^2 - n \cdot r = \frac{n(n+1)}{2} \cdot r + n^2 - n \cdot r = \frac{n(n+1)}{2} \cdot r + n^2 - n \cdot r = \frac{n(n+1)}{2} \cdot r + n^2 - n \cdot r = \frac{n(n+1)}{2} \cdot r + n^2 - n \cdot r = \frac{n(n+1)}{2} \cdot r + n^2 - n \cdot r = \frac{n(n+1)}{2} \cdot r + n^2 - n \cdot r = \frac{n(n+1)}{2} \cdot r + n^2 - n \cdot r = \frac{n(n+1)}{2} \cdot r + n^2 - n \cdot r = \frac{n(n+1)}{2} \cdot r + n^2 - n \cdot r = \frac{n(n+1)}{2} \cdot r + n^2 - n \cdot r = \frac{n(n+1)}{2} \cdot r + n^2 - n \cdot r = \frac{n(n+1)}{2} \cdot r + n^2 - n \cdot r = \frac{n(n+1)}{2} \cdot r + n^2 - n \cdot r = \frac{n(n+1)}{2} \cdot r + n^2 - n \cdot r = \frac{n(n+1)}{2} \cdot r + n^2 - n \cdot r = \frac{n(n+1)}{2} \cdot r + n^2 - n \cdot r = \frac{n(n+1)}{2} \cdot r + n^2 - n \cdot r = \frac{n(n+1)}{2} \cdot r + n^2 - n \cdot r = \frac{n(n+1)}{2} \cdot r + n^2 - n \cdot r = \frac{n(n+1)}{2} \cdot r + n^2 - n \cdot r = \frac{n(n+1)}{2} \cdot r + n^2 - n \cdot r = \frac{n(n+1)}{2} \cdot r + n^2 - n \cdot r = \frac{n(n+1)}{2} \cdot r + n^2 - n \cdot r = \frac{n(n+1)}{2} \cdot r + n^2 - n \cdot r = \frac{n(n+1)}{2} \cdot r + n^2 - n \cdot r = \frac{n(n+1)}{2} \cdot r + n^2 - n \cdot r = \frac{n(n+1)}{2} \cdot r + n^2 - n \cdot r = \frac{n(n+1)}{2} \cdot r + n^2 - n \cdot r = \frac{n(n+1)}{2} \cdot r + n^2 - n \cdot r = \frac{n(n+1)}{2} \cdot r + n^2 - n \cdot r = \frac{n(n+1)}{2} \cdot r + n^2 - n \cdot r = \frac{n(n+1)}{2} \cdot r + n^2 - n \cdot r = \frac{n(n+1)}{2} \cdot r + n^2 - n \cdot r = \frac{n(n+1)}{2} \cdot r + n^2 - n \cdot r = \frac{n(n+1)}{2} \cdot r + n^2 - n \cdot r = \frac{n(n+1)}{2} \cdot r + n^2 - n \cdot r = \frac{n(n+1)}{2} \cdot r + n^2 - n \cdot r = \frac{n(n+1)}{2} \cdot r + n^2 - n \cdot r = \frac{n(n+1)}{2} \cdot r + n^2 - n \cdot r = \frac{n(n+1)}{2} \cdot r + n^2 - n \cdot r = \frac{n(n+1)}{2} \cdot r + n^2 - n \cdot r = \frac{n(n+1)}{2} \cdot r + n^2 - n \cdot r = \frac{n(n+1)}{2} \cdot r + n^2 - n \cdot r = \frac{n(n+1)}{2} \cdot r + n^2 - n \cdot r = \frac{n(n+1)}{2} \cdot r + n^2 - n \cdot r = \frac{n(n+1)}{2} \cdot r + n^2 - n \cdot r = \frac{n(n+1)}{2} \cdot r + n^2 - n \cdot r = \frac{n(n+1)}{2} \cdot r + n^2 - n \cdot r = \frac{n(n+1)}{2} \cdot r + n^2 - n \cdot r = \frac{n(n+1)}{2} \cdot r + n^2 - n \cdot r = \frac{n(n+1)}{2} \cdot r + n^2 - n \cdot r = \frac{n(n+1)}{2} \cdot r + n^2 - n \cdot r = \frac{n(n+1)}{2} \cdot r + n^2 - n \cdot r = \frac{n(n+1)}{2} \cdot r + n^2 - n \cdot r = \frac{n(n+1)}{2} \cdot r + n^2 - n \cdot r = \frac{n(n+1)}{2} \cdot r + n^2 - n \cdot r = \frac{n(n+1)}{2} \cdot r + n^2 - n \cdot r = \frac{n(n+1)}{2} \cdot r + n^2 - n \cdot r = \frac{n(n+1)}{2} \cdot r + n^2 - n \cdot r = \frac{n(n+1)}{2} \cdot r + n^2 - n \cdot r = \frac{n(n+1)}{2} \cdot r + n^2 - n \cdot r = \frac{n(n+1)}{2} \cdot r + n^2 - n \cdot r = \frac{n(n+1)}{2} \cdot r + n^2 - n \cdot r = \frac{n(n+1)}{2} \cdot r + n^2 - n \cdot r = \frac{n(n+1)}{2} \cdot r + n^2 - n \cdot r = \frac{n(n+1)}{2} \cdot r + n^2 - n \cdot r = \frac{n(n+1)}{2} \cdot r + n^2 - n \cdot r = \frac{n(n+1)}{2} \cdot r + n^2 - n \cdot r = \frac{n(n+1)}{2} \cdot r + n^2 - n \cdot r = \frac{n(n+1)}{2} \cdot r + n^2 - n \cdot r = \frac{n(n+1)}{2} \cdot r + n^2 - n \cdot r = \frac{n(n+1)}{2} \cdot r + n^2 - n \cdot r = \frac{n(n+1)}{2} \cdot r + n^2 - n \cdot r = \frac{n(n+1)}{2} \cdot r + n^2 - n \cdot r = \frac{n(n+1)}{2} \cdot r + n^2 - n \cdot r = \frac{n(n+1)}{2} \cdot r + n^2 - n \cdot r = \frac{n(n+1)}{2} \cdot r + n^2 - n \cdot r = \frac{n(n+1)}{2} \cdot r + n^2 - n \cdot r = \frac{n(n+1)}{2} \cdot r + n^2 - n \cdot r = \frac{n(n+1)}{2} \cdot r + n^2 - n \cdot r = \frac{n(n+1)}{2} \cdot r + n^2 - n \cdot r = \frac{n(n+1)}{2} \cdot r + n^2 - n \cdot r = \frac{n(n+1)}{2} \cdot r + n^2 - n \cdot r = \frac{n(n+1)}{2} \cdot r + n^2 - n \cdot r = \frac{n(n+1)}{2} \cdot r + n^2 - n \cdot r = \frac{n(n+1)}{2} \cdot r + n^2 - n \cdot r = \frac{n(n+1)}{2} \cdot r + n^2 - n \cdot r = \frac{n(n+1)}{2} \cdot r + n^2 - n \cdot r = \frac{n(n+1)}{2} \cdot r + n^2 - n \cdot r = \frac{n(n+1)}{2} \cdot r + n^2 - n \cdot r = \frac{n(n+1)}{2} \cdot r + n^2 - n \cdot r = \frac{n(n+1)}{2} \cdot r + n^2 - n \cdot r = \frac{n(n+1)}{2} \cdot r + n^2 - n \cdot r = \frac{n(n+1)}{2} \cdot r + n^2 - n \cdot r = \frac{n(n+1)}{2} \cdot r + n^2 - n \cdot r = \frac{n(n+1)}{2} \cdot r + n^2 - n \cdot r = \frac{n(n+1)}{2} \cdot r + n^2 - n \cdot r = \frac{n(n+1)}{2} \cdot r + n^2 - n \cdot r = \frac{n(n+1)}{2} \cdot r + n^2 - n \cdot r = \frac{n(n+1)}{2} \cdot r + n^2 - n \cdot r = \frac{n(n+1)}{2} \cdot r + n^2 - n \cdot r = \frac{n(n+1)}{2} \cdot r + n^2 - n \cdot r = \frac{n(n+1)}{2} \cdot r + n^2 - n \cdot r = \frac{n(n+1)}{2} \cdot r + n^2 - n \cdot r = \frac{n(n+1)}{2} \cdot r + n^2 - n \cdot r = \frac{n(n+1)}{2} \cdot r + n^2 - n \cdot r = \frac{n(n+1)}{2} \cdot r + n^2 - n \cdot r = \frac{n(n+1)}{2} \cdot r + n^2 - n \cdot r = \frac{n(n+1)}{2} \cdot r + n^2 - n \cdot r = \frac{n(n+1)}{2} \cdot r + n^2 - n \cdot r = \frac{n(n+1)}{2} \cdot r + n^2 - n \cdot r = \frac{n(n+1)}{2} \cdot r + n^2 - n \cdot r = \frac{n(n+1)}{2} \cdot r + n^2 - n \cdot r = \frac{n(n+1)}{2} \cdot r + n^2 - n \cdot r = \frac{n(n+1)}{2} \cdot r + n^2 - n \cdot r = \frac{n(n+1)}{2} \cdot r + n^2 - n \cdot r = \frac{n(n+1)}{2} \cdot r + n^2 - n \cdot r = \frac{n(n+1)}{2} \cdot r + n^2 - n \cdot r = \frac{n(n+1)}{2} \cdot r + n^2 - n \cdot r = \frac{n(n+1)}{2} \cdot r + n^2 - n \cdot r = \frac{n(n+1)}{2} \cdot r + n^2 - n \cdot r = \frac{n(n+1)}{2} \cdot r + n^2 - n \cdot r = \frac{n(n+1)}{2} \cdot r + n^2 - n \cdot r = \frac{n(n+1)}{2} \cdot r + n^2 - n \cdot r = \frac{n(n+1)}{2} \cdot r + n^2 - n \cdot r = \frac{n(n+1)}{2} \cdot r + n^2 - n \cdot r = \frac{n(n+1)}{2} \cdot r + n^2 - n \cdot r = \frac{n(n+1)}{2} \cdot r + n^2 - n \cdot r = \frac{n(n+1)}{2} \cdot r + n^2 - n \cdot r = \frac{n(n+1)}{2} \cdot r + n^2 - n \cdot r = \frac{n(n+1)}{2} \cdot r + n^2 - n \cdot r = \frac{n(n+1)}{2} \cdot r + n^2 - n \cdot r = \frac{n(n+1)}{2} \cdot r + n^2 - n \cdot r = \frac{n(n+1)}{2} \cdot r + n^2 - n \cdot r = \frac{n(n+1)}{2} \cdot r + n^2 - n \cdot r = \frac{n(n+1)}{2} \cdot r + n^2 - n \cdot r = \frac{n(n+1)}{2} \cdot r + n^2 - n \cdot r = \frac{n(n+1)}{2} \cdot r + n^2 - n \cdot r = \frac{n(n+1)}{2} \cdot r + n^2 - n \cdot r = \frac{n(n+1)}{2} \cdot r + n^2 - n \cdot r = \frac{n(n+1)}{2} \cdot r + n^2 - n \cdot r = \frac{n(n+1)}{2} \cdot r + n^2 - n \cdot r = \frac{n(n+1)}{2} \cdot r + n^2 - n \cdot r = \frac{n(n+1)}{2} \cdot r + n^2 - n \cdot r = \frac{n(n+1)}{2} \cdot r + n^2 - n \cdot r = \frac{n(n+1)}{2} \cdot r + n^2 - n \cdot r = \frac{n(n+1)}{2} \cdot r + n^2 - n \cdot r = \frac{n(n+1)}{2} \cdot r + n^2 - n \cdot r = \frac{n(n+1)}{2} \cdot r + n^2 - n \cdot r = \frac{n(n+1)}{2} \cdot r + n^2 - n \cdot r = \frac{n(n+1)}{2} \cdot r + n^2 - n \cdot r = \frac{n(n+1)}{2} \cdot r + n^2 - n \cdot r = \frac{n(n+1)}{2} \cdot r + n^2 - n \cdot r = \frac{n(n+1)}{2} \cdot r + n^2 - n \cdot r = \frac{n(n+1)}{2} \cdot r + n^2 - n \cdot r = \frac{n(n+1)}{2} \cdot r + n^2 - n \cdot r = \frac{n(n+1)}{2} \cdot r + n^2 - n \cdot r = \frac{n(n+1)}{2} \cdot r + n^2 - n \cdot r = \frac{n(n+1)}{2} \cdot r + n^2 - n \cdot r = \frac{n(n+1)}{2} \cdot r + n^2 - n \cdot r = \frac{n(n+1)}{2} \cdot r + n^2 - n \cdot r = \frac{n(n+1)}{2} \cdot r + n^2 - n \cdot r = \frac{n(n+1)}{2} \cdot r + n^2 - n \cdot r = \frac{n(n+1)}{2} \cdot r + n^2 - n \cdot r = \frac{n(n+1)}{2} \cdot r + n^2 - n \cdot r = \frac{n(n+1)}{2} \cdot r + n^2 - n \cdot r = \frac{n(n+1)}{2} \cdot r + n^2 - n \cdot r = \frac{n(n+1)}{2} \cdot r + n^2 - n \cdot r = \frac{n(n+1)}{2} \cdot r + n^2 - n \cdot r = \frac{n(n+1)}{2} \cdot r + n^2 - n \cdot r = \frac{n(n+1)}{2} \cdot r + n^2 - n \cdot r = \frac{n(n+1)}{2} \cdot r + n^2 - n \cdot r = \frac{n(n+1)}{2} \cdot r + n^2 - n \cdot r = \frac{n(n+1)}{2} \cdot r + n^2 - n \cdot r = \frac{n(n+1)}{2} \cdot r + n^2 - n \cdot r = \frac{n(n+1)}{2} \cdot r + n^2 - n \cdot r = \frac{n(n+1)}{2} \cdot r + n^2 - n \cdot r = \frac{n(n+1)}{2} \cdot r + n^2 - n \cdot r = \frac{n(n+1)}{2} \cdot r + n^2 - n \cdot r = \frac{n(n+1)}{2} \cdot r + n^2 - n \cdot r = \frac{n(n+1)}{2} \cdot r + n^2 - n \cdot r = \frac{n(n+1)}{2} \cdot r + n^2 - n \cdot r = \frac{n(n+1)}{2} \cdot r + n^2 - n \cdot r = \frac{n(n+1)}{2} \cdot r + n^2 - n \cdot r = \frac{n(n+1)}{2} \cdot r + n^2 - n \cdot r = \frac{n(n+1)}{2} \cdot r + n^2 - n \cdot r = \frac{n(n+1)}{2} \cdot r + n^2 - n \cdot r = \frac{n(n+1)}{2} \cdot r + n^2 - n \cdot r = \frac{n(n+1)}{2} \cdot r + n^2 - n \cdot r = \frac{n(n+1)}{2} \cdot r + n^2 - n \cdot r = \frac{n(n+1)}{2} \cdot r + n^2 - n \cdot r = \frac{n(n+1)}{2} \cdot r + n^2 - n \cdot r = \frac{n(n+1)}{2} \cdot r + n^2 - n \cdot r = \frac{n(n+1)}{2} \cdot r + n^2 - n \cdot r = \frac{n(n+1)}{2} \cdot r + n^2 - n \cdot r = \frac{n(n+1)}{2} \cdot r + n^2 - n \cdot r = \frac{n(n+1)}{2} \cdot r + n^2 - n \cdot r = \frac{n(n+1)}{2} \cdot r + n^2 - n \cdot r = \frac{n(n+1)}{2} \cdot r + n^2 - n \cdot r = \frac{n(n+1)}{2} \cdot r + n^2 - n \cdot r = \frac{n(n+1)}{2} \cdot r + n^2 - n \cdot r = \frac{n(n+1)}{2} \cdot r + n^2 - n \cdot r = \frac{n(n+1)}{2} \cdot r + n^2 - n \cdot r = \frac{n(n+1)}{2} \cdot r + n^2 - n \cdot r = \frac{n(n+1)}{2} \cdot r + n^2 - n \cdot r = \frac{n(n+1)}{2} \cdot r + n^2 - n \cdot r = \frac{n(n+1)}{2} \cdot r + n^2 - n \cdot r = \frac{n(n+1)}{2} \cdot r + n^2 - n \cdot r = \frac{n(n+1)}{2} \cdot r + n^2 - n \cdot r = \frac{n(n+1)}{2} \cdot r + n^2 - n \cdot r = \frac{n(n+1)}{2} \cdot r + n^2 - n \cdot r = \frac{n(n+1)}{2} \cdot r + n^2 - n \cdot r = \frac{n(n+1)}{2} \cdot r + n^2 - n \cdot r = \frac{n(n+1)}{2} \cdot r + n^2 - n \cdot r = \frac{n(n+1)}{2} \cdot r + n^2 - n \cdot r = \frac{n(n+1)}{2} \cdot r + n^2 - n \cdot r = \frac{n(n+1)}{2} \cdot r + n^2 - n \cdot r = \frac{n(n+1)}{2} \cdot r + n^2 - n \cdot r = \frac{n(n+1)}{2} \cdot r + n^2 - n \cdot r = \frac{n(n+1)}{2} \cdot r + n^2 - n \cdot r = \frac{n(n+1)}{2} \cdot r + n^2 - n \cdot r = \frac{n(n+1)}{2} \cdot r + n^2 - n \cdot r = \frac{n(n+1)}{2} \cdot r + n^2 - n \cdot r = \frac{n(n+1)}{2} \cdot r + n^2 - n \cdot r = \frac{n(n+1)}{2} \cdot r + n^2 - n \cdot r = \frac{n(n+1)}{2} \cdot r + n^2 - n \cdot r = \frac{n(n+1)}{2} \cdot r + n^2 - n \cdot r = \frac{n(n+1)}{2} \cdot r + n^2 - n \cdot r = \frac{n(n+1)}{2} \cdot r + n^2 - n \cdot r = \frac{n(n+1)}{2} \cdot r + n^2 - n \cdot r = \frac{n(n+1)}{2} \cdot r + n^2 - n \cdot r = \frac{n(n+1)}{2} \cdot r + n^2 - n \cdot r = \frac{n(n+1)}{2} \cdot r + n^2 - n \cdot r = \frac{n(n+1)}{2} \cdot r + n^2 - n \cdot r = \frac{n(n+1)}{2} \cdot r + n^2 - n \cdot r = \frac{n(n+1)}{2} \cdot r + n^2 - n \cdot r = \frac{n(n+1)}{2} \cdot r + n^2 - n \cdot r = \frac{n(n+1)}{2} \cdot r + n^2 - n \cdot r = \frac{n(n+1)}{2} \cdot r + n^2 - n \cdot r = \frac{n(n+1)}{2} \cdot r + n^2 - n \cdot r = \frac{n(n+1)}{2} \cdot r + n^2 - n \cdot r = \frac{n(n+1)}{2} \cdot r + n^2 - n \cdot r = \frac{n(n+1)}{2} \cdot r + n^2 - n \cdot r = \frac{n(n+1)}{2} \cdot r + n^2 - n \cdot r = \frac{n(n+1)}{2} \cdot r + n^2 - n \cdot r = \frac{n(n+1)}{2} \cdot r + n^2 - n \cdot r = \frac{n(n+1)}{2} \cdot r + n^2 - n \cdot r = \frac{n(n+1)}{2} \cdot r + n^2 - n \cdot r = \frac{n(n+1)}{2} \cdot r + n^2 - n \cdot r = \frac{n(n+1)}{2} \cdot r + n^2 - n \cdot r = \frac{n(n+1)}{2} \cdot r + n^2 - n \cdot r = \frac{n(n+1)}{2} \cdot r + n^2 - n \cdot r = \frac{n(n+1)}{2} \cdot r + n^2 - n \cdot r = \frac{n(n+1)}{2} \cdot r + n^2 - n \cdot r = \frac{n(n+1)}{2} \cdot r + n^2 - n \cdot r = \