To analyze the impact of the code snippet provided, we start by understanding the initial state:

- `n` is an integer such that \(1 \leq n \leq 10^{18}\)
- `total_days` is \(2^n\)
- `numerator` is \((2^n \cdot (2^n - 1)) \cdot (2^n - 2)\)
- `denominator` is \(2^{2n}\)
- `k` is greater than 0
- `i` is 2

The code snippet modifies the `denominator` variable:

```
denominator *= total_days
```

This operation means that `denominator` is multiplied by `total_days`. Since `total_days` is defined as \(2^n\), we can substitute that into the equation:

- `denominator` was initially \(2^{2n}\)
- `total_days` is \(2^n\)

After the operation, the new value of `denominator` becomes:

\[
denominator = 2^{2n} \cdot 2^n = 2^{2n + n} = 2^{3n}
\]

The other variables (`n`, `total_days`, `numerator`, `k`, and `i`) remain unchanged.

Thus, the output state reflecting the changes will be:

Output State: **`n` is an integer such that 1 ≤ `n` ≤ 10^18, `total_days` is 2^n, `numerator` is (2^n * (2^n - 1)) * (2^n - 2), `denominator` is 2^(3n), `k` is greater than 0, `i` is 2**