Let's break down the initial state and the conditions step by step to determine what will be printed.

1. **Variables and their definitions:**
   - `t` is a positive integer such that \(1 \leq t \leq 10^4\).
   - `n` is `r[0]`.
   - `m` is `r[1]`.
   - `x1` is `r[2] + a`.
   - `y1` is either 1 or `m`.
   - `x2` is `r[4] - a`.
   - `y2` is adjusted based on the condition `y1 <= y2`.
   - `a` is `m - y1` if `y2` is less than `y1`, otherwise `a` is `y1 - 1`.
   - `b` is `x2 - x1`.
   - `c` is `m - y2` if `y2` is less than `y1`, otherwise `c` is `r[5] - m`.

2. **Conditions:**
   - `b // 2 \leq a`
   - `abs(x2 - c) < x1 + c`
   - `y1 > m` or `y1 <= 0`
   - `x1 > n` or `x1 < 1`.

Given these conditions, let's analyze the possible values for `y1`:

- `y1` can be either 1 or `m`.
- If `y1 = 1`, then `a = m - 1` (since `y2` must be greater than or equal to `y1`).
- If `y1 = m`, then `a = m - m = 0` (which contradicts the condition `b // 2 \leq a` because `b` would be negative or zero).

Therefore, `y1` must be 1, and `a = m - 1`.

Next, let's determine `y2`:
- Since `y1 = 1` and `y2` must be greater than or equal to `y1`, `y2` must be 1 (the only value that satisfies both conditions).

Now, let's find `a` again:
- `a = m - 1`.

Next, let's determine `c`:
- Since `y2 = 1`, `c = m - 1` (if `y2` is less than `y1`, which it isn't in this case).

Finally, let's check the other conditions:
- `b = x2 - x1 = (r[4] - (r[2] + (m - 1))) - (r[2] + (m - 1)) = r[4] - 2 * (r[2] + m - 1)`.
- `abs(x2 - c) = abs((r[4] - (m - 1)) - (m - 1)) = abs(r[4] - 2 * (m - 1))`.
- `abs(r[4] - 2 * (m - 1)) < (r[2] + (m - 1)) + (m - 1) = r[2] + 2 * (m - 1)`.

Given the conditions, the print statement `print('draw')` will execute.

Output: **draw**