Postcondition: ***`n` and `m` are positive integers such that 1 <= n, m <= 2 * 10^6, `T` is greater than 0, `t` is 1, `a` is the integer value of `info[0]`, `b` is the integer value of `info[1]` and must be at least 1, `i` is 1, `x` is `((a - 1 * (1 - 1)) // 1)`, and the expression `((a - i * (i - 1)) // i` has been evaluated and added to `suma`. If `((a - i * (i - 1)) % i ** 2 == 0` and `i * (i - 1) % i ** 2 == 0`, then `suma` is `((a - 1 * (1 - 1)) // 1) + 1` and `((a - i * (i - 1)) % i` remains unchanged. Otherwise, `suma` is `((a - 1 * (1 - 1)) // 1)`.***