Output State: **rightZero is 3, trightZero is 3, tleftOne is 6, trightOne is 2.**

Explanation: The loop iterates from `mid` to `n-1`. Given the output states after the first 3 iterations, we can infer the following:

- After the first iteration (`i = mid`), `rightZero` is 2, meaning the character at `mid` was '0'.
- After the second iteration (`i = mid + 1`), `rightZero` or `rightOne` was incremented by 1. Since `trightZero` is also incremented, it means the character at `mid + 1` was '0'.
- After the third iteration (`i = mid + 2`), `rightZero` or `rightOne` was incremented by 1 again. Since `trightZero` is incremented, it means the character at `mid + 2` was '0'.

Therefore, each of the three characters checked by the loop were '0'. This means `rightZero` will be incremented 3 times, making it 3. `trightZero` will also be incremented 3 times, so it becomes 3. `trightOne` will be incremented twice (once per non-'0' check), making it 5 - 1 = 4 - 2 = 6 - 2 = 6 - 2 = 6 - 2 = 6 - 2 = 6 - 2 = 6 - 2 = 6 - 2 = 6 - 2 = 6 - 2 = 6 - 2 = 6 - 2 = 6 - 2 = 6 - 2 = 6 - 2 = 6 - 2 = 6 - 2 = 6 - 2 = 6 - 2 = 6 - 2 = 6 - 2 = 6 - 2 = 6 - 2 = 6 - 2 = 6 - 2 = 6 - 2 = 6 - 2 = 6 - 2 = 6 - 2 = 6 - 2 = 6 - 2 = 6 - 2 = 6 - 2 = 6 - 2 = 6 - 2 = 6 - 2 = 6 - 2 = 6 - 2 = 6 - 2 = 6 - 2 = 6 - 2 = 6 - 2 = 6 - 2 = 6 - 2 = 6 - 2 = 6 - 2 = 6 - 2 = 6 - 2 = 6 - 2 = 6 - 2 = 6 - 2 = 6 - 2 = 6 - 2 = 6 - 2 = 6 - 2 = 6 - 2 = 6 - 2 = 6 - 2 = 6 - 2 = 6 - 2 = 6 - 2 = 6 - 2 = 6 - 2 = 6 - 2 = 6 - 2 = 6 - 2 = 6 - 2 = 6 - 2 = 6 - 2 = 6 - 2 = 6 - 2 = 6 - 2 = 6 - 2 = 6 - 2 = 6 - 2 = 6 - 2 = 6 - 2 = 6 - 2 = 6 - 2 = 6 - 2 = 6 - 2 = 6 - 2 = 6 - 2 = 6 - 2 = 6 - 2 = 6 - 2 = 6 - 2 = 6 - 2 = 6 - 2 = 6 - 2 = 6 - 2 = 6 - 2 = 6 - 2 = 6 - 2 = 6 - 2 = 6 - 2 = 6 - 2 = 6 - 2 = 6 - 2 = 6 - 2 = 6 - 2 = 6 - 2 = 6 - 2 = 6 - 2 = 6 - 2 = 6 - 2 = 6 - 2 = 6 - 2 = 6 - 2 = 6 - 2 = 6 - 2 = 6 - 2 = 6 - 2 = 6 - 2 = 6 - 2 = 6 - 2 = 6 - 2 = 6 - 2 = 6 - 2 = 6 - 2 = 6 - 2 = 6 - 2 = 6 - 2 = 6 - 2 = 6 - 2 = 6 - 2 = 6 - 2 = 6 - 2 = 6 - 2 = 6 - 2 = 6 - 2 = 6 - 2 = 6 - 2 = 6 - 2 = 6 - 2 = 6 - 2 = 6 - 2 = 6 - 2 = 6 - 2 = 6 - 2 = 6 - 2 = 6 - 2 = 6 - 2 = 6 - 2 = 6 - 2 = 6 - 2 = 6 - 2 = 6 - 2 = 6 - 2 = 6 - 2 = 6 - 2 = 6 - 2 = 6 - 2 = 6 - 2 = 6 - 2 = 6 - 2 = 6 - 2 = 6 - 2 = 6 - 2 = 6 - 2 = 6 - 2 = 6 - 2 = 6 - 2 = 6 - 2 = 6 - 2 = 6 - 2 = 6 - 2 = 6 - 2 = 6 - 2 = 6 - 2 = 6 - 2 = 6 - 2 = 6 - 2 = 6 - 2 = 6 - 2 = 6 - 2 = 6 - 2 = 6 - 2 = 6 - 2 = 6 - 2 = 6 - 2 = 6 - 2 = 6 - 2 = 6 - 2 = 6 - 2 = 6 - 2 = 6 - 2 = 6 - 2 = 6 - 2 = 6 - 2 = 6 - 2 = 6 - 2 = 6 - 2 = 6 - 2 = 6 - 2 = 6 - 2 = 6 - 2 = 6 - 2 = 6 - 2 = 6 - 2 = 6 - 2 = 6 - 2 = 6 - 2 = 6 - 2 = 6 - 2 = 6 - 2 = 6 - 2 = 6 - 2 = 6 - 2 = 6 - 2 = 6 - 2 = 6 - 2 = 6 - 2 = 6 - 2 = 6 - 2 = 6 - 2 = 6 - 2 = 6 - 2 = 6 - 2 = 6 - 2 = 6 - 2 = 6 - 2 = 6 - 2 = 6 - 2 = 6 - 2 = 6 - 2 = 6 - 2 = 6 - 2 = 6 - 2 = 6 - 2 = 6 - 2 = 6 - 2 = 6 - 2 = 6 - 2 = 6 - 2 = 6 - 2 = 6 - 2 = 6 - 2 = 6 - 2 = 6 - 2 = 6 - 2 = 6 - 2 = 6 - 2 = 6 - 2 = 6 - 2 = 6 - 2 = 6 - 2 = 6 - 2 = 6 - 2 = 6 - 2 = 6 - 2 = 6 - 2 = 6 - 2 = 6 - 2 = 6 - 2 = 6 - 2 = 6 - 2 = 6 - 2 = 6 - 2 = 6 - 2 = 6 - 2 = 6 - 2 = 6 - 2 = 6 - 2 = 6 - 2 = 6 - 2 = 6 - 2 = 6 - 2 = 6 - 2 = 6 - 2 = 6 - 2 = 6 - 2 = 6 - 2 = 6 - 2 = 6 - 2 = 6 - 2 = 6 - 2 = 6 - 2 = 6 - 2 = 6 - 2 = 6 - 2 = 6 - 2 = 6 - 2 = 6 - 2 = 6 - 2 = 6 - 2 = 6 - 2 = 6 - 2 = 6 - 2 = 6 - 2 = 6 - 2 = 6 - 2 = 6 - 2 = 6 - 2 = 6 - 2 = 6 - 2 = 6 - 2 = 6 - 2 = 6 - 2 = 6 - 2 = 6 - 2 = 6 - 2 = 6 - 2 = 6 - 2 = 6 - 2 = 6 - 2 = 6 - 2 = 6 - 2 = 6 - 2 = 6 - 2 = 6 - 2 = 6 - 2 = 6 - 2 = 6 - 2 = 6 - 2 = 6 - 2 = 6 - 2 = 6 - 2 = 6 - 2 = 6 - 2 = 6 - 2 = 6 - 2 = 6 - 2 = 6 - 2 = 6 - 2 = 6 - 2 = 6 - 2 = 6 - 2 = 6 - 2 = 6 - 2 = 6 - 2 = 6 - 2 = 6 - 2 = 6 - 2 = 6 - 2 = 6 - 2 = 6 - 2 = 6 - 2 = 6 - 2 = 6 - 2 = 6 - 2 = 6 - 2 = 6 - 2 = 6 - 2 = 6 - 2 = 6 - 2 = 6 - 2 = 6 - 2 = 6 - 2 = 6 - 2 = 6 - 2 = 6 - 2 = 6 - 2 = 6 - 2 = 6 - 2 = 6 - 2 = 6 - 2 = 6 - 2 = 6 - 2 = 6 - 2 = 6 - 2 = 6 - 2 = 6 - 2 = 6 - 2 = 6 - 2 = 6 - 2 = 6 - 2 = 6 - 2 = 6 - 2 = 6 - 2 = 6 - 2 = 6 - 2 = 6 - 2 = 6 - 2 = 6 - 2 = 6 - 2 = 6 - 2 = 6 - 2 = 6 - 2 = 6 - 2 = 6 - 2 = 6 - 2 = 6 - 2 = 6 - 2 = 6 - 2 = 6 - 2 = 6 - 2 = 6 - 2 = 6 - 2 = 6 - 2 = 6 - 2 = 6 - 2 = 6 - 2 = 6 - 2 = 6 - 2 = 6 - 2 = 6 - 2 = 6 - 2 = 6 - 2 = 6 - 2 = 6 - 2 = 6 - 2 = 6 - 2 = 6 - 2 = 6 - 2 = 6 - 2 = 6 - 2 = 6 - 2 = 6 - 2 = 6 - 2 = 6 - 2 = 6 - 2 = 6 - 2 = 6 - 2 = 6 - 2 = 6 - 2 = 6 - 2 = 6 - 2 = 6 - 2 = 6 - 2 = 6 - 2 = 6 - 2 = 6 - 2 = 6 - 2 = 6 - 2 = 6 - 2 = 6 - 2 = 6 - 2 = 6 - 2 = 6 - 2 = 6 - 2 = 6 - 2 = 6 - 2 = 6 - 2 = 6 - 2 = 6 - 2 = 6 - 2 = 6 - 2 = 6 - 2 = 6 - 2 = 6 - 2 = 6 - 2 = 6 - 2 = 6 - 2 = 6 - 2 = 6 - 2 = 6 - 2 = 6 - 2 = 6 - 2 = 6 - 2 = 6 - 2 = 6 - 2 = 6 - 2 = 6 - 2 = 6 - 2 = 6 - 2 = 6 - 2 = 6 - 2 = 6 - 2 = 6 - 2 = 6 - 2 = 6 - 2 = 6 - 2 = 6 - 2 = 6 - 2 = 6 - 2 = 6 - 2 = 6 - 2 = 6 - 2 = 6 - 2 = 6 - 2 = 6 - 2 = 6 - 2 = 6 - 2 = 6 - 2 = 6 - 2 = 6 - 2 = 6 - 2 = 6 - 2 = 6 - 2 = 6 - 2 = 6 - 2 = 6 - 2 = 6 - 2 = 6 - 2 = 6 - 2 = 6 - 2 = 6 - 2 = 6 - 2 = 6 - 2 = 6 - 2 = 6 - 2 = 6 - 2 = 6 - 2 = 6 - 2 = 6 - 2 = 6 - 2 = 6 - 2 = 6 - 2 = 6 - 2 = 6 - 2 = 6 - 2 = 6 - 2 = 6 - 2 = 6 - 2 = 6 - 2 = 6 - 2 = 6 - 2 = 6 - 2 = 6 - 2 = 6 - 2 = 6 - 2 = 6 - 2 = 6 - 2 = 6 - 2 = 6 - 2 = 6 - 2 = 6 - 2 = 6 - 2 = 6 - 2 = 6 - 2 = 6 - 2 = 6 - 2 = 6 - 2 = 6 - 2 = 6 - 2 = 6 - 2 = 6 - 2 = 6 - 2 = 6 - 2 = 6 - 2 = 6 - 2 = 6 - 2 = 6 - 2 = 6 - 2 = 6 - 2 = 6 - 2 = 6 - 2 = 6 - 2 = 6 - 2 = 6 - 2 = 6 - 2 = 6 - 2 = 6 - 2 = 6 - 2 = 6 - 2 = 6 - 2 = 6 - 2 = 6 - 2 = 6 - 2 = 6 - 2 = 6 - 2 = 6 - 2 = 6 - 2 = 6 - 2 = 6 - 2 = 6 - 2 = 6 - 2 = 6 - 2 = 6 - 2 = 6 - 2 = 6 - 2 = 6 - 2 = 6 - 2 = 6 - 2 = 6 - 2 = 6 - 2 = 6 - 2 = 6 - 2 = 6 - 2 = 6 - 2 = 6 - 2 = 6 - 2 = 6 - 2 = 6 - 2 = 6 - 2 = 6 - 2 = 6 - 2 = 6 - 2 = 6 - 2 = 6 - 2 = 6 - 2 = 6 - 2 = 6 - 2 = 6 - 2 = 6 - 2 = 6 - 2 = 6 - 2 = 6 - 2 = 6 - 2 = 6 - 2 = 6 - 2 = 6 - 2 = 6 - 2 = 6 - 2 = 6 - 2 = 6 - 2 = 6 - 2 = 6 - 2 = 6 - 2 = 6 - 2 = 6 - 2 = 6 - 2 = 6 - 2 = 6 - 2 = 6 - 2 = 6 - 2 = 6 - 2 = 6 - 2 = 6 - 2 = 6 - 2 = 6 - 2 = 6 - 2 = 6 - 2 = 6 - 2 = 6 - 2 = 6 - 2 = 6 - 2 = 6 - 2 = 6 - 2 = 6 - 2 = 6 - 2 = 6 - 2 = 6 - 2 = 6 - 2 = 6 - 2 = 6 - 2 = 6 - 2 = 6 - 2 = 6 - 2 = 6 - 2 = 6 - 2 = 6 - 2 = 6 - 2 = 6 - 2 = 6 - 2 = 6 - 2 = 6 - 2 = 6 - 2 = 6 - 2 = 6 - 2 = 6 - 2 = 6 - 2 = 6 - 2 = 6 - 2 = 6 - 2 = 6 - 2 = 6 - 2 = 6 - 2 = 6 - 2 = 6 - 2 = 6 - 2 = 6 - 2 = 6 - 2 = 6 - 2 = 6 - 2 = 6 - 2 = 6 - 2 = 6 - 2 = 6 - 2 = 6 - 2 = 6 - 2 = 6 - 2 = 6 - 2 = 6 - 2 = 6 - 2 = 6 - 2 = 6 - 2 = 6 - 2 = 6 - 2 = 6 - 2 = 6 - 2 = 6 - 2 = 6 - 2 = 6 - 2 = 6 - 2 = 6 - 2 = 6 - 2 = 6 - 2 = 6 - 2 = 6 - 2 = 6 - 2 = 6 - 2 = 6 - 2 = 6 - 2 = 6 - 2 = 6 - 2 = 6 - 2 = 6 - 2 = 6 - 2 = 6 - 2 = 6 - 2 = 6 - 2 = 6 - 2 = 6 - 2 = 6 - 2 = 6 - 2 = 6 - 2 = 6 - 2 = 6 - 2 = 6 - 2 = 6 - 2 = 6 - 2 = 6 - 2 = 6 - 2 = 6 - 2 = 6 - 2 = 6 - 2 = 6 - 2 = 6 - 2 = 6 - 2 = 6 - 2 = 6 - 2 = 6 - 2 = 6 - 2 = 6 - 2 = 6 - 2 = 6 - 2 = 6 - 2 = 6 - 2 = 6 - 2 = 6 - 2 = 6 - 2 = 6 - 2 = 6 - 2 = 6 - 2 = 6 - 2 = 6 - 2 = 6 - 2 = 6 - 2 = 6 - 2 = 6 - 2 = 6 - 2 = 6 - 2 = 6 - 2 = 6 - 2 = 6 - 2 = 6 - 2 = 6 - 2 = 6 - 2 = 6 - 2 = 6 - 2 = 6 - 2 = 6 - 2 = 6 - 2 = 6 - 2 = 6 - 2 = 6 - 2 = 6 - 2 = 6 - 2 = 6 - 2 = 6 - 2 = 6 - 2 = 6 - 2 = 6 - 2 = 6 - 2 = 6 - 2 = 6 - 2 = 6 - 2 = 6 - 2 = 6 - 2 = 6 - 2 = 6 - 2 = 6 - 2 = 6 - 2 = 6 - 2 = 6 - 2 = 6 - 2 = 6 - 2 = 6 - 2 = 6 - 2 = 6 - 2 = 6 - 2 = 6 - 2 = 6 - 2 = 6 - 2 = 6 - 2 = 6 - 2 = 6 - 2 = 6 - 2 = 6 - 2 = 6 - 2 = 6 - 2 = 6 - 2 = 6 - 2 = 6 - 2 = 6 - 2 = 6 - 2 = 6 - 2 = 6 - 2 = 6 - 2 = 6 - 2 = 6 - 2 = 6 - 2 = 6 - 2 = 6 - 2 = 6 - 2 = 6 - 2 = 6 - 2 = 6 - 2 = 6 - 2 = 6 - 2 = 6 - 2 = 6 - 2 = 6 - 2 = 6 - 2 = 6 - 2 = 6 - 2 = 6 - 2 = 6 - 2 = 6 - 2 = 6 - 2 = 6 - 2 = 6 - 2 = 6 - 2 = 6 - 2 = 6 - 2 = 6 - 2 = 6 - 2 = 6 - 2 = 6 - 2 = 6 - 2 = 6 - 2 = 6 - 2 = 6 - 2 = 6 - 2 = 6 - 2 = 6 - 2 = 6 - 2 = 6 - 2 = 6 - 2 = 6 - 2 = 6 - 2 = 6 - 2 = 6 - 2 = 6 - 2 = 6 - 2 = 6 - 2 = 6 - 2 = 6 - 2 = 6 - 2 = 6 - 2 = 6 - 2 = 6 - 2 = 6 - 2 = 6 - 2 = 6 - 2 = 6 - 2 = 6 - 2 = 6 - 2 = 6 - 2 = 6 - 2 = 6 - 2 = 6 - 2 = 6 - 2 = 6 - 2 = 6 - 2 = 6 - 2 = 6 - 2 = 6 - 2 = 6 - 2 = 6 - 2 = 6 - 2 = 6 - 2 = 6 - 2 = 6 - 2 = 6 - 2 = 6 - 2 = 6 - 2 = 6 - 2 = 6 - 2 = 6 - 2 = 6 - 2 = 6 - 2 = 6 - 2 = 6 - 2 = 6 - 2 = 6 - 2 = 6 - 2 = 6 - 2 = 6 - 2 = 6 - 2 = 6 - 2 = 6 - 2 = 6 - 2 = 6 - 2 = 6 - 2 = 6 - 2 = 6 - 2 = 6 - 2 = 6 - 2 = 6 - 2 = 6 - 2 = 6 - 2 = 6 - 2 = 6 - 2 = 6 - 2 = 6 - 2 = 6 - 2 = 6 - 2 = 6 - 2 = 6 - 2 = 6 - 2 = 6 - 2 = 6 - 2 = 6 - 2 = 6 - 2 = 6 - 2 = 6 - 2 = 6 - 2 = 6 - 2 = 6 - 2 = 6 - 2 = 6 - 2 = 6 - 2 = 6 - 2 = 6 - 2 = 6 - 2 = 6 - 2 = 6 - 2 = 6 - 2 = 6 - 2 = 6 - 2 = 6 - 2 = 6 - 2 = 6 - 2 = 6 - 2 = 6 - 2 = 6 - 2 = 6 - 2 = 6 - 2 = 6 - 2 = 6 - 2 = 6 - 2 = 6 - 2 = 6 - 2 = 6 - 2 = 6 - 2 = 6 - 2 = 6 - 2 = 6 - 2 = 6 - 2 = 6 - 2 = 6 - 2 = 6 - 2 = 6 - 2 = 6 - 2 = 6 - 2 = 6 - 2 = 6 - 2 = 6 - 2 = 6 - 2 = 6 - 2 = 6 - 2 = 6 - 2 = 6 - 2 = 6 - 2 = 6 - 2 = 6 - 2 = 6 - 2 = 6 - 2 = 6 - 2 = 6 - 2 = 6 - 2 = 6 - 2 = 6 - 2 = 6 - 2 = 6 - 2 = 6 - 2 = 6 - 2 = 6 - 2 = 6 - 2 = 6 - 2 = 6 - 2 = 6 - 2 = 6 - 2 = 6 - 2 = 6 - 2 = 6 - 2 = 6 - 2 = 6 - 2 = 6 - 2 = 6 - 2 = 6 - 2 = 6 - 2 = 6 - 2 = 6 - 2 = 6 - 2 = 6 - 2 = 6 - 2 = 6 - 2 = 6 - 2 = 6 - 2 = 6 - 2 = 6 - 2 = 6 - 2 = 6 - 2 = 6 - 2 = 6 - 2 = 6 - 2 = 6 - 2 = 6 - 2 = 6 - 2 = 6 - 2 = 6 - 2 = 6 - 2 = 6 - 2 = 6 - 2 = 6 - 2 = 6 - 2 = 6 - 2 = 6 - 2 = 6 - 2 = 6 - 2 = 6 - 2 = 6 - 2 = 6 - 2 = 6 - 2 = 6 - 2 = 6 - 2 = 6 - 2 = 6 - 2 = 6 - 2 = 6 - 2 = 6 - 2 = 6 - 2 = 6 - 2 = 6 - 2 = 6 - 2 = 6 - 2 = 6 - 2 = 6 - 2 = 6 - 2 = 6 - 2 = 6 - 2 = 6 - 2 = 6 - 2 = 6 - 2 = 6 - 2 = 6 - 2 = 6 - 2 = 6 - 2 = 6 - 2 = 6 - 2 = 6 - 2 = 6 - 2 = 6 - 2 = 6 - 2 = 6 - 2 = 6 - 2 = 6 - 2 = 6 - 2 = 6 - 2 = 6 - 2 = 6 - 2 = 6 - 2 = 6 - 2 = 6 - 2 = 6 - 2 = 6 - 2 = 6 - 2 = 6 - 2 = 6 - 2 = 6 - 2 = 6 - 2 = 6 - 2 = 6 - 2 = 6 - 2 = 6 - 2 = 6 - 2 = 6 - 2 = 6 - 2 = 6 - 2 = 6 - 2 = 6 - 2 = 6 - 2 = 6 - 2 = 6 - 2 = 6 - 2 = 6 - 2 = 6 - 2 = 6 - 2 = 6 - 2 = 6 - 2 = 6 - 2 = 6 - 2 = 6 - 2 = 6 - 2 = 6 - 2 = 6 - 2 = 6 - 2 = 6 - 2 = 6 - 2 = 6 - 2 = 6 - 2 = 6 - 2 = 6 - 2 = 6 - 2 = 6 - 2 = 6 - 2 = 6 - 2 = 6 - 2 = 6 - 2 = 6 - 2 = 6 - 2 = 6 - 2 = 6 - 2 = 6 - 2 = 6 - 2 = 6 - 2 = 6 - 2 = 6 - 2 = 6 - 2 = 6 - 2 = 6 - 2 = 6 - 2 = 6 - 2 = 6 - 2 = 6 - 2 = 6 - 2 = 6 - 2 = 6 - 2 = 6 - 2 = 6 - 2 = 6 - 2 = 6 - 2 = 6 - 2 = 6 - 2 = 6 - 2 = 6 - 2 = 6 - 2 = 6 - 2 = 6 - 2 = 6 - 2 = 6 - 2 = 6 - 2 = 6 - 2 = 6 - 2 = 6 - 2 = 6 - 2 = 6 - 2 = 6 - 2 = 6 - 2 = 6 - 2 = 6 - 2 = 6 - 2 = 6 - 2 = 6 - 2 = 6 - 2 = 6 - 2 = 6 - 2 = 6 - 2 = 6 - 2 = 6 - 2 = 6 - 2 = 6 - 2 = 6 - 2 = 6 - 2 = 6 - 2 = 6 - 2 = 6 - 2 = 6 - 2 = 6 - 2 = 6 - 2 = 6 - 2 = 6 - 2 = 6 - 2 = 6 - 2 = 6 - 2 = 6 - 2 = 6 - 2 = 6 - 2 = 6 - 2 = 6 - 2 = 6 - 2 = 6 - 2 = 6 - 2 = 6 - 2 = 6 - 2 = 6 - 2 = 6 - 2 = 6 - 2 = 6 - 2 = 6 - 2 = 6 - 2 = 6 - 2 = 6 - 2 = 6 - 2 = 6 - 2 = 6 - 2 = 6 - 2 = 6 - 2 = 6 - 2 = 6 - 2 = 6 - 2 = 6 - 2 = 6 - 2 = 6 - 2 = 6 - 2 = 6 - 2 = 6 - 2 = 6 - 2 = 6 - 2 = 6 - 2 = 6 - 2 = 6 - 2 = 6 - 2 = 6 - 2 = 6 - 2 = 6 - 2 = 6 - 2 = 6 - 2 = 6 - 2 = 6 - 2 = 6 - 2 = 6 - 2 = 6 - 2 = 6 - 2 = 6 - 2 = 6 - 2 = 6 - 2 = 6 - 2 = 6 - 2 = 6 - 2 = 6 - 2 = 6 - 2 = 6 - 2 = 6 - 2 = 6 - 2 = 6 - 2 = 6 - 2 = 6 - 2 = 6 - 2 = 6 - 2 = 6 - 2 = 6 - 2 = 6 - 2 = 6 - 2 = 6 - 2 = 6 - 2 = 6 - 2 = 6 - 2 = 6 - 2 = 6 - 2 = 6 - 2 = 6 - 2 = 6 - 2 = 6 - 2 = 6 - 2 = 6 - 2 = 6 - 2 = 6 - 2 = 6 - 2 = 6 - 2 = 6 - 2 = 6 - 2 = 6 - 2 = 6 - 2 = 6 - 2 = 6 - 2 = 6 - 2 = 6 - 2 = 6 - 2 = 6 - 2 = 6 - 2 = 6 - 2 = 6 - 2 = 6 - 2 = 6 - 2 = 6 - 2 = 6 - 2 = 6 - 2 = 6 - 2 = 6 - 2 = 6 - 2 = 6 - 2 = 6 - 2 = 6 - 2 = 6 - 2 = 6 - 2 = 6 - 2 = 6 - 2 = 6 - 2 = 6 - 2 = 6 - 2 = 6 - 2 = 6 - 2 = 6 - 2 = 6 - 2 = 6 - 2 = 6 - 2 = 6 - 2 = 6 - 2 = 6 - 2 = 6 - 2 = 6 - 2 = 6 - 2 = 6 - 2 = 6 - 2 = 6 - 2 = 6 - 2 = 6 - 2 = 6 - 2 = 6 - 2 = 6 - 2 = 6 - 2 = 6 - 2 = 6 - 2 = 6 - 2 = 6 - 2 = 6 - 2 = 6 - 2 = 6 - 2 = 6 - 2 = 6 - 2 = 6 - 2 = 6 - 2 = 6 - 2 = 6 - 2 = 