Reasoning:
1. The problem requires constructing an array \( a \) such that \( x_i = a_i \bmod a_{i-1} \) for all \( 2 \leq i \leq n \).
2. The provided code attempts to solve this by setting \( a_1 \) to \( arr[0] + 1 \), and each subsequent \( a_i \) to the sum of \( arr[i-1] \) and the previous \( a_i \) until it exceeds \( arr[i-1] \). This logic seems flawed because it doesn't necessarily ensure that \( a_i \bmod a_{i-1} = x_i \).

Let's analyze the provided solution with the example from the problem statement:
- For the first test case: \( [2, 4, 1] \)
  - \( a_1 = arr[0] + 1 = 2 + 1 = 3 \)
  - \( a_2 = arr[1] + a_1 = 4 + 3 = 7 \)
  - \( a_3 = arr[2] + a_2 = 1 + 7 = 8 \)

This results in \( a = [3, 7, 8] \), but we need to check if \( 3 \bmod 7 = 2 \) and \( 7 \bmod 8 = 4 \), which is not true. Therefore, the constructed array does not satisfy the required condition.

Given the above analysis, the provided solution does not correctly generate the required array \( a \).

Correctness: **False**