Alright, I've got this problem to solve. Let's see what it's about. So, there's this physical education lesson in a school, and students are lining up and getting assigned numbers based on their positions and a parameter K. The goal is to figure out how many possible values of K are valid given Vasya's position and the number he received.

First, I need to understand how the numbering works. It says that the first K people get numbers 1 through K, and then the next K-2 people get numbers K-1 down to 2, and this pattern repeats every 2K-2 positions.

So, for example, if K is 3, the sequence would be:

Position: 1 2 3 4 5 6 7 8 9 10...

Numbers: 1 2 3 2 1 2 3 2 1 2...

Wait, in the example for K=3:

1:1, 2:2, 3:3, 4:2, 5:1, 6:2, 7:3, 8:2, 9:1, 10:2,...

Yes, that makes sense. So, every 2K-2 positions, which for K=3 is 4 positions, the pattern repeats.

Another example, for K=2:

Positions: 1 2 3 4 5 6 7 8...

Numbers: 1 2 1 2 1 2 1 2...

So, for K=2, the pattern repeats every 2 positions.

Given that, Vasya remembers his position N and the number X he received. We need to find how many K > 1 satisfy this condition.

Constraints:

- K > 1

- 1 ≤ X < N ≤ 10^9

- T ≤ 100 test cases

First, I need to find a way to relate N and X to K.

Let's think about the pattern:

- For K=K, the period is 2K-2.

- Within each period:

- Positions 1 to K: numbers 1 to K

- Positions K+1 to 2K-2: numbers K-1 to 2

So, for a given N, we need to find in which part of the period it falls and what number it should be assigned.

But this seems a bit complicated. Maybe there's a better way.

Looking at the example in the problem:

For N=10, X=2, the possible K are 2,3,5,6.

Let's see:

- K=2: sequence is 1,2,1,2,1,2,1,2,1,2. So position 10 is 2.

- K=3: sequence is 1,2,3,2,1,2,3,2,1,2. Position 10 is 2.

- K=5: sequence is 1,2,3,4,5,4,3,2,1,2. Position 10 is 2.

- K=6: sequence is 1,2,3,4,5,6,5,4,3,2. Position 10 is 2.

So, for these K values, position 10 gets number 2.

Now, I need a general way to find all K >1 where position N is assigned number X.

First, let's try to find the formula for the number assigned to position N for a given K.

Given K, the period is 2K-2.

So, for any position N, we can find its position within its period by computing M = N mod (2K-2).

If M is between 1 and K, the number is M.

If M is between K+1 and 2K-2, the number is 2K - M.

Wait, let's verify this.

For K=3, period is 4.

- Position 1: M=1, number=1

- Position 2: M=2, number=2

- Position 3: M=3, number=3

- Position 4: M=4, number=2K - M = 6 - 4 = 2

- Position 5: M=5 mod 4 =1, number=1

- Position 6: M=2, number=2

- Position 7: M=3, number=3

- Position 8: M=4, number=2

- Position 9: M=1, number=1

- Position 10: M=2, number=2

Yes, that matches the example.

Similarly, for K=2, period=2.

- Position 1: M=1, number=1

- Position 2: M=2, number=2

- Position 3: M=1, number=1

- Position 4: M=2, number=2

- Position 5: M=1, number=1

- Position 6: M=2, number=2

- Position 7: M=1, number=1

- Position 8: M=2, number=2

- Position 9: M=1, number=1

- Position 10: M=2, number=2

Again, matches the example.

So, the general formula is:

M = N mod (2K - 2)

if M >=1 and M <=K, number = M

else, number = 2K - M

We need this number to be equal to X.

So, we have:

If M >=1 and M <=K, M = X

Else, 2K - M = X

So, two cases:

1. M = X, and M <=K

2. M = 2K - X, and M > K

Let's consider both cases.

First case: M = X and M <=K

Which implies X <=K

Also, M = N mod (2K - 2) = X

So, N mod (2K - 2) = X

Which means N - X is divisible by (2K - 2)

So, N - X = P*(2K - 2), for some integer P >=0

Solving for K:

N - X = P*(2K - 2)

N - X = 2P*K - 4P

2P*K = N - X + 4P

K = (N - X + 4P)/(2P)

Wait, this seems messy. Maybe there's a better way.

Alternatively, let's express P in terms of K.

Wait, maybe it's better to consider the periodicity.

The period is 2K - 2.

So, positions repeat every 2K - 2 positions.

So, for M = N mod (2K - 2), M can be from 1 to 2K - 2.

If M <=K, number = M

Else, number = 2K - M

We need number = X

So, two cases:

1. M = X, and M <=K

2. M = 2K - X, and M > K

Let's consider both cases separately.

First case: M = X and M <=K

Which means X <=K

And M = X

But M = N mod (2K - 2) = X

So, N mod (2K - 2) = X

Which implies N - X is divisible by (2K - 2)

So, N - X = P*(2K - 2), for some integer P >=0

But since 2K - 2 = 2(K - 1), we can write:

N - X = P*2(K - 1)

So, N - X = 2P(K - 1)

So, 2P(K - 1) = N - X

So, K - 1 = (N - X)/(2P)

So, K = (N - X)/(2P) + 1

Since K must be an integer greater than 1, (N - X) must be divisible by 2P, and K must be integer and greater than 1.

Also, since P is a non-negative integer, P >=0

But P=0 would make K=1, which is invalid since K >1

So, P >=1

So, for each P >=1, if (N - X) is divisible by 2P, then K = (N - X)/(2P) + 1

And K must be greater than X, since in the first case M <=K, and M=X.

Wait, no, in the first case, M=X and X <=K

But we need to ensure that M <=K, which is already satisfied since M=X and X <=K

So, for each P >=1, if (N - X) is divisible by 2P, then K = (N - X)/(2P) +1 is a possible K

Similarly, for the second case:

M = 2K - X, and M >K

So, M = 2K - X > K

Which implies K > X

Also, M = N mod (2K - 2) = 2K - X

So, N mod (2K - 2) = 2K - X

Which implies N - (2K - X) is divisible by (2K - 2)

So, N - 2K + X = Q*(2K - 2), for some integer Q >=0

Let's solve for K:

N - 2K + X = Q*(2K - 2)

N + X = 2K + Q*2K - 2Q - X

Wait, that seems off.

Let me rearrange:

N - 2K + X = 2QK - 2Q

Bring all terms to one side:

N + X - 2K = 2QK - 2Q

N + X - 2K - 2QK + 2Q = 0

Factor terms with K:

N + X + 2Q - K(2 + 2Q) = 0

Now, solve for K:

K = (N + X + 2Q)/(2 + 2Q)

Simplify:

K = (N + X + 2Q)/(2(1 + Q))

K = [N + X + 2Q]/[2(1 + Q)]

For K to be integer, the numerator must be divisible by the denominator.

This seems complicated. Maybe there's a better approach.

Looking back, perhaps it's better to iterate over possible K and check if N mod (2K - 2) equals X or 2K - X, depending on the conditions.

But given the constraints, N and X can be up to 1e9, and T=100, we need an efficient way, better than O(N).

Wait, T is up to 100, N is up to 1e9, so we need an O(1) or O(sqrt(N)) solution.

Looking at the provided code, it seems to be attempting something similar.

Let's look at the provided code:

It reads T, then for each test case, reads N and X.

Then, it computes Y = N + X

Checks if Y is even; if not, prints 0.

Else, computes Q = (Y - 2)/2

Then calls func_1(Q, X), and if N >= 3X -2, adds func_1((N - X)/2, X)

Then combines the results, removes duplicates, and prints the count.

Wait, this seems obscure.

I need to understand what's happening here.

First, it checks if Y = N + X is even; if not, there are no solutions.

Why is that?

Let's see.

From earlier:

In the first case:

N - X = 2P(K - 1)

So, N - X must be even, which implies N and X have the same parity.

Similarly, in the second case:

N - 2K + X = Q*(2K - 2)

Which also seems to imply some parity conditions.

Wait, perhaps the author is combining both cases into one condition.

Let me try to derive a relationship between K, N, and X.

From the first case:

N - X = 2P(K - 1)

From the second case:

N - 2K + X = Q*(2K - 2)

Let's see if I can manipulate these equations.

From the first case:

N - X = 2P(K - 1)

So, K - 1 = (N - X)/(2P)

K = (N - X)/(2P) + 1

From the second case:

N - 2K + X = Q*(2K - 2)

Let me express K in terms of Q.

N - 2K + X = Q*2(K - 1)

N + X = 2K(Q + 1) - 2Q

N + X + 2Q = 2K(Q + 1)

K = (N + X + 2Q)/(2(Q + 1))

Hmm, still complicated.

Maybe there's a better way to approach this.

Let me consider the periodicity again.

The pattern repeats every 2K - 2 positions.

So, for a given K, the number assigned to position N is determined by N mod (2K - 2).

We need N mod (2K - 2) to be equal to X or 2K - X, depending on the conditions.

Wait, perhaps I can set up the equation N mod (2K - 2) = X or N mod (2K - 2) = 2K - X.

So, N ≡ X mod (2K - 2) or N ≡ 2K - X mod (2K - 2)

Therefore, N - X is divisible by (2K - 2) or N - (2K - X) is divisible by (2K - 2).

So, either N - X ≡ 0 mod (2K - 2) or N - 2K + X ≡ 0 mod (2K - 2)

From the first condition:

N - X ≡ 0 mod (2K - 2)

Which implies N - X is divisible by 2K - 2.

So, N - X = M*(2K - 2), for some integer M >=0

From this, solve for K:

N - X = M*(2K - 2)

N - X = 2M*K - 4M

2M*K = N - X + 4M

K = (N - X + 4M)/(2M)

This seems messy.

Let me try to rearrange:

N - X = 2M(K - 2)

Wait, that's not correct.

Wait, from N - X = 2M*K - 4M

N - X = 2M(K - 2)

Then, K - 2 = (N - X)/(2M)

K = (N - X)/(2M) + 2

So, K = (N - X)/(2M) + 2

Similarly, for the second condition:

N - 2K + X ≡ 0 mod (2K - 2)

N + X - 2K ≡ 0 mod (2K - 2)

N + X - 2K = Q*(2K - 2), for some integer Q >=0

Solve for K:

N + X - 2K = Q*(2K - 2)

N + X - 2K = 2QK - 2Q

Bring like terms together:

N + X + 2Q = 2K(Q + 1)

So, K = (N + X + 2Q)/(2(Q + 1))

This seems similar to what I had earlier.

This still doesn't look very helpful.

Maybe I should think differently.

Let me consider that 2K - 2 is a divisor of either N - X or N - 2K + X.

Wait, from the first condition:

N - X is divisible by 2K - 2

Similarly, from the second condition:

N - 2K + X is divisible by 2K - 2

So, 2K - 2 divides either N - X or N - 2K + X.

Let me denote D = 2K - 2

Then, K = (D + 2)/2

Since K >1, D >=2

So, D is an even number >=2

Now, D divides either N - X or N - 2K + X

But N - 2K + X = N - 2*((D + 2)/2) + X = N - (D + 2) + X = N - D - 2 + X

So, N - 2K + X = N - D - 2 + X

But D = 2K - 2 = 2*((D + 2)/2) - 2 = D + 2 - 2 = D

Wait, that's circular.

Let me re-express N - 2K + X in terms of D.

K = (D + 2)/2

So, 2K = D + 2

Thus, N - 2K + X = N - (D + 2) + X = N - D - 2 + X

And D divides N - D - 2 + X

Which means N - D - 2 + X ≡ 0 mod D

But N - D - 2 + X ≡ 0 mod D

Which implies N - 2 + X ≡ D mod D

Wait, that seems off.

Let me think differently.

We have two conditions:

1. D divides N - X

2. D divides N - 2K + X

But K = (D + 2)/2

So, N - 2K + X = N - (D + 2) + X = N - D - 2 + X

So, D divides N - D - 2 + X

Which means D divides (N - D - 2 + X)

But D divides D, so D divides (N - 2 + X)

Therefore, D divides (N + X - 2)

Similarly, from the first condition, D divides (N - X)

So, D divides both (N - X) and (N + X - 2)

Therefore, D divides any linear combination of these two.

Let me find the greatest common divisor.

Wait, perhaps I can find a relationship between these two expressions.

Let me denote A = N - X

B = N + X - 2

Then, D divides both A and B.

Therefore, D divides gcd(A, B)

So, D must be a divisor of gcd(N - X, N + X - 2)

But gcd(N - X, N + X - 2) = gcd(N - X, (N + X - 2) - (N - X)) = gcd(N - X, 2X - 2)

So, gcd(N - X, 2X - 2)

Therefore, D must be a divisor of gcd(N - X, 2X - 2)

But D = 2K - 2, and K >1, so D >=2

So, possible D values are divisors of gcd(N - X, 2X - 2) that are >=2 and even.

Then, K = (D + 2)/2

So, for each even D >=2 that divides gcd(N - X, 2X - 2), we can compute K = (D + 2)/2

And K must be integer and greater than 1.

So, the number of such K is equal to the number of even divisors of gcd(N - X, 2X - 2) that are >=2.

Wait, but in the provided code, it's doing something different.

It's computing Y = N + X, checking if Y is even, if not, prints 0.

Else, computes Q = (Y - 2)/2, then calls func_1(Q, X), and if N >= 3X -2, adds func_1((N - X)/2, X), combines the results, removes duplicates, and prints the count.

I need to understand what's happening here.

First, it checks if Y = N + X is even; if not, there are no solutions.

This aligns with my earlier conclusion that D must divide gcd(N - X, 2X - 2), and likely Y being even is a prerequisite.

Then, it computes Q = (Y - 2)/2

So, Q = (N + X - 2)/2

Then, it calls func_1(Q, X), which seems to find some values based on Q and X.

Similarly, if N >= 3X - 2, it adds results from func_1((N - X)/2, X)

func_1 seems to find divisors of Q that are >= X -1

Then, it combines the results, removes duplicates, and counts the number of unique K.

But I'm not entirely sure about this implementation.

Let me verify with the first test case:

N=10, X=2

Y=12, which is even.

Q=(12-2)/2=5

func_1(5,2) should find divisors of 5 that are >=1 (since X-1=1)

Divisors of 5 are 1 and 5, both >=1, so M=[1,5]

Then, since N=10 >= 3*2 -2=4, which is true, so add func_1((10-2)/2=4,2)

Divisors of 4 that are >=1 are 1,2,4

So M=[1,2,4]

Combine M=[1,5,1,2,4], remove duplicates [1,2,4,5]

Print length, which is 4, matching the first test case.

Similarly, for N=3, X=1

Y=4, even.

Q=(4-2)/2=1

func_1(1,1): divisors of 1 >=0 (X-1=0, but in code, it's X-1=0, but code has X-1 >=1, so for X=1, it's 0, which is not >=1, so no M

Then, N=3 >= 3*1 -2=1, which is true, so add func_1((3-1)/2=1,1)

func_1(1,1): same as above, no M

So, M=[]

Print 0, but the sample output is 1.

Wait, that doesn't match.

Wait, sample input is 5 test cases:

10 2

3 1

76 4

100 99

1000000000 500000000

Sample output is:

4

1

9

0

1

But according to my earlier calculation, for N=3, X=1, it should print 0, but sample output is 1.

So, perhaps there's a mistake in my understanding.

Wait, perhaps the condition is X-1 >=1, which is 0 >=1 is false, so no M from first func_1

But in the code, it's q // i >= x -1, and i >=x-1

For X=1, x-1=0, so i >=0 is always true, but in code, it's i >=x-1, which is i >=0, which is always true for i>=1

So, divisors of Q=1 are i=1, q//i=1, both >=0, so M=[1]

Then, N=3 >=3*1 -2=1, which is true, so add func_1((3-1)/2=1,1)

Same as above, M=[1]

Combine M=[1,1], remove duplicates [1], count=1, which matches sample output=1

Ok, so my earlier mistake was not considering that X-1 can be 0, and i >=0 is always true for i>=1

So, in this case, M=[1], and the count is 1, matching the sample.

Alright, so the code seems to be correctly implementing this logic.

Let me see the function func_1:

def func_1(q, x):

M = []

w = math.sqrt(q)

if w == w // 1 and w >= x - 1:

M += [w]

for i in range(1, int(w // 1)):

if q % i == 0:

if i >= x - 1:

M += [i]

if q // i >= x - 1:

M += [q // i]

return M

So, it's finding all divisors