To calculate the new value of `dp[i]`, we need to use the given formula:

\[ dp[i] = (dp[i - 1] + (i - 1) * dp[i - 2] * 2) \% (10^9 + 7) \]

Given:
- `i` is 5
- `dp[1]` is 1
- `dp[2]` is 3
- `dp[3]` is 7
- `dp[4]` is 25

We need to find `dp[5]`:

\[ dp[5] = (dp[4] + (5 - 1) * dp[3] * 2) \% (10^9 + 7) \]
\[ dp[5] = (25 + 4 * 7 * 2) \% (10^9 + 7) \]
\[ dp[5] = (25 + 56) \% (10^9 + 7) \]
\[ dp[5] = 81 \% (10^9 + 7) \]
\[ dp[5] = 81 \]

The other variables remain unchanged.

Output State: **`t` is truthy, `n` is the first integer from the input, `k` is greater than 0, `dp` is a list of `m + 1` zeros with `dp[1]` set to `1`, `dp[2]` set to `3`, `dp[3]` set to `7`, `dp[4]` set to `25`, and `dp[5]` set to `81`, `i` is 5**