The code snippet provided is `k = j + 1`. This updates the value of `k` to be `j + 1`. The other variables `t`, `n`, `m`, `b`, `c`, `d`, `e`, `i`, and `j` remain unchanged.

Given that `j` is defined as `i + 3`, the new value of `k` will be `(i + 3) + 1`, which simplifies to `i + 4`.

Output State: **`t` is an integer such that 1 ≤ t ≤ 10^4; `n` and `m` are integers such that 1 ≤ n, m ≤ 2 ⋅ 10^5; `b` is an integer greater than 0; `c` is an integer obtained from the input with `a` ≥ 1; `d` and `e` are the new input strings; `i` is `i + 1`; `j` is `i + 3`; `k` is `i + 4`.**