The given code snippet modifies the value of `ans1` by subtracting `a[i] * 2` from it. The values of other variables remain unchanged.

Initial State: `t` is an integer such that 0 ≤ t-2 ≤ 10^4, `n`, `k`, `x` are integers read from the input where 1 ≤ n ≤ 2 · 10^5, 1 ≤ k ≤ n, and `x` must be greater than 0; `a` is a list of `n` integers sorted in descending order as read from the input; `i` is 1; `ans1` is `sum(a) - 2 * a[k + x - 1] - 2 * a[0]`; `ans2` is `sum(a) - 2 * (a[k-1] + a[k] + ... + a[k + x - 2])`; `ans` is the maximum of `ans1` and `ans2` observed during the loop.

After executing `ans1 -= a[i] * 2`:
- `ans1` is now `sum(a) - 2 * a[k + x - 1] - 2 * a[0] - 2 * a[i]`.
- Other variables (`t`, `n`, `k`, `x`, `a`, `i`, `ans2`, `ans`) remain unchanged.

Output State: **`t` is an integer such that 0 ≤ t-2 ≤ 10^4, `n`, `k`, `x` are integers read from the input where 1 ≤ n ≤ 2 · 10^5, 1 ≤ k ≤ n, and `x` must be greater than 0; `a` is a list of `n` integers sorted in descending order as read from the input; `i` is 1; `ans1` is `sum(a) - 2 * a[k + x - 1] - 2 * a[0] - 2 * a[i]`; `ans2` is `sum(a) - 2 * (a[k-1] + a[k] + ... + a[k + x - 2])`; `ans` is the maximum of `ans1` and `ans2` observed during the loop.**