The code `current_sum += y` increments the value of `current_sum` by `y`. Given that `current_sum` was initially `x + 3y`, after adding `y`, the new value of `current_sum` becomes `x + 4y`. 

All other variables remain unchanged. Therefore, the updated values are:

- `n` is an integer such that \(1 < n \leq 2 \cdot 10^5\),
- `x` is an integer such that \(0 \leq x \leq 2 \cdot 10^5\),
- `y` is an integer such that \(1 \leq y \leq 2 \cdot 10^5\),
- `s` is an integer such that \(0 \leq s \leq 2 \cdot 10^5\),
- `sequence` is `[x, y, 2y]`,
- `current_sum` is now `x + 4y`.

The condition `current_sum + y <= s` still holds, and the difference between `s` and `current_sum` minus `y` remains divisible by `y`.

Output State: **`n` is an integer such that \(1 < n \leq 2 \cdot 10^5\), `x` is an integer such that \(0 \leq x \leq 2 \cdot 10^5\), `y` is an integer such that \(1 \leq y \leq 2 \cdot 10^5\), `s` is an integer such that \(0 \leq s \leq 2 \cdot 10^5\), `sequence` is `[x, y, 2y]`, `current_sum` is `x + 4y`.**