The code appends the value of `sequence[-1] % y` to the `sequence` list. According to the initial state, `sequence[-1]` is `x`, so the new element added to the sequence is `x % y`.

The condition \(current_sum + y > s\) or \((s - current_sum - y) \% y \neq 0\) holds true initially. However, the code does not change the values of `current_sum`, `s`, or `y`, so this condition remains unchanged.

Therefore, the output state includes the updated `sequence` and the unchanged `current_sum`, `s`, and `y`.

Output State: **`n` is an integer such that \(1 < n \leq 2 \cdot 10^5\), `x` is an integer such that \(0 \leq x \leq 2 \cdot 10^5\), `y` is an integer such that \(1 \leq y \leq 2 \cdot 10^5\), `s` is an integer such that \(0 \leq s \leq 2 \cdot 10^5\), `sequence` is `[x, x % y]`, `current_sum` is `x`, and the condition \(current_sum + y > s\) or \((s - current_sum - y) \% y \neq 0\) holds.**