The initial state provides that `current_sum` is defined as `x + 2 * (x % y) + y`, and the condition `current_sum + y > s` or `(s - current_sum - y) % y != 0` holds true. The code snippet `current_sum += y` adds the value of `y` to `current_sum`. Given this, let's update the value of `current_sum`:

1. Initial `current_sum` is `x + 2 * (x % y) + y`.
2. After executing `current_sum += y`, the new value of `current_sum` becomes `x + 2 * (x % y) + y + y`.

Thus, the new value of `current_sum` is `x + 2 * (x % y) + 2 * y`.

All other variables remain unchanged according to the initial state.

Output State: **`n` is an integer such that \(1 < n \leq 2 \cdot 10^5\), `x` is an integer such that \(0 \leq x \leq 2 \cdot 10^5\), `y` is an integer such that \(1 \leq y \leq 2 \cdot 10^5\), `s` is an integer such that \(0 \leq s \leq 2 \cdot 10^5\), `sequence` is `[x, x % y, x % y + y]`, `current_sum` is `x + 2 * (x % y) + 2 * y`, and the condition `current_sum + y > s` or `(s - current_sum - y) % y != 0` holds, and `i` is `n`.**