The code appends the value of `sequence[-1] % y` to the list `sequence`. Given that `sequence` initially is `[x, x % y]`, appending `sequence[-1] % y` means appending `(x % y) % y`, which simplifies to `x % y` since `x % y` is already less than `y`.

Therefore, the updated `sequence` will be `[x, x % y, x % y]`.

Other variables remain unchanged. The conditions involving `current_sum`, `s`, and `i` also remain valid post-execution.

Output State: **`n` is an integer such that \(1 < n \leq 2 \cdot 10^5\), `x` is an integer such that \(0 \leq x \leq 2 \cdot 10^5\), `y` is an integer such that \(1 \leq y \leq 2 \cdot 10^5\), `s` is an integer such that \(0 \leq s \leq 2 \cdot 10^5\), `sequence` is `[x, x % y, x % y]`, `current_sum` is \(x + (x \% y)\), and the condition `current_sum + y > s` or \((s - current_sum - y) \% y \neq 0\) holds, and `i` is \(n\)**.