Let's analyze the code step by step:

1. Initial State:
   - `n` is an integer such that \(1 < n \leq 2 \cdot 10^5\)
   - `x` is an integer such that \(0 \leq x \leq 2 \cdot 10^5\)
   - `y` is an integer such that \(1 \leq y \leq 2 \cdot 10^5\)
   - `s` is an integer such that \(0 \leq s \leq 2 \cdot 10^5\)
   - `sequence` is `[x, x % y, x % y]`
   - `current_sum` is \(x + (x \% y)\)
   - The condition `current_sum + y > s` or \((s - current_sum - y) \% y \neq 0\) holds
   - `i` is \(n\)

2. Code: `current_sum += sequence[-1]`

   - `sequence[-1]` refers to the last element of the list `sequence`, which is `x % y`.
   - So, `current_sum` is updated by adding `x % y` to its current value.

3. After updating `current_sum`, the new value of `current_sum` becomes:
   - \( \text{new\_current\_sum} = \text{current\_sum} + (x \% y) \)
   - Since `current_sum` was already defined as \(x + (x \% y)\), the new value of `current_sum` is:
     - \( \text{new\_current\_sum} = (x + (x \% y)) + (x \% y) = x + 2 \cdot (x \% y) \)

4. All other variables (`n`, `x`, `y`, `s`, `sequence`, and `i`) remain unchanged.

Therefore, the output state is:

Output State: **`n` is an integer such that \(1 < n \leq 2 \cdot 10^5\), `x` is an integer such that \(0 \leq x \leq 2 \cdot 10^5\), `y` is an integer such that \(1 \leq y \leq 2 \cdot 10^5\), `s` is an integer such that \(0 \leq s \leq 2 \cdot 10^5\), `sequence` is `[x, x % y, x % y]`, `current_sum` is \(x + 2 \cdot (x \% y)\), the condition `current_sum + y > s` or \((s - current_sum - y) \% y \neq 0\) still holds, and `i` is \(n\)**