`sequence.append(sequence[-1] + y)` appends the value of the last element in the list `sequence` plus `y` to the end of `sequence`. The value of `n` is updated to `n-1`, but since `sequence` and `current_sum` are not mentioned in the initial state, they are not affected. The previous value of `i` is `n-1`, which is now `n-2`.

Given the initial state:
- `n` is an integer such that \(1 < n \leq 2 \cdot 10^5\)
- `x` is an integer such that \(0 \leq x \leq 2 \cdot 10^5\)
- `y` is an integer such that \(1 \leq y \leq 2 \cdot 10^5\)
- `s` is an integer such that \(0 \leq s \leq 2 \cdot 10^5\)
- `i` is now \(n-1\)

After executing the code:
- The last element of `sequence` is increased by `y` and appended to `sequence`.
- `n` is updated to `n-1`, making `i` equal to `n-2`.

Output State: **`n` is an integer such that \(0 < n \leq 2 \cdot 10^5\) and `i` is \(n-2`; `x` is an integer such that \(0 \leq x \leq 2 \cdot 10^5\); `y` is an integer such that \(1 \leq y \leq 2 \cdot 10^5\); `s` is an integer such that \(0 \leq s \leq 2 \cdot 10^5\); `sequence` is updated with the new element `sequence[-1] + y`**