Postcondition: ***`n` is an integer such that \(1 < n \leq 2 \cdot 10^5\), `x` is an integer such that \(0 \leq x \leq 2 \cdot 10^5\), `y` is an integer such that \(1 \leq y \leq 2 \cdot 10^5\), `s` is an integer such that \(0 \leq s \leq 2 \cdot 10^5\), `i` is now \(n-1\). If `current_sum + y <= s` and \((s - current_sum - y) \% y == 0\), then `sequence` is updated with the new element `sequence[-1] + y` and `current_sum` is `current_sum + y`. Otherwise, `sequence` is the original sequence with its last element replaced by `last_element_of_sequence \% y` and `current_sum` is increased by `sequence[-1] \% y`.***