To determine what will be printed, let's break down the given initial state and the Python code snippet step by step.

### Initial State Breakdown:

1. **`t`**: An integer such that \(1 \leq t \leq 10^4\). This represents the number of test cases or iterations, but it does not directly affect the current code snippet since the snippet focuses on a single iteration.

2. **`l`**: The length of the input list `array`.

3. **`array`**: A list of integers read from input. For example, if the input is `[3, 1, 2]`, then `array = [3, 1, 2]`.

4. **`rev_array`**: The reverse of the `array`. If `array = [3, 1, 2]`, then `rev_array = [2, 1, 3]`.

5. **`alp`**: A list of lowercase English alphabet characters. So, `alp = ['a', 'b', 'c', ..., 'z']`.

6. **`ans`**: A list of characters where each character is determined by the formula `alp[rev_array[j:].count(rev_array[j]) - 1]` for `j` from 0 to `l-1`.

   - For each index `j` in `rev_array`, count how many times `rev_array[j]` appears in the sublist starting from `j` to the end of `rev_array`.
   - Subtract 1 from this count to get an index into the `alp` list.
   - Use this index to get the corresponding character from `alp`.

7. **`j`**: Set to `l-1` initially, but this value is not used in the provided print statement.

8. **`i`**: Incremented by 1, but this variable is not used in the provided print statement.

### Code Snippet Analysis:

The code snippet provided is:
```python
print(''.join(map(str, ans)))
```

This line joins the elements of the `ans` list into a single string and prints it.

### Calculation of `ans`:

Let's illustrate with an example. Suppose `array = [3, 1, 2]`.

1. **Reverse the array**: `rev_array = [2, 1, 3]`.
2. **Calculate `ans`**:
   - For `j = 0`: `rev_array[0]` is 2. Count of 2 in `rev_array[0:]` is 1. So, `ans[0] = alp[1 - 1] = alp[0] = 'a'`.
   - For `j = 1`: `rev_array[1]` is 1. Count of 1 in `rev_array[1:]` is 1. So, `ans[1] = alp[1 - 1] = alp[0] = 'a'`.
   - For `j = 2`: `rev_array[2]` is 3. Count of 3 in `rev_array[2:]` is 1. So, `ans[2] = alp[1 - 1] = alp[0] = 'a'`.

Thus, `ans = ['a', 'a', 'a']`.

### Final Output:

The `print` statement will output the joined string of `ans`.

Output: **aaa (where each character in the string corresponds to the count of the respective element in the reversed array minus one, mapped to the alphabet)**

In general, the output will be a string of characters derived from the counts of elements in the reversed array, mapped to the alphabet as described.

Output: **[resulting_string] (where resulting_string is the string formed by mapping the counts of elements in the reversed array minus one to the alphabet)**

For the specific example `array = [3, 1, 2]`, the output would be:

Output: **aaa**