Let's break down the problem step-by-step based on the initial state provided:

### Initial State Breakdown:
1. **Loop Breaking Condition:**
   - If the loop breaks during iteration `i`:
     - `r = a[i] + k // (i + 1)`
     - `rem = k % (i + 1)`
     - `y = n - 1 - i`
     - `k = 0`
     - `ii = x + 1` where `x` is the value of `ii` at the end of the previous iteration.

2. **Loop Completion Condition:**
   - If the loop completes all iterations:
     - `r = a[n - 1]`
     - `rem = 0`
     - `y = 0`
     - `k` is updated as `k - (i + 1) * (a[i + 1] - a[i])` for each iteration.
     - `ii = x + 1` where `x` is the value of `ii` at the end of the previous iteration.
     - `k = 0`

### Print Statement Analysis:
The print statement is:
```python
print((r - 1) * n + 1 + rem + y)
```

### Case 1: Loop Breaks During Iteration `i`
- `r = a[i] + k // (i + 1)`
- `rem = k % (i + 1)`
- `y = n - 1 - i`
- `k = 0`

Substituting these into the print statement:
- Since `k = 0`, `k // (i + 1) = 0` and `k % (i + 1) = 0`.
- Therefore, `r = a[i] + 0 = a[i]`
- `rem = 0`
- `y = n - 1 - i`

So the expression becomes:
```python
(r - 1) * n + 1 + rem + y
= (a[i] - 1) * n + 1 + 0 + (n - 1 - i)
= (a[i] - 1) * n + 1 + n - 1 - i
= (a[i] - 1) * n + n - i
= (a[i] * n - n) + n - i
= a[i] * n - i
```

### Case 2: Loop Completes All Iterations
- `r = a[n - 1]`
- `rem = 0`
- `y = 0`
- `k = 0`

Substituting these into the print statement:
- `r = a[n - 1]`
- `rem = 0`
- `y = 0`

So the expression becomes:
```python
(r - 1) * n + 1 + rem + y
= (a[n - 1] - 1) * n + 1 + 0 + 0
= (a[n - 1] - 1) * n + 1
= a[n - 1] * n - n + 1
```

### Conclusion:
The output depends on whether the loop breaks during iteration `i` or completes all iterations.

- If the loop breaks during iteration `i`, the output is `a[i] * n - i`.
- If the loop completes all iterations, the output is `a[n - 1] * n - n + 1`.

Given the initial state does not specify which case occurs, we need to consider both possibilities.

Output: **(a[i] * n - i) if the loop breaks during iteration i, otherwise (a[n - 1] * n - n + 1)**