The code `ans += n // 2 - 1` increments the value of `ans` by the integer division of `n` by 2 minus 1. Since `n` is even and divisible by 2, `n // 2` will be an integer. 

Given that `n` is an input integer such that `n` > 1 and `n` ≤ 2^`h`, and `h` is an input integer such that 1 ≤ `h` ≤ 50, the initial constraints on `h` and `n` remain the same. The value of `n` being even is also unchanged. 

The only variable that changes is `ans`, which is initially 0. After the execution of the code, `ans` becomes `0 + n // 2 - 1`, which simplifies to `n // 2 - 1`. 

Output State: **`h` is an input integer such that 1 ≤ `h` ≤ 50, `n` is an even input integer such that `n` > 1 and `n` ≤ 2^`h`, and `ans` is `n // 2 - 1`.**