Given the initial state:
- `t` is a positive integer such that \(1 \leq t < 10^4\).
- `_` is 2.
- `n` is the first integer from the input.
- `a` is the second integer from the input.
- `b` is the third integer from the input.

We need to evaluate the expression inside the `print` statement:
\[ \text{int}((2 * b - n + 1) * n / 2) \]

Let's break it down step-by-step:

1. **Expression Breakdown**:
   - \(2 * b - n + 1\): This part of the expression calculates a value based on `b` and `n`.
   - \((2 * b - n + 1) * n\): This multiplies the result of the previous step by `n`.
   - \(\frac{(2 * b - n + 1) * n}{2}\): This divides the result by 2.
   - \(\text{int}(\cdot)\): This converts the result to an integer.

2. **Values of Variables**:
   - `_` is 2 (though this variable is not used in the expression).
   - `n` is the first integer from the input.
   - `b` is the third integer from the input.

3. **Calculation**:
   - Letâ€™s assume specific values for `n` and `b` to illustrate the calculation. For example, if `n = 5` and `b = 3`:
     - \(2 * b - n + 1 = 2 * 3 - 5 + 1 = 6 - 5 + 1 = 2\)
     - \((2 * b - n + 1) * n = 2 * 5 = 10\)
     - \(\frac{(2 * b - n + 1) * n}{2} = \frac{10}{2} = 5\)
     - \(\text{int}(5) = 5\)

Therefore, the output of the `print` statement will be the integer value of the evaluated expression.

Output: **int((2 * b - n + 1) * n / 2) (where the value is calculated based on the given `n` and `b` from the input)**