Correctness: **True**

Explanation: The provided program correctly implements the logic described in the problem statement. The problem requires a function that takes a positive integer \( n \) and returns the sum of even-indexed binomial coefficients. For a positive integer \( n \), the sum of even-indexed binomial coefficients can be derived using the binomial theorem and properties of binomial coefficients. Specifically, the sum of even-indexed binomial coefficients for a given \( n \) is \( 2^{n-1} \).

The program defines a function `func_1` that takes a positive integer \( n \) and returns \( 2^{(n - 1)} \). This matches the required behavior:

- When \( n = 4 \), the sum of even-indexed binomial coefficients is \( 2^{(4 - 1)} = 2^3 = 8 \).
- When \( n = 6 \), the sum of even-indexed binomial coefficients is \( 2^{(6 - 1)} = 2^5 = 32 \).
- When \( n = 2 \), the sum of even-indexed binomial coefficients is \( 2^{(2 - 1)} = 2^1 = 2 \).

These test cases confirm that the function behaves as expected for the given inputs. Therefore, the program is correct according to the problem description.