Alright, I've got this problem to solve. Let's see what it's asking for. So, I'm given two positive integers, n and m, and I need to find the number of ordered pairs (a, b) where 1 ≤ a ≤ n and 1 ≤ b ≤ m, such that a + b is a multiple of b multiplied by the greatest common divisor of a and b. That is, a + b should be divisible by b * gcd(a, b).

First, I need to understand what this condition means. Let's denote gcd(a, b) as g. Then, b * g divides a + b. So, a + b is divisible by b * g.

I know that gcd(a, b) = g, which means both a and b are multiples of g. So, I can write a = g * a' and b = g * b', where gcd(a', b') = 1.

Substituting these into the condition:

a + b = g * a' + g * b' = g(a' + b')

And b * g = g * b' * g = g^2 * b'

So, the condition becomes that g(a' + b') is divisible by g^2 * b'. Simplifying, this means that a' + b' is divisible by g * b'.

But since gcd(a', b') = 1, g is the gcd of a and b, and a' and b' are coprime.

This seems a bit tricky. Maybe there's another way to approach this.

Let me think about the condition a + b is divisible by b * gcd(a, b). That is, b * gcd(a, b) divides a + b.

Let me consider the ratio (a + b) / (b * gcd(a, b)). This should be an integer.

Let me denote d = gcd(a, b). Then, a = d * a' and b = d * b', where gcd(a', b') = 1.

Substituting, we have:

(a + b) / (b * d) = (d * a' + d * b') / (d * b' * d) = d(a' + b') / (d^2 * b') = (a' + b') / (d * b')

For this to be an integer, d * b' must divide a' + b'.

But since a' and b' are coprime, and b' divides a' + b', then b' divides a' + b'. Since b' divides b', it must also divide a'. But since gcd(a', b') = 1, the only way b' divides a' is if b' = 1.

Wait, that seems off. If b' divides a' + b', and b' divides b', then b' divides a' + b' - b' = a'. But gcd(a', b') = 1, so b' = 1.

So, b' must be 1.

That means b = d * b' = d * 1 = d. So, b = d.

Therefore, gcd(a, b) = b.

This means that b divides a.

So, the condition simplifies to b divides a.

Wait, is that correct?

Let me verify.

If b divides a, then a = k * b for some integer k.

Then, a + b = k * b + b = (k + 1) * b.

And b * gcd(a, b) = b * b, since gcd(a, b) = b.

So, (a + b) / (b * gcd(a, b)) = (k + 1) * b / (b * b) = (k + 1) / b.

For this to be an integer, b must divide (k + 1).

But since a = k * b, then k = a / b.

So, (k + 1) = (a / b) + 1.

Then, (k + 1) / b = (a / b + 1) / b = (a + b) / (b^2).

Wait, that seems different from what I had earlier.

I think there's a mistake here.

Let me go back.

Given that b divides a, so a = k * b for some integer k ≥ 1.

Then, a + b = k * b + b = (k + 1) * b.

And b * gcd(a, b) = b * b, since gcd(a, b) = b.

So, (a + b) / (b * gcd(a, b)) = (k + 1) * b / (b^2) = (k + 1) / b.

For this to be an integer, b must divide (k + 1).

But k = a / b, which is an integer since b divides a.

So, k is an integer ≥ 1.

Thus, b divides (k + 1), where k = a / b.

So, b divides (a / b + 1).

Wait, that seems tricky.

Let me think differently.

Let me consider the condition again: b * gcd(a, b) divides a + b.

Let me denote d = gcd(a, b). Then, a = d * a' and b = d * b', with gcd(a', b') = 1.

Substituting, we have:

b * d = d * b' * d = d^2 * b'

And a + b = d * a' + d * b' = d(a' + b')

So, the condition is that d^2 * b' divides d(a' + b'), which simplifies to d * b' divides a' + b'.

Since a' and b' are coprime, and b' divides a' + b', then b' divides a'.

But since gcd(a', b') = 1, b' must be 1.

Therefore, b' = 1.

So, b = d * b' = d * 1 = d.

Thus, b = d, which means b = gcd(a, b).

But since b divides a (because gcd(a, b) = b), we have b divides a.

Therefore, the condition simplifies to b divides a.

So, the problem reduces to counting the number of ordered pairs (a, b) where 1 ≤ a ≤ n, 1 ≤ b ≤ m, and b divides a.

This seems much simpler.

So, for each b from 1 to m, count how many a in 1 to n are multiples of b.

This is equivalent to floor(n / b) for each b, and sum these up for b from 1 to m.

Wait, but in the problem, n and m can be up to 2*10^6, and there can be up to 10^4 test cases, with the sum of n and m over all test cases not exceeding 2*10^6.

So, I need an efficient way to compute this.

A naive approach would be, for each test case, iterate over each b from 1 to m, and for each b, compute floor(n / b), and sum these up.

But with n and m up to 2*10^6, and t up to 10^4, this would be too slow because it would be O(t * m), which could be up to 10^4 * 2*10^6 = 2*10^10 operations, which is unacceptable.

So, I need a better approach.

I recall that the sum of floor(n / b) over b from 1 to m can be computed efficiently using divisor summation techniques, possibly with number theory optimizations or by iterating over multiples of b.

One common optimization is to iterate over possible values of b and group terms where floor(n / b) is the same.

This is similar to the technique used in the sieve of Eratosthenes, where you iterate over multiples.

So, for a given n and m, I can iterate over multiples of k, and compute the contribution of each k.

Wait, let me think.

I need to compute sum over b=1 to m of floor(n / b).

This is a standard problem in competitive programming, and there are optimized ways to compute this sum without iterating over each b individually.

One such method is to iterate over possible values of floor(n / b), which can take only O(sqrt(n)) distinct values.

For each distinct value of floor(n / b) = k, find the range of b where this k is constant, and then compute the sum for that range.

This way, the total number of operations is O(sqrt(n)) per test case, which should be efficient enough since sqrt(2*10^6) is about 1414, and with t=10^4, it's about 1.4*10^7 operations, which should be acceptable.

So, I need to implement this optimized sum.

Let me try to outline the steps:

For each test case with given n and m:

- If n < m, swap n and m, because the sum is symmetric in n and m.

- Then, iterate over b from 1 to m, and for each b, add floor(n / b) to the sum.

But using the optimization, I can group the b's where floor(n / b) is the same.

So, for k from 1 to floor(n / 1):

- Find the range of b where floor(n / b) = k.

- This range can be found as b from ceil(n / (k + 1)) to floor(n / k).

- Then, the number of b's in this range is floor(n / k) - ceil(n / (k + 1)) + 1.

- But I have to make sure that b does not exceed m.

So, I need to adjust the range to be within 1 to m.

This seems a bit involved. Maybe there's a simpler way to implement this.

I recall that in Python, there's a way to compute sum(floor(n / b) for b in 1..m) efficiently by iterating over possible k values and calculating the contribution of each k.

Let me try to implement that.

Here's a plan:

def calculate_sum(n, m):

sum = 0

a = 1

while a <= n:

b = n // a

c = m // b

sum += b * (c - a + 1)

a = c + 1

return sum

Wait, I think I need to adjust this.

I found this code snippet, but I need to make sure I understand it.

Let me see.

In this code, 'a' is the current value of floor(n / b).

We start with a = 1.

Then, b = floor(n / a), and c = floor(m / b).

Then, the number of b's where floor(n / b) = a is c - a + 1.

Then, we add a * (c - a + 1) to the sum.

Then, set a = c + 1 and repeat.

Wait, but in the code above, it's sum += b * (c - a + 1), which seems incorrect because 'b' is floor(n / a), so perhaps it should be sum += a * (c - a + 1).

Wait, I'm getting confused.

Let me look for a standard implementation of sum(floor(n / b) for b in 1..m).

I recall that the standard way is to iterate over possible values of floor(n / b) = k, find the range of b where this k is constant, and then compute the sum for that range.

Here's a step-by-step breakdown:

Given n and m, we want to compute sum_{b=1}^m floor(n / b).

We observe that floor(n / b) can take on a limited number of integer values, and for each value k = floor(n / b), there is a range of b's where this k is constant.

To find these ranges:

- For a given k, find the minimal b_min where floor(n / b) = k.

- Find the maximal b_max where floor(n / b) = k.

Then, the number of b's in this range is b_max - b_min + 1.

The sum contributed by this k is k * (b_max - b_min + 1).

We can iterate over all possible k values and sum up these contributions.

To find b_min for a given k:

- b_min = floor(n / (k + 1)) + 1

To find b_max for a given k:

- b_max = floor(n / k)

But we need to ensure that b_min and b_max are within 1 to m.

So, the actual b_min is max(1, floor(n / (k + 1)) + 1)

And b_max is min(m, floor(n / k))

Then, if b_min <= b_max, the number of b's in this range is b_max - b_min + 1, and the sum contributed is k * (b_max - b_min + 1).

We need to iterate over all k from 1 to floor(n / 1), which is n.

But this can be optimized because k can only take on values up to n.

However, in practice, we can iterate k from 1 to n, but since n can be up to 2*10^6, and t up to 10^4, this might still be too slow.

Wait, but for each k, finding b_min and b_max is O(1), and k goes up to n, which is large, but with optimizations, it should be manageable.

Alternatively, there's a way to iterate over blocks where floor(n / b) is constant, similar to the divisor summation optimization.

Here's an optimized way to compute the sum:

def optimized_sum(n, m):

sum = 0

a = 1

while a <= n:

# Find the maximal b where floor(n / b) = floor(n / a)

b = n // a

# Find the minimal d where floor(n / d) = b

# Which is d = n // b

# But in this context, we need to find c = min(m, n // b)

c = min(m, n // b)

# Then, the number of b's in this range is c - a + 1

count = c - a + 1

# And the sum contributed by this k is b * count

sum += b * count

# Set a = c + 1 to move to the next range

a = c + 1

return sum

This seems efficient because the loop runs in O(sqrt(n)) time per test case, since the number of distinct values of floor(n / b) is approximately 2 * sqrt(n).

Given that t can be up to 10^4 and n up to 2*10^6, the total time should be acceptable.

Now, looking back at the given program, it seems different.

Let's look at the given program:

import math

def func():

T = int(input())

for t in range(T):

info = input().split()

(a, b) = (int(info[0]), int(info[1]))

suma = 0

for i in range(1, b + 1):

x = (a - i * (i - 1)) // (i ** 2) + 1

if (a - i * (i - 1)) // (i ** 2) + 1 > 0:

suma += x

if (a - i * (i - 1)) % (i ** 2) == 0 and i * (i - 1) % (i ** 2) == 0:

suma += 1

print(suma - 2)

This seems quite different from what I was expecting.

It iterates over i from 1 to b, and for each i, it computes x = floor((a - i*(i-1)) / (i^2)) + 1, and adds x to suma if x > 0.

Then, if (a - i*(i-1)) % (i^2) == 0 and (i*(i-1)) % (i^2) == 0, it adds 1 to suma.

Finally, it prints suma - 2.

This seems very specific and not aligned with the standard approach I was thinking about.

I need to understand what this code is doing.

First, it's iterating over i from 1 to b, which seems like it's iterating over possible values of b.

Then, for each i (which corresponds to b), it's computing floor((a - i*(i-1)) / (i^2)) + 1.

I need to see how this relates to the number of a's that satisfy the condition for a given b.

Wait, earlier I concluded that the condition simplifies to b divides a.

So, for a given b, the number of a's where b divides a is floor(n / b).

But in this code, it's computing floor((a - i*(i-1)) / (i^2)) + 1, which doesn't seem to match floor(n / b).

Wait, perhaps there's a different approach here.

Let me try to see.

Wait, in the code, (a, b) = (n, m), so a is n and b is m.

Wait, no, in the code, it's:

(a, b) = (int(info[0]), int(info[1]))

So, a is n and b is m.

Then, it's iterating over i from 1 to b, which is m.

For each i (which represents b), it's computing floor((a - i*(i-1)) / (i^2)) + 1.

I need to see how this relates to the number of a's that are multiples of i.

Wait, let's consider that for a given b = i, we need a to be a multiple of i, and 1 ≤ a ≤ n.

The number of such a's is floor(n / i).

But in the code, it's computing floor((n - i*(i-1)) / (i^2)) + 1.

This seems off.

Let me see if there's a relationship.

Wait, perhaps the author is trying to compute the number of a's such that a + b is divisible by b * gcd(a, b), which we've established is equivalent to b divides a.

But I don't see how floor((n - i*(i-1)) / (i^2)) + 1 relates to floor(n / i).

Maybe there's a mistake in the code.

Alternatively, perhaps there's a mathematical derivation that leads to this formula.

Let me try to derive it.

Suppose b divides a, so a = k * b for some integer k ≥ 1.

Then, a + b = k * b + b = (k + 1) * b.

And b * gcd(a, b) = b * b.

So, (a + b) / (b * gcd(a, b)) = (k + 1) * b / (b^2) = (k + 1) / b.

For this to be an integer, b must divide (k + 1).

But k = a / b, which is an integer.

So, b divides (k + 1), which means b divides (a / b + 1).

So, b divides (a + b) / b.

Wait, this seems circular.

Let me try to express a in terms of b and k.

Given that b divides a, a = k * b.

Then, a + b = k * b + b = (k + 1) * b.

And b * gcd(a, b) = b * b.

So, (a + b) / (b * gcd(a, b)) = (k + 1) * b / (b^2) = (k + 1) / b.

For this to be an integer, b must divide (k + 1).

So, k + 1 is a multiple of b.

Thus, k = m * b - 1 for some integer m ≥ 1.

Therefore, a = k * b = (m * b - 1) * b = m * b^2 - b.

So, a = m * b^2 - b.

Now, a must be between 1 and n.

So, 1 ≤ m * b^2 - b ≤ n.

Let's solve for m:

1 ≤ m * b^2 - b ⇒ m * b^2 ≥ b + 1 ⇒ m ≥ (b + 1)/b^2

And m * b^2 - b ≤ n ⇒ m ≤ (n + b)/b^2

Since m must be an integer, m can range from ceil((b + 1)/b^2) to floor((n + b)/b^2).

But m must be at least 1, since k = m * b - 1 ≥ 1 implies m * b ≥ 2.

Wait, this seems complicated.

Perhaps there's a better way to approach this.

Let me consider small values and see if the given code produces the correct output.

Looking at the example:

Input:

6

1 1

2 3

3 5

10 8

100 1233

1000000 1145141

Output:

1

3

4

14

153

1643498

Let me try to compute the sum for the first test case: n=1, m=1.

According to my earlier reasoning, we need to find the number of pairs (a, b) where 1 ≤ a ≤ 1 and 1 ≤ b ≤ 1, and b divides a.

So, only (1,1) satisfies this, so the answer should be 1, which matches the first output.

Second test case: n=2, m=3.

Possible pairs:

(1,1): 1 divides 1 → yes

(1,2): 2 does not divide 1 → no

(1,3): 3 does not divide 1 → no

(2,1): 1 divides 2 → yes

(2,2): 2 divides 2 → yes

(2,3): 3 does not divide 2 → no

So, valid pairs are (1,1), (2,1), (2,2) → total 3, which matches the second output.

Third test case: n=3, m=5.

Possible pairs:

(1,1): yes

(1,2): no

(1,3): no

(1,4): no

(1,5): no

(2,1): yes

(2,2): yes

(2,3): no

(2,4): no

(2,5): no

(3,1): yes

(3,2): no

(3,3): yes

(3,4): no

(3,5): no

Valid pairs: (1,1), (2,1), (2,2), (3,1), (3,3) → total 5, but the output is 4. Hmm, that doesn't match. Maybe I'm missing something.

Wait, perhaps I miscounted.

Let me list them again:

- (1,1): 1 divides 1 → yes

- (2,1): 1 divides 2 → yes

- (2,2): 2 divides 2 → yes

- (3,1): 1 divides 3 → yes

- (3,3): 3 divides 3 → yes

That's 5 pairs. But the output is 4. So, either the output is wrong or my understanding is incorrect.

Wait, maybe I need to consider the condition more carefully.

Wait, the condition is that a + b is a multiple of b * gcd(a,b).

Let me check for (3,3):

a=3, b=3

a + b = 6

b * gcd(a,b) = 3 * 3 = 9

Is 6 a multiple of 9? 6 is not a multiple of 9. So, (3,3) does not satisfy the condition.

So, only (1,1), (2,1), (2,2), (3,1) are valid → total 4, which matches the output.

Okay, so my earlier assumption that b divides a is equivalent to the condition was incorrect.

Wait, but according to my earlier derivation, it should be equivalent.

Let me re-examine that.

Given that a + b is divisible by b * gcd(a,b).

Let d = gcd(a,b).

Then, a = d * a', b = d * b', with gcd(a', b') = 1.

Then, a + b = d(a' + b')

b * d = d * b' * d = d^2 * b'

So, d^2 * b' divides d(a' + b'), which simplifies to d * b' divides a' + b'.

Since gcd(a', b') = 1, and b' divides a' + b', then b' divides a'.

But gcd(a', b') = 1 implies b' = 1.

Therefore, b' = 1, so b = d.

Thus, b = d = gcd(a,b), which means b divides a.

But for (3,3), b=3 divides a=3, but a + b = 6 is not divisible by b * gcd(a,b) = 9.

So, there's a contradiction here.

Wait, perhaps my earlier assumption is incorrect.

Let me recast the condition.

We have a + b is divisible by b * gcd(a,b).

Given that b divides a, a = k * b.

Then, a + b = k * b + b = (k + 1) * b.

And b * gcd(a,b) = b * b.

So, (k + 1) * b is divisible by b * b, which implies that (k + 1) is divisible by b.

So, b divides (k + 1).

But k = a / b, which is an integer since b divides a.

So, k + 1 is an integer, and b divides k + 1.

Therefore, k + 1 = m * b for some integer m.

Thus, k = m * b - 1.

Therefore, a = k * b = (m * b - 1) * b = m * b^2 - b.

So, a = m * b^2 - b.

Now, a must be between 1 and n.

So, 1 ≤ m * b^2 - b ≤ n.

Solving for m:

1 ≤ m * b^2 - b ⇒ m * b^2 ≥ b + 1 ⇒ m ≥ (b + 1)/b^2

And m * b^2 - b ≤ n ⇒ m ≤ (n + b)/b^2

Since m must be an integer, m starts from ceil((b + 1)/b^2) up to floor((n + b)/b^2).

But (b + 1)/b^2 = (1/b) + (1/b^2), which is less than or equal to 1 for b ≥ 1.

So, m starts from 1.

Thus, for each b, the number of a's is the number of integer m's such that a = m * b^2 - b is within 1 to n.

So, for each b, the number of a's is floor((n + b)/b^2) - ceil((b + 1)/b^2) + 1.

But ceil((b + 1)/b^2) is ceil(1/b + 1/b^2), which for b ≥ 1 is 1.

Because 1/b + 1/b^2 ≤ 1 + 1 = 2 for b=1, and decreases as b increases.

So, ceil((b + 1)/b^2) = 1 for b ≥ 1.

And floor((n + b)/b^2) is floor((n + b)/b^2).

Therefore, the number of a's for each b is floor((n + b)/b^2) - 1 + 1 = floor((n + b)/b^2).

Wait, but actually, floor((n + b)/b^2) - ceil((b + 1)/b^2) + 1.

Since ceil((b + 1)/b^2) = 1, then floor((n + b)/b^2) - 1 + 1 = floor((n + b)/b^2).

So, the number of a's for each b is floor((n + b)/b^2).

Therefore, the total number of pairs is sum over b from 1 to m of floor((n + b)/b^2).

Now, looking back at the given code:

suma = 0

for i in range(1, b + 1):

x = (a - i * (i - 1)) // (i ** 2) + 1

if x > 0:

suma += x

if (a - i * (i - 1)) % (i ** 2) == 0 and i * (i - 1) % (i ** 2) == 0:

suma += 1

print(suma - 2)

Wait, (a - i*(i-1)) // (i**2) + 1 = floor((a - i*(i-1)) / i^2) + 1

But according to my derivation, it should be floor((n + b)/b^2).

So, is floor((n + b)/b^2) equal to floor((a - i*(i-1)) / i^2) + 1?

Wait, perhaps there's a mistake in my derivation.

Let me double-check.

I had a = m * b^2 - b.

Then, m = (a + b)/b^2.

So, floor(m) = floor((a + b)/b^2).

Yes, that matches my earlier conclusion.

But in the code, it's computing floor((a - i*(i-1))/i^2) + 1.

This doesn't seem to match floor((a + i)/i^2).

Wait, perhaps there's a different way to express it.

Alternatively, perhaps the author made a mistake in the formula.

Alternatively, maybe there's a different approach.

Let me consider that for each b, a = m * b^2 - b, and 1 ≤ a ≤ n.

So, m = ceil((b + 1)/b^2) to floor((n + b)/b^2).

But ceil((b + 1)/b^2) = 1, as we saw earlier.

So, m ranges from 1 to floor((n + b)/b^2).

Therefore, for each b, the number of a's is floor((n + b)/b^2).

So, the total sum is sum over b from 1 to m of floor((n + b)/b^2).

Now, looking back at the code, it's computing something different.

It's computing sum over i from 1 to b of floor((a - i*(i-1))/i^2) + 1, with some additional conditions.

This seems inconsistent with my derivation.

Perhaps there's a different way to express floor((n + b)/b^2).

Let me see:

floor((n + b)/b^2) = floor(n/b^2 + 1/b)

Since 1/b is less than 1, floor(n/b^2 + 1/b) = floor(n/b^2) + 0 or 1 depending on whether n/b^2 + 1/b >= floor(n/b^2) + 1.

But this seems messy.

Alternatively, perhaps the author is using a different formula.

Let me consider that floor((n + b)/b^2) = floor(n/b^2 + 1/b) = floor(n/b^2) if n/b^2 + 1/b < floor(n/b^2) + 1, otherwise floor(n/b^2) + 1.

But this seems too convoluted.

Looking back at the code, perhaps the author is trying to compute floor((n + b)/b^2) in a different way.

Let me compute floor((n + b)/b^2) directly and see if it matches the code's approach.

For example, in the first test case: n=1, m=1.

floor((1 + 1)/1^2) = floor(2/1) = 2.

But according to the earlier, there should be only 1 valid pair, but this gives 2.

Hmm, that doesn't match.

Wait, perhaps there's an adjustment needed.

In the code, it's suma - 2 at the end.

So, for n=1, m=1, suma would be 2, and suma - 2 = 0, but the correct answer is 1.

Wait, that doesn't make sense.

Maybe the code is incorrect.

Alternatively, perhaps the author is considering some inclusive/exclusive boundaries incorrectly.

Let me try to compute the sum for n=3, m=5.

According to my calculation, sum over b=1 to 5 of floor((3 + b)/b^2).

For b=1: floor((3+1)/1) = floor(4/1) = 4

b=2: floor((3+2)/4) = floor(5/4) = 1

b=3: floor((3+3)/9) = floor(6/9) = 0

b=4: floor((3+4)/16) = floor(7/16) = 0

b=5: floor((3+5)/25) = floor(8/25) = 0

Total sum = 4 + 1 + 0 + 0 + 0 = 5

But earlier we saw that there should be only 4 valid pairs, so this doesn't match.

Wait, perhaps there's an off-by-one error.

Alternatively, perhaps the formula is not correct.

Wait, perhaps the number of a's for each b is floor((n + b - 1)/b^2).

Let's try that for n=3, m=5.

b=1: floor((3 + 1 - 1)/1) = floor(3/1) = 3

b=2: floor((3 + 2 -1)/4) = floor(4/4) = 1

b=3: floor((3 + 3 -1)/9) = floor(5/9) = 0

b=4: floor((3 + 4 -1)/16) = floor(6/16) = 0

b=5: floor((3 + 5 -1)/25) = floor(7/25) = 0

Total sum = 3 + 1 + 0 + 0 + 0 = 4, which matches the expected output of 4.

Similarly, for n=1, m=1:

b=1: floor((1 + 1 -1)/1) = floor(1/1) = 1

Total sum = 1, which matches the first output.

For n=2, m=3:

b=1: floor((2 +1 -1)/1) = 2

b=2: floor((2 +2 -1)/4) = floor(3/4) = 0

b=3: floor((2 +3 -1)/9) = floor(4/9) = 0

Sum = 2 + 0 + 0 = 2, but earlier we saw there should be 3 pairs.

Wait, that doesn't match.

So, perhaps this formula is still incorrect.

Wait, perhaps it's floor((n + b -1)/b^2) + something.

This is getting too confusing.

Alternatively, perhaps the correct formula is sum over b=1 to m of floor((n + b -1)/b^2), but as shown above, it doesn't consistently match the expected outputs.

Given this discrepancy, I suspect that the given program is incorrect because it doesn't align with the standard approach or with the correct counts in the example.

Therefore, the answer is Correctness: **False**