Alright, I have this problem to solve. Let's see what it's asking for. Bob has a bakery, and on the opening day, he baked n buns that he wants to sell. The usual price for each bun is a coins. But to attract customers, he's running a promotion where he can choose some integer k (between 0 and the minimum of n and b) and sell the first k buns at a modified price. The price for the i-th bun (where i ranges from 1 to k) is (b - i + 1) coins. The remaining (n - k) buns are sold at the usual price a coins each.

My task is to help Bob determine the maximum profit he can obtain by selling all n buns.

First, I need to understand the promotion clearly. So, if Bob chooses k = 0, he sells all n buns at price a coins each. If he chooses k = 1, he sells the first bun at price b coins and the remaining (n - 1) buns at price a coins each. If he chooses k = 2, he sells the first bun at price b coins, the second bun at (b - 1) coins, and the remaining (n - 2) buns at price a coins each. This pattern continues up to k = min(n, b), where he sells k buns with decreasing prices starting from b down to (b - k + 1), and the remaining (n - k) buns at price a coins each.

My goal is to maximize the total profit, which is the sum of the prices of all buns sold.

Let me think about different scenarios to understand better.

**Scenario 1:** b <= a

In this case, the modified prices for k buns would be less than or equal to the usual price a. So, selling any bun at the modified price would result in equal or less revenue compared to selling it at price a. Therefore, the maximum profit would be achieved by setting k = 0 and selling all n buns at price a coins each. Total profit would be n * a.

**Scenario 2:** b > a

Here, the first bun in the modified pricing is b coins, which is greater than a. So, selling some buns at the modified price might increase the total profit.

But I need to find the optimal k that maximizes the profit.

Let's consider that Bob chooses to sell k buns at the modified prices. The total price for these k buns would be the sum of an arithmetic series starting from b down to (b - k + 1).

The sum of this series is:

sum = (k/2) * (first term + last term) = (k/2) * (b + (b - k + 1)) = (k/2) * (2b - k + 1)

The remaining (n - k) buns are sold at price a each, so their total price is a * (n - k).

Therefore, the total profit P for a given k is:

P = (k/2) * (2b - k + 1) + a * (n - k)

I need to maximize P with respect to k.

Constraints are:

- k is an integer between 0 and min(n, b)

- n, a, b can be up to 10^9, so I need an efficient way to compute this.

Let me think about how P changes with k.

Let's look at the expression for P:

P(k) = (k/2)*(2b - k + 1) + a*(n - k)

Simplify it:

P(k) = (k*(2b - k + 1))/2 + a*(n - k)

= (2bk - k^2 + k)/2 + a*n - a*k

= (2bk)/2 - (k^2)/2 + k/2 + a*n - a*k

= bk - (k^2)/2 + k/2 + a*n - a*k

= a*n + bk - a*k - (k^2)/2 + k/2

This seems a bit messy. Maybe there's a better way to approach this.

Alternatively, since k can be up to 10^9, I need a way to find the optimal k without iterating through all possible k values.

Let me consider the difference in profit when increasing k by 1.

Let's compute P(k+1) - P(k):

P(k+1) = ( (k+1)/2 ) * (2b - (k+1) + 1) + a*(n - (k+1))

= ( (k+1)/2 ) * (2b - k) + a*(n - k - 1)

Now, P(k+1) - P(k) = [ ( (k+1)/2 ) * (2b - k) + a*(n - k - 1) ] - [ (k/2) * (2b - k + 1) + a*(n - k) ]

Let's compute this step by step.

First, expand ( (k+1)/2 ) * (2b - k):

= (k+1)(2b - k)/2

= (2b(k+1) - k(k+1))/2

= (2bk + 2b - k^2 - k)/2

= bk + b - (k^2)/2 - k/2

Now, a*(n - k - 1) = a*n - a*k - a

So, P(k+1) = bk + b - (k^2)/2 - k/2 + a*n - a*k - a

Similarly, P(k) = (k/2)*(2b - k + 1) + a*(n - k)

= (k/2)*(2b - k + 1) + a*n - a*k

= (k*(2b - k + 1))/2 + a*n - a*k

= (2bk - k^2 + k)/2 + a*n - a*k

= bk - (k^2)/2 + k/2 + a*n - a*k

Now, P(k+1) - P(k) = [bk + b - (k^2)/2 - k/2 + a*n - a*k - a] - [bk - (k^2)/2 + k/2 + a*n - a*k]

Simplify:

= bk + b - (k^2)/2 - k/2 + a*n - a*k - a - bk + (k^2)/2 - k/2 - a*n + a*k

= b - a - k - k

= b - a - 2k

So, P(k+1) - P(k) = b - a - 2k

This is useful. This tells me how the profit changes when I increase k by 1.

To maximize P(k), I need to find the k where P(k+1) - P(k) <= 0.

So, set P(k+1) - P(k) <= 0:

b - a - 2k <= 0

=> 2k >= b - a

=> k >= ceil((b - a)/2)

But I need to be careful here because k has to be an integer between 0 and min(n, b).

Wait, actually, to maximize P(k), I should find the point where P(k+1) - P(k) changes from positive to negative.

In other words, find the k where P(k+1) - P(k) <= 0, and P(k) - P(k-1) >= 0.

From P(k+1) - P(k) = b - a - 2k

Set b - a - 2k <= 0

=> k >= ceil((b - a)/2)

And P(k) - P(k-1) = b - a - 2(k-1) = b - a - 2k + 2 >= 0

=> k <= floor((b - a + 1)/2)

So, the optimal k is between ceil((b - a)/2) and floor((b - a + 1)/2)

Wait, but this seems a bit messy. Maybe there's a better way.

Alternatively, since P(k+1) - P(k) = b - a - 2k, this is a decreasing function in k.

So, P(k+1) - P(k) starts at b - a when k=0, and decreases by 2 for each increment in k.

Therefore, as long as b - a - 2k > 0, P(k+1) > P(k), and once b - a - 2k <= 0, P(k+1) <= P(k).

So, the maximum P(k) occurs at the largest k where b - a - 2k > 0, which is k < floor((b - a)/2).

But since k must be an integer, the optimal k is floor((b - a - 1)/2) or floor((b - a)/2).

Wait, let's double-check this.

Set b - a - 2k > 0

=> k < (b - a)/2

So, the last k where P(k+1) > P(k) is k = floor((b - a - 1)/2)

Therefore, the optimal k is k = floor((b - a - 1)/2) + 1 = floor((b - a)/2)

Wait, this is getting confusing. Maybe I should consider the derivative.

But since k is integer, maybe considering it as a continuous variable and taking derivative is not directly applicable.

Alternatively, maybe I can find the value of k that maximizes P(k) by finding where the difference changes sign.

Given that P(k+1) - P(k) = b - a - 2k

So, as k increases, P(k+1) - P(k) decreases by 2 each time.

Start with k=0: P(1) - P(0) = b - a

k=1: P(2) - P(1) = b - a - 2

k=2: P(3) - P(2) = b - a - 4

...

So, as long as b - a - 2k > 0, P(k+1) > P(k), meaning P increases.

When b - a - 2k = 0 or negative, P(k+1) <= P(k), meaning P starts decreasing.

Therefore, the maximum P(k) occurs at the largest k where b - a - 2k > 0, i.e., k < floor((b - a)/2)

Wait, let's solve b - a - 2k > 0 for k:

k < (b - a)/2

Since k must be integer, k <= floor((b - a - 1)/2)

But I need to make sure that k does not exceed min(n, b).

So, the optimal k is the minimum of floor((b - a - 1)/2) and min(n, b).

Wait, but in the problem, k can be up to min(n, b), but according to this, the profit increases as long as k < floor((b - a)/2), but we need to ensure that k does not exceed min(n, b).

Wait, perhaps I need to consider the following:

- If floor((b - a)/2) < min(n, b), then set k = floor((b - a)/2)

- Else, set k = min(n, b)

But I need to verify this with some examples.

Let me consider an example.

Take the first test case:

n = 4, a = 4, b = 5

So, b - a = 1

floor((b - a)/2) = floor(1/2) = 0

So, according to this, k = 0

But in the explanation, it says that k = 1 gives 17, which is higher than k = 0 giving 16.

Wait, that doesn't match.

Wait, in the first test case, n=4, a=4, b=5

If k=0, profit = 4*4 = 16

If k=1, profit = 5 + 4*3 = 5 + 12 = 17

If k=2, profit = 5 + 4 + 4*2 = 9 + 8 = 17

If k=3, profit = 5 + 4 + 3 + 4*1 = 12 + 4 = 16

If k=4, profit = 5 + 4 + 3 + 2 = 14

So, maximum is k=1 or k=2, both giving 17.

But according to my earlier formula, floor((b - a)/2) = floor(1/2) = 0, which suggests k=0, but that's not the case.

Hmm, perhaps I made a mistake.

Let me recast the problem.

Let me consider P(k) = sum of first k terms: b, b-1, ..., b - k + 1 and (n - k) terms of a.

So, P(k) = k*(2b - k + 1)/2 + a*(n - k)

I need to maximize P(k) over k from 0 to min(n, b)

Let me treat P(k) as a quadratic in terms of k:

P(k) = (-1/2)k^2 + (2b + 1)/2 k + a*(n - k)

= (-1/2)k^2 + (2b + 1 - 2a)/2 k + a*n

= (-1/2)k^2 + (b - a + 0.5)k + a*n

This is a downward-opening parabola, so the maximum occurs at the vertex.

The vertex is at k = -(b - a + 0.5)/(2*(-1/2)) = (b - a + 0.5)/1 = b - a + 0.5

So, the optimal k is floor(b - a + 0.5) = floor(b - a) + floor(0.5) = (b - a) + 0 = b - a

But in the first example, b - a = 1, so k = 1, which matches one of the optimal k values.

In the third example:

n=10, a=10, b=5

b - a = -5, so k = 0, which matches the third test case.

In the second example:

n=5, a=5, b=9

b - a = 4, so k = 4

But in the explanation, k=5 gives 35, which is higher than k=4 giving 9 + 8 + 7 + 6 + 5 = 35, wait, k=5 gives 9 + 8 + 7 + 6 + 5 = 35, which is the same as k=4 giving 9 + 8 + 7 + 6 + 5 = 35? Wait, no, k=4 would be 9 + 8 + 7 + 6 + 5 for k=5.

Wait, perhaps I miscalculated.

Wait, for k=4: 9 + 8 + 7 + 6 + 5 for k=5.

Wait, perhaps I need to double-check.

Wait, the first k buns are sold at prices b, b-1, ..., b - k + 1.

So, for k=5: 9 + 8 + 7 + 6 + 5 = 35

For k=4: 9 + 8 + 7 + 6 = 30, and (5 - 4)=1 bun sold at a=5: 30 + 5 = 35

So, same profit.

But according to the formula, k = b - a = 9 - 5 = 4, which seems consistent.

Wait, but in the first example, k = b - a = 5 - 4 = 1, which is optimal.

In the second example, k = 9 - 5 = 4, and k=5 also gives the same profit.

So, perhaps the optimal k is min(b - a, min(n, b))

Wait, but in the first example, b - a = 1, and min(n, b) = min(4,5)=4, so k=1

In the second example, b - a = 4, and min(n, b)=5, so k=4

But choosing k=5 also gives the same profit.

Wait, in the second example, k=4 gives 9 + 8 + 7 + 6 + 5 = 35, and k=5 also gives 9 + 8 + 7 + 6 + 5 = 35

Wait, no, k=5 would be 9 + 8 + 7 + 6 + 5 = 35, same as k=4.

Wait, no, for k=4: 9 + 8 + 7 + 6 + 5 for k=5.

Wait, perhaps I'm getting confused.

Wait, for k=4: first 4 buns at 9,8,7,6 and remaining n - k =1 bun at a=5: total 9+8+7+6 +5=35

For k=5: first 5 buns at 9,8,7,6,5: total 9+8+7+6+5=35

So, both k=4 and k=5 give the same profit.

So, in this case, k = b - a =4 is optimal, but k=5 is also equally good.

So, perhaps the optimal k is min(b - a, min(n, b))

But in the first example, k = b - a =1, which is less than min(n,b)=4, so k=1 is optimal.

In the second example, k = b - a =4, and min(n,b)=5, so k=4 is optimal, but k=5 is also equally good.

So, perhaps choosing k = min(b - a, min(n, b)) would be optimal.

But in the third example:

n=10, a=10, b=5

b - a = -5, so k=0 is optimal, which matches.

Another example:

n=5, a=5, b=11

b - a =6, min(n,b)=5, so k=5

Indeed, in the fourth test case:

n=5, a=5, b=11

k=5: 11 +10 +9 +8 +7 = 45

k=4: 11 +10 +9 +8 +5=43

k=3:11+10+9 +5+5=40

So, k=5 is optimal.

So, in general, k = min(b - a, min(n, b))

Wait, but in the second example, b - a=4, min(n,b)=5, so k=4 is optimal, but k=5 is also equally good.

Wait, why is that?

Wait, in the second example, n=5, a=5, b=9

k=4: first 4 buns at 9,8,7,6 and one bun at a=5: total 9+8+7+6+5=35

k=5: first 5 buns at 9,8,7,6,5: total 9+8+7+6+5=35

So, both give the same profit.

But according to the formula k = min(b - a, min(n, b)) = min(4,5)=4

But choosing k=5 is also equally good.

So, perhaps choosing k = min(b - a, min(n, b)) or k = min(n, b), both give the same profit.

So, perhaps the maximum profit is max(P(min(b - a, min(n, b))), P(min(n, b)))

But in the second example, P(4)=35 and P(5)=35

In the fourth example, P(5)=45 and P(6)=11+10+9+8+7 +5=45 (if n=6), but n=5, so P(5)=45

Wait, but in the fourth example, n=5, a=5, b=11

k=5: 11+10+9+8+7=45

k=4:11+10+9+8 +5=43

k=3:11+10+9 +5+5=40

So, k=5 is better than k=4 in this case.

Wait, but according to the formula k = min(b - a, min(n, b)) = min(6,5)=5

So, k=5 is optimal.

Wait, but in the second example, b - a=4, min(n,b)=5, so k=4 is optimal, but k=5 gives the same profit.

Wait, perhaps I need to consider that when b - a >= n, then k = n is optimal.

Wait, in the second example, b - a=4, which is less than n=5, so k=4 is optimal.

But in the fourth example, b - a=6, which is greater than n=5, but k=5 is optimal.

Wait, perhaps when b - a >= n, then k = n is optimal.

Wait, in the third example, b - a=-5 <0, so k=0 is optimal.

In the second example, b - a=4 < n=5, so k=4 is optimal.

In the fourth example, b - a=6 > n=5, so k=5 is optimal.

So, perhaps:

If b - a >= n, then k = n is optimal.

Else, k = b - a is optimal.

Let me check this.

First example: b - a=1 < n=4, so k=1 is optimal.

Second example: b - a=4 < n=5, so k=4 is optimal.

Third example: b - a=-5 <0, so k=0 is optimal.

Fourth example: b - a=6 > n=5, so k=5 is optimal.

Seems consistent.

So, the optimal k is:

if b - a >= n:

k = n

else:

k = b - a

But in the second example, k=4 and k=5 both give the same profit.

So, in cases where b - a >= n, choosing k = n is also optimal.

So, to maximize profit, choose k = min(b - a, n)

But in the second example, b - a=4, n=5, so k=4 is optimal, but k=5 is also equally good.

Wait, why is that?

Wait, perhaps because when b - a >= k, choosing k up to n is beneficial.

Wait, perhaps I need to consider that the modified prices are higher than a up to k where b - k +1 >= a

So, the point where the modified price drops below a, it's not beneficial to choose higher k.

So, the maximum k where b - k +1 >= a is k <= b - a +1

So, the maximum k where modified prices are greater than or equal to a is k <= b - a +1

But k also cannot exceed n or b.

So, the optimal k is min(n, b, b - a +1)

In the first example, b - a +1 =2, min(n=4, b=5, 2)=2

So, k=2 gives 5+4+4+4=17, which matches the optimal.

In the second example, b - a +1=5, min(n=5, b=9,5)=5, so k=5 gives 35, which is optimal.

In the third example, b - a +1=6, min(n=10, b=5,6)=5, but in this case, modified prices are 5,4,3,2,1, which are less than a=10, so k=0 is better.

Wait, but b - a +1=6, but b=5, so min(n=10, b=5,6)=5

But in this case, choosing k=5 gives 5+4+3+2+1=15, which is less than k=0 giving 10*10=100

So, in this case, choosing k=0 is better.

Wait, so my previous assumption is incorrect.

So, perhaps the optimal k is min(n, b - a +1, b)

Wait, but in the third example, b - a +1=6, b=5, so min(n=10,5,6)=5

But choosing k=5 is suboptimal.

So, perhaps the condition is k <= b - a

Wait, in the third example, b - a=-5, so k=0 is optimal.

In the first example, b - a=1, so k=1 is optimal.

In the second example, b - a=4, so k=4 is optimal, but k=5 also gives the same profit.

In the fourth example, b - a=6, so k=5 is optimal.

Wait, perhaps the optimal k is min(n, b, b - a +1)

In the first example, min(4,5,2)=2, which matches k=1 and k=2 both giving 17.

In the second example, min(5,9,5)=5, which gives 35.

In the third example, min(10,5,6)=5, but choosing k=0 is better.

Wait, but in the third example, b - a +1=6, but b=5, so min(n=10, b=5,6)=5

But choosing k=5 gives less profit than k=0.

So, perhaps the condition is k <= b - a

In the third example, b - a=-5, so k=0 is optimal.

In the first example, b - a=1, so k=1 is optimal.

In the second example, b - a=4, so k=4 is optimal.

In the fourth example, b - a=6, so k=5 (since min(n,b)=5) is optimal.

So, perhaps the optimal k is min(n, b, b - a)

In the third example, min(10,5, -5)= -5, but k cannot be negative, so k=0.

Wait, but min with a negative number doesn't make sense, so k=0.

So, perhaps k = min(n, b, b - a, 0)

But k can be 0.

Wait, perhaps k = min(n, b, b - a)

Then, in the third example, min(10,5, -5) = -5, but k cannot be negative, so k=0.

In the first example, min(4,5,1)=1

In the second example, min(5,9,4)=4

In the fourth example, min(5,11,6)=5

Which matches the optimal k.

So, in general, k = max(0, min(n, b, b - a))

This way, k cannot be negative.

So, this seems to be the way to choose the optimal k.

Now, let's confirm this with the examples.

First test case:

n=4, a=4, b=5

k = min(4,5,1)=1

Profit = 5 + 4*3 = 5 + 12 = 17

Second test case:

n=5, a=5, b=9

k = min(5,9,4)=4

Profit = 9 +8 +7 +6 +5 = 35

Third test case:

n=10, a=10, b=5

k = min(10,5,-5)= -5 -> k=0

Profit = 10*10=100

Fourth test case:

n=5, a=5, b=11

k = min(5,11,6)=5

Profit =11 +10 +9 +8 +7=45

Seems correct.

Now, let's look at the provided program and see if it implements this logic correctly.

The program is:

def func():

t = int(input())

for _ in range(t):

(n, a, b) = map(int, input().split())

if b <= a:

print(n * a)

elif b - a >= n:

print(int((2 * b - n + 1) * n // 2))

else:

print(int((b - a) * (b - a + 1) // 2 + a * n))

So, it has two main cases:

1. if b <= a:

print(n * a)

This matches our first scenario where choosing k=0 is optimal.

2. elif b - a >= n:

print(int((2 * b - n + 1) * n // 2))

This seems to be calculating the sum of the first n modified prices when b - a >= n.

Let's see what this expression is.

(2 * b - n + 1) * n // 2

This looks like the sum of an arithmetic series where the first term is b, and the last term is b - n +1.

Sum = (first + last) * number_of_terms / 2 = (b + (b - n +1)) * n / 2 = (2b - n +1) * n / 2

Which matches the expression in the code.

So, when b - a >= n, it chooses k = n, and sells the first n buns at modified prices.

This seems correct, as in the fourth example.

3. else:

print(int((b - a) * (b - a + 1) // 2 + a * n))

This seems to be calculating the sum of the first (b - a) modified prices and selling the remaining buns at price a.

Wait, but according to our earlier analysis, the optimal k is min(n, b, b - a), which is b - a when b - a <= min(n, b)

So, in this case, k = b - a

Then, the sum of the first k modified prices is sum from i=0 to k-1 of (b - i)

Which is k*(2b - k +1)/2

And the remaining (n - k)*a

So, total profit is k*(2b - k +1)/2 + a*(n - k)

In the code, it's calculating (b - a)*(b - a +1)/2 + a*n

Wait, is this equivalent?

Wait, (b - a)*(b - a +1)/2 is the sum of the first (b - a) integers starting from 1 up to (b - a).

But in our earlier analysis, the sum of the first k modified prices is sum from i=1 to k of (b - i +1)

Which is k*(2b - k +1)/2

So, in the code, it's using (b - a)*(b - a +1)/2, which is the sum of the first (b - a) integers, not the sum of the modified prices.

Wait, this seems incorrect.

Wait, no, let's see.

The sum of the first k modified prices is sum from i=1 to k of (b - i +1) = sum from i=1 to k of (b +1 - i) = k*(b +1) - sum from i=1 to k of i = k*(b +1) - k*(k +1)/2 = k*(b +1 - (k +1)/2) = k*(2b +2 - k -1)/2 = k*(2b - k +1)/2

But in the code, it's using (b - a)*(b - a +1)/2 + a*n

Wait, but according to our earlier analysis, the optimal k is min(n, b, b - a)

Which in this else block, b - a < n (since the condition is b - a >= n is false)

So, k = min(n, b, b - a)

But since b - a < n, and b - a <= b (since b - a >=0, because else clause is executed only if b > a), so k = b - a

Therefore, sum of first k modified prices is k*(2b - k +1)/2

And remaining (n - k)*a

So, total profit is k*(2b - k +1)/2 + a*(n - k)

But in the code, it's calculating (b - a)*(b - a +1)/2 + a*n

Wait, but (b - a)*(b - a +1)/2 is equal to k*(2b - k +1)/2 when k = b - a?

Wait, let's see:

k = b - a

Then, k*(2b - k +1)/2 = (b - a)*(2b - (b - a) +1)/2 = (b - a)*(2b - b + a +1)/2 = (b - a)*(b + a +1)/2

Which is not equal to (b - a)*(b - a +1)/2

So, the code seems to be incorrect in this else block.

It should be calculating k*(2b - k +1)/2 + a*(n - k), where k = b - a

But instead, it's calculating (b - a)*(b - a +1)/2 + a*n

Which is different from the correct sum.

Wait, perhaps it's a mistake.

Let me check with the first test case.

First test case:

n=4, a=4, b=5

k = b - a =1

Correct sum: 1*(2*5 -1 +1)/2 + 4*(4 -1) = 1*10/2 + 4*3 = 5 + 12 =17

But according to the code: (5 -4)*(5 -4 +1)/2 + 4*4 =1*2/2 +16=1 +16=17

So, in this case, it gives the correct answer.

Wait, but according to my earlier calculation, k*(2b - k +1)/2 + a*(n - k) =1*(10)/2 +4*3=5+12=17

And the code calculates (b - a)*(b - a +1)/2 + a*n =1*2/2 +16=1+16=17

Which matches.

But is this always true?

Wait, in the first test case, it works, but is it general?

Let me check the second test case.

n=5, a=5, b=9

k = b - a =4

Correct sum:4*(2*9 -4 +1)/2 +5*(5 -4)=4*15/2 +5*1=30 +5=35

According to the code:(9 -5)*(9 -5 +1)/2 +5*5=4*5/2 +25=10 +25=35

Again, matches.

Another test case:

n=5, a=5, b=11

k = b - a =6

But min(n, b, b - a)= min(5,11,6)=5

So, k=5

Correct sum:5*(2*11 -5 +1)/2 +5*(5 -5)=5*17/2 +0=42.5, but since we're dealing with integers, 5*17//2=42 +0=42

But in reality, sum is 11+10+9+8+7=45, which is higher than 42.

Wait, there's a discrepancy here.

Wait, perhaps I'm miscalculating.

Wait, 2b - k +1 =2*11 -5 +1=22 -5 +1=18

sum =5*18//2=45, which matches the correct sum.

But according to the code:

(b - a)*(b - a +1)/2 + a*n =6*7/2 +5*5=21 +25=46

Which is higher than the actual sum of 45.

But in reality, choosing k=5 gives sum=45, which is higher than k=4, etc.

So, the code is giving 46, which is incorrect.

Wait, perhaps I need to see what's wrong.

Wait, in this case, b - a=6, n=5

So, k = min(n, b, b - a)= min(5,11,6)=5

So, sum should be 5*(2*11 -5 +1)/2 +5*(5 -5)=5*17/2=42.5, but integer division gives 42 +0=42

But actual sum is 11+10+9+8+7=45

So, there's a discrepancy.

Wait, perhaps I'm miscalculating the sum.

Wait, 2b - k +1=22 -5 +1=18

sum=k*18//2=5*18//2=90//2=45, which matches.

But according to the code, it's calculating (b - a)*(b - a +1)/2 + a*n =6*7/2 +25=21 +25=46

Which is higher than the actual sum of 45.

So, in this case, the code is giving an incorrect sum.

Therefore, the code is incorrect in the else block.

It should be calculating k*(2b - k +1)/2 + a*(n - k), where k = min(n, b, b - a)

But instead, it's calculating (b - a)*(b - a +1)/2 + a*n, which is incorrect.

So, the correct implementation should be:

if b <= a:

print(n * a)

elif b - a >= n:

print((2 * b - n + 1) * n // 2)

else:

k = b - a

sum_modified = k * (2 * b - k + 1) // 2

sum_remaining = a * (n - k)

print(sum_modified + sum_remaining)

But in the provided code, in the else block, it's using (b - a)*(b - a +1)/2 + a*n, which is incorrect.

Hence, the program is incorrect.

Wait, but in the first and second test cases, it gave the correct answer, but in the fourth test case, it gives 46 instead of 45.

So, it's incorrect.

Therefore, Correctness: False

**Final Answer**

\[ \boxed{\text{False}} \]