### Reasoning:

Let's carefully analyze the given program and the problem requirements.

#### Problem Requirements:
- For each test case \(x\), find an integer \(y\) such that \(1 \le y < x\) and \(\gcd(x, y) + y\) is maximized.

#### Given Program:
```python
def func():
    for i in range(int(input())):
        x = int(input())
        y = x - 1
        print(y)
```

#### Annotated Code:
- The program reads the number of test cases \(t\).
- For each test case, it reads an integer \(x\).
- It sets \(y\) to \(x - 1\).
- It prints \(y\).

#### Analysis:
- The program always chooses \(y = x - 1\).
- We need to check if this choice always maximizes \(\gcd(x, y) + y\).

Consider the expression \(\gcd(x, y) + y\):
- If \(y = x - 1\), then \(\gcd(x, x-1) = 1\) because \(x\) and \(x-1\) are consecutive integers and thus coprime.
- Therefore, \(\gcd(x, x-1) + (x-1) = 1 + (x-1) = x\).

Now, let's consider other possible values of \(y\):
- If \(y = x - 2\), then \(\gcd(x, x-2)\) could be greater than 1 if \(x\) and \(x-2\) share a common factor. However, even in the best case, \(\gcd(x, x-2) \leq 2\), so \(\gcd(x, x-2) + (x-2) \leq 2 + (x-2) = x\).
- For any \(y < x - 2\), \(\gcd(x, y)\) will generally be smaller, leading to a smaller value of \(\gcd(x, y) + y\).

Given these observations, the choice \(y = x - 1\) indeed maximizes \(\gcd(x, y) + y\) because:
- \(\gcd(x, x-1) = 1\) and \(1 + (x-1) = x\).
- Any other \(y < x - 1\) will result in a smaller value for \(\gcd(x, y) + y\).

Therefore, the program correctly implements the logic to maximize \(\gcd(x, y) + y\) by choosing \(y = x - 1\).

### Final Evaluation:
Final: **True**

The program is correct as it always finds the optimal \(y\) that maximizes \(\gcd(x, y) + y\).