Output State: `i` is 6, `n` must be at least 6, and `sum` is 210.

To understand this, let's break down the loop and its behavior:

1. The loop starts with `i` as 2 and increments `i` by 1 on each iteration.
2. The expression inside the loop is `(i * i - (i - 1) * (i - 1)) * i`, which simplifies to `2 * i * i - 2 * i + 1`.
3. This can be further simplified to `2 * i^2 - 2 * i + 1`.

Given the output states after the first 3 iterations:
- After 1st iteration (`i = 3`), `sum = 8`
- After 2nd iteration (`i = 4`), `sum = 20`
- After 3rd iteration (`i = 5`), `sum = 60`

We can observe the pattern in `sum`:
- After 1st iteration: `sum = 8` (which is `2 * 3^2 - 2 * 3 + 1`)
- After 2nd iteration: `sum = 20` (which is `8 + 2 * 4^2 - 2 * 4 + 1`)
- After 3rd iteration: `sum = 60` (which is `20 + 2 * 5^2 - 2 * 5 + 1`)

Following this pattern, the next value of `i` would be 6, and the `sum` would be calculated as:
- `sum = 60 + 2 * 6^2 - 2 * 6 + 1 = 60 + 72 - 12 + 1 = 121 + 1 = 210`.

Thus, after all iterations, `i` will be 6, `n` must be at least 6, and `sum` will be 210.