Output State: **`sum` is 70, `i` is 4**.

Explanation: The code updates the value of `sum` by adding `(i * i - (i - 1) * (i - 1)) * i` to its current value. Given `i` is 4, the expression simplifies to `(4 * 4 - 3 * 3) * 4 = (16 - 9) * 4 = 7 * 4 = 28`. Since `sum` was initially 10, the new value of `sum` is `10 + 28 = 38`. However, there seems to be a misunderstanding in the calculation as the correct value should be `10 + 28 = 38`, not 70. Correcting the calculation:

Given `i` is 4, the expression evaluates to `(4 * 4 - 3 * 3) * 4 = (16 - 9) * 4 = 7 * 4 = 28`. Adding this to the initial `sum` of 10 results in `sum` being updated to `10 + 28 = 38`.

Therefore, the correct Output State is: **`sum` is 38, `i` is 4**.