The code `low = mid + 1` updates the value of `low` to be one more than the current value of `mid`. Given the initial conditions:

- `low` is 1
- `high` is \(\min(a, b) + 1\)
- `mid` is \((\min(a, b) + 2) // 2\)

We can determine the updated value of `low` by calculating `mid` first.

Since `mid` is \((\min(a, b) + 2) // 2\), the new value of `low` will be \((\min(a, b) + 2) // 2 + 1\).

Given that `low` was initially 1, the updated value of `low` will be:

\[ \text{low} = (\min(a, b) + 2) // 2 + 1 \]

Therefore, the output state is:

Output State: **`n` is a positive integer such that \( 2 \leq n \leq a + b \); `a` and `b` are positive integers such that \( 1 \leq a \leq 100 \) and \( 1 \leq b \leq 100 \); `low` is \((\min(a, b) + 2) // 2 + 1\); `high` is \(\min(a, b) + 1\); `mid` is \((\min(a, b) + 2) // 2\)**