Let's analyze the provided code snippet step by step based on the initial state described.

Initial State: 
- `n` is a positive integer (1 ≤ n ≤ 100)
- `pos` is an integer (1 ≤ pos ≤ n)
- `l` is an integer (1 ≤ l ≤ r)
- `r` is an integer (l ≤ r ≤ n)
- `ans` is a positive integer equal to `l - pos` when `pos` is less than `l` (implying `ans` starts as a negative value since `l - pos` would be negative if `pos` is greater than or equal to `l`).
- The current value of `pos` is greater than `r`, meaning `pos > r`.

The code snippet:
```
ans += pos - r
```

Now, let's analyze the impact:

1. `ans` is being updated with the operation `ans += pos - r`.
2. Given that `pos > r`, the expression `pos - r` will yield a positive value since `pos` is greater than `r`.
3. Therefore, `ans` will be increased by this positive value, resulting in a new value for `ans`.

We will keep the rest of the variables unchanged and only update the value of `ans`. The state will now reflect the new value of `ans`.

Output State: **`n` is a positive integer (1 ≤ n ≤ 100), `pos` is an integer (1 ≤ pos ≤ n), `l` is an integer (1 ≤ l ≤ r), `r` is an integer (l ≤ r ≤ n), `ans` is a positive integer equal to the original value of `ans + (pos - r)`**.