To determine the output state, we analyze the impact of the line of code provided.

1. The line `f = factorial(n - k)` computes the factorial of `n - k`.
2. We know from the initial state:
   - `n` is a positive integer such that \(1 \leq n \leq 50\).
   - `k` is initialized to 1.
3. Therefore, we substitute `k` into the expression: \( n - k = n - 1 \).
4. The value of `f` is assigned as the factorial of \(n - 1\).

Since `n` is a positive integer within the specified range, `n - 1` is also a non-negative integer. Thus, `f` will be the factorial of a valid non-negative integer.

Hence, the output state will reflect the computed value of `f` along with the values of `n`, `k`, and other variables that remain unchanged.

Output State: **`n` is a positive integer such that 1 ≤ `n` ≤ 50; `k` is 1; `f` is factorial(n - 1)**