The initial state is defined as follows:
- `a` is the integer division of its original value by 3, and `a` must be greater than 0.
- `b` is the integer division of its value by 3 again, and `b` must be greater than 0.
- `c` is a non-negative integer such that \(0 \leq c \leq 10^9\).
- `ans` is equal to \((3 - a \% 3 + b \% 3) \% 3\).

The code snippet given is:
```python
ans *= 3
```

This line multiplies the current value of `ans` by 3. Let's determine the updated value of `ans`:

1. From the initial definition of `ans`, we know:
   \[
   ans = (3 - a \% 3 + b \% 3) \% 3
   \]
   Since \(a\) and \(b\) are integers greater than 0 and are the result of integer division by 3, their values modulo 3 can only be 0, 1, or 2.

2. The expression \((3 - a \% 3 + b \% 3) \% 3\) simplifies because:
   - \(a \% 3\) can be 0, 1, or 2.
   - \(b \% 3\) can be 0, 1, or 2.
   
   We can evaluate all possible cases:
   - If \(a \% 3 = 0\) and \(b \% 3 = 0\):
     \[
     ans = (3 - 0 + 0) \% 3 = 3 \% 3 = 0
     \]
   - If \(a \% 3 = 0\) and \(b \% 3 = 1\):
     \[
     ans = (3 - 0 + 1) \% 3 = 4 \% 3 = 1
     \]
   - If \(a \% 3 = 0\) and \(b \% 3 = 2\):
     \[
     ans = (3 - 0 + 2) \% 3 = 5 \% 3 = 2
     \]
   - If \(a \% 3 = 1\) and \(b \% 3 = 0\):
     \[
     ans = (3 - 1 + 0) \% 3 = 2 \% 3 = 2
     \]
   - If \(a \% 3 = 1\) and \(b \% 3 = 1\):
     \[
     ans = (3 - 1 + 1) \% 3 = 3 \% 3 = 0
     \]
   - If \(a \% 3 = 1\) and \(b \% 3 = 2\):
     \[
     ans = (3 - 1 + 2) \% 3 = 4 \% 3 = 1
     \]
   - If \(a \% 3 = 2\) and \(b \% 3 = 0\):
     \[
     ans = (3 - 2 + 0) \% 3 = 1 \% 3 = 1
     \]
   - If \(a \% 3 = 2\) and \(b \% 3 = 1\):
     \[
     ans = (3 - 2 + 1) \% 3 = 2 \% 3 = 2
     \]
   - If \(a \% 3 = 2\) and \(b \% 3 = 2\):
     \[
     ans = (3 - 2 + 2) \% 3 = 3 \% 3 = 0
     \]

Thus, `ans` can be 0, 1, or 2 depending on the values of \(a \% 3\) and \(b \% 3\).

After executing `ans *= 3`, the new value of `ans` is three times its previous value:
- If `ans` was 0, it becomes 0.
- If `ans` was 1, it becomes 3.
- If `ans` was 2, it becomes 6.

Therefore, the output state is:
Output State: **`a` is the integer division of its original value by 3, `b` is the integer division of its value by 3 again, both `a` and `b` must be greater than 0, `c` is a non-negative integer such that \(0 \leq c \leq 10^9\), and `ans` is equal to 0, 3, or 6.**