Given the initial state:
- `t` is an input integer such that 1 ≤ `t` ≤ 5 · 10^4
- `n` must be greater than 1
- `k` is an input integer
- `L` is a list containing one element `[m]`
- `m` is `(n + 1) // 2`

The code snippet is:
```python
n -= m
```

This operation modifies the value of `n` by subtracting `m` from it.

Since `m` is `(n + 1) // 2`, the new value of `n` will be:
\[ n_{\text{new}} = n - \frac{n + 1}{2} = \frac{2n - (n + 1)}{2} = \frac{n - 1}{2} \]

Therefore, the updated value of `n` is `(n - 1) // 2`.

The other variables (`t`, `k`, `L`, and `m`) remain unchanged.

Output State: **`t` is an input integer such that 1 ≤ `t` ≤ 5 · 10^4; `n` is `(n - 1) // 2`; `k` is an input integer; `L` is a list containing one element `[m]`; `m` is `(n + 1) // 2`**