Let's break down the initial state and the code snippet to determine what will be printed:

### Initial State:
- `n` and `m` are positive integers such that \(1 \leq n, m \leq 2 \times 10^6\).
- `T` is greater than 1.
- `t` is 2.
- `info` is a list of strings obtained from splitting the new input.
- `a` is the integer value of `info[0]`.
- `b` is the integer value of `info[1]` and must be at least 1.
- `i` is `b + 1`.
- `suma` is the sum of \((a - i * (i - 1)) // i\).

### Code Snippet:
```python
print(suma - 1)
```

### Step-by-Step Analysis:
1. **Understanding `info`**:
   - `info` is a list of strings obtained from splitting the new input. This means `info` contains at least two elements, where `info[0]` and `info[1]` are the first and second elements, respectively.

2. **Assigning Values to `a` and `b`**:
   - `a` is the integer value of `info[0]`.
   - `b` is the integer value of `info[1]` and must be at least 1.

3. **Calculating `i`**:
   - `i` is `b + 1`.

4. **Calculating `suma`**:
   - `suma` is the sum of \((a - i * (i - 1)) // i\).
   - Let's break this down further:
     - \(i = b + 1\)
     - \(i * (i - 1)\) is the product of `i` and `i - 1`.
     - \(a - i * (i - 1)\) is the difference between `a` and the product.
     - \((a - i * (i - 1)) // i\) is the integer division of the difference by `i`.
     - `suma` is the sum of this result.

5. **Final Calculation**:
   - The code snippet `print(suma - 1)` will print the value of `suma` minus 1.

### Example Calculation:
Let's assume `info` is `['10', '2']`:
- `a = 10`
- `b = 2`
- `i = b + 1 = 2 + 1 = 3`
- Calculate \(i * (i - 1) = 3 * 2 = 6\)
- Calculate \(a - i * (i - 1) = 10 - 6 = 4\)
- Calculate \((a - i * (i - 1)) // i = 4 // 3 = 1\)
- `suma` is the sum of this result, which is 1.
- `print(suma - 1) = 1 - 1 = 0`

### General Case:
- The value of `suma` depends on the specific values of `a` and `b` from the input.
- The final output will be `suma - 1`.

### Final Output:
Output: **suma - 1 (where suma is the sum of \((a - i * (i - 1)) // i\) and i is b + 1)**