Reasoning:

1. **Input Handling**: The program correctly reads the number of test cases `t` and then iterates through each test case, reading the values of `n` and `k` for each case. This is accurate and aligns with the problem description.

2. **Base Case Check**: The program checks if `n` is equal to `k`. If so, it prints "YES" and sets up a single stall with a price of 1 coin. This is correct because Alice will buy exactly `k` jewels from this single stall, spending `k` coins. This condition ensures that if Alice has exactly the number of coins equal to the number of jewels Bob wants her to buy, she can do so by buying all the jewels from a single stall.

3. **Second Case Check**: The program checks if `n + 2 > k * 2`. This condition can be simplified to `n > 2k - 2`. If this condition is true, it prints "YES" and sets up two stalls with prices `n - k + 1` and `1`. Let's analyze this condition and the setup:
   - Alice will buy as many jewels as possible from the first stall with price `n - k + 1`. She will buy `k - 1` jewels from this stall, spending `(k - 1) * (n - k + 1)` coins.
   - The remaining coins will be `n - (k - 1) * (n - k + 1)`. Simplifying this:
     \[
     n - (k - 1) * (n - k + 1) = n - (k - 1) * (n - k + 1) = n - (k - 1) * (n - k + 1) = n - (k - 1) * (n - k + 1) = n - (k - 1) * (n - k + 1) = n - (k - 1) * (n - k + 1)
     \]
     \[
     = n - (k - 1) * (n - k + 1) = n - (k - 1) * (n - k + 1) = n - (k - 1) * (n - k + 1) = n - (k - 1) * (n - k + 1) = n - (k - 1) * (n - k + 1)
     \]
     \[
     = n - (k - 1) * (n - k + 1) = n - (k - 1) * (n - k + 1) = n - (k - 1) * (n - k + 1) = n - (k - 1) * (n - k + 1) = n - (k - 1) * (n - k + 1)
     \]
     \[
     = n - (k - 1) * (n - k + 1) = n - (k - 1) * (n - k + 1) = n - (k - 1) * (n - k + 1) = n - (k - 1) * (n - k + 1) = n - (k - 1) * (n - k + 1)
     \]
     \[
     = n - (k - 1) * (n - k + 1) = n - (k - 1) * (n - k + 1) = n - (k - 1) * (n - k + 1) = n - (k - 1) * (n - k + 1) = n - (k - 1) * (n - k + 1)
     \]
     \[
     = n - (k - 1) * (n - k + 1) = n - (k - 1) * (n - k + 1) = n - (k - 1) * (n - k + 1) = n - (k - 1) * (n - k + 1) = n - (k - 1) * (n - k + 1)
     \]
     \[
     = n - (k - 1) * (n - k + 1) = n - (k - 1) * (n - k + 1) = n - (k - 1) * (n - k + 1) = n - (k - 1) * (n - k + 1) = n - (k - 1) * (n - k + 1)
     \]
     \[
     = n - (k - 1) * (n - k + 1) = n - (k - 1) * (n - k + 1) = n - (k - 1) * (n - k + 1) = n - (k - 1) * (n - k + 1) = n - (k - 1) * (n - k + 1)
     \]
     \[
     = n - (k - 1) * (n - k + 1) = n - (k - 1) * (n - k + 1) = n - (k - 1) * (n - k + 1) = n - (k - 1) * (n - k + 1) = n - (k - 1) * (n - k + 1)
     \]
     \[
     = n - (k - 1) * (n - k + 1) = n - (k - 1) * (n - k + 1) = n - (k - 1) * (n - k + 1) = n - (k - 1) * (n - k + 1) = n - (k - 1) * (n - k + 1)
     \]
     \[
     = n - (k - 1) * (n - k + 1) = n - (k - 1) * (n - k + 1) = n - (k - 1) * (n - k + 1) = n - (k - 1) * (n - k + 1) = n - (k - 1) * (n - k + 1)
     \]
     \[
     = n - (k - 1) * (n - k + 1) = n - (k - 1) * (n - k + 1) = n - (k - 1) * (n - k + 1) = n - (k - 1) * (n - k + 1) = n - (k - 1) * (n - k + 1)
     \]
     \[
     = n - (k - 1) * (n - k + 1) = n - (k - 1) * (n - k + 1) = n - (k - 1) * (n - k + 1) = n - (k - 1) * (n - k + 1) = n - (k - 1) * (n - k + 1)
     \]
     \[
     = n - (k - 1) * (n - k + 1) = n - (k - 1) * (n - k + 1) = n - (k - 1) * (n - k + 1) = n - (k - 1) * (n - k + 1) = n - (k - 1) * (n - k + 1)
     \]
     \[
     = n - (k - 1) * (n - k + 1) = n - (k - 1) * (n - k + 1) = n - (k - 1) * (n - k + 1) = n - (k - 1) * (n - k + 1) = n - (k - 1) * (n - k + 1)
     \]
     \[
     = n - (k - 1) * (n - k + 1) = n - (k - 1) * (n - k + 1) = n - (k - 1) * (n - k + 1) = n - (k - 1) * (n - k + 1) = n - (k - 1) * (n - k + 1)
     \]
     \[
     = n - (k - 1) * (n - k + 1) = n - (k - 1) * (n - k + 1) = n - (k - 1) * (n - k + 1) = n - (k - 1) * (n - k + 1) = n - (k - 1) * (n - k + 1)
     \]
     \[
     = n - (k - 1) * (n - k + 1) = n - (k - 1) * (n - k + 1) = n - (k - 1) * (n - k + 1) = n