Alright, I've got this problem to solve. Let's see what it's about. So, Polycarp has a string made up of lowercase Latin letters, and he encodes it using a specific algorithm. I need to write a program that can decode it back to the original string.

First, I need to understand the encoding process clearly. The description says that he constructs an auxiliary string 'r' which consists of all distinct letters from the string 's', arranged in alphabetical order. Then, each character in 's' is replaced by its symmetric character from 'r'. That means the first character of 'r' is replaced by the last of 'r', the second by the second last, and so on.

For example, with s = "codeforces", r is "cdefors". So, 'c' is replaced by 's', 'o' by 'e', 'd' by 'r', and so on, resulting in "serofedsoc".

Okay, so my task is to reverse this process. Given the encoded string 'b', I need to find the original string 's'.

Let me think about how to approach this.

First, since 'r' is made up of unique characters from 's' in sorted order, and 'b' is 's' with each character replaced by its symmetric character from 'r', I need to find 'r' and then reverse the replacement.

Wait, but I don't have 's', I only have 'b' and 'r'. But 'r' is derived from 's', which I don't have. Hmm.

Wait, no. Given 'b' and 'r', I can decode 'b' back to 's', because the encoding is a direct mapping from 's' to 'b' via 'r'.

But in this problem, I'm only given 'b', and I need to find 's'. That means I need to figure out 'r' from 'b', since 'b' is encoded from 's' using 'r'.

Wait, but 'r' is derived from 's', which I don't have. So, how can I find 'r' from 'b'?

Well, since 'b' is obtained by replacing each character in 's' with its symmetric character from 'r', and 'r' is the sorted unique characters of 's', maybe I can find 'r' by looking at the unique characters in 'b' and assuming that 'b' is encoded from 's' using 'r'.

Wait, but 's' and 'b' have the same set of unique characters, because the encoding is a permutation of these characters.

So, the unique characters in 'b' are the same as the unique characters in 's', just mapped differently.

Therefore, 'r' can be obtained by sorting the unique characters in 'b'.

Wait, is that correct? Let's see.

If 'r' is made up of unique characters from 's' in sorted order, and 's' and 'b' have the same unique characters, then sorting the unique characters in 'b' should give me 'r'.

Yes, that seems right.

So, step 1: From 'b', find 'r' by sorting the unique characters in 'b'.

Then, since the encoding replaces each character in 's' with its symmetric character from 'r', to decode 'b' back to 's', I need to reverse this mapping.

That is, for each character in 'b', find its symmetric character in 'r' to get back to 's'.

Wait, no. Let's think carefully.

In the encoding process:

- Each character in 's' is replaced by its symmetric character from 'r'.

So, to decode:

- Each character in 'b' should be replaced back by its original character from 's', which is its symmetric character from 'r'.

Wait, that seems a bit confusing. Let's think with the example.

Given s = "codeforces", r = "cdefors", encoded b = "serofedsoc".

Now, to decode "serofedsoc" back to "codeforces", I need to map each character in "serofedsoc" to its corresponding character in "codeforces" via 'r'.

From the encoding process, 'c' in 's' is replaced by 's' in 'b', 'o' in 's' by 'e' in 'b', and so on.

So, to decode, I need a mapping from 's' in 'b' back to 'c' in 's', from 'e' in 'b' back to 'o' in 's', etc.

Wait, but I don't have 's', I only have 'b' and 'r'.

Given 'r' = "cdefors", the symmetric mapping is:

c -> s

d -> r

e -> o

f -> f

o -> e

r -> d

s -> c

So, to decode 'b' to 's', I need to apply this mapping in reverse, meaning:

s -> c

e -> o

r -> d

f -> f

o -> e

d -> r

c -> s

Wait, no. To decode, I need to map each character in 'b' to its corresponding character in 's', which is its symmetric character from 'r'.

Wait, maybe it's better to think of it as a bijection. The mapping is a bijection between characters in 's' and 'b' via 'r'.

So, to decode, I need to apply the inverse mapping.

Wait, perhaps it's easier to construct a mapping from 'r' to its symmetric 'r'.

Let me try to formalize this.

Let 'r' be the sorted unique characters of 's'.

Let the mapping be a function map: s -> b, where map(c) = r[len(r) - 1 - idx(c)], where idx(c) is the index of c in 'r'.

So, to decode, I need a function inv_map: b -> s, where inv_map(d) = r[idx(d)], but idx(d) is the index of d in the symmetric position in 'r'.

Wait, this is getting messy. Maybe I should think of 'r' as a list, and create a mapping from encoded character back to original character based on their positions in 'r'.

Let me try.

Given 'r' = ['c', 'd', 'e', 'f', 'o', 'r', 's']

Then, the mapping for encoding is:

c -> s (position 0 -> position 6)

d -> r (position 1 -> position 5)

e -> o (position 2 -> position 4)

f -> f (position 3 -> position 3)

Similarly, for decoding, I need to map s -> c, r -> d, o -> e, f -> f, etc.

So, in other words, the decoding mapping is the inverse of the encoding mapping.

So, to decode, I need to map each character in 'b' to the character in 's' that was encoded to it.

Given that the encoding mapping is map: s -> b via map(c) = r[len(r)-1 - idx(c)], then the decoding mapping should be inv_map(d) = r[len(r)-1 - idx(d)].

Wait, does that make sense?

Let me test it with the example.

Take 's' = "codeforces", 'r' = "cdefors"

Encoding:

c -> s

o -> e

d -> r

f -> f

o -> e

r -> d

c -> s

e -> o

f -> f

e -> o

s -> c

So, b = "serofedsoc"

Now, to decode "serofedsoc" back to "codeforces", using the decoding mapping:

s -> c

e -> o

r -> d

f -> f

o -> e

d -> r

e -> o

s -> c

o -> o

c -> s

Which is "codeforces". Yes, that works.

So, the decoding mapping is the same as the encoding mapping, because the mapping is its own inverse.

Wait, is that always true?

In this case, it seems that applying the mapping twice brings us back to the original character.

Yes, because map(map(c)) = c.

Let's see:

map(c) = s

map(s) = c

map(o) = e

map(e) = o

map(d) = r

map(r) = d

map(f) = f

So, indeed, map is its own inverse.

Therefore, to decode 'b' back to 's', I can apply the same mapping again.

That simplifies things a lot.

So, in code, I can:

1. From 'b', find 'r' by sorting its unique characters.

2. Create a mapping from each character in 'r' to its symmetric character in 'r'.

3. Apply this mapping to each character in 'b' to get back 's'.

This should work, because the mapping is its own inverse.

Let me try it with the example.

b = "serofedsoc"

r = sorted(unique(b)) = "cdefors"

Mapping:

c -> s

d -> r

e -> o

f -> f

o -> e

r -> d

s -> c

Apply this mapping to "serofedsoc":

s -> c

e -> o

r -> d

o -> e

f -> f

e -> o

d -> r

s -> c

o -> o

c -> s

Which is "codeforces". Perfect.

Another example from the input:

b = "ttfh"

r = sorted(unique(b)) = "ft"

Mapping:

f -> t

t -> f

Apply to "ttfh":

t -> f

t -> f

f -> t

h -> h (assuming h is in r, but h is not in b, wait, but in this test case, it's "ttf", which corresponds to "fft"

Wait, in the sample input, one test case is:

3

ttf

So, b = "ttf"

r = sorted(unique(b)) = "ft"

Mapping:

f -> t

t -> f

Apply to "ttf":

t -> f

t -> f

f -> t

Which is "fft". Matches the sample output.

Great, seems correct.

Another test case:

b = "tlrhgmaoi"

r = sorted(unique(b)) = "aghilmort"

Wait, "tlrhgmaoi" unique letters are t, l, r, h, g, m, a, o, i -> sorted "a,g,h,i,l,m,o,r,t"

Mapping:

a -> t

g -> r

h -> o

i -> m

l -> l

m -> i

o -> h

r -> g

t -> a

Apply to "tlrhgmaoi":

t -> a

l -> l

r -> g

h -> o

g -> r

m -> i

a -> t

o -> h

i -> m

Which is "algorithm". Matches the sample output.

Excellent.

Another test case:

b = "w"

r = "w"

Mapping: w -> w

So, decoded is "w". Matches the sample output.

Last test case:

b = "hnndledmnhlttin"

r = sorted(unique(b)) = "dehilmnnt"

Mapping:

d -> t

e -> n

h -> n

i -> l

l -> h

m -> m

n -> e

t -> d

Apply to "hnndledmnhlttin":

h -> n

n -> e

n -> e

d -> t

l -> h

e -> n

d -> t

m -> m

n -> e

h -> n

l -> h

t -> d

t -> d

i -> l

n -> e

Which is "neethtmtenehdlne". Wait, that doesn't match the sample output "meetinthemiddle". Maybe I messed up.

Wait, perhaps I miscounted the positions.

Let's see, r = "dehilmnt" (unique sorted from b)

Wait, "dehilmnnt" has duplicates, but set removes duplicates, so r = "dehilmnt" sorted.

Indices:

d:0 -> t:7

e:1 -> n:6

h:2 -> t:5

i:3 -> h:4

l:4 -> i:3

m:5 -> m:2

n:6 -> e:1

t:7 -> d:0

So, mapping:

d -> t

e -> n

h -> t

i -> h

l -> i

m -> m

n -> e

t -> d

Apply to "hnndledmnhlttin":

h -> t

n -> e

n -> e

d -> t

l -> i

e -> n

d -> t

m -> m

n -> e

h -> t

l -> i

t -> d

t -> d

i -> h

n -> e

So, "teetitmtetidehne". That still doesn't match "meetinthemiddle". Maybe I messed up the sorting or the mapping.

Wait, perhaps I need to consider that 'r' should be made from 's', not 'b'. But earlier it seemed to work.

Wait, maybe my assumption that 'r' can be obtained by sorting unique characters of 'b' is wrong.

Wait, no, in the earlier test cases, it worked.

Wait, in the last test case, b = "hnndledmnhlttin"

Assuming r is sorted unique characters of b, which is "dehilmnt"

Mapping:

d -> t

e -> n

h -> m

i -> l

l -> i

m -> h

n -> e

t -> d

Wait, perhaps I miscounted the positions.

Let me index 'r' = "dehilmnt"

Indices: 0 to 7

Symmetric positions:

0 -> 7: d -> t

1 -> 6: e -> n

2 -> 5: h -> m

3 -> 4: i -> l

So, mapping is:

d -> t

e -> n

h -> m

i -> l

l -> i

m -> h

n -> e

t -> d

Apply to "hnndledmnhlttin":

h -> m

n -> e

n -> e

d -> t

l -> i

e -> n

d -> t

m -> h

n -> e

h -> m

l -> i

t -> d

t -> d

i -> l

n -> e

So, "meetinthemiddle". Yes, that matches the sample output.

I must have messed up the earlier mapping.

So, the correct approach is:

- From 'b', find 'r' by sorting its unique characters.

- Create a mapping from each character in 'r' to its symmetric character in 'r'.

- Apply this mapping to each character in 'b' to get back 's'.

This seems to work for all sample inputs.

Now, let's look at the provided program and see if it implements this correctly.

The program is:

import sys

input = sys.stdin.read

data = input().split()

index = 0

t = int(data[index])

index += 1

results = []

for _ in range(t):

n = int(data[index])

index += 1

b = data[index]

index += 1

results.append(func_1(b))

print('\n'.join(results))

def func_1(encoded):

r = ''.join(sorted(set(encoded)))

mapping = {r[i]: r[-(i + 1)] for i in range(len(r))}

return ''.join((mapping[char] for char in encoded))

So, it reads all input at once, splits it into words, and processes them one by one.

It reads t, then for each test case, reads n and then the encoded string b.

Then, it calls func_1(b) to decode it and collects the results.

In func_1:

- It creates 'r' by sorting the unique characters of 'encoded' (which is 'b').

- Then, it creates a mapping where each character in 'r' is mapped to its symmetric character in 'r'.

- Finally, it applies this mapping to each character in 'encoded' to get the decoded string.

This matches exactly the approach I just reasoned through.

Therefore, the program should be correct.

I can test it with the sample inputs to confirm.

Sample Input:

5

10

serofedsoc

3

ttf

9

tlrhgmaoi

1

w

15

hnndledmnhlttin

Sample Output:

codeforces

fft

algorithm

w

meetinthemiddle

As I verified earlier, this approach correctly decodes each 'b' back to 's'.

Hence, the program is correct.

**Final Answer**

\[ \boxed{\text{The program is correct.}} \]