To determine the output state, we need to evaluate the expression `z += z // (k - 1) + 1` using the initial values provided.

Given:
- `s` is "5 6 7"
- `k` is 5
- `x` is 6
- `a` is 7
- `z` is 3

Let's compute `z` after the operation:

1. Calculate `k - 1`:
   \[
   k - 1 = 5 - 1 = 4
   \]

2. Calculate `z // (k - 1)`:
   \[
   z // (k - 1) = 3 // 4 = 0 \quad \text{(integer division)}
   \]

3. Calculate the new value of `z`:
   \[
   z = z + z // (k - 1) + 1 = 3 + 0 + 1 = 4
   \]

The value of `z` is updated to 4. The other variables remain unchanged.

Output State: **`s` is "5 6 7", `k` is 5, `x` is 6, `a` is 7, `z` is 4**.