To determine the final output state after all iterations of the loop, we need to carefully analyze the loop and how the variables change with each iteration.

Given:
- `info` is a new list of substrings based on the user's input.
- `t` is `b + 3`.
- `T` is greater than 0.
- `a` is the integer value of `info[0]`.
- `b` is the integer value of `info[1]`.
- `i` is `b + 1` initially, but the loop starts with `i` from 1 to `b`.
- `suma` is 0 initially.

The loop runs from `i = 1` to `i = b`. For each iteration, `x` is calculated as:
\[ x = \left(\frac{a - i \cdot (i - 1)}{i^2}\right) + 1 \]
If `x > 0`, `suma` is incremented by `x`. Additionally, if \((a - i \cdot (i - 1)) \mod i^2 == 0\) and \(i \cdot (i - 1) \mod i^2 == 0\), `suma` is incremented by 1.

Let's break down the loop iterations:

1. **First Iteration (i = 1)**:
   - \( x = \left(\frac{a - 1 \cdot 0}{1^2}\right) + 1 = a + 1 \)
   - If \(a + 1 > 0\), `suma` becomes \(a + 1\).
   - The condition \((a - 1 \cdot 0) \mod 1^2 == 0\) and \(1 \cdot 0 \mod 1^2 == 0\) is always true, so `suma` becomes \(a + 2\).

2. **Second Iteration (i = 2)**:
   - \( x = \left(\frac{a - 2 \cdot 1}{2^2}\right) + 1 = \left(\frac{a - 2}{4}\right) + 1 \)
   - If \(\left(\frac{a - 2}{4}\right) + 1 > 0\), `suma` is incremented by \(\left(\frac{a - 2}{4}\right) + 1\).
   - The condition \((a - 2 \cdot 1) \mod 2^2 == 0\) and \(2 \cdot 1 \mod 2^2 == 0\) may or may not be true, so `suma` might be incremented by 1 if the condition holds.

3. **Third Iteration (i = 3)**:
   - \( x = \left(\frac{a - 3 \cdot 2}{3^2}\right) + 1 = \left(\frac{a - 6}{9}\right) + 1 \)
   - If \(\left(\frac{a - 6}{9}\right) + 1 > 0\), `suma` is incremented by \(\left(\frac{a - 6}{9}\right) + 1\).
   - The condition \((a - 3 \cdot 2) \mod 3^2 == 0\) and \(3 \cdot 2 \mod 3^2 == 0\) may or may not be true, so `suma` might be incremented by 1 if the condition holds.

This pattern continues up to `i = b`. The final value of `suma` will be the sum of all valid `x` values plus any additional 1s from the conditions.

Therefore, the output state after all iterations will be:
- `info` remains unchanged as a new list of substrings based on the user's input.
- `t` remains `b + 3`.
- `T` remains greater than 0.
- `a` remains the integer value of `info[0]`.
- `b` remains the integer value of `info[1]`.
- `i` is `b + 1` after the loop ends.
- `suma` is the sum of all valid `x` values plus any additional 1s from the conditions.

Output State: **`info` is a new list of substrings based on the user's input, `t` is `b + 3`, `T` is greater than 0, `a` is the integer value of `info[0]`, `b` is the integer value of `info[1]`, `i` is `b + 1`, `suma` is the sum of all valid `x` values plus any additional 1s from the conditions.**

In simpler terms, the final `suma` is the sum of calculated `x` values for each iteration where `x > 0`, plus an additional 1 for each iteration where the specific modulo conditions are met.