To determine the output state, we need to compute the value of `res` based on the given formula and the initial state. The formula for `res` is:

\[ \text{res} = \left| \sqrt{\text{p1}} \times \sqrt{\text{p2}} \right| \]

Where:
- \( \text{p1} = (\text{coord[1][0]} - \text{coord[0][0]}) \)
- \( \text{p2} = (\text{coord[3][0]} - \text{coord[2][0]}) \)

Let's assume the coordinates in `coord` are \((x1, y1)\), \((x2, y2)\), \((x3, y3)\), and \((x4, y4)\). Given that `coord` is sorted in ascending order first by x-coordinates and then by y-coordinates, we have:

- \( x1 \leq x2 \leq x3 \leq x4 \)
- If \( x1 = x2 \), then \( y1 \leq y2 \)
- If \( x3 = x4 \), then \( y3 \leq y4 \)

Thus:
- \( \text{p1} = x2 - x1 \)
- \( \text{p2} = x4 - x3 \)

The value of `res` will be:
\[ \text{res} = \left| \sqrt{x2 - x1} \times \sqrt{x4 - x3} \right| \]

Since `x2 - x1` and `x4 - x3` are differences of x-coordinates, they are non-negative. Therefore, the absolute value is not necessary, and we can simplify it to:
\[ \text{res} = \sqrt{(x2 - x1) \times (x4 - x3)} \]

Now, let's update the output state with the new value of `res`:

Output State: **`n` must be at least 2, `coord` is `[(x1, y1), (x2, y2), (x3, y3), (x4, y4)]` sorted in ascending order first by x-coordinates and then by y-coordinates, `res` is `sqrt((x2 - x1) * (x4 - x3))`, `i` is `3`, `x` is the first integer from the last input, `y` is the second integer from the last input, `p1` is `(coord[1][0] - coord[0][0])`, `p2` is `(coord[3][0] - coord[2][0])`**.