To determine the necessary adjustments to the program state so that the first iteration of the `while` loop can proceed, we need to analyze the condition in the loop head:

```
while (x + y) * x <= n and (x + y) * y <= m:
    # the loop body is omit
```

The loop will execute if both conditions `(x + y) * x <= n` and `(x + y) * y <= m` are true.

Given the current state:
- `n` is 5
- `m` is 20
- `x` is 2
- `y` is 1
- `cnt` is 6.1667 (though `cnt` is not used in the loop condition, it's included in the state)

Let's evaluate the conditions with the current values:
1. `(x + y) * x = (2 + 1) * 2 = 3 * 2 = 6`
   - Check if `6 <= n`: Since `n` is 5, this condition is false (`6 <= 5` is false).

2. `(x + y) * y = (2 + 1) * 1 = 3 * 1 = 3`
   - Check if `3 <= m`: Since `m` is 20, this condition is true (`3 <= 20` is true).

Since the first condition `(x + y) * x <= n` is false, we need to adjust either `x`, `y`, or `n` so that this condition becomes true.

### Adjusting the State
To make `(x + y) * x <= n` true, we can either:
- Increase `n` to be at least 6.
- Decrease `x` to be such that `(x + y) * x` is less than or equal to 5.
- Decrease `y` to be such that `(x + y) * x` is less than or equal to 5.

Let's consider the simplest adjustment: increasing `n` to be at least 6.

### New State
If we increase `n` to 6, the new state would be:
- `n` is 6
- `m` is 20
- `x` is 2
- `y` is 1
- `cnt` is 6.1667

With these values, let's re-evaluate the conditions:
1. `(x + y) * x = (2 + 1) * 2 = 3 * 2 = 6`
   - Check if `6 <= n`: Since `n` is now 6, this condition is true (`6 <= 6` is true).

2. `(x + y) * y = (2 + 1) * 1 = 3 * 1 = 3`
   - Check if `3 <= m`: Since `m` is 20, this condition is true (`3 <= 20` is true).

Both conditions are now true, so the loop can execute.

### Final Answer
State: **`n` is 6, `m` is 20, `x` is 2, `y` is 1, and `cnt` is 6.1667**