The code `n -= i * curr` updates the value of `n` by subtracting the product of `i` and `curr` from the current value of `n`. Given the initial state:

- `n` is updated to `n - i * curr`
- `k` is a positive integer such that 1 ≤ k ≤ 10^18
- `n` is not equal to `k`
- `n` is greater than or equal to `k`
- `costs` is a list containing two elements: `[n - k + 1, 1]`
- `h` is `n // (n - k + 1) + n + curr`
- `i` is `1`
- `curr` is `n`

Let's calculate the new value of `n`:

1. `i` is `1`
2. `curr` is `n`
3. `n -= i * curr` means `n -= 1 * n`, which simplifies to `n -= n`, resulting in `n` becoming `0`.

After executing the code, the updated state is:

- `n` is `0`
- `k` is a positive integer such that 1 ≤ k ≤ 10^18
- `n` is not equal to `k` (since `n` is now `0` and `k` is a positive integer)
- `n` is less than `k` (since `n` is `0` and `k` is a positive integer)
- `costs` is a list containing two elements: `[n - k + 1, 1]` (which remains unchanged because `n` was used in its initial form to create the list)
- `h` is `n // (n - k + 1) + n + curr` (which remains unchanged because `n` was used in its initial form to create `h`)
- `i` is `1`
- `curr` is `n` (which is now `0`)

Output State: **`n` is `0`, `k` is a positive integer such that 1 ≤ k ≤ 10^18, `n` is not equal to `k`, `n` is less than `k`, `costs` is `[n - k + 1, 1]`, `h` is `n // (n - k + 1) + n + curr`, `i` is `1`, `curr` is `0`**