The code snippet `nx += xx[i][j - 1]` updates the value of `nx` by adding the element at index `j-1` (which is 0) of the list `xx[i]` to `nx`.

Given the initial state:
- `n` remains an integer such that 2 ≤ n ≤ 24
- `j` is 1
- The element at index `j-1` (which is 0) of the list `xx[i]` is not equal to '?'

Let's assume `xx[i][0]` is a specific value, say `val`. The value of `nx` is updated to `nx + val`.

Therefore, the output state is:
- `n` remains an integer such that 2 ≤ n ≤ 24
- `j` is 1
- The element at index `j-1` (which is 0) of the list `xx[i]` is not equal to '?'
- `nx` is now `nx + xx[i][0]`

Output State: **`n` remains an integer such that 2 ≤ n ≤ 24, `j` is 1, the element at index 0 of the list `xx[i]` is not equal to '?', and `nx` is now `nx + xx[i][0]`.**