The value of `z` is updated using the expression `z += z // (k - 1) + 1`. Given that `z` is initially `k - 1`, we substitute `z` with `k - 1` in the expression.

The new value of `z` is calculated as:
\[ z = (k - 1) + \frac{(k - 1)}{(k - 1)} + 1 \]
\[ z = (k - 1) + 1 + 1 \]
\[ z = k + 1 \]

The values of `k`, `x`, `a`, and `i` remain unchanged.

Output State: **`k` is an integer between 2 and 30, `x` is an integer between `k` and 100 (inclusive) and not equal to `k - 1`, `a` is an integer between 1 and 10^9, `z` is `k + 1`, `i` is 1**.