Output State: **`t` must be greater than 0, `n` must be greater than or equal to 3, `sum` is 1 + (2 * 2 - 1 * 1) * 2 + (3 * 3 - 2 * 2) * 3, `i` is 3**

Explanation: The value of `sum` is updated by adding the expression `(i * i - (i - 1) * (i - 1)) * i` to its current value. Given that `i` is 3, the expression evaluates to `(3 * 3 - 2 * 2) * 3 = (9 - 4) * 3 = 5 * 3 = 15`. Therefore, the new value of `sum` is `1 + (2 * 2 - 1 * 1) * 2 + 15 = 1 + 6 + 15 = 22`. The values of `t` and `n` remain unchanged, and `i` remains 3.