Let's break down the initial state and the print statement step by step to determine what will be printed.

### Initial State:
1. `p_1`, `p_2`, and `p_3` are integers provided by the user such that \(0 \leq p_1 \leq p_2 \leq p_3 \leq 30\).
2. `t` is greater than 0 (though `t` is not used in the print statement).
3. `_` is 0 (though `_` is not used in the print statement).
4. `low` is \( \min(p_3 - p_1, p_3 - p_2) \).
5. `high` is \( \max(p_3 - p_1, p_3 - p_2) \).
6. `cur` is `low`.
7. The sum of `p_1`, `p_2`, and `p_3` is odd.
8. `p_3` is less than `p_1 + p_2`.
9. The current value of `p_1 - cur` is less than or equal to `p_2 - (p_3 - cur)`.

### Analysis:
1. **Determine `low` and `high`:**
   - Since \( p_1 \leq p_2 \leq p_3 \), the differences \( p_3 - p_1 \) and \( p_3 - p_2 \) will be non-negative.
   - `low` will be the smaller of these two differences, and `high` will be the larger.
   - Therefore, \( \text{low} = p_3 - p_2 \) and \( \text{high} = p_3 - p_1 \).

2. **Determine `cur`:**
   - `cur` is set to `low`, which is \( p_3 - p_2 \).

3. **Check the condition `p_1 - cur` is less than or equal to `p_2 - (p_3 - cur)`:**
   - Substitute `cur` with \( p_3 - p_2 \):
     \[
     p_1 - (p_3 - p_2) \leq p_2 - (p_3 - (p_3 - p_2))
     \]
   - Simplify the right side:
     \[
     p_1 - (p_3 - p_2) \leq p_2 - p_2
     \]
   - This simplifies to:
     \[
     p_1 - (p_3 - p_2) \leq 0
     \]
   - Further simplification:
     \[
     p_1 - p_3 + p_2 \leq 0
     \]
   - Rearrange:
     \[
     p_1 + p_2 \leq p_3
     \]
   - However, we are given that \( p_3 < p_1 + p_2 \), so the condition \( p_1 + p_2 \leq p_3 \) is always false. This suggests that the condition might be a constraint that is always satisfied given the other conditions.

4. **Calculate the expression `p1 - cur + p3`:**
   - Substitute `cur` with \( p_3 - p_2 \):
     \[
     p_1 - (p_3 - p_2) + p_3
     \]
   - Simplify:
     \[
     p_1 - p_3 + p_2 + p_3
     \]
   - This simplifies to:
     \[
     p_1 + p_2
     \]

### Final Output:
The print statement will output the sum of `p_1` and `p_2`.

Output: **p_1 + p_2 (where p_1 and p_2 are integers such that 0 <= p_1 <= p_2 <= p_3 <= 30, p_3 < p_1 + p_2, and the sum of p_1, p_2, and p_3 is odd)**