Let's break down the initial state and the code snippet step by step to determine what will be printed.

### Initial State:
1. `p_1`, `p_2`, and `p_3` are integers provided by the user such that:
   - \(0 \leq p_1 \leq p_2 \leq p_3 \leq 30\)
   - \(p_3 < p_1 + p_2\)
2. `t` is greater than 0 (though `t` is not used in the code snippet).
3. `_` is 0 (though `_` is not used in the code snippet).
4. `low` is \( \min(p_3 - p_1, p_3 - p_2) \).
5. `high` is \( \max(p_3 - p_1, p_3 - p_2) \).
6. `cur` is incremented by 1.
7. `high >= cur` must hold.

### Code Snippet:
```python
print(p1 - cur + p3)
```

### Step-by-Step Analysis:
1. **Initial Values:**
   - `p_1`, `p_2`, and `p_3` are integers such that \(0 \leq p_1 \leq p_2 \leq p_3 \leq 30\) and \(p_3 < p_1 + p_2\).
   - `low` is \( \min(p_3 - p_1, p_3 - p_2) \).
   - `high` is \( \max(p_3 - p_1, p_3 - p_2) \).
   - `cur` is initially 0.

2. **Incrementing `cur`:**
   - `cur` is incremented by 1, so `cur` becomes 1.
   - The condition `high >= cur` must hold, which means \( \max(p_3 - p_1, p_3 - p_2) \geq 1 \).

3. **Expression in the `print` Statement:**
   - The expression to be printed is `p1 - cur + p3`.
   - Substituting the values, we get:
     \[
     p1 - cur + p3 = p_1 - 1 + p_3
     \]

4. **Final Output:**
   - The value printed will be \( p_1 - 1 + p_3 \).
   - Given the constraints \(0 \leq p_1 \leq p_2 \leq p_3 \leq 30\) and \(p_3 < p_1 + p_2\), the value of \( p_1 - 1 + p_3 \) will be an integer within the range of the constraints.

### Conclusion:
The `print` statement will output the value of \( p_1 - 1 + p_3 \), which is an integer based on the given constraints.

Output: **\( p_1 - 1 + p_3 \) (where \( p_1 \) and \( p_3 \) are integers provided by the user such that \(0 \leq p_1 \leq p_2 \leq p_3 \leq 30\) and \(p_3 < p_1 + p_2\))**