Output State: **`c` is 2, `n` is an integer such that \(1 \leq n \leq 2 \cdot 10^5\), `i` is `n - 3`, `k` is `k - (n - 1) + 1 - (n - 3) + 1`, `l` is the result of `func_3(c, l)`**

Explanation:
- The initial value of `c` is 2.
- `n` remains an integer within the range \(1 \leq n \leq 2 \cdot 10^5\).
- `i` is calculated as `n - 3`.
- `k` is updated as `k - (n - 1) + 1 - (n - 3) + 1`, which simplifies to `k - n + 1 + 1 - n + 3 + 1` or `k - 2n + 6`.
- The line `l = func_3(c, l)` updates `l` to the result of calling `func_3` with arguments `c` (which is 2) and `l`. The exact value of `l` depends on the implementation of `func_3`, but it is now the return value of this function call.