The code `ss -= 1` decrements the value of `ss` by 1. Given that `ss` is initially the count of 'S' in the string `l`, it simply decreases by 1. The states of all other variables remain unchanged.

Therefore, the output state is:
Output State: **`n` is the count of 'N' in the string `l`, `s` is the count of 'S' in the string `l` minus 1, `w` is the count of 'W' in the string `l`, `e` is the count of 'E' in the string `l`, `nn` and `ss` are updated based on the comparison between `n` and `s` with `ss` decreased by 1, `ww` is `0` since `w` is not greater than `e`, `ee` is `e - w` since `w` is not greater than `e`, `m` is an input integer, `l` is a non-empty input string, `r` is `1` if `(ss % 2 == 1)` is true, otherwise `r` is `0`, `h` is `1` if `(ss % 2 == 1)` is false, otherwise `h` is `0`, `i` is 'S', `rr` is a list `[0, 0, 0, 0]`, `hh` is a list `[0, 0, 0, 0]`, `pp` is `['R']` if `(ss % 2 == 1)` is true, otherwise `pp` is `['H']`.**