Let's break down the problem step by step:

1. **Identify the Loop Head Variables**: The loop head variables are `i` and `b`.

2. **Current States at the End of the Previous Iteration**:
   - `b` is greater than or equal to 5.
   - `i` is 5.
   - `x` is 2.
   - `suma` is increased by 3.
   - The condition `((a - i * (i - 1)) % i ** 2 == 0 and i * (i - 1) % i ** 2 == 0)` holds true.

3. **Determine the Next State**:
   - The loop condition is `for i in range(1, b + 1)`.
   - At the end of the previous iteration, `i` is 5.
   - For the loop to continue, `i` must be less than `b + 1`.
   - Since `i` is currently 5, `b` must be greater than 5 for the loop to execute one more time.
   - After the loop increments `i` by 1, `i` will become 6.

4. **Adjust the States**:
   - `i` will be incremented to 6.
   - `b` must remain greater than 5 for the loop to continue.

Given these points, the states that need to be adjusted are `i` and `b`.

**Final Answer**:
State: **`b` is greater than 5, `i` is 6, `x` is 2, `suma` is increased by 3, and the condition `((a - i * (i - 1)) % i ** 2 == 0 and i * (i - 1) % i ** 2 == 0)` holds true.**