To determine what will be printed by the `print(result)` statement, let's break down the precondition and the formula step by step:

1. **Initial State**:
   - `p_1`, `p_2`, and `p_3` are integers where \(0 \leq p_1 \leq p_2 \leq p_3 \leq 30\).
   - `t` must be greater than 0.
   - `v` is a list of integers input by the user.
   - The sum of the first three elements of `v` is even.

2. **Formula for `result`**:
   - `result` is calculated as \((v[0] + v[1] + v[2] - \max(0, v[2] - v[0] - v[1])) // 2\).

Let's analyze the formula:

- **Sum of the first three elements**: \(v[0] + v[1] + v[2]\) is even.
- **Max function**: \(\max(0, v[2] - v[0] - v[1])\):
  - If \(v[2] - v[0] - v[1] \geq 0\), then \(\max(0, v[2] - v[0] - v[1]) = v[2] - v[0] - v[1]\).
  - If \(v[2] - v[0] - v[1] < 0\), then \(\max(0, v[2] - v[0] - v[1]) = 0\).

3. **Calculating `result`**:
   - If \(v[2] - v[0] - v[1] \geq 0\):
     \[
     \text{result} = \left(v[0] + v[1] + v[2] - (v[2] - v[0] - v[1])\right) // 2
     \]
     Simplifying inside the parentheses:
     \[
     \text{result} = \left(v[0] + v[1] + v[2] - v[2] + v[0] + v[1]\right) // 2 = (2 \cdot v[0] + 2 \cdot v[1]) // 2 = v[0] + v[1]
     \]
   - If \(v[2] - v[0] - v[1] < 0\):
     \[
     \text{result} = \left(v[0] + v[1] + v[2] - 0\right) // 2 = (v[0] + v[1] + v[2]) // 2
     \]

Since the sum \(v[0] + v[1] + v[2]\) is even, \((v[0] + v[1] + v[2]) // 2\) will be an integer.

4. **Conclusion**:
   - If \(v[2] \geq v[0] + v[1]\), the result will be \(v[0] + v[1]\).
   - If \(v[2] < v[0] + v[1]\), the result will be \((v[0] + v[1] + v[2]) // 2\).

Given the precondition, the `print(result)` statement will print one of these two values, depending on the relationship between \(v[2]\) and \(v[0] + v[1]\).

Output: **result (where result is \(v[0] + v[1]\) if \(v[2] \geq v[0] + v[1]\), otherwise result is \((v[0] + v[1] + v[2]) // 2\))**