To determine what will be printed by the `print(p1 - cur + p3)` statement, we need to carefully analyze the given initial state and deduce the values of `p1`, `p2`, `p3`, `cur`, `low`, and `high`.

### Initial State Recap:
- `t` is an integer greater than or equal to 1.
- `p1`, `p2`, and `p3` are integers such that \(0 \leq p1 \leq p2 \leq p3 \leq 30\).
- The sum of `p1`, `p2`, and `p3` is odd.
- `p3` is less than the sum of `p1` and `p2`.
- `low` is `p3 - p2`.
- `high` is `p3 - p1` and `high` must be at least `cur`.
- If `p1 - cur` is less than or equal to `p2 - (p3 - cur)`, `cur` remains `low`. Otherwise, `cur` is `low + 1` and `p1 - cur` is greater than `p2 - (p3 - cur)`.

### Step-by-Step Analysis:
1. **Determine `low` and `high`:**
   - `low = p3 - p2`
   - `high = p3 - p1`
   
2. **Determine `cur`:**
   - If `p1 - cur <= p2 - (p3 - cur)`, then `cur = low`.
   - Otherwise, `cur = low + 1`.
   
3. **Simplify the condition for `cur`:**
   - The condition `p1 - cur <= p2 - (p3 - cur)` simplifies to `p1 - cur <= p2 - p3 + cur`, which further simplifies to `p1 + p3 <= p2 + 2*cur`.
   - Thus, if `p1 + p3 <= p2 + 2*low`, then `cur = low`.
   - Otherwise, `cur = low + 1`.

4. **Calculate `p1 - cur + p3`:**
   - If `cur = low`, then `p1 - cur + p3 = p1 - (p3 - p2) + p3 = p1 + p2`.
   - If `cur = low + 1`, then `p1 - cur + p3 = p1 - (p3 - p2 + 1) + p3 = p1 + p2 - 1`.

### Conclusion:
The exact value of `p1 - cur + p3` depends on whether `cur` is `low` or `low + 1`. However, based on the conditions provided, we can describe the possible outcomes:

- If `p1 + p3 <= p2 + 2*low`, then `cur = low` and the output is `p1 + p2`.
- Otherwise, `cur = low + 1` and the output is `p1 + p2 - 1`.

Since the exact values of `p1`, `p2`, and `p3` are not provided, we must describe the output in terms of these variables.

Output: **p1 + p2 - 1 or p1 + p2 (depending on whether p1 + p3 <= p2 + 2*(p3 - p2))**