Let's carefully analyze the given initial state and the print statement to determine what will be printed.

### Initial State Recap:
1. `t` is an integer greater than or equal to 2.
2. `p1`, `p2`, and `p3` are integers such that \(0 \leq p1 \leq p2 \leq p3 \leq 30\).
3. The sum of `p1`, `p2`, and `p3` is odd.
4. `low` is the minimum of `p3 - p1` and `p3 - p2`.
5. `high` is the maximum of `p3 - p1` and `p3 - p2`.
6. `cur` is set to `low`.
7. The condition `p1 - cur <= p2 - (p3 - cur)` is true.

### Analysis:
Given the constraints and conditions, let's determine the value of `p1 - cur + p3`.

- Since `cur` is set to `low`, and `low` is the minimum of `p3 - p1` and `p3 - p2`, `cur` is either `p3 - p1` or `p3 - p2`, whichever is smaller.
- Given the condition `p1 - cur <= p2 - (p3 - cur)`, we can substitute `cur` with `low` and analyze the inequality.
- Since `cur` is `low`, and `low` is the minimum difference between `p3` and `p1` or `p3` and `p2`, the inequality `p1 - cur <= p2 - (p3 - cur)` holds true.

### Print Statement:
The print statement is `print(p1 - cur + p3)`.

- `cur` is `low`, which is either `p3 - p1` or `p3 - p2`.
- We need to consider both possibilities for `cur`.

#### Case 1: `cur = p3 - p1`
- `p1 - cur + p3` becomes `p1 - (p3 - p1) + p3` which simplifies to `p1 - p3 + p1 + p3` which further simplifies to `2 * p1`.

#### Case 2: `cur = p3 - p2`
- `p1 - cur + p3` becomes `p1 - (p3 - p2) + p3` which simplifies to `p1 - p3 + p2 + p3` which further simplifies to `p1 + p2`.

However, since `cur` is the minimum of `p3 - p1` and `p3 - p2`, and the condition `p1 - cur <= p2 - (p3 - cur)` is true, the expression `p1 - cur + p3` simplifies to `p1 + p2` in the valid case.

### Conclusion:
Given the constraints and the condition, the expression `p1 - cur + p3` simplifies to `p1 + p2`.

Output: **p1 + p2 (where p1 and p2 are integers such that 0 ≤ p1 ≤ p2 ≤ p3 ≤ 30 and the sum of p1, p2, and p3 is odd)**