The code updates `pref[i]` by adding `pref[i - 1]` to it. Given that `i` is 3, the code becomes `pref[3] += pref[2]`. The initial values are `pref[0]` is unchanged, `pref[1]` is `pref[0]`, and `pref[2]` is `2 * pref[0]`.

Since `pref[2]` is `2 * pref[0]`, and `pref[1]` is `pref[0]`, let's assume `pref[0] = x`. Then, `pref[1] = x` and `pref[2] = 2 * x`. So, `pref[3]` becomes `pref[2] + pref[2] = 2 * (2 * x) = 4 * x`.

Output State: **`i` is 3, `n` must be greater than 1, `pref[0]` is unchanged, `pref[1]` is `pref[0]`, `pref[2]` is `2 * pref[0]`, `pref[3]` is `4 * pref[0]`**