Reasoning: 

The original assessment is accurate, but let's break down the reasoning step-by-step to ensure clarity and correctness.

1. **Problem Description Analysis**:
   - We need to find the difference between the sum of cubes of the first `n` natural numbers and the sum of the first `n` natural numbers.
   - Mathematically, this can be expressed as:
     \[
     \text{Difference} = \left(\sum_{i=1}^{n} i^3\right) - \left(\sum_{i=1}^{n} i\right)
     \]

2. **Mathematical Formulas**:
   - The sum of the first `n` natural numbers is given by:
     \[
     \text{sum}_n = \frac{n(n + 1)}{2}
     \]
   - The sum of the cubes of the first `n` natural numbers is given by:
     \[
     \text{sum\_cubes}_n = \left(\frac{n(n + 1)}{2}\right)^2
     \]

3. **Function Implementation**:
   - The function `func_1(n)` calculates:
     \[
     \text{sum}_n = \frac{n(n + 1)}{2}
     \]
     \[
     \text{sum\_cubes}_n = \left(\frac{n(n + 1)}{2}\right)^2
     \]
   - It then returns the difference:
     \[
     \text{Difference} = \text{sum\_cubes}_n - \text{sum}_n
     \]

4. **Test Cases**:
   - For `n = 3`:
     \[
     \text{sum}_3 = \frac{3(3 + 1)}{2} = 6
     \]
     \[
     \text{sum\_cubes}_3 = 6^2 = 36
     \]
     \[
     \text{Difference} = 36 - 6 = 30
     \]
   - For `n = 5`:
     \[
     \text{sum}_5 = \frac{5(5 + 1)}{2} = 15
     \]
     \[
     \text{sum\_cubes}_5 = 15^2 = 225
     \]
     \[
     \text{Difference} = 225 - 15 = 210
     \]
   - For `n = 2`:
     \[
     \text{sum}_2 = \frac{2(2 + 1)}{2} = 3
     \]
     \[
     \text{sum\_cubes}_2 = 3^2 = 9
     \]
     \[
     \text{Difference} = 9 - 3 = 6
     \]

5. **Function Summary**:
   - The function summary correctly states that the function `func_1` accepts a non-negative integer `n` and returns the value \( \text{sum\_cubes}_n - \text{sum}_n \).

Given the above analysis, the function `func_1` is indeed correct and matches the problem description. The test cases provided further verify the correctness of the implementation.

Final: **True**