The given code snippet modifies the value of `c` by adding `l[i] * s - s * s / 2` to its current value. Let's determine the new value of `c` based on the initial state.

Initial State:
- `t` is an integer such that 1 ≤ t ≤ 10^4
- `n` must be greater than 1
- `m` is the second integer from the input
- `k` is `k - 2 * min(m, k)`
- `l` is a sorted list of integers read from the input
- `s` is `min(m, k)`
- `c` is `k * k / 2 + (l[0] + l[i]) * s - s * s`
- `i` is 2

The code snippet:
```python
c += l[i] * s - s * s / 2
```

This means the new value of `c` will be:
\[ c_{\text{new}} = c + l[i] * s - \frac{s * s}{2} \]

Substituting the initial value of `c` into the equation:
\[ c_{\text{new}} = \left(k * \frac{k}{2} + (l[0] + l[i]) * s - s * s\right) + l[i] * s - \frac{s * s}{2} \]
\[ c_{\text{new}} = k * \frac{k}{2} + (l[0] + l[i]) * s - s * s + l[i] * s - \frac{s * s}{2} \]
\[ c_{\text{new}} = k * \frac{k}{2} + (l[0] + l[i] + l[i]) * s - s * s - \frac{s * s}{2} \]
\[ c_{\text{new}} = k * \frac{k}{2} + (l[0] + 2 * l[i]) * s - \frac{2 * s * s}{2} - \frac{s * s}{2} \]
\[ c_{\text{new}} = k * \frac{k}{2} + (l[0] + 2 * l[i]) * s - \frac{3 * s * s}{2} \]

Therefore, the updated value of `c` is:
\[ c_{\text{new}} = k * \frac{k}{2} + (l[0] + 2 * l[i]) * s - \frac{3 * s * s}{2} \]

The other variables remain unchanged.

Output State: **`t` is an integer such that 1 ≤ t ≤ 10^4, `n` must be greater than 1, `m` is the second integer from the input, `k` is `k - 2 * min(m, k)`, `l` is a sorted list of integers read from the input, `s` is `min(m, k)`, `c` is `k * k / 2 + (l[0] + 2 * l[i]) * s - 3 * s * s / 2`, `i` is 2**