Let's break down the given initial state and the code snippet to determine what will be printed.

### Initial State:
1. `t` is at least 1.
2. `p1`, `p2`, and `p3` are integers such that:
   - \(0 \leq p1 \leq p2 \leq p3 \leq 30\)
   - The sum \(p1 + p2 + p3\) is odd.
   - \(p3\) is less than \(p1 + p2\).
3. `x` is 0.
4. `y` is equal to `p3`.
5. It holds that \(p1 - x \leq p2 - y\).

### Code Snippet:
```python
print(p1 - x + p3)
```

### Analysis:
- Given `x = 0`, the expression `p1 - x` simplifies to `p1`.
- Therefore, the expression `p1 - x + p3` simplifies to `p1 + p3`.

### Output:
The print statement will output the value of `p1 + p3`.

### Final Answer:
Output: **p1 + p3 (where p1 and p3 are integers such that 0 ≤ p1 ≤ p3 ≤ 30, p1 + p2 + p3 is odd, and p3 < p1 + p2)**