To determine what will be printed by the statement `print(p1 - x + p3)`, we need to analyze the given initial state and the conditions provided.

### Initial State and Conditions:
1. **t** is at least 1 (though `t` is not used in the print statement, it's part of the initial state).
2. **p1**, **p2**, and **p3** are integers such that:
   - \(0 \leq p1 \leq p2 \leq p3 \leq 30\)
   - The sum of \(p1\), \(p2\), and \(p3\) is odd.
   - \(p3\) is less than \(p1 + p2\).
3. The values of **x** and **y** are determined by the condition:
   - If \(p1 - x \leq p2 - y\), then \(x\) remains 0 and \(y\) remains \(p3\).
   - Otherwise, \(x\) is set to 1 and \(y\) is set to \(p3 - 1\).

### Analysis:
The print statement is `print(p1 - x + p3)`. We need to determine the values of **x** and how they affect the output.

#### Determining **x**:
- The value of \(x\) is dependent on the condition \(p1 - x \leq p2 - y\).
- Since \(y\) is always \(p3\) or \(p3 - 1\), we need to consider both scenarios:
  - If \(x = 0\), then the condition becomes \(p1 \leq p2 - y\).
  - If \(x = 1\), then the condition becomes \(p1 - 1 \leq p2 - y\).

Given the constraints \(0 \leq p1 \leq p2 \leq p3 \leq 30\) and \(p3 < p1 + p2\), the condition \(p1 \leq p2 - y\) (when \(x = 0\)) will often hold true because \(y\) is either \(p3\) or \(p3 - 1\), and \(p3 < p1 + p2\) implies \(p2 > p3 - p1\).

However, if \(p1 - 1 \leq p2 - y\) (when \(x = 1\)) does not hold, then \(x\) will be set to 1.

### Calculating the Output:
- If \(x = 0\), the expression becomes \(p1 + p3\).
- If \(x = 1\), the expression becomes \(p1 + p3 - 1\).

Since the exact values of \(p1\), \(p2\), and \(p3\) are not provided, we need to consider both possibilities based on the conditions.

### Conclusion:
The output will be either \(p1 + p3\) or \(p1 + p3 - 1\) depending on whether \(x\) is 0 or 1.

Output: **p1 + p3 - x (where x is 0 if p1 <= p2 - y, otherwise x is 1)**