To determine what will be printed by the `print(p1 - x + p3)` statement, we need to carefully analyze the given initial state and conditions.

1. **Initial State and Conditions:**
   - `t` is at least 0 (though `t` is not used in the given code snippet).
   - `p1`, `p2`, and `p3` are integers such that \(0 \leq p1 \leq p2 \leq p3 \leq 30\).
   - The sum of `p1`, `p2`, and `p3` is odd.
   - If `p3` is greater than or equal to the sum of `p1` and `p2`, `p3` remains unchanged. Otherwise, `p3` retains its original value.
   - If `p1 - x <= p2 - y`, then `x` is 0 and `y` is equal to `p3`. Otherwise, `x` is 1 and `y` is equal to `p3 - 1`.

2. **Determine `x` and `y`:**
   - The condition `p1 - x <= p2 - y` needs to be evaluated to determine the values of `x` and `y`.
   - If `p1 - x <= p2 - y` is true, then `x = 0` and `y = p3`.
   - If `p1 - x <= p2 - y` is false, then `x = 1` and `y = p3 - 1`.

3. **Evaluate the Expression `p1 - x + p3`:**
   - If `x = 0`, then `p1 - x + p3` simplifies to `p1 + p3`.
   - If `x = 1`, then `p1 - x + p3` simplifies to `p1 - 1 + p3`.

To determine which of these two cases applies, we need to consider the condition `p1 - x <= p2 - y`:

- If `x = 0` and `y = p3`, the condition becomes `p1 <= p2 - p3`. This is unlikely given the constraints \(0 \leq p1 \leq p2 \leq p3\).
- If `x = 1` and `y = p3 - 1`, the condition becomes `p1 - 1 <= p2 - (p3 - 1)`, which simplifies to `p1 - 1 <= p2 - p3 + 1` or `p1 <= p2 - p3 + 2`. Given the constraints and the fact that `p1`, `p2`, and `p3` are integers, this condition is more likely to hold true.

Therefore, `x` is likely to be 1 and `y` is likely to be `p3 - 1`. This means the expression `p1 - x + p3` simplifies to `p1 - 1 + p3`.

**Final Output:**
Output: **p1 - 1 + p3 (where p1 and p3 are integers such that 0 ≤ p1 ≤ p2 ≤ p3 ≤ 30 and the sum of p1, p2, and p3 is odd)**