Based on the initial state provided:

- `t` is an integer within the range 1 to 500.
- `_` is 3.
- `p1`, `p2`, `p3` are integers with the sum of `p1`, `p2`, and `p3` being even.
- `p3` is less than or equal to `p1 + p2`.
- `p3` is at least 3.
- `x` is 0.
- The current value of `y` is `p3`.
- `p1 - x` is less than or equal to `p2 - y`.

We need to determine the value of `p1 - x + p3` when the print statement is executed.

Given:
- `x = 0`
- `y = p3`

So, the expression simplifies to:
\[ p1 - 0 + p3 = p1 + p3 \]

From the conditions:
- `p1 + p2 + p3` is even.
- `p3` is at least 3.
- `p3` is less than or equal to `p1 + p2`.

Since `p1 + p3` must contribute to making the total sum even, and `p3` is at least 3, let's consider the simplest case where `p1` and `p2` are chosen such that `p1 + p2 + p3` is even. For example, if `p1 = 2` and `p2 = 2`, then `p3` could be 2 (since 2 + 2 + 2 = 6, which is even).

Thus, in this case:
- `p1 = 2`
- `p3 = 2`

Therefore:
\[ p1 + p3 = 2 + 2 = 4 \]

Output: **4**