Alright, I've got this problem to solve. Let's see what it's asking for. So, Anton has a permutation of size n, and he wants to find a number x using a binary search-like algorithm. But here's the twist: the array isn't sorted, and I can perform at most two swaps on the permutation before running this binary search. The goal is to rearrange the array in such a way that after performing the modified binary search, the value at position l equals x.

First, I need to understand what a permutation is. A permutation of size n is just an array containing each number from 1 to n exactly once, but in any order. So, for n=3, possible permutations are [1,2,3], [1,3,2], [2,1,3], etc.

Now, the binary search algorithm described here is a bit unusual. Normally, binary search requires a sorted array, but here, it's being applied to a potentially unsorted permutation. The steps are:

1. Initialize l = 0 and r = n.

2. While r - l > 1:

a. Calculate m = floor((r + l) / 2).

b. If p[m] <= x, set l = m.

c. Otherwise, set r = m.

After this loop, p[l] should equal x.

Wait a second, this is not a standard binary search. Normally, binary search on a sorted array would compare p[m] to x and adjust l and r accordingly until l <= r, and then check if p[m] == x.

Here, the condition is different: if p[m] <= x, set l = m; else set r = m. Also, the loop condition is r - l == 1, which is different from standard binary search.

I need to understand how this algorithm works on a permutation that isn't necessarily sorted.

Let me try to see what this algorithm is doing.

Suppose we have n=6, x=3, and the array is [1,2,3,4,5,6]. According to the example, no swaps are needed, so the output should be 0.

Let's simulate the algorithm:

- l = 0, r = 6

- While 6 - 0 > 1:

- m = floor((0 + 6)/2) = 3

- p[3] = 4, which is greater than 3, so r = 3

- Now l = 0, r = 3

- m = floor((0 + 3)/2) = 1

- p[1] = 2, which is less than or equal to 3, so l = 1

- Now l = 1, r = 3

- m = floor((1 + 3)/2) = 2

- p[2] = 3, which is equal to 3, so l = 2

- Now l = 2, r = 3

- m = floor((2 + 3)/2) = 2

- p[2] = 3, which is equal to 3, so l = 2

- Now l = 2, r = 3

- m = floor((2 + 3)/2) = 2

- p[2] = 3, which is equal to 3, so l = 2

- The loop continues until r - l == 1, which it already is (3 - 2 = 1), so it ends.

At the end, p[l] = p[2] = 3, which equals x=3. So, it works without any swaps.

Another example: n=6, x=5, array=[3,1,6,5,2,4]

Let's see what the output is: 1 swap, swapping positions 3 and 4.

So, original array: [3,1,6,5,2,4]

After swapping positions 3 and 4 (assuming 1-based indexing), the array becomes [3,1,5,6,2,4]

Let's simulate the algorithm:

- l = 0, r = 6

- m = floor((0 + 6)/2) = 3

- p[3] = 5, which is equal to 5, so l = 3

- Now l = 3, r = 6

- m = floor((3 + 6)/2) = 4

- p[4] = 6, which is greater than 5, so r = 4

- Now l = 3, r = 4

- m = floor((3 + 4)/2) = 3

- p[3] = 5, which is equal to 5, so l = 3

- Now l = 3, r = 4

- m = floor((3 + 4)/2) = 3

- p[3] = 5, which is equal to 5, so l = 3

- The loop ends, p[l] = 5, which equals x=5.

So, with one swap, we achieved the goal.

Another example: n=5, x=1, array=[3,5,4,2,1]

Output: 2 swaps.

First swap: 2 4 -> swap positions 2 and 4 (1-based: p[2]=5 and p[4]=2)

After first swap: [3,2,4,5,1]

Second swap: 1 5 -> swap positions 1 and 5 (1-based: p[1]=3 and p[5]=1)

After second swap: [1,2,4,5,3]

Now, simulate the algorithm:

- l = 0, r = 5

- m = floor((0 + 5)/2) = 2

- p[2] = 2, which is less than or equal to 1, so l = 2

- Now l = 2, r = 5

- m = floor((2 + 5)/2) = 3

- p[3] = 4, which is greater than 1, so r = 3

- Now l = 2, r = 3

- m = floor((2 + 3)/2) = 2

- p[2] = 2, which is greater than 1, so r = 2

- Now l = 2, r = 2

- m = floor((2 + 2)/2) = 2

- p[2] = 2, which is greater than 1, so r = 2

- The loop ends, p[l] = p[2] = 2, which is not equal to x=1.

Wait, this seems incorrect. The example output shows two swaps, but after performing them, p[l] = 2, which is not equal to x=1.

Hmm, maybe I did something wrong.

Wait, perhaps I misinterpreted the swap indices. Let's see:

Original array: [3,5,4,2,1]

First swap: 2 4 -> swap positions 2 and 4: p[2]=5 and p[4]=2 -> [3,2,4,5,1]

Second swap: 1 5 -> swap positions 1 and 5: p[1]=3 and p[5]=1 -> [1,2,4,5,3]

Now, simulate the algorithm:

- l = 0, r = 5

- m = floor((0 + 5)/2) = 2

- p[2] = 4, which is greater than 1, so r = 2

- Now l = 0, r = 2

- m = floor((0 + 2)/2) = 1

- p[1] = 2, which is greater than 1, so r = 1

- Now l = 0, r = 1

- m = floor((0 + 1)/2) = 0

- p[0] = 1, which is equal to 1, so l = 0

- Now l = 0, r = 1

- m = floor((0 + 1)/2) = 0

- p[0] = 1, which is equal to 1, so l = 0

- The loop ends, p[l] = p[0] = 1, which equals x=1.

Okay, so it works with two swaps.

So, the strategy seems to be: perform swaps to position x in such a way that the binary search algorithm lands on x.

But this is tricky because the binary search algorithm here isn't a standard one; it's tailored to this specific problem.

I need to understand how this binary search works.

Let me try to see what this binary search is doing.

In standard binary search on a sorted array, we have l and r as bounds, and we repeatedly halve the search space based on comparisons with the target x.

Here, the loop continues until r - l == 1, and in each step, it sets m = floor((l + r)/2), then if p[m] <= x, set l = m, else set r = m.

This seems like it's trying to find the largest index where p[m] <= x.

Wait, it's similar to finding the upper bound in standard binary search.

In standard binary search, to find the smallest element >= x, we can adjust the conditions accordingly.

But here, it's seems to be finding the smallest m where p[m] > x, and then l would be m - 1, assuming p[m - 1] <= x.

But in this problem, after the loop, p[l] should be equal to x.

So, perhaps the goal is to position x such that it's the largest element <= x.

Wait, but if p[l] == x, that means x is present in the array at position l.

Given that it's a permutation, x is guaranteed to be present exactly once.

So, the task is to rearrange the array with at most two swaps so that after the given binary search algorithm, p[l] == x.

Moreover, it's guaranteed that two swaps are always sufficient.

I need to find a way to perform at most two swaps to achieve this condition.

Let me think about how the binary search algorithm behaves.

Let's consider the initial and final positions of x, and see how swaps can adjust its position to satisfy the condition.

Let me denote pos_x as the current position of x in the array.

Let me also denote target_pos as the position where the binary search would stop, such that p[l] == x.

I need to move x to target_pos with at most two swaps.

But I need to determine what target_pos should be for p[l] to equal x after the binary search.

This is confusing because the binary search depends on the array's values, which can be arbitrary since it's a permutation.

Perhaps I need to consider where x should be placed so that the binary search converges to it.

Let me consider that the binary search is trying to find the insertion point for x in a sorted array, but since the array isn't sorted, I need to manipulate its positions.

Wait, perhaps I can think of it as placing x in a position where, according to the binary search's logic, it would be selected as p[l].

But this is still vague.

Let me consider that after the binary search, l points to x.

I need to ensure that after the search, p[l] == x.

Given that, I need to position x such that the search process leads to l being the index of x.

But the search process is dependent on the values at the indices chosen during the search.

This seems recursive and complex.

Maybe I should look for a different approach.

Let me consider that the binary search is effectively dividing the array into halves and choosing a half based on the comparison of p[m] and x.

Given that the array is a permutation, all elements are unique.

I need to ensure that the search process, with its specific rules, leads to p[l] == x.

Perhaps I can consider the binary tree structure implied by the binary search and ensure that x is placed in a position that aligns with the search's decisions.

But this seems overly complicated.

Let me consider a simpler strategy.

Since I can perform up to two swaps, I can try to bring x to a position where the binary search will select it.

One idea is to swap x directly to the position where the search would stop.

But to do that, I need to know where the search would stop if x were in a certain position.

Alternatively, perhaps I can adjust the array so that x is in a position that satisfies p[l] == x after the search.

Wait, perhaps I can ensure that x is the only element that satisfies the condition at the end of the search.

This is still too vague.

Let me consider specific cases.

Take the first example:

n=6, x=3, array=[1,2,3,4,5,6]

No swaps needed because the array is already sorted, and the search correctly identifies p[2] == 3.

Second example:

n=6, x=5, array=[3,1,6,5,2,4]

After swapping positions 3 and 4 (1-based: 6 and 5), the array becomes [3,1,5,6,2,4]

Search:

- l=0, r=6

- m=3, p[3]=5 <=5, so l=3

- m=3, p[3]=5 <=5, so l=3

- m=3, p[3]=5 <=5, so l=3

- r - l = 3, which is >1, but since m is the same, it's stuck.

Wait, in this case, l=3, r=6, m=4, p[4]=6 >5, so r=4

Then l=3, r=4, m=3, p[3]=5 <=5, so l=3

Now r - l =1, so loop ends.

p[l] = p[3] =5 ==x=5.

Okay, it works.

Third example:

n=5, x=1, array=[3,5,4,2,1]

After two swaps:

First swap 2 and 4: [3,2,4,5,1]

Second swap 1 and 5: [1,2,4,5,3]

Search:

- l=0, r=5

- m=2, p[2]=4 >1, so r=2

- m=1, p[1]=2 >1, so r=1

- m=0, p[0]=1 <=1, so l=0

- m=0, p[0]=1 <=1, so l=0

- r - l =1, loop ends.

p[l] = p[0] =1 ==x=1.

Good.

Another example:

n=6, x=3, array=[4,3,1,5,2,6]

Output: two swaps.

After swaps:

First swap 2 and 4: [4,5,1,3,2,6]

Second swap 1 and 5: [2,5,1,3,4,6]

Search:

- l=0, r=6

- m=3, p[3]=3 <=3, so l=3

- m=3, p[3]=3 <=3, so l=3

- m=3, p[3]=3 <=3, so l=3

- r - l =3, which is >1, but m is same.

Wait, l=3, r=6, m=4, p[4]=4 >3, so r=4

Now l=3, r=4, m=3, p[3]=3 <=3, so l=3

Now r - l =1, loop ends.

p[l] = p[3] =3 ==x=3.

Good.

Last example:

n=3, x=2, array=[3,2,1]

One swap: 1 and 3 -> [1,2,3]

Search:

- l=0, r=4

Wait, n=3, so r=4?

Wait, n=3, so r=3.

- l=0, r=3

- m=1, p[1]=2 <=2, so l=1

- m=1, p[1]=2 <=2, so l=1

- r - l =2, so m=1, p[1]=2 <=2, so l=1

- r - l =2, so m=1, p[1]=2 <=2, so l=1

- r - l =1, loop ends.

p[l] = p[1] =2 ==x=2.

Good.

So, in all examples, the strategy seems to work.

But I need to generalize this.

Looking at the solutions, it seems that in many cases, swapping x to its correct position in a sorted array is sufficient, or performing swaps to make the array sorted.

But the problem allows the array to be rearranged in any way, not necessarily sorted, as long as after at most two swaps, the binary search ends with p[l] == x.

Moreover, it's guaranteed that two swaps are always sufficient.

So, I need to find a way to rearrange the array with at most two swaps so that the binary search's l ends on x.

I need a systematic way to determine which swaps to make.

Let me consider the following approach:

1. Perform the binary search as described and see where it stops.

2. If p[l] == x, then no swaps are needed.

3. If p[l] != x, then find a way to swap elements so that x is moved to the position where the search stops.

But this requires understanding where the search stops.

Alternatively, perhaps I can think about the binary search's behavior and determine the final l based on the initial array.

But since the array is not sorted, predicting where l will be is tricky.

Wait, perhaps I can simulate the binary search to find where l ends up, and then swap x to that position.

If x is already at that position, then no swaps are needed.

If x is not at that position, then I can swap x with the element at the target position.

But if the target position already has the correct value, then no swap is needed.

Wait, perhaps I need to swap x to the position where l ends up.

Let me try this approach.

First, run the binary search to find the final l.

Then, if p[l] != x, swap x's current position with the target position l.

This would be one swap.

But perhaps in some cases, one swap isn't enough, and I need to perform a second swap.

Wait, let's think about it.

Suppose after running the binary search, l points to some position, say pos_l.

If p[pos_l] == x, then no swaps are needed.

If p[pos_l] != x, then I can swap x's current position with pos_l.

After this swap, p[pos_l] == x, and x is now at pos_l.

So, one swap is sufficient.

But in some cases, maybe x is not directly swappable in one step, and I need to perform two swaps.

Wait, in the examples, sometimes one swap is enough, sometimes two are needed.

So, perhaps in the general case, one swap might not be sufficient, and I need to perform two swaps to position x correctly.

But I need to confirm this.

Let me consider a case where one swap isn't enough.

Suppose n=4, x=3, array=[1,4,2,3]

Run the binary search:

- l=0, r=4

- m=2, p[2]=2 <=3, so l=2

- m=3, p[3]=3 <=3, so l=3

- m=3, p[3]=3 <=3, so l=3

- r - l =1, loop ends.

p[l] = p[3] =3 ==x=3.

So, no swaps needed.

Another case: n=4, x=2, array=[1,3,4,2]

Run the binary search:

- l=0, r=4

- m=2, p[2]=4 >2, so r=2

- m=1, p[1]=3 >2, so r=1

- m=0, p[0]=1 <=2, so l=0

- m=0, p[0]=1 <=2, so l=0

- r - l =1, loop ends.

p[l] = p[0] =1 !=2.

So, need to swap x=2 to position 0.

Current position of x=2 is 3.

Swap positions 0 and 3: [2,3,4,1]

Now, run the binary search:

- l=0, r=4

- m=2, p[2]=4 >2, so r=2

- m=1, p[1]=3 >2, so r=1

- m=0, p[0]=2 <=2, so l=0

- m=0, p[0]=2 <=2, so l=0

- r - l =1, loop ends.

p[l] = p[0] =2 ==x=2.

So, one swap suffices.

But let's consider another case.

n=5, x=3, array=[5,1,2,4,3]

Run the binary search:

- l=0, r=5

- m=2, p[2]=2 <=3, so l=2

- m=3, p[3]=4 >3, so r=3

- m=2, p[2]=2 <=3, so l=2

- m=2, p[2]=2 <=3, so l=2

- r - l =1, loop ends.

p[l] = p[2] =2 !=3.

So, need to swap x=3 to position 2.

Current position of x=3 is 4.

Swap positions 2 and 4: [5,1,3,4,2]

Now, run the binary search:

- l=0, r=5

- m=2, p[2]=3 <=3, so l=2

- m=3, p[3]=4 >3, so r=3

- m=2, p[2]=3 <=3, so l=2

- m=2, p[2]=3 <=3, so l=2

- r - l =1, loop ends.

p[l] = p[2] =3 ==x=3.

So, again, one swap suffices.

But according to the problem, two swaps are always sufficient, but it seems one swap often suffices.

Perhaps in some cases, one swap isn