Given the initial conditions, let's analyze the code step by step:

### Initial State:
- `n` is an even integer such that \(2 \leq n \leq 10^9\)
- `m` is an integer such that \(2 \leq m \leq 10^9\)
- `k` is an integer such that \(0 \leq k < n \times 2 - 2\)
- The current value of `k` is greater than or equal to \(n - 1\)
- The current value of `k` is less than \(n \times 2 - 2\)

### Code:
```python
print(n - (k - n + 1) % (n - 1) - 1, (k - n + 1) // (n - 1) + 1)
```

### Step-by-Step Analysis:
1. **Calculate the first part of the print statement:**
   - \( \text{expression} = n - (k - n + 1) \% (n - 1) - 1 \)
   - Let's break down the inner expression:
     - \( k - n + 1 \) is an integer.
     - \( (k - n + 1) \% (n - 1) \) gives the remainder when \( k - n + 1 \) is divided by \( n - 1 \).
   - Since \( k \geq n - 1 \), \( k - n + 1 \geq 0 \).
   - The remainder when \( k - n + 1 \) is divided by \( n - 1 \) will be between 0 and \( n - 2 \).

2. **Calculate the second part of the print statement:**
   - \( \text{expression} = (k - n + 1) // (n - 1) + 1 \)
   - \( (k - n + 1) // (n - 1) \) gives the quotient when \( k - n + 1 \) is divided by \( n - 1 \).
   - Since \( k < n \times 2 - 2 \), \( k - n + 1 < n - 1 \), so the quotient will be 0 or 1.

### Specific Values:
- Given \( k \geq n - 1 \) and \( k < n \times 2 - 2 \):
  - \( k - n + 1 \) ranges from 0 to \( n - 2 \).
  - The remainder \( (k - n + 1) \% (n - 1) \) will be \( k - n + 1 \) itself because \( k - n + 1 \) is less than \( n - 1 \).
  - The quotient \( (k - n + 1) // (n - 1) \) will be 0.

### Final Calculation:
- First part: \( n - (k - n + 1) - 1 \)
- Second part: \( (k - n + 1) // (n - 1) + 1 = 0 + 1 = 1 \)

### Output:
- The first part simplifies to: \( n - (k - n + 1) - 1 = n - k + n - 1 - 1 = 2n - k - 2 \)
- The second part is: 1

### Output State:
- The values of `n`, `m`, and `k` remain unchanged.
- The print statement outputs the values calculated.

Output State: **`n` is an even integer such that \(2 \leq n \leq 10^9\), `m` is an integer such that \(2 \leq m \leq 10^9\), `k` is an integer such that \(0 \leq k < n \times 2 - 2\) and the current value of `k` is greater than or equal to \(n - 1\) and less than \(n \times 2 - 2\). The print statement outputs \((2n - k - 2, 1)\)**.