Alright, I've got this problem to solve. Let's see what it's asking for. So, Rudolf has an array of integers, and he can perform a specific operation on it any number of times. The operation involves choosing an index i (where 2 ≤ i ≤ n-1) and modifying the elements at positions i-1, i, and i+1 by subtracting 1, 2, and 1 respectively. The goal is to determine whether it's possible to make all elements of the array zero by applying this operation any number of times.

First, I need to understand the operation clearly. So, for any chosen i (between 2 and n-1), I can subtract 1 from a[i-1], subtract 2 from a[i], and subtract 1 from a[i+1]. This operation can be applied any number of times, and I can choose different i's in different operations.

I need to find out if, after some sequence of these operations, all elements of the array become zero.

Let me think about what this operation does to the array. It seems like it's designed to reduce the values in a specific pattern. Maybe I can model this operation in terms of linear algebra or find some invariant that can help me determine the possibility.

One approach is to see if the system of equations derived from the operations has a solution that makes all elements zero.

Let me denote the number of times operation is applied at position i as x_i. Then, for each position in the array, the total subtraction due to all operations should equal the initial value in that position.

Let's formalize this.

Let’s define:

- x_i is the number of times operation is applied at position i (for i from 2 to n-1).

Then, for each position j from 1 to n:

- If j = 1: a[j] - x_2 = 0 → x_2 = a[1]

- If j = 2: a[j] - 2*x_2 - x_3 = 0

- If j = 3: a[j] - x_2 - 2*x_3 - x_4 = 0

- ...

- If j = n-1: a[j] - x_{n-2} - 2*x_{n-1} - x_n = 0

- If j = n: a[j] - x_{n-1} = 0 → x_{n-1} = a[n]

Wait, but in the operation, for i from 2 to n-1, we modify a[i-1], a[i], and a[i+1]. So, for each x_i, it affects a[i-1], a[i], and a[i+1].

Let me try to set up the equations properly.

For each i from 2 to n-1:

- a[i-1] -= x_i

- a[i] -= 2*x_i

- a[i+1] -= x_i

But I need to apply these operations in such a way that after all operations, a[j] = 0 for all j from 1 to n.

So, I need to solve for x_2 to x_{n-1} such that:

For j = 1: a[1] - x_2 = 0 → x_2 = a[1]

For j = 2: a[2] - 2*x_2 - x_3 = 0

For j = 3: a[3] - x_2 - 2*x_3 - x_4 = 0

...

For j = n-1: a[n-1] - x_{n-2} - 2*x_{n-1} - x_n = 0

For j = n: a[n] - x_{n-1} = 0 → x_{n-1} = a[n]

Wait, but in the operation, x_i only goes from i=2 to i=n-1, and it affects a[i-1], a[i], and a[i+1]. But for i=2, it affects a[1], a[2], a[3]; for i=3, it affects a[2], a[3], a[4]; and so on.

So, perhaps I can model this as a system of linear equations.

Let me try to write the equations in terms of x_i.

Let’s denote x_i as the number of operations applied at position i.

Then, for each position j from 1 to n:

- a[j] minus the sum of the contributions from all operations that affect it should be zero.

Let’s see:

- For j=1: a[1] - x_2 = 0 → x_2 = a[1]

- For j=2: a[2] - 2*x_2 - x_3 = 0

- For j=3: a[3] - x_2 - 2*x_3 - x_4 = 0

...

- For j=n-1: a[n-1] - x_{n-2} - 2*x_{n-1} - x_n = 0

- For j=n: a[n] - x_{n-1} = 0 → x_{n-1} = a[n]

Wait, but in the operation, x_i only goes up to i=n-1, and x_n doesn't exist because i cannot be n (since i ≤ n-1). So, perhaps the last equation is x_{n-1} = a[n].

But I need to make sure that all a[j] become zero.

Let me see if there's a pattern or a way to solve these equations step by step.

Starting from the first equation:

x_2 = a[1]

Then, plug x_2 into the second equation:

a[2] - 2*x_2 - x_3 = 0 → a[2] - 2*a[1] - x_3 = 0 → x_3 = a[2] - 2*a[1]

Then, plug x_2 and x_3 into the third equation:

a[3] - x_2 - 2*x_3 - x_4 = 0 → a[3] - a[1] - 2*(a[2] - 2*a[1]) - x_4 = 0

Simplify:

a[3] - a[1] - 2*a[2] + 4*a[1] - x_4 = 0 → x_4 = a[3] - a[1] - 2*a[2] + 4*a[1] = a[3] + 3*a[1] - 2*a[2]

This seems getting complicated. Maybe there's a better way.

Let me consider the differences or look for an invariant.

Another approach is to consider the operation as a vector subtraction and see if the target vector (all zeros) is reachable from the initial vector via linear combinations of the operation vectors.

Each operation corresponds to a vector where positions i-1, i, and i+1 are -1, -2, -1 respectively, and zeros elsewhere.

So, the problem reduces to checking if the initial vector a can be expressed as a linear combination of these operation vectors.

Given that all operations are subtracting, and we can apply them any number of times, it's effectively solving a system of linear equations where the coefficients are the operation vectors, and the solution vector is a.

But since we're dealing with integer operations and non-negative counts, it's essential to ensure that the solution has non-negative integers.

This seems like a system of linear equations with constraints.

Alternatively, perhaps there's a simpler way to check the feasibility.

Let me consider the operation as a way to reduce the array step by step.

Starting from the left, if I set x_2 = a[1], then a[1] becomes zero. Then, proceed to the next elements.

Wait, in the first equation, x_2 = a[1]. Then, in the second equation, x_3 = a[2] - 2*x_2 = a[2] - 2*a[1].

Then, in the third equation, x_4 = a[3] - x_2 - 2*x_3 = a[3] - a[1] - 2*(a[2] - 2*a[1}) = a[3] - a[1] - 2*a[2] + 4*a[1} = a[3] + 3*a[1] - 2*a[2]

This seems messy. Maybe there's a pattern or a cumulative sum that can help.

Let me consider the cumulative sum or prefix sums.

Define s[j] = a[1] + a[2] + ... + a[j]

Wait, not sure if that helps directly.

Let me think differently.

Suppose I have the array a[1], a[2], ..., a[n]

I can think of the operations as follows:

Each operation at position i reduces a[i-1], a[i], and a[i+1] by 1, 2, and 1 respectively.

I need all a[j] to become zero.

Let me consider the operation as subtracting a specific pattern from the array.

Maybe I can model this as a system where I need to find the number of times each operation is applied to reach zero.

But with large n (up to 2e5 per test case and up to 1e4 test cases), I need an efficient solution, probably O(n) per test case.

Let me think about the constraints and see if there's a pattern.

Looking at the sample input and output:

First test case:

n=5

a = [1, 3, 5, 5, 2]

Operations:

1. Apply at i=3: a[2]-2, a[3]-2, a[4]-2 => a becomes [1,1,3,3,2]

Wait, no, the operation is a[i-1]-1, a[i]-2, a[i+1]-1.

So, applying at i=3: a[2]-1, a[3]-2, a[4]-1 => [1,2,3,4,2]

Wait, but in the explanation, it's different. Maybe I need to follow the sequence in the explanation.

In the explanation:

- Apply at i=4: a[3]-1, a[4]-2, a[5]-1 => [1,3,4,3,1]

- Apply at i=3: a[2]-1, a[3]-2, a[4]-1 => [1,2,2,2,1]

- Apply at i=2: a[1]-1, a[2]-2, a[3]-1 => [0,0,1,2,1]

- Apply at i=4: a[3]-1, a[4]-2, a[5]-1 => [0,0,0,0,0]

So, it's possible.

But how to generalize this?

Maybe I can process the array from left to right, keeping track of the operations needed to make each element zero.

Let me try simulating this process.

Start from the left:

- At position 1: a[1]=1. To make it zero, need to apply operation at i=2 x_2 times where x_2 = a[1]=1.

- So, apply operation at i=2 once: a[1]-1, a[2]-2, a[3]-1 => a becomes [0,1,4,5,2]

- Now, a[1]=0.

- Move to position 2: a[2]=1. To make it zero, need to apply operation at i=3 x_3 times where x_3 = a[2]=1.

- Apply operation at i=3 once: a[2]-1, a[3]-2, a[4]-1 => [0,0,2,4,2]

- Now, a[2]=0.

- Move to position 3: a[3]=2. Apply operation at i=4 x_4 times where x_4 = a[3]=2.

- Apply operation at i=4 twice: a[3]-2, a[4]-4, a[5]-2 => [0,0,0,0,0]

- Now, a[3]=0, a[4]=0, a[5]=0.

So, it's possible.

Another test case:

n=5

a = [2,4,4,5,1]

Let's try the same approach.

- At position 1: a[1]=2. Apply operation at i=2 twice: a[1]-2, a[2]-4, a[3]-2 => [0,0,2,5,1]

- At position 2: a[2]=0. No need to apply any operation.

- At position 3: a[3]=2. Apply operation at i=4 twice: a[3]-2, a[4]-4, a[5]-2 => [0,0,0,1,-1]

- Now, a[5]=-1, which is negative. But we cannot have negative values, so this is invalid.

Hence, "NO"

Another test case:

n=5

a = [0,1,3,3,1]

- At position 1: a[1]=0. No operation needed.

- At position 2: a[2]=1. Apply operation at i=3 once: a[2]-1, a[3]-2, a[4]-1 => [0,0,1,2,1]

- At position 3: a[3]=1. Apply operation at i=4 once: a[3]-1, a[4]-2, a[5]-1 => [0,0,0,0,0]

- All zeros. "YES"

Another test case:

n=6

a = [5,6,0,2,3,0]

- At position 1: a[1]=5. Apply operation at i=2 five times: a[1]-5, a[2]-10, a[3]-5 => [-5,-4,-5,2,3,0]

- a[1]=-5, which is negative. Invalid. "NO"

Another test case:

n=4

a = [1,2,7,2]

- At position 1: a[1]=1. Apply operation at i=2 once: a[1]-1, a[2]-2, a[3]-1 => [0,0,6,2]

- At position 2: a[2]=0. No operation needed.

- At position 3: a[3]=6. Apply operation at i=4 six times: a[3]-6, a[4]-12 => [0,0,0,-10]

- a[4]=-10, which is negative. Invalid. "NO"

Another test case:

n=3

a = [7,1,0]

- At position 1: a[1]=7. Apply operation at i=2 seven times: a[1]-7, a[2]-14, a[3]-7 => [-7,-13,-7]

- Negative values. Invalid. "NO"

Last test case:

n=4

a = [1,1,1,1]

- At position 1: a[1]=1. Apply operation at i=2 once: a[1]-1, a[2]-2, a[3]-1 => [0,-1,0,1]

- a[2]=-1, which is negative. Invalid. "NO"

From these observations, it seems that if at any step, applying the necessary operations leads to negative values in the array, it's invalid, and the answer is "NO". Otherwise, if we can make all elements zero without negatives, it's "YES".

So, perhaps the condition is that the array can be made zero if and only if, when processing from left to right, subtracting the necessary operations doesn't lead to any negative values.

Let me try to formalize this.

Algorithm:

1. Start from the left of the array.

2. For each position i from 1 to n-2:

a. If a[i] < 0, return "NO"

b. Set opNum = a[i]

c. a[i] -= opNum

d. a[i+1] -= 2 * opNum

e. a[i+2] -= opNum

3. After processing up to n-2, check if a[n-1] == 0 and a[n] == 0. If yes, return "YES"; else, "NO"

Wait, but in the sample solutions, they only check a[n-1] and a[n] after processing up to n-2.

Let me see if this works for the first test case.

First test case:

n=5

a=[1,3,5,5,2]

Processing i=1:

a[1]=1 >=0

opNum=1

a[1]-=1 → 0

a[2]-=2 → 3-2=1

a[3]-=1 → 5-1=4

Now a=[0,1,4,5,2]

Processing i=2:

a[2]=1 >=0

opNum=1

a[2]-=1 →0

a[3]-=2 →4-2=2

a[4]-=1 →5-1=4

Now a=[0,0,2,4,2]

Processing i=3:

a[3]=2 >=0

opNum=2

a[3]-=2 →0

a[4]-=4 →4-4=0

a[5]-=2 →2-2=0

Now a=[0,0,0,0,0]

Check a[4]=0 and a[5]=0 → "YES"

Another test case:

n=5

a=[2,4,4,5,1]

Processing i=1:

a[1]=2 >=0

opNum=2

a[1]-=2 →0

a[2]-=4 →4-4=0

a[3]-=2 →4-2=2

Now a=[0,0,2,5,1]

Processing i=2:

a[2]=0 >=0

opNum=0

No changes

Processing i=3:

a[3]=2 >=0

opNum=2

a[3]-=2 →0

a[4]-=4 →5-4=1

a[5]-=2 →1-2=-1

Now a=[0,0,0,1,-1]

Check a[4]=1 >=0 and a[5]=-1 <0 → "NO"

Seems correct.

Another test case:

n=5

a=[0,1,3,3,1]

Processing i=1:

a[1]=0 >=0

opNum=0

No changes

Processing i=2:

a[2]=1 >=0

opNum=1

a[2]-=1 →0

a[3]-=2 →3-2=1

a[4]-=1 →3-1=2

Now a=[0,0,1,2,1]

Processing i=3:

a[3]=1 >=0

opNum=1

a[3]-=1 →0

a[4]-=2 →2-2=0

a[5]-=1 →1-1=0

Now a=[0,0,0,0,0]

Check a[4]=0 and a[5]=0 → "YES"

Another test case:

n=6

a=[5,6,0,2,3,0]

Processing i=1:

a[1]=5 >=0

opNum=5

a[1]-=5 →0

a[2]-=10 →6-10=-4

a[3]-=5 →0-5=-5

Now a=[0,-4,-5,2,3,0]

a[2]=-4 <0 → "NO"

Another test case:

n=4

a=[1,2,7,2]

Processing i=1:

a[1]=1 >=0

opNum=1

a[1]-=1 →0

a[2]-=2 →2-2=0

a[3]-=1 →7-1=6

Now a=[0,0,6,2]

Processing i=2:

a[2]=0 >=0

opNum=0

No changes

Processing i=3:

a[3]=6 >=0

opNum=6

a[3]-=6 →0

a[4]-=12 →2-12=-10

Now a=[0,0,0,-10]

Check a[4]=-10 <0 → "NO"

Another test case:

n=3

a=[7,1,0]

Processing i=1:

a[1]=7 >=0

opNum=7

a[1]-=7 →0

a[2]-=14 →1-14=-13

a[3]-=7 →0-7=-7

Now a=[0,-13,-7]

a[2]=-13 <0 → "NO"

Last test case:

n=4

a=[1,1,1,1]

Processing i=1:

a[1]=1 >=0

opNum=1

a[1]-=1 →0

a[2]-=2 →1-2=-1

a[3]-=1 →1-1=0

Now a=[0,-1,0,1]

a[2]=-1 <0 → "NO"

Seems like this algorithm works for the sample inputs.

Let me see if there are any edge cases where this might fail.

Edge case 1:

n=3

a=[0,0,0]

Processing i=1:

a[1]=0 >=0

opNum=0

No changes

Check a[2]=0 and a[3]=0 → "YES"

Edge case 2:

n=3

a=[1,2,1]

Processing i=1:

a[1]=1 >=0

opNum=1

a[1]-=1 →0

a[2]-=2 →2-2=0

a[3]-=1 →1-1=0

Check a[2]=0 and a[3]=0 → "YES"

Edge case 3:

n=3

a=[1,1,1]

Processing i=1:

a[1]=1 >=0

opNum=1

a[1]-=1 →0

a[2]-=2 →1-2=-1

a[3]-=1 →1-1=0

a[2]=-1 <0 → "NO"

Edge case 4:

n=4

a=[0,0,0,0]

Processing i=1:

a[1]=0 >=0

opNum=0

No changes

Processing i=2:

a[2]=0 >=0

opNum=0

No changes

Check a[3]=0 and a[4]=0 → "YES"

Edge case 5:

n=5

a=[0,0,0,0,0]

Similar to above, "YES"

Edge case 6:

n=3

a=[2,4,2]

Processing i=1:

a[1]=2 >=0

opNum=2

a[1]-=2 →0

a[2]-=4 →4-4=0

a[3]-=2 →2-2=0

Check a[2]=0 and a[3]=0 → "YES"

Edge case 7:

n=3

a=[1,3,1]

Processing i=1:

a[1]=1 >=0

opNum=1

a[1]-=1 →0

a[2]-=2 →3-2=1

a[3]-=1 →1-1=0

Now a=[0,1,0]

Processing i=2:

a[2]=1 >=0

opNum=1

a[2]-=1 →0

a[3]-=2 →0-2=-2

a[4]-=1 → but n=3, no a[4]

Wait, in the algorithm, for n=3, i goes up to n-2=1, so only process i=1.

Then check a[2]=1 and a[3]=1.

But in this case, after processing i=1, a=[0,1,0]

Then check a[2]=1 !=0 or a[3]=0.

Wait, in the initial processing, only i=1 is processed, and then check a[2] and a[3].

So, a[2]=1 !=0, so "NO"

But according to earlier logic, it should be "NO" because a[2]=1.

Wait, but in the earlier test case, n=3, a=[1,1,1] → "NO" because after processing i=1, a=[0,-1,0], which is negative.

But in this case, n=3, a=[1,3,1], after processing i=1, a=[0,1,0], then check a[2]=1 !=0 → "NO"

Seems consistent.

Another edge case:

n=3

a=[