The initial state is: `i` is 3, `n` is an integer where \(1 \leq n \leq 3 \cdot 10^5\), and `my_power` is equal to the original value of `my_power` minus `put_all_on_right[3]`.

The code snippet is:
```
my_power += k
```

Here, `my_power` is incremented by the value of `k`. Since the initial value of `my_power` was equal to its original value minus `put_all_on_right[3]`, after executing the code, the new value of `my_power` will be the old value of `my_power` plus `k`.

Therefore, the updated value of `my_power` is:
\[ \text{my\_power} = (\text{original value of my\_power}) - \text{put\_all\_on\_right[3]} + k \]

Other variables are not affected.

Output State: **`i` is 3, `n` is an integer where \(1 \leq n \leq 3 \cdot 10^5\), `my_power` is equal to the original value of `my_power` minus `put_all_on_right[3]` plus `k`.**