The code snippet `ma = len(s) - d` calculates the value of `ma` by subtracting `d` from the length of the string `s`.

Given:
- `s` is a string of length `n`.
- `d` is 3.

Thus, `ma` will be `n - 3`.

Output State: **`t` is an integer such that 1 <= t <= 10^4, `n` is an integer such that 1 <= n <= 10, `s` is a new input string of length `n` consisting of characters 'W' and 'B' with at least one 'B' present, `mi` is `k` if the first 'B' is at position `k`, `m` is an input integer, `c` is `k`, `d` is 3, `l` is an empty list, `j` is the next character in the reversed string `s[::-1]`, `ma` is `n - 3`.**