The code `dp[i] = tem` updates the value of `dp[i]` with the value of `tem`. Given that `tem` is defined as `dp[i - j] + abs(arr[i - j] - arr[i])`, this means that `dp[i]` will take the value of `dp[i - j] + abs(arr[i - j] - arr[i])`.

However, without knowing the exact values of `i`, `j`, `dp`, `arr`, and the specifics of how `tem` was calculated, we can only express the update in terms of these variables.

Given the initial state:
- `n` must be greater than 0.
- `k` is an integer such that \(1 \leq k \leq 100\) and \(k \leq n\).
- `arr` is updated to the value returned by `read()`.
- `dp` is a list of length `n` filled with `-1` (except `dp[0]` which is `0`).
- `tem` is assigned the value `dp[i - j] + abs(arr[i - j] - arr[i])`.

After executing `dp[i] = tem`, the value of `dp[i]` is updated to `tem`.

Therefore, the Output State is:
**`n` must be greater than 0, `k` is an integer such that \(1 \leq k \leq 100\) and \(k \leq n\), `arr` is updated to the value returned by `read()`, `dp` is a list of length `n` filled with `-1` (except `dp[0]` which is `0`), and `dp[i]` is updated to `dp[i - j] + abs(arr[i - j] - arr[i])`.**