Alright, I have this problem to solve. Let's read it carefully.

We have an array of n integers, and we need to perform exactly k operations. In each operation, we select a contiguous subarray (which can be empty) and insert the sum of this subarray anywhere in the array. Our goal is to maximize the sum of the array after k such operations, and we need to output this sum modulo 10^9 + 7.

First, I need to understand what exactly an operation does. So, in one operation, I choose a contiguous subarray, compute its sum, and then insert this sum into the array at any position I like. Importantly, the subarray can be empty, and its sum would be 0.

Let me think about what happens when I perform such an operation. Suppose I have an array [a, b, c], and I choose the subarray [b, c] with sum (b + c), and I insert this sum after a, making the array [a, (b + c), b, c]. Now, the sum of the array is a + (b + c) + b + c = a + b + c + b + c = a + 2b + 2c.

Wait, that seems interesting. By inserting the sum of a subarray, I'm effectively adding that sum to the total sum of the array.

Wait a minute, is that always the case? Let's try another example. Suppose I have [1, -2, 3], and I choose the subarray [-2], whose sum is -2, and insert it at the beginning, making [-2, 1, -2, 3]. The original sum was 1 - 2 + 3 = 2, and the new sum is -2 + 1 - 2 + 3 = 0, which is less than before. So, in this case, the sum decreased.

Hmm, so sometimes inserting a subarray sum can decrease the total sum. But our goal is to maximize the sum after k operations. So, we need a strategy that maximizes the sum.

Let me consider the opposite: how can I make the sum as large as possible? Well, if I always insert the sum of the entire array, that would seem beneficial.

Let's say I have array [a1, a2, ..., an], and I compute the sum S = a1 + a2 + ... + an. If I insert S into the array, the new sum becomes S + S = 2S. If I do this k times, I'd have S + k*S = (k+1)*S.

Wait, but I need to consider that I can choose any subarray, not just the entire array. Maybe choosing a different subarray could lead to a larger sum.

Let me think about it differently. Each operation allows me to add the sum of a chosen subarray to the total sum. So, the key is to choose the subarray with the maximum possible sum each time.

If I can choose the subarray with the maximum sum and insert it, then each operation adds the maximum possible value to the sum. Repeating this k times would give me the maximum possible sum.

So, perhaps I need to find the maximum subarray sum and add it k times to the original sum.

But wait, in the example provided, for n=2, k=2, with array [-4, -7], the output is 999,999,996, which is equivalent to -11 modulo 10^9 + 7. If I follow the above logic, the maximum subarray sum is 0 (from an empty subarray), and the original sum is -11. Adding 0 twice would give -11, which matches the example.

In another example, n=3, k=3, array [2,2,8], the output is 96. The maximum subarray sum is 12 (2+2+8), and adding it 3 times to the original sum (12) gives 12 + 3*12 = 48, which doesn't match the example. Wait, maybe I'm missing something.

Wait, in the second example, starting with [2,2,8], sum=12. If I insert 12 to get [2,2,8,12], sum=24. Then insert 24 to get [2,2,8,12,24], sum=48. Then insert 48 to get [2,2,8,12,24,48], sum=96. So, it's multiplying by 2 each time.

Wait, so it's not just adding the maximum subarray sum each time, but rather, the new sum is doubling each time because I'm adding the current sum each time.

Wait, in the first operation, I add the current sum (12) to get a new sum of 24. In the second operation, the current sum is 24, I add that to get 48, and so on.

So, it seems that if I always add the current sum to itself, the sum doubles each time.

Wait, but in the first operation, the sum becomes sum + sum = 2*sum.

After the second operation, it becomes sum + 2*sum = 3*sum.

Wait, no, wait. If I have sum S, and I insert S, the new sum is S + S = 2S.

Then, I have 2S, and I insert 2S, making it 2S + 2S = 4S.

Then, insert 4S to get 4S + 4S = 8S.

Wait, but in the example, starting from 12, after first insertion: 12 + 12 = 24.

Second insertion: 24 + 24 = 48.

Third insertion: 48 + 48 = 96.

So, it's multiplying by 2 each time.

So, it seems that if I always insert the current sum, the sum doubles each time.

So, after k insertions, the sum would be S * (2^k).

But wait, in the first example, with S = -11, and k=2, (-11) * (2^2) = -44, which is not equal to 999,999,996.

Wait, but in the first example, the output is 999,999,996, which is -4 modulo 10^9 + 7, because -4 + 10^9 + 7 = 999,999,996 + 4 = 10^9 + 7.

Wait, no, -11 modulo 10^9 + 7 is -11 + 10^9 + 7 = 10^9 - 4 = 999,999,996.

Wait, but according to the note, it's -11 modulo 10^9 + 7 is 999,999,996.

But according to my earlier assumption, S * (2^k) = -11 * 4 = -44, which is not equal to -11.

Wait, perhaps my assumption is incorrect.

Wait, in the first example, they say that they take an empty subarray twice and insert 0 each time, resulting in sum = -4 -7 +0 +0 = -11.

But according to my earlier assumption, if I insert the current sum each time, starting with -11, then insert -11 to get -11 + (-11) = -22, then insert -22 to get -22 + (-22) = -44, which is different from what they did.

So, perhaps my assumption is wrong.

Wait, maybe I need to choose which subarray to insert each time.

In the first operation, if I insert the sum of the entire array, which is -11, then the new array sum becomes -11 + (-11) = -22.

In the second operation, I insert -22 again, making the sum -22 + (-22) = -44.

But according to the problem, they inserted 0 twice, resulting in sum = -11.

So, it seems that choosing to insert the sum of an empty subarray (which is 0) is better in this case.

Wait, but in this case, inserting 0 doesn't change the sum.

Wait, but in the first operation, if I insert 0, the sum remains -11.

In the second operation, again insert 0, sum remains -11.

So, in this case, inserting 0 is better than inserting the sum of the entire array, which would make the sum worse.

So, perhaps the strategy is not always to insert the current sum, but to choose the maximum possible sum of any subarray to insert.

Wait, but in this case, the maximum subarray sum is 0 (from an empty subarray), and inserting that is better than inserting -11.

In another example, with [2,2,8], the maximum subarray sum is 12, which is positive, and inserting that repeatedly increases the sum.

So, perhaps the strategy is to find the maximum subarray sum and insert that in each operation.

But in the first example, the maximum subarray sum is 0, and inserting that is better than inserting -11.

So, perhaps the formula is: sum += max_subarray_sum * k

But in the second example, sum becomes S + k * S = S * (k + 1), but in the example, it's S * 2^k.

Wait, that's different.

Wait, perhaps it's sum *= (1 + k), but in the second example, it's S * 2^k.

Wait, perhaps it's sum *= (1 + k), but no, 12 * (1 + 3) = 48, but in the example, it's 96.

Wait, 12 * 2^3 = 96.

So, it's sum *= 2^k.

But in the first example, -11 * 2^2 = -44, which is worse than inserting 0 twice.

So, perhaps the formula is sum += max_subarray_sum * k.

In the first example, sum = -11 + 0 * 2 = -11.

In the second example, sum = 12 + 12 * 3 = 48, but in the example, it's 96.

Wait, that doesn't match.

Alternatively, maybe it's sum += max_subarray_sum * (2^k - 1).

In the second example, 12 + 12 * (2^3 - 1) = 12 + 12 * 7 = 96, which matches.

In the first example, -11 + 0 * (2^2 - 1) = -11, which matches.

So, perhaps the general formula is sum += max_subarray_sum * (2^k - 1).

Wait, but in the second example, sum += max_subarray_sum * (2^k - 1) = 12 + 12 * (8 - 1) = 12 + 84 = 96, which matches.

In the first example, -11 + 0 * (4 - 1) = -11, which matches.

Another example: n=1, k=7, array [7].

If I insert 7 each time: starting with [7], sum=7.

Insert 7: [7,7], sum=14.

Insert 14: [7,7,14], sum=28.

Insert 28: [7,7,14,28], sum=56.

Insert 56: [7,7,14,28,56], sum=112.

Insert 112: [7,7,14,28,56,112], sum=224.

Insert 224: [7,7,14,28,56,112,224], sum=448.

So, sum = 7 * (2^7 -1) = 7 * 127 = 889, but according to the formula, sum += max_subarray_sum * (2^k -1) = 7 + 7 * 127 = 7 + 889 = 896, which matches.

In the problem's output, for this case, it's 896.

So, it seems the formula is sum += max_subarray_sum * (2^k -1).

But wait, in the second example, sum += max_subarray_sum * (2^k -1) = 12 + 12 * 7 = 96, which matches.

In the first example, sum += 0 * 3 = -11 + 0 = -11, which matches.

So, the general formula seems to be sum += max_subarray_sum * (2^k -1).

Wait, but in the seventh example, with all elements being -1e9, the sum is -6e9, and according to the formula, sum += 0 * (2^k -1) = -6e9, but in the note, it's -6e9 + 42 = -6e9 + 42.

Wait, no, in the note, it says the answer is 42, because (-6e9) % (1e9 +7) = -6e9 + 7*(1e9 +7) = -6e9 + 7e9 +49 = 1e9 +49, but perhaps I misread.

Wait, in the note, it says "-6 * (1e9 +7) +42 = -6e9", which would be -6e9 -42 +42 = -6e9, but I'm getting confused.

Anyway, perhaps I should focus on the formula sum += max_subarray_sum * (2^k -1).

But in the seventh example, with all elements negative, the max_subarray_sum is 0 (from an empty subarray), so sum += 0 * (2^k -1) = sum.

But according to the note, they add 0 in each operation, so the sum remains the same, which is -6e9, and modulo 1e9+7 is 1e9+7 -6e9 = -6e9 +1e9 +7 = -5e9 +7, but I need to compute it properly.

Wait, perhaps I need to think differently.

Wait, perhaps the formula is sum += max_subarray_sum * (2^k -1), but only if max_subarray_sum > 0.

In the case where max_subarray_sum <= 0, sum remains the same.

Wait, but in the first example, sum += 0 * (2^k -1) = sum, which is correct.

In the second example, sum += 12 * 7 = 84, so total sum is 12 + 84 = 96, which matches.

In the seventh example, sum += 0 * (2^k -1) = sum, which is -6e9, and modulo 1e9+7 is -6e9 + m * (1e9+7), where m is chosen such that the result is between 0 and 1e9+7-1.

Specifically, -6e9 mod (1e9+7) = -6e9 + 7*(1e9+7)/1 = -6e9 + 7e9 +49 = 1e9 +49, but according to the note, it's 42.

Wait, perhaps I need to compute it differently.

Wait, in the note, it says "-6 * (1e9 +7) +42 = -6e9", which implies that -6*(1e9+7) +42 = -6e9 -42 +42 = -6e9.

But -6e9 modulo 1e9+7 is -6e9 + 6*(1e9+7) = -6e9 +6e9 +42 =42, which matches the note.

So, the formula seems to hold.

Wait, but in the formula sum += max_subarray_sum * (2^k -1), in the seventh example, max_subarray_sum is 0, so sum +=0, which is correct.

Hence, the general formula seems to be sum += max_subarray_sum * (2^k -1).

But wait, in the fourth example, n=5, k=1, array [4,-2,8,-12,9].

The maximum subarray sum is 4 + (-2) + 8 + (-12) +9 =17, but according to the note, they choose [4,-2,8] with sum 10, and insert it at the beginning, making [10,4,-2,8,-12,9], sum=17, which matches.

Wait, but according to my formula, sum += max_subarray_sum * (2^k -1) = 17 + 17*(2^1 -1) =17 +17=34, which doesn't match the note's 17.

Wait, perhaps I'm missing something.

Wait, in this case, k=1, so sum += max_subarray_sum * (2^1 -1) = sum += max_subarray_sum.

In the note, they choose to insert the sum of [4,-2,8]=10, and insert it at the beginning, making the array [10,4,-2,8,-12,9], sum=17.

But according to my formula, sum +=17, which would be 17 +17=34, but in reality, it's 17.

So, my formula seems incorrect.

Wait, perhaps I need to adjust the formula.

Wait, in this case, sum += max_subarray_sum * (2^k -1), but for k=1, that's sum += max_subarray_sum.

But in reality, when k=1, sum becomes sum + max_subarray_sum, which is correct.

Wait, in the second example, sum += max_subarray_sum * (2^k -1) =12 +12*(8-1)=12+84=96, which matches.

In the first example, sum +=0*(4-1)=0, which is correct.

In the fourth example, sum +=17*(2-1)=17, which would make sum=17+17=34, but according to the note, it's 17.

Wait, that's inconsistent.

Wait, perhaps I need to think differently.

Wait, in the fourth example, they choose to insert the sum of [4,-2,8]=10, and insert it at the beginning, making the array [10,4,-2,8,-12,9], sum=17.

But according to my earlier assumption, sum += max_subarray_sum, which is 17, so 17 +17=34, but in reality, it's 17.

Wait, perhaps I'm double-counting.

Wait, when I insert the sum of [4,-2,8]=10, I add 10 to the array, making the sum sum +10.

But the original sum was 4-2+8-12+9=7, not 17.

Wait, no, according to the note, the sum is 17.

Wait, let me recalculate: 4 + (-2) +8 +(-12)+9=7, but according to the note, it's 17.

Wait, perhaps I misread.

Wait, in the note, it says: "take a subarray consisting of the first three numbers (4,-2,8) and insert its sum (10) at the beginning, making [10,4,-2,8,-12,9], sum=17."

Wait, so original sum is 4-2+8-12+9=7, insert 10, sum becomes 10+4-2+8-12+9=17.

So, sum +=10, which is the sum of the chosen subarray.

So, in this case, sum +=10, not sum +=17.

Wait, but according to my formula, sum += max_subarray_sum * (2^k -1) =17*(1)=17, which would make sum=7+17=24, but in reality, sum=17.

So, my formula is incorrect.

Wait, perhaps I need to adjust the formula.

Wait, in each operation, I choose a subarray, compute its sum, and insert it into the array, which adds that sum to the total sum.

So, for k operations, I add the sum of the chosen subarrays in each operation.

To maximize the sum, I should choose the subarray with the maximum sum in each operation.

So, if the maximum subarray sum is S, then after k operations, the sum would be original_sum + k*S.

But in the second example, it's original_sum + S*(2^k -1).

Wait, that doesn't match.

Wait, in the second example, original_sum=12, S=12, k=3, sum=12 +12*7=96, which matches.

But in the fourth example, original_sum=7, S=10, k=1, sum=7 +10=17, which matches.

Wait, so perhaps the formula is sum += S*(2^k -1), where S is the maximum subarray sum.

But in the second example, sum=12 +12*(8-1)=96, which matches.

In the fourth example, sum=7 +10*(2-1)=17, which matches.

In the first example, sum=-11 +0*(4-1)=-11, which matches.

So, yes, the formula seems to be sum += S*(2^k -1), where S is the maximum subarray sum.

Hence, the final sum is original_sum + S*(2^k -1).

Then, take this sum modulo 1e9+7.

So, to solve the problem, I need to:

1. Compute the original sum of the array.

2. Find the maximum subarray sum S.

3. Compute the final sum as original_sum + S*(2^k -1).

4. Take this sum modulo 1e9+7.

Now, to compute 2^k modulo 1e9+7, I can use fast exponentiation.

Also, since S can be negative, but in cases where S is negative or zero, adding S*(2^k -1) should not make the sum worse than just the original sum.

Wait, in the first example, S=0, so sum +=0*(4-1)=0, which is correct.

In the seventh example, S=0, so sum +=0*(2^k -1)=0, which is correct.

In the fourth example, S=10, k=1, sum +=10*(2-1)=10, which makes sum=17.

Wait, but in the fourth example, the original sum is 7, and S=10, so sum=7 +10=17, which matches.

In the second example, sum=12 +12*(8-1)=96, which matches.

So, the formula seems consistent.

Hence, the approach is:

- Compute original_sum = sum of the array.

- Compute S = maximum subarray sum.

- Compute final_sum = original_sum + S*(2^k -1).

- Output final_sum modulo 1e9+7.

Now, to implement this, I need to compute the maximum subarray sum efficiently.

I can use Kadane's algorithm for this, which runs in O(n) time.

Also, I need to compute 2^k modulo 1e9+7 efficiently, which can be done using fast exponentiation.

Given that n and k can be up to 2e5, and t up to 1e4, but the sum of n and k over all test cases is up to 2e5, the total time should be acceptable.

Edge cases to consider:

- All elements are negative: in this case, S=0 (from an empty subarray), and sum +=0, so sum remains the original sum.

- All elements are positive: S equals the sum of the entire array, so sum += S*(2^k -1).

- k=0: but k >=1 as per constraints.

- n=1: simple case.

- Large values of k: up to 2e5, so need to handle large exponents efficiently.

- Negative sums: need to handle negative numbers correctly in the formula.

- Zero sum subarrays: choosing an empty subarray is allowed and its sum is zero.

Implementing this in code:

- Read t, the number of test cases.

- For each test case:

- Read n and k.

- Read the array a.

- Compute original_sum = sum(a).

- Compute S = maximum subarray sum using Kadane's algorithm.

- Compute 2^k modulo 1e9+7.

- Compute final_sum = original_sum + S*( (2^k) % mod -1 )

- Output final_sum modulo 1e9+7.

Wait, but 2^k can be large, so I need to compute (2^k -1) modulo mod, but need to handle negative numbers carefully.

Wait, (2^k -1) modulo mod is ( (2^k modulo mod) -1 ) modulo mod.

So, final_sum = original_sum + S * ( (2^k modulo mod) -1 )

Then, final_sum modulo mod = (original_sum + S * ( (2^k modulo mod) -1 )) modulo mod

This should handle large numbers correctly.

Implementing this in code should be straightforward.

Now, let's look at the given program and see if it matches this logic.

Given program:

import math

def func():

for i in range(int(input())):

(n, k) = map(int, input().split())

l = list(map(int, input().split()))

c = 0

maxi = 0

for ele in l:

if ele < 0 and c <= abs(ele):

maxi = max(c, maxi)

c = 0

else:

c += ele

maxi = max(c, maxi)

maxi = max(c, maxi)

print((2 ** k * maxi - maxi + sum(l)) % 1000000007)

So, in this program:

- It reads t, n, k, and the array l.

- It initializes c=0 and maxi=0.

- It iterates through the array:

- If ele <0 and c <= abs(ele), set maxi to max(c, maxi) and reset c=0.

- Else, c += ele.

- After the loop, it sets maxi = max(c, maxi).

- Then, it computes (2**k * maxi - maxi + sum(l)) % 1000000007.

Comparing this with my derived formula:

- original_sum = sum(l)

- S = maxi

- (2**k * maxi - maxi + sum(l)) % 1000000007

Which simplifies to:

sum + S*(2**k -1) modulo mod

Which matches my formula.

Hence, the given program seems correct.

But wait, in the implementation of finding maxi, which is supposed to be the maximum subarray sum, the code seems a bit off.

Let me verify if it correctly implements Kadane's algorithm.

Standard Kadane's algorithm:

max_current = max_global = arr[0]

for i in range(1, n):

max_current = max(arr[i], max_current + arr[i])

if max_current > max_global:

max_global = max_current

return max_global

But in the given code:

c = 0

maxi = 0

for ele in l:

if ele < 0 and c <= abs(ele):

maxi = max(c, maxi)

c = 0

else:

c += ele

maxi = max(c, maxi)

maxi = max(c, maxi)

This seems different from the standard Kadane's algorithm.

Let me test it with an example.

Example 1: [4, -2, 8, -12, 9]

Initialize c=0, maxi=0

ele=4: since 4 >=0, c +=4 => c=4, maxi=max(4,0)=4

ele=-2: -2 <0 and c=4 <= abs(-2)=2 => False, so c += (-2) => c=2, maxi=max(2,4)=4

ele=8: 8 >=0, c +=8 => c=10, maxi=max(10,4)=10

ele=-12: -12 <0 and c=10 <= abs(-12)=12 => maxi=max(10,10)=10, c=0

ele=9: 9 >=0, c +=9 => c=9, maxi=max(9,10)=10

Final maxi=10, which matches the note's maximum subarray sum.

Another example: [-4, -7]

Initialize c=0, maxi=0

ele=-4: -4 <0 and c=0 <= abs(-4)=4 => maxi=max(0,0)=0, c=0

ele=-7: -7 <0 and c=0 <= abs(-7)=7 => maxi=max(0,0)=0, c=0

Final maxi=0, which is correct.

Another example: [2,2,8]

Initialize c=0, maxi=0

ele=2: 2 >=0, c +=2 => c=2, maxi=max(2,0)=2

ele=2: 2 >=0, c +=2 => c=4, maxi=max(4,2)=4

ele=8: 8 >=0, c +=8 => c=12, maxi=max(12,4)=12

Final maxi=12, which is correct.

Seems like this implementation works correctly for these cases.

Comparing with standard Kadane's algorithm, this version seems to handle negative numbers differently, but it still finds the maximum subarray sum correctly in these examples.

Hence, the given program seems correct.

Therefore, the answer is True.

**Final Answer**

\[ \boxed{\text{True}} \]