The code `dp[i][j] = dp[i][j - 1]` assigns the value of `dp[i][j - 1]` to `dp[i][j]`. Since `j` is defined as `M + 1`, we can infer that `j - 1` equals `M`. 

This means that `dp[i][j]` will now hold the same value as `dp[i][M]`. The values of `n`, `k`, `M`, `t`, and `j` remain unchanged, but the value of `dp[i][j]` is updated based on the existing value of `dp[i][M]`.

Output State: **`n` is an integer (1 ≤ n ≤ 45), `k` is an integer (1 ≤ k ≤ 45), `M` must be greater than `M`, `t` is a sorted list of integers of length `k`, `j` is `M + 1`, `dp[i][j]` is now equal to `dp[i][M]`.**