Let's break down the problem step by step.

### Step-by-Step Analysis:

1. **Identify the Loop Condition:**
   The loop condition is given by:
   \[
   (x + y) \cdot x \leq n \quad \text{and} \quad (x + y) \cdot y \leq m
   \]

2. **Current Values at the End of the Previous Iteration:**
   - \( x = 3 \)
   - \( n \) must be at least 15
   - \( m \) is at least 7
   - \( y = 3 \)
   - \( cnt = 18 \)

3. **Evaluate the Loop Condition with Current Values:**
   Substitute the current values into the loop condition:
   \[
   (3 + 3) \cdot 3 \leq n \quad \text{and} \quad (3 + 3) \cdot 3 \leq m
   \]
   Simplify the expressions:
   \[
   6 \cdot 3 \leq n \quad \text{and} \quad 6 \cdot 3 \leq m
   \]
   Which further simplifies to:
   \[
   18 \leq n \quad \text{and} \quad 18 \leq m
   \]

4. **Determine the Conditions for the Next Iteration:**
   For the loop to continue, both conditions must be true:
   - \( (x + y) \cdot x \leq n \)
   - \( (x + y) \cdot y \leq m \)

   Given the current values, \( x = 3 \) and \( y = 3 \), the conditions become:
   - \( 18 \leq n \)
   - \( 18 \leq m \)

5. **Adjust the States:**
   Since \( n \) must be at least 15 and \( m \) must be at least 7, and the current values already satisfy these conditions, no adjustments are necessary for \( n \) and \( m \). However, the loop condition requires \( n \geq 18 \) and \( m \geq 18 \).

### Final State:
The only adjustment needed is to ensure that \( n \) and \( m \) meet the stricter condition required by the loop. Therefore, the state should be modified to reflect this.

**State:**
**`x` is 3, `n` must be at least 18, `m` must be at least 18, `y` is 3, and `cnt` is 18**