To determine the new value of `dp[i]`, we use the given formula:

\[ dp[i] = (dp[i - 1] + (i - 1) * dp[i - 2] * 2) \% (10^9 + 7) \]

Given:
- `i` is 3.
- `dp[1]` is 1.
- `dp[2]` is 3.
- `dp` is a list of zeros with length `m + 1` except for `dp[1]` and `dp[2]`.

Let's substitute the known values into the formula:

\[ dp[3] = (dp[2] + (3 - 1) * dp[1] * 2) \% (10^9 + 7) \]
\[ dp[3] = (3 + 2 * 1 * 2) \% (10^9 + 7) \]
\[ dp[3] = (3 + 4) \% (10^9 + 7) \]
\[ dp[3] = 7 \% (10^9 + 7) \]
\[ dp[3] = 7 \]

All other variables (`t`, `n`, `k`, `num`, `m`) remain unchanged.

Output State: **`t` remains the same, `n` remains the same, `k` remains the same, `num` is the sum of 1 for each iteration where `c == r` and 2 for each iteration where `c != r`, `m` is at least 2 and not equal to 0 or 1, `dp` is a list of zeros with length `m + 1` except `dp[1]` which is 1, `dp[2]` which is 3, and `dp[3]` which is 7, `i` is 3.**