To determine the new value of `dp[i]`, we need to apply the given formula to the initial state provided.

Given:
- `i` is 5
- `dp[i - 1]` is `dp[4]` which is 25
- `dp[i - 2]` is `dp[3]` which is 7
- The formula is `dp[i] = (dp[i - 1] + (i - 1) * dp[i - 2] * 2) % (10 ** 9 + 7)`

Substituting the values:
- `dp[5] = (25 + (5 - 1) * 7 * 2) % (10 ** 9 + 7)`
- `dp[5] = (25 + 4 * 7 * 2) % (10 ** 9 + 7)`
- `dp[5] = (25 + 56) % (10 ** 9 + 7)`
- `dp[5] = 81 % (10 ** 9 + 7)`
- `dp[5] = 81`

Thus, the value of `dp[5]` is updated to 81.

The other variables remain unchanged as they are not affected by the given code snippet.

Output State: **`t` is truthy minus 1, `n` is the first integer from the input, `k` is the second integer from the input, `num` is `k + y` where `y` is the number of times `c != r`, `m` is at least 5, `dp` is a list of zeros with length `m + 1` except `dp[1]` which is 1, `dp[2]` which is 3, `dp[3]` which is 7, `dp[4]` which is 25, and `dp[5]` which is 81, `i` is 5**.