Let's break down the initial state and the print statement step by step:

1. **Initial State:**
   - `p1`, `p2`, and `p3` are integers where \(0 \leq p1 \leq p2 \leq p3 \leq 30\).
   - `t` is greater than 1 (though `t` is not used in the print statement).
   - `_` is 1 (though `_` is not used in the print statement).
   - The sum of `p1`, `p2`, and `p3` is even.
   - `y` is set to `p3 - 1`.
   - `x` is set to 1.
   - `p3` must be greater than or equal to 2.

2. **Print Statement:**
   - The print statement is `print(p1 - x + p3)`.

3. **Variable Values:**
   - `x` is 1.
   - `p3` is an integer where \(2 \leq p3 \leq 30\).
   - `p1` is an integer where \(0 \leq p1 \leq p3\).

4. **Expression Calculation:**
   - The expression inside the print statement is `p1 - x + p3`.
   - Substituting `x` with 1, the expression becomes `p1 - 1 + p3`.
   - Simplifying, the expression is `p1 + p3 - 1`.

5. **Output Description:**
   - The output will be the value of `p1 + p3 - 1`.
   - Since `p1` and `p3` are integers and `p3` is at least 2, the minimum value of `p1 + p3 - 1` is \(0 + 2 - 1 = 1\).
   - The maximum value of `p1 + p3 - 1` is \(30 + 30 - 1 = 59\).

Given the constraints and the expression, the output will be the value of `p1 + p3 - 1`.

Output: **p1 + p3 - 1 (where p1 is an integer such that 0 ≤ p1 ≤ p3 and p3 is an integer such that 2 ≤ p3 ≤ 30, and the sum of p1, p2, and p3 is even)**