To determine what will be printed by the `print(p1 - x + p3)` statement, let's break down the initial state and the values of the variables involved:

1. **Initial State:**
   - `p1`, `p2`, and `p3` are integers provided by the user, where \(0 \leq p1 \leq p2 \leq p3 \leq 30\).
   - `t` is greater than 1 (though this variable is not used in the print statement).
   - `_` is 2 (though this variable is not used in the print statement).
   - The sum of `p1`, `p2`, and `p3` is even.
   - `x` is 0.
   - `y` is equal to `p3`.
   - The current value of `p1 - x` is less than or equal to the current value of `p2 - y`.

2. **Variables in the Print Statement:**
   - `p1 - x + p3`:
     - `x` is 0, so `p1 - x` simplifies to `p1`.
     - Therefore, `p1 - x + p3` simplifies to `p1 + p3`.

3. **Constraints and Conditions:**
   - Since `x` is 0, `p1 - x` is simply `p1`.
   - `y` is `p3`, so `p2 - y` is `p2 - p3`.
   - The condition `p1 - x <= p2 - y` simplifies to `p1 <= p2 - p3`.

4. **Sum of `p1`, `p2`, and `p3` is Even:**
   - This means `p1 + p2 + p3` is even.

5. **Final Calculation:**
   - The print statement will output the value of `p1 + p3`.

Given the constraints and conditions, the most precise description of the output is:

Output: **p1 + p3 (where p1 and p3 are integers such that 0 ≤ p1 ≤ p2 ≤ p3 ≤ 30, the sum of p1, p2, and p3 is even, and p1 ≤ p2 - p3)**