The code snippet updates the value of `F[i]` based on the given formula:

\[ F[i] = \min(A[i] + M[i - 1], A[i] + A[i - 1] + M[i - 2]) \]

Given the initial state:
- `t` is an integer such that 1 ≤ t ≤ 2 ⋅ 10^4
- `_` is 1
- `n` must be greater than 2
- `A` is a map object containing integers from the input line in reverse order
- `F` is a list of length `n` with `F[0] = A[0]` and `F[1] = A[1]`, and the rest elements are 0
- `M` is a list of length `n` initialized to `[0] * n`, with `M[2] = min(A[1], A[0])`
- `i` is 2

Let's calculate the new value of `F[i]`:

1. **Accessing `A[i]`:**
   - Since `i` is 2, we access `A[2]`.

2. **Accessing `M[i - 1]`:**
   - `i - 1` is 1, so we access `M[1]`. According to the initial state, `M[1]` is 0.

3. **Accessing `A[i - 1]`:**
   - `i - 1` is 1, so we access `A[1]`.

4. **Accessing `M[i - 2]`:**
   - `i - 2` is 0, so we access `M[0]`. According to the initial state, `M[0]` is 0.

5. **Calculating the two expressions:**
   - First expression: \( A[2] + M[1] \)
     - This is \( A[2] + 0 = A[2] \)
   - Second expression: \( A[2] + A[1] + M[0] \)
     - This is \( A[2] + A[1] + 0 = A[2] + A[1] \)

6. **Finding the minimum of the two expressions:**
   - \( F[2] = \min(A[2], A[2] + A[1]) \)

Thus, the updated value of `F[2]` is \( \min(A[2], A[2] + A[1]) \).

Output State: **`t` is an integer such that 1 ≤ t ≤ 2 ⋅ 10^4, `_` is 1, `n` must be greater than 2, `A` is a map object containing integers from the input line in reverse order, `F` is a list of length `n` with `F[0] = A[0]`, `F[1] = A[1]`, and `F[2] = min(A[2], A[2] + A[1])`, the rest elements are 0, `M` is a list of length `n` initialized to `[0] * n`, with `M[2] = min(A[1], A[0])`, `i` is 2**