The code snippet updates the value of `F[i]` based on the given formula. Let's analyze the impact:

1. `F[i]` is set to the minimum of two expressions: `A[i] + M[i - 1]` and `A[i] + A[i - 1] + M[i - 2]`.
2. The value of `i` is 2, so we need to evaluate `F[2]` using the elements of `A` and `M` at indices 2, 1, and 0.

Given the initial state:
- `t` is an integer such that 1 ≤ t ≤ 2 ⋅ 10^4
- `_` is 2
- `n` is an input integer greater than 2
- `A` is a map object containing integers from the new input line in the original order
- `F` is a list of length `n` with `F[0] = A[0]` and `F[1] = A[1]` and the rest initialized to `[0] * (n-2)`
- `M` is a list of length `n` initialized to `[0] * n` with `M[2] = min(A[0], A[1])`
- `i` is 2

Let's calculate the new value of `F[2]`:
- `F[2] = min(A[2] + M[1], A[2] + A[1] + M[0])`

Since `M[1]` is 0 (as `M` is initialized to `[0] * n` and only `M[2]` is updated), and `M[0]` is also 0, we have:
- `F[2] = min(A[2] + 0, A[2] + A[1] + 0)`
- `F[2] = min(A[2], A[2] + A[1])`

Thus, `F[2]` is the minimum of `A[2]` and `A[2] + A[1]`.

The updated state is:
- `t` is an integer such that 1 ≤ t ≤ 2 ⋅ 10^4
- `_` is 2
- `n` is an input integer greater than 2
- `A` is a map object containing integers from the new input line in the original order
- `F` is a list of length `n` with `F[0] = A[0]`, `F[1] = A[1]`, and `F[2] = min(A[2], A[2] + A[1])`, and the rest initialized to `[0] * (n-3)`
- `M` is a list of length `n` initialized to `[0] * n` with `M[2] = min(A[0], A[1])`
- `i` is 2

Output State: **`t` is an integer such that 1 ≤ t ≤ 2 ⋅ 10^4, `_` is 2, `n` is an input integer greater than 2, `A` is a map object containing integers from the new input line in the original order, `F` is a list of length `n` with `F[0] = A[0]`, `F[1] = A[1]`, and `F[2] = min(A[2], A[2] + A[1])`, and the rest initialized to `[0] * (n-3)`, `M` is a list of length `n` initialized to `[0] * n` with `M[2] = min(A[0], A[1])`, `i` is 2**