The code snippet updates the value of `F[i]` using the formula `F[i] = min(A[i] + M[i - 1], A[i] + A[i - 1] + M[i - 2])`. Given the initial state:

- `t` is an integer such that 1 ≤ t ≤ 2 ⋅ 10^4
- `_` is 2
- `n` is an input integer greater than 3
- `A` is a map object containing integers from the new input line in the original order
- `F` is a list of length `n` with `F[0] = A[0]`, `F[1] = A[1]`, and `F[2] = min(A[2], A[2] + A[1])`, and the rest initialized to `[0] * (n-3)`
- `M` is a list of length `n` initialized to `[0] * n` with `M[2] = min(A[0], A[1])` and `M[3] = min(min(A[2], A[2] + A[1]), A[1])`
- `i` is 3

Let's evaluate the expression for `F[i]`:

1. `A[i]` is the third element in the map object `A`.
2. `M[i - 1]` is `M[2]`, which is `min(A[0], A[1])`.
3. `A[i - 1]` is `A[2]`.
4. `M[i - 2]` is `M[1]`, which is 0 (since `M` is initialized to `[0] * n`).

Thus, the expression becomes:
\[ F[3] = \min(A[3] + M[2], A[3] + A[2] + M[1]) \]
\[ F[3] = \min(A[3] + \min(A[0], A[1]), A[3] + A[2] + 0) \]
\[ F[3] = \min(A[3] + \min(A[0], A[1]), A[3] + A[2]) \]

Therefore, the updated value of `F[3]` is:
\[ F[3] = \min(A[3] + \min(A[0], A[1]), A[3] + A[2]) \]

The output state remains the same for all other variables except for `F[3]`.

Output State: **`t` is an integer such that 1 ≤ t ≤ 2 ⋅ 10^4, `_` is 2, `n` is an input integer greater than 3, `A` is a map object containing integers from the new input line in the original order, `F` is a list of length `n` with `F[0] = A[0]`, `F[1] = A[1]`, `F[2] = min(A[2], A[2] + A[1])`, and `F[3] = min(A[3] + min(A[0], A[1]), A[3] + A[2])`, the rest initialized to `[0] * (n-4)`, `M` is a list of length `n` initialized to `[0] * n` with `M[2] = min(A[0], A[1])` and `M[3] = min(min(A[2], A[2] + A[1]), A[1])`, `i` is 3**.