Let's break down the problem step by step:

1. **Identify the Loop Variables**: The loop variable in the given `for` loop is `b`, and it ranges from `a` to `(n - a) // 2 + 1`.

2. **Understand the Initial State**:
   - `ways` is the number of pairs (a, b) such that `2 * (a + b) == n` and `a != b`.
   - `a` is initially `k + 1`.
   - `b` is initially `k + 2`.
   - There is no change in `ways` if the condition `a != b and 2 * (a + b) == n` is false.

3. **Loop Execution**:
   - The loop iterates over values of `b` starting from `a` up to `(n - a) // 2 + 1`.
   - For each value of `b`, the loop checks if `2 * (a + b) == n` and `a != b`.
   - If the condition is true, `ways` is incremented by 1.
   - `a` is set to `b` for the next iteration.
   - `b` starts from `a + 1` for the next iteration.

4. **Determine the New State**:
   - Since the loop increments `b` by 1 for each iteration, the new value of `b` will be `a + 1`.
   - `a` is set to `b` at the end of each iteration, so `a` becomes `a + 1`.
   - `ways` remains unchanged if the condition is false.

Given this information, let's adjust the states for the next iteration:

- `a` will be `k + 2` (since `a` was `k + 1` and it is incremented by 1).
- `b` will be `k + 3` (since `b` starts from `k + 2` and is incremented by 1).

Therefore, the state at the start of the next iteration should be:

State: **`ways` is the number of pairs (a, b) such that `2 * (a + b) == n` and `a != b`, and a is in the range [0, n//2], plus 1 if the condition (a != b and 2 * (a + b) == n) is satisfied; `a` is k + 2; `b` is k + 3.**