Let's analyze the given Python loop and the provided initial state and output states to determine the final output state after all executions of the loop.

### Initial State
- `ways` is the number of pairs `(a, b)` such that `2 * (a + b) == n` and `a != b`, and `a` is in the range `[0, n//2]`.
- `a` is `k + 1`.

### Code of the Loop
```python
for b in range(a, (n - a) // 2 + 1):
    if a != b and 2 * (a + b) == n:
        ways += 1
```

### Analysis
1. **Variable `a`**: The variable `a` starts at `k + 1` and remains constant within the loop as the loop body only updates `ways` based on the value of `b`.
2. **Variable `b`**: The variable `b` iterates over the range from `a` to `(n - a) // 2 + 1`. The loop increments `ways` each time it finds a valid pair `(a, b)` where `2 * (a + b) == n` and `a != b`.
3. **Invariants**:
   - `a` remains `k + 1` throughout the loop.
   - `b` changes with each iteration but always starts from `a` and goes up to `(n - a) // 2 + 1`.

### Loop Execution
- The loop runs for each valid `b` such that `a != b` and `2 * (a + b) == n`.
- Each time the condition `2 * (a + b) == n` and `a != b` is met, `ways` is incremented by 1.

### Output States Provided
- After 1 time: `ways` is incremented by 1 if the condition is met, with `b` being at least `k + 1`.
- After 2 times: `ways` is incremented by 1 again if the condition is met, with `b` being `k + 2`.
- After 3 times: `ways` is incremented by 1 again if the condition is met, with `b` being `k + 3`.

### Generalizing the Loop Behavior
- The loop will continue to increment `ways` for each valid pair `(a, b)` where `a = k + 1` and `b` ranges from `k + 1` to `(n - a) // 2 + 1` as long as the condition `2 * (a + b) == n` and `a != b` is met.

### Final Output State
To find the final value of `ways`, we need to count all valid pairs `(a, b)` where `a = k + 1` and `2 * (a + b) == n` and `a != b`.

For `a = k + 1`, the equation becomes:
\[ 2 \times ((k + 1) + b) == n \]
\[ 2k + 2 + 2b == n \]
\[ 2b == n - 2k - 2 \]
\[ b == \frac{n - 2k - 2}{2} \]

This value of `b` must also satisfy:
\[ a < b \leq \frac{n - a}{2} \]
Substituting `a = k + 1`:
\[ k + 1 < \frac{n - 2k - 2}{2} \leq \frac{n - (k + 1)}{2} \]

Simplifying:
\[ 2k + 2 < n - 2k - 2 \]
\[ 4k + 4 < n \]
\[ k < \frac{n - 4}{4} \]

And:
\[ \frac{n - 2k - 2}{2} \leq \frac{n - k - 1}{2} \]
\[ n - 2k - 2 \leq n - k - 1 \]
\[ -2k - 2 \leq -k - 1 \]
\[ -k \leq 1 \]
\[ k \geq -1 \]

Thus, `k` must be an integer such that:
\[ k < \frac{n - 4}{4} \]

If `k` satisfies this condition, the value of `b` will be valid and `ways` will be incremented by 1 for each valid `b`.

### Final Output State
Output State: **`ways` is the number of valid pairs (a, b) such that 2 * (a + b) == n, a = k + 1, and b is in the range [k + 1, (n - a) // 2 + 1] with a != b.**