The code `W += w` updates the value of `W` by adding the current value of `w` to it. Given the initial state, let's analyze the impact:

- `n` remains an integer where 1 ≤ n ≤ 100.
- `i` remains 1.
- `myBooks` is a list containing one element `[w, t]`.
- `W` was initially equal to `w`.
- `t` is the first integer from the next input pair.
- `w` is the second integer from the next input pair.
- There are `n` pairs of integers `(ti, wi)` where 1 ≤ ti ≤ 2 and 1 ≤ wi ≤ 100.

After executing `W += w`:
- `W` is now updated to `W + w`, which simplifies to `w + w` or `2 * w`.

Therefore, the output state is:
Output State: **`n` is an integer where 1 ≤ n ≤ 100, `i` is 1, `myBooks` is a list containing one element `[w, t]`, `W` is `2 * w`, `t` is the first integer from the next input pair, `w` is the second integer from the next input pair, and there are `n` pairs of integers `(ti, wi)` where 1 ≤ ti ≤ 2 and 1 ≤ wi ≤ 100**