The code `W += w` updates the value of `W` by adding the current value of `w` to it. Given the initial state, `W` is initially `2 * w`. After executing the code, `W` becomes `2 * w + w`, which simplifies to `3 * w`.

The other variables and conditions remain unchanged. The value of `n` is still an integer between 1 and 100, `i` is still 2, `myBooks` is still a list containing two elements `[w, t]` and `[w, t]`, `t` is still the first integer from the next input pair, and `w` is still the second integer from the next input pair. There are still `n` pairs of integers `(ti, wi)` where 1 ≤ ti ≤ 2 and 1 ≤ wi ≤ 100.

Output State: **`n` is an integer where 1 ≤ n ≤ 100, `i` is 2, `myBooks` is a list containing two elements `[w, t]` and `[w, t]`, `W` is `3 * w`, `t` is the first integer from the next input pair, `w` is the second integer from the next input pair, and there are `n` pairs of integers `(ti, wi)` where 1 ≤ ti ≤ 2 and 1 ≤ wi ≤ 100**