The code snippet `W -= book[0]` updates the value of `W` by subtracting the first element of the first sublist in `myBooks` from it.

Given the Initial State:
- `n` is an integer where 1 ≤ n ≤ 100
- `i` is `n-1`
- `myBooks` is a reversed sorted list containing at least 1 element, each element is a list `[w, t]` where `t` is an integer (1 ≤ t ≤ 2) and `w` is an integer (1 ≤ w ≤ 100)
- `W` is the sum of all `w` values from the input pairs
- `T` is `T + t1` where `t1` is the second element of the first sublist in `myBooks`
- There are `n` pairs of integers `(ti, wi)` where 1 ≤ ti ≤ 2 and 1 ≤ wi ≤ 100

Let's denote the first sublist in `myBooks` as `[w1, t1]`. The value of `W` is updated by subtracting `w1` from its current value.

Therefore, the Output State is:
**`n` is an integer where 1 ≤ n ≤ 100, `i` is `n-1`, `myBooks` is a reversed sorted list containing at least 1 element, each element is a list `[w, t]` where `t` is an integer (1 ≤ t ≤ 2) and `w` is an integer (1 ≤ w ≤ 100), `W` is `W - w1` where `w1` is the first element of the first sublist in `myBooks`, `T` is `T + t1` where `t1` is the second element of the first sublist in `myBooks`, and there are `n` pairs of integers `(ti, wi)` where 1 ≤ ti ≤ 2 and 1 ≤ wi ≤ 100.**