The code snippet provided decrements the value of `cnt` by 1. Given the initial state, `cnt` was initially set to `k - 1`. After executing `cnt -= 1`, the new value of `cnt` will be `(k - 1) - 1`, which simplifies to `k - 2`.

None of the other variables (`n`, `k`, `v`, `l`, `i`) are affected by this operation.

Output State: **`n` is a positive integer, `k` is an integer such that `1 <= k <= n`, `v` is the value returned by `func_2()` during the last iteration (`i = 1`), `cnt` is `k - 2`, `l` is `func_2() + 1` and must be less than `n + 1`, `i` is `2`.**