To determine the output of the `print` statement, let's break down the given initial state and the variables involved:

- `n` is a positive integer such that `n >= 3 * k`.
- `k` is an integer such that `3 <= k <= n`.
- `v` is the value returned by `func_2()` during the last iteration (`i = 1`) and `v < n`.
- `cnt` is `k - 2`.
- `l` is `func_2() + 1`.
- `i` is `3`.

The `print` statement is:
```python
print(f'? {l} {i * v}', flush=True)
```

Let's analyze the components of this statement:

1. **`l`**: According to the initial state, `l` is defined as `func_2() + 1`. Since `v` is the value returned by `func_2()` during the last iteration (`i = 1`), we can infer that `l = v + 1`.

2. **`i * v`**: Here, `i` is explicitly given as `3`. Therefore, `i * v` simplifies to `3 * v`.

Putting it all together, the `print` statement will output:
- `?` (a literal question mark)
- `l` which is `v + 1`
- `i * v` which is `3 * v`

Thus, the output will be formatted as:
Output: **? [v + 1] [3 * v] (where v is the value returned by func_2() during the last iteration i=1)**

However, since we do not have the specific value of `v`, we express the output in terms of `v`.

Final Output:
Output: **? [v + 1] [3 * v] (where v is the value returned by func_2() during the last iteration i=1)**