To determine what will be printed, let's break down the given Python code snippet and the initial state:

### Initial State:
- `n`, `a`, and `b` are integers read from the input.
- `k` is calculated as follows:
  - If `b > a`, then `k = min(n, b - a)`.
  - Otherwise (`b <= a`), then `k = min(n, 0)`.

### Code Snippet:
```python
print(b * k - k * (k - 1) // 2 + (n - k) * a)
```

### Step-by-Step Analysis:

1. **Determine `k`:**
   - If `b > a`, `k` is the smaller value between `n` and `b - a`.
   - If `b <= a`, `k` is the smaller value between `n` and `0`. Since `min(n, 0)` will always be `0` for any non-negative integer `n`, `k` will be `0` in this case.

2. **Calculate the Expression:**
   - The expression to be printed is `b * k - k * (k - 1) // 2 + (n - k) * a`.
   - We need to evaluate this expression based on the value of `k`.

#### Case 1: `b > a`
- Here, `k = min(n, b - a)`.
- Let's substitute `k` into the expression:
  - `b * k - k * (k - 1) // 2 + (n - k) * a`
  - This expression calculates a weighted sum based on the values of `a`, `b`, `n`, and `k`.

#### Case 2: `b <= a`
- Here, `k = 0`.
- Substituting `k = 0` into the expression:
  - `b * 0 - 0 * (0 - 1) // 2 + (n - 0) * a`
  - Simplifies to `0 + 0 + n * a`
  - Which further simplifies to `n * a`

### Final Output Description:
- If `b > a`, the output will be `b * k - k * (k - 1) // 2 + (n - k) * a` where `k = min(n, b - a)`.
- If `b <= a`, the output will be `n * a`.

Given these conditions, the final output can be described as follows:

Output: **`b * k - k * (k - 1) // 2 + (n - k) * a` (where `k = min(n, b - a)` if `b > a`, otherwise `k = 0`)**