The code snippet `ans += m - hmp[i]` updates the value of `ans` by adding the difference between `m` and `hmp[i]` to its current value. Given the initial state:

- `_` is `t`
- `t` is an integer input by the user (1 <= t <= 1000)
- `n` and `m` are integers provided by the user input (1 <= n <= 50 and 1 <= m <= 5)
- `a` is a string of length `n` containing characters from 'A' to 'G'
- `p` is 'ABCDEF'
- `hmp` is a Counter object that counts the occurrences of each character in the string `s` and must have at least one key-value pair
- `i` is the first key in `hmp`
- `ans` is the sum of `m` for each character in 'ABCDEF' that is not present in `hmp'
- `s` is a new non-empty string input by the user
- The value of `hmp[i]` is less than `m`

The value of `ans` is updated by adding `m - hmp[i]` to its current value. Since `hmp[i]` is less than `m`, the value added to `ans` will be a positive integer.

Output State: **`_` is `t`, `t` is an integer input by the user (1 <= t <= 1000), `n` and `m` are integers provided by the user input (1 <= n <= 50 and 1 <= m <= 5), `a` is a string of length `n` containing characters from 'A' to 'G', `p` is 'ABCDEF', `hmp` is a Counter object that counts the occurrences of each character in the string `s` and must have at least one key-value pair, `i` is the first key in `hmp`, `ans` is now `ans + (m - hmp[i])`, `s` is a new non-empty string input by the user, and the value of `hmp[i]` is less than `m`.**