To determine the output of the given print statement, we need to carefully analyze the initial state and the variables involved. Let's break down the problem step by step.

### Initial State:
- `t` is an integer such that \(1 \leq t \leq 5 \times 10^4\).
- `n` is initialized to 0.
- `k` is an integer.
- `s` is the cumulative sum of `(n + 1) // 2` values from each iteration until the loop terminates.
- `m` is \(2^i\) where `i` is the number of iterations the loop completed.

### Key Points:
- The value of `t` is the number of iterations the loop will run.
- `n` starts at 0 and is incremented in each iteration.
- `s` accumulates the value of `(n + 1) // 2` in each iteration.
- `m` is calculated as \(2^i\) where `i` is the number of iterations, which is `t`.

### Iteration Details:
- In each iteration, `n` is incremented by 1.
- The value `(n + 1) // 2` is added to `s`.
- After `t` iterations, `m` becomes \(2^t\).

### Calculation of `s`:
- In the first iteration, `n = 0`, so `(n + 1) // 2 = 1 // 2 = 0`. `s = 0`.
- In the second iteration, `n = 1`, so `(n + 1) // 2 = 2 // 2 = 1`. `s = 0 + 1 = 1`.
- In the third iteration, `n = 2`, so `(n + 1) // 2 = 3 // 2 = 1`. `s = 1 + 1 = 2`.
- In the fourth iteration, `n = 3`, so `(n + 1) // 2 = 4 // 2 = 2`. `s = 2 + 2 = 4`.
- This pattern continues, and `s` can be seen as the sum of the sequence \([0, 1, 1, 2, 2, 3, 3, \ldots]\) up to `t` terms.

### Sum Formula for `s`:
- The sequence \([0, 1, 1, 2, 2, 3, 3, \ldots]\) can be analyzed as follows:
  - For even `t`, `s` is the sum of the first \(\frac{t}{2}\) integers repeated twice.
  - For odd `t`, `s` is the sum of the first \(\frac{t-1}{2}\) integers repeated twice plus the middle term \(\frac{t+1}{2}\).

- The sum of the first \(i\) integers is \(\frac{i(i+1)}{2}\).
- Therefore, for even `t`, `s = 2 \times \frac{\frac{t}{2}(\frac{t}{2} + 1)}{2} = \frac{t(t+2)}{4}`.
- For odd `t`, `s = 2 \times \frac{\frac{t-1}{2}(\frac{t-1}{2} + 1)}{2} + \frac{t+1}{2} = \frac{(t-1)(t+1) + 2(t+1)}{4} = \frac{(t+1)(t-1+2)}{4} = \frac{(t+1)(t+1)}{4} = \frac{(t+1)^2}{4}`.

### Simplified Formula for `s`:
- Combining both cases, `s` can be expressed as:
  \[
  s = \left\lfloor \frac{t^2}{4} \right\rfloor
  \]

### Calculation of `m`:
- `m = 2^t`.

### Final Expression for the Print Statement:
- The print statement is: `print((2 * (k - s) - 1) * m)`
- Substituting the values, we get:
  \[
  \text{Output} = (2 \times (k - \left\lfloor \frac{t^2}{4} \right\rfloor) - 1) \times 2^t
  \]

### Final Output:
Output: **(2 * (k - ⌊t^2 / 4⌋) - 1) * 2^t**