To determine what will be printed by the `print(d2[y] - d2[x])` statement, let's break down the initial state and the relevant parts of the code:

### Initial State:
- `t` is an integer where \(1 \leq t \leq 10^4\).
- `i` is 1.
- `n` is equal to `t` and greater than 0.
- `l` is a list of integers provided by the user input.
- `d1` is a defaultdict initialized with default factory `int` and `d1[2]` is 1.
- `d2` is a defaultdict initialized with default factory `int` and `d2[n - 1]` is 1.
- `m` must be greater than 2.
- `j` is 2.
- `x` and `y` are updated to new integers provided by the user input.
  - If the new `y` > `x`, the condition `y` > `x` holds true.
  - If the new `y` ≤ `x`, the condition `y` ≤ `x` holds true.

### Analysis:
1. **Defaultdict Initialization**:
   - `d1` is a defaultdict with default factory `int` and `d1[2]` is 1.
   - `d2` is a defaultdict with default factory `int` and `d2[n - 1]` is 1.

2. **User Input**:
   - `x` and `y` are updated to new integers provided by the user input.
   - The relationship between `x` and `y` is determined by the user input:
     - If `y` > `x`, the condition `y` > `x` holds true.
     - If `y` ≤ `x`, the condition `y` ≤ `x` holds true.

3. **Dictionary Access**:
   - `d2[y]` and `d2[x]` are accessed.
   - Since `d2` is a defaultdict with default factory `int`, any key that is not explicitly set will return 0.

4. **Calculation**:
   - The expression `d2[y] - d2[x]` will be evaluated.
   - If `y` is equal to `n - 1`, then `d2[y]` will be 1 (since `d2[n - 1]` is 1).
   - If `x` is equal to `n - 1`, then `d2[x]` will be 1.
   - Otherwise, both `d2[y]` and `d2[x]` will be 0 if they are not equal to `n - 1`.

### Possible Scenarios:
- If `y == n - 1` and `x != n - 1`, then `d2[y]` is 1 and `d2[x]` is 0, so `d2[y] - d2[x]` is 1.
- If `x == n - 1` and `y != n - 1`, then `d2[x]` is 1 and `d2[y]` is 0, so `d2[y] - d2[x]` is -1.
- If `y == n - 1` and `x == n - 1`, then `d2[y]` is 1 and `d2[x]` is 1, so `d2[y] - d2[x]` is 0.
- If neither `y` nor `x` is equal to `n - 1`, then both `d2[y]` and `d2[x]` are 0, so `d2[y] - d2[x]` is 0.

### Conclusion:
Given the initial state and the conditions, the output of the `print(d2[y] - d2[x])` statement will depend on the values of `y` and `x` relative to `n - 1`.

Output: **d2[y] - d2[x] (where d2[y] is 1 if y == n - 1, otherwise 0, and d2[x] is 1 if x == n - 1, otherwise 0)**