According to the code, the loop iterates over `y` from 0 to `k` inclusive. The loop body increments `y` by 1 each iteration and checks if \(0 \leq \text{nokori} - (y + 1) \leq k\) is true. If the condition is true, `ct` is increased by 1. 

At the end of the previous iteration, we know:
- `nokori` is an integer.
- `y` is \(y + 1\) from the previous iteration.

For the loop to execute one more time, `y` needs to be incremented by 1 from its value at the end of the previous iteration.

Let's denote the value of `y` at the end of the previous iteration as \(y_{\text{prev}}\). Therefore, at the start of the next iteration, `y` will be \(y_{\text{prev}} + 1\).

Since the loop condition \(0 \leq \text{nokori} - (y + 1) \leq k\) must hold true for `ct` to be incremented, we need to ensure that the new value of `y` still satisfies this condition. The condition becomes:
\[ 0 \leq \text{nokori} - ((y_{\text{prev}} + 1) + 1) \leq k \]
which simplifies to:
\[ 0 \leq \text{nokori} - (y_{\text{prev}} + 2) \leq k \]

Given that the loop can execute one more time, the condition must hold true for the new value of `y`.

Therefore, the state at the start of the next iteration should be:
State: **`nokori` is an integer, `y` is \(y_{\text{prev}} + 1\), and the condition \(0 \leq \text{nokori} - (y_{\text{prev}} + 2) \leq k\) must hold true.**