Let's break down the initial state and the print statement step by step:

1. **Initial State:**
   - `k` is decreased by `2 * (tot + a_next)`.
   - `n` is 1.
   - `m` is 1.
   - `pow` is 4.
   - `t` is 1.
   - `tot` is increased by `a_next`.

2. **Variables and Their Values:**
   - `n = 1`
   - `m = 1`
   - `pow = 4`
   - `t = 1`
   - `tot` is increased by `a_next`, so `tot = tot + a_next`.
   - `k` is decreased by `2 * (tot + a_next)`, so `k = k - 2 * (tot + a_next)`.

3. **Expression to Evaluate:**
   - The print statement is `print(pow * (2 * k - 1))`.

4. **Substitute Known Values:**
   - We know `pow = 4`.
   - To find `2 * k - 1`, we need the value of `k`. Since `k` is not explicitly given, let's express it in terms of `tot` and `a_next`:
     \[
     k = k - 2 * (tot + a_next)
     \]
     Let's denote the initial value of `k` as `k_initial`. Then:
     \[
     k = k_{\text{initial}} - 2 * (tot + a_{\text{next}})
     \]

5. **Expression for `2 * k - 1`:**
   \[
   2 * k - 1 = 2 * (k_{\text{initial}} - 2 * (tot + a_{\text{next}})) - 1
   \]
   Simplifying this:
   \[
   2 * k - 1 = 2 * k_{\text{initial}} - 4 * (tot + a_{\text{next}}) - 1
   \]

6. **Final Expression to Print:**
   \[
   \text{print}(4 * (2 * k_{\text{initial}} - 4 * (tot + a_{\text{next}}) - 1))
   \]

Since the exact values of `k_initial` and `a_next` are not provided, we can only express the final printed value in terms of these variables.

Output: **4 * (2 * k_initial - 4 * (tot + a_next) - 1)**