Let's break down the code and apply it step by step to the initial state:

Initial State:
- \( x = 2 \times dx + 2 \times dx \times steps + 2 \times dx + 2 \times dx \times (2 \times steps) \)
- \( y = 2 \times dy + 2 \times dy \times steps + 2 \times dy + 2 \times dy \times (2 \times steps) \)
- \( direction\_index = ((direction\_index + 3) \% 6) \)
- \( n = n - 3 \times steps \) and \( n \) is still greater than 0

Code Block:
```python
dx, dy = directions[direction_index]
x += dx * steps
y += dy * steps
n -= steps
direction_index = (direction_index + 1) \% 6
```

### Step-by-Step Execution:

1. **Line 1: `dx, dy = directions[direction_index]`**
   - This line retrieves the values of `dx` and `dy` based on the current `direction_index`.

2. **Line 2: `x += dx * steps`**
   - This line updates `x` by adding the product of `dx` and `steps` to the current value of `x`.

3. **Line 3: `y += dy * steps`**
   - This line updates `y` by adding the product of `dy` and `steps` to the current value of `y`.

4. **Line 4: `n -= steps`**
   - This line decreases `n` by `steps`.

5. **Line 5: `direction_index = (direction_index + 1) % 6`**
   - This line updates `direction_index` to the next value in the cycle, ensuring it stays within the range [0, 5].

### Calculations:

#### Updated Values of `x` and `y`:
- Original `x`: \( 2 \times dx + 2 \times dx \times steps + 2 \times dx + 2 \times dx \times (2 \times steps) \)
- Updated `x`: \( 2 \times dx + 2 \times dx \times steps + 2 \times dx + 2 \times dx \times (2 \times steps) + dx \times steps \)

- Simplify the expression for `x`:
  \[
  x = 2 \times dx + 2 \times dx \times steps + 2 \times dx + 4 \times dx \times steps + dx \times steps = 2 \times dx + 7 \times dx \times steps + 2 \times dx = 4 \times dx + 7 \times dx \times steps
  \]

- Original `y`: \( 2 \times dy + 2 \times dy \times steps + 2 \times dy + 2 \times dy \times (2 \times steps) \)
- Updated `y`: \( 2 \times dy + 2 \times dy \times steps + 2 \times dy + 2 \times dy \times (2 \times steps) + dy \times steps \)

- Simplify the expression for `y`:
  \[
  y = 2 \times dy + 2 \times dy \times steps + 2 \times dy + 4 \times dy \times steps + dy \times steps = 2 \times dy + 7 \times dy \times steps + 2 \times dy = 4 \times dy + 7 \times dy \times steps
  \]

#### Updated Value of `n`:
- Original `n`: \( n - 3 \times steps \)
- Updated `n`: \( n - 3 \times steps - steps = n - 4 \times steps \)

Since \( n \) is still greater than 0, we keep this condition.

#### Updated Value of `direction_index`:
- Original `direction_index`: \( ((direction_index + 3) \% 6) \)
- Updated `direction_index`: \( (direction_index + 1) \% 6 \)

### Final Output State:
- \( x = 4 \times dx + 7 \times dx \times steps \)
- \( y = 4 \times dy + 7 \times dy \times steps \)
- \( direction\_index = (direction\_index + 1) \% 6 \)
- \( n = n - 4 \times steps \)

Output State: **x is \( 4 \times dx + 7 \times dx \times steps \), y is \( 4 \times dy + 7 \times dy \times steps \), direction_index is \((direction_index + 1) \% 6\), n is \( n - 4 \times steps \)**