Let's break down the code and apply it step by step to the initial state:

### Initial State:
- \( x \) is \( 4 \times dx + 7 \times dx \times steps \)
- \( y \) is \( 4 \times dy + 7 \times dy \times steps \)
- \( direction_index \) is \(((direction_index + 1) \% 6)\)
- \( n \) is \( n - 6 \times steps \)

### Code Execution:
1. **`dx, dy = directions[direction_index]`**
   - This line retrieves the direction values from the `directions` list using the updated `direction_index`.
   - Let's assume `directions` is a predefined list of tuples representing (dx, dy) for each direction. For example, `directions = [(1, 0), (0, 1), (-1, 0), (0, -1), (1, 1), (-1, -1)]`.

2. **`x += dx * n`**
   - This line updates \( x \) by adding \( dx \times n \).
   - From the initial state, \( n \) is already updated to \( n - 6 \times steps \).

3. **`y += dy * n`**
   - This line updates \( y \) by adding \( dy \times n \).
   - From the initial state, \( n \) is already updated to \( n - 6 \times steps \).

### Calculating the Final Values:
Assuming the initial state before the code block is:
- \( x = 4 \times dx + 7 \times dx \times steps \)
- \( y = 4 \times dy + 7 \times dy \times steps \)
- \( n \) is \( n - 6 \times steps \)
- \( direction_index \) is \(((direction_index + 1) \% 6)\)

After executing the code:
- \( dx \) and \( dy \) are updated from the `directions` list based on the new `direction_index`.
- \( x \) is updated by adding \( dx \times n \) to the initial value of \( x \).
- \( y \) is updated by adding \( dy \times n \) to the initial value of \( y \).
- \( n \) is further reduced by \( 6 \times steps \).
- \( direction_index \) is updated to the next direction index in the `directions` list.

Since we don't have specific values for `directions`, `steps`, and `n`, let's assume:
- `directions = [(1, 0), (0, 1), (-1, 0), (0, -1), (1, 1), (-1, -1)]`
- `steps = 1` (for simplicity)

If `direction_index` is initially 0 (meaning \( dx = 1 \) and \( dy = 0 \)):
- \( x = 4 \times 1 + 7 \times 1 \times 1 = 11 \)
- \( y = 4 \times 0 + 7 \times 0 \times 1 = 0 \)
- \( n = n - 6 \times 1 \)

After the code:
- \( dx, dy = (0, 1) \) (since `direction_index` is now 1)
- \( x = 11 + 0 \times (n - 6) = 11 \)
- \( y = 0 + 1 \times (n - 6) = n - 6 \)

### Final Output State:
- \( x \) is 11
- \( y \) is \( n - 6 \)
- \( direction_index \) is 1
- \( n \) is \( n - 6 \)

Output State: **x is 11, y is n - 6, direction_index is 1, n is n - 6**