Output State: **`t` is `T`, `info` is a list of strings obtained from splitting the input, the first element of `info` is an integer `a`, `b` must be at least `2`, `suma` is either `x + 1` or remains `0`, `i` is `3`, `x` is `1`, the current value of `((a - i * (i - 1)) // i) ** 2 + 1` is `a - 6 + 1 = a - 5`**.

Explanation: 
- The value of `t` remains `T`.
- The value of `info` remains a list of strings obtained from splitting the input.
- The first element of `info` is an integer `a`.
- The value of `b` remains at least `2`.
- The value of `suma` remains either `x + 1` or `0`.
- The value of `i` is updated to `3`.
- The value of `x` is calculated as `(a - 1) // 1 + 1 = a`.
- The value of `x` is updated to `1` because `i` is `3` and `x` is recalculated as `(a - 3 * (3 - 1)) // 3 + 1 = (a - 6) // 3 + 1 = a - 6 + 1 = a - 5`.
- The value of `((a - i * (i - 1)) // i) ** 2 + 1` is calculated as `((a - 3 * (3 - 1)) // 3) ** 2 + 1 = ((a - 6) // 3) ** 2 + 1 = (a - 5) ** 2 + 1`.