### Reasoning:

Let's break down the program to understand if it correctly implements the problem statement.

1. **Initialization**:
   - `t` is the number of test cases.
   - For each test case, `n` is the total number of cards and `k` is the position of the card we need to find.

2. **Main Loop**:
   - `s` is initialized to 0. This variable will keep track of the number of cards laid down so far.
   - `m` is initialized to 1. This variable will keep track of the multiplier for the odd numbers (initially 1 for odd numbers, then 2, 3, etc.).

3. **While Loop**:
   - The loop continues as long as `n` is greater than 0.
   - `x` is calculated as `(n + 1) // 2`. This gives the number of odd-numbered cards (or cards that can be formed by multiplying odd numbers by `m`) that are still available.
   - `n` is then halved (`n //= 2`). This step effectively reduces the problem size by considering the next set of cards that are multiples of the next integer.
   - The condition `if s < k and k <= s + x` checks if the `k`-th card lies within the current set of cards being considered (multiples of `m`).
   - If the condition is true, the loop breaks because we have found the set of cards that contains the `k`-th card.
   - Otherwise, `s` is incremented by `x` (the number of cards laid down in this iteration), and `m` is doubled to consider the next set of cards (multiples of `2m`).

4. **Output**:
   - After exiting the loop, the `k`-th card is calculated as `(2 * (k - s) - 1) * m`.
   - This formula correctly identifies the `k`-th card by first finding the position within the current set of cards (`k - s`), converting it to the appropriate card number (`2 * (k - s) - 1`), and then scaling it by the current multiplier `m`.

### Example Walkthrough:

For `n = 7` and `k = 4`:
- Initially, `s = 0`, `m = 1`.
- First iteration: `x = (7 + 1) // 2 = 4`, `n = 7 // 2 = 3`. Since `s < k <= s + x` (0 < 4 <= 4), the loop breaks.
- The `k`-th card is `(2 * (4 - 0) - 1) * 1 = 7`.

For `n = 7` and `k = 5`:
- Initially, `s = 0`, `m = 1`.
- First iteration: `x = (7 + 1) // 2 = 4`, `n = 7 // 2 = 3`. Since `s < k <= s + x` (0 < 5 <= 4) is false, `s = 4`, `m = 2`.
- Second iteration: `x = (3 + 1) // 2 = 2`, `n = 3 // 2 = 1`. Since `s < k <= s + x` (4 < 5 <= 6), the loop breaks.
- The `k`-th card is `(2 * (5 - 4) - 1) * 2 = 2`.

### Conclusion:

The program correctly implements the logic to find the `k`-th card in the sequence as described in the problem statement. It efficiently narrows down the set of cards and calculates the correct card position using the derived formula.

**Correctness: True**