Alright, I've got this problem to solve. Let's see what it's asking for. So, I'm given two positive integers, n and m, and I need to find the number of ordered pairs (a, b) where 1 ≤ a ≤ n and 1 ≤ b ≤ m, with the condition that a + b is a multiple of b multiplied by the greatest common divisor of a and b. That is, a + b should be divisible by b * gcd(a, b).

First, I need to understand what this condition means. Let's break it down. GCD stands for Greatest Common Divisor, which is the largest positive integer that divides both a and b without leaving a remainder. So, gcd(a, b) is that number.

The condition is that a + b should be divisible by b * gcd(a, b). In mathematical terms, this means that b * gcd(a, b) divides a + b without leaving a remainder.

Let me try to simplify this condition. Maybe there's a way to express this in a more manageable form.

Let’s denote d = gcd(a, b). Then, a can be written as a = d * a1, and b can be written as b = d * b1, where gcd(a1, b1) = 1. This is because d is the greatest common divisor of a and b.

Substituting these into the condition:

a + b = d * a1 + d * b1 = d * (a1 + b1)

And b * gcd(a, b) = d * b1 * d = d^2 * b1

So, the condition becomes:

d * (a1 + b1) should be divisible by d^2 * b1.

In other words, d * (a1 + b1) is divisible by d^2 * b1.

We can simplify this by dividing both sides by d (since d is not zero):

(a1 + b1) is divisible by d * b1.

But we know that gcd(a1, b1) = 1, which might help in further simplification.

Wait a minute, since a1 and b1 are coprime, meaning they have no common divisors other than 1, this could be useful.

Let’s see, if a1 and b1 are coprime, and d * b1 divides (a1 + b1), what does that imply?

Since b1 divides (a1 + b1), and gcd(a1, b1) = 1, then b1 must divide a1 + b1.

But a1 + b1 is equal to a1 + b1, which is the same as a1 + b1.

Wait, that seems obvious. Maybe I need to think differently.

Let’s consider that b1 divides a1 + b1. Since b1 divides b1, and b1 divides a1 + b1, then b1 divides a1.

But hold on, gcd(a1, b1) = 1, which means that b1 cannot divide a1 unless b1 = 1.

Wait, that seems contradictory. If b1 divides a1, and gcd(a1, b1) = 1, then b1 must be 1.

So, this suggests that b1 = 1.

If b1 = 1, then b = d * b1 = d * 1 = d.

And a = d * a1.

Also, since b1 = 1, and b1 divides a1 + b1, which is a1 + 1.

But b1 = 1, and 1 divides any integer, so this condition is always true when b1 = 1.

Therefore, the only time the condition holds is when b1 = 1.

Which means that b = d, where d = gcd(a, b).

But since d divides a, and b = d, then a must be a multiple of b.

Wait, a = d * a1, and b = d.

So, a is a multiple of b, because a = a1 * b.

Therefore, the condition a + b is a multiple of b * gcd(a, b) simplifies to a being a multiple of b.

Wait, is that correct?

Let me verify.

If a is a multiple of b, then a = k * b for some integer k.

Then, a + b = k * b + b = b * (k + 1).

And b * gcd(a, b) = b * gcd(k * b, b) = b * b, since gcd(k * b, b) = b.

So, a + b = b * (k + 1), and b * gcd(a, b) = b * b.

So, for a + b to be divisible by b * b, we need b * (k + 1) to be divisible by b * b.

Which simplifies to (k + 1) being divisible by b.

So, actually, the condition is that (k + 1) is divisible by b.

But k = a / b, so k is an integer since a is a multiple of b.

So, k + 1 is an integer, and we need k + 1 to be divisible by b.

Which means that k + 1 is a multiple of b.

So, k + 1 = m * b for some integer m.

Therefore, k = m * b - 1.

Substituting back, a = k * b = (m * b - 1) * b = m * b^2 - b.

So, a = m * b^2 - b.

Wait, this seems complicated. Maybe there's a better way to approach this.

Let me try to think differently.

Given that a + b is divisible by b * gcd(a, b), and we've established that a must be a multiple of b, but with some additional constraints.

Maybe I should iterate over possible values of b and find corresponding a that satisfy the condition.

Given that b can range from 1 to m, and for each b, a can range from 1 to n, with a being a multiple of b, and possibly some other conditions.

Wait, perhaps I need to find all pairs (a, b) where a is a multiple of b, and a + b is divisible by b * gcd(a, b).

But from earlier, if a is a multiple of b, then gcd(a, b) = b.

Wait, is that correct?

If a is a multiple of b, then gcd(a, b) = b.

Yes, because b divides a, so the greatest common divisor is b.

So, in that case, b * gcd(a, b) = b * b = b^2.

And a + b = k * b + b = b * (k + 1).

So, for a + b to be divisible by b^2, we need b * (k + 1) to be divisible by b^2.

Which simplifies to (k + 1) being divisible by b.

So, k + 1 must be a multiple of b.

Therefore, k = m * b - 1 for some integer m.

Thus, a = k * b = (m * b - 1) * b = m * b^2 - b.

So, a must be of the form m * b^2 - b, for some positive integer m, such that a is between 1 and n.

Wait, but a has to be at least 1, so m * b^2 - b >= 1.

Which implies m >= (1 + b) / b^2.

But b is at least 1, so m >= (1 + b) / b^2.

But m must be an integer, so m >= ceil((1 + b) / b^2).

But b^2 grows faster than b, so for b >= 1, (1 + b) / b^2 is less than or equal to 2.

For b = 1, (1 + 1)/1^2 = 2.

For b = 2, (1 + 2)/4 = 0.75, so m >= 1.

For b = 3, (1 + 3)/9 = 4/9 ≈ 0.44, so m >= 1.

And so on.

Therefore, for each b from 1 to m, and for m >= ceil((1 + b)/b^2), a = m * b^2 - b, and a <= n.

So, for each b, I need to find the number of integers m such that a = m * b^2 - b <= n, and a >= 1.

So, m * b^2 - b <= n.

Thus, m <= (n + b) / b^2.

And since m must be at least ceil((1 + b)/b^2), which is mostly 1 for b >= 1.

So, for each b, the number of valid m is floor((n + b)/b^2) - ceil((1 + b)/b^2) + 1.

But for b = 1, ceil((1 + 1)/1^2) = ceil(2/1) = 2.

Floor((n + 1)/1) = n + 1.

So, number of m for b=1 is n + 1 - 2 + 1 = n.

But a = m * 1^2 - 1 = m - 1.

So, a ranges from 1 to n when m ranges from 2 to n + 1.

Wait, but a = m - 1, and a >=1, so m -1 >=1 => m >=2.

And a <=n, so m -1 <=n => m <=n +1.

So, m from 2 to n+1, which is n elements, matching the earlier calculation.

For b=2, ceil((1+2)/4) = ceil(3/4) = 1.

Floor((n + 2)/4).

So, number of m is floor((n + 2)/4) - 1 + 1 = floor((n + 2)/4).

And a = m * 4 - 2.

So, a >=1: m * 4 -2 >=1 => m >= (3)/4, so m >=1.

But m starts from 1.

So, seems consistent.

Similarly, for each b, m starts from floor((1 + b)/b^2) up to floor((n + b)/b^2).

But since (1 + b)/b^2 is less than or equal to 2 for b=1 and less than 1 for b>=2, we can set m starting from 1 for b>=2, and from 2 for b=1.

But to generalize, perhaps it's better to iterate over b from 1 to m, and for each b, compute the number of m such that a = m * b^2 - b <=n and a >=1.

Which is floor((n + b)/b^2) - ceil((1 + b)/b^2) + 1.

But handling ceil and floor might be tricky.

Alternatively, we can iterate over b from 1 to m, and for each b, find the maximum m such that a = m * b^2 - b <=n and a >=1.

Then sum over all b from 1 to m of the number of such m.

But this seems computationally intensive if n and m are up to 2*10^6, and t is up to 10^4.

Wait, but the constraints say that the sum of n and m over all test cases doesn't exceed 2*10^6.

So, we need an algorithm that is linear or near-linear in the sum of n and m.

Meaning, per test case, the time should be proportional to n + m, but since t can be up to 10^4, and n and m up to 2*10^6, but sum over all test cases n and m up to 2*10^6, so per test case, n and m can be up to 2*10^6, but total over all test cases, sum of n and m is up to 2*10^6.

Wait, no. The problem says "It is guaranteed that neither the sum of n nor the sum of m over all test cases exceeds 2*10^6."

Meaning, sum of all n across test cases <=2*10^6, and sum of all m across test cases <=2*10^6.

So, in total, across all test cases, we have sum of n <=2*10^6 and sum of m <=2*10^6.

Therefore, we can have t=10^4 test cases, each with n and m up to 2*10^6, but sum of n and sum of m across all test cases <=2*10^6.

So, per test case, n and m can be up to 2*10^6, but we have to process t test cases efficiently.

Given that, we need an algorithm that is efficient per test case.

Now, going back to the earlier approach, for each b from 1 to m, compute the number of m such that a = m * b^2 - b <=n and a >=1.

Let’s see, a = m * b^2 - b >=1 => m * b^2 >= b +1 => m >= (b +1)/b^2.

And a <=n => m * b^2 - b <=n => m <= (n + b)/b^2.

So, m needs to be an integer such that ceil((b +1)/b^2) <= m <= floor((n + b)/b^2).

Then, the number of valid m for each b is floor((n + b)/b^2) - ceil((b +1)/b^2) +1.

Now, for b=1:

ceil((1 +1)/1^2) = ceil(2/1) =2

floor((n +1)/1) = n +1

So, number of m = n +1 -2 +1 = n

Which makes sense, as a = m *1 -1 = m -1, and a from 1 to n requires m from 2 to n+1, which is n elements.

For b=2:

ceil((2 +1)/4) = ceil(3/4) =1

floor((n +2)/4)

So, number of m = floor((n +2)/4) -1 +1 = floor((n +2)/4)

Which is correct.

Similarly, for b=3:

ceil((3 +1)/9) = ceil(4/9) =1

floor((n +3)/9)

Number of m = floor((n +3)/9) -1 +1 = floor((n +3)/9)

And so on.

So, in general, for each b from 1 to m, the number of valid m is floor((n + b)/b^2) - ceil((b +1)/b^2) +1.

But for b >=1, ceil((b +1)/b^2) is either 1 or 2, depending on b.

Specifically, for b=1, ceil(2/1)=2

For b=2, ceil(3/4)=1

For b=3, ceil(4/9)=1

And so on.

So, perhaps it's better to handle b=1 separately, and for b >=2, use floor((n + b)/b^2).

Wait, for b=1, number of m is n, which is floor((n +1)/1) - ceil((1 +1)/1) +1 = (n +1) -2 +1 = n

For b=2, floor((n +2)/4) - ceil(3/4) +1 = floor((n +2)/4) -1 +1 = floor((n +2)/4)

Which is correct.

Similarly for b=3: floor((n +3)/9) - ceil(4/9) +1 = floor((n +3)/9) -1 +1 = floor((n +3)/9)

So, in general, for b >=1, the number of m is floor((n + b)/b^2) - ceil((b +1)/b^2) +1.

But ceil((b +1)/b^2) can be simplified.

Let’s see:

For b >=2, b^2 >=4, and b +1 <= b^2 for b >=2.

So, (b +1)/b^2 <=1, and since b +1 <= b^2, ceil((b +1)/b^2) =1 for b >=2.

For b=1, ceil(2/1)=2.

Therefore, for b >=2, ceil((b +1)/b^2)=1, and for b=1, it's 2.

So, the general formula is:

For b from 1 to m:

If b=1:

number of m = floor((n +1)/1) -2 +1 = n

Else:

number of m = floor((n + b)/b^2) -1 +1 = floor((n + b)/b^2)

So, total number of pairs is:

For b=1: n

For b>=2: sum over b=2 to m of floor((n + b)/b^2)

Wait, but for b=1, a = m -1, and m from 2 to n+1, which gives a from 1 to n.

So, for b=1, it's simply n.

For b>=2, it's sum over b=2 to m of floor((n + b)/b^2)

So, total pairs = n + sum_{b=2 to m} floor((n + b)/b^2)

But wait, in the earlier example, for n=10, m=8, the output is 14.

Let's verify:

For b=1: n=10, so 10 pairs.

For b=2: floor((10 +2)/4) = floor(12/4)=3

b=3: floor((10 +3)/9)=floor(13/9)=1

b=4: floor((10 +4)/16)=floor(14/16)=0

b=5: floor((10 +5)/25)=floor(15/25)=0

b=6: floor((10 +6)/36)=floor(16/36)=0

b=7: floor((10 +7)/49)=floor(17/49)=0

b=8: floor((10 +8)/64)=floor(18/64)=0

So, sum for b=2 to 8 is 3 +1 +0 +0 +0 +0 +0 =4

Total pairs: 10 +4=14, which matches the sample output.

Good, so the formula seems correct.

Therefore, the total number of pairs is n + sum_{b=2 to m} floor((n + b)/b^2)

Now, I need to implement this efficiently.

Given that n and m can be up to 2*10^6, and t up to 10^4, but sum of n and m across all test cases is up to 2*10^6, I need an efficient way to compute this.

One way is to iterate over b from 2 to m, and compute floor((n + b)/b^2) for each b, and sum them up, then add n.

But this would be O(m) per test case, which could be acceptable since sum over m across all test cases is up to 2*10^6.

Alternatively, I can optimize the computation of sum_{b=2 to m} floor((n + b)/b^2)

Let’s see if I can find a way to compute this sum more efficiently.

Let’s denote s = sum_{b=2 to m} floor((n + b)/b^2)

We can observe that for large b, b^2 will be much larger than n + b, so floor((n + b)/b^2) will be 0.

So, only for b such that b^2 <= n + b, which is approximately b <= sqrt(n)

More precisely, b^2 <= n + b => b^2 - b - n <=0

Solving b^2 - b - n <=0, the roots are b = (1 ± sqrt(1 + 4n))/2

So, b <= (1 + sqrt(1 + 4n))/2

But for practical purposes, b is up to sqrt(n), since b^2 grows faster than n.

Therefore, the number of terms in the sum is up to sqrt(n), which is acceptable for n up to 2*10^6, as sqrt(2*10^6) is about 1414, so per test case, it's O(sqrt(n))

Adding to that, for b=1, we have n, which is O(1)

So, overall complexity per test case is O(sqrt(n) + m), but since m can be up to 2*10^6, and sum over all m across test cases is up to 2*10^6, it should be manageable.

But wait, m can be up to 2*10^6 per test case, but sum over all m across test cases is up to 2*10^6, so per test case, m can be up to 2*10^6, but with t up to 10^4, the total sum of m is up to 2*10^6.

Therefore, it's acceptable to have O(m) per test case, as long as the total time is acceptable.

But to optimize further, perhaps I can find a mathematical formula to compute the sum without iterating over each b.

Let’s see.

sum_{b=2 to m} floor((n + b)/b^2)

Let’s denote k = floor((n + b)/b^2)

Which is equal to floor((n + b)/b^2)

Let’s see if I can find a better way to compute this sum.

Alternatively, perhaps I can iterate over b in groups where floor((n + b)/b^2) is constant.

This is similar to the method used in computing the number of divisors up to a certain value, where you iterate over possible divisors and compute the range where the quotient is constant.

Similarly, here, I can iterate over possible values of b such that floor((n + b)/b^2) remains constant.

Let’s denote q = floor((n + b)/b^2)

Then, for a given q, find the range of b where q remains the same.

But this seems a bit complicated.

Alternatively, perhaps I can iterate over b from 2 to m, compute floor((n + b)/b^2), and sum them up.

Given that m can be up to 2*10^6 per test case, and t up to 10^4, but sum over all m across test cases is up to 2*10^6, it should be manageable with optimized code.

I need to make sure that the code runs efficiently, perhaps using fast input methods, and minimizing the number of operations per test case.

Now, looking at the provided program, it seems to be a part of a larger codebase, with multiple functions defined, but the relevant function is func_15(), which seems to implement the logic for computing the number of valid pairs for a single test case.

Let’s look at func_15():

def func_15():

(n, m) = func_7()

i = 1

ans = 0

while i <= m and i * i <= n + i:

ans += (n + i) // (i * i)

i += 1

return ans - 1

And func_16() calls func_15() for each test case.

Wait, but according to our earlier reasoning, for b=1, the number of a is n, and for b>=2, it's sum_{b=2 to m} floor((n + b)/b^2)

But in the code, it iterates i from 1 to m, and adds (n + i) // (i * i) to ans, and finally returns ans -1.

Wait, in our formula, for b=1, it's n, and for b>=2, it's sum_{b=2 to m} floor((n + b)/b^2)

But in the code, it iterates i from 1 to m, and adds floor((n + i)/i^2) each time, and then subtracts 1 at the end.

So, let's see:

sum_{i=1 to m} floor((n + i)/i^2) -1

But according to our formula, it should be n + sum_{b=2 to m} floor((n + b)/b^2)

But in the code, it's sum_{i=1 to m} floor((n + i)/i^2) -1

Wait, perhaps the -1 is to compensate for the inclusion of b=1.

Let’s see:

sum_{i=1 to m} floor((n + i)/i^2) = floor((n +1)/1) + sum_{i=2 to m} floor((n + i)/i^2)

Which is n +1 + sum_{i=2 to m} floor((n + i)/i^2)

But according to our formula, it should be n + sum_{b=2 to m} floor((n + b)/b^2)

So, the code is computing n +1 + sum_{i=2 to m} floor((n + i)/i^2) -1 = n + sum_{i=2 to m} floor((n + i)/i^2)

Which matches our formula.

Therefore, the code is correct.

Wait, but in the code, it's returning ans -1, where ans is sum_{i=1 to m} floor((n + i)/i^2)

According to the above, sum_{i=1 to m} floor((n + i)/i^2) = (n +1) + sum_{i=2 to m} floor((n + i)/i^2)

But according to our formula, we need n + sum_{b=2 to m} floor((n + b)/b^2)

So, sum_{i=1 to m} floor((n + i)/i^2) -1 = n + sum_{i=2 to m} floor((n + i)/i^2)

Which matches our formula.

Hence, the code is correct.

Additionally, in the code, it iterates i from 1 to m, but with a condition i <= m and i * i <= n + i.

Wait, why is there a condition i * i <= n + i?

Let’s see, i * i <= n + i => i * i - i <= n => i*(i -1) <=n

For i >=1, this condition is true up to a certain i, beyond which i*(i -1) > n.

So, it's optimizing the loop by stopping early when i * i > n + i, which is a valid optimization since floor((n + i)/i^2) would be 0 beyond that point.

Therefore, the code is correct.

Hence, Correctness: **True**

**Final Answer**

\[ \boxed{\text{see explanation}} \]