`cur` is decremented by 1. The value of `cur` was such that `(cur % 2 == 0)` is not equal to `(c == '1')`. After decrementing, the condition `(cur % 2 == 0)` will still not be equal to `(c == '1')` because we only changed the value of `cur` and did not modify `c`. Therefore, the output state is: `s` is a non-empty string, `(cur % 2 == 0)` is not equal to `(c == '1')`, `cur` is decreased by 1.

Output State: **`s` is a non-empty string, `(cur % 2 == 0)` is not equal to `(c == '1')`, `cur` is decreased by 1**