Let's analyze the given code block step by step to determine the final state of the variables.

### Initial State:
- `n` is a positive integer equal to its original value minus `min(k, candies)`.
- `vasya_eaten` is `min(k, candies)`.
- `petya_eaten` is `candies // 10`.
- `candies` must be greater than 0.

### Code Block:
```python
vasya_eaten += min(k, candies)
candies -= min(k, candies)
petya_eaten = candies // 10
candies -= petya_eaten
```

#### Line 1: `vasya_eaten += min(k, candies)`
- This line adds `min(k, candies)` to `vasya_eaten`.
- From the initial state, `vasya_eaten` is `min(k, candies)`.
- After this line, `vasya_eaten` becomes `2 * min(k, candies)`.

#### Line 2: `candies -= min(k, candies)`
- This line subtracts `min(k, candies)` from `candies`.
- From the initial state, `candies` is greater than 0.
- After this line, `candies` becomes `candies - min(k, candies)`.

#### Line 3: `petya_eaten = candies // 10`
- This line sets `petya_eaten` to `candies // 10`.
- After the previous line, `candies` is now `candies - min(k, candies)`.
- Therefore, `petya_eaten` is `(candies - min(k, candies)) // 10`.

#### Line 4: `candies -= petya_eaten`
- This line subtracts `petya_eaten` from `candies`.
- From the previous line, `petya_eaten` is `(candies - min(k, candies)) // 10`.
- After this line, `candies` becomes `candies - (candies - min(k, candies)) // 10`.

### Final State Calculation:
- Let's denote `min(k, candies)` as `m` for simplicity.
- Initially, `vasya_eaten = m`.
- After the first line, `vasya_eaten = 2m`.
- After the second line, `candies = candies - m`.
- After the third line, `petya_eaten = (candies - m) // 10`.
- After the fourth line, `candies = candies - (candies - m) // 10`.

Given that `candies` is initially greater than 0 and we are subtracting a value from it, letâ€™s assume `candies` starts at some value \( C \). Then:
- After the second line, `candies = C - m`.
- `petya_eaten = (C - m) // 10`.
- After the fourth line, `candies = (C - m) - ((C - m) // 10)`.

Let's simplify the final expression for `candies`:
- `candies = (C - m) - (C - m) // 10`.
- `candies = (C - m) - (C // 10 - m // 10)`.
- `candies = C - m - C // 10 + m // 10`.
- `candies = C - C // 10 - m + m // 10`.

Since `m = min(k, candies)`, the final value of `candies` will depend on the exact initial value of `candies` and `k`.

### Output State:
- `n` remains unchanged as no operations were performed on `n`.
- `vasya_eaten` becomes `2 * min(k, candies)`.
- `petya_eaten` becomes `(candies - min(k, candies)) // 10`.
- `candies` becomes `candies - (candies - min(k, candies)) // 10`.

Output State: **n is a positive integer equal to its original value minus min(k, candies), vasya_eaten is 2 * min(k, candies), petya_eaten is (candies - min(k, candies)) // 10, and candies becomes candies - (candies - min(k, candies)) // 10**