Let's break down the given state and the for loop step by step to determine the necessary adjustments for the next iteration.

### Given State at the End of the Previous Iteration
- \( a \) is such that \( l \leq a + 1 < r \)
- There does not exist an integer \( b \) such that \( b = b_end + 1 \) and \( b_end + 2 < b \leq r \) and \( \text{func\_5}(r, b) == 1 \) and \( \text{func\_5}(b, b_end + 1) != 1 \), and \( a + 1 < r \) and \( (\text{func\_5}(r, b_end + 1) != 1 \text{ or } \text{func\_5}(b_end + 1, a) == 1) \)
- \( b = b_end + 1 \)
- If \( \text{func\_5}(r, b) == 1 \) and \( \text{func\_5}(b, a) != 1 \), no changes are made to \( a \) and \( b \).

### For Loop
```
for b in range(a + 1, r + 1):
    # the loop body is omitted
```

### Analysis
1. **Loop Condition**: The loop runs from \( a + 1 \) to \( r \). Since \( b = b_end + 1 \) and we don't know if this value of \( b \) was updated during the loop, we need to consider the range \( [a + 1, r] \).
2. **Update of `b`**: The loop updates \( b \) as it iterates through the range \( [a + 1, r] \). Therefore, \( b \) will increment by 1 in each iteration.
3. **Condition for Next Iteration**: The loop continues until \( b \) reaches \( r \).

### Step-by-Step Adjustment
- **Initial Value of `b`**: From the given state, \( b = b_end + 1 \).
- **Next Value of `b`**: Since the loop runs from \( a + 1 \) to \( r \), the next value of \( b \) will be \( b + 1 \).
- **State Adjustments**:
  - \( b \) will be incremented to \( b + 1 \).
  - The loop will continue as long as \( b < r \).

### Conclusion
The state at the start of the next iteration of the loop should reflect the updated value of \( b \).

### Final Answer
State: **\( a \) is such that \( l \leq a + 1 < r \) and there does not exist an integer \( b \) such that \( b = b_end + 2 \) and \( b_end + 3 < b \leq r \) and \( \text{func\_5}(r, b) == 1 \) and \( \text{func\_5}(b, b_end + 1) != 1 \), and \( a + 1 < r \) and \( (\text{func\_5}(r, b_end + 1) != 1 \text{ or } \text{func\_5}(b_end + 1, a) == 1) \), and \( b = b_end + 2 \)**.