Let's break down the initial state and the print statement step by step:

1. **Initial State:**
   - `p1`, `p2`, and `p3` are integers provided by user input.
   - `p1` ≤ `p2` ≤ `p3` ≤ 30.
   - The sum of `p1`, `p2`, and `p3` is odd.
   - `t` is greater than 2.
   - `_` is 2.
   - `x` is 1.
   - `y` is `p3 - 1`.

2. **Print Statement:**
   ```python
   print(p1 - x + p3)
   ```

3. **Explanation:**
   - `p1` is an integer such that `p1` ≤ `p2` ≤ `p3` ≤ 30.
   - `x` is explicitly given as 1.
   - `p3` is an integer such that `p1` ≤ `p2` ≤ `p3` ≤ 30.
   - The expression `p1 - x + p3` simplifies to `p1 - 1 + p3`.

4. **Output Calculation:**
   - The value of `p1 - 1 + p3` will be printed.
   - Since `p1` and `p3` are integers and `x` is 1, the expression `p1 - 1 + p3` will result in an integer value.

5. **Final Output:**
   - The exact numerical value of `p1 - 1 + p3` cannot be determined without knowing the specific values of `p1` and `p3`, but we can describe it based on the given conditions.
   - The output will be the result of the expression `p1 - 1 + p3`.

Output: **p1 - 1 + p3 (where p1 and p3 are integers such that p1 ≤ p2 ≤ p3 ≤ 30 and the sum of p1, p2, and p3 is odd)**