To determine the new value of `t` after executing the given code snippet, we need to follow the calculation step-by-step:

Given:
- `t` is initially calculated based on whether it's even or odd.
- `a` is the first integer from the input.
- `b` is the second integer from the input.
- `n` is greater than 0.
- For each of the `t` test cases, there are two integers `x` and `y` such that 0 ≤ `x`, `y` ≤ 99.
- `i` is `i + 1`.
- `t1` is `t * 15 - b * 4`.
- `t2` is `a - (t * 15 - b * 4)`.

The code snippet modifies `t` as follows:
```python
t = t + t2 // 15 + 1
```

Let's substitute the expression for `t2` into the equation:
```python
t = t + (a - (t * 15 - b * 4)) // 15 + 1
```

Simplifying the expression inside the parentheses:
```python
t = t + (a - t * 15 + b * 4) // 15 + 1
```

Distributing the division by 15:
```python
t = t + (a // 15 - t + b * 4 // 15) + 1
```

Combining like terms:
```python
t = t + a // 15 - t + b * 4 // 15 + 1
t = a // 15 + b * 4 // 15 + 1
```

So, the new value of `t` is:
```python
t = a // 15 + b * 4 // 15 + 1
```

The other variables (`a`, `b`, `n`, `i`, `t1`, `t2`) remain unchanged.

Output State: **`t` is `a // 15 + b * 4 // 15 + 1`, `a` is the first integer from the input, `b` is the second integer from the input, `n` is greater than 0, for each of the `t` test cases, there are two integers `x` and `y` such that 0 ≤ `x`, `y` ≤ 99, `i` is `i + 1`, `t1` is `t * 15 - b * 4`, `t2` is `a - (t * 15 - b * 4)`**.