`ans` is updated by adding the value of `(3 - a % 3 + b % 3) % 3` to its current value. Given the initial state, we know that `a` is a positive integer, `b` is a positive integer, and `c` is a non-negative integer such that \(0 \leq c \leq 10^9\). The value of `ans` starts at 0.

Let's break down the expression `(3 - a % 3 + b % 3) % 3`:

1. `a % 3` gives the remainder when `a` is divided by 3. Since `a` is a positive integer, `a % 3` can be 0, 1, or 2.
2. `b % 3` gives the remainder when `b` is divided by 3. Similarly, `b % 3` can be 0, 1, or 2.

Combining these, the expression `3 - a % 3 + b % 3` can take on several values depending on the remainders of `a` and `b` when divided by 3:

- If `a % 3` is 0 and `b % 3` is 0, then `3 - 0 + 0 = 3`, and `3 % 3 = 0`.
- If `a % 3` is 0 and `b % 3` is 1, then `3 - 0 + 1 = 4`, and `4 % 3 = 1`.
- If `a % 3` is 0 and `b % 3` is 2, then `3 - 0 + 2 = 5`, and `5 % 3 = 2`.
- If `a % 3` is 1 and `b % 3` is 0, then `3 - 1 + 0 = 2`, and `2 % 3 = 2`.
- If `a % 3` is 1 and `b % 3` is 1, then `3 - 1 + 1 = 3`, and `3 % 3 = 0`.
- If `a % 3` is 1 and `b % 3` is 2, then `3 - 1 + 2 = 4`, and `4 % 3 = 1`.
- If `a % 3` is 2 and `b % 3` is 0, then `3 - 2 + 0 = 1`, and `1 % 3 = 1`.
- If `a % 3` is 2 and `b % 3` is 1, then `3 - 2 + 1 = 2`, and `2 % 3 = 2`.
- If `a % 3` is 2 and `b % 3` is 2, then `3 - 2 + 2 = 3`, and `3 % 3 = 0`.

Given these possible values, we can summarize the expression as follows:

- If `a % 3` is 0, `b % 3` is 0, then `ans += 0`.
- If `a % 3` is 0, `b % 3` is 1, then `ans += 1`.
- If `a % 3` is 0, `b % 3` is 2, then `ans += 2`.
- If `a % 3` is 1, `b % 3` is 0, then `ans += 2`.
- If `a % 3` is 1, `b % 3` is 1, then `ans += 0`.
- If `a % 3` is 1, `b % 3` is 2, then `ans += 1`.
- If `a % 3` is 2, `b % 3` is 0, then `ans += 1`.
- If `a % 3` is 2, `b % 3` is 1, then `ans += 2`.
- If `a % 3` is 2, `b % 3` is 2, then `ans += 0`.

Since `ans` starts at 0, the value of `ans` after the operation will depend on the specific values of `a % 3` and `b % 3`. However, the output state will include the updated value of `ans` based on the above calculations.

Output State: **`a` is a positive integer, `b` is a positive integer, `c` is a non-negative integer such that \(0 \leq c \leq 10^9\), `ans` is the value calculated from `(3 - a % 3 + b % 3) % 3` added to the initial value of `ans` (which was 0)**.