Output State: **`suma` is increased by 1, `b` must be at least 1, `x` is `(a - i * (i - 1)) // i`, and the value of `x` is such that `((a - i * (i - 1)) % i ** 2 == 0 and i * (i - 1) % i ** 2 == 0)`**.

Explanation: The code `suma += 1` increments the value of `suma` by 1. The other conditions and the value of `x` remain unchanged from the initial state. Therefore, `b` must still be at least 1, `x` is still defined as `(a - i * (i - 1)) // i`, and `x` must satisfy the condition `((a - i * (i - 1)) % i ** 2 == 0 and i * (i - 1) % i ** 2 == 0)`.