The code snippet `c[i] = c[i - 1] + d[i]` updates the value of `c[i]` by adding the value of `d[i]` to `c[i - 1]`. Given the initial state:

- `n` is an integer where \(2 \leq n \leq 2000\)
- `a` is a list of `n` distinct integers where \(1 \leq a_i \leq 5000\)
- `d` is a list of 5000 integers
- `c` is a list of 5000 elements where `c[1] = d[1]` and the rest are zeros
- `i` is 2

The value of `c[2]` is updated to `c[1] + d[2]`. Since `c[1] = d[1]`, the new value of `c[2]` is `d[1] + d[2]`.

Therefore, the output state is:
Output State: **`n` is an integer where \(2 \leq n \leq 2000\), `a` is a list of `n` distinct integers where \(1 \leq a_i \leq 5000\), `d` is a list of 5000 integers, `c` is a list of 5000 elements where `c[1] = d[1]` and `c[2] = d[1] + d[2]` and the rest are zeros, `i` is 2**