The value of `c[i]` is updated to be the sum of `c[i - 1]` and `d[i]`. Given that `i` is 3, this means `c[3]` is set to `c[2] + d[3]`.

From the initial state, we know:
- `c[1] = d[1]`
- `c[2] = d[1] + d[2]`

Therefore, `c[3]` will be:
- `c[3] = c[2] + d[3]`
- `c[3] = (d[1] + d[2]) + d[3]`
- `c[3] = d[1] + d[2] + d[3]`

All other variables remain unchanged.

Output State: **`n` is an integer where \(2 \leq n \leq 2000\), `a` is a list of `n` distinct integers where \(1 \leq a_i \leq 5000\), `d` is a list of 5000 integers, `c` is a list of 5000 elements where `c[1] = d[1]`, `c[2] = d[1] + d[2]`, and `c[3] = d[1] + d[2] + d[3]`, the rest of `c` are zeros, `i` is 3**