The given code snippet updates the variable `ans` by adding to it the value of the expression `d[i] / m * (d[j] / m) * (c[i - j - 1] / m)`.

- `ans` was initially \((d[4999] / m) * (d[0] / m) * (c[4998] / m)\).
- `i` is 4999.
- `j` is 1.
- `m` is the sum of all elements in `d` as a float.
- `c` is a list of 5000 elements where `c[0]` is 0 and for \(1 \leq i \leq 4999\), `c[i]` is the cumulative sum of `d` from `d[1]` to `d[i]`.

The new value of `ans` is calculated as follows:
\[ \text{new\_ans} = \text{old\_ans} + \frac{d[4999]}{m} * \left(\frac{d[1]}{m}\right) * \left(\frac{c[4997]}{m}\right) \]

Therefore, the updated value of `ans` is:
\[ \text{ans} = \left(\frac{d[4999]}{m} * \frac{d[0]}{m} * \frac{c[4998]}{m}\right) + \left(\frac{d[4999]}{m} * \frac{d[1]}{m} * \frac{c[4997]}{m}\right) \]

All other variables remain unchanged.

Output State: **`n` is an integer where \(2 \leq n \leq 2000\), `a` is a list of `n` distinct integers where \(1 \leq a_i \leq 5000\), `d` is a list of 5000 integers, `c` is a list of 5000 elements where `c[0]` is 0 and for \(1 \leq i \leq 4999\), `c[i]` is the cumulative sum of `d` from `d[1]` to `d[i]`, `i` is 4999, `ans` is \(\left(\frac{d[4999]}{m} * \frac{d[0]}{m} * \frac{c[4998]}{m}\right) + \left(\frac{d[4999]}{m} * \frac{d[1]}{m} * \frac{c[4997]}{m}\right)\), `m` is the sum of all elements in `d` as a float, `j` is 1**