The given code snippet updates the value of `ans` using the formula:

\[ \text{ans} += \frac{d[i]}{m} \times \left(\frac{d[j]}{m}\right) \times \left(\frac{c[i - j - 1]}{m}\right) \]

Given the initial state:
- `n` is an integer where \(2 \leq n \leq 2000\)
- `a` is a list of `n` distinct integers where \(1 \leq a_i \leq 5000\)
- `d` is a list of 5000 integers
- `c` is a list of 5000 elements where `c[0]` is 0 and for \(1 \leq i \leq 4999\), `c[i]` is the cumulative sum of `d` from `d[1]` to `d[i]`
- `i` is 4998
- `ans` is the sum of \(\left(\frac{d[4999]}{m} * \frac{d[j]}{m} * \frac{c[4999 - j - 1]}{m}\right)\) for all \(0 \leq j < 4999\) where `d[j]` is not 0
- `m` is the sum of all elements in `d` as a float
- `j` is 0

The code snippet modifies `ans` by adding the value of the expression:

\[ \frac{d[4998]}{m} \times \left(\frac{d[0]}{m}\right) \times \left(\frac{c[4997]}{m}\right) \]

Let's break down the calculation:

1. **Calculate each term in the expression:**
   - \(\frac{d[4998]}{m}\)
   - \(\frac{d[0]}{m}\)
   - \(\frac{c[4997]}{m}\)

2. **Combine these terms:**
   - \(\frac{d[4998]}{m} \times \left(\frac{d[0]}{m}\right) \times \left(\frac{c[4997]}{m}\right)\)

3. **Add this result to `ans`:**

Let's denote the original value of `ans` as \( \text{ans}_{\text{original}} \). The new value of `ans` will be:

\[ \text{ans}_{\text{new}} = \text{ans}_{\text{original}} + \left( \frac{d[4998]}{m} \times \frac{d[0]}{m} \times \frac{c[4997]}{m} \right) \]

Therefore, the updated state is:

Output State: **`n` is an integer where \(2 \leq n \leq 2000\), `a` is a list of `n` distinct integers where \(1 \leq a_i \leq 5000\), `d` is a list of 5000 integers, `c` is a list of 5000 elements where `c[0]` is 0 and for \(1 \leq i \leq 4999\), `c[i]` is the cumulative sum of `d` from `d[1]` to `d[i]`, `i` is 4998, `ans` is the sum of \(\left(\frac{d[4999]}{m} * \frac{d[j]}{m} * \frac{c[4999 - j - 1]}{m}\right)\) for all \(0 \leq j < 4999\) where `d[j]` is not 0 plus \(\left(\frac{d[4998]}{m} * \frac{d[0]}{m} * \frac{c[4997]}{m}\right)\), `m` is the sum of all elements in `d` as a float, `j` is 0**.