The code snippet updates the value of `ans` using the formula `ans += d[i] / m * (d[j] / m) * (c[i - j - 1] / m)`.

Given:
- `n` is an integer where \(2 \leq n \leq 2000\)
- `a` is a list of `n` distinct integers where \(1 \leq a_i \leq 5000\)
- `d` is a list of 5000 integers
- `c` is a list of 5000 elements where `c[0]` is 0 and for \(1 \leq i \leq 4999\), `c[i]` is the cumulative sum of `d` from `d[1]` to `d[i]`
- `i` is 4998
- `ans` is the sum of \(\left(\frac{d[4999]}{m} * \frac{d[j]}{m} * \frac{c[4999 - j - 1]}{m}\right)\) for all \(0 \leq j < 4999\) where `d[j]` is not 0 plus \(\left(\frac{d[4998]}{m} * \frac{d[0]}{m} * \frac{c[4997]}{m}\right)\)
- `m` is the sum of all elements in `d` as a float
- `j` is 1

The code snippet modifies `ans` by adding the value of `d[i] / m * (d[j] / m) * (c[i - j - 1] / m)` to it.

Let's break down the calculation:
- `i` is 4998
- `j` is 1
- `m` is the sum of all elements in `d` as a float
- `c[i - j - 1]` is `c[4998 - 1 - 1]` which is `c[4996]`

So, the new value added to `ans` is:
\[ \text{new\_value} = \frac{d[4998]}{m} * \frac{d[1]}{m} * \frac{c[4996]}{m} \]

Therefore, the updated value of `ans` is:
\[ \text{ans} = \text{ans} + \frac{d[4998]}{m} * \frac{d[1]}{m} * \frac{c[4996]}{m} \]

The other variables remain unchanged.

Output State: **`n` is an integer where \(2 \leq n \leq 2000\), `a` is a list of `n` distinct integers where \(1 \leq a_i \leq 5000\), `d` is a list of 5000 integers, `c` is a list of 5000 elements where `c[0]` is 0 and for \(1 \leq i \leq 4999\), `c[i]` is the cumulative sum of `d` from `d[1]` to `d[i]`, `i` is 4998, `ans` is the sum of \(\left(\frac{d[4999]}{m} * \frac{d[j]}{m} * \frac{c[4999 - j - 1]}{m}\right)\) for all \(0 \leq j < 4999\) where `d[j]` is not 0 plus \(\left(\frac{d[4998]}{m} * \frac{d[0]}{m} * \frac{c[4997]}{m}\right)\) plus \(\left(\frac{d[4998]}{m} * \frac{d[1]}{m} * \frac{c[4996]}{m}\right)\), `m` is the sum of all elements in `d` as a float, `j` is 1**