The given code snippet updates the variable `ans` based on the current values of `i`, `j`, `d`, `c`, and `m`. Let's break down the steps:

1. **Check if `d[i]` is 0**: The condition `if d[4997] is 0, no changes are made to `ans`' means that if `d[4997]` is 0, the operation does not affect `ans`. Given `i` is 4997, we need to check the value of `d[4997]`.

2. **Calculate the new value of `ans`**: If `d[4997]` is not 0, the new value of `ans` is updated using the formula:
   \[
   \text{ans} += \frac{d[4997]}{m} \times \frac{d[4998]}{m} \times \frac{c[4997 - 4998 - 1]}{m}
   \]
   Simplifying the indices:
   \[
   \text{ans} += \frac{d[4997]}{m} \times \frac{d[4998]}{m} \times \frac{c[-2]}{m}
   \]
   Since `c` is defined as a list of 5000 elements, `c[-2]` is equivalent to `c[4998]`.

3. **Update the value of `ans`**:
   \[
   \text{ans} += \frac{d[4997]}{m} \times \frac{d[4998]}{m} \times \frac{c[4998]}{m}
   \]

Given the initial state:
- `n` is an integer where \(2 \leq n \leq 2000\)
- `a` is a list of `n` distinct integers where \(1 \leq a_i \leq 5000\)
- `d` is a list of 5000 integers
- `c` is a list of 5000 elements where `c[0]` is 0 and for \(1 \leq i \leq 4999\), `c[i]` is the cumulative sum of `d` from `d[1]` to `d[i]`
- `i` is 4997
- `ans` is the sum of \(\left(\frac{d[4999]}{m} * \frac{d[j]}{m} * \frac{c[4999 - j - 1]}{m}\right)\) for all \(0 \leq j < 4999\) where `d[j]` is not 0 plus the sum of \(\left(\frac{d[4998]}{m} * \frac{d[j]}{m} * \frac{c[4998 - j - 1]}{m}\right)\) for all \(0 \leq j < 4998\)
- `m` is the sum of all elements in `d` as a float
- `j` is 4998

If `d[4997]` is not 0, the new value of `ans` is:
\[
\text{ans} = \text{ans} + \frac{d[4997]}{m} \times \frac{d[4998]}{m} \times \frac{c[4998]}{m}
\]

Output State: **`n` is an integer where \(2 \leq n \leq 2000\), `a` is a list of `n` distinct integers where \(1 \leq a_i \leq 5000\), `d` is a list of 5000 integers, `c` is a list of 5000 elements where `c[0]` is 0 and for \(1 \leq i \leq 4999\), `c[i]` is the cumulative sum of `d` from `d[1]` to `d[i]`, `i` is 4997, `ans` is the sum of \(\left(\frac{d[4999]}{m} * \frac{d[j]}{m} * \frac{c[4999 - j - 1]}{m}\right)\) for all \(0 \leq j < 4999\) where `d[j]` is not 0 plus the sum of \(\left(\frac{d[4998]}{m} * \frac{d[j]}{m} * \frac{c[4998 - j - 1]}{m}\right)\) for all \(0 \leq j < 4998\) plus \(\frac{d[4997]}{m} \times \frac{d[4998]}{m} \times \frac{c[4998]}{m}\), `m` is the sum of all elements in `d` as a float, `j` is 4998.**