The given code updates the value of `ans` using the formula:

\[ \text{ans} += \frac{d[i]}{m} \times \left(\frac{d[j]}{m}\right) \times \left(\frac{c[i - j - 1]}{m}\right) \]

Given the initial state:
- `n` is an integer where \(2 \leq n \leq 2000\)
- `a` is a list of `n` distinct integers where \(1 \leq a_i \leq 5000\)
- `d` is a list of 5000 integers
- `c` is a list of 5000 elements where `c[0]` is 0 and for \(1 \leq i \leq 4999\), `c[i]` is the cumulative sum of `d` from `d[1]` to `d[i]`
- `i` is 4997
- `ans` is the original value of `ans` plus \(\frac{d[4997]}{m} \times \frac{d[0]}{m} \times \frac{c[4996]}{m}\)
- `m` is the sum of all elements in `d` as a float
- `j` is 1

Let's break down the impact of the code:

1. **Calculate the new value of `ans`:**
   - `d[i]` is `d[4997]`
   - `d[j]` is `d[1]`
   - `c[i - j - 1]` is `c[4997 - 1 - 1]` which is `c[4995]`
   - `m` is the sum of all elements in `d`

   The new value of `ans` is updated as follows:
   \[
   \text{ans} += \frac{d[4997]}{m} \times \left(\frac{d[1]}{m}\right) \times \left(\frac{c[4995]}{m}\right)
   \]

2. **Update the state:**
   - `ans` is updated to its new value.
   - All other variables remain unchanged.

Therefore, the output state is:
- `n` is an integer where \(2 \leq n \leq 2000\)
- `a` is a list of `n` distinct integers where \(1 \leq a_i \leq 5000\)
- `d` is a list of 5000 integers
- `c` is a list of 5000 elements where `c[0]` is 0 and for \(1 \leq i \leq 4999\), `c[i]` is the cumulative sum of `d` from `d[1]` to `d[i]`
- `i` is 4997
- `ans` is the original value of `ans` plus \(\frac{d[4997]}{m} \times \frac{d[1]}{m} \times \frac{c[4995]}{m}\)
- `m` is the sum of all elements in `d` as a float
- `j` is 1

Output State: **`n` is an integer where \(2 \leq n \leq 2000\), `a` is a list of `n` distinct integers where \(1 \leq a_i \leq 5000\), `d` is a list of 5000 integers, `c` is a list of 5000 elements where `c[0]` is 0 and for \(1 \leq i \leq 4999\), `c[i]` is the cumulative sum of `d` from `d[1]` to `d[i]`, `i` is 4997, `ans` is the original value of `ans` plus \(\frac{d[4997]}{m} \times \frac{d[1]}{m} \times \frac{c[4995]}{m}\), `m` is the sum of all elements in `d` as a float, `j` is 1**