The given code snippet updates the value of `dp[i]` using the formula `(dp[i - 1] + 2 * (i - 1) * dp[i - 2]) % 1000000007`. This means that the value of `dp[i]` is now calculated based on the previous two values in the `dp` array.

Given the initial state:
- `t` is an integer such that 1 ≤ t ≤ 10^4
- `n` is an integer such that 3 ≤ n ≤ 3 · 10^5
- `k` is an integer such that 0 ≤ k ≤ n
- `dp[1]` is 1
- `dp[2]` is 3
- `dp[i]` is `(dp[i - 1] + 2 * (i - 1) * dp[i - 2]) % 1000000007`
- `i` is incremented by 1

After executing the line `dp[i] = (dp[i - 1] + 2 * (i - 1) * dp[i - 2]) % 1000000007`, the value of `dp[i]` is updated. The values of `t`, `n`, `k`, `dp[1]`, and `dp[2]` remain unchanged.

Output State: **`t` is an integer such that 1 ≤ t ≤ 10^4, `n` is an integer such that 3 ≤ n ≤ 3 · 10^5, `k` is an integer such that 0 ≤ k ≤ n, `dp[1]` is 1, `dp[2]` is 3, `dp[i]` is `(dp[i - 1] + 2 * (i - 1) * dp[i - 2]) % 1000000007, `i` is incremented by 1**