Let's break down the problem step by step based on the given initial state and the provided code snippet.

### Initial State Recap
- `t` is an input integer such that \(0 \leq t \leq 499\).
- `p1`, `p2`, and `p3` are integers obtained from the input.
- The sum of `p1`, `p2`, and `p3` is odd.
- `low` is the minimum of `p3 - p1` and `p3 - p2`.
- `high` must be at least `cur`.
- `cur` is set according to the condition:
  - If `p1 - cur` is less than or equal to `p2 - (p3 - cur)`, `cur` remains equal to `low`.
  - Otherwise, `cur` is set to `low + 1`.

### Code Analysis
The code snippet to analyze is:
```python
print(p1 - cur + p3)
```

### Step-by-Step Calculation
1. **Determine `low`:**
   - `low` is the minimum of `p3 - p1` and `p3 - p2`.
   - Let's denote `low = min(p3 - p1, p3 - p2)`.

2. **Determine `cur`:**
   - `cur` is set based on the condition:
     - If `p1 - cur` is less than or equal to `p2 - (p3 - cur)`, `cur` remains `low`.
     - Otherwise, `cur` is set to `low + 1`.
   - Simplifying the condition:
     - `p1 - cur` is less than or equal to `p2 - (p3 - cur)`
     - `p1 - cur` is less than or equal to `p2 - p3 + cur`
     - `p1 + p3` is less than or equal to `p2 + 2 * cur`
     - `cur` is greater than or equal to `(p1 + p3 - p2) / 2`
   - Since `cur` is an integer, we can rewrite the condition as:
     - `cur` is the smallest integer such that `cur >= (p1 + p3 - p2) / 2`
     - If `(p1 + p3 - p2) / 2` is an integer, `cur` is this value.
     - If `(p1 + p3 - p2) / 2` is not an integer, `cur` is the next integer up.

3. **Determine `p1 - cur + p3`:**
   - Based on the value of `cur` determined above, we need to compute `p1 - cur + p3`.

### Final Output
To provide the most precise description, we need to consider the two cases for `cur`:

- **Case 1:** If `cur = low`
  - `p1 - cur + p3 = p1 - low + p3`
  - Since `low = min(p3 - p1, p3 - p2)`, we have two sub-cases:
    - If `low = p3 - p1`, then `p1 - cur + p3 = p1 - (p3 - p1) + p3 = 2 * p1`
    - If `low = p3 - p2`, then `p1 - cur + p3 = p1 - (p3 - p2) + p3 = p1 + p2`

- **Case 2:** If `cur = low + 1`
  - `p1 - cur + p3 = p1 - (low + 1) + p3 = p1 - low + p3 - 1`
  - Using the same sub-cases for `low`:
    - If `low = p3 - p1`, then `p1 - cur + p3 = 2 * p1 - 1`
    - If `low = p3 - p2`, then `p1 - cur + p3 = p1 + p2 - 1`

### Conclusion
The exact value of `p1 - cur + p3` depends on whether `cur` is `low` or `low + 1`, which in turn depends on the specific values of `p1`, `p2`, and `p3`. However, we can describe the output in terms of these variables and conditions.

Output: **p1 - cur + p3 (where cur is determined by the conditions given and low = min(p3 - p1, p3 - p2))**