To determine the output state after the loop has finished executing, we need to carefully walk through each iteration of the loop. The loop iterates `n` times, where `n` is the length of the string `s`. Since the string `s` is not provided, we will assume it's a string of length 4, as the initial states of `A` and `idx_A` have 4 elements. We will also assume that `s` is a string that contains the characters '<' in such a way that the loop logic can be followed.

Let's assume `s = '<<>>'` for this example. This assumption will help us follow the logic of the loop step-by-step.

### Iteration 1 (j = 0):
- `i = n - 1 - j = 4 - 1 - 0 = 3`
- `s[i] = s[3] = '>'`, so the `if s[i] == '<'` condition is not met.
- No changes to `B` or `idx_B`.

### Iteration 2 (j = 1):
- `i = n - 1 - j = 4 - 1 - 1 = 2`
- `s[i] = s[2] = '>'`, so the `if s[i] == '<'` condition is not met.
- No changes to `B` or `idx_B`.

### Iteration 3 (j = 2):
- `i = n - 1 - j = 4 - 1 - 2 = 1`
- `s[i] = s[1] = '<'`, so the `if s[i] == '<'` condition is met.
- `len(idx_B) == 0` is true, so `B.append(0)` and `idx_B.append(1)`.
- `B` becomes `[0]` and `idx_B` becomes `[1]`.

### Iteration 4 (j = 3):
- `i = n - 1 - j = 4 - 1 - 3 = 0`
- `s[i] = s[0] = '<'`, so the `if s[i] == '<'` condition is met.
- `len(idx_B) == 0` is false, so we calculate `x = B[len(B) - 1] + (idx_B[len(B) - 1] - i) * len(idx_B)`.
- `x = 0 + (1 - 0) * 1 = 1`.
- `B.append(1)` and `idx_B.append(0)`.
- `B` becomes `[0, 1]` and `idx_B` becomes `[1, 0]`.

### Final Output State:
After the loop has finished executing, the final state of the variables `B` and `idx_B` is `B = [0, 1]` and `idx_B = [1, 0]`. The other variables `A` and `idx_A` remain unchanged.

Output State: **A is [0, 1, 3, 12]; idx_A is [0, 1, 2, 5]; B is [0, 1]; idx_B is [1, 0].**