To determine the output state after the loop has finished executing, we need to carefully analyze the given code and the initial state. However, the variable `n` and the string `s` are not defined in the initial state provided. Since the loop iterates over `range(0, n)` and the conditionals inside the loop depend on the characters of `s`, we need to assume some values for `n` and `s` to proceed. 

For this example, let's assume `n` is `6` and `s` is a string of length `6` such as `">><><<"` to illustrate the loop's behavior. This assumption allows us to demonstrate how the loop operates and how the variables change.

Let's walk through the loop with these assumptions:

### Initial State:
- `A` is `[0, 1, 3, 12]`
- `idx_A` is `[0, 1, 2, 5]`
- `B` is `[0, 1]`
- `idx_B` is `[1, 0]`
- `l` is `0`
- `r` is `2`
- `n` is `6`
- `s` is `">><><<"`

### Loop Execution:
1. **Iteration 1 (i=0, s[0]='>')**:
   - `l < r` is `True`
   - `a = A[l] = A[0] = 0`
   - `x = r - (l + 2) = 2 - (0 + 2) = 0`
   - `b = B[r - 1] = B[1] = 1`
   - `x >= 0` is `True`
   - `b = b - B[x] = 1 - B[0] = 1 - 0 = 1`
   - `b = b - (idx_B[x] - idx_B[r - 1]) * (x + 1) = 1 - (idx_B[0] - idx_B[1]) * (0 + 1) = 1 - (1 - 0) * 1 = 0`
   - `b = (idx_B[r - 1] - i) * (l + 1) = (0 - 0) * (0 + 1) = 0`
   - `print(a * 2 + b * 2 + i + 1) = print(0 * 2 + 0 * 2 + 0 + 1) = print(1)`
   - `l += 1` → `l = 1`

2. **Iteration 2 (i=1, s[1]='>')**:
   - `l < r` is `True`
   - `a = A[l] = A[1] = 1`
   - `x = r - (l + 2) = 2 - (1 + 2) = -1`
   - `b = B[r - 1] = B[1] = 1`
   - `x >= 0` is `False`
   - `b = (idx_B[r - 1] - i) * (l + 1) = (0 - 1) * (1 + 1) = -2`
   - `print(a * 2 + b * 2 + i + 1) = print(1 * 2 + (-2) * 2 + 1 + 1) = print(1 * 2 - 4 + 2) = print(-1)`
   - `l += 1` → `l = 2`

3. **Iteration 3 (i=2, s[2]='<')**:
   - `r -= 1` → `r = 1`
   - `l <= r` is `True`
   - `l == 0` is `False`
   - `a = A[l - 1] = A[1] = 1`
   - `a = a + (i - idx_A[l - 1]) * l = 1 + (2 - 1) * 2 = 1 + 2 = 3`
   - `b = B[r] = B[1] = 1`
   - `r - l >= 0` is `False`
   - `b = b + (idx_B[r] - i) * l = 1 + (0 - 2) * 2 = 1 - 4 = -3`
   - `print(a * 2 + b * 2 + i + 1) = print(3 * 2 + (-3) * 2 + 2 + 1) = print(6 - 6 + 3) = print(3)`
   - `r -= 1` → `r = 0`

4. **Iteration 4 (i=3, s[3]='>')**:
   - `l < r` is `False`
   - `r == 0` is `True`
   - `print(n - i) = print(6 - 3) = print(3)`
   - `l += 1` → `l = 3`

5. **Iteration 5 (i=4, s[4]='<')**:
   - `r -= 1` → `r = -1` (This is out of bounds, but for the sake of illustration, assume it doesn't affect the logic here)
   - `l <= r` is `False`
   - `r == 0` is `False`
   - `a = B[r] = B[-1]` (out of bounds, assume it doesn't affect the logic here)
   - `b = A[l - 1] = A[2] = 3`
   - `l - r - 1 > 0` is `True`
   - `b = b - A[l - r - 2] = 3 - A[3 - (-1) - 2] = 3 - A[2] = 3 - 3 = 0`
   - `b = b - (idx_A[l - 1] - idx_A[l - r - 2]) * (l - r - 1) = 0 - (idx_A[2] - idx_A[2]) * (3 - (-1) - 1) = 0 - 0 * 3 = 0`
   - `b = b + (i - idx_A[l - 1]) * (r + 1) = 0 + (4 - 2) * (0 + 1) = 0 + 2 * 1 = 2`
   - `print(a * 2 + b * 2 + (n - i)) = print(0 * 2 + 2 * 2 + (6 - 4)) = print(0 + 4 + 2) = print(6)`
   - `r -= 1` → `r = -2`

6. **Iteration 6 (i=5, s[5]='<')**:
   - `r -= 1` → `r = -3` (This is out of bounds, but for the sake of illustration, assume it doesn't affect the logic here)
   - `l <= r` is `False`
   - `r == 0` is `False`
   - `a = B[r] = B[-3]` (out of bounds, assume it doesn't affect the logic here)
   - `b = A[l - 1] = A[2] = 3`
   - `l - r - 1 > 0` is `True`
   - `b = b - A[l - r - 2] = 3 - A[3 - (-3) - 2] = 3 - A[4]` (out of bounds, assume it doesn't affect the logic here)
   - `b = b - (idx_A[l - 1] - idx_A[l - r - 2]) * (l - r - 1) = 3 - (idx_A[2] - idx_A[4]) * (3 - (-3) - 1)` (out of bounds, assume it doesn't affect the logic here)
   - `b = b + (i - idx_A[l - 1]) * (r + 1) = 3 + (5 - 2) * (0 + 1) = 3 + 3 * 1 = 6`
   - `print(a * 2 + b * 2 + (n - i)) = print(0 * 2 + 6 * 2 + (6 - 5)) = print(0 + 12 + 1) = print(13)`
   - `r -= 1` → `r = -4`

### Final Output State:
The values of `A`, `idx_A`, `B`, `idx_B` remain unchanged as they are not modified within the loop. The values of `l` and `r` are modified based on the loop's execution. The output of the loop is printed values, but we are only interested in the final state of the variables.

Output State: **A is [0, 1, 3, 12]; idx_A is [0, 1, 2, 5]; B is [0, 1]; idx_B is [1, 0]; l is 3; r is -4