Alright, I've got this problem to solve. Let's see what it's asking for. So, there's this one-dimensional grid with cells, each containing either a '<' or a '>'. When a pinball is placed on one of these cells, it moves according to the direction of the arrow in that cell. If it's '<', it moves left, if '>', it moves right. But here's the twist: after moving, the arrow in the cell it was in flips. So, if it was '<', it becomes '>', and vice versa.

The task is to figure out how many seconds it takes for the pinball to leave the grid when placed on each cell, one at a time. The pinball stops when it goes off either end of the grid.

First, I need to understand the behavior of the pinball. Let's consider a simple example to see how it works.

Take n=3 with s="><<".

- If I place the pinball on cell 1 (which has '>'), it moves right to cell 2. After moving, the arrow in cell 1 flips to '<'.

- Now, cell 2 has '<', so the pinball moves left to cell 1. But cell 1 now has '<', so it moves left again, off the grid. Total steps: 3.

According to the example, it should take 3 seconds, which matches.

Another example: n=3 with s="><<", placing on cell 2.

- Cell 2 has '<', so it moves left to cell 1. Cell 2 flips to '>'.

- Cell 1 has '<', so it moves left, off the grid. But wait, according to the example, it takes 6 seconds. Hmm, maybe I'm missing something.

Wait, perhaps the flipping affects future moves. Let's try again.

- Place on cell 2: '<', moves left to cell 1, cell 2 flips to '>'.

- Now, cell 1 has '<', moves left, off the grid. Total steps: 2.

But the example says it takes 6 seconds. So, I must be misunderstanding.

Let me look at the example more carefully. Oh, the example says for n=3 with s="><<", the answers are 3, 6, 5 for each starting position.

Hmm, maybe my initial approach is too simplistic. There must be something more to it.

Perhaps I need to simulate the process for each starting position to see the pattern.

Let me try simulating for n=3 with s="><<".

- Starting at cell 1: '>' moves right to cell 2, s becomes "<<>".

- At cell 2: '<' moves left to cell 1, s becomes "<<>".

- At cell 1: '<' moves left, off the grid. Total steps: 3.

- Starting at cell 2: '<' moves left to cell 1, s becomes ">><".

- At cell 1: '<' moves left, off the grid. Total steps: 2.

But according to the example, it should be 6 seconds. Wait, maybe I need to consider that the arrow flips after each move.

Wait, in the first step, starting at cell 2 with '<', move left to cell 1, and flip cell 2 to '>'. So s becomes "<><".

Then, at cell 1 with '<', move left, off the grid. Total steps: 2.

But the example says it's 6 seconds. There's clearly something wrong with my simulation.

Let me check the second example: n=4 with s="<<<<".

- Starting at cell 1: '<' moves left, off the grid. Takes 1 second.

- Starting at cell 2: '<' moves left to cell 1, s becomes "<<>>".

- At cell 1: '<' moves left, off the grid. Total steps: 2.

- Starting at cell 3: '<' moves left to cell 2, s becomes "<><>".

- At cell 2: '<' moves left to cell 1, s becomes "><><".

- At cell 1: '<' moves left, off the grid. Total steps: 3.

- Starting at cell 4: '<' moves left to cell 3, s becomes "<<><".

- At cell 3: '<' moves left to cell 2, s becomes "<><>".

- At cell 2: '<' moves left to cell 1, s becomes "><><".

- At cell 1: '<' moves left, off the grid. Total steps: 4.

Which matches the sample output: 1 2 3 4.

So, in the first test case, something must be different in my simulation.

Wait, in the first test case, s="><<".

- Starting at cell 1: '>' moves right to cell 2, s becomes "<<<".

- At cell 2: '<' moves left to cell 1, s becomes "<<>".

- At cell 1: '<' moves left, off the grid. Total steps: 3.

- Starting at cell 2: '<' moves left to cell 1, s becomes "><<".

- At cell 1: '<' moves left, off the grid. Total steps: 2.

But according to the sample, it's 3,6,5. So, I must be missing something.

Wait, maybe the flipping affects the path differently.

Let me try tracing again for starting at cell 2 in the first test case.

- Start at cell 2: '<', move left to cell 1, s becomes ">><".

- At cell 1: '<' moves left, off the grid. Total steps: 2.

But sample output is 6. So, clearly, my simulation is incorrect.

I need a better approach.

Perhaps I should consider that each move affects the grid, and future moves depend on these changes.

This seems complex to simulate for large n, as n can be up to 5e5, and t up to 1e5, with total n across test cases up to 5e5.

I need an efficient algorithm, probably O(n) per test case.

Looking at the provided program, it seems to precompute two arrays A and B, tracking positions of '>' and '<' respectively, and then computes the answer for each position using these arrays.

I need to understand what A and B represent.

In func_1(s):

- n = len(s)

- A = [], idx_A = []

- For each i in 0 to n-1:

- if s[i] == '>':

- if idx_A is empty, A.append(0)

- else:

- x = A[-1] + (i - idx_A[-1]) * len(idx_A)

- A.append(x)

- idx_A.append(i)

Similarly for B:

- B = [], idx_B = []

- For j in 0 to n-1:

- i = n-1 - j

- if s[i] == '<':

- if idx_B is empty, B.append(0)

- else:

- x = B[-1] + (idx_B[-1] - i) * len(idx_B)

- B.append(x)

- idx_B.append(i)

Then, l = 0, r = len(B)

For each i in 0 to n-1:

- if s[i] == '>':

- if l < r:

- a = A[l]

- x = r - (l + 2)

- b = B[r - 1]

- if x >= 0:

- b = b - B[x]

- b = b - (idx_B[x] - idx_B[r - 1]) * (x + 1)

- b = b + (idx_B[r - 1] - i) * (l + 1)

- print(a * 2 + b * 2 + i + 1, end=' ')

- elif r == 0:

- print(n - i, end=' ')

- else:

- a = B[r - 1] + (idx_B[r - 1] - i) * r

- b = A[l - 1]

- if l - r > 0:

- b = b - A[l - r - 1]

- b = b - (idx_A[l - 1] - idx_A[l - r - 1]) * (l - r)

- b = b + (i - idx_A[l - 1]) * r

- print(a * 2 + b * 2 + (n - i), end=' ')

- l += 1

- else:

- r -= 1

- if l <= r:

- if l == 0:

- print(i + 1, end=' ')

- else:

- a = A[l - 1] + (i - idx_A[l - 1]) * l

- b = B[r]

- if r - l >= 0:

- b = b - B[r - l]

- b = b - (idx_B[r - l] - i) * (r - l)

- b = b + (idx_B[r] - i) * l

- print(a * 2 + b * 2 + i + 1, end=' ')

- elif r == 0:

- print(n - i + (i - idx_A[l - 1]) * 2, end=' ')

- else:

- a = B[r]

- b = A[l - 1]

- if l - r - 1 > 0:

- b = b - A[l - r - 2]

- b = b - (idx_A[l - 1] - idx_A[l - r - 2]) * (l - r - 1)

- b = b + (i - idx_A[l - 1]) * (r + 1)

- print(a * 2 + b * 2 + (n - i), end=' ')

This seems quite involved. I need to understand what A and B represent.

Looking at A:

- For each position i where s[i] == '>', it computes A[i], which seems to accumulate some kind of distance or step count, considering the number of '>' before it and the positions.

Similarly, B seems to do the same for '<' from the end.

Then, for each position i, depending on s[i], it computes the answer using A and B, with different cases based on the values of l and r.

This seems like an attempt to precompute the contributions from '>' and '<' directions and then combine them appropriately for each starting position.

I need to verify if this logic correctly computes the number of steps for each starting position.

Given the complexity of the provided code, and without a clear understanding of the variables and their meanings, it's challenging to verify its correctness directly.

An alternative approach might be to model the problem using graphs or dynamic programming, but given the constraints, efficiency is key.

Perhaps a better way is to consider the movement of the pinball and how the flipping of arrows affects its path.

Let's think about the pinball's movement:

- When the pinball is at a cell with '>', it moves right, and the arrow flips to '<'.

- When it's at a cell with '<', it moves left, and the arrow flips to '>'.

This flipping changes the behavior of future pinballs.

However, since each query is independent, meaning a new pinball is placed on the grid in its original state each time, the flips don't persist between queries.

Wait, no. The problem states: "Note that we always place a pinball on the initial grid." So, for each query, the grid is reset to its original state before placing the pinball.

Therefore, the flips made by one pinball don't affect the next one.

Hence, each query can be considered independently, starting from the original grid.

Given that, perhaps we can precompute for each position how long it takes for the pinball to leave the grid.

But with n up to 5e5 and t up to 1e5, with total n across test cases up to 5e5, we need an O(n) per test case solution.

Let me think about the movement in more detail.

Suppose we have a grid with cells from 0 to n-1.

- If s[i] == '>', the pinball moves to i+1, and s[i] flips to '<'.

- If s[i] == '<', the pinball moves to i-1, and s[i] flips to '>'.

But since each query is independent and the grid is reset each time, the flips don't affect subsequent moves of the same pinball.

Wait, no. For each query, the pinball moves, flips the arrow, moves again, flips again, and so on, until it leaves the grid.

But the grid is reset before each query, so each query is independent in terms of grid state, but within a query, the flips do affect the subsequent moves of that pinball.

Wait, no. The problem says: "Note that we always place a pinball on the initial grid."

But, during the movement of a single pinball, the arrows it leaves behind flip.

So, for a single query, the grid changes as the pinball moves.

Wait, but the problem says: "Note that we always place a pinball on the initial grid."

Does this mean that for each query, the grid is reset to its original state before placing the pinball?

If so, then in each query, the pinball moves, flips the arrow, moves again, flips again, and so on, but since it's a new pinball each time, the grid is reset to its original state for each query.

Wait, but the movement depends on the current arrow, which flips after each move.

So, for a single query, the grid changes as the pinball moves.

But across different queries, the grid is reset to its original state.

Given that, the movement for each query is deterministic based on the original grid.

I need to find a way to compute, for each starting position, how many steps it takes for the pinball to leave the grid, considering the flipping of arrows as it moves.

This seems tricky because the flipping changes the path.

I need a smarter way to model this.

Perhaps I can think of the movement in terms of cycles or something.

Wait, another idea: since the grid is reset for each query, and the movement is deterministic, perhaps I can precompute for each position how long it takes to leave the grid.

But directly simulating for each position would be too slow for n=5e5.

I need a smarter way.

Let me consider that the flipping of arrows effectively reverses the direction of future pinballs.

Wait, but each query is independent, so perhaps I can model the movement in some way.

Another approach: think of the grid as a graph where each cell has an outgoing edge based on its arrow, and the flipping changes the direction for future moves.

But since each query is independent, and the grid is reset each time, perhaps I can model the movement without worrying about the flips affecting future moves.

Wait, but in reality, the flips do affect the path of the current pinball.

This is confusing.

Let me try to think differently.

Suppose I have a grid with n cells.

I need to compute, for each starting position i, the number of steps until the pinball leaves the grid.

Let's denote f(i) as the number of steps for the pinball starting at position i.

I need to compute f(0), f(1), ..., f(n-1).

Given the constraints, I need an O(n) solution.

Looking back at the provided code, it seems to be attempting to compute these values efficiently using precomputed arrays A and B.

I need to understand what A and B represent.

Looking at A:

- For each position i where s[i] == '>', it computes A[i] based on the previous A value and the number of '>' before it.

Similarly for B with '<'.

Then, for each position, it computes f(i) based on A and B, with different cases depending on l and r.

I need to see if this logic correctly computes f(i) for each i.

Given that the sample input and output match, it seems to be correct.

But to be thorough, I should verify it with another example.

Take n=4 with s="<<<<".

According to the sample, the output should be "1 2 3 4".

Let's see what the provided code does for this input.

First, t=1 (though t is not used in the function, but in the loop).

Then, n=4, s="<<<<".

Compute A:

- s[0]=='<', skip

- s[1]=='<', skip

- s[2]=='<', skip

- s[3]=='<', skip

So, A is empty.

Compute B:

- For j=0, i=3, s[3]=='<', append 0, idx_B=[3]

- For j=1, i=2, s[2]=='<', x = B[0] + (3 - 2)*1 = 0 + 1*1 = 1, B=[0,1], idx_B=[3,2]

- For j=2, i=1, s[1]=='<', x = B[1] + (2 - 1)*2 = 1 + 1*2 = 3, B=[0,1,3], idx_B=[3,2,1]

- For j=3, i=0, s[0]=='<', x = B[2] + (1 - 0)*3 = 3 + 1*3 = 6, B=[0,1,3,6], idx_B=[3,2,1,0]

Then, l=0, r=4.

For i=0 to 3:

- i=0, s[0]=='<':

- since l <= r (0 <= 4):

- since l != 0:

- a = A[l-1] + (0 - idx_A[l-1])*l

- but A is empty, l=0, so l-1 is invalid.

Wait, l=0, so it should print i+1=1, which matches the sample output.

- i=1, s[1]=='<':

- r=4-1=3

- l <= r (0 <= 3):

- a = A[l-1] + (1 - idx_A[l-1])*l

- l=0, so a=0

- b = B[r] - B[r-l] - (idx_B[r-l]-1)*(r-l) + (idx_B[r]-1)*l

- r=3, r-l=3-0=3

- b = B[3] - B[3] - (idx_B[3]-1)*(3) + (idx_B[3]-1)*0

- idx_B[3]=0, so b=6 - 6 - (0-1)*3 + (0-1)*0 = 0 - (-1)*3 + 0 = 0 - (-3) + 0 = 3

- print a*2 + b*2 + i+1 = 0*2 + 3*2 + 2 = 0 + 6 + 2 = 8, which doesn't match the sample output of 2.

Wait, that's not matching. There must be a mistake in my calculation.

Wait, the code prints a*2 + b*2 + i + 1.

In this case, a=0, b=3, i=1, so 0*2 + 3*2 + 1 + 1 = 0 + 6 + 2 = 8, but sample output is 2.

So, perhaps my understanding is incorrect.

Wait, perhaps B is indexed differently.

Looking back, B is [0,1,3,6], idx_B=[3,2,1,0]

And r=4, but in the code, r=len(B)=4.

Wait, B has 4 elements, indices from 0 to 3.

When i=1, r=4-1=3.

l=0.

So, a = A[l-1] + (i - idx_A[l-1])*l

But l=0, l-1 is invalid, so a=0.

b = B[r] - B[r - l] - (idx_B[r - l] - i)*(r - l) + (idx_B[r] - i)*l

r - l = 3 - 0 = 3

B[3] = 6

B[3] = 6

idx_B[3] = 0

So, b = 6 - B[3] - (0 - 1)*3 + (0 - 1)*0 = 6 - 6 - (-1)*3 + 0 = 0 - (-3) + 0 = 3

Then, print 0*2 + 3*2 + 1 + 1 = 0 + 6 + 2 = 8, but sample output is 2.

This discrepancy suggests that the provided code might be incorrect.

Wait, perhaps I misread the code.

Looking back at the code:

When s[i]=='<':

if l <= r:

if l == 0:

print(i + 1, end=' ')

else:

a = A[l - 1] + (i - idx_A[l - 1]) * l

b = B[r] - B[r - l] - (idx_B[r - l] - i) * (r - l) + (idx_B[r] - i) * l

print(a * 2 + b * 2 + i + 1, end=' ')

In this case, l=0, so it should print i+1=2, which matches the sample output.

Wait, but in my earlier calculation, I thought l was incremented only when s[i]=='>', but in the code, l is incremented only when s[i]=='>'.

So, for i=0, s[0]=='<', r is decremented to 3.

Then, for i=1, s[1]=='<', r is decremented to 2.

So, when i=1, l=0, r=2.

Thus, l <= r (0 <= 2), and l != 0, so it should compute a and b.

Wait, l=0, so a=0, and b = B[2] - B[2] - (idx_B[2] - 1)*2 + (idx_B[2] - 1)*0

idx_B[2]=1

So, b = B[2] - B[2] - (1 - 1)*2 + (1 - 1)*0 = 3 - 3 - 0 + 0 = 0

Then, print a*2 + b*2 + i +1 = 0*2 + 0*2 + 1 +1 = 2, which matches the sample.

Ah, I see. I must have misread the code earlier.

So, in this case, it correctly prints 2.

Similarly, for i=2, s[2]=='<', r is now 1.

l=0, r=1.

l <= r, l !=0, so a = A[-1] + (2 - idx_A[-1])*0 = 0 + (2 - undefined)*0 = 0

b = B[1] - B[1] - (idx_B[1] - 2)*1 + (idx_B[1] - 2)*0 = 1 - 1 - (2 - 2)*1 + 0 = 0 - 0 + 0 = 0

print 0*2 + 0*2 + 2 +1 = 3, which matches the sample.

And for i=3, s[3]=='<', r=0.

l=0, r=0.

l <= r, l !=0, so a = A[-1] + (3 - idx_A[-1])*0 = 0

b = B[0] - B[0] - (idx_B[0] - 3)*0 + (idx_B[0] - 3)*0 = 0 - 0 - (3 - 3)*0 + 0 = 0

print 0*2 + 0*2 + 3 +1 =4, which matches.

So, in this case, the code works correctly.

In the first test case, n=3, s="><<"

Compute A:

- i=0, s[0]=='>', A=[0], idx_A=[0]

- i=1, s[1]=='<', skip

- i=2, s[2]=='<', skip

Compute B:

- j=0, i=2, s[2]=='<', B=[0], idx_B=[2]

- j=1, i=1, s[1]=='<', x=0 + (2-1)*1=1, B=[0,1], idx_B=[2,1]

- j=2, i=0, s[0]=='>', skip

So, B=[0,1], idx_B=[2,1]

Then, l=0, r=2.

For i=0 to 2:

- i=0, s[0]=='>':

- l < r (0 < 2):

- a = A[0] = 0

- x = r - (l + 2) = 2 - 2 =0

- b = B[1] =1

- x >=0, so b = 1 - B[0] - (idx_B[0] - idx_B[1])*1 =1 -0 - (2 -1)*1 =1 -0 -1 =0

- b = 0 + (idx_B[1] - 0)*1 =1 -0 =1

- print 0*2 +1*2 +0 +1=0 +2 +1=3, which matches the sample.

- i=1, s[1]=='<':

- r=2-1=1

- l <= r (0 <=1):

- since l !=0, a = A[-1] + (1 - idx_A[-1])*0 =0

- b = B[1] - B[1 - 0] - (idx_B[1 - 0] -1)*1 + (idx_B[1] -1)*0 =1 -1 - (1 -1)*1 +0 =0 -0 +0=0

- print 0*2 +0*2 +1 +1=0+0+2=2, which should be 6 according to the sample, but in the sample, it's 6. Wait, discrepancy again.

Wait, no. In the sample, for n=3, s="><<", outputs are 3,6,5.

But according to my calculation, it prints 3,2,5. Which doesn't match.

Wait, perhaps I'm miscounting.

Wait, in the first test case, n=3, s="><<", outputs are 3,6,5.

But according to the code:

- For i=0: 3

- For i=1: 6

- For i=2: 5

But in my calculation above, for i=1, s[1]=='<', it prints 2, but sample is 6.

So, perhaps the code is incorrect.

Wait, perhaps I'm not correctly implementing the logic.

Looking back at the code:

For s[i]=='>':

if l < r:

a = A[l]

x = r - (l + 2)

b = B[r - 1]

if x >=0:

b = b - B[x]

b = b - (idx_B[x] - idx_B[r - 1]) * (x + 1)

b = b + (idx_B[r - 1] - i) * (l + 1)

print(a * 2 + b * 2 + i + 1, end=' ')

else:

...

For s[i]=='<':

if l <= r:

if l ==0:

print(i +1, end=' ')

else:

a = A[l -1] + (i - idx_A[l -1]) * l

b = B[r] - B[r - l] - (idx_B[r - l] - i) * (r - l) + (idx_B[r] -i) * l

print(a *2 + b *2 + i +1, end=' ')

else:

...

In the first test case:

n=3, s="><<"

A=[0], idx_A=[0]

B=[0,1], idx_B=[2,1]

l=0, r=2

For i=0, s[0]=='>':

l < r (0 < 2):

a = A[0]=0

x = r - (l +2) =2 -2=0

b = B[1]=1

x >=0:

b =1 - B[0]=1 -0=1

b =1 - (idx_B[0] - idx_B[1])*1=1 - (2 -1)*1=1 -1=0

b =0 + (idx_B[1] -0)*1=1*1=1

print 0*2 +1*2 +0 +1=0 +2 +1=3, matches sample.

Then, l +=1, l=1

For i=1, s[1]=='<':

r=2-1=1

l <=r (1 <=1):

l !=0, so:

a = A[0] + (1 - idx_A[0])*1 =0 + (1 -0)*1=1

b = B[1] - B[1 -1] - (idx_B[1 -1] -1)*(1 -1) + (idx_B[1] -1)*1

=1 -0 - (idx_B[0] -1)*0 + (1 -1)*1=1 -0 - (2 -1)*0 +0=1 -0 -0 +0=1

print 1*2 +1*2 +1 +1=2 +2 +1 +1=6, matches sample.

For i=2, s[2]=='<':

r=1-1=0

l <=r (1 <=0)? No.

else:

if r ==0:

print(n -i + (i - idx_A[l -1])*2)

l=1, idx_A=[0], l-1=0, idx_A[0]=0

print(3 -2 + (2 -0)*2)=1 +4=5, matches sample.

So, in this case, it does produce the correct output.

I must have made a mistake in my earlier simulation.

Therefore, the code seems to be correct for this test case.

Let me check another test case.

n=6, s="<><<<>"

Compute A:

- i=0, s[0]=='<', skip

- i=1, s[1]=='>', A=[0], idx_A=[1]

- i=2, s[2]=='<', skip

- i=3, s[3]=='<', skip

- i=4, s[4]=='<', skip

- i=5, s[5]=='>', x=A[0] + (5 -1)*1=0 +4*1=4, A=[0,4], idx_A=[1,5]

Compute B:

- j=0, i=5, s[5]=='>', skip

- j=1, i=4, s[4]=='<', B=[0], idx_B=[4]

- j=2, i=3, s[3]=='<', x=B[0] + (4 -3)*1=0 +1*1=1, B=[0,1], idx_B=[4,3]

- j=3, i=2, s[2]=='<', x=B[1] + (3 -2)*2=1 +1*2=3, B=[0,1,3], idx_B=[4,3,2]

- j=4, i=1, s[1]=='>', skip

- j=5, i=0, s[0]=='<', x=B[2] + (2 -0)*3=3 +2*3=9, B=[0,1,3,9], idx_B=[4,3,2,0]

Then, l=0, r=4

For i=0 to 5:

- i=0, s[0]=='<':

- l <=r (0 <=4):

- l ==0, print i+1=1, matches sample.

- i=1, s[1]=='>':

- l < r (0 <4):

- a = A[0]=0

- x = r - (l +2)=4 -2=2

- b = B[3]=9

- x >=0:

- b =9 - B[2]=9 -3=6

- b =6 - (idx_B[2] - idx_B[3])*3=6 - (2 -0)*3=6 -6=0

- b =0 + (idx_B[3] -1)*1= (0 -1)*1=-1

- print 0*2 + (-1)*2 +1 +1=0 -2 +2=0, but sample is 4.

Wait, discrepancy again.

Wait, perhaps I misread the code.

Looking back:

b = b - (idx_B[x] - idx_B[r -1]) * (x +1)

x = r - (l +2)=4 -2=2

idx_B[x]=idx_B[2]=2

idx_B[r -1]=idx_B[3]=0

So, b =9 - B[2]=9 -3=6

Then, b=6 - (2 -0)*3=6 -6=0

Then, b=0 + (0 -1)*1=0 -1=-1

Then, print 0*2 + (-1)*2 +1 +1=0 -2 +2=0, but sample is 4.

This doesn't match.

Wait, perhaps I'm miscounting indices.

Let's double-check.

n=6, s="<><<<>"

A=[0,4], idx_A=[1,5]

B=[0,1,3,9], idx_B=[4,3,2,0]

l=0, r=4

For i=1, s[1]=='>':

l < r (0 <4):

a = A[0]=0

x = r - (l +2)=4 -2=2

b = B[3]=9

if x >=0:

b =9 - B[2]=9 -3=6

b =6 - (idx_B[2] - idx_B[3])*3=6 - (2 -0)*3=6 -6=0

b =0 + (idx_B[3] -1)*1= (0 -1)*1=-1

print 0*2 + (-1)*2 +1 +1=0 -2 +2=0, but sample is 4.

This suggests a mistake in the code or my understanding.

Wait, perhaps the formula is different.

Looking back at the code:

b = b - (idx_B[x] - idx_B[r -1]) * (x +1)

b = b + (idx_B[r -1] -i) * (l +1)

So, in this case:

b =9 -3 - (2 -0)*3 + (0 -1)*1=6 -6 + (-1)=-1

Then, a*2 + b*2 +i +1=0*2 + (-1)*2 +1 +1=0 -2 +2=0, but sample is 4.

So, perhaps the code is incorrect.

Alternatively, maybe I'm miscounting something.

Wait, perhaps r -1 is 3-1=2, idx_B[2]=2.

Wait, r=4, idx_B[3]=0.

Wait, r=4, but B has indices from 0 to 3.

x = r - (l +2)=4 -2=2

idx_B[x]=idx_B[2]=2

idx_B[r -1]=idx_B[3]=0

So, b=9 -3 - (2 -0)*3 + (0 -1)*1=6 -6 + (-1)=-1

Then, a*2 + b*2 +i +1=0*2 + (-1)*2 +1 +1=0 -2 +2=0, but sample is 4.

This indicates an error in the code.

Given this discrepancy, it seems the provided code is incorrect.

Therefore, the answer is Correctness: **False**