Alright, I've got this problem to solve. I need to determine if a given Python program correctly calculates the number of ordered pairs (a, b) that satisfy certain conditions based on the input values n and m. The conditions are that 1 ≤ a ≤ n, 1 ≤ b ≤ m, and a + b is a multiple of b multiplied by the greatest common divisor (GCD) of a and b. Whew, that sounds a bit tricky, but let's break it down step by step.

First, I need to understand the problem clearly. For each test case, I'm given two positive integers, n and m, and I need to find the number of ordered pairs (a, b) where a is between 1 and n, and b is between 1 and m, inclusive. The tricky part is the condition that a + b must be a multiple of b * GCD(a, b).

Let me try to rephrase that condition to make sure I get it. So, a + b should be divisible by b times the GCD of a and b. In mathematical terms, that means (a + b) mod (b * GCD(a, b)) == 0.

Hmm, that seems a bit complicated. Maybe there's a way to simplify this condition. Let's think about what GCD(a, b) represents. The GCD of a and b is the largest positive integer that divides both a and b without leaving a remainder.

Let me see if I can find a relationship or a pattern that can help simplify this condition.

Let's consider that GCD(a, b) divides both a and b. So, we can write a = GCD(a, b) * k and b = GCD(a, b) * l, where k and l are integers that are co-prime (their GCD is 1).

Wait, actually, that's a standard way to represent a and b in terms of their GCD. So, a = d * k and b = d * l, where d = GCD(a, b), and GCD(k, l) = 1.

Substituting these into the condition:

a + b = d * k + d * l = d * (k + l)

And b * GCD(a, b) = d * l * d = d^2 * l

So, the condition becomes:

d * (k + l) must be a multiple of d^2 * l

In other words, d * (k + l) is divisible by d^2 * l.

Simplifying this, we can divide both sides by d (since d is positive and non-zero):

k + l must be divisible by d * l.

Wait a minute, but d is GCD(a, b), and a = d * k, b = d * l, with GCD(k, l) = 1.

So, k and l are co-prime.

I need to find when k + l is divisible by d * l.

But k and l are co-prime, and d divides both a and b.

This seems a bit messy. Maybe there's another way to approach this.

Let's consider the condition again: a + b is a multiple of b * GCD(a, b).

Which means a + b = c * (b * GCD(a, b)), for some integer c.

So, a + b = c * b * GCD(a, b)

Let me solve for a:

a = c * b * GCD(a, b) - b

a = b * (c * GCD(a, b) - 1)

Now, since a must be a positive integer between 1 and n, and b is between 1 and m, we can think of a in terms of b and c.

But this seems a bit convoluted. Maybe I should look for a different approach.

Perhaps I can fix b and see what constraints that puts on a.

So, for a fixed b, I need to find a such that 1 ≤ a ≤ n, and a + b is a multiple of b * GCD(a, b).

Hmm.

Alternatively, maybe I can think about the ratio a/b.

Wait, not sure.

Let me try plugging in some small values to see if I can find a pattern.

Take the first example in the problem: n = 1, m = 1.

So, only possible pair is (1, 1).

Check the condition: a + b = 2, and b * GCD(1, 1) = 1 * 1 = 1.

Is 2 a multiple of 1? Yes. So, only one valid pair, which matches the sample output.

Second sample: n = 2, m = 3.

Possible pairs: (1,1), (1,2), (1,3), (2,1), (2,2), (2,3).

Let's check each:

(1,1): 1+1=2, 1*1=1 → 2 is a multiple of 1 → yes

(1,2): 1+2=3, 2*1=2 → 3 is not a multiple of 2 → no

(1,3): 1+3=4, 3*1=3 → 4 is not a multiple of 3 → no

(2,1): 2+1=3, 1*1=1 → 3 is a multiple of 1 → yes

(2,2): 2+2=4, 2*2=4 → 4 is a multiple of 4 → yes

(2,3): 2+3=5, 3*1=3 → 5 is not a multiple of 3 → no

So, valid pairs are (1,1), (2,1), (2,2) → total 3, which matches the sample output.

Another sample: n = 3, m = 5.

Possible pairs: (1,1), (1,2), (1,3), (1,4), (1,5), (2,1), (2,2), (2,3), (2,4), (2,5), (3,1), (3,2), (3,3), (3,4), (3,5).

Checking each:

(1,1): 2, 1*1=1 → yes

(1,2): 3, 2*1=2 → no

(1,3): 4, 3*1=3 → no

(1,4): 5, 4*1=4 → no

(1,5): 6, 5*1=5 → no

(2,1): 3, 1*1=1 → yes

(2,2): 4, 2*2=4 → yes

(2,3): 5, 3*1=3 → no

(2,4): 6, 4*2=8 → 6 is not a multiple of 8 → no

(2,5): 7, 5*1=5 → no

(3,1): 4, 1*1=1 → yes

(3,2): 5, 2*1=2 → no

(3,3): 6, 3*3=9 → no

(3,4): 7, 4*1=4 → no

(3,5): 8, 5*1=5 → no

Valid pairs: (1,1), (2,1), (2,2), (3,1) → total 4, matches the sample.

Okay, so from these small examples, I can see a pattern. It seems that for b = 1, a can be from 1 to n, and it's always valid. For b > 1, it's more restrictive.

Wait, in the second sample, b = 1: (1,1), (2,1), (3,1) are valid. b = 2: (2,2) is valid, but (1,2), (3,2) are not. b = 3: none are valid. b = 4: none. b = 5: none.

In the third sample, similar pattern.

So, perhaps there's a way to generalize this.

Let me try to find a mathematical relationship.

Given that a + b is a multiple of b * GCD(a, b), let's denote d = GCD(a, b).

Then, a = d * k and b = d * l, where GCD(k, l) = 1.

Then, a + b = d * k + d * l = d * (k + l)

And b * GCD(a, b) = d * l * d = d^2 * l

So, d * (k + l) must be a multiple of d^2 * l.

Dividing both sides by d (since d > 0), we get:

k + l is a multiple of d * l.

But GCD(k, l) = 1, which means k and l share no common factors other than 1.

So, k + l being a multiple of d * l implies that d * l divides k + l.

But l divides k + l only if l divides k, but since GCD(k, l) = 1, l can only divide k if l = 1.

Wait, but l = 1 would mean b = d * 1 = d, so b = GCD(a, b).

In other words, b divides a.

Wait, that seems interesting.

If b divides a, then GCD(a, b) = b, since b divides a.

So, a = m * b for some integer m.

Then, a + b = m * b + b = (m + 1) * b

And b * GCD(a, b) = b * b = b^2

So, (m + 1) * b must be a multiple of b^2, which implies that m + 1 must be a multiple of b.

So, m + 1 = p * b for some integer p.

Thus, m = p * b - 1.

But m = a / b, since a = m * b.

Wait, this seems a bit tangled.

Let me try to summarize:

If b divides a, then GCD(a, b) = b, and a = k * b for some integer k.

Then, a + b = k * b + b = (k + 1) * b

And b * GCD(a, b) = b * b = b^2

So, (k + 1) * b must be a multiple of b^2, which means k + 1 must be a multiple of b.

So, k + 1 = m * b for some integer m.

Thus, k = m * b - 1

Therefore, a = k * b = (m * b - 1) * b = m * b^2 - b

Now, a must be between 1 and n, so:

1 ≤ m * b^2 - b ≤ n

This seems a bit messy. Maybe there's a better way to approach this.

Alternatively, perhaps I can iterate over possible values of b and find the corresponding a that satisfy the condition.

Given that b is from 1 to m, for each b, I need to find a in 1 to n such that a + b is a multiple of b * GCD(a, b).

This seems computationally intensive if n and m are large, but given the constraints, the sum of n and m over all test cases doesn't exceed 2 * 10^6, and t can be up to 10^4, so I need an efficient solution.

Perhaps I can precompute some values or find a mathematical formula that allows me to compute the number of valid pairs quickly.

Looking back at the condition, a + b is a multiple of b * GCD(a, b).

Let me consider that b * GCD(a, b) divides a + b.

Which means a + b is divisible by b * GCD(a, b).

Let me see if I can write this condition in terms of a.

So, a + b ≡ 0 mod (b * GCD(a, b))

Which implies a ≡ -b mod (b * GCD(a, b))

But I'm not sure if that helps.

Maybe I should consider that GCD(a, b) divides a, so GCD(a, b) divides a + b.

But GCD(a, b) divides a and b, so it divides a + b automatically.

Wait, but the condition is that a + b is divisible by b * GCD(a, b), which is stronger than just being divisible by GCD(a, b).

So, it's not just that GCD(a, b) divides a + b, but b * GCD(a, b) divides a + b.

Which is a stronger condition.

So, perhaps I need to find pairs where b * GCD(a, b) divides a + b.

Let me consider that b * GCD(a, b) divides a + b.

Which implies that b * GCD(a, b) divides a + b.

Let me divide both sides by GCD(a, b):

Then, b divides (a + b) / GCD(a, b)

But (a + b) / GCD(a, b) = (a / GCD(a, b)) + (b / GCD(a, b))

Let me denote a' = a / GCD(a, b) and b' = b / GCD(a, b), where a' and b' are co-prime.

So, (a + b) / GCD(a, b) = a' + b'

Therefore, b divides a' + b'

But a' and b' are co-prime.

So, b divides a' + b'

Since b' divides b, and a' and b' are co-prime, perhaps there's a way to use this.

Wait, b' divides b, since b = GCD(a, b) * b'

But I'm getting a bit tangled here.

Maybe I should try a different approach.

Let me consider fixing b and finding the number of a in [1, n] that satisfy the condition for that b.

So, for a fixed b, I need to find the number of a in [1, n] such that a + b is a multiple of b * GCD(a, b).

Let me think about GCD(a, b).

For a fixed b, GCD(a, b) can take on values that are divisors of b.

Let me denote d = GCD(a, b), so d divides b.

Then, a must be a multiple of d, and a must be in [1, n].

Moreover, a + b must be a multiple of b * d.

So, for each possible d that divides b, I can find the number of a in [1, n] that are multiples of d and satisfy a + b is a multiple of b * d.

Wait, but d = GCD(a, b), and since d divides b, b * d is b * GCD(a, b) = b * d.

So, for each d that divides b, I need to find a in [1, n], where a is a multiple of d, and a + b is a multiple of b * d.

Let me write a ≡ -b mod (b * d)

Since a is a multiple of d, let a = k * d, where k is an integer.

Then, a + b = k * d + b ≡ 0 mod (b * d)

So, k * d + b ≡ 0 mod (b * d)

Which implies k * d ≡ -b mod (b * d)

But b is a multiple of d, since d divides b.

Let me denote b = c * d, where c is an integer.

Then, k * d ≡ -c * d mod (b * d) ⇒ k * d ≡ -c * d mod (c * d^2)

Dividing both sides by d (since d > 0), we get:

k ≡ -c mod (c * d)

But c = b / d.

So, k ≡ - (b / d) mod (b * d / d) ⇒ k ≡ - (b / d) mod b

Wait, simplifying:

Since c = b / d, then k ≡ -c mod (c * d)

But this seems a bit convoluted.

Maybe there's a better way to approach this.

Let me consider that a + b is a multiple of b * GCD(a, b), and GCD(a, b) divides b.

So, b * GCD(a, b) divides a + b.

Given that GCD(a, b) divides a and b, it divides a + b, but the condition is stronger.

Perhaps I can consider the ratio a + b over b * GCD(a, b).

Let me denote that ratio as an integer, say m.

So, (a + b) / (b * GCD(a, b)) = m, where m is an integer.

Then, a + b = m * b * GCD(a, b)

Since a = k * GCD(a, b), and b = l * GCD(a, b), with GCD(k, l) = 1.

Substituting back:

k * d + l * d = m * l * d * d ⇒ d(k + l) = m * l * d^2 ⇒ k + l = m * l * d

But GCD(k, l) = 1.

This seems complicated.

Maybe I need to look for a different approach altogether.

Let me consider small values of b and see if I can find a pattern.

For b = 1:

Then, a + 1 must be a multiple of 1 * GCD(a, 1).

Since GCD(a, 1) = 1, so a + 1 must be a multiple of 1, which it always is, because any integer is a multiple of 1.

Therefore, for b = 1, all a in [1, n] are valid.

For b = 2:

a + 2 must be a multiple of 2 * GCD(a, 2).

If a is even, GCD(a, 2) = 2, so a + 2 must be a multiple of 4.

If a is odd, GCD(a, 2) = 1, so a + 2 must be a multiple of 2.

Wait, let's check that.

For a even:

GCD(a, 2) = 2, so a + 2 must be a multiple of 4.

For a odd:

GCD(a, 2) = 1, so a + 2 must be a multiple of 2.

But any a + 2 where a is odd is odd + even = odd, which is not a multiple of 2, since it's odd.

Wait, but 1 + 2 = 3, which is not a multiple of 2. Indeed, 3 is not even.

So, for b = 2:

- If a is even, a + 2 must be a multiple of 4.

- If a is odd, a + 2 must be a multiple of 2, but since a + 2 is odd, this is never true.

Therefore, only even a where a + 2 is a multiple of 4 are valid.

Which means a is a multiple of 2, and a + 2 is a multiple of 4.

Let me see: if a is a multiple of 2, say a = 2k, then a + 2 = 2k + 2 = 2(k + 1)

For this to be a multiple of 4, 2(k + 1) must be divisible by 4, which implies k + 1 is even, so k is odd.

Therefore, a = 2k = 2*(2m + 1) = 4m + 2, for integer m.

So, a is of the form 4m + 2.

Wait, but in the second sample, n = 2, m = 3, and for b = 2, only a = 2 is valid, which is 4*0 + 2 = 2.

In the third sample, n = 3, m = 5, for b = 2, a = 2 is valid, which is again 4*0 + 2 = 2.

So, for b = 2, only a = 2, 6, 10, etc., are valid.

Wait, but 2 = 4*0 + 2, 6 = 4*1 + 2, 10 = 4*2 + 2, and so on.

So, for b = 2, a must be of the form 4k + 2.

Got it.

Similarly, for b = 3:

a + 3 must be a multiple of 3 * GCD(a, 3).

If a is a multiple of 3, GCD(a, 3) = 3, so a + 3 must be a multiple of 9.

If a is not a multiple of 3, GCD(a, 3) = 1, so a + 3 must be a multiple of 3.

So, for a multiple of 3, a + 3 must be a multiple of 9.

For a not multiple of 3, a + 3 must be a multiple of 3, which is always true since a + 3 is a multiple of 3 if a is not a multiple of 3.

Wait, no.

If a is not a multiple of 3, then a mod 3 is 1 or 2.

If a mod 3 = 1, then a + 3 mod 3 = 1 + 0 = 1, which is not 0.

If a mod 3 = 2, then a + 3 mod 3 = 2 + 0 = 2, which is not 0.

So, only when a is a multiple of 3 does a + 3 be a multiple of 3.

Wait, but according to the condition, for b = 3, a + 3 must be a multiple of 3 * GCD(a, 3).

If a is a multiple of 3, GCD(a, 3) = 3, so a + 3 must be a multiple of 9.

If a is not a multiple of 3, GCD(a, 3) = 1, so a + 3 must be a multiple of 3.

But as shown above, if a is not a multiple of 3, a + 3 is not a multiple of 3.

Therefore, only a that are multiples of 3 satisfy the condition for b = 3, and among those, a + 3 must be a multiple of 9.

So, a is a multiple of 3, and a + 3 is a multiple of 9.

Let me set a = 3k.

Then, a + 3 = 3k + 3 = 3(k + 1), which needs to be a multiple of 9.

So, 3(k + 1) ≡ 0 mod 9 ⇒ k + 1 ≡ 0 mod 3 ⇒ k ≡ 2 mod 3.

Therefore, k = 3m + 2, so a = 3*(3m + 2) = 9m + 6.

So, a is of the form 9m + 6.

In the third sample, n = 3, m = 5.

Possible b from 1 to 5.

For b = 3, a must be of the form 9m + 6.

But for m = 0, a = 6, which is greater than n = 3, so no valid a for b = 3.

Similarly, for b = 4 and b = 5, no valid a in n = 3.

Hence, only a = 1,2,3 for b = 1; a = 2 for b = 2; total 4 valid pairs.

This seems consistent.

So, generalizing this, for each b from 1 to m, and for each possible d that divides b, we can find the number of a in [1, n] that satisfy the condition for that d.

Wait, perhaps inclusion-exclusion could be applied here, but I'm not sure.

Alternatively, maybe we can iterate over b and find the number of a that satisfy the condition for each b, then sum over all b.

Given the time constraints, I need an efficient way to compute this.

Looking back at the sample solutions, it seems that for each b, the number of valid a can be computed based on some arithmetic progression.

For b = 1: all a in [1, n]

For b = 2: a = 4k + 2, for k >= 0, such that a <= n

For b = 3: a = 9k + 6, for k >= 0, such that a <= n

And so on.

So, for general b, it seems that a must be of the form LCM(b, GCD(a, b)) * m - b, for some integer m.

Wait, that seems too vague.

Let me think differently.

Suppose I fix b and d = GCD(a, b), then d divides b.

So, for each d that divides b, I can find the number of a in [1, n] such that GCD(a, b) = d and a + b is a multiple of b * d.

Given that GCD(a, b) = d, then a is a multiple of d, so a = d * k, where k is an integer such that GCD(k, b/d) = 1 (since GCD(a, b) = d).

Then, a + b = d * k + b.

But b is a multiple of d, since d divides b.

Let b = d * l, where l = b / d.

So, a + b = d * k + d * l = d * (k + l)

And b * d = d * l * d = d^2 * l

So, d * (k + l) must be a multiple of d^2 * l, which simplifies to k + l must be a multiple of d * l.

But k and l are co-prime, since GCD(k, l) = 1.

So, k + l must be a multiple of d * l.

Given that k and l are co-prime, and l divides k + l only if l divides k, but since GCD(k, l) = 1, l can only divide k if l = 1.

Therefore, unless l = 1, which implies b = d, meaning b = GCD(a, b), which implies that b divides a.

So, in this case, b divides a, and GCD(a, b) = b.

Then, a = b * m for some integer m.

Then, a + b = b * m + b = b * (m + 1)

And b * GCD(a, b) = b * b = b^2

So, b * (m + 1) must be a multiple of b^2, which implies that m + 1 must be a multiple of b.

So, m + 1 = p * b for some integer p.

Thus, m = p * b - 1

Therefore, a = b * (p * b - 1) = p * b^2 - b

Now, a must be in [1, n], so:

1 ≤ p * b^2 - b ≤ n

Solving for p:

Lower bound: p * b^2 - b ≥ 1 ⇒ p * b^2 ≥ b + 1 ⇒ p ≥ (b + 1) / b^2

Upper bound: p * b^2 - b ≤ n ⇒ p * b^2 ≤ n + b ⇒ p ≤ (n + b) / b^2

So, p must be an integer in the range:

ceil((b + 1)/b^2) ≤ p ≤ floor((n + b)/b^2)

Now, since b is at least 1, and p must be an integer, we can compute the number of valid p for each b, and thus the number of valid a for each b.

Then, sum over all b from 1 to m.

This seems feasible.

Let me try to compute this for the second sample input.

n = 2, m = 3

For b = 1:

p ≥ (1 + 1)/1^2 = 2/1 = 2 ⇒ p ≥ 2

p ≤ (2 + 1)/1^2 = 3/1 = 3 ⇒ p ≤ 3

So, p = 2, 3

a = 1 * (2 * 1 - 1) = 1 * (2 - 1) = 1 → valid

a = 1 * (3 * 1 - 1) = 1 * (3 - 1) = 2 → valid

So, a = 1, 2 for b = 1

For b = 2:

p ≥ (2 + 1)/4 = 3/4 ⇒ p ≥ 1

p ≤ (2 + 2)/4 = 4/4 = 1 ⇒ p ≤ 1

