To determine what will be printed by the `print(suma - 2)` statement, we need to carefully analyze the initial state and the formula provided for `suma`.

### Initial State:
- `n` and `m` are positive integers such that \(1 \leq n, m \leq 2 \times 10^6\).
- `T` is greater than 0.
- `t` is 1.
- `info` is a list of strings from the input.
- `a` is the integer value of the first string in `info`.
- `b` is the integer value of the second string in `info` and must be greater than or equal to 1.
- `suma` is the sum of the values of \((a - i \times (i - 1)) // i^2 + 1\) for each `i` from 1 to `b` where \((a - i \times (i - 1)) // i^2 + 1 > 0\), and an additional 1 is added to `suma` for each `i` where \((a - i \times (i - 1)) % i^2 == 0\) and \(i \times (i - 1) % i^2 == 0\).

### Step-by-Step Calculation:
1. **Understanding the Formula for `suma`:**
   - For each `i` from 1 to `b`, compute \((a - i \times (i - 1)) // i^2 + 1\).
   - Add this value to `suma` if it is greater than 0.
   - Additionally, add 1 to `suma` if \((a - i \times (i - 1)) % i^2 == 0\) and \(i \times (i - 1) % i^2 == 0\).

2. **Simplifying the Conditions:**
   - The condition \((a - i \times (i - 1)) % i^2 == 0\) means that \(a - i \times (i - 1)\) is divisible by \(i^2\).
   - The condition \(i \times (i - 1) % i^2 == 0\) means that \(i \times (i - 1)\) is divisible by \(i^2\). This is only true when \(i = 1\) because for any \(i > 1\), \(i \times (i - 1)\) is not divisible by \(i^2\).

3. **Evaluating the Formula:**
   - For \(i = 1\):
     - \((a - 1 \times (1 - 1)) // 1^2 + 1 = (a - 0) // 1 + 1 = a + 1\).
     - Since \(a + 1 > 0\), this value is added to `suma`.
     - Additionally, since \(i = 1\) satisfies both conditions, an extra 1 is added to `suma`.
   - For \(i > 1\):
     - \((a - i \times (i - 1)) // i^2 + 1\) is computed.
     - This value is added to `suma` if it is greater than 0.
     - The additional condition \(i \times (i - 1) % i^2 == 0\) is not satisfied for \(i > 1\), so no extra 1 is added.

4. **Summarizing `suma`:**
   - `suma` starts with \(a + 1 + 1 = a + 2\) from \(i = 1\).
   - For \(i > 1\), the value \((a - i \times (i - 1)) // i^2 + 1\) is added to `suma` if it is greater than 0.

5. **Final Calculation:**
   - The `print(suma - 2)` statement will print `suma` minus 2.
   - Since `suma` starts with \(a + 2\) and additional values are added based on the formula for \(i > 1\), the final value of `suma` will be \(a + 2 + \text{additional values}\).
   - Therefore, `suma - 2` will be \(a + \text{additional values}\).

### Output:
The `print(suma - 2)` statement will print the value of `a` plus the sum of the values of \((a - i \times (i - 1)) // i^2 + 1\) for each `i` from 2 to `b` where \((a - i \times (i - 1)) // i^2 + 1 > 0\).

Output: **a + \(\sum_{i=2}^{b} ((a - i \times (i - 1)) // i^2 + 1)\) where \((a - i \times (i - 1)) // i^2 + 1 > 0\)**