The code `t = t - 1` decrements the value of `t` by 1. All other variables remain unchanged. The initial state specifies that `t` is `t + (n - 1)`, so after the operation, `t` becomes `t + (n - 1) - 1`, which simplifies to `t + n - 2`.

Output State: **`t` is `t + n - 2`, `n` remains the same input integer such that 2 <= n <= 500, `x` remains the same list of n-1 integers where each element `x_i` satisfies 1 <= `x_i` <= 500, `T` is a list of integers derived from splitting and converting `line`, `a` is a list containing the elements `[1000, 1000 + T[0], 1000 + T[0] + T[1], ..., 1000 + T[0] + T[1] + ... + T[i-1]]` for all 1 <= i <= n-1, `result` is a string formed by joining the elements of `a` with spaces, `line` is the input string.**