Let's break down the problem step by step:

### Step 1: Understand the Loop Condition
The loop condition is:
```python
while j + p + 1 < n and i - p - 1 >= 0:
```

### Step 2: Analyze the Initial Values
- `i = (z + 1) // 2`
- `j = z // 2`
- `p = 0` if `i >= r` else `\(\min(r - i, res[2 * (l + r) - z])\)`
- `l = (z + 2) // 2 - p` if `((z + 1) // 2) + p > r` else `res[z + 1]` is equal to `p`.

### Step 3: Determine the Necessary Adjustments
To ensure the loop executes at least once, we need to satisfy both parts of the loop condition:
1. \( j + p + 1 < n \)
2. \( i - p - 1 \geq 0 \)

#### Part 1: \( j + p + 1 < n \)
- \( j = z // 2 \)
- \( p \) depends on the value of `i` relative to `r`.

For the loop to start, \( j + p + 1 \) should be less than `n`. Since \( j = z // 2 \), the critical part here is \( p \). We need to ensure \( p \) is such that \( j + p + 1 < n \).

#### Part 2: \( i - p - 1 \geq 0 \)
- \( i = (z + 1) // 2 \)
- \( p \) depends on the value of `i` relative to `r`.

For the loop to start, \( i - p - 1 \) should be non-negative. This means \( p \) should be such that \( i - p - 1 \geq 0 \).

### Step 4: Combine Conditions
Given the values:
- \( i = (z + 1) // 2 \)
- \( j = z // 2 \)
- \( p \) depends on `i` and `r`

We need to ensure:
- \( (z // 2) + p + 1 < n \)
- \( (z + 1) // 2 - p - 1 \geq 0 \)

To simplify, let's assume \( p \) is adjusted such that both conditions hold.

### Final Answer
State: **`i` is \((z + 1) // 2\), `j` is \(z // 2\), `p` is 0 if `i >= r` else \(\min(r - i, res[2 * (l + r) - z])\), `l` is \((z + 2) // 2 - p\)` if `((z + 1) // 2) + p > r` holds, otherwise `res[z + 1]` is equal to `p`, and `j + p + 1 < n` and `i - p - 1 \geq 0`**.

However, since the exact value of `p` might vary based on the conditions, the most precise way to represent this in the given format is:

State: **`i` is \((z + 1) // 2\), `j` is \(z // 2\), `p` is 0 if `i >= r` else \(\min(r - i, res[2 * (l + r) - z])\), `l` is \((z + 2) // 2 - p\)` if `((z + 1) // 2) + p > r` holds, otherwise `res[z + 1]` is equal to `p`, and `j + p + 1 < n` and `i - p - 1 \geq 0`**.