The code snippet `p += 1` increments the value of `p` by 1. The value of `p` was previously defined based on certain conditions involving `i`, `r`, `res`, and other variables. Since the exact initial value of `p` is not explicitly given in the initial state, we'll refer to it as the initial value of `p`.

The conditions and relationships between the variables are as follows:

- `i = (z + 1) // 2`
- `j = z // 2`
- `p = 0` if `i >= r` else \(\min(r - i, res[2 * (l + r) - z])\)
- `l = (z + 2) // 2 - p` if `((z + 1) // 2) + p > r` holds, otherwise `res[z + 1] = p`
- `j + p + 1 < n` and `i - p - 1 \geq 0`
- If \(s[j + p + 1] \neq s[i - p - 1]\), we break out of the most internal loop or if statement.

Given this, the only change after executing `p += 1` is that the value of `p` is incremented by 1. All other variables remain unchanged unless they are directly dependent on the updated value of `p`, which is not specified in the given conditions.

Therefore, the output state is:

Output State: **`i` is \((z + 1) // 2\), `j` is \(z // 2\), `p` is `p + 1`, `l` is \((z + 2) // 2 - (p + 1)\) if `((z + 1) // 2) + (p + 1) > r` holds, otherwise `res[z + 1]` is equal to `p + 1`, and `j + (p + 1) + 1 < n` and `i - (p + 1) - 1 \geq 0`.**