The code assigns the values of `i - p` to `l` and `j + p` to `r`. We know from the initial state that:

- `i = (z + 1) // 2`
- `j = z // 2`
- `p` is determined by the conditions involving `n`, `i`, and `j`.
- `l` is calculated based on the value of `p` and the condition involving `r`.

Given that `(j + p) > r` is true, we know that the loop condition `(j + p + 1 < n) and (i - p - 1 >= 0)` is satisfied, and `s[j + p + 1] == s[i - p - 1]` holds.

After executing the code, the new values for `l` and `r` are:

- `l = i - p`
- `r = j + p`

The other variables remain unchanged in their expressions or conditions based on the initial state.

Output State: **`i` is \((z + 1) // 2\), `j` is \(z // 2\), `p` is the maximum value of `p` such that `j + p + 1 < n` and `i - p - 1 >= 0`, `l` is `i - p`, `r` is `j + p`, and the loop terminates when either `j + p + 1 >= n` or `i - p - 1 < 0` or `s[j + p + 1] != s[i - p - 1]`. Additionally, the condition `(j + p) > r` is true.**