Output State: **`i` is \((z + 1) // 2\), `j` is \(z // 2\), `p` is \((z + 1) // 2 + (n - z - 2.5)\), and \(n > z + 2.5\)**

Explanation:
1. **Initialization**: The initial values of `i`, `j`, and `p` are given. Specifically, `i = (z + 1) // 2`, `j = z // 2`, and `p` depends on whether \((z + 1) // 2 < r\).
2. **Loop Condition**: The loop continues as long as \(j + p + 1 < n\) and \(i - p - 1 \geq 0\).
3. **Loop Iterations**:
   - After 1 iteration: `p` increases by 1, so `p = (z + 1) // 2`.
   - After 2 iterations: `p` increases by another 1, so `p = (z + 1) // 2 + 1`.
   - After 3 iterations: `p` increases by another 1, so `p = (z + 1) // 2 + 2`.

From the provided states, we observe that `p` increases by 1 with each iteration, and the loop continues until \(j + p + 1 \geq n\). Since \(j = z // 2\), the loop continues until \(z // 2 + p + 1 \geq n\), which simplifies to \(p \geq n - z - 1.5\).

Given the final state after 3 iterations, we infer that \(p\) will eventually reach \((z + 1) // 2 + (n - z - 2.5)\), ensuring the condition \(n > z + 2.5\) is met for the loop to continue until the end.

Thus, after the loop has executed all its iterations, `p` will be \((z + 1) // 2 + (n - z - 2.5)\), and the condition \(n > z + 2.5\) must hold true. The other variables `i` and `j` remain unchanged throughout the loop.