The code `i += 2 * k + 1` increments the value of `i` by `2 * k + 1`. From the initial state, we know that `i` is equal to `2 * k + 3`. Therefore, after executing the code, the new value of `i` will be `(2 * k + 3) + (2 * k + 1)`, which simplifies to `4 * k + 4`.

All other variables remain unchanged according to the initial state.

Output State: **`n` is an integer such that \(1 \leq n \leq 1000\) and \(n \geq 2 \cdot k + 3\); `k` is an integer such that \(0 \leq k \leq 1000\); `positions` is a list containing `[1, 2 \cdot k + 3]`; `i` is `4 * k + 4`**