Let's break down the initial state and the print statement step by step:

### Initial State:
- `n` and `k` are positive integers such that \(1 \leq k \leq n \leq 10^4\).
- `v` is the value returned by `func_2()`.
- `i` is `n - 2`.

### Print Statement:
```python
print(f'? 1 {i * n}', flush=True)
```

### Step-by-Step Analysis:
1. **Determine the value of `i`:**
   - According to the initial state, `i` is `n - 2`.
   - Therefore, `i = n - 2`.

2. **Calculate the expression `i * n`:**
   - Substitute `i` with `n - 2` in the expression `i * n`.
   - This gives us `(n - 2) * n`.

3. **Simplify the expression:**
   - `(n - 2) * n` simplifies to `n^2 - 2n`.

4. **Construct the print statement:**
   - The print statement is `f'? 1 {i * n}'`.
   - Substituting `i * n` with `n^2 - 2n`, the print statement becomes `f'? 1 {n^2 - 2n}'`.

### Final Output:
The print statement will output the string `? 1` followed by the value of `n^2 - 2n`.

Output: **? 1 n^2 - 2n (where n is a positive integer such that 1 <= k <= n <= 10^4)**