The code snippet provided is:

```python
l = func_2() + 1
```

Given the initial state:
- `n` and `k` are positive integers such that \( 1 \leq k \leq n \leq 10^4 \) and `k > 2`.
- `v` is the value of `i` when `v` equals `n` or 1 if no such `i` exists.
- `i` is 1.
- `cnt` is `k - 2`.
- `l` is `func_2() + 1` and `func_2() < n`.

Step-by-step analysis:
1. The line `l = func_2() + 1` is executed.
2. The function `func_2()` returns a value that is less than `n`.
3. This value is then incremented by 1 and assigned to `l`.

Since `func_2()` returns a value less than `n`, let's denote this value as `x` where \( x < n \). Therefore, `l` becomes `x + 1`.

The updated state of the variables is:
- `n` remains a positive integer such that \( 1 \leq k \leq n \leq 10^4 \).
- `k` remains a positive integer such that \( k > 2 \).
- `v` remains the value of `i` when `v` equals `n` or 1 if no such `i` exists.
- `i` remains 1.
- `cnt` remains `k - 2`.
- `l` is now `func_2() + 1`, which is `x + 1` where \( x < n \).

Output State: **`n` and `k` are positive integers such that \( 1 \leq k \leq n \leq 10^4 \) and `k > 2`, `v` is the value of `i` when `v` equals `n` or 1 if no such `i` exists, `i` is 1, `cnt` is `k - 2`, `l` is `func_2() + 1` (a value less than `n + 1`).**