To determine the final output state after all iterations of the loop, we need to understand the loop's behavior and how the variable `z` changes with each iteration.

The loop runs for `x - k + 3` iterations. In each iteration, `z` is updated using the formula:

\[ z = z + \left(\frac{z}{k - 1}\right) + 1 \]

Given the initial state:
- `z` starts as `k - 2`.

Let's denote:
- `z_0 = k - 2` (initial value of `z`).
- `z_1 = z_0 + \left(\frac{z_0}{k - 1}\right) + 1` (value of `z` after 1 iteration).
- `z_2 = z_1 + \left(\frac{z_1}{k - 1}\right) + 1` (value of `z` after 2 iterations).
- `z_3 = z_2 + \left(\frac{z_2}{k - 1}\right) + 1` (value of `z` after 3 iterations).
- And so on...

The value of `z` after `n` iterations can be expressed as:

\[ z_n = z_{n-1} + \left(\frac{z_{n-1}}{k - 1}\right) + 1 \]

The loop runs for `x - k + 3` iterations, so the final value of `z` after all iterations is:

\[ z_{\text{final}} = z_{x - k + 2} \]

The exact value of `z_{\text{final}}` can be calculated iteratively using the above formula. However, the problem asks for the output state in a specific format, and we can express the final state in terms of the number of iterations.

Output State: **`t` is an integer such that 1 <= t <= 1000, `k`, `x`, and `a` are integers obtained by splitting and converting the string `s`, `x` is greater than or equal to `k - 1` and `x` is not equal to `k - 1`, `z` is the value obtained after `x - k + 3` iterations of the loop where `z` is updated as `z = z + (z // (k - 1)) + 1` starting from `z = k - 2`.**

In simpler terms, the final value of `z` is the result of applying the loop's update rule `x - k + 3` times starting from `z = k - 2`.