Alright, I've got this task to verify the correctness of a given Python program based on its problem description. The program is supposed to rearrange a permutation array so that after performing a specific binary search, the value at position `l` equals the target value `x`. The program can perform up to two swaps on the array before running the binary search.

First, I need to make sure I understand the problem completely. We have a permutation of size `n`, which means it's an array containing each number from 1 to `n` exactly once, but in any order. The goal is to adjust this array by swapping elements at most twice so that after these swaps, a particular binary search algorithm will end with `p_l` equal to `x`, the target number we're trying to find.

I need to understand the binary search algorithm described in the problem because it's not a standard binary search. Let's see:

- Initialize `l = 1` and `r = n + 1`.

- While `r - l != 1`:

- Calculate `m = floor((r + l) / 2)`.

- If `p_m <= x`, set `l = m`.

- Else, set `r = m`.

- After the loop, `p_l` should equal `x`.

This is interesting because in standard binary search, we're looking for a specific value, and we adjust `l` and `r` based on whether the middle element is less than or greater than the target. Here, it seems like we're adjusting `l` and `r` based on `p_m` compared to `x`, but the stopping condition is when `r - l = 1`.

I need to make sure I understand how this search works. Let's take an example.

Suppose `n = 6`, `x = 3`, and `array = [1, 2, 3, 4, 5, 6]`.

Starting with `l = 1`, `r = 7`.

First iteration:

- `m = floor((1 + 7)/2) = 4`.

- `p_4 = 4`, which is greater than `x = 3`, so `r = 4`.

Now `l = 1`, `r = 4`.

Second iteration:

- `m = floor((1 + 4)/2) = 2`.

- `p_2 = 2`, which is less than or equal to `x = 3`, so `l = 2`.

Now `l = 2`, `r = 4`.

Third iteration:

- `m = floor((2 + 4)/2) = 3`.

- `p_3 = 3`, which is less than or equal to `x = 3`, so `l = 3`.

Now `l = 3`, `r = 4`.

Fourth iteration:

- `m = floor((3 + 4)/2) = 3`.

- `p_3 = 3`, which is less than or equal to `x = 3`, so `l = 3`.

Now `l = 3`, `r = 4`.

Since `r - l = 1`, the loop stops, and `p_l = p_3 = 3`, which equals `x = 3`. So, in this case, no swaps are needed.

Another example: `n = 6`, `x = 5`, `array = [3, 1, 6, 5, 2, 4]`.

Let's perform the search without any swaps.

Start with `l = 1`, `r = 7`.

First iteration:

- `m = floor((1 + 7)/2) = 4`.

- `p_4 = 5`, which is equal to `x = 5`, so `l = 4`.

Now `l = 4`, `r = 7`.

Second iteration:

- `m = floor((4 + 7)/2) = 5`.

- `p_5 = 2`, which is less than `x = 5`, so `l = 5`.

Now `l = 5`, `r = 7`.

Third iteration:

- `m = floor((5 + 7)/2) = 6`.

- `p_6 = 4`, which is less than `x = 5`, so `l = 6`.

Now `l = 6`, `r = 7`.

Fourth iteration:

- `m = floor((6 + 7)/2) = 6`.

- `p_6 = 4`, which is less than `x = 5`, so `l = 6`.

Now `l = 6`, `r = 7`.

Loop stops, `p_l = p_6 = 4`, which is not equal to `x = 5`. So, swaps are needed.

We can try swapping indices 3 and 4: swap `p_3 = 6` and `p_4 = 5`, so array becomes `[3, 1, 5, 6, 2, 4]`.

Perform the search again:

Start with `l = 1`, `r = 7`.

First iteration:

- `m = 4`.

- `p_4 = 6`, which is greater than `x = 5`, so `r = 4`.

Now `l = 1`, `r = 4`.

Second iteration:

- `m = 2`.

- `p_2 = 1`, which is less than or equal to `x = 5`, so `l = 2`.

Now `l = 2`, `r = 4`.

Third iteration:

- `m = 3`.

- `p_3 = 5`, which is less than or equal to `x = 5`, so `l = 3`.

Now `l = 3`, `r = 4`.

Fourth iteration:

- `m = 3`.

- `p_3 = 5`, which is less than or equal to `x = 5`, so `l = 3`.

Loop stops, `p_l = p_3 = 5`, which equals `x = 5`. So, one swap suffices.

Another example: `n = 5`, `x = 1`, `array = [3, 5, 4, 2, 1]`.

Perform the search without swaps:

`l = 1`, `r = 6`.

First iteration:

- `m = floor((1 + 6)/2) = 3`.

- `p_3 = 4`, which is greater than `x = 1`, so `r = 3`.

Now `l = 1`, `r = 3`.

Second iteration:

- `m = floor((1 + 3)/2) = 1`.

- `p_1 = 3`, which is greater than `x = 1`, so `r = 1`.

Now `l = 1`, `r = 1`.

Loop stops, `p_l = p_1 = 3`, which is not equal to `x = 1`.

Need to perform swaps.

Let's try swapping `p_1 = 3` and `p_5 = 1`, so array becomes `[1, 5, 4, 2, 3]`.

Perform the search:

`l = 1`, `r = 6`.

First iteration:

- `m = 3`.

- `p_3 = 4`, which is greater than `x = 1`, so `r = 3`.

Now `l = 1`, `r = 3`.

Second iteration:

- `m = 1`.

- `p_1 = 1`, which is less than or equal to `x = 1`, so `l = 1`.

Now `l = 1`, `r = 3`.

Third iteration:

- `m = floor((1 + 3)/2) = 1`.

- `p_1 = 1`, which is less than or equal to `x = 1`, so `l = 1`.

Loop stops, `p_l = p_1 = 1`, which equals `x = 1`. So, one swap suffices.

Another example: `n = 6`, `x = 3`, `array = [4, 3, 1, 5, 2, 6]`.

Perform the search without swaps:

`l = 1`, `r = 7`.

First iteration:

- `m = 4`.

- `p_4 = 5`, which is greater than `x = 3`, so `r = 4`.

Now `l = 1`, `r = 4`.

Second iteration:

- `m = 2`.

- `p_2 = 3`, which is less than or equal to `x = 3`, so `l = 2`.

Now `l = 2`, `r = 4`.

Third iteration:

- `m = 3`.

- `p_3 = 1`, which is less than or equal to `x = 3`, so `l = 3`.

Now `l = 3`, `r = 4`.

Fourth iteration:

- `m = 3`.

- `p_3 = 1`, which is less than or equal to `x = 3`, so `l = 3`.

Loop stops, `p_l = p_3 = 1`, which is not equal to `x = 3`.

Need to perform swaps.

Let's try swapping `p_3 = 1` and `p_2 = 3`, so array becomes `[4, 1, 3, 5, 2, 6]`.

Perform the search:

`l = 1`, `r = 7`.

First iteration:

- `m = 4`.

- `p_4 = 5`, which is greater than `x = 3`, so `r = 4`.

Now `l = 1`, `r = 4`.

Second iteration:

- `m = 2`.

- `p_2 = 1`, which is less than or equal to `x = 3`, so `l = 2`.

Now `l = 2`, `r = 4`.

Third iteration:

- `m = 3`.

- `p_3 = 3`, which is less than or equal to `x = 3`, so `l = 3`.

Now `l = 3`, `r = 4`.

Fourth iteration:

- `m = 3`.

- `p_3 = 3`, which is less than or equal to `x = 3`, so `l = 3`.

Loop stops, `p_l = p_3 = 3`, which equals `x = 3`. So, one swap suffices.

Last example: `n = 3`, `x = 2`, `array = [3, 2, 1]`.

Perform the search without swaps:

`l = 1`, `r = 4`.

First iteration:

- `m = floor((1 + 4)/2) = 2`.

- `p_2 = 2`, which is less than or equal to `x = 2`, so `l = 2`.

Now `l = 2`, `r = 4`.

Second iteration:

- `m = floor((2 + 4)/2) = 3`.

- `p_3 = 1`, which is less than or equal to `x = 2`, so `l = 3`.

Now `l = 3`, `r = 4`.

Third iteration:

- `m = 3`.

- `p_3 = 1`, which is less than or equal to `x = 2`, so `l = 3`.

Loop stops, `p_l = p_3 = 1`, which is not equal to `x = 2`.

Need to perform swaps.

Let's try swapping `p_1 = 3` and `p_2 = 2`, so array becomes `[2, 3, 1]`.

Perform the search:

`l = 1`, `r = 4`.

First iteration:

- `m = 2`.

- `p_2 = 3`, which is greater than `x = 2`, so `r = 2`.

Now `l = 1`, `r = 2`.

Second iteration:

- `m = 1`.

- `p_1 = 2`, which is less than or equal to `x = 2`, so `l = 1`.

Now `l = 1`, `r = 2`.

Third iteration:

- `m = 1`.

- `p_1 = 2`, which is less than or equal to `x = 2`, so `l = 1`.

Loop stops, `p_l = p_1 = 2`, which equals `x = 2`. So, one swap suffices.

From these examples, it seems that one swap is often sufficient to make the binary search end with `p_l` equal to `x`. Sometimes, no swaps are needed if the array is already set up correctly for the binary search to find `x` at the right position.

Now, looking at the provided program, I need to see if it correctly implements the logic to perform up to two swaps to achieve the desired result.

Looking at the program:

- It reads the number of test cases `t`.

- For each test case, it reads `n` and `x`, then reads the permutation array.

- It calls a function `func_1(array, find)` where `find` is `x`.

- `func_1` performs a binary search similar to the one described in the problem, but with some differences.

Wait a minute, in the problem description, the binary search is performed on the array after possible swaps, and we need to output the swaps performed.

But in this program, `func_1` seems to perform some kind of search on the array and then decide whether to perform a swap or not.

Looking closer at `func_1`:

- It sets `l = 0` and `r = n - 1` (0-based indexing).

- It performs a while loop while `l <= r`:

- Calculates `mid = (l + r) // 2`.

- If `array[mid] >= find`, set `r = mid - 1`.

- Else, set `l = mid + 1`.

- After the loop, it checks if `l` is not equal to the index of `find` in the array.

- If not, it prints `1` and returns a string with `l + 1` and `index of find + 1` (1-based indexing).

- If yes, it prints `0`.

Wait, this seems different from the problem's binary search algorithm.

In the problem's binary search:

- `l` starts at `1`, `r` at `n + 1`.

- Loop continues until `r - l == 1`.

- `m = floor((r + l) / 2)`.

- If `p_m <= x`, set `l = m`.

- Else, set `r = m`.

- After loop, check `p_l == x`.

In `func_1`:

- `l` starts at `0`, `r` at `n - 1`.

- Loop continues while `l <= r`.

- `mid = floor((l + r) / 2)`.

- If `array[mid] >= find`, set `r = mid - 1`.

- Else, set `l = mid + 1`.

- After loop, check if `l` is not equal to the index of `find`.

- If not, perform one swap between `l` and the index of `find`.

This seems like a standard binary search to find the position where `find` should be inserted, but adjusted to find the exact position of `find` in the array.

However, the problem requires us to adjust the array through swaps so that the specific binary search ends with `p_l` equal to `x`.

I think there's a mismatch here. The program seems to be trying to find the position of `x` in the array and swap it to position `l` if necessary. But the binary search in the problem is different from the one in `func_1`.

I need to ensure that after performing the swaps (if any), when the problem's binary search is applied, it ends with `p_l` equal to `x`.

But in the program, `func_1` is performing a different binary search and deciding based on that.

This is confusing. Maybe I need to understand what the program is doing step by step.

Let's take the first example:

Input:

5

6 3

1 2 3 4 5 6

Output:

0

So, no swaps are needed, which is correct because in this case, the binary search already ends with `p_l = 3`.

Another example:

Input:

6 5

3 1 6 5 2 4

Output:

1

3 4

So, it's performing one swap between positions 3 and 4 (1-based indexing), which corresponds to swapping `p_3 = 6` and `p_4 = 5`, resulting in the array [3, 1, 5, 6, 2, 4].

As I saw earlier, this makes the binary search end with `p_l = 5`, which is correct.

Another example:

Input:

5 1

3 5 4 2 1

Output:

2

2 4

1 5

So, performing two swaps: first swap positions 2 and 4 (1-based: `p_2 = 5` and `p_4 = 2`), resulting in [3, 2, 4, 5, 1]. Then swap positions 1 and 5 (1-based: `p_1 = 3` and `p_5 = 1`), resulting in [1, 2, 4, 5, 3]. Now, the binary search should end with `p_l = 1`, which is correct.

Another example:

Input:

6 3

4 3 1 5 2 6

Output:

2

4 5

2 4

So, first swap positions 4 and 5 (1-based: `p_4 = 5` and `p_5 = 2`), resulting in [4, 3, 1, 2, 5, 6]. Then swap positions 2 and 4 (1-based: `p_2 = 3` and `p_4 = 2`), resulting in [4, 2, 1, 3, 5, 6]. Now, the binary search should end with `p_l = 3`, which is correct.

Last example:

Input:

3 2

3 2 1

Output:

1

1 3

So, swap positions 1 and 3 (1-based: `p_1 = 3` and `p_3 = 1`), resulting in [1, 2, 3]. Now, the binary search should end with `p_l = 2`, which is correct.

So, in all these examples, the program seems to be working correctly, producing the right number of swaps and the right swaps to make the binary search end with `p_l = x`.

But I need to verify if this is always the case.

Let me try to think of a tricky case.

Suppose `n = 4`, `x = 2`, and `array = [4, 1, 3, 2]`.

Let's perform the binary search without swaps:

`l = 1`, `r = 5`.

First iteration:

- `m = floor((1 + 5)/2) = 3`.

- `p_3 = 3`, which is greater than `x = 2`, so `r = 3`.

Now `l = 1`, `r = 3`.

Second iteration:

- `m = floor((1 + 3)/2) = 1`.

- `p_1 = 4`, which is greater than `x = 2`, so `r = 1`.

Now `l = 1`, `r = 1`.

Loop stops, `p_l = p_1 = 4`, which is not equal to `x = 2`.

Need to perform swaps.

Let's see what swaps the program would perform.

According to the program, `func_1` would perform a binary search to find where `x = 2` should be, and if it's not at position `l`, perform one swap.

But in this case, I need to see what `l` would be after the search.

Wait, I need to simulate the program's `func_1`.

Given `array = [4, 1, 3, 2]`, `find = 2`.

Initialize `l = 0`, `r = 3`.

First iteration:

- `mid = floor((0 + 3)/2) = 1`.

- `array[1] = 1`, which is less than `2`, so `l = 1 + 1 = 2`.

Now `l = 2`, `r = 3`.

Second iteration:

- `mid = floor((2 + 3)/2) = 2`.

- `array[2] = 3`, which is greater than or equal to `2`, so `r = 2 - 1 = 1`.

Now `l = 2`, `r = 1`.

Since `l > r`, loop ends.

The index `l` is 2, but `array[2] = 3`, which is not `x = 2`.

So, the program would perform one swap between position `l = 2` and the position of `x = 2`, which is position 4.

Swap positions 2 and 4: `array` becomes [4, 2, 3, 1].

Now, perform the problem's binary search:

`l = 1`, `r = 5`.

First iteration:

- `m = floor((1 + 5)/2) = 3`.

- `p_3 = 3`, which is greater than `x = 2`, so `r = 3`.

Now `l = 1`, `r = 3`.

Second iteration:

- `m = floor((1 + 3)/2) = 1`.

- `p_1 = 4`, which is greater than `x = 2`, so `r = 1`.

Now `l = 1`, `r = 1`.

Loop stops, `p_l = p_1 = 4`, which is not equal to `x = 2`.

Hmm, in this case, one swap was performed, but the binary search still doesn't end with `p_l = x`.

So, perhaps the program is incorrect in this case.

Wait, according to the program, it would perform one swap between `l = 2` and the position of `x = 2`, which is position 4.

After swap, array is [4, 2, 3, 1].

Performing the binary search:

- `l = 1`, `r = 5`.

- `m = 3`, `p_3 = 3 >= 2`, so `l = 3`.

- `m = floor((3 + 5)/2) = 4`.

- `p_4 = 1 < 2`, so `l = 4`.

- `m = 4`, `p_4 = 1 < 2`, so `l = 4`.

Loop stops, `p_l = p_4 = 1 != 2`.

So, it's incorrect. The program performs one swap, but the binary search doesn't end with `p_l = x`.

Perhaps the program is incorrect in this case.

But according to the problem statement, it's guaranteed that two operations are always sufficient. So, maybe performing two swaps would fix it.

In this case, after the first swap, array is [4, 2, 3, 1].

We can perform a second swap between positions 1 and 4: swap `p_1 = 4` and `p_4 = 1`, resulting in [1, 2, 3, 4].

Now, perform the binary search:

- `l = 1`, `r = 5`.

- `m = 3`, `p_3 = 3 >= 2`, so `l = 3`.

- `m = floor((3 + 5)/2) = 4`.

- `p_4 = 4 >= 2`, so `l = 4`.

- `m = 4`, `p_4 = 4 >= 2`, so `l = 4`.

Loop stops, `p_l = p_4 = 4 != 2`.

Hmm, still not correct.

Wait, maybe different swaps are needed.

Alternatively, maybe swapping positions 2 and 4, then positions 1 and 2:

First swap: positions 2 and 4: [4, 2, 3, 1].

Second swap: positions 1 and 2: [2, 4, 3, 1].

Now, perform the binary search:

- `l = 1`, `r = 5`.

- `m = 3`, `p_3 = 3 >= 2`, so `l = 3`.

- `m = floor((3 + 5)/2) = 4`.

- `p_4 = 1 < 2`, so `l = 4`.

- `m = 4`, `p_4 = 1 < 2`, so `l = 4`.

Loop stops, `p_l = p_4 = 1 != 2`.

Still incorrect.

Another attempt: swap positions 1 and 3: [3, 1, 4, 