To determine the final output state after all iterations of the loop, we need to understand the pattern of how the `answer` list and the `a` list are modified in each iteration.

Given:
- `answer` starts as `[1]`.
- `a` starts as `[1, -1]`.
- `n` is the length of `array`, which is a list of integers from 1 to `n`.
- The loop runs from `i = 1` to `i = n-1`.

Let's break down the loop behavior:
- For odd `i`, `answer.append(array[a[-1]])` and `a[-1] -= 1`. This means we append the element at the index `a[-1]` of `array` to `answer` and then decrement `a[-1]`.
- For even `i`, `answer.append(array[a[0]])` and `a[0] += 1`. This means we append the element at the index `a[0]` of `array` to `answer` and then increment `a[0]`.

Initially, `a` is `[1, -1]`. The loop runs `n-1` times, so let's see how `answer` and `a` evolve:

1. **First Iteration (i = 1, odd)**:
   - `answer.append(array[a[-1]])` → `answer.append(array[-1])` → `answer.append(n)`
   - `a[-1] -= 1` → `a[-1] = -2`
   - `answer` becomes `[1, n]`
   - `a` becomes `[1, -2]`

2. **Second Iteration (i = 2, even)**:
   - `answer.append(array[a[0]])` → `answer.append(array[1])` → `answer.append(2)`
   - `a[0] += 1` → `a[0] = 2`
   - `answer` becomes `[1, n, 2]`
   - `a` becomes `[2, -2]`

3. **Third Iteration (i = 3, odd)**:
   - `answer.append(array[a[-1]])` → `answer.append(array[-2])` → `answer.append(n-1)`
   - `a[-1] -= 1` → `a[-1] = -3`
   - `answer` becomes `[1, n, 2, n-1]`
   - `a` becomes `[2, -3]`

Following this pattern:
- For each odd `i`, we append the element at index `a[-1]` of `array` to `answer` and decrement `a[-1]`.
- For each even `i`, we append the element at index `a[0]` of `array` to `answer` and increment `a[0]`.

By the end of the loop (`i = n-1`):
- `a[-1]` will have decremented to `-n` (since it starts at `-1` and decrements `n-1` times).
- `a[0]` will have incremented to `n` (since it starts at `1` and increments `n-2` times).

The `answer` list will contain elements from `n` down to `2` in alternating order with elements from `2` up to `n-1` in the remaining positions.

Thus, the final `answer` list will be `[1, n, 2, n-1, 3, n-2, ..., (n+1)//2, (n+1)//2]` if `n` is odd, or `[1, n, 2, n-1, 3, n-2, ..., n//2, n//2+1]` if `n` is even.

For simplicity, the final `answer` list will be `[1] + [n, 2, n-1, 3, n-2, ..., (n+1)//2, (n+1)//2]` if `n` is odd, or `[1] + [n, 2, n-1, 3, n-2, ..., n//2, n//2+1]` if `n` is even.

Output State: **[1] + [n, 2, n-1, 3, n-2, ..., (n+1)//2, (n+1)//2] if n is odd, or [1] + [n, 2, n-1, 3, n-2, ..., n//2, n//2+1] if n is even.**

In natural language: The final `answer` list will start with `1`, followed by a sequence of numbers that alternates between the largest remaining number in `array` and the smallest remaining number in `array`, until all numbers from `2` to `n` are included. The `a` list will end up as `[n, -n]`.