The code snippet `rem = k % (i + 1)` calculates the remainder of `k` divided by `(i + 1)` and assigns it to the variable `rem`.

Given the initial state:
- `t` is an integer where \(1 \leq t \leq 100\)
- `ii` is 0
- `n` is an integer greater than 1
- `k` is an integer greater than 0
- `a` is a sorted list of integers in ascending order
- `r` is `r + k`
- `rem` is 0
- `y` is 0
- `i` is 0
- The condition \((i + 1) * (a[i + 1] - a[i]) > k\) is true

Let's calculate the new value of `rem`:
- `i` is 0
- `k` is an integer greater than 0
- Therefore, `rem = k % (0 + 1) = k % 1 = 0`

The value of `rem` is now 0.

The other variables remain unchanged.

Output State: **`t` is an integer where \(1 \leq t \leq 100\), `ii` is 0, `n` is an integer greater than 1, `k` is an integer greater than 0, `a` is a sorted list of integers in ascending order, `r` is `r + k`, `rem` is 0, `y` is 0, `i` is 0, and the condition \((i + 1) * (a[i + 1] - a[i]) > k\) is true.**