To determine the output state, we need to evaluate the expression `ans = ans + (n + b) // (b * b)` given the initial state.

Given:
- `t` is an input integer such that 1 ≤ `t` ≤ 10^4.
- `n` and `m` are integers such that `min(n, m) >= 2`.
- `ans` is initially equal to `n`.
- `T` is incremented by 1.

The line of code modifies the value of `ans` using the formula `ans = ans + (n + b) // (b * b)`.

Let's break down the changes:
- `ans` was initially `n`.
- Now `ans` is updated to `n + (n + b) // (b * b)`.

Since `b` is not defined in the initial state, we'll keep it as `b` in our expression.

Therefore, the new value of `ans` is `n + (n + b) // (b * b)`.

The other variables (`t`, `m`, and `T`) remain unchanged except for `T` which was incremented by 1 in the initial state but no further changes are made to it in the provided code snippet.

Output State: **`t` is an input integer such that 1 ≤ `t` ≤ 10^4, `n` and `m` are integers such that `min(n, m) >= 2`, `ans` is `n + (n + b) // (b * b)`, `T` is incremented by 1.**