Correctness: **False**

### Explanation:
The provided solution does not correctly generate the array \(a\) that satisfies the given conditions. Specifically, the logic used to compute \(a_i\) from \(a_{i-1}\) and \(x_i\) is flawed. The current implementation sets \(a_0 = 500\) and then calculates \(a_i = a_{i-1} + x_{i-1}\), which does not ensure that \(x_i = a_i \bmod a_{i-1}\).

To fix this, we need to ensure that \(a_i\) is chosen such that \(x_i = a_i \bmod a_{i-1}\). One way to achieve this is to set \(a_i = x_i \cdot a_{i-1} + a_{i-1}\), ensuring that \(x_i = a_i \bmod a_{i-1}\).

Here's a corrected version of the function:

```python
def func():
    for _ in range(int(input())):
        n = int(input())
        x = list(map(int, input().split()))
        a = [0] * n
        a[0] = 1  # Start with a[0] as 1, can be any positive integer but 1 simplifies calculations
        for i in range(1, n):
            a[i] = x[i - 1] * a[i - 1] + a[i - 1]  # Ensure x_i = a_i % a_{i-1}
        print(*a)
```

This version ensures that the conditions are met by constructing \(a_i\) such that \(x_i = a_i \bmod a_{i-1}\).