To determine the output of the `print` statement, we need to carefully evaluate the expressions for `a`, `b`, and the final expression `a * 2 + b * 2 + (n - i)` based on the given initial state.

### Step-by-Step Evaluation:

1. **Identify the Values of Relevant Variables:**
   - `A = [0, 2, 4, 7]`
   - `idx_A = [3, 5, 6, 7]`
   - `B = [0, 1, 3, 6]`
   - `idx_B = [3, 2, 1, 0]`
   - `n > 0` (specific value of `n` is not provided)
   - `s[i]` is either '>' or not '>', but its specific value is not needed for this calculation.
   - `i = 1`
   - `r` and `l` are not explicitly defined in the initial state, so we need to assume their values based on typical usage in such problems.

2. **Evaluate `a`:**
   - `a = B[r - 1] + (idx_B[r - 1] - 1) * r`
   - Since `r` is not specified, let's assume `r = 2` for demonstration purposes (as it is a common choice for such indices).
     - `B[r - 1] = B[1] = 1`
     - `idx_B[r - 1] = idx_B[1] = 2`
     - Therefore, `a = 1 + (2 - 1) * 2 = 1 + 2 = 3`

3. **Evaluate `b`:**
   - `b = b + (1 - idx_A[l - 1]) * r`
   - Since `b` is not initialized, let's assume `b = 0` initially.
   - Also, `l` is not specified, so let's assume `l = 2` for demonstration purposes.
     - `idx_A[l - 1] = idx_A[1] = 5`
     - Therefore, `b = 0 + (1 - 5) * 2 = 0 + (-4) * 2 = -8`

4. **Evaluate the Final Expression:**
   - `a * 2 + b * 2 + (n - i)`
   - Substituting the values of `a`, `b`, and `i`:
     - `a * 2 = 3 * 2 = 6`
     - `b * 2 = -8 * 2 = -16`
     - `(n - i) = n - 1`
     - Therefore, the final expression becomes `6 - 16 + (n - 1) = -10 + (n - 1) = n - 11`

### Conclusion:
Given the assumptions for `r` and `l`, the output of the `print` statement will be `n - 11`. Since the exact value of `n` is not provided, we express the output in terms of `n`.

Output: **n - 11 (where n is a positive integer greater than 0)**