Reasoning:  
The problem requires calculating the difference between the sum of cubes of the first `n` natural numbers and the sum of the first `n` natural numbers. The formula for the sum of the first `n` natural numbers is \( \text{sum\_n} = \frac{n(n+1)}{2} \). The sum of the cubes of the first `n` natural numbers is \( \left(\frac{n(n+1)}{2}\right)^2 \), which is the square of the sum of the first `n` natural numbers.

The function `func_1` correctly calculates `sum_n` and `sum_cubes_n`:
- `sum_n` is calculated as `n * (n + 1) // 2`.
- `sum_cubes_n` is calculated as `sum_n ** 2`.

The function then returns the difference `sum_cubes_n - sum_n`.

Let's verify the correctness with the provided test cases:
- For `n = 3`:
  - `sum_n = 3 * (3 + 1) // 2 = 6`
  - `sum_cubes_n = 6 ** 2 = 36`
  - Difference: `36 - 6 = 30`
  - Test case `func_1(3) == 30` passes.

- For `n = 5`:
  - `sum_n = 5 * (5 + 1) // 2 = 15`
  - `sum_cubes_n = 15 ** 2 = 225`
  - Difference: `225 - 15 = 210`
  - Test case `func_1(5) == 210` passes.

- For `n = 2`:
  - `sum_n = 2 * (2 + 1) // 2 = 3`
  - `sum_cubes_n = 3 ** 2 = 9`
  - Difference: `9 - 3 = 6`
  - Test case `func_1(2) == 6` passes.

All test cases pass, and the function behaves as expected according to the problem description.

Correctness: **True**