The code snippet `b[i] = b[i - 1] + x` updates the value of `b[i]` based on the previous value of `b[i - 1]` and the value of `x`.

Given:
- `b` is a list of `n + 1` integers, all initialized to 0.
- `i` is 1.
- `x` is 1 if `a[1] > 1` else 2.

Since `b` is initialized to all zeros, `b[i - 1]` is `b[0]`, which is 0. Therefore, `b[i]` becomes `0 + x`, which is simply `x`.

So, `b[1]` is now equal to `x`.

Output State: **`t` is an integer such that 1 <= t <= 10^4; `n` is an integer such that 1 <= n <= 3 * 10^5; `q` is an integer such that 1 <= q <= 3 * 10^5; `c` is a list of `n` integers where each element is greater than 0 (1 <= c_i <= 10^9); `a` is a list of `n + 1` integers where the first element is 0 and the remaining `n` elements are the integers read from the input; `b` is a list of `n + 1` integers, with `b[1]` equal to `x` and all other elements still 0; `i` is 1; `x` is 1 if `a[1] > 1` else 2.**