The code snippet updates the value of `b[i]` based on the previous value of `b[i-1]` and the value of `x`. Given the initial state, `b[1]` is `x` and all other elements of `b` are 0. Since `i` is initially 2, the code updates `b[2]` to be `b[1] + x`.

Here are the specific changes:
- `b[2]` is updated to `b[1] + x`, which is `x + x` since `b[1]` is `x`.
- The value of `x` is determined by the condition `x = 1 if a[2] > 1 else 2`.

Therefore, `b[2]` will be `2 * x`.

Output State: **`t` is an integer such that 1 <= t <= 10^4; `n` is an integer such that 1 <= n <= 3 * 10^5; `q` is an integer such that 1 <= q <= 3 * 10^5; `c` is a list of `n` integers where each element is greater than 0 (1 <= c_i <= 10^9); `a` is a list of `n + 1` integers where the first element is 0 and the remaining `n` elements are the integers read from the input; `b` is a list of `n + 1` integers, with `b[1]` equal to `x` and `b[2]` equal to `2 * x`, and all other elements still 0; `i` is 2; `x` is 1 if `a[2] > 1` else 2**