Let's break down the initial state and the code snippet step by step to determine what will be printed.

### Initial State:
1. `t` is greater than 0.
2. `_` is 0.
3. `p1`, `p2`, and `p3` are input integers.
4. The sum of `p1`, `p2`, and `p3` is odd.
5. `p3` is less than `p1 + p2`.
6. `low` is the minimum of `p3 - p1` and `p3 - p2`.
7. `high` is the maximum of `p3 - p1` and `p3 - p2`.
8. `cur` is `low` or `low + 1`.
9. `high` must be greater than or equal to `low + 1`.

### Code Snippet:
```python
print(p1 - cur + p3)
```

### Step-by-Step Analysis:
1. **Determine `low` and `high`**:
   - `low` is the minimum of `p3 - p1` and `p3 - p2`.
   - `high` is the maximum of `p3 - p1` and `p3 - p2`.

2. **Determine `cur`**:
   - `cur` can be either `low` or `low + 1`.
   - Given that `high` must be greater than or equal to `low + 1`, `cur` can be either `low` or `low + 1`.

3. **Expression to Print**:
   - The expression `p1 - cur + p3` will be evaluated.
   - Since `cur` can be either `low` or `low + 1`, we need to consider both cases.

### Case 1: `cur = low`
- The expression becomes `p1 - low + p3`.
- `low` is the minimum of `p3 - p1` and `p3 - p2`.

### Case 2: `cur = low + 1`
- The expression becomes `p1 - (low + 1) + p3`.
- Simplifying, this becomes `p1 - low - 1 + p3`.

### Simplifying the Expression:
- **Case 1**: `p1 - low + p3`
  - If `low = p3 - p1`, then `p1 - (p3 - p1) + p3 = p1 - p3 + p1 + p3 = 2 * p1`.
  - If `low = p3 - p2`, then `p1 - (p3 - p2) + p3 = p1 - p3 + p2 + p3 = p1 + p2`.

- **Case 2**: `p1 - (low + 1) + p3`
  - If `low = p3 - p1`, then `p1 - (p3 - p1 + 1) + p3 = p1 - p3 + p1 - 1 + p3 = 2 * p1 - 1`.
  - If `low = p3 - p2`, then `p1 - (p3 - p2 + 1) + p3 = p1 - p3 + p2 - 1 + p3 = p1 + p2 - 1`.

### Conclusion:
- The expression `p1 - cur + p3` will print either `2 * p1` or `p1 + p2` if `cur = low`.
- The expression `p1 - cur + p3` will print either `2 * p1 - 1` or `p1 + p2 - 1` if `cur = low + 1`.

Since `cur` can be either `low` or `low + 1`, the output can be one of the following:
- `2 * p1`
- `p1 + p2`
- `2 * p1 - 1`
- `p1 + p2 - 1`

### Final Output:
Output: **p1 - cur + p3 (where `cur` is either `low` or `low + 1`, and `low` is the minimum of `p3 - p1` and `p3 - p2`)**