To provide the output state after the loop executes all the iterations, I need specific values for the variables `s`, `A`, `B`, `n`, `idx_B`, and `idx_A`. Since these values are not provided, I will assume some example values to demonstrate how to calculate the output state.

Let's assume:
- `s = "><>><<"`
- `A = [1, 2, 3, 4, 5]`
- `B = [6, 7, 8, 9, 10]`
- `n = 5`
- `idx_B = [4, 3, 2, 1]`
- `idx_A = [0, 1, 2, 3, 4]`
- `r = 5`
- `l = 0`

Now, let's go through the loop with these values:

1. `i = 0`: `s[0] == '<'`, so `r -= 1` and `r = 4`.
2. `i = 1`: `s[1] == '>'`, so we enter the if block with `l < r` (0 < 4).
   - `a = A[0] = 1`
   - `x = r - (l + 2) = 4 - (0 + 2) = 2`
   - `b = B[r - 1] = B[3] = 9`
   - `b = b - B[x] = 9 - 8 = 1`
   - `b = b - (idx_B[x] - idx_B[r - 1]) * (x + 1) = 1 - (2 - 3) * 3 = 1 + 3 = 4`
   - `b = (idx_B[r - 1] - i) * (l + 1) = (3 - 1) * 1 = 2`
   - `print(1 * 2 + 2 * 2 + 1 + 1) = 8`
3. `i = 2`: `s[2] == '>'`, so we enter the if block with `l < r` (0 < 4).
   - `a = A[0] = 1`
   - `x = r - (l + 2) = 4 - (0 + 2) = 2`
   - `b = B[r - 1] = B[3] = 9`
   - `b = b - B[x] = 9 - 8 = 1`
   - `b = b - (idx_B[x] - idx_B[r - 1]) * (x + 1) = 1 - (2 - 3) * 3 = 1 + 3 = 4`
   - `b = (idx_B[r - 1] - i) * (l + 1) = (3 - 2) * 1 = 1`
   - `print(1 * 2 + 1 * 2 + 2 + 1) = 7`
4. `i = 3`: `s[3] == '>'`, so we enter the if block with `l < r` (0 < 4).
   - `a = A[0] = 1`
   - `x = r - (l + 2) = 4 - (0 + 2) = 2`
   - `b = B[r - 1] = B[3] = 9`
   - `b = b - B[x] = 9 - 8 = 1`
   - `b = b - (idx_B[x] - idx_B[r - 1]) * (x + 1) = 1 - (2 - 3) * 3 = 1 + 3 = 4`
   - `b = (idx_B[r - 1] - i) * (l + 1) = (3 - 3) * 1 = 0`
   - `print(1 * 2 + 0 * 2 + 3 + 1) = 6`
5. `i = 4`: `s[4] == '<'`, so `r -= 1` and `r = 3`.
6. `i = 5`: `s[5] == '>'`, so we enter the if block with `l < r` (0 < 3).
   - `a = A[0] = 1`
   - `x = r - (l + 2) = 3 - (0 + 2) = 1`
   - `b = B[r - 1] = B[2] = 8`
   - `b = b - B[x] = 8 - 7 = 1`
   - `b = b - (idx_B[x] - idx_B[r - 1]) * (x + 1) = 1 - (3 - 2) * 2 = 1 - 2 = -1`
   - `b = (idx_B[r - 1] - i) * (l + 1) = (2 - 4) * 1 = -2`
   - `print(1 * 2 + (-1) * 2 + 5 + 1) = 4`

Output State: **8 7 6 4**