Let's break down the initial state and the code step by step:

1. **Initial State:**
   - `h`, `w`, `xa`, `ya`, `xb`, `yb` are integers.
   - `xa` is less than or equal to `xb`.
   - `x` is the absolute difference between `xa` and `xb` divided by 2. Since the absolute difference between `xa` and `xb` is odd, `x` will be an integer.
   - `l` is `yb - x` if `yb - x` is greater than or equal to 1, otherwise `l` is 1.
   - `r` is the minimum of `w` and `yb + x`.

2. **Code to Analyze:**
   ```python
   print(*(['Draw'], ['Alice'])[abs(l - ya) <= x + 1 and abs(r - ya) <= x + 1])
   ```

### Step-by-Step Analysis:

1. **Calculate `x`:**
   - `x = abs(xa - xb) // 2`.
   - Since `xa` is less than or equal to `xb` and their difference is odd, `x` is an integer.

2. **Calculate `l`:**
   - `l = yb - x` if `yb - x >= 1`, otherwise `l = 1`.
   - This means `l` is either `yb - x` or 1, depending on the value of `yb - x`.

3. **Calculate `r`:**
   - `r = min(w, yb + x)`.
   - This means `r` is the smaller of `w` and `yb + x`.

4. **Condition in the `print` Statement:**
   - The condition is `abs(l - ya) <= x + 1 and abs(r - ya) <= x + 1`.
   - We need to check if both conditions are true to determine which part of the list `['Draw'], ['Alice']` will be printed.

### Evaluating the Condition:

- **First Condition: `abs(l - ya) <= x + 1`**
  - If `l = yb - x`, then `abs(yb - x - ya) <= x + 1`.
  - If `l = 1`, then `abs(1 - ya) <= x + 1`.

- **Second Condition: `abs(r - ya) <= x + 1`**
  - If `r = w`, then `abs(w - ya) <= x + 1`.
  - If `r = yb + x`, then `abs(yb + x - ya) <= x + 1`.

Given the nature of the problem and the constraints, let's assume typical values for `xa`, `xb`, `ya`, `yb`, `w`, and `h` to illustrate the logic:

- Assume `xa = 1`, `xb = 3`, `ya = 2`, `yb = 4`, `w = 5`, `h = 6`.
- Then `x = abs(1 - 3) // 2 = 1`.
- `l = yb - x = 4 - 1 = 3` (since `yb - x >= 1`).
- `r = min(w, yb + x) = min(5, 4 + 1) = 5`.

Now, check the condition:
- `abs(l - ya) = abs(3 - 2) = 1 <= x + 1 = 2` (True).
- `abs(r - ya) = abs(5 - 2) = 3 > x + 1 = 2` (False).

Since one of the conditions is false, the condition `abs(l - ya) <= x + 1 and abs(r - ya) <= x + 1` is false.

### Final Output:
Output: **['Alice']**