Let's break down the initial state and the print statement step by step:

1. **Initial State Variables:**
   - `h`, `w`, `xa`, `xb`, `yb` are integers.
   - `r` is the minimum of `w` and `yb + x`. Here, `x` seems to be a typo and should likely be `xa` (since `xa` is used elsewhere). So, `r = min(w, yb + xa)`.
   - `xa` is less than or equal to `xb`.
   - The absolute difference between `xa` and `xb` is even.
   - `l` is the maximum of 1 and `ya - xa`. Here, `ya` is not defined in the initial state, so let's assume it is a typo and should be `yb`.

2. **Print Statement Analysis:**
   ```python
   print(*(['Draw'], ['Bob'])[abs(l - yb) <= x and abs(r - yb) <= x])
   ```
   - The expression inside the square brackets `[abs(l - yb) <= x and abs(r - yb) <= x]` determines which list to print from.
   - If `abs(l - yb) <= x` and `abs(r - yb) <= x` are both true, then the list `['Bob']` will be printed. Otherwise, the list `['Draw']` will be printed.

3. **Conditions to Determine the Printed List:**
   - `l = max(1, yb - xa)`.
   - `r = min(w, yb + xa)`.
   - We need to check if `abs(l - yb) <= x` and `abs(r - yb) <= x` are both true.

Given the conditions:
- Since `xa` is less than or equal to `xb` and the absolute difference between `xa` and `xb` is even, let's assume `xa` and `xb` are such that the conditions hold.
- Let's assume `yb - xa >= 1` (so `l = yb - xa`), and `yb + xa <= w` (so `r = yb + xa`).

For simplicity, let's assume:
- `yb - xa = 2` (so `l = 2`).
- `yb + xa = 4` (so `r = 4`).
- `x = 1` (a reasonable assumption for the context).

Then:
- `abs(l - yb) = abs(2 - yb)`.
- `abs(r - yb) = abs(4 - yb)`.

For `abs(l - yb) <= x` and `abs(r - yb) <= x` to be true:
- `abs(2 - yb) <= 1` implies `1 <= yb <= 3`.
- `abs(4 - yb) <= 1` implies `3 <= yb <= 5`.

Combining these, `yb` must be 3. With `yb = 3`:
- `l = 2` and `r = 4`.
- Both conditions `abs(2 - 3) <= 1` and `abs(4 - 3) <= 1` are true.

Therefore, the list `['Bob']` will be printed.

Output: **['Bob']**