Let's analyze the code step by step:

1. `total_sum` is updated to be the sum of its current value and `num`, modulo `MOD`.
2. The value of `num` is `l + 2`.
3. The value of `l` is an integer such that 1 <= `l` + 1 <= `r` < 10^18.
4. The initial value of `total_sum` is either `(l + 1) % MOD`, `(total_sum + 2*l + 1) % MOD`, or remains unchanged, either 0 or `(total_sum + l) % MOD`.

Now, let's calculate the new value of `total_sum`:

`total_sum` = (`total_sum` + `num`) % MOD
= (`total_sum` + `l` + 2) % MOD

Since `total_sum` can take multiple initial values, we'll consider each case separately:

* If `total_sum` is initially `(l + 1) % MOD`, then:
`total_sum` = (`(l + 1) % MOD` + `l` + 2) % MOD
= (`2*l` + 3) % MOD
* If `total_sum` is initially `(total_sum + 2*l + 1) % MOD`, then:
`total_sum` = (`(total_sum + 2*l + 1) % MOD` + `l` + 2) % MOD
= (`total_sum` + 3*l + 3) % MOD
* If `total_sum` is initially 0, then:
`total_sum` = (0 + `l` + 2) % MOD
= (`l` + 2) % MOD
* If `total_sum` is initially `(total_sum + l) % MOD`, then:
`total_sum` = (`(total_sum + l) % MOD` + `l` + 2) % MOD
= (`total_sum` + 2*l + 2) % MOD

In all cases, the value of `total_sum` is updated to a new value that depends on the initial value of `total_sum`, `l`, and `MOD`.

The output state is: `l` and `r` are integers such that 1 <= `l` + 1 <= `r` < 10^18, `k` is an integer such that 1 <= `k` <= 10, `num` is equal to `l + 2`, and `total_sum` is either (`2*l` + 3) % MOD, (`total_sum` + 3*l + 3) % MOD, (`l` + 2) % MOD, or (`total_sum` + 2*l + 2) % MOD.

Output State: **`l` and `r` are integers such that 1 <= `l` + 1 <= `r` < 10^18, `k` is an integer such that 1 <= `k` <= 10, `num` is equal to `l + 2`, and `total_sum` is either (`2*l` + 3) % MOD, (`total_sum` + 3*l + 3) % MOD, (`l` + 2) % MOD, or (`total_sum` + 2*l + 2) % MOD**