To understand what will be printed, let's break down the given information and the code step by step.

### Initial State:
- `p1` will contain the original elements of `vx` plus all `v1` values from `ops` where the condition `p1[-1] != v2` was true.
- `p2` will contain all `v1` values from `ops` where the condition `p1[-1] == v2` was true.

### Output Statement:
```
print('! %s' % ' '.join(map(str, p1[::-1] + p2)), flush=True)
```

### Analysis:
1. **`p1[::-1]`**: This reverses the list `p1`. The `[::-1]` slice notation is used to reverse the list.
2. **`p1[::-1] + p2`**: This concatenates the reversed `p1` list with the `p2` list.
3. **`map(str, ...)`**: This converts each element in the concatenated list to a string.
4. **`' '.join(...)`**: This joins all the string elements of the concatenated list into a single string, separated by spaces.
5. **`'! %s' % ...`**: This formats the string to include an exclamation mark followed by the joined string.

### Final Output Description:
The code prints a string that starts with an exclamation mark, followed by the elements of the reversed `p1` list concatenated with the `p2` list, all separated by spaces.

### Output:
Output: **! [reversed elements of p1] [elements of p2] (where [reversed elements of p1] are the elements of p1 in reverse order and [elements of p2] are the elements of p2)**

To make it more precise, let's assume some hypothetical values for `vx` and `ops` to illustrate how this would look:

#### Hypothetical Example:
- `vx = [1, 2, 3]`
- `ops = [(4, 3), (5, 2), (6, 3), (7, 4)]`

#### Step-by-Step Calculation:
1. **Initial `p1`**: `p1 = [1, 2, 3]`
2. **Processing `ops`**:
   - `(4, 3)`: `p1[-1] == 3` (True), so `p2 = [4]`
   - `(5, 2)`: `p1[-1] == 3` (True), so `p2 = [4, 5]`
   - `(6, 3)`: `p1[-1] == 3` (True), so `p2 = [4, 5, 6]`
   - `(7, 4)`: `p1[-1] == 3` (True), so `p2 = [4, 5, 6, 7]`
3. **Final `p1` and `p2`**:
   - `p1 = [1, 2, 3]`
   - `p2 = [4, 5, 6, 7]`
4. **Reversed `p1`**:
   - `p1[::-1] = [3, 2, 1]`
5. **Concatenated and Formatted Output**:
   - `' '.join(map(str, p1[::-1] + p2)) = '3 2 1 4 5 6 7'`
   - Final output: `'! 3 2 1 4 5 6 7'`

### Final Output:
Output: **! 3 2 1 4 5 6 7 (where 3 2 1 are the reversed elements of p1 and 4 5 6 7 are the elements of p2)**

However, since the exact values of `vx` and `ops` are not provided, the general answer is:

Output: **! [reversed elements of p1] [elements of p2] (where [reversed elements of p1] are the elements of p1 in reverse order and [elements of p2] are the elements of p2)**