To solve this, let's break down the given code and its impact on the variables:

1. **Initial State:**
   - `t` is an integer where 0 ≤ t ≤ 10^4
   - `n` is an integer where 2 ≤ n ≤ 10^5
   - `a` is a list of `n` integers where 0 ≤ a_1 < a_2 < ... < a_n ≤ 10^9
   - `m` is an integer where 1 ≤ m ≤ 10^5
   - `b` is now `[0, 0, v]`, where `v` is `y - x`
   - `v` is `y - x`
   - `w` and `z` are not defined in the initial state, so we assume they are known constants or variables.

2. **Code Execution:**
   ```python
   b += b[-2] + v ** (v > x - w), b[-1] + v ** (v > z - y)
   ```

3. **Step-by-Step Impact:**
   - `b[-2]` is the second last element of `b`, which is `0`.
   - `b[-1]` is the last element of `b`, which is `v`.
   - `v ** (v > x - w)` evaluates to `v` if `v > x - w` is true, otherwise it evaluates to `1` (since `v ** 0` is `1`).
   - `v ** (v > z - y)` evaluates to `v` if `v > z - y` is true, otherwise it evaluates to `1`.

4. **Calculations:**
   - The new elements added to `b` are:
     - `b[-2] + v ** (v > x - w) = 0 + v ** (v > x - w)`
     - `b[-1] + v ** (v > z - y) = v + v ** (v > z - y)`

5. **Final State:**
   - If `v > x - w` is true, the first new element is `v`.
   - If `v > x - w` is false, the first new element is `1`.
   - If `v > z - y` is true, the second new element is `2v`.
   - If `v > z - y` is false, the second new element is `v + 1`.

Therefore, the updated list `b` will be:
- If `v > x - w` and `v > z - y` are both true: `b = [0, 0, v, v, 2v]`
- If `v > x - w` is true and `v > z - y` is false: `b = [0, 0, v, v, v + 1]`
- If `v > x - w` is false and `v > z - y` is true: `b = [0, 0, v, 1, 2v]`
- If `v > x - w` and `v > z - y` are both false: `b = [0, 0, v, 1, v + 1]`

Output State: **`t` is an integer where 0 ≤ t ≤ 10^4, `n` is an integer where 2 ≤ n ≤ 10^5, `a` is a list of `n` integers where 0 ≤ a_1 < a_2 < ... < a_n ≤ 10^9, `m` is an integer where 1 ≤ m ≤ 10^5, `b` is now `[0, 0, v, v ** (v > x - w), v + v ** (v > z - y)]`.**