Let's break down the initial state and the print statement to determine what will be printed:

### Initial State:
- `t` is an integer where 0 ≤ t ≤ 10^4.
- `n` is an integer where 2 ≤ n ≤ 10^5.
- `a` is a list of `n` integers where 0 ≤ a_1 < a_2 < ... < a_n ≤ 10^9.
- `m` is an integer where 1 ≤ m ≤ 10^5.
- `b` is a list with length `n-3` appended to the initial `[0, 0]`. Each element in `b` from index 2 onwards is calculated as follows: `b[i] = b[i-2] + (y - x)`, where `y` and `x` are elements from the list `a`.

### Print Statement:
```python
print(b, 'B')
```

### Step-by-Step Analysis:
1. **Initialization of `b`:**
   - `b` starts as `[0, 0]`.
   - The length of `b` is extended to `n-3` elements, making the total length of `b` equal to `n-1`.

2. **Calculation of `b` elements:**
   - For each index `i` starting from 2 (since `b[0]` and `b[1]` are already 0), the value of `b[i]` is calculated as `b[i-2] + (y - x)`.
   - Here, `y` and `x` are elements from the list `a`. Specifically, `y` is `a[i+1]` and `x` is `a[i-1]`.

3. **Final Structure of `b`:**
   - The first two elements of `b` are always `[0, 0]`.
   - The subsequent elements are calculated based on the formula `b[i] = b[i-2] + (a[i+1] - a[i-1])`.

### Example Calculation:
Let's assume `a = [1, 2, 3, 4, 5]` and `n = 5`:
- `b` starts as `[0, 0]`.
- For `i = 2`:
  - `b[2] = b[0] + (a[3] - a[1]) = 0 + (4 - 2) = 2`.
- For `i = 3`:
  - `b[3] = b[1] + (a[4] - a[2]) = 0 + (5 - 3) = 2`.
- For `i = 4`:
  - `b[4] = b[2] + (a[5] - a[3]) = 2 + (6 - 4) = 4`.

So, `b` would be `[0, 0, 2, 2, 4]`.

### General Output:
Given the initial state and the calculation method, the print statement will output the list `b` followed by the string `'B'`.

Output: **[0, 0, b[2], b[3], ..., b[n-1]] B (where b[i] = b[i-2] + (a[i+1] - a[i-1]) for i ≥ 2)**

This output describes the list `b` with its elements calculated as specified, followed by the string `'B'`.