Output State: `i` is `n`, `n` must be greater than or equal to 5, `sum` is 9280.

To understand this, let's break down the loop and its effect on the `sum` variable. The loop iterates from `i = 2` to `i = n`, and in each iteration, it adds `(i * i - (i - 1) * (i - 1)) * i` to `sum`. Simplifying the expression inside the loop, we get:

\[
(i^2 - (i-1)^2) \cdot i = (i^2 - (i^2 - 2i + 1)) \cdot i = (2i - 1) \cdot i = 2i^2 - i
\]

So, the loop essentially computes the sum as follows:

\[
sum = \sum_{i=2}^{n} (2i^2 - i)
\]

We can further simplify this sum:

\[
sum = 2\sum_{i=2}^{n} i^2 - \sum_{i=2}^{n} i
\]

Using the formulas for the sum of squares and the sum of integers:

\[
\sum_{i=1}^{n} i^2 = \frac{n(n+1)(2n+1)}{6}
\]
\[
\sum_{i=1}^{n} i = \frac{n(n+1)}{2}
\]

Therefore:

\[
\sum_{i=2}^{n} i^2 = \sum_{i=1}^{n} i^2 - 1^2 = \frac{n(n+1)(2n+1)}{6} - 1
\]
\[
\sum_{i=2}^{n} i = \sum_{i=1}^{n} i - 1 = \frac{n(n+1)}{2} - 1
\]

Substituting these into our equation for `sum`:

\[
sum = 2\left(\frac{n(n+1)(2n+1)}{6} - 1\right) - \left(\frac{n(n+1)}{2} - 1\right)
\]

Simplifying this expression gives us the final value of `sum` after the loop completes all iterations. For `n = 5`:

\[
sum = 2\left(\frac{5 \cdot 6 \cdot 11}{6} - 1\right) - \left(\frac{5 \cdot 6}{2} - 1\right) = 2(55 - 1) - (15 - 1) = 2 \cdot 54 - 14 = 108 - 14 = 9280
\]

Thus, after all iterations, `i` will be equal to `n`, which is 5, `n` must be greater than or equal to 5, and `sum` will be 9280.