Based on the initial state described:

- `sum` is the sum calculated by the loop for the given `n`.
- The loop runs from `i = 2` to `i = n`, and the final value of `sum` is the result of the expression \((i * i - (i - 1) * (i - 1)) * i\) for each `i` from 2 to `n`, summed up.
- After the loop, `j` remains `n+1` as it is not affected by the loop.
- After the loop, `i` will be `n+1`.
- `n` remains unchanged as it is an input parameter.

For the example where `n` is 5, the loop calculates `sum` as follows:
- For `i = 2`: \(2^2 - 1^2) * 2 = 6\)
- For `i = 3`: \(3^2 - 2^2) * 3 = 15\)
- For `i = 4`: \(4^2 - 3^2) * 4 = 28\)
- For `i = 5`: \(5^2 - 4^2) * 5 = 45\)

So, `sum` will be \(6 + 15 + 28 + 45 = 94\).

After the loop, `j` is `n + 1 = 5 + 1 = 6`, `i` is `n + 1 = 5 + 1 = 6`, and `n` remains 5.

The print statement `print(sum, n + n)` will output the values of `sum` and `n + n`.

Output: **94, 10**