# Test 1
**Input**: 
```
1
10
```
**Output**: 
```
5
```
*Explanation*: For \(x = 10\), the value of \(y\) that maximizes \(\gcd(10, y) + y\) is \(5\). Here, \(\gcd(10, 5) + 5 = 5 + 5 = 10\).

# Test 2
**Input**: 
```
1
7
```
**Output**: 
```
6
```
*Explanation*: For \(x = 7\), the value of \(y\) that maximizes \(\gcd(7, y) + y\) is \(6\). Here, \(\gcd(7, 6) + 6 = 1 + 6 = 7\).

# Test 3
**Input**: 
```
1
21
```
**Output**: 
```
18
```
*Explanation*: For \(x = 21\), the value of \(y\) that maximizes \(\gcd(21, y) + y\) is \(18\). Here, \(\gcd(21, 18) + 18 = 3 + 18 = 21\).

# Test 4
**Input**: 
```
1
100
```
**Output**: 
```
98
```
*Explanation*: For \(x = 100\), the value of \(y\) that maximizes \(\gcd(100, y) + y\) is \(98\). Here, \(\gcd(100, 98) + 98 = 2 + 98 = 100\).

# Test 5
**Input**: 
```
1
2
```
**Output**: 
```
1
```
*Explanation*: For \(x = 2\), the value of \(y\) that maximizes \(\gcd(2, y) + y\) is \(1\). Here, \(\gcd(2, 1) + 1 = 1 + 1 = 2\).

# Test 6
**Input**: 
```
1
1000
```
**Output**: 
```
750
```
*Explanation*: For \(x = 1000\), the value of \(y\) that maximizes \(\gcd(1000, y) + y\) is \(750\). Here, \(\gcd(1000, 750) + 750 = 250 + 750 = 1000\).

# Test 7
**Input**: 
```
1
6
```
**Output**: 
```
3
```
*Explanation*: For \(x = 6\), the value of \(y\) that maximizes \(\gcd(6, y) + y\) is \(3\). Here, \(\gcd(6, 3) + 3 = 3 + 3 = 6\).

# Test 8
**Input**: 
```
3
11
13
17
```
**Output**: 
```
6
6
8
```
*Explanation*: For \(x = 11\), the value of \(y\) that maximizes \(\gcd(11, y) + y\) is \(6\). Here, \(\gcd(11, 6) + 6 = 1 + 6 = 7\).
For \(x = 13\), the value of \(y\) that maximizes \(\gcd(13, y) + y\) is \(6\). Here, \(\gcd(13, 6) + 6 = 1 + 6 = 7\).
For \(x = 17\), the value of \(y\) that maximizes \(\gcd(17, y) + y\) is \(8\). Here, \(\gcd(17, 8) + 8 = 1 + 8 = 9\).

# Test 9
**Input**: 
```
3
1001
1002
1003
```
**Output**: 
```
501
501
502
```
*Explanation*: For \(x = 1001\), the value of \(y\) that maximizes \(\gcd(1001, y) + y\) is \(501\). Here, \(\gcd(1001, 501) + 501 = 1 + 501 = 502\).
For \(x = 1002\), the value of \(y\) that maximizes \(\gcd(1002, y) + y\) is \(501\). Here, \(\gcd(1002, 501) + 501 = 3 + 501 = 504\).
For \(x = 1003\), the value of \(y\) that maximizes \(\gcd(1003, y) + y\) is \(502\). Here, \(\gcd(1003, 502) + 502 = 1 + 502 = 503\).

# Test 10
**Input**: 
```
3
2
3
4
```
**Output**: 
```
1
1
2
```
*Explanation*: For \(x = 2\), the value of \(y\) that maximizes \(\gcd(2, y) + y\) is \(1\). Here, \(\gcd(2, 1) + 1 = 1 + 1 = 2\).
For \(x = 3\), the value of \(y\) that maximizes \(\gcd(3, y) + y\) is \(1\). Here, \(\gcd(3, 1) + 1 = 1 + 1 = 2\).
For \(x = 4\), the value of \(y\) that maximizes \(\gcd(4, y) + y\) is \(2\). Here, \(\gcd(4, 2) + 2 = 2 + 2 = 4\).