To determine the final output state after all iterations of the loop, we need to understand how the `sum` variable is updated in each iteration. The loop runs from `i = 2` to `i = n`, and in each iteration, the `sum` is updated as follows:

\[ \text{sum} += (i^2 - (i-1)^2) \times i \]

Let's simplify the expression inside the loop:

\[ i^2 - (i-1)^2 = i^2 - (i^2 - 2i + 1) = 2i - 1 \]

So the expression becomes:

\[ \text{sum} += (2i - 1) \times i = 2i^2 - i \]

Now, let's calculate the final `sum` for a general `n`. We need to sum up the expression \(2i^2 - i\) from \(i = 2\) to \(i = n\).

\[ \text{sum} = 1 + \sum_{i=2}^{n} (2i^2 - i) \]

We can split this sum into two separate sums:

\[ \text{sum} = 1 + 2\sum_{i=2}^{n} i^2 - \sum_{i=2}^{n} i \]

Using the formulas for the sum of squares and the sum of the first \(n\) integers:

\[ \sum_{i=1}^{n} i^2 = \frac{n(n+1)(2n+1)}{6} \]
\[ \sum_{i=1}^{n} i = \frac{n(n+1)}{2} \]

So,

\[ \sum_{i=2}^{n} i^2 = \sum_{i=1}^{n} i^2 - 1^2 = \frac{n(n+1)(2n+1)}{6} - 1 \]
\[ \sum_{i=2}^{n} i = \sum_{i=1}^{n} i - 1 = \frac{n(n+1)}{2} - 1 \]

Substituting these into the expression for `sum`:

\[ \text{sum} = 1 + 2\left(\frac{n(n+1)(2n+1)}{6} - 1\right) - \left(\frac{n(n+1)}{2} - 1\right) \]
\[ \text{sum} = 1 + \frac{n(n+1)(2n+1)}{3} - 2 - \frac{n(n+1)}{2} + 1 \]
\[ \text{sum} = \frac{n(n+1)(2n+1)}{3} - \frac{n(n+1)}{2} \]
\[ \text{sum} = \frac{2n(n+1)(2n+1) - 3n(n+1)}{6} \]
\[ \text{sum} = \frac{n(n+1)(4n+2 - 3)}{6} \]
\[ \text{sum} = \frac{n(n+1)(4n-1)}{6} \]

This is the final expression for the `sum` after the loop completes.

Given the initial state and the loop logic, the final output state is:

Output State: **`n` is an input integer, `j` is an input integer + 1, `t` is t - 1, `sum` is \(\frac{n(n+1)(4n-1)}{6}\)**.

In natural language, the final state of the variables after the loop completes is that `n` remains the input integer, `j` remains the input integer plus one, `t` remains the initial value minus one, and `sum` is calculated as \(\frac{n(n+1)(4n-1)}{6}\).