`a2` is assigned the value `y * (a - (n - b1))`. Given the conditions in the initial state:

- `a1 = a - x`
- `b1 = b - y`
- `min(a1, b1) < n`
- `max(a1, b1) != n`
- The current value of `max(a1, b1)` is greater than `n`
- `a1 >= b1`

Since `a1 >= b1` and `max(a1, b1)` is greater than `n`, `a1` must be the maximum and therefore `a1 > n`.

Let's substitute `a1` and `b1` into the expression for `a2`:

- `a1 = a - x`
- `b1 = b - y`

Thus, `a2 = y * (a - (n - b1))` can be rewritten using `b1` as:

- `a2 = y * (a - (n - (b - y)))`
- `a2 = y * (a - n + b - y)`
- `a2 = y * (a + b - n - y)`

Therefore, the output state is:

Output State: **`a`, `b`, `x`, `y`, and `n` are updated with the values returned by `func_3()`, `(a - x + (b - y)) > n`, `a1 = a - x`, `b1 = b - y`, `min(a1, b1) < n`, `max(a1, b1) != n`, `max(a1, b1) > n`, `a1 >= b1`, `a2 = y * (a + b - n - y)`**