The code snippet `b2 = b * (a - n)` assigns a new value to the variable `b2`. This value is calculated as `b` multiplied by the difference between `a` and `n`.

Given the initial state:
- `a`, `b`, `x`, `y`, and `n` are updated with the values returned by `func_3()`.
- `(a - x + (b - y)) > n`
- `a1 = a - x`
- `b1 = b - y`
- `min(a1, b1) < n`
- `max(a1, b1) != n`
- `max(a1, b1) > n`
- `a1 >= b1`
- `a2 = y * (a + b - n - y)`

After executing the code snippet:
- `b2` is now assigned the value of `b * (a - n)`.

The rest of the conditions and values remain unchanged. Therefore, the output state is:

Output State: **`a`, `b`, `x`, `y`, and `n` are updated with the values returned by `func_3()`, `(a - x + (b - y)) > n`, `a1 = a - x`, `b1 = b - y`, `min(a1, b1) < n`, `max(a1, b1) != n`, `max(a1, b1) > n`, `a1 >= b1`, `a2 = y * (a + b - n - y)`, `b2 = b * (a - n)`**