`a2` is assigned the value of `x * (b - (n - a1))`. 

Given the preconditions:
- `a1 = a - x`
- `b1 = b - y`
- `min(a1, b1) < n`
- `max(a1, b1) <= n`
- `a1 < b1`

We know that `a1 < b1` and both `a1` and `b1` are less than or equal to `n`.

Thus, the expression `b - (n - a1)` simplifies to `b - n + a1`.

So, `a2` becomes `x * (b - n + a1)`.

Since `a1` is `a - x`, the expression for `a2` is `x * (b - n + (a - x))`, which simplifies to `x * (b - n + a - x)`.

Therefore, the Output State is:
**`a`, `b`, `x`, `y`, and `n` are updated with the values returned by `func_3()`, `(a - x + (b - y)) > n`, `a1 = a - x`, `b1 = b - y`, `min(a1, b1) < n`, `max(a1, b1) <= n`, `a1 < b1`, `a2 = x * (b - n + a - x)`**