The given code snippet is:
```python
b2 = a * (b - n)
```

From the initial state, we know:
- `a1 = a - x`
- `b1 = b - y`
- `min(a1, b1) < n`
- `max(a1, b1) <= n`
- `a1 < b1`
- `a2 = x * (b - n + a - x)`

The new variable `b2` is introduced and assigned the value `a * (b - n)`.

Let's update the state accordingly:

- `a`, `b`, `x`, `y`, and `n` remain unchanged.
- `a1` remains `a - x`.
- `b1` remains `b - y`.
- `a2` remains `x * (b - n + a - x)`.
- `b2` is now `a * (b - n)`.

The conditions `min(a1, b1) < n`, `max(a1, b1) <= n`, and `a1 < b1` are still valid as they do not depend on the new assignment.

Therefore, the Output State is:
**`a`, `b`, `x`, `y`, and `n` are updated with the values returned by `func_3()`, `(a - x + (b - y)) > n`, `a1 = a - x`, `b1 = b - y`, `min(a1, b1) < n`, `max(a1, b1) <= n`, `a1 < b1`, `a2 = x * (b - n + a - x)`, `b2 = a * (b - n)`**