The code `a2 = x * (a - (n - b1))` updates the value of `a2`. To determine the new value of `a2`, we need to evaluate the expression `x * (a - (n - b1))`.

Given the initial state:
- `a`, `b`, `x`, `y`, and `n` are updated with the values returned by `func_3()`.
- `(a - x + (b - y)) > n`.
- `a1 = a - x`.
- `b1 = b - y`.
- `min(a1, b1) < n`.
- `max(a1, b1) <= n`.
- `a1 >= b1`.

From the given conditions:
- `a1 = a - x`.
- `b1 = b - y`.
- `a1 >= b1`.

We can substitute `a1` and `b1` into the expression for `a2`:
- `a2 = x * (a - (n - b1))`.
- Since `b1 = b - y`, we can rewrite the expression as:
  - `a2 = x * (a - (n - (b - y)))`.
  - Simplifying further:
    - `a2 = x * (a - n + b - y)`.

Therefore, the value of `a2` is `x * (a - n + b - y)`.

The other conditions remain unchanged:
- `(a - x + (b - y)) > n`.
- `a1 = a - x`.
- `b1 = b - y`.
- `min(a1, b1) < n`.
- `max(a1, b1) <= n`.
- `a1 >= b1`.

Output State: **`a`, `b`, `x`, `y`, and `n` are updated with the values returned by `func_3()`, `(a - x + (b - y)) > n`, `a1 = a - x`, `b1 = b - y`, `min(a1, b1) < n`, `max(a1, b1) <= n`, `a1 >= b1`, `a2 = x * (a - n + b - y)`**.