To determine the new value of `b` after executing the given code snippet, we will use the provided initial state values.

Given:
- `x` is 2
- `r` is 4
- `idx_B` is [3, 2, 1, 0]

The expression for `b` is:
\[ b = b - (\text{idx\_B}[x] - \text{idx\_B}[r - 1]) \times (x + 1) \]

Substituting the known values:
\[ b = 3 - (\text{idx\_B}[2] - \text{idx\_B}[3]) \times (2 + 1) \]
\[ b = 3 - (1 - 0) \times 3 \]
\[ b = 3 - 1 \times 3 \]
\[ b = 3 - 3 \]
\[ b = 0 \]

All other variables remain unchanged.

Output State: **`A` is [0, 2, 4, 7], `idx_A` is [3, 5, 6, 7], `B` is [0, 1, 3, 6], `idx_B` is [3, 2, 1, 0], `l` is 0, `r` is 4, `n` is greater than 0, `s[i]` is `'>'`, `a` is 0, `x` is 2, `b` is 0, and `l` is less than `r`. Additionally, `x` is greater than or equal to 0.**