To determine what will be printed, let's break down the given initial state and the print statement step by step:

### Initial State Breakdown:
- `A = [0, 2, 4, 7]`
- `idx_A = [3, 5, 6, 7]`
- `B = [0, 1, 3, 6]`
- `idx_B = [3, 2, 1, 0]`
- `n` is greater than 0 (specific value not provided, but it exists and is positive).
- `s[i]` is either '>' or not '>', specifically `i` is 1 (so `s[1]` is relevant, but its exact value is not provided).
- `r` is defined based on the conditions involving `r_initial` and `l`.
- `a` is defined as `B[r_initial - 1]`.
- `b` is defined as `-8` if `r_initial` is 2 and `l` is 1.

### Print Statement Analysis:
The print statement is:
```python
print(a * 2 + b * 2 + (n - i), end=' ')
```

Let's break down the expression inside the print statement:
1. **`a * 2`**: Since `a = B[r_initial - 1]`, we need the value of `r_initial` to determine `a`. However, `r_initial` is not directly provided. Let's assume `r_initial` is such that we can determine `a`.
2. **`b * 2`**: `b` is `-8` if `r_initial` is 2 and `l` is 1. If this condition is met, `b * 2` will be `-16`. Otherwise, `b` is not specified, so we'll consider the condition met for this example.
3. **`(n - i)`**: Given `i = 1`, this becomes `(n - 1)`.

### Determining Values:
- Assume `r_initial = 2` and `l = 1` to satisfy the condition for `b = -8`.
- Therefore, `a = B[r_initial - 1] = B[1] = 1`.

Now we can substitute these values into the expression:
- `a * 2 = 1 * 2 = 2`
- `b * 2 = -8 * 2 = -16`
- `(n - i) = (n - 1)`

So the expression becomes:
\[ 2 + (-16) + (n - 1) = 2 - 16 + n - 1 = n - 15 \]

### Final Output:
The print statement will output `n - 15` followed by a space.

Output: **n - 15 ** (where n is a positive integer greater than 0)