To determine the output state, let's break down the given code and apply the initial conditions:

Initial State:
- `A` is `[0, 2, 4, 7]`
- `idx_A` is `[3, 5, 6, 7]`
- `B` is `[0, 1, 3, 6]`
- `idx_B` is `[3, 2, 1, 0]`
- `n` is greater than 0
- `s[i]` is either `'>'` or not `'>'`
- `i` is 2
- `a` is 4
- `x` is `r - (l + 2)`
- `b` is `B[r - 1] - B[x]`

Given Code:
```python
b = b - (idx_B[x] - idx_B[r - 1]) * (x + 1)
```

We need to find the new value of `b` after executing the code.

First, let's identify the current values of `x` and `r`. Since `x` is defined as `r - (l + 2)`, we need to know the values of `r` and `l`. However, `r` and `l` are not explicitly defined in the initial state. For the sake of this example, let's assume hypothetical values for `r` and `l` that would make `x` a valid index within the bounds of `idx_B`.

Let's assume `r = 3` and `l = 0` for simplicity:
- `x = r - (l + 2) = 3 - (0 + 2) = 1`

Now, we can compute the value of `b` before the operation:
- `b = B[r - 1] - B[x] = B[2] - B[1] = 3 - 1 = 2`

Next, we substitute the values into the given code:
- `b = b - (idx_B[x] - idx_B[r - 1]) * (x + 1)`
- `b = 2 - (idx_B[1] - idx_B[2]) * (1 + 1)`
- `b = 2 - (2 - 1) * 2`
- `b = 2 - 1 * 2`
- `b = 2 - 2`
- `b = 0`

Thus, the new value of `b` is 0.

Output State: **`A` is `[0, 2, 4, 7]`; `idx_A` is `[3, 5, 6, 7]`; `B` is `[0, 1, 3, 6]`; `idx_B` is `[3, 2, 1, 0]`; `n` is greater than 0; `s[i]` is either `'>'` or not `'>'`; `i` is 2; `a` is 4; `x` is `r - (l + 2)`; `b` is 0**.