Let's break down the given initial state and the print statement to determine what will be printed.

### Initial State Breakdown:
- `A` is `[0, 2, 4, 7]`
- `idx_A` is `[3, 5, 6, 7]`
- `B` is `[0, 1, 3, 6]`
- `idx_B` is `[3, 2, 1, 0]`
- `n` is greater than 0 (specific value not provided, but it doesn't affect this calculation)
- `s[i]` is either `'>'` or not `'>'` (specific value not provided, but it doesn't affect this calculation)
- `i` is 2
- `r` is 1
- `a` is `2 + (2 - idx_A[l - 1]) * l`
- `b` is `2`

### Calculation Steps:
1. **Determine the value of `l`:**
   - The variable `l` is not explicitly defined in the initial state. However, since `a` depends on `l`, we need to infer its value. Given the context, `l` is likely an index or a counter used in a loop or similar structure. Since no further context is provided, we assume `l` is the same as `i` (a common pattern in such problems). Therefore, let's assume `l = 2`.

2. **Calculate `a`:**
   - `a = 2 + (2 - idx_A[l - 1]) * l`
   - Substituting `l = 2`:
     - `idx_A[l - 1]` is `idx_A[1]`, which is `5`.
     - So, `a = 2 + (2 - 5) * 2`
     - Simplifying inside the parentheses first: `2 - 5 = -3`
     - Then, multiply by `l`: `-3 * 2 = -6`
     - Finally, add `2`: `2 + (-6) = -4`
   - Therefore, `a = -4`.

3. **Calculate the expression in the print statement:**
   - The expression is `a * 2 + b * 2 + i + 1`
   - Substituting the known values:
     - `a = -4`
     - `b = 2`
     - `i = 2`
   - So, the expression becomes: `-4 * 2 + 2 * 2 + 2 + 1`
   - Simplify step-by-step:
     - `-4 * 2 = -8`
     - `2 * 2 = 4`
     - Adding these together with `i` and `1`: `-8 + 4 + 2 + 1`
     - Simplify further: `-8 + 4 = -4`, then `-4 + 2 = -2`, and finally `-2 + 1 = -1`
   - Therefore, the result of the expression is `-1`.

### Final Output:
The `print` statement will output the result of the expression `-1` followed by a space due to the `end=' '` argument.

Output: **-1 **