Output State: **`j` is 5, `sum` is 20, `i` is 2**

Explanation: The code updates the value of `sum` by adding `(i * i - (i - 1) * (i - 1)) * i` to the current value of `sum`. Given that `i` is initially 2, the expression `(i * i - (i - 1) * (i - 1)) * i` simplifies to `(2 * 2 - 1 * 1) * 2 = (4 - 1) * 2 = 3 * 2 = 6`. Therefore, `sum` is updated to `1 + 6 = 7`. However, since the problem does not specify that `i` should increment, we assume `i` remains 2. The values of `j` and `n` remain unchanged.