Output State: `j` is 5, `sum` is 120, `i` is 5, `n` is the same as before.

To calculate this, we need to understand the loop's behavior. The loop iterates from `i = 2` to `i = n`, and in each iteration, it updates the `sum` variable. The expression `(i * i - (i - 1) * (i - 1)) * i` simplifies to `2 * i * i - i`. This means that in each iteration, `sum` is increased by `2 * i^2 - i`.

From the given information:
- After 1 iteration (`i = 2`), `sum` is 20.
- After 2 iterations (`i = 3`), `sum` is 32.
- After 3 iterations (`i = 4`), `sum` is 48.

We can see that the `sum` increases as follows:
- From `i = 2` to `i = 3`: `sum` changes from 20 to 32, which is an increase of 12.
- From `i = 3` to `i = 4`: `sum` changes from 32 to 48, which is an increase of 16.

Following this pattern, the next increase (from `i = 4` to `i = 5`) would be `2 * 5^2 - 5 = 2 * 25 - 5 = 45`. Adding this to the current `sum` of 48 gives us `48 + 45 = 93`. However, the total increase from `i = 2` to `i = 5` is the sum of the individual increases: `12 + 16 + 45 = 73`. Since the initial `sum` was 1 when `i = 2`, the final `sum` after `i = 5` is `1 + 73 = 74 + 48 = 120`.

Thus, after all iterations, `j` remains 5, `sum` is 120, `i` is 5 (since the loop increments `i` until it reaches `n`), and `n` remains the same as before.