Output State: **`i` is 3, `n` must be at least 2, and `sum` is 2 * (2 * 2 - 1 * 1) * 2 = 6**.

Explanation: The code updates the `sum` variable by adding the value of `(i * i - (i - 1) * (i - 1)) * i`. Given that `i` is initially 2, the expression evaluates to `(2 * 2 - 1 * 1) * 2 = (4 - 1) * 2 = 3 * 2 = 6`. Thus, `sum` is updated to 6. After this operation, `i` is incremented to 3 (though this increment is not shown in the given code snippet, it is implied by the problem's nature). The precondition that `n` must be at least 2 remains unchanged.