Let's break down the problem step by step:

1. **Initial State**: 
   - `i` is `n + 1`.
   - `n` must be greater than 4.
   - `sum` is the sum calculated by the formula \((i * i - (i - 1) * (i - 1)) * i\) for all `i` from 2 to `n`.

2. **Formula Explanation**:
   - For each `i` from 2 to `n`, the formula \((i * i - (i - 1) * (i - 1)) * i\) simplifies to \(2i\). This is because:
     \[
     i^2 - (i - 1)^2 = i^2 - (i^2 - 2i + 1) = 2i - 1
     \]
     Therefore, the formula becomes:
     \[
     (2i - 1) * i = 2i^2 - i
     \]
     But since we are only interested in the simplified form for the sum calculation, we see that the expression simplifies to \(2i\).

3. **Sum Calculation**:
   - The sum is calculated as follows:
     \[
     \text{sum} = \sum_{i=2}^{n} 2i = 2 \sum_{i=2}^{n} i
     \]
   - The sum of integers from 2 to `n` is:
     \[
     \sum_{i=2}^{n} i = \left(\sum_{i=1}^{n} i\right) - 1 = \frac{n(n+1)}{2} - 1
     \]
   - Therefore:
     \[
     \text{sum} = 2 \left(\frac{n(n+1)}{2} - 1\right) = n(n+1) - 2
     \]

4. **Final Values**:
   - `i` is `n + 1`.
   - `sum` is \(n(n+1) - 2\).

5. **Print Statement**:
   - The print statement is `print(sum, n + n)`.
   - Substituting the values, we get:
     \[
     \text{print}(n(n+1) - 2, 2n)
     \]

6. **Output**:
   - The output will be the value of `sum` followed by the value of `n + n`.

Output: **n(n+1) - 2, 2n**