The code assigns new values to `l` and `r` based on the values of `i` and `p`. Specifically, `l` is set to `i - p` and `r` is set to `j + p`.

Given the initial conditions:
- `i` is \(2 * p + 1\)
- `j` is 0
- `p` is the maximum value satisfying the conditions \(j + p + 1 < n\) and \(i - p - 1 \geq 0\)

Let's calculate the new values for `l` and `r`:
- `l = i - p = (2 * p + 1) - p = p + 1`
- `r = j + p = 0 + p = p`

The values of other variables remain unchanged: `n`, `s`, `res`, `l`, `r`, `z`, `i`, `j`, `p`.

Therefore, the Output State is:
**`n` is the length of the string `s`, `s` is a string with a length greater than 0, `res` is a list of \(2 * n - 1\) elements, all set to 0, `l` is \(p + 1\), `r` is \(p\), `z` is 0, `i` is \(2 * p + 1\), `j` is 0, `p` is the maximum value that satisfies the condition \(j + p + 1 < n\) and \(i - p - 1 \geq 0\)**.