The code assigns the value of `(z + 1) // 2` to `i`. Given that `z` is `2 * n - 1`, we can substitute this into the equation to find the new value of `i`.

Let's calculate it:

- `z = 2 * n - 1`
- `i = (z + 1) // 2 = ((2 * n - 1) + 1) // 2 = (2 * n) // 2 = n`

So, the new value of `i` is `n`. The states of the other variables are not affected.

Output State: **`n` is the length of the string `s`, `s` is a string with a length greater than 0, `res` is a list of \(2 * n - 1\) elements, all set to 0 except for the first element which is now `p`, `l` is \(p + 1\), `r` is \(p\), `z` is \(2 * n - 1\), `i` is `n`, `j` is 0, `p` is the maximum value that satisfies the condition \(j + p + 1 < n\) and \(i - p - 1 \geq 0\)**