To determine what will be printed by the `print(p1 - cur + p3)` statement, let's break down the given initial state and the relationships between the variables.

1. **Variables and Initial State:**
   - `p1`, `p2`, `p3` are integers read from the input.
   - The sum of `p1`, `p2`, and `p3` is odd.
   - `p3` remains unchanged.
   - `low` is defined as the minimum of `p3 - p1` and `p3 - p2`.
   - `high` is defined as the maximum of `p3 - p1` and `p3 - p2`.
   - `cur` is set to `low`.
   - The condition `p1 - cur <= p2 - (p3 - cur)` holds true.

2. **Understanding `low` and `high`:**
   - `low = min(p3 - p1, p3 - p2)`
   - `high = max(p3 - p1, p3 - p2)`
   - `cur = low`

3. **Condition Analysis:**
   - Given `cur = low`, the condition `p1 - cur <= p2 - (p3 - cur)` must hold true.
   - This translates to `p1 - low <= p2 - (p3 - low)`, which simplifies to `p1 - low <= p2 - p3 + low`.
   - Rearranging, we get `p1 + p3 <= 2 * low + p2`.

4. **Expression to Print:**
   - The expression to be printed is `p1 - cur + p3`.
   - Since `cur = low`, the expression becomes `p1 - low + p3`.

5. **Substitute `low`:**
   - Recall that `low = min(p3 - p1, p3 - p2)`.
   - Therefore, `p1 - low + p3` can be analyzed based on the value of `low`.

6. **Two Cases for `low`:**
   - **Case 1:** `low = p3 - p1`
     - Then `p1 - low + p3 = p1 - (p3 - p1) + p3 = p1 - p3 + p1 + p3 = 2 * p1`.
   - **Case 2:** `low = p3 - p2`
     - Then `p1 - low + p3 = p1 - (p3 - p2) + p3 = p1 - p3 + p2 + p3 = p1 + p2`.

7. **Condition Verification:**
   - We need to verify which case satisfies the condition `p1 - cur <= p2 - (p3 - cur)`.
   - For `low = p3 - p1`:
     - The condition becomes `p1 - (p3 - p1) <= p2 - (p3 - (p3 - p1))` which simplifies to `2 * p1 - p3 <= p2 - p1` or `3 * p1 - p3 <= p2`.
   - For `low = p3 - p2`:
     - The condition becomes `p1 - (p3 - p2) <= p2 - (p3 - (p3 - p2))` which simplifies to `p1 - p3 + p2 <= p2 - p2` or `p1 - p3 <= 0` or `p1 <= p3`.

Given the condition `p1 - cur <= p2 - (p3 - cur)` and the fact that the sum of `p1`, `p2`, and `p3` is odd, the more likely scenario that satisfies the condition is `low = p3 - p2` leading to the expression `p1 + p2`.

Thus, the final output is:
Output: **p1 + p2**