Output State: **`S0` is the 0th term of the sequence defined by the recurrence relation \(S_{i+1} = 2S_1 + S_0\) starting with \(S_0 = 1\) and \(S_1 = 1\), `S1` is the 1st term of the same sequence, `i` is `n`, `n` is a positive integer greater than or equal to 2.**

Explanation:
- The loop starts with \(S_0 = 1\) and \(S_1 = 1\).
- The recurrence relation inside the loop is \(S_{next} = 2 \cdot S1 + S0\).
- After each iteration, \(S0\) is updated to the previous value of \(S1\) and \(S1\) is updated to the value of \(S_{next}\).

Let's analyze the sequence generated by the loop:
1. Initial values: \(S0 = 1\), \(S1 = 1\)
2. First iteration (i = 2):
   - \(S_next = 2 \cdot 1 + 1 = 3\)
   - \(S0 = 1\), \(S1 = 3\)
3. Second iteration (i = 3):
   - \(S_next = 2 \cdot 3 + 1 = 7\)
   - \(S0 = 3\), \(S1 = 7\)
4. Third iteration (i = 4):
   - \(S_next = 2 \cdot 7 + 3 = 17\)
   - \(S0 = 7\), \(S1 = 17\)

From these observations, we can generalize that after \(n-1\) iterations, the values of \(S0\) and \(S1\) follow the recurrence relation:
\[ S0 \text{ is the 0th term}, \]
\[ S1 \text{ is the 1st term}. \]

Since the loop runs from \(i = 2\) to \(i = n\), it executes \(n-1\) times, and the final value of \(i\) is \(n\). Therefore, the output state after all iterations is that \(S0\) and \(S1\) follow the sequence defined by the recurrence relation, and \(i\) is \(n\).

If the loop does not execute (i.e., \(n < 2\)), then \(S0 = 1\) and \(S1 = 1\) since the initial conditions do not change. However, this case is excluded based on the initial state where \(n\) is a positive integer and \(n \geq 2\).