Postcondition: `t` is 0, `info` is a list of strings obtained from splitting the input string, `a` is an integer equal to the first element of `info`, `b` must be a positive integer, `suma` is `x` + 1, `i` is 2, `x` is `(a - 1) // 2`, and the current value of `x` satisfies `((a - 1) % 4 == 0 and 1 % 4 == 0`.

This means that if the condition `(a - i * (i - 1)) % i ** 2 == 0 and i * (i - 1) % i ** 2 == 0` is true, then `t` remains 0, `info` remains unchanged, `a` remains the same, `b` remains a positive integer, `suma` becomes `x + 1`, `i` becomes 2, `x` becomes `(a - 1) // 2`, and `x` satisfies `((a - 1) % 4 == 0 and 1 % 4 == 0)`. Since there is no else part, these changes apply regardless of the condition's truth value.