The code snippet modifies the `sum` variable by adding the result of the expression `(i * i - (i - 1) * (i - 1)) * i` to it. Given that `i` is 5, we can compute this expression as follows:

1. Calculate `i * i`: \(5 * 5 = 25\)
2. Calculate `(i - 1) * (i - 1)`: \(4 * 4 = 16\)
3. Subtract the second result from the first: \(25 - 16 = 9\)
4. Multiply the result by `i`: \(9 * 5 = 45\)

Thus, `sum` is incremented by 45. Given that `sum` was initially 57, it becomes \(57 + 45 = 102\).

The other variables (`n`, `j`, `t`, and `i`) remain unchanged.

Output State: **`n` must be at least 5, `j` is an input integer + 1, `t` is `t - 1`, `sum` is 102, `i` is 5**.