The code `j -= 1` decrements the value of `j` by 1. The values of the other variables remain unchanged. Since `j` was initially a valid index such that `ais[j - 1] > ais[i] + d`, after decrementing `j` by 1, the new value of `j` will be `j - 1`.

Therefore, the Output State is: `n` is greater than 0, `i` is `n - 2`, `k` is an integer such that 1 ≤ k ≤ n, `d` is an integer such that 0 ≤ d ≤ 10^9, `a` is a list of `n` integers where 1 ≤ ai ≤ 10^9, `ais` is a list of `n` integers sorted in ascending order, `cando` is a list of `n` values where `cando[i]` is `True`, `j` is a valid index such that `ais[j - 1] > ais[i] + d`, `j` is now `j - 1`.

Output State: **`n` is greater than 0, `i` is `n - 2`, `k` is an integer such that 1 ≤ k ≤ n, `d` is an integer such that 0 ≤ d ≤ 10^9, `a` is a list of `n` integers where 1 ≤ ai ≤ 10^9, `ais` is a list of `n` integers sorted in ascending order, `cando` is a list of `n` values where `cando[i]` is `True`, `j` is now `j - 1`.**