The code snippet `n -= m` modifies the value of `n` by subtracting `m` from it. Given that `m` is `(n + 1) // 2`, the new value of `n` will be `n - (n + 1) // 2`.

Output State: **`t` is an integer input such that 1 ≤ `t` ≤ 5 · 10^4, `n` is `n - (n + 1) // 2`, `k` is an integer such that 1 ≤ `k` ≤ `n` ≤ 10^9, `L` is an empty list, `m` is `(n + 1) // 2`**

In natural language: The value of `n` is updated to `n - (n + 1) // 2`. The values of `t`, `k`, `L`, and `m` remain unchanged as per the given conditions.