The code `x += int(c) * n ** i` updates the value of `x` by adding `int(c) * n ** i` to its current value. Here, `c` is a digit from the string `k` (a number in base `n`), and `i` is the index of this digit.

Given:
- `n` is an integer such that \(2 \leq n \leq 10^9\).
- `k` is a string representing a number in a base-n numeral system with no more than 60 digits and contains only valid digits less than `n`.
- `x` is initially `int(c) * n`.

After executing the line `x += int(c) * n ** i`, `x` is updated to `x + int(c) * n ** i`. Since `x` was initially `int(c) * n`, the new value of `x` becomes:

\[ x = int(c) * n + int(c) * n ** i \]

We can factor out `int(c)` from the expression:

\[ x = int(c) * (n + n ** i) \]

Since the values of `n`, `k`, and `i` remain unchanged, they stay in their original form. The updated value of `x` is now `int(c) * (n + n ** i)`.

Output State: **`n` is an integer such that \(2 \leq n \leq 10^9\); `k` is a string representing a number in a base-n numeral system with no more than 60 digits and contains only valid digits less than `n`; `x` is `int(c) * (n + n ** i)`**