Given the code snippet `p = p * v`, we know that the value of `p` is updated to be the product of its current value and the value of `v`. The other variables remain unchanged unless they are directly affected by this operation.

Here's the breakdown:

- `t` remains an integer such that 1 ≤ t ≤ 10^4.
- `n` and `m` remain integers such that 1 ≤ n ≤ 2·10^5 and 1 ≤ m ≤ 10^4.
- `a` remains a list of `n` integers where each integer `a_i` satisfies 1 ≤ `a_i` ≤ 10^4.
- `s` remains a string of length `n` consisting of the characters 'L' and 'R'.
- `b` remains a list containing all elements of `a` in the order specified by `s`.
- `l` remains `n`.
- `r` remains `-1`.
- `ans` remains a list containing `p` and `p * v * v`.
- `p` is updated to `p * v`.
- `v` remains the next element in the reversed list `b` after the current `v`.

Therefore, the updated output state is:

Output State: **`t` is an integer such that 1 ≤ t ≤ 10^4, `n` and `m` are integers such that 1 ≤ n ≤ 2·10^5 and 1 ≤ m ≤ 10^4, `a` is a list of `n` integers where each integer `a_i` satisfies 1 ≤ `a_i` ≤ 10^4, `s` is a string of length `n` consisting of the characters 'L' and 'R', `b` is a list containing all elements of `a` in the order specified by `s`, `l` is `n`, `r` is `-1`, `ans` is a list containing `p` and `p * v * v`, `p` is `p * v`, `v` is the next element in the reversed list `b` after the current `v`.**