The code `cur = cur + 1` increments the value of `cur` by 1. Since `cur` satisfies the condition \((cur \mod 2 == 0) == (c == '1')\), and `c` is the first character of the binary string `s`, we need to consider two cases:

1. If `c == '1'`, then \((cur \mod 2 == 0)\) should be `True`.
2. If `c == '0'`, then \((cur \mod 2 == 0)\) should be `False`.

Since `cur` is initially set to satisfy this condition based on `c`, incrementing `cur` by 1 will change its parity (odd/even nature). This means that if `cur` was even, it will become odd, and if it was odd, it will become even.

Therefore, the updated condition will be:
- If `c == '1'`, then after incrementing, \((cur \mod 2 == 0)\) will be `False`.
- If `c == '0'`, then after incrementing, \((cur \mod 2 == 0)\) will be `True`.

Output State: **`t` is an integer such that \(1 \leq t \leq 10^4\) and must be greater than 0, `n` is an integer such that \(1 \leq n \leq 2 \cdot 10^5\), `s` is a binary string of length `n`, `mn` is 0, `mx` is 0, `cur` is `cur + 1`, `c` is the first character of `s`, and the current value of `cur` satisfies the condition \((cur \mod 2 == 0) == (c == '0')\)**