The code `cur = cur - 1` decrements the value of `cur` by 1. According to the precondition, `cur` is initially equal to `0` (either because `cur % 2 == 0` and `c != '1'` or `cur % 2 != 0` and `c == '1'`). Therefore, after executing the code, `cur` will be `cur - 1`, which means `cur` is now `-1`.

All other variables remain unchanged according to the given initial state.

Output State: **`t` is an integer such that \(1 \leq t \leq 10^4\) and must be greater than 0, `n` is an integer such that \(1 \leq n \leq 2 \cdot 10^5\), `s` is a binary string of length `n`, `mn` is 0, `mx` is 0, `cur` is -1, `c` is the first character of `s`, and either (`cur % 2 == 0` and `c != '1')` or (`cur % 2 != 0` and `c == '1')**