To determine the new state after the code execution, we need to evaluate the expression `ans = ans + (n + b) // (b * b)` given the initial state.

Initial State:
- `t` is an input integer such that 1 ≤ `t` ≤ 10^4
- `n` and `m` are integers such that `min(n, m) ≥ 2`
- `ans` is equal to `n`

The code modifies `ans` by adding the result of `(n + b) // (b * b)` to its current value. Since `b` is not defined in the initial state, we will keep it as `b` in our calculations.

New value of `ans`:
- `ans` was initially `n`.
- It is now `n + (n + b) // (b * b)`.

Other variables (`t` and `m`) remain unchanged.

Output State: **`t` is an input integer such that 1 ≤ `t` ≤ 10^4, `n` and `m` are integers such that `min(n, m) ≥ 2, `ans` is `n + (n + b) // (b * b)`**.