The code snippet `b[i] = b[i - 1] + x` updates the value of `b[i]` based on the value of `b[i - 1]` and `x`. Given that `i` is 4, we need to update `b[4]` using the value of `b[3]` and `x`. The value of `x` is determined by whether `a[4] > 1` or not. Since the specific value of `a[4]` is not provided, we will express `x` in terms of `a[4]`.

If `a[4] > 1`, then `x = 1`; otherwise, `x = 2`. Therefore, the value of `b[4]` will be `b[3] + 1` if `a[4] > 1`, or `b[3] + 2` if `a[4] ≤ 1`.

Output State: **`t` is an integer such that 1 ≤ t ≤ 10^4; `n` is an integer such that 1 ≤ n ≤ 3 · 10^5; `q` is an integer such that 1 ≤ q ≤ 3 · 10^5; `c` is a list of `n` integers where each element `c_i` satisfies 1 ≤ `c_i` ≤ 10^9; `a` is a list where `a[0]` is 0 and `a[1]` to `a[n]` are the integers read from the input; For each query, `l_i` and `r_i` are integers such that 1 ≤ `l_i` ≤ `r_i` ≤ `n`; `b` is a list of `n + 1` integers where `b[0]` is 0 and `b[i]` for `i` from 1 to `n` is `b[i - 1] + x`, with `x` being 1 if `a[i] > 1` else 2; `i` is 4; `x` is 1 if `a[4] > 1` else 2; `b[4]` is `b[3] + 1` if `a[4] > 1` else `b[3] + 2`.**