The code snippet `k = j + 1` updates the value of `k` to be `j + 1`. No other variables are affected by this line of code.

Given the initial state, `j` is defined as `i + 2`. Therefore, the new value of `k` becomes `(i + 2) + 1`, which simplifies to `i + 3`.

Output State: **`t` is an integer such that 1 ≤ t ≤ 10^4, `n` and `m` are integers such that 1 ≤ n, m ≤ 2 ⋅ 10^5, `b` is an integer greater than 0, `c` is an integer, `d` is the new input string, `j` is `i + 2`, `i` is `i + 1`, `e` is the value of the input, `k` is `i + 3`.**