Output State: **`i` is 2, `idx` is 1, `nums` is a list with elements [2, k - 1, k + 1]**.

Explanation: The code appends a new element to the list `nums`. The new element is calculated as `k + nums[idx] + 1`. Given that `idx` is 1, `nums[idx]` is `k - nums[1]`, which is `k - (k - 1) = 1`. Therefore, the new element is `k + 1 + 1 = k + 2`. However, since the initial list `nums` was `[2, k - nums[1], k + 1]` and `nums[1]` is `k - 1`, the new element is `k + 1 + 1 = k + 2`, but the list already contains `k + 1`, so the correct new element is simply `k + 1 + 1 = k + 2 - 1 = k + 1`. Thus, the updated list is `[2, k - 1, k + 1]`. The variables `i` and `idx` remain unchanged.