The code snippet `t = abs(y2 - y1)` updates the value of `t` to the absolute difference between `y2` and `y1`.

Given the initial state:
- `t` is an integer where 1 ≤ t ≤ 10^4
- `n` is `r[0]`
- `m` is `r[1]`
- `x1` is `r[2] + 1`
- `x2` is `r[4]`
- `y2` is `r[5]`
- `r` is a list of six integers [h, w, x_a, y_a, x_b, y_b] where 1 ≤ x_a, x_b ≤ h ≤ 10^6, 1 ≤ y_a, y_b ≤ w ≤ 10^9, and either x_a ≠ x_b or y_a ≠ y_b
- `x2` is greater than `x1`, the difference between `x2` and `x1` is even, and `y1` is not equal to `y2`
- If `y1` ≥ `y2`, then `a` is `r[5] - 1`. Otherwise, `y1` is less than `y2`, and `a` is `r[1] - r[5]`
- `b` is `x2 - x1`

After executing the code:
- `t` is updated to `abs(y2 - y1)`

Therefore, the output state is:
Output State: **`t` is `abs(y2 - y1)`, `n` is `r[0]`, `m` is `r[1]`, `x1` is `r[2] + 1`, `x2` is `r[4]`, `y2` is `r[5]`, `r` is a list of six integers [h, w, x_a, y_a, x_b, y_b] where 1 ≤ x_a, x_b ≤ h ≤ 10^6, 1 ≤ y_a, y_b ≤ w ≤ 10^9, and either x_a ≠ x_b or y_a ≠ y_b, `x2` is greater than `x1`, the difference between `x2` and `x1` is even, and `y1` is not equal to `y2`, if `y1` ≥ `y2`, then `a` is `r[5] - 1`. Otherwise, `y1` is less than `y2`, and `a` is `r[1] - r[5]`, `b` is `x2 - x1`.**