The value of `res` is updated to the expression `i * h2 + (c - i * w2) / w1 * h1`. The values of the other variables remain unchanged. Since the initial state specifies that `res` is 0 and `i` is 0, and given that `c` is an integer such that \(10 < c \leq 10^5 \times w2\), the calculation of `res` will depend on the values of `h1`, `h2`, `w1`, and `w2`.

Given that `i` is 0, the term `i * h2` and `i * w2` will both be 0, simplifying the expression to:
\[ res = (c / w1) * h1 \]

Therefore, the Output State is:
**`C` is an integer such that \(1 \leq C \leq 10^9\), `Hr` is an integer such that \(1 \leq Hr \leq 10^9\), `Hb` is an integer such that \(1 \leq Hb \leq 10^9\), `Wr` is an integer such that \(1 \leq Wr \leq 10^9\), `Wb` is an integer such that \(1 \leq Wb \leq 10^9\), `c` is an integer such that \(10 < c \leq 10^5 \times w2\), `h1` is an input integer, `h2` is an input integer, `w1` is an input integer divided by `g`, `w2` is an input integer divided by `g`, `g` is gcd(w1, w2), `res` is \((c / w1) * h1\), `i` is 0, and the current value of `res` is \((c / w1) * h1\).**