In the provided code snippet, `f` is assigned the value of `factorial(n - k)`. Given that `k` is initially 1, the expression simplifies to `factorial(n - 1)`. The value of `n` is a positive integer that can range from 1 to 50. Therefore, `n - 1` will range from 0 to 49.

The factorial of a non-negative integer `x` is defined as the product of all positive integers up to `x`, with `factorial(0)` defined as 1.

Thus, the output state will reflect the computed value of `f` based on the value of `n`. 

1. If `n = 1`, then `f = factorial(0) = 1`
2. If `n = 2`, then `f = factorial(1) = 1`
3. If `n = 3`, then `f = factorial(2) = 2`
4. If `n = 4`, then `f = factorial(3) = 6`
5. If `n = 5`, then `f = factorial(4) = 24`
6. ...
7. If `n = 50`, then `f = factorial(49)`, which is a very large number.

Since `n` can take any positive integer value from 1 to 50, `f` will take values accordingly. Therefore, we cannot specify a single value for `f` without knowing the exact value of `n`.

Thus, the output state is:
Output State: **`n` is a positive integer such that 1 ≤ `n` ≤ 50; `f` is the factorial of `n - 1` which varies based on `n`.**