To determine the new value of `sum`, we need to perform the calculation step-by-step using the given initial state.

Given:
- `sum` is initially 93.
- `i` is initially 5.

The code snippet:
```
sum += (i * i - (i - 1) * (i - 1)) * i
```

Let's break down the expression:
1. Calculate `i * i`:
   - `5 * 5 = 25`

2. Calculate `(i - 1) * (i - 1)`:
   - `(5 - 1) * (5 - 1) = 4 * 4 = 16`

3. Subtract the second result from the first:
   - `25 - 16 = 9`

4. Multiply the result by `i`:
   - `9 * 5 = 45`

5. Add this result to `sum`:
   - `93 + 45 = 138`

Now, the value of `sum` is 138. The values of `t`, `n`, and `i` remain unchanged.

Output State: **`t` is an input integer representing the number of test cases and must be greater than 0; `n` must be at least 2; `sum` is 138; `i` is 5**.