To determine the output state after the loop has completed all its iterations, we need to understand the pattern in the loop and how the `sum` is being updated.

The loop iterates from `i = 2` to `i = n`. In each iteration, the `sum` is updated by adding the value `(i * i - (i - 1) * (i - 1)) * i`, which simplifies to `i^3`.

Let's break down the iterations:

- When `i = 2`, `sum += 2^3 = 8`, so `sum = 1 + 8 = 9`.
- When `i = 3`, `sum += 3^3 = 27`, so `sum = 9 + 27 = 36`.
- When `i = 4`, `sum += 4^3 = 64`, so `sum = 36 + 64 = 100`.
- When `i = 5`, `sum += 5^3 = 125`, so `sum = 100 + 125 = 225`.

Following this pattern, the final `sum` after the loop completes all iterations up to `i = n` will be the sum of cubes of all integers from 2 to `n`.

The formula for the sum of cubes of the first `n` natural numbers is \((\frac{n(n+1)}{2})^2\). However, since we start from 2, we need to subtract the cube of 1 from this sum.

Therefore, the final `sum` is \((\frac{n(n+1)}{2})^2 - 1\).

Given the output states after the first 3 iterations, we can verify that the loop runs for `n` iterations. Therefore, the final `sum` after all iterations is:

\[
\text{sum} = \left(\frac{n(n+1)}{2}\right)^2 - 1
\]

Let's calculate this for the given `n`.

Output State: **the output state you calculate.**

To compute the exact final sum, we need the value of `n`. Since we don't have the exact value of `n` from the problem statement, let's assume `n` is provided and calculate the final `sum` based on the given pattern.

Let's say `n` is 5 for demonstration purposes (as it matches the given output states after 3 iterations):

\[
\text{sum} = \left(\frac{5(5+1)}{2}\right)^2 - 1 = \left(\frac{5 \cdot 6}{2}\right)^2 - 1 = 15^2 - 1 = 225 - 1 = 224
\]

Thus, the final output state is:

Output State: **t is an input integer representing the number of test cases and must be greater than 0; n is an input integer; sum is (n(n+1)/2)^2 - 1.**

In simple terms, the final `sum` after all iterations of the loop is the sum of cubes of all integers from 2 to `n`, which can be expressed as \((\frac{n(n+1)}{2})^2 - 1\).