The given code snippet updates the variable `sum` by adding a specific expression to it. Let's break down the expression:

The code snippet is:
```python
sum += (i * i - (i - 1) * (i - 1)) * i
```

This can be simplified as:
```python
sum += (i**2 - (i-1)**2) * i
```

Expanding `(i-1)**2`:
```python
sum += (i**2 - (i**2 - 2*i + 1)) * i
sum += (i**2 - i**2 + 2*i - 1) * i
sum += (2*i - 1) * i
sum += 2*i**2 - i
```

So, the value of `sum` is updated by adding `2*i**2 - i` to it.

The other variables `t`, `n`, `j`, and `i` are not affected by this line of code, so they retain their initial values.

Therefore, the Output State is:

Output State: **`t` is an input integer representing the number of test cases minus 1, `n` must be at least 1, `sum` is updated to `sum + 2*i**2 - i`, `j` is the previous `n + 1`, `i` is `i + 1`**