To determine the final output state after all iterations of the loop, we need to understand the loop's behavior. The loop iterates from `i = 2` to `i = n` and updates the `sum` variable in each iteration according to the formula:
\[ \text{sum} += (i * i - (i - 1) * (i - 1)) * i \]

This can be simplified as:
\[ \text{sum} += (i^2 - (i-1)^2) * i \]
\[ \text{sum} += (i^2 - (i^2 - 2i + 1)) * i \]
\[ \text{sum} += (2i - 1) * i \]
\[ \text{sum} += 2i^2 - i \]

The loop starts with `i = 2` and continues until `i = n`. Therefore, the final value of `sum` will be the cumulative sum of `2i^2 - i` from `i = 2` to `i = n`.

Let's determine the final `sum` value by iterating through the loop and updating the `sum` accordingly:

1. **Initial State**: `t` is an input integer representing the number of test cases minus 1; `n` is a new input integer; `sum` is 1; `j` is the previous `n + 1`.

2. **Loop Iterations**:
   - For `i = 2`: `sum += 2*2^2 - 2 = 2*4 - 2 = 8 - 2 = 6`. So, `sum = 1 + 6 = 7`.
   - For `i = 3`: `sum += 2*3^2 - 3 = 2*9 - 3 = 18 - 3 = 15`. So, `sum = 7 + 15 = 22`.
   - For `i = 4`: `sum += 2*4^2 - 4 = 2*16 - 4 = 32 - 4 = 28`. So, `sum = 22 + 28 = 50`.
   - This continues until `i = n`.

The final `sum` after all iterations will be the sum of `2i^2 - i` from `i = 2` to `i = n`.

**Output State**: **`t` is an input integer representing the number of test cases minus 1; `n` is a new input integer; `sum` is the cumulative sum of `2i^2 - i` from `i = 2` to `i = n`; `j` is the previous `n + 1`.**

In natural language, the final output state is that `t` remains the same as the input integer representing the number of test cases minus 1, `n` remains the input integer, `sum` is the total accumulated value from the loop iterations, and `j` remains the previous `n + 1`.