To determine the final output state after all iterations of the loop have finished, we need to understand how the loop modifies the variables `sum` and `i`.

The loop iterates from `i = 2` to `i = n`, updating `sum` in each iteration according to the formula:
\[ \text{sum} += (i \times i - (i - 1) \times (i - 1)) \times i \]

Simplifying the expression inside the loop:
\[ i \times i - (i - 1) \times (i - 1) = i^2 - (i^2 - 2i + 1) = 2i - 1 \]
Thus, the update to `sum` in each iteration can be rewritten as:
\[ \text{sum} += (2i - 1) \times i = 2i^2 - i \]

The loop starts with `i = 2` and increments `i` by 1 in each iteration until `i` reaches `n`. Therefore, the final value of `sum` is the sum of the series:
\[ \text{sum} = 1 + \sum_{i=2}^{n} (2i^2 - i) \]

Let's compute the final value of `sum` step-by-step:
\[ \text{sum} = 1 + \sum_{i=2}^{n} (2i^2 - i) \]
\[ \text{sum} = 1 + 2\sum_{i=2}^{n} i^2 - \sum_{i=2}^{n} i \]

Using the formulas for the sum of squares and the sum of the first `n` natural numbers:
\[ \sum_{i=1}^{n} i^2 = \frac{n(n + 1)(2n + 1)}{6} \]
\[ \sum_{i=1}^{n} i = \frac{n(n + 1)}{2} \]

Subtracting the `i = 1` terms:
\[ \sum_{i=2}^{n} i^2 = \frac{n(n + 1)(2n + 1)}{6} - 1 \]
\[ \sum_{i=2}^{n} i = \frac{n(n + 1)}{2} - 1 \]

Substituting these into the expression for `sum`:
\[ \text{sum} = 1 + 2\left(\frac{n(n + 1)(2n + 1)}{6} - 1\right) - \left(\frac{n(n + 1)}{2} - 1\right) \]
\[ \text{sum} = 1 + \frac{n(n + 1)(2n + 1)}{3} - 2 - \frac{n(n + 1)}{2} + 1 \]
\[ \text{sum} = \frac{n(n + 1)(2n + 1)}{3} - \frac{n(n + 1)}{2} \]

Combining the fractions:
\[ \text{sum} = \frac{2n(n + 1)(2n + 1) - 3n(n + 1)}{6} \]
\[ \text{sum} = \frac{n(n + 1)(4n + 2 - 3)}{6} \]
\[ \text{sum} = \frac{n(n + 1)(4n - 1)}{6} \]

The variable `j` remains unchanged throughout the loop, so `j` is still the previous `n + 1`.

Thus, the final output state is:
Output State: **`t` is an input integer representing the number of test cases minus 1, `n` is a new input integer, `sum` is \(\frac{n(n + 1)(4n - 1)}{6}\), `j` is the previous `n + 1`.**

In simple terms, after all iterations, `sum` is calculated as \(\frac{n(n + 1)(4n - 1)}{6}\), and `j` remains the previous value of `n + 1`.