Let's break down the problem step by step:

1. **Identify the loop condition**: The loop condition is given by the expression `(x + y) * x <= n` and `(x + y) * y <= m`.

2. **Current states at the end of the previous iteration**:
   - `x` is 1
   - `n` must be at least 2
   - `m` must be at least 7
   - `cnt` is 2
   - `y` is increased by 1 (implying `y` is 1 at this point)

3. **Determine the new values for `x` and `y` for the next iteration**:
   - Since `y` is increased by 1, at the start of the next iteration, `y` will be 2.
   - We need to check if the loop condition holds with `x = 1` and `y = 2`.

4. **Evaluate the loop condition with `x = 1` and `y = 2`**:
   - `(x + y) * x <= n` becomes `(1 + 2) * 1 <= n` or `3 <= n`.
   - `(x + y) * y <= m` becomes `(1 + 2) * 2 <= m` or `6 <= m`.

5. **Check the constraints on `n` and `m`**:
   - From the current state, `n` must be at least 2.
   - From the current state, `m` must be at least 7.
   - Both conditions `3 <= n` and `6 <= m` are satisfied because `n` must be at least 2 and `m` must be at least 7.

Since both conditions are satisfied, the loop can execute one more time. Therefore, no adjustments are needed for `n` or `m`.

6. **Adjust the state for the next iteration**:
   - `x` remains 1.
   - `y` becomes 2.
   - `cnt` remains 2 (since the loop body is omitted and no changes are made to `cnt`).

So, the state for the next iteration should be:

State: **`x` is 1, `y` is 2, `cnt` is 2**