Output State: `x` is 3, `n` must be at least 24, `m` is at least 7, `y` is 6, and `cnt` is 30.

Explanation: The loop continues as long as \((x + y) * x \leq n\) and \((x + y) * y \leq m\). Given the initial conditions and the output states after the first three iterations, we can deduce the following:

- After the first iteration, \(x = 3\), \(y = 2\), and \(cnt = 16\).
- After the second iteration, \(x = 3\), \(y = 3\), and \(cnt = 18\).
- After the third iteration, \(x = 3\), \(y = 4\), and \(cnt = 20\).

Following this pattern, we see that \(x\) remains constant at 3, and \(y\) increases by 1 each time the loop runs. Therefore, after all iterations, \(y\) will be 6. 

To find the final value of `cnt`, we need to consider the condition \(\text{math.gcd}(x, y) == 1\). Since \(x = 3\) and \(y\) starts from 2 and increments by 1, the gcd condition will be satisfied until \(y = 6\) (since \(\text{math.gcd}(3, 6) \neq 1\)). For each valid \(y\), \(cnt\) is incremented by the minimum value between \(n / ((x + y) * x)\) and \(m // ((x + y) * y)\).

Given the output states after the first three iterations, we can infer that \(n\) must be at least 24 (since \(n / ((x + y) * x)\) needs to be large enough to contribute to the increase in `cnt` up to the third iteration). Therefore, after all iterations, the final state will be \(x = 3\), \(n \geq 24\), \(m \geq 7\), \(y = 6\), and \(cnt = 30\).