To determine the new state after executing the given Python code snippet, we need to focus on the calculation of `dp[i]`. The formula used is:

\[ dp[i] = (dp[i - 1] + (i - 1) \times dp[i - 2] \times 2) \% (10^9 + 7) \]

Given:
- `i` is 5
- `dp[1]` is 1
- `dp[2]` is 3
- `dp[4]` is 18

We need to compute `dp[5]` using the above formula.

Substituting the known values into the formula:

\[ dp[5] = (dp[4] + (5 - 1) \times dp[3] \times 2) \% (10^9 + 7) \]

However, `dp[3]` is not explicitly given. Since it's not specified, we assume it follows the same pattern or is initialized to 0 unless otherwise stated. Given the problem context, we'll assume `dp[3]` is 0 (as it's not mentioned and typically such problems initialize all unspecified elements to 0).

So, the equation simplifies to:

\[ dp[5] = (18 + (5 - 1) \times 0 \times 2) \% (10^9 + 7) \]
\[ dp[5] = (18 + 0) \% (10^9 + 7) \]
\[ dp[5] = 18 \% (10^9 + 7) \]
\[ dp[5] = 18 \]

Therefore, `dp[5]` is updated to 18.

All other variables remain unchanged as per the given initial state.

Output State: **`t` is an input integer such that 0 ≤ `t` ≤ 10^4 - 1; `n` is the first integer read from the input, such that 1 ≤ `n` ≤ 3 · 10^5; `k` is the second integer read from the input, such that 0 ≤ `k` ≤ `n`; `num` is the sum of 1s and 2s based on whether `c` equals `r` in each of the `k` iterations; `m` is `n - num` and `m` must be at least 3; `dp` is a list of length `m + 1` with all elements initialized to 0 except `dp[1]` which is 1, `dp[2]` which is 3, `dp[4]` which is 18, and `dp[5]` which is 18; `i` is 5**