To determine what will be printed by the `print(dp[m])` statement, let's break down the initial state and the calculation process step by step:

### Initial State:
- `dp` is a list of length `m + 1` initialized with zeros.
- `dp[1]` is set to 1.
- `dp[2]` is set to 3.
- Subsequent elements are calculated using the formula: `dp[i] = (dp[i - 1] + (i - 1) * dp[i - 2] * 2) % 10`.

### Calculation Process:
1. **Initialization:**
   - `dp[0] = 0`
   - `dp[1] = 1`
   - `dp[2] = 3`

2. **Subsequent Elements:**
   - For `i = 3`:
     \[
     dp[3] = (dp[2] + (3 - 1) * dp[1] * 2) \% 10 = (3 + 2 * 1 * 2) \% 10 = (3 + 4) \% 10 = 7
     \]
   - For `i = 4`:
     \[
     dp[4] = (dp[3] + (4 - 1) * dp[2] * 2) \% 10 = (7 + 3 * 3 * 2) \% 10 = (7 + 18) \% 10 = 5
     \]
   - For `i = 5`:
     \[
     dp[5] = (dp[4] + (5 - 1) * dp[3] * 2) \% 10 = (5 + 4 * 7 * 2) \% 10 = (5 + 56) \% 10 = 1
     \]
   - Continue this process until `i = m`.

### Final Output:
The value of `dp[m]` will be the result of the above calculations up to the `m`-th element.

Since the exact value of `m` is not provided, we cannot compute the exact numerical value of `dp[m]`. However, based on the structure of the problem and the formula used, the print statement will output the value of `dp[m]` calculated using the given formula.

Output: **dp[m] (where dp[m] is the value of the m-th element in the dp list calculated using the formula dp[i] = (dp[i - 1] + (i - 1) * dp[i - 2] * 2) % 10)**