Let's break down the initial state and the print statement step by step:

1. **Initial State:**
   - `p1`, `p2`, and `p3` are integers provided by user input.
   - `p1` ≤ `p2` ≤ `p3` ≤ 30.
   - The sum of `p1`, `p2`, and `p3` is odd.
   - `p3` must be greater than or equal to 4.
   - `x` is 2.
   - `y` is `p3 - 2`.

2. **Print Statement:**
   ```
   print(p1 - x + p3)
   ```

3. **Determine the Values:**
   - `x` is explicitly given as 2.
   - `p1` and `p3` are integers provided by user input, but they must satisfy the conditions `p1` ≤ `p2` ≤ `p3` ≤ 30 and `p3` ≥ 4.
   - The sum of `p1`, `p2`, and `p3` is odd, which means the sum of `p1 + p2 + p3` must be an odd number.

4. **Calculate the Expression:**
   - The expression to be printed is `p1 - x + p3`.
   - Substituting `x` with 2, the expression becomes `p1 - 2 + p3`.
   - Simplifying, the expression is `p1 + p3 - 2`.

5. **Output Description:**
   - The value of `p1 + p3 - 2` will be printed.
   - Since `p1` and `p3` are integers and `p3` is at least 4, the minimum value of `p1 + p3 - 2` is `p1 + 4 - 2 = p1 + 2`.
   - The maximum value of `p1 + p3 - 2` is `p1 + 30 - 2 = p1 + 28`.
   - Given that `p1` ≤ `p2` ≤ `p3` and the sum of `p1`, `p2`, and `p3` is odd, the exact values of `p1` and `p3` are not specified, but they must be chosen such that the sum is odd.

Output: **p1 + p3 - 2 (where p1 and p3 are integers such that p1 ≤ p2 ≤ p3 ≤ 30, p3 ≥ 4, and the sum of p1, p2, and p3 is odd)**