The code snippet `pd[i] += pd[i - 1]` updates the value of `pd[i]` by adding the value of `pd[i - 1]` to it. Given the initial state:

- `t` is an input integer where 1 ≤ t ≤ 10^4
- `n` is an integer where 1 ≤ n ≤ 2 · 10^5 for each test case
- `N` is 200001
- `pd` is a list of length 200001 with `pd[0]` set to 0
- `pd[i]` (where `i` is `N`) is now the sum of `pd[N-1]` and the sum of the digits of `N`
- `i` is `N`

After executing the code snippet:

- The value of `pd[i]` is updated to `pd[i] + pd[i - 1]`.
- Since `i` is `N`, the new value of `pd[N]` is `pd[N] + pd[N - 1]`.

The values of `t`, `n`, `N`, and the rest of the list `pd` remain unchanged except for the updated value of `pd[N]`.

Output State: **`t` is an input integer where 1 ≤ t ≤ 10^4, `n` is an integer where 1 ≤ n ≤ 2 · 10^5 for each test case, `N` is 200001, `pd` is a list of length 200001 with `pd[0]` set to 0, `pd[N]` is now the sum of `pd[N-1]` and the sum of the digits of `N` plus `pd[N-1]`, `i` is `N`.**