The value of `s` is decremented by 1. Since `s` is equal to the input integer `b - 1`, this operation changes `s` to `(b - 1) - 1`, which simplifies to `b - 2`. The other variables `t` and `n` remain unaffected. The condition for the loop to execute again is that `b` must be greater than 2 and even, which remains unchanged. Therefore, the Output State is: `t` is an integer such that 1 ≤ `t` ≤ 100; `n` is an integer such that 2 ≤ `n` ≤ 100; `s` is equal to `b - 2`.

Output State: **`t` is an integer such that 1 ≤ `t` ≤ 100; `n` is an integer such that 2 ≤ `n` ≤ 100; `s` is equal to `b - 2**