The code snippet modifies the value of `x_w` using the formula provided. Let's analyze the impact of this operation:

- `x_w` is assigned the value of `xb - 2 * (yb - y_goal_mid) * (xb - 0) / (y_goal_mid - yb)`.

Given the initial state:
- `y1, y2, yw, xb, yb, r` are integers such that 1 ≤ y1, y2, yw, xb, yb ≤ 10^6, y1 < y2 < yw, yb + r < yw, 2·r < y2 - y1, and (yb + r < yw and y1 < y2 and y1 + r < y2 - r).
- `y_goal_mid` is a float equal to `(y1 + y2) / 2`.
- \( y_goal_mid - r \geq y1 \) and \( y_goal_mid + r \leq y2 \).

Let's break down the formula for `x_w`:
- `x_w = xb - 2 * (yb - y_goal_mid) * (xb - 0) / (y_goal_mid - yb)`
- Simplifying the formula:
  - The term `(yb - y_goal_mid)` is the difference between `yb` and `y_goal_mid`.
  - The term `(y_goal_mid - yb)` is the same as `- (yb - y_goal_mid)`.
  - Therefore, the formula simplifies to:
    - `x_w = xb - 2 * (yb - y_goal_mid) * xb / (-(yb - y_goal_mid))`
    - `x_w = xb + 2 * xb`
    - `x_w = 3 * xb`

Thus, the value of `x_w` is calculated as `3 * xb`.

The values of `y1, y2, yw, xb, yb, r, y_goal_mid` remain unchanged, and the conditions specified in the initial state are still valid.

Output State: **`y1, y2, yw, xb, yb, r` are integers such that 1 ≤ y1, y2, yw, xb, yb ≤ 10^6, y1 < y2 < yw, yb + r < yw, 2·r < y2 - y1, and (yb + r < yw and y1 < y2 and y1 + r < y2 - r); `y_goal_mid` is a float equal to `(y1 + y2) / 2`; \( y_goal_mid - r \geq y1 \) and \( y_goal_mid + r \leq y2 \); `x_w` is `3 * xb`**