Let's go through the code step by step:

1. **Initial State**: 
   - `n` is an integer.
   - `m` is an integer.
   - `k` is an integer such that \(0 \leq k < 2n - 2\) and \(k \geq n - 1\).

2. **Code Snippet**:
   ```python
   print(n - (k - n + 1) % (n - 1) - 1, (k - n + 1) // (n - 1) + 1)
   ```

3. **Impact Analysis**:
   - The expression `(k - n + 1) % (n - 1)` calculates the remainder when `(k - n + 1)` is divided by `(n - 1)`.
   - The expression `(k - n + 1) // (n - 1)` performs integer division of `(k - n + 1)` by `(n - 1)`.
   - The final print statement outputs two values derived from these expressions.

4. **Calculating the Result**:
   - Let's denote `r = (k - n + 1) % (n - 1)`. So, the first value printed is `n - r - 1`.
   - The second value printed is `(k - n + 1) // (n - 1) + 1`.

5. **Simplifying the Expressions**:
   - Since \(0 \leq k < 2n - 2\) and \(k \geq n - 1\), we know \(0 \leq k - n + 1 < n - 1\).
   - This means \(r = (k - n + 1) % (n - 1)\) is simply `k - n + 1` because `k - n + 1` is already within the range \(0 \leq k - n + 1 < n - 1\).

6. **Final Values**:
   - The first value printed is `n - (k - n + 1) - 1 = n - k + n - 2 = 2n - k - 2`.
   - The second value printed is \((k - n + 1) // (n - 1) + 1 = 0 + 1 = 1` because \(0 \leq k - n + 1 < n - 1\) ensures the quotient is 0.

7. **Output State**:
   - The values of `n`, `m`, and `k` remain unchanged.
   - The output state includes the printed values: `2n - k - 2` and `1`.

Output State: **`n` is an integer, `m` is an integer, `k` is an integer such that \(0 \leq k < 2n - 2\) and \(k \geq n - 1\); the output is `2n - k - 2` and `1`.**