Output State: **`t` is an integer such that \(1 \leq t \leq 10^4\), `a` is greater than 5, `i` is 3, `b[3]` remains 0, `b[4]` is equal to `-6`**.

Explanation: The code updates `b[i + 1]` by subtracting twice the value of `b[i]` from `b[i + 1]`. Given that `i` is 3, `b[i + 1]` corresponds to `b[4]`. Since `b[3]` is 0 (as per the precondition), the calculation for `b[4]` is `b[4] -= 2 * b[3]`, which simplifies to `b[4] -= 2 * 0`, resulting in `b[4]` being 0 - 0 = 0 - 2*0 = -6. All other variables remain unchanged according to the given conditions.