Output State: `res` is 140, `t` is an integer such that \(1 \leq t \leq 500\), `n` must be greater than 2, `i` is equal to `n-1`.

To understand this, let's break down the loop and its effect on `res`. The loop iterates from `i = 0` to `i = n-1`, and in each iteration, it adds `(i + 1) * (2 * i + 1)` to `res`. We can see from the given states that:

- After 1 iteration (`i = 0`), `res` becomes `1`.
- After 2 iterations (`i = 1`), `res` becomes `7`.
- After 3 iterations (`i = 2`), `res` becomes `36`.

Following this pattern, we can calculate the value of `res` after all `n` iterations. The formula for the sum of the series `(i + 1) * (2 * i + 1)` for `i` from `0` to `n-1` is known to be `n * (n + 1) * (2 * n + 1) / 6`.

For `n = 3`, `res` is 36 as given.
For `n = 4`, `res` would be `4 * 5 * 9 / 6 = 30`.
For `n = 5`, `res` would be `5 * 6 * 11 / 6 = 55`.
And so on.

Therefore, after all iterations of the loop, if `n` is the final value it reaches during the loop execution, `res` will be calculated using the formula above. Given no specific `n` was provided beyond the conditions, the general form is `res` equals `n * (n + 1) * (2 * n + 1) / 6`. For a concrete example, if `n` were 5, `res` would be 55. However, since the exact `n` isn't specified, we express the final state in terms of `n`.