The code snippet appends the current value of `p` to the list `ans`. This means that `ans` will now contain two elements: the original `p` and the newly appended `p`.

Given the initial state, the value of `p` is calculated as `(p * v) % m`, but since `v` is not defined in the initial state, we will keep `p` as it is in terms of its expression.

Here's the updated state:

- `t` remains an integer such that 1 ≤ t ≤ 10^4.
- `n` remains an integer such that 1 ≤ n ≤ 2·10^5.
- `m` remains an integer such that 1 ≤ m ≤ 10^4.
- `a` remains a list of `n` integers where each integer `a_i` satisfies 1 ≤ `a_i` ≤ 10^4.
- `s` remains a string of length `n` consisting only of the characters 'L' and 'R'.
- `b` remains a list containing all `n` elements from `a`, ordered according to the sequence specified by `s`.
- `l` remains `n`.
- `r` remains -1.
- `i` remains `n - 2`.
- `ans` now contains two elements: `[p, p]`.
- `p` remains `(p * v) % m`.

Output State: **`t` is an integer such that 1 ≤ t ≤ 10^4; `n` is an integer such that 1 ≤ n ≤ 2·10^5; `m` is an integer such that 1 ≤ m ≤ 10^4; `a` is a list of `n` integers where each integer `a_i` satisfies 1 ≤ `a_i` ≤ 10^4; `s` is a string of length `n` consisting only of the characters 'L' and 'R'; `b` is a list containing all `n` elements from `a`, ordered according to the sequence specified by `s`; `l` is `n`; `r` is -1; `i` is `n - 2`; `ans` is `[p, p]`; `p` is `(p * v) % m`.**