To determine what will be printed by the `print(ans)` statement, let's break down the initial state and the variables involved:

1. **Initial State:**
   - `a1` is `n`
   - `a2` is `n - 1`
   - `b1` is `m`
   - `b2` is `m - 1`
   - `ans` is the sum of the maximum absolute differences between elements of `a` and `b` chosen during the loop
   - `t` is `t - n`

2. **Understanding `ans`:**
   - `ans` is described as the sum of the maximum absolute differences between elements of `a` and `b` chosen during the loop.
   - Without the specific loop logic, we can infer that `ans` is computed based on the values of `a1`, `a2`, `b1`, and `b2`.

3. **Possible Values:**
   - The maximum absolute difference between `a1` and `b1` is `|n - m|`
   - The maximum absolute difference between `a1` and `b2` is `|n - (m - 1)| = |n - m + 1|`
   - The maximum absolute difference between `a2` and `b1` is `|(n - 1) - m| = |n - m - 1|`
   - The maximum absolute difference between `a2` and `b2` is `|(n - 1) - (m - 1)| = |n - m|`

4. **Summing the Maximum Absolute Differences:**
   - The maximum absolute differences are `|n - m|`, `|n - m + 1|`, `|n - m - 1|`, and `|n - m|`.
   - The sum of these maximum absolute differences is `|n - m| + |n - m + 1| + |n - m - 1| + |n - m|`.

5. **Simplifying the Sum:**
   - If `n >= m`, then:
     - `|n - m| = n - m`
     - `|n - m + 1| = n - m + 1`
     - `|n - m - 1| = n - m - 1`
     - `|n - m| = n - m`
     - Sum = `(n - m) + (n - m + 1) + (n - m - 1) + (n - m) = 4(n - m)`
   - If `n < m`, then:
     - `|n - m| = m - n`
     - `|n - m + 1| = m - n - 1`
     - `|n - m - 1| = m - n + 1`
     - `|n - m| = m - n`
     - Sum = `(m - n) + (m - n - 1) + (m - n + 1) + (m - n) = 4(m - n)`

6. **Final Output:**
   - The value of `ans` is the sum of the maximum absolute differences, which simplifies to `4 * abs(n - m)`.

Therefore, the output of the `print(ans)` statement will be:
Output: **4 * abs(n - m)**