The value of `r` is updated by multiplying its current value by `p`. Given that `r` is equal to `n * (n - 1)` and `p` is equal to `n - 2`, we can express the new value of `r` as:

```
r = (n * (n - 1)) * (n - 2)
```

Since `n` is an integer such that 5 <= `n` <= 100, the specific numeric values of `r` will depend on `n`. However, the overall relationship can still be described without knowing the exact value of `n`. The other variables (`s`, `g`, `a`, and `i`) remain unaffected.

Therefore, the Output State is: `n` is an integer such that 5 <= `n` <= 100; `r` is now equal to (n * (n - 1)) * (n - 2); `s` is 2; `p` is `n - 2`; `g` is 3; `i` is 3.

Output State: **`n` is an integer such that 5 <= `n` <= 100; `r` is now equal to (n * (n - 1)) * (n - 2); `s` is 2; `p` is `n - 2`; `g` is 3; `i` is 3.**