`p` is decremented by 1. The previous value of `p` is `n - 2`, so after execution, `p` becomes `(n - 2) - 1`, which simplifies to `n - 3`. The values of the other variables remain unchanged. Therefore, the Output State is: `n` is an integer such that 5 <= `n` <= 100; `r` is now equal to (n * (n - 1)) * (n - 2); `s` is 2; `p` is `n - 3`; `g` is 3; `i` is 3.

Output State: **`n` is an integer such that 5 <= `n` <= 100; `r` is now equal to (n * (n - 1)) * (n - 2); `s` is 2; `p` is `n - 3`; `g` is 3; `i` is 3**