Based on the initial state provided:

- `a` is explicitly given as 1.
- `L` is a list `[1, 3, 2]`.
- `tot` is a value such that `tot` is less than `k` and `k` is less than or equal to `tot` plus 1.

From the condition given for `tot` and `k`, let's analyze the possible values:

- Since `tot < k` and `k <= tot + 1`, the only possible integer values for `tot` and `k` that satisfy both conditions are `tot = 1` and `k = 2`.

Now, substituting these values into the expression `pow * (2 * (k - tot) - 1)`:

- `k = 2`
- `tot = 1`

So, the expression becomes:
\[ \text{pow} \times (2 \times (2 - 1) - 1) = \text{pow} \times (2 \times 1 - 1) = \text{pow} \times (2 - 1) = \text{pow} \times 1 = \text{pow} \]

Since `pow` is not defined in the initial state, it must be a variable that is expected to have a value. Given no further context, we assume `pow` is meant to be evaluated as `1` (since it's a common placeholder for 1 in such expressions).

Thus, the expression simplifies to:
\[ 1 \]

Output: **1**