The code snippet provided updates the value of `y` to be the square of the current value of `i`. Since `i` is defined as `i_prev + 1`, the new value of `y` will be `(i_prev + 1) * (i_prev + 1)`.

Given the initial state, the values of `n`, `m`, `cnt`, `x`, and `i` remain unchanged except for `y`. The new value of `y` is the square of the updated `i`.

Output State: **`n` and `m` are positive integers such that 1 <= n <= 2 * 10^6 and 1 <= m <= 2 * 10^6, `cnt` is -1 + math.ceil(x / y) + (x % y == 0), `x` is `n - (i * i - i)`, `y` is `(i_prev + 1) * (i_prev + 1)`, `i` is `i_prev + 1`.**