Let's break down the code execution based on the provided initial state and the code snippet.

Initial State:
- `n` and `m` are positive integers such that 1 <= n <= 2 * 10^6 and 1 <= m <= 2 * 10^6
- `cnt` is calculated as `-1 + math.ceil(x / y) + (x % y == 0)`
- `x` is `n - (i * i - i)`
- `y` is `(i_prev + 1) * (i_prev + 1)`
- `i` is `i_prev + 1`

The code snippet:
```python
cnt = cnt + math.ceil(x / y) + (x % y == 0)
```

The code snippet modifies the value of `cnt` by adding `math.ceil(x / y) + (x % y == 0)` to its current value.

Let's denote the original value of `cnt` as `cnt_original`. Then the new value of `cnt` will be:
```python
cnt = cnt_original + math.ceil(x / y) + (x % y == 0)
```

Since `x`, `y`, and `cnt` are all derived from `n`, `m`, `i`, and `i_prev`, we can express the new value of `cnt` in terms of these variables:
- `x` is `n - (i * i - i)`
- `y` is `(i_prev + 1) * (i_prev + 1)`
- `i` is `i_prev + 1`

Therefore, the new value of `cnt` can be written as:
```python
cnt = cnt + math.ceil((n - (i * i - i)) / ((i_prev + 1) * (i_prev + 1))) + ((n - (i * i - i)) % ((i_prev + 1) * (i_prev + 1)) == 0)
```

The other variables (`n`, `m`, `x`, `y`, `i`, `i_prev`) remain unchanged.

Output State: **`n` and `m` are positive integers such that 1 <= n <= 2 * 10^6 and 1 <= m <= 2 * 10^6; `cnt` is updated to `cnt + math.ceil((n - (i * i - i)) / ((i_prev + 1) * (i_prev + 1))) + ((n - (i * i - i)) % ((i_prev + 1) * (i_prev + 1)) == 0); `x` is `n - (i * i - i)`; `y` is `(i_prev + 1) * (i_prev + 1)`; `i` is `i_prev + 1`.**