To determine the output state, let's analyze the given code snippet and the initial state.

Given:
- `A = [0, 1, 3]`
- `idx_A = [3, 4, 5]`
- `B` is a non-empty list
- `idx_B` is a non-empty list
- `n` must be greater than 0
- `i = n - 1 - j`
- `s[i] == '<'`

Code snippet:
```python
x = B[len(B) - 1] + (idx_B[len(B) - 1] - i) * len(idx_B)
```

Here, `x` is being assigned a new value based on the elements of `B` and `idx_B`, and the value of `i`.

Let's break down the expression:
- `B[len(B) - 1]`: This is the last element of the list `B`.
- `idx_B[len(B) - 1]`: This is the last element of the list `idx_B`.
- `len(idx_B)`: This is the length of the list `idx_B`.
- `i = n - 1 - j`: This is the value of `i` which depends on `n` and `j`.

The expression for `x` can be written as:
\[ x = \text{last element of } B + (\text{last element of } idx_B - i) \times \text{length of } idx_B \]

Since the exact values of `B`, `idx_B`, `n`, and `j` are not specified, we will keep them in their symbolic form.

Therefore, the output state will be:
- `A = [0, 1, 3]` (unchanged)
- `idx_A = [3, 4, 5]` (unchanged)
- `B` is a non-empty list (unchanged)
- `idx_B` is a non-empty list (unchanged)
- `n` must be greater than 0 (unchanged)
- `i = n - 1 - j` (unchanged)
- `s[i] == '<'` (unchanged)
- `x` is calculated as `B[len(B) - 1] + (idx_B[len(B) - 1] - i) * len(idx_B)`

Output State: **`A = [0, 1, 3], idx_A = [3, 4, 5], B` is a non-empty list, `idx_B` is a non-empty list, `n` must be greater than 0, `i = n - 1 - j`, `s[i] == '<', x = B[len(B) - 1] + (idx_B[len(B) - 1] - i) * len(idx_B)`**