Let's analyze the given code snippet and the initial state:

Initial State:
- `A = [0, 1, 3]`
- `idx_A = [3, 4, 5]`
- `B = [0, 1, 3]`
- `idx_B = [2, 1, 0]`
- `l = 0`
- `r = 3`
- `n` is greater than 0
- `s[i]` is `'>'`
- `a = 3 - 3 * i`
- `b = 3`

Code Snippet:
```python
b = b - (idx_A[l - 1] - idx_A[l - r - 1]) * (l - r)
```

Let's substitute the values of `l` and `r` into the equation:
- `l = 0`
- `r = 3`

Substituting these values into the indices:
- `idx_A[l - 1]` translates to `idx_A[0 - 1]` which is `idx_A[-1]` and equals `5`.
- `idx_A[l - r - 1]` translates to `idx_A[0 - 3 - 1]` which is `idx_A[-4]`. However, since `idx_A` only has three elements, this index is out of bounds. In Python, negative indices wrap around, so `idx_A[-4]` is equivalent to `idx_A[-1]` which is `5`.

Now, let's compute the expression:
- `(idx_A[l - 1] - idx_A[l - r - 1]) * (l - r)` translates to `(5 - 5) * (0 - 3)` which equals `0 * -3` which equals `0`.

Finally, updating `b`:
- `b = b - 0` which means `b` remains `3`.

Therefore, the only variable that changes is `b`.

Output State: **`A = [0, 1, 3], idx_A = [3, 4, 5], B = [0, 1, 3], idx_B = [2, 1, 0], l = 0, r = 3, n` is greater than 0, `s[i]` is `'>'`, `a = 3 - 3 * i`, `b = 3`**