Let's break down the given initial state and the print statement to determine what will be printed.

### Initial State:
- `A = [0, 1, 3]`
- `idx_A = [3, 4, 5]`
- `B = [0, 1, 3]`
- `idx_B = [2, 1, 0]`
- `l = 0`
- `r = 2`
- `a = 3`
- `n` is greater than 0
- `s[i]` is not equal to `'>'`
- `l` is greater than `r` (False)
- `r` is not equal to `0`
- `b = (i - 3) * 3`

### Print Statement:
```python
print(a * 2 + b * 2 + (n - i), end=' ')
```

### Analysis:
1. **Variable `a`:**
   - Given: `a = 3`
   - Calculation: `a * 2 = 3 * 2 = 6`

2. **Variable `b`:**
   - Given: `b = (i - 3) * 3`
   - However, the value of `i` is not provided in the initial state.
   - Since `i` is not explicitly defined, we cannot compute the exact value of `b`.
   - We'll keep `b` in its formulaic form: `b = (i - 3) * 3`
   - Calculation: `b * 2 = ((i - 3) * 3) * 2 = (i - 3) * 6`

3. **Variable `n` and `i`:**
   - Given: `n` is greater than 0
   - Given: `s[i]` is not equal to `'>'`
   - Given: `r` is not equal to `0`
   - However, the exact values of `n` and `i` are not provided.
   - Since `i` is not explicitly defined, we cannot compute the exact value of `(n - i)`.
   - We'll keep `(n - i)` in its formulaic form: `(n - i)`

### Combining the Calculations:
- The expression to be printed is: `a * 2 + b * 2 + (n - i)`
- Substituting the known and unknown values:
  - `a * 2 = 6`
  - `b * 2 = (i - 3) * 6`
  - `(n - i) = (n - i)`
- Therefore, the combined expression is: `6 + (i - 3) * 6 + (n - i)`

### Final Output Description:
The print statement will output the result of the expression `6 + (i - 3) * 6 + (n - i)`, where `i` is an undefined variable and `n` is a positive integer greater than 0.

Output: **6 + (i - 3) * 6 + (n - i) (where i is an undefined variable and n is a positive integer greater than 0)**