To determine the new value of `b` after executing the given line of code, we need to substitute the expressions and values into the equation.

Given:
- `b = B[r] - B[r - l]`
- The new assignment: `b = b - (idx_B[r - l] - i) * (r - l)`

Let's break down the calculation:

1. **Original `b` Calculation**:
   - `b = B[r] - B[r - l]`

2. **New `b` Calculation**:
   - `b = (B[r] - B[r - l]) - (idx_B[r - l] - i) * (r - l)`

Since the exact values of `r` and `l` are not specified, let's assume some values to illustrate the calculation. For example, let's assume `r = 2` and `l = 1` (these are hypothetical values for demonstration purposes).

Given `r = 2` and `l = 1`:
- `b = B[2] - B[1]` (from the original `b` calculation)
- `b = (B[2] - B[1]) - (idx_B[0] - i) * (2 - 1)`
- `b = (B[2] - B[1]) - (idx_B[0] - i)`

Substituting the values from the initial state:
- `B = [0, 1, 3]`
- `idx_B = [2, 1, 0]`

So,
- `b = (3 - 1) - (2 - i)`
- `b = 2 - (2 - i)`
- `b = 2 - 2 + i`
- `b = i`

Thus, if `r = 2` and `l = 1`, the new value of `b` would be `i`.

However, since the exact values of `r` and `l` are not provided, we'll express the final `b` in terms of `r`, `l`, `i`, and the lists `B` and `idx_B`.

The updated `b` is:
- `b = (B[r] - B[r - l]) - (idx_B[r - l] - i) * (r - l)`

Therefore, the Output State is:

Output State: **`A = [0, 1, 3]`, `idx_A = [3, 4, 5]`, `B = [0, 1, 3]`, `idx_B = [2, 1, 0]`, `n` is greater than 0, `s[i]` is either `'>'` or not `'>'`, `i` is incremented by 1, `r` is decreased by 1, `a` is `i - 3` if `l = 1`, `2i - 7` if `l = 2`, `3i - 12` if `l = 3`, `b` is `(B[r] - B[r - l]) - (idx_B[r - l] - i) * (r - l)`**.