Let's analyze the given code snippet and its impact on the variables:

Initial State: 
- `A = [0, 1, 3]`
- `idx_A = [3, 4, 5]`
- `B = [0, 1, 3]`
- `idx_B = [2, 1, 0]`
- `n` is greater than 0
- `s[i]` is either `'>'` or not `'>'`
- `i` is incremented by 1
- `r` is decreased by 1
- `a` is calculated based on `l`:
  - `a = i - 3` if `l = 1`
  - `a = 2i - 7` if `l = 2`
  - `a = 3i - 12` if `l = 3`
- `b` is calculated based on `r` and `l`:
  - If `r - l >= 0`, then `b = (B[r] - B[r - l]) - (idx_B[r - l] - i) * (r - l)`
  - Otherwise, `b = B[r]`

Code Snippet:
```python
b = b + (idx_B[r] - i) * l
```

Impact of the Code:
- The value of `b` is updated by adding `(idx_B[r] - i) * l` to its current value.

Given the initial conditions, let's consider the possible values for `b` before the update:
- If `r - l >= 0`, `b` was initially calculated as `(B[r] - B[r - l]) - (idx_B[r - l] - i) * (r - l)`.
- If `r - l < 0`, `b` was initially `B[r]`.

After the code snippet executes, the new value of `b` will be:
- `b = (B[r] - B[r - l]) - (idx_B[r - l] - i) * (r - l) + (idx_B[r] - i) * l` if `r - l >= 0`
- `b = B[r] + (idx_B[r] - i) * l` if `r - l < 0`

Since the exact values of `r` and `l` are not specified, we'll keep the expressions general.

Output State: **`A = [0, 1, 3]`, `idx_A = [3, 4, 5]`, `B = [0, 1, 3]`, `idx_B = [2, 1, 0]`, `n` is greater than 0, `s[i]` is either `'>'` or not `'>'`, `i` is incremented by 1, `r` is decreased by 1, `a` is `i - 3` if `l = 1`, `2i - 7` if `l = 2`, `3i - 12` if `l = 3`, `b` is updated to `(B[r] - B[r - l]) - (idx_B[r - l] - i) * (r - l) + (idx_B[r] - i) * l` if `r - l >= 0` or `B[r] + (idx_B[r] - i) * l` if `r - l < 0`.**

In simple terms, the value of `b` is adjusted by adding `(idx_B[r] - i) * l` to its previous value, while all other variables remain unchanged.