Postcondition: **`A = [0, 1, 3]`, `idx_A = [3, 4, 5]`, `B = [0, 1, 3]`, `idx_B = [2, 1, 0]`, `n` is greater than 0, `s[i]` is either `'>'` or not `'>'`, `i` is incremented by 1. If `s[i] == '>'`, then if `l < r`, `a` is set to `A[l]`, `x` is set to `r - (l + 2)`, and `b` is set to `(idx_B[r - 1] - i) * (l + 1)`. If `l >= r`, and `r` is not equal to 0, `a` is set to `B[r - 1] + (idx_B[r - 1] - i) * r`, and `b` is updated to its previous value plus `(i - idx_A[l - 1]) * r`. `l` is incremented by 1. If `s[i] != '>'`, then `r` is decreased by 1 unless `r` was initially 0 or `l > r`, in which case `r` remains 0 or is set to 1. If `l <= r`, `a` is set to `i - 3` if `l = 1`, `2i - 7` if `l = 2`, `3i - 12` if `l = 3`, and `b` is updated to `(B[r] - B[r - l]) - (idx_B[r - l] - i) * (r - l) + (idx_B[r] - i) * l` if `r - l >= 0` or `B[r] + (idx_B[r] - i) * l` if `r - l < 0`. If `l > r`, `a` is either `0` or `1` depending on the new value of `r`, and `b` is `A[l - 1] + (i - idx_A[l - 1]) * (r + 1)`**