To determine the new value of `b`, we need to substitute the given expressions into the equation:

Given:
- `b = 2`
- `x = r - (l + 2)`
- `idx_B = [2, 1, 0]`

The equation to evaluate is:
```
b = b - (idx_B[x] - idx_B[r - 1]) * (x + 1)
```

Let's break down the expression step by step:

1. Calculate `idx_B[x]`:
   - Since `x = r - (l + 2)`, we need to know the values of `r` and `l`. However, these values are not provided directly, so we'll assume `x` is within the bounds of `idx_B` (0, 1, or 2).

2. Calculate `idx_B[r - 1]`:
   - Similarly, `r - 1` should also be within the bounds of `idx_B`.

Since the exact values of `r` and `l` are not provided, let's consider the possible values of `x` and `r - 1` and see how `b` changes.

### Case Analysis:
#### Case 1: Assume `x = 0` and `r - 1 = 2`
- `idx_B[x] = idx_B[0] = 2`
- `idx_B[r - 1] = idx_B[2] = 0`
- `b = 2 - (2 - 0) * (0 + 1) = 2 - 2 * 1 = 0`

#### Case 2: Assume `x = 1` and `r - 1 = 1`
- `idx_B[x] = idx_B[1] = 1`
- `idx_B[r - 1] = idx_B[1] = 1`
- `b = 2 - (1 - 1) * (1 + 1) = 2 - 0 * 2 = 2`

#### Case 3: Assume `x = 2` and `r - 1 = 0`
- `idx_B[x] = idx_B[2] = 0`
- `idx_B[r - 1] = idx_B[0] = 2`
- `b = 2 - (0 - 2) * (2 + 1) = 2 - (-2) * 3 = 2 + 6 = 8`

Without specific values for `r` and `l`, we cannot definitively determine the exact value of `b`. However, we can express the updated `b` in terms of `x` and `r`.

Given the general form:
- `b = 2 - (idx_B[x] - idx_B[r - 1]) * (x + 1)`

We can write the output state as:

Output State: **`A = [0, 1, 3]`, `idx_A = [3, 4, 5]`, `B = [0, 1, 3]`, `idx_B = [2, 1, 0]`, `n` is greater than 0, `s[i]` is either `'>'` or not `'>'`, `i` is 1, `a` is 1, `x` is `r - (l + 2)`, `b` is `2 - (idx_B[x] - idx_B[r - 1]) * (x + 1)`**