To determine the output of the given print statement, we need to carefully analyze the initial state and the calculations involved in determining the values of `a` and `b`.

### Initial State Recap:
- `A = [0, 1, 3]`
- `idx_A = [3, 4, 5]`
- `B = [0, 1, 3]`
- `idx_B = [2, 1, 0]`
- `n` is greater than 0
- `s[i]` is either `'>'` or not `'>'`
- `i` is 1
- `a` is calculated as `B[r - 1] + (idx_B[r - 1] - i) * r`
- `b` is updated to `b + (1 - idx_A[l - 1]) * r`

### Analysis:

#### Determining `r` and `l`:
The variables `r` and `l` are not explicitly defined in the initial state. However, since they are used in the calculations of `a` and `b`, we need to make assumptions based on typical usage patterns in such problems. Given that `i` is 1, it's reasonable to assume that `r` and `l` are also indices related to the lists `B` and `A`, respectively.

For simplicity, let's assume:
- `r = 2` (since `B` has 3 elements, and `r - 1` should be a valid index)
- `l = 2` (similarly, `A` has 3 elements)

#### Calculating `a`:
Given `a = B[r - 1] + (idx_B[r - 1] - i) * r`:
- `r = 2`
- `B[r - 1] = B[1] = 1`
- `idx_B[r - 1] = idx_B[1] = 1`
- `i = 1`
- Therefore, `a = 1 + (1 - 1) * 2 = 1 + 0 = 1`

#### Calculating `b`:
Given `b` is updated to `b + (1 - idx_A[l - 1]) * r`:
- `l = 2`
- `idx_A[l - 1] = idx_A[1] = 4`
- `r = 2`
- Therefore, the update to `b` is `b + (1 - 4) * 2 = b - 6`
- Assuming `b` was initially 0 (since no initial value is given), `b` becomes `-6`

#### Final Calculation for Print Statement:
The print statement is `print(a * 2 + b * 2 + (n - i), end=' ')`:
- `a = 1`
- `b = -6`
- `i = 1`
- `n` is greater than 0, but its exact value is not specified. Let's denote it as `n`.

Thus, the expression evaluates to:
\[ a * 2 + b * 2 + (n - i) = 1 * 2 + (-6) * 2 + (n - 1) = 2 - 12 + n - 1 = n - 11 \]

### Conclusion:
The output of the print statement depends on the value of `n`, which is not explicitly given. Therefore, the most precise description of the output is:

Output: **n - 11 (where n is greater than 0)**