To determine the output state, let's analyze the given code snippet and the initial state:

Given Code:
```python
b = b - (idx_A[l - 1] - idx_A[l - r - 2]) * (l - r - 1)
```

Initial State:
- `A = [0, 1, 3]`
- `idx_A = [3, 4, 5]`
- `B = [0, 1, 3]`
- `idx_B = [2, 1, 0]`
- `n` is greater than 0
- `s[i]` is either `'>'` or not `'>'`
- `i` is 1
- `r` is 2
- `a` is 3
- `b` is -2

From the initial state, we know the following:
- `l` is not defined in the initial state, so we need to assume it from the context. Given the indices used (`l - 1` and `l - r - 2`), `l` should be at least 3 to avoid index errors. Let's assume `l` is 3 for this calculation.
- `r` is 2.

Let's substitute the values into the equation:
- `b = b - (idx_A[l - 1] - idx_A[l - r - 2]) * (l - r - 1)`
- `b = -2 - (idx_A[3 - 1] - idx_A[3 - 2 - 2]) * (3 - 2 - 1)`
- `b = -2 - (idx_A[2] - idx_A[-1]) * (0)`

Since `idx_A` only has indices from 0 to 2, `idx_A[-1]` would refer to the last element of the list, which is `idx_A[2]`. Thus:
- `b = -2 - (idx_A[2] - idx_A[2]) * (0)`
- `b = -2 - (5 - 5) * (0)`
- `b = -2 - 0 * 0`
- `b = -2`

Therefore, the value of `b` remains `-2`.

Output State: **`A = [0, 1, 3]`, `idx_A = [3, 4, 5]`, `B = [0, 1, 3]`, `idx_B = [2, 1, 0]`, `n` is greater than 0, `s[i]` is either `'>'` or not `'>'`, `i` is 1, `r` is 2, `a` is 3, `b` is -2**