Correctness: False

The code does not follow the problem description for all potential cases. The issue lies in the condition `((b - a) % c == 0 and (b - a) / c >= 0)`. This condition assumes that the difference between `b` and `a` is divisible by `c`, and the result is non-negative, which may not always be true. 

For example, if `a = 1`, `b = 7`, and `c = 3`, the condition `((b - a) % c == 0 and (b - a) / c >= 0)` evaluates to `((7 - 1) % 3 == 0 and (7 - 1) / 3 >= 0)`, which simplifies to `(6 % 3 == 0 and 6 / 3 >= 0)` -> `(0 == 0 and 2 >= 0)`, which is true. However, this condition gives a false positive result for this input, as 7 is not actually a valid element in the sequence starting from 1 with a difference of 3 between each element. 

Therefore, the code is incorrect as it fails to handle all potential cases as required by the problem description.