Let's break down the initial state and the code snippet step by step to determine what will be printed.

### Initial State:
- `t` is an integer such that \(1 \leq t \leq 1000\).
- `_` is 1 (this variable is not used in the calculation, it's just a placeholder).
- `k` is an input integer.
- `x` is an input integer.
- `a` is an input integer.
- `i` is set to `x`.
- `s` is the result of the expression `1 + sum((s // (k - 1) + 1) for _ in range(x))` where `s` starts at 1.

### Expression for `s`:
The expression for `s` is:
\[ s = 1 + \sum_{i=0}^{x-1} \left( \frac{s_i}{k-1} + 1 \right) \]
where \( s_i \) is the value of `s` at the \(i\)-th iteration, starting with \( s_0 = 1 \).

### Calculation of `s`:
1. **Initialization**: \( s = 1 \).
2. **Loop**: For each iteration from 0 to \( x-1 \):
   - Calculate \( \frac{s}{k-1} + 1 \).
   - Add this value to `s`.

Let's break down the loop:
- For the first iteration (\( i = 0 \)):
  \[ s = 1 + \left( \frac{1}{k-1} + 1 \right) \]
  \[ s = 1 + \left( \frac{1}{k-1} + 1 \right) = 1 + \frac{1}{k-1} + 1 = 2 + \frac{1}{k-1} \]

- For the second iteration (\( i = 1 \)):
  \[ s = 2 + \frac{1}{k-1} + \left( \frac{2 + \frac{1}{k-1}}{k-1} + 1 \right) \]
  \[ s = 2 + \frac{1}{k-1} + \left( \frac{2(k-1) + 1}{(k-1)^2} + 1 \right) \]
  \[ s = 2 + \frac{1}{k-1} + \left( \frac{2k - 2 + 1}{(k-1)^2} + 1 \right) \]
  \[ s = 2 + \frac{1}{k-1} + \left( \frac{2k - 1}{(k-1)^2} + 1 \right) \]
  \[ s = 2 + \frac{1}{k-1} + \frac{2k - 1}{(k-1)^2} + 1 \]
  \[ s = 3 + \frac{1}{k-1} + \frac{2k - 1}{(k-1)^2} \]

This pattern continues for each iteration, and the final value of `s` after \( x \) iterations can be described as:
\[ s = 1 + \sum_{i=0}^{x-1} \left( \frac{s_i}{k-1} + 1 \right) \]

### Print Statement:
The print statement is:
```python
print('Yes' if a >= s else 'No')
```

### Determining the Output:
- The value of `s` is calculated based on the input values of `k` and `x`.
- The value of `a` is an input integer.
- The print statement will output 'Yes' if `a` is greater than or equal to `s`, and 'No' otherwise.

Since the exact values of `k` and `x` are not provided, we can't compute the exact numerical value of `s`. However, we can describe the output based on the given conditions.

### Final Output:
Output: **'Yes' if \( a \geq s \) else 'No' (where \( s \) is the result of the expression \( 1 + \sum_{i=0}^{x-1} \left( \frac{s_i}{k-1} + 1 \right) \) and \( s \) starts at 1)**