Alright, I've got this problem to figure out. So, let's see what it's asking.

We have a little boy named Nikita who has some cubes, and he wants to build a tower using these cubes. He can perform two types of moves: either add one cube to the top of the tower or remove one cube from the top. He does this for a total of n moves, and we need to determine if it's possible, after these n moves, to have exactly m cubes in the tower.

First, I need to understand the operations he can perform. Each move is either adding one cube or removing one cube. So, starting from zero cubes, he alternates between adding and removing cubes in a sequence of n steps.

I need to think about how the number of cubes in the tower changes with each move. Let's consider a few examples to get a feel for the problem.

Take the first example from the problem:

n = 3, m = 3

So, Nikita makes 3 moves, and we want to end up with 3 cubes.

Possible sequences of moves:

1. Add, Add, Add → tower has 3 cubes.

2. Add, Add, Remove → tower has 2 cubes.

3. Add, Remove, Add → tower has 2 cubes.

4. Add, Remove, Remove → tower has 0 cubes.

5. Remove, Add, Add → tower has 2 cubes (since removing from an empty tower doesn't make sense, but maybe in this problem, removing from an empty tower just does nothing).

Wait, the problem says "remove exactly 1 cube from the top of the tower", so if the tower is empty, removing a cube shouldn't do anything, essentially it's a no-op.

So, in the sequence, if he tries to remove a cube when there are none, nothing happens.

So, for n=3, m=3:

Only the sequence Add, Add, Add works, which indeed gives us 3 cubes. So, "Yes".

Second example:

n=2, m=4

Possible sequences:

1. Add, Add → tower has 2 cubes.

2. Add, Remove → tower has 1 cube.

3. Remove, Add → tower has 1 cube.

4. Remove, Remove → tower has 0 cubes.

In none of these sequences do we reach 4 cubes. So, "No".

Third example:

n=5, m=3

Possible sequences:

1. Add, Add, Add, Remove, Remove → 3 cubes.

2. Add, Add, Remove, Add, Remove → 2 cubes.

3. Add, Remove, Add, Add, Remove → 2 cubes.

4. And so on.

So, it's possible to end up with 3 cubes, hence "Yes".

From these examples, I need to find a general condition that determines whether it's possible to end up with m cubes after n moves.

Let's think in terms of the net effect of the moves. Each add operation increases the number of cubes by 1, and each remove operation decreases it by 1, but only if there is at least one cube to remove.

So, if I let a be the number of add operations and r be the number of remove operations, with a + r = n.

The number of cubes in the tower would be a - r, but with the constraint that you can't remove more cubes than are present.

So, the effective number of remove operations is limited by the number of cubes available.

This seems a bit tricky. Maybe there's a better way to approach this.

Another way to look at it is to consider that the maximum number of cubes you can have after n moves is n (if you add a cube in every move).

The minimum number of cubes you can have is max(0, n - 2*m). Wait, that doesn't seem right.

Wait, let's think differently. Each remove operation can only remove a cube that has been previously added.

So, the number of remove operations cannot exceed the number of add operations.

In other words, r ≤ a.

Since a + r = n, and r ≤ a, we can substitute r = n - a into the inequality:

n - a ≤ a ⇒ n ≤ 2a ⇒ a ≥ n/2.

So, the number of add operations must be at least half the total number of moves.

The number of cubes in the tower at the end is a - r = a - (n - a) = 2a - n.

We want 2a - n = m.

So, 2a - n = m ⇒ 2a = m + n ⇒ a = (m + n)/2.

Since a must be an integer (number of add operations), (m + n) must be even.

Also, a must be at least n/2 and at least 0, and at most n.

So, the condition is:

- (m + n) is even.

- (m + n)/2 is an integer between 0 and n, inclusive.

Given that m and n are both positive integers from 1 to 100, we can check these conditions.

So, in the first example:

n=3, m=3.

m + n = 6, which is even. (m + n)/2 = 3, which is between 0 and 3, inclusive. So, "Yes".

Second example:

n=2, m=4.

m + n = 6, which is even. (m + n)/2 = 3, which is between 0 and 2? No, 3 > 2. So, "No".

Third example:

n=5, m=3.

m + n = 8, which is even. (m + n)/2 = 4, which is between 0 and 5, inclusive. So, "Yes".

This seems to align with the examples.

So, the general condition is:

If (m + n) is even and 0 ≤ (m + n)/2 ≤ n, then "Yes", else "No".

But, since m and n are both at least 1, and m can be up to 100, we need to ensure that (m + n)/2 is an integer and within the range [0, n].

Wait, actually, since a = (m + n)/2, and a must be an integer, (m + n) must be even.

Also, a must be at least n/2 (from earlier), but given a = (m + n)/2, and a ≤ n, this is already covered by the condition.

Moreover, a must be at least 0, which implies (m + n)/2 ≥ 0, which is always true since m and n are positive.

So, the condition simplifies to:

- (m + n) is even.

- (m + n)/2 ≤ n.

But, (m + n)/2 ≤ n ⇒ m ≤ n.

Wait, is that correct?

Let's check:

(m + n)/2 ≤ n ⇒ m + n ≤ 2n ⇒ m ≤ n.

So, the condition is that (m + n) is even and m ≤ n.

Wait, but in the third example, n=5, m=3, m ≤ n, and (m + n)=8 is even, which matches "Yes".

In the second example, m=4, n=2, m > n, but (m + n)=6 is even, but m > n, so "No".

Wait, but according to the condition, m ≤ n and (m + n) is even.

But in the first example, m=3, n=3, m ≤ n, and (m + n)=6 is even, "Yes".

Third example, m=3, n=5, m ≤ n, and (m + n)=8 is even, "Yes".

Another test case: n=4, m=2.

(m + n)=6 is even, m ≤ n, so "Yes".

n=4, m=4.

(m + n)=8 is even, m ≤ n, "Yes".

n=4, m=0.

(m + n)=4 is even, m ≤ n, "Yes".

n=1, m=1.

(m + n)=2 is even, m ≤ n, "Yes".

n=1, m=2.

(m + n)=3 is odd, m > n, "No".

Seems consistent.

So, the condition is:

If (m + n) is even and m ≤ n, then "Yes", else "No".

Wait, but in the second example, n=2, m=4, m > n, and (m + n)=6 is even, which should be "No", as per our condition.

Another test case: n=4, m=0.

(m + n)=4 is even, m ≤ n, "Yes".

n=3, m=0.

(m + n)=3 is odd, m ≤ n, "No".

n=2, m=0.

(m + n)=2 is even, m ≤ n, "Yes".

n=1, m=0.

(m + n)=1 is odd, m ≤ n, "No".

n=5, m=1.

(m + n)=6 is even, m ≤ n, "Yes".

n=5, m=2.

(m + n)=7 is odd, m ≤ n, "No".

Seems consistent.

So, the condition can be simplified to:

If (m + n) is even and m ≤ n, then "Yes", else "No".

This seems to cover all cases.

Now, looking at the given program:

kreker = int(input())

for i in range(kreker):

func_1()

def func_1():

(n, m) = map(int, input().split())

if n >= m:

print('Yes')

else:

print('No')

So, the program checks if n >= m and prints "Yes" if it is, otherwise "No".

But according to our earlier reasoning, the condition should be:

If (m + n) is even and m ≤ n, then "Yes", else "No".

Wait, but the program only checks if n >= m, without checking if (m + n) is even.

This is a problem.

Looking back at the examples:

First example: n=3, m=3.

n >= m is True, but we also need (m + n) to be even, which it is (6), so "Yes".

Second example: n=2, m=4.

n >= m is False (2 >= 4 is False), so program prints "No", which is correct.

Third example: n=5, m=3.

n >= m is True, and (m + n)=8 is even, so "Yes".

Another test case: n=4, m=2.

n >= m is True, (m + n)=6 is even, "Yes".

n=4, m=4.

n >= m is True, (m + n)=8 is even, "Yes".

n=4, m=0.

n >= m is True, (m + n)=4 is even, "Yes".

n=1, m=1.

n >= m is True, (m + n)=2 is even, "Yes".

n=1, m=0.

n >= m is True, (m + n)=1 is odd, but program prints "Yes" since n >= m, which is incorrect because (m + n) is odd.

According to our condition, it should be "No" because although m ≤ n, (m + n) is odd.

Hence, the program is incorrect in this case.

Similarly, n=3, m=0.

(m + n)=3 is odd, m ≤ n, should be "No", but program prints "Yes" because n >= m.

Another test case: n=2, m=0.

(m + n)=2 is even, m ≤ n, should be "Yes", and program prints "Yes" because n >= m.

n=3, m=1.

(m + n)=4 is even, m ≤ n, should be "Yes", program prints "Yes" because n >= m.

n=3, m=2.

(m + n)=5 is odd, m ≤ n, should be "No", program prints "Yes" because n >= m.

Hence, the program is incorrect because it doesn't check the parity of (m + n).

It only checks if n >= m, which is part of the condition, but misses the condition that (m + n) must be even.

Therefore, the program is incorrect.

**Final Answer**

\[ \boxed{\text{False}} \]

