The code snippet `ans += (a[i] - a[i - 1]) // 2` updates the value of `ans` by adding half the difference between the elements at indices `i` and `i-1` of the list `a`. Given the initial state:

- `t` is a positive integer such that 1 ≤ t ≤ 10^4
- `n` is an input integer
- `x` is an input integer where 2 ≤ x ≤ min(n, 2 · 10^5)
- `y` is an input integer where 0 ≤ y ≤ n - x
- `tt` must be greater than 0
- `ii` is 1
- `a` is a sorted list of integers in ascending order that must have at least 4 elements
- `i` is 3
- `tmp` now contains the value `(a[3] - a[2]) // 2`

The value of `ans` is updated as follows:
- The difference between `a[3]` and `a[2]` is calculated.
- This difference is divided by 2 using integer division.
- The result is added to the current value of `ans`.

Since the initial value of `ans` is not specified, we assume it is initially 0. Therefore, the new value of `ans` is `(a[3] - a[2]) // 2`.

The output state is:
Output State: **`t` is a positive integer such that 1 ≤ t ≤ 10^4, `n` is an input integer, `x` is an input integer where 2 ≤ x ≤ min(n, 2 · 10^5), `y` is an input integer where 0 ≤ y ≤ n - x, `tt` must be greater than 0, `ii` is 1, `a` is a sorted list of integers in ascending order that must have at least 4 elements, `i` is 3, `tmp` is `(a[3] - a[2]) // 2`, `ans` is `(a[3] - a[2]) // 2`.**