Based on the initial state provided:

- `p1` is an integer entered by the user.
- `p2` is an integer entered by the user.
- `p3` must be an odd number and at least 3.
- `t` is a positive integer such that \(1 \leq t \leq 500\).
- `_` is 2.
- `x` is either 0 or 2.
- `y` is either `p3` or `p3 - 1`, and `y` is greater than or equal to 2.

We need to determine the value of `p1 - x + p3`.

### Step-by-Step Analysis:

1. **Value of `x`:**
   - `x` is either 0 or 2. Since no specific value is given, we consider both possibilities.

2. **Value of `p3`:**
   - `p3` must be an odd number and at least 3. Therefore, `p3` could be any odd number starting from 3 (e.g., 3, 5, 7, ...).

3. **Expression Evaluation:**
   - If `x = 0`, then `p1 - x + p3 = p1 + p3`.
   - If `x = 2`, then `p1 - x + p3 = p1 - 2 + p3`.

Given these possibilities, the exact output cannot be determined precisely without knowing the specific values of `p1` and `p3`. However, we can describe the possible outputs based on the given conditions.

### Possible Outputs:
- If `x = 0`, the output will be `p1 + p3`.
- If `x = 2`, the output will be `p1 - 2 + p3`.

Since we don't have the exact values of `p1` and `p3`, we express the output in terms of these variables.

Output: **p1 + p3 (if x = 0) or p1 - 2 + p3 (if x = 2)**