The given code snippet calculates the `next_year` based on the `current_year` and the first element `ai` from the list `a` of the first test case in `test_cases`. Given that `current_year` is 0 initially, the calculation simplifies as follows:

```
next_year = (current_year // ai + 1) * ai
```

Since `current_year` is 0, `current_year // ai` will be 0 for any positive integer `ai`. Therefore, the expression simplifies to:

```
next_year = (0 + 1) * ai = ai
```

This means `next_year` will be equal to the first element `ai` in the list `a` of the first test case.

Output State: **`t` is an integer such that 1 <= t <= 1000, `test_cases` is a list of `t` test cases where each test case is a tuple (n, a) with `n` being an integer such that 1 <= `n` <= 100 and `a` being a list of `n` integers where each integer `a_i` satisfies 1 <= `a_i` <= 10^6, `results` is an empty list, `n` is the first element of the first test case in `test_cases`, `a` is the second element of the first test case in `test_cases`, `current_year` is 0, `next_year` is equal to the first element of `a` in the first test case.**