The code snippet appends `b[i]` to the list `ans1`. Given that `b[i] == b[i - 1]` is true for the current value of `i`, `b[i]` is the same as the last element added to `ans1`. Therefore, `ans1` will now have an additional instance of `b[i]`.

Here is the updated output state:

Output State: **`n` must be greater than 2; `ans1` is a list containing the elements it originally had with `b[i]` appended twice; `ans2` is an empty list; `l` is a list containing the first element of `b` if `b[0] != b[1]`, and if `b[n - 2] != b[n - 1]`, `l` also contains `b[n - 1]`; `q` is `q + 1`; `a` is a list of integers derived from the input; `b` is the sorted first `n` elements of `a`; `c` is the sorted elements of `a[n:]`; `req` is `2 * k`. If `k` is 0, `k` remains unchanged; `b[i] == b[i - 1]` is true for the current value of `i`.**