The provided code appends `l[i]` to `ans2`. Given the initial state, `i` is 1, so `l[i]` refers to the second element of `l`. 

Here is the updated output state with the changes applied:

Output State: **`ans1` contains elements from `b` that are repeated based on the condition `b[i] == b[i - 1]` plus the element `l[i]`, and now includes `l[1]` at the end; `ans2` contains elements from `c` that are repeated based on the condition `c[i] == c[i - 1]` until `k` reaches 0, plus `l[i]`; `k` is -2; `l` contains at least one unique element from `b` based on the conditions `b[i] != b[i - 1]` and `b[i] != b[i + 1]`; `q` is incremented based on the number of times `b[i] != b[i + 1]` occurs; `i` is 1; `ans2` now includes `l[0]` and `l[1]` at the end.**

In simple terms, `ans2` now includes an additional element from `l` at index 1, while all other variables remain unchanged.