Let's break down the problem step by step:

1. **Identify the Loop Condition**: The loop condition is `j >= i and s < j - i + 1`.
2. **Current States**: 
   - `i` is `m`
   - `j` is `m - 1`
   - `s` is either `-1` or `0`

3. **Check the First Part of the Loop Condition (`j >= i`)**:
   - Currently, `j = m - 1` and `i = m`. This means `j >= i` is false because `m - 1 < m`.

4. **Check the Second Part of the Loop Condition (`s < j - i + 1`)**:
   - For `j = m - 1` and `i = m`, we have `j - i + 1 = (m - 1) - m + 1 = -1 + 1 = 0`.
   - Therefore, the second part of the condition becomes `s < 0`.
   - Since `s` can be either `-1` or `0`, `s < 0` is true only when `s = -1`.

5. **Determine What Needs to Be Adjusted**:
   - The loop will not execute because both parts of the condition are not met.
   - To make the loop execute one more time, we need to adjust the state such that at least one part of the condition is true.

6. **Possible Adjustments**:
   - Make `j >= i` true: This can be achieved by setting `j` to a value greater than or equal to `i` (which is `m`).
   - Make `s < j - i + 1` true: This can be achieved by setting `s` to a value less than `0` (since `j - i + 1 = 0`).

Given these conditions, let's set `j` to `m` (making `j >= i` true) and `s` to `-1` (since `s < 0` is true in this case).

State: **`i` is `m`, `j` must be greater than or equal to `m`, and `s` must be `-1`**