Let's break down the problem step by step:

1. **Initial States:**
   - `i` is `m - 1`
   - `j` is `0`
   - `s` is `s + c[m - 1]`
   - `ans[j - i + 1]` is incremented by 1 since `j <= m` is true.

2. **Loop Condition:**
   - The loop condition is `while j >= i and s < j - i + 1`.

3. **Analyze the Loop Condition:**
   - For the loop to execute, two conditions must be met:
     1. `j >= i`
     2. `s < j - i + 1`

4. **Current Values:**
   - Given `i = m - 1` and `j = 0`, we check the first condition: `j >= i` becomes `0 >= (m - 1)`, which is false unless `m` is 1.
   - Since `m` is not specified to be 1, let's assume `m > 1` for general consideration. Thus, `j >= i` is not satisfied initially.
   - Next, consider `s < j - i + 1`. With `j = 0` and `i = m - 1`, this becomes `s < 1 - (m - 1) + 1` or `s < 3 - m`.

5. **Adjusting the State:**
   - To satisfy `j >= i`, we need to increase `j` to be at least as large as `i`. Since `i = m - 1`, we need `j >= m - 1`.
   - The current value of `s` is `s + c[m - 1]`, and we need to ensure that `s < j - i + 1` holds after adjusting `j`.

Given these points, we need to adjust the state such that `j` is at least `m - 1` and the condition `s < j - i + 1` is satisfied.

**Adjusted State:**
- `i` remains `m - 1`
- `j` is set to `m - 1` (or higher)
- `s` remains `s + c[m - 1]`

Thus, the final state before the loop can proceed is:
State: **`i` is `m - 1`, `j` is `m - 1`, `s` is `s + c[m - 1]`**