Let's break down the problem step by step:

1. **Initial States**: 
   - `i` is `m - 1`
   - `j` is `m - 2`
   - `s` is updated based on the value of `b[j]`:
     - If `b[j]` is `True`, then `s = s + c[m - 1] - 1`
     - If `b[j]` is `False`, then `s = s + c[m - 1]`

2. **Loop Condition**: 
   The loop continues as long as `j >= i` and `s < j - i + 1`.

3. **Current Values**:
   - `i = m - 1`
   - `j = m - 2`
   - `s` is either `s + c[m - 1] - 1` (if `b[j]` is `True`) or `s + c[m - 1]` (if `b[j]` is `False`)

4. **Loop Execution Condition**:
   - `j >= i` will always be true because `j = m - 2` and `i = m - 1`.
   - We need to check the condition `s < j - i + 1`.

5. **Calculating `j - i + 1`**:
   - `j - i + 1 = (m - 2) - (m - 1) + 1 = m - 2 - m + 1 + 1 = 0`.

6. **Loop Condition Simplified**:
   - Since `j - i + 1` simplifies to `0`, the condition `s < j - i + 1` becomes `s < 0`.

7. **Adjusting the State**:
   - For the loop to continue, `s` must be less than `0`.
   - Given `s` is updated as `s + c[m - 1] - 1` or `s + c[m - 1]`, `s` must be negative.

8. **Conclusion**:
   - The only state that needs to be adjusted is `s` to ensure it is less than `0`.

Therefore, the final state required for the loop to execute one more time is:

**State: `i` is `m - 1`, `j` is `m - 2`, `s` is less than `0`**