Let's break down the initial state and the print statement step by step:

1. **Initial State**:
   - `t` must be greater than 0.
   - `p1`, `p2`, and `p3` are integers obtained from the input split by spaces.
   - The sum of `p1`, `p2`, and `p3` is odd.
   - `p3` is less than `p1 + p2`.
   - `low` is `p3 - p1` if `p3 - p1 < p3 - p2` else `p3 - p2`.
   - `high` is `p3 - p1` if `p3 - p1 > p3 - p2` else `p3 - p2`.
   - `cur` is equal to `low`.
   - `high` must be greater than or equal to `low`.
   - The condition `(p1 - cur <= p2 - (p3 - cur))` is also true.

2. **Print Statement**:
   - We need to evaluate `p1 - cur + p3`.

Given the conditions:
- Since `cur` is equal to `low`, we need to determine the value of `low`.
- `low` is defined as `p3 - p1` if `p3 - p1 < p3 - p2` else `p3 - p2`.
- `high` is defined similarly but it doesn't affect `cur` directly.

To find `low`:
- If `p3 - p1 < p3 - p2`, then `low = p3 - p1`.
- Otherwise, `low = p3 - p2`.

Since `cur` is `low`, we substitute `cur` with either `p3 - p1` or `p3 - p2` depending on the condition.

Now, let's consider the expression `p1 - cur + p3`:
- If `p3 - p1 < p3 - p2`, then `cur = p3 - p1`, so the expression becomes `p1 - (p3 - p1) + p3 = p1 - p3 + p1 + p3 = 2 * p1`.
- If `p3 - p1 >= p3 - p2`, then `cur = p3 - p2`, so the expression becomes `p1 - (p3 - p2) + p3 = p1 - p3 + p2 + p3 = p1 + p2`.

Given the condition `(p1 - cur <= p2 - (p3 - cur))`, we can infer that:
- If `cur = p3 - p1`, then `p1 - (p3 - p1) <= p2 - (p3 - (p3 - p1))` simplifies to `2 * p1 - p3 <= p2 + p1 - p3`, which simplifies to `p1 <= p2`. This is consistent with our earlier assumption.
- If `cur = p3 - p2`, then `p1 - (p3 - p2) <= p2 - (p3 - (p3 - p2))` simplifies to `p1 - p3 + p2 <= p2 + p2 - p3`, which simplifies to `p1 <= p2`. This is also consistent with our earlier assumption.

Therefore, the expression `p1 - cur + p3` will evaluate to either `2 * p1` or `p1 + p2`.

Since the exact values of `p1` and `p2` are not specified, we can only express the result in terms of these values.

Output: **2 * p1 or p1 + p2 (depending on the condition between p3 - p1 and p3 - p2)**