Let's break down the problem step by step based on the initial state and the operations performed:

1. **Initial State**:
   - `t > 1`
   - `p1`, `p2`, `p3` are integers obtained from the input split by spaces.
   - The sum of `p1`, `p2`, and `p3` is odd.
   - `low` is updated to the minimum of `p3 - p1` and `p3 - p2`.
   - `high` is updated to the maximum of `p3 - p1` and `p3 - p2`.
   - `cur` is set to either `low` or `high` depending on whether `p1 - cur` is less than or equal to `p2 - (p3 - cur)`.
   - `cur` is increased by 1 if it was set to `high`.
   - `high` must be greater than or equal to `cur - 1`.

2. **Determine the Values of `low` and `high`**:
   - Since `p3 - p1` and `p3 - p2` are being compared to determine `low` and `high`, let's denote:
     - `a = p3 - p1`
     - `b = p3 - p2`
   - Without loss of generality, assume `a <= b` (if `a > b`, the roles of `low` and `high` would simply be swapped).
   - Therefore, `low = a` and `high = b`.

3. **Determine the Value of `cur`**:
   - `cur` is set to `low` or `high` based on the condition `p1 - cur <= p2 - (p3 - cur)`.
   - Let's analyze this condition:
     - If `cur = low = a`, then the condition becomes `p1 - a <= p2 - (p3 - a)`.
     - Simplifying, `p1 - a <= p2 - p3 + a` or `p1 + p3 - a <= p2 + a` or `p1 + p3 <= p2 + 2a`.
     - Similarly, if `cur = high = b`, then the condition becomes `p1 - b <= p2 - (p3 - b)`.
     - Simplifying, `p1 - b <= p2 - p3 + b` or `p1 - b <= p2 - p3 + b` or `p1 + p3 <= p2 + 2b`.
   - Given that `a <= b`, if `p1 + p3 <= p2 + 2a`, then `cur` will be `a` (low). Otherwise, `cur` will be `b` (high).

4. **Determine the Final Value of `cur`**:
   - If `p1 + p3 <= p2 + 2a`, then `cur = a`.
   - If `p1 + p3 > p2 + 2a`, then `cur = b`.
   - After setting `cur`, `cur` is increased by 1 if it was set to `high` (i.e., if `cur = b`), so `cur` becomes `b + 1`.

5. **Calculate the Final Expression**:
   - The expression to evaluate is `p1 - cur + p3`.
   - If `cur = a`, then `p1 - cur + p3 = p1 - a + p3`.
   - If `cur = b + 1`, then `p1 - cur + p3 = p1 - (b + 1) + p3 = p1 - b - 1 + p3`.

Given the above steps, we need to consider both cases:

- **Case 1**: If `cur = a` (i.e., `p1 + p3 <= p2 + 2a`), then the expression evaluates to `p1 - a + p3`.
- **Case 2**: If `cur = b + 1` (i.e., `p1 + p3 > p2 + 2a`), then the expression evaluates to `p1 - b - 1 + p3`.

Since the exact values of `p1`, `p2`, and `p3` are not provided, we cannot determine which case applies without additional information. However, we know that `low` and `high` are derived from `p3 - p1` and `p3 - p2`, and `cur` is determined based on the condition involving these differences.

Output: **p1 - [low or high + 1] + p3** (where `[low or high + 1]` depends on the condition `p1 + p3 <= p2 + 2a` or `p1 + p3 > p2 + 2a`).