Alright, I've got this problem to solve. I need to determine if a given Python program is correct based on the provided problem description. The problem is about counting the number of ordered pairs (a, b) that satisfy certain conditions, and there are multiple test cases to handle.

First, I need to understand the problem clearly. I'm given two positive integers, n and m, and I need to find the number of ordered pairs (a, b) where 1 ≤ a ≤ n and 1 ≤ b ≤ m, such that b * gcd(a, b) is a multiple of a + b.

Okay, so for each test case, I'll get n and m, and I have to count how many pairs (a, b) meet the condition that b * gcd(a, b) is divisible by a + b.

I need to think about how to approach this efficiently, especially since n and m can be up to 2 million, and there can be up to 10,000 test cases, with the sum of n and m across all test cases not exceeding 2 million.

Looking at the example, for n=10 and m=8, there are 6 valid pairs: (2,2), (3,6), (4,4), (6,3), (6,6), and (8,8). I need to see if the given program correctly counts these pairs.

Now, let's look at the provided program. There are two functions: func_1 and func_2. func_2 reads the number of test cases and calls func_1 for each test case. func_1 seems to implement the logic to count the valid pairs.

In func_1, it initializes x to 1 and cnt to 0. Then it reads n and m from input. There's a while loop that runs as long as x * x is less than or equal to n. Inside this loop, there's another while loop for y, which increments from 1 until (x + y) * x is less than or equal to n and (x + y) * y is less than or equal to m.

Within this inner loop, it checks if gcd(x, y) equals 1, and if so, it adds the minimum of n // ((x + y) * x) and m // ((x + y) * y) to cnt.

After the loops, it prints the count.

Hmm, this seems optimized, but I need to verify if this logic correctly counts the pairs that satisfy the given condition.

Let me try to understand the logic behind this implementation.

First, the condition is that b * gcd(a, b) is a multiple of a + b. Let's denote d = gcd(a, b). Then a = d * x and b = d * y, where gcd(x, y) = 1.

Substituting into the condition: b * d = d * y * d = d^2 * y should be a multiple of a + b = d * x + d * y = d (x + y).

So, d^2 * y should be a multiple of d (x + y), which simplifies to d * y being a multiple of x + y.

Since d = gcd(a, b), and a = d * x, b = d * y, with gcd(x, y) = 1.

So, the condition becomes d * y is a multiple of x + y.

But d is gcd(a, b), which is d = gcd(d * x, d * y) = d * gcd(x, y) = d * 1 = d.

Wait, that seems a bit circular. Let me think differently.

Given that a = d * x and b = d * y, with gcd(x, y) = 1, the condition is b * d = d * y * d = d^2 * y is a multiple of a + b = d * x + d * y = d (x + y).

So, d^2 * y is a multiple of d (x + y), which means d * y is a multiple of x + y.

Since gcd(x, y) = 1, x and y are coprime.

Now, I need to find when d * y is a multiple of x + y.

Let me see if I can express d in terms of x and y.

Since a = d * x and b = d * y, and d = gcd(a, b), which is the largest integer dividing both a and b.

Given that, d is determined by a and b, but in terms of x and y, since a = d * x and b = d * y, and x and y are coprime, d is the greatest common divisor of a and b.

Wait, perhaps I need to approach this differently.

Let me consider the condition: b * gcd(a, b) is a multiple of a + b.

Substituting a = d * x and b = d * y, with gcd(x, y) = 1:

Condition becomes: (d * y) * d is a multiple of d * x + d * y, which simplifies to d^2 * y is a multiple of d (x + y), which further simplifies to d * y is a multiple of x + y.

Now, since x and y are coprime, and d is a multiple of x + y divided by y.

Wait, this seems complicated. Maybe I need to find another way.

Let me consider that d * y is a multiple of x + y.

Since x and y are coprime, x + y and y are also coprime, because any common divisor of x + y and y would also divide x, but x and y are coprime.

Wait, is x + y and y coprime?

Let’s see: suppose p divides y and p divides x + y, then p divides x (since p divides y and x + y), but since gcd(x, y) = 1, p must be 1.

Therefore, x + y and y are coprime, meaning that y and x + y are coprime.

Therefore, for d * y to be a multiple of x + y, since x + y and y are coprime, x + y must divide d.

So, x + y divides d.

But d is gcd(a, b) = gcd(d * x, d * y) = d * gcd(x, y) = d.

Wait, that doesn't make sense.

Wait, gcd(d*x, d*y) = d * gcd(x, y) = d * 1 = d.

Yes, d = gcd(a, b).

So, if x + y divides d, then d is a multiple of x + y.

Therefore, d >= x + y.

But d is gcd(a, b), and a = d * x, b = d * y.

Given that a <= n and b <= m, meaning d * x <= n and d * y <= m.

Given that d >= x + y, we can write d * x >= x * (x + y) and d * y >= y * (x + y).

But a <= n and b <= m, so x * (x + y) <= n and y * (x + y) <= m.

Wait, this seems promising.

So, for each pair (x, y) where x and y are coprime, and x * (x + y) <= n and y * (x + y) <= m, there exists d >= x + y, and d * x <= n and d * y <= m.

Wait, but d must be a multiple of x + y, since x + y divides d.

Wait, earlier I concluded that x + y divides d, so d is a multiple of x + y.

Let’s set d = k * (x + y), for some integer k >= 1.

Then, a = d * x = k * (x + y) * x

b = d * y = k * (x + y) * y

Given that a <= n and b <= m, we have:

k * (x + y) * x <= n

and

k * (x + y) * y <= m

Since k is a positive integer, the maximum k for each (x, y) is the minimum of floor(n / ((x + y) * x)) and floor(m / ((x + y) * y)).

Therefore, for each (x, y) pair where x and y are coprime, and x * (x + y) <= n and y * (x + y) <= m, the number of valid d's (or k's) is min(floor(n / ((x + y) * x)), floor(m / ((x + y) * y))).

Hence, the total count is the sum over all such (x, y) pairs of this minimum value.

Looking back at the code, it seems to implement exactly this logic.

It iterates over x starting from 1, while x * x <= n.

Then, for each x, it iterates y from 1, while (x + y) * x <= n and (x + y) * y <= m.

For each (x, y) pair where gcd(x, y) == 1, it adds min(n // ((x + y) * x), m // ((x + y) * y)) to the count.

This matches the logic I just derived.

Now, I need to verify if this implementation is correct and efficient enough given the constraints.

Given that n and m can be up to 2*10^6, and t can be up to 10^4, with the sum of n and m across all test cases not exceeding 2*10^6, the implementation seems acceptable in terms of time complexity.

The double loop over x and y, with y incrementing until (x + y) * x > n or (x + y) * y > m, should be efficient because for larger x, y will be smaller, and vice versa.

Also, since the sum of n and m across all test cases is limited to 2*10^6, the total computational complexity should be manageable.

Looking back at the example, for n=10 and m=8, the valid pairs are (2,2), (3,6), (4,4), (6,3), (6,6), and (8,8), totaling 6 pairs.

I need to see if the code correctly counts these pairs.

Let's map these pairs to (x, y) where a = d * x and b = d * y, with d = x + y.

For (2,2): Let's see, a=2, b=2. Then d = gcd(2,2)=2. So x = a/d=1, y=b/d=1.

Check if 1* (1+1) = 2 <= 10 and 1 * (1+1) = 2 <= 8. Yes.

Then k = d / (x + y) = 2 / (1 + 1) = 1.

So min(10 // (2 * 1), 8 // (2 * 1)) = min(5, 4) = 4.

But in reality, there's only one pair (2,2), but according to this, it seems to count 4, which is not matching.

Wait, perhaps I'm misunderstanding the mapping.

Wait, in the code, x and y are loop variables representing the multipliers.

Wait, maybe I need to think differently.

Let me consider the pair (2,2):

Here, a=2, b=2.

Check if 2 * gcd(2,2) = 2 * 2 = 4 is a multiple of a + b = 4. Yes, 4 is a multiple of 4.

So, (2,2) is a valid pair.

Similarly, (3,6):

a=3, b=6.

gcd(3,6)=3.

b * gcd(a,b) = 6 * 3 = 18.

a + b = 9.

18 is a multiple of 9, so yes.

(4,4):

a=4, b=4.

gcd=4.

4*4=16, a+b=8.

16 is a multiple of 8.

Yes.

(6,3):

a=6, b=3.

gcd=3.

3*3=9, a+b=9.

9 is a multiple of 9.

Yes.

(6,6):

a=6, b=6.

gcd=6.

6*6=36, a+b=12.

36 is a multiple of 12.

Yes.

(8,8):

a=8, b=8.

gcd=8.

8*8=64, a+b=16.

64 is a multiple of 16.

Yes.

So, these are the 6 valid pairs.

Now, in the code, for x=1:

y=1:

(x,y)=(1,1):

a = k*(1+1)*1 = 2k

b = k*(1+1)*1 = 2k

So, a=b=2k.

For k=1: a=2, b=2 -> valid.

k=2: a=4, b=4 -> valid.

k=3: a=6, b=6 -> valid.

k=4: a=8, b=8 -> valid.

So, for (x,y)=(1,1), it adds min(10//2, 8//2)=min(5,4)=4 to cnt.

But in reality, only k=1,2,3,4 correspond to valid pairs (2,2),(4,4),(6,6),(8,8).

So, cnt increases by 4.

Next, x=2:

y=1:

(x,y)=(2,1):

a = k*(2+1)*2 = 6k

b = k*(2+1)*1 = 3k

a <=10, b<=8.

6k <=10 and 3k <=8.

k <=1 (since 6*1=6<=10, 3*1=3<=8)

So, k=1: a=6, b=3 -> valid.

min(10//6, 8//3)=1, so cnt increases by 1.

y=2:

(x,y)=(2,2):

a = k*(2+2)*2 = 8k

b = k*(2+2)*2 = 8k

a <=10, b<=8.

8k <=10 and 8k <=8 => k=1.

a=8, b=8 -> valid.

min(10//8, 8//8)=1, so cnt increases by 1.

y=3:

(x,y)=(2,3):

a = k*(2+3)*2 =10k

b = k*(2+3)*3 =15k

a <=10, b<=8.

10k <=10 and 15k <=8.

k=1: a=10, b=15 -> b>8, invalid.

k=0 is not considered.

So, no addition to cnt.

Thus, total cnt =4+1+1=6, which matches the example.

Therefore, the code seems correct.

I need to confirm if this logic holds for other test cases as well.

Looking back at the code, it seems to correctly implement the logic I derived.

Hence, the program is correct.

**Final Answer**

\[\boxed{\text{True}}\]

