The code snippet modifies the value of `s`. The other variables (`k`, `x`, `a`, and `i`) remain unchanged. The new value of `s` is calculated as `s += s // (k - 1) + 1`.

Given:
- `s` is initially `4 + (3 / (k - 1))`
- `s` is then updated to `s + s // (k - 1) + 1`

Let's denote the initial value of `s` as `s_initial = 4 + (3 / (k - 1))`. After the code execution, the new value of `s` becomes:
- `s_new = s_initial + s_initial // (k - 1) + 1`

Therefore, the final output state is:
Output State: **`k`, `x`, and `a` are integers read from the input with the constraints 2 ≤ k ≤ 30, 1 ≤ x ≤ 100, and 1 ≤ a ≤ 10^9; `s` is `4 + (3 / (k - 1)) + (4 + (3 / (k - 1))) // (k - 1) + 1`; `i` is 3**