Output State: **`t` is an integer such that \(1 \leq t \leq 10^4\), `a` is greater than 5, `i` is 3, `b[3]` remains 0, `b[4]` is equal to `-6`, `b[5]` is equal to `-6**.

Explanation: The code `b[i + 2] -= b[i]` updates the value of `b[i + 2]` by subtracting `b[i]` from it. Given that `i` is 3, `i + 2` equals 5. Since `b[3]` is 0 and `b[4]` is -6, the operation `b[5] -= b[3]` simplifies to `b[5] -= 0`, which does not change the value of `b[5]`. Therefore, `b[5]` remains -6. All other variables retain their initial conditions.