To determine the new value of `cnt`, we need to evaluate the expression `min(n // ((x + y) * x), m // ((x + y) * y))`.

Given:
- `x` is 2
- `y` is 1
- `n` is at least 6
- `m` is at least 3

First, compute `(x + y) * x`:
\[ (x + y) * x = (2 + 1) * 2 = 3 * 2 = 6 \]

Next, compute `n // ((x + y) * x)`:
Since `n` is at least 6, let's consider the minimum possible value for `n` which is 6.
\[ n // 6 = 6 // 6 = 1 \]

Then, compute `(x + y) * y`:
\[ (x + y) * y = (2 + 1) * 1 = 3 * 1 = 3 \]

Next, compute `m // ((x + y) * y)`:
Since `m` is at least 3, let's consider the minimum possible value for `m` which is 3.
\[ m // 3 = 3 // 3 = 1 \]

Now, compute `min(n // ((x + y) * x), m // ((x + y) * y))`:
\[ \text{min}(1, 1) = 1 \]

Finally, update `cnt`:
\[ cnt += 1 \]
\[ cnt = 5 + 1 = 6 \]

The values of `x`, `y`, `n`, `m`, and the greatest common divisor condition remain unchanged.

Output State: **`x` is 2, `y` is 1, `cnt` is 6, `n` is at least 6, `m` is at least 3, and the greatest common divisor of `x` and `y` is 1.**