The code snippet `a[r] -= a[l]` reduces the value of `a[r]` by the value of `a[l]`. Given the initial state, the values of `n`, `k`, `a`, `l`, and `r` remain unchanged except for `a[r]`.

Output State: **`n` is an integer such that 1 <= n <= 2 * 10^5, `k` is an integer such that 1 <= k <= 10^15 and `k` has been decreased by `a[l] * 2`, `a` is a list of `n` integers where each integer `a_i` is such that 1 <= `a_i` <= 10^9, the sum of `n` across all test cases does not exceed 2 * 10^5; `l` and `r` are integers, and `a[l]` is less than or equal to `a[r]`. Additionally, `k` is greater than or equal to `a[l] * 2`; `a[r]` is now `a[r] - a[l]`.**