Let's break down the initial state and the expression to be printed step by step:

1. **Initial Values:**
   - `i = 7`
   - `n > 8` (we don't know the exact value of `n`, but we know it is greater than 8)
   - `k = 0`
   - `r = a[7]` (assuming `a` is a list and `a[7]` refers to the 8th element of the list if the list is zero-indexed)
   - `rem = 0`
   - `y = n - 3` (since `n > 8`, `y` will be greater than 5)
   - `ii = 0`
   - `k = 0` (repeated, but we already know this from the initial state)

2. **Expression to Evaluate:**
   \[
   (r - 1) \times n + 1 + rem + y
   \]

3. **Substitute Known Values:**
   - `r = a[7]`
   - `rem = 0`
   - `y = n - 3`

   So the expression becomes:
   \[
   (a[7] - 1) \times n + 1 + 0 + (n - 3)
   \]
   Simplifying further:
   \[
   (a[7] - 1) \times n + n - 2
   \]
   \[
   (a[7] - 1 + 1) \times n - 2
   \]
   \[
   a[7] \times n - 2
   \]

4. **Final Expression:**
   The expression simplifies to \(a[7] \times n - 2\).

Given the initial state, the exact value of `a[7]` and `n` are not specified, but we can describe the output in terms of these variables.

Output: **a[7] * n - 2**