The code snippet `y2 -= a` updates the value of `y2` by subtracting `a` from its current value. Given the initial state, let's break down the impact:

- `a` is defined as `y1 - 1`, and since `y1` is 1, `a` is `1 - 1 = 0`.
- `y2` is initially equal to `y_b`.

Since `a` is 0, subtracting `a` from `y2` does not change the value of `y2`. Therefore, `y2` remains equal to `y_b`.

The rest of the variables and conditions remain unchanged.

Output State: **`t` is the absolute difference between `y2` and `y1`, and `t` is a positive integer such that 1 <= t <= 10^4. `r` is a list of six integers [h, w, x_a, y_a, x_b, y_b] where 1 <= x_a, x_b <= h <= 10^6, 1 <= y_a, y_b <= w <= 10^9, and either x_a != x_b or y_a != y_b. `n` is equal to `h`, `m` is equal to `w`, `x1` is equal to `x_a + a` (where `a` is `y1 - 1` because `y2 >= y1`), `y1` is 1, `x2` is equal to `x_b - a`, and `y2` is equal to `y_b`. Additionally, `x2` is greater than `x1`. The difference between `x2` and `x1` is even. `y1` is not equal to `y2`. `b` is equal to `x2 - x1`. `x2` is greater than `x1`, `x1` is greater than or equal to 1, and `x2` is less than or equal to `n`. The current value of `y1` is 1.**