Let's analyze the given if condition:

The if condition is:
```
if ((a - b == -a, a) or (b - a == -b, b)):
```

This condition seems to have a syntax error because the tuple `(a - b == -a, a)` and `(b - a == -b, b)` are not valid expressions for an `if` statement. It appears that the intention might have been to check two separate conditions using logical OR. Let's assume the intended condition was:

```
if (a - b == -a) or (b - a == -b):
```

Now, let's simplify these conditions:
- `a - b == -a` simplifies to `2a == b`
- `b - a == -b` simplifies to `2b == a`

So the if condition essentially checks if either `a` is twice `b` or `b` is twice `a`.

Given this understanding, we can now formulate the postcondition.

Precondition: `t` is an integer such that 1 ≤ t ≤ 10^4; `a` and `b` are integers read from the input. At least one of `a` or `b` is odd.

Postcondition: **`t` is an integer such that 1 ≤ t ≤ 10^4; `a` and `b` are integers read from the input, at least one of `a` or `b` is odd, and either `a` is twice `b` or `b` is twice `a`.**

This postcondition includes all the information from the precondition and incorporates the logic of the if condition.