To determine the postcondition, we need to ensure that the if condition is false while retaining all the information provided in the precondition. 

The if condition is:
```python
if ((a - b == -a, a) or (b - a == -b, b)):
```

This condition seems to contain a tuple comparison which might be a mistake since tuples are compared lexicographically. However, assuming the intention was to check if either `(a - b == -a)` or `(b - a == -b)`, we'll negate this condition for the postcondition.

Let's break down the if condition:
- `(a - b == -a)` simplifies to `2a == b`
- `(b - a == -b)` simplifies to `2b == a`

So the if condition is checking if either `2a == b` or `2b == a`. The negation of this condition would be that neither `2a == b` nor `2b == a`.

Given the precondition:
- `t` is an integer such that \(1 \leq t \leq 10^4\)
- `a` and `b` are integers read from the input
- At least one of `a` or `b` is odd

The postcondition must include all these details and also specify that neither `2a == b` nor `2b == a`.

Postcondition: **`t` is an integer such that \(1 \leq t \leq 10^4\); `a` and `b` are integers read from the input; at least one of `a` or `b` is odd; neither `2a == b` nor `2b == a`**