Alright, I've got this problem to solve. It's about a game between Alice and Bob where they have some coins in their wallets and they take turns making moves according to certain rules. The goal is to determine who will win if both play optimally.

First, I need to understand the problem completely. Alice and Bob start with a certain number of coins in their wallets, let's say a and b respectively. They take turns, with Alice going first. In each turn, the player can choose to either exchange wallets with the opponent or keep their current wallet, and then remove one coin from their current wallet. Importantly, the wallet cannot have zero coins before removing one coin.

The player who cannot make a valid move loses. So, if a player is in a situation where their wallet has zero coins and they can't swap to a non-zero wallet, they lose.

I need to determine, for given values of a and b, who will win the game if both play optimally.

Let me think about the game mechanics. Each move consists of two steps: choosing to swap wallets or not, and then removing one coin from the current wallet. The swap is optional, but it might be strategically useful in certain situations.

I should consider the game as a sequence of states, where each state is defined by the number of coins in Alice's and Bob's wallets. Since the game is turn-based and deterministic, I can model it as a impartial game, similar to Nim or other impartial games where the rules are the same for both players.

However, in this game, the players have asymmetric roles because Alice moves first. So, I need to account for that in my analysis.

Let me consider some small values of a and b to see if I can find a pattern or a general rule.

**Example 1:**

a = 1, b = 1

- Alice's turn:

- Option 1: Swap wallets. Now a=1, b=1. Remove 1 coin from her wallet. Now a=0, b=1.

- Option 2: Keep wallet. Remove 1 coin. Now a=0, b=1.

- In both cases, after Alice's move, a=0 and b=1.

- Bob's turn:

- Bob has a wallet with 1 coin and Alice has 0.

- Option 1: Swap wallets. Now a=1, b=0. Remove 1 coin. Now a=0, b=0.

- Option 2: Keep wallet. Remove 1 coin. Now a=0, b=0.

- In both cases, after Bob's move, a=0 and b=0.

- Alice's turn:

- Both wallets are empty. Alice cannot make a move. So, Bob wins.

This matches the first test case in the example.

**Example 2:**

a = 1, b = 4

- Alice's turn:

- Option 1: Swap wallets. Now a=4, b=1. Remove 1 coin. Now a=3, b=1.

- Option 2: Keep wallet. Remove 1 coin. Now a=0, b=4.

- Let's say Alice chooses to swap and have a=4, b=1, then a=3, b=1.

- Bob's turn:

- Now a=3, b=1.

- Option 1: Swap wallets. Now a=1, b=3. Remove 1 coin. Now a=0, b=3.

- Option 2: Keep wallet. Remove 1 coin. Now a=2, b=1.

- Suppose Bob chooses to swap and have a=0, b=3.

- Alice's turn:

- Now a=0, b=3.

- Option 1: Swap wallets. Now a=3, b=0. Remove 1 coin. Now a=2, b=0.

- Option 2: Keep wallet. Remove 1 coin. Now a=0, b=2.

- If Alice swaps, a=2, b=0.

- Bob's turn:

- Now a=2, b=0.

- Option 1: Swap wallets. Now a=0, b=2. Remove 1 coin. Now a=0, b=1.

- Option 2: Keep wallet. Remove 1 coin. Now a=1, b=0.

- Suppose Bob chooses to swap, a=0, b=1.

- Alice's turn:

- Now a=0, b=1.

- Option 1: Swap wallets. Now a=1, b=0. Remove 1 coin. Now a=0, b=0.

- Option 2: Keep wallet. Remove 1 coin. Now a=0, b=0.

- In both cases, after Alice's move, a=0, b=0.

- Bob's turn:

- Both wallets are empty. Bob cannot make a move. So, Alice wins.

This matches the second test case in the example.

From these examples, it seems that the winner depends on the parity of the sum of a and b.

Wait, in the first example, a + b = 2, which is even, and Bob wins.

In the second example, a + b = 5, which is odd, and Alice wins.

Let me check another example.

**Example 3:**

a = 2, b = 2

- Alice's turn:

- Option 1: Swap wallets. Now a=2, b=2. Remove 1 coin. Now a=1, b=2.

- Option 2: Keep wallet. Remove 1 coin. Now a=1, b=2.

- In both cases, a=1, b=2.

- Bob's turn:

- Now a=1, b=2.

- Option 1: Swap wallets. Now a=2, b=1. Remove 1 coin. Now a=1, b=1.

- Option 2: Keep wallet. Remove 1 coin. Now a=0, b=2.

- Suppose Bob chooses to swap, a=1, b=1.

- Alice's turn:

- Now a=1, b=1.

- Option 1: Swap wallets. Now a=1, b=1. Remove 1 coin. Now a=0, b=1.

- Option 2: Keep wallet. Remove 1 coin. Now a=0, b=1.

- In both cases, a=0, b=1.

- Bob's turn:

- Now a=0, b=1.

- Option 1: Swap wallets. Now a=1, b=0. Remove 1 coin. Now a=0, b=0.

- Option 2: Keep wallet. Remove 1 coin. Now a=0, b=0.

- In both cases, a=0, b=0.

- Alice's turn:

- Both wallets are empty. Alice cannot make a move. So, Bob wins.

Here, a + b = 4, which is even, and Bob wins.

Another example:

**Example 4:**

a = 2, b = 3

- Alice's turn:

- Option 1: Swap wallets. Now a=3, b=2. Remove 1 coin. Now a=2, b=2.

- Option 2: Keep wallet. Remove 1 coin. Now a=1, b=3.

- Suppose Alice chooses to swap, a=3, b=2, then remove 1 coin, a=2, b=2.

- Bob's turn:

- Now a=2, b=2.

- Option 1: Swap wallets. Now a=2, b=2. Remove 1 coin. Now a=1, b=2.

- Option 2: Keep wallet. Remove 1 coin. Now a=1, b=2.

- In both cases, a=1, b=2.

- Alice's turn:

- Now a=1, b=2.

- Option 1: Swap wallets. Now a=2, b=1. Remove 1 coin. Now a=1, b=1.

- Option 2: Keep wallet. Remove 1 coin. Now a=0, b=2.

- Suppose Alice chooses to swap, a=1, b=1.

- Bob's turn:

- Now a=1, b=1.

- Option 1: Swap wallets. Now a=1, b=1. Remove 1 coin. Now a=0, b=1.

- Option 2: Keep wallet. Remove 1 coin. Now a=0, b=1.

- In both cases, a=0, b=1.

- Alice's turn:

- Now a=0, b=1.

- Option 1: Swap wallets. Now a=1, b=0. Remove 1 coin. Now a=0, b=0.

- Option 2: Keep wallet. Remove 1 coin. Now a=0, b=0.

- In both cases, a=0, b=0.

- Bob's turn:

- Both wallets are empty. Bob cannot make a move. So, Alice wins.

Here, a + b = 5, which is odd, and Alice wins.

It seems that when a + b is even, Bob wins, and when a + b is odd, Alice wins.

Let me check another example to confirm.

**Example 5:**

a = 3, b = 3

- Alice's turn:

- Option 1: Swap wallets. Now a=3, b=3. Remove 1 coin. Now a=2, b=3.

- Option 2: Keep wallet. Remove 1 coin. Now a=2, b=3.

- In both cases, a=2, b=3.

- Bob's turn:

- Now a=2, b=3.

- Option 1: Swap wallets. Now a=3, b=2. Remove 1 coin. Now a=2, b=2.

- Option 2: Keep wallet. Remove 1 coin. Now a=1, b=3.

- Suppose Bob chooses to swap, a=2, b=2.

- Alice's turn:

- Now a=2, b=2.

- Option 1: Swap wallets. Now a=2, b=2. Remove 1 coin. Now a=1, b=2.

- Option 2: Keep wallet. Remove 1 coin. Now a=1, b=2.

- In both cases, a=1, b=2.

- Bob's turn:

- Now a=1, b=2.

- Option 1: Swap wallets. Now a=2, b=1. Remove 1 coin. Now a=1, b=1.

- Option 2: Keep wallet. Remove 1 coin. Now a=0, b=2.

- Suppose Bob chooses to swap, a=1, b=1.

- Alice's turn:

- Now a=1, b=1.

- Option 1: Swap wallets. Now a=1, b=1. Remove 1 coin. Now a=0, b=1.

- Option 2: Keep wallet. Remove 1 coin. Now a=0, b=1.

- In both cases, a=0, b=1.

- Bob's turn:

- Now a=0, b=1.

- Option 1: Swap wallets. Now a=1, b=0. Remove 1 coin. Now a=0, b=0.

- Option 2: Keep wallet. Remove 1 coin. Now a=0, b=0.

- In both cases, a=0, b=0.

- Alice's turn:

- Both wallets are empty. Alice cannot make a move. So, Bob wins.

Here, a + b = 6, which is even, and Bob wins.

This seems consistent with the earlier observations.

Let me consider a case where a + b is odd.

**Example 6:**

a = 2, b = 1

- Alice's turn:

- Option 1: Swap wallets. Now a=1, b=2. Remove 1 coin. Now a=0, b=2.

- Option 2: Keep wallet. Remove 1 coin. Now a=1, b=1.

- Suppose Alice chooses to swap, a=1, b=2, then remove 1 coin, a=0, b=2.

- Bob's turn:

- Now a=0, b=2.

- Option 1: Swap wallets. Now a=2, b=0. Remove 1 coin. Now a=1, b=0.

- Option 2: Keep wallet. Remove 1 coin. Now a=0, b=1.

- Suppose Bob chooses to swap, a=1, b=0.

- Alice's turn:

- Now a=1, b=0.

- Option 1: Swap wallets. Now a=0, b=1. Remove 1 coin. Now a=0, b=0.

- Option 2: Keep wallet. Remove 1 coin. Now a=0, b=0.

- In both cases, a=0, b=0.

- Bob's turn:

- Both wallets are empty. Bob cannot make a move. So, Alice wins.

Here, a + b = 3, which is odd, and Alice wins.

This further confirms the pattern.

It seems that the sum of a and b determines the winner:

- If a + b is even, Bob wins.

- If a + b is odd, Alice wins.

This seems too straightforward. Is there any scenario where this doesn't hold?

Let me think about larger numbers.

**Example 7:**

a = 5, b = 3

- a + b = 8, which is even. According to the pattern, Bob should win.

Let's simulate:

- Alice's turn:

- Option 1: Swap wallets. a=3, b=5. Remove 1 coin. a=2, b=5.

- Option 2: Keep wallet. Remove 1 coin. a=4, b=3.

- Suppose Alice chooses to swap, a=3, b=5, then remove 1 coin, a=2, b=5.

- Bob's turn:

- Now a=2, b=5.

- Option 1: Swap wallets. a=5, b=2. Remove 1 coin. a=4, b=2.

- Option 2: Keep wallet. Remove 1 coin. a=1, b=5.

- Suppose Bob chooses to swap, a=4, b=2.

- Alice's turn:

- Now a=4, b=2.

- Option 1: Swap wallets. a=2, b=4. Remove 1 coin. a=1, b=4.

- Option 2: Keep wallet. Remove 1 coin. a=3, b=2.

- Suppose Alice chooses to swap, a=1, b=4.

- Bob's turn:

- Now a=1, b=4.

- Option 1: Swap wallets. a=4, b=1. Remove 1 coin. a=3, b=1.

- Option 2: Keep wallet. Remove 1 coin. a=0, b=4.

- Suppose Bob chooses to swap, a=3, b=1.

- Alice's turn:

- Now a=3, b=1.

- Option 1: Swap wallets. a=1, b=3. Remove 1 coin. a=0, b=3.

- Option 2: Keep wallet. Remove 1 coin. a=2, b=1.

- Suppose Alice chooses to swap, a=0, b=3.

- Bob's turn:

- Now a=0, b=3.

- Option 1: Swap wallets. a=3, b=0. Remove 1 coin. a=2, b=0.

- Option 2: Keep wallet. Remove 1 coin. a=0, b=2.

- Suppose Bob chooses to swap, a=2, b=0.

- Alice's turn:

- Now a=2, b=0.

- Option 1: Swap wallets. a=0, b=2. Remove 1 coin. a=0, b=1.

- Option 2: Keep wallet. Remove 1 coin. a=1, b=0.

- Suppose Alice chooses to swap, a=0, b=1.

- Bob's turn:

- Now a=0, b=1.

- Option 1: Swap wallets. a=1, b=0. Remove 1 coin. a=0, b=0.

- Option 2: Keep wallet. Remove 1 coin. a=0, b=0.

- In both cases, a=0, b=0.

- Alice's turn:

- Both wallets are empty. Alice cannot make a move. So, Bob wins.

This matches the pattern.

Another example:

**Example 8:**

a = 11, b = 9

- a + b = 20, which is even. According to the pattern, Bob should win.

Let's see:

- Alice's turn:

- Option 1: Swap wallets. a=9, b=11. Remove 1 coin. a=8, b=11.

- Option 2: Keep wallet. Remove 1 coin. a=10, b=9.

- Suppose Alice chooses to swap, a=9, b=11, then remove 1 coin, a=8, b=11.

- Bob's turn:

- Now a=8, b=11.

- Option 1: Swap wallets. a=11, b=8. Remove 1 coin. a=10, b=8.

- Option 2: Keep wallet. Remove 1 coin. a=7, b=11.

- Suppose Bob chooses to swap, a=10, b=8.

- Alice's turn:

- Now a=10, b=8.

- Option 1: Swap wallets. a=8, b=10. Remove 1 coin. a=7, b=10.

- Option 2: Keep wallet. Remove 1 coin. a=9, b=8.

- Suppose Alice chooses to swap, a=7, b=10.

- Bob's turn:

- Now a=7, b=10.

- Option 1: Swap wallets. a=10, b=7. Remove 1 coin. a=9, b=7.

- Option 2: Keep wallet. Remove 1 coin. a=6, b=10.

- Suppose Bob chooses to swap, a=9, b=7.

- Alice's turn:

- Now a=9, b=7.

- Option 1: Swap wallets. a=7, b=9. Remove 1 coin. a=6, b=9.

- Option 2: Keep wallet. Remove 1 coin. a=8, b=7.

- Suppose Alice chooses to swap, a=6, b=9.

- Bob's turn:

- Now a=6, b=9.

- Option 1: Swap wallets. a=9, b=6. Remove 1 coin. a=8, b=6.

- Option 2: Keep wallet. Remove 1 coin. a=5, b=9.

- Suppose Bob chooses to swap, a=8, b=6.

- Alice's turn:

- Now a=8, b=6.

- Option 1: Swap wallets. a=6, b=8. Remove 1 coin. a=5, b=8.

- Option 2: Keep wallet. Remove 1 coin. a=7, b=6.

- Suppose Alice chooses to swap, a=5, b=8.

- Bob's turn:

- Now a=5, b=8.

- Option 1: Swap wallets. a=8, b=5. Remove 1 coin. a=7, b=5.

- Option 2: Keep wallet. Remove 1 coin. a=4, b=8.

- Suppose Bob chooses to swap, a=7, b=5.

- Alice's turn:

- Now a=7, b=5.

- Option 1: Swap wallets. a=5, b=7. Remove 1 coin. a=4, b=7.

- Option 2: Keep wallet. Remove 1 coin. a=6, b=5.

- Suppose Alice chooses to swap, a=4, b=7.

- Bob's turn:

- Now a=4, b=7.

- Option 1: Swap wallets. a=7, b=4. Remove 1 coin. a=6, b=4.

- Option 2: Keep wallet. Remove 1 coin. a=3, b=7.

- Suppose Bob chooses to swap, a=6, b=4.

- Alice's turn:

- Now a=6, b=4.

- Option 1: Swap wallets. a=4, b=6. Remove 1 coin. a=3, b=6.

- Option 2: Keep wallet. Remove 1 coin. a=5, b=4.

- Suppose Alice chooses to swap, a=3, b=6.

- Bob's turn:

- Now a=3, b=6.

- Option 1: Swap wallets. a=6, b=3. Remove 1 coin. a=5, b=3.

- Option 2: Keep wallet. Remove 1 coin. a=2, b=6.

- Suppose Bob chooses to swap, a=5, b=3.

- Alice's turn:

- Now a=5, b=3.

- Option 1: Swap wallets. a=3, b=5. Remove 1 coin. a=2, b=5.

- Option 2: Keep wallet. Remove 1 coin. a=4, b=3.

- Suppose Alice chooses to swap, a=2, b=5.

- Bob's turn:

- Now a=2, b=5.

- Option 1: Swap wallets. a=5, b=2. Remove 1 coin. a=4, b=2.

- Option 2: Keep wallet. Remove 1 coin. a=1, b=5.

- Suppose Bob chooses to swap, a=4, b=2.

- Alice's turn:

- Now a=4, b=2.

- Option 1: Swap wallets. a=2, b=4. Remove 1 coin. a=1, b=4.

- Option 2: Keep wallet. Remove 1 coin. a=3, b=2.

- Suppose Alice chooses to swap, a=1, b=4.

- Bob's turn:

- Now a=1, b=4.

- Option 1: Swap wallets. a=4, b=1. Remove 1 coin. a=3, b=1.

- Option 2: Keep wallet. Remove 1 coin. a=0, b=4.

- Suppose Bob chooses to swap, a=3, b=1.

- Alice's turn:

- Now a=3, b=1.

- Option 1: Swap wallets. a=1, b=3. Remove 1 coin. a=0, b=3.

- Option 2: Keep wallet. Remove 1 coin. a=2, b=1.

- Suppose Alice chooses to swap, a=0, b=3.

- Bob's turn:

- Now a=0, b=3.

- Option 1: Swap wallets. a=3, b=0. Remove 1 coin. a=2, b=0.

- Option 2: Keep wallet. Remove 1 coin. a=0, b=2.

- Suppose Bob chooses to swap, a=2, b=0.

- Alice's turn:

- Now a=2, b=0.

- Option 1: Swap wallets. a=0, b=2. Remove 1 coin. a=0, b=1.

- Option 2: Keep wallet. Remove 1 coin. a=1, b=0.

- Suppose Alice chooses to swap, a=0, b=1.

- Bob's turn:

- Now a=0, b=1.

- Option 1: Swap wallets. a=1, b=0. Remove 1 coin. a=0, b=0.

- Option 2: Keep wallet. Remove 1 coin. a=0, b=0.

- In both cases, a=0, b=0.

- Alice's turn:

- Both wallets are empty. Alice cannot make a move. So, Bob wins.

Again, this matches the pattern.

Let me consider a case where a + b is odd.

**Example 9:**

a = 83, b = 91

- a + b = 174, which is even. According to the pattern, Bob should win.

But according to the sample output, for a=83, b=91, the output is "Bob", which matches the pattern.

Wait, but according to my earlier observation, when a + b is even, Bob wins, and when it's odd, Alice wins.

But in the sample input, for a=1, b=4 (sum=5, odd), Alice wins, and for a=83, b=91 (sum=174, even), Bob wins, which matches.

Another sample input: a=1000000000, b=1000000000 (sum=2000000000, even), Bob wins.

Wait, but in the sample output, for a=1000000000, b=1000000000, the output is "Bob", which matches the pattern.

So, all the sample inputs seem to confirm that if a + b is even, Bob wins, else Alice wins.

Is there any scenario where this doesn't hold?

Let me think about a=1, b=1 (sum=2, even), Bob wins.

a=1, b=4 (sum=5, odd), Alice wins.

a=5, b=3 (sum=8, even), Bob wins.

a=4, b=5 (sum=9, odd), Alice wins.

a=11, b=9 (sum=20, even), Bob wins.

a=83, b=91 (sum=174, even), Bob wins.

a=1032, b=9307 (sum=10339, odd), Alice wins.

a=839204, b=7281 (sum=846485, odd), Alice wins.

a=1000000000, b=1000000000 (sum=2000000000, even), Bob wins.

a=53110, b=2024 (sum=55134, even), Bob wins.

All these match the pattern.

I think the game can be modeled as a Nim game with one heap where the number of coins is (a + b). The player who takes the last coin wins.

Wait, but in this game, players are reducing the total number of coins by one each turn, and they have the option to swap wallets, which effectively just swaps a and b.

Since swapping doesn't change the sum, the sum remains invariant under swaps.

Therefore, the total number of moves possible is equal to the initial sum of a and b.

Since Alice moves first, if the total number of moves is even, Bob will make the last move and win. If it's odd, Alice will make the last move and win.

Wait, but in the earlier examples, when a + b is even, Bob wins, and when it's odd, Alice wins.

This seems consistent with the above reasoning.

Let me formalize this.

Let s = a + b.

Since each move reduces the total by one, there will be s moves in total.

If s is even, Bob makes the last move and wins.

If s is odd, Alice makes the last move and wins.

Hence, the winner can be determined solely by the parity of a + b.

This seems to be a correct conclusion.

Therefore, the given program is correct.

In the program:

def func():

t = int(input())

for i in range(t):

s = input()

a = int(list(s.split())[0])

b = int(list(s.split())[1])

if (a + b) % 2 == 0:

print('Bob')

else:

print('Alice')

It correctly calculates the sum of a and b and determines the winner based on the parity of the sum.

Hence, the program is correct.

**Final Answer**

\[ \boxed{\text{The program is correct.}} \]

**Correctness: True**