Initial State: `n` and `m` are positive integers such that 1 ≤ n, m ≤ 2 · 10^6, `x` is 1, `y` is 3, `cnt` is updated to `min(n // 2, m // 2) + min(n // 3, m // 6)` if the GCD of `x` and `y` is 1, otherwise `cnt` remains 0.

Given the initial state, let's analyze the provided code snippet:

```python
cnt += min(n // ((x + y) * x), m // ((x + y) * y))
```

### Step-by-Step Analysis:

1. **Initial Values:**
   - `x` = 1
   - `y` = 3
   - `cnt` is updated based on the GCD condition. Since the GCD of 1 and 3 is 1, `cnt` is set to:
     \[
     \text{cnt} = \min\left(\frac{n}{2}, \frac{m}{2}\right) + \min\left(\frac{n}{3}, \frac{m}{6}\right)
     \]

2. **Expression Evaluation:**
   - Calculate `(x + y) * x`:
     \[
     (x + y) * x = (1 + 3) * 1 = 4
     \]
   - Calculate `(x + y) * y`:
     \[
     (x + y) * y = (1 + 3) * 3 = 12
     \]
   - Evaluate `min(n // 4, m // 12)`:
     \[
     \text{min}(n // 4, m // 12)
     \]

3. **Update `cnt`:**
   - Add the result of `min(n // 4, m // 12)` to `cnt`:
     \[
     \text{cnt} += \min\left(\frac{n}{4}, \frac{m}{12}\right)
     \]

### Final Output State:

- `n` and `m` remain positive integers such that 1 ≤ n, m ≤ 2 · 10^6.
- `x` remains 1.
- `y` remains 3.
- `cnt` is updated to:
  \[
  \text{cnt} = \min\left(\frac{n}{2}, \frac{m}{2}\right) + \min\left(\frac{n}{3}, \frac{m}{6}\right) + \min\left(\frac{n}{4}, \frac{m}{12}\right)
  \]

Output State: **`n` and `m` are positive integers such that 1 ≤ n, m ≤ 2 · 10^6, `x` is 1, `y` is 3, `cnt` is now `min(n // 2, m // 2) + min(n // 3, m // 6) + min(n // 4, m // 12)`**.