In the given initial state, we have:

- `n` is an input integer such that `1 ≤ n ≤ 100`.
- `a` is a list of `n` integers where each integer `a[i]` satisfies `-100 ≤ a[i] ≤ 100`.
- `B` is the sum of all positive integers in `a`.
- `C` is the sum of all negative integers in `a`.

The code snippet calculates:

```
result = B - C
```

Now, let's analyze the impact of this code.

1. `result` is assigned the value of `B - C`, which means `result` becomes the value of the sum of all positive integers in `a` minus the sum of all negative integers in `a`.
2. The values of `B` and `C` remain unchanged after this assignment; only `result` is modified based on their values.

Therefore, the output state will reflect the unchanged values of `n`, `a`, `B`, and `C`, along with the new value of `result`.

Output State: **`n` is an input integer such that 1 ≤ `n` ≤ 100; `a` is a list of `n` integers where each integer `a[i]` satisfies -100 ≤ `a[i]` ≤ 100; `B` is the sum of all positive integers in `a`; `C` is the sum of all negative integers in `a`; `result` is equal to `B - C`.**