Let's break down the initial state and the code snippet to determine what will be printed:

### Initial State:
- `_` is 1 (This variable is not used in the code snippet).
- `t` is an integer such that 1 ≤ t ≤ 10^4 (This variable is not used in the code snippet).
- `n` is an input integer.
- `ar` is a list of integers with at least 1 element.
- `res` is a list of `n` elements where each element at index `i` is `mex - ar[i]` starting from the last element to the first.
- `mex` is the result of subtracting all elements of `ar` from `n` (i.e., `n - sum(ar)`).
- `i` is -1 (This variable is not used in the code snippet).

### Code Snippet:
```python
print(' '.join(str(x) for x in res))
```

### Step-by-Step Analysis:
1. **Calculate `mex`:**
   - `mex` is defined as `n - sum(ar)`.
   - This means `mex` is the difference between `n` and the sum of all elements in the list `ar`.

2. **Construct `res`:**
   - `res` is a list of `n` elements.
   - Each element at index `i` in `res` is calculated as `mex - ar[i]`, but the elements are added to `res` starting from the last element of `ar` to the first.
   - Therefore, the first element of `res` will be `mex - ar[-1]`, the second element will be `mex - ar[-2]`, and so on.

3. **Print `res`:**
   - The `print` statement converts each element of `res` to a string and joins them with a space.
   - The output will be a space-separated string of the elements in `res`.

### Example Calculation:
Let's assume:
- `n = 10`
- `ar = [1, 2, 3, 4]`

1. **Calculate `mex`:**
   - `sum(ar) = 1 + 2 + 3 + 4 = 10`
   - `mex = n - sum(ar) = 10 - 10 = 0`

2. **Construct `res`:**
   - `res[0] = mex - ar[-1] = 0 - 4 = -4`
   - `res[1] = mex - ar[-2] = 0 - 3 = -3`
   - `res[2] = mex - ar[-3] = 0 - 2 = -2`
   - `res[3] = mex - ar[-4] = 0 - 1 = -1`
   - Therefore, `res = [-4, -3, -2, -1]`

3. **Print `res`:**
   - The output will be: `-4 -3 -2 -1`

### General Output:
Given the initial state and the code snippet, the output will be a space-separated string of the elements in `res`, where each element is calculated as `mex - ar[i]` starting from the last element of `ar` to the first.

Output: **' '.join(str(mex - ar[i]) for i in range(len(ar)-1, -1, -1)) (where mex is n - sum(ar) and ar is the list of integers)**

In simpler terms:
Output: **space-separated list of (mex - ar[i]) for each i from len(ar)-1 to 0**