Alright, I've got this problem to solve. Let's see what it's asking for. So, I'm given two positive integers, n and m, and I need to find the number of ordered pairs (a, b) where 1 ≤ a ≤ n and 1 ≤ b ≤ m, with the condition that a + b is a multiple of b multiplied by the greatest common divisor of a and b. That is, a + b should be divisible by b * gcd(a, b).

First, I need to understand what this condition means. Let's break it down. GCD of a and b is the greatest common divisor of a and b, which I'll denote as gcd(a, b). So, b * gcd(a, b) should divide a + b.

Let me try to rephrase this. If b * gcd(a, b) divides a + b, then there exists some integer k such that a + b = k * b * gcd(a, b).

Hmm, that seems a bit complicated. Maybe I can simplify this condition.

Let me consider the properties of gcd. I know that gcd(a, b) divides both a and b. So, let's denote d = gcd(a, b). Then, a = d * a1 and b = d * b1, where gcd(a1, b1) = 1.

Substituting these into the condition:

a + b = d * a1 + d * b1 = d * (a1 + b1)

And b * gcd(a, b) = d * b1 * d = d^2 * b1

So, the condition becomes that d * (a1 + b1) is divisible by d^2 * b1.

Simplifying, this means that a1 + b1 is divisible by d * b1.

But since a1 and b1 are coprime (gcd(a1, b1) = 1), and d = gcd(a, b), I need to see how these relate.

Wait a minute, since a = d * a1 and b = d * b1, and a1 and b1 are coprime, then gcd(a, b) = d, which matches our earlier definition.

So, the condition is that a1 + b1 is divisible by d * b1.

But a1 and b1 are coprime, so a1 + b1 being divisible by b1 would imply that a1 is divisible by b1, but since gcd(a1, b1) = 1, unless b1 = 1, this isn't possible.

Wait, that seems off. Let's think differently.

Maybe I should consider the ratio a/b. Since a = d * a1 and b = d * b1, then a/b = a1 / b1.

But I'm not sure if that helps directly.

Let me try plugging in some small values to see if I can find a pattern.

Take n = 1, m = 1. Then the only pair is (1,1). So, a + b = 2, and b * gcd(a,b) = 1 * 1 = 1. Since 2 is divisible by 1, this works. So, answer is 1.

Next, n = 2, m = 3.

Possible pairs:

(1,1): 1+1=2, 1*1=1, 2 is divisible by 1 → valid

(1,2): 1+2=3, 2*1=2, 3 is not divisible by 2 → invalid

(1,3): 1+3=4, 3*1=3, 4 is not divisible by 3 → invalid

(2,1): 2+1=3, 1*1=1, 3 is divisible by 1 → valid

(2,2): 2+2=4, 2*2=4, 4 is divisible by 4 → valid

(2,3): 2+3=5, 3*1=3, 5 is not divisible by 3 → invalid

So, valid pairs are (1,1), (2,1), (2,2) → total 3.

This matches the example.

Another example: n=3, m=5.

Possible pairs:

(1,1): valid

(1,2): invalid

(1,3): invalid

(1,4): invalid

(1,5): invalid

(2,1): valid

(2,2): valid

(2,3): invalid

(2,4): invalid

(2,5): invalid

(3,1): valid

(3,2): invalid

(3,3): 3+3=6, 3*3=9, 6 is not divisible by 9 → invalid

(3,4): invalid

(3,5): invalid

So, valid pairs are (1,1), (2,1), (2,2), (3,1) → total 4.

Again, matches the example.

Now, looking at the pattern, it seems that for each b, there are certain a's that satisfy the condition.

But checking each pair individually is not efficient, especially since n and m can be up to 2*10^6, and t can be up to 10^4.

So, I need a smarter way to compute the number of valid pairs without iterating through each pair.

Let me try to find a mathematical formula or a way to count the valid pairs efficiently.

Going back to the condition: a + b is divisible by b * gcd(a,b).

Expressed differently: b * gcd(a,b) divides a + b.

Let d = gcd(a,b), then a = d * a1, b = d * b1, with gcd(a1, b1) = 1.

Substituting, a + b = d * a1 + d * b1 = d * (a1 + b1)

And b * gcd(a,b) = d * b1 * d = d^2 * b1

So, d^2 * b1 divides d * (a1 + b1), which simplifies to d * b1 divides a1 + b1.

But a1 and b1 are coprime, so a1 + b1 and b1 are coprime except for the common factor of b1.

Wait, no. a1 and b1 are coprime, but a1 + b1 and b1 may have common factors.

Actually, gcd(a1 + b1, b1) = gcd(a1, b1) = 1, since a1 and b1 are coprime.

So, a1 + b1 and b1 are coprime.

Therefore, d * b1 divides a1 + b1, and since b1 divides a1 + b1, and a1 + b1 and b1 are coprime, this implies that b1 = 1.

Wait, that can't be right. If b1 divides a1 + b1, and gcd(a1 + b1, b1) = 1, then b1 must be 1.

So, b1 = 1.

Which means that b = d * b1 = d * 1 = d.

So, b = d = gcd(a,b).

Therefore, b divides a, because gcd(a,b) divides a.

Wait, if b divides a, then a is a multiple of b.

So, a = k * b for some integer k.

But since b = d, and a = d * a1, then a1 = k.

But a1 and b1 are coprime, and b1 = 1, so a1 can be any positive integer.

Wait, this seems to suggest that a is a multiple of b.

Wait, but in the earlier examples, for n=2, m=3:

Valid pairs: (1,1), (2,1), (2,2)

In these:

- (1,1): 1 divides 1

- (2,1): 1 divides 2

- (2,2): 2 divides 2

So, in all valid pairs, b divides a.

Is this always the case?

Looking back, yes, because b divides a.

Wait, but in the condition, b * gcd(a,b) divides a + b.

If b divides a, then a = k * b for some integer k.

So, a + b = k * b + b = (k + 1) * b

And b * gcd(a,b) = b * gcd(k * b, b) = b * b, since gcd(k * b, b) = b.

So, b^2 divides (k + 1) * b.

Simplifying, b divides (k + 1).

Since a = k * b and a ≤ n, k ≤ n / b.

Also, b ≤ m.

So, for each b, k can be from 1 to floor(n / b), such that b divides (k + 1).

Wait, that seems manageable.

So, for each b from 1 to m:

For each k from 1 to floor(n / b):

a = k * b

Condition: b divides (k + 1)

Which means k ≡ -1 mod b

Or, k ≡ (b - 1) mod b

So, for each b, the number of k's satisfying k ≡ (b - 1) mod b, and 1 ≤ k ≤ floor(n / b)

This seems like an arithmetic sequence.

Let me see.

k ≡ (b - 1) mod b

So, k = b * t + (b - 1), for some integer t ≥ 0

We need 1 ≤ k ≤ floor(n / b)

So, 1 ≤ b * t + (b - 1) ≤ floor(n / b)

Let me solve for t:

1 ≤ b * t + (b - 1) ⇒ t ≥ ceil((1 - (b - 1)) / b) = ceil((1 - b + 1)/b) = ceil((2 - b)/b)

But 2 - b ≤ 1 for b ≥ 1, so ceil((2 - b)/b) = 0 for b ≥ 1

And b * t + (b - 1) ≤ floor(n / b)

⇒ t ≤ floor( (floor(n / b) - (b - 1)) / b )

So, t can be from 0 to floor( (floor(n / b) - (b - 1)) / b )

Let me see an example.

Take n=2, m=3

For b=1:

k ≡ 0 mod 1, which is always true.

So, k can be from 1 to floor(2 / 1) = 2

So, k=1,2 → a=1*1=1, a=2*1=2 → pairs (1,1), (2,1)

For b=2:

k ≡ 1 mod 2

So, k=1,3,5,...

But floor(n / 2) = 1

So, k=1 → a=2*1=2 → pair (2,2)

k=3 is >1, so invalid

For b=3:

k ≡ 2 mod 3

k=2,5,8,...

floor(n / 3)=0, since 2/3 <1

So, no valid k

Total pairs: (1,1),(2,1),(2,2) → 3, which matches the example.

Another example: n=3, m=5

b=1:

k ≡ 0 mod 1, always true

k from 1 to floor(3/1)=3 → k=1,2,3 → a=1,2,3 → pairs (1,1),(2,1),(3,1)

b=2:

k ≡1 mod 2

k from 1 to floor(3/2)=1

k=1 → a=2*1=2 → pair (2,2)

k=3 >1, invalid

b=3:

k ≡2 mod 3

k from 1 to floor(3/3)=1

k=2 >1, invalid

b=4:

k ≡3 mod 4

k from 1 to floor(3/4)=0

no k

b=5:

k ≡4 mod 5

k from 1 to floor(3/5)=0

no k

Total pairs: (1,1),(2,1),(3,1),(2,2) → 4, matches the example.

So, this seems correct.

Now, to compute this efficiently, especially since t can be up to 10^4 and n and m up to 2*10^6, with sum of n and m over all test cases up to 2*10^6.

So, per test case, time should be roughly O(m), but with optimizations.

I need to find, for each b from 1 to m, the number of k's satisfying k ≡ (b - 1) mod b, and 1 ≤ k ≤ floor(n / b)

This is equivalent to finding the number of integers k in [1, floor(n/b)] such that k ≡ (b - 1) mod b

This is an arithmetic sequence with first term a1 = (b - 1), difference d = b

So, the number of terms is floor( (floor(n/b) - (b - 1)) / b ) + 1, if (b - 1) ≤ floor(n/b), else 0

Wait, in the earlier example with n=2, m=3, b=1:

floor(n / b)=2, (b -1)=0

So, floor( (2 - 0)/1 ) +1 = 3, which is correct.

For b=2:

floor(n / b)=1, (b -1)=1

floor( (1 -1)/2 ) +1 = floor(0/2) +1 = 0 +1 =1, which is correct.

For b=3:

floor(n / b)=0, (b -1)=2

floor( (0 -2)/3 ) +1 = floor(-2/3) +1 = (-1) +1 =0, which is correct.

Another example: n=3, m=5

b=1: floor(3/1)=3, (1-1)=0

floor( (3 -0)/1 ) +1 =3 +1=4, but in reality, k=1,2,3 →3. Wait, seems off.

Wait, maybe it's floor( (floor(n/b) - (b -1)) / b ) +1

So, floor( (3 -0)/1 ) +1 =3 +1=4, but in reality, k=1,2,3 →3.

Wait, that seems one extra.

Wait, perhaps it's floor( (floor(n/b) - (b -1)) / b ) +1, but only if floor(n/b) >= (b -1), else 0.

In this case, floor(n/b)=3 >=0, so 3.

Wait, floor( (3 -0)/1 ) +1=3 +1=4, but k can be 1,2,3, which are all valid, since b=1 divides (k+1) for k=1,2,3.

Wait, maybe it's correct.

For b=1, k can be 1,2,3, which are all valid.

Wait, but in the earlier calculation, for b=1, floor( (floor(n/b)-(b-1)) / b ) +1 = floor( (3-0)/1 ) +1 =3 +1=4, but there are only k=1,2,3.

Wait, perhaps I need to adjust the formula.

Wait, perhaps it's floor( (floor(n/b) - (b -1)) / b ) +1, but ensuring that (b -1) <= floor(n/b)

In this case, b=1, floor(n/b)=3 >=0, so 3 -0 /1 +1=4, but only 3 k's are valid.

Wait, perhaps the correct formula is floor( (floor(n/b) - (b -1)) / b ) +1, but clipped to be at most floor(n/b)

In this case, for b=1, floor(n/b)=3, so min(floor( (3-0)/1 ) +1, floor(n/b)) = min(4,3)=3, which is correct.

Wait, but in previous example, for b=2, floor(n/b)=1, (b-1)=1

floor( (1-1)/2 ) +1=0 +1=1, which is correct.

For b=3, floor(n/b)=0, (b-1)=2

floor( (0-2)/3 ) +1= floor(-2/3) +1= (-1) +1=0, which is correct.

So, the general formula is:

For each b from 1 to m:

Compute floor(n / b)

Let upper = floor(n / b)

If upper < (b -1), then no k's satisfy.

Else, the number of k's is floor( (upper - (b -1)) / b ) +1

Wait, but in the b=1 case, this gave me 4, but only 3 k's are valid.

Wait, perhaps I need to ensure that k >=1.

Wait, perhaps the formula should be floor( (upper - (b -1)) / b ) +1, but only if upper >= (b -1), else 0.

In the b=1 case, upper=3 >=0, so floor( (3-0)/1 ) +1=3 +1=4, but k can be 0,1,2,3.

Wait, but k should be >=1, so k=1,2,3 are valid, but k=0 is invalid because a=k*b=0*1=0, which is not >=1.

So, in this case, I need to adjust the formula to count only k >=1.

Similarly, in b=2, floor(n/b)=1 >=1, floor( (1-1)/2 ) +1=0 +1=1, which is k=1.

In b=3, floor(n/b)=0 <2, so 0.

So, perhaps the formula is floor( (floor(n/b) - (b -1)) / b ) +1, but adjusted to be >=1.

Wait, perhaps it's ceiling( (floor(n/b) - (b -1)) / b ) +1, but I need to think carefully.

Alternatively, perhaps it's floor( (floor(n/b) - (b -1) + b -1) / b ), which simplifies to floor( (floor(n/b) + b -1 - (b -1)) / b )=floor( floor(n/b) / b ), but that seems off.

Wait, maybe I need to use the standard formula for the number of terms in an arithmetic sequence.

The number of k's such that k ≡ (b -1) mod b, and 1 <= k <= floor(n/b)

This is equivalent to k = (b -1) + t * b, for t >=0, and k <= floor(n/b)

So, (b -1) + t * b <= floor(n/b)

Thus, t <= (floor(n/b) - (b -1)) / b

So, t <= floor( (floor(n/b) - (b -1)) / b )

Therefore, t can be from 0 to floor( (floor(n/b) - (b -1)) / b )

Hence, the number of k's is floor( (floor(n/b) - (b -1)) / b ) +1, provided that floor(n/b) >= (b -1), else 0.

In the b=1 case, floor(n/b)=3 >=0, so floor( (3 -0)/1 ) +1=3 +1=4, but k=0 is invalid, so I need to adjust the lower bound.

Wait, perhaps I need to ensure that k >=1, so t >= ceil( (1 - (b -1)) / b )

Let me calculate t >= ceil( (1 - (b -1)) / b )=ceil( (1 -b +1)/b )=ceil( (2 -b)/b )

For b >=1, (2 -b)/b <=1/b <=1, so ceil((2 -b)/b)=1 for b=1, and 0 for b>1.

Wait, no.

For b=1: (2 -1)/1=1/1=1 → ceil(1)=1

For b=2: (2 -2)/2=0/2=0 → ceil(0)=0

For b=3: (2 -3)/3=-1/3 → ceil(-1/3)=0

So, for b=1, t >=1, for b>=2, t >=0.

Wait, but in b=1, t >=0, since k=0 is possible, but k=0 is invalid because a=0 is not allowed.

Wait, perhaps I need to set t >= ceil( (1 - (b -1)) / b )

For b=1: ceil( (1 -0)/1 )=1

For b=2: ceil( (1 -1)/2 )=ceil(0/2)=0

For b=3: ceil( (1 -2)/3 )=ceil(-1/3)=0

So, for b=1, t starts from 1 (k=1), for b>=2, t starts from 0.

Wait, but in b=1, t=0 gives k=0, which is invalid, so t starts from 1.

For b>=2, t starts from 0.

Hence, the number of k's is floor( (floor(n/b) - (b -1)) / b ) - ceil( (1 - (b -1)) / b ) +1

Wait, that might be complicated.

Alternatively, perhaps it's easier to compute the number of k's satisfying k ≡ (b -1) mod b, and 1 <= k <= floor(n/b), directly.

Given that, for b=1, k can be any integer from 1 to floor(n/b), since b=1 divides all k.

For b>=2, k can be from ceil((1 - (b -1))/b) to floor( (floor(n/b) - (b -1)) / b )

But this seems messy.

Maybe I can precompute for each b, the number of k's satisfying the condition.

Alternatively, perhaps there's a better way to count this.

Let me consider that a = k * b, and k ≡ (b -1) mod b.

Wait, but k ≡ (b -1) mod b is the same as k ≡ -1 mod b.

So, k = t * b -1, for some integer t >=1.

Wait, but k must be >=1, so t >= ceil( (1 +1)/b )= ceil(2/b), which is 1 for b>=1.

Wait, for t=1, k=b*1 -1=b -1

For t=2, k=2b -1, and so on, up to k <= floor(n/b)

So, the number of t's such that k = t * b -1 <= floor(n / b)

Which implies t * b -1 <= floor(n / b)

So, t <= (floor(n / b) +1) / b

Hence, t <= floor( (floor(n / b) +1) / b )

Therefore, the number of t's is floor( (floor(n / b) +1) / b )

Wait, let's test this with n=2, m=3

For b=1:

floor(n / b)=2

floor( (2 +1)/1 )=3

So, t=1,2,3 → k=1*1 -1=0, 2*1 -1=1, 3*1 -1=2

But k=0 is invalid, but k=1 and k=2 are valid.

So, number of valid k's is 2, but the formula gives floor( (2 +1)/1 )=3, which is overcounting.

Wait, perhaps I need to adjust for k >=1.

Wait, in this case, t starts from 1, and k=t*b -1

So, for t=1, k=b -1

For t=2, k=2b -1, etc.

So, k >= b -1

But k must also be >=1.

So, if b -1 >=1, i.e., b >=2, then k >=1.

For b=1, b -1=0, which is invalid, so we need to handle b=1 separately.

For b=1:

k can be any integer from 1 to floor(n / 1)=n, since b=1 divides a for any a.

So, number of k's is floor(n /1)=n.

For b >=2:

Number of t's such that k = t * b -1 <= floor(n / b)

Which is t <= floor( (floor(n / b) +1)/b )

So, number of k's is floor( (floor(n / b) +1)/b )

Wait, in the example n=2, m=3:

For b=1: n=2, m=3

Number of k's: n=2

For b=2:

floor(n / b)=1

floor( (1 +1)/2 )=floor(2/2)=1

Which corresponds to k=1*2 -1=1, which is valid.

For b=3:

floor(n / b)=0

floor( (0 +1)/3 )=floor(1/3)=0

No k's, which is correct.

Total: 2 (from b=1) +1 (from b=2) +0=3, which matches.

Another example: n=3, m=5

b=1: n=3 →3 k's:1,2,3

b=2: floor(3/2)=1 → floor( (1+1)/2 )=floor(2/2)=1 → k=1*2 -1=1, which is valid.

b=3: floor(3/3)=1 → floor( (1+1)/3 )=floor(2/3)=0 → no k's.

b=4: floor(3/4)=0 → floor( (0+1)/4 )=floor(1/4)=0 → no k's.

b=5: floor(3/5)=0 → floor( (0+1)/5 )=floor(1/5)=0 → no k's.

Total:3+1+0+0+0=4, which matches.

Another example: n=10, m=8

From the note, valid pairs are:

(1,1), (2,1), (2,2), (3,1), (4,1), (5,1), (6,1), (6,2), (6,3), (7,1), (8,1), (9,1), (10,1), (10,2)

Total 14, which matches the example.

Let me compute using the formula.

For b=1: floor(n /1)=10 →10 k's:1 through10

For b=2: floor(10 /2)=5 → floor( (5 +1)/2 )=floor(6/2)=3 → t=1,2,3 → k=1*2 -1=1, 2*2 -1=3, 3*2 -1=5 → a=2,6,10 → pairs (2,2), (6,2), (10,2)

Wait, but in the note, only (2,2), (6,2), (10,2) are listed.

But according to this, k=1,3,5 are valid, corresponding to a=2,6,10.

But in the note, only (2,2), (6,2), (10,2) are listed, but actually for b=2, k=1,3,5 are valid, but a=2,6,10 are <=n=10.

Wait, but in the note, only (2,2), (6,2), (10,2) are listed, which corresponds to a=2,6,10.

So, seems correct.

Total for b=1:10 pairs (a,1) for a=1 to10

For b=2:3 pairs: (2,2), (6,2), (10,2)

For b=3: floor(10/3)=3 → floor( (3+1)/3 )=floor(4/3)=1 → t=1 → k=2 → a=6 → pair (6,3)

But in the note, only (6,3) is not listed, but according to the condition, b=3, k=2, a=6, which should be valid.

Wait, but in the note, only (1,1),(2,1),(2,2),(3,1),(4,1),(5,1),(6,1),(6,2),(6,3),(7,1),(8,1),(9,1),(10,1),(10,2)

So, it seems (6,3) is included, but perhaps it was missed in the note.

Or maybe I miscounted.

Anyway, moving on.

So, the total number of pairs is sum over b from 1 to m of the number of k's satisfying the condition.

For b=1: n

For b>=2: floor( (floor(n / b) +1)/b )

Wait, but in the earlier calculation for b=3 in n=10,m=8, I got one pair (6,3), which is correct.

So, the formula seems to hold.

Now, to implement this efficiently, I need to iterate over b from 1 to m, and for each b, compute floor(n / b), then compute floor( (floor(n / b) +1)/b ) if b >=2, and add n for b=1.

But since t can be up to 10^4 and n and m up to 2*10^6, with sum of n and m over all test cases up to 2*10^6, I need an efficient way to compute this.

One way is to iterate over b from 1 to m, and for each b, compute floor(n / b), then compute floor( (floor(n / b) +1)/b )

But this would be O(m) per test case, which with t=10^4 and m=2*10^6, would be too slow.

So, I need a better way.

Let me consider the values of floor(n / b). These are known as the harmonic parts or something similar in number theory.

I recall that the number of unique values of floor(n / b) for b from 1 to m is around 2 * sqrt(n), which is much smaller than m.

So, perhaps I can iterate over the ranges where floor(n / b) is constant.

Wait, but in this problem, for each b, I need to compute floor(n / b), which can be grouped by the value of floor(n / b).

But in this case, since for each b, I need to compute floor(n / b) and then floor( (floor(n / b) +1)/b ), it's a bit more involved.

Wait, perhaps I can find a way to group the b's by the value of floor(n / b), and compute the sum in blocks.

Let me think differently.

Let me denote q = floor(n / b)

Then, for a fixed q, find the range of b's where floor(n / b) = q.

This is standard in divisor sum computations.

Specifically, for q from 1 to n, find the minimum b_min where floor(n / b) <= q, and maximum b_max where floor(n / b) >= q.

Wait, more precisely, for q = floor(n / b), we have q <= n / b < q +1

Which implies floor(n / q) >= b > floor(n / (q +1))

So, for each q, the b's where floor(n / b) = q are from ceil(n / (q +1)) to floor(n / q)

But in this problem, I need to compute for each b from 1 to m, floor(n / b), then floor( (floor(n / b) +1)/b )

So, perhaps I can iterate over q from 1 to n, and for each q, compute the range of b's where floor(n / b) = q, and then compute the sum over those b's of floor( (q +1)/b )

But this seems complicated.

Alternatively, perhaps I can iterate over b in blocks where floor(n / b) is constant.

Let me try to implement the standard divisor sum optimization.

I'll write a function to iterate over the blocks where floor(n / b) is constant.

Here's how it works:

- Initialize sum =0

- For b from 1 to m:

- q = floor(n / b)

- Find the maximum b where floor(n / b) = q, which is floor(n / q)

- But more precisely, the upper limit is floor(n / q)

- So, for this q, add q to the sum, multiplied by the number of b's in this range.

Wait, but in this problem, for each b, the term is floor( (q +1)/b ), where q = floor(n / b)

So, it's not a standard divisor sum.

This seems tricky.

Maybe I need to find a different approach.

Let me consider that for b from 1 to m, and for each b, add floor( (floor(n / b) +1)/b )

This is similar to adding floor(n / (b * k)) for some k, but I'm not sure.

Alternatively, perhaps I can consider a change of variables.

Let me set k = t * b -1, as before.

Then, a = k * b = (t * b -1) * b = t * b^2 - b

But I'm not sure if that helps.

Wait, perhaps I can consider that a + b = k * b * gcd(a,b) = k * b * b = k * b^2

Wait, earlier I set a + b = k * b * gcd(a,b), but with a = d * a1, b = d * b1, and d = b, since b = gcd(a,b), as derived earlier.

Wait, earlier I concluded that b = gcd(a,b), and a is a multiple of b.

So, a = m * b for some integer m >=1

Then, a + b = m * b + b = (m +1) * b

And b * gcd(a,b) = b * b = b^2

So, b^2 divides (m +1) * b ⇒ b divides (m +1)

So, m ≡ -1 mod b

But m = a / b, which is integer since a is multiple of b.

Wait, but a = m * b, so m = a / b

Wait, perhaps I need to use different variables.

Let me set m = a / b, since a is multiple of b.

Then, m = a / b, and a + b = m * b + b = (m +1) * b

And b * gcd(a,b) = b * b = b^2

So, b^2 divides (m +1) * b ⇒ b divides (m +1)

So, m ≡ -1 mod b

Which means m = t * b -1 for some integer t >=1

Then, a = m * b = (t * b -1) * b = t * b^2 - b

And since a <=n, we have t * b^2 - b <=n ⇒ t <= floor( (n +b)/b^2 )

So, for each b, t can be from1 to floor( (n +b)/b^2 )

Therefore, the number of valid a's for each b is floor( (n +b)/b^2 )

Wait, is that correct?

Let me check with n=2, m=3

For b=1:

floor( (2 +1)/1 )=3 → a=1,2,3*1 -1=0,1,2 → but a must be >=1, so a=1,2 →2 pairs

For b=2:

floor( (2 +2)/4 )=floor(4/4)=1 → a=2*1 -1=1*2=2 → pair (2,2)

For b=3:

floor( (2 +3)/9 )=floor(5/9)=0 → no a's

Total:2+1+0=3, matches the example.

Another example: n=3, m=5

b=1: floor( (3 +1)/1 )=4 → a=1,2,3 →3 pairs

b=2: floor( (3 +2)/4 )=floor(5/4)=1 → a=2*1 -1=1*2=2 → pair (2,2)

b=3: floor( (3 +3)/9 )=floor(6/9)=0 → no a's

b=4: floor( (3 +4)/16 )=floor(7/16)=0 → no a's

b=5: floor( (3 +5)/25 )=floor(8/25)=0 → no a's

Total:3+1+0+0+0=4, matches the example.

Another example: n=10, m=8

b=1: floor( (10 +1)/1 )=11 → a=1,2,3,4,5,6,7,8,9,10 →10 pairs

b=2: floor( (10 +2)/4 )=floor(12/4)=3 → a=2*1 -1=1*2=2, a=2*2 -1=3*2=6, a=2*3 -1=5*2=10 → pairs (2,2), (6,2), (10,2)

b=3: floor( (10 +3)/9 )=floor(13/9)=1 → a=3*1 -1=2*3=6 → pair (6,3)

b=4: floor( (10 +4)/16 )=floor(14/16)=0 → no a's

b=5: floor( (10 +5)/25 )=floor(15/25)=0 → no a's

b=6: floor( (10 +6)/36 )=floor(16/36)=0 → no a's

b=7: floor( (10 +7)/49 )=floor(17/49)=0 → no a's

b=8: floor( (10 +8)/64 )=floor(18/64)=0 → no a's

Total:10 +3 +1 +0 +0 +0 +0 +0=14, matches the example.

So, the number of valid a's for each b is floor( (n +b)/b^2 )

Therefore, the total number of valid pairs is sum over b from1 to m of floor( (n +b)/b^2 )

For b=1, this is floor( (n +1)/1 )=n +1, but in reality, a can be from1 to n, so n values.

Wait, in the earlier calculation for b=1, floor( (n +1)/1 )=n +1, but a must be >=1 and <=n, so it's n.

So, perhaps for b>=1, the number of a's is floor( (n +b)/b^2 ), but for b=1, it's n.

Wait, perhaps it's min(n, floor( (n +b)/b^2 ) * b)

Wait, for b=1, floor( (n +1)/1 )=n +1, but a can be from1 to n, so min(n, floor( (n +1)/1 ) *1 )=n

Wait, perhaps it's floor( (n +b)/b^2 ) * b, but clipped to <=n.

Wait, in the b=1 case, floor( (n +1)/1 )=n +1, and b=1, so (n +1)*1=n +1, but a can be up to n, so min(n, n +1)=n.

Similarly, for b=2, floor( (n +2)/4 ), and b=2, so floor( (n +2)/4 ) *2

In the n=2, m=3 case:

b=1: min(2, 3*1)=2

b=2: floor( (2 +2)/4 )=1 →1*2=2, but a=2 is <=n=2, so 1 pair

b=3: floor( (2 +3)/9 )=0 →0*3=0, no a's

Total:2+1+0=3

Wait, but earlier, for b=2, floor( (2 +2)/4 )=1, and b=2, so number of a's=1*2=2, but in reality, only a=2 is valid, since a=2*1 -1=1*2=2.

Wait, seems like it's not directly floor( (n +b)/b^2 ) * b.

Wait, perhaps it's floor( (n +b)/b^2 )

In the n=2, m=3 case:

b=1: floor( (2 +1)/1 )=3, but only 2 a's are valid.

Wait, perhaps it's min(floor( (n +b)/b^2 ), floor(n / b))

For b=1: min(floor( (2 +1)/1 ), floor(2 /1 ))=min(3,2)=2

b=2: min(floor( (2 +2)/4 ), floor(2 /2 ))=min(1,1)=1

b=3: min(floor( (2 +3)/9 ), floor(2 /3 ))=min(0,0)=0

Total:2+1+0=3, which matches.

Another example: n=3, m=5

b=1: min(floor( (3 +1)/1 ), floor(3 /1 ))=min(4,3)=3

b=2: min(floor( (3 +2)/