Alright, I've got this problem to solve. Let's see what it's about. So, Polycarp has a string made up of lowercase Latin letters, and he encodes it using a specific algorithm. The encoding process involves creating an auxiliary string 'r' which consists of all the distinct letters from the original string 's', sorted in alphabetical order. Then, each character in 's' is replaced by its symmetric counterpart from 'r'. For example, the first character of 'r' is replaced by the last character of 'r', the second by the second last, and so on.

Given the encoded string, I need to write a program that decodes it back to the original string 's'. The input consists of multiple test cases, each containing the length of the encoded string and the encoded string itself. The output should be the decoded string for each test case.

First, I need to understand the encoding process thoroughly to reverse it correctly. Let's take the example provided:

Original string: "codeforces"

Auxiliary string 'r': "cdefors"

Encoding replacements:

- 'c' -> 's'

- 'o' -> 'e'

- 'd' -> 'r'

- 'e' -> 'o'

- 'f' -> 'f'

- 'o' -> 'e'

- 'r' -> 'd'

- 'c' -> 's'

- 'e' -> 'o'

- 's' -> 'c'

So, the encoded string is "serofedsoc".

Now, to decode "serofedsoc" back to "codeforces", I need to reverse this process. Given the encoded string and the auxiliary string 'r', I can create a mapping from each character in 'r' to its symmetric counterpart in 'r'. Then, for each character in the encoded string, I can replace it with its corresponding character in the original string based on this mapping.

Wait, but in the decoding process, I don't have the original string 's' or the auxiliary string 'r'. I only have the encoded string. How do I reconstruct 'r' from the encoded string?

Well, the problem states that the encoded string is obtained by replacing each character in 's' with its symmetric counterpart from 'r'. Since 'r' is constructed by taking all distinct characters from 's' and sorting them, I can reconstruct 'r' from the encoded string because the encoded string is essentially a permutation of 's', and thus contains the same distinct characters.

So, for the encoded string, I can extract the distinct characters, sort them to get 'r', and then create the symmetric mapping to decode each character.

Let me try this with the example:

Encoded string: "serofedsoc"

Distinct characters: 'c', 'd', 'e', 'f', 'o', 'r', 's'

Sorted 'r': "cdefors"

Now, the symmetric mapping would be:

'c' -> 's'

'd' -> 'r'

'e' -> 'o'

'f' -> 'f'

'o' -> 'e'

'r' -> 'd'

's' -> 'c'

So, to decode, I need a mapping from 's' to 'c', 'e' to 'o', 'r' to 'd', etc., which is the reverse of the encoding mapping.

Wait, no. Actually, since the encoding is replacing each character in 's' with its symmetric counterpart in 'r', the decoding should be replacing each character in the encoded string with its symmetric counterpart in 'r' to get back to 's'.

Wait, maybe I need to think about it differently.

Let me consider that 'r' is a sorted list of unique characters from 's'. The encoding process replaces each character in 's' with its symmetric counterpart in 'r'. So, to decode, I need to replace each character in the encoded string with its symmetric counterpart in 'r'.

Wait, but in the example, if I have 's' corresponding to 'c', 'e' to 'o', 'r' to 'd', etc., then to decode 's' back to 'c', 'e' back to 'o', etc., I need the same mapping as the encoding process.

Wait, no. In the encoding process, each character is replaced by its symmetric counterpart in 'r'. So, in decoding, I need to replace each character in the encoded string with its symmetric counterpart in 'r' to get back to the original character in 's'.

Wait, maybe I need to confirm this with the example.

Given 's' = "codeforces", 'r' = "cdefors"

Encoding mapping:

'c' -> 's'

'o' -> 'e'

'd' -> 'r'

'e' -> 'o'

'f' -> 'f'

'o' -> 'e'

'r' -> 'd'

'c' -> 's'

'e' -> 'o'

's' -> 'c'

So, encoded string is "serofedsoc"

Now, to decode "serofedsoc" back to "codeforces", I need to apply the same mapping again because:

's' -> 'c'

'e' -> 'o'

'r' -> 'd'

'o' -> 'e'

'f' -> 'f'

'e' -> 'o'

'd' -> 'r'

's' -> 'c'

'o' -> 'o'

'c' -> 's'

Wait, that gives "codedefors", which is not the original "codeforces". Hmm, that's not matching.

Wait, maybe I misunderstood the mapping.

Let me think again.

Given 'r' = "cdefors"

The symmetric mapping would pair:

'c' with 's'

'd' with 'r'

'e' with 'o'

'f' with 'f'

'o' with 'e'

'r' with 'd'

's' with 'c'

So, encoding replaces each character in 's' with its pair in this mapping.

To decode, I need to apply the same mapping again because applying the mapping twice should bring me back to the original character.

Wait, in the example, applying the mapping to "serofedsoc" gives "codedefors", which is not "codeforces". So, perhaps this approach is incorrect.

Wait, maybe I need to create a mapping from encoded characters back to original characters.

Given that 'r' is the same for both encoding and decoding, perhaps I need to create a mapping from the symmetric counterpart to the original character.

Wait, perhaps I need to invert the mapping.

In the encoding mapping, 'c' is replaced by 's', so in decoding, 's' should be replaced by 'c'.

Similarly, 'o' is replaced by 'e', so in decoding, 'e' should be replaced by 'o'.

So, the decoding mapping is the inverse of the encoding mapping.

Therefore, to decode, I need to create a mapping where each character in 'r' is mapped to its original counterpart in 'r'.

Given 'r' = "cdefors"

Mapping for encoding:

'c' -> 's'

'd' -> 'r'

'e' -> 'o'

'f' -> 'f'

'o' -> 'e'

'r' -> 'd'

's' -> 'c'

So, decoding mapping:

's' -> 'c'

'e' -> 'o'

'r' -> 'd'

'o' -> 'e'

'f' -> 'f'

'd' -> 'r'

'c' -> 's'

Yes, that makes sense.

So, to decode, I need to create this decoding mapping and apply it to each character in the encoded string.

Now, in the program provided, it seems to be doing something similar.

Looking at the code:

- It reads all input at once using sys.stdin.read() and splits it into a list called data.

- It then parses the number of test cases t from data[index] and increments index.

- For each test case, it reads n (length of encoded string) and the encoded string b from data[index] and increments index accordingly.

- It calls func_1(b) for each test case and collects the results.

- Finally, it prints all the decoded strings joined by newline.

Now, func_1(encoded) is defined as follows:

- It constructs 'r' by sorting the unique characters in the encoded string.

- It creates a mapping where each character in 'r' is mapped to its symmetric counterpart in 'r'.

- It then decodes the encoded string by replacing each character with its corresponding character in the mapping.

Wait a minute, in the earlier analysis, I thought that to decode, I need to map each character in the encoded string to its original counterpart based on the symmetric mapping.

But in the code, it's creating a mapping where r[i] is mapped to r[-(i+1)], which is exactly the symmetric mapping.

Then, it applies this mapping to each character in the encoded string to get the decoded string.

Wait, but in my earlier example, this seemed to not work correctly, as applying the same mapping twice did not return to the original string.

Wait, perhaps I made a mistake in applying the mapping.

Let me try again with the example.

Given encoded string: "serofedsoc"

'r' = "cdefors"

Decoding mapping:

's' -> 'c'

'e' -> 'o'

'r' -> 'd'

'f' -> 'f'

'o' -> 'e'

'd' -> 'r'

'c' -> 's'

Applying this mapping to "serofedsoc":

- 's' -> 'c'

- 'e' -> 'o'

- 'r' -> 'd'

- 'o' -> 'e'

- 'f' -> 'f'

- 'e' -> 'o'

- 'd' -> 'r'

- 's' -> 'c'

- 'o' -> 'e'

- 'c' -> 's'

So, the decoded string would be "codedefors", but the original string was "codeforces". This doesn't match.

Hmm, there's a discrepancy here. Maybe the mapping is not correctly applied or there's a misunderstanding in the process.

Let me re-examine the encoding process.

Given original string 's' = "codeforces"

'r' = "cdefors"

Encoding mapping:

'c' -> 's'

'o' -> 'e'

'd' -> 'r'

'e' -> 'o'

'f' -> 'f'

'o' -> 'e'

'r' -> 'd'

'c' -> 's'

'e' -> 'o'

's' -> 'c'

So, encoded string is "serofedsoc"

Now, to decode "serofedsoc" back to "codeforces", I need to map each character in "serofedsoc" to its original character in 's'.

Given that 'r' is "cdefors", the decoding mapping should be:

's' -> 'c'

'e' -> 'o'

'r' -> 'd'

'f' -> 'f'

'o' -> 'e'

'd' -> 'r'

'c' -> 's'

Applying this to "serofedsoc":

- 's' -> 'c'

- 'e' -> 'o'

- 'r' -> 'd'

- 'o' -> 'e'

- 'f' -> 'f'

- 'e' -> 'o'

- 'd' -> 'r'

- 's' -> 'c'

- 'o' -> 'e'

- 'c' -> 's'

So, the decoded string is "codedefors", but the original was "codeforces". This doesn't match.

Wait, there must be a mistake here. Maybe the mapping is incorrect.

Wait, perhaps I need to consider that the mapping is a bijection, and applying it twice should return to the original if it's an involution.

In this case, applying the mapping twice:

- 'c' -> 's' -> 'c'

- 'o' -> 'e' -> 'o'

- 'd' -> 'r' -> 'd'

- 'e' -> 'o' -> 'e'

- 'f' -> 'f' -> 'f'

- 'r' -> 'd' -> 'r'

- 's' -> 'c' -> 's'

So, it seems that applying the mapping twice returns to the original character, which suggests that the encoding and decoding mappings are the same.

But in the example, applying the mapping to "serofedsoc" gives "codedefors", which is not "codeforces". So, perhaps there's a mistake in assuming that 'r' is the same for encoding and decoding.

Wait, in encoding, 'r' is constructed from the original string 's', but in decoding, I reconstruct 'r' from the encoded string. Since the encoded string is a permutation of 's' with some replacements, its distinct characters should be the same as 's', so 'r' should be the same in both encoding and decoding.

Given that, the mapping should be the same in both encoding and decoding, and applying it twice should return to the original.

But in the example, it's not working as expected. Maybe I made a mistake in constructing 'r' or the mapping.

Let me check the sorted unique characters of "serofedsoc":

Distinct characters: 'c', 'd', 'e', 'f', 'o', 'r', 's'

Sorted 'r': "cdefors"

Mapping:

'c' -> 's'

'd' -> 'r'

'e' -> 'o'

'f' -> 'f'

'o' -> 'e'

'r' -> 'd'

's' -> 'c'

Applying this mapping to "serofedsoc":

- 's' -> 'c'

- 'e' -> 'o'

- 'r' -> 'd'

- 'o' -> 'e'

- 'f' -> 'f'

- 'e' -> 'o'

- 'd' -> 'r'

- 's' -> 'c'

- 'o' -> 'e'

- 'c' -> 's'

So, "codedefors"

But the original was "codeforces". So, where is the mistake?

Wait, perhaps the mapping is correct, but I miscounted the characters.

Wait, "codeforces" has two 'e's, but in "codedefors", I have only one 'e'. Wait, no, "codedefors" has one 'e', but "codeforces" has two 'e's. So, perhaps the mapping is not correctly applied.

Wait, perhaps I need to ensure that the mapping is applied correctly to each character in the encoded string.

Let me list the positions:

Encoded string: s e r o f e d s o c

Mapping:

s -> c

e -> o

r -> d

o -> e

f -> f

e -> o

d -> r

s -> c

o -> e

c -> s

So, decoded string: c o d e f o r c e s

Which is "codeforces"

Wait, that matches the original string.

I must have miscounted earlier. So, "codedefors" was a typo; it should be "codeforces". Yes, that makes sense now.

So, the mapping works correctly.

Therefore, the approach in the code seems correct.

The code constructs 'r' by sorting the unique characters of the encoded string, creates a symmetric mapping, and applies it to each character in the encoded string to get the decoded string.

Given that this works for the example, I can conclude that the program is correct.

**Final Answer**

\[ \boxed{\text{The given program is correct.}} \]