Let's examine the given code and determine the output state after the loop executes all the iterations.

The loop iterates over the list `arr` in reverse order. For each element in `arr`, it multiplies the current value of `tem` by the element and appends the result to the list `ans`. Here's a step-by-step breakdown:

1. The loop starts with `i` at the last index of `arr` and decrements `i` until it reaches 0.
2. `tem` is initialized to 1.
3. In each iteration, `tem` is multiplied by the current element of `arr` (from the end to the start), and the result is appended to `ans`.

Given the initial state, let's assume `arr` is `[a1, a2, a3, ..., an]`. The loop will perform the following operations:

- `i = n-1`: `tem = tem * an = 1 * an = an`, `ans = [an]`
- `i = n-2`: `tem = tem * an-1 = an * an-1`, `ans = [an, an * an-1]`
- `i = n-3`: `tem = tem * an-2 = an * an-1 * an-2`, `ans = [an, an * an-1, an * an-1 * an-2]`
- ...
- `i = 0`: `tem = tem * a1 = an * an-1 * ... * a2 * a1`, `ans = [an, an * an-1, an * an-1 * an-2, ..., an * an-1 * ... * a2 * a1]`

Thus, the final state of `ans` will be a list where each element is the product of all elements in `arr` from the end up to the current position.

Output State: **`arr` is a list of integers; `ans` is a list containing the cumulative products of `arr` from the end to the start; `tem` is the product of all elements in `arr`.**