To determine the final output state after all the iterations of the loop have finished, let's analyze the loop step by step.

The loop runs from `i = 1` to `i = n-1`. The behavior of the loop depends on the value of `(-1) ** i`:
- If `i` is odd, `(-1) ** i == -1`, and the loop appends `array[a[-1]]` to `answer` and decrements `a[-1]`.
- If `i` is even, `(-1) ** i == 1`, and the loop appends `array[a[0]]` to `answer` and increments `a[0]`.

Given the initial state:
- `answer` starts as `[1]`.
- `a` starts as `[1, -1]`.
- `array` is a list from `1` to `n`.

Let's trace the loop for a general `n`:

1. **First Iteration (i=1)**:
   - `(-1) ** 1 == -1` → `answer.append(array[a[-1]])` → `answer.append(array[-1])` → `answer.append(n)` → `answer = [1, n]`
   - Decrement `a[-1]` → `a = [1, -2]`

2. **Second Iteration (i=2)**:
   - `(-1) ** 2 == 1` → `answer.append(array[a[0]])` → `answer.append(array[1])` → `answer.append(2)` → `answer = [1, n, 2]`
   - Increment `a[0]` → `a = [2, -2]`

3. **Third Iteration (i=3)**:
   - `(-1) ** 3 == -1` → `answer.append(array[a[-1]])` → `answer.append(array[-2])` → `answer.append(n-1)` → `answer = [1, n, 2, n-1]`
   - Decrement `a[-1]` → `a = [2, -3]`

4. **Fourth Iteration (i=4)**:
   - `(-1) ** 4 == 1` → `answer.append(array[a[0]])` → `answer.append(array[2])` → `answer.append(3)` → `answer = [1, n, 2, n-1, 3]`
   - Increment `a[0]` → `a = [3, -3]`

This pattern continues. We observe that the loop appends elements from both ends of the `array` to `answer` alternately. The `a` list keeps track of the indices from which the next elements will be appended.

After `n-1` iterations, the `answer` list will contain all elements from `array` in a specific order: starting from the last element, then the first, then the second last, and so on.

Thus, the final `answer` list after all iterations will be a list of numbers from `n` down to `1`, and then from `2` up to `n-1` in alternating fashion.

For example, if `n = 5`, the `answer` list will be `[1, 5, 2, 4, 3]`.

The `a` list at the end will be `[n-1, -n]`.

Output State: **`answer` is `[1, n, 2, n-1, 3, n-2, ..., (n+1)//2, (n-1)//2 + 1]` and `a` is `[(n-1)//2 + 1, -n]`.**

In simpler terms, the `answer` list will have the numbers from `n` down to `1` and then from `2` up to `n-1` in an alternating pattern, and `a` will have the indices `[(n-1)//2 + 1, -n]`.