The code snippet `ans += (a[i] - a[i - 1]) // 2` updates the variable `ans` by adding the value of `(a[i] - a[i - 1]) // 2` to its current value.

Given the initial state:
- `t` is a positive integer where 1 ≤ t ≤ 10^4
- `n` is an input integer where 4 ≤ n ≤ 10^9
- `x` is an input integer where 2 ≤ x ≤ min(n, 2 · 10^5)
- `y` is an input integer where 0 ≤ y ≤ n - x
- `tt` is greater than 1
- `ii` is 1
- `i` is 2
- `a` is a sorted list of integers in ascending order with at least 3 elements
- `tmp` is a list containing the value `(a[2] - a[1]) // 2`

Let's analyze the impact of the code:

1. The variable `i` is 2.
2. The variable `a` is a sorted list of integers in ascending order with at least 3 elements.
3. The expression `(a[i] - a[i - 1]) // 2` calculates the integer division of the difference between the third element (`a[2]`) and the second element (`a[1]`) of the list `a`.

Therefore, the value added to `ans` is `(a[2] - a[1]) // 2`.

Since `ans` was not mentioned in the initial state, we assume it is initially 0.

Thus, the new value of `ans` is:
\[ \text{ans} = 0 + (a[2] - a[1]) // 2 \]

The updated state is:
- `t` is a positive integer where 1 ≤ t ≤ 10^4
- `n` is an input integer where 4 ≤ n ≤ 10^9
- `x` is an input integer where 2 ≤ x ≤ min(n, 2 · 10^5)
- `y` is an input integer where 0 ≤ y ≤ n - x
- `tt` is greater than 1
- `ii` is 1
- `i` is 2
- `a` is a sorted list of integers in ascending order with at least 3 elements
- `tmp` is a list containing the value `(a[2] - a[1]) // 2`
- `ans` is now equal to `(a[2] - a[1]) // 2`

Output State: **`t` is a positive integer where 1 ≤ t ≤ 10^4, `n` is an input integer where 4 ≤ n ≤ 10^9, `x` is an input integer where 2 ≤ x ≤ min(n, 2 · 10^5), `y` is an input integer where 0 ≤ y ≤ n - x, `tt` is greater than 1, `ii` is 1, `i` is 2, `a` is a sorted list of integers in ascending order with at least 3 elements, `tmp` is a list containing the value `(a[2] - a[1]) // 2`, `ans` is `(a[2] - a[1]) // 2`.**