Let's break down the initial state and the print statement step by step:

1. **Initial State:**
   - `p1`, `p2`, and `p3` are integers provided by the user such that \(0 \leq p1 \leq p2 \leq p3 \leq 30\).
   - `t` is greater than 1 (but not used in the print statement).
   - `_` is 1 (but not used in the print statement).
   - `low` is the minimum of `p3 - p1` and `p3 - p2`.
   - `high` is the maximum of `p3 - p1` and `p3 - p2`.
   - `cur` is equal to `low + 2`.

2. **Calculating `low` and `high`:**
   - Since \(p1 \leq p2 \leq p3\), the difference `p3 - p1` will always be greater than or equal to `p3 - p2`.
   - Therefore, `low` will be `p3 - p2` and `high` will be `p3 - p1`.

3. **Calculating `cur`:**
   - `cur` is `low + 2`, which means `cur` is `p3 - p2 + 2`.

4. **Expression in the print statement:**
   - The expression to be printed is `p1 - cur + p3`.
   - Substituting `cur` with `p3 - p2 + 2`, we get:
     \[
     p1 - (p3 - p2 + 2) + p3
     \]
   - Simplifying the expression:
     \[
     p1 - p3 + p2 - 2 + p3
     \]
     \[
     p1 + p2 - 2
     \]

5. **Final Output:**
   - The print statement will output the value of `p1 + p2 - 2`.

Output: **p1 + p2 - 2 (where p1 and p2 are integers provided by the user such that 0 <= p1 <= p2 <= p3 <= 30)**