Correctness: **False**.

Explanation: The program does not correctly implement the logic required to solve the problem. Specifically, the formula used in the `suma` calculation does not accurately determine the number of valid pairs \((a, b)\) that satisfy the condition \(a + b\) being a multiple of \(b \cdot \gcd(a, b)\).

To illustrate, let's consider a specific example:

- For the input \(n = 10\) and \(m = 8\), the expected output is \(14\). However, the provided code gives a different result.

Let's manually check a few pairs to see where the code might fail:

1. For \(a = 1\) and \(b = 1\):
   - \(a + b = 2\)
   - \(b \cdot \gcd(a, b) = 1 \cdot 1 = 1\)
   - \(2 \mod 1 = 0\), so \((1, 1)\) is valid.

2. For \(a = 2\) and \(b = 1\):
   - \(a + b = 3\)
   - \(b \cdot \gcd(a, b) = 1 \cdot 1 = 1\)
   - \(3 \mod 1 = 0\), so \((2, 1)\) is valid.

3. For \(a = 2\) and \(b = 2\):
   - \(a + b = 4\)
   - \(b \cdot \gcd(a, b) = 2 \cdot 2 = 4\)
   - \(4 \mod 4 = 0\), so \((2, 2)\) is valid.

4. For \(a = 3\) and \(b = 1\):
   - \(a + b = 4\)
   - \(b \cdot \gcd(a, b) = 1 \cdot 1 = 1\)
   - \(4 \mod 1 = 0\), so \((3, 1)\) is valid.

5. For \(a = 4\) and \(b = 1\):
   - \(a + b = 5\)
   - \(b \cdot \gcd(a, b) = 1 \cdot 1 = 1\)
   - \(5 \mod 1 = 0\), so \((4, 1)\) is valid.

6. For \(a = 5\) and \(b = 1\):
   - \(a + b = 6\)
   - \(b \cdot \gcd(a, b) = 1 \cdot 1 = 1\)
   - \(6 \mod 1 = 0\), so \((5, 1)\) is valid.

7. For \(a = 6\) and \(b = 1\):
   - \(a + b = 7\)
   - \(b \cdot \gcd(a, b) = 1 \cdot 1 = 1\)
   - \(7 \mod 1 = 0\), so \((6, 1)\) is valid.

8. For \(a = 6\) and \(b = 2\):
   - \(a + b = 8\)
   - \(b \cdot \gcd(a, b) = 2 \cdot 2 = 4\)
   - \(8 \mod 4 = 0\), so \((6, 2)\) is valid.

9. For \(a = 6\) and \(b = 3\):
   - \(a + b = 9\)
   - \(b \cdot \gcd(a, b) = 3 \cdot 3 = 9\)
   - \(9 \mod 9 = 0\), so \((6, 3)\) is valid.

10. For \(a = 7\) and \(b = 1\):
    - \(a + b = 8\)
    - \(b \cdot \gcd(a, b) = 1 \cdot 1 = 1\)
    - \(8 \mod 1 = 0\), so \((7, 1)\) is valid.

11. For \(a = 8\) and \(b = 1\):
    - \(a + b = 9\)
    - \(b \cdot \gcd(a, b) = 1 \cdot 1 = 1\)
    - \(9 \mod 1 = 0\), so \((8, 1)\) is valid.

12. For \(a = 9\) and \(b = 1\):
    - \(a + b = 10\)
    - \(b \cdot \gcd(a, b) = 1 \cdot 1 = 1\)
    - \(10 \mod 1 = 0\), so \((9, 1)\) is valid.

13. For \(a = 10\) and \(b = 1\):
    - \(a + b = 11\)
    - \(b \cdot \gcd(a, b) = 1 \cdot 1 = 1\)
    - \(11 \mod 1 = 0\), so \((10, 1)\) is valid.

14. For \(a = 10\) and \(b = 2\):
    - \(a + b = 12\)
    - \(b \cdot \gcd(a, b) = 2 \cdot 2 = 4\)
    - \(12 \mod 4 = 0\), so \((10, 2)\) is valid.

Thus, there are indeed 14 valid pairs, but the code does not produce this result, indicating a logical error in the implementation.