Given the initial state where `N` is a positive integer such that 1 ≤ N ≤ 10^6; `n` is an input integer; `x` is the integer square root of `n`; and `x` squared is equal to `n`, we proceed with the code:

The variable `answr` is assigned the value of `x * 4`. Since `x` is defined as the integer square root of `n`, we can express `answr` in terms of `n`. Specifically, since `x` squared equals `n`, it follows that `x = sqrt(n)`. Thus, `answr = sqrt(n) * 4`.

The output state does not change the values of `N`, `n`, and `x` but computes a new value for `answr`.

Output State: **`N` is a positive integer such that 1 ≤ N ≤ 10^6; `n` is an input integer; `x` is the integer square root of `n`; `answr` is calculated as `x * 4`.**