`answr` is assigned the value of `(x + x + 1) * 2`. Since `x` is defined as the integer square root of `n` and meets the condition that `x * (x + 1) > n`, the expression evaluates to a specific value based on `x`. The calculation results in `answr = (2x + 1) * 2 = 4x + 2`. The states of other variables are not affected. Therefore, the Output State is: `N` is a positive integer such that 1 ≤ N ≤ 10^6; `n` is an input integer; `x` is the integer square root of `n`; `answr` is `4x + 2`.

Output State: **`N` is a positive integer such that 1 ≤ N ≤ 10^6; `n` is an input integer; `x` is the integer square root of `n`; `answr` is `4x + 2`**