The code snippet `ma = len(s) - d` updates the value of `ma` to be the length of the string `s` minus the value of `d`. Given that `d` is 3, `ma` becomes `n - 3` (since `len(s)` is equal to `n`).

Output State: **`t` is an integer such that 1 <= t <= 10^4, `n` is an integer such that 1 <= n <= 10, `s` is a string of length `n` consisting of characters 'W' or 'B', with at least one 'B' in the string, `ma` is `n - 3`, `mi` is the position of the first 'B' in the string `s`, `m` is an input integer, `c` is the position of the first 'B' in the string `s`, `d` is 3, `l` is an empty list, `j` is the third last character of `s`.**