The code `a *= 3` multiplies the current value of `a` by 3. Since `a` was initially 3 times its original value between 3 and 30 inclusive, let's denote the original value of `a` as `a_original`. Therefore, `a = 3 * a_original`.

After executing `a *= 3`, the new value of `a` will be `a * 3 = 3 * (3 * a_original) = 9 * a_original`. 

The value of `b` remains unchanged because the code only modifies `a`.

Output State: **`a` is 9 times its original value (between 9 and 90 inclusive); `b` is 2 times its original value (between 2 and 20 inclusive)**