Let's break down the initial state and the print statement step by step:

1. **Initial State**:
   - `cnt` is 0.
   - `l` is defined as `func_2() + 3`.
   - The condition `(cnt == 0 and l == n + 1)` is true.

2. From the condition `(cnt == 0 and l == n + 1)` being true, we can deduce:
   - Since `cnt` is 0, the first part of the condition `cnt == 0` is satisfied.
   - Therefore, `l == n + 1` must also be true, meaning `func_2() + 3 == n + 1`.

3. The print statement is:
   ```
   print(f'! {i * v}', flush=True)
   ```

4. To determine what will be printed, we need to know the values of `i` and `v`. However, these variables are not defined in the initial state provided. Given the context, let's assume that `i` and `v` are such that they form a valid expression that can be evaluated.

Since the exact values of `i` and `v` are not specified, we can only describe the format of the output. The print statement will output a string that includes the product of `i` and `v`, with a leading exclamation mark.

Output: **! [i * v]**