Let's break down the initial state and the print statement step by step:

1. **Initial State**:
   - `cnt` is 0.
   - `l` is defined as `func_2() + 1`.
   - The condition `cnt == 0 and l == n + 1` is true.

2. **Understanding `l`**:
   - Since `l` is defined as `func_2() + 1`, we need to determine the value of `func_2()`.
   - Given the condition `cnt == 0 and l == n + 1` is true, and knowing that `cnt` is 0, it implies that `l` must be `n + 1`.

3. **Determine `func_2()`**:
   - From the condition `l == n + 1`, we can deduce that `func_2()` must return `n`.
   - Therefore, `func_2()` returns `n`, and `l = n + 1`.

4. **Print Statement**:
   - The print statement is `print(f'! {i * v}', flush=True)`.
   - However, the initial state does not provide any information about `i` or `v`.

Given the information, we cannot determine the exact values of `i` and `v`. Therefore, the output will include placeholders for these variables.

Output: **! [i * v]**