The code snippet provided reassigns the variable `v` to the value returned by the function `func_2()`. This means the previous value of `v` is overwritten by whatever `func_2()` returns.

Given the initial state:
- `n` and `k` are the values returned by `func_3()`, which are positive integers such that \(1 \leq k \leq n \leq 10^4\).
- `i` is \(n - 2\).
- `v` is the value returned by `func_2()`.

After executing the line `v = func_2()`, the new value of `v` is the value returned by `func_2()`. The values of `n`, `k`, and `i` remain unchanged.

Output State: **`n` and `k` are the values returned by `func_3()`, which are positive integers such that \(1 \leq k \leq n \leq 10^4\); `i` is \(n - 2\); `v` is the value returned by `func_2()`.**