The code snippet `c = str(b[-1::-1])` reverses the string `b` and assigns it to `c`. Let's analyze this step-by-step:

- `b` is a string entered by the user, which means its value is unknown initially.
- `c` is assigned the value of `b` reversed and converted to a string (which it already is).

Therefore, the only change in the variables is that `c` now holds the reversed string of `b`.

Output State: **`t` is a positive integer such that \(1 \leq t \leq 10^4\), `n` is a positive integer such that \(1 \leq n \leq 10\), `s` is a string of length `n` consisting of characters 'W' and 'B' with at least one 'B', `a` is an integer, `b` is the string entered by the user, `c` is the reversed string of `b`**