The code `c = str(b[-1::-1])` reverses the string `b` and assigns the reversed string to `c`. Given the initial state:

- `t` is a positive integer such that \(1 \leq t \leq 10^4\)
- `n` is a positive integer such that \(1 \leq n \leq 10\)
- `s` is a string of length `n` consisting of characters 'W' and 'B' with at least one 'B'
- `a` is the integer entered by the user
- `b` is the string entered by the user
- `c` is the reversed string of `b`

After executing the code:

- The value of `c` is now the reversed version of the string `b`.
- The values of `t`, `n`, `s`, `a`, and `b` remain unchanged.

Output State: **`t` is a positive integer such that \(1 \leq t \leq 10^4\), `n` is a positive integer such that \(1 \leq n \leq 10\), `s` is a string of length `n` consisting of characters 'W' and 'B' with at least one 'B', `a` is the integer entered by the user, `b` is the string entered by the user, `c` is the reversed string of `b`.**