Alright, I've got this problem to solve. Let's see what it's asking for. So, I have an array of integers, and I need to perform exactly K operations on it. In each operation, I can select any contiguous subarray (which could even be empty) and insert the sum of that subarray anywhere in the array. My goal is to maximize the sum of the array after K operations, and since the sum can be very large, I need to output it modulo 10^9 + 7.

First, I need to understand what exactly an operation does. When I select a contiguous subarray and insert its sum into the array, I'm essentially adding that sum to the total sum of the array because I'm inserting a new element equal to the sum of some subarray. But, I need to think about how this affects the overall sum after K operations.

Let me consider a simple example to get a better understanding. Suppose I have an array [1, 2, 3] and K=1. If I select the entire array as the subarray, its sum is 6, and I can insert 6 anywhere in the array, say at the beginning, making the new array [6, 1, 2, 3], which has a sum of 12. Alternatively, if I select an empty subarray, its sum is 0, and inserting 0 doesn't change the sum. So, in this case, it's better to select the entire array.

Wait, but in the first test case of the example, they have negative numbers, and selecting an empty subarray leads to adding zero, which is better than adding negative sums. So, maybe I need to be careful about the subarrays I choose.

Let me think about what subarray sum would be best to insert. Since I want to maximize the sum of the array, I should choose the subarray with the maximum possible sum to add in each operation. That sounds like a maximum subarray sum problem.

Yes, in each operation, I should compute the maximum sum of any contiguous subarray, and insert that sum into the array. By doing this, I'm adding the largest possible value to the array's sum in each operation.

So, for the first operation, I find the maximum subarray sum, insert it, and add that value to the total sum. For the next operation, I can again find the maximum subarray sum, which would now include the newly inserted sum, and insert that again, and so on, for K operations.

But wait, in each operation, after inserting the sum, the array changes, so the maximum subarray sum could change. I need to consider how the array evolves with each operation.

Let's denote S as the initial sum of the array. After the first operation, I insert the maximum subarray sum, say M1, so the new sum is S + M1. Then, in the second operation, I can insert the new maximum subarray sum, which could be M1 or a larger sum that includes M1, and so on.

This seems a bit recursive and could be complicated to compute directly, especially since K can be up to 2*10^5, and T (the number of test cases) is up to 10^4, with the total sum of N and K across all test cases being up to 2*10^5. So, I need an efficient way to compute this.

Maybe there's a pattern or a formula that can help me compute the final sum after K operations without simulating each operation.

Let me consider that in each operation, I'm adding the maximum subarray sum to the total sum. So, if I can find a way to compute the total addition after K operations based on the initial array, that would be great.

Wait, perhaps I can think of it as the initial sum plus K times the maximum subarray sum. But that might not be accurate because after adding the maximum subarray sum, the new array has a new maximum subarray sum, which could be larger.

Let me consider an example to see the pattern.

Take the second test case:

N=3, K=3

Array: [2, 2, 8]

Sum S = 12

Maximum subarray sum M = 12 (the entire array)

After first operation: insert 12, array becomes [2, 2, 8, 12], sum = 24

Second operation: maximum subarray sum is now 24 (the entire new array), insert 24, array becomes [2, 2, 8, 12, 24], sum = 48

Third operation: maximum subarray sum is 48, insert 48, array becomes [2, 2, 8, 12, 24, 48], sum = 96

So, the final sum is 96, which matches the sample output.

In this case, it seems like in each operation, the maximum subarray sum is doubling the previous sum.

Wait, more precisely, each new sum is twice the previous sum.

Wait, no:

Operation 1: sum = 12 + 12 = 24

Operation 2: sum = 24 + 24 = 48

Operation 3: sum = 48 + 48 = 96

So, it's like sum doubles in each operation.

But why is the maximum subarray sum equal to the current sum in this case?

Because all elements are positive, so the maximum subarray sum is the sum of the entire array.

So, in this case, each insertion adds the current sum to the array, making the new sum double the previous sum.

Wait, not quite. If I have sum S, and I insert S, the new sum is S + S = 2S.

Yes, that's correct.

So, in this scenario, where all elements are positive, the maximum subarray sum is the sum of the entire array, and inserting that sum increases the total sum by S, making it 2S.

Then, in the next operation, the maximum subarray sum is again the sum of the entire array, which is 2S, and inserting it makes the sum 4S, and so on.

So, after K operations, the sum would be S * 2^K.

But wait, in the sample input, for N=3, K=3, sum S=12, and the final sum is 96, which is 12 * 8, i.e., 12 * 2^3, which matches this pattern.

Similarly, in the seventh test case, all elements are negative, so the maximum subarray sum is zero (from an empty subarray), and inserting zero doesn't change the sum. So, the sum remains the initial sum, which is -42, and modulo 10^9 + 7 is 42, as given in the sample output.

Wait, in the seventh test case, the initial sum is -42, but modulo operation is tricky with negative numbers. Actually, -42 modulo 10^9 + 7 is equivalent to 10^9 + 7 - 42 = 999999958, but in the sample output, it's 42. Wait, maybe I need to handle the modulo operation carefully for negative sums.

Wait, in the code provided, they have ((s + t) % MOD + MOD) % MOD, which seems to handle negative sums properly by adding MOD twice and taking modulo again to ensure a non-negative result.

So, in the case where all elements are negative, the maximum subarray sum is zero (from an empty subarray), and adding zero in each operation doesn't change the sum. So, the final sum is the initial sum, handled with modulo.

In the fourth test case, N=5, K=1, array=[4, -2, 8, -12, 9], sum S=7.

Maximum subarray sum is 4 + (-2) + 8 = 10 (from subarray [4, -2, 8]).

After inserting 10, the array becomes [4, -2, 8, -12, 9, 10], sum=17, which matches the sample output.

So, in this case, with K=1, we just add the maximum subarray sum once.

Wait, but in the earlier case with K=3, we had to add the sum multiple times, and it was doubling each time.

So, perhaps there's a pattern based on whether K is 1 or greater than 1.

Let me try to generalize this.

If all elements are positive, the maximum subarray sum is the sum of the entire array, and each insertion doubles the sum.

If there are negative elements, the maximum subarray sum might be less than the total sum, and inserting it would increase the sum by that amount.

But in the case where the maximum subarray sum is less than the total sum, it's still better to add the maximum subarray sum in each operation.

Wait, but in the fourth test case, with K=1, we added the maximum subarray sum once, which was 10, to the initial sum of 7, making it 17. But actually, inserting 10 to the array makes the sum 17, not adding 10 to the sum.

Wait, I think I need to clarify the difference between adding the sum to the array and adding the sum to the total sum.

When I insert the sum of a subarray, I'm adding that value to the array, which increases the total sum by that amount.

So, if I have sum S, and I insert a value M (the sum of some subarray), the new sum is S + M.

Then, in the next operation, I can insert another M, making the sum S + M + M = S + 2M.

Wait, but in the second test case, it's S + M + 2M + 4M, and so on.

Wait, no, in the second test case, with K=3, S=12, M=12, after first insertion, sum=24, then M=24, insert to make sum=48, then M=48, insert to make sum=96.

So, it's S * 2^K.

But in the fourth test case, with K=1, S=7, M=10, sum after insertion is 17, which is S + M.

So, it seems that in each operation, we can choose a new M, which is the current maximum subarray sum.

But in the second test case, M changes in each operation because we're adding larger and larger sums.

So, perhaps in general, after the first operation, M becomes equal to the current sum, and in each subsequent operation, M doubles.

Wait, in the second test case, after the first insertion, the array is [2,2,8,12], and M=12+2+2+8=24, then insert 24 to make [2,2,8,12,24], and M=24+12+8+2+2=48, and so on.

Wait, but actually, in each operation, the maximum subarray sum is the sum of the entire array, which is S + M from previous operations.

Wait, perhaps I need to model this mathematically.

Let me denote:

S0 = initial sum

M0 = initial maximum subarray sum

After first operation: sum S1 = S0 + M0

M1 = maximum subarray sum of the new array, which is S1

After second operation: sum S2 = S1 + M1 = S1 + S1 = 2*S1 = 2*(S0 + M0)

M2 = maximum subarray sum of the new array, which is S2

...

After K operations: sum SK = S0 + M0 + M1 + ... + MK-1

But since in each operation, Mi = Si-1, then SK = S0 + M0 + M1 + ... + MK-1 = S0 + S0 + S1 + S2 + ... + SK-2

Wait, this seems complicated.

Alternatively, perhaps I can see that after the first operation, sum S1 = S0 + M0

After second operation, S2 = S1 + M1 = S1 + S1 = 2*S1 = 2*(S0 + M0)

After third operation, S3 = S2 + M2 = S2 + S2 = 2*S2 = 4*(S0 + M0)

...

After K operations, SK = (S0 + M0) * 2^(K-1)

Wait, in the second test case, S0=12, M0=12, SK=12 + 12 + 24 + 48 = 96, which is 12 * 8 = 12 * 2^3.

But according to this formula, (12 + 12) * 2^(3-1) = 24 * 4 = 96, which matches.

In the fourth test case, K=1, SK = (7 + 10) * 2^(1-1) = 17 * 1 = 17, which matches.

So, it seems that the general formula is SK = (S0 + M0) * 2^(K-1)

Wait, but in the seventh test case, S0=-42, M0=0 (since the maximum subarray sum is zero from an empty subarray), so SK = (-42 + 0) * 2^(1000-1) = -42 * 2^999, which is a very large negative number, but in the sample output, it's 42.

Wait, perhaps I need to consider that M0 is zero when all elements are negative, and inserting zero in each operation doesn't change the sum.

Wait, but according to the formula, it would be S0 * 2^(K-1), which for negative S0 and large K would be a very large negative number, but in the sample output, it's 42.

Wait, perhaps I need to take modulo at each step, considering that modulo operation can handle negative numbers by adding MOD until it's positive.

Wait, in the code, they have ((s + t) % MOD + MOD) % MOD, which ensures a non-negative result.

So, -42 modulo 10^9 + 7 is equivalent to 10^9 + 7 - 42 = 999999958, but in the sample output, it's 42.

Wait, perhaps there's something wrong with my understanding.

Wait, in the seventh test case, N=6, K=1000, array=[-10^9, -10^9, -10^9, -10^9, -10^9, -10^9], sum S0=-6*10^9.

M0=0 (from empty subarray).

After first operation: insert 0, sum remains -6*10^9.

After second operation: insert 0, sum remains -6*10^9.

...

After 1000 operations: sum is still -6*10^9.

But -6*10^9 modulo 10^9+7 is (-6*10^9) % (10^9+7) = (-6*10^9 + 6*10^9 + 7*10^9) % (10^9+7) = (7*10^9) % (10^9+7) = 7*10^9 - 7*10^9 - 7 = -7, which is incorrect.

Wait, perhaps I need to add MOD multiple times to make it positive.

Actually, in the code, they have ((s + t) % MOD + MOD) % MOD, which ensures a non-negative result.

So, (-6*10^9) % (10^9+7) = -6*10^9 + 6*10^9 + 7 = 7, but in the sample output, it's 42.

Wait, perhaps I'm miscalculating.

Wait, in the sample output for the seventh test case, it's 42, but according to my calculation, it should be 7.

Wait, maybe I need to look back at the sample input and output.

Looking back at the sample input and output, for the seventh test case, the output is 42.

Wait, perhaps I need to verify my understanding.

Wait, in the seventh test case, N=6, K=1000, array=[-1000000000, -1000000000, -1000000000, -1000000000, -1000000000, -1000000000], sum S0=-6*10^9.

M0=0 (from empty subarray).

After each operation, we insert 0, so the sum remains -6*10^9.

Then, (-6*10^9) % (10^9+7) = -6*10^9 + 6*10^9 + 7 = 7, but the sample output is 42.

Wait, maybe I need to check the sample input and output again.

Wait, in the sample input and output provided in the problem, the seventh test case has output 42, but according to my calculation, it should be 7.

Wait, perhaps there's a mistake in my calculation.

Wait, let's compute (-6*10^9) modulo (10^9 + 7).

We know that a modulo m is a - m * floor(a/m).

So, -6*10^9 divided by 10^9 + 7 is -6 + (-ve adjustment).

Wait, floor(-6*10^9 / 10^9 +7) = floor(-5.999... ) = -6.

So, -6*10^9 - (-6)*(10^9 +7) = -6*10^9 +6*10^9 +42 = 42.

Yes, so (-6*10^9) % (10^9 +7) = 42.

I see, so my earlier calculation was incorrect. It's actually 42, which matches the sample output.

So, in this case, where M0=0, and we insert 0 in each operation, the sum remains S0, and S0 modulo 10^9+7 is 42.

Therefore, the general approach seems to be:

- Compute the initial sum S0.

- Compute the initial maximum subarray sum M0.

- Then, the final sum SK = S0 + M0 * (2^{K-1})

Wait, but in the second test case, S0=12, M0=12, SK=12 + 12*(2^{3-1})=12 + 12*4=12+48=60, but the sample output is 96.

Wait, that doesn't match.

Wait, perhaps I need to adjust the formula.

Wait, in the second test case:

Operation 1: insert M0=12, sum becomes 24

Operation 2: insert M1=24, sum becomes 48

Operation 3: insert M2=48, sum becomes 96

So, total addition is M0 + M1 + M2 = 12 + 24 + 48 = 84, plus initial sum 12, total 96.

But according to my previous formula, it's S0 + M0 * (2^{K-1}) = 12 + 12*4=60, which is incorrect.

So, perhaps that's not the correct formula.

Wait, maybe it's S0 + M0 * (2^K -1 )

In the second test case, S0 + M0*(2^3 -1 ) = 12 + 12*7 = 96, which matches.

Similarly, in the fourth test case, S0 + M0*(2^1 -1 ) = 7 + 10*1 = 17, which matches.

In the seventh test case, S0 + M0*(2^{1000}-1) = -42 + 0*(2^{1000}-1) = -42, which modulo 10^9+7 is 42, which matches.

So, the general formula seems to be SK = S0 + M0 * (2^K -1 )

This seems consistent with the sample inputs and outputs.

Therefore, my approach should be:

1. Compute the initial sum S0 of the array.

2. Compute the initial maximum subarray sum M0.

3. Compute the final sum SK = S0 + M0 * (2^K -1 )

4. Take SK modulo 10^9+7, ensuring it's a non-negative value.

Now, to compute M0, the initial maximum subarray sum, I can use Kadane's algorithm, which efficiently finds the maximum sum of a contiguous subarray in O(N) time.

Given that N can be up to 2*10^5 and T up to 10^4, with the total sum of N and K across all test cases up to 2*10^5, I need to ensure that my solution is efficient.

Since the total sum of N and K across all test cases is up to 2*10^5, and T is up to 10^4, individual test cases can have N and K up to 2*10^5, but not simultaneously due to the constraint on the sum.

Therefore, my solution should be O(N) per test case, which should be acceptable.

Now, let's look at the provided code and see if it implements this approach correctly.

Looking at the code:

- It reads T, the number of test cases.

- For each test case, it reads N and K, then reads the array A.

- It computes S = sum(A), which is S0.

- It computes T, which seems to be the initial maximum subarray sum M0, using a loop that implements Kadane's algorithm.

- Then, it computes ans = ((S + T) % MOD + MOD) % MOD

- Then, for i in range(K-1), it updates T = (T * 2) % MOD and adds T to ans, taking modulo each time.

Wait, this seems different from my earlier formula.

According to my formula, SK = S0 + M0 * (2^K -1 )

But in the code, it's computing ans = S + M0, then adding M0 * 2^1, M0 * 2^2, ..., M0 * 2^{K-1}, each time taking modulo.

Wait, let's see:

ans = S + M0

Then, for K-1 times, it's adding M0 * 2^i for i from 1 to K-1.

Wait, no, in the code, it's:

ans = S + M0

Then, for i in range(K-1):

T = (T * 2) % MOD

ans = (ans + T) % MOD

So, it's adding M0 * 2^i for i from 0 to K-1.

Wait, but according to my formula, it should be M0 * (2^K -1 ), which is M0 * (1 + 2 + 4 + ... + 2^{K-1} )

So, the code is adding M0 * 1 + M0 * 2 + M0 * 4 + ... + M0 * 2^{K-1}, which is M0 * (2^K -1 ), which matches my formula.

Wait, but in the second test case, with K=3, it's adding M0 * 1 + M0 * 2 + M0 * 4, which is M0 * 7, same as M0 * (2^3 -1 ) = 7*M0.

Yes, that matches.

Therefore, the code is correctly implementing the formula SK = S0 + M0 * (2^K -1 )

It also handles the modulo operation properly for negative sums by using ((s + t) % MOD + MOD) % MOD.

Therefore, the given program is correct.

**Final Answer**

\boxed{\text{The given program is correct.}}