To determine the final output state after all iterations of the loop, we need to analyze the loop's behavior and the conditions under which it terminates.

The loop continues as long as both `(x + y) * x <= n` and `(x + y) * y <= m` are true. Given the initial state `x = 1`, the loop will increment `y` in each iteration and check these conditions. The loop will also update `cnt` if the greatest common divisor (gcd) of `x` and `y` is 1.

Let's break down the loop iterations:

1. **First Iteration**:
   - `x = 1`, `y = 2`
   - `(x + y) * x = 3` and `(x + y) * y = 6`
   - Since `3 <= n` and `6 <= m` (given `n >= 2` and `m >= 2`), the loop executes.
   - `gcd(1, 2) == 1`, so `cnt` is incremented by `min(n // 3, m // 6)`.

2. **Second Iteration**:
   - `x = 1`, `y = 3`
   - `(x + y) * x = 4` and `(x + y) * y = 9`
   - Since `4 <= n` and `9 <= m` (given `n >= 3` and `m >= 6`), the loop executes.
   - `gcd(1, 3) == 1`, so `cnt` is incremented by `min(n // 4, m // 9)`.

3. **Third Iteration**:
   - `x = 1`, `y = 4`
   - `(x + y) * x = 5` and `(x + y) * y = 12`
   - Since `5 <= n` and `12 <= m` (given `n >= 3` and `m >= 12`), the loop executes.
   - `gcd(1, 4) == 1`, so `cnt` is incremented by `min(n // 5, m // 12)`.

The loop will continue until either `(x + y) * x > n` or `(x + y) * y > m`. Given the initial conditions and the increments, the loop will terminate when `y` becomes large enough that `(x + y) * y` exceeds `m`. Since `x` is fixed at 1, the loop will terminate when `y` is such that `(1 + y) * y > m`.

Let's assume `m` is large enough that the loop can run several iterations, but we need to find the point where it stops. For simplicity, let's assume `n` and `m` are sufficiently large to allow several iterations, and we need to find the final state.

Given the pattern, the loop will terminate when `(1 + y) * y > m`. The final value of `y` will be the smallest integer such that `(1 + y) * y > m`.

The final output state will be:
- `x` remains 1.
- `y` is the smallest integer such that `(1 + y) * y > m`.
- `cnt` is the sum of `min(n // ((1 + y) * 1), m // ((1 + y) * y))` for all valid `y` values.

For the sake of this problem, let's assume the loop terminates after `y` reaches a value such that `(1 + y) * y > m`. The final `cnt` will be the sum of the increments from each valid iteration.

Let's assume `m` is large enough that the loop runs until `y` reaches a value where `(1 + y) * y > m`. For example, if `m = 12`, the loop will run until `y = 4` (since `(1 + 4) * 4 = 20 > 12`).

The final output state will be:
- `x = 1`
- `y` is the smallest integer such that `(1 + y) * y > m`
- `cnt` is the sum of the increments from each valid iteration

For `m = 12`, the final `y` is 4, and `cnt` is the sum of the increments from `y = 2`, `y = 3`, and `y = 4`.

Let's calculate the final `cnt`:
- For `y = 2`: `cnt += min(n // 3, m // 6)`
- For `y = 3`: `cnt += min(n // 4, m // 9)`
- For `y = 4`: `cnt += min(n // 5, m // 12)`

Assuming `n` and `m` are sufficiently large, the final `cnt` will be the sum of these increments.

Output State: **x is 1, y is the smallest integer such that (1 + y) * y > m, cnt is the sum of the increments from each valid iteration.**

For a specific example with `m = 12`:
- `y = 4`
- `cnt = min(n // 3, 12 // 6) + min(n // 4, 12 // 9) + min(n // 5, 12 // 12)`

Assuming `n` is large enough:
- `cnt = min(n // 3, 2) + min(n // 4, 1) + min(n // 5, 1)`

If `n >= 15`:
- `cnt = 2 + 1 + 1 = 4`

Output State: **x is 1, y is 4, cnt is 4.**

This is the final output state after all iterations of the loop have finished, assuming `n` and `m` are sufficiently large.