To determine what will be printed by the given `print` statement, let's break down the initial state and the logic of the statement step by step.

### Initial State:
- `neg` is the number of '-' characters in the string `s`.
- The value of `s` remains unchanged.

### Code Snippet:
```python
print(n - 2 * neg if n != neg else n)
```

### Analysis:
1. **Determine the value of `neg`**:
   - `neg` is the count of '-' characters in the string `s`.

2. **Determine the value of `n`**:
   - The value of `n` is not explicitly given in the initial state. However, we can infer that `n` is likely the length of the string `s` because the condition `n != neg` suggests a comparison between the length of the string and the number of '-' characters.

3. **Evaluate the condition `n != neg`**:
   - If `n` (the length of `s`) is not equal to `neg` (the number of '-' characters in `s`), the expression `n - 2 * neg` will be printed.
   - If `n` is equal to `neg`, the value of `n` will be printed.

### Possible Scenarios:
- **Scenario 1**: `n != neg`
  - In this case, the expression `n - 2 * neg` will be printed.
  - For example, if `s = "a-b-c"`, then `n = 5` and `neg = 2`. The expression `5 - 2 * 2` evaluates to `1`.

- **Scenario 2**: `n == neg`
  - In this case, the value of `n` will be printed.
  - For example, if `s = "---"`, then `n = 3` and `neg = 3`. The condition `n == neg` is true, so `3` will be printed.

### Final Output:
- The output will depend on the specific values of `n` and `neg` based on the string `s`.
- If `n != neg`, the output will be `n - 2 * neg`.
- If `n == neg`, the output will be `n`.

Since the exact string `s` is not provided, we can't compute the exact numerical value. However, we can describe the output based on the given conditions.

Output: **n - 2 * neg if n != neg else n (where n is the length of the string s and neg is the number of '-' characters in the string s)**