The code snippet `max_diff = max(max_diff, abs(e - s))` updates the value of `max_diff` to be the maximum between its current value and the absolute difference between `e` and `s`. Let's analyze this step-by-step:

1. **Initial Values**: 
   - `b` is 1
   - `max_diff` is 0
   - `e` is the sum of `tabs[i-1] == 1` for all `i` where `(i - 1) % k != 0`
   - `s` is the sum of `tabs[i-1] == -1` for all `i` where `(i - 1) % k != 0`
   - `n` is the total number of iterations
   - `i` is `n + 1`

2. **Impact of the Code**:
   - The code calculates `abs(e - s)` which is the absolute difference between `e` and `s`.
   - It then updates `max_diff` to be the maximum of its current value (`0`) and the calculated absolute difference.

3. **Calculation**:
   - Since `max_diff` was initially 0, the new value of `max_diff` will be `max(0, abs(e - s))`. Given that `abs(e - s)` is a non-negative value, the updated value of `max_diff` will be `abs(e - s)`.

4. **Updated Variables**:
   - `max_diff` is now `abs(e - s)`
   - The values of `b`, `e`, `s`, `n`, and `i` remain unchanged.

Therefore, the output state is:

Output State: **`b` is 1, `max_diff` is `abs(e - s)`, `e` is the sum of `tabs[i-1] == 1` for all `i` where `(i - 1) % k != 0`, `s` is the sum of `tabs[i-1] == -1` for all `i` where `(i - 1) % k != 0`, `n` is the total number of iterations, `i` is `n + 1`.**