Given the initial state and the code snippet, let's analyze the situation step by step:

**Initial State:**
- `i` is `i + 1` (This is a placeholder indicating that `i` should be incremented by 1 from its original value, but we don't know the exact original value)
- `b` is `b`
- `k` is `k`
- `e` is `e`
- `s` is `s`
- `n` is `n`

**Code Snippet:**
```python
e += tabs[i - 1] == 1
s += tabs[i - 1] == -1
```

Since the exact values of `i`, `tabs`, `e`, and `s` are not provided, let's consider the logical implications of the code:

1. `e += tabs[i - 1] == 1`:
   - This line checks if `tabs[i - 1]` is equal to 1.
   - If `tabs[i - 1]` is 1, then `e` is incremented by 1.
   - If `tabs[i - 1]` is not 1, then `e` remains unchanged.

2. `s += tabs[i - 1] == -1`:
   - This line checks if `tabs[i - 1]` is equal to -1.
   - If `tabs[i - 1]` is -1, then `s` is incremented by 1.
   - If `tabs[i - 1]` is not -1, then `s` remains unchanged.

Without the actual values of `tabs`, we can't determine the exact numerical values of `e` and `s`, but we can describe their updated states relative to their original values.

**Final Output State:**
- `i` is `i + 1` (incremented by 1 from its original value)
- `b` is `b` (unchanged)
- `k` is `k` (unchanged)
- `e` is `e + (tabs[i - 1] == 1)` (incremented by 1 if `tabs[i - 1]` is 1, otherwise unchanged)
- `s` is `s + (tabs[i - 1] == -1)` (incremented by 1 if `tabs[i - 1]` is -1, otherwise unchanged)
- `n` is `n` (unchanged)

Thus, the final output state is:
Output State: **i is i + 1, b is b, k is k, e is e + (tabs[i - 1] == 1), s is s + (tabs[i - 1] == -1), n is n**