Output State: **i is N, j is N + 2, x1 is x2, y1 is y2, c1 is c2, x2 is x1, y2 is y1, c2 is c1, d is (c1 * T - c2 * T) / (c1 * c2), cx is (x1 + x2) / 2, cy is (y1 + y2) / 2, dx is (x1 - x2) / 2, dy is (y1 - y2) / 2, d2 is (x1 - x2)**^2 / 4 + (y1 - y2)**^2 / 4**

Explanation:
- The value of `d` is updated by dividing it by `c1 * c2`. Given `d = c1 * T - c2 * T`, after division, `d` becomes `(c1 * T - c2 * T) / (c1 * c2)`.
- `cx` is calculated as the average of `x1` and `x2`, so `cx = (x1 + x2) / 2`.
- `cy` is calculated as the average of `y1` and `y2`, so `cy = (y1 + y2) / 2`.
- `dx` is calculated as half the difference between `x1` and `x2`, so `dx = (x1 - x2) / 2`.
- `dy` is calculated as half the difference between `y1` and `y2`, so `dy = (y1 - y2) / 2`.
- `d2` is the sum of squares of `dx` and `dy`, so `d2 = dx * dx + dy * dy = ((x1 - x2) / 2)^2 + ((y1 - y2) / 2)^2 = (x1 - x2)^2 / 4 + (y1 - y2)^2 / 4`.

All other variables remain unchanged.