Let's break down the given initial state and the code snippet to determine what will be printed.

### Initial State:
- `u` is a non-zero value minus 2.
- The list `b` is defined as `[0, 0, y - x, y - x, y - x + v, y - x + v, y - x + v]`.
- `c` and `d` are the values returned by the function `r()`.
- There is a conditional statement that checks if `c` is less than `d`. If true, it states `c` is less than `d`; otherwise, it states `c` is greater than or equal to `d`.

### Code Snippet:
```python
print(b[c * 2 - 1] - b[d * 2 - 1])
```

### Analysis:
1. **List `b`:**
   - The list `b` contains 7 elements: `[0, 0, y - x, y - x, y - x + v, y - x + v, y - x + v]`.
   
2. **Indices Calculation:**
   - The expression `c * 2 - 1` calculates the index for the first element in the list `b`.
   - The expression `d * 2 - 1` calculates the index for the second element in the list `b`.
   
3. **Values at Indices:**
   - Since the list `b` has a specific pattern, let's map out the indices to their respective values:
     - `b[0] = 0`
     - `b[1] = 0`
     - `b[2] = y - x`
     - `b[3] = y - x`
     - `b[4] = y - x + v`
     - `b[5] = y - x + v`
     - `b[6] = y - x + v`
   
4. **Conditional Statement:**
   - The conditional statement does not affect the calculation of the print statement directly but provides context about the relationship between `c` and `d`.
   
5. **Print Statement:**
   - The print statement computes the difference between the elements at indices `c * 2 - 1` and `d * 2 - 1` in the list `b`.

### Possible Values of Indices:
- Given the list `b` has 7 elements, valid indices are from 0 to 6.
- The expressions `c * 2 - 1` and `d * 2 - 1` must yield valid indices within this range.

### Calculation of Output:
- Let's consider the possible values for `c` and `d`:
  - If `c` and `d` are such that both `c * 2 - 1` and `d * 2 - 1` are valid indices, the output will be the difference between the corresponding elements in the list `b`.

### Example Calculation:
- Suppose `c = 1` and `d = 2`:
  - `c * 2 - 1 = 1 * 2 - 1 = 1` → `b[1] = 0`
  - `d * 2 - 1 = 2 * 2 - 1 = 3` → `b[3] = y - x`
  - The print statement would output `0 - (y - x) = - (y - x) = x - y`.

### General Case:
- The output depends on the specific values of `c` and `d`, but it will always be the difference between the elements at the calculated indices in the list `b`.

### Final Output:
Given the general nature of `c` and `d` and the structure of the list `b`, the output can be described as follows:

Output: **b[c * 2 - 1] - b[d * 2 - 1] (where b is the list [0, 0, y - x, y - x, y - x + v, y - x + v, y - x + v] and c, d are values returned by r())**