To determine what will be printed, let's break down the initial conditions and how they affect the values of the variables involved.

### Step-by-Step Breakdown:

1. **Determine the Value of `ind`:**
   - If `n` is odd, `ind = 1 + n % 2 + 2 * (n - 1) = 1 + 1 + 2 * (n - 1) = 3 + 2 * (n - 1) = 2 * n - 1`.
   - If `n` is even, `ind = 1 + n % 2 + 2 * (n - 2) = 1 + 0 + 2 * (n - 2) = 2 * n - 3`.

2. **Determine the Values of `i` for Even and Odd `n`:**
   - For odd `n`, `i` starts at `n - 1` and increments by 1 until it reaches `n - 1`.
   - For even `n`, `i` starts at `n - 2` and increments by 1 until it reaches `n - 2`.

3. **Calculate the Values of `p[i]`:**
   - For each `i` from 0 to `n-2` (for even `n`) or `n-1` (for odd `n`), `p[i] = ind - 2 * i`.
   - Given the formulas for `ind` and `i`, we can substitute these into the formula for `p[i]`.

### Example Calculations:

#### Case 1: `n` is Odd
- Let's take `n = 5` as an example.
  - `ind = 2 * 5 - 1 = 9`.
  - `i` ranges from 0 to 4.
  - `p[0] = 9 - 2 * 0 = 9`.
  - `p[1] = 9 - 2 * 1 = 7`.
  - `p[2] = 9 - 2 * 2 = 5`.
  - `p[3] = 9 - 2 * 3 = 3`.
  - `p[4] = 9 - 2 * 4 = 1`.

So, `p = [9, 7, 5, 3, 1]`.

#### Case 2: `n` is Even
- Let's take `n = 6` as an example.
  - `ind = 2 * 6 - 3 = 9`.
  - `i` ranges from 0 to 4.
  - `p[0] = 9 - 2 * 0 = 9`.
  - `p[1] = 9 - 2 * 1 = 7`.
  - `p[2] = 9 - 2 * 2 = 5`.
  - `p[3] = 9 - 2 * 3 = 3`.
  - `p[4] = 9 - 2 * 4 = 1`.

So, `p = [9, 7, 5, 3, 1]`.

### Conclusion:
In both cases (whether `n` is odd or even), the resulting list `p` will be `[9, 7, 5, 3, 1]` for `n = 5` and `[9, 7, 5, 3, 1]` for `n = 6`. This pattern continues for any `n`.

### Final Output:
Output: **9 7 5 3 1**