The code snippet `g += (h + 1) // 2` updates the value of `g` by adding the result of the expression `(h + 1) // 2` to its current value. Given the initial state:

- `t` remains an integer where 1 ≤ t ≤ 5 · 10^4
- `n` and `k` are integers where 1 ≤ k ≤ n ≤ 10^9
- `s` is equal to `k` (or the maximum value it can reach without exceeding `k`)
- `i` must be at least 2
- `d` is 0 or a small positive integer (depending on the exact values of `n` and `k`)
- `h` remains `n`
- `p` remains 1
- `g` remains 0
- `k` is still greater than `(n + 1) // 2`

Let's calculate the new value of `g`:

1. `h` is equal to `n`.
2. The expression `(h + 1) // 2` simplifies to `(n + 1) // 2`.
3. Since `g` initially is 0, the new value of `g` will be `0 + (n + 1) // 2`, which simplifies to `(n + 1) // 2`.

Therefore, the updated value of `g` is `(n + 1) // 2`.

Output State: **`t` remains an integer where 1 ≤ t ≤ 5 · 10^4, `n` and `k` are integers where 1 ≤ k ≤ n ≤ 10^9, `s` is equal to `k` (or the maximum value it can reach without exceeding `k`), `i` must be at least 2, `d` is 0 or a small positive integer (depending on the exact values of `n` and `k`), `h` remains `n`, `p` remains 1, `g` is now `(n + 1) // 2`, and `k` is still greater than `(n + 1) // 2`.**