Reasoning:

1. **Understanding the Problem:**
   - The problem requires us to maximize the sum of an \( n \times n \) matrix initially filled with zeroes.
   - We can perform Type 1 and Type 2 operations, each of which involves assigning a permutation of integers from 1 to \( n \) to either a row or a column.
   - The goal is to achieve the maximum possible sum, which is \( n^3 \), and to do so using no more than \( 2n \) operations.

2. **Maximum Sum Calculation:**
   - The maximum sum of the matrix is indeed \( n^3 \), as each cell can be filled with the maximum value \( n \), and there are \( n^2 \) cells in total.

3. **Operations to Achieve the Maximum Sum:**
   - To achieve the maximum sum, we need to fill each row and each column with the permutation \( [1, 2, \ldots, n] \).
   - This can be done by performing \( n \) Type 1 operations (one for each row) and \( n \) Type 2 operations (one for each column), totaling \( 2n \) operations.

4. **Analyzing the Given Program:**
   - The program reads the number of test cases \( t \).
   - For each test case, it reads the size of the matrix \( n \).
   - It calculates the sum using the formula \( \text{sum} = 1 + \sum_{i=2}^{n} (i^2 - (i-1)^2) \times i \).
   - It prints the sum and \( 2n \) as the number of operations.
   - It then prints \( n \) Type 1 operations and \( n \) Type 2 operations, each using the permutation \( [1, 2, \ldots, n] \).

5. **Correctness of the Sum Calculation:**
   - The formula used in the program is \( \text{sum} = 1 + \sum_{i=2}^{n} (i^2 - (i-1)^2) \times i \).
   - Simplifying the term inside the sum:
     \[
     i^2 - (i-1)^2 = i^2 - (i^2 - 2i + 1) = 2i - 1
     \]
   - Therefore, the sum becomes:
     \[
     \text{sum} = 1 + \sum_{i=2}^{n} (2i - 1) \times i
     \]
   - This can be further simplified to:
     \[
     \text{sum} = 1 + \sum_{i=2}^{n} (2i^2 - i)
     \]
   - The sum of \( 2i^2 \) from \( i=2 \) to \( n \) is:
     \[
     2 \sum_{i=2}^{n} i^2 = 2 \left( \sum_{i=1}^{n} i^2 - 1 \right) = 2 \left( \frac{n(n+1)(2n+1)}{6} - 1 \right)
     \]
   - The sum of \( i \) from \( i=2 \) to \( n \) is:
     \[
     \sum_{i=2}^{n} i = \sum_{i=1}^{n} i - 1 = \frac{n(n+1)}{2} - 1
     \]
   - Combining these, the sum becomes:
     \[
     \text{sum} = 1 + 2 \left( \frac{n(n+1)(2n+1)}{6} - 1 \right) - \left( \frac{n(n+1)}{2} - 1 \right)
     \]
   - Simplifying further:
     \[
     \text{sum} = 1 + \frac{n(n+1)(2n+1)}{3} - 2 - \frac{n(n+1)}{2} + 1 = \frac{n(n+1)(2n+1)}{3} - \frac{n(n+1)}{2}
     \]
   - This is not equal to \( n^3 \), which is the correct maximum sum.

6. **Correctness of the Operations:**
   - The program correctly prints \( 2n \) operations, each using the permutation \( [1, 2, \ldots, n] \).
   - However, the sum calculation is incorrect, which means the program does not correctly compute the maximum sum.

Conclusion:
The program is incorrect because the sum calculation does not match the expected maximum sum \( n^3 \).

Final: **False**