Based on the initial state provided:

- `i` is set to `m-1`
- `k` is greater than 0
- `u` is an integer entered by the user
- `v` is an integer entered by the user
- `f` is an integer entered by the user
- `a` is the sum of all `f` values entered over the course of the loop's iterations
- `s` is the sum of `c * i * c * m + c * a` for each `i` from 0 to `m-1`

The expression for `s` is:
\[ s = \sum_{i=0}^{m-1} (c \cdot i \cdot c \cdot m + c \cdot a) \]

This simplifies to:
\[ s = \sum_{i=0}^{m-1} (c^2 \cdot i \cdot m + c \cdot a) \]
\[ s = c^2 \cdot m \cdot \sum_{i=0}^{m-1} i + c \cdot a \cdot m \]

The sum of the first `m-1` integers is:
\[ \sum_{i=0}^{m-1} i = \frac{(m-1)m}{2} \]

So,
\[ s = c^2 \cdot m \cdot \frac{(m-1)m}{2} + c \cdot a \cdot m \]
\[ s = \frac{c^2 \cdot m^2 \cdot (m-1)}{2} + c \cdot a \cdot m \]

Finally, the expression to be printed is `s % M`, which means the remainder when `s` is divided by `M`.

Output: **(c^2 * m^2 * (m-1) / 2 + c * a * m) % M**