Let's break down the initial state and the calculation step-by-step:

1. **Initial Values:**
   - `t` is 0.
   - `n` is an integer converted from input.
   - `m` is an integer converted from input.
   - `ans` is initialized to `n + 1 + (n + 3) // 9 + (n + 4) // 16 + (n + 5) // 25 + ... + (n + min(n, m)) // (min(n, m) * min(n, m))`.

2. **Loop Calculation:**
   - The loop starts with `b = min(n, m) + 1` and increments `b` by 1 in each iteration.
   - The loop runs until `b` exceeds `min(n, m)`.
   - In each iteration, `ans` is updated by adding `(n + b) // (b * b)` to it.

Given that `min(n, m) >= 2`, let's assume the smallest possible values for `n` and `m` to simplify the explanation. Let's assume `n = 2` and `m = 3` (since `min(n, m) >= 2`).

- **Initialization:**
  - `ans = 2 + 1 + (2 + 3) // 9 + (2 + 4) // 16 + (2 + 5) // 25 + (2 + 6) // 36`
  - Simplifying the expression:
    - `ans = 3 + 5 // 9 + 6 // 16 + 7 // 25 + 8 // 36`
    - Since all divisions result in 0 (as the numerators are less than the denominators):
      - `ans = 3 + 0 + 0 + 0 + 0 = 3`

- **Loop Execution:**
  - `b` starts at `min(2, 3) + 1 = 3`.
  - The loop runs until `b` exceeds `3`.
  - For `b = 3`:
    - `ans += (2 + 3) // (3 * 3) = 5 // 9 = 0`
  - For `b = 4`:
    - `ans += (2 + 4) // (4 * 4) = 6 // 16 = 0`
  - For `b = 5`:
    - `ans += (2 + 5) // (5 * 5) = 7 // 25 = 0`
  - For `b = 6`:
    - `ans += (2 + 6) // (6 * 6) = 8 // 36 = 0`

Since all additions in the loop result in 0, `ans` remains 3.

Therefore, the final value of `ans` is 3.

Output: **3**