To determine what will be printed, let's break down the given initial state and the Python code snippet step by step.

### Initial State Breakdown:

1. **Variable `i`**:
   - `i` is defined as `b + 1`.

2. **Variable `suma`**:
   - `suma` is the sum of all `x` values where the condition `a - i * (i - 1) > 0` holds true for `i` ranging from 1 to `b`.
   - Here, `x` is not explicitly defined in the problem statement, but it seems to be the same as `i` in the context of the summation, as no other variable `x` is mentioned. Therefore, we assume `x = i`.

### Calculation of `suma`:

- We need to sum up all `i` values from 1 to `b` such that `a - i * (i - 1) > 0`.
- This means for each `i` from 1 to `b`, we check if `a - i * (i - 1) > 0`. If true, we add `i` to `suma`.

### Example Calculation:

Let's consider an example to make this clearer. Suppose `a = 10` and `b = 4`.

- For `i = 1`: `a - i * (i - 1) = 10 - 1 * 0 = 10 > 0` → Add 1 to `suma`.
- For `i = 2`: `a - i * (i - 1) = 10 - 2 * 1 = 8 > 0` → Add 2 to `suma`.
- For `i = 3`: `a - i * (i - 1) = 10 - 3 * 2 = 4 > 0` → Add 3 to `suma`.
- For `i = 4`: `a - i * (i - 1) = 10 - 4 * 3 = -2 < 0` → Do not add 4 to `suma`.

So, `suma = 1 + 2 + 3 = 6`.

### Final Calculation:

The code snippet then prints `suma - 1`.

- Continuing with our example, `suma - 1 = 6 - 1 = 5`.

### General Case:

Given the general case, `suma` is the sum of all `i` values from 1 to `b` that satisfy the condition `a - i * (i - 1) > 0`. The final output will be `suma - 1`.

### Conclusion:

Output: **suma - 1 (where suma is the sum of all i values from 1 to b such that a - i * (i - 1) > 0)**