To determine what will be printed by the given Python code snippet, let's break down the initial state and the operations step by step:

### Initial State:
- `t` must be greater than 0.
- `i` is 0.
- `a`, `b`, and `m` are input integers.
- `mn` is the minimum of `a` and `b` plus `m`.
- `m` is divisible by both `a` and `b`.
- Neither `a` nor `b` is equal to 1.

### Code Snippet:
```python
print(mn // a + mn // b + 1)
```

### Step-by-Step Analysis:
1. **Determine `mn`**:
   - `mn` is defined as the minimum of `a` and `b` plus `m`.
   - Let's denote the minimum of `a` and `b` as `min(a, b)`.
   - Therefore, `mn = min(a, b) + m`.

2. **Divisibility Condition**:
   - `m` is divisible by both `a` and `b`.
   - This means `m % a == 0` and `m % b == 0`.

3. **Calculate `mn // a` and `mn // b`**:
   - `mn // a` is the integer division of `mn` by `a`.
   - `mn // b` is the integer division of `mn` by `b`.

4. **Sum and Add 1**:
   - The expression inside the `print` statement is `mn // a + mn // b + 1`.

### Simplifying the Expression:
- Since `m` is divisible by both `a` and `b`, we can write `m = k * a` and `m = l * b` for some integers `k` and `l`.
- Let's assume without loss of generality that `a <= b` (since `mn` uses the minimum of `a` and `b`).
- Then `mn = a + m`.

5. **Substitute `m`**:
   - If `m = k * a`, then `mn = a + k * a = (k + 1) * a`.
   - Similarly, if `m = l * b`, then `mn = b + l * b = (l + 1) * b`.

6. **Calculate Integer Divisions**:
   - `mn // a = ((k + 1) * a) // a = k + 1`.
   - `mn // b = ((l + 1) * b) // b = l + 1`.

7. **Sum and Add 1**:
   - The expression becomes `(k + 1) + (l + 1) + 1 = k + l + 3`.

### Final Output:
- The value printed will be `k + l + 3`, where `k` and `l` are the integers such that `m = k * a` and `m = l * b`.

However, since the exact values of `k` and `l` are not provided, we can only express the output in terms of these variables.

Output: **k + l + 3 (where k and l are integers such that m = k * a and m = l * b)**