The code updates the value of `right_product[i]` to be the product of `right_product[i + 1]` and `cards[i]`. Here, `i` is `n-1`, so the equation becomes `right_product[n-1] = right_product[n] * cards[n-1]`. Since `right_product[n]` is initially set to 1, the new value of `right_product[n-1]` is simply `cards[n-1]`.

The initial state of `right_product` is a list of `n + 1` elements, each set to 1. After the assignment, the first element (at index `n-1`) of `right_product` is updated to `cards[n-1]`, while the rest of the list remains unchanged.

Output State: **`n` is a positive integer such that \(1 \leq n \leq 100,000\), `k` is a positive integer such that \(1 \leq k \leq 10^9\), `cards` is a list of `n` positive integers such that \(1 \leq a_i \leq 10^9\) for all `i`, `total_product` is the product of all elements in `cards`, `right_product` is a list of `n + 1` elements where the first element is `cards[n-1]` and the rest are 1, and `i` is equal to `n-1`.**