Reasoning:  
The given program defines a function `func_1` that calculates the difference between the sum of cubes of the first `n` natural numbers and the sum of the first `n` natural numbers. Let's break down the steps:

1. **Sum of the First `n` Natural Numbers (`sum_n`)**:
   The formula for the sum of the first `n` natural numbers is:
   \[
   \text{sum\_n} = \frac{n \times (n + 1)}{2}
   \]
   This is correctly implemented in the function as:
   ```python
   sum_n = n * (n + 1) // 2
   ```

2. **Sum of Cubes of the First `n` Natural Numbers (`sum_cubes_n`)**:
   The sum of the cubes of the first `n` natural numbers is given by the square of the sum of the first `n` natural numbers:
   \[
   \text{sum\_cubes\_n} = \left(\frac{n \times (n + 1)}{2}\right)^2
   \]
   This is also correctly implemented in the function as:
   ```python
   sum_cubes_n = sum_n ** 2
   ```

3. **Difference Calculation**:
   The function then returns the difference between `sum_cubes_n` and `sum_n`:
   ```python
   return sum_cubes_n - sum_n
   ```

Let's verify the test cases:
- For `n = 3`:
  \[
  \text{sum\_n} = \frac{3 \times 4}{2} = 6
  \]
  \[
  \text{sum\_cubes\_n} = 6^2 = 36
  \]
  \[
  \text{result} = 36 - 6 = 30
  \]
  This matches the test case `func_1(3) == 30`.

- For `n = 5`:
  \[
  \text{sum\_n} = \frac{5 \times 6}{2} = 15
  \]
  \[
  \text{sum\_cubes\_n} = 15^2 = 225
  \]
  \[
  \text{result} = 225 - 15 = 210
  \]
  This matches the test case `func_1(5) == 210`.

- For `n = 2`:
  \[
  \text{sum\_n} = \frac{2 \times 3}{2} = 3
  \]
  \[
  \text{sum\_cubes\_n} = 3^2 = 9
  \]
  \[
  \text{result} = 9 - 3 = 6
  \]
  This matches the test case `func_1(2) == 6`.

Since all the test cases are correct and the logic of the function is sound, the program is correct.

Correctness: **True**