Let's break down the initial state and the provided Python code snippet step by step to determine what will be printed.

### Initial State Breakdown:
1. **`t`**: Must be greater than 0.
2. **`n`**: Is 0.
3. **`k`**: Is an input integer that must be at least 1.
4. **`L`**: Is a list containing the sequence of values `[m1, m2, ..., mk]` where each `mi` is the value of `(ni + 1) // 2` for the corresponding iteration, and `ni` is the value of `n` at the start of each iteration.
5. **`tot`**: Is `a + a`, where `a` is the third element in `L`.
6. **`pow`**: Is 4.
7. **`a`**: Is the third element in `L`.

### Step-by-Step Calculation:
1. **Determine the values of `L`**:
   - Since `n` starts at 0 and each `mi` is `(ni + 1) // 2`, let's calculate the first few elements of `L`:
     - For `i = 0`: `m1 = (0 + 1) // 2 = 0`
     - For `i = 1`: `m2 = (0 + 1) // 2 = 0`
     - For `i = 2`: `m3 = (0 + 1) // 2 = 0`
   - Therefore, `L = [0, 0, 0, ...]` (assuming `k` is at least 3).

2. **Determine the value of `a`**:
   - `a` is the third element in `L`, which is `0`.

3. **Determine the value of `tot`**:
   - `tot = a + a = 0 + 0 = 0`.

4. **Check the postcondition**:
   - The postcondition states that if `tot < k` and `k <= tot + a`, then the postcondition remains unchanged.
   - Given `tot = 0` and `a = 0`, the conditions become:
     - `0 < k` (which is true since `k` is at least 1).
     - `k <= 0 + 0` (which simplifies to `k <= 0`).
   - Since `k` must be at least 1, the condition `k <= 0` is false. Therefore, the postcondition does not apply, and we proceed with the given values.

5. **Calculate the expression in the `print` statement**:
   - The expression is `pow * (2 * (k - tot) - 1)`.
   - Substituting the known values:
     - `pow = 4`
     - `tot = 0`
     - The expression becomes: `4 * (2 * (k - 0) - 1) = 4 * (2 * k - 1) = 4 * (2k - 1) = 8k - 4`.

### Final Output:
The `print` statement will output the value of the expression `8k - 4`.

Output: **8k - 4 (where k is the input integer)**