Let's analyze the given code step by step:

1. **Initial State**: 
   - `a` is an integer such that \(1 \leq a \leq n \cdot m \cdot k\)
   - `b` is an integer such that \(1 \leq b \leq n \cdot m \cdot k\) and `a ≠ b`
   - `m` is a positive integer between 1 and 1000
   - `a_floor` is `(a - 1) % m + 1`

2. **Code Execution**:
   - The code assigns a new value to `a_block` using the formula: `a_block = (a - 1) // (m * k) + 1`

   Let's break down the formula:
   - `(a - 1)` computes `a - 1`.
   - `// (m * k)` performs integer division by `m * k`.
   - `+ 1` adds 1 to the result.

   Therefore, `a_block` is calculated as:
   \[
   a_block = \left(\frac{a - 1}{m \cdot k}\right) + 1
   \]

3. **Impact on Variables**:
   - `a_floor` remains unchanged as it was defined earlier and its value does not depend on the calculation of `a_block`.
   - `a` and `b` remain unchanged as they are not modified in the given code.
   - `m` remains unchanged as it is a constant in this context.
   - `a_block` is the newly computed value based on the formula.

4. **Output State**:
   - `a` is unchanged: \(1 \leq a \leq n \cdot m \cdot k\)
   - `b` is unchanged: \(1 \leq b \leq n \cdot m \cdot k\) and `a ≠ b`
   - `m` is unchanged: \(1 \leq m \leq 1000\)
   - `a_floor` is unchanged: `a_floor = (a - 1) % m + 1`
   - `a_block` is the new value computed as \(\left(\frac{a - 1}{m \cdot k}\right) + 1\)

Output State: **`a` is an integer such that \(1 \leq a \leq n \cdot m \cdot k\); `b` is an integer such that \(1 \leq b \leq n \cdot m \cdot k\) and `a ≠ b`; `m` is a positive integer between 1 and 1000; `a_floor` is \((a - 1) \% m + 1\); `a_block` is \(\left(\frac{a - 1}{m \cdot k}\right) + 1\)**