Given the initial state and the provided Python code snippet, let's determine the output state.

Initial State:
- `t` is an integer such that 1 <= t <= 500.
- `cas_de_test` is a list of tuples where each tuple contains three integers (p_1, p_2, p_3) such that 0 <= p_1 <= p_2 <= p_3 <= 30, and `cas_de_test` must contain at least one tuple.
- If `total_points` (which is the sum of the first tuple in `cas_de_test`) is odd, `resultats` is a list containing the elements [-1, -1] if `total_matchs > 3 or p3 > total_matchs` is true, otherwise `resultats` is a list containing the element [-1].
- `total_matchs` is `total_points // 2`.

Code Snippet:
```python
egalites = total_points - 2 * (p3 - p2) - 2 * (p3 - p1)
```

Impact of the Code:
- The variable `egalites` is calculated using the formula provided in the code snippet.
- `total_points` is the sum of the first tuple in `cas_de_test`.
- `p1`, `p2`, and `p3` are the elements of the first tuple in `cas_de_test`.

Let's denote the first tuple in `cas_de_test` as `(p1, p2, p3)`. Therefore, `total_points = p1 + p2 + p3`.

The calculation for `egalites` becomes:
\[ \text{egalites} = (p1 + p2 + p3) - 2 \times (p3 - p2) - 2 \times (p3 - p1) \]
\[ \text{egalites} = p1 + p2 + p3 - 2p3 + 2p2 - 2p3 + 2p1 \]
\[ \text{egalites} = 3p1 + 3p2 - 3p3 \]
\[ \text{egalites} = 3 \times (p1 + p2 - p3) \]

Since the values of `p1`, `p2`, and `p3` are part of the initial state and are not modified by the code, `egalites` is now defined as `3 * (p1 + p2 - p3)`.

Output State: **`t` is an integer such that 1 <= t <= 500, `cas_de_test` is a list of tuples where each tuple contains three integers (p_1, p_2, p_3) such that 0 <= p_1 <= p_2 <= p_3 <= 30, and `cas_de_test` must contain at least one tuple. If `total_points` (which is the sum of the first tuple in `cas_de_test`) is odd, `resultats` is a list containing the elements [-1, -1] if `total_matchs > 3 or p3 > total_matchs` is true, otherwise `resultats` is a list containing the element [-1]. `total_matchs` is `total_points // 2`. `egalites` is `3 * (p1 + p2 - p3)` where `(p1, p2, p3)` is the first tuple in `cas_de_test`.**