The code snippet `current_sum += a[i]` updates the value of `current_sum` by adding the value of `a[i]` to it. Given the initial state:

- `n` is a positive integer such that \(1 \leq n \leq 3 \times 10^5\)
- `i` is 1
- `m` is a positive integer such that \(1 \leq m \leq 10\)
- `k` is a positive integer such that \(1 \leq k \leq 10^9\)
- `a` is a list of `n` integers where each integer \(a_i\) satisfies \(-10^9 \leq a_i \leq 10^9\)
- `current_sum` is \(a[0]\)
- If `i + 1 >= m`, `current_cost` is \(a[0] - k\)
- `max_cost` is \(max(0, a[0] - k)\)
- `min_prefix` is \(min(0, a[0] - k)\)

After executing the code snippet, the value of `current_sum` is updated to `a[0] + a[1]`. The other variables remain unchanged.

Output State: **`n` is a positive integer such that \(1 \leq n \leq 3 \times 10^5\), `i` is 1, `m` is a positive integer such that \(1 \leq m \leq 10\), `k` is a positive integer such that \(1 \leq k \leq 10^9\), `a` is a list of `n` integers where each integer \(a_i\) satisfies \(-10^9 \leq a_i \leq 10^9\), `current_sum` is \(a[0] + a[1]\), if `i + 1 >= m`, `current_cost` is \(a[0] - k\), `max_cost` is \(max(0, a[0] - k)\), and `min_prefix` is \(min(0, a[0] - k)\)**