The code updates the value of `_acc` by adding the value of `_acc + _max` modulo `MOD`. Given that `_acc` is initially equal to `(_max % 10 + _max) % 10`, let's calculate the new value of `_acc`.

First, let's denote `_max` as `M` and `_acc` as `A`. The initial value of `_acc` is \( A = (M \mod 10 + M) \mod 10 \).

The updated value of `_acc` is:
\[ A_{\text{new}} = (A + M) \mod 10 \]

Substituting \( A = (M \mod 10 + M) \mod 10 \) into the equation:
\[ A_{\text{new}} = ((M \mod 10 + M) \mod 10 + M) \mod 10 \]

Since \( (a + b) \mod c = ((a \mod c) + (b \mod c)) \mod c \):
\[ A_{\text{new}} = ((M \mod 10 + M) \mod 10 + M) \mod 10 = ((M \mod 10 + M) \mod 10 + M) \mod 10 \]

This simplifies to:
\[ A_{\text{new}} = (2M \mod 10 + M \mod 10) \mod 10 \]
\[ A_{\text{new}} = (2M + M \mod 10) \mod 10 \]

Given that `MOD` is 10, the final value of `_acc` is:
\[ A_{\text{new}} = (2M + M \mod 10) \mod 10 \]

Therefore, the updated values are:
- `_acc` is now \((2M + M \mod 10) \mod 10\)
- `_max` remains unchanged as `M`
- `i` is 2 (unchanged)

Output State: **`_sum` is the maximum cumulative sum starting from 0 and considering each element of `a` up to index `n-1`, `_max` is the maximum value of `_sum` across all iterations of the loop, `n` is the number of iterations (which is the same as the length of the list `a` up to the n-th index), `k` is greater than or equal to 2, `t` is the original value read from the standard input, `a` is a list of integers where each element satisfies \(-10^9 \leq a_i \leq 10^9\), `MOD` is 10, `_acc` is \((2M + M \mod 10) \mod 10\), `i` is 2**