The code `k -= u` subtracts the value of `u` from `k`. Given the initial conditions, `u` can either be the new last element of `lit` (if `lastState == -1`) or the second element of `lit` (if `lastState == 0`). After executing this line of code, the value of `k` will be updated by subtracting `u` from its previous value. The other variables remain unchanged.

Since `u` is defined differently based on `lastState`, we need to consider both cases:

1. If `lastState == -1`, then `u` is the new last element of `lit`.
2. If `lastState == 0`, then `u` is the second element of `lit`.

In either case, the value of `k` is updated by subtracting `u` from its previous value. The other variables (`t`, `a`, `n`, `lit`, `sunk`, and `lastState`) remain in their initial or described states.

Therefore, the output state is:
Output State: **`t` is a positive integer, `a` is an empty list, `n` is an input integer, `lit` is either a list or a deque with one less element than before, `sunk` is incremented by 1, `lastState` is either `0` or `-1` depending on whether the `if` condition (`lastState == -1`) is true or false, and `k` is updated by subtracting `u` from its previous value.**