The code snippet `sum += (i * i - (i - 1) * (i - 1)) * i` updates the value of `sum` based on the current values of `i` and `n`. Let's break down the impact:

1. **Initial Values**:
   - `t` must be greater than 1.
   - `n` is an input integer and must be greater than or equal to 2.
   - `sum` is 1.
   - `i` is 2.
   - `j` is `n`.

2. **Calculation**:
   - The expression `(i * i - (i - 1) * (i - 1)) * i` is evaluated.
   - `i * i` is `2 * 2 = 4`.
   - `(i - 1) * (i - 1)` is `1 * 1 = 1`.
   - `4 - 1 = 3`.
   - `3 * i` is `3 * 2 = 6`.
   - `sum` is updated by adding 6 to its current value: `sum += 6`.

3. **Final Values**:
   - `sum` is now `1 + 6 = 7`.
   - The values of `t`, `n`, `i`, and `j` remain unchanged.

Output State: **`t` must be greater than 1, `n` is an input integer and must be greater than or equal to 2, `sum` is 7, `i` is 2, `j` is `n`.**