The code snippet `sum += (i * i - (i - 1) * (i - 1)) * i` updates the value of `sum` by adding the result of the expression `(i * i - (i - 1) * (i - 1)) * i` to the current value of `sum`.

Initial State:
- `t` must be greater than 0
- `n` must be greater than or equal to 3
- `sum` is 1 + (2 * 2 - 1 * 1) * 2 = 1 + (4 - 1) * 2 = 1 + 3 * 2 = 1 + 6 = 7
- `i` is 3
- `j` is \(\text{previous\_n}\)

Step-by-step calculation:
1. Calculate the expression `(i * i - (i - 1) * (i - 1)) * i`:
   - `i * i` is 3 * 3 = 9
   - `(i - 1) * (i - 1)` is (3 - 1) * (3 - 1) = 2 * 2 = 4
   - `i * i - (i - 1) * (i - 1)` is 9 - 4 = 5
   - `(i * i - (i - 1) * (i - 1)) * i` is 5 * 3 = 15

2. Update `sum`:
   - `sum` was initially 7
   - `sum` is now 7 + 15 = 22

Output State: **`t` must be greater than 0, `n` must be greater than or equal to 3, `sum` is 22, `i` is 3, `j` is \(\text{previous\_n}\)**.