The code snippet `ans += dp[step - prev]` increments the value of `ans` by the value of `dp[step - prev]`. To determine the exact value added to `ans`, we need to evaluate `dp[step - prev]`.

Given the initial state:
- `prev` is 2
- `ans` is updated based on the condition `step - prev >= 0` and `dp[step - prev] >= 0` from the previous iteration.

### Step-by-Step Calculation:
1. **Calculate `step - prev`:**
   - `prev` is 2.
   - `step - prev` is `step - 2`.

2. **Check the condition:**
   - The condition `step - prev >= 0` simplifies to `step - 2 >= 0`, which means `step >= 2`.
   - The condition `dp[step - prev] >= 0` simplifies to `dp[step - 2] >= 0`.

3. **Update `ans`:**
   - If both conditions are met (`step >= 2` and `dp[step - 2] >= 0`), then `ans` is incremented by `dp[step - 2]`.
   - If the conditions are not met, `ans` retains its value.

### Output State:
- If `step >= 2` and `dp[step - 2] >= 0`, then `ans` is incremented by `dp[step - 2]`.
- Otherwise, `ans` retains its value.

Therefore, the output state is:
Output State: **`N`, `M`, `n`, `m`, `a`, `dp`, `i`, `step`, `prev` is 2, `ans` is incremented by `dp[step - 2]` if `step >= 2` and `dp[step - 2] >= 0`, otherwise `ans` retains its value.**