Output State: **`t` is `initial t - 2 * k`, `n` remains unchanged, `k` is 0, `num` is 0, `i` is 4, `m` is at least 3, `dp` is a list containing elements 0, 1, and the third element dp[2] is 5, `dp[4]` is 14.**

Explanation: 
- Initially, `dp` is a list with elements `[0, 1, 5]`.
- The code updates `dp[i]` where `i` is 4.
- The formula used is `dp[i] = (dp[i - 1] + (i - 1) * dp[i - 2] * 2) % (10 ** 9 + 7)`.
- Substituting the values, we get `dp[4] = (dp[3] + 3 * dp[2] * 2) % (10 ** 9 + 7)`.
- Since `dp[3]` is 0 (as the list only has three elements initially), the equation simplifies to `dp[4] = (0 + 3 * 5 * 2) % (10 ** 9 + 7) = 30 % (10 ** 9 + 7) = 30`.
- All other variables remain unchanged.