The code snippet `y -= (a[i] - a[i - 1]) // 2 - 1` updates the value of `y` by subtracting the result of the expression `(a[i] - a[i - 1]) // 2 - 1` from its current value. Let's break down the impact:

1. **Initial Values:**
   - `t` is an integer where 1 ≤ t ≤ 10^4.
   - `n` is the first input integer (4 ≤ n ≤ 10^9).
   - `x` is the second input integer (2 ≤ x ≤ min(n, 2 * 10^5)).
   - `y` is the third input integer (0 ≤ y ≤ n - x).
   - `a` is a sorted list of integers read from the input with at least 3 elements.
   - `i` is 3.
   - `tmp` is a list containing one element which is `(a[3] - a[2]) // 2`.
   - `ans` is increased by `(a[3] - a[2]) // 2`.

2. **Expression Calculation:**
   - `a[i]` is `a[3]`.
   - `a[i - 1]` is `a[2]`.
   - The expression `(a[3] - a[2]) // 2 - 1` calculates the difference between `a[3]` and `a[2]`, divides it by 2, and then subtracts 1.

3. **Update `y`:**
   - `y` is updated by subtracting the result of the expression from its current value.

Let's denote the value of `a[3] - a[2]` as `diff`. The expression becomes `(diff // 2) - 1`.

Therefore, the new value of `y` is:
\[ y = y - \left( \frac{a[3] - a[2]}{2} - 1 \right) \]

The rest of the variables remain unchanged.

Output State: **`t` is an integer where 1 ≤ t ≤ 10^4, `n` is the first input integer (4 ≤ n ≤ 10^9), `x` is the second input integer (2 ≤ x ≤ min(n, 2 * 10^5)), `y` is updated to `y - ((a[3] - a[2]) // 2 - 1)`, `a` is a sorted list of integers read from the input with at least 3 elements, `i` is 3, `tmp` is a list containing one element which is `(a[3] - a[2]) // 2`, `ans` is increased by `(a[3] - a[2]) // 2`.**