Given the initial state:
- `t` is an input integer such that 1 ≤ `t` ≤ 5 · 10^4
- `n` must be at least 2
- `k` is an input integer
- `L` is a list containing two elements `[m, m]`
- `m` is `(n + 1) // 2`

The code snippet is:
```python
n -= m
```

This operation reduces the value of `n` by `m`. Since `m` is `(n + 1) // 2`, we can substitute this into the equation to find the new value of `n`.

Let's calculate the new value of `n`:
- `m = (n + 1) // 2`
- `n -= m` implies `n = n - m`
- Substituting `m`: `n = n - (n + 1) // 2`

If `n` is even, `(n + 1) // 2` is equivalent to `n / 2` rounded down, which is `n / 2`.
If `n` is odd, `(n + 1) // 2` is equivalent to `(n + 1) / 2` rounded down, which is `(n + 1) / 2`.

Thus, the new value of `n` depends on whether `n` was initially even or odd.

However, without knowing the exact value of `n`, we can express the new value of `n` in terms of its original value:
- If `n` is even: `n = n - n/2 = n/2`
- If `n` is odd: `n = n - (n+1)/2 = (2n - n - 1) / 2 = (n - 1) / 2`

Since the exact parity of `n` is not specified, we can describe the new value of `n` as `n - (n + 1) // 2`.

The other variables (`t`, `k`, `L`, and `m`) remain unchanged.

Output State: **`t` is an input integer such that 1 ≤ `t` ≤ 5 · 10^4; `n` is `n - (n + 1) // 2`; `k` is an input integer; `L` is a list containing two elements `[m, m]`; `m` is `(n + 1) // 2`**