The code snippet `ans[i + 1] += ans[i]` increments the value of `ans[i + 1]` by the value of `ans[i]`. Given the initial state, we know the values of `ans[0]`, `ans[1]`, and `ans[2]`, and all other elements in `ans` are 0 initially.

Let's calculate the new value of `ans[i + 1]` based on the provided initial state.

Initial State Recap:
- `arr` is a list of integers where each integer \( x_i \) satisfies \( 1 \leq x_i \leq 500 \).
- `n` is an integer such that \( 3 \leq n \leq 500 \).
- `ans[0]` is `arr[0] + 1`.
- `ans[1]` is `2 * arr[0] + 1`.
- `ans[2]` is `2 * arr[0] + 1`.
- The rest of the elements in `ans` are 0.

Given the code `ans[i + 1] += ans[i]`, let's assume `i` is 1 (as it will be the first iteration where `ans[i + 1]` is not 0, and it makes sense in the context of the provided initial state).

So, `ans[2] += ans[1]` translates to `ans[2] = ans[2] + ans[1]`.

Since `ans[2]` is initially `2 * arr[0] + 1` and `ans[1]` is `2 * arr[0] + 1`, the new value of `ans[2]` will be:
\[ \text{new } ans[2] = (2 * arr[0] + 1) + (2 * arr[0] + 1) = 4 * arr[0] + 2 \]

Output State: **`arr` is a list of integers where each integer \( x_i \) satisfies \( 1 \leq x_i \leq 500 \), `n` is an integer such that \( 3 \leq n \leq 500 \), `ans[0]` is `arr[0] + 1`, `ans[1]` is `2 * arr[0] + 1`, `ans[2]` is `4 * arr[0] + 2`, and the rest of the elements in `ans` are 0.**