The given code snippet modifies the value of `ans[i + 1]` by adding `ans[i]` to it. 

Initial State: 
- `arr` is a list of integers where each integer \( x_i \) satisfies \( 1 \leq x_i \leq 500 \).
- `n` is an integer such that \( 3 \leq n \leq 500 \).
- `ans` is a list of integers where `ans[i + 1]` is now `arr[i] + 2 * ans[i]`, `i` is `k + 1`, `ans[k + 1]` is 0, and `arr[k + 2]` is at least `arr[k + 1]`.

The code snippet provided is:
```
ans[i + 1] += ans[i]
```

This modifies `ans[i + 1]` to be `ans[i + 1] + ans[i]`. Since `ans[i + 1]` was initially `arr[i] + 2 * ans[i]`, after the operation, `ans[i + 1]` becomes `arr[i] + 2 * ans[i] + ans[i]`, which simplifies to `arr[i] + 3 * ans[i]`.

Therefore, the Output State is:
Output State: **`arr` is a list of integers where each integer \( x_i \) satisfies \( 1 \leq x_i \leq 500 \); `n` is an integer such that \( 3 \leq n \leq 500 \); `ans` is a list of integers where `ans[i + 1]` is now `arr[i] + 3 * ans[i]`, `i` is `k + 1`, `ans[k + 1]` is 0, and `arr[k + 2]` is at least `arr[k + 1]`.**