Let's go through the steps:

1. Initial State:
   - `m` is an integer such that \(1 \leq m \leq 10^9\)
   - `a` is an integer such that \(1 \leq a \leq 10^5\)
   - `b` is an integer such that \(1 \leq b \leq 10^5\)
   - `g` is equal to 1
   - `k` is `a + b - 1`
   - `sum_k` is \((a + b - 1) * (a + b) // 2\)

2. Code Execution:
   - The code assigns `sum_m` the value of `m * (m + 1) // 2 - k * (k - 1) // 2`.
   - `m * (m + 1) // 2` is the sum of the first `m` integers.
   - `k * (k - 1) // 2` is the sum of the first `k` integers, where `k = a + b - 1`.

3. Calculating the Impact:
   - `sum_m = m * (m + 1) // 2 - k * (k - 1) // 2`
   - Since `k = a + b - 1`, substitute `k` into the equation:
     - `sum_m = m * (m + 1) // 2 - (a + b - 1) * (a + b - 2) // 2`

The output state will include the updated value of `sum_m` along with the unchanged values of `m`, `a`, `b`, `g`, `k`, and `sum_k`.

Output State: **`m` is an integer such that \(1 \leq m \leq 10^9\), `a` is an integer such that \(1 \leq a \leq 10^5\), `b` is an integer such that \(1 \leq b \leq 10^5\), `g` is equal to 1, `k` is `a + b - 1`, `sum_k` is \((a + b - 1) * (a + b) // 2`, `sum_m` is `m * (m + 1) // 2 - (a + b - 1) * (a + b - 2) // 2**