Alright, I have this problem to solve. Let's see what it's about. So, Nikita has some cubes, and he wants to build a tower using these cubes. He can either add one cube on top of the tower or remove one cube from the top in each move. The question is, after a certain number of moves, can he end up with exactly m cubes in the tower?

Okay, so the input consists of multiple test cases. The first line is t, which is the number of test cases. Then, for each test case, there are two integers, n and m, where n is the number of moves and m is the desired number of cubes in the tower at the end.

I need to determine, for each test case, whether it's possible to achieve exactly m cubes in the tower after n moves.

Let me think about how the tower evolves with each move.

Initially, the tower has 0 cubes.

Each move can be either:

1. Add one cube on top.

2. Remove one cube from the top.

Important points:

- You can only remove a cube if there is at least one cube in the tower.

- Moves are sequential.

I need to find out if, after n such moves, the tower can have exactly m cubes.

Let's consider some examples to understand the problem better.

Example 1:

Input:

3

3 3

2 4

5 3

Output:

Yes

No

Yes

Let's see why:

First test case: n=3, m=3

Possible sequence:

Add, Add, Add → 3 cubes

So, "Yes"

Second test case: n=2, m=4

Possible sequences:

Add, Add → 2 cubes

Add, Remove → 1 cube

Remove, Add → If there's no cube initially, Remove can't be done. So, only Add, Add is possible, leading to 2 cubes.

So, can't get 4 cubes with only 2 moves. Hence, "No"

Wait, but according to the note, it's possible to have 0 or 2 cubes, but not 4. Maybe I misread.

Wait, with n=2, m=4, it's impossible because you can't have more than n cubes if you only add cubes, which would be n cubes maximum.

But in the first test case, n=3, m=3 is possible by adding three times.

Third test case: n=5, m=3

Possible sequence:

Add, Add, Add, Add, Remove → 4 cubes

Add, Add, Add, Remove, Add → 4 cubes

Wait, but the output is "Yes", so there must be a sequence that results in 3 cubes.

Let me think differently.

Let's consider that each add operation increases the cube count by 1, and each remove operation decreases it by 1, but only if there's at least one cube.

So, if I have n moves, consisting of a adds and b removes, where a + b = n, and a - b = m.

Because each add increases the cube count by 1, and each remove decreases it by 1.

So, a - b = m

And a + b = n

Solving these two equations:

a = (n + m)/2

b = (n - m)/2

For a and b to be non-negative integers, (n + m) must be even, and (n - m) must be even, and n >= m.

Wait, n doesn't necessarily have to be >= m, because you can remove cubes.

Wait, but you can't remove more cubes than you have.

So, the effective number of removes can't exceed the number of adds.

So, b <= a.

Which implies that (n - m)/2 <= (n + m)/2

Which simplifies to n - m <= n + m, which is always true since m >= 0.

But actually, m can be less than n.

Wait, m can be less than n, but m can't be negative.

So, the conditions are:

1. a and b are integers.

2. a >= 0

3. b >= 0

4. b <= a

From a = (n + m)/2 and b = (n - m)/2

So, for a and b to be integers, (n + m) must be even, and (n - m) must be even.

Wait, (n + m) and (n - m) are both even only if n and m are both even or both odd.

Because:

- If n and m are both even, n + m is even, n - m is even.

- If n and m are both odd, n + m is even, n - m is even.

- If one is even and the other is odd, n + m is odd, n - m is odd.

So, a and b are integers only if n and m are both even or both odd.

Additionally, a >= 0 and b >= 0.

So, (n + m)/2 >= 0 and (n - m)/2 >= 0

Which implies that n + m >= 0 (always true since n and m are positive) and n - m >= 0, so n >= m.

But in the third test case, n=5 and m=3.

5 >= 3, and both are odd, so a = (5 + 3)/2 = 4, b = (5 - 3)/2 = 1.

Which are both non-negative integers, and b <= a (1 <= 4).

So, it's possible.

In the second test case, n=2 and m=4.

n < m (2 < 4), so n - m = -2, which would make b = -1, which is invalid.

Hence, "No"

In the first test case, n=3 and m=3.

a = (3 + 3)/2 = 3, b = (3 - 3)/2 = 0.

Which is valid.

So, the general condition is:

- n >= m

- n and m are both even or both odd.

Wait, but in the third test case, n=5 and m=3, both are odd, so it's valid.

In the first test case, n=3 and m=3, both odd, valid.

In the second test case, n=2 and m=4, both even, but n < m, which is invalid.

Wait, but according to the earlier condition, n >= m and both even or both odd.

But in the second test case, n=2 and m=4, both even, but n < m, so invalid.

So, the condition should be:

- n >= m

- (n - m) is even

Wait, but in the earlier derivation, (n + m) and (n - m) must be even for a and b to be integers.

But n >= m to have b >= 0.

Wait, but in the third test case, n=5 and m=3, n - m = 2, which is even.

In the first test case, n=3 and m=3, n - m = 0, which is even.

In the second test case, n=2 and m=4, n - m = -2, which is even, but n < m.

So, perhaps the condition is that (n - m) is even, and n >= m.

But, in the sample input, there's a case where m > n, and the output is "No".

Hence, the condition is:

- n >= m

- (n - m) is even

Wait, but in the third test case, n=5 and m=3, n - m = 2, which is even, and n >= m.

In the second test case, n=2 and m=4, n - m = -2, which is even, but n < m, so "No".

In the first test case, n=3 and m=3, n - m = 0, which is even, and n >= m.

So, the condition seems to be:

If n >= m and (n - m) is even, then "Yes", else "No".

Wait, but in the problem statement, it says:

"You can output each letter in any case (lowercase or uppercase). For example, the strings "yEs", "yes", "Yes", and "YES" will be accepted as a positive answer."

But in the sample output, it's "Yes" and "No".

So, I need to output "Yes" or "No" accordingly.

So, the condition is:

If n >= m and (n - m) % 2 == 0, then "Yes", else "No".

Wait, but in the sample input, there's a case where n=5 and m=3, which satisfies n >= m and (n - m) % 2 == 0, so "Yes".

Another case where n=2 and m=4, n < m, so "No".

And n=3 and m=3, n >= m and (n - m) % 2 == 0, so "Yes".

Seems consistent.

Wait, but in the note, it says:

"In the second test case, Nikita can only end up with either a tower with no blocks or a tower with 2 blocks, so the answer is "No"."

Wait, with n=2 and m=4, it's impossible to have m > n, because you can't have more cubes than the number of moves you make, assuming you can only add or remove one cube per move.

Wait, but actually, you can have m > n, if you add and remove cubes in a certain sequence.

Wait, for example, n=3, m=1:

Add, Add, Remove → 2 cubes

Add, Remove, Add → 2 cubes

Add, Add, Add → 3 cubes

Add, Remove, Remove → 1 cube

Wait, but in this case, n=3, m=1, n >= m and (n - m) = 2, which is even, so "Yes".

Wait, but in n=2, m=4, n < m, so "No".

Hence, the condition seems to hold.

Another way to look at it is:

The net effect of the moves is m cubes.

Each add operation increases the cube count by 1, each remove operation decreases it by 1.

So, if you have a adds and b removes, then a - b = m and a + b = n.

Solving, a = (n + m)/2, b = (n - m)/2.

For a and b to be integers, (n + m) must be even, and (n - m) must be even.

Which is equivalent to n and m being both even or both odd.

Additionally, a >= 0 and b >= 0, which implies n >= m.

Wait, but in the earlier example, n=5 and m=3, both odd, a=4, b=1, which is valid.

n=2 and m=4, both even, a=3, b=-1, which is invalid.

n=3 and m=3, both odd, a=3, b=0, which is valid.

So, the condition is:

- n >= m

- (n + m) is even

- (n - m) is even

But (n + m) and (n - m) being even is equivalent to n and m being both even or both odd.

So, the condition simplifies to:

- n >= m

- n and m are both even or both odd.

Which is the same as (n - m) is even and n >= m.

Because if n and m are both even or both odd, then (n - m) is even.

Hence, the condition is:

If n >= m and (n - m) % 2 == 0, then "Yes", else "No".

Now, looking at the provided program:

def func():

t = int(input())

for i in range(t):

(n, m) = [int(i) for i in input().split()]

if n == m:

print('Yes')

elif m > n:

print('No')

elif m == n - 1:

print('Yes')

elif m % 2 == 0 and n % 2 == 0:

print('Yes')

elif m % 2 != 0 and n % 2 != 0:

print('Yes')

else:

print('No')

Let's see if this aligns with the condition I derived.

First, if n == m:

According to my condition, n >= m and (n - m) % 2 == 0.

Since n == m, (n - m) = 0, which is even, and n >= m, so "Yes".

The program prints "Yes" in this case, which is correct.

Second, if m > n:

According to my condition, n >= m is false, so "No".

The program prints "No", which is correct.

Third, if m == n - 1:

According to my condition, n >= m, which is true, and (n - m) = 1, which is odd.

So, if m == n - 1, then (n - m) = 1, which is odd, so should be "No".

But the program prints "Yes" in this case, which seems incorrect.

Wait, but according to my earlier reasoning, it should be "No".

For example, n=3, m=2.

n >= m, but (n - m) = 1, which is odd.

So, should be "No".

But according to the program, it would print "Yes" because m == n - 1.

This seems to be a mistake in the program.

Wait, but in my earlier example, n=3 and m=1, (n - m)=2, which is even, so "Yes".

n=3 and m=2, (n - m)=1, which is odd, so "No".

So, the program would incorrectly answer "Yes" for n=3 and m=2.

Hence, the program is incorrect.

Wait, but in the sample input, there is n=5 and m=3, which should be "Yes", because (5 - 3)=2, which is even, and n >= m.

The program would reach the elif m == n - 1, which is not true here, so it would check m % 2 == 0 and n % 2 == 0.

m=3 is odd, n=5 is odd, so it would print "Yes", which is correct.

But in the case where m == n - 1, like n=3 and m=2, which should be "No", the program would print "Yes", which is incorrect.

Hence, the program is incorrect.

Wait, but maybe the condition m == n - 1 is handled correctly in some cases.

Wait, let's consider n=3 and m=2.

According to the program:

n != m → go to next

m > n? 2 > 3? No → go to next

m == n - 1? 2 == 3 - 1? Yes → print "Yes"

But according to my condition, (n - m)=1, which is odd, so should be "No"

Hence, the program is incorrect in this case.

Another way to think about it is that m == n - 1 is only possible if n and m are both even or both odd.

Wait, but in the case n=3 (odd), m=2 (even), which are different parity, so should be "No"

Which aligns with my earlier condition that n and m must be both even or both odd.

Hence, the condition should not just check m == n - 1 and print "Yes", but also check the parity.

So, the program is incorrect in this aspect.

Looking further, the next conditions are:

elif m % 2 == 0 and n % 2 == 0:

print('Yes')

elif m % 2 != 0 and n % 2 != 0:

print('Yes')

else:

print('No')

This seems to cover the cases where n and m are both even or both odd.

But, according to my earlier condition, we also need n >= m.

But in the program, these conditions are checked after checking if m > n and m == n - 1.

But, as we saw, m == n - 1 can lead to incorrect "Yes" if (n - m) is odd.

Hence, the program is flawed.

A better way to implement it would be:

- If n >= m and (n - m) % 2 == 0, then "Yes", else "No"

Or, equivalently:

- If n >= m and n and m are both even or both odd, then "Yes", else "No"

But the program doesn't correctly implement this.

Hence, the program is incorrect.

**Final Answer**

\[ \boxed{\text{False}} \]