Let's break down the initial state and the calculation step by step:

1. **Initial State:**
   - `t` is an integer such that \(1 \leq t \leq 10^4\).
   - `ap` is an input integer.
   - `k` is 0.
   - `x` is an input integer - `bxsfory` * 15 + `y` * 4, where `bxsfory` is the ceiling of `y` divided by 2.
   - `y` is an input integer.
   - `bxsfory1` is 0 if `x` is less than or equal to 0 else the ceiling of `x` divided by 15.

2. **Calculating `bxsfory`:**
   - `bxsfory` = \(\left\lceil \frac{y}{2} \right\rceil\).

3. **Calculating `x`:**
   - `x` = `input_integer` - `bxsfory` * 15 + `y` * 4.

4. **Calculating `bxsfory1`:**
   - If `x` <= 0, then `bxsfory1` = 0.
   - Otherwise, `bxsfory1` = \(\left\lceil \frac{x}{15} \right\rceil\).

5. **Expression to be printed:**
   - `print(bxsfory1 + bxsfory)`.

Given the above, let's determine the values of `bxsfory` and `bxsfory1`:

- Suppose `y` is an input integer. For simplicity, let's assume `y = 6` (an arbitrary value to illustrate the calculation).
  - `bxsfory` = \(\left\lceil \frac{6}{2} \right\rceil = 3\).

- Now, let's assume `input_integer` (which we'll call `x_input`) is another input integer. For simplicity, let's assume `x_input = 45` (another arbitrary value to illustrate the calculation).
  - `x` = `x_input` - `bxsfory` * 15 + `y` * 4 = 45 - 3 * 15 + 6 * 4 = 45 - 45 + 24 = 24.
  - Since `x` > 0, `bxsfory1` = \(\left\lceil \frac{24}{15} \right\rceil = 2\).

Therefore, `bxsfory1 + bxsfory` = 2 + 3 = 5.

Output: **5**