Let's break down the initial state and the print statement step by step:

1. **Initial State:**
   - `t` is greater than 0 (though `t` is not used in the print statement).
   - `n` and `k` are input integers.
   - The relationship between `n` and `k` is given by the equation: `4 * n - 2 == k`.

2. **Print Statement:**
   - The print statement is: `print(k // 2 + 1)`.

3. **Determine the Value of `k`:**
   - From the equation `4 * n - 2 == k`, we can express `k` in terms of `n`:
     \[
     k = 4n - 2
     \]

4. **Calculate the Expression `k // 2 + 1`:**
   - Substitute `k` with `4n - 2` in the expression:
     \[
     k // 2 + 1 = (4n - 2) // 2 + 1
     \]
   - Simplify the expression:
     \[
     (4n - 2) // 2 = 2n - 1
     \]
     \[
     2n - 1 + 1 = 2n
     \]

5. **Final Output:**
   - The expression `k // 2 + 1` simplifies to `2n`.

Therefore, the print statement will output the value of `2n`.

Output: **2n (where n is the input integer)**