To determine the final output state after all iterations of the loop have finished, let's analyze the loop step by step and understand the transformations applied to the variables.

### Initial State:
- `fact` = [1, 1 % mod, 2 % mod, (2 % mod) * 3 % mod, ..., (19! % mod)]
- `i` is 19
- `ifact` = [0] * 105
- `ifact[104]` = `pow(fact[104], mod - 2, mod)`

### Loop Code:
```python
for i in range(104, 0, -1):
    ifact[i - 1] = i * ifact[i] % mod
```

### Step-by-Step Analysis:
1. **First Iteration (i = 104):**
   - `ifact[103] = 104 * ifact[104] % mod`
   - `ifact[104]` remains `pow(fact[104], mod - 2, mod)`

2. **Second Iteration (i = 103):**
   - `ifact[102] = 103 * ifact[103] % mod`
   - `ifact[103]` is now `104 * ifact[104] % mod`

3. **Third Iteration (i = 102):**
   - `ifact[101] = 102 * ifact[102] % mod`
   - `ifact[102]` is now `103 * ifact[103] % mod`

Continuing this pattern, each iteration updates `ifact[i - 1]` based on the previous value of `ifact[i]`.

### Final State After All Iterations:
- The loop runs from `i = 104` down to `i = 1`, updating `ifact` in reverse order.
- By the end of the loop, `ifact[0]` will be the last value updated.

### Detailed Final State:
- `ifact[104]` remains `pow(fact[104], mod - 2, mod)`
- For each `j` from 103 down to 0:
  - `ifact[j] = (j + 1) * ifact[j + 1] % mod`

### Summary:
- `ifact[104]` = `pow(fact[104], mod - 2, mod)`
- `ifact[103]` = `104 * ifact[104] % mod`
- `ifact[102]` = `103 * ifact[103] % mod`
- ...
- `ifact[1]` = `2 * ifact[2] % mod`
- `ifact[0]` = `1 * ifact[1] % mod`

### Output State:
**`fact` = [1, 1 % mod, 2 % mod, (2 % mod) * 3 % mod, ..., (19! % mod)], `i` is 0, `ifact` = [0] * 105, `ifact[104]` = `pow(fact[104], mod - 2, mod)`, `ifact[103]` = `104 * ifact[104] % mod`, `ifact[102]` = `103 * ifact[103] % mod`, ..., `ifact[0]` = `1 * ifact[1] % mod`**