Based on the initial state and the conditions provided:

1. `t` is greater than 1.
2. `p1`, `p2`, and `p3` are integers obtained from the input, and their sum is odd.
3. `low` is set to the minimum of `p3 - p1` and `p3 - p2`.
4. `high` is set to the maximum of `p3 - p1` and `p3 - p2`.
5. `cur` is set to `low`.
6. The current value of `p1 - cur` is less than or equal to the current value of `p2 - (p3 - cur)`.

We need to determine the value of `p1 - cur + p3`.

Let's break down the expression `p1 - cur + p3`:

- `cur` is set to `low`, which is the minimum of `p3 - p1` and `p3 - p2`.
- Since `p1 - cur` is less than or equal to `p2 - (p3 - cur)`, let's consider the two cases for `cur`:

**Case 1:** If `cur = p3 - p1`:
- Then `p1 - cur = p1 - (p3 - p1) = 2*p1 - p3`.
- And `p2 - (p3 - cur) = p2 - (p3 - (p3 - p1)) = p2 - p1`.
- Given that `2*p1 - p3 <= p2 - p1`, this simplifies to `2*p1 - p3 <= p2 - p1` which is consistent with our condition.

**Case 2:** If `cur = p3 - p2`:
- Then `p1 - cur = p1 - (p3 - p2) = p1 - p3 + p2`.
- And `p2 - (p3 - cur) = p2 - (p3 - (p3 - p2)) = p2 - p2 = 0`.
- Given that `p1 - p3 + p2 <= 0`, this simplifies to `p1 - p3 + p2 <= 0` which is also consistent with our condition.

In both cases, the expression `p1 - cur + p3` simplifies to either:
- `2*p1 - p3 + p3 = 2*p1` (if `cur = p3 - p1`)
- `p1 - p3 + p2 + p3 = p1 + p2` (if `cur = p3 - p2`)

Given the condition that the sum of `p1`, `p2`, and `p3` is odd, one of them must be odd and the other two even, or vice versa. This ensures that the simplified expressions `2*p1` or `p1 + p2` will be valid based on the parity of the numbers.

Therefore, the output will be either `2*p1` or `p1 + p2` depending on the value of `cur`.

Output: **2*p1 (or p1 + p2) where p1, p2, and p3 are integers such that their sum is odd and the conditions for `cur` are met.**