Let's break down the initial state and the code snippet step by step:

1. **Initial State:**
   - `eta` is a list containing the integers `1`, `1`, and `3`. So, `eta = [1, 1, 3]`.
   - `q` is a list where each element `q[j]` (for `j` from `0` to `n`) has been decremented by `1` for each iteration where `q[j]` was greater than `0`. Since the exact initial values of `q` are not provided, we need to infer them based on the operations described.
   - `rho` is `q[1]`.
   - `j` is `n + 1`.
   - `n` remains unchanged.
   - `eta_ln` is equal to `1`.

2. **Code Snippet:**
   ```python
   print(n * (n - 1) * (n - 2) // 6)
   ```

From the initial state, we know that `eta` is `[1, 1, 3]`. The value of `n` must be the length of `eta`, which is `3`. Therefore, `n = 3`.

Now, let's substitute `n = 3` into the expression `n * (n - 1) * (n - 2) // 6`:
- `n = 3`
- `n - 1 = 2`
- `n - 2 = 1`

So, the expression becomes:
\[ 3 \times 2 \times 1 // 6 \]

Calculating this:
\[ 3 \times 2 \times 1 = 6 \]
\[ 6 // 6 = 1 \]

Therefore, the output of the print statement will be `1`.

Output: **1**