The code snippet `n -= m` updates the value of `n` by subtracting the value of `m` from it. Given the initial state:

- `t` is an input integer such that 1 ≤ t ≤ 5 · 10^4
- `n` is `n - (n + 1) // 2`
- `k` is an input integer
- `L` is a list containing the values `(n + 1) // 2` and `(n + 1) // 2`
- `m` is `(n + 1) // 2`

Let's analyze the impact of the code:

1. `m` is defined as `(n + 1) // 2`.
2. `n` is updated to `n - m`.

Since `m` is `(n + 1) // 2`, the new value of `n` becomes:
\[ n = n - ((n + 1) // 2) \]

This simplifies to:
\[ n = (n - (n + 1) // 2) - ((n + 1) // 2) \]
\[ n = (n - (n + 1) // 2) - (n + 1) // 2 \]
\[ n = n - (n + 1) // 2 - (n + 1) // 2 \]
\[ n = n - (n + 1) \]

Since `(n + 1) // 2` is an integer division, the final value of `n` will be:
\[ n = n - (n + 1) \]
\[ n = -1 \]

Therefore, the output state is:
Output State: **`t` is an input integer such that 1 ≤ t ≤ 5 · 10^4, `n` is -1, `k` is an input integer, `L` is a list containing the values `(n + 1) // 2` and `(n + 1) // 2`, `m` is `(n + 1) // 2`.**