The value of `remainder` is decremented by 1. The previous value of `remainder` is equal to \( n - d \cdot min_sum - 2 \), so the new value of `remainder` becomes \( (n - d \cdot min_sum - 2) - 1 = n - d \cdot min_sum - 3 \). Other variables remain unchanged. 

Output State: **`n` is a positive integer such that \( 1 \leq n \leq 10^{10} \); `k` is a positive integer such that \( k \geq 3 \); `min_sum` is equal to \( \frac{k \cdot (k + 1)}{2} \) and \( min_sum \leq n \); `d` is equal to \( \frac{n}{min_sum} \); `sequence` is a list containing \( [d, 2d, 3d, \ldots, (k-1)d + 2] \); `i` is \( k - 3 \); `remainder` is equal to \( n - d \cdot min_sum - 3 \).**