Postcondition: ***`n` and `m` are positive integers such that 1 <= n, m <= 2 * 10^6, `T` is greater than 0, `t` is 0, `a` is the integer value of `info[0]`, `b` is the integer value of `info[1]` and must be greater than or equal to 2, `i` is 2, `x` is the result of the expression `(a - 2 * (2 - 1)) // 2`. If the condition `(a - i * (i - 1)) % i ** 2 == 0 and i * (i - 1) % i ** 2 == 0` is true, then `suma` is the result of the expression `(a - 2 * (2 - 1)) // 2 + 1`. Otherwise, `suma` remains the result of the expression `(a - 2 * (2 - 1)) // 2`.***