Output State: **`n` and `m` are positive integers such that \(1 \leq n, m \leq 2 \times 10^6\), `T` is greater than 0, `t` is 1, `a` is the integer value of `info[0]`, `b` is the integer value of `info[1]` and must be greater than or equal to `a` and 2, `i` is 3, `x` is \((a - 3 \times 2) // 9 + 1\). If \((a - 3 \times 2) // 9 + 1 > 0\), then `suma` is \((a - 2 \times 1) // 4 + 2\) if \((a - 3 \times 2) \% 9 == 0\) and \((3 \times 2) \% 9 == 0\). Otherwise, `suma` remains \((a - 2 \times 1) // 4 + 1\). If \((a - 3 \times 2) // 9 + 1 \leq 0\), `suma` remains \((a - 2 \times 1) // 4 + 1\). Now, `suma` is incremented by 1.**

In natural language:
- `n` and `m` are still positive integers within the range \(1 \leq n, m \leq 2 \times 10^6\).
- `T` is still greater than 0.
- `t` is still 1.
- `a` is still the integer value of `info[0]`.
- `b` is still the integer value of `info[1]` and must be greater than or equal to `a` and 2.
- `i` is still 3.
- `x` is still \((a - 3 \times 2) // 9 + 1\).
- The value of `suma` is incremented by 1. If \((a - 3 \times 2) // 9 + 1 > 0\) and \((a - 3 \times 2) \% 9 == 0\) and \((3 \times 2) \% 9 == 0\), then `suma` was initially \((a - 2 \times 1) // 4 + 2\) and is now \((a - 2 \times 1) // 4 + 3\). Otherwise, if \((a - 3 \times 2) // 9 + 1 > 0\) and the conditions \((a - 3 \times 2) \% 9 == 0\) and \((3 \times 2) \% 9 == 0\) are not met, then `suma` was initially \((a - 2 \times 1) // 4 + 1\) and is now \((a - 2 \times 1) // 4 + 2\). If \((a - 3 \times 2) // 9 + 1 \leq 0\), `suma` was initially \((a - 2 \times 1) // 4 + 1\) and is now \((a - 2 \times 1) // 4 + 2\).