Output State: **`n` and `m` are positive integers such that \(1 \leq n, m \leq 2 \times 10^6\), `T` is greater than 2, `t` is 2, `info` is a list of strings from user input, `a` is the integer value of `info[0]`, `b` is the integer value of `info[1]` and must be greater than or equal to `a` and at least 1, `i` is 2, `x` is \(\frac{a - 2 \cdot 1}{2^2} + 1\), `suma` is \(a + 1 + x\) if the conditions \((a - i \cdot (i - 1)) \% i^2 == 0\) and \(i \cdot (i - 1) \% i^2 == 0\) are not both satisfied, otherwise `suma` is \(a + 2 + x\).**

Explanation:
- The value of `suma` is updated by adding `x` to it.
- The initial value of `suma` is \(a + 1\) if the conditions \((a - i \cdot (i - 1)) \% i^2 == 0\) and \(i \cdot (i - 1) \% i^2 == 0\) are not both satisfied, otherwise it is \(a + 2\).
- Therefore, after the code `suma += x` is executed, `suma` becomes \(a + 1 + x\) or \(a + 2 + x\) depending on the initial conditions.