The code snippet `cnt -= 1` decrements the value of `cnt` by 1. Given the initial state, `cnt` was `k - 2`. After decrementing, `cnt` becomes `(k - 2) - 1` which simplifies to `k - 3`.

The other variables remain unchanged:
- `n` is still a positive integer.
- `k` is still an integer such that `3 <= k <= n`.
- `v` is still the value returned by `func_2()` during the last iteration (`i = 1`).
- `l` is still `func_2() + 1` and must be less than `n + 1`.
- `i` is still `2`.

Therefore, the Output State is:
Output State: **`n` is a positive integer, `k` is an integer such that `3 <= k <= n`, `v` is the value returned by `func_2()` during the last iteration (`i = 1`), `cnt` is `k - 3`, `l` is `func_2() + 1` and must be less than `n + 1`, `i` is `2`.**