To determine the output state after the loop executes all the iterations, we need to understand the loop's behavior based on the provided initial state and the code. However, the code snippet provided includes variables `A`, `idx_A`, `s`, and `n` that are not defined in the initial state. For the purpose of this exercise, I will assume some plausible values for these variables to illustrate the process.

Let's assume:
- `A` is `[0, 1]`
- `idx_A` is `[0, 1]`
- `s` is a string of `>` and `<` characters, for example, `">><<"`
- `n` is the length of the string `s`, which is `4` in this case.

Given the initial state and the assumed values:

Initial State: `B` is `[0, 1]`, `idx_B` is `[1, 0]`, `l` is `0`, `r` is `2`, `A` is `[0, 1]`, `idx_A` is `[0, 1]`, `s` is `">><<"`.

Let's walk through the loop iterations:

1. **Iteration 1 (i=0, s[0] = '>')**:
   - `l < r` (0 < 2) is true.
   - `a = A[l] = A[0] = 0`
   - `x = r - (l + 2) = 2 - (0 + 2) = 0`
   - `b = B[r - 1] = B[1] = 1`
   - Since `x >= 0` (0 >= 0) is true:
     - `b = b - B[x] = 1 - B[0] = 1 - 0 = 1`
     - `b = b - (idx_B[x] - idx_B[r - 1]) * (x + 1) = 1 - (idx_B[0] - idx_B[1]) * (0 + 1) = 1 - (1 - 0) * 1 = 0`
   - `b = b + (idx_B[r - 1] - i) * (l + 1) = 0 + (0 - 0) * (0 + 1) = 0`
   - `print(a * 2 + b * 2 + i + 1, end=' ') = print(0 * 2 + 0 * 2 + 0 + 1, end=' ') = print(1, end=' ')`
   - `l += 1` → `l` becomes `1`

2. **Iteration 2 (i=1, s[1] = '>')**:
   - `l < r` (1 < 2) is true.
   - `a = A[l] = A[1] = 1`
   - `x = r - (l + 2) = 2 - (1 + 2) = -1`
   - `b = B[r - 1] = B[1] = 1`
   - Since `x >= 0` (-1 >= 0) is false:
     - We skip the inner if block.
   - `b = b + (idx_B[r - 1] - i) * (l + 1) = 1 + (0 - 1) * (1 + 1) = 1 - 2 = -1`
   - `print(a * 2 + b * 2 + i + 1, end=' ') = print(1 * 2 + (-1) * 2 + 1 + 1, end=' ') = print(1, end=' ')`
   - `l += 1` → `l` becomes `2`

3. **Iteration 3 (i=2, s[2] = '<')**:
   - `r -= 1` → `r` becomes `1`
   - `l <= r` (2 <= 1) is false.
   - `r == 0` (1 == 0) is false.
   - `a = B[r] = B[1] = 1`
   - `b = A[l - 1] = A[1] = 1`
   - Since `l - r - 1 > 0` (2 - 1 - 1 > 0) is false:
     - We skip the inner if block.
   - `b = b + (i - idx_A[l - 1]) * (r + 1) = 1 + (2 - 1) * (1 + 1) = 1 + 2 = 3`
   - `print(a * 2 + b * 2 + (n - i), end=' ') = print(1 * 2 + 3 * 2 + (4 - 2), end=' ') = print(10, end=' ')`

4. **Iteration 4 (i=3, s[3] = '<')**:
   - `r -= 1` → `r` becomes `0`
   - `l <= r` (2 <= 0) is false.
   - `r == 0` (0 == 0) is true.
   - `print(n - i + (i - idx_A[l - 1]) * 2, end=' ') = print(4 - 3 + (3 - 1) * 2, end=' ') = print(5, end=' ')`

After the loop finishes, the values of `B`, `idx_B`, `l`, and `r` remain unchanged because the loop does not modify them directly. The variables `A` and `idx_A` are also not modified within the loop.

Output State: **B is [0, 1], idx_B is [1, 0], l is 2, r is 0.**