Let's break down the given code snippet step by step:

1. The initial state is defined as follows:
   - `t` is a positive integer between 0 and \(10^4\).
   - `t` is equal to `k - 1`.
   - There are conditions related to `b % 3 == 0`, `c` being greater than or equal to certain values, etc., which may have already modified `tents` in a previous step.

2. The code snippet to be executed is:
   ```python
   tents += c // 3 + (1 if c % 3 > 0 else 0)
   ```

This line of code updates the value of `tents` based on the value of `c`. Specifically, it adds `c // 3` plus 1 if `c % 3` is greater than 0 to `tents`.

- If `c % 3 > 0`, the expression `(1 if c % 3 > 0 else 0)` evaluates to 1, so `tents += c // 3 + 1`.
- If `c % 3 == 0`, the expression `(1 if c % 3 > 0 else 0)` evaluates to 0, so `tents += c // 3`.

Given this, let's summarize the impact:

- `t` remains unchanged and is still equal to `k - 1`.
- `tents` is updated according to the above logic based on the value of `c`.

Therefore, the Output State is:
Output State: **`t` is `k - 1`, `tents` is updated based on the condition `tents += c // 3 + (1 if c % 3 > 0 else 0)`**