Let's analyze the given loop step by step to determine the final state of the variables after all iterations have finished.

### Initial State
- \( n \) is a non-negative integer and \( n \neq 0 \) and \( n \neq 1 \).
- \( a = 2 \)
- \( b = 1 \)

### Loop Code
```python
for _ in range(2, n + 1):
    a, b = b, a + b
```

### Observations from the First Few Iterations
1. **After 1 iteration (n=2):**
   - \( n \geq 2 \)
   - \( a = 1 \)
   - \( b = 3 \)

2. **After 2 iterations (n=3):**
   - \( n \geq 3 \)
   - \( a = 3 \)
   - \( b = 4 \)

3. **After 3 iterations (n=4):**
   - \( n \geq 4 \)
   - \( a = 7 \)
   - \( b = 4 \)

### Analysis
From the observations, we can see that the loop runs from 2 to \( n \). Each iteration updates the values of \( a \) and \( b \) based on the Fibonacci sequence starting from \( b = 1 \) and \( a = 2 \).

- After the first iteration (\( n = 2 \)):
  - \( a = b \) (initial \( b = 1 \))
  - \( b = a + b = 1 + 2 = 3 \)
- After the second iteration (\( n = 3 \)):
  - \( a = b \) (previous \( b = 3 \))
  - \( b = a + b = 3 + 1 = 4 \)
- After the third iteration (\( n = 4 \)):
  - \( a = b \) (previous \( b = 4 \))
  - \( b = a + b = 4 + 3 = 7 \)

### General Pattern
Each iteration of the loop adds the previous \( a \) and \( b \) to form the next pair:
- After \( k \) iterations, \( a \) becomes the \( k+1 \)-th Fibonacci number starting from \( F_2 = 1 \) (since \( b = 1 \) initially and \( a = 2 \)).
- After \( k \) iterations, \( b \) becomes the \( (k+2) \)-th Fibonacci number starting from \( F_2 = 1 \).

### Final State
- Since the loop runs from 2 to \( n \), it will run exactly \( n - 1 \) times.
- After \( n - 1 \) iterations, \( a \) will be the \( n \)-th Fibonacci number.
- \( b \) will be the \( (n+1) \)-th Fibonacci number.

Thus, the final state of the loop is:
Output State: **`n` is a non-negative integer and \( n \neq 0 \) and \( n \neq 1 \); `a` is the \( n \)-th Fibonacci number; `b` is the \( (n+1) \)-th Fibonacci number.**