Output State: `total` is 0, `l` is `n - 3`, `r` is `n - 2`, `a` is a list of integers where `a[1] == a[2]` and `a[2] == a[3]` and so on until `a[n-4] == a[n-3]`, `le` is the length of list `a`, `st` is `le - (n - 2)`, `end` is 1, `ans` is `le - (n - 1 + 1)`.

Explanation: The loop continues as long as `l < r` and the elements at indices `l` and `l+1` are equal. Each iteration increments `l` and `st`. After the loop terminates, `l` will be one more than `r`, meaning `l = n - 3` if `r = n - 2`. This implies that the sequence of equal consecutive elements starts from index 0 and goes up to `n-4` (inclusive), making `st` equal to `le - (n - 2)`. The value of `ans` remains as initially defined.