Reasoning: 

The original assessment contains a critical misunderstanding of the mathematical formulas used in the function. The function `func_1(n)` indeed uses the correct formula for the sum of the first `n` natural numbers, which is \( \text{sum}_n = \frac{n(n + 1)}{2} \). However, it incorrectly assumes that the sum of the cubes of the first `n` natural numbers is the square of the sum of the first `n` natural numbers, which is \( \left(\frac{n(n + 1)}{2}\right)^2 \).

This assumption is incorrect. The correct formula for the sum of the cubes of the first `n` natural numbers is actually:
\[ \text{sum\_cubes}_n = \left(\frac{n(n + 1)}{2}\right)^2 \]

However, the problem requires the difference between the sum of the cubes of the first `n` natural numbers and the sum of the first `n` natural numbers. The correct formula for the difference should be:
\[ \text{difference} = \left(\frac{n(n + 1)}{2}\right)^2 - \frac{n(n + 1)}{2} \]

The function as written does not compute this difference correctly. Instead, it computes:
\[ \left(\frac{n(n + 1)}{2}\right)^2 - \frac{n(n + 1)}{2} \]

But due to a mistake in the annotation, it seems to suggest that both `sum_cubes_n` and `sum_n` are equal, which is incorrect. They are not equal; they are different quantities.

Let's re-evaluate the function with the correct formulas:

1. **Sum of the first `n` natural numbers**:
   \[ \text{sum}_n = \frac{n(n + 1)}{2} \]

2. **Sum of the cubes of the first `n` natural numbers**:
   \[ \text{sum\_cubes}_n = \left(\frac{n(n + 1)}{2}\right)^2 \]

3. **Difference**:
   \[ \text{difference} = \left(\frac{n(n + 1)}{2}\right)^2 - \frac{n(n + 1)}{2} \]

Given the test cases:
- For \( n = 3 \):
  \[ \text{sum}_n = \frac{3(3 + 1)}{2} = 6 \]
  \[ \text{sum\_cubes}_n = 6^2 = 36 \]
  \[ \text{difference} = 36 - 6 = 30 \]

- For \( n = 5 \):
  \[ \text{sum}_n = \frac{5(5 + 1)}{2} = 15 \]
  \[ \text{sum\_cubes}_n = 15^2 = 225 \]
  \[ \text{difference} = 225 - 15 = 210 \]

- For \( n = 2 \):
  \[ \text{sum}_n = \frac{2(2 + 1)}{2} = 3 \]
  \[ \text{sum\_cubes}_n = 3^2 = 9 \]
  \[ \text{difference} = 9 - 3 = 6 \]

The function correctly implements these calculations, and the test cases provided verify the correctness of the implementation.

Therefore, the original assessment is accurate, and the function is correct.

Final: **True**