`k` is between 0 and 3 inclusive; `i` is \(i + 1\); `j` and `ans` are unchanged. The code updates `j` to the value of \((k - 3 \times i) // 2\). Given that `k` is between 0 and 3 inclusive and `i` is now \(i + 1\), let's evaluate the expression for `j`.

- If `k = 0` and `i = 1`, then `j = (0 - 3 * 1) // 2 = -3 // 2 = -1`.
- If `k = 1` and `i = 1`, then `j = (1 - 3 * 1) // 2 = -2 // 2 = -1`.
- If `k = 2` and `i = 1`, then `j = (2 - 3 * 1) // 2 = -1 // 2 = -1`.
- If `k = 3` and `i = 1`, then `j = (3 - 3 * 1) // 2 = 0 // 2 = 0`.

In each case, the value of `j` depends on the specific values of `k` and `i`. However, since the exact value of `i` was not given initially and only that it was \(i + 1\), we express `j` in terms of `k` and `i`.

Therefore, the output state is:
Output State: **`k` is between 0 and 3 inclusive; `i` is \(i + 1\); `j` is \((k - 3 \times i) // 2\); `ans` is unchanged**.