First, let's break down the initial state and the code snippet:

- Initial State:
  - `k` is between 0 and 3 inclusive.
  - `i` is incremented by 1.
  - `j` is calculated as \((k - 3 \times i) // 2\).
  - `ans` remains unchanged.

- Code Snippet:
  ```python
  ans = min(ans, 3 * i * c + j * b + (k - 3 * i - 2 * j) * a)
  ```

Step-by-step analysis:

1. Since `i` is incremented by 1 in the initial state, we have \(i = i + 1\).

2. Calculate `j` using the formula \(j = \frac{k - 3 \times i}{2}\). Since `i` is now \(i + 1\), substitute this into the equation:
   \[
   j = \frac{k - 3(i + 1)}{2} = \frac{k - 3i - 3}{2}
   \]

3. Substitute \(i\) and \(j\) into the expression `3 * i * c + j * b + (k - 3 * i - 2 * j) * a`:
   \[
   3(i + 1) * c + \left(\frac{k - 3i - 3}{2}\right) * b + \left(k - 3(i + 1) - 2 \left(\frac{k - 3i - 3}{2}\right)\right) * a
   \]

4. Simplify the expression:
   \[
   3i * c + 3c + \frac{k - 3i - 3}{2} * b + \left(k - 3i - 3 - (k - 3i - 3)\right) * a
   \]
   \[
   3i * c + 3c + \frac{k - 3i - 3}{2} * b + 0 * a
   \]
   \[
   3i * c + 3c + \frac{k - 3i - 3}{2} * b
   \]

5. The `ans` variable is updated to be the minimum of its current value and the calculated expression:
   \[
   ans = \min(ans, 3i * c + 3c + \frac{k - 3i - 3}{2} * b)
   \]

Given the initial constraints on `k` (0 to 3), let's consider each case:

- If `k = 0`, then \(i = i + 1\), \(j = \frac{0 - 3(i + 1)}{2}\), and the expression becomes:
  \[
  3i * c + 3c + \frac{-3(i + 1)}{2} * b
  \]

- If `k = 1`, then \(i = i + 1\), \(j = \frac{1 - 3(i + 1)}{2}\), and the expression becomes:
  \[
  3i * c + 3c + \frac{1 - 3(i + 1)}{2} * b
  \]

- If `k = 2`, then \(i = i + 1\), \(j = \frac{2 - 3(i + 1)}{2}\), and the expression becomes:
  \[
  3i * c + 3c + \frac{2 - 3(i + 1)}{2} * b
  \]

- If `k = 3`, then \(i = i + 1\), \(j = \frac{3 - 3(i + 1)}{2}\), and the expression becomes:
  \[
  3i * c + 3c + \frac{3 - 3(i + 1)}{2} * b
  \]

In all cases, `ans` is updated to the minimum value of itself and the calculated expression. The final state is:
Output State: **`k` is between 0 and 3 inclusive; `i` is \(i + 1\); `j` is \(\frac{k - 3i - 3}{2}\); `ans` is the minimum of its current value and \(3i * c + 3c + \frac{k - 3i - 3}{2} * b\)**.