The initial state is defined as follows:
- `k` is between 0 and 3 inclusive.
- `i` is updated to `i + 1`.
- `j` is recalculated based on the new value of `i`.
- `ans` remains the same.

The code snippet updates `i` to `i + 1` and then calculates `j` using the formula `j = (k - 3 * i) // 2`.

Let's break down the impact:

1. `i` is incremented by 1, so the new value of `i` is `i + 1`.
2. `j` is recalculated using the new value of `i`. The formula `j = (k - 3 * i) // 2` means `j` is now `(k - 3 * (i + 1)) // 2`.

Since `k` is between 0 and 3 inclusive, let's consider each possible value of `k`:

- If `k = 0`: `j = (0 - 3 * (i + 1)) // 2 = (-3 * (i + 1)) // 2 = -3 * (i + 1) // 2`.
- If `k = 1`: `j = (1 - 3 * (i + 1)) // 2 = (1 - 3 * (i + 1)) // 2 = (1 - 3 * i - 3) // 2 = (-2 - 3 * i) // 2`.
- If `k = 2`: `j = (2 - 3 * (i + 1)) // 2 = (2 - 3 * (i + 1)) // 2 = (2 - 3 * i - 3) // 2 = (-1 - 3 * i) // 2`.
- If `k = 3`: `j = (3 - 3 * (i + 1)) // 2 = (3 - 3 * (i + 1)) // 2 = (3 - 3 * i - 3) // 2 = (-3 * i) // 2`.

Given these recalculations, the final output state is:
- `k` is between 0 and 3 inclusive.
- `i` is updated to `i + 1`.
- `j` is updated based on the formula `j = (k - 3 * (i + 1)) // 2`.
- `ans` remains the same.

Output State: **`k` is between 0 and 3 inclusive; `i` is `i + 1`; `j` is `(k - 3 * (i + 1)) // 2`; `ans` remains the same**