The expression `dp[n, k] += 9 * 10 ** (i - 1) * (10 ** (k - i) - 10 ** (i - 1))` updates the value of `dp[n, k]`. The variable `i` is 2, therefore `10 ** (i - 1)` is `10 ** 1`, which equals `10`. The term `10 ** (k - i)` represents `10 ** (k - 2)`, and the term `10 ** (i - 1)` is `10`. Thus, the equation simplifies to:

```
dp[n, k] += 9 * 10 * (10 ** (k - 2) - 10)
```

Other variables (`l`, `r`, `k`) are not directly affected by this operation. Therefore, the output state can be described as:

Output State: **`l` is an integer such that 1 <= `l` <= `r` < 10^18, `r` is an integer such that 1 <= `l` <= `r` < 10^18, `k` is greater than 1, `i` is 2, and `dp[n, k]` is updated by adding `9 * 10 * (10 ** (k - 2) - 10)`**.