The value of `m` is assigned the result of `n - num`. Given that `n` is an input integer such that \(1 \leq n \leq 3 \cdot 10^5\) and `num` is the sum of 1s and 2s from each of the `k` iterations (i.e., `k + y` where `y` is the number of times `c != r`), the value of `m` will be `n - (k + y)`. The values of `n`, `k`, `t`, `i`, and `num` remain unchanged except for the new value of `m`.

Output State: **`n` is an input integer such that 1 ≤ n ≤ 3 · 10^5, `k` is an input integer such that 0 ≤ k ≤ n, `t` is at least 1 and has been decremented by 1, `i` is -1, `num` is the sum of 1s and 2s from each of the `k` iterations (i.e., `k + y` where `y` is the number of times `c != r`), `m` is `n - num`.**