Postcondition: ***`a`, `b`, `c`, and `d` are non-negative integers. `s1` is `b - a`, `s2` is `c - d`. If `s1 == s2`, then `out` is `[1, 0] * a + [1, 2] * (b - a) + [3, 2] * d`. If `s1 + 1 == s2` and `d > 0`, then `a` decreases by 1 (if `a > 0`), and `out` is constructed as `[1, 0] * a + [1, 2] * (b - a) + [3, 2] * d + [3]`. If `s1 + 1 == s2` and `d <= 0`, then `b` increases by 1, `d` resets to 0, and `c` is set to a non-zero value other than 1, with `out` being `[1, 0] * a + [1]`. Otherwise, if `s1 + 1 != s2` and `d > 0`, then `d` decreases by 1, and `out` remains `[1, 0] * a + [1, 2] * (b - a) + [3, 2] * d`. If `s1 + 1 != s2` and `d <= 0`, then `b` increases by 1, `d` resets to 0, and `c` is set to a non-zero value other than 1, with `out` being `[1, 0] * a + [1]`.***