To determine the new value of `dp[i]`, we use the given formula:

\[ dp[i] = (dp[i - 1] + (i - 1) \times dp[i - 2] \times 2) \% (10^9 + 7) \]

Given:
- `i` is 8
- `dp[7]` is 0
- `dp[6]` is 0

Substituting these values into the formula:

\[ dp[8] = (dp[7] + (8 - 1) \times dp[6] \times 2) \% (10^9 + 7) \]
\[ dp[8] = (0 + 7 \times 0 \times 2) \% (10^9 + 7) \]
\[ dp[8] = 0 \% (10^9 + 7) \]
\[ dp[8] = 0 \]

The other variables (`t`, `n`, `k`, `num`, `m`) remain unchanged.

Output State: **`t` is at least 0, `n` is the first integer read from the input, `k` is the second integer read from the input, `num` is `2k - x` where `x` is the number of times `c == r` during the `k` iterations, `m` is at least 3, `dp` is a list of `m + 1` zeros except `dp[1]` which is 1, `dp[2]` which is 3, `dp[6]` which is 0, `dp[7]` which is 0, and `dp[8]` which is 0, `i` is 8.**