The code snippet `ma = len(s) - d` calculates the value of `ma` by subtracting the value of `d` (which is 1) from the length of the string `s`. Given that `s` is a string of length `n`, `ma` will be `n - 1`.

Output State: **`t` is an integer (1 ≤ t ≤ 10^4), `n` is an integer (1 ≤ n ≤ 10), `s` is a string of length n consisting of 'W' and 'B' with at least one 'B', `ma` is `n - 1`, `mi` is the 1-based index of the first 'B' in `s`, `m` is the number of test cases, `c` is the 1-based index of the first 'B' in `s`, `d` is 1, and `l` is an empty list. The current character `j` is 'B'.**