Let's break down the initial state and the print statement step by step:

1. **Initial State Analysis:**
   - `b` is a list with three elements:
     - First element: `0 + v_3`
     - Second element: `v_3 + v_3`
     - Third element: `v_3 + v_3`
   - `x` is `w_3`
   - `y` is `x`, so `y` is also `w_3`
   - `z` is `y`, so `z` is also `w_3`
   - `v` is `v_3`
   - `u` is `u - 1`
   - `c` is the return value from function `r()`
   - `d` is the return value from function `r()`

2. **Print Statement Analysis:**
   - The expression inside the print statement is `b[(d - 1) * 2] - b[(c - 1) * 2]`.

3. **Evaluating the Expression:**
   - `b[(d - 1) * 2]`: This means we need to find the element at the index `(d - 1) * 2` in the list `b`.
   - `b[(c - 1) * 2]`: This means we need to find the element at the index `(c - 1) * 2` in the list `b`.

4. **List `b` Elements:**
   - `b[0] = 0 + v_3`
   - `b[1] = v_3 + v_3`
   - `b[2] = v_3 + v_3`

5. **Index Calculation:**
   - For `b[(d - 1) * 2]`:
     - If `d` is 1, then `(d - 1) * 2 = 0`, so it refers to `b[0] = 0 + v_3`.
     - If `d` is 2, then `(d - 1) * 2 = 2`, so it refers to `b[2] = v_3 + v_3`.
     - If `d` is 3, then `(d - 1) * 2 = 4`, but since the list only has 3 elements, this would be out of bounds, so let's assume `d` is within the valid range.
   - For `b[(c - 1) * 2]`:
     - If `c` is 1, then `(c - 1) * 2 = 0`, so it refers to `b[0] = 0 + v_3`.
     - If `c` is 2, then `(c - 1) * 2 = 2`, so it refers to `b[2] = v_3 + v_3`.
     - If `c` is 3, then `(c - 1) * 2 = 4`, but again, this would be out of bounds.

6. **Possible Values:**
   - If both `d` and `c` are either 1 or 2, the expression simplifies to:
     - `b[0] - b[0] = (0 + v_3) - (0 + v_3) = 0`
     - `b[2] - b[2] = (v_3 + v_3) - (v_3 + v_3) = 0`

Therefore, the print statement will output `0`.

Output: **0**