The code snippet `end += 1` increments the value of the variable `end` by 1. The other variables remain unchanged.

Given the initial state:
- `t` is an integer such that \(1 \leq t \leq 10^4\)
- `n` is the length of the list `a`
- `a` is the list of integers where `a[n - 1] == a[n - 2]`
- `le` is the length of the list `a`
- `l` is `n - 2`
- `r` is `n - 2`
- `st` is `n - 1`
- `end` is `1`
- `ans` is `0` if `a[0]` is equal to `a[-1]`, otherwise `ans` is `1`

After executing `end += 1`, the value of `end` becomes `2`.

Output State: **`t` is an integer such that \(1 \leq t \leq 10^4\); `n` is the length of the list `a`; `a` is the list of integers where `a[n - 1] == a[n - 2]`; `le` is the length of the list `a`; `l` is `n - 2`; `r` is `n - 2`; `st` is `n - 1`; `end` is `2`; `ans` is `0` if `a[0]` is equal to `a[-1]`, otherwise `ans` is `1`**.