Given the initial state where `n`, `pos`, `l`, `r` are integers with the conditions specified, and the information that `pos` is greater than `r`, we can analyze the impact of the provided code snippet.

1. Initially, since `pos > r`, we know that `ans` has a value of either `l - pos` (if `pos < l`) or 0 (if `pos >= l`). However, since `pos` cannot be less than `l` because it is either equal to or greater than `l` (from the condition involving `pos`, `l`, and `r`), we establish that `ans` must be 0 before the operation.

2. The statement `ans += pos - r` modifies `ans`. Since `ans` is initially 0, the new value is directly dependent on the calculation of `pos - r`.

3. Therefore, `ans` becomes `0 + (pos - r)`, which simplifies to just `pos - r`.

Thus, the output state will reflect the updated value of `ans`, indicating its new computed value based on the relationship between `pos` and `r`.

Output State: **`n`, `pos`, `l`, `r` are integers with `1 ≤ pos ≤ n`, `1 ≤ l ≤ r ≤ n`, `1 ≤ r ≤ n`; `ans` is equal to `pos - r`.**