The code updates the value of `my` using the formula `my = cy - dx * math.sqrt(d2 * d - d * d) / d2`. Let's break this down:

1. The initial value of `my` is `cy - sqrt(d)`.
2. The new value of `my` is calculated as `cy - dx * math.sqrt(d2 * d - d * d) / d2`.

We can simplify the expression inside the square root:
\[ d2 \times d - d \times d = d2 \times d - d^2 = d2 \times d - d^2 \]
So the expression becomes:
\[ my = cy - dx \times \frac{\sqrt{d2 \times d - d^2}}{d2} \]

Given the initial values:
- `dx = (x1 - x2) / 2`
- `dy = (y1 - y2) / 2`
- `d2 = ((x1 - x2) / 2)^2 + ((y1 - y2) / 2)^2`
- `mx = cx + dy * sqrt(d2 * d - d * d) / d2`
- `my = cy - sqrt(d)`
- `j = i + 1`
- `x2 = meats[j][0]`
- `y2 = meats[j][1]`
- `c2 = meats[j][2]`
- `x1 = meats[j][1]`
- `y1 = meats[j][2]`
- `c1 = meats[j][0]`
- `d = c1 * T - c2 * T / (c1 * c2)`
- `cx = (x2 + x1) / 2`
- `cy = (y1 + y2) / 2`

After executing the code, `my` is updated according to the formula provided. All other variables remain unchanged.

Output State: **`dx` is `(x1 - x2) / 2`, `dy` is `(y1 - y2) / 2`, `d2` is `((x1 - x2) / 2)^2 + ((y1 - y2) / 2)^2`, `mx` is `cx + dy * sqrt(d2 * d - d * d) / d2`, `my` is `cy - dx * math.sqrt(d2 * d - d^2) / d2`, `j` is `i + 1`, `x2` is `meats[j][0]`, `y2` is `meats[j][1]`, `c2` is `meats[j][2]`, `x1` is `meats[j][1]`, `y1` is `meats[j][2]`, `c1` is `meats[j][0]`, `d` is `c1 * T - c2 * T / (c1 * c2)`, `cx` is `(x2 + x1) / 2`, `cy` is `(y1 + y2) / 2`**