Let's break down the initial state and the code snippet step by step to determine what will be printed.

### Initial State:
- `n` and `m` are positive integers such that \(1 \leq n, m \leq 2 \times 10^6\).
- `T` is greater than 0.
- `t` is 0.
- `info` is a list of strings obtained from the input.
- `a` is the integer value of `info[0]`.
- `b` is the integer value of `info[1]` and must be at least 1.
- `i` is `b`.
- `suma` is the sum of \((a - i * (i - 1)) // i\).

### Code Snippet:
```python
print(suma - 1)
```

### Step-by-Step Analysis:
1. **Understanding `info`**:
   - `info` is a list of strings obtained from the input. For example, if the input is `["10", "3"]`, then `info = ["10", "3"]`.

2. **Assigning Values to `a` and `b`**:
   - `a` is the integer value of `info[0]`. So, if `info[0]` is `"10"`, then `a = 10`.
   - `b` is the integer value of `info[1]` and must be at least 1. So, if `info[1]` is `"3"`, then `b = 3`.

3. **Assigning Value to `i`**:
   - `i` is set to `b`. So, if `b = 3`, then `i = 3`.

4. **Calculating `suma`**:
   - `suma` is the sum of \((a - i * (i - 1)) // i\).
   - Let's break this down further:
     - \(i * (i - 1)\) is \(3 * (3 - 1) = 3 * 2 = 6\).
     - \(a - i * (i - 1)\) is \(10 - 6 = 4\).
     - \((a - i * (i - 1)) // i\) is \(4 // 3 = 1\).
   - Therefore, `suma` is the sum of 1, which is simply 1.

5. **Printing `suma - 1`**:
   - `suma` is 1.
   - `suma - 1` is \(1 - 1 = 0\).

### Final Output:
The code will print the value of `suma - 1`, which is 0.

Output: **0**