The code snippet calculates a new value `x` based on the current state of `A` and `idx_A`. The new value of `x` is appended to `A`.

Given the initial state, `x` is calculated as:
\[ x = A[\text{len}(A) - 1] + (i - \text{idx\_A}[\text{len}(\text{idx\_A}) - 1]) * \text{len}(\text{idx\_A}) \]

After this calculation, `x` is added to the end of the list `A`.

Output State: **`s` is a string consisting of characters '<' and '>' with length `n`, where 1 ≤ `n` ≤ 5 · 10^5; `n` is the length of `s`; `i` is `i_prev + 2`; `A` has a new element `x` appended, where `x = A[len(A) - 1] + (i - idx_A[len(idx_A) - 1]) * len(idx_A)`; `idx_A` is unchanged from the end of the previous iteration, except that if `s[i] == '>'`, `idx_A` has `i` appended to it.**