
Given a Python loop, an initial execution state, and the output states after the first 3 iterations of the loop, determine the output state after all the executions of the loop have finished. 

You must adhere to the text format: Output State: **output state.**

Initial State: `A` contains values calculated based on positions of '>' in `s`, `idx_A` contains indices of all '>' characters in `s`, `B` contains cumulative values calculated based on the positions of '<' in `s` from right to left, `idx_B` contains indices of all '<' characters in `s` in decreasing order (from right to left), `l` is 0, `r` is the length of `B`.
Code of the loop:
for i in range(0, n):
    if s[i] == '>':
        if l < r:
            a = A[l]
            x = r - (l + 2)
            b = B[r - 1]
            if x >= 0:
                b = b - B[x]
                b = b - (idx_B[x] - idx_B[r - 1]) * (x + 1)
            b = (idx_B[r - 1] - i) * (l + 1)
            print(a * 2 + b * 2 + i + 1, end=' ')
        elif r == 0:
            print(n - i, end=' ')
        else:
            a = B[r - 1] + (idx_B[r - 1] - i) * r
            b = A[l - 1]
            if l - r > 0:
                b = b - A[l - r - 1]
                b = b - (idx_A[l - 1] - idx_A[l - r - 1]) * (l - r)
            b = b + (i - idx_A[l - 1]) * r
            print(a * 2 + b * 2 + (n - i), end=' ')
        l += 1
    else:
        r -= 1
        if l <= r:
            if l == 0:
                print(i + 1, end=' ')
            else:
                a = A[l - 1]
                a = a + (i - idx_A[l - 1]) * l
                b = B[r]
                if r - l >= 0:
                    b = b - B[r - l]
                    b = b - (idx_B[r - l] - i) * (r - l)
                b = b + (idx_B[r] - i) * l
                print(a * 2 + b * 2 + i + 1, end=' ')
        elif r == 0:
            print(n - i + (i - idx_A[l - 1]) * 2, end=' ')
        else:
            a = B[r]
            b = A[l - 1]
            if l - r - 1 > 0:
                b = b - A[l - r - 2]
                b = b - (idx_A[l - 1] - idx_A[l - r - 2]) * (l - r - 1)
            b = b + (i - idx_A[l - 1]) * (r + 1)
            print(a * 2 + b * 2 + (n - i), end=' ')


The output state after the loop executes the first 3 of times includes what needed to be true for the loop to execute at least that number of times:

Output State after the loop executes 1 time: `A` contains values calculated based on positions of '>' in `s`, `idx_A` contains indices of all '>' characters in `s`, `B` contains cumulative values calculated based on the positions of '<' in `s` from right to left, `idx_B` contains indices of all '<' characters in `s` in decreasing order (from right to left), `n` must be greater than 0. If `s[i]` is '>', `l` is set to 1, and if `l < r`, `a` is set to `A[0]` and `x` is set to `len(B) - 2`, and `b` is set to `idx_B[r - 1] - i`. If `l` is not less than `r`, `a` is set to `B[r - 1] + (idx_B[r - 1] - i) * r`. If `l - r` is greater than 0, `b` is updated to `A[l - 1] - A[l - r - 1] - (idx_A[l - 1] - idx_A[l - r - 1]) * (l - r) + (i - idx_A[l - 1]) * r`. Otherwise, `b` is updated to `(i - idx_A[l - 1]) * r`. If `s[i]` is not '>', `a` is `A[l - 1] + (i - idx_A[l - 1]) * l` if `l` is greater than 0, and `b` is `B[r] - B[r - l] - (idx_B[r - l] - i) * (r - l) + (idx_B[r] - i) * l` if `r - l >= 0`. If `l` is less than or equal to `r`, `r` remains the length of `B` minus 1. If `l` is greater than `r`, `a` is set to `B[r]` and `b` is updated to `b + (i - idx_A[l - 1]) * (r + 1)`. If `r` is 0, `r` remains 0.

**Output State after the loop executes 2 times**: `A` contains values calculated based on positions of '>' in `s`, `idx_A` contains indices of all '>' characters in `s`, `B` contains cumulative values calculated based on the positions of '<' in `s` from right to left, `idx_B` contains indices of all '<' characters in `s` in decreasing order (from right to left), `n` is greater than 0, `i` is `n`. If `s[i] == '>'`, the value of `l` and `r` are adjusted based on the conditions provided, updating `a` and `b` accordingly. If `l < r`, `a` is set to `A[l]` and `b` is updated based on the value of `x`. If `l` is not less than `r` and `r` is not 0, `a` and `b` are updated based on the provided conditions. If `s[i]` is not '>', `r` is decreased by 1, and `a` and `b` are updated based on the new value of `r` and `l`. `l` is incremented by 1 in the if part.

**Output State after the loop executes 3 times**: `A` contains values calculated based on positions of '>' in `s`, `idx_A` contains indices of all '>' characters in `s`, `B` contains cumulative values calculated based on the positions of '<' in `s` from right to left, `idx_B` contains indices of all '<' characters in `s` in decreasing order (from right to left), `n` is greater than 0, `i` is 0. If `s[i] == '>'`, `l` is incremented by 1, and if `l < r`, `a` is set to `A[l]` and `x` is set to `r - (l + 2)` and `b` is set to `(idx_B[r - 1] - i) * (l + 1)`. Otherwise, if `r` is not 0, `a` is set to `B[r - 1] + (idx_B[r - 1] - i) * r` and `b` is set to `A[l - 1] - A[l - r - 1] - (idx_A[l - 1] - idx_A[l - r - 1]) * (l - r) + (i - idx_A[l - 1]) * r` if `l - r > 0`, otherwise `b` is set to `B[r - 1] + (idx_B[r - 1] - i) * r + (i - idx_A[l - 1]) * r`. If `s[i] != '>'`, `r` is decremented by 1, and if `l` is not 0, `b` is updated to its previous value plus `(idx_B[r] - i) * l`. If `l` is 0 and `r` is not 0, `a` is set to `B[r]` and `b` is updated to `b + (i - idx_A[l - 1]) * (r + 1)`. If `r` is 0, no further changes are made to `a` or `b`.




What is the ouput state after the loop executes all the iterations? Change the values of only the variables in the loop head and body.The state of the other variables in the precondition that are not affected by the loop head and body must remain unchanged.
In your response strictly use the format: Output State: **the output state you calculate.**, and describe this output state in Natural language easily understandable by humans.

