The code snippet `g += (h + 1) // 2` updates the value of `g` by adding the result of `(h + 1) // 2` to its current value.

Let's break down the impact of this code:

1. **Initial Values:**
   - `t` is an integer such that 1 ≤ t ≤ 5 · 10^4.
   - `n` is the first integer input by the user.
   - `k` is the second integer input by the user.
   - `s` is `k`.
   - `i` must be at least 3.
   - `d` is 0.
   - `h` is `(n + 1) // 4 - ((n + 1) // 4 + 1) // 2`.
   - `p` is 2.
   - `g` is `(n + 1) // 2 + ((n + 1) // 4 + 1) // 2`.
   - `k` is less than or equal to \((n + 1) // 2\).

2. **Calculation of `h`:**
   - `h` is calculated as `(n + 1) // 4 - ((n + 1) // 4 + 1) // 2`.
   - Let's denote \( q = (n + 1) // 4 \).
   - Then, `h` becomes \( q - (q + 1) // 2 \).

3. **Calculation of `g` before the update:**
   - `g` is initially \( (n + 1) // 2 + ((n + 1) // 4 + 1) // 2 \).
   - Let's denote \( r = (n + 1) // 2 \) and \( s = ((n + 1) // 4 + 1) // 2 \).
   - Then, `g` is \( r + s \).

4. **Update of `g`:**
   - The code `g += (h + 1) // 2` adds the result of `(h + 1) // 2` to `g`.
   - We need to calculate `(h + 1) // 2`.

5. **Final Calculation:**
   - `h` is \( q - (q + 1) // 2 \).
   - Adding 1 to `h` gives \( h + 1 = q - (q + 1) // 2 + 1 \).
   - Simplifying, \( h + 1 = q - (q // 2 + 1) + 1 = q - q // 2 \).
   - Therefore, \( (h + 1) // 2 = (q - q // 2) // 2 \).

6. **Final Value of `g`:**
   - The new value of `g` is \( g + (h + 1) // 2 \).
   - Substituting the values, \( g = r + s + (q - q // 2) // 2 \).

Therefore, the output state is:
Output State: **`t` is an integer such that 1 ≤ t ≤ 5 · 10^4, `n` is the first integer input by the user, `k` is the second integer input by the user, `s` is `k`, `i` must be at least 3, `d` is 0, `h` is `(n + 1) // 4 - ((n + 1) // 4 + 1) // 2`, `p` is 2, `g` is `(n + 1) // 2 + ((n + 1) // 4 + 1) // 2 + ((n + 1) // 4 - ((n + 1) // 4 + 1) // 2 + 1) // 2`, and `k` is less than or equal to \((n + 1) // 2\).**