To determine what will be printed by the `print(y)` statement, let's break down the initial state and the calculations step by step:

1. **Initial State:**
   - `t` is an integer such that \(1 \leq t \leq 5 \cdot 10^4\).
   - `n` is the first integer input by the user.
   - `k` is the second integer input by the user.
   - `s` is initialized to `k`.
   - `i` is the number of iterations required to reach `s = k`.
   - `d` is 0.
   - `h` is 0.
   - `p` is `i`.
   - `g` is the sum of the series \(\sum_{j=0}^{i-1} \left( \left( \frac{n + 1}{2^j} + 1 \right) // 2 \right)\).
   - `k` is less than or equal to \((n + 1) // 2\).
   - `f` is `k - g`.
   - `y` is \(2^{(i - 1)} \times (2 \times f - 1)\).

2. **Understanding the Variables:**
   - `i` is the number of iterations required to reach `s = k`. Since `s` starts as `k` and no further operations are described to change `s`, `i` is effectively 1.
   - `g` is the sum of the series \(\sum_{j=0}^{i-1} \left( \left( \frac{n + 1}{2^j} + 1 \right) // 2 \right)\). Given `i = 1`, the series only has one term:
     \[
     g = \left( \frac{n + 1}{2^0} + 1 \right) // 2 = \left( n + 1 + 1 \right) // 2 = (n + 2) // 2
     \]
   - `f` is `k - g`. Therefore:
     \[
     f = k - \left( (n + 2) // 2 \right)
     \]
   - `y` is \(2^{(i - 1)} \times (2 \times f - 1)\). Given `i = 1`, this simplifies to:
     \[
     y = 2^{(1 - 1)} \times (2 \times f - 1) = 2^0 \times (2 \times f - 1) = 1 \times (2 \times f - 1) = 2 \times f - 1
     \]

3. **Final Calculation:**
   - Substituting the value of `f`:
     \[
     y = 2 \times \left( k - \left( (n + 2) // 2 \right) \right) - 1
     \]

Therefore, the value of `y` is determined by the formula:
\[
y = 2 \times \left( k - \left( (n + 2) // 2 \right) \right) - 1
\]

Output: **2 \times (k - ((n + 2) // 2)) - 1 (where k is the second integer input by the user and n is the first integer input by the user)**