Based on the initial state provided:

- `a` is explicitly given as 1.
- `L` is a list containing the values `[1, 0, 1]`.
- `tot` is a value less than `k` and `k` is less than or equal to `tot` plus 1.

Given these conditions, let's break down the expression inside the `print` statement:

```python
print(pow * (2 * (k - tot) - 1))
```

Here, `pow` is not defined in the initial state, so it must be a variable that is not mentioned in the initial state. Since no value for `pow` is provided, we cannot determine its exact value. However, we can infer that `pow` is a variable that holds some value, and the expression will be evaluated based on the values of `k` and `tot`.

Since `k` is less than or equal to `tot` plus 1, and `tot` is less than `k`, this implies that `k` and `tot` are consecutive integers. Given the constraints, the only possible values for `k` and `tot` that satisfy both conditions are `k = tot + 1` or `k = tot`.

Let's consider the two cases:

1. If `k = tot + 1`, then `k - tot = 1`, and the expression becomes:
   \[
   pow * (2 * (1) - 1) = pow * (2 - 1) = pow * 1 = pow
   \]

2. If `k = tot`, then `k - tot = 0`, and the expression becomes:
   \[
   pow * (2 * (0) - 1) = pow * (-1) = -pow
   \]

Since `k` and `tot` are consecutive integers and `k` is greater than `tot`, the more likely scenario is `k = tot + 1`. Therefore, the expression simplifies to `pow`.

However, since `pow` is not defined in the initial state, we cannot determine its exact value. Thus, the output will depend on the value of `pow`.

Output: **pow (where pow is the value of the variable pow)**