The given code modifies the value of `list[i]` based on the value of `list[i - 1]`. Specifically, `list[i]` is decreased by twice the value of `list[i - 1]`.

Given the initial state, we know:
- `list[2]` is 1
- `list[1]` is 1
- `list[3]` is 1
- `list[4]` is 1
- The remaining elements are either 0 or 1, with no element greater than 1.

Let's consider the impact of the code on `list[i]`:

1. If `i = 2`, then `list[2] -= 2 * list[1]` → `list[2] -= 2 * 1` → `list[2] -= 2` → `list[2] = 1 - 2` → `list[2] = -1`
2. If `i = 3`, then `list[3] -= 2 * list[2]` → `list[3] -= 2 * (-1)` → `list[3] += 2` → `list[3] = 1 + 2` → `list[3] = 3` (But this contradicts the initial state condition that no element is greater than 1, so we need to consider the constraints carefully.)
3. If `i = 4`, then `list[4] -= 2 * list[3]` → `list[4] -= 2 * (1)` → `list[4] -= 2` → `list[4] = 1 - 2` → `list[4] = -1`

Given the constraints, the only feasible change within the given conditions is when `i = 2`, making `list[2] = -1`. The other elements remain unchanged or need to be reconsidered under the constraint that no element is greater than 1.

Therefore, the Output State is:
Output State: **The list is a list of integers where `list[2]` is -1, `list[1]` is 1, `list[3]` is 1, `list[4]` is 1, and the remaining elements are either 0 or 1, with no element greater than 1.**