To determine the postcondition, we need to ensure that the negation of the if condition is included while retaining all the information from the precondition.

Given:
- Precondition: `t` is an integer such that 1 ≤ t ≤ 10^4, `a` is the first integer read from the input, and `b` is the second integer read from the input. At least one of `a` or `b` is odd.
- If condition: `if ((a - b == -a, a) or (b - a == -b, b)):`

First, let's simplify the if condition:
- `(a - b == -a, a)` is a tuple where the first element is the result of the comparison `a - b == -a`, and the second element is `a`. This condition seems incorrect as written because it doesn't make logical sense in Python. It might be intended to be `a - b == -a`.
- Similarly, `(b - a == -b, b)` is a tuple where the first element is the result of the comparison `b - a == -b`, and the second element is `b`. This condition might be intended to be `b - a == -b`.

Assuming the correct if condition is:
- `if (a - b == -a) or (b - a == -b):`

This simplifies to:
- `if (a - b == -a) or (b - a == -b):`
- `if (2a == b) or (2b == a):`

The negation of this condition would be:
- `not ((2a == b) or (2b == a))`
- `not (2a == b) and not (2b == a)`

Now, combining this with the precondition:

Postcondition: **`t` is an integer such that 1 ≤ t ≤ 10^4, `a` is the first integer read from the input, and `b` is the second integer read from the input. At least one of `a` or `b` is odd, and neither `2a` equals `b` nor `2b` equals `a`.**