Alright, I've got this problem to solve. Let's see what it's asking for. So, Anton has a permutation of size n, and he wants to find a number x using a binary search-like algorithm. But here's the twist: the array isn't sorted, and I can only perform up to two swaps on the permutation before running this binary search. The goal is to rearrange the permutation in such a way that after performing the modified binary search, the value at position l equals x.

First, I need to understand what a permutation is. A permutation of size n is just an array containing each number from 1 to n exactly once, but in any order. So, for example, [2, 3, 1] is a permutation of size 3.

Now, the binary search algorithm described here is a bit unusual. It initializes l to 1 and r to n+1. Then, in each step, if r - l == 1, it stops. Otherwise, it calculates m as the floor of (r + l)/2. If p_m <= x, it sets l = m; otherwise, r = m. This continues until the loop condition is met.

I need to ensure that after performing up to two swaps, when this binary search is run, p_l equals x.

Given that n can be up to 2*10^5 and t (the number of test cases) can be up to 2*10^4, efficiency is key here.

Let me think about how binary search works on a sorted array. In a sorted array, binary search efficiently finds the position where x would be located. However, in this problem, the array isn't sorted, and I can perform up to two swaps to make the binary search yield the correct result.

I need to find a way to adjust the positions of at most two elements so that the binary search process, as defined, leads to p_l being equal to x.

Let me consider the steps of the binary search:

1. Initialize l = 1, r = n + 1.

2. While r - l != 1:

a. Compute m = floor((r + l)/2).

b. If p_m <= x, set l = m.

c. Else, set r = m.

After this loop, p_l should be equal to x.

I need to ensure that after at most two swaps, this condition holds.

First, I should understand what the current behavior is without any swaps. I can simulate the binary search on the given permutation and see where it ends up. If it already ends up with p_l == x, then no swaps are needed, and I can output 0.

If not, I need to perform swaps to make it so.

Let's think about performing one swap. By swapping two elements, I can change the path that the binary search takes. I need to choose which elements to swap such that the binary search ends up at the correct position.

One approach could be to swap the element at the final l position with the element that should be there, which is x. But I need to ensure that this swap doesn't disrupt the previous steps of the binary search.

Alternatively, I could try to bring x to a position where the binary search would naturally find it, by adjusting its position relative to the other elements.

Wait, but since the array isn't sorted, the binary search may not behave as expected.

Let me consider a small example to get a better understanding.

Take n = 3, x = 2, permutation = [3, 2, 1].

Let's simulate the binary search:

Initialize l = 1, r = 4.

First loop:

m = floor((1 + 4)/2) = 2.

p_m = p[2] = 2.

Since 2 <= 2, set l = 2.

Check r - l = 4 - 2 = 2 != 1, so continue.

Second loop:

m = floor((2 + 4)/2) = 3.

p_m = p[3] = 1.

Since 1 <= 2, set l = 3.

Check r - l = 4 - 3 = 1, stop.

Now, p_l = p[3] = 1, which is not equal to x = 2.

So, the binary search ends up at p[3] = 1, but we need it to end up at p_l = x = 2.

One way to fix this is to swap p[3] = 1 with p[2] = 2.

After swapping, the permutation becomes [3, 1, 2].

Now, simulate the binary search again:

Initialize l = 1, r = 4.

First loop:

m = floor((1 + 4)/2) = 2.

p_m = p[2] = 1.

Since 1 <= 2, set l = 2.

Check r - l = 4 - 2 = 2 != 1, continue.

Second loop:

m = floor((2 + 4)/2) = 3.

p_m = p[3] = 2.

Since 2 <= 2, set l = 3.

Check r - l = 4 - 3 = 1, stop.

Now, p_l = p[3] = 2, which matches x = 2.

So, with one swap, we achieved the desired result.

Another example: n = 6, x = 3, permutation = [4, 3, 1, 5, 2, 6].

Simulate binary search:

l = 1, r = 7.

First loop:

m = floor((1 + 7)/2) = 4.

p_m = p[4] = 5.

5 > 3, so r = 4.

Check r - l = 4 - 1 = 3 != 1, continue.

Second loop:

m = floor((1 + 4)/2) = 2.

p_m = p[2] = 3.

3 <= 3, so l = 2.

Check r - l = 4 - 2 = 2 != 1, continue.

Third loop:

m = floor((2 + 4)/2) = 3.

p_m = p[3] = 1.

1 <= 3, so l = 3.

Check r - l = 4 - 3 = 1, stop.

p_l = p[3] = 1 != 3.

Need to perform swaps.

Option 1: Swap p[3] = 1 with p[2] = 3.

New permutation: [4, 1, 3, 5, 2, 6].

Simulate binary search:

l = 1, r = 7.

First loop:

m = 4, p_m = 5 > 3, r = 4.

Second loop:

m = 2, p_m = 1 <= 3, l = 2.

Third loop:

m = 3, p_m = 3 <= 3, l = 3.

p_l = p[3] = 3 == x.

So, one swap suffices.

Another option: Swap p[4] = 5 with p[2] = 3.

New permutation: [4, 5, 1, 3, 2, 6].

Simulate binary search:

l = 1, r = 7.

First loop:

m = 4, p_m = 3 <= 3, l = 4.

Second loop:

m = floor((4 + 7)/2) = 5, p_m = 2 <= 3, l = 5.

Third loop:

m = floor((5 + 7)/2) = 6, p_m = 6 > 3, r = 6.

Check r - l = 6 - 5 = 1, stop.

p_l = p[5] = 2 != 3.

So, this swap doesn't help.

Hence, choosing the right swap is important.

From these examples, it seems that swapping the final p_l with x works.

In the first example, swapping p[3] = 1 with p[2] = 2 made p_l = 2, which is x.

In the second example, swapping p[3] = 1 with p[2] = 3 achieved the same.

So, a general strategy could be:

1. Run the binary search to find the final l.

2. If p_l == x, do nothing.

3. Else, swap p_l with x in the permutation.

This seems to work in the examples above.

But I need to confirm if this always works.

Suppose in the permutation, x is at position pos, and after running the binary search, p_l is some other value.

By swapping p_l and x, p_l becomes x, and x's original position gets p_l's value.

Now, running the binary search again should land on p_l = x.

Wait, but in the second example above, this worked with one swap.

But is there any case where one swap isn't enough, and I need two swaps?

Let me think of a case where one swap isn't sufficient.

Consider n = 4, x = 3, permutation = [1, 4, 2, 3].

Run binary search:

l = 1, r = 5.

First loop:

m = floor((1 + 5)/2) = 3.

p_m = p[3] = 2 <= 3, l = 3.

Check r - l = 5 - 3 = 2 != 1, continue.

Second loop:

m = floor((3 + 5)/2) = 4.

p_m = p[4] = 3 <= 3, l = 4.

Check r - l = 5 - 4 = 1, stop.

p_l = p[4] = 3 == x.

So, no swap needed.

Another case: n = 4, x = 2, permutation = [3, 1, 4, 2].

Run binary search:

l = 1, r = 5.

First loop:

m = 3, p_m = 4 > 2, r = 3.

Second loop:

m = floor((1 + 3)/2) = 2.

p_m = 1 <= 2, l = 2.

Check r - l = 3 - 2 = 1, stop.

p_l = p[2] = 1 != 2.

So, need to swap p[2] = 1 with x = 2.

New permutation: [3, 2, 4, 1].

Run binary search again:

l = 1, r = 5.

First loop:

m = 3, p_m = 4 > 2, r = 3.

Second loop:

m = floor((1 + 3)/2) = 2.

p_m = 2 <= 2, l = 2.

Check r - l = 3 - 2 = 1, stop.

p_l = p[2] = 2 == x.

So, one swap suffices.

Another case: n = 5, x = 3, permutation = [5, 1, 2, 4, 3].

Run binary search:

l = 1, r = 6.

First loop:

m = floor((1 + 6)/2) = 3.

p_m = p[3] = 2 <= 3, l = 3.

Second loop:

m = floor((3 + 6)/2) = 4.

p_m = 4 > 3, r = 4.

Third loop:

m = floor((3 + 4)/2) = 3.

p_m = 2 <= 3, l = 3.

Check r - l = 4 - 3 = 1, stop.

p_l = p[3] = 2 != 3.

Need to swap p[3] = 2 with x = 3.

New permutation: [5, 1, 3, 4, 2].

Run binary search:

l = 1, r = 6.

First loop:

m = 3, p_m = 3 <= 3, l = 3.

Second loop:

m = floor((3 + 6)/2) = 4.

p_m = 4 > 3, r = 4.

Third loop:

m = floor((3 + 4)/2) = 3.

p_m = 3 <= 3, l = 3.

Check r - l = 4 - 3 = 1, stop.

p_l = p[3] = 3 == x.

Again, one swap suffices.

Wait, but the problem says that two operations are always sufficient. In all these cases, one swap was enough. Is there a case where one swap isn't enough?

Let me think of a more tricky case.

Consider n = 4, x = 2, permutation = [4, 3, 1, 2].

Run binary search:

l = 1, r = 5.

First loop:

m = 3, p_m = 1 <= 2, l = 3.

Second loop:

m = floor((3 + 5)/2) = 4.

p_m = 2 <= 2, l = 4.

Check r - l = 5 - 4 = 1, stop.

p_l = p[4] = 2 == x.

No swap needed.

Another case: n = 4, x = 3, permutation = [4, 2, 1, 3].

Run binary search:

l = 1, r = 5.

First loop:

m = 3, p_m = 1 <= 3, l = 3.

Second loop:

m = floor((3 + 5)/2) = 4.

p_m = 3 <= 3, l = 4.

Check r - l = 5 - 4 = 1, stop.

p_l = p[4] = 3 == x.

No swap needed.

Wait, maybe in these cases, no swap is needed.

Let me try n = 4, x = 1, permutation = [4, 3, 2, 1].

Run binary search:

l = 1, r = 5.

First loop:

m = 3, p_m = 2 <= 1? No, 2 > 1, so r = 3.

Second loop:

m = floor((1 + 3)/2) = 2.

p_m = 3 <= 1? No, 3 > 1, so r = 2.

Check r - l = 2 - 1 = 1, stop.

p_l = p[1] = 4 != 1.

Need to swap p[1] = 4 with x = 1.

New permutation: [1, 3, 2, 4].

Run binary search:

l = 1, r = 5.

First loop:

m = 3, p_m = 2 <= 1? No, so r = 3.

Second loop:

m = floor((1 + 3)/2) = 2.

p_m = 3 <= 1? No, r = 2.

Check r - l = 2 - 1 = 1, stop.

p_l = p[1] = 1 == x.

So, again, one swap suffices.

Is there a case where one swap isn't enough?

Let me try n = 5, x = 3, permutation = [5, 4, 2, 1, 3].

Run binary search:

l = 1, r = 6.

First loop:

m = 3, p_m = 2 <= 3, l = 3.

Second loop:

m = floor((3 + 6)/2) = 4.

p_m = 1 <= 3, l = 4.

Third loop:

m = floor((4 + 6)/2) = 5.

p_m = 3 <= 3, l = 5.

Check r - l = 6 - 5 = 1, stop.

p_l = p[5] = 3 == x.

No swap needed.

Another case: n = 5, x = 2, permutation = [5, 4, 3, 1, 2].

Run binary search:

l = 1, r = 6.

First loop:

m = 3, p_m = 3 <= 2? No, r = 3.

Second loop:

m = floor((1 + 3)/2) = 2.

p_m = 4 <= 2? No, r = 2.

Check r - l = 2 - 1 = 1, stop.

p_l = p[1] = 5 != 2.

Need to swap p[1] = 5 with x = 2.

New permutation: [2, 4, 3, 1, 5].

Run binary search:

l = 1, r = 6.

First loop:

m = 3, p_m = 3 <= 2? No, r = 3.

Second loop:

m = floor((1 + 3)/2) = 2.

p_m = 4 <= 2? No, r = 2.

Check r - l = 2 - 1 = 1, stop.

p_l = p[1] = 2 == x.

Again, one swap suffices.

Wait, perhaps in all cases, one swap is enough. But the problem says that two operations are always sufficient, implying that sometimes one might not be enough. But in all my examples, one swap suffices.

Let me try a more tricky case.

n = 6, x = 3, permutation = [6, 5, 4, 3, 2, 1].

Run binary search:

l = 1, r = 7.

First loop:

m = floor((1 + 7)/2) = 4.

p_m = 3 <= 3, l = 4.

Second loop:

m = floor((4 + 7)/2) = 5.

p_m = 2 <= 3, l = 5.

Third loop:

m = floor((5 + 7)/2) = 6.

p_m = 1 <= 3, l = 6.

Check r - l = 7 - 6 = 1, stop.

p_l = p[6] = 1 != 3.

Need to swap p[6] = 1 with x = 3.

New permutation: [6, 5, 4, 3, 2, 3].

Wait, but 3 appears twice, which violates the permutation property. Oh, wait, in the original permutation, x is present only once, so swapping p[6] = 1 with p[pos_of_3] = 3.

Original permutation: [6, 5, 4, 3, 2, 1].

Pos of 3 is 4.

Swap p[6] and p[4]: [6, 5, 4, 1, 2, 3].

Now, run binary search:

l = 1, r = 7.

First loop:

m = 4, p_m = 1 <= 3, l = 4.

Second loop:

m = floor((4 + 7)/2) = 5.

p_m = 2 <= 3, l = 5.

Third loop:

m = floor((5 + 7)/2) = 6.

p_m = 3 <= 3, l = 6.

Check r - l = 7 - 6 = 1, stop.

p_l = p[6] = 3 == x.

So, again, one swap suffices.

Is there a case where one swap isn't enough?

Let me consider n = 4, x = 2, permutation = [3, 4, 1, 2].

Run binary search:

l = 1, r = 5.

First loop:

m = 3, p_m = 1 <= 2, l = 3.

Second loop:

m = floor((3 + 5)/2) = 4.

p_m = 2 <= 2, l = 4.

Check r - l = 5 - 4 = 1, stop.

p_l = p[4] = 2 == x.

No swap needed.

Another case: n = 4, x = 1, permutation = [3, 4, 2, 1].

Run binary search:

l = 1, r = 5.

First loop:

m = 3, p_m = 2 <= 1? No, r = 3.

Second loop:

m = floor((1 + 3)/2) = 2.

p_m = 4 <= 1? No, r = 2.

Check r - l = 2 - 1 = 1, stop.

p_l = p[1] = 3 != 1.

Need to swap p[1] = 3 with x = 1.

New permutation: [1, 4, 2, 3].

Run binary search:

l = 1, r = 5.

First loop:

m = 3, p_m = 2 <= 1? No, r = 3.

Second loop:

m = floor((1 + 3)/2) = 2.

p_m = 4 <= 1? No, r = 2.

Check r - l = 2 - 1 = 1, stop.

p_l = p[1] = 1 == x.

Again, one swap suffices.

Wait, maybe in all cases, one swap is enough. But the problem mentions that two operations are always sufficient, suggesting that there might be cases where one swap isn't enough.

Is there a case where swapping p_l with x doesn't lead to p_l being x after the binary search?

Let me think of such a case.

Suppose n = 5, x = 2, permutation = [4, 3, 5, 1, 2].

Run binary search:

l = 1, r = 6.

First loop:

m = 3, p_m = 5 > 2, r = 3.

Second loop:

m = floor((1 + 3)/2) = 2.

p_m = 3 > 2, r = 2.

Check r - l = 2 - 1 = 1, stop.

p_l = p[1] = 4 != 2.

Swap p[1] = 4 with x = 2.

New permutation: [2, 3, 5, 1, 4].

Run binary search:

l = 1, r = 6.

First loop:

m = 3, p_m = 5 > 2, r = 3.

Second loop:

m = floor((1 + 3)/2) = 2.

p_m = 3 > 2, r = 2.

Check r - l = 2 - 1 = 1, stop.

p_l = p[1] = 2 == x.

Again, one swap suffices.

Wait, perhaps in all cases, one swap is enough. Maybe the problem's mention of two operations being sufficient is just to be safe, although in practice, one swap often suffices.

Alternatively, maybe in some cases, no swap is needed, as in some of the earlier examples.

But I need to confirm if there exists any case where one swap isn't enough to make p_l equal to x.

Let me consider n = 5, x = 3, permutation = [1, 2, 4, 5, 3].

Run binary search:

l = 1, r = 6.

First loop:

m = 3, p_m = 4 > 3, r = 3.

Second loop:

m = floor((1 + 3)/2) = 2.

p_m = 2 <= 3, l = 2.

Check r - l = 3 - 2 = 1, stop.

p_l = p[2] = 2 != 3.

Need to swap p[2] = 2 with x = 3.

New permutation: [1, 3, 4, 5, 2].

Run binary search:

l = 1, r = 6.

First loop:

m = 3, p_m = 4 > 3, r = 3.

Second loop:

m = floor((1 + 3)/2) = 2.

p_m = 3 <= 3, l = 2.

Check r - l = 3 - 2 = 1, stop.

p_l = p[2] = 3 == x.

Again, one swap suffices.

Another case: n = 5, x = 4, permutation = [1, 2, 3, 5, 4].

Run binary search:

l = 1, r = 6.

First loop:

m = 3, p_m = 3 <= 4, l = 3.

Second loop:

m = floor((3 + 6)/2) = 4.

p_m = 5 > 4, r = 4.

Third loop:

m = floor((3 + 4)/2) = 3.

p_m = 3 <= 4, l = 3.

Check r - l = 4 - 3 = 1, stop.

p_l = p[3] = 3 != 4.

Need to swap p[3] = 3 with x = 4.

New permutation: [1, 2, 4, 5, 3].

Run binary search:

l = 1, r = 6.

First loop:

m = 3, p_m = 4 <= 4, l = 3.

Second loop:

m = floor((3 + 6)/2) = 4.

p_m = 5 > 4, r = 4.

Third loop:

m = floor((3 + 4)/2) = 3.

p_m = 4 <= 4, l = 3.

Check r - l = 4 - 3 = 1, stop.

p_l = p[3] = 4 == x.

Again, one swap suffices.

Wait, maybe in all cases, one swap is enough. Perhaps the problem's statement about two operations being sufficient is just to ensure that it's always possible, even in the most complicated cases.

But based on my examples, it seems that one swap is enough when changes are needed.

Perhaps the only case where two swaps are needed is when swapping p_l with x affects the path the binary search takes in a way that requires another swap to correct.

Let me think of such a case.

Consider n = 6, x = 3, permutation = [4, 5, 1, 2, 6, 3].

Run binary search:

l = 1, r = 7.

First loop:

m = floor((1 + 7)/2) = 4.

p_m = 2 <= 3, l = 4.

Second loop:

m = floor((4 + 7)/2) = 5.

p_m = 6 > 3, r = 5.

Third loop:

m = floor((4 + 5)/2) = 4.

p_m = 2 <= 3, l = 4.

Check r - l = 5 - 4 = 1, stop.

p_l = p[4] = 2 != 3.

Need to swap p[4] = 2 with x = 3.

New permutation: [4, 5, 1, 3, 6, 2].

Run binary search again:

l = 1, r = 7.

First loop:

m = 4, p_m = 3 <= 3, l = 4.

Second loop:

m = floor((4 + 7)/2) = 5.

p_m = 6 > 3, r = 5.

Third loop:

m = floor((4 + 5)/2) = 4.

p_m = 3 <= 3, l = 4.

Check r - l = 5 - 4 = 1, stop.

p_l = p[4] = 3 == x.

So, again, one swap suffices.

Wait, maybe in all cases, one swap is enough. Perhaps the problem allows up to two swaps just to make it easier.

But to be safe, I should consider the possibility of needing two swaps.

Let me think about a case where swapping p_l with x doesn't lead to p_l being x after the binary search, and I need an additional swap.

Suppose n = 7, x = 4, permutation = [6, 5, 3, 7, 2, 1, 4].

Run binary search:

l = 1, r = 8.

First loop:

m = floor((1 + 8)/2) = 4.

p_m = 7 > 4, r = 4.

Second loop:

m = floor((1 + 4)/2) = 2.

p_m = 5 > 4, r = 2.

Third loop:

m = floor((1 + 2)/2) = 1.

p_m = 6 > 4, r = 1.

Check r - l = 1 - 1 = 0, stop.

p_l = p[1] = 6 != 4.

Need to swap p[1] = 6 with x = 4.

New permutation: [4, 5, 3, 7, 2, 1, 6].

Run binary search:

l = 1, r = 8.

First loop:

m = 4, p_m = 7 > 4, r = 4.

Second loop:

m = floor((1 + 4)/2) = 2.

p_m = 5 > 4, r = 2.

Third loop:

m = floor((1 + 2)/2) = 1.

p_m = 4 <= 4, l = 1.

Check r - l = 2 - 1 = 1, stop.

p_l = p[1] = 4 == x.

So, again, one swap suffices.

Wait, maybe in all cases, one swap is enough. Perhaps the problem allows two swaps to cover all possible cases, but in practice, one swap is sufficient.

Alternatively, maybe in some cases, no swap is needed.

Looking back at the examples, it seems that one swap is enough when a swap is needed.

Hence, perhaps the general strategy is:

- Run the binary search to find the final l.

- If p_l == x, do nothing.

- Else, swap p_l with x.

- After this swap, running the binary search should result in p_l == x.

But to confirm, I need to think about whether there could be a case where swapping p_l with x doesn't lead to p_l == x after the binary search.

Suppose that after swapping p_l with x, the binary search takes a different path due to the changed values, leading to a different l where p_l != x.

Is that possible?

Let me consider n = 5, x = 2, permutation = [3, 4, 1, 5, 2].

Run binary search:

l = 1, r = 6.

First loop:

m = 3, p_m = 1 <= 2, l = 3.

Second loop:

m = floor((3 + 6)/2) = 4.

p_m = 5 > 2, r = 4.

Third loop:

m = floor((3 + 4)/2) = 3.

p_m = 1 <= 2, l = 3.

Check r - l = 4 - 3 = 1, stop.

p_l = p[3] = 1 != 2.

Swap p[3] = 1 with x = 2.

New permutation: [3, 4, 2, 5, 1].

Run binary search:

l = 1, r = 6.

First loop:

m = 3, p_m = 2 <= 2, l = 3.

Second loop:

m = floor((3 + 6)/2) = 4.

p_m = 5 > 2, r = 4.

Third loop:

m = floor((3 + 4)/2) = 3.

p_m = 2 <= 2, l = 3.

Check r - l = 4 - 3 = 1, stop.

p_l = p[3] = 2 == x.

Again, one swap suffices.

Wait, perhaps in all cases, one swap is enough. Maybe the problem allows up to two swaps to cover cases where two swaps are needed, but in practice, one swap suffices when changes are needed.

Alternatively, maybe in some cases, no swaps are needed.

Looking back at the earlier examples, it seems that one swap is sufficient when a swap is needed.

Hence, perhaps the general strategy is:

- Perform the binary search to find the final l.

- If p_l == x, do nothing.

- Else, swap p_l with x.

- Output the number of swaps (1 in this case) and the swap operation.

This seems straightforward and efficient, which is good given the constraints.

Now, considering the time constraints, with t up to