To determine what will be printed by the given `print` statement, let's break down the initial state and the logic step by step:

### Initial State:
- `t` is an integer such that \(1 \leq t \leq 10^4\).
- `_` is 0 (this variable is not used in the given context).
- `n` is an input integer.
- `ar` is a list of integers provided by the user input.
- `res` is a list of integers where each element `res[i]` is equal to `mex - ar[i]` for each index `i` from 0 to `n-1`.
- `mex` is the result of repeatedly subtracting each element of `ar` from the initial value `n` as long as `mex > mex - ar[i]` holds true. The final value of `mex` will be the smallest non-negative integer that is not present in the list `ar` after all iterations.

### Step-by-Step Analysis:
1. **Determine `mex`**:
   - Start with `mex = n`.
   - For each element `ar[i]` in the list `ar`, check if `mex > mex - ar[i]`.
   - If the condition holds, update `mex` to `mex - ar[i]`.
   - Continue this process until `mex` is the smallest non-negative integer that is not present in the list `ar`.

2. **Construct `res`**:
   - For each index `i` from 0 to `n-1`, compute `res[i] = mex - ar[i]`.

3. **Print `res`**:
   - Convert each element of `res` to a string.
   - Join these strings with a space.
   - Print the resulting string.

### Example Calculation:
Let's assume the following inputs for clarity:
- `n = 5`
- `ar = [0, 1, 2, 3, 4]`

#### Step 1: Determine `mex`:
- Start with `mex = 5`.
- Check each element in `ar`:
  - `ar[0] = 0`: `mex > mex - 0` is true, so `mex = 5 - 0 = 5`.
  - `ar[1] = 1`: `mex > mex - 1` is true, so `mex = 5 - 1 = 4`.
  - `ar[2] = 2`: `mex > mex - 2` is true, so `mex = 4 - 2 = 2`.
  - `ar[3] = 3`: `mex > mex - 3` is false, so `mex` remains 2.
  - `ar[4] = 4`: `mex > mex - 4` is false, so `mex` remains 2.

The smallest non-negative integer not in `ar` is 5, but since we are updating `mex` to the smallest value that is not in `ar`, `mex` will be 5.

#### Step 2: Construct `res`:
- `res[0] = mex - ar[0] = 5 - 0 = 5`
- `res[1] = mex - ar[1] = 5 - 1 = 4`
- `res[2] = mex - ar[2] = 5 - 2 = 3`
- `res[3] = mex - ar[3] = 5 - 3 = 2`
- `res[4] = mex - ar[4] = 5 - 4 = 1`

So, `res = [5, 4, 3, 2, 1]`.

#### Step 3: Print `res`:
- Convert each element of `res` to a string: `['5', '4', '3', '2', '1']`.
- Join these strings with a space: `'5 4 3 2 1'`.

### Final Output:
Output: **5 4 3 2 1**

This is the output based on the given initial state and the logic described.