Alright, I've got this problem to solve. Let's see what it's asking for. So, I have an array of integers, and I can perform exactly k operations on it. In each operation, I select a contiguous subarray (which could be empty) and insert the sum of this subarray anywhere in the array. My goal is to maximize the sum of the array after k operations, and since the sum can be very large, I need to output it modulo 10^9 + 7.

First, I need to understand what exactly an operation is. So, I select a contiguous subarray, calculate its sum, and then insert that sum back into the array at any position. This means the array can grow in size with each operation, right? Because I'm inserting a new element equal to the sum of the subarray.

Wait, but the problem says "insert the sum anywhere in the array." Does that mean I'm adding a new element to the array, or am I replacing some existing elements? Based on the wording, it seems like I'm adding a new element to the array. So, with each operation, the array size increases by one.

But let's look at the first test case in the example:

Input:

2 2

-4 -7

Output:

999999996

Explanation:

It's advantageous to take an empty subarray twice and insert the sum (zero) anywhere, resulting in the array [-4, -7, 0, 0], with a sum of -11, which modulo 10^9 + 7 is 999,999,996.

Okay, so in this case, they're choosing the empty subarray and inserting zero each time. So, the array starts with two elements, and after two operations, it has four elements.

Another test case:

Input:

3 3

2 2 8

Output:

96

Explanation:

Take the sum of the entire array (12) and insert it three times, resulting in the array [2, 2, 8, 12, 24, 48], with a sum of 96.

Wait, but in the first operation, they take the sum of the entire array (12) and insert it, making the array [2, 2, 8, 12]. Then, they take the sum again (2 + 2 + 8 + 12 = 24) and insert 24, making [2, 2, 8, 12, 24]. Finally, take the sum again (2+2+8+12+24=48) and insert 48, making [2, 2, 8, 12, 24, 48], with a total sum of 96.

But hold on, the problem says to insert the sum of a subarray anywhere in the array. In this explanation, they're always inserting the sum at the end, but according to the problem, I can insert the sum anywhere in the array. Does the position where I insert the sum matter?

In the first test case, they inserted zeros at the end, but presumably, inserting them elsewhere wouldn't change the total sum. So, maybe the position doesn't matter for the sum.

Let me think about this. The sum of the array is just the sum of all its elements, regardless of the order. So, no matter where I insert the sum of a subarray, the total sum of the array will increase by that subarray's sum.

Wait, but when I insert the sum of a subarray into the array, that sum becomes another element in the array, which can be part of future subarrays. So, it's not just adding the sum to the total; it's adding an element that can be included in future operations.

This seems a bit tricky. Let's try to find a pattern or a mathematical formula to maximize the sum after k operations.

First, observe that each operation allows me to select any contiguous subarray (including empty) and insert its sum into the array.

An empty subarray has a sum of zero, as shown in the first test case.

So, one strategy is to always choose the empty subarray and insert zero. But in the first test case, that leads to a sum of -11, which is better than the sum of the original array (-4 + -7 = -11), but in other cases, it might not be optimal.

In the second test case, they're choosing the entire array each time and inserting its sum, leading to exponential growth in the sum.

Wait, in the second test case, the sum after each operation is:

Initial: [2,2,8], sum=12

After first operation: [2,2,8,12], sum=24

After second operation: [2,2,8,12,24], sum=48

After third operation: [2,2,8,12,24,48], sum=96

So, each time, the sum doubles.

Wait, 12, 24, 48, 96... yes, it's doubling each time.

Wait, but actually, 12 to 24 is doubling, 24 to 48 is doubling, 48 to 96 is doubling. But according to the explanation, they're inserting the sum of the array at each step, which includes the sums inserted in previous steps.

Wait, but 12 is the sum of the initial array, then they insert 12, making the new sum 24, then insert 24, making it 48, and so on.

So, it seems like each insertion adds the current sum of the array, which includes the sums inserted in previous steps.

Wait, but in the first test case, they insert zero twice, and the sum remains -11. So, in that case, inserting zero doesn't change the sum.

So, perhaps the optimal strategy is to choose the subarray with the maximum sum and insert it multiple times.

Let me think about this.

Suppose I have an array with both positive and negative numbers. If I choose a subarray with a positive sum and insert it, the total sum increases by that subarray's sum. Then, in the next operation, if I choose the same subarray again and insert it, the sum increases by the same amount again.

Wait, but in the second test case, they're choosing the entire array each time, which includes the sums inserted in previous steps, leading to exponential growth.

So, perhaps there's a way to choose subarrays in such a way that the sum inserted in each step is maximized based on previous insertions.

This seems complicated. Maybe I need to find a way to model this mathematically.

Let me denote S as the sum of the current array.

Initially, S = sum of a.

In each operation, I choose a subarray with sum x, and insert x into the array, which increases S by x.

So, after one operation, S becomes S + x.

Then, in the next operation, I can choose another subarray with sum y and insert y, making S = S + x + y.

But, if I choose to insert S itself, then S becomes S + S = 2S.

Wait, in the second test case, they're choosing the entire array each time and inserting S, leading to S, 2S, 4S, 8S, and so on.

Wait, but in the second test case, after the first insertion, the array becomes [2,2,8,12], with S=24.

Then, inserting S=24 makes the array [2,2,8,12,24], with S=48.

Then, inserting S=48 makes the array [2,2,8,12,24,48], with S=96.

So, S is doubling each time.

Wait, but 12 to 24 is doubling, 24 to 48 is doubling, 48 to 96 is doubling.

Wait, but 12 is the initial sum, then after first insertion, S=24, which is 12 + 12.

Wait, but according to the explanation, they're inserting the sum of the array at each step, which is S.

So, in each step, S becomes S + S = 2S.

Hence, after k insertions, S becomes S * 2^k.

Wait, but in the first test case, they insert zero twice, so S remains -11, which is -11 + 0 + 0.

So, in that case, it's not doubling; it's just adding zero each time.

So, perhaps the general formula is S + x1 + x2 + ... + xk, where each xi is the sum of some subarray.

But in the second test case, by choosing xi = S each time, S becomes S + S + 2S + ... , which is S * 2^k.

Wait, but in the second test case, they're choosing xi = S each time, so S becomes S + S, then S + 2S, and so on.

Wait, but in terms of the sum, it's S + S = 2S after first insertion, then 2S + 2S = 4S after second insertion, and so on, up to S * 2^k after k insertions.

So, in that case, choosing xi = S each time leads to S * 2^k.

Is this always the maximum possible sum?

Well, in the second test case, yes, because S is positive, and doubling it each time maximizes the sum.

But in the first test case, S is negative, so doubling it would make it more negative, which is worse.

Hence, in that case, it's better to insert zero each time, which doesn't change the sum.

So, perhaps the general strategy is:

- If S > 0, then insert S each time, leading to S * 2^k.

- If S <= 0, then insert zero each time, leading to S + 0 * k = S.

But wait, in the first test case, S = -4 + -7 = -11, which is less than zero, so inserting zero each time is better than inserting negative sums.

But, is there a case where S > 0, but inserting a subarray sum larger than S is possible?

Wait, in the second test case, S = 2 + 2 + 8 = 12, and inserting S each time leads to S * 2^k.

Is there a way to get a larger sum by inserting a different subarray sum?

For example, suppose I insert the sum of a subarray with a sum larger than S.

But, since S is the sum of the entire array, any subarray sum would be less than or equal to S.

Wait, unless there are positive and negative numbers in such a way that a subarray sum can be larger than S.

Wait, no, the sum of any subarray cannot be larger than the sum of the entire array if all elements are positive.

But if there are negative elements, it's possible that a subarray sum is larger than S.

Wait, no, if S is the sum of the entire array, and a subarray is a part of it, its sum should be less than or equal to S.

Unless the subarray sum is negative, in which case, excluding that subarray would make the sum larger.

But, in this problem, when inserting a subarray sum, I'm adding that sum to the array, not replacing anything.

Wait, perhaps I'm missing something.

Let me think differently.

Let me consider that in each operation, I can choose any contiguous subarray, compute its sum x, and insert x into the array.

This inserted x can then be part of future subarrays in future operations.

So, the array grows with each operation, and the new elements can be included in future subarrays.

Hence, the sum S after k operations is the initial sum plus the sum of the inserted elements.

Each inserted element is the sum of some subarray from the previous array.

So, to maximize S, I need to maximize the sum of the inserted elements.

Now, in each operation, I can choose any contiguous subarray, compute its sum, and insert it.

So, to maximize the inserted sum in each operation, I should choose the subarray with the maximum sum available in the current array.

Hence, in each operation, I should find the subarray with the maximum sum in the current array and insert it.

This way, in each step, I'm adding the largest possible sum to the array.

In the second test case, the entire array has the maximum sum, so inserting S each time is optimal.

In the first test case, the maximum subarray sum is zero (from an empty subarray), so inserting zero each time is optimal.

But, is there a case where inserting a subarray sum larger than S is possible?

Wait, perhaps not, because S is the sum of the entire array, and any subarray sum is less than or equal to S.

Wait, unless there are negative elements.

Wait, suppose the array is [1, -2, 3].

The sum S = 1 + (-2) + 3 = 2.

But the subarray [3] has sum 3, which is larger than S.

Wait, no, [3] has sum 3, which is larger than S=2.

Wait, but in this case, if I insert 3, the new array is [1, -2, 3, 3], with sum 1 -2 +3 +3 = 5.

If I had inserted S=2, the new array would be [1, -2, 3, 2], with sum 1 -2 +3 +2 = 4.

So, inserting the maximum subarray sum (3) is better than inserting S (2).

Hence, in this case, inserting the maximum subarray sum is better than inserting S.

Hence, my previous assumption that inserting S each time is always optimal is wrong.

So, perhaps the strategy should be to, in each operation, find the maximum subarray sum and insert it.

In the previous example, starting with [1, -2, 3], S=2.

Insert 3, new array [1, -2, 3, 3], S=5.

Then, find the maximum subarray sum, which is 3 again, insert 3, new array [1, -2, 3, 3, 3], S=8.

And so on, leading to S = 2 + 3*k.

Whereas, if I had inserted S each time, S would be 2, then 4, then 8, etc., which is 2^(k+1) - 2.

Wait, but in this case, inserting the maximum subarray sum leads to S = 2 + 3*k, whereas inserting S each time leads to S = 2 * 2^k.

For k=1, S=5 vs 4.

For k=2, S=8 vs 8.

For k=3, S=11 vs 16.

So, for k >=2, inserting S is better.

Hence, perhaps there's a trade-off, and inserting S is better in the long run when S is positive.

But in this specific case, inserting the maximum subarray sum leads to S = 2 + 3*k.

Whereas inserting S each time leads to S = 2 * (2^k).

Clearly, for k >=2, 2 * (2^k) > 2 + 3*k.

Hence, inserting S each time is better for k >=2.

Wait, but in the earlier example with k=2, inserting the maximum subarray sum gives S=8, which matches inserting S each time.

For k=3, inserting the maximum subarray sum gives S=11, but inserting S each time gives S=16, which is better.

Hence, perhaps inserting S each time is better in the long run.

So, perhaps the general strategy is:

- Find the maximum possible sum that can be inserted in each operation, considering that inserting S each time leads to exponential growth.

But, in the case where the maximum subarray sum is larger than S, inserting the maximum subarray sum can be better in the short term, but in the long term, inserting S leads to better growth.

Wait, in the previous example, inserting S=2 leads to S = 2 * 2^k, while inserting the maximum subarray sum of 3 leads to S=2 + 3*k.

For k=1: 4 vs 5.

For k=2: 8 vs 8.

For k=3: 16 vs 11.

So, for k=1, inserting the maximum subarray sum is better, but for k>=2, inserting S is better.

Hence, perhaps the optimal strategy is:

- If k=1, insert the maximum subarray sum.

- If k>=2, insert S each time.

But, in the second test case, with k=3, inserting S each time leads to S * 2^3 = 12 * 8 = 96, which matches the example.

In the first test case, with k=2, inserting zero each time leads to S=-11, which is better than inserting the maximum subarray sum of zero.

In the third test case, with n=1, a=[7], k=7.

Inserting S=7 each time leads to S * 2^7 = 7 * 128 = 896, which matches the example.

In the fourth test case, n=5, a=[4, -2, 8, -12, 9], k=1.

Since k=1, insert the maximum subarray sum.

The maximum subarray sum is 4 + (-2) + 8 = 10.

Insert 10, new array is [4, -2, 8, -12, 9, 10], sum=17.

Which matches the example.

Hence, the general strategy seems to be:

- If k >=1, insert the maximum subarray sum once.

- If k >=2, insert S each subsequent time.

Wait, but in the first test case, k=2, and they insert zero twice.

But according to this strategy, for k>=2, insert S each time.

In the first test case, S=-11, so inserting S each time would lead to S + S + S = -33, which is worse than inserting zero twice (-11).

Hence, perhaps the strategy needs to be adjusted.

Perhaps:

- If S > 0, insert S each time.

- If S <=0, insert the maximum subarray sum, which could be zero or positive.

Wait, in the first test case, S=-11, which is less than zero, so insert the maximum subarray sum, which is zero, k times.

In the second test case, S=12 >0, so insert S each time, leading to S * 2^k.

In the third test case, S=7 >0, so insert S each time, leading to S * 2^k.

In the fourth test case, S=4 + (-2) + 8 + (-12) +9 = 7, which is positive, but since k=1, insert the maximum subarray sum once, which is 10, leading to S=17.

Wait, but according to the earlier strategy, if S>0, insert S each time.

In the fourth test case, S=7, k=1, inserting S would lead to S + S =14, but the example shows sum=17 by inserting the maximum subarray sum of 10.

Hence, perhaps for k=1, it's better to insert the maximum subarray sum, and for k>=2, insert S each time.

In that case, for the fourth test case, with k=1, inserting the maximum subarray sum of 10 leads to S=17, which is better than inserting S=7, which would lead to S=14.

Similarly, in the first test case, with k=2, inserting the maximum subarray sum (zero) twice leads to S=-11, which is better than inserting S=-11 twice, leading to S=-33.

Hence, perhaps the strategy is:

- If k=1, insert the maximum subarray sum once.

- If k>=2, insert S each time.

But, in the second test case, with k=3, inserting S each time leads to S * 2^3 = 96, which matches the example.

In the third test case, with k=7, inserting S each time leads to S * 2^7 =7*128=896, which matches the example.

In the fourth test case, with k=1, inserting the maximum subarray sum leads to S=17, which is better than inserting S=7, leading to S=14.

Hence, perhaps the general formula is:

- Find the maximum subarray sum, let's call it M.

- If k=1, then S += M.

- Else, S becomes S * 2^(k-1) + M * (2^(k-1) -1).

Wait, let's think differently.

If k >=1, we can insert M once, and then insert S each time after that.

So, after the first insertion of M, S becomes S + M.

Then, for the remaining k-1 operations, we insert S each time, which doubles S each time.

Hence, after k-1 insertions of S, S becomes (S + M) * 2^(k-1).

But, in the fourth test case, S=7, M=10, k=1.

So, S += M = 7 +10 =17.

Which matches the example.

In the first test case, S=-11, M=0, k=2.

Insert M=0 once, S becomes -11 +0 =-11.

Then, insert S=-11 once, S becomes -11 + (-11) =-22.

But in the example, they insert zero twice, leading to S=-11.

Wait, perhaps there is a better strategy.

Wait, in the first test case, if we insert zero twice, S remains -11.

But according to the above formula, inserting M=0 first, then inserting S=-11, leading to S=-22, which is worse.

Hence, perhaps the strategy