The code snippet `ans += (n + i) // cnt` modifies the value of `ans` by adding the result of the expression `(n + i) // cnt`. The other variables `n`, `m`, `root`, and `cnt` remain unchanged.

Given the initial state:
- `n` is a positive integer (1 ≤ `n` ≤ 2 · 10^6)
- `m` is a positive integer (1 ≤ `m` ≤ 2 · 10^6)
- `ans` is `n`
- `root` is `int(math.sqrt(n)) + 1`
- `cnt` is `i * i`

After the code execution:
- `ans` is updated to `n + (n + i) // cnt`
- `n`, `m`, `root`, and `cnt` retain their initial values

Output State: **`n` is a positive integer (1 ≤ `n` ≤ 2 · 10^6); `m` is a positive integer (1 ≤ `m` ≤ 2 · 10^6); `ans` is `n + (n + i) // cnt`; `root` is `int(math.sqrt(n)) + 1`; `cnt` is `i * i`**