Based on the initial state provided:

- `t` remains 0
- `T` remains as the initial positive integer
- `info` remains unchanged
- `a` remains as the first element of `info` converted to an integer
- `b` remains as the second element of `info` converted to an integer
- `suma` is the sum of all `x` values calculated during the loop's iterations until `a - i * (i - 1) <= 0` for all `i` in the range 1 to `b`

We need to determine what `suma` is. The loop calculates the sum of `x` values where `x` is derived from the formula `a - i * (i - 1)` for each `i` in the range from 1 to `b`.

Let's break it down:

1. For `i = 1`: `a - 1 * (1 - 1) = a - 0 = a`
2. For `i = 2`: `a - 2 * (2 - 1) = a - 2`
3. For `i = 3`: `a - 3 * (3 - 1) = a - 6`
4. Continue this pattern up to `i = b`.

So, `suma` is the sum of these values:
\[ suma = a + (a - 2) + (a - 6) + \ldots + (a - b(b-1)/2) \]

This simplifies to:
\[ suma = b \cdot a - (0 + 2 + 6 + \ldots + b(b-1)/2) \]
\[ suma = b \cdot a - \frac{b(b-1)(b+1)}{6} \]

Given the print statement `print(suma - 1)`, we need to subtract 1 from `suma`.

Therefore, the output will be:
Output: **suma - 1 (where suma is the sum of all x values calculated as described)**