To determine the final output state after the loop completes all its iterations, we need to understand how the `sum` variable is being updated in each iteration.

The loop iterates from `i = 2` to `i = n` (inclusive), and in each iteration, it updates the `sum` variable according to the formula:
\[ \text{sum} += (i \times i - (i - 1) \times (i - 1)) \times i \]

This simplifies to:
\[ \text{sum} += (i^2 - (i - 1)^2) \times i \]
\[ \text{sum} += (i^2 - (i^2 - 2i + 1)) \times i \]
\[ \text{sum} += (2i - 1) \times i \]
\[ \text{sum} += 2i^2 - i \]

Let's calculate the `sum` step by step for a general `n`:

1. For `i = 2`, the increment to `sum` is:
\[ 2 \times 2^2 - 2 = 8 - 2 = 6 \]
\[ \text{sum} = 1 + 6 = 7 \]

2. For `i = 3`, the increment to `sum` is:
\[ 2 \times 3^2 - 3 = 18 - 3 = 15 \]
\[ \text{sum} = 7 + 15 = 22 \]

3. For `i = 4`, the increment to `sum` is:
\[ 2 \times 4^2 - 4 = 32 - 4 = 28 \]
\[ \text{sum} = 22 + 28 = 50 \]

We can generalize this to say that for each `i` from 2 to `n`, the `sum` is incremented by \(2i^2 - i\). The final value of `sum` after the loop completes all iterations is the sum of these increments starting from `i = 2` to `i = n`.

The formula for the final `sum` can be written as:
\[ \text{sum} = 1 + \sum_{i=2}^{n} (2i^2 - i) \]

This can be simplified further, but for the sake of this problem, we can just compute it iteratively for a given `n`.

Given the initial state and the increments described, the final output state after the loop completes all iterations is:

Output State: **the sum is calculated as 1 plus the sum of (2i^2 - i) for i from 2 to n.**

To express this more concretely, if `n` were a specific value, we could compute the exact sum. However, without a specific `n`, we express the final state in terms of `n`.

In natural language, the final state is that `t` remains greater than or equal to 1, `n` remains the input integer, and `sum` is the result of starting at 1 and adding \(2i^2 - i\) for each `i` from 2 to `n`.