Let's break down the problem step by step:

1. **Identify the loop condition**: The loop condition is `(x + y) * x <= n` and `(x + y) * y <= m`.

2. **Current values**:
   - `x` is 2
   - `y` is 1
   - `n` must be at least 5
   - `m` must be at least 7
   - `cnt` is 12 (this variable is not part of the loop condition and does not need adjustment)

3. **Calculate `(x + y) * x` and `(x + y) * y` with current values**:
   - `(x + y) * x = (2 + 1) * 2 = 3 * 2 = 6`
   - `(x + y) * y = (2 + 1) * 1 = 3 * 1 = 3`

4. **Check the loop condition with current values**:
   - `(x + y) * x <= n` becomes `6 <= n`
   - `(x + y) * y <= m` becomes `3 <= m`

5. **Determine necessary adjustments**:
   - For `6 <= n` to be true, `n` must be at least 6.
   - For `3 <= m` to be true, `m` must be at least 3. However, since `m` must already be at least 7 (from the given state), this condition is already satisfied.

Therefore, the only necessary adjustment is to ensure that `n` is at least 6.

**Final Answer**:
State: **`x` is 2, `n` must be at least 6, `m` must be at least 7, `y` is 1, and `cnt` is 12**