Reasoning:  
The function `func_1` is intended to compute the difference between the sum of cubes of the first `n` natural numbers and the sum of the first `n` natural numbers. However, the implementation in the provided code calculates the sum of the first `n` natural numbers (`sum_n`) and then squares it to get `sum_cubes_n`. The final step is to subtract `sum_n` from `sum_cubes_n`.

The formula for the sum of the first `n` natural numbers is:
\[ \text{sum\_n} = \frac{n(n + 1)}{2} \]

The formula for the sum of the cubes of the first `n` natural numbers is:
\[ \text{sum\_cubes\_n} = \left( \frac{n(n + 1)}{2} \right)^2 \]

Thus, the function should return:
\[ \text{sum\_cubes\_n} - \text{sum\_n} = \left( \frac{n(n + 1)}{2} \right)^2 - \frac{n(n + 1)}{2} \]

However, the provided implementation correctly computes this difference. Let's verify the correctness with the given test cases:

1. For `n = 3`:
   - Sum of the first 3 natural numbers: \( \text{sum\_n} = \frac{3(3 + 1)}{2} = 6 \)
   - Sum of the cubes of the first 3 natural numbers: \( \text{sum\_cubes\_n} = 6^2 = 36 \)
   - Difference: \( 36 - 6 = 30 \)

2. For `n = 5`:
   - Sum of the first 5 natural numbers: \( \text{sum\_n} = \frac{5(5 + 1)}{2} = 15 \)
   - Sum of the cubes of the first 5 natural numbers: \( \text{sum\_cubes\_n} = 15^2 = 225 \)
   - Difference: \( 225 - 15 = 210 \)

3. For `n = 2`:
   - Sum of the first 2 natural numbers: \( \text{sum\_n} = \frac{2(2 + 1)}{2} = 3 \)
   - Sum of the cubes of the first 2 natural numbers: \( \text{sum\_cubes\_n} = 3^2 = 9 \)
   - Difference: \( 9 - 3 = 6 \)

All test cases match the expected results, so the function is correct.

Correctness: **True**