Let's break down the initial state and the print statement step by step:

1. **Initial State:**
   - `v` is the return value of `func_2()`.
   - `n` must be at least 1.
   - `k` is the return value of `func_3()`.
   - `i` is `n - 2`.

2. **Print Statement:**
   ```python
   print(f'? 1 {i * n}', flush=True)
   ```

Given the initial state:
- `i` is defined as `n - 2`.
- Therefore, `i * n` becomes `(n - 2) * n`.

Since `n` must be at least 1, let's consider the smallest possible value for `n`, which is 1:
- If `n = 1`, then `i = 1 - 2 = -1`, and `i * n = -1 * 1 = -1`.

However, since `n` can be any integer greater than or equal to 1, the expression `i * n` will depend on the actual value of `n`.

To generalize, if `n` is any integer greater than or equal to 1, then `i = n - 2` and `i * n = (n - 2) * n`.

Thus, the print statement will output a string with the value of `i * n` inserted into it.

Output: **'? 1 [i * n]' where i = n - 2 and i * n = (n - 2) * n**