Let's break down the initial state and the print statement step by step:

1. **Initial State Variables:**
   - `i` is 1.
   - `n` is 1.
   - `k` must be 1 (though it's not used in the print statement).
   - `cnt` is 0.
   - `l` is `func_2() + 1`.
   - The condition `cnt == 0 and l == n + 1` is true.

2. **Determine the Value of `l`:**
   - Since `cnt` is 0 and the condition `cnt == 0 and l == n + 1` is true, it implies that `l == n + 1`.
   - Given `n` is 1, `l` must be `1 + 1 = 2`.

3. **Determine the Value of `v`:**
   - The value of `v` is not explicitly given, but it must be such that the condition holds true. Since `l` is 2, and `l` is `func_2() + 1`, `func_2()` must return 1 (because `1 + 1 = 2`).

4. **Evaluate the Print Statement:**
   - The print statement is `print(f'! {i * v}', flush=True)`.
   - We know `i` is 1, so `i * v` is simply `v`.
   - Therefore, the print statement becomes `print(f'! {v}', flush=True)`.

Given the above steps, the value of `v` must be such that the condition holds, but since it's not explicitly defined, we can only say that `v` is a value that satisfies the condition. However, based on the context, if `func_2()` returns 1, then `v` could be any value that does not contradict this, but typically in such problems, `v` would be 1 unless otherwise specified.

Thus, the most precise description based on the given information is:

Output: **! 1**