Let's break down the initial state and the print statement step by step:

1. **Initial State:**
   - `i` is 2.
   - `n` is 1.
   - `k` must be 1.
   - `cnt` is 0.
   - `l` is `func_2()` + 1.
   - The condition `cnt == 0 and l == n + 1` is true.

2. **Determine the Value of `l`:**
   - Since `cnt` is 0 and the condition `cnt == 0 and l == n + 1` is true, it implies that `l == n + 1`.
   - Given `n` is 1, `l` must be `1 + 1 = 2`.

3. **Determine the Value of `v`:**
   - The value of `v` is not explicitly given, but it is used in the print statement as `i * v`.
   - Since `i` is 2, the expression `i * v` becomes `2 * v`.

4. **Print Statement:**
   - The print statement is `print(f'! {i * v}', flush=True)`.
   - Substituting the value of `i`, it becomes `print(f'! {2 * v}', flush=True)`.

Given the information, the print statement will output a string that includes the product of `2` and `v`.

Output: **! 2 * v**