Output State: **`gaps` is an empty list, `ans` is 0, `i` is 0, `next_elem` is `a[1] + (n if 0 == x - 1 else 0)`, `gap` is `next_elem - a[0] - 1`**

Explanation: The code calculates the value of `gap` as `next_elem - a[i] - 1`. Given the initial state, `i` is 0, so `a[i]` is `a[0]`. The value of `next_elem` is defined as `a[(0 + 1) % x] + (n if 0 == x - 1 else 0)`, which simplifies to `a[1] + (n if 0 == x - 1 else 0)` since `(0 + 1) % x` equals 1. Thus, `gap` is calculated as `next_elem - a[0] - 1`, which is `a[1] + (n if 0 == x - 1 else 0) - a[0] - 1`. All other variables remain unchanged.