Let's break down the initial state and the code snippet step by step:

### Initial State:
- `n` remains unchanged.
- `i` is `n-1`.
- `res` is the sum of `(i + 1) * (2 * i + 1)` for all `i` from 0 to `n-1`.

### Code Snippet:
```python
print(res, n << 1)
```

### Step-by-Step Analysis:
1. **Understanding `n` and `i`**:
   - `n` is a given integer that remains unchanged.
   - `i` is defined as `n-1`.

2. **Calculating `res`**:
   - `res` is the sum of the expression `(i + 1) * (2 * i + 1)` for all `i` from 0 to `n-1`.
   - Let's break down the expression:
     - For `i = 0`: `(0 + 1) * (2 * 0 + 1) = 1 * 1 = 1`
     - For `i = 1`: `(1 + 1) * (2 * 1 + 1) = 2 * 3 = 6`
     - For `i = 2`: `(2 + 1) * (2 * 2 + 1) = 3 * 5 = 15`
     - For `i = 3`: `(3 + 1) * (2 * 3 + 1) = 4 * 7 = 28`
     - And so on...

   - The general formula for each term in the sum is:
     \[
     (i + 1) * (2 * i + 1)
     \]
   - The sum of these terms from `i = 0` to `i = n-1` can be written as:
     \[
     \sum_{i=0}^{n-1} (i + 1) * (2 * i + 1)
     \]

3. **Bitwise Shift Operation**:
   - `n << 1` is a bitwise left shift operation, which multiplies `n` by 2.
   - Therefore, `n << 1` is equivalent to `2 * n`.

### Final Output:
- The `print` statement will output the value of `res` and the value of `n << 1`.
- `res` is the sum of the terms \((i + 1) * (2 * i + 1)\) for all `i` from 0 to `n-1`.
- `n << 1` is `2 * n`.

Output: **res, 2 * n (where res is the sum of (i + 1) * (2 * i + 1) for all i from 0 to n-1 and n is the given integer)**