Let's break down the initial state and the code snippet step by step to determine what will be printed.

### Initial State:
1. **`n`**: This is the input integer.
2. **`i`**: This is `n-1`.
3. **`res`**: This is the sum of `(i + 1) * (2 * i + 1)` for `i` from 0 to `n-1`.
4. **`mat`**: This is a list of `n` lists, where each list contains integers from 1 to `n`.

### Code Snippet:
```python
print(res, n << 1)
```

### Step-by-Step Analysis:
1. **`n`**: This is the input integer. Let's denote it as `n`.

2. **`i`**: This is `n-1`. So, `i` is `n-1`.

3. **`res`**: This is the sum of `(i + 1) * (2 * i + 1)` for `i` from 0 to `n-1`. Let's compute this sum:
   - For `i = 0`: `(0 + 1) * (2 * 0 + 1) = 1 * 1 = 1`
   - For `i = 1`: `(1 + 1) * (2 * 1 + 1) = 2 * 3 = 6`
   - For `i = 2`: `(2 + 1) * (2 * 2 + 1) = 3 * 5 = 15`
   - For `i = 3`: `(3 + 1) * (2 * 3 + 1) = 4 * 7 = 28`
   - And so on...

   The general term for the sum is:
   \[
   \text{res} = \sum_{i=0}^{n-1} (i + 1) * (2 * i + 1)
   \]

   Let's simplify this sum:
   \[
   (i + 1) * (2 * i + 1) = 2i^2 + 3i + 1
   \]
   So,
   \[
   \text{res} = \sum_{i=0}^{n-1} (2i^2 + 3i + 1)
   \]

   This can be broken down into:
   \[
   \text{res} = 2 \sum_{i=0}^{n-1} i^2 + 3 \sum_{i=0}^{n-1} i + \sum_{i=0}^{n-1} 1
   \]

   Using the formulas for the sum of squares and the sum of integers:
   \[
   \sum_{i=0}^{n-1} i^2 = \frac{(n-1) * n * (2n-1)}{6}
   \]
   \[
   \sum_{i=0}^{n-1} i = \frac{(n-1) * n}{2}
   \]
   \[
   \sum_{i=0}^{n-1} 1 = n
   \]

   Substituting these into the equation for `res`:
   \[
   \text{res} = 2 \left( \frac{(n-1) * n * (2n-1)}{6} \right) + 3 \left( \frac{(n-1) * n}{2} \right) + n
   \]
   Simplifying further:
   \[
   \text{res} = \frac{(n-1) * n * (2n-1)}{3} + \frac{3 * (n-1) * n}{2} + n
   \]
   \[
   \text{res} = \frac{2(n-1) * n * (2n-1) + 9(n-1) * n + 6n}{6}
   \]
   \[
   \text{res} = \frac{(n-1) * n * (4n - 2 + 9) + 6n}{6}
   \]
   \[
   \text{res} = \frac{(n-1) * n * (4n + 7) + 6n}{6}
   \]
   \[
   \text{res} = \frac{(n-1) * n * (4n + 7) + 6n}{6}
   \]
   \[
   \text{res} = \frac{(n-1) * n * (4n + 7) + 6n}{6}
   \]

   This is the formula for `res`.

4. **`n << 1`**: This is a bitwise left shift operation, which is equivalent to multiplying `n` by 2. So, `n << 1` is `2 * n`.

### Final Output:
The `print(res, n << 1)` statement will print the value of `res` and `2 * n`.

Output: **\(\frac{(n-1) * n * (4n + 7) + 6n}{6}\), 2 * n (where \( n \) is the input integer)**