Let's break down the initial state and the code snippet step by step to determine what will be printed.

### Initial State:
- `n` remains unchanged.
- `i` is `n-1`.
- `res` is the sum of \((i + 1) \times (2 \times i + 1)\) for \(i\) from 0 to \(n-1\).

### Code Snippet:
```python
print(res, n << 1)
```

### Step-by-Step Analysis:
1. **Understanding `res`**:
   - `res` is calculated as the sum of \((i + 1) \times (2 \times i + 1)\) for \(i\) ranging from 0 to \(n-1\).
   - Let's break down the formula:
     - For \(i = 0\): \((0 + 1) \times (2 \times 0 + 1) = 1 \times 1 = 1\)
     - For \(i = 1\): \((1 + 1) \times (2 \times 1 + 1) = 2 \times 3 = 6\)
     - For \(i = 2\): \((2 + 1) \times (2 \times 2 + 1) = 3 \times 5 = 15\)
     - And so on...

   - The general term for each \(i\) is \((i + 1) \times (2 \times i + 1)\).
   - The sum of these terms from \(i = 0\) to \(i = n-1\) is:
     \[
     \text{res} = \sum_{i=0}^{n-1} (i + 1) \times (2 \times i + 1)
     \]

2. **Understanding `n << 1`**:
   - The `<<` operator is a bitwise left shift operator.
   - Shifting `n` left by 1 bit is equivalent to multiplying `n` by 2.
   - Therefore, `n << 1` is \(2 \times n\).

### Final Output:
- The `print` statement will output the value of `res` and the value of `n << 1`.
- Since `res` is the sum of the terms \((i + 1) \times (2 \times i + 1)\) for \(i\) from 0 to \(n-1\), and `n << 1` is \(2 \times n\), the output will be:

Output: **res, 2 * n (where res is the sum of (i + 1) * (2 * i + 1) for i from 0 to n-1 and n is the value of n)**