To determine what will be printed, we need to carefully analyze the initial state and the provided Python code snippet.

### Initial State Breakdown:

1. **List `b`**:
   - The list `b` is defined with specific elements and conditions:
     - `b[0] = -1000000000.0`
     - `b[1] = r1`
     - `b[2] = r2`
     - `b[3] = 2000000000.0`
     - `b[4] = 2000000000.0`
     - `b[5] = 2000000000.0 if 2000000000.0 - r2 > r2 - r1 else r2 + 1`
     - `b[6] = 4000000000.0 - r2 if 2000000000.0 - r2 > 2000000000.0 - (2000000000.0 - r2) else 2000000000.0 + 1`
     - `b[7] = (4000000000.0 - r2) + (2000000000.0 - r2) if 2000000000.0 - r2 > r2 - r1 else (4000000000.0 - r2) + 1`
     - `b[8] = (2000000000.0 if 2000000000.0 - r2 > r2 - r1 else r2 + 1) + (2000000000.0 - r2)`

2. **Variable `u`**:
   - `u` is set to 0.

3. **Variables `c` and `d`**:
   - `c` and `d` are the values returned by the function `r()`.
   - The relationship between `c` and `d` is described: if `c < d`, then `c < d`; otherwise, `c >= d`.

### Code Analysis:

The print statement is:
```python
print(b[(d - 1) * 2] - b[(c - 1) * 2])
```

- `(d - 1) * 2` and `(c - 1) * 2` are indices into the list `b`.
- We need to determine the values of these indices based on the values of `c` and `d`.

### Determining Indices:

- Since `c` and `d` are returned by `r()` and their relationship is given (`c < d` or `c >= d`), we need to consider the possible values of `c` and `d` relative to the length of the list `b`, which is 9.
- The valid indices for `b` are from 0 to 8.

### Possible Values of Indices:

- `(d - 1) * 2` must be an even number between 0 and 8.
- `(c - 1) * 2` must also be an even number between 0 and 8.

### Evaluating the Expression:

Given the constraints and the nature of the indices, let's assume `c` and `d` are such that they map to valid indices in `b`.

- For example, if `c = 1` and `d = 2`:
  - `(d - 1) * 2 = (2 - 1) * 2 = 2`
  - `(c - 1) * 2 = (1 - 1) * 2 = 0`
  - The expression becomes `b[2] - b[0] = r2 - (-1000000000.0) = r2 + 1000000000.0`

- If `c = 2` and `d = 3`:
  - `(d - 1) * 2 = (3 - 1) * 2 = 4`
  - `(c - 1) * 2 = (2 - 1) * 2 = 2`
  - The expression becomes `b[4] - b[2] = 2000000000.0 - r2`

### General Case:

Without specific values for `c` and `d`, we can generalize the output as the difference between the elements at the calculated indices in the list `b`.

### Final Output:

Based on the general case and the structure of the problem, the output will be the difference between the elements at the indices `(d - 1) * 2` and `(c - 1) * 2` in the list `b`.

Output: **b[(d - 1) * 2] - b[(c - 1) * 2] (where b is the list defined in the initial state and c, d are values returned by r())**