Alright, I've got this problem to solve. Let me read it carefully.

So, there's this physical education lesson where students line up and are assigned numbers based on a specific pattern involving a parameter k, where k > 1. The pattern repeats every 2k - 2 positions. The first k positions are numbered 1 through k, and the next k-2 positions are numbered k-1 down to 2. Then this pattern repeats.

For example, if k=3, the pattern would be: 1,2,3,2,1,2,3,2,1,2,3,2,1,...

Given Vasya's position n and the number x he received, I need to find how many natural numbers k > 1 satisfy the condition that at position n, the number assigned is x.

Constraints:

- t (number of test cases) is between 1 and 100.

- For each test case, n and x are integers where 1 ≤ x < n ≤ 10^9.

First, I need to understand the pattern of numbering.

Let's take k=3 as an example:

Positions: 1,2,3,4,5,6,7,8,9,10,...

Numbers: 1,2,3,2,1,2,3,2,1,2,...

Pattern repeats every 2k-2 = 4 positions: [1,2,3,2]

Similarly, for k=2: [1,2,1,2,...] repeats every 2 positions.

For k=4: [1,2,3,4,3,2] repeats every 6 positions.

Wait, for k=4, 2k-2=6, so the pattern is [1,2,3,4,3,2].

I need to generalize this pattern.

Given any k > 1, the pattern is:

- Positions 1 to k: numbers 1 to k

- Positions k+1 to 2k-2: numbers k-1 down to 2

- Then the pattern repeats.

So, the period is 2k - 2.

Now, for a given n and x, I need to find all k > 1 such that at position n, the number is x.

First, I need to find the position n within one period.

Since the period is 2k - 2, the position n modulo (2k - 2) will give me the position within the pattern.

Let m = 2k - 2.

Then, position n in the pattern is equivalent to n mod m.

But m = 2k - 2, so m + 2 = 2k.

Thus, k = (m + 2)/2.

But k must be an integer, so m must be even.

Wait, k is an integer greater than 1, so m = 2k - 2 is even only if k is integer, which it is.

But I need to ensure that k is integer, so m must be even.

Wait, m = 2k - 2, which is even for integer k.

So, I need to consider m such that m = 2k - 2, where k is integer >1.

Now, n mod m corresponds to a position in the pattern.

The pattern is:

- Positions 1 to k: numbers 1 to k

- Positions k+1 to 2k-2: numbers k-1 down to 2

So, if n mod m is p, then:

- If 1 ≤ p ≤ k, number is p

- If k+1 ≤ p ≤ 2k-2, number is 2k - p

Wait, let's verify that.

For k=3:

m = 4

Pattern:

p=1: 1

p=2: 2

p=3: 3

p=4: 2

Which is 2k - p = 6 - p:

For p=4: 6-4=2, which matches.

For p=3: 6-3=3, which matches.

For p=2: 6-2=4, which doesn't match the pattern. Wait, that's wrong.

Wait, for p from k+1 to 2k-2, the number is k - (p - k)

Wait, let's think differently.

In the first k positions, numbers are 1 to k.

In the next k-2 positions, numbers are k-1 down to 2.

So, for p from 1 to k: number = p

For p from k+1 to 2k-2: number = 2k - p

Let's check for k=3:

p=1: 1

p=2:2

p=3:3

p=4:2k - p =6-4=2

Which matches the pattern.

For k=4:

m=6

p=1:1

p=2:2

p=3:3

p=4:4

p=5:3

p=6:2

Which matches 2k - p for p from 5 to 6: 8-5=3, 8-6=2.

So, general formula:

If p = n mod m

If 1 ≤ p ≤ k, number = p

If k+1 ≤ p ≤ m, number = 2k - p

Now, m = 2k - 2

So, k = (m + 2)/2

Now, given n and x, I need to find k such that at position n, the number is x.

First, find p = n mod m

But m = 2k - 2, and k is unknown.

This seems tricky.

Alternatively, let's think in terms of m.

Let m be the period, m = 2k - 2.

Then, k = (m + 2)/2

Now, p = n mod m

If 1 ≤ p ≤ k, x = p

Else, x = 2k - p

So, for given n and x, and unknown m (period), I need to find m such that:

Case 1: 1 ≤ p ≤ k, x = p

Which implies p = x, and 1 ≤ x ≤ k

Since k = (m + 2)/2, so x ≤ (m + 2)/2

Also, p = n mod m = x

So, n ≡ x mod m

Moreover, m must divide n - x, i.e., m divides n - x.

Similarly, from x ≤ (m + 2)/2, we have m ≥ 2x - 2

Also, since k > 1, m > 0

Case 2: k+1 ≤ p ≤ m, x = 2k - p

With p = n mod m

And k = (m + 2)/2

So, x = 2*(m + 2)/2 - p = m + 2 - p

Thus, x = m + 2 - p

Which implies p = m + 2 - x

Also, since p = n mod m, p ∈ [1, m]

So, n mod m = m + 2 - x

Which implies n ≡ m + 2 - x mod m

But n ≡ m + 2 - x mod m ⇒ n ≡ 2 - x mod m

Because m ≡ 0 mod m

So, n ≡ 2 - x mod m

Which implies m divides n - (2 - x)

i.e., m divides n + x - 2

Also, from p = m + 2 - x ≤ m, which is always true since x ≥ 1, m ≥ 2

And p ≥ k + 1 = (m + 2)/2 + 1 = (m + 4)/2

So, m + 2 - x ≥ (m + 4)/2

Which simplifies to:

m + 2 - x ≥ (m + 4)/2

Multiply both sides by 2:

2m + 4 - 2x ≥ m + 4

Subtract m + 4 from both sides:

m - 2x ≥ 0 ⇒ m ≥ 2x

So, m ≥ 2x

But earlier, from case 1, m ≥ 2x - 2

But in case 2, m ≥ 2x

So, overall, m ≥ 2x - 2

Now, summarizing both cases:

- Case 1: m divides n - x and m ≥ 2x - 2

- Case 2: m divides n + x - 2 and m ≥ 2x

Also, m must be even because m = 2k - 2, and k is integer >1.

So, m is even.

Now, to find all m that satisfy either:

1. m divides n - x and m ≥ 2x - 2

2. m divides n + x - 2 and m ≥ 2x

And m is even.

Then, for each such m, k = (m + 2)/2

Since k must be integer >1, m must be even and m ≥ 2.

Now, to find the number of such m, which are even divisors of either n - x or n + x - 2, satisfying the respective inequalities.

So, first, find all even divisors m of n - x such that m ≥ 2x - 2

And all even divisors m of n + x - 2 such that m ≥ 2x

Then, the total number is the number of unique m satisfying either condition.

But need to make sure that m is positive, since m = 2k - 2 > 0 for k >1.

Also, m must be even.

Now, to implement this efficiently, considering that n and x can be up to 1e9, I need an efficient way to find the divisors.

First, I need to find the divisors of n - x and n + x - 2.

But n and x can be up to 1e9, so n - x can be up to 1e9, and n + x - 2 up to 2e9 - 2.

Factoring numbers up to 1e9 efficiently requires an efficient divisor function.

I can write a function to find all divisors of a number up to 1e9.

Given that t is up to 100, and for each test case, n and x are up to 1e9, I need an efficient way to factorize these numbers.

An efficient way is to iterate from 1 to sqrt(x), and for each i that divides x, add both i and x/i to the list of divisors, unless i == x/i.

Then, sort the list of divisors.

But since m must be even, I only consider even divisors.

Now, for each test case:

- Compute n - x and n + x - 2

- Find all even divisors of n - x that are >= 2x - 2

- Find all even divisors of n + x - 2 that are >= 2x

- Combine these lists and count the unique m

- Then, for each m, k = (m + 2)/2, which should be integer.

Wait, m must be even, so (m + 2)/2 is integer.

Now, implement a function to find all even divisors of a number.

Also, need to handle cases where n - x or n + x - 2 is zero or negative.

Wait, n > x, as per constraints, since 1 ≤ x < n ≤ 1e9, so n - x >=1

And n + x - 2 >= 1 + 1 - 2 = 0

But n + x - 2 can be zero, but in the divisor function, zero is not handled.

So, need to handle n + x - 2 == 0 separately.

If n + x - 2 == 0, then m must divide 0, which is undefined, but m >0, so no solution in this case.

Wait, m divides 0 means m can be any divisor of 0, but m >0, so perhaps m can be any positive integer, but in practice, m must divide n + x - 2, which is 0.

But m must divide 0, which is true for any m, but m must be positive.

But in programming terms, we cannot find divisors of 0.

So, need to handle n + x - 2 == 0 separately.

Similarly, n - x can be 1 or higher.

Wait, n - x >=1, since n > x >=1.

Wait, no, if n=2, x=1, then n - x=1

n + x -2 =2 +1 -2=1

So, n + x -2 can be 1 or higher.

Wait, but if x=1, n=2, then n + x -2=1

If x=1, n=1, but n > x, so n >=2, x >=1

So, n + x -2 >=1

Hence, n + x -2 >=1

So, no need to handle n + x -2 ==0

Wait, but according to constraints, n > x >=1, so n -x >=1

And n + x -2 >= n -x >=1, wait no.

Wait, n + x -2 can be less than n -x

Wait, for n=2, x=1, n + x -2=1

For n=3, x=1, n + x -2=2

For n=3, x=2, n + x -2=3

Wait, n + x -2 can be as low as 1.

But in the divisor function, I need to find divisors of n -x and n +x -2, which are both >=1.

So, no problem.

Now, in the code, there is a function func_1(x) which seems to return all divisors of x.

Let me look at it.

def func_1(x):

output1 = []

output2 = []

for i in range(1, int(x ** 0.5) +1):

if x % i ==0:

output1.append(i)

output2.append(int(x /i))

output1.reverse()

return output2 + output1

This function finds all divisors of x by iterating from 1 to sqrt(x), appending i and x/i if x % i ==0, then reversing output1 and concatenating output2 + output1.

This should give all divisors in ascending order.

Now, in the main loop:

for each test case:

read n and x

initialize output list

check if (n + x -2) %2 ==0

if yes, call func_1(n + x -2) to get all divisors

for each divisor s:

if (s +2) %2 ==0 and (s +2)/2 >=x

append (s +2)/2 to output

then, check if (n -x) %2 ==0

if yes, call func_1(n -x) to get all divisors

for each divisor s:

if (s +2) %2 ==0 and (s +2)/2 >=x

append (s +2)/2 to output

then, make output a set to remove duplicates, then list(set(output))

Finally, print the length of output.

Wait, but in the code provided, it's missing the print statements.

It should be:

print(len(output))

But in the given program, it's not there.

Wait, the code provided is incomplete, as it ends with the list(set(output)) line without printing anything.

Assuming that the print statement is there in the actual code, but missing in the provided snippet.

Now, let's verify if this approach is correct.

Recall that:

- For case 1: m divides n -x and m >=2x -2

- For case 2: m divides n +x -2 and m >=2x

And m must be even.

In the code:

- If (n + x -2) %2 ==0, get divisors s of n +x -2

For each s, if (s +2) %2 ==0 and (s +2)/2 >=x, append (s +2)/2 to output

Similarly, if (n -x) %2 ==0, get divisors s of n -x

For each s, if (s +2) %2 ==0 and (s +2)/2 >=x, append (s +2)/2 to output

Then, remove duplicates and count.

Wait, but m must be even, and m = s, where s is a divisor.

Then, k = (m +2)/2 = (s +2)/2

Condition (s +2)/2 >=x implies k >=x

Also, (s +2) %2 ==0 ensures that s is even, since m must be even.

Wait, m = s, and m must be even, so s must be even.

But in the code, it checks (s +2) %2 ==0, which is equivalent to s being even.

Because s +2 is even only if s is even.

Wait, s is even if s %2 ==0

And (s +2) %2 ==0 iff s %2 ==0

So, this is correct.

Also, m >=2x -2 for case 1, which translates to s >=2x -2

But in the code, it's checking (s +2)/2 >=x, which is equivalent to s >=2x -2

Because (s +2)/2 >=x ⇒ s +2 >=2x ⇒ s >=2x -2

Similarly, for case 2, m >=2x, which is s >=2x

But in the code, it's using the same condition (s +2)/2 >=x, which is s >=2x -2

Wait, but for case 2, m >=2x, which is s >=2x

But (s +2)/2 >=x is s >=2x -2

So, for case 2, it should be s >=2x, but the code has s >=2x -2

This seems incorrect.

Wait, perhaps I missed something.

Wait, in case 2, m >=2x

But the condition in the code is (s +2)/2 >=x, which is s >=2x -2

But for case 2, m must be >=2x

So, the condition should be s >=2x

But in the code, it's s >=2x -2

Which allows s >=2x -2 for both cases.

But for case 2, it should be s >=2x

So, perhaps it's incorrect.

Wait, maybe I need to reconcile this.

In case 1: m divides n -x and m >=2x -2

In case 2: m divides n +x -2 and m >=2x

But in the code, for both cases, it's using (s +2)/2 >=x, which is s >=2x -2

So, for case 2, it's allowing s >=2x -2, but it should be s >=2x

So, perhaps it's incorrect.

Wait, maybe not.

Wait, for case 2, m >=2x

And k = (m +2)/2 >=x +1

Wait, k >=x +1?

Wait, k = (m +2)/2 >=x

Because (m +2)/2 >=x ⇒ m >=2x -2

Wait, but for case 2, m >=2x

So, perhaps there is confusion here.

Wait, perhaps I need to re-express the conditions.

Given that for case 1: m divides n -x and m >=2x -2

For case 2: m divides n +x -2 and m >=2x

But in the code, it's combining both conditions into (s +2)/2 >=x, which is s >=2x -2

But for case 2, m >=2x, which is stronger than s >=2x -2

So, perhaps it's incorrect.

Wait, perhaps the condition needs to be adjusted.

Wait, perhaps in case 2, since m >=2x, and m is even, so s >=2x

But in the code, it's s >=2x -2

Which would allow s =2x -2, but for case 2, s must be >=2x

So, it's incorrect.

Wait, perhaps the condition (s +2)/2 >=x is not sufficient for case 2.

Because for case 2, m >=2x, but (s +2)/2 >=x is equivalent to s >=2x -2

Which is weaker than m >=2x

So, perhaps I need to adjust the condition.

Wait, maybe I need to handle the two cases separately.

For case 1: m divides n -x and m >=2x -2

For case 2: m divides n +x -2 and m >=2x

And m is even.

So, for case 1, collect m from divisors of n -x where m is even and m >=2x -2

For case 2, collect m from divisors of n +x -2 where m is even and m >=2x

Then, take the union of these m's and count them.

In the code, it's collecting m's where m is even and m >=2x -2 for both cases.

Which is incorrect for case 2, because it should be m >=2x

So, to fix this, need to adjust the condition for case 2 to m >=2x

But in the code, it's m >=2x -2 for both cases.

So, it's incorrect.

To fix this, need to have:

- For case 1: m divides n -x and m >=2x -2

- For case 2: m divides n +x -2 and m >=2x

And m is even.

So, in code, for case 1:

if (n -x) % m ==0 and m >=2x -2 and m is even

For case 2:

if (n +x -2) % m ==0 and m >=2x and m is even

So, perhaps the code needs to separate these conditions properly.

But in the given code, it's combining both cases with m >=2x -2

Which is incorrect for case 2.

So, the program is incorrect.

Wait, but perhaps there is a mathematical equivalence that I'm missing.

Let me check with an example.

Take the first test case:

n=10, x=2

Compute n -x =8, n +x -2=10

Find even divisors of 8 and 10, with m >=2x -2=2 and m >=2x=4 for case 2.

For case 1: even divisors of 8 that are >=2

Divisors of 8:1,2,4,8

Even divisors:2,4,8

All >=2

So, m=2,4,8

For case 2: even divisors of 10 that are >=4

Divisors of 10:1,2,5,10

Even divisors:2,10

Those >=4:10

So, m=10

Total m's:2,4,8,10

Which matches the first test case output of 4.

But according to the code, it's collecting m's where m >=2x -2 for both cases.

Wait, in the code, for case 1: m >=2x -2

For case 2: m >=2x -2

But in reality, for case 2, it should be m >=2x

But in this example, 2x=4, 2x -2=2

So, for case 1: m >=2

For case 2: m >=4

But in the code, it's m >=2 for both, which would include m=2 in case 2, but according to the correct condition, m >=4 for case 2.

But in the example, m=2 is only included in case 1, and m=10 in case 2.

So, perhaps in the code, it's correctly handling it because m=2 is only included if it divides n -x, and m=10 is included in case 2.

Wait, but according to the code, for case 2, it includes m=2 if it divides n +x -2 and m >=2x -2, which would be m >=2

But in reality, for case 2, m should be >=2x=4

So, m=2 should not be included in case 2.

But in the example, m=2 divides n +x -2=10, but m=2 <2x=4, so it should be excluded.

But in the code, it includes m=2 if m >=2x -2=2

So, it includes m=2, which is incorrect.

But in the example, m=2 is only included in case 1, where m >=2x -2=2

So, in case 1, m=2,4,8

In case 2, m=10

Total unique m's:2,4,8,10

Which is correct.

So, perhaps it works in this case.

Wait, but according to the correct logic, for case 2, m should be >=2x=4, so m=2 should be excluded from case 2.

But in the code, it includes m=2 in case 2 if m >=2x -2=2

But in the example, m=2 is only included in case 1, which is correct because m=2 <2x=4, so it should not be included in case 2.

But in the code, for case 2, it checks m >=2x -2, which is incorrect.

Wait, perhaps in the code, for case 2, it should be m >=2x

But it's written as m >=2x -2

Which is incorrect.

But in the first test case, it happens to work because m=2 is only included in case 1, and in case 2, m=10 is included, which is >=4.

But in other test cases, it might include m's that should not be included.

Let me check another test case.

Take the second test case:

n=3, x=1

Compute n -x=2, n +x -2=2

Case 1: m divides 2 and m >=2*1 -2=0

But m must be >=2x -2=0, but m >=2 anyway, since m=2k -2 and k>=2 ⇒ m>=2

So, m divides 2 and m >=2

Divisors of 2:1,2

Even divisors:2

So, m=2

Case 2: m divides n +x -2=2 and m >=2x=2

So, m=2

So, m=2 is included in both cases.

But in reality, k=(m +2)/2

For m=2, k=2

Check if for k=2, position 3 is assigned number 1.

For k=2, pattern is [1,2,1,2,...]

Position 3:1, which matches x=1

So, m=2 is valid.

Hence, output=1

Which matches the second test case.

But according to the code, it would include m=2 in both cases, but since it's the same m, it's included once.

So, again, it works.

But is this always correct?

Let me consider a case where m >=2x -2 includes m's that should not be included in case 2.

Take n=76, x=4

Compute n -x=72, n +x -2=78

Case 1: m divides 72 and m >=6 (since 2x -2=6)

Even divisors of 72 that are >=6:

Divisors of 72:1,2,3,4,6,8,9,12,18,24,36,72

Even divisors:2,4,6,8,12,18,24,36,72

Those >=6:6,8,12,18,24,36,72

Case 2: m divides 78 and m >=8 (since 2x=8)

Divisors of 78:1,2,3,6,13,26,39,78

Even divisors:2,6,26,78

Those >=8:26,78

So, total m's:6,8,12,18,24,36,72,26,78

Unique m's:6,8,12,18,24,26,36,72,78 ⇒9 m's

Which matches the third test case output of 9.

But according to the code, it would include m >=2x -2=6 for both cases, which in case 1 is correct, and in case 2, it should be m >=8, but the code uses m >=6 for both.

So, in this case, it would include m=6 in case 2, which should not be included because m >=8.

But for m=6, let's check:

For case 1: m=6 divides 72 and m>=6 ⇒ included

For case 2: m=6 divides 78 and m>=6 ⇒ included

But according to the correct condition, in case 2, m >=8.

So, m=6 should not be included in case 2.

But in the code, it includes m=6 in case 2 because m >=2x -2=6

Which is incorrect.

But in this particular test case, m=6 is also included in case 1, so it's already included.

So, the unique m's remain the same.

Hence, the code happens to produce the correct output.

But this seems like a coincidence.

Let me think of a test case where this would cause an error.

Suppose n=100, x=99

Compute n -x=1, n +x -2=97

Case 1: m divides 1 and m >=196 -2=194

Divisors of 1:1

But 1 <194, so no m in case 1

Case 2: m divides 97 and m >=198

Divisors of 97:1,97

Even divisors: none (97 is odd)

So, no m in case 2

Hence, output=0

Which matches the fourth test case.

But according to the code, for case 1:

If (n -x) %2 ==0, which is 1 %2 ==0? No, so skip

For case 2: (n +x -2) %2 ==0, 97 %2 ==1, so skip

Hence, output=0

Which is correct.

Another test case: n=1000000000, x=500000000

Compute n -x=500000000, n +x -2=999999998

Case 1: m divides 500000000 and m >=999999998

But m must divide 500000000 and m >=999999998

So, m=1000000000 (assuming it divides 500000000, but 1000000000 >500000000, so no

Wait, m must divide 500000000 and m >=999999998

But 500000000 <999999998, so no m in case 1

Case 2: m divides 999999998 and m >=1000000000

So, m >=1000000000 and m divides 999999998

But 999999998 <1000000000, so no m in case 2

Hence, output=0

But according to the example, output=1

Wait, the fifth test case in the example is:

1000000000 500000000

Output:1

Wait, but according to my reasoning, output should be 0

But in the example, it's 1

So, perhaps I'm missing something.

Wait, perhaps there is a k that satisfies the conditions.

Let me check.

For k=500000001

m=2k -2=1000000000

Now, check if m divides n -x or n +x -2

n -x=500000000

m=1000000000 divides 500000000? No, 1000000000 does not divide 500000000

Wait, 500000000 /1000000000=0.5, not integer

Similarly, n +x -2=999999998

Does m=1000000000 divide 999999998? No

So, no m satisfies the conditions.

But according to the example, output=1

Wait, perhaps I'm missing a k.

Wait, maybe k=500000001 is not the only possible k.

Wait, perhaps k=2

m=2k -2=2

Check if m divides n -x=500000000 and m >=2x -2=999999998

But m=2 <999999998, so no

Or m divides n +x -2=999999998 and m >=2x=1000000000

m=2 <1000000000, so no

Wait, perhaps there is another k.

Wait, maybe k=1000000001

m=2*1000000001 -2=2000000000

Does m divide n -x=500000000? 2000000000 does not divide 500000000

Wait, 500000000 /2000000000=0.25, not integer

Does m divide n +x -2=999999998? 999999998 /2000000000 not integer

So, no.

I must be missing something.

Wait, perhaps k=500000000

m=2*500000000 -2=999999998

Check if m divides n -x=500000000: 999999998 does not divide 500000000

Check if m divides n +x -2=999999998: yes, m=999999998 divides 999999998

And m >=2x=1000000000? 999999998 <1000000000, so no

Hence, not valid.

Wait, but according to the example, output=1, so there must be one k that satisfies.

Wait, perhaps k=500000000 is acceptable.

Wait, k must be integer >1

k=500000000

m=2*500000000 -2=999999998

Check case 2: m divides n +x -2=999999998 and m >=2x=1000000000

m=999999998 divides 999999998, but m <1000000000, so not acceptable.

Hence, output should be 0, but according to the example, it's 1.

Wait, perhaps I'm missing another k.

Wait, perhaps k=1

But k must be >1

So, indeed, output should be 0, but the example shows 1.

Wait, perhaps the example is incorrect.

Or perhaps I'm misunderstanding something.

Wait, maybe k=500000000 is acceptable.

Wait, k=500000000

m=999999998

Case 2: m divides n +x -2=999999998, which it does.

And m >=2x=1000000000? 999999998 <1000000000, so not acceptable.

Hence, output should be 0, but the example shows 1.

Wait, perhaps there is a mistake in the example.

Wait, perhaps for k=500000000, m=999999998

But m >=2x=1000000000 is not satisfied, so it should not be included.

Hence, output should be 0, but the example shows 1.

Wait, perhaps the example is incorrect.

Alternatively, perhaps there is a misinterpretation in the condition.

Wait, perhaps in case 2, m >=2x is not necessary.

Wait, going back to the original condition.

In case 2, m >=2x is derived from p = m +2 -x >=k +1 = (m +2)/2 +1

Wait, perhaps I made a mistake in deriving the condition for case 2.

Let me re-examine the condition for case 2.

In case 2, p = m +2 -x

And p >=k +1 = (m +2)/2 +1

So, m +2 -x >= (m +2)/2 +1

Multiply both sides by 2:

2m +4 -2x >= m +2 +2

Simplify: 2m -2x >= m +2

Subtract m from both sides: m -2x >=2 ⇒ m >=2x +2

Wait, earlier I had m >=2x

But according to this, m >=2x +2

So, perhaps I made a mistake in the inequality.

Let me check again.

From p >=k +1

p = m +2 -x

k +1 = (m +2)/2 +1 = (m +2 +2)/2 = (m +4)/2

So, m +2 -x >= (m +4)/2

Multiply both sides by 2:

2m +4 -2x >= m +4

Subtract m +4 from both sides:

m -2x >=0 ⇒ m >=2x

So, m >=2x

Hence, in case 2, m >=2x

But in the earlier calculation, I got m >=2x +2

Wait, perhaps I messed up.

Wait, p = m +2 -x

k +1 = (m +2)/2 +1 = (m +2 +2)/2 = (m +4)/2

So, p >=k +1 ⇒ m +2 -x >= (m +4)/2

Multiply both sides by 2:

2m +4 -2x >= m +4

Subtract m +4 from both sides:

m -2x >=0 ⇒ m >=2x

So, m >=2x

Hence, in case 2, m >=2x

But in the code, it's using m >=2x -2

Which is too lenient.

So, it should be m >=2x

Hence, the code is incorrect.

In the fifth test case, n=1000000000, x=500000000

Compute n -x=500000000, n +x -2=999999998

Case 1: m divides 500000000 and m >=999999998

No such m, since m must divide 500000000 and m >=999999998, but 500000000 <999999998

Case 2: m divides 999999998 and m >=1000000000

No such m, since m must divide 999999998 and m >=1000000000, but 999999998 <1000000000

Hence, output should be 0, but the example shows 1.

Wait, perhaps there is a k that satisfies.

Wait, for k=500000000

m=2*500000000 -2=999999998

Check if m divides n +x -2=999999998 ⇒ yes

And m >=2x=1000000000 ⇒ 999999998 <1000000000 ⇒ not acceptable

Hence, output should be 0

But according to the example, it's 1

Wait, perhaps the example is wrong.

Alternatively, perhaps I'm missing something.

Wait, perhaps for k=500000000, m=9999