To determine what will be printed, let's break down the initial state and the operations performed:

1. **Initial State**: 
   - `a` is a sorted list of integers.
   - `i` is set to `len(a)`, which means `i` starts at the length of the list `a`.
   - `kq` is the sum of `a[len(a) - i - 1] - a[i]` for all iterations from `i=0` to `i=len(a)//2-1`.

2. **Loop Execution**:
   - The loop runs from `i=0` to `i=len(a)//2-1`.
   - In each iteration, `i` increases by 1.
   - For each `i`, the expression `a[len(a) - i - 1] - a[i]` is computed and added to `kq`.

3. **Understanding the Expression**:
   - `a[len(a) - i - 1]` refers to the element at the position from the end of the list.
   - `a[i]` refers to the element at the current position from the start of the list.
   - The difference `a[len(a) - i - 1] - a[i]` is added to `kq` for each `i`.

4. **Final Value of `kq`**:
   - Since `i` starts at `len(a)` and decreases to `len(a)//2`, the loop effectively calculates the sum of differences between elements symmetrically positioned from both ends of the list up to the middle.

Given the above, let's assume a specific example to illustrate the calculation. Suppose `a = [1, 2, 3, 4, 5]` (a sorted list):

- When `i = len(a) = 5`, the loop doesn't run because `i` must be less than `len(a)//2 = 2.5` (which is 2).
- The loop runs from `i=0` to `i=1`:
  - For `i=0`: `a[len(a) - 0 - 1] - a[0] = a[4] - a[0] = 5 - 1 = 4`
  - For `i=1`: `a[len(a) - 1 - 1] - a[1] = a[3] - a[1] = 4 - 2 = 2`

So, `kq = 4 + 2 = 6`.

Therefore, the output will be:

Output: **6**