The expression `current_cost += length - (t + 1)` indicates that the value of `current_cost` is being updated by adding the result of `length - (t + 1)` to its previous value. The variables affected are `current_cost`, `length`, and `t`.

From the initial state:
- `n` remains an integer such that `1 <= n <= 1000`
- `a` remains a list of `n + 1` integers where each integer `a_i` is in the range `1 <= a_i <= 100`
- `length` is the next integer in the list `a`
- `t` is some integer whose value is not specified here.

The result of the operation `length - (t + 1)` will be added to the original value of `current_cost`, but we do not have specific values for `current_cost`, `length`, or `t`, only the relationships established in the initial state.

Since `length` is defined as the next integer in the list `a`, we can express the change in terms of those variables.

Output State: **`n` is an integer such that 1 <= `n` <= 1000; `a` is a list of `n + 1` integers where each integer `a_i` is in the range 1 <= `a_i` <= 100; `length` is the next integer in the list `a`; `current_cost` is updated to `current_cost + (length - (t + 1))`.**