Let's break down the given code and determine the output state.

Initial State:
- `t` must be greater than 0
- `k` is the first integer from the input
- `x` is the second integer from the input and must be at least 0
- `a` is the third integer from the input
- `z` is `1 + 1 + 1 // (k - 1)`
- `i` is `x + 1`

The given code snippet is:
```python
z += z // (k - 1) + 1
```

First, we need to understand the initial value of `z`:
- `z = 1 + 1 + 1 // (k - 1)`
- Since `1 // (k - 1)` is integer division, it will be `1` if `k > 2`, `0` if `k = 2`, and undefined if `k = 1` (which is not possible since `k - 1` would be `0` and division by zero is not allowed).
- Therefore, `z` simplifies to:
  - `z = 3` if `k > 2`
  - `z = 2` if `k = 2`

Next, we apply the code snippet:
- `z += z // (k - 1) + 1`
- We need to calculate `z // (k - 1)`:
  - If `k > 2`, `z // (k - 1)` will be `0` or `1` depending on the value of `z` and `k`.
  - If `k = 2`, `z // (k - 1)` will be `z // 1`, which is `z`.

Let's consider both cases:

1. **If `k > 2`:**
   - `z = 3` initially.
   - `z // (k - 1)` will be `0` (since `3 // (k - 1)` where `k - 1 > 1`).
   - `z += 0 + 1` → `z = 4`.

2. **If `k = 2`:**
   - `z = 2` initially.
   - `z // (k - 1)` will be `2 // 1 = 2`.
   - `z += 2 + 1` → `z = 5`.

Given the initial state and the code, we can now state the output state:

- If `k > 2`, `z` becomes `4`.
- If `k = 2`, `z` becomes `5`.

The other variables (`t`, `k`, `x`, `a`, `i`) remain unchanged.

Output State: **`t` must be greater than 0, `k` is the first integer from the input, `x` is the second integer from the input and must be at least 0, `a` is the third integer from the input, `i` is `x + 1`, `z` is `4` if `k > 2` or `5` if `k = 2`.**