The code snippet `ans += t` increments the value of `ans` by `t`. Given the initial state, `ans` is initially calculated as `((s + t) % MOD + MOD) % MOD`. After adding `t` to `ans`, the new value of `ans` becomes `(((s + t) % MOD + MOD) % MOD + t) % MOD`.

To simplify, let's denote the initial value of `ans` as `initial_ans = ((s + t) % MOD + MOD) % MOD`. After executing `ans += t`, the new value of `ans` is `(initial_ans + t) % MOD`.

Therefore, the updated value of `ans` is `(((s + t) % MOD + MOD) % MOD + t) % MOD`.

Output State: **`T` is greater than or equal to 1; `t` is `(2 times the maximum subarray sum of `a`) % 1000000007; `tmp` is 0; `n` is an integer read from input where 1 ≤ n ≤ 2 · 10^5; `k` is an integer read from input where 2 ≤ k ≤ 2 · 10^5; `a` is a list of `n` integers read from input where each integer `a_i` satisfies -10^9 ≤ `a_i` ≤ 10^9; `MOD` is 1000000007; `s` is the sum of all elements in the list `a`; `ans` is `(((s + t) % MOD + MOD) % MOD + t) % MOD`.**