Let's break down the problem step by step:

1. **Initial State**:
   - `count` is `m + 1`.
   - `i` is 1.
   - `n` is an input integer.
   - `m` is an integer such that `m` is at least 4.
   - `countmins` is `m - 1`.
   - `g` is `int(n / (m + 1)) - m + 1`.
   - `ans` is initialized to 0 (since no initial value is given).

2. **Loop Execution**:
   - The loop runs from `2` to `m` (inclusive).
   - In each iteration, `count` is incremented by 1.
   - `countmins` is set to `count - 1`.
   - `g` is recalculated as `int(n / count) - m + 1`.
   - If `g` becomes less than `countmins`, the loop breaks early. Otherwise, `ans` is updated by adding `int(g / count) + 1` to its current value.

3. **Final Values**:
   - After the loop completes, `count` will be `m + 1`.
   - `ans` will be the cumulative sum of `int(g / count) + 1` for each iteration from 2 to `m`.

4. **Calculation of `ans`**:
   - For `count = 2`: `g = int(n / 3) - m + 1`, `ans += int(g / 2) + 1`.
   - For `count = 3`: `g = int(n / 2) - m + 1`, `ans += int(g / 3) + 1`.
   - For `count = 4`: `g = int(n / 1) - m + 1`, `ans += int(g / 4) + 1`.
   - This process continues until `count = m`.

5. **Output**:
   - The final value of `ans` is printed.

Given the above steps, let's express the final output:

Output: **ans (where ans is the cumulative sum of int(g / count) + 1 for each iteration from 2 to m, with g = int(n / count) - m + 1)**