Alright, I have this problem to solve. Let's understand what's being asked here. We have n signs of the apocalypse, each occurring every a_i years. These signs must occur sequentially, meaning each sign must happen one after the other in order. So, the first sign occurs at year a_1, then the second sign occurs right after the first one, and so on.

Wait, no. Actually, reading it again, it says that the i-th sign occurs every a_i years, in years a_i, 2*a_i, 3*a_i, and so on. So, the signs are recurring at their own intervals. But, for the apocalypse to happen, they must occur sequentially, meaning that after the first sign occurs, we start waiting for the second sign to occur in its next available year, and so on, up to the n-th sign.

So, it's not about all signs happening in the same year, but rather a sequence where each sign happens one after the other, following their own periodicity.

Let me try to rephrase the problem to make sure I understand it correctly. We have a sequence of signs, each with their own periodicity a_i. We need to find the year when the n-th sign occurs, given that each sign must occur after the previous one has occurred.

In other words, we need to find the smallest year y such that for each sign from the first to the n-th, there exists a multiple of a_i that is greater than the year the previous sign occurred and less than or equal to y.

This sounds like we need to chain the occurrences of each sign, ensuring that each sign occurs after the previous one.

Let me look at the example to understand better.

In the first test case:

n = 6

a = [3, 2, 4, 5, 9, 18]

And the output is 36.

Let's see:

- The first sign occurs at year 3.

- Then, we wait for the second sign after year 3. The second sign occurs every 2 years, so the next occurrence after year 3 is at year 4.

- Then, wait for the third sign after year 4. The third sign occurs every 4 years. The next occurrence after year 4 is at year 4 + 4 = 8.

- Then, wait for the fourth sign after year 8. The fourth sign occurs every 5 years. The next occurrence after year 8 is at year 10.

- Then, wait for the fifth sign after year 10. The fifth sign occurs every 9 years. The next occurrence after year 10 is at year 18.

- Finally, wait for the sixth sign after year 18. The sixth sign occurs every 18 years. The next occurrence after year 18 is at year 36.

So, the apocalyse happens in year 36.

Another test case:

n = 5

a = [1, 2, 3, 4, 5]

Output: 5

Let's see:

- First sign at year 1.

- Second sign after year 1, next occurrence of sign 2 is at year 2.

- Third sign after year 2, next occurrence of sign 3 is at year 3.

- Fourth sign after year 3, next occurrence of sign 4 is at year 4.

- Fifth sign after year 4, next occurrence of sign 5 is at year 5.

So, apocalyse happens in year 5.

Another test case:

n = 5

a = [1, 1, 1, 1, 1]

Output: 5

Similar to above, each sign occurs every year, so they can occur sequentially from year 1 to year 5.

Last test case:

n = 6

a = [50, 30, 711, 200, 503, 1006]

Output: 2012

Let's verify:

- First sign at year 50.

- Second sign after year 50, next occurrence at year 60.

- Third sign after year 60, next occurrence at year 711.

- Fourth sign after year 711, next occurrence at year 800.

- Fifth sign after year 800, next occurrence at year 1006.

- Sixth sign after year 1006, next occurrence at year 2012.

Wait, year 1006 plus 1006 is 2012.

So, seems like the pattern is to find the next multiple of a_i after the previous sign's year for each sign, and the year when the n-th sign occurs is the answer.

Now, looking at the provided program:

def func():

num_tests = int(input())

while num_tests > 0:

num_tests -= 1

n = int(input())

nums = [int(x) for x in input().split(' ')]

start_year = 0

for x in range(0, len(nums)):

start_year = ((start_year + 1) // nums[x] + 1) * nums[x]

print(start_year)

So, it reads the number of test cases, then for each test case, it reads n and the list of a_i's.

It initializes start_year to 0.

Then, for each sign from 1 to n, it updates start_year as follows:

start_year = ((start_year + 1) // nums[x] + 1) * nums[x]

And finally, prints start_year.

I need to verify if this logic correctly computes the year when the n-th sign occurs, following the sequential occurrence rules.

Let's try to understand the logic inside the loop:

start_year = ((start_year + 1) // nums[x] + 1) * nums[x]

This seems to be calculating the next multiple of nums[x] after start_year.

Let's break it down:

- (start_year + 1) // nums[x]: This computes the smallest integer k such that k * nums[x] >= start_year + 1.

- Then, ((start_year + 1) // nums[x] + 1) * nums[x]: This computes (k + 1) * nums[x], which is the next multiple of nums[x] after start_year.

Wait, actually, (start_year + 1) // nums[x] gives the ceiling of (start_year + 1) divided by nums[x], which is the smallest integer greater than or equal to (start_year + 1)/nums[x]. Multiplying this by nums[x] gives the smallest multiple of nums[x] that is greater than or equal to start_year + 1.

So, yes, this correctly computes the next occurrence of the sign after the previous sign's year.

Let's test this with the first example:

n = 6

a = [3, 2, 4, 5, 9, 18]

start_year initialized to 0.

First sign: ((0 + 1) // 3 + 1) * 3 = (1 // 3 + 1) * 3 = (0 + 1) * 3 = 3

Second sign: ((3 + 1) // 2 + 1) * 2 = (4 // 2 + 1) * 2 = (2 + 1) * 2 = 6

Wait, but in the example, the second sign should occur at year 4, not 6.

Hmm, discrepancy here.

Wait, perhaps I misunderstood the logic.

In the first iteration, start_year becomes 3.

In the second iteration, start_year = ((3 + 1) // 2 + 1) * 2 = (4 // 2 + 1) * 2 = (2 + 1) * 2 = 6

But in the example, it should be 4.

So, maybe the logic is incorrect.

Wait, perhaps I need to adjust the formula.

Let me think differently.

Given that we need the next occurrence of the sign after the previous year, it should be the smallest multiple of a_i that is greater than the previous year.

So, for a given a_i and a previous year y, the next occurrence is ceil((y + 1)/a_i) * a_i.

In Python, ceil((y + 1)/a_i) can be computed as ((y + 1) // a_i + bool((y + 1) % a_i)) * a_i, but since // operator already gives the floor division, ((y + 1) // a_i) * a_i gives the largest multiple less than or equal to y + 1, and ((y + 1) // a_i + 1) * a_i gives the next multiple.

Wait, no. If y + 1 is divisible by a_i, then ((y + 1) // a_i) * a_i = y + 1.

Otherwise, ((y + 1) // a_i + 1) * a_i is the next multiple.

So, the formula start_year = ((start_year + 1) // a_i + 1) * a_i seems correct.

In the first iteration:

start_year = 0

next occurrence of first sign: ((0 + 1) // 3 + 1) * 3 = (1 // 3 + 1) * 3 = (0 + 1) * 3 = 3

Second iteration:

start_year = 3

next occurrence of second sign: ((3 + 1) // 2 + 1) * 2 = (4 // 2 + 1) * 2 = (2 + 1) * 2 = 6

But in the example, it should be 4.

Wait, perhaps the formula is incorrect.

In the example, after the first sign at year 3, the second sign should occur at the smallest multiple of 2 that is greater than 3, which is 4.

But according to the formula, it's computing 6.

So, there's a mistake here.

Wait, maybe I need to adjust the formula.

Let me compute the smallest multiple of a_i greater than y.

This can be computed as:

if y % a_i == 0:

next_occurrence = y + a_i

else:

next_occurrence = y - (y % a_i) + a_i

Or more simply, next_occurrence = ceil((y + 1)/a_i) * a_i

In Python, ceil division can be done with -(-y // a_i) * a_i, but that's for negative numbers.

Wait, perhaps using math.ceil.

But in integer operations, ((y + a_i - 1) // a_i) * a_i gives the smallest multiple of a_i greater than or equal to y.

But in the code, it's using ((start_year + 1) // nums[x] + 1) * nums[x], which seems to be adding one extra period.

Wait, let's compute it step by step for the first example.

Iteration 1:

start_year = 0

next_occurrence = ((0 + 1) // 3 + 1) * 3 = (1 // 3 + 1) * 3 = (0 + 1) * 3 = 3

This is correct, first sign at year 3.

Iteration 2:

start_year = 3

next_occurrence = ((3 + 1) // 2 + 1) * 2 = (4 // 2 + 1) * 2 = (2 + 1) * 2 = 6

But in the example, it should be 4.

Wait, maybe the formula should be ((start_year + 1) // a_i) * a_i

Let's try that:

Iteration 1:

start_year = 0

next_occurrence = ((0 + 1) // 3) * 3 = (1 // 3) * 3 = 0 * 3 = 0

Which is not correct, should be 3.

Wait, that's worse.

Alternatively, maybe start_year = ((start_year + 1) // a_i) * a_i

No, in the first iteration, that would give ((0 + 1) // 3) * 3 = 0 * 3 = 0, which is incorrect.

Wait, perhaps start_year = ((start_year + 1 + a_i - 1) // a_i) * a_i

Which is ceil((start_year + 1)/a_i) * a_i

Let's try:

Iteration 1:

start_year = 0

next_occurrence = ((0 + 1 + 3 - 1) // 3) * 3 = (3 // 3) * 3 = 1 * 3 = 3

Correct.

Iteration 2:

start_year = 3

next_occurrence = ((3 + 1 + 2 - 1) // 2) * 2 = (5 // 2) * 2 = 2 * 2 = 4

Correct.

Iteration 3:

start_year = 4

next_occurrence = ((4 + 1 + 4 - 1) // 4) * 4 = (8 // 4) * 4 = 2 * 4 = 8

Correct.

Iteration 4:

start_year = 8

next_occurrence = ((8 + 1 + 5 - 1) // 5) * 5 = (13 // 5) * 5 = 2 * 5 = 10

Correct.

Iteration 5:

start_year = 10

next_occurrence = ((10 + 1 + 9 - 1) // 9) * 9 = (19 // 9) * 9 = 2 * 9 = 18

Correct.

Iteration 6:

start_year = 18

next_occurrence = ((18 + 1 + 18 - 1) // 18) * 18 = (36 // 18) * 18 = 2 * 18 = 36

Correct.

So, the formula should be:

start_year = ((start_year + 1 + a_i - 1) // a_i) * a_i

Which simplifies to:

start_year = ((start_year + 1) // a_i + bool((start_year + 1) % a_i)) * a_i

But in the original code, it's using:

start_year = ((start_year + 1) // nums[x] + 1) * nums[x]

Which, in the second iteration, gave 6 instead of 4.

Wait, in the second iteration, with a_i=2:

start_year = ((3 + 1) // 2 + 1) * 2 = (4 // 2 + 1) * 2 = (2 + 1) * 2 = 6

But according to the correct formula:

start_year = ((3 + 1 + 2 - 1) // 2) * 2 = (6 // 2) * 2 = 3 * 2 = 6

Wait, but in the example, it should be 4, not 6.

Wait, perhaps I'm misunderstanding.

Wait, no. In the correct formula, it's ((start_year + 1 + a_i - 1) // a_i) * a_i = ((start_year + a_i) // a_i) * a_i

Wait, no, it's ceil((start_year + 1)/a_i) * a_i, which is equivalent to ((start_year + a_i - 1) // a_i) * a_i

Let's compute it:

For start_year=3, a_i=2:

((3 + 2 - 1) // 2) * 2 = (4 // 2) * 2 = 2 * 2 = 4

Which is correct.

But in the original code, it's using ((start_year + 1) // nums[x] + 1) * nums[x] = ((3 + 1) // 2 + 1) * 2 = (4 // 2 + 1) * 2 = (2 + 1) * 2 = 6

Which is incorrect, as per the example.

So, the original code is wrong here.

Wait, perhaps it's a mistake in the code.

Let me check with another test case.

Take n=5, a=[1,2,3,4,5], output should be 5.

Initialize start_year=0

Iteration 1: start_year = ((0 + 1) // 1 + 1) * 1 = (1 // 1 + 1) * 1 = (1 + 1) * 1 = 2

Iteration 2: start_year = ((2 + 1) // 2 + 1) * 2 = (3 // 2 + 1) * 2 = (1 + 1) * 2 = 4

Iteration 3: start_year = ((4 + 1) // 3 + 1) * 3 = (5 // 3 + 1) * 3 = (1 + 1) * 3 = 6

Iteration 4: start_year = ((6 + 1) // 4 + 1) * 4 = (7 // 4 + 1) * 4 = (1 + 1) * 4 = 8

Iteration 5: start_year = ((8 + 1) // 5 + 1) * 5 = (9 // 5 + 1) * 5 = (1 + 1) * 5 = 10

But according to the example, it should be 5, not 10.

So, the code is producing wrong output here.

Another test case: n=5, a=[1,1,1,1,1], output should be 5.

Initialize start_year=0

Iteration 1: start_year = ((0 + 1) // 1 + 1) * 1 = (1 // 1 + 1) * 1 = (1 + 1) * 1 = 2

Iteration 2: start_year = ((2 + 1) // 1 + 1) * 1 = (3 // 1 + 1) * 1 = (3 + 1) * 1 = 4

Iteration 3: start_year = ((4 + 1) // 1 + 1) * 1 = (5 // 1 + 1) * 1 = (5 + 1) * 1 = 6

Iteration 4: start_year = ((6 + 1) // 1 + 1) * 1 = (7 // 1 + 1) * 1 = (7 + 1) * 1 = 8

Iteration 5: start_year = ((8 + 1) // 1 + 1) * 1 = (9 // 1 + 1) * 1 = (9 + 1) * 1 = 10

Again, according to the example, it should be 5, but the code outputs 10.

So, clearly, the code is incorrect.

The correct formula should be start_year = ((start_year + 1 + a_i - 1) // a_i) * a_i

Which simplifies to start_year = ((start_year + a_i) // a_i) * a_i

Let's test this formula with the first test case:

n=6, a=[3,2,4,5,9,18]

start_year=0

Iteration 1: ((0 + 3) // 2) * 2 = (3 // 2) * 2 = 1 * 2 = 2

Wait, that can't be right.

Wait, I think I messed up the formula.

Actually, the correct formula to find the smallest multiple of a_i greater than start_year is:

if start_year % a_i == 0:

next_occurrence = start_year + a_i

else:

next_occurrence = start_year - (start_year % a_i) + a_i

Or, equivalently, next_occurrence = ceil((start_year + 1)/a_i) * a_i

In integer arithmetic, this is ((start_year + a_i - 1) // a_i) * a_i

Let's apply this correctly:

Iteration 1: start_year=0, a_i=3

next_occurrence = ((0 + 3 - 1) // 3) * 3 = (2 // 3) * 3 = 0 * 3 = 0

Wait, that's not right, should be 3.

Wait, maybe I need to adjust the formula.

Actually, the correct formula is ceil((start_year + 1)/a_i) * a_i

In integer arithmetic, ceil(a/b) is (a + b - 1) // b

So, ceil((start_year + 1)/a_i) = (start_year + 1 + a_i - 1) // a_i = (start_year + a_i) // a_i

Then, next_occurrence = ((start_year + a_i) // a_i) * a_i

Let's try:

Iteration 1: start_year=0, a_i=3

next_occurrence = ((0 + 3) // 3) * 3 = (3 // 3) * 3 = 1 * 3 = 3

Correct.

Iteration 2: start_year=3, a_i=2

next_occurrence = ((3 + 2) // 2) * 2 = (5 // 2) * 2 = 2 * 2 = 4

Correct.

Iteration 3: start_year=4, a_i=4

next_occurrence = ((4 + 4) // 4) * 4 = (8 // 4) * 4 = 2 * 4 = 8

Correct.

Iteration 4: start_year=8, a_i=5

next_occurrence = ((8 + 5) // 5) * 5 = (13 // 5) * 5 = 2 * 5 = 10

Correct.

Iteration 5: start_year=10, a_i=9

next_occurrence = ((10 + 9) // 9) * 9 = (19 // 9) * 9 = 2 * 9 = 18

Correct.

Iteration 6: start_year=18, a_i=18

next_occurrence = ((18 + 18) // 18) * 18 = (36 // 18) * 18 = 2 * 18 = 36

Correct.

So, the correct formula is start_year = ((start_year + a_i) // a_i) * a_i

But in the original code, it's start_year = ((start_year + 1) // nums[x] + 1) * nums[x]

Which is different.

Let's see:

start_year = ((start_year + 1) // nums[x] + 1) * nums[x]

In the first iteration:

start_year = ((0 + 1) // 3 + 1) * 3 = (1 // 3 + 1) * 3 = (0 + 1) * 3 = 3

Correct.

Second iteration:

start_year = ((3 + 1) // 2 + 1) * 2 = (4 // 2 + 1) * 2 = (2 + 1) * 2 = 6

But should be 4.

So, incorrect.

Hence, the formula in the code is wrong.

The correct formula should be start_year = ((start_year + nums[x]) // nums[x]) * nums[x]

So, the code is incorrect.

**Final Answer**

\[ \boxed{\text{False}} \]