To determine what will be printed by the `print(suma - 1)` statement, let's break down the initial state and the logic involved:

### Initial State Breakdown:
- `t` is an integer such that \(2 \leq t \leq 10^4\). This variable seems to indicate the number of test cases or iterations but does not directly influence the current context.
- `T` is an integer read from the input and must be greater than or equal to 1. This could represent another form of iteration count or a specific value used in calculations.
- `info` is a list of strings obtained by splitting the new input line. This implies that the input line contains space-separated values.
- `a` is the integer value of `info[0]`, which is the first value from the split input line.
- `b` is the integer value of `info[1]`, which is the second value from the split input line and must be at least 1.
- `suma` is the sum of all `x` values calculated during the iterations where `a - i * (i - 1) > 0`.

### Calculation of `suma`:
The variable `suma` is the result of summing up all `x` values in iterations where the condition `a - i * (i - 1) > 0` holds true. Here, `i` likely ranges over some sequence, possibly from 1 upwards, and `x` is typically defined as `a - i * (i - 1)`.

Let's analyze the condition `a - i * (i - 1) > 0`:
- For each `i`, if `a - i * (i - 1) > 0`, then `x = a - i * (i - 1)` is added to `suma`.
- This condition will hold true for a certain range of `i` values, starting from `i = 1` and continuing until `a - i * (i - 1) <= 0`.

### Example Calculation:
Suppose `a = 10`:
- For `i = 1`: `a - i * (i - 1) = 10 - 1 * 0 = 10 > 0` → `x = 10` → `suma += 10`
- For `i = 2`: `a - i * (i - 1) = 10 - 2 * 1 = 8 > 0` → `x = 8` → `suma += 8`
- For `i = 3`: `a - i * (i - 1) = 10 - 3 * 2 = 4 > 0` → `x = 4` → `suma += 4`
- For `i = 4`: `a - i * (i - 1) = 10 - 4 * 3 = -2 <= 0` → Condition fails, stop iterating.

In this example, `suma` would be `10 + 8 + 4 = 22`.

### Final Output:
The `print(suma - 1)` statement will output the value of `suma` minus 1.

### Conclusion:
Given the above analysis, the output of the `print(suma - 1)` statement is the sum of all valid `x` values (where `x = a - i * (i - 1)` and `a - i * (i - 1) > 0`) minus 1.

Output: **suma - 1 (where suma is the sum of all x values calculated during the iterations where a - i * (i - 1) > 0)**