The code snippet updates the value of `ans` by multiplying it with `nums_left` and taking the modulus with `MOD`. Let's go through the details:

- `ans` was initially the result of `func_1(N - 1, L[-1] - 1)`.
- `nums_left` is defined as `L[-1] - 3`.
- The new value of `ans` is calculated as `ans * nums_left % MOD`.

Given the initial state:
- `N`, `M1`, and `M2` are positive integers such that 1 ≤ M1, M2 ≤ N ≤ 2 * 10^5.
- `L` is a list of integers of length M1, where 1 ≤ L[i] ≤ N and L is strictly increasing.
- `R` is a list of integers provided by the user input, with the last element of L equal to the first element of R, L[0] is 1, and R[-1] is N.
- Either M1 ≤ 1, or M2 ≤ 1, or (L[-2] ≠ R[1]).
- `ans` is the result of `func_1(N - 1, L[-1] - 1)`.
- `cur` is `M1 - 3` if `i` is equal to `L[cur + 1]`, otherwise `cur` remains `M1 - 2`.
- `nums_left` is `L[-1] - 3`.
- `M1` is greater than 1.
- `i` is `L[-1] - 2` and `L[-1]` must be at least 3.

After executing the code snippet:
- `ans` is updated to `ans * (L[-1] - 3) % MOD`.

Therefore, the output state is:
Output State: **`N`, `M1`, and `M2` are positive integers such that 1 ≤ M1, M2 ≤ N ≤ 2 * 10^5. `L` is a list of integers of length M1, where 1 ≤ L[i] ≤ N and L is strictly increasing. `R` is a list of integers provided by the user input, with the last element of L equal to the first element of R, L[0] is 1, and R[-1] is N. Either M1 ≤ 1, or M2 ≤ 1, or (L[-2] ≠ R[1]). `ans` is now `ans * (L[-1] - 3) % MOD`. `cur` is `M1 - 3` if `i` is equal to `L[cur + 1]`, otherwise `cur` remains `M1 - 2`. `nums_left` is `L[-1] - 3`. `M1` is greater than 1. `i` is `L[-1] - 2` and `L[-1]` must be at least 3.**