Postcondition: `i` is `n-3`, `el` is `s1[n-3]`, `ol` is `totalOne - 1` or `totalOne`, `zr` is `len(suffZero) - 1`, `preOne` is the list obtained by removing the last element from the original `preOne` list, and `ans[i]` is calculated as follows:
- If `el == '>'` and `zr <= ol`, then `ans[i]` is `zeroInd - oneInd + n + 1` where `zeroInd` is `suffZero[-1] + suffZero[-2]` and `oneInd` is `2 * func_1(preOne, zr)`.
- If `el == '>'` and `zr > ol`, then `ans[i]` is `zeroInd - oneInd + n + 1 - fi` where `zeroInd` is `zeroInd` or `2 * func_1(suffZero, totalOne + 1) - func_1(suffZero, 1)` and `oneInd` is `oneInd` or `2 * preOne[-1] - func_1(preOne, 1) + func_1(preOne, zr + 1) - func_1(preOne, zr) + func_1(preOne, zr) - func_1(preOne, 1)`.
- If `el != '>'` and `zr <= ol`, then `ans[i]` is `zeroInd - oneInd + n + 1` where `zeroInd` is `2 * func_1(suffZero, ol + 1) - func_1(suffZero, 1)` and `oneInd` is `2 * func_1(preOne, zr)`.
- If `el != '>'` and `zr > ol`, then `ans[i]` is `zeroInd - oneInd` where `zeroInd` is `2 * func_1(suffZero, ol + 1) - func_1(suffZero, 1)` and `oneInd` is `2 * preOne[-1]`.