Let's break down the initial state and the code snippet step by step to determine what will be printed.

### Initial State:
1. `n` is at least 1.
2. `m` is at least 1.
3. `b` is defined as `min(n, m) + 1`.
4. `t` is a positive integer greater than 0.
5. `T` is 0.
6. `ans` is the sum of `n // b + 1` for each `b` from 1 to `min(n, m)`.

### Step-by-Step Calculation:

1. **Determine `min(n, m)`**:
   - Let's denote `min(n, m)` as `k`. Since both `n` and `m` are at least 1, `k` is also at least 1.

2. **Calculate `b`**:
   - `b` is defined as `min(n, m) + 1`, which means `b = k + 1`.

3. **Calculate `ans`**:
   - `ans` is the sum of `n // b + 1` for each `b` from 1 to `k`.
   - We need to evaluate the expression `n // b + 1` for each `b` from 1 to `k` and sum these values.

### Detailed Calculation of `ans`:
- For each `b` from 1 to `k`:
  - Compute `n // b + 1`.
  - Sum these values to get `ans`.

Let's denote the sum as:
\[ \text{ans} = \sum_{b=1}^{k} (n // b + 1) \]

### Example Calculation:
Suppose `n = 5` and `m = 3`:
- `k = min(5, 3) = 3`.
- `b` ranges from 1 to 3.
- Calculate `ans`:
  - For `b = 1`: \( n // 1 + 1 = 5 // 1 + 1 = 5 + 1 = 6 \)
  - For `b = 2`: \( n // 2 + 1 = 5 // 2 + 1 = 2 + 1 = 3 \)
  - For `b = 3`: \( n // 3 + 1 = 5 // 3 + 1 = 1 + 1 = 2 \)
- Sum these values: \( 6 + 3 + 2 = 11 \)

So, `ans` is 11 in this example.

### General Case:
For any `n` and `m` where `n` and `m` are at least 1:
- `k = min(n, m)`.
- `ans` is the sum of `n // b + 1` for each `b` from 1 to `k`.

### Final Output:
The `print(ans)` statement will print the sum of `n // b + 1` for each `b` from 1 to `min(n, m)`.

Output: **ans (where ans is the sum of n // b + 1 for each b from 1 to min(n, m))**