First, let's break down the initial state and the code snippet:

- Initial State: `n` is a positive integer such that \(1 \leq n \leq 2 \cdot 10^9\) and \(n \geq 6\), `count` is either 1 or 2, `rem` is \(n - 2 \cdot (n // 2 + 2)\), `a` is \(a + 1\), `b` is \(n // 4 + 1\).
- Code: `b = a`

Step-by-step analysis:
1. The value of `a` is not explicitly defined in the initial state, but it is stated that `a` is \(a + 1\). This implies that `a` is initially 0 because adding 1 to 0 gives us the next integer.
2. The value of `b` is initially calculated as \(n // 4 + 1\).
3. The code `b = a` assigns the current value of `a` to `b`.

Since `a` is initially 0, after executing `b = a`, `b` will also be 0. The values of `n`, `count`, `rem`, and `a` remain unchanged.

Therefore, the output state is:
Output State: **`n` is a positive integer such that \(1 \leq n \leq 2 \cdot 10^9\) and \(n \geq 6\), `count` is either 1 or 2, `rem` is \(n - 2 \cdot (n // 2 + 2)\), `a` is 1, `b` is 0.**