First, let's analyze the given initial state and the code snippet.

Initial State:
- `n` is a positive integer such that \(1 \leq n \leq 2 \cdot 10^9\) and \(n \geq 6\).
- `count` is either 1 or 2.
- `rem` is \(n - 2 \cdot (n // 2 + 2)\).
- `a` is 1.
- `b` is 0.

Code Snippet:
```python
rem = n - 2 * (a + b)
```

Let's calculate the updated value of `rem` based on the initial values of `a` and `b`.

Given `a = 1` and `b = 0`, the expression `2 * (a + b)` simplifies to `2 * (1 + 0) = 2 * 1 = 2`. So the new value of `rem` will be:

\[ rem = n - 2 \]

Now, we can list the output state after executing the code.

Output State: **`n` is a positive integer such that \(1 \leq n \leq 2 \cdot 10^9\) and \(n \geq 6\); `count` is either 1 or 2; `rem` is `n - 2`; `a` is 1; `b` is 0.**