The code snippet `list[i] -= 2 * list[i - 1]` modifies the value of `list[i]` by subtracting twice the value of `list[i - 1]` from it. Let's determine the impact on the list based on the given initial state.

Given:
- `list[2]` is 2
- `list[1]` is 1
- `list[3]` is 0
- The remaining elements are either 0 or 1, with no element greater than 1.

The code modifies `list[i]` based on the value of `i`. Since the specific value of `i` is not provided, we will consider the possible values of `i` that can affect the list as per the given initial state.

### Case Analysis:

1. **If `i` is 2:**
   - `list[2] -= 2 * list[1]`
   - `list[2] -= 2 * 1`
   - `list[2] -= 2`
   - `list[2] = 2 - 2`
   - `list[2] = 0`

2. **If `i` is 3:**
   - `list[3] -= 2 * list[2]`
   - `list[3] -= 2 * 2`
   - `list[3] -= 4`
   - `list[3] = 0 - 4`
   - `list[3] = -4` (However, this contradicts the precondition that no element is greater than 1, so `i` cannot be 3 in this context.)

Since `i` cannot be 3 without violating the precondition, we'll assume `i` is 2.

### Output State:
The only change in the list is that `list[2]` is now 0. All other conditions remain the same.

Output State: **The list is a list of integers where `list[2]` is 0, `list[1]` is 1, `list[3]` is 0, and the remaining elements are either 0 or 1, with no element greater than 1.**