To determine the output of the `print(ans)` statement, let's break down the given initial state and the calculation of `ans`.

### Initial State Breakdown:
- `t`: An input integer that must be greater than 0. This variable does not directly affect the calculation of `ans`.
- `n`: The first number from a new input, converted to an integer.
- `m`: The second number from the same new input, converted to an integer.
- `ans`: Calculated as `n + Σ((n + b) // (b * b))` for `b` ranging from 2 to `min(n, m)`.
- `T`: Incremented by 1, but it is not used in the calculation of `ans` or in the print statement.

### Calculation of `ans`:
The variable `ans` is computed using the formula:
\[ \text{ans} = n + \sum_{b=2}^{\min(n, m)} \left\lfloor \frac{n + b}{b \cdot b} \right\rfloor \]

Here's a step-by-step breakdown:
1. Start with `ans` initialized to `n`.
2. For each integer `b` from 2 up to `min(n, m)`:
   - Compute the term \(\left\lfloor \frac{n + b}{b \cdot b} \right\rfloor\).
   - Add this term to `ans`.

### Example Calculation:
Let's assume `n = 10` and `m = 5` for illustration purposes (the actual values of `n` and `m` would be provided during execution).

- Initialize `ans` to `n`: `ans = 10`.
- Calculate the summation part:
  - For `b = 2`: \(\left\lfloor \frac{10 + 2}{2 \cdot 2} \right\rfloor = \left\lfloor \frac{12}{4} \right\rfloor = 3\)
  - For `b = 3`: \(\left\lfloor \frac{10 + 3}{3 \cdot 3} \right\rfloor = \left\lfloor \frac{13}{9} \right\rfloor = 1\)
  - For `b = 4`: \(\left\lfloor \frac{10 + 4}{4 \cdot 4} \right\rfloor = \left\lfloor \frac{14}{16} \right\rfloor = 0\)
  - For `b = 5`: \(\left\lfloor \frac{10 + 5}{5 \cdot 5} \right\rfloor = \left\lfloor \frac{15}{25} \right\rfloor = 0\)

Summing these values: \(3 + 1 + 0 + 0 = 4\).

Thus, `ans` becomes \(10 + 4 = 14\).

### General Case:
Given `n` and `m`, the value of `ans` will be:
\[ \text{ans} = n + \sum_{b=2}^{\min(n, m)} \left\lfloor \frac{n + b}{b \cdot b} \right\rfloor \]

### Final Output:
The `print(ans)` statement will output the value of `ans` as calculated above.

Output: **ans (where ans is calculated as n + Σ((n + b) // (b * b)) for b from 2 to min(n, m))**