Alright, I have this problem to solve. Let's understand what's being asked here. So, Polycarp has a string `s` consisting of lowercase Latin letters, and he encodes it using a specific algorithm. My task is to write a program that decodes the encoded string back to the original string `s`.

First, I need to understand the encoding algorithm clearly. The algorithm has two main steps:

1. **Construct the auxiliary string `r`**: This string consists of all distinct letters from `s`, arranged in alphabetical order.

2. **Encoding the string `s`**: Each character in `s` is replaced by its symmetric character from the string `r`. That means the first character of `r` is replaced by the last character of `r`, the second by the second last, and so on.

For example, given `s = "codeforces"`, the auxiliary string `r` is "cdefors". Then, each character in `s` is replaced as follows:

- 'c' -> 's'

- 'o' -> 'e'

- 'd' -> 'r'

- 'f' -> 'o'

- 'e' -> 'f'

- 'c' -> 's'

- 'o' -> 'e'

- 'r' -> 'd'

- 'c' -> 's'

- 'e' -> 'f'

- 's' -> 'c'

So, the encoded string is "serofedsoc".

Now, my task is to decode the encoded string back to the original string `s`. Given the encoded string `b`, I need to find the original string `s`.

Looking at the encoding process, it seems that the mapping from `s` to `b` is done using the string `r`, which is derived from `s`. But in decoding, I only have `b`, so I need to figure out how to reconstruct `s` from `b`.

Let me think about the properties of the encoding process:

- The string `r` is determined by the distinct characters in `s`, sorted alphabetically.

- The encoding replaces each character in `s` with its symmetric counterpart in `r`.

- Therefore, the mapping is a one-to-one correspondence between characters in `r` and their symmetric partners in `r`.

Given that, to decode, I need to reverse this mapping. That is, for each character in `b`, I need to find out which character in `r` it corresponds to, and then map it back to the original character in `s`.

Wait a minute, but I don't have `r` directly. I only have `b`, which is the encoded version of `s`. However, `r` is derived from `s`, which is what I'm trying to find. So, I have a chicken and egg problem here.

Let me think differently. Suppose I consider that the encoding is a mapping based on the sorted unique characters of `s`. If I can determine what `r` is from `b`, then I can reverse the mapping to get back to `s`.

Given that `b` is obtained by replacing each character in `s` with its symmetric counterpart in `r`, and `r` is derived from `s`, perhaps I can infer `r` from `b` because `b` should also be encoded using the same `r`.

Wait, but `b` is the encoded version of `s`, so the characters in `b` are mapped from `s` based on `r`. If I can find the unique sorted characters in `b`, that should be the same as `r`, because `r` is based on the unique characters in `s`, and the encoding just maps them symmetrically.

Is that correct? Let's see.

Take the example:

`s = "codeforces"`

`r = "cdefors"`

Encoded `b = "serofedsoc"`

Unique sorted characters in `b` are "cdefors", which is the same as `r`.

So, in this case, the unique sorted characters in `b` match `r`.

Therefore, I can derive `r` from `b` by taking the unique characters in `b` and sorting them.

Once I have `r`, I can create a mapping from each character in `r` to its symmetric counterpart in `r`.

Then, to decode `b` back to `s`, I need to reverse this mapping. That is, for each character in `b`, find out which character in `r` it corresponds to in the symmetric mapping, and map it back to that character.

Wait, actually, since the encoding is a direct mapping from `s` to `b` based on `r`, to decode, I just need to apply the same mapping again, because mapping twice should bring me back to the original.

Let me test this idea.

Take `s = "codeforces"`

Encoded `b = "serofedsoc"`

Now, if I apply the same mapping to `b`, using `r = "cdefors"`, mapping each character in `b` to its symmetric counterpart in `r`:

- 's' -> 'c'

- 'e' -> 'o'

- 'r' -> 'd'

- 'o' -> 'f'

- 'f' -> 'e'

- 'e' -> 'o'

- 'd' -> 'r'

- 's' -> 'c'

- 'o' -> 'e'

- 'c' -> 's'

So, applying the mapping again to `b` gives me back `"codeforces"`, which is `s`.

Amazing! So, decoding is just applying the same mapping again.

Therefore, the decoding process is identical to the encoding process.

Hence, to decode `b` back to `s`, I can use the same function `func_1` that encodes `s` to `b`, because applying it twice should give me back `s`.

Looking at the provided program:

```python

import sys

input = sys.stdin.read

data = input().split()

index = 0

t = int(data[index])

index += 1

results = []

for _ in range(t):

n = int(data[index])

index += 1

b = data[index]

index += 1

results.append(func_1(b))

for result in result s:

print(result)

def func_1(encoded):

unique_chars = sorted(set(encoded))

char_map = {}

len_unique = len(unique_chars)

for i in range(len_unique):

char_map[unique_chars[i]] = unique_chars[len_unique - 1 - i]

decoded = ''.join((char_map[ch] for ch in encoded))

return decoded

```

It seems that `func_1` takes the encoded string `b`, derives `r` from it by taking the unique sorted characters, creates a mapping from each character in `r` to its symmetric counterpart, and applies this mapping to `b` to get back `s`.

Given my earlier reasoning, this should work, because applying the mapping twice should return the original string.

Let's verify this with the example:

Given `b = "serofedsoc"`, unique sorted characters are "cdefors".

The mapping is:

- 'c' -> 's'

- 'd' -> 'r'

- 'e' -> 'o'

- 'f' -> 'f'

- 'o' -> 'e'

- 'r' -> 'd'

- 's' -> 'c'

Applying this mapping to `b`:

- 's' -> 'c'

- 'e' -> 'o'

- 'r' -> 'd'

- 'o' -> 'e'

- 'f' -> 'f'

- 'e' -> 'o'

- 'd' -> 'r'

- 's' -> 'c'

- 'o' -> 'e'

- 'c' -> 's'

Which gives `"codeforces"`, which matches the original `s`.

Great, it works for this example.

Let's check another example from the provided test case:

Input:

5

10

serofedsoc

3

ttf

9

tlrhgmaoi

1

w

15

hnndledmnhlttin

Output:

codeforces

fft

algorithm

w

meetinthemiddle

Let's take the second test case:

`n = 3`

`b = "ttf"`

Unique sorted characters in `b` are "ft".

Mapping:

- 'f' -> 't'

- 't' -> 'f'

Applying this mapping to `b`:

- 't' -> 'f'

- 't' -> 'f'

- 'f' -> 't'

Which gives "fft", matching the provided output.

Another test case:

`n = 9`

`b = "tlrhgmaoi"`

Unique sorted characters in `b` are "aghilmort".

Mapping:

- 'a' -> 't'

- 'g' -> 'r'

- 'h' -> 'o'

- 'i' -> 'm'

- 'l' -> 'l'

- 'm' -> 'i'

- 'o' -> 'h'

- 'r' -> 'g'

- 't' -> 'a'

Applying this mapping to `b`:

- 't' -> 'a'

- 'l' -> 'l'

- 'r' -> 'g'

- 'h' -> 'o'

- 'g' -> 'r'

- 'm' -> 'i'

- 'a' -> 't'

- 'o' -> 'h'

- 'i' -> 'm'

Which gives "algorithm", matching the provided output.

Seems correct.

Another test case:

`n = 1`

`b = "w"`

Unique sorted characters in `b` are "w".

Mapping:

- 'w' -> 'w'

Applying this mapping to `b`:

- 'w' -> 'w'

Which gives "w", matching the provided output.

Last test case:

`n = 15`

`b = "hnndledmnhlttin"`

Unique sorted characters in `b` are "dehilmnnt".

Mapping:

- 'd' -> 't'

- 'e' -> 'n'

- 'h' -> 'l'

- 'i' -> 'm'

- 'l' -> 'h'

- 'm' -> 'i'

- 'n' -> 'e'

- 't' -> 'd'

Applying this mapping to `b`:

- 'h' -> 'l'

- 'n' -> 'e'

- 'n' -> 'e'

- 'd' -> 't'

- 'l' -> 'h'

- 'e' -> 'n'

- 'd' -> 't'

- 'm' -> 'i'

- 'n' -> 'e'

- 'h' -> 'l'

- 'l' -> 'h'

- 't' -> 'd'

- 't' -> 'd'

- 'i' -> 'm'

- 'n' -> 'e'

Which gives "leetinhdmee", but the provided output is "meetinthemiddle". Hmm, that doesn't match.

Wait, perhaps I made a mistake in the mapping.

Let's list the unique sorted characters: "dehilmnnt". So, the mapping should be:

Index 0: 'd' -> Index 7: 't'

Index 1: 'e' -> Index 6: 'n'

Index 2: 'h' -> Index 5: 'm'

Index 3: 'i' -> Index 4: 'l'

Index 4: 'l' -> Index 3: 'i'

Index 5: 'm' -> Index 2: 'h'

Index 6: 'n' -> Index 1: 'e'

Index 7: 't' -> Index 0: 'd'

Now, applying this mapping to "hnndledmnhlttin":

- 'h' -> 'm'

- 'n' -> 'e'

- 'n' -> 'e'

- 'd' -> 't'

- 'l' -> 'i'

- 'e' -> 'n'

- 'd' -> 't'

- 'm' -> 'h'

- 'n' -> 'e'

- 'h' -> 'm'

- 'l' -> 'i'

- 't' -> 'd'

- 't' -> 'd'

- 'i' -> 'l'

- 'n' -> 'e'

So, the decoded string would be "meetinthemiddle", which matches the provided output.

Alright, so my earlier mistake was in the mapping; I miscounted the indices.

Therefore, the provided program seems to be correct, as it follows the logic I've described.

It reads all input at once using `sys.stdin.read`, splits it into words, and processes each test case accordingly.

For each test case, it reads `n` (the length of the string) and the encoded string `b`.

It then calls `func_1(b)` to decode `b` back to `s`.

In `func_1`, it sorts the unique characters of `b` to get `r`, creates a mapping from each character in `r` to its symmetric counterpart, and applies this mapping to `b` to get the decoded string.

Since applying this mapping twice should return the original string, this approach is correct.

Hence, the program is correct.

**Final Answer**

\[ \boxed{\text{The program is correct.}} \]

**Correctness:** **True**