Let's analyze the given code and its impact on the initial state:

### Initial State:
- `n` and `m` are positive integers such that \(1 \leq n, m \leq 2 \times 10^6\)
- `T` is greater than 0
- `t` is 1
- `info` is a list of strings obtained from the input
- `a` is the integer value of `info[0]`
- `b` is the integer value of `info[1]` and must be at least 3
- `i` is 3
- `x` is \((a - 2) // 4 + 1\)
- If `a - i * (i - 1) > 0`, then `suma` is updated to `a + (a - 2) // 4 + 1` if `a` is not 1, otherwise `suma` is \((a - 2) // 4 + 1\). If `a - i * (i - 1) <= 0`, `suma` remains unchanged.

### Code Snippet:
```python
x = (a - i * (i - 1)) // i ** 2 + 1
```

### Step-by-Step Analysis:
1. **Initial Values:**
   - `i` is 3
   - `x` is \((a - 2) // 4 + 1\)

2. **Expression Calculation:**
   - Calculate `i * (i - 1)`: 
     \[
     i * (i - 1) = 3 * (3 - 1) = 3 * 2 = 6
     \]
   - Calculate `a - i * (i - 1)`:
     \[
     a - 6
     \]
   - Calculate `i ** 2`:
     \[
     i ** 2 = 3 ** 2 = 9
     \]
   - Calculate \((a - 6) // 9\):
     \[
     (a - 6) // 9
     \]
   - Add 1 to the result:
     \[
     x = (a - 6) // 9 + 1
     \]

### Updated Values:
- `x` is now \((a - 6) // 9 + 1\)

### Output State:
- `n` and `m` are positive integers such that \(1 \leq n, m \leq 2 \times 10^6\)
- `T` is greater than 0
- `t` is 1
- `info` is a list of strings obtained from the input
- `a` is the integer value of `info[0]`
- `b` is the integer value of `info[1]` and must be at least 3
- `i` is 3
- `x` is \((a - 6) // 9 + 1\)
- If `a - i * (i - 1) > 0`, then `suma` is updated to `a + (a - 2) // 4 + 1` if `a` is not 1, otherwise `suma` is \((a - 2) // 4 + 1\). If `a - i * (i - 1) <= 0`, `suma` remains unchanged.

Output State: **`n` and `m` are positive integers such that \(1 \leq n, m \leq 2 \times 10^6\), `T` is greater than 0, `t` is 1, `info` is a list of strings obtained from the input, `a` is the integer value of `info[0]`, `b` is the integer value of `info[1]` and must be at least 3, `i` is 3, `x` is \((a - 6) // 9 + 1\), if `a - i * (i - 1) > 0`, then `suma` is updated to `a + (a - 2) // 4 + 1` if `a` is not 1, otherwise `suma` is \((a - 2) // 4 + 1\). If `a - i * (i - 1) <= 0`, `suma` remains unchanged.**