To determine the final output state, we need to evaluate the given code snippet in the context of the initial state. Let's break down the code and compute the final state step-by-step, while keeping the initial conditions in mind.

Initial State:
- `n` is an integer such that \(2 \leq k \leq n \leq 10^9\)
- `m` is an integer such that \(0 \leq m \leq n\)
- `k` is an integer such that \(2 \leq k \leq n\)
- `max_full_sets` is \(m // k\)
- `remaining_correct` is \(m \% k\)
- \((m > n - n // k)\)

Given Code:
```python
excess_full_sets = max_full_sets - (n - m) // (k - 1)
remaining_correct_answers = m - excess_full_sets * k
score = (remaining_correct_answers + k * (pow(2, excess_full_sets, MOD) - 1) * pow(2, MOD - 2, MOD)) % MOD
```

### Step-by-Step Analysis:

1. **Calculate `excess_full_sets`:**
   \[
   \text{excess\_full\_sets} = \text{max\_full\_sets} - \left(\frac{n - m}{k - 1}\right)
   \]
   - `max_full_sets` is \(m // k\)
   - \((n - m) // (k - 1)\) is the integer division of \(n - m\) by \(k - 1\)

2. **Calculate `remaining_correct_answers`:**
   \[
   \text{remaining\_correct\_answers} = m - \text{excess\_full\_sets} \times k
   \]

3. **Calculate `score`:**
   \[
   \text{score} = (\text{remaining\_correct\_answers} + k \times (2^{\text{excess\_full\_sets}} - 1) \times 2^{MOD - 2}) \mod MOD
   \]
   - `pow(2, excess_full_sets, MOD)` computes \(2^{\text{excess\_full\_sets}} \mod MOD\)
   - `pow(2, MOD - 2, MOD)` computes \(2^{MOD - 2} \mod MOD\), which is the modular inverse of 2 modulo MOD

### Final Output State:

Combining all the changes from the code execution, the final state is:

Output State: **n is an integer such that \(2 \leq k \leq n \leq 10^9\), m is an integer such that \(0 \leq m \leq n\), k is an integer such that \(2 \leq k \leq n\), max_full_sets is \(m // k\), remaining_correct is \(m \% k\), (m > n - n // k), excess_full_sets is \(m // k - (n - m) // (k - 1)\), remaining_correct_answers is \(m - (m // k - (n - m) // (k - 1)) \times k\), score is \((m - (m // k - (n - m) // (k - 1)) \times k + k \times (2^{(m // k - (n - m) // (k - 1))} - 1) \times 2^{MOD - 2}) \mod MOD\)**
```