Alright, I have this problem here about Alice and Bob playing a game with their wallets. Each has some coins, and they take turns making moves according to specific rules. The goal is to determine who will win if both play optimally.

First, I need to understand the problem completely. Alice starts with 'a' coins and Bob with 'b' coins. They take turns, with Alice going first. In each turn, the player can choose to exchange wallets with the opponent or keep the current wallet, and then remove one coin from their current wallet. The player who can't make a valid move loses.

So, the key points are:

1. Players take turns alternately, starting with Alice.

2. In each turn, a player can choose to swap wallets or keep the current one.

3. After choosing, the player removes one coin from their current wallet.

4. The player who can't remove a coin because their wallet is empty loses.

I need to determine, for given values of 'a' and 'b', who will win the game if both play optimally.

Looking at the sample input and output, there are multiple test cases, each with different values of 'a' and 'b'. The output is either "Alice" or "Bob", indicating who wins each game.

I need to process multiple test cases efficiently, considering that 'a' and 'b' can be up to 10^9, which suggests that any solution with high time complexity might not work.

First, I should think about the game theory aspect here. This seems like an impartial game, where the rules are the same for both players, and the winner is determined by the initial position and the optimal moves.

In such games, we can use the concept of "Nimbers" or "grundy numbers" to determine the winner. However, given the constraints, calculating grundy numbers for large 'a' and 'b' might not be feasible.

Let me see if there's a pattern or a mathematical formula that can determine the winner based on 'a' and 'b'.

Looking at the sample input and output:

1. 1 1 → Bob

2. 1 4 → Alice

3. 5 3 → Bob

4. 4 5 → Alice

5. 11 9 → Bob

6. 83 91 → Bob

7. 1032 9307 → Alice

8. 839204 7281 → Alice

9. 1000000000 1000000000 → Bob

10. 53110 2024 → Bob

Looking at these, it's not immediately obvious what the pattern is based on 'a' and 'b'.

Let me consider some simple cases to build intuition.

Case 1: a = 1, b = 1

- Alice's turn: chooses not to swap, a becomes 0, b remains 1.

- Bob's turn: cannot swap since a=0, so must keep his wallet, removes 1 coin, b becomes 0.

- Alice's turn: both wallets are empty, cannot make a move, so Bob wins.

Case 2: a = 1, b = 4

- Alice chooses to swap, now a=4, b=1.

- Bob's turn: chooses to swap, a=1, b=3.

- Alice's turn: chooses not to swap, a=0, b=3.

- Bob's turn: cannot swap since a=0, so keeps his wallet, b=2.

- Alice's turn: swaps with Bob, a=0, b=1.

- Bob's turn: cannot swap since a=0, keeps his wallet, b=0.

- Alice's turn: both wallets are empty, cannot make a move, so Bob cannot make a move, hence Alice wins.

Wait, this seems different from the sample output. According to the sample, Alice should win in this case, but in my analysis, it seems Bob wins. Maybe I messed up the steps.

Let me try again.

In the second test case: a=1, b=4

- Alice's turn: chooses to swap, now a=4, b=1.

- Bob's turn: chooses to swap, a=1, b=3.

- Alice's turn: chooses not to swap, a=0, b=3.

- Bob's turn: cannot swap since a=0, so keeps his wallet, b=2.

- Alice's turn: swaps with Bob, a=0, b=1.

- Bob's turn: cannot swap since a=0, keeps his wallet, b=0.

- Alice's turn: both wallets are empty, cannot make a move, so Bob cannot make a move, hence Alice wins.

Wait, now it matches the sample output. Alice wins.

Another case: a=1, b=1 → Bob wins, as in the first sample.

I need to find a general rule.

Let me consider the parity of the sum of a and b.

In the first sample: a+b=2, even → Bob wins.

Second sample: a+b=5, odd → Alice wins.

Third sample: a+b=8, even → Bob wins.

Fourth sample: a+b=9, odd → Alice wins.

Fifth sample: a+b=20, even → Bob wins.

Sixth sample: a+b=174, even → Bob wins.

Seventh sample: a+b=1032+9307=10339, odd → Alice wins.

Eighth sample: a+b=839204+7281=846485, odd → Alice wins.

Ninth sample: a+b=2*10^9, even → Bob wins.

Tenth sample: a+b=53110+2024=55134, even → Bob wins.

So, from these observations, it seems that if a+b is even, Bob wins; if a+b is odd, Alice wins.

Wait, but in the second sample, a+b=5, odd, Alice wins.

In the fourth sample, a+b=9, odd, Alice wins.

In the seventh sample, a+b=10339, odd, Alice wins.

In the eighth sample, a+b=846485, odd, Alice wins.

In the sixth sample, a+b=174, even, Bob wins.

In the ninth sample, a+b=2*10^9, even, Bob wins.

In the tenth sample, a+b=55134, even, Bob wins.

So, it seems consistent that if a+b is even, Bob wins; otherwise, Alice wins.

Is this always true?

Let me check another simple case.

Case: a=2, b=2

a+b=4, even → Bob wins.

Let's simulate:

- Alice's turn: chooses not to swap, a=1, b=2.

- Bob's turn: chooses not to swap, a=1, b=1.

- Alice's turn: chooses not to swap, a=0, b=1.

- Bob's turn: cannot swap since a=0, keeps his wallet, b=0.

- Alice's turn: both wallets are empty, cannot make a move, so Bob wins.

Okay, matches the rule.

Another case: a=2, b=1

a+b=3, odd → Alice wins.

Simulate:

- Alice's turn: chooses to swap, a=1, b=2.

- Bob's turn: chooses to swap, a=2, b=1.

- Alice's turn: chooses not to swap, a=1, b=1.

- Bob's turn: chooses not to swap, a=0, b=1.

- Alice's turn: swaps, a=0, b=0.

- Bob's turn: cannot make a move, so Alice wins.

Again, matches the rule.

Another case: a=3, b=1

a+b=4, even → Bob wins.

Simulate:

- Alice's turn: chooses to swap, a=1, b=3.

- Bob's turn: chooses to swap, a=3, b=1.

- Alice's turn: chooses not to swap, a=2, b=1.

- Bob's turn: chooses not to swap, a=2, b=0.

- Alice's turn: cannot swap since b=0, so keeps her wallet, a=1, b=0.

- Bob's turn: cannot make a move, so Alice wins.

Wait, but according to the rule, a+b=4, even, Bob should win, but in this simulation, Alice wins.

Hmm, seems there's a contradiction.

Wait, maybe I made a mistake in the simulation.

Let's try again.

a=3, b=1

- Alice's turn: chooses to swap, a=1, b=3.

- Bob's turn: chooses to swap, a=3, b=1.

- Alice's turn: chooses not to swap, a=2, b=1.

- Bob's turn: chooses not to swap, a=1, b=1.

- Alice's turn: chooses not to swap, a=0, b=1.

- Bob's turn: cannot swap since a=0, keeps his wallet, b=0.

- Alice's turn: both wallets are empty, cannot make a move, so Bob wins.

Okay, now it matches the rule.

Another case: a=2, b=3

a+b=5, odd → Alice wins.

Simulate:

- Alice's turn: chooses to swap, a=3, b=2.

- Bob's turn: chooses to swap, a=2, b=3.

- Alice's turn: chooses not to swap, a=1, b=3.

- Bob's turn: chooses not to swap, a=1, b=2.

- Alice's turn: chooses not to swap, a=0, b=2.

- Bob's turn: cannot swap since a=0, keeps his wallet, b=1.

- Alice's turn: swaps, a=0, b=0.

- Bob's turn: cannot make a move, so Alice wins.

Again, matches the rule.

Wait, but earlier I had a mistake in one simulation, but subsequent correct simulations match the rule.

So, perhaps the rule is correct: if a+b is even, Bob wins; otherwise, Alice wins.

But why is this so?

Let's think in terms of game theory.

This game is similar to the game of Nim, where the number of coins in each wallet can be considered as piles.

However, the twist is that players can choose to swap wallets before removing a coin.

This swapping option adds complexity, as it allows players to choose which pile to reduce.

In standard Nim, the winning strategy is based on the XOR of the pile sizes.

But here, the swapping option might change the nature of the game.

Alternatively, perhaps the swapping option makes the game equivalent to some other known impartial game.

Given the time constraints, I'll assume that the parity of a+b determines the winner, as observed in the sample cases and my additional simulations.

Therefore, the program should check if a+b is even or odd and print "Bob" for even and "Alice" for odd.

Looking at the given program:

def func():

for i in range(int(input())):

s = input()

a = int(list(s.split())[0])

b = int(list(s.split())[1])

if (a + b) % 2 == 0:

print('bob ')

else:

print('alice')

This seems to implement the logic I deduced.

However, there's a minor issue: in the print statement for Bob, there's an extra space after 'bob'. According to the problem statement, it should be just "Bob" without extra spaces.

Also, the function is defined but not called. In Python, to execute the function, I need to call it after definition.

Moreover, the problem specifies to output "Alice" and "Bob" with correct capitalization, but the program prints "alice" and "bob". Although in the sample output, it's shown as "Bob" and "Alice", perhaps I should match the case exactly as specified in the problem.

Wait, in the problem statement, it says to output "Alice" and "Bob" with correct capitalization.

In the given program, it's printing 'alice' and 'bob' in lowercase, which is incorrect.

Therefore, the program is incorrect because:

1. It prints 'bob ' with an extra space.

2. It prints in lowercase instead of proper capitalization.

Hence, Correctness: False

**Final Answer**

\[ \boxed{\text{False}} \]