To determine the output of the `print(p1 - cur + p3)` statement, let's break down the given initial state and derive the necessary values step by step.

1. **Variables and Conditions:**
   - `t` is an input integer such that \(1 \leq t \leq 500\).
   - `p1`, `p2`, and `p3` are integers obtained from the input.
   - The sum of `p1`, `p2`, and `p3` is odd: \(p1 + p2 + p3\) is odd.
   - `p3` is less than the sum of `p1` and `p2`: \(p3 < p1 + p2\).
   - `low` is the minimum of `p3 - p1` and `p3 - p2`: \(low = \min(p3 - p1, p3 - p2)\).
   - `high` is the maximum of `p3 - p1` and `p3 - p2`: \(high = \max(p3 - p1, p3 - p2)\).
   - `cur` is equal to `low`: \(cur = low\).
   - `p1 - cur` is less than or equal to `p2 - (p3 - cur)`: \(p1 - cur \leq p2 - (p3 - cur)\).

2. **Analysis:**
   - Since `low` is the minimum of `p3 - p1` and `p3 - p2`, it means `cur` will take the smaller of these two values.
   - The condition \(p1 - cur \leq p2 - (p3 - cur)\) can be simplified as follows:
     \[
     p1 - cur \leq p2 - p3 + cur \implies p1 + p3 \leq p2 + 2cur
     \]
     Since `cur` is the minimum of `p3 - p1` and `p3 - p2`, it ensures that the inequality holds true.

3. **Expression to Print:**
   - The expression to print is `p1 - cur + p3`.
   - Substituting `cur = low`, we get `p1 - low + p3`.

4. **Determining the Value:**
   - Given that `low` is the minimum of `p3 - p1` and `p3 - p2`, we need to consider the possible values of `low`:
     - If \(p3 - p1 \leq p3 - p2\), then \(low = p3 - p1\).
     - If \(p3 - p2 \leq p3 - p1\), then \(low = p3 - p2\).
   - In either case, the expression `p1 - low + p3` simplifies to:
     - If \(low = p3 - p1\), then \(p1 - (p3 - p1) + p3 = p1 - p3 + p1 + p3 = 2p1\).
     - If \(low = p3 - p2\), then \(p1 - (p3 - p2) + p3 = p1 - p3 + p2 + p3 = p1 + p2\).

5. **Conclusion:**
   - Given the condition that the sum of `p1`, `p2`, and `p3` is odd, and considering the constraints, the expression `p1 - cur + p3` will always simplify to \(p1 + p2\).

Therefore, the output of the `print(p1 - cur + p3)` statement is:

Output: **p1 + p2**