Let's break down the problem step-by-step using the given initial state and the code snippet.

### Initial State:
- `t` is an integer such that \(1 \leq t \leq 500\).
- `p1`, `p2`, and `p3` are integers.
- The sum of `p1`, `p2`, and `p3` is odd.
- `low` is the minimum of `p3 - p1` and `p3 - p2`.
- `high` is the maximum of `p3 - p1` and `p3 - p2` and must be greater than `low + 1`.
- `cur` is determined by the condition: If `p1 - cur` is less than or equal to `p2 - (p3 - cur)`, `cur` remains `low`. Otherwise, `cur` is set to `low + 1`.

### Code Snippet:
```python
print(p1 - cur + p3)
```

### Step-by-Step Analysis:

1. **Determine `low` and `high`:**
   - `low = min(p3 - p1, p3 - p2)`
   - `high = max(p3 - p1, p3 - p2)`
   - It is given that `high > low + 1`.

2. **Determine `cur`:**
   - The condition to determine `cur` is:
     - If `p1 - cur` ≤ `p2 - (p3 - cur)`, then `cur = low`.
     - Otherwise, `cur = low + 1`.

3. **Simplify the condition:**
   - The condition `p1 - cur` ≤ `p2 - (p3 - cur)` can be rewritten as:
     - `p1 - cur` ≤ `p2 - p3 + cur`
     - `p1 + p3` ≤ `p2 + 2*cur`
     - `cur` ≥ `(p1 + p3 - p2) / 2`

4. **Determine the value of `cur`:**
   - If `(p1 + p3 - p2) / 2` is less than or equal to `low`, then `cur = low`.
   - If `(p1 + p3 - p2) / 2` is greater than `low`, then `cur = low + 1`.

5. **Calculate the output:**
   - The output is `p1 - cur + p3`.
   - Substitute the value of `cur` based on the condition.

### Output Determination:

Given the conditions and the formula for `cur`, we can express the output in terms of `p1`, `p2`, and `p3`.

- If `cur = low`, then the output is `p1 - low + p3`.
- If `cur = low + 1`, then the output is `p1 - (low + 1) + p3`.

Since `low` is `min(p3 - p1, p3 - p2)`, we can express the output in terms of `p1`, `p2`, and `p3` as follows:

- If `cur = low`, the output is `p1 - min(p3 - p1, p3 - p2) + p3`.
- If `cur = low + 1`, the output is `p1 - (min(p3 - p1, p3 - p2) + 1) + p3`.

### Final Output:

The final output depends on the condition `(p1 + p3 - p2) / 2`. However, we can describe the output precisely as:

- `p1 - cur + p3` where `cur` is determined by the condition `p1 - cur` ≤ `p2 - (p3 - cur)`.

Given the initial state, the output can be expressed as:

Output: **p1 - cur + p3 (where cur is determined by the condition p1 - cur ≤ p2 - (p3 - cur))**