The code snippet `y -= 1` decrements the value of `y` by 1. Given the initial state, `y` was equal to `p3`. After the decrement, `y` becomes `p3 - 1`.

The other variables (`t`, `p1`, `p2`, `p3`, and `x`) remain unchanged. The preconditions that `t` is at least 1, `p1`, `p2`, and `p3` are integers such that 0 ≤ `p1` ≤ `p2` ≤ `p3` ≤ 30, the sum of `p1`, `p2`, and `p3` is odd, and `p3` is less than `p1 + p2` are still valid. The value of `x` remains 1.

Output State: **`t` is at least 1; `p1`, `p2`, and `p3` are integers such that 0 ≤ `p1` ≤ `p2` ≤ `p3` ≤ 30, the sum of `p1`, `p2`, and `p3` is odd, and `p3` is less than `p1 + p2`; `x` is 1; `y` is `p3 - 1`.**