Let's break down the problem step by step.

### Step-by-Step Analysis

1. **Identify the Loop Condition:**
   The loop condition is given by:
   \[
   (x + y) \cdot x \leq n \quad \text{and} \quad (x + y) \cdot y \leq m
   \]

2. **Current States:**
   - \( x = 1 \)
   - \( n \geq 1 \)
   - \( m \geq 2 \)
   - \( cnt = 0 + \min(n // (2 \cdot 1), m // (2 \cdot 1)) \)
   - \( y = 2 \)

3. **Evaluate the Loop Condition with Current States:**
   Substitute the current values into the loop condition:
   \[
   (1 + 2) \cdot 1 \leq n \quad \Rightarrow \quad 3 \leq n
   \]
   \[
   (1 + 2) \cdot 2 \leq m \quad \Rightarrow \quad 6 \leq m
   \]

4. **Determine the Next Iteration Requirements:**
   For the loop to execute one more time, both conditions must still hold true after the next iteration. Therefore, we need to ensure:
   - \( (x + y) \cdot x \leq n \)
   - \( (x + y) \cdot y \leq m \)

5. **Adjust the States:**
   - Since \( x \) and \( y \) are constants in this context (1 and 2 respectively), they cannot be changed.
   - We need to ensure that \( n \) and \( m \) are such that the conditions are still met after the next iteration.

Given that \( x = 1 \) and \( y = 2 \), the conditions simplify to:
   - \( 3 \leq n \)
   - \( 6 \leq m \)

Since these conditions must hold true for the next iteration, we need to ensure that \( n \) and \( m \) are at least 3 and 6 respectively.

### Final State Adjustment

State: **`x` is 1, `n` must be at least 3, `m` must be at least 6, `cnt` is 0 + min(n // 2, m // 2), and `y` is 2**