Output State: `r` is `k * (n - 1) - sum(b[1:n])`.

To understand this, let's break down the loop and its effect on the variable `r`:

- The loop runs from `i = 1` to `i = n`.
- In each iteration, `r` is incremented by `k`.
- Then, it checks if `r` is less than `b[i]`. If it is, the loop prints 'NO' and returns, otherwise, it subtracts `b[i]` from `r`.

Given the output states after the first three iterations:

1. After 1 iteration: `r = k - b[1]`
2. After 2 iterations: `r = k - 2*b[1] + k = 2*k - 2*b[1]`
3. After 3 iterations: `r = k - 2*b[1] - b[3] + k = 2*k - 2*b[1] - b[3]`

Following this pattern, after `n` iterations, `r` will be:

\[ r = k \times (n - 1) - \sum_{i=1}^{n} b[i] \]

This is because `r` starts with `0`, gets incremented by `k` for each of the `n` iterations, and then subtracts `b[i]` for each `i` from `1` to `n`. Hence, the final value of `r` is `k * (n - 1)` minus the sum of `b[1]` through `b[n]`.