The code calculates the sum of the first `k` integers using the formula `k * (k + 1) // 2`. Given that `k` is defined as `a + b - 1`, the value of `sum_k` will be the sum of the first `k` integers. The other variables (`m`, `a`, `b`, `g`) are not affected by this calculation.

Let's break down the steps:

1. `k` is defined as `a + b - 1`.
2. `sum_k` is assigned the value of `k * (k + 1) // 2`.

Given the initial conditions:
- `m` is an integer such that \(1 \leq m \leq 10^9\).
- `a` is an integer such that \(1 \leq a \leq 10^5\).
- `b` is an integer such that \(1 \leq b \leq 10^5\).
- `g` is equal to 1.
- `k` is `a + b - 1`.
- \(m \geq a + b - 1\).

After executing the code:
- `m` remains unchanged, so it is still an integer such that \(1 \leq m \leq 10^9\).
- `a` remains unchanged, so it is still an integer such that \(1 \leq a \leq 10^5\).
- `b` remains unchanged, so it is still an integer such that \(1 \leq b \leq 10^5\).
- `g` remains unchanged, so it is still equal to 1.
- `k` is updated to `a + b - 1`.
- `sum_k` is calculated as `k * (k + 1) // 2`, which is `(a + b - 1) * (a + b) // 2`.

Therefore, the Output State is:
Output State: **`m` is an integer such that \(1 \leq m \leq 10^9\); `a` is an integer such that \(1 \leq a \leq 10^5\); `b` is an integer such that \(1 \leq b \leq 10^5\); `g` is equal to 1; `k` is `a + b - 1`; `sum_k` is \((a + b - 1) * (a + b) // 2**.