The line of code updates the value of `prefix_sum[i + 1]`. Here, `i` is initially 0. Therefore, we are calculating `prefix_sum[1]` by adding `prefix_sum[0]` and `a[0]`. Since `prefix_sum[0]` is 0 (as stated in the initial state), we have:

`prefix_sum[1] = prefix_sum[0] + a[0]`  
`prefix_sum[1] = 0 + a[0]`  
`prefix_sum[1] = a[0]`

Now, `i` is still 0 after this operation, but we need to note that the value of `prefix_sum[1]` has changed based on the first element of list `a`.

Output State: **`n` is a positive integer (1 ≤ n ≤ 100), `a` is a list of `n` integers, `prefix_sum` is a list where `prefix_sum[0]` is 0 and `prefix_sum[1]` is equal to `a[0]`, `i` is 0**