Reasoning:

The program is designed to solve the problem of reconstructing a permutation \( p \) from the array \( a \) where \( a_i = \texttt{MEX}(p_1, p_2, \ldots, p_i) - p_i \). Let's break down the logic and verify if it correctly reconstructs \( p \):

1. **Initialization**:
   - `t` is the number of test cases.
   - For each test case, `n` is the length of the permutation \( p \) and array \( a \).
   - `a` is a list of integers read from the input.

2. **Reconstruction of \( p \)**:
   - `p` is initialized as a list of \(-1\) of length \( n \).
   - `mex` is initialized to \( n \). This is because initially, the \(\texttt{MEX}\) of the empty array is \( 0 \), and as we add elements, the \(\texttt{MEX}\) will decrease.

3. **Backward Construction**:
   - The loop iterates from \( n-1 \) to \( 0 \) (inclusive).
   - For each index \( i \), the value \( p_i \) is set to \( \texttt{MEX}(p_1, p_2, \ldots, p_i) - a_i \).
   - The \(\texttt{MEX}\) is updated to the minimum of the current \(\texttt{MEX}\) and \( p_i \).

4. **Output**:
   - After the loop, the constructed permutation \( p \) is printed.

Let's verify the correctness with the provided example:

### Example Test Case 1:
- Input: \( n = 5 \), \( a = [1, 1, -2, 1, 2] \)
- Expected Output: \( p = [0, 1, 4, 2, 3] \)

#### Step-by-Step Execution:
- Initialize `p` as \([-1, -1, -1, -1, -1]\) and `mex` as \(5\).
- Iterate from \( i = 4 \) to \( i = 0 \):
  - \( i = 4 \): \( p_4 = \texttt{MEX}(p_1, p_2, p_3, p_4) - a_4 = 5 - 2 = 3 \)
  - \( i = 3 \): \( p_3 = \texttt{MEX}(p_1, p_2, p_3) - a_3 = 3 - 1 = 2 \)
  - \( i = 2 \): \( p_2 = \texttt{MEX}(p_1, p_2) - a_2 = 2 - (-2) = 4 \)
  - \( i = 1 \): \( p_1 = \texttt{MEX}(p_1) - a_1 = 4 - 1 = 1 \)
  - \( i = 0 \): \( p_0 = \texttt{MEX}() - a_0 = 1 - 1 = 0 \)

The final \( p \) is \([0, 1, 4, 2, 3]\), which matches the expected output.

### Example Test Case 2:
- Input: \( n = 5 \), \( a = [1, 1, 1, 1, 1] \)
- Expected Output: \( p = [0, 1, 2, 3, 4] \)

#### Step-by-Step Execution:
- Initialize `p` as \([-1, -1, -1, -1, -1]\) and `mex` as \(5\).
- Iterate from \( i = 4 \) to \( i = 0 \):
  - \( i = 4 \): \( p_4 = \texttt{MEX}(p_1, p_2, p_3, p_4) - a_4 = 5 - 1 = 4 \)
  - \( i = 3 \): \( p_3 = \texttt{MEX}(p_1, p_2, p_3) - a_3 = 4 - 1 = 3 \)
  - \( i = 2 \): \( p_2 = \texttt{MEX}(p_1, p_2) - a_2 = 3 - 1 = 2 \)
  - \( i = 1 \): \( p_1 = \texttt{MEX}(p_1) - a_1 = 2 - 1 = 1 \)
  - \( i = 0 \): \( p_0 = \texttt{MEX}() - a_0 = 1 - 1 = 0 \)

The final \( p \) is \([0, 1, 2, 3, 4]\), which matches the expected output.

### Example Test Case 3:
- Input: \( n = 3 \), \( a = [-2, 1, 2] \)
- Expected Output: \( p = [2, 0, 1] \)

#### Step-by-Step Execution:
- Initialize `p` as \([-1, -1, -1]\) and `mex` as \(3\).
- Iterate from \( i = 2 \) to \( i = 0 \):
  - \( i = 2 \): \( p_2 = \texttt{MEX}(p_1, p_2) - a_2 = 3 - 2 = 1 \)
  - \( i = 1 \): \( p_1 = \texttt{MEX}(p_1) - a_1 = 1 - 1 = 0 \)
  - \( i = 0 \): \( p_0 = \texttt{MEX}() - a_0 = 0 - (-2) = 2 \)

The final \( p \) is \([2, 0, 1]\), which matches the expected output.

### Conclusion:
The program correctly reconstructs the permutation \( p \) from the array \( a \) based on the given problem description and the provided examples. The logic of updating the \(\texttt{MEX}\) and constructing \( p \) in reverse order is sound and produces valid results.

Correctness: **True**