To determine the final output state after the loop has executed all its iterations, we need to understand how the loop progresses and affects the variables involved.

The loop runs from `i = 1` to `i = b`. For each iteration, it calculates `x` using the formula `(a - i * (i - 1)) // i ** 2 + 1`. If `a - i * (i - 1) > 0`, it adds `x` to `suma`.

Let's break down the loop's behavior:

1. **Initialization**:
   - `suma` starts at 0.
   - The loop runs from `i = 1` to `i = b`.

2. **Iteration Process**:
   - For each `i`, compute `x` using the given formula.
   - If `a - i * (i - 1) > 0`, add `x` to `suma`.

3. **Termination**:
   - The loop terminates when `i` exceeds `b`.

### Detailed Iteration Analysis:

- **First Iteration (`i = 1`)**:
  - `x = (a - 1 * (1 - 1)) // 1 ** 2 + 1 = (a - 0) // 1 + 1 = a + 1`
  - Since `a - 1 * (1 - 1) = a > 0` (assuming `a > 0`), `suma` becomes `a + 1`.

- **Second Iteration (`i = 2`)**:
  - `x = (a - 2 * (2 - 1)) // 2 ** 2 + 1 = (a - 2) // 4 + 1`
  - If `a - 2 > 0`, add `x` to `suma`.

- **Third Iteration (`i = 3`)**:
  - `x = (a - 3 * (3 - 1)) // 3 ** 2 + 1 = (a - 6) // 9 + 1`
  - If `a - 6 > 0`, add `x` to `suma`.

This pattern continues until `i = b`.

### Final Output State:

After all iterations, `i` will be `b + 1`, and `suma` will be the cumulative sum of all valid `x` values calculated during the loop.

**Output State: **`i` is `b + 1`; `suma` is the sum of all `x` values where `a - i * (i - 1) > 0` for `i` from 1 to `b`.**

In natural language, this means that after the loop finishes executing all its iterations, the variable `i` will be one more than `b` (since the loop runs from 1 to `b` inclusive), and `suma` will hold the total sum of all `x` values computed in each iteration where the condition `a - i * (i - 1) > 0` is satisfied.