The code snippet `b[i] = b[i - 1] + x` updates the value of `b[i]` based on the previous value of `b[i - 1]` and the value of `x`. Given the initial state, `b` is a list of cumulative sums, and `x` is determined by the condition `a[n] > 1`. 

Here's the updated output state:

- `b[i]` is updated to `b[i - 1] + x`.
- All other variables retain their initial values unless explicitly updated.

Natural language explanation: The value of `b[i]` is now the sum of the previous value `b[i - 1]` and `x`. All other variables remain unchanged.

Output State: **`t` is an integer such that 1 ≤ t ≤ 10^4, `n` is an integer such that 1 ≤ n ≤ 3 · 10^5, `q` is an integer such that 1 ≤ q ≤ 3 · 10^5, the array `c` is a list of `n` integers where each element is greater than 0 and less than or equal to 10^9, for each query `i`, `l_i` and `r_i` are integers such that 1 ≤ `l_i` ≤ `r_i` ≤ `n`, the sum of `n` over all test cases does not exceed 3 · 10^5 and the sum of `q` over all test cases does not exceed 3 · 10^5, `a` is a list where the first element is `0` and the subsequent elements are integers read from the input, `b` is a list of `n + 1` integers where `b[i]` is the cumulative sum of `x` from `b[1]` to `b[i]` and `b[i]` has been updated to `b[i - 1] + x`, `x` is 1 if `a[n] > 1` else 2, `i` is `n`.**