Let's break down the initial state and the code snippet step by step:

1. **Initial State:**
   - `n = 0`
   - `h = (n - k + 1) // (n - k + 1) + (n - k + 1) // 1`
   - `costs = [n - k + 1, 1]`
   - `h` is greater than or equal to `k`

2. **Calculate `h`:**
   - First, let's simplify the expression for `h`:
     - `n - k + 1` is a common term in the expression.
     - Let's denote `n - k + 1` as `x`. So, `x = 0 - k + 1 = 1 - k`.
   - Now, the expression for `h` becomes:
     - `h = x // x + x // 1`
     - Since `x = 1 - k`, we substitute:
     - `h = (1 - k) // (1 - k) + (1 - k) // 1`
   - The integer division `(1 - k) // (1 - k)` is 1 (as long as `1 - k` is not zero).
   - The integer division `(1 - k) // 1` is `1 - k`.
   - Therefore, `h = 1 + (1 - k)`.

3. **Condition `h >= k`:**
   - We need to ensure that `h >= k`.
   - Substituting the value of `h`:
     - `1 + (1 - k) >= k`
     - Simplifying: `2 - k >= k`
     - Rearranging: `2 >= 2k`
     - Dividing by 2: `1 >= k`
   - This implies that `k` must be 1 or less. Since `k` is typically an integer, the only valid value for `k` is 1.

4. **Calculate `costs`:**
   - `costs = [n - k + 1, 1]`
   - Substituting `n = 0` and `k = 1`:
     - `costs = [0 - 1 + 1, 1]`
     - `costs = [0, 1]`

5. **Print Statement:**
   - The print statement is `print(*costs)`.
   - The `*` operator unpacks the list `costs`, so the elements of the list are printed separated by spaces.

Output: **0 1**