Let's break down the given initial state and the print statement step by step:

1. **Initial State:**
   - `i` is 0.
   - `n` must be greater than 0.
   - The character at index `i` of string `s` is '>'.
   - The condition `l < r` is still false.
   - `b` is defined based on the formula:
     - If `l - r > 0`, then `b = A[l - 1] - A[l - r - 1] - (idx_A[l - 1] - idx_A[l - r - 1]) * (l - r) + (0 - idx_A[l - 1]) * r`.
     - If `l - r <= 0`, then `b = A[l - 1] + (0 - idx_A[l - 1]) * r`.

2. **Print Statement:**
   ```python
   print(a * 2 + b * 2 + (n - i), end=' ')
   ```

From the initial state, we know:
- `i` is 0.
- Since `l < r` is false, it means `l >= r`.

However, the value of `a` is not explicitly mentioned in the initial state. Given that `a` is not defined in the initial state and there's no other context to determine its value, we assume `a` is a variable that needs to be evaluated in the expression `a * 2 + b * 2 + (n - i)`.

Since `i` is 0, the term `(n - i)` simplifies to `n`.

Given that `b` is defined based on conditions involving `l` and `r`, and since `l >= r`, we need to consider both cases for `b`:
- If `l - r > 0`, then `b = A[l - 1] - A[l - r - 1] - (idx_A[l - 1] - idx_A[l - r - 1]) * (l - r) + (0 - idx_A[l - 1]) * r`.
- If `l - r <= 0`, then `b = A[l - 1] + (0 - idx_A[l - 1]) * r`.

Since `l >= r`, let's assume the simplest case where `l - r = 0` (which satisfies `l - r <= 0`):
- In this case, `b = A[l - 1] + (0 - idx_A[l - 1]) * r`.

Given that `r` is not specified but must be a non-negative integer, and assuming `r` is 0 for simplicity (since `l >= r` and `r` must be non-negative), we get:
- `b = A[l - 1] + (0 - idx_A[l - 1]) * 0 = A[l - 1]`.

Now, substituting these into the print statement:
- `a * 2 + b * 2 + (n - i) = a * 2 + A[l - 1] * 2 + n`.

Since `a` is not defined, we cannot determine its exact value. However, the expression simplifies to:
- `2a + 2A[l - 1] + n`.

Given that `n` must be greater than 0, and without knowing the exact value of `a` and `A[l - 1]`, we can represent the final output as:
- `2a + 2A[l - 1] + n`.

Output: **2a + 2A[l - 1] + n**