Let's break down the initial state and the print statement step by step:

1. **Initial State Analysis:**
   - `i` is `i + 1` if `i` was not 0. This means that `i` is now 1 (assuming `i` was 0 initially).
   - `n` must be greater than 0. This doesn't affect the current calculation directly but ensures `n > 0`.
   - `r` is decreased by 1. We need to know the initial value of `r` to determine this, but it's not provided. Let's assume `r` was initially `r0`.
   - `a` is calculated as `A[l - 1] + (i - idx_A[l - 1]) * l`. Here, `l` and `idx_A[l - 1]` are not provided, so let's assume `l = 2` and `idx_A[l - 1] = 1` for simplicity (these values would be specific to the actual problem context).
     - If `l = 2` and `idx_A[l - 1] = 1`, then `a = A[1] + (1 - 1) * 2 = A[1] + 0 = A[1]`.
   - `b` is calculated as `B[r] - B[r - l] - (idx_B[r - l] - i) * (r - l) + (idx_B[r] - i) * l`. Again, `l`, `r`, `idx_B[r - l]`, and `idx_B[r]` are not provided, so let's assume `l = 2`, `r = r0 - 1`, `idx_B[r - l] = 1`, and `idx_B[r] = 2` for simplicity.
     - If `l = 2`, `r = r0 - 1`, `idx_B[r - l] = 1`, and `idx_B[r] = 2`, then `b = B[r0 - 1] - B[r0 - 3] - (1 - 1) * (r0 - 2) + (2 - 1) * 2 = B[r0 - 1] - B[r0 - 3] + 2`.

2. **Print Statement Analysis:**
   - The print statement is `print(a * 2 + b * 2 + i + 1, end=' ')`.
   - Substituting the assumed values:
     - `a = A[1]`
     - `b = B[r0 - 1] - B[r0 - 3] + 2`
     - `i = 1`
   - Therefore, `a * 2 + b * 2 + i + 1 = 2 * A[1] + 2 * (B[r0 - 1] - B[r0 - 3] + 2) + 1 + 1 = 2 * A[1] + 2 * B[r0 - 1] - 2 * B[r0 - 3] + 4 + 1 + 1 = 2 * A[1] + 2 * B[r0 - 1] - 2 * B[r0 - 3] + 6`.

Given the assumptions and the lack of specific values for `A[1]`, `B[r0 - 1]`, and `B[r0 - 3]`, the output will be expressed in terms of these variables.

Output: **2 * A[1] + 2 * B[r0 - 1] - 2 * B[r0 - 3] + 6**