To determine the output of the `print` statement, let's analyze the given initial state and the code snippet step by step:

### Initial State Analysis:
- `t` is set to 0.
- `a` is a tuple with values `(-1000000000.0, 2000000000.0)`.
- `b` is a list with values `[0, 0]`.
- `u` is set to 0.
- `c` and `d` are the values returned by the function `r()`, and it is specified that `c` is greater than or equal to `d`.

### Code Snippet:
```python
print(b[c * 2 - 1] - b[d * 2 - 1])
```

### Step-by-Step Explanation:
1. **Values of `c` and `d`:**
   - Since `c` and `d` are the values returned by `r()`, their exact values are not provided in the initial state.
   - However, we know that `c >= d`.

2. **Index Calculation:**
   - The expression `c * 2 - 1` calculates an index for the list `b`.
   - Similarly, `d * 2 - 1` calculates another index for the list `b`.

3. **List `b` Access:**
   - The list `b` has only two elements: `[0, 0]`.
   - Therefore, the valid indices for `b` are 0 and 1.

4. **Possible Values of Indices:**
   - Since `c >= d`, and both `c` and `d` must result in valid indices for the list `b` (which are 0 and 1), the possible values for `c` and `d` are limited to 0 and 1.
   - Given `c >= d`, the possible pairs `(c, d)` are `(0, 0)` and `(1, 0)` and `(1, 1)`.

5. **Calculating the Output:**
   - For the pair `(0, 0)`:
     - `b[c * 2 - 1] = b[0 * 2 - 1] = b[-1] = 0` (since Python allows negative indexing, `-1` refers to the last element).
     - `b[d * 2 - 1] = b[0 * 2 - 1] = b[-1] = 0`.
     - The result is `0 - 0 = 0`.
   - For the pair `(1, 0)`:
     - `b[c * 2 - 1] = b[1 * 2 - 1] = b[1] = 0`.
     - `b[d * 2 - 1] = b[0 * 2 - 1] = b[-1] = 0`.
     - The result is `0 - 0 = 0`.
   - For the pair `(1, 1)`:
     - `b[c * 2 - 1] = b[1 * 2 - 1] = b[1] = 0`.
     - `b[d * 2 - 1] = b[1 * 2 - 1] = b[1] = 0`.
     - The result is `0 - 0 = 0`.

In all valid cases, the expression evaluates to `0`.

### Final Output:
Output: **0**