Let's analyze the given initial state and the print statement step by step:

### Initial State:
- `A = [0, 1, 3]`
- `idx_A = [3, 4, 5]`
- `B = [0, 1, 3]`
- `idx_B = [2, 1, 0]`
- `l = 0`
- `r = 3`
- `n` is greater than 0
- `s[i]` is `'>'`
- `a = 3 - 3 * i`
- `b = 3`

### Print Statement:
```python
print(a * 2 + b * 2 + (n - i), end=' ')
```

### Analysis:
To determine the output, we need to evaluate the expression inside the `print` statement. However, the variable `i` is not explicitly defined in the initial state. Since it is not provided, let's assume `i` could take any valid value within a reasonable range, but typically in such problems, `i` is often iterated over a sequence. For the sake of this problem, let's consider `i` to be a specific value that fits within the context, such as `i = 0` (since no other constraints are given).

Given `i = 0`:
- `a = 3 - 3 * i = 3 - 3 * 0 = 3`
- `b = 3`
- `n` is greater than 0, so let's assume `n = 1` for simplicity (since no specific value is given).

Now, substituting these values into the expression:
- `a * 2 + b * 2 + (n - i) = 3 * 2 + 3 * 2 + (1 - 0) = 6 + 6 + 1 = 13`

### Conclusion:
The output of the `print` statement, assuming `i = 0` and `n = 1`, will be `13`.

However, since the exact value of `i` and `n` are not specified, the most precise description based on the given information would be:

Output: **a * 2 + b * 2 + (n - i) (where a = 3 - 3 * i, b = 3, and n > 0)**

If we assume specific values for `i` and `n` as mentioned above, then:

Output: **13 (assuming i = 0 and n = 1)**

But adhering strictly to the format without assumptions about `i` and `n`:

Output: **a * 2 + b * 2 + (n - i) (where a = 3 - 3 * i, b = 3, and n > 0)**