Given the initial state and the code snippet, let's determine the new state after executing the code.

Initial State: 
- `A = [0, 1, 3]`
- `idx_A = [3, 4, 5]`
- `B = [0, 1, 3]`
- `idx_B = [2, 1, 0]`
- `l = 0`
- `r = 2`
- `n` is greater than 0
- `s[i]` is not equal to `'>'`
- `l` is less than or equal to `r`
- `l` is not equal to 0
- `a = 3`
- `b = 3`
- `r - l` is greater than or equal to 0

Code Snippet:
```python
b = b - B[r - l]
```

From the initial state, we know:
- `r = 2`
- `l = 0`
- `B = [0, 1, 3]`

So, `r - l` equals `2 - 0` which is `2`. Therefore, `B[r - l]` is `B[2]` which is `3`.

The code snippet updates `b` by subtracting `B[r - l]` from `b`. Since `b` was initially `3` and `B[r - l]` is `3`, the new value of `b` will be `3 - 3` which is `0`.

All other variables remain unchanged.

Output State: **`A = [0, 1, 3]`, `idx_A = [3, 4, 5]`, `B = [0, 1, 3]`, `idx_B = [2, 1, 0]`, `l = 0`, `r = 2`, `n` is greater than 0, `s[i]` is not equal to `'>'`, `l` is less than or equal to `r`, `l` is not equal to 0, `a = 3`, `b = 0`, and `r - l` is greater than or equal to 0**.