To determine the output state, let's analyze the given code snippet and the initial state.

Given:
- `A = [0, 1, 3]`
- `idx_A = [3, 4, 5]`
- `B = [0, 1, 3]`
- `idx_B = [2, 1, 0]`
- `l = 0`
- `r = 2`
- `n` is greater than 0
- `s[i]` is not equal to `'>'`
- `l` is less than or equal to `r`
- `l` is not equal to 0
- `a = 3`
- `b = 0`
- `r - l` is greater than or equal to 0

Code snippet:
```python
b = b - (idx_B[r - l] - i) * (r - l)
```

First, calculate the indices and values used in the equation:
- `r - l` is `2 - 0` which equals `2`.
- `idx_B[r - l]` is `idx_B[2]` which equals `0`.
- The expression `(idx_B[r - l] - i)` becomes `(0 - i)`, but since `i` is not defined in the initial state, we cannot compute a specific value for this part. However, we can express `b` in terms of `i`.

The equation now looks like:
```python
b = 0 - (0 - i) * 2
```
Which simplifies to:
```python
b = -(-i * 2)
b = 2 * i
```

Thus, `b` is updated to `2 * i`.

Since `i` is not defined in the initial state, we express `b` in terms of `i`. All other variables remain unchanged.

Output State: **`A = [0, 1, 3]`, `idx_A = [3, 4, 5]`, `B = [0, 1, 3]`, `idx_B = [2, 1, 0]`, `l = 0`, `r = 2`, `n` is greater than 0, `s[i]` is not equal to `'>'`, `l` is less than or equal to `r`, `l` is not equal to 0, `a = 3`, `b = 2 * i`, and `r - l` is greater than or equal to 0**.