To determine what will be printed by the given `print` statement, let's break down the variables and their relationships based on the initial state and the conditions provided:

### Initial State Recap:
- `A = [0, 1, 3]`
- `idx_A = [3, 4, 5]`
- `B = [0, 1, 3]`
- `idx_B = [2, 1, 0]`
- `n` is greater than 0
- `s[i]` is either `'>'` or not `'>'`
- `i` is incremented by 1
- `a` is `A[l]` where `l` is an undefined index
- `x` is `r - (l + 2)`
- `b` is `(idx_B[r - 1] - i) * (l + 1)`

### Analysis:
1. **Variable `a`**: This is defined as `A[l]`, where `l` is an undefined index. Since `l` is not specified, `a` could be any of the elements in `A`, i.e., `0`, `1`, or `3`.

2. **Variable `b`**: This is defined as `(idx_B[r - 1] - i) * (l + 1)`. Here, `r` is also undefined, but `idx_B` is `[2, 1, 0]`. The value of `b` depends on the values of `r`, `i`, and `l`.

3. **Variable `i`**: This is incremented by 1, but its initial value is not specified. Let's denote its initial value as `i_initial`. Therefore, `i = i_initial + 1`.

4. **Expression to be printed**: `a * 2 + b * 2 + i + 1`

### Calculation:
Given the undefined nature of `l` and `r`, let's consider a specific scenario to illustrate the calculation. Suppose:
- `l = 1` (arbitrarily chosen from the indices of `A`)
- `r = 2` (arbitrarily chosen from the indices of `idx_B`)
- `i_initial = 0` (arbitrarily chosen)

Then:
- `a = A[1] = 1`
- `b = (idx_B[2 - 1] - i) * (1 + 1) = (idx_B[1] - 1) * 2 = (1 - 1) * 2 = 0`
- `i = i_initial + 1 = 0 + 1 = 1`

Substituting these into the expression:
- `a * 2 + b * 2 + i + 1 = 1 * 2 + 0 * 2 + 1 + 1 = 2 + 0 + 1 + 1 = 4`

### General Case:
While the specific values of `l`, `r`, and `i_initial` were chosen arbitrarily, the expression `a * 2 + b * 2 + i + 1` will always depend on these variables. The precise value cannot be determined without knowing the exact values of `l`, `r`, and `i_initial`.

### Conclusion:
The output will be a value derived from the expression `a * 2 + b * 2 + i + 1`, where `a` is an element from `A`, `b` is calculated based on `idx_B`, `r`, and `i`, and `i` is incremented by 1 from its initial value.

Output: **a * 2 + b * 2 + i + 1 (where a is A[l], b is (idx_B[r - 1] - i) * (l + 1), and i is incremented by 1 from its initial value)**