To determine the new value of `b` after the given operation, let's first express `b` before the operation and then apply the operation.

Initial State:
- `A = [0, 1, 3]`
- `idx_A = [3, 4, 5]`
- `B = [0, 1, 3]`
- `idx_B = [2, 1, 0]`
- `n` is greater than 0
- `s[i]` is either `'>'` or not `'>'`
- `i` is incremented by 1
- `a = B[r - 1] + (idx_B[r - 1] - i) * r`
- `b = A[l - 1] - A[l - r - 1]`

The operation to perform:
```python
b = b - (idx_A[l - 1] - idx_A[l - r - 1]) * (l - r)
```

Let's denote:
- `b_initial = A[l - 1] - A[l - r - 1]`
- `delta_idx_A = idx_A[l - 1] - idx_A[l - r - 1]`
- `factor = l - r`

Then the new value of `b` will be:
- `b_new = b_initial - delta_idx_A * factor`

Since the exact values of `l` and `r` are not specified, we'll keep them as variables in the final expression. However, we can express the updated value of `b` in terms of these variables.

Output State: **`A = [0, 1, 3]`, `idx_A = [3, 4, 5]`, `B = [0, 1, 3]`, `idx_B = [2, 1, 0]`, `n` is greater than 0, `s[i]` is either `'>'` or not `'>'`, `i` is incremented by 1, `a = B[r - 1] + (idx_B[r - 1] - i) * r`, `b = A[l - 1] - A[l - r - 1] - (idx_A[l - 1] - idx_A[l - r - 1]) * (l - r)`**

In natural language: The value of `b` is updated to its initial value minus the product of the difference between `idx_A[l - 1]` and `idx_A[l - r - 1]` and the difference between `l` and `r`. All other variables remain unchanged.