Let's analyze the given code snippet and its impact on the variables:

The code snippet is:
```python
b = b + (i - idx_A[l - 1]) * r
```

From the initial state, we know:
- `A = [0, 1, 3]`
- `idx_A = [3, 4, 5]`
- `B = [0, 1, 3]`
- `idx_B = [2, 1, 0]`
- `n` is greater than 0
- `s[i]` is either `'>'` or not `'>'`
- `i` is incremented by 1
- `a = B[r - 1] + (idx_B[r - 1] - i) * r`
- If `l - r > 0`, then `b = A[l - 1] - A[l - r - 1] - (idx_A[l - 1] - idx_A[l - r - 1]) * (l - r)`. Otherwise, `b = A[l - 1]`.

The value of `b` is updated by adding `(i - idx_A[l - 1]) * r` to it.

To determine the new value of `b`, we need to consider the expressions for `b` and the updated value of `b`:

1. **If `l - r > 0`:**
   \[
   b = A[l - 1] - A[l - r - 1] - (idx_A[l - 1] - idx_A[l - r - 1]) * (l - r)
   \]
   After updating:
   \[
   b = b + (i - idx_A[l - 1]) * r
   \]

2. **If `l - r <= 0`:**
   \[
   b = A[l - 1]
   \]
   After updating:
   \[
   b = b + (i - idx_A[l - 1]) * r
   \]

Since the exact values of `l`, `r`, and `i` are not specified, we'll keep the expressions in terms of these variables.

The updated value of `b` is:
\[
b = \text{previous\_value\_of\_b} + (i - idx_A[l - 1]) * r
\]

Given the initial state, the only variable that changes is `b`.

Output State: **`A = [0, 1, 3]`, `idx_A = [3, 4, 5]`, `B = [0, 1, 3]`, `idx_B = [2, 1, 0]`, `n` is greater than 0, `s[i]` is either `'>'` or not `'>'`, `i` is incremented by 1, `a = B[r - 1] + (idx_B[r - 1] - i) * r`, `b = \text{previous\_value\_of\_b} + (i - idx_A[l - 1]) * r`**