To determine what will be printed by the given Python code snippet, let's break down the expression step-by-step using the provided initial state:

### Given Initial State:
- `A = [0, 1, 3]`
- `idx_A = [3, 4, 5]`
- `B = [0, 1, 3]`
- `idx_B = [2, 1, 0]`
- `n` is greater than 0 (the exact value of `n` is not specified)
- `s[i]` is either `'>'` or not `'>'` (the exact value of `s[i]` is not specified)
- `i` is incremented by 1 (the exact value of `i` is not specified but it is incremented from its previous value)
- `r` is decreased by 1 (the exact value of `r` is not specified but it is decremented from its previous value)

### Expression to Evaluate:
```python
print(n - i + (i - idx_A[l - 1]) * 2, end=' ')
```

### Analysis:
1. **Variable `l`:** This variable is not defined in the initial state. However, since it is used as an index for `idx_A`, we need to assume a valid value for `l` that does not cause an `IndexError`. Let's assume `l` is 1, 2, or 3 (since these are valid indices for `idx_A`).

2. **Expression Breakdown:**
   - `n - i`: This part depends on the current values of `n` and `i`.
   - `(i - idx_A[l - 1]) * 2`: This part depends on the value of `i` and the value of `idx_A[l - 1]`.

Let's consider a specific case where `l = 2` for demonstration purposes. This means `idx_A[l - 1]` would be `idx_A[1]`, which is `4`.

3. **Substituting Values:**
   - Assume `n = 10` (since `n` is greater than 0).
   - Assume `i = 5` (since `i` is incremented by 1 from some initial value).
   - `idx_A[l - 1] = idx_A[1] = 4`.

4. **Evaluate the Expression:**
   - `n - i = 10 - 5 = 5`
   - `i - idx_A[l - 1] = 5 - 4 = 1`
   - `(i - idx_A[l - 1]) * 2 = 1 * 2 = 2`
   - Final expression value: `5 + 2 = 7`

### Conclusion:
Given the assumptions (`n = 10`, `i = 5`, `l = 2`), the expression evaluates to `7`. However, without specific values for `n`, `i`, and `l`, we can only describe the output in terms of these variables.

### General Output Description:
The expression `n - i + (i - idx_A[l - 1]) * 2` will be evaluated based on the current values of `n`, `i`, and `l`. Since `l` is used as an index for `idx_A`, it must be a valid index (1, 2, or 3).

Output: **n - i + (i - idx_A[l - 1]) * 2 (where n is greater than 0, i is incremented by 1, and l is a valid index for idx_A)**