To determine the output state, let's break down the given code snippet and apply it to the initial state:

Initial State:
- `A = [0, 1, 3]`
- `idx_A = [3, 4, 5]`
- `B = [0, 1, 3]`
- `idx_B = [2, 1, 0]`
- `n` is greater than 0
- `s[i]` is either `'>'` or not `'>'`
- `i` is incremented by 1
- `r` is decreased by 1
- `a` is either `0` or `1` depending on the new value of `r`
- `b` is `3`

Code Snippet:
```python
b = b - (idx_A[l - 1] - idx_A[l - r - 2]) * (l - r - 1)
```

From the code, we see that `b` is being updated based on the values of `idx_A`, `l`, and `r`. However, the variables `l` and `r` are not defined in the initial state, so we need to assume they have some specific values to proceed with the calculation.

Let's assume some plausible values for `l` and `r` that fit the context. Since `r` is decreased by 1 and `a` depends on `r`, let's assume `r` was initially 2 (so it becomes 1 after decrementing). For `l`, since it is used as an index, it should be within the bounds of the lists. Let's assume `l` is 3.

With these assumptions:
- `r` is 1 (after decrementing from 2)
- `l` is 3

Now, substitute these values into the equation:
```python
b = b - (idx_A[3 - 1] - idx_A[3 - 1 - 2]) * (3 - 1 - 1)
b = 3 - (idx_A[2] - idx_A[0]) * (1)
b = 3 - (5 - 3) * 1
b = 3 - 2 * 1
b = 3 - 2
b = 1
```

So, `b` is updated to 1. All other variables remain unchanged.

Output State: **`A = [0, 1, 3]`, `idx_A = [3, 4, 5]`, `B = [0, 1, 3]`, `idx_B = [2, 1, 0]`, `n` is greater than 0, `s[i]` is either `'>'` or not `'>'`, `i` is incremented by 1, `r` is 1, `a` is either `0` or `1` depending on the new value of `r`, `b` is 1**.