Given the initial state and the provided code snippet, we need to determine the new state after executing the line `b = B[r - 1]`.

The initial state provides the following information:
- `A = [0, 1, 3]`
- `idx_A = [3, 4, 5]`
- `B = [0, 1, 3]`
- `idx_B = [2, 1, 0]`
- `n` is greater than 0
- `s[i]` is either `'>'` or not `'>'`
- `i` is 1
- `a` is 1
- `x` is `r - (l + 2)`

The code snippet assigns the value of `B[r - 1]` to `b`. To find the exact value of `b`, we need to know the value of `r`. However, since the value of `r` is not specified in the initial state, we can only express `b` in terms of `r`.

Thus, after executing the code, the new state is:

Output State: **`A = [0, 1, 3]`, `idx_A = [3, 4, 5]`, `B = [0, 1, 3]`, `idx_B = [2, 1, 0]`, `n` is greater than 0, `s[i]` is either `'>'` or not `'>'`, `i` is 1, `a` is 1, `x` is `r - (l + 2)`, `b` is `B[r - 1]`**

In natural language, the output state remains largely the same except that a new variable `b` is introduced and assigned the value of `B[r - 1]`, where `r` is an unspecified variable from the initial conditions.