Given the initial state and the provided code snippet, we need to determine the new value of `b` after executing the line `b = (idx_B[r - 1] - i) * (l + 1)`.

From the initial state, we know:
- `A = [0, 1, 3]`
- `idx_A = [3, 4, 5]`
- `B = [0, 1, 3]`
- `idx_B = [2, 1, 0]`
- `n` is greater than 0
- `s[i]` is either `'>'` or not `'>'`
- `i` is 1
- `a` is 1
- `x` is `r - (l + 2)`
- If `x` is greater than or equal to 0, `b` is updated to `2 - (idx_B[x] - idx_B[r - 1]) * (x + 1)`

The code snippet updates `b` to `(idx_B[r - 1] - i) * (l + 1)`.

Since `i` is 1, the expression simplifies to `b = (idx_B[r - 1] - 1) * (l + 1)`.

We don't have specific values for `r` and `l`, but we can express the new value of `b` in terms of these variables.

Therefore, the new value of `b` is `(idx_B[r - 1] - 1) * (l + 1)`.

Other variables remain unchanged.

Output State: **`A = [0, 1, 3]`, `idx_A = [3, 4, 5]`, `B = [0, 1, 3]`, `idx_B = [2, 1, 0]`, `n` is greater than 0, `s[i]` is either `'>'` or not `'>'`, `i` is 1, `a` is 1, `x` is `r - (l + 2)`, `b` is `(idx_B[r - 1] - 1) * (l + 1)`**.