To determine the output state, let's first identify which variables are involved in the given code snippet and their initial values:

- `A = [0, 1, 3]`
- `idx_A = [3, 4, 5]`
- `B = [0, 1, 3]`
- `idx_B = [2, 1, 0]`
- `n` is greater than 0
- `s[i]` is either `'>'` or not `'>'`
- `i` is 1
- `a` is `B[r - 1] + (idx_B[r - 1] - i) * r`
- `b` is 3

The code snippet modifies the variable `b`:

```python
b = b - (idx_A[l - 1] - idx_A[l - r - 1]) * (l - r)
```

From the initial state, we know the value of `b` is 3. However, the values of `l` and `r` are not provided in the initial state. Since these variables are not defined in the initial state, we cannot compute the exact new value of `b`. We'll assume `l` and `r` are defined elsewhere in the program and proceed with the general form.

Given the formula, the new value of `b` depends on the values of `l` and `r`. Let's denote the new value of `b` as:

\[ b_{\text{new}} = 3 - (\text{idx\_A}[l - 1] - \text{idx\_A}[l - r - 1]) \times (l - r) \]

Since `l` and `r` are not specified, we cannot simplify further. The other variables remain unchanged.

Output State: **`A = [0, 1, 3]`, `idx_A = [3, 4, 5]`, `B = [0, 1, 3]`, `idx_B = [2, 1, 0]`, `n` is greater than 0, `s[i]` is either `'>'` or not `'>'`, `i` is 1, `a` is `B[r - 1] + (idx_B[r - 1] - i) * r`, `b` is `3 - (idx_A[l - 1] - idx_A[l - r - 1]) * (l - r)`**.