To determine the output state, we need to evaluate the given code snippet in the context of the initial state provided.

The code snippet is:
```python
a = a + (i - idx_A[l - 1]) * l
```

Given the initial state:
- `A = [0, 1, 3]`
- `idx_A = [3, 4, 5]`
- `B = [0, 1, 3]`
- `idx_B = [2, 1, 0]`
- `n` is greater than 0
- `s[i]` is either `'>'` or not `'>'`
- `i` is 1
- `r` is decreased by 1 (though `r` is not used in the code snippet)
- `a` is 0

The variable `l` is not defined in the initial state, so we cannot proceed without knowing its value. However, since `l` is used as an index for `idx_A`, it must be a valid index for the list `idx_A`, which has three elements. Let's assume `l` is one of the indices 1, 2, or 3 (since Python uses 0-based indexing, `l` would be 1, 2, or 3).

Let's consider each possible value for `l`:

1. If `l = 1`:
   ```python
   a = a + (i - idx_A[0]) * 1
   a = 0 + (1 - 3) * 1
   a = 0 + (-2) * 1
   a = -2
   ```

2. If `l = 2`:
   ```python
   a = a + (i - idx_A[1]) * 2
   a = 0 + (1 - 4) * 2
   a = 0 + (-3) * 2
   a = -6
   ```

3. If `l = 3`:
   ```python
   a = a + (i - idx_A[2]) * 3
   a = 0 + (1 - 5) * 3
   a = 0 + (-4) * 3
   a = -12
   ```

Since the value of `l` is not specified, we cannot determine a single definitive output state. However, we can express the output state in terms of `l`.

If `l` is 1, then `a` becomes -2.
If `l` is 2, then `a` becomes -6.
If `l` is 3, then `a` becomes -12.

Thus, the output state can be expressed as:
Output State: **`A = [0, 1, 3]`, `idx_A = [3, 4, 5]`, `B = [0, 1, 3]`, `idx_B = [2, 1, 0]`, `n` is greater than 0, `s[i]` is either `'>'` or not `'>'`, `i` is 1, `r` is decreased by 1, `a` is `-2` if `l` is 1, `a` is `-6` if `l` is 2, `a` is `-12` if `l` is 3**.