To determine the output state, let's analyze the given code snippet and the initial state:

Given:
- `A = [0, 1, 3]`
- `idx_A = [3, 4, 5]`
- `B = [0, 1, 3]`
- `idx_B = [2, 1, 0]`
- `n` is greater than 0
- `s[i]` is either `'>'` or not `'>'`
- `i` is 1
- `r` is decreased by 1 (so `r` is now `r - 1`)
- `a` is `-2` if `l` is 1, `a` is `-6` if `l` is 2, `a` is `-12` if `l` is 3
- `b` is `B[r]` which is either `0`, `1`, or `3` depending on the value of `r` after the decrement.

The code snippet is:
```python
b = b - B[r - l]
```

Let's break down the changes:
- `b` is initially `B[r]`. Since `r` was decremented, `b` could be `B[r]` where `r` is now `r - 1`.
- The new value of `b` is calculated as `b - B[r - l]`.

Since the exact values of `r` and `l` are not specified, we need to consider the possible values for `b` and `B[r - l]` based on the possible values of `r` and `l`.

Let's assume `r` was originally 2 (since `r` is decreased by 1, it could have been 3 originally). This means:
- `b` was initially `B[2]` which is `3`.
- Now, `r` is `1` (since `r` was decreased by 1).

We need to consider the possible values of `l`:
- If `l` is 1, `b = 3 - B[1 - 1] = 3 - B[0] = 3 - 0 = 3`.
- If `l` is 2, `b = 3 - B[1 - 2] = 3 - B[-1]`. However, since `B` does not have a negative index, this case is invalid.
- If `l` is 3, `b = 3 - B[1 - 3] = 3 - B[-2]`. Again, this is invalid because `B` does not have a negative index.

So, the only valid case is when `l` is 1, and `b` remains `3`.

Therefore, the updated output state is:
Output State: **`A = [0, 1, 3]`, `idx_A = [3, 4, 5]`, `B = [0, 1, 3]`, `idx_B = [2, 1, 0]`, `n` is greater than 0, `s[i]` is either `'>'` or not `'>'`, `i` is 1, `r` is `r - 1`, `a` is `-2` if `l` is 1, `a` is `-6` if `l` is 2, `a` is `-12` if `l` is 3, `b` is `3`**.