To determine the new value of `b`, we need to evaluate the expression `b = b + (idx_B[r] - i) * l`. 

Given the initial state:
- `A = [0, 1, 3]`
- `idx_A = [3, 4, 5]`
- `B = [0, 1, 3]`
- `idx_B = [2, 1, 0]`
- `n` is greater than 0
- `s[i]` is either `'>'` or not `'>'`
- `i` is 1
- If `r - l >= 0`, then `r` is decreased by 1 and `b` is set to 3. Otherwise, `r` and `b` remain unchanged.
- `a` is `-2` if `l` is 1, `a` is `-6` if `l` is 2, `a` is `-12` if `l` is 3.

From the conditions given, we know that `b` was initially set to 3 because `r - l >= 0`.

Let's assume `r` and `l` have values that satisfy `r - l >= 0` and `r` has been decremented by 1, and `b` has been set to 3. Now we need to compute the new value of `b` using the formula provided.

We need the values of `idx_B[r]` and `i`:
- `i` is given as 1.
- Since `r` was decremented by 1, let's assume the original `r` was 2 (as it's the highest index in `idx_B`). After decrementing, `r` would be 1.
- `idx_B[r]` when `r` is 1 is `idx_B[1]`, which is 1.

Now we substitute these values into the equation:
\[ b = 3 + (1 - 1) * l \]
\[ b = 3 + 0 * l \]
\[ b = 3 \]

Thus, the value of `b` remains 3.

Output State: **`A = [0, 1, 3]`, `idx_A = [3, 4, 5]`, `B = [0, 1, 3]`, `idx_B = [2, 1, 0]`, `n` is greater than 0, `s[i]` is either `'>'` or not `'>'`, `i` is 1, `b` is 3, `a` is `-2` if `l` is 1, `a` is `-6` if `l` is 2, `a` is `-12` if `l` is 3.**