To determine what will be printed, let's break down the expression inside the `print` statement step by step using the provided initial state:

Given:
- `A = [0, 1, 3]`
- `idx_A = [3, 4, 5]`
- `B = [0, 1, 3]`
- `idx_B = [2, 1, 0]`
- `n` is greater than 0 (the exact value is not specified, so we'll keep it as `n`)
- `s[i]` is either `'>'` or not `'>'` (not directly relevant to this print statement)
- `i = 1`
- `r` is decreased by 1 (not directly relevant to this print statement)

The print statement is:
```python
print(n - i + (i - idx_A[l - 1]) * 2, end=' ')
```

However, there is a variable `l` in the expression `idx_A[l - 1]` that is not defined in the initial state. Since `l` is not provided, we cannot determine its exact value. But for the sake of explanation, let's assume `l` is a valid index for the list `idx_A`.

Let's consider different possible values for `l` and see how the output changes:

1. If `l = 1`:
   - `idx_A[l - 1] = idx_A[0] = 3`
   - Expression becomes: `n - 1 + (1 - 3) * 2 = n - 1 + (-2) * 2 = n - 1 - 4 = n - 5`

2. If `l = 2`:
   - `idx_A[l - 1] = idx_A[1] = 4`
   - Expression becomes: `n - 1 + (1 - 4) * 2 = n - 1 + (-3) * 2 = n - 1 - 6 = n - 7`

3. If `l = 3`:
   - `idx_A[l - 1] = idx_A[2] = 5`
   - Expression becomes: `n - 1 + (1 - 5) * 2 = n - 1 + (-4) * 2 = n - 1 - 8 = n - 9`

Since the exact value of `l` is not provided, we cannot determine a single numerical output. However, we can describe the output in terms of `n` and `l`.

Output: **n - 1 + (1 - idx_A[l - 1]) * 2 (where l is a valid index for the list idx_A)**