Correctness: **False**

### Explanation:
The provided solution has a logical error in the `func_1` function. The approach used to calculate `ans[i]` is incorrect because it assumes that \( a_{i+1} - x_i \) will always yield a valid \( a_i \) such that \( x_i = a_i \bmod a_{i+1} \). This assumption does not hold in general and can lead to invalid results.

To correctly solve this problem, we need to ensure that \( a_i \) is chosen such that \( x_i = a_i \bmod a_{i-1} \). One correct approach is to set \( a_i \) to be at least \( a_{i-1} + x_i \), ensuring that the modulo condition holds.

Here's a corrected version of the code:

```python
t = int(input())
while t:
    n = int(input())
    arr = [int(x) for x in input().split(' ')]
    ans = func_1(arr, n)
    for i in ans:
        print(i, end=' ')
    print()
    t -= 1

def func_1(arr, n):
    ans = [10 ** 9] * n
    ans[n - 1] = 1  # Initialize the last element of ans to 1
    for i in range(n - 2, -1, -1):
        ans[i] = ans[i + 1] + arr[i]
    return ans
```

This corrected code initializes the last element of `ans` to 1 and then iterates backward through the array, setting each `ans[i]` to be at least `ans[i + 1] + x_i`, ensuring the modulo condition is satisfied.