Based on the initial state provided:

- `t` is an integer such that 1 ≤ t ≤ 1000.
- `n` is an integer such that 1 ≤ n ≤ 10^18.
- `k` is an integer such that 1 ≤ k ≤ 10^18.
- `n` is greater than `k`.
- The condition `k - 1 < n - k + 1` is satisfied.

We need to evaluate the expression `n - k + 1` and the number `1`.

Given the constraints, we know that `n` and `k` are positive integers with `n > k`. The expression `n - k + 1` will result in a positive integer since `n` is greater than `k`.

The second part of the print statement is simply the integer `1`.

Therefore, the output of the print statement will be the value of `n - k + 1` followed by the integer `1`.

Output: **n - k + 1, 1**