The code calculates the `triangular_number` based on the value of `k`. Given that `k` is 1, we can substitute this value into the formula to find the `triangular_number`. 

`triangular_number = k * (k + 1) // 2` becomes 
`triangular_number = 1 * (1 + 1) // 2` which simplifies to 
`triangular_number = 1 * 2 // 2` and further to 
`triangular_number = 2 // 2` resulting in 
`triangular_number = 1`.

The value of `n` is not affected by the code, so it remains a positive integer. The value of `k` is also not changed by the code, so it remains 1.

Output State: **`n` is a positive integer, `k` is 1, `triangular_number` is 1**