Let's break down the initial state and the print statement step by step:

1. **Initial State:**
   - `n` and `k` are positive integers such that \(1 \leq n \leq 26\) and \(1 \leq k \leq 26\).
   - `t` is greater than 0.
   - `i` is 0.
   - `s` is the string containing the first `k` letters of the alphabet starting from 'a'.
   - `j` is `k` + 96.
   - `k` is not equal to 1.

2. **Print Statement:**
   ```python
   print((2 - (n == 1)) * s)
   ```

3. **Explanation:**
   - The expression `(2 - (n == 1))` is a conditional expression that evaluates to 1 if `n` is 1, and 2 if `n` is not 1.
   - Since `k` is not equal to 1, `s` is a string containing the first `k` letters of the alphabet starting from 'a'. For example, if `k` is 3, `s` would be "abc".
   - The expression `(2 - (n == 1)) * s` will either print `s` once (if `n` is 1) or `s` twice (if `n` is not 1).

4. **Final Output:**
   - If `n` is 1, the output will be `s` once.
   - If `n` is not 1, the output will be `s` twice.

Since `k` is not equal to 1, `s` will always be a non-empty string containing the first `k` letters of the alphabet. Therefore, the output will be:

Output: **s (if n is 1) or s + s (if n is not 1) (where s is the string containing the first k letters of the alphabet starting from 'a')**