The code snippet `y2 -= a` modifies the value of `y2` by subtracting `a` from it. Given that `a` is initially set to `y1 - 1` and `y1` is 1, `a` is 0. Therefore, `y2` remains unchanged after the operation.

Here is the updated output state:

Output State: **`t` is `abs(y2 - 1)`, `h` and `w` are positive integers such that 1 <= h <= 10^6 and 1 <= w <= 10^9; `x_a`, `y_a`, `x_b`, and `y_b` are positive integers such that 1 <= x_a, x_b <= h and 1 <= y_a, y_b <= w; it is guaranteed that x_a != x_b or y_a != y_b; the sum of h over all test cases does not exceed 10^6; `r` is a list of integers read from input; `n` is `r[0]`, `m` is `r[1]`, `x1` is `r[2] + a`, `y1` is 1, `x2` is `r[4] - a`, `y2` is `r[5]`; `x2` is greater than `x1`; and (x2 - x1) is even; `y1` is not equal to `y2`. `a` is `y1 - 1` because `y2` is greater than or equal to `y1`. `b` is `x2 - x1`.**

In simpler terms, the value of `y2` remains the same as it was before the operation, and all other variables retain their initial values.