The code snippet `num = list0[i + 1] - list0[i] - 1` calculates the difference between the second element and the first element of the sorted list `list0`, and then subtracts 1 from this difference. This value is then assigned to the variable `num`.

Given the initial state:
- `t` is an integer where \(1 \leq t \leq 10^4\)
- `n` is an input integer where \(4 \leq n \leq 10^9\)
- `x` is an input integer where \(2 \leq x \leq \min(n, 2 \times 10^5)\)
- `y` is an input integer
- `_` is 2
- `T` must be greater than 0
- `list0` is a sorted list of integers derived from the input
- `i` is 0
- `count` is 0

After executing the code snippet:
- `num` is assigned the value `list0[1] - list0[0] - 1`
- All other variables remain unchanged.

Therefore, the output state is:
Output State: **`t` is an integer where \(1 \leq t \leq 10^4\), `n` is an input integer where \(4 \leq n \leq 10^9\), `x` is an input integer where \(2 \leq x \leq \min(n, 2 \times 10^5)\), `y` is an input integer, `_` is 2, `T` must be greater than 0, `list0` is a sorted list of integers derived from the input, `i` is 0, `count` is 0, `num` is `list0[1] - list0[0] - 1`.**