The code calculates `my` using the formula `my = cy - dx * math.sqrt(d2 * d - d * d) / d2`. Let's break down the variables:

- `dx` is `(x1 - x2) / 2`
- `dy` is `(y1 - y2) / 2`
- `d2` is `((x1 - x2) / 2)` (same as `dx`)
- `mx` is `cx + dy * math.sqrt(d2 * d - d * d) / d2`

The new variable `my` is calculated as:
\[ my = cy - dx \cdot \frac{\sqrt{d2 \cdot d - d \cdot d}}{d2} \]

Given that `d2 = dx`, the equation simplifies to:
\[ my = cy - dx \cdot \frac{\sqrt{dx \cdot d - d \cdot d}}{dx} \]
\[ my = cy - dx \cdot \frac{\sqrt{d(x - d)}}{dx} \]
\[ my = cy - \frac{\sqrt{d(x - d)}}{\sqrt{x - d}} \]
\[ my = cy - \sqrt{d} \]

Therefore, `my` is calculated as `cy - sqrt(d)`, where `d` is derived from the expression involving `x1`, `x2`, and `y1`, `y2`.

Output State: **`dx` is `(x1 - x2) / 2`, `dy` is `(y1 - y2) / 2`, `d2` is `((x1 - x2) / 2)`, `mx` is `cx + dy * math.sqrt(d2 * d - d * d) / d2`, `my` is `cy - sqrt(d)`**