`mx` is assigned the value `cx + dy * math.sqrt(d2 * d - d * d) / d2`. Given the initial state, we know that:

- `cx = (x1 + x2) / 2`
- `cy = (y1 + y2) / 2`
- `dx = (x1 - x2) / 2`
- `dy = (meats[j][1] - meats[i][1]) / 2`
- `d2 = \left( \frac{x1 - x2}{2} \right)^2 + \left( \frac{meats[j][1] - meats[i][1]}{2} \right)^2`

Let's break down the calculation:

1. Calculate `d2` from the given values:
   \[
   d2 = \left( \frac{x1 - x2}{2} \right)^2 + \left( \frac{meats[j][1] - meats[i][1]}{2} \right)^2
   \]

2. Calculate `d` (which is unchanged):
   \[
   d = \text{some value}
   \]

3. Substitute into the formula for `mx`:
   \[
   mx = cx + dy * \frac{\sqrt{d2 * d - d * d}}{d2}
   \]
   Simplify the term under the square root:
   \[
   d2 * d - d * d = d2 * d - d^2
   \]
   So,
   \[
   mx = cx + dy * \frac{\sqrt{d2 * d - d^2}}{d2}
   \]

Since `d2 * d - d^2 = d2 * d - d * d`, this further simplifies to:
   \[
   mx = cx + dy * \frac{\sqrt{d2 * (d - d)}}{d2} = cx + dy * \frac{\sqrt{0}}{d2} = cx + dy * 0 = cx
   \]

Therefore, `mx` ends up being equal to `cx`.

Output State: **`dx` is \((x1 - x2) / 2\), `dy` is \((meats[j][1] - meats[i][1]) / 2\), `d2` is \(\left( \frac{x1 - x2}{2} \right)^2 + \left( \frac{meats[j][1] - meats[i][1]}{2} \right)^2\), `d` retains its value, `cx` is \((x1 + x2) / 2\), `cy` is \((y1 + y2) / 2\), `count` retains its value, `j` is `i + 1`, `x2` is equal to `meats[i][0]`, `y2` is equal to `meats[i][1]`, `c2` is equal to `meats[i][2]`, `x1` is equal to `meats[j][0]`, `y1` is equal to `meats[j][1]`, `c1` is equal to `meats[j][2]`, and `mx` is equal to `cx`.