Let's break down the initial state and the print statement step by step:

1. **Initial State:**
   - `p1`, `p2`, and `p3` are integers.
   - The constraints are: \(0 \leq p1 \leq p2 \leq p3 \leq 30\).
   - `t` is greater than 0 (though it is not used in the print statement).
   - `_` is 0 (though it is not used in the print statement).
   - The sum of `p1`, `p2`, and `p3` is even.
   - `p3` is greater than or equal to the sum of `p1` and `p2`.

2. **Print Statement:**
   - The statement `print(p1 + p2)` will print the sum of `p1` and `p2`.

Given the constraints:
- `p1` and `p2` are integers such that \(0 \leq p1 \leq p2 \leq 30\).
- The sum \(p1 + p2 + p3\) is even.
- \(p3 \geq p1 + p2\).

Since `p1` and `p2` are both integers and \(p3 \geq p1 + p2\), the sum \(p1 + p2\) must be an integer. Additionally, because the sum \(p1 + p2 + p3\) is even, the sum \(p1 + p2\) must be even as well (since an even number minus an even number is even, and an odd number minus an odd number is even).

Therefore, the value of `p1 + p2` will be an even integer, and it will be less than or equal to 30 (since \(p1 \leq p2 \leq 30\)).

Output: **p1 + p2 (where p1 + p2 is an even integer and 0 ≤ p1 + p2 ≤ 30)**