Let's break down the initial state and the print statement step by step:

1. **Initial State:**
   - `p1`, `p2`, and `p3` are integers provided by the user, where \(0 \leq p1 \leq p2 \leq p3 \leq 30\).
   - `t` is greater than 1 (though `t` is not used in the print statement).
   - `_` is 2 (though `_` is not used in the print statement).
   - The sum of `p1`, `p2`, and `p3` is even.
   - `x` is 1.
   - `y` is `p3 - 1`.
   - `p3` must be greater than or equal to 2.

2. **Print Statement:**
   ```
   print(p1 - x + p3)
   ```

3. **Step-by-Step Calculation:**
   - `x` is given as 1.
   - `p1` is an integer where \(0 \leq p1 \leq p2 \leq p3 \leq 30\).
   - `p3` is an integer where \(2 \leq p3 \leq 30\).
   - The expression `p1 - x + p3` simplifies to `p1 - 1 + p3`.

4. **Final Output:**
   - The value of `p1 - 1 + p3` will be printed.
   - Since `p1` and `p3` are integers and `p3` is at least 2, the minimum value of `p1 - 1 + p3` is \(0 - 1 + 2 = 1\).
   - The maximum value of `p1 - 1 + p3` is \(30 - 1 + 30 = 59\).

Given the constraints, the output will be a specific integer value within the range from 1 to 59, depending on the values of `p1` and `p3`.

Output: **p1 - 1 + p3 (where p1 and p3 are integers such that 0 ≤ p1 ≤ p2 ≤ p3 ≤ 30, p3 ≥ 2, and the sum of p1, p2, and p3 is even)**