### Reasoning:

1. **Sum Calculation**:
   - The program calculates the sum using the formula:
     \[
     \text{sum} = 1 + \sum_{i=2}^{n} (i^2 - (i-1)^2) \times i
     \]
   - Simplifying the term inside the sum:
     \[
     i^2 - (i-1)^2 = i^2 - (i^2 - 2i + 1) = 2i - 1
     \]
   - Therefore, the sum becomes:
     \[
     \text{sum} = 1 + \sum_{i=2}^{n} (2i - 1) \times i
     \]
   - Expanding the sum:
     \[
     \text{sum} = 1 + \sum_{i=2}^{n} (2i^2 - i)
     \]
   - This can be further simplified:
     \[
     \text{sum} = 1 + 2 \sum_{i=2}^{n} i^2 - \sum_{i=2}^{n} i
     \]
   - Using the formulas for the sum of squares and the sum of integers:
     \[
     \sum_{i=1}^{n} i^2 = \frac{n(n+1)(2n+1)}{6}
     \]
     \[
     \sum_{i=1}^{n} i = \frac{n(n+1)}{2}
     \]
   - Adjusting the indices:
     \[
     \sum_{i=2}^{n} i^2 = \frac{n(n+1)(2n+1)}{6} - 1
     \]
     \[
     \sum_{i=2}^{n} i = \frac{n(n+1)}{2} - 1
     \]
   - Substituting back:
     \[
     \text{sum} = 1 + 2 \left( \frac{n(n+1)(2n+1)}{6} - 1 \right) - \left( \frac{n(n+1)}{2} - 1 \right)
     \]
     \[
     \text{sum} = 1 + \frac{2n(n+1)(2n+1)}{6} - 2 - \frac{n(n+1)}{2} + 1
     \]
     \[
     \text{sum} = \frac{2n(n+1)(2n+1)}{6} - \frac{n(n+1)}{2}
     \]
     \[
     \text{sum} = \frac{n(n+1)(2n+1)}{3} - \frac{n(n+1)}{2}
     \]
     \[
     \text{sum} = \frac{n(n+1)(4n+2 - 3)}{6}
     \]
     \[
     \text{sum} = \frac{n(n+1)(4n - 1)}{6}
     \]
   - This formula is not equivalent to the correct maximum sum \( \frac{n^2 (n + 1)}{2} \).

2. **Operations Output**:
   - The program always outputs \( 2n \) operations, which is more than necessary for \( n = 1 \).
   - For \( n = 1 \), the correct output should be:
     \[
     1 1
     1 1 1
     \]
   - The program outputs:
     \[
     1 2
     1 1 1
     2 1 1
     \]
   - This is incorrect because it outputs 2 operations instead of 1.

3. **Correct Maximum Sum**:
   - The correct maximum sum for an \( n \times n \) matrix, where each element can be a distinct integer from 1 to \( n \), is:
     \[
     \frac{n^2 (n + 1)}{2}
     \]
   - For \( n = 2 \), the correct maximum sum is:
     \[
     \frac{2^2 (2 + 1)}{2} = \frac{4 \times 3}{2} = 6
     \]
   - The program outputs 7, which is incorrect.

### Final Evaluation:
The original assessment is accurate. The program does not correctly compute the maximum sum of the matrix for all potential cases, and it does not handle the case \( n = 1 \) correctly. Therefore, the program is incorrect.

Final: **False**