To analyze the impact of the provided code on the initial state, let's break down the calculations step by step.

1. The initial state provides the following:
   - `m` is a positive integer such that \(1 \leq m \leq 10^9\).
   - `a` is a positive integer such that \(1 \leq a \leq 10^5\).
   - `b` is a positive integer such that \(1 \leq b \leq 10^5\).
   - `g` is equal to 1.
   - `k` is equal to \(a + b - 1\).
   - `m` is greater than or equal to `k`.
   - `sum_k` is equal to \(k \times (k + 1) // 2\).

2. The code snippet calculates `sum_m` using the formula:

   \[
   sum_m = m \times (m + 1) // 2 - k \times (k - 1) // 2
   \]

   To determine `sum_m`, we need to compute the following:
   - \(m \times (m + 1) // 2\): This gives the sum of the first `m` integers.
   - \(k \times (k - 1) // 2\): This gives the sum of the first `k-1` integers.

3. The value of `sum_m` will be a positive integer, derived from the specific values of `m` and `k`.

Since we have not been provided specific values for `m`, `a`, or `b`, we cannot determine exact numeric values but can express `sum_m` in terms of these variables.

Based on the calculations:
- We now have `sum_m` calculated.
- The other variables remain unchanged.

Thus, the output state would reflect the computation done for `sum_m`, while maintaining the values of all other initial variables.

Output State: **`m` is a positive integer such that \(1 \leq m \leq 10^9\); `a` is a positive integer such that \(1 \leq a \leq 10^5\); `b` is a positive integer such that \(1 \leq b \leq 10^5\); `g` is equal to 1; `k` is equal to \(a + b - 1\); `m` is greater than or equal to `k`; `sum_k` is equal to \(k \times (k + 1) // 2\); `sum_m` is equal to \(m \times (m + 1) // 2 - k \times (k - 1) // 2\).**