The code appends a tuple `(i + 1, j + 1)` to the list `ops`. Since `i` and `j` are part of the initial conditions and the operations do not affect their values, the only change is the addition of this tuple to the `ops` list. 

Given the initial conditions:
- `j` is 0
- `A` contains at least one element such that \(A[i][j] == 1\) and \(A[i + 1][j] == 1\) and \(A[i][j + 1] == 1\) and \(A[i + 1][j + 1] == 1\)
- The condition for the if part is met, i.e., \(A[i][j] == 1\) or \(A[i + 1][j] == 1\) or \(A[i][j + 1] == 1\) or \(A[i + 1][j + 1] == 1\)

After executing the code, the new value of `ops` will include the tuple `(i + 1, j + 1)`. Since `j` is 0, `j + 1` is 1.

Therefore, the updated value of `ops` will be the original `ops` list plus the tuple `(i + 1, 1)`.

Output State: **`j` is 0; `A` contains at least one element such that \(A[i][j] == 1\) and \(A[i + 1][j] == 1\) and \(A[i][j + 1] == 1\) and \(A[i + 1][j + 1] == 1\); the condition for the if part is met, i.e., \(A[i][j] == 1\) or \(A[i + 1][j] == 1\) or \(A[i][j + 1] == 1\) or \(A[i + 1][j + 1] == 1\); and `ops` now includes the tuple \((i + 1, 1)\).**