To provide the correct output state, I need specific values for the initial variables `n`, `s`, `A`, `idx_A`, `B`, `idx_B`, and their initial states. Since these values are not provided in the question, I will assume some example values to demonstrate how to calculate the output state.

Let's assume:
- `n = 5`
- `s = "><<><"`
- `A = [0, 1, 3, 6, 10]`
- `idx_A = [1, 3]`
- `B = [0, 2, 4, 6]`
- `idx_B = [0, 2]`

Now, let's go through the loop with these values:

1. `i = 0`: `s[0] = ">"`
   - `l = 0`, `r = 4`
   - `a = A[0] = 0`
   - `x = 4 - (0 + 2) = 2`
   - `b = B[3] = 6`
   - `b = 6 - B[2] = 6 - 4 = 2`
   - `b = 2 - (idx_B[2] - idx_B[3]) * (2 + 1) = 2 - 0 = 2`
   - `b = 2 + (idx_B[3] - 0) * (0 + 1) = 2 + 4 = 6`
   - Print `0 * 2 + 6 * 2 + 0 + 1 = 13`

2. `i = 1`: `s[1] = "<"`
   - `r = 3`
   - `a = B[3] + (1 - idx_A[0]) * 1 = 6 + (1 - 1) * 1 = 6`
   - `b = A[0] = 0`
   - `Print 6 * 2 + 0 * 2 + 1 + 1 = 13`

3. `i = 2`: `s[2] = "<"`
   - `r = 2`
   - `a = B[1] + (2 - idx_A[0]) * 2 = 2 + (2 - 1) * 2 = 4`
   - `b = A[0] = 0`
   - `Print 4 * 2 + 0 * 2 + 2 + 1 = 9`

4. `i = 3`: `s[3] = ">"`
   - `l = 1`, `r = 2`
   - `a = A[1] = 1`
   - `x = 2 - (1 + 2) = -1` (not valid, so skip)
   - `a = B[1] + (2 - idx_A[1]) * 2 = 2 + (2 - 3) * 2 = 0`
   - `b = A[0] = 0`
   - `Print 0 * 2 + 0 * 2 + 3 + 1 = 7`

5. `i = 4`: `s[4] = "<"`
   - `r = 1`
   - `a = B[0] + (4 - idx_A[1]) * 1 = 0 + (4 - 3) * 1 = 1`
   - `b = A[0] = 0`
   - `Print 1 * 2 + 0 * 2 + 4 + 1 = 9`

Output State: **13 13 9 7 9**

This output state represents the sequence of values printed during the loop execution based on the assumed initial values.