To determine what will be printed, let's break down the initial state and the logic of the code step by step:

1. **Initial State:**
   - `t` is an integer between 0 and 499.
   - `n` is greater than 0.
   - `i` is `n + 1`.
   - `j` is `n + 1`.
   - `r` is the largest integer `i` such that `n * (n + 1) // 2 > i * n`.
   - `sum` is the total sum of `n * (n + 1) // 2` for all `i` where the condition `n * (n + 1) // 2 > i * n` is true, plus the total sum of `i * n` for all `i` where the condition `n * (n + 1) // 2 > i * n` is false.

2. **Understanding `r`:**
   - `r` is the largest integer `i` such that `n * (n + 1) // 2 > i * n`.
   - Let's simplify the condition: `n * (n + 1) // 2 > i * n`.
   - Dividing both sides by `n` (since `n > 0`), we get: `(n + 1) // 2 > i`.
   - Therefore, `r` is the largest integer `i` such that `i < (n + 1) // 2`.

3. **Calculating `sum`:**
   - We need to sum `n * (n + 1) // 2` for all `i` where `i < (n + 1) // 2`.
   - We also need to sum `i * n` for all `i` where `i >= (n + 1) // 2`.

4. **Summing the values:**
   - For `i < (n + 1) // 2`, the sum is `sum_true = (n * (n + 1) // 2) * r`.
   - For `i >= (n + 1) // 2`, the sum is `sum_false = n * (i - r) * (i - r + 1) // 2`.
   - The total `sum` is `sum_true + sum_false`.

5. **Final Calculation:**
   - `r` is the largest integer less than `(n + 1) // 2`, so `r = (n + 1) // 2 - 1`.
   - `sum_true = (n * (n + 1) // 2) * r`.
   - `sum_false = n * (i - r) * (i - r + 1) // 2`.
   - `sum = sum_true + sum_false`.

6. **Substituting `i` and `r`:**
   - `i = n + 1`.
   - `r = (n + 1) // 2 - 1`.
   - `sum_true = (n * (n + 1) // 2) * ((n + 1) // 2 - 1)`.
   - `sum_false = n * ((n + 1) - ((n + 1) // 2 - 1)) * ((n + 1) - ((n + 1) // 2 - 1) + 1) // 2`.

7. **Simplifying `sum_false`:**
   - `sum_false = n * ((n + 1) - (n // 2)) * ((n + 1) - (n // 2) + 1) // 2`.
   - `sum_false = n * (n // 2 + 1) * (n // 2 + 2) // 2`.

8. **Combining `sum_true` and `sum_false`:**
   - `sum = (n * (n + 1) // 2) * ((n + 1) // 2 - 1) + n * (n // 2 + 1) * (n // 2 + 2) // 2`.

9. **Printing `sum` and `n + r`:**
   - `n + r = n + ((n + 1) // 2 - 1) = n + (n // 2)`.

Therefore, the final output will be:
Output: **sum, n + (n // 2) (where sum is the total sum of `n * (n + 1) // 2` for all `i` where `i < (n + 1) // 2`, plus the total sum of `i * n` for all `i` where `i >= (n + 1) // 2`, and `n + (n // 2)` is the value of `n + r`)**.