Alright, I've got this problem to solve. Let's see what it's asking for. So, I'm given two positive integers, n and m, and I need to find the number of ordered pairs (a, b) where 1 ≤ a ≤ n and 1 ≤ b ≤ m, with the condition that a + b is a multiple of b times the greatest common divisor of a and b. That is, a + b should be divisible by b * gcd(a, b).

First, I need to understand what this condition means. Let's break it down. GCD stands for Greatest Common Divisor, which is the largest positive integer that divides both a and b without leaving a remainder. So, gcd(a, b) is that number.

The condition is that a + b should be divisible by b * gcd(a, b). In other words, (a + b) mod (b * gcd(a, b)) should be 0.

Hmm, this seems a bit tricky. Maybe I can simplify this condition.

Let me think about the relationship between a and b. If I can find a relationship or a pattern that satisfies this condition, I might be able to count the number of such pairs efficiently.

Let's consider that gcd(a, b) divides both a and b. Let’s denote d = gcd(a, b). Then, a = d * a1 and b = d * b1, where a1 and b1 are coprime integers (i.e., gcd(a1, b1) = 1).

Substituting these into the condition:

a + b = d * a1 + d * b1 = d * (a1 + b1)

And b * gcd(a, b) = d * b1 * d = d^2 * b1

So, the condition becomes:

d * (a1 + b1) should be divisible by d^2 * b1

Simplifying, (a1 + b1) should be divisible by d * b1

But since a1 and b1 are coprime, and d = gcd(a, b), I need to see how these relate.

Wait, maybe there's a better way to approach this.

Let’s consider the ratio a/b. Since a = d * a1 and b = d * b1, then a/b = a1/b1, where a1 and b1 are coprime.

But I'm not sure if that helps directly.

Let me try plugging in some small values for n and m to see if I can find a pattern.

Take the first example in the problem: n=1, m=1.

So, only pair is (1,1). Let's check the condition:

a + b = 1 + 1 = 2

b * gcd(a,b) = 1 * gcd(1,1) = 1 * 1 = 1

2 is divisible by 1, so it satisfies the condition. Output is 1, which matches the example.

Second example: n=2, m=3.

Possible pairs: (1,1), (1,2), (1,3), (2,1), (2,2), (2,3)

Let's check each one:

(1,1): 1+1=2, 1*1=1, 2 is divisible by 1 → yes

(1,2): 1+2=3, 2*1=2, 3 is not divisible by 2 → no

(1,3): 1+3=4, 3*1=3, 4 is not divisible by 3 → no

(2,1): 2+1=3, 1*1=1, 3 is divisible by 1 → yes

(2,2): 2+2=4, 2*2=4, 4 is divisible by 4 → yes

(2,3): 2+3=5, 3*1=3, 5 is not divisible by 3 → no

So, valid pairs are (1,1), (2,1), (2,2) → total 3, which matches the example.

Another example: n=3, m=5

Possible pairs: (1,1), (1,2), (1,3), (1,4), (1,5), (2,1), (2,2), (2,3), (2,4), (2,5), (3,1), (3,2), (3,3), (3,4), (3,5)

Checking each:

(1,1): 1+1=2, 1*1=1, 2%1==0 → yes

(1,2): 1+2=3, 2*1=2, 3%2 !=0 → no

(1,3): 1+3=4, 3*1=3, 4%3 !=0 → no

(1,4): 1+4=5, 4*1=4, 5%4 !=0 → no

(1,5): 1+5=6, 5*1=5, 6%5 !=0 → no

(2,1): 2+1=3, 1*1=1, 3%1==0 → yes

(2,2): 2+2=4, 2*2=4, 4%4==0 → yes

(2,3): 2+3=5, 3*1=3, 5%3 !=0 → no

(2,4): 2+4=6, 4*2=8, 6%8 !=0 → no

(2,5): 2+5=7, 5*1=5, 7%5 !=0 → no

(3,1): 3+1=4, 1*1=1, 4%1==0 → yes

(3,2): 3+2=5, 2*1=2, 5%2 !=0 → no

(3,3): 3+3=6, 3*3=9, 6%9 !=0 → no

(3,4): 3+4=7, 4*1=4, 7%4 !=0 → no

(3,5): 3+5=8, 5*1=5, 8%5 !=0 → no

So, valid pairs are (1,1), (2,1), (2,2), (3,1) → total 4, which matches the example.

From these examples, it seems like pairs where b divides a+1 often satisfy the condition, but I need to generalize this.

Wait, let's look at the condition again:

a + b is divisible by b * gcd(a,b)

Given that gcd(a,b) divides both a and b, let's denote d = gcd(a,b), and a = d*a1, b = d*b1, with gcd(a1,b1)=1.

Then, a + b = d*(a1 + b1)

And b * gcd(a,b) = d * b1 * d = d^2 * b1

So, d*(a1 + b1) should be divisible by d^2 * b1

Simplify by dividing both sides by d (since d >=1):

a1 + b1 should be divisible by d * b1

But a1 and b1 are coprime, so a1 + b1 being divisible by b1 implies that a1 is divisible by b1, but since a1 and b1 are coprime, b1 must be 1.

Wait, if b1 >1, and b1 divides a1, but a1 and b1 are coprime, then b1 must be 1.

So, b1 =1.

Therefore, for the condition to hold, b1 must be 1, meaning that b = d * 1 = d, so b = d = gcd(a,b)

Therefore, b = gcd(a,b)

So, the condition simplifies to b = gcd(a,b)

But gcd(a,b) divides b, so this means that gcd(a,b) = b, which implies that b divides a.

Wait, yes, if gcd(a,b) = b, then b divides a.

So, the condition a + b divisible by b * gcd(a,b) simplifies to b divides a.

Therefore, the condition is equivalent to b divides a.

Wait, is that possible? Let me verify.

If b divides a, then a = k * b for some integer k >=1.

Then, gcd(a,b) = gcd(k*b, b) = b

So, a + b = k*b + b = (k+1)*b

And b * gcd(a,b) = b * b = b^2

So, (k+1)*b should be divisible by b^2, which means (k+1)/b should be an integer.

That is, b divides (k+1).

But a = k*b, and a <=n, b<=m.

So, k <= n/b

And b divides (k+1).

So, for each b, k can be from 1 to floor(n/b), and among these, k such that b divides (k+1), i.e., k ≡ -1 mod b.

So, k can be of the form k = b*t -1 for some integer t >=1, and k >=1.

Wait, k = b*t -1 >=1 ⇒ b*t >=2 ⇒ t >= ceil(2/b)

But b >=1, so t >=1.

But k = b*t -1 <= floor(n/b)

So, b*t -1 <= floor(n/b)

This seems a bit messy.

Wait, maybe there's a better way.

Given that the condition simplifies to b divides a, and a <=n, b<=m.

So, for each b, the number of a such that b divides a and 1 <= a <=n is floor(n/b).

So, total number of pairs should be sum over b from 1 to m of floor(n/b).

But, wait, according to the problem, it's not just sum floor(n/b) for b from 1 to m.

Because in the first test case, n=1, m=1, floor(1/1)=1, which matches the output.

In the second test case, n=2, m=3:

floor(2/1)=2

floor(2/2)=1

floor(2/3)=0

Total: 2+1+0=3, which matches the output.

In the third test case, n=3, m=5:

floor(3/1)=3

floor(3/2)=1

floor(3/3)=1

floor(3/4)=0

floor(3/5)=0

Total: 3+1+1+0+0=5, but the output is 4. Wait, that doesn't match.

Wait, in the note for the fourth test case, it lists 14 pairs for n=10, m=8.

Let's calculate sum floor(10/b) for b from 1 to 8:

floor(10/1)=10

floor(10/2)=5

floor(10/3)=3

floor(10/4)=2

floor(10/5)=2

floor(10/6)=1

floor(10/7)=1

floor(10/8)=1

Total: 10+5+3+2+2+1+1+1=25, but the note says only 14 pairs satisfy the condition.

Wait, this contradicts my earlier assumption.

So, perhaps the condition is not simply b divides a.

Wait, perhaps I made a mistake in simplifying the condition.

Let me go back.

Given that a + b is divisible by b * gcd(a,b), and we have that b = gcd(a,b).

Wait, earlier I thought that the condition simplifies to b = gcd(a,b), which implies that b divides a.

But according to the note, for n=10, m=8, there are only 14 pairs, not 25.

So, my assumption is incorrect.

I must have made a mistake in simplifying the condition.

Let me re-examine that step.

We have a + b divisible by b * gcd(a,b)

With a = d * a1, b = d * b1, where d = gcd(a,b), and a1 and b1 are coprime.

Then, a + b = d*(a1 + b1)

And b * gcd(a,b) = d * b1 * d = d^2 * b1

So, d*(a1 + b1) should be divisible by d^2 * b1

Divide both sides by d (since d >=1):

a1 + b1 should be divisible by d * b1

Now, since a1 and b1 are coprime, and b1 divides a1 + b1, then b1 divides a1.

But a1 and b1 are coprime, so b1 must be 1.

Therefore, b1 =1.

Thus, b = d * 1 = d, so b = d = gcd(a,b)

Therefore, b = gcd(a,b)

This means that b divides a, since gcd(a,b) divides a.

But in the earlier test case, sum floor(n/b) for b from 1 to m gives 25, but the correct answer is 14.

So, perhaps not all pairs where b divides a satisfy the original condition.

Wait, perhaps I need to revisit the simplification.

Given that b = gcd(a,b), and b divides a, but perhaps there are additional constraints.

Let me check the fourth test case mentioned in the note: n=10, m=8.

The valid pairs are:

(1,1),(2,1),(2,2),(3,1),(4,1),(5,1),(6,1),(6,2),(6,3),(7,1),(8,1),(9,1),(10,1),(10,2)

That's 14 pairs.

Let's see what these pairs have in common.

For b=1:

a can be from 1 to 10, since 1 divides all a.

So, pairs (1,1),(2,1),(3,1),(4,1),(5,1),(6,1),(7,1),(8,1),(9,1),(10,1) → 10 pairs

But in the list, only 10 pairs are listed, but according to the note, only 14 pairs in total.

Wait, b can be up to 8.

For b=1: 10 pairs

For b=2: pairs where 2 divides a, and a <=10: a=2,4,6,8,10 → 5 pairs

But in the note, only (2,2),(6,2),(10,2) are listed, which is 3 pairs.

Wait, but according to my calculation, there should be 5 pairs where b=2 divides a.

But in the note, only 3 pairs are considered valid.

So, perhaps not all pairs where b divides a satisfy the original condition.

Wait, perhaps I need to plug in the values for b=2.

For b=2:

a must be divisible by 2, so a=2,4,6,8,10

Now, check the original condition: a + b divisible by b * gcd(a,b)

For b=2:

- If a=2: a+b=4, b*gcd(2,2)=2*2=4, 4 divisible by 4 → yes

- If a=4: a+b=6, b*gcd(4,2)=2*2=4, 6 not divisible by 4 → no

- If a=6: a+b=8, b*gcd(6,2)=2*2=4, 8 divisible by 4 → yes

- If a=8: a+b=10, b*gcd(8,2)=2*2=4, 10 not divisible by 4 → no

- If a=10: a+b=12, b*gcd(10,2)=2*2=4, 12 divisible by 4 → yes

So, for b=2, only a=2,6,10 satisfy the condition, which matches the note's listed pairs.

Therefore, my earlier assumption that all pairs where b divides a satisfy the condition is incorrect.

There are additional constraints.

So, let's revisit the condition.

Given that b = gcd(a,b), and from above, b divides a.

But in the case of b=2, not all a divisible by 2 satisfy a + b divisible by b * gcd(a,b).

Wait, for b=2:

a + b divisible by b * gcd(a,b) = 2 * gcd(a,2)

But gcd(a,2) is either 1 or 2, depending on whether a is odd or even.

Wait, a is divisible by b=2, so a is even, so gcd(a,2)=2.

Therefore, b * gcd(a,b) = 2 * 2 = 4

So, a + b must be divisible by 4.

Therefore, for b=2, a must be even, and a + 2 must be divisible by 4, which means a must be congruent to 2 mod 4.

Wait, a + 2 ≡ 0 mod 4 ⇒ a ≡ -2 mod 4 ⇒ a ≡ 2 mod 4

So, a must be of the form 4k + 2 for some integer k >=0.

In the range 1 to 10, a=2,6,10 satisfy this.

Which matches the valid pairs in the note.

So, for b=2, a must be of the form 4k + 2.

Similarly, for general b, perhaps a must be of the form b*k + c, for some c.

Wait, let's generalize this.

Given that b divides a, so a = k*b for some integer k >=1.

Then, the condition a + b divisible by b * gcd(a,b) becomes:

a + b = k*b + b = (k+1)*b

And b * gcd(a,b) = b * gcd(k*b, b) = b * b = b^2

So, (k+1)*b divisible by b^2 ⇒ (k+1)/b is an integer.

Therefore, b divides (k+1).

So, k+1 is divisible by b.

Therefore, k ≡ -1 mod b.

So, k = b*t -1 for some integer t >=1.

Then, a = k*b = (b*t -1)*b = b^2*t - b

With a >=1 and a <=n.

So, b^2*t - b >=1 and b^2*t - b <=n

Solving for t:

b^2*t >= b +1 ⇒ t >= ceil((b +1)/b^2)

And b^2*t - b <=n ⇒ t <= floor((n + b)/b^2)

So, t ranges from ceil((b +1)/b^2) to floor((n + b)/b^2)

But since b >=1, ceil((b +1)/b^2) = ceil(1/b + 1/b^2) = ceil(some fraction less than or equal to 2) which is 1.

And floor((n + b)/b^2) is floor(n/b^2 + 1/b), which is floor(n/b^2)

Because n/b^2 + 1/b < floor(n/b^2) +1 in general.

Wait, perhaps it's better to write it directly.

Given a = b^2*t - b

We have a >=1 and a <=n

So, b^2*t - b >=1 ⇒ t >= ceil((b +1)/b^2)

And b^2*t - b <=n ⇒ t <= floor((n + b)/b^2)

But this seems complicated.

Alternatively, since k = b*t -1, and a = k*b = (b*t -1)*b = b^2*t - b

Then, a <=n ⇒ b^2*t - b <=n ⇒ b^2*t <=n + b ⇒ t <= floor((n + b)/b^2)

And a >=1 ⇒ b^2*t - b >=1 ⇒ b^2*t >= b +1 ⇒ t >= ceil((b +1)/b^2)

Given that b >=1, (b +1)/b^2 <=2 for b=1, and decreases as b increases.

So, ceil((b +1)/b^2) =1 for b >=1.

Therefore, t ranges from 1 to floor((n + b)/b^2)

So, for each b from 1 to m, the number of valid t is floor((n + b)/b^2)

Then, the total number of valid pairs is sum over b from 1 to m of floor((n + b)/b^2)

Wait, in the first test case, n=1, m=1:

floor((1 +1)/1^2)= floor(2/1)=2, but the output is 1.

Wait, that doesn't match.

So, perhaps I have miscalculated.

Wait, perhaps there's an error here.

Let me check for n=1, m=1:

b=1:

t ranges from 1 to floor((1 +1)/1^2)= floor(2/1)=2

Then, t=1 and t=2

For t=1: a =1^2*1 -1=1-1=0, which is not >=1

For t=2: a=1^2*2 -1=2-1=1, which is >=1 and <=1

So, only t=2 is valid, giving a=1

Hence, only one valid pair: (1,1)

So, in this case, although floor((n + b)/b^2)=2, only t=2 is valid because t=1 gives a=0, which is invalid.

So, perhaps we need to adjust the lower bound for t.

Similarly, for n=2, m=3:

For b=1:

t from 1 to floor((2 +1)/1^2)=3

t=1: a=1*1 -1=0 → invalid

t=2: a=2*1 -1=1 → valid

t=3: a=3*1 -1=2 → valid

So, two valid a's for b=1: a=1,2

For b=2:

t from 1 to floor((2 +2)/2^2)= floor(4/4)=1

t=1: a=2*1 -1=1 → but a=1 is less than b=2, which is invalid since a must be >=b to have b divides a.

Wait, no, a must be >=1, which it is.

But in this case, a=1, b=2: a=1 < b=2, but b divides a only if a is a multiple of b, which 1 is not a multiple of 2.

Wait, 1 is not divisible by 2.

Wait, but according to the earlier condition, t=1 gives a=1, which is less than b=2, and 2 does not divide 1.

Hence, no valid pairs for b=2 in this case.

Wait, but earlier I thought that for b=2, t=1 gives a=1, which is invalid because a < b, but in reality, a must be >=b to have b divides a.

Wait, no, a can be less than b, but in this case, b divides a only if a is a multiple of b.

But 1 is not a multiple of 2.

Hence, no valid pairs for b=2.

Wait, but according to earlier calculations, for b=2, t=1 gives a=1, which is invalid.

So, perhaps the lower bound for t should be such that a >=1.

Given a = b^2*t - b >=1 ⇒ t >= ceil((b +1)/b^2)

Which for b >=1 is t >=1, but we need to ensure that a >=1, which may require t >= ceil((b +1)/b^2)

But in the case of b=1, ceil((1+1)/1)=2, which would make t start from 1, but a=1*1 -1=0 invalid, so t starts from 2.

Wait, for b=1, ceil((1+1)/1)=2, which is correct, as t starts from 2.

For b=2, ceil((2+1)/4)= ceil(0.75)=1, but a=1 is invalid, so perhaps we need to adjust t to start from ceil((b +1)/b^2)

Wait, for b=2, ceil((2+1)/4)= ceil(0.75)=1, but a=1 is invalid.

Wait, perhaps we need to set t >= ceil((b +1)/b^2), but in this case, ceil((2+1)/4)=1, which gives a=1 invalid.

Maybe we need to set t >= ceil((b +1)/b^2) and ensure a >=1.

Alternatively, perhaps it's easier to iterate over b and find k such that k*b -1 is divisible by b, which seems odd.

This seems too complicated.

Maybe there's a better way to approach this.

Let me consider that the condition is equivalent to b divides a and b divides a + b.

Wait, if b divides a, then b divides a + b, since b divides b and b divides a.

So, b divides a + b is automatically satisfied if b divides a.

But earlier, that led to sum floor(n/b), which didn't match the sample inputs.

Wait, but according to the note, for n=10, m=8, sum floor(10/b) from b=1 to 8 is 25, but the correct answer is 14.

So, perhaps the condition is not just b divides a.

Wait, perhaps I need to look back at the original condition.

Original condition: a + b is a multiple of b * gcd(a,b)

Which is equivalent to b * gcd(a,b) divides a + b

From earlier, with a = d * a1, b = d * b1, d = gcd(a,b), and a1 and b1 are coprime.

Then, a + b = d*(a1 + b1)

And b * gcd(a,b) = d * b1 * d = d^2 * b1

So, d*(a1 + b1) divisible by d^2 * b1 ⇒ (a1 + b1) divisible by d * b1

Since a1 and b1 are coprime, and b1 divides a1 + b1, then b1 divides a1.

But a1 and b1 are coprime, so b1 must be 1.

Therefore, b1 =1, which implies b = d * 1 = d, so b = gcd(a,b)

Hence, b divides a.

But in addition, from the earlier analysis for b=2, not all a divisible by b satisfy the original condition.

Wait, for b=2, a must be such that a + b is divisible by b * gcd(a,b) = b * b = 4

So, a must be such that a +2 is divisible by 4, which is a ≡2 mod 4

Hence, a =4*k +2 for some integer k >=0

So, a=2,6,10 for k=0,1,2 respectively, within a<=10

Hence, for b=2, there are floor((n -2)/(4)) +1 = floor((10 -2)/4)+1= floor(8/4)+1=2+1=3 pairs

Wait, but (n - b)/(b^2 / b) ?

Wait, perhaps I need to generalize this.

For general b, a must satisfy a ≡ -b mod (b * gcd(a,b))

But since b = gcd(a,b), then a ≡ -b mod (b * b)

That is, a + b is divisible by b^2

So, a ≡ -b mod b^2

Therefore, a = b^2 * k - b for some integer k >=1

With a >=1 and a <=n

So, b^2 * k - b >=1 ⇒ k >= ceil((b +1)/b^2)

And a <=n ⇒ b^2 *k - b <=n ⇒ k <= floor((n + b)/b^2)

So, for each b, the number of valid k is floor((n + b)/b^2) - ceil((b +1)/b^2) +1

But for b >=1, ceil((b +1)/b^2) =1, because (b +1)/b^2 <=2 for b=1, and decreases for larger b.

Hence, the number of k is floor((n + b)/b^2) -1 +1 = floor((n + b)/b^2)

But in the first test case, b=1, floor((1 +1)/1)=2, but only one pair is valid.

So, perhaps when floor((n + b)/b^2) >0, then number of k is floor((n + b)/b^2) -1

Wait, no, in the first test case, floor((1 +1)/1)=2, but only one pair is valid.

Wait, perhaps we need to adjust the formula to floor((n + b)/b^2) -1 if b=1, else floor((n + b)/b^2)

But that doesn't seem consistent.

Wait, perhaps the correct formula is floor((n + b)/b^2) - ceil((b +1)/b^2) +1

For b=1: floor((1 +1)/1)=2, ceil((1 +1)/1)=2, so 2 -2 +1=1, which matches the first test case.

For b=2: floor((2 +2)/4)=1, ceil((2 +1)/4)=1, so 1 -1 +1=1, but in n=2, m=3, for b=2, there is only one valid pair, which matches.

Wait, but earlier for n=2, m=3, b=2 should have one valid pair, which is (2,2)

But according to sum floor((n + b)/b^2) - ceil((b +1)/b^2) +1 for b from 1 to m.

Wait, perhaps the general formula is sum over b from 1 to m of floor((n + b)/b^2) - ceil((b +1)/b^2) +1

But for b=1: floor((10 +1)/1)=11, ceil((1 +1)/1)=2, 11-2+1=10, which matches the number of pairs where b=1.

For b=2: floor((10 +2)/4)=3, ceil((2 +1)/4)=1, 3-1+1=3, which matches the valid pairs for b=2.

Similarly for b=3: floor((10 +3)/9)=1, ceil((3 +1)/9)=1, 1-1+1=1

b=4: floor((10 +4)/16)=1, ceil((4 +1)/16)=1, 1-1+1=1

b=5: floor((10 +5)/25)=1, ceil((5 +1)/25)=1, 1-1+1=1

b=6: floor((10 +6)/36)=0, ceil((6 +1)/36)=1, 0-1+1=0

b=7: floor((10 +7)/49)=0, ceil((7 +1)/49)=1, 0-1+1=0

b=8: floor((10 +8)/64)=0, ceil((8 +1)/64)=1, 0-1+1=0

Total: 10 +3 +1 +1 +1 +0 +0 +0 =16, but the note says 14 pairs.

Hmm, discrepancy.

Wait, perhaps the formula should be floor((n + b)/b^2) - floor((b +1)/b^2)

For b=1: floor(11/1)=11, floor(2/1)=1, 11-1=10

b=2: floor(12/4)=3, floor(3/4)=0, 3-0=3

b=3: floor(13/9)=1, floor(4/9)=0, 1-0=1

b=4: floor(14/16)=0, floor(5/16)=0, 0-0=0

b=5: floor(15/25)=0, floor(6/25)=0, 0-0=0

b=6: floor(16/36)=0, floor(7/36)=0, 0-0=0

b=7: floor(17/49)=0, floor(8/49)=0, 0-0=0

b=8: floor(18/64)=0, floor(9/64)=0, 0-0=0

Total: 10 +3 +1 +0 +0 +0 +0 +0=14, which matches the note.

So, the correct formula seems to be sum over b from 1 to m of floor((n + b)/b^2) - floor((b +1)/b^2)

This seems to work for the fourth test case.

Let's verify for n=3, m=5.

Sum for b=1: floor((3 +1)/1)=4, floor((1 +1)/1)=1, 4-1=3

b=2: floor((3 +2)/4)=1, floor((2 +1)/4)=0, 1-0=1

b=3: floor((3 +3)/9)=0, floor((3 +1)/9)=0, 0-0=0

b=4: floor((3 +4)/16)=0, floor((4 +1)/16)=0, 0-0=0

b=5: floor((3 +5)/25)=0, floor((5 +1)/25)=0, 0-0=0

Total: 3 +1 +0 +0 +0=4, which matches the sample output.

Great, so this seems to be the correct formula.

Hence, the number of valid pairs is sum over b from 1 to m of floor((n + b)/b^2) - floor((b +1)/b^2)

Now, to implement this efficiently, considering that n and m can be up to 2*10^6, and the sum is over b from 1 to m, which could be up to 2*10^6, we need an efficient way to compute this sum.

Let’s consider that floor((n + b)/b^2) = floor((n)/b^2) + floor((b)/b^2) - floor((n mod b^2 + b)/b^2)

But that might not help directly.

Alternatively, we can iterate over b from 1 to m, and for each b, compute floor((n + b)/b^2) and floor((b +1)/b^2), and sum their difference.

However, since n and m can be up to 2*10^6, and t can be up to 10^4, with the sum of n and m over all test cases up to 2*10^6, we need an efficient way to compute this sum for each test case.

One way to optimize this is to iterate over b in blocks, similar to the divisor summation techniques.

But perhaps there's a smarter way.

Looking back at the formula:

sum over b from 1 to m of floor((n + b)/b^2) - floor((b +1)/b^2)

We can split this into two sums:

sum over b from 1 to m of floor((n + b)/b^2) minus sum over b from 1 to m of floor((b +1)/b^2)

Now, floor((b +1)/b^2) is equal to ceil((b +1)/b^2) -1

But for b >=1, (b +1)/b^2 is less than or equal to 2 for b=1, and decreases for larger b.

So, floor((b +1)/b^2) is 2 for b=1, and 0 for b >=2.

Wait, let's check:

For b=1: (1 +1)/1=2, floor(2)=2

For b=2: (2 +1)/4=0.75, floor(0.75)=0

For b=3: (3 +1)/9=0.444, floor(0.444)=0

And so on.

Hence, sum over b from 1 to m of floor((b +1)/b^2) is 2 for b=1, and 0 for b >=2.

Therefore, the total sum is sum over b from 1 to m of floor((n + b)/b^2) minus 2.

But in the fourth test case, n=10, m=8:

sum floor((10 + b)/b^2) for b=1 to 8 is floor(11/1)=11 + floor(12/4)=3 + floor(13/9)=1 + floor(14/16)=0 + floor(15/25)=0 + floor(16/36)=0 + floor(17/49)=0 + floor(18/64)=0 =15

Then, sum floor((b +1)/b^2) for b=1 to 8 is 2 +0 +0 +0 +0 +0 +0 +0=2

So, total pairs =15 -2=13, but according to the note, it's 14.

Wait, discrepancy again.

Wait, perhaps I miscalculated floor((10 +1)/1)=11, floor((10 +2)/4)=3, floor((10 +3)/9)=1, floor((10 +4)/16)=1, floor((10 +5)/25)=0, floor((10 +6)/36)=0, floor((10 +7)/49)=0, floor((10 +8)/64)=0

So, sum is 11 +3 +1 +1 +0 +0 +0 +0=16

Then, sum floor((b +1)/b^2)=2 +0 +0 +0 +0 +0 +0 +0=2

Hence, 16 -2=14, which matches the note.

Earlier, I mistakenly thought floor((10 +4)/16)=0, but it's floor(14/16)=0, which is correct.

Hence, the formula is sum over b=1 to m of floor((n + b)/b^2) - sum over b=1 to m of floor((b +1)/b^2)

Which simplifies to sum over b=1 to m of floor((n + b)/b^2) -2

Because sum over b=1 to m of floor((b +1)/b^2) is 2 for b=1 and 0 for b >=2.

Hence, total pairs = sum over b=1 to m of floor((n + b)/b^2) -2

But in the first test case, n=1, m=1:

sum floor((1 +1)/1)=2, sum floor((1 +1)/1)=2, so 2 -2=0, but the output should be 1.

Wait, discrepancy.

Wait, perhaps I have miscounted.

Wait, for n=1, m=1:

sum floor((1 +1)/1)=2

sum floor((1 +1)/1)=2

So, 2 -2=0, but the output is 1.

This suggests that the formula is incorrect.

Wait, perhaps the formula should be sum floor((n + b)/b^2) - sum ceil((b +1)/b^2) +1

For b=1: ceil((1 +1)/1)=2, so sum ceil((b +1)/b^2)=2

Hence, total pairs = sum floor((n + b)/b^2) - sum ceil((b +1)/b^2) +1

For n=1, m=1: 2 -2 +1=1, which matches.

For n=10, m=8:

sum floor((10 + b)/b^2)=11 +3 +1 +1 +0 +0 +0 +0=16

sum ceil((b +1)/b^2)=2 +1 +1 +1 +1 +1 +1 +1=2 +7=9

Hence, 16 -9 +1=8, but according to the note, it should be 14.

Wait, not matching.

So, perhaps this is not the correct formula.

I need to think differently.

Let’s consider that for each b, the number of valid a is floor((n + b)/b^2) - floor((b +1)/b^2)

Wait, for b=1: floor((10 +1)/1)=11, floor((1 +1)/1)=2, 11 -2=9, but in reality, for b=1, there are 10 pairs: a=1 to10

Wait, but earlier we saw that for b=1, t ranges from ceil((1 +1)/1)=2 to floor((10 +1)/1)=11

Then, a =1^2*t -1= t -1, with t from 2 to11

So, a=1,2,3,4,5,6,7,8,9,10 →10 values

But according to floor((n + b)/b^2) - floor((b +1)/b^2)=11 -2=9, which is one less than actual.

So, perhaps the formula is floor((n + b)/b^2) - floor((b +1)/b^2) + c, where c is adjusted based on some condition.

This is getting too complicated.

Maybe I should look for an alternative approach.

Let’s consider iterating b from 1 to m, and for each b, compute floor((n + b)/b^2)

This is equivalent to floor(n/b^2 + b