Output State: j = 3 * n + 3, n = initial n, r = 3, sum = 3 * n * n + n * (n + 1) // 2.

After the loop executes all its iterations, `j` will be `3 * n + 3` because it increments by 1 in each iteration of the loop. The value of `n` remains unchanged as it is not modified within the loop. The value of `r` is set to 3 based on the last iteration's conditions. The value of `sum` accumulates by adding `3 * n + n * (n + 1) // 2` for each iteration, resulting in a total sum of `3 * n * n + n * (n + 1) // 2`.