The code snippet `r -= 1` decrements the value of `r` by 1. Let's analyze the impact of this code on the program:

- Initially, `r` is set to `n - 1` if `s[0]` is 'L' or `n - 2` if `s[0]` is 'R'.
- After executing `r -= 1`, the new value of `r` will be:
  - If `s[0]` is 'L': `r` was `n - 1`, so now `r` is `n - 2`.
  - If `s[0]` is 'R': `r` was `n - 2`, so now `r` is `n - 3`.

All other variables (`n`, `m`, `a`, `s`, `b`, `l`, `i`) remain unchanged.

Therefore, the Output State is:
**`n` and `m` are positive integers such that 1 ≤ `n` ≤ 2·10^5 and 1 ≤ `m` ≤ 10^4, `a` is a list of `n` integers where 1 ≤ `a_i` ≤ 10^4, `s` is a string of length `n` consisting only of the characters 'L' and 'R', `b` is a list containing the first element of `a` if `s[0]` is 'L', or the last element of `a` if `s[0]` is 'R', followed by the element `a[r]`, `l` is 1 if `s[0]` is 'L' or remains 0 if `s[0]` is 'R', `r` is `n - 2` if `s[0]` is 'L' or `n - 3` if `s[0]` is 'R', `i` is 1, and `n` must be greater than 1.**