Let's break down the initial state and the print statement step by step:

1. **Initial State:**
   - `t` is greater than 0.
   - `n` is 0.
   - `k` is an input integer.
   - `L` is a list containing the sequence of values of `(n + 1) // 2` calculated during each iteration and must have at least 1 element.
   - `m` is the last value of `(n + 1) // 2` calculated.
   - `tot` is 0.
   - `pow` is 1.
   - `a` is the first element in `L`.
   - The current value of `tot` is less than `k` and `k` is less than or equal to `tot + a`.

2. **Understanding the Variables:**
   - `L` is a list that contains at least one element, which is the result of `(n + 1) // 2` for some value of `n`.
   - `a` is the first element of `L`, so `a = (n + 1) // 2` for the initial value of `n` (which is 0).
   - `a = (0 + 1) // 2 = 1 // 2 = 0` (since integer division `//` truncates the decimal part).
   - `tot` is 0.
   - `k` is an integer such that `0 < k <= 0 + 1`, which means `k` must be 1 (since `k` is an integer and `tot + a = 0 + 1 = 1`).

3. **Evaluating the Print Statement:**
   - The print statement is `print(pow * (2 * (k - tot) - 1))`.
   - `pow` is 1.
   - `k` is 1.
   - `tot` is 0.
   - Substituting these values into the expression:
     \[
     \text{pow} * (2 * (k - \text{tot}) - 1) = 1 * (2 * (1 - 0) - 1) = 1 * (2 * 1 - 1) = 1 * (2 - 1) = 1 * 1 = 1
     \]

4. **Final Output:**
   - The print statement will output the value of the expression `1 * (2 * (1 - 0) - 1)`, which is 1.

Output: **1**