The code snippet `ans += (n - k) * a` updates the value of `ans` by adding `(n - k) * a` to its current value. Given that the initial value of `ans` is `k * b`, the new value of `ans` will be `k * b + (n - k) * a`.

Here's the updated state:
- `k` is an integer such that 0 <= k <= min(n, b)
- `a` and `b` are integers such that 1 <= a, b <= 10^9
- `n` is an integer such that 1 <= n <= 10^9
- `ans` is now `k * b + (n - k) * a`

Output State: **`k` is an integer such that 0 <= k <= min(n, b); `a` and `b` are integers such that 1 <= a, b <= 10^9; `n` is an integer such that 1 <= n <= 10^9; `ans` is `k * b + (n - k) * a`.**