The expression `dp[n, k] += 9 * 10 ** (i - 1) * (10 ** (k - i) - 10 ** (i - 1))` modifies the `dp[n, k]` value based on a calculation involving the integers `i`, `k`, and `n`. 

Initially, we have:
- `l` is an integer such that `1 ≤ l ≤ r < 10^18`
- `r` is an integer such that `1 ≤ l ≤ r < 10^18`
- `k` is an integer such that `4 ≤ k ≤ 10`
- `n` is greater than or equal to 10
- `i` is 3
- `dp[n, k]` is updated by the calculation specified.

Now, let's break down the calculation:
1. The value of `10 ** (i - 1)` is `10 ** (3 - 1)`, which equals `10 ** 2 = 100`.
2. The value of `10 ** (k - i)` needs `k` to evaluate further, but it is bounded by the constraints of `k`.
3. The overall term becomes `9 * 100 * (10 ** (k - 3) - 100)`.

The variable `dp[n, k]` is updated based on these calculations, but we do not have the initial value of `dp[n, k]`, so we can't specify the exact new value. However, we can express the change generically.

Thus, the output state reflects the changes made to `dp[n, k]` without altering the other variables. The variables `l`, `r`, `k`, and `n` remain unchanged.

Output State: **`l` is an integer such that 1 ≤ `l` ≤ `r` < 10^18; `r` is an integer such that 1 ≤ `l` ≤ `r` < 10^18; `k` is an integer such that 4 ≤ `k` ≤ 10; `n` is greater than or equal to 10; `i` is 3; `dp[n, k]` is updated by adding `9 * 100 * (10 ** (k - 3) - 100)`**.