To determine the final output state after all iterations of the loop, we need to understand the behavior of the loop and how the `res` variable changes with each iteration.

The loop iterates from `i = 0` to `i = n-1`, and in each iteration, it updates `res` by adding `(i + 1) * (2 * i + 1)` to it. We can calculate the final value of `res` by summing up the contributions from each iteration.

Let's calculate the final value of `res` for a general `n`:

- For `i = 0`, `res` becomes `res + (0 + 1) * (2 * 0 + 1) = res + 1`
- For `i = 1`, `res` becomes `res + (1 + 1) * (2 * 1 + 1) = res + 6`
- For `i = 2`, `res` becomes `res + (2 + 1) * (2 * 2 + 1) = res + 15`
- For `i = 3`, `res` becomes `res + (3 + 1) * (2 * 3 + 1) = res + 28`
- And so on...

The general term for each iteration is `(i + 1) * (2 * i + 1)`. Summing these terms from `i = 0` to `i = n-1` gives us the final value of `res`.

The formula for the sum of the series `(i + 1) * (2 * i + 1)` from `i = 0` to `i = n-1` is known to be:

\[ \text{res} = \sum_{i=0}^{n-1} (i + 1) * (2 * i + 1) = \frac{n(n+1)(2n+1)}{6} \]

Given that `res` is initialized to 0, the final value of `res` after `n` iterations is:

\[ \text{res} = \frac{n(n+1)(2n+1)}{6} \]

Since the initial state specifies that `res` is 0, `i` is 0, and `n` is an input integer, and `t` must be greater than 0, the final output state will be:

- `t` remains greater than 0
- `n` remains the input integer
- `mat` remains a list of `n` lists where each inner list contains integers from 1 to `n`
- `res` will be \(\frac{n(n+1)(2n+1)}{6}\)
- `i` will be `n-1` after the loop completes

Let's calculate the final output state using the formula for a general `n`. For the sake of clarity, let's assume `n` is a specific value, say `n = 5` (we can generalize later).

If `n = 5`:
\[ \text{res} = \frac{5(5+1)(2 \cdot 5 + 1)}{6} = \frac{5 \cdot 6 \cdot 11}{6} = 55 \]

So, if `n = 5`, the final output state would be:
- `t` must be greater than 0
- `n` is 5
- `mat` is a list of 5 lists where each inner list contains integers from 1 to 5
- `res` is 55
- `i` is 4

Generalizing for any `n`, the final output state is:

Output State: **`t` must be greater than 0, `n` is an input integer, `mat` is a list of `n` lists where each inner list contains integers from 1 to `n`, `res` is \(\frac{n(n+1)(2n+1)}{6}\), `i` is `n-1`.**

In natural language, this means that after all iterations of the loop, the value of `res` will be the sum of the series `(i + 1) * (2 * i + 1)` from `i = 0` to `i = n-1`, which is \(\frac{n(n+1)(2n+1)}{6}\), and `i` will be `n-1`. The other variables `t` and `mat` remain unchanged as per the initial conditions.