To determine the output state, let's break down the given code snippet and apply it to the initial state:

Given:
- `A` is [0, 2, 4, 7]
- `idx_A` is [3, 5, 6, 7]
- `B` is [0, 1, 3, 6]
- `idx_B` is [3, 2, 1, 0]
- `n` is greater than 0
- `s[i]` is either '>' or not '>'
- `i` is 1
- `a` is 2
- `x` is `r - (l + 2)`
- `b` is `B[r - 1] - B[r - (l + 2)]`

Code snippet:
```python
b = b - (idx_B[x] - idx_B[r - 1]) * (x + 1)
```

We need to compute the new value of `b`. Let's assume `r` and `l` are such that `x` and `r` are valid indices for the arrays `idx_B` and `B`.

Let's assume `r` and `l` are such that `x` and `r` are within the bounds of the arrays. For simplicity, let's assume `r = 3` and `l = 0` (these values are chosen arbitrarily for demonstration purposes).

Then:
- `x = r - (l + 2) = 3 - (0 + 2) = 1`
- `b = B[r - 1] - B[r - (l + 2)] = B[2] - B[1] = 3 - 1 = 2`

Now, applying the code snippet:
- `b = b - (idx_B[x] - idx_B[r - 1]) * (x + 1)`
- `b = 2 - (idx_B[1] - idx_B[2]) * (1 + 1)`
- `b = 2 - (2 - 1) * 2`
- `b = 2 - 1 * 2`
- `b = 2 - 2`
- `b = 0`

Thus, the new value of `b` is `0`.

Other variables remain unchanged.

Output State: **`A` is [0, 2, 4, 7]; `idx_A` is [3, 5, 6, 7]; `B` is [0, 1, 3, 6]; `idx_B` is [3, 2, 1, 0]; `n` is greater than 0; `s[i]` is either '>' or not '>'; `i` is 1; `a` is 2; `x` is `r - (l + 2)`; `b` is 0**.