To determine the new value of `b` after executing the given line of code, we need to substitute the known values into the expression `(idx_B[r - 1] - i) * (l + 1)`.

Given:
- `idx_B` is `[3, 2, 1, 0]`.
- `i` is `1`.
- `r` is not explicitly given, but we know it is used as an index for `idx_B`. Since `idx_B` has 4 elements, `r` can be `1`, `2`, `3`, or `4`.
- `l` is not explicitly given, but it is used in the expression `(l + 1)`.

Let's consider the possible values of `r` and `l`:

### Case Analysis:
1. **If `r = 1`:**
   - `idx_B[r - 1]` becomes `idx_B[0]`, which is `3`.
   - The expression becomes `(3 - 1) * (l + 1) = 2 * (l + 1)`.
   
2. **If `r = 2`:**
   - `idx_B[r - 1]` becomes `idx_B[1]`, which is `2`.
   - The expression becomes `(2 - 1) * (l + 1) = 1 * (l + 1) = l + 1`.

3. **If `r = 3`:**
   - `idx_B[r - 1]` becomes `idx_B[2]`, which is `1`.
   - The expression becomes `(1 - 1) * (l + 1) = 0 * (l + 1) = 0`.

4. **If `r = 4`:**
   - `idx_B[r - 1]` becomes `idx_B[3]`, which is `0`.
   - The expression becomes `(0 - 1) * (l + 1) = -1 * (l + 1) = -(l + 1)`.

Since the exact values of `r` and `l` are not specified, we express `b` in terms of these variables:

- If `r = 1`, then `b = 2 * (l + 1)`.
- If `r = 2`, then `b = l + 1`.
- If `r = 3`, then `b = 0`.
- If `r = 4`, then `b = -(l + 1)`.

Other variables remain unchanged.

Output State: **`A` is [0, 2, 4, 7]; `idx_A` is [3, 5, 6, 7]; `B` is [0, 1, 3, 6]; `idx_B` is [3, 2, 1, 0]; `n` is greater than 0; `s[i]` is either '>' or not '>'; `i` is 1; `a` is 2; `x` is `r - (l + 2)`; `b` is `(idx_B[r - 1] - i) * (l + 1)`**