To determine the new value of `b` after the given operation, we need to substitute the known values into the expression.

Given:
- `A` is [0, 2, 4, 7]
- `idx_A` is [3, 5, 6, 7]
- `B` is [0, 1, 3, 6]
- `idx_B` is [3, 2, 1, 0]
- `n` is greater than 0
- `s[i]` is either '>' or not '>'
- `i` is 1
- `a` is `B[r - 1] + (idx_B[r - 1] - 1) * r`
- `b` is `A[l - 1] - A[l - r - 1]`
- The operation to perform: `b = b - (idx_A[l - 1] - idx_A[l - r - 1]) * (l - r)`

We need to know the values of `l` and `r` to compute `b`. Since they are not provided, we'll assume hypothetical values for `l` and `r` to illustrate the calculation. Let's assume `l` is 3 and `r` is 2 for the sake of this example.

Given `l = 3` and `r = 2`:
- `b` is initially `A[3 - 1] - A[3 - 2 - 1]` which is `A[2] - A[0]` = `4 - 0` = `4`
- The operation to perform is `b = b - (idx_A[3 - 1] - idx_A[3 - 2 - 1]) * (3 - 2)`
- This simplifies to `b = 4 - (idx_A[2] - idx_A[0]) * 1`
- Substituting the values from `idx_A`: `b = 4 - (6 - 3) * 1` = `4 - 3` = `1`

Therefore, the new value of `b` is `1`.

Output State: **`A` is [0, 2, 4, 7], `idx_A` is [3, 5, 6, 7], `B` is [0, 1, 3, 6], `idx_B` is [3, 2, 1, 0], `n` is greater than 0, `s[i]` is either '>' or not '>', `i` is 1, `a` is `B[r - 1] + (idx_B[r - 1] - 1) * r`, `b` is 1**