To determine the new value of `b` after the given code executes, we need to substitute the known values into the expression `(idx_B[r - 1] - i) * (l + 1)`.

Given:
- `i` is 2.
- `idx_B` is `[3, 2, 1, 0]`.
- `r` is not explicitly defined, but it must be within the bounds of `idx_B` (0 to 3).
- `l` is not explicitly defined, but it appears in the expression.

Let's assume `r` and `l` are such that they fit within the constraints and produce a valid calculation. Since `r` is not specified, we cannot determine its exact value, but we can express `b` in terms of `r` and `l`.

The expression for `b` is:
\[ b = (idx_B[r - 1] - i) * (l + 1) \]

Substituting `i = 2`:
\[ b = (idx_B[r - 1] - 2) * (l + 1) \]

Since `idx_B` is `[3, 2, 1, 0]`, `idx_B[r - 1]` depends on the value of `r`. Let's consider the possible values of `r`:

- If `r = 1`, then `idx_B[r - 1] = idx_B[0] = 3`, so \( b = (3 - 2) * (l + 1) = 1 * (l + 1) = l + 1 \).
- If `r = 2`, then `idx_B[r - 1] = idx_B[1] = 2`, so \( b = (2 - 2) * (l + 1) = 0 * (l + 1) = 0 \).
- If `r = 3`, then `idx_B[r - 1] = idx_B[2] = 1`, so \( b = (1 - 2) * (l + 1) = -1 * (l + 1) = -(l + 1) \).
- If `r = 4`, then `idx_B[r - 1] = idx_B[3] = 0`, so \( b = (0 - 2) * (l + 1) = -2 * (l + 1) = -2(l + 1) \).

Without a specific value for `r` and `l`, we can only express `b` in terms of these variables. However, since the problem asks for the output state, we'll express `b` in terms of `r` and `l`.

Output State: **`A` is `[0, 2, 4, 7]`; `idx_A` is `[3, 5, 6, 7]`; `B` is `[0, 1, 3, 6]`; `idx_B` is `[3, 2, 1, 0]`; `n` is greater than 0; `s[i]` is either `'>'` or not `'>'`; `i` is 2; `a` is 4; `x` is `r - (l + 2)`; `b` is `(idx_B[r - 1] - 2) * (l + 1)`**.