The value of `l` is calculated as `(n + k - 1) // (k * 2 + 1)`. Given the initial conditions where `n` is an integer between 1 and 1000 inclusive, and `k` is an integer between 0 and 1000 inclusive, the value of `l` depends on the specific values of `n` and `k`.

- If `k` is 0, then `l = (n - 1) // 1 = n - 1`.
- If `k` is not 0, then `l` will be calculated based on the division of `(n + k - 1)` by `(k * 2 + 1)`.

Since we don't have specific values for `n` and `k`, we can only express `l` in terms of `n` and `k`.

Output State: **`n` is an integer where 1 ≤ n ≤ 1000; `k` is an integer where 0 ≤ k ≤ 1000; `l` is equal to `(n + k - 1) // (k * 2 + 1)`**