The code appends the value of `i * (k * 2 + 1) + 1` to the list `res`. Since the initial state does not specify a specific value for `i`, we consider `i` as an unspecified integer. The value of `k` and `n` remains unchanged, and `l` also remains unchanged because it was calculated before the code execution.

Given the initial conditions:
- `n` is an integer where \(1 \leq n \leq 1000\) and \(n > k + 2\)
- `k` is an integer where \(0 \leq k \leq 1000\)
- `l` is \(\frac{n + k - 1}{k * 2 + 1}\) and \(l > 0\)
- `res` is an empty list

After executing the line `res.append(i * (k * 2 + 1) + 1)`, the list `res` now contains one element which is `i * (k * 2 + 1) + 1`.

Output State: **`n` is an integer where \(1 \leq n \leq 1000\) and \(n > k + 2\); `k` is an integer where \(0 \leq k \leq 1000\); `l` is \(\frac{n + k - 1}{k * 2 + 1}\) and \(l > 0\); `res` is a list containing `[i * (k * 2 + 1) + 1]`**