The code appends a new value to the list `res`. The new value is calculated as `i * (k * 2 + 1) + 1`. Since `i` is equal to `l`, and `l` is defined as \(\frac{n + k - 1}{k * 2 + 1}\), the new value added to `res` will be:

\[ l * (k * 2 + 1) + 1 = \left( \frac{n + k - 1}{k * 2 + 1} \right) * (k * 2 + 1) + 1 = n + k - 1 + 1 = n + k \]

The other variables remain unchanged. Therefore, the updated states are:
- `n` remains an integer where \(1 \leq n \leq 1000\) and \(n > k + 2\)
- `k` remains an integer where \(0 \leq k \leq 1000\)
- `l` remains \(\frac{n + k - 1}{k * 2 + 1}\) and \(l > 0\)
- `res` is a list containing `[i * (k * 2 + 1) + 1, n + k]`

Output State: **`n` is an integer where \(1 \leq n \leq 1000\) and \(n > k + 2\); `k` is an integer where \(0 \leq k \leq 1000\); `l` is \(\frac{n + k - 1}{k * 2 + 1}\) and \(l > 0\); `res` is a list containing `[i * (k * 2 + 1) + 1, n + k]`**