The code snippet `r -= 1` decrements the value of `r` by 1. Given the initial state, let's analyze the impact:

- `n` and `k` remain unchanged.
- `a` remains the same list.
- `l` remains 0.
- `r` was initially `n - 1`. After executing `r -= 1`, `r` becomes `n - 2`.
- `sunks` remains 1.
- The condition `a[l]` is less than or equal to `a[r]` might no longer hold true, but we don't have enough information to determine if it does or doesn't.
- `k` remains `k - 2 * a[l]`.
- `a[r]` remains 0.

Therefore, the output state is:
Output State: **`n` and `k` are positive integers where 1 ≤ `n` ≤ 2 · 10^5 and 1 ≤ `k` ≤ 10^15, `a` is a list of `n` positive integers where 1 ≤ `a_i` ≤ 10^9, `l` is 0, `r` is `n - 2`, `sunks` is 1, `a[l]` is less than or equal to `a[r]` (if applicable), `k` is `k - 2 * a[l]`, `a[r]` is 0.**