To determine the new state after the given code executes, we need to calculate the new value of `dp[i]` using the provided formula:

`dp[i] = (dp[i - 1] + (i - 1) * dp[i - 2] * 2) % (10 ** 9 + 7)`

Given:
- `i` is 4
- `dp[1]` is 1
- `dp[2]` is 3
- `dp[3]` is calculated previously as `(dp[2] + (2) * dp[1] * 2) % (10 ** 9 + 7) = (3 + 2 * 1 * 2) % (10 ** 9 + 7) = (3 + 4) % (10 ** 9 + 7) = 7`

Now, let's calculate `dp[4]`:

`dp[4] = (dp[3] + (3) * dp[2] * 2) % (10 ** 9 + 7)`
`dp[4] = (7 + 3 * 3 * 2) % (10 ** 9 + 7)`
`dp[4] = (7 + 18) % (10 ** 9 + 7)`
`dp[4] = 25 % (10 ** 9 + 7)`
`dp[4] = 25`

The value of `dp[4]` is now 25. All other variables remain unchanged.

Output State: **`t` is at least 1, `n` is the first integer from the input, `k` is the number of iterations from the input, `m` is at least 3, `num` is the sum of 1 for each iteration where `c == r` and 2 for each iteration where `c != r`, `dp` is a list of length `m + 1` with all elements initialized to 0 except `dp[1]` which is 1, `dp[2]` which is 3, `dp[3]` which is 7, and `dp[4]` which is 25, `i` is 4**