Alright, I've got this problem to solve. Let's see what it's asking for. So, Nikita has some cubes and he wants to build a tower using these cubes. He can either add one cube on top of the tower or remove one cube from the top in each move. The question is, after a certain number of moves, can he end up with exactly m cubes in the tower?

First, I need to understand the initial state. The tower starts with no cubes, right? So, it's empty at the beginning. Now, Nikita makes n moves, and in each move, he either adds one cube or removes one cube. I need to figure out if, after these n moves, the tower can have exactly m cubes.

Let me think about this step by step. Each move is either adding one cube or removing one cube. So, if he adds a cube, the height of the tower increases by one, and if he removes a cube, the height decreases by one, provided there is at least one cube to remove.

So, if he makes n moves, some of which are adding cubes and some are removing cubes, I need to find out if the net result can be m cubes in the tower.

Let's denote the number of addition moves as a and the number of removal moves as b. Then, a + b = n, since each move is either an addition or a removal.

The net number of cubes added to the tower would be a - b, because for each addition, we add one cube, and for each removal, we subtract one cube.

But wait, initially, the tower has no cubes. So, the final number of cubes in the tower would be a - b.

According to the problem, we want a - b = m.

But we also have a + b = n.

Now, I have two equations:

1. a - b = m

2. a + b = n

I can solve these equations for a and b.

Adding both equations: 2a = m + n => a = (m + n)/2

Subtracting the first equation from the second: 2b = n - m => b = (n - m)/2

Now, since a and b represent the number of moves, they must be non-negative integers.

Therefore, a >= 0, b >= 0, and a and b must be integers.

So, for a to be non-negative: (m + n)/2 >= 0

Similarly, for b to be non-negative: (n - m)/2 >= 0

Also, (m + n) must be even, because a must be an integer.

Similarly, (n - m) must be even, because b must be an integer.

Wait a minute, actually, if (m + n) is even, then (n - m) is also even, because:

(m + n) - (n - m) = 2m, which is always even.

So, if (m + n) is even, then (n - m) is also even.

Therefore, I only need to check if (m + n) is even and n >= m.

Wait, n >= m because b = (n - m)/2 >= 0, which implies n >= m.

Also, since a = (m + n)/2, and a >= 0, then m + n >= 0, which is always true since n and m are positive integers.

So, in summary, the conditions are:

1. n >= m

2. (m + n) is even

If these two conditions are satisfied, then it's possible to have exactly m cubes in the tower after n moves.

Looking back at the example:

Test case 1: n=3, m=3

Is n >= m? 3 >= 3, yes.

Is (m + n) even? 3 + 3 = 6, which is even.

So, output "Yes".

Test case 2: n=2, m=4

Is n >= m? 2 >= 4? No.

So, output "No".

Test case 3: n=5, m=3

Is n >= m? 5 >= 3, yes.

Is (m + n) even? 5 + 3 = 8, which is even.

So, output "Yes".

Seems consistent with the sample output.

Now, let's look at the provided program:

def func():

for _ in range(int(input())):

(n, m) = map(int, input().split())

if n >= m and (n - m) % 2 == 0:

print('YES')

else:

print('NO')

Hmm, interesting.

Wait, in my earlier reasoning, I had that (m + n) should be even and n >= m.

But in the code, it's checking n >= m and (n - m) % 2 == 0.

Is that the same as (m + n) % 2 == 0?

Let me see.

We have (n - m) % 2 == 0.

But n - m is even.

And m + n is even only if both m and n are even or both are odd.

Similarly, n - m is even only if both m and n are even or both are odd.

Wait, no.

Let me recall:

If n and m are both even, then n - m is even.

If n and m are both odd, then n - m is even.

If one is even and the other is odd, then n - m is odd.

Similarly, m + n:

If both even, m + n is even.

Both odd, m + n is even.

One even and one odd, m + n is odd.

So, (n - m) % 2 == 0 is equivalent to (m + n) % 2 == 0.

Therefore, the condition in the code is equivalent to my earlier condition.

So, the code is correct.

Wait, but in my earlier reasoning, I had that (m + n) should be even and n >= m.

But in the code, it's checking n >= m and (n - m) % 2 == 0, which is equivalent to (m + n) % 2 == 0.

So, it's the same as my conditions.

Therefore, the program is correct.

I think that's all.

**Final Answer**

\[ \boxed{\text{Yes}} \]

**Correctness:**

\[ \boxed{\text{True}} \]