Let's break down the initial state and the code snippet to determine what will be printed:

### Initial State:
- `t` is an input integer where \(1 \leq t \leq 999\).
- `n` and `k` are the first and second integers provided in the input line, respectively.
- If `n` is equal to `k`, the current value of `n` is equal to the current value of `k`.
- If `n` is not equal to `k`, the condition `n + 2 > k * 2` or `n + 2 ≤ k * 2` holds true.
- `t` must be greater than 1 for the loop to execute again.

### Code Snippet:
```
print(n - k + 1, end=' ')
```

### Analysis:
1. **Case 1: `n` is equal to `k`**
   - If `n == k`, then `n - k + 1` simplifies to `0 + 1`, which is `1`.
   - Therefore, the output will be `1`.

2. **Case 2: `n` is not equal to `k`**
   - If `n != k`, we need to consider the conditions `n + 2 > k * 2` or `n + 2 ≤ k * 2`.

   - **Sub-case 2.1: `n + 2 > k * 2`**
     - This condition can be rewritten as `n > 2k - 2`.
     - The value of `n - k + 1` will be greater than `k - 1`.
     - Therefore, `n - k + 1` will be a positive integer greater than `k - 1`.

   - **Sub-case 2.2: `n + 2 ≤ k * 2`**
     - This condition can be rewritten as `n ≤ 2k - 2`.
     - The value of `n - k + 1` will be less than or equal to `k - 1`.
     - Therefore, `n - k + 1` will be a non-negative integer less than or equal to `k - 1`.

### Conclusion:
- If `n == k`, the output will be `1`.
- If `n != k`, the output will be a non-negative integer that is either greater than `k - 1` or less than or equal to `k - 1`, depending on the specific values of `n` and `k`.

### Final Output:
Output: **n - k + 1 (where n and k are the first and second integers provided in the input line, respectively, and n - k + 1 is either 1 if n == k, or a non-negative integer greater than k - 1 if n + 2 > k * 2, or a non-negative integer less than or equal to k - 1 if n + 2 ≤ k * 2)**