Correctness: **False**

Explanation: The provided program does not correctly implement the problem description. Specifically, the program incorrectly handles the calculation of the product's remainder at each step. Instead of calculating the product of the current array elements and taking the remainder at each step, the program appends elements to a list `b` based on the command ('L' or 'R') and then calculates the product of this list in reverse order.

Here is a detailed breakdown of the issues:

1. **Incorrect Product Calculation**: The program constructs a list `b` by appending elements from the original array `a` based on the commands. It then calculates the product of the elements in `b` in reverse order and takes the remainder. This approach does not reflect the actual product of the current state of the array `a` at each step.

2. **Misunderstanding of Commands**: The commands 'L' and 'R' dictate which element to remove from the array `a`, but the program does not actually modify `a` during the process. Instead, it builds a separate list `b` which is not representative of the current state of `a`.

### Example to Illustrate the Issue:

Let's consider the first test case from the problem statement:

**Input:**
```
4 6
3 1 4 2
LRRL
```

**Expected Output:**
```
0 2 4 1
```

**Explanation of Expected Output:**
- Initial array: `[3, 1, 4, 2]`
- Command 'L': Remove `3`, remaining array `[1, 4, 2]`. Product modulo 6: `(3 * 1 * 4 * 2) % 6 = 24 % 6 = 0`
- Command 'R': Remove `2`, remaining array `[1, 4]`. Product modulo 6: `(1 * 4 * 2) % 6 = 8 % 6 = 2`
- Command 'R': Remove `4`, remaining array `[1]`. Product modulo 6: `(1 * 4) % 6 = 4 % 6 = 4`
- Command 'L': Remove `1`, remaining array `[]`. Product modulo 6: `(1) % 6 = 1`

However, the provided program would not produce this output because it does not correctly calculate the product of the current array at each step.

### Correct Approach:

To fix the program, we need to calculate the product of the current array elements and take the remainder at each step without constructing a separate list `b`. Here is a corrected version of the program:

```python
for _ in range(int(input())):
    (n, m) = map(int, input().split())
    a = list(map(int, input().split()))
    s = input()
    
    product = 1
    for num in a:
        product = (product * num) % m
    
    result = []
    left = 0
    right = n - 1
    
    for command in s:
        result.append(product)
        if command == 'L':
            product = (product * pow(a[left], m - 2, m)) % m  # Modular inverse
            left += 1
        else:
            product = (product * pow(a[right], m - 2, m)) % m  # Modular inverse
            right -= 1
    
    print(*result)
```

This corrected program maintains the product of the current array elements and updates it correctly based on the commands, ensuring that the product modulo `m` is calculated accurately at each step.