The given code snippet appends `'a' * (n - cnt - 1)` to the `ans` string. This means `ans` will now include its previous value concatenated with `'a'` repeated `(n - cnt - 1)` times.

Here's the updated state of the variables:

- `t` remains an integer such that 1 <= t <= 10^5.
- `n` and `k` are integers with 1 <= n <= 26 and 1 <= k <= 26.
- `m` is an integer with 1 <= m <= 1000.
- `s` is a non-empty string.
- `i` is k-1.
- `cur` is the bitwise representation of the unique characters seen in the last incomplete set (or 0 if complete).
- `cnt` is the number of times k unique characters were seen consecutively and `cnt` is less than n.
- `tmp` remains unchanged (either an empty string or a specific character).
- `ans` is now the concatenation of its previous value and `'a' * (n - cnt - 1)`.

Output State: **`t` remains an integer such that 1 <= t <= 10^5; `n` and `k` are integers with 1 <= n <= 26 and 1 <= k <= 26; `m` is an integer with 1 <= m <= 1000; `s` is a non-empty string; `i` is k-1; `cur` is the bitwise representation of the unique characters seen in the last incomplete set (or 0 if complete); `cnt` is the number of times k unique characters were seen consecutively and `cnt` is less than n; `tmp` remains unchanged; `ans` is the concatenation of its previous value and `'a' * (n - cnt - 1)`**.