Let's break down the initial state and the calculation step by step:

1. **Initial State:**
   - `t` is set to `t - 2`. This means `t` is reduced by 2.
   - `n` is an input integer.
   - `a` is an input integer.
   - `b` is an input integer.
   - `k` is the minimum value between `b - a + 1` and `n`.
   - `ans` is calculated as `int((b + (b - k + 1)) / 2 * k)`.
   - `p2` is calculated as `(n - k) * a`.

2. **Calculating `k`:**
   - `k` is the minimum value between `b - a + 1` and `n`.
   - If `b - a + 1 <= n`, then `k = b - a + 1`.
   - Otherwise, `k = n`.

3. **Calculating `ans`:**
   - `ans` is calculated as `int((b + (b - k + 1)) / 2 * k)`.
   - Simplifying the expression inside `ans`:
     - If `k = b - a + 1`, then `ans = int((b + (b - (b - a + 1) + 1)) / 2 * (b - a + 1)) = int((b + a) / 2 * (b - a + 1))`.
     - If `k = n`, then `ans = int((b + (b - n + 1)) / 2 * n) = int((2b - n + 1) / 2 * n)`.

4. **Calculating `p2`:**
   - `p2` is calculated as `(n - k) * a`.
   - If `k = b - a + 1`, then `p2 = (n - (b - a + 1)) * a`.
   - If `k = n`, then `p2 = (n - n) * a = 0`.

5. **Final Expression:**
   - The print statement outputs `ans + p2`.
   - Combining the expressions:
     - If `k = b - a + 1`, then `ans + p2 = int((b + a) / 2 * (b - a + 1)) + (n - (b - a + 1)) * a`.
     - If `k = n`, then `ans + p2 = int((2b - n + 1) / 2 * n) + 0`.

Given the above calculations, the final output will be:

Output: **int((b + a) / 2 * (b - a + 1)) + (n - (b - a + 1)) * a** if `k = b - a + 1`, or **int((2b - n + 1) / 2 * n)** if `k = n`.