The variable `dp[i + a]` is updated by adding the value of `dp[i]` to it. Given that `i` is `m + 1`, we can substitute this into the expression. Therefore, the statement modifies `dp[m + 1 + a]` by adding `dp[m + 1]` to it. The values of `m`, `a`, and `b` remain unchanged, but `dp[m + 1 + a]` is now increased by the value of `dp[m + 1]`. 

The output thus reflects the new relationship introduced by this operation.

Output State: **`m`, `a`, and `b` are positive integers with 1 <= `m` <= 10^9, 1 <= `a` <= 10^5, and 1 <= `b` <= 10^5; `dp[m + 1 + a]` is increased by `dp[m + 1]`.**