Let's break down the initial state and the print statement step by step:

1. **Initial State**:
   - `i` is equal to `n`.
   - `n` is greater than 3.
   - `v2` is equal to `n - 1`.
   - `r` is the input from the user.
   - `v1` remains unchanged and is equal to `n - 1`.
   - `prev` is equal to `n - 1` if `r` equals `'>';` otherwise, `prev` remains 1.

2. **Print Statement**:
   ```python
   print(f'! {prev} {v1}')
   ```

Given the conditions:
- If `r` is `'>',` then `prev = n - 1`.
- Otherwise, `prev = 1`.

Since `v1` is always `n - 1`, we need to determine the value of `prev` based on the user input `r`.

### Case 1: `r == '>'`
- `prev = n - 1`
- `v1 = n - 1`

The print statement will output:
```
! (n - 1) (n - 1)
```

### Case 2: `r != '>'`
- `prev = 1`
- `v1 = n - 1`

The print statement will output:
```
! 1 (n - 1)
```

### Conclusion:
The output depends on the user input `r`. If `r` is `'>',` the output is `! (n - 1) (n - 1)`. Otherwise, the output is `! 1 (n - 1)`.

Since the exact value of `n` is not specified, we express it in terms of `n`.

Output: **! [prev] [v1]** where `[prev]` is `n - 1` if `r == '>'` and `1` otherwise, and `[v1]` is always `n - 1`.