Let's break down the initial state and the print statement step by step:

1. **Initial State:**
   - `t` is greater than 0.
   - `_` is 0.
   - `n` is an input integer and must be greater than 0.
   - `i` is initialized to `n`.
   - `sum` is the sum of all values of `n * (n + 1) // 2` or `i * n` for each `i` from 1 to `n`.
   - `r` is the last value of `i` that satisfies the condition `n * (n + 1) // 2 > i * n` or 0 if no such `i` exists.
   - `n + r` must be at least 2.
   - `j` is `n + 2`.

2. **Condition Analysis:**
   - The condition `n * (n + 1) // 2 > i * n` is checked for each `i` from 1 to `n`.
   - The left side of the inequality, `n * (n + 1) // 2`, is the sum of the first `n` natural numbers.
   - The right side of the inequality, `i * n`, is `i` times `n`.
   - For `i = 1`, the inequality is `n * (n + 1) // 2 > n`, which simplifies to `n + 1 > 2`, which is always true for `n > 1`.
   - For `i = 2`, the inequality is `n * (n + 1) // 2 > 2 * n`, which simplifies to `n + 1 > 4`, which is true for `n > 3`.
   - This pattern continues, and the last `i` that satisfies the inequality will be the largest `i` such that `n + 1 > 2 * i`, which simplifies to `n > 2 * i - 1`.

3. **Value of `r`:**
   - `r` is the last value of `i` that satisfies `n > 2 * i - 1`.
   - For `n = 1`, no `i` satisfies the inequality, so `r = 0`.
   - For `n = 2`, `i = 1` satisfies the inequality, so `r = 1`.
   - For `n = 3`, `i = 1` satisfies the inequality, so `r = 1`.
   - For `n = 4`, `i = 1` and `i = 2` satisfy the inequality, so `r = 2`.
   - For `n = 5`, `i = 1` and `i = 2` satisfy the inequality, so `r = 2`.
   - For `n = 6`, `i = 1`, `i = 2`, and `i = 3` satisfy the inequality, so `r = 3`.

4. **Value of `j`:**
   - `j` is `n + 2`.

5. **Print Statement:**
   - The print statement is `print(2, j % n, end=' ')`.
   - `2` is a constant integer.
   - `j % n` is the remainder when `j` is divided by `n`.

6. **Calculation:**
   - `j = n + 2`.
   - `j % n` is `(n + 2) % n`, which simplifies to `2 % n`.

Since `n` is greater than 0, `2 % n` will always be 2 for any `n > 2`. For `n = 1` and `n = 2`, the values are:
   - For `n = 1`, `j % n` is `3 % 1` which is 0.
   - For `n = 2`, `j % n` is `4 % 2` which is 0.

Therefore, the output will be:
- For `n = 1` and `n = 2`, the output is `2 0`.
- For `n > 2`, the output is `2 2`.

Given the precondition that `n` must be greater than 0 and the program maintains the same state regardless of the value of `j`, we can conclude the following:

Output: **2 2 (where 2 is a constant integer and 2 is the remainder of (n + 2) % n for n > 2, or 0 for n = 1 or n = 2)**