The code snippet provided increments the variable `ans` by the value of `t`. Given the initial state, the new value of `ans` will be the old value of `ans` plus `t`.

Initial State: 
- `T` is greater than or equal to 1
- `t` is `(((2 times the maximum subarray sum of `a`) % 1000000007) * 2 % 1000000007) * 2 % 1000000007`
- `tmp` is 0
- `n` is an integer read from input where 1 ≤ n ≤ 2 · 10^5
- `k` is an integer read from input where 2 ≤ k ≤ 2 · 10^5
- `a` is a list of `n` integers read from input where each integer `a_i` satisfies -10^9 ≤ `a_i` ≤ 10^9
- `MOD` is 1000000007
- `s` is the sum of all elements in the list `a`
- `ans` is `(((s + t) % MOD + MOD) % MOD + t) % MOD + t`
- `i` is 2

After executing `ans += t`, the new value of `ans` will be `(((s + t) % MOD + MOD) % MOD + t) % MOD + t + t`.

Output State: **`T` is greater than or equal to 1; `t` is `(((2 times the maximum subarray sum of `a`) % 1000000007) * 2 % 1000000007) * 2 % 1000000007`; `tmp` is 0; `n` is an integer read from input where 1 ≤ n ≤ 2 · 10^5; `k` is an integer read from input where 2 ≤ k ≤ 2 · 10^5; `a` is a list of `n` integers read from input where each integer `a_i` satisfies -10^9 ≤ `a_i` ≤ 10^9; `MOD` is 1000000007; `s` is the sum of all elements in the list `a`; `ans` is `(((s + t) % MOD + MOD) % MOD + t) % MOD + t + t`; `i` is 2**.