The code snippet provided decrements the value of `r` by 1. Let's determine the new value of `r` based on the initial conditions:

- If `s[1]` is 'L', `r` is initially `n - 1`.
- If `s[1]` is 'R', `r` is initially `n - 2`.

After executing `r -= 1`, the new value of `r` will be:
- If `s[1]` is 'L', `r` becomes `(n - 1) - 1 = n - 2`.
- If `s[1]` is 'R', `r` becomes `(n - 2) - 1 = n - 3`.

All other variables remain unchanged.

Therefore, the Output State is:
Output State: **`t` is an integer such that 1 ≤ t ≤ 10^4; for each test case, `n` is an integer such that 1 ≤ n ≤ 2·10^5, `m` is an integer such that 1 ≤ m ≤ 10^4, `a` is a list of `n` integers where each integer `a_i` satisfies 1 ≤ `a_i` ≤ 10^4, and `s` is a string of length `n` consisting only of the characters 'L' and 'R'. If `s[1]` is 'L', `b` is `[a[0], a[1], a[n-1]]`; if `s[1]` is 'R', `b` is `[a[n-1], a[n-2], a[n-2]]`; `l` is 2 if `s[1]` is 'L' and 1 if `s[1]` is 'R'; `r` is `n - 2` if `s[1]` is 'L' and `r` is `n - 3` if `s[1]` is 'R'; `i` is 2.**