The code assigns the value of `(a - 1) % m + 1` to `a_floor`. This means `a_floor` is calculated based on the value of `a` and `m`. The values of `n`, `m`, `k`, `a`, `b`, and the relationship between `a` and `b` remain unchanged.

Given the calculation for `a_floor`:
- `a_floor` is the remainder when `(a - 1)` is divided by `m`, plus 1.

Therefore, the output state is:
Output State: **`n` is an input integer, `m` is an input integer, `k` is an input integer, `a` is an input integer, `b` is an input integer and a ≠ b, 1 ≤ a ≤ n·m·k, 1 ≤ b ≤ n·m·k, `a_floor` = (a - 1) % m + 1**