The code calculates `a_block` using the formula `(a - 1) // (m * k) + 1`. The value of `a_floor` is given as `(a - 1) % m + 1`. The code does not change the value of `a_floor`, so it remains unchanged.

Given the initial state:
- `n` is an input integer
- `m` is an input integer
- `k` is an input integer
- `a` is an input integer, with \(1 \leq a \leq n \cdot m \cdot k\)
- `b` is an input integer, with \(1 \leq b \leq n \cdot m \cdot k\)
- `a_floor` = \((a - 1) \% m + 1\)

After executing the code:
- `a_block` is assigned the value \((a - 1) // (m * k) + 1\)

The output state is:
**`n` is an input integer, `m` is an input integer, `k` is an input integer, `a` is an input integer, `b` is an input integer and a â‰  b, `a_floor` = (a - 1) % m + 1, `a_block` = (a - 1) // (m * k) + 1**