After executing the code snippet, the values of `nx` and `ny` are updated based on the current values of `x`, `y`, `dx`, and `dy`. Specifically, `nx` and `ny` will take on values derived from `x` and `y` with the respective changes dictated by each pair in `dx` and `dy`.

Given that `dx` and `dy` take values from [(-1, -1), (-1, 1), (1, -1), (1, 1)], this means that for each combination, `nx` and `ny` will be calculated as follows:

- For `dx = -1, dy = -1`: `nx = x - 1`, `ny = y - 1`
- For `dx = -1, dy = 1`: `nx = x - 1`, `ny = y + 1`
- For `dx = 1, dy = -1`: `nx = x + 1`, `ny = y - 1`
- For `dx = 1, dy = 1`: `nx = x + 1`, `ny = y + 1`

Since `x` and `y` are both initialized to `1`, we can calculate `nx` and `ny` for each pair:

1. For `(-1, -1)`: `nx = 1 - 1 = 0`, `ny = 1 - 1 = 0`
2. For `(-1, 1)`: `nx = 1 - 1 = 0`, `ny = 1 + 1 = 2`
3. For `(1, -1)`: `nx = 1 + 1 = 2`, `ny = 1 - 1 = 0`
4. For `(1, 1)`: `nx = 1 + 1 = 2`, `ny = 1 + 1 = 2`

Thus, `nx` and `ny` will take on values depending on the specific `dx` and `dy` being used during iteration.

Output State: **`N` is between 3 and 10, `x` is 1, `y` is 1, `nx` varies as follows: 0 or 2, and `ny` varies as follows: 0 or 2 depending on the values taken from `dx` and `dy`.**