Reasoning:  
The function `func_1` is intended to calculate the difference between the sum of the cubes of the first `n` natural numbers and the sum of the first `n` natural numbers. The formula for the sum of the first `n` natural numbers is \( \frac{n(n + 1)}{2} \), which is correctly used in the function. However, the sum of the cubes of the first `n` natural numbers is given by \( \left(\frac{n(n + 1)}{2}\right)^2 \), which is also correctly implemented in the function as `sum_cubes_n`.

The final step is to return the difference between `sum_cubes_n` and `sum_n`. The provided assertions check the function with different values of `n` and confirm that the function returns the expected results.

Let's verify the correctness of the function with the provided test cases:
- For `n = 3`:
  - Sum of the first 3 natural numbers: \( 1 + 2 + 3 = 6 \)
  - Sum of the cubes of the first 3 natural numbers: \( 1^3 + 2^3 + 3^3 = 1 + 8 + 27 = 36 \)
  - Difference: \( 36 - 6 = 30 \)

- For `n = 5`:
  - Sum of the first 5 natural numbers: \( 1 + 2 + 3 + 4 + 5 = 15 \)
  - Sum of the cubes of the first 5 natural numbers: \( 1^3 + 2^3 + 3^3 + 4^3 + 5^3 = 1 + 8 + 27 + 64 + 125 = 225 \)
  - Difference: \( 225 - 15 = 210 \)

- For `n = 2`:
  - Sum of the first 2 natural numbers: \( 1 + 2 = 3 \)
  - Sum of the cubes of the first 2 natural numbers: \( 1^3 + 2^3 = 1 + 8 = 9 \)
  - Difference: \( 9 - 3 = 6 \)

All the test cases match the expected results, confirming that the function is correct.

Correctness: **True**