Output State: **`i` is 4, `n` must be at least 4, sum is 20**

Explanation: The code updates the `sum` variable. Given `i` is 4, the expression `(i * i - (i - 1) * (i - 1)) * i` evaluates to `(4 * 4 - 3 * 3) * 4 = (16 - 9) * 4 = 7 * 4 = 28`. Since `sum` was initially not specified, it is assumed to be 0 before this line of code is executed. After executing `sum += 28`, `sum` becomes 28. However, since the initial state mentions `n` must be at least 4, this condition remains unchanged. Thus, the final state includes `i` is 4, `n` must be at least 4, and `sum` is 28.