Postcondition: ***`i` is 1, `n` is greater than 1. If `s[i] == '>'`, and `l < r`, `a` is the element at index `l` of list `A`, `x` is `r - (l + 2)`, and `b` is `(idx_B[r - 1] - 1) * (l + 1)`. If `l >= r` and `r == 0`, no changes are made. Otherwise, `a` is set to `B[r - 1] + (idx_B[r - 1] - 1) * r`, and `b` is initially set to `A[l - 1] + (i - idx_A[l - 1]) * r`. If `l - r > 0`, `b` is updated to `A[l - 1] - A[l - r - 1] - (idx_A[l - 1] - idx_A[l - r - 1]) * (l - r) + (i - idx_A[l - 1]) * r`. Otherwise, `b` remains as `A[l - 1] + (i - idx_A[l - 1]) * r`. `l` is now `l + 1`. If `s[i] != '>'`, `r` is decreased by 1. If `l` is 0, no further changes occur. If `l` is greater than 0 and `l <= r`, `a` is set to `A[l - 1] + (1 - idx_A[l - 1]) * l`. If `r - l >= 0`, `b` is updated to `B[r] - B[r - l] - (idx_B[r - l] - 1) * (r - l) + (idx_B[r] - 1) * l`. Otherwise, `b` is updated to `B[r] + (idx_B[r] - 1) * l`. If `l` is greater than 0 and `l > r`, `a` is set to the value of `B[r]`, and `b` is updated to `b + (1 - idx_A[l - 1]) * r`. If `r` was initially 0, no further changes occur.***