To determine the output state, let's analyze the loop provided:

- We start with `i` initialized to `len(arr) - 1`, which is the last index of the list `arr`.
- The loop runs while `i` is greater than or equal to `0`.
- Inside the loop, the value of `ans[i]` is updated to be `ans[i + 1] - arr[i]`.
- After each iteration, `i` is decremented by `1`.

The initial state of `ans` is a list of `n` elements, each set to `10`. The length of `ans` is `n = len(arr) + 1`.

Let's break down the iterations:

1. **First Iteration** (`i = len(arr) - 1`):
   - `ans[i] = ans[i + 1] - arr[i]`
   - `ans[len(arr) - 1] = ans[len(arr)] - arr[len(arr) - 1]`
   - Since `ans[len(arr)]` is `10` (as it is the last element of `ans` and initially all elements are `10`), this simplifies to:
   - `ans[len(arr) - 1] = 10 - arr[len(arr) - 1]`

2. **Second Iteration** (`i = len(arr) - 2`):
   - `ans[i] = ans[i + 1] - arr[i]`
   - `ans[len(arr) - 2] = ans[len(arr) - 1] - arr[len(arr) - 2]`
   - From the first iteration, `ans[len(arr) - 1] = 10 - arr[len(arr) - 1]`, so:
   - `ans[len(arr) - 2] = (10 - arr[len(arr) - 1]) - arr[len(arr) - 2]`
   - `ans[len(arr) - 2] = 10 - arr[len(arr) - 1] - arr[len(arr) - 2]`

3. **Continuing this pattern**:
   - For each subsequent iteration, `ans[i]` is computed as:
   - `ans[i] = 10 - (arr[i + 1] + arr[i + 2] + ... + arr[len(arr) - 1])`

4. **Final Iteration** (`i = 0`):
   - `ans[0] = ans[1] - arr[0]`
   - `ans[0] = 10 - (arr[1] + arr[2] + ... + arr[len(arr) - 1]) - arr[0]`
   - `ans[0] = 10 - (arr[0] + arr[1] + ... + arr[len(arr) - 1])`

Thus, after all iterations, the `ans` list will be:
- `ans[0] = 10 - (arr[0] + arr[1] + ... + arr[len(arr) - 1])`
- `ans[1] = 10 - (arr[1] + arr[2] + ... + arr[len(arr) - 1])`
- `ans[2] = 10 - (arr[2] + ... + arr[len(arr) - 1])`
- ...
- `ans[len(arr) - 1] = 10 - arr[len(arr) - 1]`
- `ans[len(arr)] = 10` (remains unchanged)

In natural language, the output state is that the first `len(arr)` elements of `ans` are each `10` minus the sum of the corresponding suffix of `arr`, starting from the full sum of `arr` for `ans[0]` and decreasing by one element of `arr` for each subsequent element of `ans`. The last element of `ans` remains `10`.

Output State: **ans[0] = 10 - sum(arr), ans[1] = 10 - sum(arr[1:]), ..., ans[len(arr)-1] = 10 - arr[len(arr)-1], ans[len(arr)] = 10**