Let's break down the initial state and the print statement to determine what will be printed:

### Initial State:
- `n` is a positive integer such that \(1 \leq k \leq n \leq 10^4\).
- `v` is the return value of `func_2()`, but this value is not used in the print statement.
- `i` is `n - 1`.

### Print Statement:
```python
print(f'? 1 {i * n}', flush=True)
```

### Step-by-Step Analysis:
1. **Determine the value of `i`:**
   - According to the initial state, `i` is `n - 1`.
   - Therefore, `i = n - 1`.

2. **Calculate the expression `i * n`:**
   - Substitute `i` with `n - 1` in the expression `i * n`.
   - This gives us `(n - 1) * n`.

3. **Formulate the print statement:**
   - The print statement is `f'? 1 {i * n}'`.
   - Substituting `i * n` with `(n - 1) * n`, the print statement becomes `f'? 1 {(n - 1) * n}'`.

### Final Output:
The print statement will output the string `? 1` followed by the value of `(n - 1) * n`.

Output: **? 1 (n - 1) * n (where n is a positive integer such that 1 ≤ k ≤ n ≤ 10^4)**