Alright, I have this problem to solve. Let's see what it's asking for. So, Timur is in a car traveling on a number line from point 0 to point n. The car starts at minute 0. There are k+1 signs at points 0, a1, a2, ..., ak, and the car arrives at these points at minutes 0, b1, b2, ..., bk, respectively. The sequences a and b are strictly increasing, and a_k equals n.

So, between any two adjacent signs, the car travels at a constant speed. Timur has q queries, each with an integer d, and I need to find out how many minutes it takes the car to reach point d, rounded down to the nearest integer.

First, I need to understand the input and what's being asked. The input consists of multiple test cases, each with n, k, and q, followed by the a and b sequences, and then q distances d.

The constraints are:

- t ≤ 10^4 (number of test cases)

- k ≤ n ≤ 10^9

- 1 ≤ k, q ≤ 10^5

- Sum of k and q over all test cases doesn't exceed 10^5.

So, efficiency is key here because the input sizes can be large.

Let me think about how to approach this.

We have points a0 to ak with times b0 to bk. Between a0 and a1, the car travels at a constant speed, between a1 and a2 at another constant speed, and so on.

Given that, for any query d, I need to find out which segment d falls into and calculate the time based on the speed in that segment.

First, I need to find out in which segment d lies. Since a is strictly increasing, I can use binary search to find the segment.

Let me define segments as [a0, a1), [a1, a2), ..., [a_{k-1}, ak].

For each segment [a_{i-1}, ai], the speed is (ai - a_{i-1}) / (bi - b_{i-1}).

Wait, no. Actually, the car arrives at a_{i-1} at time b_{i-1} and at ai at time bi. So, the time taken to travel from a_{i-1} to ai is (bi - b_{i-1}), and the distance is (ai - a_{i-1}). Therefore, the speed in that segment is (ai - a_{i-1}) / (bi - b_{i-1}).

Wait, that doesn't make sense. If the car travels from a_{i-1} to ai in time (bi - b_{i-1}), then the speed should be (ai - a_{i-1}) / (bi - b_{i-1}).

Wait, no. Speed is distance over time, so speed = (ai - a_{i-1}) / (bi - b_{i-1}).

But, in reality, if the car travels from a_{i-1} to ai in time (bi - b_{i-1}), then the speed is (ai - a_{i-1}) / (bi - b_{i-1}).

But, in the problem, it says that between any two adjacent signs, the car travels with a constant speed. So, in each segment [a_{i-1}, ai], the speed is constant and equals (ai - a_{i-1}) / (bi - b_{i-1}).

Wait, but that would mean that the time to travel from a_{i-1} to ai is (bi - b_{i-1}), which matches the given information.

So, for a query d, I need to find which segment d lies in, calculate the time to reach d based on the speed in that segment, and add up the times from previous segments.

Let me formalize this.

Let’s say d lies in segment [a_{s-1}, as).

Then, the time to reach d is:

- Time to reach a_{s-1}: b_{s-1}

- Time to travel from a_{s-1} to d: (d - a_{s-1}) / speed in segment [a_{s-1}, as)

- speed in segment [a_{s-1}, as) is (as - a_{s-1}) / (bs - b_{s-1})

- So, time to travel from a_{s-1} to d is (d - a_{s-1}) * (bs - b_{s-1}) / (as - a_{s-1})

- Therefore, total time is b_{s-1} + (d - a_{s-1}) * (bs - b_{s-1}) / (as - a_{s-1})

Then, I need to floor this total time to get the answer.

Also, if d exactly matches some a_s, then the time is b_s.

So, I need to handle that case separately.

Let me think about implementing this.

First, for each test case, I need to read n, k, q, then the a sequence and b sequence.

Then, for each query d, I need to find s such that a_{s-1} < d <= a_s, or d == a_s.

If d == a_s, then time is b_s.

Else, time is b_{s-1} + (d - a_{s-1}) * (b_s - b_{s-1}) / (a_s - a_{s-1})

Then, floor that value.

I need to handle multiple test cases efficiently.

Given that k and q can be up to 1e5 per test case, and t up to 1e4, but sum of k and q over all test cases doesn't exceed 1e5, I need an efficient way to process this.

Let me think about the implementation.

I can precompute the speeds for each segment.

But actually, I don't need to precompute speeds; I can compute the time formula directly.

Let me think about the binary search to find the segment s for each d.

In Python, I can use bisect_left to find the insertion point for d in the a sequence.

Let me recall how bisect_left works.

bisect_left(a, d) returns the index s such that a[s-1] < d <= a[s], assuming a is sorted.

If d == a[s], it returns s.

So, if d exactly matches a[s], then s is returned.

In that case, time is b_s.

Else, s = bisect_left(a, d)

Then, s-1 is the index of a_{s-1}, and a_s is a[s]

Then, time is b_{s-1} + (d - a_{s-1}) * (b_s - b_{s-1}) / (a_s - a_{s-1})

Then, floor that value.

I need to be careful with integer division, but in Python, division is float division, so I need to make sure to floor the final result.

Also, need to handle the case when d == 0, which should return time 0.

Wait, a includes 0, and b includes 0.

Let me look at the example to verify.

First test case:

n=10, k=1, q=3

a: 10

b: 10

Queries: 0,6,7

Output: 0 6 7

So, a is [0,10], b is [0,10]

So, between 0 and 10, time is 10 minutes for 10 units, so speed is 1 unit per minute.

So, at d=0, time=0

d=6, time=6

d=7, time=7

Second test case:

n=10, k=2, q=4

a:4 10

b:4 7

Queries:6,4,2,7

Output:5 4 2 5

So, a is [0,4,10], b is [0,4,7]

So, between 0 and 4, time=4 minutes, distance=4, speed=1 unit per minute

Between 4 and 10, time=3 minutes, distance=6, speed=2 units per minute

So, for d=6:

It's between 4 and 10

Time to reach 4 is 4 minutes

Time to reach 6 from 4 is 2 units at 2 units per minute, so 1 minute

Total time=4+1=5 minutes

For d=4: time=4 minutes

For d=2: between 0 and 4, time=2 minutes

For d=7: between 4 and 10, time=4 + (7-4)/2 = 4 + 1.5 = 5.5, floor to 5

So, output is 5 4 2 5

Third test case:

n=1e9, k=1, q=1

a:1e9

b:1e9

Query:99999999

So, a is [0,1e9], b is [0,1e9]

Speed is 1 unit per minute

Time for d=99999999 is 99999999 minutes

Fourth test case:

n=6, k=1, q=3

a:6

b:5

Queries:2,6,5

So, a is [0,6], b is [0,5]

Speed is 6/5 = 1.2 units per minute

For d=2: time=2/1.2=1.666, floor to 1

For d=6: time=5

For d=5: time=5/1.2=4.166, floor to 4

Output:1 5 4

So, my formula seems correct.

Now, let's look at the given program and see if it implements this correctly.

Looking at the program:

def func():

t = int(input())

for _ in range(t):

(n, k, q) = map(int, input().split())

a = [0] + list(map(int, input().split()))

b = [0] + list(map(int, input().split()))

ad = [0]

bd = [0]

for i in range(1, len(a)):

ad.append(a[i] - a[i - 1])

for i in range(1, len(b)):

bd.append(b[i] - b[i - 1])

v = [0]

for i in range(1, len(a)):

v.append(ad[i] / bd[i])

for l in range(q):

m = 0

i = 1

ql = int(input())

s = bisect_left(a, ql)

if a[s] == ql:

print(b[s], end=' ')

continue

ql -= a[s - 1]

m += b[s - 1]

m += bd[s] * ql / ad[s]

print(int(m), end=' ')

print()

So, let's analyze this.

First, it reads t, then for each test case, reads n, k, q, then a sequence, then b sequence.

It prepends 0 to a and b.

Then, it computes ad, which is the differences between consecutive a's, starting with 0.

Similarly, bd is differences between consecutive b's, starting with 0.

Then, v is speeds, which is ad[i] / bd[i] for each segment.

Then, for each query ql:

- It uses bisect_left to find s such that a[s-1] < ql <= a[s]

- If ql == a[s], it prints b[s]

- Else, it calculates m = b[s-1] + (bd[s] * (ql - a[s-1]) / ad[s])

Wait, this seems incorrect.

According to my earlier reasoning, it should be:

time = b[s-1] + (ql - a[s-1]) * (b[s] - b[s-1]) / (a[s] - a[s-1])

But in the code, it's m += b[s-1] + bd[s] * ql / ad[s]

Wait, bd[s] is (b[s] - b[s-1]), ad[s] is (a[s] - a[s-1])

So, bd[s] * ql / ad[s] is (b[s] - b[s-1]) * ql / (a[s] - a[s-1])

But, according to my formula, it should be (d - a[s-1]) * (b[s] - b[s-1]) / (a[s] - a[s-1])

So, ql is d, so ql - a[s-1] is (d - a[s-1])

But in the code, it's ql instead of ql - a[s-1]

Wait, no, in the code, it does ql -= a[s - 1] before m += b[s - 1] + bd[s] * ql / ad[s]

Wait, ql -= a[s - 1] means ql = ql - a[s - 1]

Then, m += b[s - 1] + bd[s] * ql / ad[s]

So, m = b[s - 1] + (b[s] - b[s-1]) * (ql - a[s-1]) / (a[s] - a[s-1])

Wait, ql -= a[s - 1] means ql is now (d - a[s-1])

Then, m += b[s - 1] + bd[s] * ql / ad[s]

Which is b[s - 1] + (b[s] - b[s-1]) * (d - a[s-1]) / (a[s] - a[s-1])

Which matches my formula.

So, it seems correct.

Wait, but in the code, it's m += b[s - 1], then m += bd[s] * ql / ad[s]

Which is equivalent to m = b[s - 1] + (b[s] - b[s-1]) * (d - a[s-1]) / (a[s] - a[s-1])

Which is correct.

Then, it prints int(m), which is floor of the time.

So, it seems correct.

Let me check with the first test case.

First test case:

n=10, k=1, q=3

a:10

b:10

Queries:0,6,7

So, a = [0,10], b = [0,10]

ad = [0,10]

bd = [0,10]

v = [0,1.0]

For ql=0:

bisect_left(a,0) = 0

a[0] == 0, so print b[0] = 0

For ql=6:

bisect_left(a,6) = 1 (since 6 < a[1]=10)

So, s=1

ql -= a[s-1] = 0, so ql = 6

m = b[0] + bd[1] * ql / ad[1] = 0 + 10 * 6 / 10 = 6

print(6)

For ql=7:

similarly, s=1

ql -= 0 -> ql=7

m = 0 + 10*7/10 = 7

print(7)

Which matches the first test case.

Second test case:

n=10, k=2, q=4

a:4 10

b:4 7

Queries:6,4,2,7

a = [0,4,10]

b = [0,4,7]

ad = [0,4,6]

bd = [0,4,3]

v = [0,1.0,0.5]

For ql=6:

bisect_left(a,6) = 1 (since a[1]=4 < 6 < a[2]=10)

s=1

ql -= a[1-1]=0, so ql=6

m = b[0] + bd[1] * ql / ad[1] = 0 + 4*6/4 = 6

Wait, but according to the example, it should be 5.

Wait, perhaps I'm making a mistake.

Wait, in the second test case, a=[0,4,10], b=[0,4,7]

So, ad=[0,4,6], bd=[0,4,3], v=[0,1.0,0.5]

For ql=6:

s=1 (since a[1]=4 < 6 < a[2]=10)

ql -= a[0]=0, ql=6

m = b[0] + bd[1] * ql / ad[1] = 0 + 4*6/4 = 6

But according to the example, it should be 5.

Wait, perhaps I need to adjust the indices.

Wait, in the code, a includes 0, so a=[0,4,10], b=[0,4,7]

s = bisect_left(a,ql), which for ql=6 is 1, since a[1]=4 < 6 < a[2]=10

Then, ql -= a[s-1] = 0, ql=6

m = b[s-1] + bd[s] * ql / ad[s] = b[0] + bd[1] * 6 / ad[1] = 0 + 4*6/4 = 6

But according to the example, it should be 5.

Wait, perhaps I need to recast the formula.

Wait, in the second segment, from a=4 to a=10, time from b=4 to b=7, which is 3 minutes for 6 units, so speed is 2 units per minute.

So, time to reach d=6 is time to reach a=4 (which is b=4), plus time to reach from 4 to 6, which is (6-4)/2 = 1 minute, total 5 minutes.

But according to the code, it's calculating m = 0 + 4*6/4 = 6, which is incorrect.

Wait, there's a mistake in the code.

In the second test case, according to the code, for ql=6:

m = b[0] + bd[1] * ql / ad[1] = 0 + 4*6/4 = 6

But according to the correct calculation, it should be 5.

So, the code is wrong.

Wait, perhaps I misread the code.

Wait, in the code, it's m += b[s - 1], then m += bd[s] * ql / ad[s]

But in this case, s=1, bd[s]=bd[1]=4, ad[s]=ad[1]=4, ql=6

So, m = 0 + 4*6/4 = 6

But according to the correct formula, it should be b[s-1] + (ql - a[s-1]) * (b[s] - b[s-1]) / (a[s] - a[s-1]) = 4 + (6-4)*(7-4)/(10-4) = 4 + 2*3/6 = 4 + 1 = 5

So, the code is using m = b[s-1] + bd[s] * ql / ad[s], but it should be m = b[s-1] + bd[s] * (ql - a[s-1]) / ad[s]

Wait, but in the code, ql -= a[s - 1], so ql is now ql - a[s-1]

Then, m += b[s - 1] + bd[s] * ql / ad[s]

Which is m = b[s - 1] + bd[s] * (ql - a[s-1]) / ad[s]

Wait, but in the example above, for ql=6, s=1, a[s-1]=0, so ql -= 0, ql remains 6

Then, m = 0 + 4*6/4 = 6, which is incorrect, as per the example.

Wait, but according to my calculation, it should be m = 4 + (6-4)*3/6 = 4 + 1 = 5

So, the code is incorrect.

It seems that the code is not correctly calculating the time.

It's using m = b[s - 1] + bd[s] * (ql - a[s - 1]) / ad[s]

But according to the correct formula, it should be m = b[s - 1] + (ql - a[s - 1]) * (b[s] - b[s - 1]) / (a[s] - a[s - 1])

Wait, but bd[s] = b[s] - b[s - 1], and ad[s] = a[s] - a[s - 1]

So, bd[s] * (ql - a[s - 1]) / ad[s] = (b[s] - b[s - 1]) * (ql - a[s - 1]) / (a[s] - a[s - 1])

Which matches the correct formula.

Wait, but in the example, it's giving m = 0 + 4*6/4 = 6, but according to the correct calculation, it should be m = 0 + 3*6/6 = 3, but that's not matching either.

Wait, I'm getting confused.

Wait, let's recalculate.

Given a=[0,4,10], b=[0,4,7]

For d=6:

s=1 (since a[1]=4 < 6 < a[2]=10)

ql -= a[s-1] = 0, so ql=6

m = b[s-1] + bd[s] * ql / ad[s] = 0 + 4*6/4 = 6

But according to the correct formula:

time = b[s-1] + (ql - a[s-1]) * (b[s] - b[s-1]) / (a[s] - a[s-1]) = 4 + (6 - 4)*(7 - 4)/(10 - 4) = 4 + 2*3/6 = 4 + 1 = 5

But in the code, it's m = b[s - 1] + bd[s] * ql / ad[s] = 0 + 4*6/4 = 6

Wait, it seems that the code is incorrect.

It should be m = b[s - 1] + (ql - a[s - 1]) * bd[s] / ad[s]

But in the code, it's m += b[s - 1], then m += bd[s] * ql / ad[s]

Which is equivalent to m = b[s - 1] + bd[s] * ql / ad[s]

But according to the correct formula, it should be m = b[s - 1] + bd[s] * (ql - a[s - 1]) / ad[s]

So, the code is missing the subtraction of a[s - 1] in ql.

Wait, but in the code, it does ql -= a[s - 1] before calculating m.

Wait, ql -= a[s - 1] means ql = ql - a[s - 1]

Then, m += b[s - 1] + bd[s] * ql / ad[s]

Which is m = b[s - 1] + bd[s] * (ql - a[s - 1]) / ad[s]

Wait, no, ql -= a[s - 1] is done before m += b[s - 1] + bd[s] * ql / ad[s]

So, ql is now ql - a[s - 1]

So, m = b[s - 1] + bd[s] * (ql - a[s - 1]) / ad[s]

Which matches the correct formula.

Wait, but in the example, a[s - 1] = 0, ql = 6, bd[s] = 3, ad[s] = 6

Wait, no, in the second test case:

a = [0,4,10]

b = [0,4,7]

ad = [0,4,6]

bd = [0,4,3]

v = [0,1.0,0.5]

For ql=6:

s = bisect_left(a,6) = 1 (since a[1]=4 < 6 < a[2]=10)

ql -= a[s - 1] = 0, so ql=6

m = b[s - 1] + bd[s] * ql / ad[s] = 0 + 3*6/6 = 3

But according to the example, it should be 5.

Wait, this is confusing.

Wait, perhaps I need to re-examine the correct formula.

The correct formula should be:

time = b[s - 1] + (ql - a[s - 1]) * (b[s] - b[s - 1]) / (a[s] - a[s - 1])

Which is b[s - 1] + (ql - a[s - 1]) * bd[s] / ad[s]

But in the code, it's m += b[s - 1], then m += bd[s] * ql / ad[s]

Which is m = b[s - 1] + bd[s] * ql / ad[s]

But according to the correct formula, it should be m = b[s - 1] + bd[s] * (ql - a[s - 1]) / ad[s]

So, the code is missing the subtraction of a[s - 1] in ql.

Wait, but in the code, it does ql -= a[s - 1] before calculating m.

Wait, ql -= a[s - 1] means ql = ql - a[s - 1]

Then, m += b[s - 1] + bd[s] * ql / ad[s]

Which is m = b[s - 1] + bd[s] * (ql - a[s - 1]) / ad[s]

Wait, no, ql has already been reduced by a[s - 1], so it's ql = ql - a[s - 1]

So, m = b[s - 1] + bd[s] * (ql - a[s - 1]) / ad[s]

Wait, but ql has already been reduced by a[s - 1], so it should be m = b[s - 1] + bd[s] * ql / ad[s], where ql is already ql - a[s - 1]

Wait, perhaps I need to look at the variable names.

Let me re-express it.

After ql -= a[s - 1], ql is now (d - a[s - 1])

Then, m = b[s - 1] + bd[s] * ql / ad[s]

Which is b[s - 1] + (b[s] - b[s - 1]) * (d - a[s - 1]) / (a[s] - a[s - 1])

Which is correct.

Wait, but in the second test case, for d=6:

s=1, a[s - 1]=0, ql -= 0, so ql=6

m = 0 + 3*6/6 = 3

But according to the correct calculation, it should be 5.

Wait, bd[s] = bd[1] = 4, not 3.

Wait, b = [0,4,7], so bd = [0,4,3]

So, bd[1] = 4, ad[1] = 4

So, m = 0 + 4*6/4 = 6

But according to the correct formula, it should be m = 4 + (6 - 4)*3/6 = 4 + 1 = 5

Wait, in the code, m = b[s - 1] + bd[s] * ql / ad[s] = 0 + 4*6/4 = 6

But according to the correct formula, it's m = b[s - 1] + (ql - a[s - 1]) * bd[s] / ad[s]

But ql has already been reduced by a[s - 1], so m = b[s - 1] + bd[s] * (ql - a[s - 1]) / ad[s]

Wait, but in the code, ql -= a[s - 1] is done before calculating m.

Wait, perhaps there's a mistake in indexing.

Wait, a = [0,4,10], b = [0,4,7]

s = bisect_left(a,6) = 1

So, s=1, a[s - 1]=0, a[s]=4

Wait, but a[s]=4 < 6, so s=2

Wait, a[1]=4 < 6 < a[2]=10, so s=2

Then, ql -= a[s - 1] = 4, so ql=6-4=2

m = b[s - 1] + bd[s] * ql / ad[s] = 4 + 3*2/6 = 4 + 1 = 5

Which matches the example.

So, in the code, s = bisect_left(a, ql)

If a[s] == ql, print b[s]

Else, ql -= a[s - 1], m = b[s - 1] + bd[s] * ql / ad[s], print floor(m)

In the second test case, for ql=6, s=2, ql -= a[1]=4, ql=2

m = b[1] + bd[2] * 2 / ad[2] = 4 + 3*2/6 = 4 + 1 = 5

Which matches the example.

So, the code is correct.

I must have misread the indices earlier.

Therefore, the given program is correct.

**Final Answer**

\[ \boxed{\text{Correctness: } \text{True}} \]