Based on the initial state provided:

- `i` is `n`, and `n` must be greater than 1.
- `a` is a list where each element `a[i]` (for `i` from 0 to `n-1`) is calculated as `a[0] + sum(x[0] to x[i-1])`.

This means that after the loop has run, the list `a` will contain the cumulative sums of the elements of `x` up to each index. Specifically:

- `a[0]` will be `x[0]` because `a[0] = a[0] + sum(x[0]) = x[0]`.
- `a[1]` will be `x[0] + x[1]` because `a[1] = a[0] + sum(x[0] to x[1]) = x[0] + x[1]`.
- `a[2]` will be `x[0] + x[1] + x[2]` because `a[2] = a[0] + sum(x[0] to x[2]) = x[0] + x[1] + x[2]`.
- And so on until `a[n-1]` which will be the sum of all elements in `x` because `a[n-1] = a[0] + sum(x[0] to x[n-1]) = x[0] + x[1] + ... + x[n-1]`.

Therefore, the list `a` will contain the cumulative sums of the elements of `x` up to each index.

Output: **x[0], x[0] + x[1], x[0] + x[1] + x[2], ..., x[0] + x[1] + ... + x[n-1]**