Alright, I've got this problem to solve. Let's see what it's asking for. So, I'm given two positive integers, n and m, and I need to find the number of ordered pairs (a, b) where 1 ≤ a ≤ n and 1 ≤ b ≤ m, such that a + b is a multiple of b multiplied by the greatest common divisor of a and b. That is, a + b should be divisible by b * gcd(a, b).

First, I need to understand what this condition means. Let's break it down.

We have a + b ≡ 0 mod (b * gcd(a, b)), which means that b * gcd(a, b) divides a + b without leaving a remainder.

Let me denote gcd(a, b) as d. So, d divides both a and b. That means a = d * a' and b = d * b', where gcd(a', b') = 1.

Substituting these into the condition:

a + b = d * a' + d * b' = d(a' + b')

And b * gcd(a, b) = d * b' * d = d^2 * b'

So, the condition becomes d(a' + b') is divisible by d^2 * b'.

Simplifying, this means that a' + b' is divisible by d * b'.

But since a' and b' are coprime (gcd(a', b') = 1), and b' divides a' + b', it must be that b' divides a'. But since a' and b' are coprime, the only way b' divides a' is if b' = 1.

So, b' = 1.

That implies that b = d * b' = d * 1 = d.

So, b = d, which is gcd(a, b).

So, the condition simplifies to b = gcd(a, b).

Wait, that's interesting.

So, the condition a + b is a multiple of b * gcd(a, b) reduces to b = gcd(a, b).

So, now the problem is to count the number of pairs (a, b) where 1 ≤ a ≤ n, 1 ≤ b ≤ m, and b = gcd(a, b).

This seems simpler.

Now, since b = gcd(a, b), that means that b divides a, and b divides b (which is obvious), and b is the greatest such divisor.

But since b divides a, we can write a = k * b for some integer k ≥ 1.

Also, since b = gcd(a, b), and a = k * b, it follows that gcd(k * b, b) = b.

But gcd(k * b, b) = b * gcd(k, 1) = b, which holds as long as k and 1 are coprime, which they always are since 1 is coprime to everything.

So, the condition holds as long as b divides a.

Therefore, the problem reduces to counting the number of pairs (a, b) where 1 ≤ a ≤ n, 1 ≤ b ≤ m, and b divides a.

This is a standard problem in number theory.

So, for each b from 1 to m, we need to count how many a in 1 to n are divisible by b.

The number of such a is floor(n / b).

So, the total number of pairs is the sum over b from 1 to m of floor(n / b).

But wait, in the code provided, it's doing something different.

Let me look at the code.

The code reads T, the number of test cases, and then for each test case, it reads a and b (which correspond to n and m in the problem statement), and then it initializes suma to 0.

Then it loops over i from 1 to b (inclusive), and for each i, it computes x = (a - i * (i - 1)) // (i ** 2) + 1.

If x > 0, it adds x to suma.

Additionally, if (a - i * (i - 1)) // (i ** 2) + 1 > 0 and (a - i * (i - 1)) % (i ** 2) == 0 and i * (i - 1) % (i ** 2) == 0, it adds 1 to suma.

Finally, it prints suma - 2.

This seems quite different from what I expected.

Based on my earlier reasoning, I thought the answer should be the sum over b from 1 to m of floor(n / b).

But here, it's iterating over i from 1 to b, and computing some expression involving a and i.

I need to understand what this code is doing.

Let me try to see if this code is equivalent to summing floor(n / b) for b from 1 to m.

First, in the standard approach, for each b from 1 to m, we add floor(n / b) to the sum.

In the code, it's iterating over i from 1 to b, and for each i, computing x = (a - i * (i - 1)) // (i ** 2) + 1.

If x > 0, it adds x to suma.

Additionally, there's a condition to add 1 more if (a - i * (i - 1)) % (i ** 2) == 0 and (i * (i - 1)) % (i ** 2) == 0.

Finally, it prints suma - 2.

This doesn't look like the standard approach.

Maybe the code is implementing some optimized or transformed version of the standard approach.

Alternatively, perhaps there's a mistake in the code.

Let me try to test the code with the sample input provided in the problem.

Sample Input:

6

1 1

2 3

3 5

10 8

100 1233

1000000 1145141

Sample Output:

1

3

4

14

153

1643498

Let me take the first test case: n=1, m=1.

According to the standard approach, sum floor(1 / b) for b from 1 to 1, which is floor(1 / 1) = 1.

So, the output should be 1, which matches the sample output.

Now, let's see what the code does for n=1, m=1.

It loops over i from 1 to 1.

For i=1:

x = (1 - 1*(1-1)) // (1**2) + 1 = (1 - 0) // 1 + 1 = 1 // 1 + 1 = 1 + 1 = 2

Since x > 0, add 2 to suma.

Additionally, check if (1 - 0) % 1 == 0 and (0) % 1 == 0, which is true, so add 1 more to suma.

So, suma = 2 + 1 = 3.

Then, print suma - 2 = 3 - 2 = 1.

Okay, that matches the sample output.

Now, let's check another test case.

Take n=2, m=3.

Standard approach: sum floor(2 / b) for b from 1 to 3.

b=1: floor(2 / 1) = 2

b=2: floor(2 / 2) = 1

b=3: floor(2 / 3) = 0

Total: 2 + 1 + 0 = 3.

Sample output is 3.

Now, see what the code does.

Loop over i from 1 to 3.

i=1:

x = (2 - 1*0) // 1 + 1 = (2 - 0) // 1 + 1 = 2 // 1 + 1 = 2 + 1 = 3

x > 0, so add 3 to suma.

Check if (2 - 0) % 1 == 0 and (0) % 1 == 0, which is true, so add 1 more to suma.

So, suma = 3 + 1 = 4.

i=2:

x = (2 - 2*1) // 4 + 1 = (2 - 2) // 4 + 1 = 0 // 4 + 1 = 0 + 1 = 1

x > 0, add 1 to suma.

Check if (2 - 2) % 4 == 0 and (2*1) % 4 == 0, which is 0 % 4 == 0 and 2 % 4 == 0.

0 % 4 == 0 is true, but 2 % 4 == 0 is false, so don't add extra 1.

So, suma = 4 + 1 = 5.

i=3:

x = (2 - 3*2) // 9 + 1 = (2 - 6) // 9 + 1 = (-4) // 9 + 1 = -1 + 1 = 0

x is not > 0, so don't add anything.

So, suma = 5.

Then, print suma - 2 = 5 - 2 = 3.

Which matches the sample output.

Okay, so for n=2, m=3, it gives the correct answer.

Let's try n=3, m=5.

Standard approach: sum floor(3 / b) for b=1 to 5.

b=1: 3

b=2: 1

b=3: 1

b=4: 0

b=5: 0

Total: 3 + 1 + 1 + 0 + 0 = 5.

But sample output is 4.

Wait, contradiction.

Wait, sample output for n=3, m=5 is 4.

But according to my calculation, it should be 5.

Wait, perhaps I miscounted.

Wait, b=1: floor(3/1)=3

b=2: floor(3/2)=1

b=3: floor(3/3)=1

b=4: floor(3/4)=0

b=5: floor(3/5)=0

Total: 3 + 1 + 1 + 0 + 0 = 5.

But sample output is 4.

Hmm, maybe I'm missing something.

Wait, in the note for the fourth test case, it lists 14 pairs for n=10, m=8.

But according to the standard approach, sum floor(10 / b) for b=1 to 8:

b=1: 10

b=2: 5

b=3: 3

b=4: 2

b=5: 2

b=6: 1

b=7: 1

b=8: 1

Total: 10 + 5 + 3 + 2 + 2 + 1 + 1 + 1 = 25.

But the sample output for n=10, m=8 is 14.

So, there's a discrepancy.

This suggests that my initial simplification is incorrect.

Perhaps the condition b = gcd(a, b) is not equivalent to b divides a.

Wait, but gcd(a, b) divides b, and if b = gcd(a, b), then b divides a.

Wait, but maybe there are additional constraints.

Let me revisit the condition.

We have a + b is a multiple of b * gcd(a, b).

Let me set d = gcd(a, b).

Then a = d * a', b = d * b', with gcd(a', b') = 1.

Then a + b = d(a' + b').

b * gcd(a, b) = d * b' * d = d^2 * b'.

So, d(a' + b') must be divisible by d^2 * b'.

Thus, a' + b' must be divisible by d * b'.

But b' = 1, because b = d.

Wait, b = d, so b' = 1.

So, a' + 1 must be divisible by d * 1 = d.

But a' and b' are coprime, and b' = 1.

Wait, a' and 1 are always coprime.

So, a' + 1 must be divisible by d.

But a' = a / d, and d = b.

So, a' = a / b.

So, a / b + 1 must be divisible by b.

Wait, that doesn't make sense.

Wait, a / b + 1 is (a + b)/b.

And we need (a + b)/b to be divisible by b.

Wait, no.

Wait, a + b must be divisible by b * gcd(a, b) = b * b, since gcd(a, b) = b.

So, a + b must be divisible by b^2.

So, a + b ≡ 0 mod b^2.

Thus, a ≡ -b mod b^2.

But since b divides a, a = k * b for some integer k.

So, k * b + b = b(k + 1) ≡ 0 mod b^2.

Thus, b(k + 1) is divisible by b^2.

So, k + 1 is divisible by b.

Thus, k ≡ -1 mod b.

So, k = m * b - 1 for some integer m ≥ 1.

Thus, a = k * b = (m * b - 1) * b = m * b^2 - b.

So, a = m * b^2 - b.

Now, since a must be ≥ 1, m * b^2 - b ≥ 1 ⇒ m ≥ (b + 1)/b^2.

And a ≤ n ⇒ m * b^2 - b ≤ n ⇒ m ≤ (n + b)/b^2.

So, m can be from ceil((b + 1)/b^2) to floor((n + b)/b^2).

But m must be an integer ≥ 1.

So, for each b from 1 to m, the number of valid m is floor((n + b)/b^2) - ceil((b + 1)/b^2) + 1.

But this seems complicated.

Alternatively, since a = m * b^2 - b, and a ≥ 1 and a ≤ n, then m can be from ceil((b + 1)/b^2) to floor((n + b)/b^2).

But this might not be the easiest way to compute it.

Let me see if there's a better way.

Alternatively, from a = m * b^2 - b, we can write a + b = m * b^2.

So, a + b must be a multiple of b^2.

Thus, a + b is a multiple of b^2, and since a = k * b, then k * b + b = b(k + 1) is a multiple of b^2.

Thus, k + 1 is a multiple of b.

So, k ≡ -1 mod b.

So, k = t * b - 1 for some integer t ≥ 1.

Thus, a = (t * b - 1) * b = t * b^2 - b.

Now, 1 ≤ a ≤ n ⇒ 1 ≤ t * b^2 - b ≤ n.

So, t * b^2 - b ≥ 1 ⇒ t * b^2 ≥ b + 1 ⇒ t ≥ (b + 1)/b^2.

And t * b^2 - b ≤ n ⇒ t * b^2 ≤ n + b ⇒ t ≤ (n + b)/b^2.

So, t can be from ceil((b + 1)/b^2) to floor((n + b)/b^2).

Now, for each b from 1 to m, we need to count the number of integer t in this range.

Let's define x_b = floor((n + b)/b^2) - ceil((b + 1)/b^2) + 1.

But we have to make sure that t is at least 1.

Wait, t must be at least ceil((b + 1)/b^2).

And floor((n + b)/b^2) is the upper limit.

So, the number of valid t is floor((n + b)/b^2) - ceil((b + 1)/b^2) + 1, provided that ceil((b + 1)/b^2) ≤ floor((n + b)/b^2).

Otherwise, there are no solutions for that b.

This seems a bit messy, but perhaps there's a better way to compute this.

Looking back at the code, it seems to be implementing something similar, but I need to map its variables to my notations.

In the code, it's iterating over i from 1 to b (which is m in the problem, but in my notation, m is the upper limit for b).

For each i (which corresponds to b), it computes x = (a - i * (i - 1)) // (i ** 2) + 1.

Let's see what this corresponds to.

Given a = t * i^2 - i, we can solve for t:

a = t * i^2 - i ⇒ t = (a + i) / i^2.

But in the code, x = (a - i * (i - 1)) // (i ** 2) + 1.

Wait, perhaps there's a different transformation.

Let me compute (a - i*(i - 1)) // (i^2) + 1.

Given a = t * i^2 - i, then a - i*(i - 1) = t * i^2 - i - i*(i - 1) = t * i^2 - i - i^2 + i = t * i^2 - i^2 = (t - 1) * i^2.

So, (a - i*(i - 1)) // (i^2) = (t - 1) * i^2 // i^2 = t - 1.

Then, x = t - 1 + 1 = t.

So, x = t.

So, in the code, x is equal to t.

Then, if x > 0, it adds x to suma.

Additionally, if (a - i*(i - 1)) // (i^2) + 1 > 0 and (a - i*(i - 1)) % (i^2) == 0 and i*(i - 1) % (i^2) == 0, it adds 1 to suma.

Wait, but (a - i*(i - 1)) // (i^2) + 1 is x, which is t.

So, if t > 0, it adds t to suma.

Then, if t > 0 and (a - i*(i - 1)) % (i^2) == 0 and i*(i - 1) % (i^2) == 0, it adds 1 more to suma.

But (a - i*(i - 1)) % (i^2) == 0 means that a - i*(i - 1) is divisible by i^2, which we've already established as (t - 1) * i^2, which is always divisible by i^2. So, this condition is always true when t is an integer.

Moreover, i*(i - 1) % (i^2) == 0.

i*(i - 1) is i^2 - i, and i^2 - i % i^2 == -i % i^2.

This is zero only if i divides i^2, which it always does, but -i % i^2 is zero only if i divides i, which it does, but actually, -i % i^2 = i^2 - i.

Wait, no.

In Python, negative modulo is handled by (-i % i^2) which is equivalent to i^2 - i if i != 0.

So, this condition i*(i - 1) % i^2 == 0 is equivalent to i^2 - i % i^2 == 0, which is i^2 - i ≡ 0 mod i^2, which simplifies to -i ≡ 0 mod i^2, which means that i divides i^2, which is always true.

Wait, but actually, -i ≡ 0 mod i^2 implies that i^2 divides i, which is only true if i = 1.

Wait, no, -i ≡ 0 mod i^2 means that i^2 divides i, which is only true if i = 1.

Because for i > 1, i^2 does not divide i.

Wait, no, i^2 divides i means that i divides 1, which is only true for i = 1.

So, this condition i*(i - 1) % i^2 == 0 is only true when i = 1.

Therefore, the additional +1 is only added when t > 0 and (a - i*(i - 1)) % i^2 == 0 and i = 1.

But we've already seen that (a - i*(i - 1)) % i^2 == 0 is always true when t is an integer.

So, effectively, the additional +1 is only added when i = 1 and t > 0.

So, in summary, for each i from 1 to b:

- Compute t = x = (a - i*(i - 1)) // i^2 + 1

- If t > 0, add t to suma

- If i = 1 and t > 0, add 1 more to suma

Finally, print suma - 2.

Wait, but in the first test case, n=1, m=1:

- i=1:

- t = (1 - 1*0)//1 + 1 = (1 - 0)//1 + 1 = 1//1 + 1 = 1 + 1 = 2

- t > 0, so add 2 to suma → suma=2

- i=1 and t > 0, so add 1 more to suma → suma=3

- Then print suma - 2 = 1, which matches the sample output.

In the second test case, n=2, m=3:

- i=1:

- t = (2 - 1*0)//1 + 1 = 2//1 + 1 = 2 + 1 = 3

- t > 0, add 3 to suma → suma=3

- i=1 and t > 0, add 1 more to suma → suma=4

- i=2:

- t = (2 - 2*1)//4 + 1 = (2 - 2)//4 + 1 = 0//4 + 1 = 0 + 1 = 1

- t > 0, add 1 to suma → suma=5

- i=3:

- t = (2 - 3*2)//9 + 1 = (-4)//9 + 1 = (-1) + 1 = 0

- t <= 0, do nothing

- Finally, print suma - 2 = 5 - 2 = 3, which matches the sample output.

Now, for n=3, m=5:

- i=1:

- t = (3 - 1*0)//1 + 1 = 3//1 + 1 = 3 + 1 = 4

- t > 0, add 4 to suma → suma=4

- i=1 and t > 0, add 1 more to suma → suma=5

- i=2:

- t = (3 - 2*1)//4 + 1 = (3 - 2)//4 + 1 = 1//4 + 1 = 0 + 1 = 1

- t > 0, add 1 to suma → suma=6

- i=3:

- t = (3 - 3*2)//9 + 1 = (3 - 6)//9 + 1 = (-3)//9 + 1 = (-1) + 1 = 0

- t <= 0, do nothing

- i=4:

- t = (3 - 4*3)//16 + 1 = (3 - 12)//16 + 1 = (-9)//16 + 1 = (-1) + 1 = 0

- t <= 0, do nothing

- i=5:

- t = (3 - 5*4)//25 + 1 = (3 - 20)//25 + 1 = (-17)//25 + 1 = (-1) + 1 = 0

- t <= 0, do nothing

- Finally, print suma - 2 = 6 - 2 = 4, which matches the sample output of 4.

Wait, but according to my earlier calculation using the standard approach, sum floor(3 / b) for b=1 to 5 is 3 + 1 + 1 + 0 + 0 = 5, but the code outputs 4.

Wait, but according to the sample output, it's 4, which matches the code's output.

So, perhaps my standard approach is incorrect.

Wait, perhaps I miscounted the pairs.

Let's list all possible pairs (a, b) for n=3, m=5:

b=1:

a can be 1,2,3

Check a + b divisible by b * gcd(a, b) = 1 * gcd(a,1) = 1

So, a + 1 divisible by 1, which is always true.

So, all (1,1), (2,1), (3,1) are valid.

b=2:

a can be 2

Check a + 2 divisible by 2 * gcd(a,2)

If a=2, gcd(2,2)=2

So, 2 + 2 = 4, and 2 * 2 = 4, which divides 4.

So, (2,2) is valid.

a=1: 1 + 2 = 3, and 2 * gcd(1,2) = 2 * 1 = 2, which does not divide 3.

So, invalid.

a=2: already checked.

a=3: 3 + 2 = 5, and 2 * gcd(3,2)=2*1=2, which does not divide 5.

So, invalid.

So, only (2,2)

b=3:

a can be 3

Check a + 3 divisible by 3 * gcd(a,3)

If a=3, gcd(3,3)=3

So, 3 + 3 = 6, and 3 * 3 = 9, which does not divide 6.

Wait, 9 does not divide 6.

So, (3,3) is invalid.

a=1: 1 + 3 = 4, 3 * gcd(1,3)=3*1=3, which does not divide 4.

a=2: 2 + 3 = 5, 3 * gcd(2,3)=3*1=3, which does not divide 5.

a=3: already checked.

So, no valid pairs for b=3.

b=4:

a can be 4, but n=3, so no a.

b=5:

a can be 5, but n=3, so no a.

So, total valid pairs: (1,1), (2,1), (3,1), (2,2)

Which is 4 pairs, matching the sample output.

Earlier, I mistakenly thought that for b=3, a=3 was valid, but actually, it's invalid because 6 is not divisible by 9.

So, the standard approach of summing floor(n / b) for b from 1 to m is incorrect in this context.

Therefore, my initial simplification was wrong.

Hence, the condition a + b is a multiple of b * gcd(a,b) does not simply reduce to b divides a.

I need to find a different way to count the valid pairs.

Looking back, perhaps the code is implementing the correct approach.

Let me try to understand the expression in the code.

From earlier, we have a = t * b^2 - b.

Then, t = (a + b)/b^2.

In the code, x = (a - i*(i - 1)) // (i**2) + 1.

As we saw, this corresponds to t.

Then, the number of valid t is floor((n + b)/b^2) - ceil((b + 1)/b^2) + 1.

But in the code, it seems to be summing t for each b, where t ranges from 1 to floor((n + b)/b^2), but with some adjustments.

Moreover, it's subtracting 2 at the end.

I'm not entirely sure why it's subtracting 2.

Perhaps there are some overcounted or undercounted cases.

Alternatively, maybe the initial suma includes some invalid pairs, and subtracting 2 corrects for that.

Given that in the first test case, suma is 3 +1 (for i=1) =4, then subtract 2 to get 2, but the sample output is 1.

Wait, earlier I thought it was 3 -2=1, but actually, in n=1,m=1, suma=3, then subtract 2 to get 1.

In n=2,m=3, suma=5, subtract 2 to get 3.

In n=3,m=5, suma=5, subtract 2 to get 3, but sample output is 4.

Wait, no, earlier I saw that for n=3,m=5, suma=5, subtract 2 to get 3, but sample output is 4.

Wait, perhaps I miscalculated.

Wait, in n=3,m=5:

- i=1: t=4, add 4, plus 1 more because i=1, so suma=5

- i=2: t=1, add 1, suma=6

- i=3: t=0, do nothing

- i=4: t=0, do nothing

- i=5: t=0, do nothing

- Finally, print suma -2 =4, which matches sample output.

Wait, but earlier I thought suma=5, but actually, suma=4 +1 (from i=1) +1 (from i=2) =6, then subtract 2 to get 4.

Wait, perhaps I need to trace it again.

Wait, in n=3,m=5:

- i=1: t=(3 -0)//1 +1=4, add 4, since i=1 and t>0, add 1 more, suma=5

- i=2: t=(3 -2)//4 +1=0//4 +1=0+1=1, add 1, suma=6

- i=3: t=(3 -6)//9 +1=-1+1=0, do nothing

- i=4: t=(3 -12)//16 +1=-9//16 +1=0 +1=1, but a = t*16 -4, which is negative, so invalid

Wait, a = t*b^2 - b =1*16 -4=12, which is less than or equal to n=3? No, 12 >3, so t=1 is invalid.

Wait, but according to the code, it adds t=1, but in reality, a=1*4 -2=2, which is <=3.

Wait, for i=2, t=1, a=1*4 -2=2, which is <=3.

Wait, a = t*b^2 - b =1*4 -2=2.

Similarly, for i=1, t=4, a=4*1 -1=3, which is <=3.

Wait, but earlier I thought t=(a + b)/b^2, but actually, t=(a + b)/b^2.

Wait, perhaps I need to revisit the expression for t.

Given a = t*b^2 - b, then a + b = t*b^2.

Thus, t = (a + b)/b^2.

We need t to be an integer >=1.

Also, a = t*b^2 - b >=1 and <=n.

So, t*b^2 - b >=1 and t*b^2 - b <=n.

Thus, t >= (b +1)/b^2 and t <= (n +b)/b^2.

So, t ranges from ceil((b +1)/b^2) to floor((n +b)/b^2).

Hence, the number of valid t for each b is floor((n +b)/b^2) - ceil((b +1)/b^2) +1, if ceil((b +1)/b^2) <= floor((n +b)/b^2).

Otherwise, 0.

Now, in the code, for each i (b), it computes x = (a - i*(i -1)) // (i^2) +1.

Given that a = t*i^2 -i, then a -i*(i -1) = t*i^2 -i -i*(i -1) = t*i^2 -i -i^2 +i = t*i^2 -i^2 = (t -1)*i^2.

Thus, (a -i*(i -1)) // (i^2) = t -1.

Hence, x = t -1 +1 =t.

So, x =t.

Then, if x >0, add x to suma.

Additionally, if i=1 and x>0, add 1 more to suma.

Finally, print suma -2.

I need to understand why this is correct.

Looking back at n=3,m=5:

- i=1: t=4, add 4, plus 1 more, suma=5

- i=2: t=1, add 1, suma=6

- i=3: t=0, do nothing

- i=4: t=0, do nothing

- i=5: t=0, do nothing

- print suma -2=4, which matches sample output.

Wait, but according to the earlier manual count, there are 4 valid pairs.

So, perhaps it's correct.

Similarly, for n=10,m=8:

- i=1: t=(10 -0)//1 +1=10+1=11, add 11, plus 1 more, suma=12

- i=2: t=(10 -2)//4 +1=8//4 +1=2+1=3, add 3, suma=15

- i=3: t=(10 -6)//9 +1=4//9 +1=0+1=1, add 1, suma=16

- i=4: t=(10 -12)//16 +1=-2//16 +1=0 +1=1, a=1*16 -4=12>10, invalid, so don't add

- i=5: t=(10 -20)//25 +1=-10//25 +1=0 +1=1, a=1*25 -5=20>10, invalid

- i=6: t=(10 -30)//36 +1=-20//36 +1=0 +1=1, a=1*36 -6=30>10, invalid

- i=7: t=(10 -42)//49 +1=-32//49 +1=0 +1=1, a=1*49 -7=42>10, invalid

- i=8: t=(10 -56)//64 +1=-46//64 +1=0 +1=1, a=1*64 -8=56>10, invalid

- suma=16, suma -2=14, which matches the sample output.

So, it seems correct.

Hence, the code is correct.

Therefore, Correctness: **True**