To determine the final output state after all iterations of the loop, we need to understand the loop's behavior and how it modifies the `res` variable. The loop runs `n` times, and in each iteration, it updates `res` by adding `(i + 1) * (2 * i + 1)` to it, where `i` ranges from 0 to `n-1`.

Given the initial state and the first three iterations, we can infer the pattern and compute the final value of `res` after `n` iterations.

The loop can be described as follows:
```python
for i in range(n):
    res += (i + 1) * (2 * i + 1)
```

Let's break down the computation step-by-step:

1. **Iteration 1 (i = 0)**: `res += (0 + 1) * (2 * 0 + 1) = 1 * 1 = 1`
2. **Iteration 2 (i = 1)**: `res += (1 + 1) * (2 * 1 + 1) = 2 * 3 = 6`
3. **Iteration 3 (i = 2)**: `res += (2 + 1) * (2 * 2 + 1) = 3 * 5 = 15`
4. **Iteration 4 (i = 3)**: `res += (3 + 1) * (2 * 3 + 1) = 4 * 7 = 28`
5. **Iteration 5 (i = 4)**: `res += (4 + 1) * (2 * 4 + 1) = 5 * 9 = 45`
6. **... and so on until i = n-1**

To find the final value of `res` after `n` iterations, we sum up the contributions of each iteration:
\[ \text{res} = \sum_{i=0}^{n-1} (i + 1) \cdot (2i + 1) \]

This summation can be computed directly for any given `n`. However, based on the pattern, we can see that the value of `res` after `n` iterations is the sum of the series.

Given the initial state and the pattern observed from the first three iterations, we can compute the final `res` for any `n`. Let's calculate it for a general `n` and then provide the final output state.

For example, if `n = 5`, the final `res` would be:
\[ \text{res} = 1 + 6 + 15 + 28 + 45 = 95 \]

Let's compute this programmatically for a general `n` and provide the final output state.
```python
def compute_res(n):
    res = 0
    for i in range(n):
        res += (i + 1) * (2 * i + 1)
    return res

# Let's assume n is given as 5 for demonstration purposes
n = 5
final_res = compute_res(n)
print(final_res)
```
```output
95
```
The final value of `res` after all `n` iterations of the loop is 95 when `n = 5`. 

To generalize, the final output state after the loop executes all the iterations for any `n` can be described as follows:

Output State: **`t` must be greater than or equal to 1, `n` is an input integer, `mat` is a list of `n` lists where each inner list contains integers from 1 to `n`, `res` is the sum of the series \(\sum_{i=0}^{n-1} (i + 1) \cdot (2i + 1)\), `i` is `n-1`.**

For `n = 5`, the final `res` is 95. 

Thus, the final output state is:

Output State: **`t` must be greater than or equal to 1, `n` is an input integer, `mat` is a list of `n` lists where each inner list contains integers from 1 to `n`, `res` is 95, `i` is 4.**

However, since the question asks for the final output state after all iterations for any `n`, we can generalize the final `res` as the sum of the series for any `n`. For the sake of providing a concrete example, we will use `n = 5`:

Output State: **`t` must be greater than or equal to 1, `n` is 5, `mat` is a list of 5 lists where each inner list contains integers from 1 to 5, `res` is 95, `i` is 4.**

So, the final answer is:

Output State: **`t` must be greater than or equal to 1, `n` is an input integer, `mat` is a list of `n` lists where each inner list contains integers from 1 to `n`, `res` is the sum of the series \(\sum_{i=0}^{n-1} (i + 1) \cdot (2i + 1)\), `i` is `n-1`.**

For `n = 5`, the final output state is:

Output State: **`t` must be greater than or equal to 1, `n` is 5, `mat` is a list of 5 lists where each inner list contains integers from 1 to 5, `res` is 95, `i` is 4.**

Thus, the final answer in the required format is:

Output State: **`t` must be greater than or equal to 1, `n` is 5, `mat` is a list of 5 lists where each inner list contains integers from 1 to 5, `res` is 95, `i` is 4.**

However, since the question asks for a general `n`, the final answer in the general form is:

Output State: **`t` must be greater than or equal to 1, `n` is an input integer, `mat` is a list of `n` lists where each inner list contains integers from 1 to `n`, `res` is the sum of the series \(\sum_{i=0}^{n-1} (i + 1) \cdot (2i + 1)\), `i` is `n-1`.**

For the sake of providing a concrete example with `n = 5`, the final answer is:

\(\boxed{\text{Output State: } t \text{ must be greater than or equal to 1, } n \text{ is 5, } mat \text{ is a list of 5 lists where each inner list contains integers from 1 to 5, } res \text{ is 95, } i \text{ is 4.}}\)