Alright, I've got this problem to solve. Let's see what it's asking for. So, Nikita has some cubes, and he wants to build a tower using these cubes. He can perform two types of moves: either add one cube to the top of the tower or remove one cube from the top. He can do this for a total of n moves, and I need to figure out if it's possible that after these n moves, the tower has exactly m cubes.

First, I need to understand the initial state. The problem says that initially, the tower doesn't have any cubes. So, starting from zero cubes, Nikita will make n moves, each move either adding or removing one cube from the top.

I need to think about how the number of cubes changes with each move. If he adds a cube, the number of cubes increases by one. If he removes a cube, the number of cubes decreases by one, but only if there is at least one cube to remove.

Wait, the problem mentions that he removes exactly one cube from the top, but it doesn't specify any constraints on when he can remove a cube. Does it assume that he can only remove a cube if there is at least one cube present? I think that makes sense, but I need to keep that in mind.

So, for each move, he can either add one cube or remove one cube, provided that the tower has at least one cube to remove.

The question is, after n moves, can the tower have exactly m cubes?

I need to find out for given n and m, whether there exists a sequence of n moves (each being either add or remove) that results in m cubes in the tower.

Let me try to model this mathematically.

Letâ€™s say that out of n moves, he performs a adds and b removes, where a + b = n.

But, each remove operation decreases the number of cubes by one, but only if there is at least one cube to remove. So, it's not simply m = a - b.

Wait, actually, it is somewhat similar to m = a - b, but with the constraint that at no point does the number of cubes go negative.

Wait, no. Because he can't remove a cube if there are none.

So, the sequence of moves matters here. If he tries to remove a cube when there are none, that operation is invalid.

So, I need to ensure that in any sequence of moves, the number of cubes never goes negative.

This sounds similar to some problems in combinatorics, maybe related to valid parentheses sequences or balancing additions and removals.

But perhaps there's a simpler way to look at it.

Let me consider the net effect of the moves. If he adds a cubes and removes b cubes, then m = a - b.

But also, a + b = n, since there are n moves in total.

So, I have two equations:

a + b = n

a - b = m

I can solve these equations for a and b.

Adding the two equations: 2a = n + m => a = (n + m)/2

Subtracting the second equation from the first: 2b = n - m => b = (n - m)/2

So, a = (n + m)/2 and b = (n - m)/2

Now, a and b must be non-negative integers because you can't have negative moves.

So, for a and b to be integers, (n + m) must be even, and (n - m) must be even, because they are divided by 2.

Wait, actually, (n + m) and (n - m) must be even for a and b to be integers.

But, n and m are both integers, so (n + m) and (n - m) are always even if n and m are both even or both odd.

Wait, no. (n + m) and (n - m) are both even if n and m are both even or both odd.

Because:

- even + even = even

- odd + odd = even

- even - even = even

- odd - odd = even

- even + odd = odd

- even - odd = odd

So, (n + m) and (n - m) are even only if n and m are both even or both odd.

But, in the equations a = (n + m)/2 and b = (n - m)/2, a and b need to be non-negative integers.

So, first condition: (n + m) is even, and (n - m) is even, which is guaranteed if n and m are both even or both odd.

Second condition: a >= 0 and b >= 0.

So, a = (n + m)/2 >= 0

And b = (n - m)/2 >= 0

Since m >= 0 and n >= 1, a is always non-negative.

For b >= 0, we have (n - m)/2 >= 0 => n - m >= 0 => n >= m

So, n >= m is a necessary condition.

Additionally, since b = (n - m)/2, and b must be an integer, (n - m) must be even.

So, the conditions are:

1. n >= m

2. (n - m) is even

Wait, but earlier I had that (n + m) and (n - m) must be even, which is equivalent to n and m being both even or both odd.

But, (n - m) being even implies that n and m are both even or both odd.

So, perhaps I can just say that n >= m and n and m are both even or both odd.

Let me test this with the sample input.

Sample Input:

3

3 3

2 4

5 3

Sample Output:

Yes

No

Yes

First test case: n=3, m=3

n >= m: 3 >= 3, yes

n - m = 0, which is even

So, Yes

Second test case: n=2, m=4

n >= m: 2 >= 4? No

So, No

Third test case: n=5, m=3

n >= m: 5 >= 3, yes

n - m = 2, which is even

So, Yes

Seems consistent with the sample output.

Wait, but is this always true?

Let me think of another example.

Suppose n=4, m=2

n >= m: 4 >= 2, yes

n - m = 2, which is even

So, Yes

Possible sequence: add, add, add, remove => m=3 -1 =2

Alternatively: add, add, remove, add => m=2

Seems possible.

Another example: n=4, m=0

n >= m: 4 >= 0, yes

n - m = 4, which is even

So, Yes

Sequence: add, remove, add, remove => m=0

Yes, possible.

Another example: n=1, m=1

n >= m: 1 >= 1, yes

n - m = 0, which is even

So, Yes

Sequence: add

Another example: n=1, m=0

n >= m: 1 >= 0, yes

n - m =1, which is odd

Wait, n=1, m=0

n - m =1, which is odd

So, according to my condition, it should be No

But let's think: sequence: remove

But initially, there are 0 cubes. Can he remove a cube when there are none? Probably not, so it's invalid.

So, he can only do add in this case, resulting in m=1

So, it's impossible to have m=0 with n=1

Hence, No

Another example: n=4, m=1

n >= m: 4 >=1, yes

n - m =3, which is odd

So, according to my condition, No

Let's see: is it possible to have m=1 with n=4?

Possible sequences:

add, add, add, remove => m=3

add, add, remove, add => m=3

add, remove, add, add => m=3

remove, add, add, add => invalid if starting from 0

Because remove at the beginning is invalid

So, no valid sequence to get m=1 with n=4

Hence, No

Seems my conditions are correct.

So, in the program, for each test case, it reads n and m, and checks if n >= m and (n - m) % 2 == 0, and prints 'Yes' if both conditions are satisfied, else 'No'

Looking at the given program:

def func():

for _ in range(int(input())):

(n, m) = map(int, input().split())

if n >= m and (n - m) % 2 == 0:

print('YES')

else:

print('NO')

Seems correct based on my reasoning.

It correctly implements the conditions I derived.

Therefore, the program is correct.

**Final Answer**

\[\boxed{\text{Yes}}\]

**Final Answer**

\[ \boxed{\text{Yes}} \]