To analyze the provided Python code snippet, let's break down the impact on the initial state:

1. The variable `k` is already defined as `a + b - 1`.
2. The code calculates `sum_k` using the formula `k * (k + 1) // 2`, which computes the sum of the first `k` natural numbers.
3. The result of that calculation does not change any of the existing variables except `sum_k`.

Given that `k` is defined as `a + b - 1`, we can substitute that value into the formula for `sum_k`.

Thus, `sum_k` will be calculated as follows:
- `sum_k = (a + b - 1) * (a + b) // 2`

The key variables remain unchanged, and we now know `sum_k`.

Output State: **`m` is a positive integer such that 1 <= m <= 10^9, `a` is a positive integer such that 1 <= a <= 10^5, `b` is a positive integer such that 1 <= b <= 10^5, `g` is equal to 1, `k` is equal to `a + b - 1`, `m` is greater than or equal to `k`, `sum_k` is equal to `(a + b - 1) * (a + b) // 2`.**