The expression `(n * n - 1) / 2` calculates the result of the square of `n` minus 1, divided by 2. The expression `(n * n + 1) / 2` calculates the result of the square of `n` plus 1, divided by 2. Given that `n` is an input positive odd integer larger than 2, we can evaluate these expressions directly.

Letâ€™s denote `n` as an odd integer greater than 2. The output will be two numbers derived from the calculations.

Assuming `n` is an odd integer, for example, if `n = 3`, the calculations would be:
1. `n * n - 1 = 3 * 3 - 1 = 9 - 1 = 8`
2. `8 / 2 = 4`
3. `n * n + 1 = 3 * 3 + 1 = 9 + 1 = 10`
4. `10 / 2 = 5`

Thus, for any odd integer `n`, the output will always yield two specific results based on the value of `n`.

The output state will reflect the calculated results based on the input odd integer.

Output State: **`n` is an input positive odd integer larger than 2; the results are (n * n - 1) / 2 and (n * n + 1) / 2.**