The given code appends a new element to the list `bd`. Specifically, it calculates the difference between `b[i]` and `b[i - 1]` and adds this difference to the end of the `bd` list.

Given the initial state, `bd` initially contains two elements: `[0, b[1] - b[0]]`. After executing the line `bd.append(b[i] - b[i - 1])`, `bd` will now contain three elements: `[0, b[1] - b[0], b[i] - b[i - 1]]`.

The values of the other variables (`t`, `n`, `k`, `q`, `a`, `b`, `ad`, and `i`) remain unchanged.

Output State: **`t` is an input integer such that 1 ≤ `t` ≤ 10^4; `n` is an integer read from input such that `k` ≤ `n` ≤ 10^9; `k` is an integer read from input such that 1 ≤ `k` ≤ 10^5 and `k > 0`; `q` is an integer read from input such that 1 ≤ `q` ≤ 10^5; `a` is a list of `k+1` integers where `a_0` = 0, 1 ≤ `a_i` ≤ `n` for 1 ≤ `i` ≤ `k`, `a_i` < `a_{i+1}` for every 1 ≤ `i` ≤ `k`, and `a_k` = `n`; `b` is a list of `k+1` integers where `b_0` = 0, 1 ≤ `b_i` ≤ 10^9, `b_i` < `b_{i+1}` for every 1 ≤ `i` ≤ `k`; `ad` is a list containing `k+1` elements `[0, a[1] - a[0], a[2] - a[1], ..., a[k] - a[k-1]]`; `bd` is a list containing three elements `[0, b[1] - b[0], b[i] - b[i - 1]]`; `i` is `i + 1`**.