To determine the final output state after all iterations of the loop, let's analyze the loop's behavior and the given initial and intermediate states.

The loop iterates from `i = 1` to `i = b` (inclusive). For each `i`, it calculates `x` as:
\[ x = \left(\frac{a - i \cdot (i - 1)}{i^2}\right) + 1 \]

If `x` is greater than 0, it adds `x` to `suma`. Additionally, if both \((a - i \cdot (i - 1)) \% i^2 == 0\) and \(i \cdot (i - 1) \% i^2 == 0\), it increments `suma` by 1.

Let's break down the provided states:

1. **Output State after the loop executes 1 time:**
   - `suma` is 4 if `x` is 3.

2. **Output State after the loop executes 2 times:**
   - `x` is calculated as \(\left(\frac{a - i \cdot (i - 1)}{i^2}\right) + 1\).
   - The conditions for `suma` incrementation are not detailed further.

3. **Output State after the loop executes 3 times:**
   - Similar to the second state, `x` is calculated similarly, and conditions for `suma` incrementation are not detailed further.

Given these, we need to calculate the final `suma` after all iterations (i.e., `i` from 1 to `b`).

Let's assume the values of `a` and `b` from the initial state and iterate through the loop to compute the final `suma`.

### Example Calculation

Let's assume `a = 10` and `b = 5` for the sake of example.

1. **Iteration 1 (i = 1):**
   \[
   x = \left(\frac{10 - 1 \cdot (1 - 1)}{1^2}\right) + 1 = \left(\frac{10}{1}\right) + 1 = 10 + 1 = 11
   \]
   Since \(x > 0\), `suma` becomes 11.
   The additional condition for `suma` incrementation is not met.

2. **Iteration 2 (i = 2):**
   \[
   x = \left(\frac{10 - 2 \cdot (2 - 1)}{2^2}\right) + 1 = \left(\frac{10 - 2}{4}\right) + 1 = \left(\frac{8}{4}\right) + 1 = 2 + 1 = 3
   \]
   Since \(x > 0\), `suma` becomes 14.
   The additional condition for `suma` incrementation is not met.

3. **Iteration 3 (i = 3):**
   \[
   x = \left(\frac{10 - 3 \cdot (3 - 1)}{3^2}\right) + 1 = \left(\frac{10 - 6}{9}\right) + 1 = \left(\frac{4}{9}\right) + 1 \approx 1.44
   \]
   Since \(x > 0\), `suma` becomes approximately 15.44, but since `x` must be an integer, `suma` remains 15.
   The additional condition for `suma` incrementation is not met.

4. **Iteration 4 (i = 4):**
   \[
   x = \left(\frac{10 - 4 \cdot (4 - 1)}{4^2}\right) + 1 = \left(\frac{10 - 12}{16}\right) + 1 = \left(\frac{-2}{16}\right) + 1 = -0.125 + 1 = 0.875
   \]
   Since \(x \leq 0\), `suma` remains 15.
   The additional condition for `suma` incrementation is not met.

5. **Iteration 5 (i = 5):**
   \[
   x = \left(\frac{10 - 5 \cdot (5 - 1)}{5^2}\right) + 1 = \left(\frac{10 - 20}{25}\right) + 1 = \left(\frac{-10}{25}\right) + 1 = -0.4 + 1 = 0.6
   \]
   Since \(x \leq 0\), `suma` remains 15.
   The additional condition for `suma` incrementation is not met.

Thus, the final `suma` after all iterations is 15.

### Final Output State
Output State: **suma is 15.**

In natural language, the final output state is that the variable `suma` will hold the value 15 after the loop has completed all its iterations, given the example values of `a = 10` and `b = 5`. The exact value of `suma` will vary based on the specific values of `a` and `b`, but the process to determine it remains the same.