Alright, I've got this problem to solve. Let's see what it's asking for. So, I'm given an array `a` of length `n`, a positive integer `m`, and a string `s` of commands consisting of 'L's and 'R's. For each command in the string `s`, I need to output the remainder of the product of all elements in the array `a` when divided by `m`, and then remove either the leftmost or the rightmost element from `a`, depending on whether the command is 'L' or 'R'.

First, I need to understand what exactly is being asked. For each step:

1. Calculate the product of all elements in the current array `a`, take that product modulo `m`, and output that value.

2. Then, based on the current command in `s`, remove either the first element ('L') or the last element ('R') from `a`.

This process repeats for each command in `s`, and since `s` is of length `n`, and we remove one element each time, we'll end up with an empty array at the end.

I need to make sure that for each step, I'm correctly calculating the product modulo `m` and then removing the correct element.

Looking at the provided program, it seems to have a function `func_1` that takes `n`, `m`, `a`, and `s` as inputs and is supposed to return the sequence of remainders as described.

Let's dive into the function `func_1`:

1. It initializes an empty list `b`.

2. It sets two pointers, `l` and `r`, to the start and end of the array `a`.

3. It iterates through each command in `s`:

- If the command is 'L', it appends the leftmost element (`a[l]`) to `b` and increments `l`.

- If the command is 'R', it appends the rightmost element (`a[r]`) to `b` and decrements `r`.

4. After collecting all elements that are to be removed in order, it initializes an empty list `ans` and a variable `p` to 1.

5. It then iterates through the list `b` in reverse:

- For each value `v` in reversed `b`, it multiplies `p` by `v` and appends the result to `ans`.

6. Finally, it returns the reversed `ans`.

Wait a minute, this seems a bit convoluted. Let's see if this logic aligns with what the problem is asking for.

The problem requires that for each step, before removing any element, we calculate the product of the current array modulo `m` and then remove either the leftmost or rightmost element based on the command.

However, in the provided code:

- It first simulates the entire process of removing elements according to `s` and collects these removed elements in `b`.

- Then, it calculates the cumulative product of these removed elements in reverse order, storing intermediate products in `ans`.

- Finally, it returns the reversed `ans`.

This seems incorrect because:

- The product being calculated in `ans` is of the removed elements, not the remaining elements in the array at each step.

- The problem asks for the product of the current state of the array before any removal in each step.

So, the code is calculating the product of the elements that have been removed so far, which is not what is being asked. It should be calculating the product of the elements that are still in the array before each removal.

This suggests that the given program is incorrect.

Wait, maybe I'm misunderstanding something. Let's look at the example provided in the problem to verify.

Example Input:

4

4 6

3 1 4 2

LRRL

5 1

1 1 1 1 1

LLLLL

6 8

1 2 3 4 5 6

RLLLRR

1 10000

10000

R

Example Output:

0 2 4 1

0 0 0 0 0

0 0 0 4 4 4

0

Looking at the first test case:

n=4, m=6, a=[3,1,4,2], s=LRRL

According to the problem:

- Initial a: [3,1,4,2]

- Product: 3*1*4*2 = 24, 24 mod 6 = 0

- Output: 0

- Command 'L': remove leftmost element (3), a becomes [1,4,2]

- Product: 1*4*2 = 8, 8 mod 6 = 2

- Output: 2

- Command 'R': remove rightmost element (2), a becomes [1,4]

- Product: 1*4 = 4, 4 mod 6 = 4

- Output: 4

- Command 'R': remove rightmost element (4), a becomes [1]

- Product: 1, 1 mod 6 = 1

- Output: 1

- Command 'L': remove leftmost element (1), a becomes empty

So, the output should be: 0 2 4 1

Now, looking at the provided program's output for this case, it matches: 0 2 4 1

But according to my earlier reasoning, the program seems to be calculating the product of removed elements, not the remaining elements. However, in this case, it's producing the correct output.

Hmm, maybe there's a different way to interpret this.

Let me try to simulate what the program is doing for this first test case.

Initialize:

b = []

l = 0, r = 3

Iterate through s:

- s[0] = 'L': append a[0] = 3, l = 1

- s[1] = 'R': append a[3] = 2, r = 2

- s[2] = 'R': append a[2] = 4, r = 1

- s[3] = 'L': append a[1] = 1, l = 2

So, b = [3,2,4,1]

Then, p = 1

Reversed b: [1,4,2,3]

For each v in reversed b:

- v=1: p=1*1=1, ans=[1]

- v=4: p=1*4=4, ans=[1,4]

- v=2: p=4*2=8, ans=[1,4,8]

- v=3: p=8*3=24, ans=[1,4,8,24]

Then, return reversed(ans): [24,8,4,1]

Finally, print each element modulo 6:

24 mod 6 = 0

8 mod 6 = 2

4 mod 6 = 4

1 mod 6 = 1

Which matches the expected output: 0 2 4 1

So, in this case, it works.

But is this a general solution, or just coincidentally correct for this test case?

Let's try another test case.

Second test case:

n=5, m=1, a=[1,1,1,1,1], s=LLLLL

According to the problem:

- Initial a: [1,1,1,1,1]

- Product: 1*1*1*1*1=1, 1 mod 1=0

- Output: 0

- Command 'L': remove leftmost element (1), a becomes [1,1,1,1]

- Product: 1*1*1*1=1, 1 mod 1=0

- Output: 0

- Command 'L': remove leftmost element (1), a becomes [1,1,1]

- Product: 1*1*1=1, 1 mod 1=0

- Output: 0

- Command 'L': remove leftmost element (1), a becomes [1,1]

- Product: 1*1=1, 1 mod 1=0

- Output: 0

- Command 'L': remove leftmost element (1), a becomes [1]

- Product: 1, 1 mod 1=0

- Output: 0

- Command 'L': remove leftmost element (1), a becomes empty

So, output should be: 0 0 0 0 0

Now, according to the provided program:

Initialize:

b = []

l = 0, r = 4

Iterate through s:

- s[0] = 'L': append a[0] = 1, l = 1

- s[1] = 'L': append a[1] = 1, l = 2

- s[2] = 'L': append a[2] = 1, l = 3

- s[3] = 'L': append a[3] = 1, l = 4

- s[4] = 'L': append a[4] = 1, l = 5

So, b = [1,1,1,1,1]

Then, p = 1

Reversed b: [1,1,1,1,1]

For each v in reversed b:

- v=1: p=1*1=1, ans=[1]

- v=1: p=1*1=1, ans=[1,1]

- v=1: p=1*1=1, ans=[1,1,1]

- v=1: p=1*1=1, ans=[1,1,1,1]

- v=1: p=1*1=1, ans=[1,1,1,1,1]

Then, return reversed(ans): [1,1,1,1,1]

Print each element modulo 1:

1 mod 1 = 0 for each, so output: 0 0 0 0 0

Which matches the expected output.

Okay, so for this test case, it also works.

Let's look at the third test case:

n=6, m=8, a=[1,2,3,4,5,6], s=RLLLRR

According to the problem:

- Initial a: [1,2,3,4,5,6]

- Product: 1*2*3*4*5*6=720, 720 mod 8=0

- Output: 0

- Command 'R': remove rightmost element (6), a becomes [1,2,3,4,5]

- Product: 1*2*3*4*5=120, 120 mod 8=0

- Output: 0

- Command 'L': remove leftmost element (1), a becomes [2,3,4,5]

- Product: 2*3*4*5=120, 120 mod 8=0

- Output: 0

- Command 'L': remove leftmost element (2), a becomes [3,4,5]

- Product: 3*4*5=60, 60 mod 8=4

- Output: 4

- Command 'L': remove leftmost element (3), a becomes [4,5]

- Product: 4*5=20, 20 mod 8=4

- Output: 4

- Command 'R': remove rightmost element (5), a becomes [4]

- Product: 4, 4 mod 8=4

- Output: 4

- Command 'R': remove rightmost element (4), a becomes empty

So, output should be: 0 0 0 4 4 4

Now, according to the provided program:

Initialize:

b = []

l = 0, r = 5

Iterate through s:

- s[0] = 'R': append a[5] = 6, r = 4

- s[1] = 'L': append a[0] = 1, l = 1

- s[2] = 'L': append a[1] = 2, l = 2

- s[3] = 'L': append a[2] = 3, l = 3

- s[4] = 'R': append a[4] = 5, r = 3

- s[5] = 'R': append a[3] = 4, r = 2

So, b = [6,1,2,3,5,4]

Then, p = 1

Reversed b: [4,5,3,2,1,6]

For each v in reversed b:

- v=4: p=1*4=4, ans=[4]

- v=5: p=4*5=20, ans=[4,20]

- v=3: p=20*3=60, ans=[4,20,60]

- v=2: p=60*2=120, ans=[4,20,60,120]

- v=1: p=120*1=120, ans=[4,20,60,120,120]

- v=6: p=120*6=720, ans=[4,20,60,120,120,720]

Then, return reversed(ans): [720,120,120,60,20,4]

Print each element modulo 8:

720 mod 8 = 0

120 mod 8 = 0

120 mod 8 = 0

60 mod 8 = 4

20 mod 8 = 4

4 mod 8 = 4

Which matches the expected output: 0 0 0 4 4 4

So, for this test case, it also works.

Let's look at the fourth test case:

n=1, m=10000, a=[10000], s=R

According to the problem:

- Initial a: [10000]

- Product: 10000, 10000 mod 10000=0

- Output: 0

- Command 'R': remove rightmost element (10000), a becomes empty

So, output should be: 0

According to the provided program:

Initialize:

b = []

l = 0, r = 0

Iterate through s:

- s[0] = 'R': append a[0] = 10000, r = -1

So, b = [10000]

Then, p = 1

Reversed b: [10000]

For each v in reversed b:

- v=10000: p=1*10000=10000, ans=[10000]

Then, return reversed(ans): [10000]

Print 10000 mod 10000 = 0

Which matches the expected output.

So, all the test cases provided in the example are correctly handled by the program.

But I still feel like the logic is counterintuitive. Let's try to understand why this works.

The key insight seems to be that the product of the remaining elements in the array at each step is equal to the product of all elements divided by the product of the elements that have been removed up to that point.

Wait, but that's not exactly it, because division isn't straightforward with modular arithmetic, especially since m could be any positive integer.

Actually, in modular arithmetic, direct division isn't always possible, especially if the divisor and modulus are not coprime.

But in this approach, it seems like the program is calculating the product of the removed elements in reverse order and keeping a cumulative product.

Wait, no, let's see:

In the function `func_1`:

- It collects the elements to be removed in order into list `b`.

- Then, it initializes `p` to 1 and iterates through `b` in reverse, multiplying `p` by each element and appending the result to `ans`.

- Finally, it returns the reversed `ans`.

So, effectively, `ans` ends up being the product of all removed elements up to each step.

But wait, in the first test case:

b = [3,2,4,1]

reversed b: [1,4,2,3]

Then:

- p=1*1=1, ans=[1]

- p=1*4=4, ans=[1,4]

- p=4*2=8, ans=[1,4,8]

- p=8*3=24, ans=[1,4,8,24]

Then, reversed(ans) = [24,8,4,1]

Which corresponds to the products of the removed elements up to each step:

- After first removal: 3

- But in ans, it's 24, which is 3*2*4*1

Wait, no, reversed(ans) is [24,8,4,1], which corresponds to:

- 24: product of all removed elements up to this point (3*2*4*1=24)

- 8: product of the last three removed elements (2*4*1=8)

- 4: product of the last two removed elements (4*1=4)

- 1: the last removed element (1)

But in the problem, we need the product of the remaining elements at each step.

Wait, perhaps there's a relationship between the product of the remaining elements and the product of the removed elements.

Let me think about it mathematically.

Let’s denote the entire product of the array as P.

At each step, the product of the remaining elements is P divided by the product of the removed elements so far.

But in modular arithmetic, division isn't straightforward.

However, if m is a prime or if P and the product of removed elements are coprime with m, we could use modular inverses.

But in general, since m can be any positive integer, and P and the product of removed elements may not be coprime with m, direct division isn't possible.

So, perhaps the approach in the code is incorrect, but it happens to work for the given test cases.

But in reality, it's flawed.

Let me try to find a counterexample where this approach fails.

Consider n=3, m=4, a=[2,2,2], s=RRR

According to the problem:

- Initial a: [2,2,2]

- Product: 2*2*2=8, 8 mod 4=0

- Output: 0

- Command 'R': remove rightmost element (2), a becomes [2,2]

- Product: 2*2=4, 4 mod 4=0

- Output: 0

- Command 'R': remove rightmost element (2), a becomes [2]

- Product: 2, 2 mod 4=2

- Output: 2

- Command 'R': remove rightmost element (2), a becomes empty

So, output should be: 0 0 2

Now, according to the provided program:

Initialize:

b = []

l = 0, r = 2

Iterate through s:

- s[0] = 'R': append a[2] = 2, r = 1

- s[1] = 'R': append a[1] = 2, r = 0

- s[2] = 'R': append a[0] = 2, r = -1

So, b = [2,2,2]

Then, p = 1

Reversed b: [2,2,2]

For each v in reversed b:

- v=2: p=1*2=2, ans=[2]

- v=2: p=2*2=4, ans=[2,4]

- v=2: p=4*2=8, ans=[2,4,8]

Then, reversed(ans): [8,4,2]

Print each element modulo 4:

8 mod 4 = 0

4 mod 4 = 0

2 mod 4 = 2

Which matches the expected output: 0 0 2

So, even in this case, it works.

Let's try another example: n=2, m=2, a=[1,1], s=LR

According to the problem:

- Initial a: [1,1]

- Product: 1*1=1, 1 mod 2=1

- Output: 1

- Command 'L': remove leftmost element (1), a becomes [1]

- Product: 1, 1 mod 2=1

- Output: 1

- Command 'R': remove rightmost element (1), a becomes empty

So, output should be: 1 1

Now, according to the provided program:

Initialize:

b = []

l = 0, r = 1

Iterate through s:

- s[0] = 'L': append a[0] = 1, l = 1

- s[1] = 'R': append a[1] = 1, r = 0

So, b = [1,1]

Then, p = 1

Reversed b: [1,1]

For each v in reversed b:

- v=1: p=1*1=1, ans=[1]

- v=1: p=1*1=1, ans=[1,1]

Then, reversed(ans): [1,1]

Print each element modulo 2: 1 1

Which matches the expected output.

Hmm, it seems to be working for these cases.

Let me try a case where m is not a prime and elements are not coprime with m.

n=3, m=6, a=[2,3,4], s=LRL

According to the problem:

- Initial a: [2,3,4]

- Product: 2*3*4=24, 24 mod 6=0

- Output: 0

- Command 'L': remove leftmost element (2), a becomes [3,4]

- Product: 3*4=12, 12 mod 6=0

- Output: 0

- Command 'R': remove rightmost element (4), a becomes [3]

- Product: 3, 3 mod 6=3

- Output: 3

- Command 'L': remove leftmost element (3), a becomes empty

So, output should be: 0 0 3

Now, according to the provided program:

Initialize:

b = []

l = 0, r = 2

Iterate through s:

- s[0] = 'L': append a[0] = 2, l = 1

- s[1] = 'R': append a[2] = 4, r = 1

- s[2] = 'L': append a[1] = 3, l = 2

So, b = [2,4,3]

Then, p = 1

Reversed b: [3,4,2]

For each v in reversed b:

- v=3: p=1*3=3, ans=[3]

- v=4: p=3*4=12, ans=[3,12]

- v=2: p=12*2=24, ans=[3,12,24]

Then, reversed(ans): [24,12,3]

Print each element modulo 6:

24 mod 6 = 0

12 mod 6 = 0

3 mod 6 = 3

Which matches the expected output: 0 0 3

So, it works in this case as well.

Wait, maybe this approach is correct after all, despite my initial confusion.

Let me try to understand why this works.

In the function `func_1`:

- It collects the elements to be removed in the order they are removed into list `b`.

- Then, it calculates the cumulative product of these removed elements in reverse order.

- The idea seems to be that the product of the remaining elements at each step is equal to the product of all elements divided by the product of the removed elements up to that point.

- However, as mentioned earlier, division in modular arithmetic is tricky.

- But in this approach, it's calculating the product of the removed elements up to each step and using that to derive the product of the remaining elements.

Wait, perhaps there's a better way to see this.

Let’s denote:

- P: product of all elements in the initial array.

- For each step i from 0 to n-1:

- Let R_i: product of elements removed up to step i.

- Then, the product of remaining elements at step i is P / R_i.

- But again, division is problematic in modular arithmetic.

However, in the code:

- It collects the removed elements in `b`.

- Then, it calculates the cumulative product of `b` in reverse order, which effectively gives the product of all removed elements up to each step.

- Finally, it returns these cumulative products in the order corresponding to each step.

But wait, in the first test case:

- b = [3,2,4,1]

- reversed b: [1,4,2,3]

- cumulative products in ans: [1,4,8,24]

- reversed ans: [24,8,4,1]

- Which correspond to the product of removed elements up to each step:

- Step 0: removed elements up to step 0: [3], product=3

- Step 1: removed elements up to step 1: [3,2], product=6

- Step 2: removed elements up to step 2: [3,2,4], product=24

- Step 3: removed elements up to step 3: [3,2,4,1], product=24

- But in reversed ans: [24,8,4,1], which seem to be the products in reverse order.

Wait, perhaps I need to think differently.

Let’s consider that the product of the remaining elements at each step is equal to P / R_i, where R_i is the product of removed elements up to step i.

But since direct division isn't possible in modular arithmetic, this approach seems flawed.

However, in the examples, it's working correctly.

Let me think about another approach.

An alternative correct approach would be to precompute the product of all elements, and then iteratively divide by the removed elements, taking care with modular inverses when necessary.

But this requires that the removed elements are coprime with m, which isn't guaranteed.

Wait, actually, in the provided program, it seems to be calculating the product of the removed elements and using that to compute the product of the remaining elements indirectly.

But I'm still not sure how this works correctly in the examples.

Let me consider another test case.

n=2, m=3, a=[2,1], s=LR

According to the problem:

- Initial a: [2,1]

- Product: 2*1=2, 2 mod 3=2

- Output: 2

- Command 'L': remove leftmost element (2), a becomes [1]

- Product: 1, 1 mod 3=1

- Output: 1

- Command 'R': remove rightmost element (1), a becomes empty

So, output should be: 2 1

Now, according to the provided program:

Initialize:

b = []

l = 0, r = 1

Iterate through s:

- s[0] = 'L': append a[0] = 2, l = 1

- s[1] = 'R': append a[1] = 1, r = 0

So, b = [2,1]

Then, p = 1

Reversed b: [1,2]

For each v in reversed b:

- v=1: p=1*1=1, ans=[1]

- v=2: p=1*2=2, ans=[1,2]

Then, reversed(ans): [2,1]

Print each element modulo 3: 2 1

Which matches the expected output.

Another example where it works.

Let me try a case where m is smaller than some elements.

n=3, m=5, a=[3,4,2], s=RLR

According to the problem:

- Initial a: [3,4,2]

- Product: 3*4*2=24, 24 mod 5=4

- Output: 4

- Command 'R': remove rightmost element (2), a becomes [3,4]

- Product: 3*4=12, 12 mod 5=2

- Output: 2

- Command 'L': remove leftmost element (3), a becomes [4]

- Product: 4, 4 mod 5=4

- Output: 4

- Command 'R': remove rightmost element (4), a becomes empty

So, output should be: 4 2 4

Now, according to the provided program:

Initialize:

b = []

l = 0, r = 2

Iterate through s:

- s[0] = 'R': append a[2] = 2, r = 1

- s[1] = 'L': append a[0] = 3, l = 1

- s[2] = 'R': append a[1] = 4, r = 0

So, b = [2,3,4]

Then, p = 1

Reversed b: [4,3,2]

For each v in reversed b:

- v=4: p=1*4=4, ans=[4]

- v=3: p=4*3=12, ans=[4,12]

- v=2: p=12*2=24, ans=[4,12,24]

Then, reversed(ans): [24,12,4]

Print each element modulo 5: 24 mod 5=4, 12 mod 5=2, 4 mod 5=4

Which matches the expected output: 4 2 4

So, it works in this case as well.

Given that it works for all the test cases I've tried, including ones where m is not a prime and elements are not coprime with m, it seems that this approach is correct.

But I still don't understand why this works. Let's try to find out the mathematical justification.

In the function `func_1`:

- It collects the removed elements in `b`.

- Then, it calculates the cumulative product of `b` in reverse order.

- The reversed `ans` is then returned, which seems to correspond to the product of removed elements up to each step.

But in the examples, this approach gives the correct output, which is the product of the remaining elements at each step.

How is this possible?

Wait, perhaps there's a relationship between the product of removed elements and the product of remaining elements through the total product.

Let’s denote:

- P: product of all elements in the initial array.

- R_i: product of elements removed up to step i.

- Then, the product of remaining elements at step i should be P / R_i.

But in modular arithmetic, P / R_i is equivalent to P * (R_i^{-1}), assuming R_i has an inverse modulo m.

However, if R_i does not have an inverse modulo m, this approach would fail.

But in the provided program, it's not calculating P / R_i; instead, it's calculating R_i for each step and returning those values.

Wait, no, it's returning the cumulative product of the removed elements in reverse order.

Wait, perhaps I need to look at it differently.

Let’s consider that the product of the remaining elements at each step is equal to P / R_i, but since direct division isn't possible, perhaps there's a different way to look at it.

Wait, perhaps the approach is correct because the product of the remaining elements is equal to the product of all elements divided by the product of the removed elements, and in modular arithmetic, if we consider the cumulative product of removed elements, it might relate to the remaining product in some way.

But I'm still not seeing it clearly.

Let me consider a small example.

Take n=2, m=3, a=[2,1], s=LR

- Initial a: [2,1]

- P = 2*1=2

- s[0] = 'L': remove 2, remaining a: [1]

- Product of remaining: 1

- According to the program:

- b = [2,1]

- reversed b: [1,2]

- ans: [1,2]

- reversed ans: [2,1]

- Output: 2 mod 3=2, 1 mod 3=1

Which matches: 2 1

Now, in this case, the reversed ans seems to correspond to the product of removed elements up to each step.

Wait, in this case:

- Step 0: removed elements up to step 0: [2], product=2

- Step 1: removed elements up to step 1: [2,1], product=2*1=2

- But reversed ans: [2,1]

Wait, no, in the previous step, for n=2, m=3, a=[2,1], s=LR:

- b = [2,1]

- reversed b: [1,2]

- For v in reversed b:

- v=1: p=1*1=1, ans=[1]

- v=2: p=1*2=2, ans=[1,2]

- reversed ans: [2,1]

Which corresponds to the product of all removed elements up to each step, but in reverse order.

Wait, perhaps there's a pattern here that I'm missing.

Let me consider the cumulative product of removed elements in the order they are removed.

For n=2, m=3, a=[2,1], s=LR:

- b = [2,1]

- Cumulative product in order: [2,2]

- But the program returns [2,1], which seems different.

Wait, perhaps it's not directly the cumulative product in order.

Let me look back at the first test case:

n=4, m=6, a=[3,1,4,2], s=LRRL

- b = [3,2,4,1]

- Cumulative product in order: [3,6,24,24]

- But the program returns [24,8,4,1]

Which are 24, 24/3=8, 8/2=4, 4/4=1

Wait, it's like dividing the total product by the cumulative product of removed elements up to that step.

Wait, in the first test case:

- Total product P = 3*1*4*2=24

- Step 0: removed elements up to step 0: [3], R_0=3

- Remaining product: P / R_0 = 24 / 3 = 8

- But 8 mod 6 = 2

- Step 1: removed elements up to step 1: [3,2], R_1=6

- Remaining product: 24 / 6 = 4

- 4 mod 6 = 4

- Step 2: removed elements up to step 2: [3,2,4], R_2=24

- Remaining product: 24 / 24 = 1

- 1 mod 6 = 1

- Step 3: removed elements up to step 3: [3,2,4,1], R_3=24

- Remaining product: 24 / 24 = 1

- 1 mod 6 = 1

But in the program's output: 0 2 4 1

Wait, in the first step, it's 0, which is 24 mod 6=0

Then 2, which is 8 mod 6=2

Then 4, which is 4 mod 6=4

Then 1, which is 1 mod 6=1

So, it seems that the program is calculating P / R_i mod m, where R_i is the product of removed elements up to step i.

But how is the program achieving this without directly dividing?

Wait, perhaps it's because it's calculating R_i in reverse order and then returning the reversed list.

Wait, I'm still confused.

Let me look at the implementation again.

In `func_1`:

- Collect removed elements in `b` in the order they are removed.

- Then, iterate through `b` in reverse, calculating cumulative product in `ans`.

- Finally, return reversed `ans`.

So, effectively, `ans` is the cumulative product of removed elements in the order they were removed.

But in the first test case:

- b = [3,2,4,1]

- reversed b: [1,4,2,3]

- ans: [1,4,8,24]

- reversed ans: [24,8,4,1]

Which corresponds to P / R_i mod m.

But how?

Wait, perhaps P is 24, and:

- 24 / 3 = 8

- 24 / 6 = 4

- 24 / 24 = 1

- 24 / 24 = 1

But the program is calculating R_i in a cumulative way and returning P / R_i using some property of cumulative products.

I think I need to accept that this approach, although counterintuitive to me, is working for all the test cases I've tried.

Therefore, the given program is correct.

**Final Answer**

\[ \boxed{\text{see explanation}} \]