The code calculates two expressions using the variable `n`. Since `n` is an input integer greater than 2 and is even, we can denote `n` as `2k` for some integer `k`, which means `n * n` is `(2k) * (2k) = 4k^2`. 

Now, we evaluate the two expressions:

1. For the first expression: 
   \[
   \frac{n * n}{4} - 1 = \frac{4k^2}{4} - 1 = k^2 - 1
   \]

2. For the second expression:
   \[
   \frac{n * n}{4} + 1 = \frac{4k^2}{4} + 1 = k^2 + 1
   \]

Thus, the output state reflects the values of the expressions based on the even integer `n`. 

Output State: **`n` is an input integer greater than 2 and even; the expressions evaluate to `k^2 - 1` and `k^2 + 1`**.