The code snippet `y -= i - 1` modifies the value of `y` by subtracting `i - 1` from it. The other variables remain unchanged.

Given the initial state:
- `t` is an integer such that 1 ≤ t ≤ 10^4
- `tt` is greater than or equal to 1
- `n`, `x`, and `y` are integers
- `a` is a list of integers sorted in ascending order
- `tmp` is a sorted list containing at least one element
- `y` is greater than or equal to `i - 1`
- `ans` is increased by `i`

After executing `y -= i - 1`, the value of `y` becomes `y - (i - 1)`.

Output State: **`t` is an integer such that 1 ≤ t ≤ 10^4, `tt` is greater than or equal to 1, `n`, `x`, and `y` are integers, `a` is a list of integers sorted in ascending order, `tmp` is a sorted list containing at least one element, `y` is `y - (i - 1)`, and `ans` is increased by `i`.**