Output State: **`i` is 2, `ones[2]` is `ones[1]` + (1 if `nums[0]` == 1 else 0) + (1 if `nums[1]` == 1 else 0), `sum[2]` is `sum[1]` + `nums[0]`**

Explanation: The code updates the value of `ones[i]` to be `ones[i - 1]` plus 1 if `nums[i - 1]` is 1, otherwise 0. Given that `i` is 2, `ones[i]` becomes `ones[1]` plus 1 if `nums[1]` is 1, otherwise 0. The initial state of `ones[2]` is `ones[1]` + (1 if `nums[0]` == 1 else 0), so after the code runs, `ones[2]` becomes `ones[1]` + (1 if `nums[0]` == 1 else 0) + (1 if `nums[1]` == 1 else 0). The value of `sum[2]` remains unchanged as the code does not affect it.