The code appends the value of `x` to the list `B`. The value of `x` is calculated as `B[len(B) - 1] + (idx_B[len(B) - 1] - i) * len(idx_B)`. Since `B` and `idx_B` are non-empty lists, and `i` is defined as `n - 1 - j`, the new element added to `B` is dependent on these variables.

After the execution of the code, `B` will have one additional element, which is the value of `x`.

Output State: **`A = [0, 1, 3], idx_A = [3, 4, 5], B` is a non-empty list with one more element appended, `idx_B` is a non-empty list, `n` must be greater than 0, `i = n - 1 - j`, `s[i] == '<', x = B[len(B) - 2] + (idx_B[len(B) - 2] - i) * len(idx_B)`**

Natural Language Explanation: The list `B` now contains one more element, which is the value of `x`. All other variables remain unchanged except for the updated list `B`.