To determine the new value of `b` after executing the given line of code, we substitute the known values into the expression:

Given:
- `b = 2`
- `idx_B = [2, 1, 0]`
- `x = 1`
- `r = 3`

The expression to evaluate is:
```python
b = b - (idx_B[x] - idx_B[r - 1]) * (x + 1)
```

Substituting the values:
- `idx_B[x]` where `x = 1` gives `idx_B[1] = 1`
- `idx_B[r - 1]` where `r = 3` gives `idx_B[2] = 0`
- `(x + 1)` where `x = 1` gives `(1 + 1) = 2`

So the expression becomes:
```python
b = 2 - (1 - 0) * 2
```
Which simplifies to:
```python
b = 2 - 1 * 2
b = 2 - 2
b = 0
```

Therefore, the new value of `b` is `0`.

All other variables remain unchanged.

Output State: **`A = [0, 1, 3]`, `idx_A = [3, 4, 5]`, `B = [0, 1, 3]`, `idx_B = [2, 1, 0]`, `l = 0`, `r = 3`, `n` is greater than 0, `s[i]` is `'>'`, `a = 0`, `x` is a non-negative integer with the current value of 1, `b = 0`**.