To determine the new state after executing the given code, let's break down the calculation:

Given:
- `A = [0, 1, 3]`
- `idx_A = [3, 4, 5]`
- `B = [0, 1, 3]`
- `idx_B = [2, 1, 0]`
- `l = 0`
- `r = 3`
- `n` is greater than 0
- `s[i]` is `'>'`
- `a = 0`
- `x = 1`
- `b = 0`

The code snippet is:
```python
b = (idx_B[r - 1] - i) * (l + 1)
```

From the given information, we know:
- `r = 3`
- `idx_B = [2, 1, 0]`
- `l = 0`
- `i` is not explicitly defined in the initial state, but since `s[i]` is `'>'`, we can infer that `i` is an index within the bounds of the arrays involved. However, since `i` is not specified, we'll assume it's provided in the context of the loop or condition that uses `s[i]`. For the sake of this example, let's assume `i` is a valid index, say `i = 0` (since `s[i]` is `'>'` and `i` is used in the context of array indexing).

So, substituting the known values:
- `idx_B[r - 1]` translates to `idx_B[2]` which is `0`
- `i` is assumed to be `0`
- `l + 1` translates to `0 + 1` which is `1`

Thus, the calculation becomes:
```python
b = (0 - 0) * 1
b = 0
```

Since `b` was initially `0` and the calculation results in `0`, `b` remains `0`.

Output State: **`A = [0, 1, 3]`, `idx_A = [3, 4, 5]`, `B = [0, 1, 3]`, `idx_B = [2, 1, 0]`, `l = 0`, `r = 3`, `n` is greater than 0, `s[i]` is `'>'`, `a = 0`, `x = 1`, `b = 0`**