Let's analyze the given code snippet and initial state step by step:

### Initial State:
- `A = [0, 1, 3]`
- `idx_A = [3, 4, 5]`
- `B = [0, 1, 3]`
- `idx_B = [2, 1, 0]`
- `l = 0`
- `r = 3`
- `n` is greater than 0 (the exact value of `n` is not specified, but it doesn't affect the current print statement)
- `s[i]` is `'>'` (the exact index `i` is not specified, but it doesn't affect the current print statement)
- `a = 0`
- `x = 1`
- `b = 0`

### Code Snippet:
```python
print(a * 2 + b * 2 + i + 1, end=' ')
```

### Analysis:
- The expression inside the `print` statement is `a * 2 + b * 2 + i + 1`.
- We know the values of `a` and `b`:
  - `a = 0`
  - `b = 0`
- Therefore, `a * 2 + b * 2` simplifies to `0 * 2 + 0 * 2 = 0`.
- The expression now becomes `0 + i + 1`, which simplifies to `i + 1`.

However, the value of `i` is not explicitly provided in the initial state. Since `i` is used in the expression but not defined, we cannot determine its exact value from the given information. Therefore, the output will depend on the value of `i`.

### Conclusion:
Given the lack of a specific value for `i`, the output will be `i + 1`, where `i` is an undefined variable in the context provided.

Output: **i + 1 (where i is an undefined variable in the context provided)**