To determine the output state, let's evaluate the given code snippet with the provided initial state.

Given:
- `A = [0, 1, 3]`
- `idx_A = [3, 4, 5]`
- `B = [0, 1, 3]`
- `idx_B = [2, 1, 0]`
- `l = 0`
- `r = 3`
- `n` is greater than 0
- `s[i]` is `'>'`
- `l` is not less than `r`, and `r` is not equal to 0

The code snippet is:
```python
a = B[r - 1] + (idx_B[r - 1] - i) * r
```

Since `r` is 3, we substitute `r` into the equation:
```python
a = B[3 - 1] + (idx_B[3 - 1] - i) * 3
a = B[2] + (idx_B[2] - i) * 3
```

From the initial state, we know:
- `B[2]` is `3`
- `idx_B[2]` is `0`

Substituting these values in:
```python
a = 3 + (0 - i) * 3
a = 3 + (-i) * 3
a = 3 - 3 * i
```

Therefore, the value of `a` is `3 - 3 * i`.

The other variables (`A`, `idx_A`, `B`, `idx_B`, `l`, `r`, `n`, and `s[i]`) remain unchanged.

Output State: **`A = [0, 1, 3]`, `idx_A = [3, 4, 5]`, `B = [0, 1, 3]`, `idx_B = [2, 1, 0]`, `l = 0`, `r = 3`, `n` is greater than 0, `s[i]` is `'>'`, `a = 3 - 3 * i`**