To determine the output of the given print statement, let's break down the expression step-by-step using the provided initial state:

Given:
- `A = [0, 1, 3]`
- `idx_A = [3, 4, 5]`
- `B = [0, 1, 3]`
- `idx_B = [2, 1, 0]`
- `l = 0`
- `r = 0`
- `n` is greater than 0
- `s[i]` is not equal to `'>'`
- `l` is not greater than `r` (since `r` is also 0)

The print statement is:
```python
print(n - i + (i - idx_A[l - 1]) * 2, end=' ')
```

Let's analyze the expression inside the `print` function:

1. `l - 1`: Since `l = 0`, this evaluates to `0 - 1 = -1`.
2. `idx_A[l - 1]`: Using the result from the previous step, this becomes `idx_A[-1]`. In Python, negative indexing starts from the end of the list, so `idx_A[-1]` is `5`.
3. `i - idx_A[l - 1]`: This translates to `i - 5`. However, the value of `i` is not provided in the initial state, so we'll keep it as `i - 5`.
4. `(i - idx_A[l - 1]) * 2`: This becomes `(i - 5) * 2`.
5. `n - i + (i - idx_A[l - 1]) * 2`: Substituting the previous results, this becomes `n - i + (i - 5) * 2`.

Simplifying the expression:
- `n - i + (i - 5) * 2` 
- `= n - i + 2i - 10` 
- `= n + i - 10`

Since the exact value of `n` and `i` are not provided, we can only express the output in terms of these variables.

Output: **n + i - 10 (where n is greater than 0 and i is an integer)**