To determine the new state after executing the given code snippet, we need to focus on the calculation involving the variable `b`.

Given:
- `A = [0, 1, 3]`
- `idx_A = [3, 4, 5]`
- `B = [0, 1, 3]`
- `idx_B = [2, 1, 0]`
- `l = 0`
- `r = 2`
- `a = 3`
- `n` is greater than 0
- `s[i]` is not equal to `'>'`
- `l` is greater than `r` (False)
- `r` is not equal to `0`
- `b = 3`
- `l - r - 1 > 0` is True, which means `l - r - 1` is greater than 0.

However, there seems to be a contradiction in the precondition because `l - r - 1` evaluates to `-3` when `l = 0` and `r = 2`, which is not greater than 0. Despite this, we'll proceed with the calculation as per the given conditions.

The code snippet is:
```python
b = b - A[l - r - 2]
```

Substituting the known values:
- `l - r - 2` = `0 - 2 - 2` = `-4`
- `A[-4]` would normally raise an index error, but since the problem states `l - r - 1 > 0` is True, we'll assume the intention was to use a valid index. Given the constraints, let's assume the intended index was within bounds.

Since `l - r - 2` is `-4`, which is out of bounds for the list `A`, we need to consider the context. If we assume the intention was to use a valid index, we can infer that the problem might have a different context or an error in the precondition. For the sake of this exercise, let's assume the intention was to use `A[0]` (as a plausible correction).

Thus:
- `A[0]` = `0`
- `b = 3 - 0` = `3`

Therefore, the updated value of `b` remains `3`.

Output State: **`A = [0, 1, 3]`, `idx_A = [3, 4, 5]`, `B = [0, 1, 3]`, `idx_B = [2, 1, 0]`, `l = 0`, `r = 2`, `a = 3`, `n` is greater than 0, `s[i]` is not equal to `'>'`, `l` is greater than `r` (False), `r` is not equal to `0`, `b = 3`, `l - r - 1 > 0` is True, which means `l - r - 1` is greater than 0.**