To determine the output state, we need to evaluate the expression `b = b + (i - idx_A[l - 1]) * (r + 1)` given the initial state.

Given:
- `A = [0, 1, 3]`
- `idx_A = [3, 4, 5]`
- `B = [0, 1, 3]`
- `idx_B = [2, 1, 0]`
- `l = 0`
- `r = 2`
- `a = 3`
- `n` is greater than 0
- `s[i]` is not equal to `'>'`
- `l` is greater than `r` (False)
- `r` is not equal to `0`
- If `l - r - 1 > 0` is True, then `b` is set to 1. Otherwise, `b` remains unchanged.

Since `l - r - 1 = 0 - 2 - 1 = -3`, which is not greater than 0, `b` remains unchanged initially.

Now, let's evaluate the expression `b = b + (i - idx_A[l - 1]) * (r + 1)`:
- `l = 0`, so `l - 1 = -1`. However, since `idx_A` is indexed from 0 to 2, `idx_A[l - 1]` would be out of bounds. Given the context, we assume `l - 1` should be a valid index, and since `l` is 0, `l - 1` should logically refer to the last element in the list when considering circular indexing or similar logic, but typically in such problems, it's assumed to be an error unless specified otherwise. For the sake of this problem, let's assume it refers to the first element when `l` is 0, which is `idx_A[0] = 3`.
- `r = 2`, so `r + 1 = 3`.
- The expression becomes `b = b + (i - 3) * 3`.

Since the value of `i` is not provided, we cannot compute the exact numerical value of `b`. However, we can express the new value of `b` in terms of `i`.

If `b` was initially 0 (as it was not explicitly set to 1 due to the condition `l - r - 1 > 0` being false), the new value of `b` would be `(i - 3) * 3`.

Output State: **`A = [0, 1, 3]`, `idx_A = [3, 4, 5]`, `B = [0, 1, 3]`, `idx_B = [2, 1, 0]`, `l = 0`, `r = 2`, `a = 3`, `n` is greater than 0, `s[i]` is not equal to `'>'`, `l` is greater than `r` (False), `r` is not equal to `0`, `b = (i - 3) * 3`**.