To determine the output state, let's analyze the given code snippet and the initial state.

The code snippet is:
```python
b = b - B[x]
```

From the initial state, we know:
- `A = [0, 1, 3]`
- `idx_A = [3, 4, 5]`
- `B = [0, 1, 3]`
- `idx_B = [2, 1, 0]`
- `n` is greater than 0
- `s[i]` is either `'>'` or not `'>'`
- `i` is incremented by 1
- `a` is `A[l]` where `l` is an undefined index
- `x` is `r - (l + 2)`
- `b` is `B[r - 1]` which could be `0`, `1`, or `3` depending on the value of `r`

The only variable that changes in the code snippet is `b`. The new value of `b` is calculated as `b - B[x]`.

Since `b` is initially `B[r - 1]` and `x` is `r - (l + 2)`, the new value of `b` will be `B[r - 1] - B[r - (l + 2)]`.

Let's denote the new value of `b` as `b_new`. Therefore, `b_new = B[r - 1] - B[r - (l + 2)]`.

The values of `A`, `idx_A`, `B`, `idx_B`, `n`, `s[i]`, `i`, `a`, `x`, and `r` remain unchanged.

Output State: **`A = [0, 1, 3]`, `idx_A = [3, 4, 5]`, `B = [0, 1, 3]`, `idx_B = [2, 1, 0]`, `n` is greater than 0, `s[i]` is either `'>'` or not `'>'`, `i` is incremented by 1, `a` is `A[l]` where `l` is an undefined index, `x` is `r - (l + 2)`, `b` is `B[r - 1] - B[r - (l + 2)]`**.