To determine the output state, we need to evaluate the expression `a = B[r - 1] + (idx_B[r - 1] - i) * r`. However, the variable `r` is not defined in the initial state, so we cannot compute a specific value for `a`. We can only express `a` in terms of `r`, `i`, `B`, and `idx_B`.

Given:
- `A = [0, 1, 3]`
- `idx_A = [3, 4, 5]`
- `B = [0, 1, 3]`
- `idx_B = [2, 1, 0]`
- `n` is greater than 0
- `s[i]` is either `'>'` or not `'>'`
- `i` is incremented by 1

The new variable `a` is calculated as:
\[ a = B[r - 1] + (idx_B[r - 1] - i) \times r \]

Since `r` is not specified, we cannot determine a numerical value for `a`. However, we know the expression it follows.

Output State: **`A = [0, 1, 3]`, `idx_A = [3, 4, 5]`, `B = [0, 1, 3]`, `idx_B = [2, 1, 0]`, `n` is greater than 0, `s[i]` is either `'>'` or not `'>'`, `i` is incremented by 1, `a = B[r - 1] + (idx_B[r - 1] - i) * r`**.