To determine the output state, we need to evaluate the given code snippet with respect to the initial state provided.

The code snippet is:
```python
a = a + (i - idx_A[l - 1]) * l
```

Given the initial state:
- `A = [0, 1, 3]`
- `idx_A = [3, 4, 5]`
- `B = [0, 1, 3]`
- `idx_B = [2, 1, 0]`
- `n` is greater than 0
- `s[i]` is either `'>'` or not `'>'`
- `i` is incremented by 1
- `r` is decreased by 1
- `a = A[l - 1]`

We need to find the new value of `a`. According to the code, `a` is updated using the formula:
\[ a = a + (i - \text{idx\_A}[l - 1]) \times l \]

From the initial state, we know:
- `a = A[l - 1]`. Since `A = [0, 1, 3]`, the value of `a` depends on the value of `l`.

Let's assume `l` can take values from 1 to 3 (since `A` and `idx_A` have 3 elements).

### Case 1: \( l = 1 \)
- `a = A[0] = 0`
- `idx_A[l - 1] = idx_A[0] = 3`
- New value of `a`:
\[ a = 0 + (i - 3) \times 1 = i - 3 \]

### Case 2: \( l = 2 \)
- `a = A[1] = 1`
- `idx_A[l - 1] = idx_A[1] = 4`
- New value of `a`:
\[ a = 1 + (i - 4) \times 2 = 1 + 2(i - 4) = 2i - 7 \]

### Case 3: \( l = 3 \)
- `a = A[2] = 3`
- `idx_A[l - 1] = idx_A[2] = 5`
- New value of `a`:
\[ a = 3 + (i - 5) \times 3 = 3 + 3(i - 5) = 3i - 12 \]

Since `l` can be 1, 2, or 3, the value of `a` will depend on `l` and `i`.

Other variables (`A`, `idx_A`, `B`, `idx_B`, `n`, `s[i]`, `r`) remain unchanged.

Therefore, the Output State is:
Output State: **`A = [0, 1, 3]`, `idx_A = [3, 4, 5]`, `B = [0, 1, 3]`, `idx_B = [2, 1, 0]`, `n` is greater than 0, `s[i]` is either `'>'` or not `'>'`, `i` is incremented by 1, `r` is decreased by 1, `a` is `i - 3` if `l = 1`, `2i - 7` if `l = 2`, `3i - 12` if `l = 3`**.