To determine the output of the `print` statement, we need to carefully analyze the given initial state and how the variables `a`, `b`, `i`, and `r` are defined and manipulated. Let's break down the information step by step:

### Initial State Recap:
- `A = [0, 1, 3]`
- `idx_A = [3, 4, 5]`
- `B = [0, 1, 3]`
- `idx_B = [2, 1, 0]`
- `n` is greater than 0
- `s[i]` is either `'>'` or not `'>'`
- `i` is incremented by 1
- `r` is decreased by 1
- `a` is defined based on the value of `l`:
  - If `l = 1`, `a = i - 3`
  - If `l = 2`, `a = 2i - 7`
  - If `l = 3`, `a = 3i - 12`
- `b` is updated based on the value of `r` and `l`:
  - If `r - l >= 0`, `b = (B[r] - B[r - l]) - (idx_B[r - l] - i) * (r - l) + (idx_B[r] - i) * l`
  - If `r - l < 0`, `b = B[r] + (idx_B[r] - i) * l`

### Analysis:
1. **Determine `i` and `r`:**
   - Since `i` is incremented by 1 and `r` is decreased by 1, let's assume initial values for `i` and `r`. Without specific initial values, we can assume `i` starts at 0 and `r` starts at the length of `B` minus 1 (which is 2).
   - After one iteration, `i = 1` and `r = 1`.

2. **Determine `a`:**
   - We need the value of `l` to determine `a`. Let's assume `l` is given or can be derived from the context. For this example, let's assume `l = 1` (since no specific value is given, we can choose any valid value for demonstration).
   - If `l = 1`, then `a = i - 3 = 1 - 3 = -2`.

3. **Determine `b`:**
   - We need to check the condition `r - l >= 0`:
     - Here, `r = 1` and `l = 1`, so `r - l = 0` which is `>= 0`.
     - Therefore, `b = (B[r] - B[r - l]) - (idx_B[r - l] - i) * (r - l) + (idx_B[r] - i) * l`
     - Substituting the values:
       - `B[r] = B[1] = 1`
       - `B[r - l] = B[0] = 0`
       - `idx_B[r - l] = idx_B[0] = 2`
       - `idx_B[r] = idx_B[1] = 1`
       - `r - l = 0`
       - `l = 1`
       - So, `b = (1 - 0) - (2 - 1) * 0 + (1 - 1) * 1 = 1 - 0 + 0 = 1`.

4. **Calculate the expression to be printed:**
   - The expression is `a * 2 + b * 2 + i + 1`.
   - Substituting the values:
     - `a = -2`
     - `b = 1`
     - `i = 1`
     - So, `a * 2 + b * 2 + i + 1 = (-2) * 2 + 1 * 2 + 1 + 1 = -4 + 2 + 1 + 1 = 0`.

### Final Output:
Based on the above calculations, the output of the `print` statement will be:
Output: **0**