To determine the new state after executing the given code, let's analyze the variables involved and the operation performed:

- Initial State: 
  - `A = [0, 1, 3]`
  - `idx_A = [3, 4, 5]`
  - `B = [0, 1, 3]`
  - `idx_B = [2, 1, 0]`
  - `n` is greater than 0
  - `s[i]` is either `'>'` or not `'>'`
  - `i` is 1
  - `a` is `B[r - 1] + (idx_B[r - 1] - i) * r`
  - `b` is `A[l - 1]`

The code snippet modifies `b` as follows:
```python
b = b - A[l - r - 1]
```

From the initial state, we know:
- `b` is `A[l - 1]`
- The new value of `b` is `A[l - 1] - A[l - r - 1]`

However, the values of `l` and `r` are not specified in the initial state. To proceed, we need to assume plausible values for `l` and `r` that fit within the bounds of the lists `A` and `B`.

Let's assume:
- `l` is 3 (since `A` has 3 elements)
- `r` is 1 (a common small value for demonstration)

Given these assumptions:
- `b` is initially `A[l - 1]` which is `A[2]` = 3
- The new value of `b` is `A[2] - A[2 - 1 - 1]` = `A[2] - A[0]` = 3 - 0 = 3

Since the value of `b` does not change in this specific example, the output state remains the same for `b`. However, the general form of the output state considering the operation would be:

Output State: **`A = [0, 1, 3]`, `idx_A = [3, 4, 5]`, `B = [0, 1, 3]`, `idx_B = [2, 1, 0]`, `n` is greater than 0, `s[i]` is either `'>'` or not `'>'`, `i` is 1, `a` is `B[r - 1] + (idx_B[r - 1] - i) * r`, `b` is `A[l - 1] - A[l - r - 1]`**

For the assumed values of `l` and `r`:
Output State: **`A = [0, 1, 3]`, `idx_A = [3, 4, 5]`, `B = [0, 1, 3]`, `idx_B = [2, 1, 0]`, `n` is greater than 0, `s[i]` is either `'>'` or not `'>'`, `i` is 1, `a` is `B[r - 1] + (idx_B[r - 1] - i) * r`, `b` is 3**