Let's break down the given information and the print statement step-by-step to determine the output:

### Initial State:
- `A = [0, 1, 3]`
- `idx_A = [3, 4, 5]`
- `B = [0, 1, 3]`
- `idx_B = [2, 1, 0]`
- `n` is greater than 0 (but the specific value of `n` is not needed for this calculation).
- `s[i]` is either `'>'` or not `'>'` (the specific value of `s[i]` is not needed for this calculation).
- `i = 1`
- `b = 3`
- `a` is determined by the value of `l`:
  - If `l = 1`, then `a = -2`
  - If `l = 2`, then `a = -6`
  - If `l = 3`, then `a = -12`

### Print Statement:
```python
print(a * 2 + b * 2 + i + 1, end=' ')
```

### Analysis:
To determine the output, we need to know the value of `a`. Since the value of `l` is not specified, we cannot determine the exact value of `a`. However, we can express the output in terms of `a`.

Given:
- `a` can be `-2`, `-6`, or `-12` depending on the value of `l`.
- `b = 3`
- `i = 1`

Let's calculate the expression `a * 2 + b * 2 + i + 1` for each possible value of `a`:

1. If `a = -2`:
   \[
   a * 2 + b * 2 + i + 1 = (-2) * 2 + 3 * 2 + 1 + 1 = -4 + 6 + 1 + 1 = 4
   \]

2. If `a = -6`:
   \[
   a * 2 + b * 2 + i + 1 = (-6) * 2 + 3 * 2 + 1 + 1 = -12 + 6 + 1 + 1 = -4
   \]

3. If `a = -12`:
   \[
   a * 2 + b * 2 + i + 1 = (-12) * 2 + 3 * 2 + 1 + 1 = -24 + 6 + 1 + 1 = -16
   \]

Since the exact value of `l` (and thus `a`) is not provided, the output can be one of these three values. However, we can describe the output in terms of `a`.

### Final Output:
Output: **a * 2 + b * 2 + i + 1 (where a is -2, -6, or -12 depending on the value of l, b is 3, and i is 1)**

This description captures all possible outputs based on the given conditions.