Let's break down the initial state and the print statement step by step:

1. **Initial State Variables:**
   - `t` is an integer within the range 1 to 500.
   - `_` is 2.
   - `p1`, `p2`, `p3` are integers such that their sum is even and `p3` is less than or equal to `p1 + p2`.
   - `x` is 0.
   - `y` is `p3 - 1` and `y` must be greater than or equal to `x`.

2. **Expression to Evaluate:**
   - The expression to evaluate is `p1 - x + p3`.

Given these conditions:
- Since `x` is 0, the expression simplifies to `p1 + p3`.
- `y` is defined as `p3 - 1`, and it must be greater than or equal to `x` (which is 0). This means `p3 - 1 >= 0`, so `p3` must be at least 1.

Since `p1`, `p2`, and `p3` must have an even sum and `p3` is less than or equal to `p1 + p2`, let's consider a simple example where `p1 = 1`, `p2 = 1`, and `p3 = 1` (since 1 + 1 + 1 = 3, which is odd, we need to adjust to make the sum even, e.g., `p1 = 1`, `p2 = 1`, `p3 = 2`).

For simplicity, let's assume `p1 = 1`, `p2 = 1`, and `p3 = 2`:
- `p1 + p3 = 1 + 2 = 3`.

However, since the sum needs to be even, we can adjust to `p1 = 2`, `p2 = 1`, and `p3 = 1`:
- `p1 + p3 = 2 + 1 = 3` (still not even).
- Adjusting further to `p1 = 2`, `p2 = 2`, and `p3 = 2`:
- `p1 + p3 = 2 + 2 = 4` (even).

Thus, a valid set of values could be `p1 = 2`, `p2 = 2`, and `p3 = 2`.

Therefore, the expression `p1 - x + p3` evaluates to `2 - 0 + 2 = 4`.

Output: **4**