Postcondition: `ol` is `totalOne`, `zr` is `len(suffZero) - 1`, `el` is equal to `s1[1]`, `totalOne` is unchanged, `suffZero` is unchanged, `preOne` is unchanged, `ans` is unchanged, `zeroInd` and `oneInd` are calculated differently based on the condition `ol <= zr`. If `ol <= zr`, then `zeroInd = 2 * func_1(suffZero, totalOne)` and `oneInd = 2 * preOne[-1] - func_1(preOne, 1)`, leading to `ans[2] = zeroInd - oneInd`. Otherwise, `zeroInd = 2 * suffZero[-1]` and `oneInd = func_1(preOne, 1) + func_1(preOne, zr + 1) - func_1(preOne, zr)`, resulting in `ans[i] = zeroInd - oneInd + n + 1 - fi` where `i` is 3. `fi` is unchanged and `n` remains unchanged.