The code `dp[j] += dp[j - 1]` updates the value of `dp[j]` by adding the value of `dp[j - 1]` to it. Given the initial conditions:

- `n` is an integer such that \(2 \leq n \leq 10^6\)
- `f_max_n` is an integer representing the maximum value of \(f(p)\) for permutations of length `n`
- `MOD` is 10
- `dp` is a list of length `f_max_n + 1` initialized to 0 with `dp[0] = 1` and `dp[f_max_n] = dp[f_max_n] % 10`
- `j` is `f_max_n - 2`
- `dp[j]` is `(dp[f_max_n - 3] + dp[f_max_n - 2]) % 10`

The operation `dp[j] += dp[j - 1]` modifies `dp[j]` to include the value of `dp[j - 1]`. Specifically:

- Initially, `dp[j]` is \((dp[f_max_n - 3] + dp[f_max_n - 2]) \% 10\).
- After the operation, `dp[j]` becomes \(((dp[f_max_n - 3] + dp[f_max_n - 2]) \% 10) + dp[j - 1] \mod 10\).

Since `j` is `f_max_n - 2`, `j - 1` would be `f_max_n - 3`. Therefore, the updated value of `dp[j]` is:

\[ dp[j] = ((dp[f_max_n - 3] + dp[f_max_n - 2]) \% 10 + dp[f_max_n - 3]) \% 10 \]

Other variables remain unchanged.

Output State: **`n` is an integer such that \(2 \leq n \leq 10^6\), `f_max_n` is an integer representing the maximum value of \(f(p)\) for permutations of length `n`, `MOD` is 10, `dp` is a list of length `f_max_n + 1` initialized to 0 with `dp[0] = 1` and `dp[f_max_n] = dp[f_max_n] \% 10`, `j` is `f_max_n - 2`, `dp[j]` is \(((dp[f_max_n - 3] + dp[f_max_n - 2]) \% 10 + dp[f_max_n - 3]) \% 10)**