Let's go through the code step by step:

1. Initial State:
   - `n` is a positive integer such that \(1 \leq n \leq 2 \times 10^9\) and \(n \geq 6\)
   - `count` is 0
   - `a` is `a + 1`, which means `a` was previously calculated as `a + 1`. However, since no specific value is given, we can denote `a` as `a + 1`.
   - `b` is `a`, meaning `b` is also `a + 1`.
   - `rem` is `n - 4`

2. Code Execution:
   ```python
   rem = n - 2 * (a + b)
   ```
   Substitute the values of `a` and `b` into the equation:
   - `a + b` becomes `(a + 1) + (a + 1) = 2a + 2`
   - Therefore, `rem = n - 2 * (2a + 2) = n - 4a - 4`

3. Updated Variables:
   - `n` remains unchanged: \(1 \leq n \leq 2 \times 10^9\) and \(n \geq 6\)
   - `count` remains 0
   - `a` remains `a + 1`
   - `b` remains `a + 1`
   - `rem` is updated to `n - 4a - 4`

Output State: **`n` is a positive integer such that \(1 \leq n \leq 2 \times 10^9\) and \(n \geq 6\); `count` is 0; `a` is `a + 1`; `b` is `a + 1`; `rem` is `n - 4a - 4`**