The code `c += a[i]` increments `c` by the value of `a[i]`. Since `i` is initially 0 and \(i \mod 2 \neq 0\), `i` is odd (let's say `i` is 1 for simplicity, although the exact value doesn't affect the logic). `a` is a list of `n` integers sorted in descending order. Therefore, `a[i]` is the second element in the list (since `i` starts from 0).

Given that the initial state is:
- `n` is an integer where \(1 \leq n \leq 100\)
- `a` is a list of `n` integers sorted in descending order
- `b` is 0
- `c` is 0
- `i` is 0, and \(i \mod 2 \neq 0\)

After executing the line `c += a[i]`, the value of `c` will be the second element of the list `a`.

Output State: **`n` is an integer where \(1 \leq n \leq 100\), `a` is a list of `n` integers sorted in descending order, `b` is 0, `c` is the second element of `a`, `i` is 0 and \(i \mod 2 \neq 0\)**