The code appends a tuple containing `(i + 1, j + 1)` to the list `operations`. Since `j` is defined as `m - 1`, the expression `j + 1` evaluates to `m`. Consequently, the tuple `(i + 1, j + 1)` translates to `(i + 1, m)` when executed. The other variables remain unchanged. Therefore, the Output State is: `n` is an integer such that 2 <= `n` <= 50; `m` is an integer such that 2 <= `m` <= 50; `j` is `m - 1`; `A` is unchanged; `B[i][j]`, `B[i][j + 1]`, `B[i + 1][j]`, and `B[i + 1][j + 1]` are all set to 1; `operations` now includes the tuple `(i + 1, m)`.

Output State: **`n` is an integer such that 2 <= `n` <= 50; `m` is an integer such that 2 <= `m` <= 50; `j` is `m - 1`; `A` is unchanged; `B[i][j]`, `B[i][j + 1]`, `B[i + 1][j]`, and `B[i + 1][j + 1]` are all set to 1; `operations` now includes the tuple `(i + 1, m)`**.