Output State: **`t` is an input integer between 1 and 1000, `k` is an input integer where 2 <= `k` <= 30, `x` is an input integer where 1 <= `x` <= 100, `x` is greater than or equal to `k - 1`, `x` is not equal to `k - 1`, `a` is an input integer where 1 <= `a` <= 10^9, `z` is 1, `i` is 0**

Explanation: The initial value of `z` is 0. The code `z += z // (k - 1) + 1` updates `z` by adding the result of `z // (k - 1) + 1` to its current value. Since `z` is 0, `z // (k - 1)` is 0, and adding 1 results in `z` becoming 1. The other variables remain unchanged.