# Test 1
**Input**: 
```
1
2 1
1 2 2 1
```
**Output**: 
```
2 1
2 1
```
*Explanation*: This is a basic test case where `n = 2` and `k = 1`. The array `a` consists of the integers from 1 to 2, each appearing twice. We select `l = [2, 1]` and `r = [2, 1]`, which satisfy the condition since `2 ^ 1 = 2 ^ 1 = 3`.

# Test 2
**Input**: 
```
1
6 1
6 4 2 1 2 3 1 6 3 5 5 4
```
**Output**: 
```
6 4
1 3
```
*Explanation*: Here, `n = 6` and `k = 1`. The array `a` includes numbers from 1 to 6, each appearing twice. We select `l = [6, 4]` and `r = [1, 3]`, which satisfy the condition since `6 ^ 4 = 1 ^ 3 = 2`.

# Test 3
**Input**: 
```
1
4 1
1 2 3 4 1 2 3 4
```
**Output**: 
```
1 2
3 4
```
*Explanation*: In this case, `n = 4` and `k = 1`. The array `a` includes numbers from 1 to 4, each appearing twice. We select `l = [1, 2]` and `r = [3, 4]`, which satisfy the condition since `1 ^ 2 = 3 ^ 4 = 3`.

# Test 4
**Input**: 
```
1
6 2
5 1 3 3 5 1 2 6 4 6 4 2
```
**Output**: 
```
5 1 3 3
6 4 2 4
```
*Explanation*: Here, `n = 6` and `k = 2`. The array `a` includes numbers from 1 to 6, each appearing twice. We select `l = [5, 1, 3, 3]` and `r = [6, 4, 2, 4]`, which satisfy the condition since `5 ^ 1 ^ 3 ^ 3 = 6 ^ 4 ^ 2 ^ 4 = 0`.

# Test 5
**Input**: 
```
1
2 2
1 2 2 1
```
**Output**: 
```
1 2
2 1
```
*Explanation*: In this case, `n = 2` and `k = 2`. The array `a` includes numbers from 1 to 2, each appearing twice. We select `l = [1, 2]` and `r = [2, 1]`, which satisfy the condition since `1 ^ 2 = 2 ^ 1 = 3`.

# Test 6
**Input**: 
```
1
6 3
6 4 2 1 2 3 1 6 3 5 5 4
```
**Output**: 
```
6 4 2
1 3 5
```
*Explanation*: Here, `n = 6` and `k = 3`. The array `a` includes numbers from 1 to 6, each appearing twice. We select `l = [6, 4, 2]` and `r = [1, 3, 5]`, which satisfy the condition since `6 ^ 4 ^ 2 = 1 ^ 3 ^ 5 = 7`.

# Test 7
**Input**: 
```
1
4 2
1 2 3 4 1 2 3 4
```
**Output**: 
```
1 2 3 4
1 2 3 4
```
*Explanation*: In this case, `n = 4` and `k = 2`. The array `a` includes numbers from 1 to 4, each appearing twice. We select `l = [1, 2, 3, 4]` and `r = [1, 2, 3, 4]`, which satisfy the condition since `1 ^ 2 ^ 3 ^ 4 = 1 ^ 2 ^ 3 ^ 4 = 0`.

# Test 8
**Input**: 
```
1
10 5
1 2 3 4 5 6 7 8 9 10 6 7 8 9 10 5 4 3 2 1
```
**Output**: 
```
6 7 8 9 10
5 4 3 2 1
```
*Explanation*: Here, `n = 10` and `k = 5`. The array `a` includes numbers from 1 to 10, each appearing twice. We select `l = [6, 7, 8, 9, 10]` and `r = [5, 4, 3, 2, 1]`, which satisfy the condition since `6 ^ 7 ^ 8 ^ 9 ^ 10 = 5 ^ 4 ^ 3 ^ 2 ^ 1 = 15`.

# Test 9
**Input**: 
```
1
2 1
1 1 2 2
```
**Output**: 
```
1 2
1 2
```
*Explanation*: In this case, `n = 2` and `k = 1`. The array `a` includes numbers from 1 to 2, each appearing twice. We select `l = [1, 2]` and `r = [1, 2]`, which satisfy the condition since `1 ^ 2 = 1 ^ 2 = 3`.

# Test 10
**Input**: 
```
1
4 2
1 1 2 2 3 3 4 4
```
**Output**: 
```
1 2 3 4
1 2 3 4
```
*Explanation*: Here, `n = 4` and `k = 2`. The array `a` includes numbers from 1 to 4, each appearing twice. We select `l = [1, 2, 3, 4]` and `r = [1, 2, 3, 4]`, which satisfy the condition since `1 ^ 2 ^ 3 ^ 4 = 1 ^ 2 ^ 3 ^ 4 = 0`.

# Test 11
**Input**: 
```
1
6 3
1 1 2 2 3 3 4 4 5 5 6 6
```
**Output**: 
```
1 2 3 4 5 6
1 2 3 4 5 6
```
*Explanation*: In this case, `n = 6` and `k = 3`. The array `a` includes numbers from 1 to 6, each appearing twice. We select `l = [1, 2, 3, 4, 5, 6]` and `r = [1, 2, 3, 4, 5, 6]`, which satisfy the condition since `1 ^ 2 ^ 3 ^ 4 ^ 5 ^ 6 = 1 ^ 2 ^ 3 ^ 4 ^ 5 ^ 6 = 0`.

These test cases cover a range of scenarios including basic and edge cases to ensure the solution's correctness and robustness.