To determine what will be printed by the `print(d2[y] - d2[x])` statement, let's break down the initial state and the relevant parts of the code:

1. **Initial State:**
   - `t` is an integer where 1 ≤ t ≤ 10^4.
   - `i` is 1.
   - `n` is equal to `t` and greater than 0.
   - `l` is a list of integers provided by the user input.
   - `d1` is a defaultdict initialized with default factory `int` and `d1[2]` is 1.
   - `d2` is a defaultdict initialized with default factory `int` and `d2[n - 1]` is 1.
   - `m` must be greater than 1.
   - `j` is 1.
   - `x` and `y` are integers provided by the user input.
   - If `y` > `x`, the condition `y` > `x` holds true.
   - If `y` ≤ `x`, the condition `y` ≤ `x` holds true.

2. **Relevant Variables:**
   - `d2` is a defaultdict with default factory `int`, meaning any key that does not exist in `d2` will return 0.
   - `d2[n - 1]` is explicitly set to 1.

3. **Print Statement Analysis:**
   - The statement `print(d2[y] - d2[x])` will print the difference between the values of `d2[y]` and `d2[x]`.

4. **Possible Values:**
   - Since `d2` is a defaultdict with default factory `int`, if `y` or `x` is not a key in `d2`, the value will be 0.
   - The only explicitly set key in `d2` is `n - 1`, which is set to 1.

5. **Scenarios:**
   - If `y == n - 1` and `x != n - 1`, then `d2[y] = 1` and `d2[x] = 0`, so `d2[y] - d2[x] = 1 - 0 = 1`.
   - If `y != n - 1` and `x == n - 1`, then `d2[y] = 0` and `d2[x] = 1`, so `d2[y] - d2[x] = 0 - 1 = -1`.
   - If both `y` and `x` are not equal to `n - 1`, then `d2[y] = 0` and `d2[x] = 0`, so `d2[y] - d2[x] = 0 - 0 = 0`.
   - If both `y` and `x` are equal to `n - 1`, then `d2[y] = 1` and `d2[x] = 1`, so `d2[y] - d2[x] = 1 - 1 = 0`.

Given these scenarios, the output will depend on the values of `y` and `x` relative to `n - 1`.

Output: **d2[y] - d2[x] (where d2[y] and d2[x] are the values of y and x in the defaultdict d2, respectively, and d2[n - 1] is 1, and all other keys default to 0)**

For a more specific answer:
- If `y == n - 1` and `x != n - 1`, Output: **1**
- If `y != n - 1` and `x == n - 1`, Output: **-1**
- If `y != n - 1` and `x != n - 1`, Output: **0**
- If `y == n - 1` and `x == n - 1`, Output: **0**