The code snippet `cnt[i] = cnt[i - 1]` assigns the value of `cnt[i - 1]` to `cnt[i]`. Given that `i` is 3, this means `cnt[3]` will be set to the value of `cnt[2]`.

From the initial state:
- `i` is 3
- `n` must be greater than 3
- If `numbers[i] == numbers[s]`, then `cnt[2]` is `v + 1`, where `v` is the value of `cnt[1]`. Otherwise, `cnt[2]` is equal to `cnt[1]`

After executing the code snippet:
- `cnt[3]` is now equal to `cnt[2]`

Therefore, the Output State is:
**`i` is 3, `n` must be greater than 3, if `numbers[i] == numbers[s]`, then `cnt[2]` is `v + 1` and `cnt[3]` is `v + 1`, where `v` is the value of `cnt[1]`. Otherwise, `cnt[2]` is equal to `cnt[1]` and `cnt[3]` is equal to `cnt[1]`.**