The code snippet `a[m + 1] += 1` increments the value of `a[m + 1]` by 1. Given the initial conditions, `a[m + 1]` is currently one more than `a[m]`. Therefore, after executing the code, `a[m + 1]` will be two more than `a[m]`.

Let's summarize the changes:

- The value of `a[m + 1]` is increased by 1.
- The values of `a`, `t`, `n`, `m`, `a[m]`, `cnt`, and the conditions \(1 \leq t \leq 10^4\) and \(n \geq m + 2\) remain unchanged.

Thus, the updated values are:

- `a[m + 1]` is now `a[m] + 2`.

The Output State is: **`a` is a list of integers sorted in ascending order, `t` is an integer such that \(1 \leq t \leq 10^4\), `n` must be at least \(m + 2\), `m` is now \(m + 1\), `a[m]` is a value, `a[m + 1]` is a value + 2, `cnt` is 3**.