The code snippet `dp[i] = n - i + dp[i + 1]` updates the value of `dp[i]` based on the values of `n`, `i`, and `dp[i + 1]`. Here's the step-by-step calculation:

- `i` is initially set to `n - 2`.
- `dp` is a list of length `n + 1` initialized with zeros.
- The equation `dp[i] = n - i + dp[i + 1]` is applied to update `dp[i]`.

Since `dp[i + 1]` is the next element in the list, which is `dp[n - 1]`, and given that `dp` is initialized with zeros, `dp[n - 1]` is 0.

Let's substitute the known values into the equation:

- `i = n - 2`
- `dp[i + 1] = dp[n - 1] = 0`

So, the equation becomes:
\[ dp[n - 2] = n - (n - 2) + 0 \]
\[ dp[n - 2] = 2 \]

This means `dp[i]` is updated to 2. All other values of `dp` remain 0 because no other parts of the list have been updated yet.

The output state after this line of code is executed is:
Output State: **`t` is an integer such that \(1 \leq t \leq 500\), `n` is a positive integer, `s` is the value of `data[3]`, `data` is a list of strings resulting from splitting the input read from `sys.stdin.read`, `index` is 4, `num_cases` is a positive integer, `results` is an empty list, `dp` is a list of length `n + 1` with `dp[n - 2] = 2` and all other elements equal to 0, `result` is 0, `i` is `n - 2`.**