Alright, I have this task to verify the correctness of a given Python program based on a problem description. If the program meets all the requirements correctly for every potential case, I should print "True"; otherwise, "False". Partially correct programs are considered incorrect.

First, I need to understand the problem description thoroughly. Let's read it carefully.

Polycarp has a string `s` consisting of lowercase Latin letters. He encodes this string using the following algorithm:

1. Construct a new auxiliary string `r`, which consists of all distinct letters of the string `s`, written in alphabetical order.

2. Then, encode the string `s` by replacing each character in `s` with its symmetric character from the string `r`. That is, the first character of `r` is replaced by the last character of `r`, the second by the second last, and so on.

For example, for `s = "codeforces"`:

- `r = "cdefors"`

- Encoding:

  - 'c' -> 's'

  - 'o' -> 'e'

  - 'd' -> 'r'

  - 'e' -> 'o'

  - 'f' -> 'f'

  - 'o' -> 'e'

  - 'r' -> 'd'

  - 'c' -> 's'

  - 'e' -> 'o'

  - 's' -> 'c'

- So, the encoded string is "serofedsoc".

Given the encoded string `b`, the task is to decode it back to the original string `s`.

Input:

- The first line contains an integer `t` (1 ≤ t ≤ 10^4) — the number of test cases.

- For each test case:

  - The first line contains an integer `n` (1 ≤ n ≤ 2⋅10^5) — the length of the string `b`.

  - The second line contains the string `b` of length `n`, consisting of lowercase Latin letters — the encoding result of the original string `s`.

- It's guaranteed that the sum of `n` over all test cases doesn't exceed 2⋅10^5.

Output:

- For each test case, output the decoded string `s`.

Now, let's look at the provided program and see if it correctly decodes the encoded strings back to the original strings as per the problem description.

Program code:

```python
import sys
from typing import List

input = sys.stdin.readline
if __name__ == '__main__':
    num_cases = int(input().strip())
    for _ in range(num_cases):
        n = int(input().strip())
        encoded = input().strip()
        decoded = func_1(encoded)
        print(decoded)

def func_1(encoded: str) -> str:
    mapping = {}
    decoded = []
    for char in encoded:
        if char in mapping:
            decoded.append(mapping[char])
        else:
            for c in range(ord('a'), ord('z') + 1):
                if chr(c) not in mapping.values():
                    mapping[chr(c)] = char
                    break
            decoded.append(chr(c))
    return ''.join(decoded)
```

I need to verify if this program correctly decodes any encoded string `b` back to the original string `s` as per the encoding algorithm described.

First, I need to understand the encoding algorithm:

1. Create `r`: sorted unique characters of `s`.

2. Replace each character in `s` with its symmetric character in `r`.

So, for decoding, given `b`, I need to reverse this process:

- Find the string `r` from `b`.

- Map each character in `b` back to its original character in `s` using the symmetric relationship in `r`.

Looking at the provided `func_1`, it seems to be attempting to build a mapping from the encoded characters back to the original characters. However, I need to check if this mapping correctly reverses the encoding process as described.

Let me analyze `func_1`:

- It initializes an empty mapping dictionary and an empty list for the decoded string.

- For each character in the encoded string:

- If the character is already in the mapping, append its mapped value to `decoded`.

- If not, find the first available lowercase letter not yet used in the mapping values, map it to the current encoded character, and append it to `decoded`.

This seems similar to creating a substitution cipher where each unique character in the encoded string is mapped to a unique character not yet used.

But, according to the problem, the encoding is based on the symmetric mapping in `r`. So, the decoding should reverse this symmetric mapping.

Wait a minute, this doesn't seem to be correctly implementing the decoding process as per the problem's encoding algorithm.

Let me think about how the decoding should actually work.

Given the encoded string `b`, to decode it back to `s`, I need to:

1. Determine the string `r` used for encoding.

2. For each character in `b`, find its position in `r` and map it back to the corresponding character in `s`.

But here's the catch: `r` is derived from the original string `s`, which is unknown. However, since `r` consists of unique sorted characters from `s`, and the encoding is a symmetric mapping based on `r`, I need to find a way to reconstruct `r` from `b`.

Wait, since `r` is sorted unique characters from `s`, and the encoding maps each character in `s` to its symmetric counterpart in `r`, then in the encoded string `b`, the unique sorted characters should be the same as `r`, because encoding is a permutation within `r`.

So, `r` can be obtained by extracting all unique characters from `b` and sorting them.

Then, to decode, for each character in `b`, find its position in `r` and map it back to the corresponding character in `s`, which is the symmetric character in `r`.

Wait, but actually, since the encoding is replacing each character in `s` with its symmetric character in `r`, decoding should be the same as encoding, because applying the symmetric mapping twice should return to the original.

Wait, no. Let's think carefully.

If `s` is encoded to `b` by replacing each character in `s` with its symmetric character in `r`, then to decode `b` back to `s`, I need to apply the same symmetric mapping again, because mapping twice should return to the original.

Wait, but is that true?

Let's take an example.

Given `s = "codeforces"`, `r = "cdefors"`, encoding is:

- 'c' -> 's'

- 'o' -> 'e'

- 'd' -> 'r'

- 'e' -> 'o'

- 'f' -> 'f'

- 'o' -> 'e'

- 'r' -> 'd'

- 'c' -> 's'

- 'e' -> 'o'

- 's' -> 'c'

So, `b = "serofedsoc"`

Now, to decode "serofedsoc" back to "codeforces", I need to apply the same symmetric mapping again.

Take 's' -> 'c'

'e' -> 'o'

'r' -> 'd'

'o' -> 'e'

'f' -> 'f'

'e' -> 'o'

'd' -> 'r'

's' -> 'c'

'o' -> 'o'

'c' -> 's'

Wait, that gives "codorfedorcs", which is not the original "codeforces". So, my assumption is incorrect.

Hmm, seems like just applying the symmetric mapping again doesn't give back the original string.

Wait, perhaps I made a mistake in the mapping.

Let's see:

Given `r = "cdefors"`

The symmetric mapping is:

- 'c' -> 's'

- 'd' -> 'r'

- 'e' -> 'o'

- 'f' -> 'f'

- 'o' -> 'e'

- 'r' -> 'd'

- 's' -> 'c'

So, encoding "codeforces" gives "serofedsoc".

Now, to decode "serofedsoc", I need to map each character back using the same mapping:

- 's' -> 'c'

- 'e' -> 'o'

- 'r' -> 'd'

- 'o' -> 'e'

- 'f' -> 'f'

- 'e' -> 'o'

- 'd' -> 'r'

- 's' -> 'c'

- 'o' -> 'o'

- 'c' -> 's'

So, decoded string is "codorfedorcs", which is not "codeforces".

This suggests that just applying the symmetric mapping again doesn't give back the original string. So, my initial assumption is wrong.

Therefore, decoding is not the same as encoding.

Wait, perhaps I need to reverse the mapping.

That is, for decoding, I need to map from the encoded character back to the original character using the same symmetric relationship.

So, in the mapping:

- 'c' -> 's'

- 'd' -> 'r'

- 'e' -> 'o'

- 'f' -> 'f'

- 'o' -> 'e'

- 'r' -> 'd'

- 's' -> 'c'

For decoding, I need a reverse mapping:

- 's' -> 'c'

- 'r' -> 'd'

- 'o' -> 'e'

- 'f' -> 'f'

- 'e' -> 'o'

- 'd' -> 'r'

- 'c' -> 's'

So, in decoding, I need to use the reverse of the symmetric mapping.

In other words, if encoding is mapping each character in `s` to its symmetric counterpart in `r`, then decoding is mapping each character in `b` to its symmetric counterpart in `r`.

Wait, but in the example above, applying the reverse mapping gave me back the original string.

Wait, no, in the above, applying the reverse mapping to "serofedsoc" using the reverse mapping:

- 's' -> 'c'

- 'e' -> 'o'

- 'r' -> 'd'

- 'o' -> 'e'

- 'f' -> 'f'

- 'e' -> 'o'

- 'd' -> 'r'

- 's' -> 'c'

- 'o' -> 'o'

- 'c' -> 's'

Which is "codorfedorcs", which is not "codeforces".

Wait, that's strange.

Wait, perhaps I need to think differently.

Let me think about how to correctly decode.

Given the encoded string `b`, and knowing that `b` is obtained by replacing each character in `s` with its symmetric character in `r`, I need to map each character in `b` back to its original character in `s` using the same symmetric mapping.

So, to decode, I need to apply the symmetric mapping again, but apparently, in the example, it didn't work.

Wait, perhaps I made a mistake in constructing `r`.

Let me double-check.

Given `s = "codeforces"`, `r = "cdefors"`.

Symmetric mapping:

- 'c' -> 's'

- 'd' -> 'r'

- 'e' -> 'o'

- 'f' -> 'f'

- 'o' -> 'e'

- 'r' -> 'd'

- 's' -> 'c'

So, encoding "codeforces" gives "serofedsoc".

Now, to decode "serofedsoc", I need to apply the same mapping:

- 's' -> 'c'

- 'e' -> 'o'

- 'r' -> 'd'

- 'o' -> 'e'

- 'f' -> 'f'

- 'e' -> 'o'

- 'd' -> 'r'

- 's' -> 'c'

- 'o' -> 'o'

- 'c' -> 's'

Which is "codorfedorcs", which is not "codeforces".

Wait, that's odd.

But according to the problem, encoding and decoding should be inverses of each other.

Perhaps I'm misunderstanding the symmetric mapping.

Let me think differently.

Suppose `r` has length `k`. Then, the symmetric mapping pairs the first character with the last, the second with the second last, and so on.

So, to decode, I need to map each character in `b` to the character in `s` that was encoded to it.

But since the encoding is based on `r`, which is unique sorted characters from `s`, and `b` is encoded from `s` using `r`, perhaps I can reconstruct `r` from `b` because `b` should contain the same unique characters as `s`, just encoded.

Wait, yes, `b` is encoded from `s` using `r`, which is the sorted unique characters of `s`. So, the unique sorted characters of `b` should be the same as `r`.

Therefore, for decoding, I can:

1. Extract the unique sorted characters from `b` to get `r`.

2. For each character in `b`, find its position in `r` and map it to the corresponding character in `r` but from the other end.

Wait, but that's essentially applying the symmetric mapping again.

In the earlier example, that gave me "codorfedorcs" instead of "codeforces". So, perhaps there's a mistake in this approach.

Wait, perhaps the issue is that the mapping is not one-to-one in all cases.

Wait, in the symmetric mapping, each character in `r` is mapped to another unique character in `r`, so it should be a bijection.

So, applying the mapping twice should return to the original character.

Wait, in the example:

- 'c' -> 's' -> 'c'

- 'd' -> 'r' -> 'd'

- 'e' -> 'o' -> 'e'

- 'f' -> 'f' -> 'f'

- 'o' -> 'e' -> 'o'

- 'r' -> 'd' -> 'r'

- 's' -> 'c' -> 's'

So, for each character, applying the mapping twice returns to the original.

But in the decoding process, when I applied the mapping to "serofedsoc", I got "codorfedorcs", which is not "codeforces".

Wait, perhaps I made a mistake in applying the mapping.

Let me map "serofedsoc" back using the symmetric mapping:

- 's' -> 'c'

- 'e' -> 'o'

- 'r' -> 'd'

- 'o' -> 'e'

- 'f' -> 'f'

- 'e' -> 'o'

- 'd' -> 'r'

- 's' -> 'c'

- 'o' -> 'o'

- 'c' -> 's'

So, "codorfedorcs", which is not "codeforces".

Wait, that's strange. There must be a mistake in this approach.

Wait, perhaps the issue is that the mapping is based on the position in `r`, and when there are an even number of characters, the mapping is straightforward, but with an odd number, there might be a central character that maps to itself.

In the example, `r = "cdefors"`, which has 7 characters:

Positions:

0: 'c' -> 6: 's'

1: 'd' -> 5: 'r'

2: 'e' -> 4: 'o'

3: 'f' -> 3: 'f'

So, 'f' maps to itself.

This seems correct.

But applying the mapping twice should return to the original.

Wait, in the example, it didn't.

Wait, perhaps I made a mistake in the mapping.

Wait, "serofedsoc" mapped back:

- 's' -> 'c'

- 'e' -> 'o'

- 'r' -> 'd'

- 'o' -> 'e'

- 'f' -> 'f'

- 'e' -> 'o'

- 'd' -> 'r'

- 's' -> 'c'

- 'o' -> 'o'

- 'c' -> 's'

So, "codorfedorcs"

But the original is "codeforces"

Wait, perhaps the issue is that the mapping is correct, but I have repeated characters in `s`.

Wait, in "codeforces", the second 'o' should map to 'e', and in the decoded string, it's 'o', which matches.

Wait, but in the decoded string "codorfedorcs", the fifth character is 'f', which should correspond to 'f' in "codeforces", which is correct.

Wait, but the fourth character is 'd', which should be 'e'.

Wait, perhaps I messed up the mapping.

Wait, no, 'o' maps to 'e', and 'e' maps to 'o'.

Wait, in the mapping:

- 'c' -> 's'

- 'd' -> 'r'

- 'e' -> 'o'

- 'f' -> 'f'

- 'o' -> 'e'

- 'r' -> 'd'

- 's' -> 'c'

So, in "serofedsoc":

- 's' -> 'c'

- 'e' -> 'o'

- 'r' -> 'd'

- 'o' -> 'e'

- 'f' -> 'f'

- 'e' -> 'o'

- 'd' -> 'r'

- 's' -> 'c'

- 'o' -> 'o'

- 'c' -> 's'

So, "codorfedorcs"

But "codeforces" is "c o d e f o r c e s"

Positions:

1. c -> s

2. o -> e

3. d -> r

4. e -> o

5. f -> f

6. o -> e

7. r -> d

8. c -> s

9. e -> o

10. s -> c

So, "s e r o f e d s o c"

Wait, no, in the example, it's "serofedsoc", which is 10 characters: 's','e','r','o','f','e','d','s','o','c'

Mapping back:

- 's' -> 'c'

- 'e' -> 'o'

- 'r' -> 'd'

- 'o' -> 'e'

- 'f' -> 'f'

- 'e' -> 'o'

- 'd' -> 'r'

- 's' -> 'c'

- 'o' -> 'o'

- 'c' -> 's'

So, "c o d e f o r c o s"

Which is "codeforcos", not "codeforces".

Wait, that's different from what I wrote earlier.

Wait, perhaps I miscounted.

Wait, "serofedsoc" has 10 characters: s,e,r,o,f,e,d,s,o,c

Mapping back:

- s -> c

- e -> o

- r -> d

- o -> e

- f -> f

- e -> o

- d -> r

- s -> c

- o -> o

- c -> s

So, "c o d e f o r c o s"

Which is "codeforcos", not "codeforces".

So, there's a mistake somewhere.

Wait, perhaps the mapping is incorrect.

Wait, in the encoding, 'e' in position 4 is mapped to 'o', and 'o' is mapped to 'e'.

But in the decoded string, the eighth character is 's', which should correspond to 'c', but in "codeforces", it's 'c'.

Wait, but in "codeforces", the tenth character is 's', which is mapped to 'c'.

Wait, perhaps I need to map back correctly.

Wait, maybe I need to map each character in `b` to the character in `s` that was encoded to it.

But according to the encoding process, each character in `s` is replaced by its symmetric character in `r`.

So, to decode, I need to replace each character in `b` by its symmetric character in `r`.

Wait, but in the example, that's not giving me back the original string.

Wait, perhaps I need to think about the positions in `r`.

Let's index `r` from 0 to len(r)-1.

For each character in `s`, find its index in `r`, and replace it with the character at position len(r)-1 - index in `r`.

So, to decode, for each character in `b`, find its index in `r`, and replace it with the character at position len(r)-1 - index in `r`.

Wait, but that's the same as the encoding step.

So, encoding and decoding are the same operation.

But in the example, applying it twice doesn't give back the original string.

Wait, perhaps there's a misunderstanding.

Let me try to formalize it.

Let `r` be the sorted unique characters of `s`.

Let `m` be the length of `r`.

For each character in `s`, find its index `i` in `r` (0-based), and replace it with `r[m-1-i]`.

To decode, for each character in `b`, find its index `j` in `r`, and replace it with `r[m-1-j]`.

So, applying this decoding step should give back `s`.

But in the example, it's not working.

Wait, perhaps I need to reconstruct `r` from `b`.

Given `b`, which is encoded from `s` using `r`, and `r` is the sorted unique characters of `s`, which is the same as the sorted unique characters of `b`, since encoding is a permutation within `r`.

So, from `b`, extract `r` by sorting its unique characters.

Then, for each character in `b`, find its position in `r` and map it to `r[m-1-j]`.

This should give back `s`.

But in the example, it's not working.

Wait, perhaps I need to look at another example.

Take `s = "fft"`, `r = "ft"`, encoding:

- 'f' -> 't'

- 'f' -> 't'

- 't' -> 'f'

So, `b = "ttf"`

Now, to decode "ttf":

- 't' -> 'f'

- 't' -> 'f'

- 'f' -> 't'

So, "fft", which matches the original `s`.

So, in this case, it works.

Another example: `s = "algorithm"`, `r = "aghlmoirt"`

Wait, sorted unique characters of "algorithm" are "aghilmort", so `r = "aghilmort"`

Symmetric mapping:

- 'a' -> 't'

- 'g' -> 'r'

- 'h' -> 'o'

- 'i' -> 'm'

- 'l' -> 'i'

- 'm' -> 'l'

- 'o' -> 'h'

- 'r' -> 'g'

- 't' -> 'a'

So, encoding "algorithm":

- 'a' -> 't'

- 'l' -> 'i'

- 'g' -> 'r'

- 'o' -> 'h'

- 'r' -> 'g'

- 'i' -> 'm'

- 't' -> 'a'

- 'h' -> 'o'

- 'm' -> 'l'

So, encoded string is "tirhgmagl"

Now, to decode "tirhgmagl":

- 't' -> 'a'

- 'i' -> 'm'

- 'r' -> 'g'

- 'h' -> 'o'

- 'g' -> 'r'

- 'm' -> 'l'

- 'a' -> 't'

- 'g' -> 'r'

- 'l' -> 'i'

So, decoded string is "amgolortri", which is not "algorithm".

Wait, that's incorrect.

This suggests that simply applying the symmetric mapping again doesn't give back the original string.

Wait, but in the previous example, it did work.

Wait, perhaps I made a mistake in constructing `r`.

Let me check.

For `s = "algorithm"`, unique sorted characters are "aghilmort", so `r = "aghilmort"`

Symmetric mapping:

- 'a' -> 't'

- 'g' -> 'r'

- 'h' -> 'o'

- 'i' -> 'm'

- 'l' -> 'i'

- 'm' -> 'l'

- 'o' -> '