Based on the initial state provided:

- `cnt` is `0`
- `l` is `func_2() + 1`
- The condition `(cnt == 0 and l == n + 1)` holds true

Given this information, let's break down the print statement:

- The `print` statement is `print('! -1', flush=True)`
- `'! -1'` is a string that will be printed
- `flush=True` ensures the output is flushed immediately

Since the condition `(cnt == 0 and l == n + 1)` holds true, we know that `l` must be equal to `n + 1`. Given that `l = func_2() + 1`, it implies that `func_2()` returns `n`.

Therefore, the print statement will output the string `! -1`.

Output: **! -1**