Output State: **After all iterations of the loop, `cnt` is `0`, `l` is `func_2() + 1`, and the condition `(cnt == 0 and l == func_2() + 2)` holds true.**

Explanation: The function `func_2()` is called, and its return value is used to update the variable `l`. Since the initial state had `l` as `func_2() + 1`, calling `func_2()` again updates `l` to `func_2() + 1 + 1`, which simplifies to `func_2() + 2`. The conditions involving `cnt` remain unchanged as `cnt` was initially `0` and no operation altered it.