The code snippet `ans += dif2` increments the value of `ans` by the value of `dif2`. Given the initial state, `dif2` is defined as `abs(a[a1] - b[b2])`.

Therefore, the updated value of `ans` is `ans + abs(a[a1] - b[b2])`.

The rest of the variables and conditions remain unchanged.

Output State: **`t` is an input integer where 0 ≤ t ≤ 99, `n` and `m` are integers where 1 ≤ n ≤ m ≤ 2 * 10^5, the sum of `m` over all test cases does not exceed 2 * 10^5, `a` is a sorted list of integers, `b` is a sorted list of integers read from user input, `dif1` is `abs(a[a1] - b[b1])`, `dif2` is `abs(a[a1] - b[b2])`, `dif3` is `abs(a[a2] - b[b1])`, `dif4` is `abs(a[a2] - b[b2])`, `a1` is less than or equal to `a2`, `b1` and `b2` are as set in the if-else block, and `ans` is now `ans + abs(a[a1] - b[b2])`.**