In the given code, `triangular_num` is calculated as `idx * (idx + 1) // 2`. Given that `idx` is 1, we can substitute this value into the expression.

Calculating `triangular_num`:
- `triangular_num = 1 * (1 + 1) // 2`
- `triangular_num = 1 * 2 // 2`
- `triangular_num = 2 // 2`
- `triangular_num = 1`

Thus, `triangular_num` becomes 1.

The other variables, `n` and `idx`, remain unchanged. 

Therefore, the output state is:
Output State: **`n` is a positive integer representing the number of digits; `idx` is 1; `triangular_num` is 1**.