Let's break down the initial state and the print statement step by step:

1. **Initial State:**
   - `p1`, `p2`, and `p3` are integers provided by user input.
   - `p1` ≤ `p2` ≤ `p3` ≤ 30.
   - The sum of `p1`, `p2`, and `p3` is odd.
   - `t` is greater than 2 (but not used in the print statement).
   - `_` is 2 (but not used in the print statement).
   - `x` is 0.
   - `y` is equal to `p3`.
   - The difference between `p1` and `x` is less than or equal to the difference between `p2` and `y`.

2. **Print Statement:**
   - `print(p1 - x + p3)`

3. **Variable Values:**
   - `x` is 0.
   - `y` is `p3`.
   - `p1 - x` simplifies to `p1 - 0`, which is just `p1`.
   - Therefore, `p1 - x + p3` simplifies to `p1 + p3`.

4. **Conditions:**
   - `p1` ≤ `p2` ≤ `p3` ≤ 30.
   - The sum of `p1`, `p2`, and `p3` is odd.
   - The difference between `p1` and `x` (which is `p1`) is less than or equal to the difference between `p2` and `y` (which is `p2 - p3`).

5. **Analysis:**
   - Since `x` is 0, `p1 - x` is simply `p1`.
   - The print statement will output `p1 + p3`.
   - The condition `p1 - x <= p2 - y` translates to `p1 <= p2 - p3`. Given that `p1` ≤ `p2` and `p2` ≤ `p3`, this condition is always true because `p2 - p3` is non-positive (since `p2` ≤ `p3`).

6. **Conclusion:**
   - The print statement will output the sum of `p1` and `p3`.

Output: **p1 + p3 (where p1 and p3 are integers such that p1 ≤ p2 ≤ p3 ≤ 30 and the sum of p1, p2, and p3 is odd)**