Alright, I've got this problem to solve. Let's see what it's asking for. So, Nikita has a three-letter word, all lowercase Latin letters, and he encodes it by summing up the positions of each letter in the alphabet. For example, "cat" is 3 + 1 + 20 = 24. But this encoding is ambiguous because other words can have the same sum, like "ava" also sums to 24. Now, given the sum, I need to find the lexicographically smallest three-letter word that could have resulted in that sum.

First, I need to understand what lexicographical order means. It's basically dictionary order. So, the smallest word is the one that would appear first in the dictionary. That means preferring letters as early in the alphabet as possible.

Given that, I need a strategy to assign letters to the three positions in the word such that their positions are as small as possible, but the sum is still equal to the given number n.

Let's think about the constraints. Each letter corresponds to a number from 1 to 26. So, each position in the word can have a value between 1 and 26. The total sum n is between 3 and 78, since the smallest sum is 1+1+1=3 and the largest is 26+26+26=78.

I need to distribute the sum n across three letters, minimizing the word lexicographically. That means I should try to minimize the first letter, then the second, and then the third.

One way to approach this is to iterate from the first letter to the third, assigning the smallest possible value to each position and calculating the remaining sum for the subsequent letters.

Let me try to formalize this:

1. Assign the smallest possible value to the first letter (starting with 'a' which is 1), and then recursively assign the smallest possible values to the remaining letters such that their sum is n minus the value of the first letter.

2. If at any point the remaining sum is impossible to achieve with the remaining letters (i.e., remaining sum is less than the number of letters times 1 or greater than the number of letters times 26), backtrack and increase the current letter's value.

This seems like a recursive approach, but since it's a small problem (only three letters), I can probably do it iteratively as well.

Let me consider the example from the problem: n=24.

I need to find the smallest word that sums to 24.

Start with the first letter as 'a' (1). Then, the remaining sum is 23 for the next two letters.

Now, assign the smallest possible value to the second letter. Let's try 'a' again (1). Then, the third letter would need to be 22, which is 'v'. So, the word is "aav", which sums to 1+1+22=24.

Is there a smaller word than "aav"? If I try to make the first letter 'a', second letter 'a', and third letter 'v', that seems fine. Is there any combination where changing the letters could make it smaller?

If I try to make the first letter 'a', and the second letter 'b' (2), then the third letter would need to be 21, which is 'u'. So, "abu" sums to 1+2+21=24, but "abu" is lexicographically larger than "aav" because 'b' comes after 'a'.

Similarly, if I make the first letter 'a', and the second letter 'a', and third letter 'v', that's "aav", which is smaller.

So, "aav" seems correct for n=24.

Another example: n=70.

I need to find the smallest word that sums to 70.

Start with the first letter as 'a' (1). Then, the remaining sum is 69 for the next two letters.

Assign the smallest possible value to the second letter, which is 'a' (1). Then, the third letter would need to be 68, but 'z' is only 26, so that's not possible.

So, increase the second letter. If second letter is 'b' (2), third letter needs to be 67, still too big.

Continue increasing the second letter until the third letter is within 1 to 26.

So, second letter as 'z' (26), then third letter needs to be 69 - 26 = 43, which is still too big.

Wait, 69 - 26 = 43, but 43 is larger than 26, which is invalid.

So, need to increase the first letter.

Make first letter 'b' (2). Then, remaining sum is 68 for the next two letters.

Second letter 'z' (26), third letter needs to be 68 - 26 = 42, still too big.

Continue increasing the first letter.

First letter 'c' (3), remaining sum 67.

Second letter 'z' (26), third letter 67 - 26 = 41, still too big.

Continue this way until the remaining sum for two letters is between 2 and 52 (since 1+1=2 and 26+26=52).

Eventually, when first letter is 'r' (18), remaining sum is 70 - 18 = 52.

Second letter 'z' (26), third letter 52 - 26 = 26, which is 'z'.

So, "rzz" sums to 18+26+26=70.

Is there a smaller word than "rzz"? If I try first letter 'q' (17), remaining sum 70 - 17 = 53.

But 53 is greater than 52, which is not possible with two letters. So, 'r' is the smallest possible first letter.

Hence, "rzz" is correct.

Another example: n=3.

Smallest possible sum, which is 'aaa' (1+1+1=3). So, that's straightforward.

n=55.

First letter 'a' (1), remaining sum 54 for two letters.

Second letter 'a' (1), third letter 53, which is invalid.

Increase second letter to 'z' (26), third letter 54 - 26 = 28, which is invalid.

Increase first letter to 'b' (2), remaining sum 53.

Second letter 'z' (26), third letter 53 - 26 = 27, which is invalid.

Continue increasing first letter.

First letter 'c' (3), remaining sum 52.

Second letter 'z' (26), third letter 52 - 26 = 26, which is 'z'.

So, "czz" sums to 3+26+26=55.

But the example output shows "a uz", which sums to 1 + 21 + 26 = 48, but wait, n=55 is supposed to be "czz".

Wait, in the example, for n=48, it's "auz" (1 + 21 + 26 = 48), but for n=55, it's "czz" (3 + 26 + 26 = 55).

Wait, but in the example output, for n=55, it's "czz", but in my calculation, it's "czz". Maybe it's a typo in the explanation.

Anyway, moving on.

I need to generalize this approach.

So, the strategy is:

- Start with the first letter as small as possible.

- Then, for the second letter, start as small as possible given the first letter.

- Finally, the third letter is determined by the remaining sum.

- If the remaining sum for the last letter is within 1 to 26, it's valid; otherwise, adjust the previous letters.

This seems a bit tedious for a program. Maybe there's a smarter way.

Looking at the reference solution:

def func():

alphabet = string.ascii_lowercase

for i in range(int(input())):

n = int(input())

word = ''

if n > 52:

word += alphabet[n - 53] + 'zz'

elif n > 27:

word += 'a' + alphabet[n - 28] + 'z'

elif n == 27:

word = 'aay'

else:

word += 'aa' + alphabet[n - 3]

print(word)

This seems concise, but I need to verify if it works correctly for all cases.

Let's test it with n=24.

According to the code:

n = 24

24 > 52? No.

24 > 27? Yes.

So, word = 'a' + alphabet[24 - 28] + 'z'

24 - 28 = -4, which is invalid for alphabet indexing.

Wait, that can't be right.

Wait, maybe I'm misunderstanding the indexing.

In Python, string.ascii_lowercase is 'abcdefghijklmnopqrstuvwxyz', indexed from 0 to 25.

So, alphabet[n - 28] would be alphabet[-4], which in Python wraps around due to negative indexing.

But alphabet[-1] is 'z', alphabet[-2] is 'y', etc.

So, alphabet[-4] would be 'w'.

But in the example, for n=24, it should be 'aav', not 'a w z'.

Wait, that doesn't match.

Wait, perhaps there's a mistake in the reference solution.

Let's check the example output:

For n=24, output is "aav".

According to the reference solution:

n = 24

24 > 52? No.

24 > 27? Yes.

word = 'a' + alphabet[24 - 28] + 'z'

24 - 28 = -4

alphabet[-4] = 'w'

So, word = 'a' + 'w' + 'z' = "awz", but the correct answer is "aav".

This suggests that the reference solution is incorrect for n=24.

Wait, but in the example, for n=24, it's "aav", not "awz".

So, the reference solution is giving "awz", which is incorrect.

Wait, perhaps I'm misinterpreting the code.

Wait, let's look again.

alphabet = string.ascii_lowercase

n = 24

if n > 52:

word += alphabet[n - 53] + 'zz'

elif n > 27:

word += 'a' + alphabet[n - 28] + 'z'

elif n == 27:

word = 'aay'

else:

word += 'aa' + alphabet[n - 3]

So, for n=24:

n > 52? No.

n > 27? 24 > 27? No.

n == 27? No.

So, it goes to the else clause: word += 'aa' + alphabet[n - 3]

n - 3 = 21

alphabet[21] is 'v'

So, word = 'aa' + 'v' = "aav", which matches the example.

Wait, earlier I thought it would take the elif n > 27 clause, but actually, 24 is not greater than 27, so it takes the else clause.

Okay, my mistake in following the code.

Let's verify for n=70.

n = 70

70 > 52? 52 is 26 + 26 = 52, which is 'zzz' summing to 78 - but wait, 26 + 26 + 26 = 78, 26 + 26 + 25 = 77, etc.

Wait, in the code, for n > 52:

word += alphabet[n - 53] + 'zz'

Wait, n - 53 for n=70: 70 - 53 = 17

alphabet[17] = 'r'

So, word = 'r' + 'zz' = "rzz", which matches the example.

Okay, that seems correct.

Let's check n=3:

n = 3

3 > 52? No.

3 > 27? No.

n == 27? No.

Else clause: word += 'aa' + alphabet[3 - 3] = 'aa' + alphabet[0] = 'aa' + 'a' = "aaa", which is correct.

n=55:

55 > 52? 52 is for 'zzz' which is 78 - wait, 26 + 26 + 26 = 78, so 55 is less than 78.

But the condition is n > 52, which is 55 > 52? Yes.

So, word += alphabet[55 - 53] + 'zz' = alphabet[2] + 'zz' = 'c' + 'zz' = "czz", which seems correct.

But in the example, for n=55, it's "czz", which is the same as "czz". Maybe a typo in the explanation.

n=48:

48 > 52? No.

48 > 27? Yes.

So, word += 'a' + alphabet[48 - 28] + 'z' = 'a' + alphabet[20] + 'z' = 'a' + 'u' + 'z' = "auz", which matches the example.

Okay, so it seems the reference solution is correct.

But earlier I thought there was a mistake, but actually, I misread the code flow.

So, the logic in the reference solution is:

- If n > 52: Assign the first letter as alphabet[n - 53], and the next two letters as 'z'.

- Elif n > 27: Assign the first letter as 'a', the second letter as alphabet[n - 28], and the third letter as 'z'.

- Elif n == 27: Directly assign 'aay'.

- Else: Assign 'aa' followed by alphabet[n - 3].

I need to verify if this covers all possible cases correctly.

Let's consider n=27.

According to the code, word = 'aay', which is correct because 'a' + 'a' + 'y' = 1 + 1 + 25 = 27.

n=28:

n > 52? No.

n > 27? Yes.

word = 'a' + alphabet[28 - 28] + 'z' = 'a' + alphabet[0] + 'z' = 'a' + 'a' + 'z' = "aaz", which sums to 1 + 1 + 26 = 28. Correct.

n=52:

n > 52? 52 > 52? No.

n > 27? Yes.

word = 'a' + alphabet[52 - 28] + 'z' = 'a' + alphabet[24] + 'z' = 'a' + 'x' + 'z' = "axz", which sums to 1 + 24 + 26 = 51, which is less than 52. Wait, that's incorrect.

Wait, there's a mistake here.

For n=52, according to the code, it should go to the n > 27 clause:

word = 'a' + alphabet[52 - 28] + 'z' = 'a' + alphabet[24] + 'z' = 'a' + 'x' + 'z' = "axz", which sums to 1 + 24 + 26 = 51, but n=52.

That's not matching. So, for n=52, the correct word should be 'ayz': 'a' + 'y' + 'z' = 1 + 25 + 26 = 52.

But according to the code, it's producing "axz" which sums to 51.

That seems like an error in the reference solution.

Similarly, for n=53:

n > 52? 53 > 52? Yes.

word = alphabet[53 - 53] + 'zz' = alphabet[0] + 'zz' = 'a' + 'zz' = "azz", which sums to 1 + 26 + 26 = 53. Correct.

Wait, but for n=52, it's producing "axz" which is 51, but it should be "ayz" which is 52.

So, there's an inconsistency here.

Let's see what's going wrong.

The condition for n > 52 is word += alphabet[n - 53] + 'zz'

For n=53, it's 'a' + 'zz' = 1 + 26 + 26 = 53, correct.

For n=52, it should be 'a' + 'y' + 'z' = 1 + 25 + 26 = 52.

But according to the code, for n=52, since 52 > 52 is False, it goes to the n > 27 clause:

word = 'a' + alphabet[52 - 28] + 'z' = 'a' + alphabet[24] + 'z' = 'a' + 'x' + 'z' = "axz" = 1 + 24 + 26 = 51, which is incorrect.

So, for n=52, it's producing "axz" which sums to 51, but it should be "ayz" which sums to 52.

This suggests that the reference solution is flawed for n=52.

Similarly, for n=27, it directly assigns 'aay', which is correct.

For n=28, it assigns "aaz" which sums to 51, but n=52 should be "ayz".

Wait, no, n=28 is different from n=52.

Wait, in n=28, according to the code, it's "aaz" which sums to 1+1+26=28, which is correct.

But for n=52, it should go to the n > 27 clause and produce 'a' + alphabet[24] + 'z' = 'a' + 'x' + 'z' = "axz" which sums to 1+24+26=51, which is less than 52.

So, it's incorrect for n=52.

Wait, but in the initial examples, n=70 is handled correctly as "rzz", which sums to 18+26+26=70.

n=48 is "auz" which is 1+21+26=48, correct.

n=55 is "czz" which is 3+26+26=55, correct.

n=52 should be "ayz" which is 1+25+26=52.

But according to the code, it produces "axz" which is 1+24+26=51.

So, it's off by 1.

Wait, perhaps there's an off-by-one error in the indexing.

Let's check the indexing.

alphabet = string.ascii_lowercase, which is 'abcdefghijklmnopqrstuvwxyz'

alphabet[0] = 'a', alphabet[1] = 'b', ..., alphabet[25] = 'z'

For n > 52:

word += alphabet[n - 53] + 'zz'

For n=53, n - 53 = 0 -> 'a' + 'zz' = "azz" = 1 + 26 + 26 = 53, correct.

For n=52, it should be 'ayz' = 1 + 25 + 26 = 52.

But according to the condition, since 52 > 52 is False, it goes to the n > 27 clause.

So, perhaps the condition should be n >= 53 instead of n > 52.

Wait, let's adjust the condition to n >= 53.

Then, for n=53, it's 'a' + 'zz' = 1 + 26 + 26 = 53, correct.

For n=52, it goes to n > 27 clause.

word = 'a' + alphabet[52 - 28] + 'z' = 'a' + alphabet[24] + 'z' = 'a' + 'x' + 'z' = "axz" = 1 + 24 + 26 = 51, which is still incorrect.

But actually, for n=52, the correct word is 'ayz' = 1 + 25 + 26 = 52.

So, perhaps there's an off-by-one error in the calculation for the second letter.

Wait, let's calculate the required index.

We need to have first letter 'a' (1),