To determine the output state after all iterations of the loop have finished, we need to understand how the loop evolves over time. The loop runs for `x + 1` iterations, and in each iteration, the value of `z` is updated according to the formula `z += z // (k - 1) + 1`.

Let's break down the process:

1. **Initial State**: 
   - `z = 0`
   - The loop runs `x + 1` times.

2. **First Iteration**:
   - `i = 0`
   - `z += z // (k - 1) + 1` → `z = 0 + 0 // (k - 1) + 1` → `z = 1`

3. **Second Iteration**:
   - `i = 1`
   - `z += z // (k - 1) + 1` → `z = 1 + 1 // (k - 1) + 1` → `z = 2 + 1 // (k - 1)`

4. **Third Iteration**:
   - `i = 2`
   - `z += z // (k - 1) + 1` → `z = 2 + 1 // (k - 1) + 1 + (2 + 1 // (k - 1)) // (k - 1) + 1`

This pattern continues until `i = x`. The final value of `z` after `x + 1` iterations can be expressed as the accumulation of the updates in each iteration.

Given the pattern, after `x + 1` iterations, the value of `z` is the result of repeatedly applying the update formula. We can represent the final value of `z` as follows:

- For each iteration `i` from `0` to `x`, `z` is incremented by `z // (k - 1) + 1`.

To find the exact final value of `z`, we need to compute the cumulative effect of these updates. This can be complex to express in a closed form without knowing specific values of `k` and `x`. However, we can describe the final state in terms of the loop's behavior.

**Output State**: **`t` is an integer input such that 0 <= t < 1000; `k`, `x`, and `a` are integers provided in the input with `x` being at least 0; `z` is the result of the loop after `x + 1` iterations where `z` is incremented by `z // (k - 1) + 1` in each iteration; `i` is `x`**

In simpler terms, the final value of `z` is determined by the loop running `x + 1` times, updating `z` in each iteration according to the given formula. The values of `t`, `k`, and `a` remain unchanged as they are not affected by the loop.