To determine the output state, we start by analyzing the provided initial conditions and the impact of the code snippet.

Initial State: 
- `x`, `y`, and `z` are real numbers such that 0.1 ≤ `x`, `y`, `z` ≤ 200.0
- `a1` is equal to `x` raised to the power of `y` raised to the power of `z` (i.e., `a1 = x ** (y ** z)`)
- `a2` is equal to `x` raised to the power of `z` raised to the power of `y` (i.e., `a2 = x ** (z ** y)`)

Code:
```
a3 = (x ** y) ** z
```

Now, let's evaluate the impact of the code:
1. `a3` is assigned the value of `(x ** y) ** z`.
2. The expression `(x ** y) ** z` can be simplified using the power of a power rule: `(a ** b) ** c = a ** (b * c)`, which gives us `a3 = x ** (y * z)`.

The values of `x`, `y`, and `z`, and the calculations for `a1` and `a2` remain unchanged. Therefore, we update only the value of `a3`.

Output State: **`x`, `y`, and `z` are real numbers such that 0.1 ≤ `x`, `y`, `z` ≤ 200.0; `a1` is equal to `x` raised to the power of `y` raised to the power of `z`; `a2` is equal to `x` raised to the power of `z` raised to the power of `y`; `a3` is equal to `x` raised to the power of `y * z`.**