In the given code, `a` is assigned the value of `i * x`. Given the initial state, we have:

- `i` is `k + 1`.
- `k + 1` must be ≤ `int(math.sqrt(z))`.
- `x` is an integer such that 1 ≤ `x`.

Since `i` is `k + 1`, we can write `a = (k + 1) * x`.

The conditions for `l`, `r`, `x`, `y`, and `z` remain unchanged, as they do not directly affect the computation of `a`, and only `a` is updated due to the operation.

Therefore, the Output State will be as follows:

Output State: **`l` and `r` are integers such that 1 ≤ `l` ≤ `r`, `x` is an integer such that 1 ≤ `x`, `y` is an integer such that `x` ≤ `y`, `z` is an integer such that `z` ≥ 4, `i` is `k + 1`, `a` is equal to `(k + 1) * x`.**