Let's break down the given information and the code to determine what will be printed.

### Initial State:
- `t` must be greater than or equal to 1 (though `t` is not used in the provided code snippet, it's mentioned for completeness).
- `n` is an input integer.
- `mat` is a list of `n` lists, where each inner list contains integers from 1 to `n`. However, `mat` is not used in the provided code snippet.
- `res` is the sum of the series \(\sum_{i=0}^{n-1} (i + 1) \cdot (2i + 1)\).
- `i` is set to `n-1`.

### Code to Execute:
```python
print(res, n << 1)
```

### Calculation of `res`:
The variable `res` is the sum of the series \(\sum_{i=0}^{n-1} (i + 1) \cdot (2i + 1)\). Let's expand this series:

\[
\begin{align*}
res &= \sum_{i=0}^{n-1} (i + 1) \cdot (2i + 1) \\
&= \sum_{i=0}^{n-1} (2i^2 + 3i + 1) \\
&= 2\sum_{i=0}^{n-1} i^2 + 3\sum_{i=0}^{n-1} i + \sum_{i=0}^{n-1} 1 \\
&= 2\left(\frac{(n-1)n(2n-1)}{6}\right) + 3\left(\frac{(n-1)n}{2}\right) + n \\
&= \frac{(n-1)n(2n-1)}{3} + \frac{3(n-1)n}{2} + n \\
&= \frac{(n-1)n(4n-2 + 9)}{6} + n \\
&= \frac{(n-1)n(4n+7)}{6} + n \\
&= \frac{(n-1)n(4n+7) + 6n}{6} \\
&= \frac{n((n-1)(4n+7) + 6)}{6} \\
&= \frac{n(4n^2 + 3n - 7 + 6)}{6} \\
&= \frac{n(4n^2 + 3n - 1)}{6}
\end{align*}
\]

### Calculation of `n << 1`:
The expression `n << 1` is a bitwise left shift operation, which is equivalent to multiplying `n` by 2.

### Final Output:
The `print` statement will output the value of `res` and the value of `n << 1`.

Output: **res (where res is the sum of the series \(\frac{n(4n^2 + 3n - 1)}{6}\)), n << 1 (where n << 1 is 2 * n)**