To determine what will be printed by the `print(*a)` statement, let's break down the initial state and the transformations applied to the variables:

### Initial State:
- `n` remains the same.
- `q` remains the same.
- `a` is now a list of cumulative sums of its original values.
- `c` remains the same.
- `b` is a list of length `n + 1` where each element `b[i]` (for `i` from 1 to `n`) is the cumulative sum of `1` or `2` based on the condition `a[i] > 1` starting from `b[0] = 0`.

### Explanation:
1. **`a` is a list of cumulative sums of its original values:**
   - Suppose the original list `a` was `[a1, a2, a3, ..., an]`.
   - The new list `a` will be `[a1, a1 + a2, a1 + a2 + a3, ..., a1 + a2 + a3 + ... + an]`.

2. **`b` is a list of length `n + 1`:**
   - The first element `b[0]` is `0`.
   - For each subsequent element `b[i]` (where `i` ranges from 1 to `n`), the value is the cumulative sum of `1` or `2` based on the condition `a[i] > 1`.
   - If `a[i] > 1`, then `b[i]` is incremented by `2`.
   - If `a[i] <= 1`, then `b[i]` is incremented by `1`.

### Example Calculation:
Let's assume the original list `a` was `[1, 2, 3, 4]`.

1. **Transform `a` to cumulative sums:**
   - `a[0] = 1`
   - `a[1] = 1 + 2 = 3`
   - `a[2] = 1 + 2 + 3 = 6`
   - `a[3] = 1 + 2 + 3 + 4 = 10`
   - So, the new list `a` is `[1, 3, 6, 10]`.

2. **Transform `b` based on `a`:**
   - `b[0] = 0`
   - `b[1] = b[0] + 1` (since `a[1] = 3 > 1`)
   - `b[2] = b[1] + 2` (since `a[2] = 6 > 1`)
   - `b[3] = b[2] + 2` (since `a[3] = 10 > 1`)
   - So, the list `b` is `[0, 1, 3, 5]`.

### Final Output:
The `print(*a)` statement will print the elements of the list `a` separated by spaces. Since `a` is now a list of cumulative sums of its original values, the output will be the cumulative sums of the original values of `a`.

Output: **1 3 6 10 (where the values are the cumulative sums of the original values of list `a`)**

If the original list `a` had different values, the cumulative sums would be different, but the format of the output would remain the same. The output will always be the cumulative sums of the original values of `a` separated by spaces.