Alright, I've got this problem to solve. Let's see what it's asking for. So, Nikita has a three-letter word, all lowercase Latin letters, and he encodes it by summing the positions of each letter in the alphabet. For example, "cat" is 3 + 1 + 20 = 24. But this encoding is ambiguous because other words like "ava" also sum to 24. My task is to, given the sum, find the lexicographically smallest three-letter word that could have resulted in that sum.

First, I need to understand what "lexicographically smallest" means. It means that among all possible combinations of three letters that sum to the given number, I need to find the one that would come first in a dictionary. So, for example, "aav" comes before "ava" because the first two letters are 'a' and 'a', and only the third letter differs.

Okay, so I need to minimize the word in lexicographical order given that the sum of the positions of the three letters is n.

Let's think about the constraints. Each letter is a lowercase Latin letter, so from 'a' to 'z', which correspond to positions 1 to 26.

So, for three letters, the minimum sum is 1 + 1 + 1 = 3 ('aaa'), and the maximum sum is 26 + 26 + 26 = 78 ('zzz'). The problem states that n is between 3 and 78, inclusive, which makes sense.

Now, I need to find the smallest word that sums to n. To make the word lexicographically smallest, I should try to make the first letter as small as possible, then the second, and so on.

Let me consider the first letter. To make the whole word as small as possible, I should choose the smallest possible first letter, which is 'a' if possible.

If I choose 'a' for the first letter, which is 1, then the sum of the next two letters should be n - 1. But the next two letters must each be between 1 and 26, so n - 1 must be between 2 and 52.

Wait, but n can be as small as 3, so n - 1 = 2, which is achievable with two 'a's. And n can be up to 78, but if I choose 'a' for the first letter, n - 1 can be up to 77, which would require the next two letters to sum to 77, which is possible only if both are 'z' (26 + 26 = 52), but 52 < 77, so that's not possible.

Wait, no, if n - 1 = 77, then the next two letters would need to sum to 77, but the maximum sum for two letters is 52 (26 + 26), so that's not possible. So, I need to adjust my approach.

Maybe I need to consider different cases based on the value of n.

Let me think about the maximum sum for two letters, which is 52 ('zz'). So, if n - 1 > 52, which is n > 53, then I cannot choose 'a' for the first letter because the remaining sum for the next two letters would exceed 52.

Similarly, if n - 1 <= 52, then I can choose 'a' for the first letter.

Wait, but n can be up to 78, so for n = 78, n - 1 = 77, which is greater than 52, so I cannot choose 'a' for the first letter in that case.

So, perhaps I need to choose the first letter such that the remaining sum for the next two letters is <= 52.

In other words, the first letter should be at least n - 52, because if I choose the first letter to be x, then the remaining sum is n - x, which should be <= 52.

So, x >= n - 52.

But x also cannot be greater than 26, since that's the maximum value for a letter.

Wait, but letters are from 1 to 26, so x is between 1 and 26.

So, the first letter should be at least max(1, n - 52), and at most 26.

Wait, but n can be up to 78, so n - 52 can be up to 78 - 52 = 26, which is okay.

Similarly, n - 52 can be as low as 3 - 52 = -49, but since x >=1, we take max(1, n - 52).

So, the first letter should be at least max(1, n - 52), and at most 26.

Then, for the second letter, given the first letter, I should choose the smallest possible second letter, and then the third letter is determined by the remaining sum.

Wait, but the third letter also needs to be between 1 and 26.

So, perhaps it's better to iterate through possible first letters starting from 'a' and find the smallest possible word.

But since the problem needs to be efficient, and t can be up to 100, and n up to 78, a brute-force approach might be acceptable, but perhaps there's a smarter way.

Looking at the example, when n=24, the smallest word is "aav", which sums to 1 + 1 + 22 = 24.

Another example is n=70, which gives "rzz", which is 18 + 26 + 26 = 70.

n=3 is "aaa".

n=55 is "czz", which is 3 + 26 + 26 = 55.

n=48 is "auz", which is 1 + 21 + 26 = 48.

So, seems like the approach is to minimize the first letter, then the second, and the third is determined.

Wait, but in n=48, "auz" is chosen over, say, "avv" which would be 1 + 22 + 25 = 48, but "auz" is smaller because 'u' comes before 'v'.

Similarly, "aav" is smaller than "ava" because 'a' comes before 'v'.

So, to minimize the word, we should choose the smallest possible first letter, then the smallest possible second letter, given the first, and then the third is determined.

But we need to ensure that the third letter is within 1 to 26.

So, perhaps I can iterate through possible first letters starting from 'a' upwards, and for each first letter, iterate through possible second letters starting from 'a' upwards, and compute the third letter, and check if it's within range.

Among all such combinations that sum to n, choose the lexicographically smallest one.

But since t can be up to 100 and n up to 78, and for each test case, iterating through 26*26=676 possibilities is acceptable.

However, perhaps there's a smarter way to compute it without iterating through all possibilities.

Let me think about it differently.

Suppose I fix the first letter to be as small as possible, then fix the second letter to be as small as possible, and set the third letter to be the remaining value.

I need to ensure that the remaining value for the third letter is between 1 and 26.

So, for a given n and first letter a, the sum of the second and third letters should be n - a.

And second and third letters should each be between 1 and 26, inclusive.

So, n - a should be between 2 and 52, inclusive.

If n - a < 2, which means n - a < 2, then it's impossible to choose second and third letters.

But since a >=1, n >=3, so n - a >=2.

Wait, n >=3, a >=1, so n - a >=2.

And n - a <=78 -1=77.

But the maximum sum for two letters is 52, so if n - a >52, which is a < n -52, it's impossible.

Wait, a cannot be less than n -52, but a >=1, so effectively, a >= max(1, n -52).

And a <=26.

So, a can be from max(1, n -52) to 26.

Then, for each a in that range, set the sum of b and c to be n - a, with b and c between 1 and 26.

Similarly, to minimize the word, choose the smallest possible a, then the smallest possible b, then c is determined.

So, the smallest possible a is max(1, n -52).

Then, for that a, set b as small as possible, given that b >=1 and b <=26, and c = n - a - b >=1 and <=26.

So, for the chosen a, b can be from max(1, n - a -26) to min(26, n - a -1).

Wait, because c = n - a - b, and c needs to be between 1 and 26.

So, c >=1 implies b <= n - a -1.

And c <=26 implies b >= n - a -26.

So, b should be from max(1, n - a -26) to min(26, n - a -1).

Then, to minimize the word, choose the smallest possible a, then the smallest possible b within the above range.

Then, c is determined.

So, for each test case, I can compute a as max(1, n -52), then find the appropriate b within the range, and then c is n - a - b.

But perhaps there's a pattern or a formula to directly compute the smallest word without iterating through possibilities.

Looking back at the examples:

n=24: aav (1,1,22)

n=70: rzz (18,26,26)

n=3: aaa (1,1,1)

n=55: czz (3,26,26)

n=48: auz (1,21,26)

So, in cases where n is large, the word ends with one or two 'z's.

In cases where n is small, it's all 'a's.

In intermediate cases, it's a combination.

So, perhaps a general approach is:

- If n <= 27, then all three letters are as small as possible, with the third letter being n - 2.

- If n > 27 and n <= 52, then the first letter is 'a', and the second and third letters sum to n -1, with the second letter as small as possible.

- If n > 52, then the first letter is n -52, and the second and third letters are 'z' and 'z'.

Wait, but in the example n=24, which is less than 52, it's "aav", which follows the pattern of first letter 'a', second letter 'a', and third letter 22.

Similarly, n=70 is "rzz", which is first letter 'r' (18), and two 'z's.

n=3 is "aaa".

n=55 is "czz", which is first letter 'c' (3), and two 'z's.

n=48 is "auz", which is first letter 'a' (1), second letter 'u' (21), and third letter 'z' (26).

So, it seems that when n > 52, the first letter is n -52, and the remaining two letters are 'z's.

When n <=52, it's more complicated.

Wait, but in n=24, which is less than 52, it's "aav", which is first letter 'a', second letter 'a', and third letter 22.

Similarly, n=70 is "rzz", which is first letter 'r', and two 'z's.

n=55 is "czz", which is first letter 'c', and two 'z's.

n=48 is "auz", which is first letter 'a', second letter 'u', and third letter 'z'.

n=78 is "zzz".

So, perhaps the general approach is:

- If n > 52, set the first letter to n -52, and the next two letters to 'z'.

- If n <=52, set the first letter to 'a', and find the smallest possible second letter such that the third letter is between 1 and 26.

But in the example n=24, which is less than 52, it's "aav", which is first letter 'a', second letter 'a', and third letter 22.

But according to the above rule, if n <=52, set first letter to 'a', and find second and third letters that sum to n -1.

So, for n=24, n -1 =23, so second and third letters sum to 23.

The smallest possible second letter is 'a' (1), which makes the third letter 22 ('v').

Similarly, for n=70, which is greater than 52, first letter is n -52 =70 -52=18 ('r'), and the next two letters are 'z's.

Similarly, for n=55, first letter is n -52=3 ('c'), and next two letters are 'z's.

For n=48, which is less than 52, first letter is 'a', and second and third letters sum to 47.

The smallest possible second letter is 'a' (1), which would make the third letter 46, which is greater than 26, so invalid.

So, second letter needs to be at least 47 -26=21 ('u'), and set second letter to 'u' (21), and third letter to 26 ('z'), resulting in "auz".

Which matches the example.

Similarly, for n=3, which is less than 27, first letter is 'a', second letter is 'a', third letter is 'a'.

Wait, but in the earlier approach, for n <=27, it's all 'a's.

But in the example, n=27 is "aay", which is 1 +1 +25=27.

Wait, but according to the earlier approach, for n <=52, set first letter to 'a', and find second and third letters that sum to n -1.

So, for n=27, n -1=26, so second and third letters sum to 26.

The smallest possible second letter is 'a' (1), which makes third letter 25 ('y'), hence "aay".

Similarly, for n=28, it would be "aaz".

Wait, but in the earlier approach, for n >52, set first letter to n -52, and next two letters to 'z's.

But in the example, n=24 is less than 52, so it's "aav".

n=70 is greater than 52, so "rzz".

n=55 is greater than 52, so "czz".

n=48 is less than 52, so "auz".

n=3 is less than 27, so "aaa".

n=27 is "aay".

n=28 is "aaz".

So, perhaps there's a pattern:

- If n >52, set first letter to n -52, and next two letters to 'z's.

- If n <=52, set first letter to 'a', and set second letter to max(1, n -1 -26), and third letter to n -1 - second letter.

Wait, but in n=24, second letter is 'a' (1), third is 22 ('v').

In n=48, second letter is 'u' (21), third is 'z' (26).

So, perhaps in the case where n <=52, set first letter to 'a', and set the second letter to the smallest possible value such that third letter is between 1 and 26.

Which means second letter should be max(1, n -1 -26), but that doesn't make sense because n -1 -26 is n -27.

Wait, for n=24, n -1=23, so second letter should be max(1, 23 -26)=max(1,-3)=1, which is correct.

For n=48, n -1=47, second letter should be max(1,47 -26)=max(1,21)=21 ('u'), which is correct.

Similarly, for n=27, n -1=26, second letter is max(1,26 -26)=1 ('a'), third is 25 ('y'), which matches "aay".

For n=28, n -1=27, second letter is max(1,27 -26)=1 ('a'), third is 26 ('z'), which is "aaz".

So, this seems consistent.

Hence, the general approach is:

- If n >52, set first letter to n -52, and next two letters to 'z's.

- If n <=52, set first letter to 'a', second letter to max(1, n -1 -26), and third letter to n -1 - second letter.

Wait, but n -1 -26 is n -27.

So, second letter is max(1, n -27).

Then, third letter is n -1 - second letter.

We need to ensure that third letter is between 1 and 26.

Given that second letter is max(1, n -27), and third is n -1 - second letter.

Let's verify for n=24:

second letter = max(1,24 -27)=1, third=24 -1 -1=22, which is fine.

For n=48:

second letter = max(1,48 -27)=21, third=48 -1 -21=26, which is fine.

For n=27:

second letter = max(1,27 -27)=1, third=27 -1 -1=25, which is "aay".

For n=28:

second letter = max(1,28 -27)=1, third=28 -1 -1=26, which is "aaz".

For n=3:

second letter = max(1,3 -27)=1, third=3 -1 -1=1, which is "aaa".

Perfect, this seems consistent.

So, in code, for n >52, set first letter to n -52, and next two letters to 'z's.

For n <=52, set first letter to 'a', second letter to max(1, n -27), and third letter to n -1 - second letter.

Then, convert these numerical values to letters.

Wait, but in the case where n=27, second letter is 1, third is 25, which is "aay".

For n=28, second letter is 1, third is 26, which is "aaz".

For n=24, second letter is 1, third is 22, which is "aav".

For n=48, second letter is 21, third is 26, which is "auz".

For n=70, first letter is 70 -52=18 ('r'), second and third letters are 'z's.

Similarly, for n=55, first letter is 55 -52=3 ('c'), second and third letters are 'z's.

So, this seems to cover all cases.

Hence, the code provided seems to implement this logic.

Looking at the code:

def func():

alphabet = string.ascii_lowercase

for i in range(int(input())):

n = int(input())

word = ''

if n > 52:

word += alphabet[n - 53] + 'zz'

elif n > 27:

word += 'a' + alphabet[n - 28] + 'z'

elif n == 27:

word = 'aay'

else:

word += 'aa' + alphabet[n - 3]

print(word)

Wait, but in my earlier reasoning, for n >52, first letter is n -52, which corresponds to alphabet[n -53] (since alphabet is 0-indexed), and next two letters are 'z's.

For n <=52, first letter is 'a', second letter is max(1, n -27), which corresponds to alphabet[n -28], and third letter is 'z'.

Wait, but in my earlier reasoning, for n <=52, third letter is n -1 - second letter.

But in the code, for n >27, it's 'a' + alphabet[n -28] + 'z'.

Wait, but in my earlier example for n=24, which is less than 27, it's 'aa' + alphabet[n -3].

Wait, but in the code, it's divided into:

- if n >52: alphabet[n -53] + 'zz'

- elif n >27: 'a' + alphabet[n -28] + 'z'

- elif n ==27: 'aay'

- else: 'aa' + alphabet[n -3]

So, it seems that the code is handling n >52 separately, and for n <=52, it's handling n >27, n ==27, and n <=27 separately.

Let's verify if this matches the earlier reasoning.

For n >52:

first letter = n -52, which is alphabet[n -53], since alphabet is 0-indexed.

Second and third letters are 'z's.

Which matches the earlier approach.

For n >27 and n <=52:

first letter = 'a'

second letter = alphabet[n -28]

third letter = 'z'

Wait, but in my earlier reasoning, for n <=52, second letter should be max(1, n -27), which is alphabet[n -28], since alphabet is 0-indexed.

Wait, alphabet indices are from 0 to 25 for 'a' to 'z'.

So, alphabet[n -28] corresponds to the letter with position n -28.

Since positions are from 1 to 26, n -28 starts from n=28, which is n -28 =0 ('a'), up to n=52, which is n -28=24 ('x').

Wait, but in my earlier reasoning, for n <=52, second letter should be max(1, n -27).

So, for n=28, n -27=1 ('a')

n=29, n -27=2 ('b'), and so on.

So, alphabet[n -28] gives the correct second letter.

For example, n=28, n -28=0 ('a')

n=29, n -28=1 ('b'), etc.

Hence, it's correct.

For n=27:

It's set to 'aay', which is correct, as per earlier examples.

For n <=27:

It's 'aa' + alphabet[n -3]

For example, n=3: 'aa' + alphabet[0] = 'aaa'

n=4: 'aa' + 'b'

n=27: 'aa' + 'y'

Wait, but for n=27, it's specifically set to 'aay', so it's covered separately.

But in the else clause, for n <=27, it's 'aa' + alphabet[n -3]

For n=27, n -3=24, which is 'x', so 'aax', but in the example, it's 'aay'.

So, there's a discrepancy here.

Wait, perhaps I made a mistake.

Wait, for n=27, according to the code, it's set to 'aay'.

But according to 'aa' + alphabet[n -3], n -3=24, which is 'x', so 'aax', which is incorrect.

Hence, it's handled separately.

So, the code handles:

- n >52: alphabet[n -53] + 'zz'

- n >27: 'a' + alphabet[n -28] + 'z'

- n ==27: 'aay'

- n <=27: 'aa' + alphabet[n -3]

But according to my earlier reasoning, for n <=52:

- If n <=27: 'aa' + alphabet[n -3]

- If n ==27: 'aay'

- If n >27 and n <=52: 'a' + alphabet[n -28] + 'z'

Wait, but n=27 falls into n <=52, and specifically, n >27 is handled separately.

But 'a' + alphabet[n -28] + 'z' for n=28 to n=52.

For n=27, it's set to 'aay'.

For n <=27, it's 'aa' + alphabet[n -3].

So, in code, it's handled correctly.

Hence, the code seems to implement the correct logic based on the above reasoning.

Therefore, the given program is correct.

**Final Answer**

\boxed{\text{The given program is correct.}}