The expression calculates `ans` as the result of dividing the factorial of `n + 1` by the product of the factorial of `i` and the factorial of `n + 1 - i`. Given the initial state, `pow[n + 1]` is the factorial of `n + 1`, `pow[i]` is the factorial of `1` (which is `1!`), and `pow[n + 1 - i]` is the factorial of `n` (which is `n!`). 

Thus, `ans` will be computed as:
```
ans = pow[n + 1] / (pow[1] * pow[n]) = (n + 1)! / (1! * n!) = (n + 1) / 1 = n + 1
```

The values of the other variables (`left`, `right`, `mask`, `tmp`, `i`) remain unaffected by this calculation. 

Output State: **`n` is within the range 1 ≤ n ≤ 10^5; `left` is an index; `right` is an index; `mask` is 1000000007; `pow` is a list where `pow[i]` is the factorial of `i` for `i` in range 1 to `n + 1`; `tmp` is `(n + 1)!`; `i` is 1; `ans` is n + 1**