Example Answer:
`b` is updated to `(previous value of b) - (k - 1)`. Since `b` is greater than or equal to `k`, the value of `b` after execution is `(previous value of b) - (k - 1)`. The value of `a` is updated to `(previous value of a) - (k * v)`. Therefore, the Output State is: `k`, `a`, `b`, `v` are integers such that 2 <= k <= 1000, 1 <= a, b, v <= 1000; `res` is 1. `b` is greater than or equal to `k`. `a` is updated to the value of `(previous value of a) - (k * v)`, `b` is updated to `(previous value of b) - (k - 1)`.
Output State: **`k`, `a`, `b`, `v` are integers such that 2 <= k <= 1000, 1 <= a, b, v <= 1000; `res` is 1. `b` is greater than or equal to `k`. `a` is updated to the value of `(previous value of a) - (k * v)`, `b` is updated to `(previous value of b) - (k - 1)`**