Let's analyze the given loop and the provided output states step by step.

### Initial State:
- \( n \) is a non-negative integer and \( n \neq 0 \), \( n \neq 1 \)
- \( a = 2 \)
- \( b = 1 \)

### Code of the Loop:
```python
for _ in range(2, n + 1):
    a, b = b, a + b
```

### Understanding the Loop:
- The loop runs from 2 to \( n \) (inclusive).
- In each iteration, \( a \) is updated to the current value of \( b \), and \( b \) is updated to the sum of the previous \( a \) and \( b \).

### Observing the Output States:
- After 1 iteration:
  - \( n \) must be at least 2
  - \( a = 3 \) (initial \( b \))
  - \( b = 1 \) (initial \( a \))

- After 2 iterations:
  - \( n \) must be at least 3
  - \( a = 1 \) (previous \( b \))
  - \( b = 4 \) (previous \( a + b \))

- After 3 iterations:
  - \( n \) must be at least 4
  - \( a = 4 \) (previous \( b \))
  - \( b = 5 \) (previous \( a + b \))

### General Pattern:
- Each iteration updates \( a \) and \( b \) such that \( a \) becomes the previous \( b \), and \( b \) becomes the sum of the previous \( a \) and \( b \).
- The sequence generated by this loop is known as the Fibonacci sequence starting from \( a = 2 \) and \( b = 1 \).

### Final Output State:
- When the loop finishes, \( a \) will be the \( (n-1) \)-th Fibonacci number starting from \( a = 2 \) and \( b = 1 \).
- \( b \) will be the \( n \)-th Fibonacci number starting from \( a = 2 \) and \( b = 1 \).

### Conclusion:
- The loop will execute exactly \( n-1 \) times if \( n \geq 2 \).
- If \( n < 2 \), the loop does not execute, so \( a \) remains 2 and \( b \) remains 1.

### Output State:
**Output State:**
- If \( n \geq 2 \), \( a \) is the \( (n-1) \)-th Fibonacci number starting from 2 and 1, and \( b \) is the \( n \)-th Fibonacci number starting from 2 and 1.
- If \( n < 2 \), \( a = 2 \) and \( b = 1 \).

Thus, the final output state is:
Output State: **If \( n \geq 2 \), \( a \) is the \( (n-1) \)-th Fibonacci number starting from 2 and 1, and \( b \) is the \( n \)-th Fibonacci number starting from 2 and 1; otherwise, \( a = 2 \) and \( b = 1 \).**