Output State: **`z` is 0, `i` is 1, `j` is 0, `p` is 1**

Explanation:
1. **Initial State**: 
   - `z = 0`
   - `i = 0`
   - `j = 0`
   - `p` is determined based on the condition: `p = 0` if `i >= r` else `p = min(r - i, res[2 * (l + r) - z])`.

2. **Loop Condition**: 
   - The loop continues as long as `j + p + 1 < n` and `i - p - 1 >= 0`.

3. **First Iteration**:
   - After the first iteration, `p` is incremented by 1, so `p` becomes `min(r - i, res[2 * (l + r) - z]) + 1`.
   - Given the output state after 1 iteration, `p` is `min(r - i, res[2 * (l + r) - z]) + 1`.
   - Since `i` remains unchanged and starts at 0, and considering the condition `i - p - 1 >= 0`, we can infer that `p` must be incremented only once to satisfy the loop condition, making `p = 1`.

4. **Subsequent Iterations**:
   - The output state after the second and third iterations remains the same (`p = 1`), indicating that the loop breaks immediately after the first iteration due to the condition inside the loop.

5. **Break Condition**:
   - The loop breaks when `s[j + p + 1] != s[i - p - 1]`, which means that the characters at positions `j + p + 1` and `i - p - 1` are not equal.

6. **Final Values**:
   - `z` remains 0 because there is no update to this variable in the loop.
   - `i` remains 1 because it is incremented within the loop, but since the loop breaks after the first iteration, `i` does not change further.
   - `j` remains 0 because it is not updated in the loop.
   - `p` is 1 because the loop increments `p` by 1 during its first and final iteration.

Therefore, the loop terminates with `z = 0`, `i = 1`, `j = 0`, and `p = 1`.