`k` is decremented by `n - 1`. Given the initial state where `n` is an even positive integer between 2 and \(10^9\), and `k` is an integer such that \(0 \leq k < n \cdot m\) and \(k \geq n - 1\), after decrementing `k` by `n - 1`, the new value of `k` will be in the range from 0 to \(n \cdot m - (n - 1)\) but will now satisfy \(k \geq 0\) since the decrement is by `n - 1` which is positive.

Therefore, the updated conditions are:
- `n` remains an even positive integer between 2 and \(10^9\).
- `m` remains a positive integer such that \(2 \leq n, m \leq 10^9\).
- `k` is an integer such that \(0 \leq k < n \cdot m\) and \(k \geq 0\) after decrementing by `n - 1`.

Output State: **`n` is an even positive integer between 2 and \(10^9\); `m` is a positive integer such that \(2 \leq n, m \leq 10^9\); `k` is an integer such that \(0 \leq k < n \cdot m\) and \(k \geq 0` after decrementing by `n - 1`.**