The expression `total_sum = (total_sum + num) % MOD` updates the value of `total_sum`. The initial value of `total_sum` is 0, and `num` is given as `l + 1`. Therefore, the new value of `total_sum` will be `(0 + (l + 1)) % MOD`, which simplifies to `(l + 1) % MOD`. The value of `MOD` is not specified, so we cannot determine the exact result of the modulo operation, but we can express it in terms of `l` and `MOD`.

The output state is: `total_sum` is `(l + 1) % MOD`, `l` and `r` are integers such that 1 <= l <= r < 10^18, and `num` is `l + 1`.

Output State: **`total_sum` is `(l + 1) % MOD`, `l` and `r` are integers such that 1 <= l <= r < 10^18, `num` is `l + 1`**