To determine what will be printed by the `print` statement, let's break down the given initial state and the code snippet step-by-step:

### Initial State Breakdown:
- `a`: This is a list with six elements, but only the first three elements (`first_value_from_r`, `second_value_from_r`, `last_value_from_r`) and the fourth element (`2000000000.0`) are explicitly mentioned. The last two elements are `new_value` and `next_new_value`.
- `u`: This is a non-zero number decreased by 1. However, this variable is not used in the `print` statement, so we can ignore it for this specific task.
- `t`: This is set to `new_t_value`, but it is also not used in the `print` statement, so we can ignore it for this specific task.
- `b`: This is a list with eight elements:
  - `b[0] = 0`
  - `b[1] = 0`
  - `b[2] = y - x`
  - `b[3] = y - x + v_or_1`
  - `b[4] = 2 * (y - x) + v_or_1`
  - `b[5] = (y - x + v_or_1) + v_or_1`
  - `b[6] = v`
  - `b[7] = v`
- `c` and `d`: These are the return values from the function `r()`. The relationship between `c` and `d` is given by the condition: if `c < d`, then `c` is less than `d`; otherwise, `c` is greater than or equal to `d`.

### Code Snippet Analysis:
The `print` statement is:
```python
print(b[(d - 1) * 2] - b[(c - 1) * 2])
```

Let's analyze the indices:
- `(d - 1) * 2`: Since `d` is a return value from `r()`, we don't know its exact value. However, it must be a positive integer because `d` is compared with `c` and both are used as indices.
- `(c - 1) * 2`: Similarly, `c` is another return value from `r()` and must be a positive integer.

Given that `b` is indexed from 0 to 7, the valid values for `(d - 1) * 2` and `(c - 1) * 2` must be within the range of 0 to 6 (inclusive).

### Calculation of Output:
- `b[(d - 1) * 2]`: This will access an even-indexed element of the list `b`.
- `b[(c - 1) * 2]`: This will access another even-indexed element of the list `b`.

The possible even indices for `b` are 0, 2, 4, and 6.

- If `d = 1`, then `(d - 1) * 2 = 0` → `b[0] = 0`
- If `d = 2`, then `(d - 1) * 2 = 2` → `b[2] = y - x`
- If `d = 3`, then `(d - 1) * 2 = 4` → `b[4] = 2 * (y - x) + v_or_1`
- If `d = 4`, then `(d - 1) * 2 = 6` → `b[6] = v`

Similarly,
- If `c = 1`, then `(c - 1) * 2 = 0` → `b[0] = 0`
- If `c = 2`, then `(c - 1) * 2 = 2` → `b[2] = y - x`
- If `c = 3`, then `(c - 1) * 2 = 4` → `b[4] = 2 * (y - x) + v_or_1`
- If `c = 4`, then `(c - 1) * 2 = 6` → `b[6] = v`

### Final Output:
The `print` statement calculates the difference between two elements of `b` at even indices based on the values of `c` and `d`. The exact numerical value depends on the specific values of `c` and `d`, but we can describe the output in terms of these variables.

Output: **b[(d - 1) * 2] - b[(c - 1) * 2] (where b[(d - 1) * 2] and b[(c - 1) * 2] are elements of the list b at even indices determined by the values of d and c respectively)**