The given code snippet updates the value of `p` using the formula `p = (p * v) % m`. Here, `v` is the next element in the reversed list `b`.

Given the initial state, the only variable that changes is `p`. The new value of `p` is calculated as `(p * v) % m`.

Output State: **`t` is an integer such that 1 ≤ t ≤ 10^4; `n` is an integer such that 1 ≤ n ≤ 2·10^5; `m` is an integer such that 1 ≤ m ≤ 10^4; `a` is a list of `n` integers where each integer `a_i` satisfies 1 ≤ a_i ≤ 10^4 and `n` is at least 1; `s` is a string of length `n` consisting of the characters 'L' and 'R'; `b` is a list containing all elements of `a` in the order specified by `s` and `b` has at least one element; `l` is `n`; `r` is `-1`; `ans` is a list containing the value of `p` twice; `p` is `(p * v) % m`; `v` is the next element in the reversed list `b`.**