Let's break down the code step by step:

- Initial State: `t` is 1, `n` is an integer such that \(1 \leq n \leq 1000\), `a` is a list of integers where each integer is between 1 and 100 and the length of `a` is equal to \(n - 1\), and `current_cost` is \(\text{len}(a) - 2\) if \(\text{len}(a) > 0\), otherwise `current_cost` is 0.

- Code: `current_cost += t - 1 - length`

  Here, `length` refers to the length of the list `a`, which is \(n - 1\).

- The calculation inside the code: `t - 1 - length` translates to `1 - 1 - (n - 1)`, which simplifies to `-n + 1`.

- Therefore, `current_cost += -n + 1`. 

- Since `current_cost` is initially \(\text{len}(a) - 2\) (or 0 if \(\text{len}(a) = 0\)), the new value of `current_cost` will be \(\text{len}(a) - 2 - n + 1\), which simplifies to \(\text{len}(a) - n - 1\).

- Given that \(\text{len}(a) = n - 1\), substituting this into the expression gives us \((n - 1) - n - 1 = -2\).

Thus, the final value of `current_cost` is -2, and all other variables remain unchanged.

Output State: **`t` is 1, `n` is an integer such that \(1 \leq n \leq 1000\), `a` is a list of integers where each integer is between 1 and 100 and the length of `a` is equal to \(n - 1\), and `current_cost` is -2.**