The code appends the value of `gap` to the list `even`. Let's analyze the impact of this operation:

1. The initial value of `gap` is either `(a[0] + n) - a[i] - 1` if `i == x - 1` else `a[i + 1] - a[i] - 1`.
2. After executing `even.append(gap)`, the value of `gap` remains unchanged, but `even` now contains the value of `gap`.

Therefore, the output state is: `next_elem` is `a[0] + n` if `i == x - 1` else `a[i + 1]`, `gap` is `(a[0] + n) - a[i] - 1` if `i == x - 1` else `a[i + 1] - a[i] - 1`, `odd` is `[-1]`, and `even` is a list containing one element which is the value of `gap`.

Output State: **`next_elem` is `a[0] + n` if `i == x - 1` else `a[i + 1]`, `gap` is `(a[0] + n) - a[i] - 1` if `i == x - 1` else `a[i + 1] - a[i] - 1`, `odd` is `[-1]`, `even` is `[gap]`**