Given the initial state and the code snippet:

- Initial State: `i` is 0; `x` must be greater than 0; `next_elem` is either `a[0] + n` if `x` is 1, or `a[1]` if `x` is not 1.

The code snippet to analyze is:
```python
gap = next_elem - a[i] - 1
```

Let's break this down:

1. **Condition for `next_elem`:**
   - If `x` is 1, `next_elem = a[0] + n`.
   - If `x` is not 1, `next_elem = a[1]`.

2. **Value of `i`:**
   - `i` is 0.

Now, let's substitute these into the equation `gap = next_elem - a[i] - 1`:

- **Case 1: `x` is 1**
  - `next_elem = a[0] + n`
  - `a[i] = a[0]` (since `i` is 0)
  - So, `gap = (a[0] + n) - a[0] - 1 = n - 1`

- **Case 2: `x` is not 1**
  - `next_elem = a[1]`
  - `a[i] = a[0]` (since `i` is 0)
  - So, `gap = a[1] - a[0] - 1`

In both cases, the value of `i` remains unchanged at 0, and the value of `x` is still greater than 0.

Therefore, the output state is:
**`i` is 0; `x` must be greater than 0; `next_elem` is either `a[0] + n` if `x` is 1, or `a[1]` if `x` is not 1; `gap` is either `n - 1` if `x` is 1, or `a[1] - a[0] - 1` if `x` is not 1.**

Output State: **`i` is 0; `x` must be greater than 0; `next_elem` is either `a[0] + n` if `x` is 1, or `a[1]` if `x` is not 1; `gap` is either `n - 1` if `x` is 1, or `a[1] - a[0] - 1` if `x` is not 1.**