Alright, I've got this problem to solve. Let me read it carefully.

So, there's this physical education lesson in a school, and students are lining up and getting assigned numbers based on their positions and a parameter K. The way the numbers are assigned is a bit tricky. For the first K positions, they get numbers 1 to K, then the next K-2 positions get numbers K-1 down to 2, and this pattern repeats every 2K-2 positions.

For example, if K is 3, the sequence would be 1,2,3,2,1,2,3,2,1,... and so on.

Vasya remembers his position in the line (N) and the number he received (X), and he wants to figure out how many possible values of K are consistent with this information.

Given multiple test cases, each with N and X, I need to output the number of possible K values for each test case.

Constraints:

- T (number of test cases) is between 1 and 100.

- For each test case, N and X are integers where 1 ≤ X < N ≤ 10^9.

Note that K must be greater than 1.

First, I need to understand how the numbering works.

Given a position N and a K, how do we determine the number X assigned to that position?

The pattern repeats every 2K-2 positions. Within each cycle:

- Positions 1 to K: numbers 1 to K.

- Positions K+1 to 2K-2: numbers K-1 down to 2.

So, for K=3:

- Positions 1 to 3: 1,2,3

- Positions 4 to 5: 2,1

- Positions 6 to 8: 2,3,2,1

Wait, no, for K=3, the cycle length is 4 (2K-2=4).

Let's confirm with the example in the problem:

In the first test case:

N=10, X=2

Possible K values are 2,3,5,6.

Let's verify:

For K=2:

Sequence: 1,2,1,2,1,2,1,2,1,2

At position 10: 2

For K=3:

Sequence: 1,2,3,2,1,2,3,2,1,2

At position 10: 2

For K=5:

Sequence: 1,2,3,4,5,4,3,2,1,2

At position 10: 2

For K=6:

Sequence: 1,2,3,4,5,6,5,4,3,2

At position 10: 2

So, in all these cases, at position 10, X=2.

Now, for K=4:

Sequence: 1,2,3,4,3,2,1,2,3,4

At position 10: 4, which is not equal to X=2, so K=4 is invalid.

Similarly, K=7:

Sequence: 1,2,3,4,5,6,7,6,5,4

At position 10: 4, not 2.

So, only K=2,3,5,6 are valid for N=10, X=2.

Another test case: N=3, X=1

Only K=2 is valid.

Wait, let's check:

For K=2:

Sequence: 1,2,1

At position 3: 1

For K=3:

Sequence: 1,2,3

At position 3: 3, which is not X=1.

For K=4:

Sequence: 1,2,3,4,3,2,1,2,3,4,...

Position 3: 3, not 1.

So, only K=2 is valid.

Alright, now I need to find a general way to find all possible K for given N and X.

First, I need to understand the pattern of the sequence for a given K.

For a given K:

- The sequence repeats every 2K-2 positions.

- Within each cycle:

- Positions 1 to K: numbers 1 to K.

- Positions K+1 to 2K-2: numbers K-1 down to 2.

So, for a position N, I need to find out, for which K, the number at position N is X.

Given that the sequence repeats every 2K-2 positions, I can find the position within the cycle.

Let’s denote:

Cycle length = 2K - 2

Then, the position within the cycle is N mod (2K - 2)

However, need to handle the case when N is a multiple of the cycle length.

Wait, more carefully:

Position in cycle = (N - 1) mod (2K - 2) + 1

Then, determine the number assigned to that position based on its position within the cycle.

If position in cycle <= K, then number is position in cycle

Else, number is 2K - position in cycle

Wait, let's formalize this.

Let’s define:

Let M = (N - 1) mod (2K - 2)

Then, position in cycle = M + 1

If position in cycle <= K, then X = position in cycle

Else, X = 2K - position in cycle

We need X to be equal to the given X.

So, we have:

If position in cycle <= K, then X = position in cycle

Else, X = 2K - position in cycle

We need X to be equal to the given X.

So, we can set up equations based on this.

Case 1: position in cycle <= K

Then, X = position in cycle

Which means M + 1 = X

So, M = X - 1

But M = (N - 1) mod (2K - 2)

So, (N - 1) mod (2K - 2) = X - 1

Which implies that (N - 1) - (X - 1) is divisible by (2K - 2)

So, N - X is divisible by (2K - 2)

Therefore, (2K - 2) divides (N - X)

Similarly, (2K - 2) divides (N - X)

So, 2K - 2 is a divisor of N - X

Thus, 2K - 2 divides N - X

So, 2K - 2 | N - X

Similarly, K = (N - X)/(2K - 2) + something

Wait, perhaps it's better to express it as:

2K - 2 divides N - X

So, 2K - 2 is a divisor of N - X

Therefore, for each divisor D of N - X, we can set 2K - 2 = D

Then, K = (D + 2)/2

But K must be an integer greater than 1.

So, D must be even because 2K - 2 is even for K integer greater than 1.

Wait, is that true?

Wait, 2K - 2 is even only if K is integer.

Wait, K must be integer because it's a number of positions.

Wait, but K must be integer, as it's a parameter defining the pattern.

So, K is integer, K > 1.

Then, 2K - 2 is even.

So, D must be even.

But N - X could be odd or even.

If N - X is odd, then there are no solutions in this case because D must be even to divide N - X.

Wait, but D must divide N - X, and D is even, so N - X must be even in this case.

Wait, no, D can be any divisor of N - X, but 2K - 2 is even, so D is even only if K is integer greater than 1.

Wait, K is integer, K > 1, so 2K - 2 is even.

Therefore, D must be even.

Hence, N - X must be even in this case.

Wait, no, D divides N - X, and D is even, so N - X must be even.

Wait, no, if D is even and D divides N - X, then N - X must be divisible by D, which is even, so N - X must be even.

Wait, no, if D is even and D divides N - X, then N - X must be even because even divides even.

But N - X could be odd, in which case there are no solutions in this case.

Wait, but in this case, we have 2K - 2 divides N - X, and 2K - 2 is even, so N - X must be even.

But in the problem, N and X can be such that N - X is odd or even.

So, in the case where N - X is odd, there are no solutions in this case.

But perhaps there are other cases.

Wait, perhaps there are two cases.

Wait, in the problem, it's mentioned that the settling exists only if K > 1.

So, K >= 2.

Now, in the first case, where position in cycle <= K, we have X = position in cycle = M + 1 = X

Then, (N - 1) mod (2K - 2) = X - 1

Which implies that (N - 1) - (X - 1) is divisible by (2K - 2)

So, (N - X) is divisible by (2K - 2)

Hence, (2K - 2) divides (N - X)

So, 2K - 2 is a divisor of N - X.

Therefore, for each divisor D of N - X, we can set 2K - 2 = D, hence K = (D + 2)/2

We need K to be integer >= 2.

So, D must be even, because 2K - 2 is even.

Hence, D must be even.

Therefore, N - X must be even.

Wait, but N - X can be odd or even.

If N - X is odd, then there are no solutions in this case.

But perhaps there is another case.

Looking back at the problem, perhaps there is another case.

In the sequence, for positions beyond the first cycle, it repeats every 2K - 2 positions.

But in the first cycle, it's positions 1 to 2K - 2.

Wait, perhaps I need to consider the general formula for X in terms of N and K.

Let me try to derive a general formula.

Given K, and position N, what is X?

Let’s define:

Cycle length = 2K - 2

Then, the position within the cycle is P = (N - 1) mod (2K - 2) + 1

Then, if P <= K, X = P

Else, X = 2K - P

So, X = P if P <= K, else X = 2K - P

We need X to be equal to the given X.

So, we have two cases:

1. P <= K and P = X

2. P > K and 2K - P = X

Let’s consider each case separately.

Case 1: P <= K and P = X

Then, P = X

Which means (N - 1) mod (2K - 2) + 1 = X

So, (N - 1) mod (2K - 2) = X - 1

Which implies that (N - 1) - (X - 1) is divisible by (2K - 2)

So, N - X is divisible by (2K - 2)

Hence, (2K - 2) divides (N - X)

Therefore, 2K - 2 is a divisor of N - X

So, for each divisor D of N - X, we can set 2K - 2 = D, hence K = (D + 2)/2

We need K to be integer >= 2, so D must be even.

Therefore, N - X must be even.

But in the problem, N and X can be such that N - X is odd or even.

So, in this case, if N - X is odd, there are no solutions in this case.

Case 2: P > K and 2K - P = X

Then, P = 2K - X

But P = (N - 1) mod (2K - 2) + 1

So, (N - 1) mod (2K - 2) + 1 = 2K - X

Therefore, (N - 1) mod (2K - 2) = 2K - X - 1

Which implies that (N - 1) - (2K - X - 1) is divisible by (2K - 2)

So, N - 1 - 2K + X + 1 = N - 2K + X is divisible by (2K - 2)

Hence, (N - 2K + X) is divisible by (2K - 2)

So, (2K - 2) divides (N - 2K + X)

Simplify N - 2K + X:

N + X - 2K

So, (2K - 2) divides (N + X - 2K)

Let’s rearrange:

(2K - 2) divides (N + X - 2K)

Which can be written as:

(2K - 2) divides -(2K - 2 - (N + X - 2K)) = -(N + X - 2)

So, (2K - 2) divides (N + X - 2)

Therefore, 2K - 2 divides N + X - 2

Hence, for each divisor D of N + X - 2, we can set 2K - 2 = D, hence K = (D + 2)/2

Again, K must be integer >= 2, so D must be even.

Therefore, N + X - 2 must be even.

But N and X can be such that N + X - 2 is odd or even.

So, in this case, if N + X - 2 is odd, there are no solutions in this case.

Now, to find all possible K, we need to consider both cases and find K that satisfy either case.

But we have to make sure that K is integer >= 2, and that in both cases, K satisfies the conditions.

Also, we need to make sure that in both cases, K is consistent with the position and the number assigned.

Wait, but in the first case, we have (2K - 2) divides (N - X), and in the second case, (2K - 2) divides (N + X - 2).

So, for each divisor D of N - X, we can compute K = (D + 2)/2, and check if K is integer >= 2, and also check that P <= K in the first case.

Similarly, for each divisor D of N + X - 2, we can compute K = (D + 2)/2, and check if K is integer >= 2, and also check that P > K in the second case.

But to make it efficient, especially since N and X can be up to 10^9, we need an efficient way to find the divisors of N - X and N + X - 2.

But N can be up to 10^9, so we need an efficient way to find the divisors of large numbers.

Wait, but T is up to 100, so for each test case, we can find the divisors of N - X and N + X - 2 efficiently, as long as we implement an efficient divisor function.

So, I need to implement a function that, given a number, returns all its divisors in O(sqrt(number)) time.

Then, for each test case, I can find all divisors of N - X and N + X - 2, compute K = (D + 2)/2 for each divisor D, check if K is integer >= 2, and also check the conditions P <= K or P > K accordingly.

But perhaps I can combine both cases.

Let’s see.

So, for each divisor D of N - X, compute K = (D + 2)/2, and check if K is integer >= 2 and P <= K.

Similarly, for each divisor D of N + X - 2, compute K = (D + 2)/2, and check if K is integer >= 2 and P > K.

But to check P <= K or P > K, I need to compute P for each K.

Wait, but P is (N - 1) mod (2K - 2) + 1.

But since (2K - 2) divides (N - X) in the first case, and (2K - 2) divides (N + X - 2) in the second case, perhaps I can simplify P.

Wait, in the first case, since (2K - 2) divides (N - X), and P = X, which is given.

In the second case, P = 2K - X.

But perhaps I need to ensure that K >= X, since in the first K positions, numbers are from 1 to K.

Wait, in the first K positions, numbers are from 1 to K, and in the next K - 2 positions, numbers are from K - 1 down to 2.

So, X can be from 1 to K.

But X is given to be less than N, and N >= 2, since X < N.

Also, K > 1.

So, K can be from 2 up to some value.

Now, in the first case, when P <= K, X = P = X, which is consistent.

In the second case, when P > K, X = 2K - P.

So, P = 2K - X.

But P must be greater than K, so 2K - X > K, which implies K > X.

Therefore, in the second case, K > X.

So, in the first case, K >= X (since P can be equal to K), and in the second case, K > X.

But in the first case, when P <= K, K can be equal to X.

Wait, P <= K, and P = X, so K >= X.

In the second case, P > K, and P = 2K - X, so 2K - X > K, which implies K > X.

Therefore, in the second case, K > X.

So, in the first case, K >= X, and in the second case, K > X.

Now, in terms of finding K, perhaps it's better to consider both cases separately.

First, consider the first case where (2K - 2) divides (N - X), and K >= X.

Second, consider the second case where (2K - 2) divides (N + X - 2), and K > X.

Then, for each divisor D of N - X, compute K = (D + 2)/2, and check if K is integer >= 2 and K >= X.

Similarly, for each divisor D of N + X - 2, compute K = (D + 2)/2, and check if K is integer >= 2 and K > X.

But also, need to ensure that D is positive, since K > 1 implies D = 2K - 2 >= 2.

So, D >= 2.

Also, D must be even, since 2K - 2 is even for K >= 2.

Therefore, when finding divisors of N - X and N + X - 2, we only consider even divisors D >= 2.

Then, for each such D, compute K = (D + 2)/2, and check the conditions.

Now, to implement this efficiently, I need to:

1. For each test case, read N and X.

2. Compute N - X and N + X - 2.

3. Find all even divisors D of N - X that are >= 2.

4. For each such D, compute K = (D + 2)/2, and check if K >= X.

5. Similarly, find all even divisors D of N + X - 2 that are >= 2.

6. For each such D, compute K = (D + 2)/2, and check if K > X.

7. Collect all valid K from both cases, remove duplicates, and count them.

Now, considering that N and X can be up to 10^9, and T is up to 100, I need an efficient way to find the even divisors of N - X and N + X - 2.

I can implement a function that returns all even divisors of a given number M.

The function should find all divisors of M that are even and >= 2.

Given that M can be up to 2*10^9 (since N <= 10^9 and X <= N-1), finding divisors in O(sqrt(M)) time is acceptable, as sqrt(10^9) is about 31623, which is manageable.

Now, I need to handle the cases where N - X is zero or negative, but according to the constraints, X < N, so N - X is at least 1.

Similarly, N + X - 2 can be less than 1, but since X >=1 and N >=2, N + X - 2 >=1.

So, no issues there.

Now, in the code provided, there is a function func_1(x) that seems to return all divisors of x.

But in the main loop, it's using this function to find divisors of N + X - 2 and N - X, and then computing K = (D + 2)/2, and checking some conditions.

But there are some issues in the code.

First, the function func_1(x) seems correct; it finds all divisors of x.

However, in the main loop:

- It checks if (n + x - 2) % 2 == 0, then finds divisors of N + X - 2.

- For each divisor s, if (s + 2) % 2 == 0 and (s + 2)/2 >= X, it appends K = (s + 2)/2 to output.

- Similarly, if (n - x) % 2 == 0, it finds divisors of N - X.

- For each divisor s, if (s + 2) % 2 == 0 and (s + 2)/2 >= X, it appends K = (s + 2)/2 to output.

- Then, it removes duplicates by using set(output).

But there are some problems here.

First, in the first case, it should be checking (N - X) % D == 0, but in the code, it's checking (N + X - 2) % 2 == 0, which is different.

Wait, no, in the code, it's checking if (N + X - 2) % 2 == 0, which corresponds to the second case where (2K - 2) divides (N + X - 2).

Similarly, it checks if (N - X) % 2 == 0 for the first case.

But in reality, it should be checking if D divides (N - X) or D divides (N + X - 2), where D is 2K - 2.

Wait, no, in the code, it's finding divisors of N + X - 2 and N - X, assuming D = 2K - 2.

But in the first case, it should be checking if D divides (N - X), and in the second case, if D divides (N + X - 2).

But in the code, it's directly using the divisors of N + X - 2 and N - X as D.

Wait, perhaps I need to look again.

In the code:

if (n + x - 2) % 2 == 0:

sep = func_1(n + x - 2)

for s in sep:

if (s + 2) % 2 == 0 and (s + 2)/2 >= x:

output.append((s + 2)/2)

Similarly for (n - x) % 2 == 0.

But according to our earlier analysis, in the first case, (2K - 2) divides (N - X), and in the second case, (2K - 2) divides (N + X - 2).

So, in the code, it's considering D = 2K - 2 as a divisor of N - X or N + X - 2.

But actually, D should be a divisor of N - X or N + X - 2.

So, in the first case, for D dividing N - X, set D = 2K - 2, hence K = (D + 2)/2.

Similarly, in the second case, for D dividing N + X - 2, set D = 2K - 2, hence K = (D + 2)/2.

Then, check if K >= X in the first case and K > X in the second case.

But in the code, it's checking if (n + x - 2) % 2 == 0, which is equivalent to checking if N + X - 2 is even, which corresponds to D being even, since D = 2K - 2 is even for K >= 2.

Similarly, for (n - x) % 2 == 0, which should be equivalent to N - X being even, which again corresponds to D being even.

But in the code, it's directly using the divisors of N + X - 2 and N - X, assuming D is even, and computing K = (D + 2)/2, then checking if K >= X or K > X.

Wait, perhaps the checks are misplaced.

Wait, perhaps the conditions should be:

- If (N - X) is even, proceed with the first case.

- If (N + X - 2) is even, proceed with the second case.

Because D = 2K - 2 must be even for K >= 2.

Hence, (N - X) and (N + X - 2) must be even for there to be solutions in their respective cases.

Therefore, the checks (N - X) % 2 == 0 and (N + X - 2) % 2 == 0 are correct.

Then, for each even divisor D of N - X, compute K = (D + 2)/2, and check if K >= X.

Similarly, for each even divisor D of N + X - 2, compute K = (D + 2)/2, and check if K > X.

In the code, it's appending K to output if these conditions are met.

Then, it removes duplicates by using set(output).

But in the code, it's using output = list(set(output)), which is correct.

However, in the first case, it should be checking that K >= X, and in the second case, K > X.

But in the code, for both cases, it's checking (s + 2)/2 >= X.

Wait, in the second case, it should be checking K > X, but in the code, it's checking K >= X.

This might be a mistake.

Wait, in the second case, K > X, so it should be checking (s + 2)/2 > X, which is equivalent to (s + 2)/2 >= X + 1.

But in the code, it's (s + 2)/2 >= X.

So, perhaps there is an off-by-one error here.

Wait, let's see.

In the second case, we have K > X.

But in the code, it's appending K if (s + 2)/2 >= X.

Which includes K >= X, but we need K > X.

So, it should be (s + 2)/2 > X, which is equivalent to (s + 2)/2 >= X + 1.

But in the code, it's (s + 2)/2 >= X.

So, this is incorrect.

It should be (s + 2)/2 > X, which is (s + 2)/2 >= X + 1.

Therefore, the code is incorrect in this aspect.

Moreover, in the first case, it should be K >= X, which is correctly checked as (s + 2)/2 >= X.

But in the second case, it should be K > X, which should be (s + 2)/2 > X.

But in the code, it's (s + 2)/2 >= X, which includes K = X, but in the second case, K > X.

Hence, it's incorrect.

Additionally, in the code, it's using float division (s + 2)/2, but K should be an integer.

So, it should be checking if (s + 2) is divisible by 2, which it is, since s is even.

But it's better to use integer division.

Moreover, the function func_1(x) returns all divisors of x, but it's not clear if it returns them in a specific order.

But since we're only interested in unique K values, the order doesn't matter.

Also, the code has a logical error in the second case where it should check K > X instead of K >= X.

Therefore, the code is incorrect.

To fix it, in the second case, when appending K, it should check (s + 2)/2 > X, which is equivalent to (s + 2)/2 >= X + 1.

Hence, the condition should be (s + 2)/2 > X.

Additionally, to ensure that K is an integer, we need to make sure that (s + 2) is divisible by 2, which it is since s is even.

Therefore, the corrected code should be:

if (n + x - 2) % 2 == 0:

sep = func_1(n + x - 2)

for s in sep:

if (s + 2) % 2 == 0 and (s + 2)/2 > x:

output.append((s + 2)/2)

Similarly, for the first case:

if (n - x) % 2 == 0:

sep = func_1(n - x)

for s in sep:

if (s + 2) % 2 == 0 and (s + 2)/2 >= x:

output.append((s + 2)/2)

Also, need to ensure that K >= 2, but since s >= 2, and K = (s + 2)/2, and s is even, K >= 2.

Hence, no need for additional checks.

Moreover, need to make sure that s is positive, but since s is a divisor of N - X or N + X - 2, and N - X >=1, and N + X - 2 >=1, s is positive.

Therefore, the main issue is the incorrect condition in the second case.

Hence, the code is incorrect.

Therefore, the answer is Correctness: **False**

**Final Answer**

\[ \boxed{\text{Correctness: } \text{False}} \]