In the given code snippet, `rem` is assigned the value of `n - 2 * (a + b)`. Since `a` and `b` both have the value of 3, we can calculate the expression step by step:

1. Calculate `a + b`: 
   - \( a + b = 3 + 3 = 6 \)

2. Multiply the result by 2:
   - \( 2 * (a + b) = 2 * 6 = 12 \)

3. Subtract this from `n` to find `rem`:
   - \( rem = n - 12 \)

From the initial state, we know that `rem` is equal to \( n - 8 \). Therefore, setting both equations for `rem` equal gives us:
- \( n - 8 = n - 12 \)
- This implies \( -8 = -12 \), which holds true if `n - 8` yields a valid positive even integer when evaluated. 

Thus, since `rem` has now been redefined in terms of \( n \):
- \( rem \) will always be the positive even integer \( n - 12 \), where \( n \) is guaranteed to be at least 12.

The new context is:
- `rem` is now specifically defined as \( n - 12 \), which maintains the positivity of `rem` given that `n` is at least 12.

Therefore, the outputs that change in this state are just the value of `rem`.

Output State: **`n` is a positive integer such that 1 ≤ `n` ≤ 2·10^9 and `n` is greater than or equal to 12; `rem` is now equal to `n - 12`, `count` is 2, `a` is 3, `b` is 3.**