The code `mid = (low + high) // 2` updates the value of `mid` by calculating the floor division of the sum of `low` and `high`. Given the initial conditions:

- `n` is a positive integer such that \(2 \leq n \leq a + b\),
- `a` is a positive integer such that \(1 \leq a \leq 100\),
- `b` is a positive integer such that \(1 \leq b \leq 100\),
- `low` is either \(1\) or \(\left(\frac{\min(a, b) + 2}{2} + 1\right)\),
- `high` is \(\min(a, b) + 1\),
- `mid` is \(\left(\frac{\min(a, b) + 2}{2}\right)\).

We need to determine the updated value of `mid` based on the possible values of `low` and `high`.

Let's consider the two cases for `low`:

**Case 1:** `low = 1`
- `high = \min(a, b) + 1`
- `mid = (1 + (\min(a, b) + 1)) // 2 = \left(\frac{1 + \min(a, b) + 1}{2}\right) = \left(\frac{\min(a, b) + 2}{2}\right)`

This matches the initial value of `mid`.

**Case 2:** `low = \left(\frac{\min(a, b) + 2}{2} + 1\right)`
- `high = \min(a, b) + 1`
- `mid = \left(\left(\frac{\min(a, b) + 2}{2} + 1\right) + (\min(a, b) + 1)\right) // 2 = \left(\frac{\left(\frac{\min(a, b) + 2}{2} + 1\right) + (\min(a, b) + 1)}{2}\right) = \left(\frac{\frac{\min(a, b) + 2}{2} + 1 + \min(a, b) + 1}{2}\right) = \left(\frac{\frac{\min(a, b) + 2 + 2\min(a, b) + 4}{2}}{2}\right) = \left(\frac{\frac{3\min(a, b) + 6}{2}}{2}\right) = \left(\frac{3\min(a, b) + 6}{4}\right)`

In both cases, the value of `n` remains unchanged, and the other variables remain as per their initial conditions.

Therefore, the Output State is:
Output State: **`n` is a positive integer such that \(2 \leq n \leq a + b\); `a` is a positive integer such that \(1 \leq a \leq 100\); `b` is a positive integer such that \(1 \leq b \leq 100\); `low` is either \(1\) or \(\left(\frac{\min(a, b) + 2}{2} + 1\right)\); `high` is \(\min(a, b) + 1\); `mid` is \(\left(\frac{\min(a, b) + 2}{2}\right) or \left(\frac{3\min(a, b) + 6}{4}\right)**