The initial state is given as follows:
- `n` is a positive integer such that \(2 \leq n \leq a + b\);
- `a` is a positive integer such that \(1 \leq a \leq 100\);
- `b` is a positive integer such that \(1 \leq b \leq 100\);
- `low` is either \(1\) or \(\left(\frac{\min(a, b) + 2}{2} + 1\right)\);
- `high` is \(\min(a, b) + 1\);
- `mid` is \(\left(\frac{\min(a, b) + 2}{2}\right) or \left(\frac{3\min(a, b) + 6}{4}\right)\).

The code snippet updates the value of `low` by setting it to `mid + 1`. We need to consider the two cases for `mid`:

1. If `mid` is \(\left(\frac{\min(a, b) + 2}{2}\right)\), then `low` becomes \(\left(\frac{\min(a, b) + 2}{2}\right) + 1\).
2. If `mid` is \(\left(\frac{3\min(a, b) + 6}{4}\right)\), then `low` becomes \(\left(\frac{3\min(a, b) + 6}{4}\right) + 1\).

Let's denote \(\min(a, b)\) as `m`.

- In the first case, `low` is updated to \(\left(\frac{m + 2}{2}\right) + 1\).
- In the second case, `low` is updated to \(\left(\frac{3m + 6}{4}\right) + 1\).

Since `m` can vary depending on the values of `a` and `b`, we need to express the final state in terms of these expressions.

Output State: **`n` is a positive integer such that \(2 \leq n \leq a + b\); `a` is a positive integer such that \(1 \leq a \leq 100\); `b` is a positive integer such that \(1 \leq b \leq 100\); `low` is either \(\left(\frac{m + 2}{2} + 1\right)\) or \(\left(\frac{3m + 6}{4} + 1\right)\); `high` is \(m + 1\); `mid` is \(\left(\frac{m + 2}{2}\right) or \left(\frac{3m + 6}{4}\right)**.