The code snippet `b -= 1` decreases the value of `b` by 1. Let's analyze the impact of this operation on the given initial state:

- `a`, `b`, `c`, and `d` are non-negative integers such that 0 < a + b + c + d ≤ 10^5.
- They have been updated to the values returned by `func_3()`.
- `s1` is equal to `b - a`.
- `s2` is equal to `c - d`.
- `s1` is not equal to `s2`.
- `s1 + 1` is not equal to `s2`.
- The current value of `s1` is `s2 + 1`.
- `d` is 0.

After executing `b -= 1`:
- The value of `b` is decreased by 1.
- `s1` is recalculated as `s1 = (b - 1) - a = b - a - 1`.

Since `s1` was initially equal to `s2 + 1`, after decrementing `b` by 1, the new value of `s1` will be:
- `s1 = s2 + 1 - 1 = s2`.

Thus, the new state is:
- `a`, `b - 1`, `c`, and `d` are non-negative integers such that 0 < a + (b - 1) + c + d ≤ 10^5.
- `s1` is now equal to `s2`.
- `s2` remains `c - d`.
- `s1 + 1` is not equal to `s2` (since `s1` is now equal to `s2`).
- `d` is 0.

Output State: **`a`, `b - 1`, `c`, and `d` are non-negative integers such that 0 < a + (b - 1) + c + d ≤ 10^5, `s1` is equal to `s2`, `s2` is equal to `c - d`, `s1 + 1` is not equal to `s2`, `d` is 0.**