The variable `ans` is updated by adding the value of `n - 2 - i`. Given that `i` is `n - 1`, we can substitute this into the expression: 

`ans += n - 2 - (n - 1)`

This simplifies to:

`ans += n - 2 - n + 1` 
`ans += -1`

Since `ans` is initially 0, we have:

`ans = 0 - 1`
`ans = -1`

The other variables `n`, `cnt`, and `i` remain unchanged. Therefore, the output state is: `n` is greater than 0, `ans` is -1, `cnt` is 1, `i` is `n - 1`.

Output State: **`n` is greater than 0, `ans` is -1, `cnt` is 1, `i` is `n - 1`**