The expression `ans += n - 2 - i` updates the value of `ans` by adding the result of `n - 2 - i`. Given that `i` is defined as `n - 2`, we can substitute this directly into the expression. Therefore, we have:

```
ans += n - 2 - (n - 2)
```

This simplifies to:

```
ans += n - 2 - n + 2
```

Which results in:

```
ans += 0
```

Thus, `ans` remains unchanged. The other variables `n` and `i` are not affected by this operation. 

Output State: **`n` is greater than 0; `i` is `n - 2`; `ans` remains unchanged.**