Let's break down the given code snippet and the initial state to determine what will be printed.

### Initial State:
- `func_1` is defined with parameters `t` and `test_cases`.
- `n` is an input integer.
- `s` is an input string.
- `neg` is the number of '-' characters in the string `s`.

### Code Snippet:
```python
print(n - 2 * neg if n != neg else n)
```

### Step-by-Step Analysis:
1. **Determine the value of `neg`**:
   - `neg` is the number of '-' characters in the string `s`.
   - For example, if `s = "--++-"`, then `neg = 3`.

2. **Evaluate the condition `n != neg`**:
   - This condition checks if the integer `n` is not equal to the number of '-' characters in the string `s`.

3. **Determine the output based on the condition**:
   - If `n != neg`, the expression `n - 2 * neg` will be printed.
   - If `n == neg`, the value of `n` will be printed.

### Final Output:
- If `n` is not equal to `neg`, the output will be `n - 2 * neg`.
- If `n` is equal to `neg`, the output will be `n`.

### Example Scenarios:
- **Scenario 1**: If `n = 5` and `s = "--++-"`, then `neg = 3`.
  - Condition: `5 != 3` (True)
  - Output: `5 - 2 * 3 = 5 - 6 = -1`
  - Final Output: **-1**

- **Scenario 2**: If `n = 3` and `s = "---"`, then `neg = 3`.
  - Condition: `3 == 3` (True)
  - Output: `3`
  - Final Output: **3**

### General Output:
Based on the initial state and the given code snippet, the output will be:
- `n - 2 * neg` if `n` is not equal to `neg`.
- `n` if `n` is equal to `neg`.

Output: **n - 2 * neg if n != neg else n (where n is the input integer and neg is the number of '-' characters in the input string s)**