To analyze the given code snippet, we have:

Initial State: `n` is a positive integer (1 <= `n` <= 1000), `a` is a list of `n` positive integers (1 <= `a[i]` <= 100), length is equal to `a[2]`

The code provided is:
```
current_cost += t - 1 - length
```

Step-by-step analysis:
- `current_cost` is incremented by the value `t - 1 - length`.
- `length` is defined as equal to `a[2]`.

Thus, `current_cost` is affected here. Given that we're unaware of the values of `current_cost`, `t`, or the actual content of the list `a`, we can't provide specific values for them. However, we know:
- `length` is the value of `a[2]`.
- `current_cost` increases based on the expression involving `t` and `a[2]`.

Output State: **`n` is a positive integer (1 <= `n` <= 1000), `a` is a list of `n` positive integers (1 <= `a[i]` <= 100), `length` is equal to `a[2], current_cost` is increased by `t - 1 - length.**