Alright, I've got this problem to solve. Let me read it carefully.

So, there's this physical education lesson where students line up and are assigned numbers based on a specific pattern involving a parameter k, where k > 1. The pattern repeats every 2k - 2 positions. The first k positions are numbered 1 through k, and the next k-2 positions are numbered k-1 down to 2. Then this pattern repeats.

For example, if k=3, the pattern would be: 1,2,3,2,1,2,3,2,1,2,3,2,1,...

Given that Vasya is in position n and was assigned number x, I need to find out how many natural numbers k (greater than 1) satisfy these conditions.

The input consists of multiple test cases, each with n and x, and I need to output the count of such k for each test case.

First, I need to understand the pattern of numbering.

Let's take k=3 as an example:

Positions: 1,2,3,4,5,6,7,8,9,10,...

Numbers: 1,2,3,2,1,2,3,2,1,2,...

So, the pattern repeats every 2*3 - 2 = 4 positions: 1,2,3,2.

Similarly, for k=4:

Positions: 1,2,3,4,5,6,7,8,9,10,11,12,...

Numbers: 1,2,3,4,3,2,1,2,3,4,3,2,...

Pattern repeats every 6 positions: 1,2,3,4,3,2.

Given n and x, I need to find all k >1 such that the number assigned to position n is x.

Constraints:

- k is a natural number greater than 1.

- 1 ≤ x < n ≤ 10^9

- t (number of test cases) ≤ 100

First, I need to find a way to model this pattern mathematically.

Observations:

1. The pattern repeats every 2k - 2 positions.

2. Within each cycle of 2k - 2 positions:

- Positions 1 to k: numbers 1 to k

- Positions k+1 to 2k-2: numbers k-1 to 2

So, for any position n, I can find out which number is assigned to it based on k.

I need to find all k where the number at position n is x.

Approach:

1. Find the general formula for the number at position n for a given k.

2. Solve for k given that the number at position n is x.

Let's try to find a formula for the number at position n for a given k.

Given k, the pattern repeats every 2k - 2 positions.

So, the number at position n is the same as the number at position n mod (2k - 2).

Let m = n mod (2k - 2)

If m is between 1 and k, inclusive, then number is m.

If m is between k+1 and 2k-2, inclusive, then number is 2k - m.

Wait, let's verify this.

Take k=3:

m = n mod 4

- m=1: number=1

- m=2: number=2

- m=3: number=3

- m=4: number=2

Which matches the pattern.

Take k=4:

m = n mod 6

- m=1: number=1

- m=2: number=2

- m=3: number=3

- m=4: number=4

- m=5: number=3

- m=6: number=2

Which matches the pattern.

So, the formula is:

m = n mod (2k - 2)

if m <= k:

number = m

else:

number = 2k - m

But we have to handle the case where m=0 separately.

If m=0, it means n is a multiple of the period (2k - 2), so m = 2k - 2

So, adjust m to be 2k - 2 if m=0.

So, the formula is:

m = n mod (2k - 2)

if m == 0:

m = 2k - 2

if m <= k:

number = m

else:

number = 2k - m

Given that number = x, we can set up equations to solve for k.

So, we have:

Case 1: m <= k => m = x

Case 2: m > k => 2k - m = x => m = 2k - x

We need to find k such that:

- k >1

- m = n mod (2k - 2)

- if m <=k, then m =x

- else, m =2k -x

Also, since m = n mod (2k - 2), m ranges from 1 to 2k -2.

Let's consider both cases.

Case 1: m <=k => m =x

So, n mod (2k -2) =x

But m cannot exceed 2k -2, so x <= 2k -2

Also, since m <=k, x <=k

But x <=k and x <= 2k -2

But since k >1, 2k -2 >=k for k >=2

So, x <=k

So, n mod (2k -2) =x

Which means n -x is divisible by (2k -2)

So, n -x = t*(2k -2) for some integer t >=0

But n and x are positive integers, n >x

So, t can be 0 or positive integers.

Wait, n -x must be non-negative, since n >x

So, t >=0

But t=0 would imply n -x =0, which is possible only if n=x, but n >x, so t >=1

Wait, but in the formula, n -x = t*(2k -2)

But n >x, so t >=1

So, for each t >=1, we can solve for k:

n -x = t*(2k -2)

So, 2k -2 = (n -x)/t

So, k = [(n -x)/t +2]/2

Similarly, we need k to be integer >1

So, (n -x)/t must be even, since 2k -2 is even.

Wait, 2k -2 is even because 2k is even and subtracting 2 keeps it even.

So, 2k -2 is divisible by 2.

So, (n -x)/t must be even.

Wait, perhaps I need to think differently.

Let me consider that 2k -2 divides n -x.

So, 2k -2 is a divisor of n -x.

Let me denote d =2k -2

So, d divides n -x, and d >=2 since k >=2

So, d is an even divisor of n -x, because d=2k -2 is even for k >=2

Wait, d=2k -2 =2(k -1), which is even for k >=2

So, d is an even divisor of n -x, and d >=2

Then, k =(d +2)/2

We need k to be integer >1

So, d must be even, and d >=2

So, for each even divisor d of n -x, where d >=2, we can set k =(d +2)/2

But we also have constraints based on the position of m.

Wait, perhaps I need to consider both cases.

Wait, perhaps there are two scenarios:

1. When m <=k, which leads to n -x being divisible by 2k -2

2. When m >k, which leads to a different equation.

Wait, perhaps I need to consider both cases separately.

Let me consider the two cases based on m.

Case 1: m <=k => m =x

So, n mod (2k -2) =x

Which means n -x is divisible by 2k -2

So, n -x = t*(2k -2) for some integer t >=1

So, 2k -2 divides n -x

Hence, 2k -2 is a divisor of n -x

Let me denote d =2k -2

So, d divides n -x, and d >=2 since k >=2

So, for each d that divides n -x and d >=2 and d even, we can set k =(d +2)/2

But wait, d=2k -2=2(k -1), which is even for k >=2

So, d is even, and d >=2

So, for each even divisor d of n -x where d >=2, set k =(d +2)/2

Then, we need to ensure that m <=k, which is already satisfied because m =x and x <=k in this case.

Case 2: m >k => m =2k -x

So, n mod (2k -2) =2k -x

Similarly, n -(2k -x) is divisible by 2k -2

Wait, n mod (2k -2) =2k -x

Which implies n - (2k -x) is divisible by 2k -2

So, n -2k +x = t*(2k -2) for some integer t >=0

Let me rearrange:

n +x -2k = t*(2k -2)

Hmm, this seems complicated.

Alternatively, perhaps it's better to consider m = n mod (2k -2)

If m >k, then m =2k -x

So, n mod (2k -2) =2k -x

Which implies n - (2k -x) is divisible by 2k -2

So, n -2k +x ≡0 mod (2k -2)

Which implies n +x -2k ≡0 mod (2k -2)

But 2k -2 divides n +x -2k

So, 2k -2 divides (n +x -2k)

Which means n +x -2k = t*(2k -2) for some integer t >=0

Let me solve for k:

n +x -2k = t*(2k -2)

n +x -2k = t*2k -2t

n +x = 2k + t*2k -2t

n +x = 2k(1 + t) -2t

This seems messy.

Maybe there's a better way to approach this.

Let me consider that in this case, m =2k -x

But m =n mod (2k -2)

So, n mod (2k -2) =2k -x

But 2k -x must be <=2k -2, since m <=2k -2

So, 2k -x <=2k -2

Which implies x >=2

Also, since m >k, and m =2k -x, we have 2k -x >k

So, k >x

Therefore, in this case, k >x and x >=2

So, k >x >=2

Now, n mod (2k -2) =2k -x

Which can be written as n ≡2k -x mod (2k -2)

But 2k -x is equivalent to -x mod (2k -2), since 2k -x = -x +2k

But 2k ≡0 mod (2k -2), because 2k =2(k -1) +2 ≡2 mod (2k -2)

Wait, this might not help.

Alternatively, perhaps I can express it as:

n ≡2k -x mod (2k -2)

Which implies n - (2k -x) is divisible by (2k -2)

So, n -2k +x = m*(2k -2) for some integer m >=0

Let me rearrange:

n +x -2k = m*(2k -2)

So, n +x -2k = m*(2k -2)

Let me solve for k:

n +x -2k = m*(2k -2)

n +x -2k = 2m*k -2m

n +x =2m*k +2k -2m

n +x =k*(2m +2) -2m

n +x +2m =k*(2m +2)

So, k=(n +x +2m)/(2m +2)

Simplify:

k=(n +x +2m)/(2(m +1))

k=(n +x +2m)/(2m +2)

This still seems complicated.

Maybe I need to find another way.

Let me consider that in both cases, m =n mod (2k -2)

In case 1: m <=k => m =x

In case 2: m >k => m =2k -x

So, for each possible k, I can compute m =n mod (2k -2)

Then, check if m <=k and m =x, or m >k and m =2k -x

But solving this directly seems tricky.

An alternative approach is to iterate over possible d, where d=2k -2 divides either n -x or n +x -2k

Wait, but n +x -2k involves k, which is what we're solving for.

This seems circular.

Wait, perhaps I can consider d=2k -2 divides n -x for case 1 and d=2k -2 divides n +x -2k for case 2.

But in case 2, it's still complicated.

Maybe I need to find a better way to handle case 2.

Let me consider that in case 2, k >x, since m >k implies 2k -x >k, which simplifies to k >x

But k >x, and x >=2

So, perhaps I can handle case 1 and case 2 separately.

For case 1: m <=k => m =x

So, n -x is divisible by d=2k -2

Hence, d divides n -x, d=2(k -1), k=(d +2)/2

Constraints: d divides n -x, d >=2, d even, k=(d +2)/2 >x (since k >x in this case)

Wait, no, in case 1, k can be <=x or >x, but according to earlier analysis, in case 1, m <=k, which is x <=k

So, in case 1, k >=x

But in case 2, k >x

Wait, I need to reconcile this.

Wait, in case 1: m <=k => m =x, and x <=k

In case 2: m >k => m =2k -x, and k >x

So, in case 1: k >=x

In case 2: k >x

So, overall, k >=x for case 1, and k >x for case 2.

Now, for case 1: d=2k -2 divides n -x, k=(d +2)/2, d >=2, d even

Similarly, for case 2: d=2k -2 divides n +x -2k, but k=(d +2)/2

Substituting k in terms of d:

n +x -2*((d +2)/2) = n +x -d -2

So, n +x -d -2 is divisible by d

Wait, but d divides n +x -d -2

Which implies d divides (n +x -d -2)

Which implies d divides (n +x -2 -d)

Which implies d divides (n +x -2) -d

Which implies d divides (n +x -2) -d

But d divides d, so d divides (n +x -2)

Wait, this seems inconsistent.

Wait, if d divides (n +x -2 -d), then d divides (n +x -2)

Because d divides d, and d divides (n +x -2 -d), so d divides (n +x -2)

So, in case 2, d=2k -2 divides (n +x -2)

And k=(d +2)/2

Constraints: d >=2, d even, k >x

So, k=(d +2)/2 >x

Which implies d +2 >2x

So, d >2x -2

Also, since d=2k -2 and k >x, d=2k -2 >2x -2

But k >=2, d >=2

So, for case 2: d divides (n +x -2), d >=2, d even, d >2x -2

Similarly, for case 1: d divides (n -x), d >=2, d even, k=(d +2)/2 >=x

Which implies d +2 >=2x, so d >=2x -2

But d >=2, so d >= max(2, 2x -2)

But x >=1, n >=x +1 >=2, so d >=2

So, in practice, d >=2

So, for case 1: d divides (n -x), d >=2, d even, k=(d +2)/2 >=x

For case 2: d divides (n +x -2), d >=2, d even, k=(d +2)/2 >x

Now, to find all k that satisfy either case, I need to:

- For case 1: find all even d that divide (n -x), and k=(d +2)/2 >=x

- For case 2: find all even d that divide (n +x -2), and k=(d +2)/2 >x

Then, combine the results from both cases, making sure to avoid duplicates.

But since d=2(k -1), and k >=2, d >=2, and d even.

So, for case 1: d divides (n -x), d >=2, d even, and (d +2)/2 >=x

Similarly, for case 2: d divides (n +x -2), d >=2, d even, and (d +2)/2 >x

Now, I need to find all such d for both cases and count unique k.

Potential optimizations:

- Since d divides (n -x) or (n +x -2), and d >=2, d even,

- I can find all divisors of (n -x) and (n +x -2), select the even ones >=2,

- Then compute k=(d +2)/2, and check the constraints for each case.

- Finally, count unique k that satisfy either case.

Edge cases to consider:

- n -x =0: but n >x, so n -x >=1

- n +x -2 <0: but n >x >=1, so n +x -2 >=0 only if n +x >=2, which is true for n >=2, x >=1

- k must be integer >1

- x=1: in case 1, k >=x=1, but k >1, so k >=2

- x >=2: in case 2, k >x

Implementing this efficiently is crucial, given the constraints n and x up to 1e9.

So, I need an efficient way to find divisors of (n -x) and (n +x -2).

An efficient way to find all divisors of a number is to iterate up to sqrt(number), which is feasible since n up to 1e9.

So, in code, for each test case:

- Compute n -x and n +x -2

- Find all even divisors d >=2 of n -x (for case 1)

- For each d, compute k=(d +2)/2, check if k >=x, if so, include it in output

- Find all even divisors d >=2 of n +x -2 (for case 2)

- For each d, compute k=(d +2)/2, check if k >x, if so, include it in output

- Combine both lists, remove duplicates, and count the number of unique k

Now, to implement this, I need a function to find all even divisors >=2 of a given number.

Let's write a function func_1(x) that returns all even divisors of x that are >=2.

Implementation:

- Iterate i from 1 to sqrt(x)

- If x % i ==0:

- If i is even, add i to output

- If x/i is even and x/i !=i, add x/i to output

- Return the list of divisors

Then, for each test case:

- Compute n -x and n +x -2

- Find even divisors of n -x and n +x -2 using func_1

- For case 1: for each d in even divisors of n -x, k=(d +2)/2, if k >=x, include k in output

- For case 2: for each d in even divisors of n +x -2, k=(d +2)/2, if k >x, include k in output

- Combine both lists, remove duplicates, and count the number of unique k

Also, need to make sure that k is integer and k >1, but since d >=2 and d even, k=(d +2)/2 is integer >=2

Now, implement this logic in code.

Looking at the given code:

t = int(input())

for i in range(t):

(n, x) = map(int, input().split())

output = []

if (n + x -2) % 2 == 0:

sep = func_1(n + x -2)

for s in sep:

if (s + 2) % 2 == 0 and (s + 2) / 2 >= x:

output.append((s + 2) / 2)

if (n - x) % 2 == 0:

sep = func_1(n - x)

for s in sep:

if (s + 2) % 2 == 0 and (s + 2) / 2 >= x:

output.append((s + 2) / 2)

output = list(set(output))

print(len(output))

def func_1(x):

output1 = []

output2 = []

for i in range(1, int(x ** 0.5) +1):

if x % i ==0:

output1.append(i)

output2.append(int(x / i))

output1.reverse()

return output2 + output1

Analysis of the given code:

- For each test case, read n and x

- Initialize an empty list output to store possible k values

- Check if (n + x -2) % 2 ==0

- If true, find even divisors of (n + x -2) using func_1

- For each even divisor s, if (s +2) %2 ==0 and (s +2)/2 >=x, append (s +2)/2 to output

- Check if (n -x) %2 ==0

- If true, find even divisors of (n -x) using func_1

- For each even divisor s, if (s +2) %2 ==0 and (s +2)/2 >=x, append (s +2)/2 to output

- Remove duplicates by converting output to a set, then to a list

- Print the length of the output list

Function func_1(x):

- Find all divisors of x by iterating from 1 to sqrt(x)

- For each i that divides x, append i to output1 and x/i to output2

- Reverse output1 and concatenate with output2 to get all divisors

Issues with the code:

- The condition (n + x -2) % 2 ==0 is checked before finding even divisors of (n + x -2)

- Similarly, (n -x) %2 ==0 is checked before finding even divisors of (n -x)

- However, in our earlier analysis, for case 1, we need d=2k -2 divides (n -x), and d even

- Similarly, for case 2, d=2k -2 divides (n +x -2), and d even

- But d=2k -2 is always even for k >=2

- So, why check (n + x -2) % 2 ==0 and (n - x) % 2 ==0?

- Perhaps there's a mistake here.

Let me verify.

Wait, (n + x -2) % 2 ==0 is equivalent to n + x even.

Similarly, (n - x) % 2 ==0 is equivalent to n and x both even or both odd.

But in our earlier analysis, d=2k -2 divides (n -x) or (n +x -2), and d even.

But d=2k -2 is always even for k >=2.

So, why is the code checking if (n + x -2) is even before finding even divisors?

Wait, perhaps the code is trying to ensure that (n + x -2) is divisible by 2, so that even divisors can be found.

But d=2k -2 is always even, so d divides (n +x -2) implies (n +x -2) is even only if d is even.

Wait, no, d even divides (n +x -2) only if (n +x -