To calculate the output, we first examine the expressions being printed. The variable `n` is a positive odd integer greater than 2. Let's denote `n` as an odd integer, for example, 3, 5, 7, etc.

The expressions are:
1. `(n * n - 1) / 2`
2. `(n * n + 1) / 2`

For an odd integer `n`, we can compute these expressions step by step.

For example, if `n = 3`:
1. `n * n` = `3 * 3` = `9`
   - Thus, `(n * n - 1) / 2` = `(9 - 1) / 2` = `8 / 2` = `4`
   - And `(n * n + 1) / 2` = `(9 + 1) / 2` = `10 / 2` = `5`

If `n = 5`:
1. `n * n` = `5 * 5` = `25`
   - Thus, `(n * n - 1) / 2` = `(25 - 1) / 2` = `24 / 2` = `12`
   - And `(n * n + 1) / 2` = `(25 + 1) / 2` = `26 / 2` = `13`

Since `n` can be any odd integer greater than 2, the results will vary. However, we can summarize the output state as follows:

Output State: **`n` is a positive odd integer greater than 2; the outputs are `(n * n - 1) / 2` and `(n * n + 1) / 2`.**