Reasoning:
The provided function `func_1` is supposed to calculate the difference between the sum of cubes of the first `n` natural numbers and the sum of the first `n` natural numbers. However, there are a few issues with the implementation:

1. The calculation for the sum of the first `n` natural numbers (`sum_n`) is correct: `sum_n = n * (n + 1) // 2`.
2. The calculation for the sum of cubes of the first `n` natural numbers (`sum_cubes_n`) is incorrect. The formula for the sum of cubes of the first `n` natural numbers is \((\frac{n(n+1)}{2})^2\), which is correctly implemented as `sum_cubes_n = sum_n ** 2`.
3. The function returns `sum_cubes_n - sum_n`, which should indeed be the difference between the sum of cubes and the sum of the first `n` natural numbers.

However, the provided test cases do not match the expected output based on the correct formula. Let's verify the test cases:

- For `n = 3`:
  - Sum of the first 3 natural numbers: \(1 + 2 + 3 = 6\)
  - Sum of cubes of the first 3 natural numbers: \(1^3 + 2^3 + 3^3 = 1 + 8 + 27 = 36\)
  - Difference: \(36 - 6 = 30\) (Correct)

- For `n = 5`:
  - Sum of the first 5 natural numbers: \(1 + 2 + 3 + 4 + 5 = 15\)
  - Sum of cubes of the first 5 natural numbers: \(1^3 + 2^3 + 3^3 + 4^3 + 5^3 = 1 + 8 + 27 + 64 + 125 = 225\)
  - Difference: \(225 - 15 = 210\) (Correct)

- For `n = 2`:
  - Sum of the first 2 natural numbers: \(1 + 2 = 3\)
  - Sum of cubes of the first 2 natural numbers: \(1^3 + 2^3 = 1 + 8 = 9\)
  - Difference: \(9 - 3 = 6\) (Correct)

Given that the test cases are correct and the function implementation matches the expected logic, the program is correct.

Correctness: **True**