The given code snippet modifies the variable `p` by updating its value based on the current values of `p`, `v`, and `m`. Here's the updated state:

The new value of `p` is calculated as `(p * v) % m`.

Given that `v` is `b[n-1]`, the new value of `p` is `(p * b[n-1]) % m`.

All other variables remain unchanged.

Output State: **`t` is an integer such that 1 ≤ t ≤ 10^4; `n` is an integer such that 1 ≤ n ≤ 2·10^5; `m` is an integer such that 1 ≤ m ≤ 10^4; `a` is a list of `n` integers where each integer `a_i` satisfies 1 ≤ `a_i` ≤ 10^4; `s` is a string of length `n` consisting only of the characters 'L' and 'R'; `b` is a list containing all `n` elements from `a`, ordered according to the sequence specified by `s`; `l` is `n`; `r` is -1; `i` is `n - 2`; `ans` is `[p, p]`; `p` is `(p * b[n-1]) % m`; `v` is `b[n-1]`**