Output State: **`k` is an integer such that \(2 \leq k \leq 30\), `x` is an integer such that \(1 \leq x \leq 100\), `a` is an integer such that \(1 \leq a \leq 10^9\), `t` is now `t - 1`, `z` is 3, `i` is `i_value + 1`, `x` must be a positive integer within the range \(1 \leq x \leq 100\)**.

Explanation: The value of `z` is updated by adding `z // (k - 1) + 1` to its current value. Given that `z` was initially 2, `z // (k - 1)` will be 0 because \(k - 1\) is at least 1, making the entire expression `0 + 1 = 1`. Thus, `z` becomes `2 + 1 = 3`. All other variables remain unchanged.