Let's break down the initial state and the code snippet to understand what will be printed.

### Initial State:
1. `n` is at least 1.
2. `root` is the integer part of the square root of `n` plus 1.
3. `i` is `root + 1`.
4. `cnt` is `root * root`.
5. `ans` is increased by the sum of `(n + i) // (i * i)` for all `i` from 2 to `root`.

### Step-by-Step Analysis:
1. **Calculate `root`**:
   - `root` is the integer part of the square root of `n` plus 1.
   - For example, if `n = 10`, then `root = int(sqrt(10)) + 1 = 3 + 1 = 4`.

2. **Calculate `i`**:
   - `i` is `root + 1`.
   - Using the example, if `root = 4`, then `i = 4 + 1 = 5`.

3. **Calculate `cnt`**:
   - `cnt` is `root * root`.
   - Using the example, if `root = 4`, then `cnt = 4 * 4 = 16`.

4. **Calculate `ans`**:
   - `ans` is increased by the sum of `(n + i) // (i * i)` for all `i` from 2 to `root`.
   - Let's break this down further:
     - For each `i` from 2 to `root`, compute `(n + i) // (i * i)`.
     - Sum these values to get the final `ans`.

### Example Calculation:
Let's use `n = 10` as an example to illustrate the calculation of `ans`:
- `root = 4`
- `i` ranges from 2 to 4.

For each `i`:
- When `i = 2`:
  - `(n + i) // (i * i) = (10 + 2) // (2 * 2) = 12 // 4 = 3`
- When `i = 3`:
  - `(n + i) // (i * i) = (10 + 3) // (3 * 3) = 13 // 9 = 1`
- When `i = 4`:
  - `(n + i) // (i * i) = (10 + 4) // (4 * 4) = 14 // 16 = 0`

Summing these values:
- `ans = 3 + 1 + 0 = 4`

### General Case:
- The exact value of `ans` depends on the value of `n`.
- The formula for `ans` is:
  \[
  \text{ans} = \sum_{i=2}^{\text{root}} \left( \frac{n + i}{i^2} \right)
  \]
- `root` is the integer part of the square root of `n` plus 1.

### Final Output:
The `print(ans)` statement will print the value of `ans`, which is the sum of \((n + i) // (i * i)\) for all `i` from 2 to `root`.

Output: **ans (where ans is the sum of \((n + i) // (i * i)\) for all \(i\) from 2 to \(\text{root}\), and \(\text{root}\) is the integer part of the square root of \(n\) plus 1)**