The code `h -= (h + 1) // 2` updates the value of `h`. Let's break down the calculation:

1. `h` is initially set to `n`.
2. `(h + 1) // 2` computes the integer division of `h + 1` by 2.
3. `h` is then updated by subtracting the result of the integer division from its current value.

Let's calculate the new value of `h`:

- Initial value of `h` is `n`.
- `(h + 1) // 2` is equivalent to `(n + 1) // 2`.
- Therefore, `h -= (n + 1) // 2` means `h = n - (n + 1) // 2`.

To simplify further:
- If `n` is even, `(n + 1) // 2` is `n // 2 + 1`.
- If `n` is odd, `(n + 1) // 2` is `(n + 1) // 2`.

So, the new value of `h` is:
- If `n` is even: `h = n - (n // 2 + 1) = n - n // 2 - 1`.
- If `n` is odd: `h = n - (n + 1) // 2 = n - (n + 1) // 2`.

In both cases, the new value of `h` is `n - (n + 1) // 2`.

Therefore, the output state is:
Output State: **`t` remains an integer such that 1 ≤ t ≤ 5 · 10^4, `n` and `k` are integers such that 1 ≤ k ≤ n ≤ 10^9, `n` and `k` are the values read from the input, `s` is equal to `k`, `d` is 0, `h` is `n - (n + 1) // 2`, `p` is 1, `g` is (`n` + 1) // 2, `f` is undefined, `y` is undefined, and `i` is at least 2.**