Output State: **`t` remains an integer such that 1 ≤ t ≤ 5 · 10^4, `n` and `k` are integers such that 1 ≤ k ≤ n ≤ 10^9, `s` is equal to `k`, `d` is 0, `h` is now `n - (n + 1) // 2 - ((n - (n + 1) // 2 + 1) // 2) - ((n - (n + 1) // 2 - ((n - (n + 1) // 2 + 1) // 2) + 1) // 2)`, `p` is 3, `g` is (`n` + 1) // 2 + (`h` + 1) // 2 + (`h` + 1) // 2, `f` is undefined, `y` is undefined, and `i` is at least 4.**

Explanation:
- The value of `h` is updated by subtracting `(h + 1) // 2` from its current value.
- All other variables remain unchanged.
- The new value of `h` is calculated as `h -= (h + 1) // 2`, which simplifies to the expression given in the output state.