Example Answer:
`a` is decreased by the value of `k * v`, so `a` becomes `a - k * v`. Then, `b` is updated by subtracting `(k - 1)` from its previous value. The Output State is: `k, a, b, and v` are integers such that 2 ≤ k ≤ 1000, 1 ≤ a, b, v ≤ 1000; `res` is 2, `a` is decreased by the value of `k * v`, `b` is updated by subtracting `(k - 1)`.
Output State: **`k, a, b, and v` are integers such that 2 ≤ k ≤ 1000, 1 ≤ a, b, v ≤ 1000; `res` is 2, `a` is decreased by the value of `k * v`, `b` is updated by subtracting `(k - 1)`**