The code snippet provided is:
```python
sum[i] = sum[i - 1] + nums[i - 1] - 1
```

Given the initial state, `i` is `n + 1`. So, the code modifies the `sum` list at index `i` (which is `n + 1`), setting its value to `sum[n] + nums[n] - 1`.

The initial state specifies that `sum` is a list of `n + 1` integers where `sum[i] = sum[i - 1] + nums[i - 1] - 1` for `1 ≤ i ≤ n`. Therefore, `sum[n]` is already defined based on the previous elements of `nums`.

The impact of the code is that it calculates the value for `sum[n + 1]` and assigns it. The other variables remain unchanged.

Output State: **`t` is an integer such that 1 ≤ t ≤ 10^4; `n` is an input integer where 1 ≤ n ≤ 3 · 10^5; `q` is an input integer where 1 ≤ q ≤ 3 · 10^5; `c` is a list of `n` integers where each element `c_i` satisfies 1 ≤ `c_i` ≤ 10^9; `nums` is a list of integers read from the input; `ones` is a list of `n + 1` integers where `ones[i]` is the cumulative count of 1s from `nums[0]` to `nums[i-1]` and `ones[n + 1]` is equal to `ones[n]`; `sum` is a list of `n + 1` integers where `sum[i] = sum[i - 1] + nums[i - 1] - 1` for 1 ≤ i ≤ n and `sum[n + 1] = sum[n] + nums[n] - 1`; `i` is `n + 1`.**