Let's break down the initial state and the code step by step:

1. **Initial State**:
   - `t` is an integer such that \(1 \leq t \leq 5 \times 10^4\).
   - `n` becomes 1 (since it is continuously halved and will reach 1 when fully divided).
   - `k` is the input integer.
   - `s` is the sum of all `x` values calculated during each iteration.
   - `m` is \(2^3 = 8\) (as `m` is multiplied by 2 for each iteration, and the loop executes 3 times).
   - `x` is \((n + 1) // 2 = (1 + 1) // 2 = 1\).

2. **Code Snippet**:
   ```python
   print((2 * (k - s) - 1) * m)
   ```

3. **Analysis**:
   - `n` is 1, so `x` is \((1 + 1) // 2 = 1\).
   - Since `n` is 1, there are no further iterations, so `s` remains 1 (the sum of all `x` values from each iteration).
   - `m` is 8.
   - `k` is the input integer, but its exact value is not specified, so we'll keep it as `k`.

4. **Calculation**:
   - Substitute the known values into the expression:
     \[
     (2 * (k - s) - 1) * m = (2 * (k - 1) - 1) * 8
     \]
   - Simplify the expression inside the parentheses:
     \[
     2 * (k - 1) - 1 = 2k - 2 - 1 = 2k - 3
     \]
   - Multiply by `m`:
     \[
     (2k - 3) * 8 = 16k - 24
     \]

5. **Final Output**:
   - The expression evaluates to \(16k - 24\).

Output: **16k - 24**