The code `dp[i][j] = dp[i][j - 1]` updates the value of `dp[i][j]` to be equal to the value of `dp[i][j - 1]`. Given the initial state, `i` is 3 and `j` is 1. 

So, `dp[3][1]` becomes equal to `dp[3][0]`. The values of the other variables are not affected.

Therefore, the Output State is: `n` is an input integer (1 ≤ n ≤ 45), `k` is an input integer (1 ≤ k ≤ 45) and must be greater than 2, `M` is an input integer (1 ≤ M ≤ 2*10^9), `t` is a sorted list of `k` integers representing the time in minutes required to solve each subtask in ascending order, `dp` is a `(k + 1) x (M + 1)` 2D list where `dp[3][1]` is equal to `dp[3][0]`, `i` is 3, `j` is 1.

Output State: **`n` is an input integer (1 ≤ n ≤ 45), `k` is an input integer (1 ≤ k ≤ 45) and must be greater than 2, `M` is an input integer (1 ≤ M ≤ 2*10^9), `t` is a sorted list of `k` integers representing the time in minutes required to solve each subtask in ascending order, `dp` is a `(k + 1) x (M + 1)` 2D list where `dp[3][1]` is equal to `dp[3][0]`, `i` is 3, `j` is 1**