The given code `dp[i][j] = dp[i][j - 1]` updates the value of `dp` at index `[i][j]` to be equal to the value of `dp` at index `[i][j - 1]`. 

Given the initial state: 
- `n` is an input integer (1 ≤ n ≤ 45)
- `k` is an input integer (1 ≤ k ≤ 45) and must be greater than 2
- `M` is an input integer (1 ≤ M ≤ 2*10^9)
- `t` is a sorted list of `k` integers representing the time in minutes required to solve each subtask in ascending order
- `dp` is a `(k + 1) x (M + 1)` 2D list
- `i` is 3
- `j` is 2

The value of `dp[3][2]` becomes equal to `dp[3][1]`. 

The states of the other variables are not affected. 

Therefore, the Output State is: 
`n` is an input integer (1 ≤ n ≤ 45), 
`k` is an input integer (1 ≤ k ≤ 45) and must be greater than 2, 
`M` is an input integer (1 ≤ M ≤ 2*10^9), 
`t` is a sorted list of `k` integers representing the time in minutes required to solve each subtask in ascending order, 
`dp` is a `(k + 1) x (M + 1)` 2D list where `dp[3][2]` equals `dp[3][1]`, 
`i` is 3, 
`j` is 2.

Output State: **`n` is an input integer (1 ≤ n ≤ 45), `k` is an input integer (1 ≤ k ≤ 45) and must be greater than 2, `M` is an input integer (1 ≤ M ≤ 2*10^9), `t` is a sorted list of `k` integers representing the time in minutes required to solve each subtask in ascending order, `dp` is a `(k + 1) x (M + 1)` 2D list where `dp[3][2]` equals `dp[3][1]`, `i` is 3, `j` is 2**