Let's break down the initial state and the provided code snippet step by step to determine what will be printed.

### Initial State:
1. `c` and `r` are integers provided by user input.
2. `t` is now `t - 2` and must be greater than 0.
3. `n` and `k` are integers provided by user input.
4. Each of the `k` moves is represented by two integers `r_i` and `c_i`, where `1 <= r_i, c_i <= n`, and all moves are valid.
5. `i` is `k-1`.
6. `k` must be greater than or equal to 3.
7. `num` is the total number of times `c` was equal to `r` plus twice the number of times `c` was not equal to `r` over all `k` iterations.
8. `m` is `n - num`.
9. `m` is equal to 1.

### Analysis:
- `c` and `r` are user inputs, so their values are not explicitly known.
- `t` is adjusted to `t - 2` and must be greater than 0, but this does not affect the print statement.
- `n` and `k` are user inputs, and `k` must be at least 3.
- Each move is represented by `r_i` and `c_i`, and all moves are valid within the range `1 <= r_i, c_i <= n`.
- `i` is set to `k-1`, which is the last index of the moves list.
- `num` is calculated based on the moves:
  - `num` is the sum of the number of times `c` was equal to `r` plus twice the number of times `c` was not equal to `r`.
- `m` is `n - num`, and it is given that `m` is equal to 1.

### Calculation:
- Since `m` is equal to 1, we have:
  \[
  m = n - num = 1
  \]
  Therefore:
  \[
  num = n - 1
  \]

- `num` is the total number of times `c` was equal to `r` plus twice the number of times `c` was not equal to `r` over all `k` iterations. Let's denote:
  - `eq` as the number of times `c` was equal to `r`.
  - `neq` as the number of times `c` was not equal to `r`.

  Then:
  \[
  num = eq + 2 \times neq
  \]

- Given that `num = n - 1`, we have:
  \[
  eq + 2 \times neq = n - 1
  \]

- Since `k` is the total number of moves and `k >= 3`, we know:
  \[
  eq + neq = k
  \]

- We can solve these two equations:
  \[
  eq + 2 \times neq = n - 1
  \]
  \[
  eq + neq = k
  \]

  Subtract the second equation from the first:
  \[
  (eq + 2 \times neq) - (eq + neq) = (n - 1) - k
  \]
  \[
  neq = n - 1 - k
  \]

- Substitute `neq` back into the second equation:
  \[
  eq + (n - 1 - k) = k
  \]
  \[
  eq = k - (n - 1 - k)
  \]
  \[
  eq = 2k - n + 1
  \]

- Since `m` is equal to 1, the print statement will output 1.

### Final Output:
Output: **1**