The expressions involve calculations based on the value of `n`. Here, `n` is a positive odd integer greater than 2. 

1. The expression `n * n - 1` computes the square of `n` and subtracts 1.
2. The expression `n * n + 1` computes the square of `n` and adds 1.
3. Both results are then divided by 2.

Since `n` is an odd integer greater than 2, let's denote `n` as an odd integer value, for example, `n = 3, 5, 7, ..., 999999999`. 

- For example, if `n = 3`: 
  - `n * n - 1` = `3 * 3 - 1` = `9 - 1` = `8`
  - `n * n + 1` = `3 * 3 + 1` = `9 + 1` = `10`
  - After division: `8 / 2 = 4` and `10 / 2 = 5`
  
- If `n = 5`: 
  - `n * n - 1` = `5 * 5 - 1` = `25 - 1` = `24`
  - `n * n + 1` = `5 * 5 + 1` = `25 + 1` = `26`
  - After division: `24 / 2 = 12` and `26 / 2 = 13`

Thus, the output consists of two parts based on the calculations involving `n`.

Output State: **`n` is a positive integer such that 1 ≤ `n` ≤ 10^9, `n` is greater than 2, and `n` is an odd integer; outputs are (n * n - 1) / 2 and (n * n + 1) / 2**.