`value` is incremented by `q ** (n - i - 1)`. Given that `q` is 5, the expression `q ** (n - i - 1)` calculates `5 ** (n - i - 1)`. Since `s[i] == '1'`, the index `i` points to a character '1' in the string `s`. The value of `n` is greater than 0, so `n - i - 1` is a non-negative integer. The value of `value` is updated accordingly.

Output State: **`s` is a non-empty string, `q` is 5, `value` is 0 plus 5 raised to the power of (n - i - 1), `n` is greater than 0, the current value of `i` satisfies `s[i] == '1'`**