The code snippet `ls += nums[i]` adds the value of `nums[i]` to the current value of `ls`. Given that `i` is 2, this means `ls` will be updated by adding `nums[2]` to it.

From the initial state, we know:
- `ls` is initially `nums[0] + nums[1]`.
- `nums[2]` is `nums[2] - (nums[0] + nums[1])`.

After executing `ls += nums[i]`, `ls` becomes:
\[ \text{ls} = (\text{nums}[0] + \text{nums}[1]) + (\text{nums}[2] - (\text{nums}[0] + \text{nums}[1])) = \text{nums}[2] \]

The other variables (`t`, `n`, the list of integers `a_1, a_2, ..., a_n`, `N`, `nums`, and `i`) remain unchanged.

Output State: **`t` is an integer such that 1 ≤ t ≤ 10^4; `n` is an integer such that 1 ≤ n ≤ 2·10^5, and a list of n integers a_1, a_2, ..., a_n where each a_i is an integer such that 1 ≤ a_i ≤ 10^9; `N` is an input integer; `nums` is a sorted list of unique integers obtained from the input string and includes the integer `0`, with `nums[i]` reduced by `nums[0]` and `nums[2]` is now `nums[2] - (nums[0] + nums[1])`; `ls` is `nums[2]`; `i` is 2.**