To determine the output of the given `print` statement, we need to analyze the provided initial state and understand how the variables are defined and computed.

### Initial State Breakdown:
1. **`t`**: An integer such that \(1 \leq t \leq 10^4\). This variable represents the number of test cases or iterations.
2. **`T`**: Greater than 0. This variable is not directly used in the provided code snippet, so it doesn't affect the output.
3. **`info`**: A list of strings obtained from splitting an input line. This list contains two elements.
4. **`a`**: The integer value of `info[0]`. This is the first integer from the input line.
5. **`b`**: The integer value of `info[1]`. This is the second integer from the input line.
6. **`suma`**: The accumulated sum of \(x\) for each iteration where \(a - i \cdot (i - 1) > 0\).

### Calculation of `suma`:
The variable `suma` is calculated through an iterative process. Let's break down the loop condition and the summation:

- The loop runs for \(i = 1, 2, 3, \ldots\) until the condition \(a - i \cdot (i - 1) \leq 0\) is met.
- For each valid \(i\), the term \(x\) is added to `suma`. The value of \(x\) is not explicitly defined in the problem statement, but based on typical problems of this nature, \(x\) is often \(i\). Therefore, we assume \(x = i\).

Thus, `suma` can be expressed as:
\[ \text{suma} = \sum_{i=1}^{k} i \]
where \(k\) is the largest integer such that \(a - k \cdot (k - 1) > 0\).

### Deriving the Output:
The `print` statement outputs `suma - 1`.

Let's summarize the steps:
1. Determine the maximum \(k\) such that \(a - k \cdot (k - 1) > 0\).
2. Calculate `suma` as the sum of integers from 1 to \(k\).
3. Subtract 1 from `suma` to get the final output.

### Example Calculation:
Assume \(a = 10\):
- For \(i = 1\): \(10 - 1 \cdot 0 = 10 > 0\)
- For \(i = 2\): \(10 - 2 \cdot 1 = 8 > 0\)
- For \(i = 3\): \(10 - 3 \cdot 2 = 4 > 0\)
- For \(i = 4\): \(10 - 4 \cdot 3 = -2 \leq 0\) (stop here)

So, \(k = 3\), and `suma` is:
\[ \text{suma} = 1 + 2 + 3 = 6 \]

Finally, the output is:
\[ \text{suma} - 1 = 6 - 1 = 5 \]

### General Case:
For any given \(a\), the output will be the sum of the first \(k\) integers minus 1, where \(k\) is the largest integer such that \(a - k \cdot (k - 1) > 0\).

### Final Output Description:
The `print` statement will output the value of `suma - 1`, where `suma` is the sum of integers from 1 to the largest \(k\) such that \(a - k \cdot (k - 1) > 0\).

Output: **suma - 1 (where suma is the sum of integers from 1 to the largest k such that a - k * (k - 1) > 0)**