The code updates the value of `triangular_number` to `k * (k + 1) // 2`. Given the initial state where `k` is 2, we can calculate the new value of `triangular_number` as follows:

- Initial value of `k` is 2.
- Calculation: `triangular_number = k * (k + 1) // 2` becomes `triangular_number = 2 * (2 + 1) // 2 = 2 * 3 // 2 = 6 // 2 = 3`.

So, the new value of `triangular_number` is 3. The other variables (`n` and `k`) remain unchanged.

Output State: **`n` is a positive integer, `k` is 2, `triangular_number` is 3, and the length of the string representation of `triangular_number` must eventually be equal to `n`**