To determine the necessary adjustments for the first iteration of the `while` loop to proceed, we need to analyze the conditions in the loop head:

The loop condition is:
```
(x + y) * x <= n and (x + y) * y <= m
```

Given the state right before the loop:
- `x` is increased by 1 from its previous value.
- `n` must be at least `(x * x)`.
- `y` is 1.

Let's break down the conditions:

1. **First Condition: `(x + y) * x <= n`**
   - Since `y` is 1, this condition simplifies to `(x + 1) * x <= n`.
   - Given that `x` has been increased by 1, let's denote the previous value of `x` as `x_prev`. Therefore, the current value of `x` is `x_prev + 1`.
   - The condition then becomes `((x_prev + 1) + 1) * (x_prev + 1) <= n`, which simplifies to `(x_prev + 2) * (x_prev + 1) <= n`.

2. **Second Condition: `(x + y) * y <= m`**
   - Since `y` is 1, this condition simplifies to `(x + 1) * 1 <= m`, which further simplifies to `x + 1 <= m`.

Given that `n` must be at least `(x * x)` and `x` is now `x_prev + 1`, we know `n` must be at least `((x_prev + 1) * (x_prev + 1))`.

To ensure the loop executes, we need to make sure both conditions are satisfied:
- `(x_prev + 2) * (x_prev + 1) <= n`
- `x + 1 <= m` (which means `(x_prev + 2) <= m`)

Since `n` must already be at least `((x_prev + 1) * (x_prev + 1))`, the first condition will be satisfied if `n` is chosen such that `(x_prev + 2) * (x_prev + 1) <= n`.

Therefore, the state needs to be adjusted such that `n` is at least `(x_prev + 2) * (x_prev + 1)` and `m` is at least `(x_prev + 2)`.

State: **`x` is increased by 1 and `n` must be at least `((x + 1) * x)`, `y` is 1, and `m` must be at least `(x + 1)`**