Output State: **`t` is an integer such that 1 <= t <= 500, `n` is an input integer such that 1 <= n <= 500 and `n` must be at least 1, `mat` is a list of `n` lists, each containing integers from 1 to `n` inclusive, `res` is 4, `i` is 1**

Explanation:
- `res` is initially 1.
- `i` is initially 1.
- The expression `(i + 1) * (2 * i + 1)` evaluates to `(1 + 1) * (2 * 1 + 1) = 2 * 3 = 6`.
- `res` is updated to `res + 6`, which is `1 + 6 = 7`.
- However, there was a mistake in the calculation. The correct value of `res` after the update is `1 + 6 = 7`, not 4. Let's correct this:

Output State: **`t` is an integer such that 1 <= t <= 500, `n` is an input integer such that 1 <= n <= 500 and `n` must be at least 1, `mat` is a list of `n` lists, each containing integers from 1 to `n` inclusive, `res` is 7, `i` is 1**