The code snippet `res += k % (i + 1)` updates the value of `res` by adding the result of `k % (i + 1)` to its current value. Let's break down the impact:

1. `res` is initially `n - 1`.
2. `k % (i + 1)` computes the remainder of `k` divided by `i + 1`.
3. `res` is then updated to `n - 1 + k % (i + 1)`.

The other variables and conditions remain unchanged. Therefore, the output state is:

Output State: **`ans_list` is an empty list, `t` is an integer where 1 ≤ t ≤ 100, `n` is an integer provided by the user input where 2 ≤ n ≤ 2 · 10^5, `k` is an integer provided by the user input where 0 ≤ k ≤ 10^12, `a` is a sorted list of integers where 1 ≤ a_i ≤ 10^12, the sum of `n` over all test cases does not exceed 5 · 10^5, `_` is 0, `ans` is equal to the first element of `a` plus `k // (i + 1)`, `i` is not 0, `dif` is not 0, `k` is less than `dif * (i + 1)`, and `res` is equal to `n - 1 + k % (i + 1)`.**