Alright, I have this problem to solve. Let me try to understand it step by step. So, the problem is about helping Vasya remember the possible values of k based on his position in the line and the number he received during the settling.

First, I need to understand what "settling in 'the firstâ€“k -th' position" means. From the description, it seems like the line is divided into segments of 2k - 2 people, and within each segment, the first k people are numbered 1 to k, and the next k-2 people are numbered k-1 down to 2. This pattern repeats every 2k - 2 positions.

So, for a given position n and number x, I need to find all possible k > 1 such that at position n, the number assigned is x.

Let me look at the example provided:

Input:

5

10 2

3 1

76 4

100 99

1000000000 500000000

Output:

4

1

9

0

1

For the first test case, n=10 and x=2, the possible k values are 2,3,5,6.

Looking at the table:

k | 1 | 2 | 3 | 4 | 5 | 6 | 7 | 8 | 9 |10

---|---|---|---|---|---|---|---|---|---|---

2 | 1 | 2 |1 |2 |1 |2 |1 |2 |1 |2

3 | 1 |2 |3 |2 |1 |2 |3 |2 |1 |2

5 |1 |2 |3 |4 |5 |4 |3 |2 |1 |2

6 |1 |2 |3 |4 |5 |6 |5 |4 |3 |2

Indeed, for k=2,3,5,6, the 10th position has x=2.

Now, I need to generalize this for any n and x.

First, I need to find a way to express the number at position n for a given k.

Let's observe the pattern:

- For k=2: the sequence is 1,2,1,2,1,2,...

- For k=3: 1,2,3,2,1,2,3,2,1,...

- For k=5: 1,2,3,4,5,4,3,2,1,2,3,4,5,4,3,2,1,...

- For k=6: 1,2,3,4,5,6,5,4,3,2,1,2,3,4,5,6,5,4,3,2,...

I see that the pattern repeats every 2k - 2 positions.

For example, for k=3, the pattern is 1,2,3,2,1 and repeats every 4 positions (2*3 - 2=4).

Similarly, for k=5, the pattern is 1,2,3,4,5,4,3,2,1 and repeats every 8 positions (2*5 - 2=8).

So, the repeating block has length 2k - 2.

Within each block:

- Positions 1 to k: numbers 1 to k

- Positions k+1 to 2k-2: numbers k-1 down to 2

So, for a given position n, I can find its position within the block by computing (n-1) mod (2k - 2) +1.

Let me denote m = (n-1) mod (2k - 2) +1

Then:

- If 1 <= m <= k, number is m

- If k < m <= 2k - 2, number is 2k - m

So, for a given k, the number at position n is:

if m <= k:

x = m

else:

x = 2k - m

Now, given n and x, I need to find all k >1 such that this equation holds.

So, I have:

m = (n-1) mod (2k - 2) +1

if m <= k:

x = m

else:

x = 2k - m

So, two cases:

1. m <= k => x = m => m = x

2. m > k => x = 2k - m => m = 2k - x

In both cases, m is determined by n and k via m = (n-1) mod (2k - 2) +1

So, I can set up equations based on these cases.

Let me consider case 1: m <= k => m = x

So, (n-1) mod (2k - 2) +1 = x

=> (n-1) mod (2k - 2) = x -1

Since a mod b = r, where 0 <= r < b

So, 0 <= x -1 < 2k -2 => x -1 < 2k -2 => x < 2k -1 => k > (x+1)/2

Also, since k >1, so k >= max(2, ceil((x+1)/2))

Also, since m = x, and m <= k, so x <= k

So, k >= x

Combining, k >= max(2, x)

Now, (n-1) mod (2k - 2) = x -1

This implies that n-1 = q*(2k -2) + (x -1) for some integer q >=0

So, n-1 = q*(2k -2) + x -1

=> n - x = q*(2k -2)

=> n - x must be divisible by 2k -2

So, 2k -2 divides n -x

Similarly, since 2k -2 >0, and n -x can be positive or negative, but in the problem, it's given that 1 <= x < n <= 10^9, so n -x >0

So, n -x >0

So, q >=0

Now, 2k -2 divides n -x

So, 2k -2 is a divisor of n -x

Let me denote d = 2k -2

Then, d divides n -x

So, d | n -x

Also, k = (d +2)/2

Since k must be an integer >1, d must be an even number >=2

Because k >=2 => d >=2, and d must be even so that k is integer.

So, for each even divisor d of n -x, where d >=2, set k = (d +2)/2

But wait, d = 2k -2 => k = (d +2)/2

Also, k must satisfy k >= x (from earlier)

So, (d +2)/2 >=x => d +2 >=2x => d >=2x -2

Also, d must be even and >=2

So, for case 1, the possible k are those where d is an even divisor of n -x, d >=2x -2, and d >=2

Similarly, for case 2: m > k

So, m = 2k - x

And m = (n-1) mod (2k -2) +1

So, (n-1) mod (2k -2) +1 = 2k -x

=> (n-1) mod (2k -2) = 2k -x -1

Again, (n-1) = q*(2k -2) + (2k -x -1)

=> n -1 = q*(2k -2) + 2k -x -1

=> n -1 -2k +x +1 = q*(2k -2)

=> n -2k +x = q*(2k -2)

But since q >=0, and 2k -2 >0, n -2k +x >=0

Wait, but in this case, m > k, which means m >=k+1

But m = (n-1) mod (2k -2) +1 <= 2k -2

So, k+1 <= m <=2k -2

So, k+1 <= 2k -x -1 <=2k -2

From k+1 <=2k -x -1 => k >=x +2

And 2k -x -1 <=2k -2 => -x -1 <= -2 => x >=1, which is always true since x >=1

So, additional constraint: k >= x +1

Also, from m = 2k -x, and m <=2k -2 => 2k -x <=2k -2 => -x <= -2 => x >=2

So, for case 2 to be possible, x >=2

In this case, n -2k +x is divisible by 2k -2

Let me denote d = 2k -2 => k = (d +2)/2

Then, n -2*( (d +2)/2 ) +x = n -d -2 +x = (n +x -2 -d)

This should be divisible by d, since q is integer.

So, (n +x -2 -d) / d is integer, which implies that d divides n +x -2 -d

=> d divides n +x -2 -d

=> d divides n +x -2 -d

=> d divides (n +x -2 -d)

=> d divides (n +x -2) - d

=> d divides (n +x -2) - d

So, d divides (n +x -2) - d

But since d divides itself, and d divides (n +x -2) - d, then d divides n +x -2

Wait, that's interesting.

So, d divides n +x -2

But earlier, in case 1, d divides n -x

So, in case 1: d | (n -x)

In case 2: d | (n +x -2)

And d = 2k -2, where d is even and >=2

Also, in case 1: d >= 2x -2

In case 2: k >= x +1, which translates to d >= 2(x +1) -2 = 2x

So, in case 2: d >=2x

Wait, let's summarize:

Case 1:

- d divides (n -x)

- d >= 2x -2

- d >=2

- d even

Case 2:

- d divides (n +x -2)

- d >=2x

- d >=2

- d even

So, to find all possible k, I need to consider both cases and ensure that d meets the criteria in each case.

Then, for each case, collect the possible d, ensure they are even and >= the required minimum, and then compute k = (d +2)/2

Finally, combine the results from both cases, remove duplicates, and count the number of distinct k.

Looking at the provided code:

t = int(input())

for i in range(t):

(n, x) = map(int, input().split())

output = []

if (n + x - 2) % 2 == 0:

sep = func_1(n + x - 2)

for s in sep:

if (s + 2) % 2 == 0 and (s + 2) / 2 >= x:

output.append((s + 2) / 2)

if (n - x) % 2 == 0:

sep = func_1(n - x)

for s in sep:

if (s + 2) % 2 == 0 and (s + 2) / 2 >= x:

output.append((s + 2) / 2)

output = list(set(output))

def func_1(x):

output1 = []

output2 = []

for i in range(1, int(x ** 0.5) + 1):

if x % i == 0:

output1.append(i)

output2.append(int(x / i))

output1.reverse()

return output2 + output1

Let's analyze this code.

First, it reads the number of test cases t.

Then, for each test case, it reads n and x.

It initializes an empty list output to store possible k values.

Then, it checks if (n + x - 2) % 2 == 0. If true, it calls func_1(n + x - 2) to get the divisors, iterates through them, and for each s (divisor), if (s + 2) is even and (s + 2)/2 >= x, it appends (s + 2)/2 to output.

Similarly, it checks if (n - x) % 2 == 0. If true, it calls func_1(n - x) to get the divisors, iterates through them, and for each s, if (s + 2) is even and (s + 2)/2 >= x, it appends (s + 2)/2 to output.

Finally, it converts output to a set to remove duplicates and then back to a list.

At the end, there's a function func_1(x) that returns all divisors of x in ascending order.

Now, comparing this to our earlier reasoning:

In case 1, d divides (n -x), d >=2x -2, d even.

In case 2, d divides (n +x -2), d >=2x, d even.

In the code:

- For case 1 (d divides n -x):

It checks if (n -x) % 2 == 0 before calling func_1(n -x). Wait, but d = 2k -2, which is always even, and d divides n -x.

But in the code, it checks (n -x) % 2 == 0, which is not necessarily the same as d divides n -x.

Wait, perhaps it's a mistake.

Similarly, for case 2, it checks (n +x -2) % 2 == 0 before calling func_1(n +x -2).

Again, d divides (n +x -2), but d is even, so (n +x -2) must be even for d to divide it.

Wait, no. If d is even and d divides (n +x -2), then (n +x -2) must be divisible by d, which is even.

But the code checks if (n +x -2) is even before proceeding.

Wait, perhaps it's to ensure that d is even.

Wait, but d is always even in this problem, since k >1 and d=2k-2.

So, d is even and >=2.

Hence, when d divides (n -x) or (n +x -2), and d is even, the code is trying to find such d and then compute k=(d+2)/2.

But the condition (n +x -2) % 2 ==0 is not necessarily required for d to divide (n +x -2), because d is even.

Wait, perhaps the code is trying to ensure that (n +x -2) is even so that d can divide it, since d is even.

But actually, if d is even, and d divides (n +x -2), then (n +x -2) must be even.

Similarly, if d divides (n -x), and d is even, then (n -x) must be even.

So, the code is checking if (n +x -2) is even before considering divisors of (n +x -2), and similarly for (n -x).

This seems logical.

Then, it calls func_1 to get the divisors of (n +x -2) or (n -x), and for each divisor s, checks if (s +2) is even and (s +2)/2 >=x.

Wait, s is a divisor of (n +x -2) or (n -x), and s=d=2k-2.

So, k=(s+2)/2.

Then, it checks if (s +2)/2 >=x, which corresponds to k >=x in case 1 and k >=x+1 in case 2.

Wait, in case 1, k >=x, and in case 2, k >=x+1.

But in the code, it's (s +2)/2 >=x for both cases.

Wait, perhaps it's a mistake.

Wait, in case 2, k >=x+1, which is (s +2)/2 >=x+1, but in the code, it's (s +2)/2 >=x.

So, perhaps it's incorrect.

Wait, let's verify.

From d=2k-2, k=(d+2)/2.

In case 1: k >=x => (d+2)/2 >=x => d >=2x -2

In case 2: k >=x+1 => (d+2)/2 >=x+1 => d >=2(x+1) -2 =2x

Which matches the earlier conditions.

But in the code, it's checking (s +2)/2 >=x for both cases.

Wait, perhaps it's because in case 2, k >=x+1, and (s +2)/2 >=x+1, but the code has (s +2)/2 >=x, which would include some k that are less than x+1.

So, perhaps it's incorrect.

Wait, maybe I'm missing something.

Let me re-examine.

In case 1: k >=x

In case 2: k >=x+1

But in the code, for both cases, it's (s +2)/2 >=x

Which would include k>=x for both cases, but in case 2, it should be k>=x+1.

So, perhaps it's incorrectly including some k in case 2 that should not be included.

Wait, but in the code, for case 1, it's (n -x) % 2 ==0, and for case 2, (n +x -2) %2 ==0.

And it's using the same condition (s +2)/2 >=x for both.

Perhaps it needs to adjust the condition based on the case.

Alternatively, maybe it's compensating for the difference in the constraints.

Wait, perhaps it's correct because in case 2, d >=2x, and (s +2)/2 >=x+1, which is equivalent to s >=2x.

But in the code, it's (s +2)/2 >=x, which is s >=2x -2.

But in case 2, d >=2x, so s >=2x.

But in the code, it's s >=2x -2.

So, it's including s >=2x -2 for both cases, but in case 2, it should be s >=2x.

Hence, it's incorrectly including s >=2x -2 in both cases, whereas for case 2, it should be s >=2x.

Therefore, the code is incorrect because it doesn't account for the stricter condition in case 2.

Wait, but in case 1, d >=2x -2, and in case 2, d >=2x.

But in the code, it's using (s +2)/2 >=x, which is s >=2x -2 for both cases.

But for case 2, it should be s >=2x.

So, it's incorrectly including s >=2x -2 in both cases, which means in case 2, it's including s >=2x -2 instead of s >=2x.

Therefore, it's including some s that don't satisfy the condition for case 2.

Wait, but in case 2, k >=x+1, which is (s +2)/2 >=x+1, which is s >=2x.

So, the code should have (s +2)/2 >=x+1 for case 2, but it has (s +2)/2 >=x for both cases.

Hence, it's incorrect.

Therefore, the given program is incorrect.

**Final Answer**

\[ \boxed{\text{false}} \]