To determine the new value of `dp[i]` based on the given formula, we need to compute `(dp[i - 1] + (i - 1) * dp[i - 2] * 2) % (10 ** 9 + 7)`.

Given:
- `i` is 6
- `dp` is a list of `m + 1` zeros except `dp[1]` which is 1 and `dp[2]` which is 3

We need the values of `dp[5]` and `dp[4]` to proceed with the calculation:
- `dp[3]` is not provided directly, but since it's initialized as 0, we assume `dp[3] = 0`.
- `dp[4]` is not provided directly, but since it's initialized as 0, we assume `dp[4] = 0`.
- `dp[5]` is not provided directly, but since it's initialized as 0, we assume `dp[5] = 0`.

Using these assumptions:
- `dp[5] = 0`
- `dp[4] = 0`

Now, substituting the values into the formula:
- `dp[6] = (dp[5] + (6 - 1) * dp[4] * 2) % (10 ** 9 + 7)`
- `dp[6] = (0 + 5 * 0 * 2) % (10 ** 9 + 7)`
- `dp[6] = 0 % (10 ** 9 + 7)`
- `dp[6] = 0`

Thus, the updated `dp` list will have `dp[6]` set to 0.

Other variables (`t`, `n`, `k`, `num`, `m`) remain unchanged.

Output State: **`t` is at least 0, `n` is the first integer read from the input, `k` is the second integer read from the input, `num` is `2k - x` where `x` is the number of times `c == r` during the `k` iterations, `m` is at least 3, `dp` is a list of `m + 1` zeros except `dp[1]` which is 1, `dp[2]` which is 3, and `dp[6]` which is 0, `i` is 6**.