To determine the new value of `z` after executing the given line of code, we need to consider its current value and how it changes based on the formula provided.

Given:
- `z` is initially set to either `(y + 1) // 2` or `(y + 1) // 2 + (x - m + 14) // 15`.
- `m` is recalculated as `15 * z - y * 4`.

The line of code modifies `z` as follows:
```
z = z + (x - m + 15 - 1) // 15
```

Let's break down the new value of `z`:
- The original value of `z` remains part of the new value.
- The term `(x - m + 15 - 1) // 15` is added to `z`.

Since `m` is recalculated as `15 * z - y * 4`, we substitute this into the equation:
- `m = 15 * z - y * 4`
- Therefore, `x - m + 15 - 1 = x - (15 * z - y * 4) + 14 = x - 15 * z + y * 4 + 14`

Thus, the new value of `z` is:
- `z = z + (x - 15 * z + y * 4 + 14) // 15`

Simplifying further:
- `z = z + ((x + y * 4 + 14) - 15 * z) // 15`
- `z = z + (x + y * 4 + 14) // 15 - z`
- `z = (x + y * 4 + 14) // 15`

So, the new value of `z` is `(x + y * 4 + 14) // 15`.

The values of `t`, `a`, `x`, `y`, and `m` remain unchanged except for `z` which is recalculated.

Output State: **`t` is an integer such that 1 ≤ t ≤ 10^4, `a` is greater than 0, `x` and `y` are integers read from the input, `z` is `(x + y * 4 + 14) // 15`, `m` is recalculated as `15 * z - y * 4`.**