The code snippet `n -= i * curr` updates the value of `n` by subtracting the product of `i` and `curr` from it. Given the initial state, we know the values of `n`, `i`, and `curr`.

Let's break down the changes:
- `n` was initially `n - i * curr`.
- `i` is `n - k + 1`.
- `curr` is `n // (n - k + 1)`.

Now, the new value of `n` becomes:
\[ n = (n - i * curr) - i * curr \]
\[ n = n - 2 * i * curr \]

Since `i` and `curr` are defined in terms of `n` and `k`, the new value of `n` can be expressed as:
\[ n = n - 2 * (n - k + 1) * \left(\frac{n}{n - k + 1}\right) \]
\[ n = n - 2 * n \]
\[ n = -n \]

The values of `k`, `costs`, `h`, and `curr` remain unchanged.

Output State: **`n` is `-n`, `k` is a positive integer such that 1 ≤ k ≤ 10^{18}, `costs` is `[n - k + 1, 1]`, `h` is `curr`, `curr` is `n // (n - k + 1)`, `i` is `n - k + 1`**.