To determine the final output state after all iterations of the loop, we need to analyze the loop and how the variables change with each iteration.

The loop iterates `k` times, and in each iteration, the variable `s` is updated as follows:
\[ s = s + c \times i \times c \times m + c \times a \]
where `i` starts at `m + k` and decreases by 1 in each iteration.

Let's break down the changes in `s` for each iteration:
- After the 1st iteration, `s` becomes:
  \[ s = s + c \times (m + k) \times c \times m + c \times a \]
- After the 2nd iteration, `s` becomes:
  \[ s = s + c \times (m + k) \times c \times m + c \times a + c \times (m + k - 1) \times c \times m + c \times a \]
- After the 3rd iteration, `s` becomes:
  \[ s = s + c \times (m + k) \times c \times m + c \times a + c \times (m + k - 1) \times c \times m + c \times a + c \times (m + k - 2) \times c \times m + c \times a \]

Generalizing this, after `k` iterations, `s` will be:
\[ s = s + \sum_{j=0}^{k-1} \left( c \times (m + k - j) \times c \times m + c \times a \right) \]
\[ s = s + \sum_{j=0}^{k-1} c \times (m + k - j) \times c \times m + \sum_{j=0}^{k-1} c \times a \]
\[ s = s + c \times c \times m \times \sum_{j=0}^{k-1} (m + k - j) + c \times a \times k \]
\[ s = s + c^2 \times m \times \left( (m + k) \times k - \sum_{j=0}^{k-1} j \right) + c \times a \times k \]
\[ s = s + c^2 \times m \times \left( (m + k) \times k - \frac{k \times (k - 1)}{2} \right) + c \times a \times k \]
\[ s = s + c^2 \times m \times \left( m \times k + k^2 - \frac{k \times (k - 1)}{2} \right) + c \times a \times k \]
\[ s = s + c^2 \times m \times \left( m \times k + \frac{2k^2 - k^2 + k}{2} \right) + c \times a \times k \]
\[ s = s + c^2 \times m \times \left( m \times k + \frac{k^2 + k}{2} \right) + c \times a \times k \]
\[ s = s + c^2 \times m \times k \times \left( m + \frac{k + 1}{2} \right) + c \times a \times k \]
\[ s = s + c^2 \times m \times k \times \left( \frac{2m + k + 1}{2} \right) + c \times a \times k \]
\[ s = s + \frac{c^2 \times m \times k \times (2m + k + 1)}{2} + c \times a \times k \]

The value of `i` remains `m + k` after the loop finishes.

Thus, the final output state is:
Output State: **s is s + (c^2 * m * k * (2m + k + 1)) // 2 + c * a * k, n is the first integer from the input, m is the second integer from the input, k is the third integer from the input, M is 1000000007, c is the modular multiplicative inverse of n * (n - 1) // 2 modulo 1000000007, a is the sum of all f values read from the input during the m iterations, i is m + k.**

In natural language, after all iterations, the value of `s` is updated based on the sum of a series involving `c`, `m`, `k`, and `a`. The other variables remain unchanged.