To determine what will be printed by the `print(int(ans))` statement, let's break down the initial state and the code step by step.

### Initial State:
- `n` and `m` are positive integers such that \(1 \leq n, m \leq 2 \times 10^6\).
- `t` must be greater than 0 (though it is not used in the given code snippet).
- `i` is 0 (though it is not used in the given code snippet).
- `count` is \(m + 1\).
- `ans` is calculated as:
  \[
  \text{ans} = n + \sum_{k=2}^{m+1} \left( \frac{n}{k} - \frac{(k - 1)}{k} + 1 \right) \text{ for } k \text{ such that } \left( \frac{n}{k} - (k - 1) \right) \geq (k - 1)
  \]
- `countmins` is `m`.
- `g` is calculated as:
  \[
  g = \frac{n}{m} - (m - 1)
  \]
  If `g` is less than `countmins`, the loop breaks.

### Step-by-Step Calculation:
1. **Calculate `g`**:
   \[
   g = \frac{n}{m} - (m - 1)
   \]
   Since `g` is less than `countmins` (which is `m`), the loop breaks. This means the condition `g < m` is true.

2. **Calculate `ans`**:
   - The formula for `ans` is:
     \[
     \text{ans} = n + \sum_{k=2}^{m+1} \left( \frac{n}{k} - \frac{(k - 1)}{k} + 1 \right) \text{ for } k \text{ such that } \left( \frac{n}{k} - (k - 1) \right) \geq (k - 1)
     \]
   - Simplify the term inside the sum:
     \[
     \frac{n}{k} - \frac{(k - 1)}{k} + 1 = \frac{n - (k - 1) + k}{k} = \frac{n + 1}{k}
     \]
   - The condition for the sum is:
     \[
     \left( \frac{n}{k} - (k - 1) \right) \geq (k - 1)
     \]
     Simplify the condition:
     \[
     \frac{n}{k} \geq 2(k - 1)
     \]
     \[
     n \geq 2k(k - 1)
     \]

3. **Summation**:
   - The summation will only include terms where \( n \geq 2k(k - 1) \).
   - For each valid `k`, the term added to `ans` is \( \frac{n + 1}{k} \).

4. **Final Calculation**:
   - The final value of `ans` is:
     \[
     \text{ans} = n + \sum_{k=2}^{m+1} \left( \frac{n + 1}{k} \right) \text{ for } k \text{ such that } n \geq 2k(k - 1)
     \]

### Output:
Since the exact values of `n` and `m` are not provided, we can't compute the exact numerical value of `ans`. However, based on the given formula and conditions, the `print(int(ans))` statement will output the integer value of `ans`.

Output: **int(ans) (where ans is the sum of n and the sum of (n + 1) / k for all k from 2 to m + 1 such that n >= 2k(k - 1))**