Let's analyze the initial state and the provided Python code snippet step by step:

### Initial State:
- `i` is 0.
- `a` and `b` are integer values from the input.
- At least one of `a` or `b` is odd.
- Neither `(a - b == -a, a)` nor `(b - a == -b, b)` is true.
- The difference between `a` and `b` (`a - b`) is not divisible by 2, meaning it is odd.

### Code Snippet:
```python
print('yes')
```

### Analysis:
1. **Variables and Conditions:**
   - `i` is 0, but it is not used in the code snippet.
   - `a` and `b` are integers where at least one is odd.
   - The conditions `(a - b == -a, a)` and `(b - a == -b, b)` being false imply that the differences `a - b` and `b - a` do not simplify to `-a` or `-b` respectively.
   - The difference `a - b` is odd.

2. **Print Statement:**
   - The `print` statement simply prints the string `'yes'`.

### Conclusion:
The `print` statement does not depend on any of the variables or conditions mentioned in the initial state. It simply prints the string `'yes'`.

Output: **yes**