First, let's analyze the given code snippet:

```python
ans += 2 * y
```

Given the initial state:
- `y` is `0 - ((last_gap + 2) // 2)`
- `ans` is `ans + (last_gap + 2)`

We need to substitute the value of `y` into the equation and update `ans`.

Step 1: Calculate `y`.
\[ y = 0 - \left(\frac{last\_gap + 2}{2}\right) \]

Step 2: Update `ans` using the value of `y`.
\[ ans = ans + 2 \times y \]
Substituting `y`:
\[ ans = ans + 2 \times \left(0 - \left(\frac{last\_gap + 2}{2}\right)\right) \]
\[ ans = ans + 2 \times \left(-\frac{last\_gap + 2}{2}\right) \]
\[ ans = ans - (last\_gap + 2) \]

So, the updated value of `ans` is the original value of `ans` minus `(last_gap + 2)`.

Output State: **`y` is \(0 - \left(\frac{last\_gap + 2}{2}\right)\), `ans` is `ans - (last\_gap + 2)`**