Let's break down the initial state and the print statement step by step:

### Initial State:
- `t` must be greater than 0.
- `n` is 0.
- `k` is an input integer that must be at least 1.
- `L` is a list containing the sequence of values `[m1, m2, ..., mk]` where each `mi` is the value of `(ni + 1) // 2` for the corresponding iteration, and `ni` is the value of `n` at the start of each iteration.
- `tot` is 0.
- `pow` is 1.
- `a` is the first element in `L`.
- `tot` is less than `k` and `k` is less than or equal to `tot + a`.

### Step-by-Step Analysis:
1. **Initialization:**
   - `n = 0`
   - `k` is an integer ≥ 1.
   - `L` is a list where each element `mi` is calculated as `(ni + 1) // 2` for each iteration.
   - `tot = 0`
   - `pow = 1`
   - `a` is the first element of `L`.

2. **List `L` Construction:**
   - Since `n` starts at 0, the first element `m1` of `L` is `(0 + 1) // 2 = 0`.
   - Therefore, `a = 0`.

3. **Conditions:**
   - `tot < k` and `k ≤ tot + a`.
   - Given `a = 0`, the condition `k ≤ tot + a` simplifies to `k ≤ 0`, which is impossible since `k` is at least 1.
   - This implies there might be a misunderstanding in the initial state, but let's proceed with the given conditions.

4. **Print Statement:**
   - The print statement is `print(pow * (2 * (k - tot) - 1))`.
   - Substituting the known values:
     - `pow = 1`
     - `tot = 0`
     - `k` is an integer ≥ 1
   - The expression inside the print statement becomes:
     - `1 * (2 * (k - 0) - 1) = 2 * k - 1`

### Final Output:
The print statement will output the value of `2 * k - 1`.

Output: **2 * k - 1 (where k is the input integer and k ≥ 1)**