Based on the initial state provided:

- `n` and `k` are input integers.
- `k` is less than or equal to \((n + 1) // 2\).

The print statement is:
```python
print(2 * k - 1)
```

To determine what will be printed, we need to evaluate the expression `2 * k - 1`:

1. **Value of `k`**: According to the precondition, `k` is an integer and it is less than or equal to \((n + 1) // 2\). This means `k` can take any integer value from 1 up to \((n + 1) // 2\).

2. **Expression `2 * k - 1`**: 
   - If `k = 1`, then `2 * 1 - 1 = 1`.
   - If `k = 2`, then `2 * 2 - 1 = 3`.
   - If `k = 3`, then `2 * 3 - 1 = 5`.
   - And so on...

The expression `2 * k - 1` will always produce an odd number because `2 * k` is even, and subtracting 1 from an even number results in an odd number.

Therefore, the output of the print statement will be an odd number, specifically the value of `2 * k - 1`.

Output: **2 * k - 1 (where k is an integer such that 1 ≤ k ≤ (n + 1) // 2)**