Step-by-step reasoning:

1. Initial State: `j` is explicitly given as 2.
2. The expression `n + r + 1` is derived from the condition where `r` is the largest integer such that \( r \times n < \frac{n \times (n + 1)}{2} \).

To determine `r`, let's assume a value for `n` and find the corresponding `r`.

For simplicity, let's take `n = 3` (you can choose any positive integer for `n`):

- Calculate \(\frac{n \times (n + 1)}{2}\):
  \[
  \frac{3 \times (3 + 1)}{2} = \frac{3 \times 4}{2} = 6
  \]

- Find the largest integer `r` such that \( r \times n < 6 \):
  \[
  r \times 3 < 6 \implies r < 2
  \]
  The largest integer `r` satisfying this condition is 1.

So, if `n = 3`, then `r = 1` and `n + r + 1 = 3 + 1 + 1 = 5`.

Since the initial state does not specify `n`, but only provides the formula for `n + r + 1`, we can conclude that `n + r + 1` will be the value derived from the given condition.

Therefore, the print statement will output:
Output: **1 2**