Let's break down the initial state and the code snippet step by step:

1. **Initial State:**
   - `j` is explicitly given as 2.
   - `n + r + 1` is derived from the condition where \( r \) is the largest integer such that \( r \times n < \frac{n \times (n + 1)}{2} \).

2. **Determine \( r \):**
   - To find \( r \), we need to solve the inequality \( r \times n < \frac{n \times (n + 1)}{2} \).
   - This can be rewritten as \( r < \frac{n \times (n + 1)}{2n} = \frac{n + 1}{2} \).
   - Since \( r \) must be an integer, \( r \) is the floor of \( \frac{n + 1}{2} \).

3. **Calculate \( n + r + 1 \):**
   - We know \( r = \lfloor \frac{n + 1}{2} \rfloor \).
   - Therefore, \( n + r + 1 = n + \lfloor \frac{n + 1}{2} \rfloor + 1 \).

4. **Evaluate the expression:**
   - Let's consider different cases for \( n \):
     - If \( n \) is even, say \( n = 2k \):
       - \( r = k \)
       - \( n + r + 1 = 2k + k + 1 = 3k + 1 \)
     - If \( n \) is odd, say \( n = 2k + 1 \):
       - \( r = k \)
       - \( n + r + 1 = (2k + 1) + k + 1 = 3k + 2 \)

5. **Print Statement:**
   - The code snippet is `print(2, j % n, end=' ')`.
   - We already know \( j = 2 \).
   - We need to determine \( j \% n \):
     - \( j \% n = 2 \% n \).

6. **Final Output:**
   - Since \( j = 2 \), \( 2 \% n \) will always be 2 if \( n \geq 2 \) because 2 is less than any \( n \geq 2 \).

Therefore, the print statement will output:
Output: **2 2**