To determine what will be printed, let's break down the initial state and the code snippet step by step.

1. **Initial State Analysis:**
   - `j` is explicitly given as 3.
   - `n + r + 1` is derived from the condition where \( r \) is the largest integer such that \( r \times n < \frac{n \times (n + 1)}{2} \).

2. **Finding the Value of \( r \):**
   - We need to find the largest integer \( r \) such that \( r \times n < \frac{n \times (n + 1)}{2} \).
   - This inequality can be rearranged to \( r < \frac{n \times (n + 1)}{2n} = \frac{n + 1}{2} \).
   - Therefore, \( r \) is the largest integer less than \( \frac{n + 1}{2} \), which is \( \left\lfloor \frac{n + 1}{2} \right\rfloor \).

3. **Expression for \( n + r + 1 \):**
   - Substituting \( r = \left\lfloor \frac{n + 1}{2} \right\rfloor \) into \( n + r + 1 \):
     \[
     n + r + 1 = n + \left\lfloor \frac{n + 1}{2} \right\rfloor + 1
     \]
   - Since \( r \) is the largest integer less than \( \frac{n + 1}{2} \), if \( n \) is even, \( r = \frac{n}{2} \); if \( n \) is odd, \( r = \frac{n - 1}{2} \).

4. **Determining the Value of \( n \):**
   - From the expression \( n + r + 1 \), we need to find \( n \). Let's assume \( n \) is such that it satisfies the condition and leads to a valid integer result for \( r \).
   - For simplicity, let's assume \( n = 3 \) (since \( j = 3 \) and we need a consistent value for \( n \)).

5. **Calculating \( r \) for \( n = 3 \):**
   - \( r = \left\lfloor \frac{3 + 1}{2} \right\rfloor = \left\lfloor 2 \right\rfloor = 2 \).
   - Therefore, \( n + r + 1 = 3 + 2 + 1 = 6 \).

6. **Evaluating the Print Statement:**
   - The print statement is `print(2, j % n, end=' ')`.
   - \( j = 3 \) and \( n = 3 \).
   - \( j \% n = 3 \% 3 = 0 \).

7. **Final Output:**
   - The print statement will output `2 0`.

Output: **2 0**