Alright, I've got this problem to solve. Let's see what it's asking for. So, Rudolf has an array of integers, and he can perform a specific operation on it any number of times. The operation involves choosing an index i (between 2 and n-1) and modifying the elements at positions i-1, i, and i+1 by subtracting 1, 2, and 1 respectively. The goal is to make all elements of the array zero.

First, I need to understand what this operation does. It seems like it's a way to reduce the values in the array, particularly targeting the center element more heavily since it's reduced by 2, while its neighbors are reduced by 1 each. The operation can be applied multiple times, and to any index between 2 and n-1, meaning the endpoints can't be directly targeted.

I need to figure out if it's possible to apply these operations in such a way that all elements become zero. The problem is, with large n (up to 2*10^5 per test case and up to 10^4 test cases), efficiency is crucial. So, any solution that's O(n^2) is probably not going to work.

Let me think about this operation in terms of linear algebra or some kind of system of equations. Each operation can be seen as subtracting a specific "mask" from the array: [-1, -2, -1] at positions i-1, i, i+1. Applying this operation multiple times would be like subtracting multiples of this mask at different positions.

To make all elements zero, it's like solving a system where the sum of these masked operations equals the original array. This sounds similar to solving a system of linear equations, but it's probably too slow for the given constraints.

Maybe there's a smarter way to approach this. Let's consider the array as a sequence and see if there's a pattern or a way to propagate the operations.

Looking at the first example:

Original array: [1, 3, 5, 5, 2]

After operation at i=4: [1, 3, 5-2=3, 5-2=3, 2-1=1]

Then operation at i=3: [1, 3-2=1, 3-2=1, 3-1=2, 1-1=0]

Then operation at i=2: [1-1=0, 1-2=-1, 1-1=0, 2, 0]

Wait, this doesn't match the description. Maybe I miscounted the indices. Let's try again.

Wait, in the first operation, choosing i=4: a[3]=5-1=4, a[4]=5-2=3, a[5]=2-1=1. So the array becomes [1,3,4,3,1].

Then, operation at i=3: a[2]=3-1=2, a[3]=4-2=2, a[4]=3-1=2. Array is [1,2,2,2,1].

Then, operation at i=2: a[1]=1-1=0, a[2]=2-2=0, a[3]=2-1=1. Array is [0,0,1,2,1].

Then, operation at i=4: a[3]=1-1=0, a[4]=2-2=0, a[5]=1-1=0. Array is [0,0,0,0,0].

Okay, that makes sense.

So, the operations can be applied in a way that propagates changes through the array.

I need to find a general way to determine if such a sequence of operations can zero out the entire array.

One approach is to consider the operations as a form of Gaussian elimination, where each operation affects three consecutive elements. However, given the constraints, this might not be efficient enough.

Another way is to iterate through the array and apply operations greedily whenever possible.

Let me look at the provided program and see what it's doing.

The function `func` reads the number of test cases and then processes each test case individually.

For each test case, it reads the integer n (the size of the array) and then reads the array itself.

Then, it loops from i=0 to i=a-2 (where a is n), which is from 0 to n-2 inclusive.

Inside the loop, it checks if b[i] is less than 0. If so, it prints 'NO' and breaks out of the loop.

Otherwise, it updates b[i+1] by subtracting b[i]*2, and b[i+2] by subtracting b[i], and sets b[i] to zero.

After the loop, if the last two elements are both zero, it prints 'YES'; otherwise, it prints 'NO'.

Wait, but in the loop, it's modifying the array based on the current element b[i]. It's seems like it's trying to eliminate b[i] by applying operations that affect b[i], b[i+1], and b[i+2].

Let me see if this makes sense.

Suppose I have an array [a0, a1, a2, ..., an-1].

The operation is to choose i (from 1 to n-2, since indices start at 0 in Python), and perform:

a[i-1] -= 1

a[i] -= 2

a[i+1] -= 1

But in the code, it's updating b[i+1] -= b[i]*2 and b[i+2] -= b[i], and sets b[i] to zero.

Wait, that doesn't seem to match the operation described in the problem.

In the problem, the operation is to subtract 1 from a[i-1], 2 from a[i], and 1 from a[i+1].

But in the code, it's subtracting b[i]*2 from b[i+1] and b[i] from b[i+2], and setting b[i] to zero.

This seems different.

Let me think differently.

Maybe the code is trying to simulate the operations in reverse. Instead of applying operations to reduce the array to zero, it's trying to see if the array can be built up from zero by adding the operation masks.

But I'm not sure.

Let me consider the effect of the operations.

Each operation subtracts 1 from a[i-1], 2 from a[i], and 1 from a[i+1].

So, to reverse it, adding an operation would add 1 to a[i-1], 2 to a[i], and 1 to a[i+1].

So, if I think of the array as a system of equations, where each operation adds a specific pattern to the array, I need to find coefficients for each operation such that the sum equals the original array.

But with large n, solving a system of equations isn't feasible.

Another approach is to use a difference array or prefix sums.

Let me consider the operations in terms of how they affect the array.

If I apply an operation at position i, it's like adding [-1, -2, -1] to positions i-1, i, i+1.

Wait, no, it's subtracting those values.

But in terms of solving for the number of operations, it's better to think of it as adding [1, 2, 1] to the array.

But I'm getting confused.

Let me try to think of it differently.

Suppose I have the array [a0, a1, a2, ..., an-1].

I need to make all ai = 0 by applying operations that subtract [1,2,1] from three consecutive elements at a time.

This is similar to solving a system where each operation affects three consecutive elements.

This seems like a system of linear equations, but with constraints on the number of operations being integers.

But with n up to 2e5, this approach is not practical.

Maybe there's a smarter way.

Let me look at the differences between consecutive elements.

Define d0 = a0, d1 = a1 - a0, d2 = a2 - a1, ..., dn-1 = an-1 - an-2.

Wait, that's the difference array.

But I'm not sure if that helps directly.

Another idea: since operations can only be applied to indices from 2 to n-1 (in 1-based indexing), which correspond to indices 1 to n-2 in 0-based indexing.

Wait, the problem says 2 <= i <= n-1, which in 1-based indexing is positions 2 to n-1.

In 0-based indexing, that's indices 1 to n-2.

Each operation at index i (0-based) subtracts 1 from a[i-1], 2 from a[i], and 1 from a[i+1].

Wait, in 0-based indexing:

- a[i-1] -= 1 (for i >=1)

- a[i] -= 2

- a[i+1] -=1 (for i <= n-2)

So, operations can only be applied to i from 1 to n-2.

Now, the code provided loops from i=0 to i=a-2, which in 0-based indexing is from 0 to n-2.

But in the problem, operations can only be applied for i from 1 to n-2.

There's a discrepancy here.

In the code, it's looping from i=0 to i=n-2, but operations can't be applied at i=0 (in 0-based indexing, which corresponds to i=1 in 1-based indexing).

Wait, no. The problem says 2 <= i <= n-1 in 1-based indexing, which is 1 <= i <= n-2 in 0-based indexing.

But the code is looping from i=0 to i=n-2.

So, it's applying the operation to i from 0 to n-2, but operations can only be applied from i=1 to n-2.

This might be a mistake.

Wait, perhaps the code is trying to simulate something else, not directly applying the operations.

Let me look at what the code does inside the loop.

For each i from 0 to n-2:

- If b[i] < 0, print 'NO' and break.

- Else, b[i+1] -= b[i]*2

- b[i+2] -= b[i]

- b[i] -= b[i] (which sets b[i] to 0)

So, it's modifying b[i+1] and b[i+2] based on b[i], and zeroing out b[i].

It's not directly applying the operations as described in the problem.

Perhaps there's a mathematical justification for this approach.

Let me consider what this loop does.

It starts from the leftmost elements and propagates changes to the right.

It seems like it's trying to eliminate the current element by adjusting the next two elements.

Let me see what happens with the first example:

Initial array: [1,3,5,5,2]

n=5

Loop from i=0 to i=3

i=0:

b[0]=1 >=0

b[1] -= 1*2 => b[1]=3-2=1

b[2] -= 1 => b[2]=5-1=4

b[0]=0

Array: [0,1,4,5,2]

i=1:

b[1]=1 >=0

b[2] -=1*2 => b[2]=4-2=2

b[3] -=1 => b[3]=5-1=4

b[1]=0

Array: [0,0,2,4,2]

i=2:

b[2]=2 >=0

b[3] -=2*2 => b[3]=4-4=0

b[4] -=2 => b[4]=2-2=0

b[2]=0

Array: [0,0,0,0,0]

After the loop, b[-1]=0 and b[-2]=0, so it prints 'YES'

This matches the expected outcome.

Let's see another example where the answer should be 'NO'.

Take the second example:

n=5

Array: [2,4,4,5,1]

Apply the loop:

i=0:

b[0]=2 >=0

b[1]-=2*2 => b[1]=4-4=0

b[2]-=2 => b[2]=4-2=2

b[0]=0

Array: [0,0,2,5,1]

i=1:

b[1]=0 >=0

b[2]-=0*2 => b[2]=2-0=2

b[3]-=0 => b[3]=5-0=5

b[1]=0

Array: [0,0,2,5,1]

i=2:

b[2]=2 >=0

b[3]-=2*2 => b[3]=5-4=1

b[4]-=2 => b[4]=1-2=-1

b[2]=0

Array: [0,0,0,1,-1]

After the loop, b[-1]=-1 <0, so it should print 'NO'

Wait, but according to the problem's sample output, it's 'NO', which matches.

Another example:

n=5

Array: [0,1,3,3,1]

Apply the loop:

i=0:

b[0]=0 >=0

b[1]-=0*2 => b[1]=1-0=1

b[2]-=0 => b[2]=3-0=3

b[0]=0

Array: [0,1,3,3,1]

i=1:

b[1]=1 >=0

b[2]-=1*2 => b[2]=3-2=1

b[3]-=1 => b[3]=3-1=2

b[1]=0

Array: [0,0,1,2,1]

i=2:

b[2]=1 >=0

b[3]-=1*2 => b[3]=2-2=0

b[4]-=1 => b[4]=1-1=0

b[2]=0

Array: [0,0,0,0,0]

After the loop, b[-1]=0 and b[-2]=0, so it prints 'YES'

Which should be correct.

Another test case:

n=6

Array: [5,6,0,2,3,0]

Apply the loop:

i=0:

b[0]=5 >=0

b[1]-=5*2 => b[1]=6-10=-4

Since b[1]=-4 <0, it prints 'NO'

Which matches the sample output.

Seems correct.

Another test case:

n=4

Array: [1,2,7,2]

Apply the loop:

i=0:

b[0]=1 >=0

b[1]-=1*2 => b[1]=2-2=0

b[2]-=1 => b[2]=7-1=6

b[0]=0

Array: [0,0,6,2]

i=1:

b[1]=0 >=0

b[2]-=0*2 => b[2]=6-0=6

b[3]-=0 => b[3]=2-0=2

b[1]=0

Array: [0,0,6,2]

i=2:

b[2]=6 >=0

b[3]-=6*2 => b[3]=2-12=-10

b[4]-=6 => but b[4] doesn't exist, so only b[3] is updated.

Array: [0,0,6,-10]

After the loop, b[-1]=-10 <0, so it prints 'NO'

Which matches the sample output.

Another test case:

n=3

Array: [7,1,0]

Apply the loop:

i=0:

b[0]=7 >=0

b[1]-=7*2 => b[1]=1-14=-13

Since b[1]=-13 <0, it prints 'NO'

Which matches the sample output.

Last test case:

n=4

Array: [1,1,1,1]

Apply the loop:

i=0:

b[0]=1 >=0

b[1]-=1*2 => b[1]=1-2=-1 <0

Prints 'NO'

Which matches the sample output.

So, from these observations, it seems like the provided code correctly identifies whether it's possible to zero out the array or not.

But why does this approach work?

Let's try to understand the logic behind the code.

The loop iterates from the beginning of the array to the third-to-last element.

For each element b[i], if it's negative, it's impossible to reach an all-zero array, so it prints 'NO'.

Otherwise, it adjusts the next two elements based on b[i].

Specifically:

- Subtract b[i]*2 from b[i+1]

- Subtract b[i] from b[i+2]

- Set b[i] to zero

This seems like it's trying to eliminate b[i] by adjusting the future elements accordingly.

After the loop, it checks if the last two elements are zero.

If they are, it prints 'YES'; otherwise, 'NO'.

This approach seems to work for the provided examples, but I need to understand why it works in general.

Let's consider the operations allowed.

Each operation subtracts [1,2,1] from three consecutive elements.

This can be seen as subtracting a specific pattern from the array.

The code's approach seems to be a form of Gaussian elimination or solving the system of equations represented by these operations.

By iterating from left to right and eliminating each element by adjusting the future elements, it's effectively solving for the operations needed to zero out the array.

The condition b[i] < 0 at any step indicates that it's impossible to achieve the desired result because it would require a negative number of operations, which isn't feasible.

Hence, this approach seems correct.

Therefore, the answer is **True**.

**Final Answer**

\boxed{\text{True}}