The code assigns `max_jump` the greater value between its current value and the result of the expression `i - prev_pos`. The initial value of `max_jump` is 1, `prev_pos` is -1, and `i` is 0. 

Calculating `i - prev_pos`:
- `i - prev_pos` = 0 - (-1) = 0 + 1 = 1.

Now we find the maximum:
- `max(max_jump, i - prev_pos)` = max(1, 1) = 1.

Since the value of `max_jump` does not change, the output state will maintain its previous values.

Output State: **`s` is a non-empty string consisting of capital English letters, `vowels` is {'A', 'E', 'I', 'O', 'U', 'Y'}, `max_jump` is 1, `prev_pos` is -1, `i` is 0**.