Alright, I've got this problem to solve. Let's see what it's asking for. So, I'm given two positive integers, n and m, and I need to find the number of ordered pairs (a, b) where 1 ≤ a ≤ n and 1 ≤ b ≤ m, with the condition that a + b is a multiple of b multiplied by the greatest common divisor (GCD) of a and b. That condition sounds a bit tricky, so I need to break it down.

First, let's understand the condition: a + b should be a multiple of b * GCD(a, b). In mathematical terms, this means that b * GCD(a, b) divides a + b without leaving a remainder. So, (a + b) mod (b * GCD(a, b)) == 0.

I need to find all pairs (a, b) that satisfy this. Let's try to simplify this condition to make it easier to compute, especially since n and m can be up to 2 million, and there can be up to 10,000 test cases. Efficiency is key here.

Let me denote GCD(a, b) as g. So, a = g * k and b = g * l, where k and l are coprime integers (since g is the GCD).

Substituting into the condition:

a + b = g*k + g*l = g*(k + l)

b * GCD(a, b) = g*l * g = g*g*l

So, the condition becomes: g*(k + l) is a multiple of g*g*l.

Dividing both sides by g (since g != 0), we get:

k + l is a multiple of g*l.

Wait, but k and l are coprime, since GCD(k, l) = 1.

This seems useful. So, k + l is a multiple of g*l.

Let me think about what this means.

Since k and l are coprime, and l divides k + l, then l must divide k. But k and l are coprime, so the only way l divides k is if l = 1.

Wait, that seems off. If l divides k + l and GCD(k, l) = 1, then l divides k + l implies l divides k, but since GCD(k, l) = 1, l must be 1.

So, does this mean that l must be 1 for the condition to hold?

Let me check with some examples.

Take b = 1, then g = GCD(a, 1) = 1.

So, a + 1 should be a multiple of 1 * 1 = 1, which is always true, since any integer is a multiple of 1.

So, all pairs where b = 1 satisfy the condition.

Now, take b = 2.

Let’s say a = 2, g = GCD(2, 2) = 2.

Then, a + b = 4, and b * g = 2 * 2 = 4, which divides 4, so it satisfies.

Another pair: a = 4, b = 2, g = 2.

a + b = 6, b * g = 4.

6 divided by 4 is 1 with a remainder of 2, so it doesn't satisfy.

Wait, but according to earlier, l must be 1, which in this case would mean b = g * l = g * 1 = g.

But g = GCD(a, b), and b = g, so b divides a.

Wait, maybe I need to think differently.

Let me consider that b * GCD(a, b) divides a + b.

Let me denote d = GCD(a, b), so a = d * a1 and b = d * b1, with GCD(a1, b1) = 1.

Then, b * d = d * b1 * d = d^2 * b1.

And a + b = d * a1 + d * b1 = d * (a1 + b1).

So, d * (a1 + b1) must be divisible by d^2 * b1.

Simplify by d: a1 + b1 must be divisible by d * b1.

But a1 and b1 are coprime.

So, d * b1 divides a1 + b1.

Since b1 divides b1, and a1 + b1 is divisible by b1, then a1 must be divisible by b1.

But a1 and b1 are coprime, so b1 must be 1.

Therefore, b1 = 1, which implies that b = d * 1 = d, so b = d = GCD(a, b).

Thus, b = GCD(a, b), which means that b divides a.

So, the condition simplifies to b divides a.

Wait, is that correct?

Let me verify.

If b divides a, then GCD(a, b) = b, since b divides a.

Then, b * GCD(a, b) = b * b.

And a + b must be divisible by b * b.

But a is a multiple of b, so a = k * b.

Then, a + b = k * b + b = b * (k + 1).

This needs to be divisible by b * b, so b * (k + 1) / (b * b) = (k + 1)/b needs to be an integer.

So, b divides (k + 1).

But a = k * b, so a + b = b * (k + 1).

So, b * b divides b * (k + 1) implies that b divides (k + 1).

Therefore, the condition is that b divides (a + b), which simplifies to b divides a, as a = k * b.

Wait, I'm getting a bit tangled here.

Let me try to rephrase.

Given that a + b is a multiple of b * GCD(a, b), and using the substitution a = d * a1, b = d * b1, with GCD(a1, b1) = 1, we arrived at d * (a1 + b1) must be divisible by d^2 * b1.

Simplifying, a1 + b1 must be divisible by d * b1.

Since a1 and b1 are coprime, and b1 divides a1 + b1, then b1 divides a1, which implies b1 = 1.

Therefore, b1 = 1, meaning b = d * 1 = d, so b = GCD(a, b).

But since GCD(a, b) = d = b, this means that b divides a.

So, the condition reduces to b divides a.

Therefore, the pairs (a, b) where b divides a are the ones that satisfy the given condition.

Wait, but in the initial example, when n = 10 and m = 8, the sample output is 14, which matches the count of pairs where b divides a.

Let me verify this.

For b = 1, a can be from 1 to 10, so 10 pairs.

For b = 2, a can be 2,4,6,8,10, so 5 pairs.

For b = 4, a can be 4,8, so 2 pairs.

For b = 5, a can be 5,10, so 2 pairs.

For b = 8, a can be 8, so 1 pair.

Total: 10 + 5 + 2 + 2 + 1 = 20, but the sample output is 14. Hmm, discrepancy here.

Wait, maybe I miscounted.

Wait, perhaps not all b up to m are considered if they don't divide a.

Wait, no, if b divides a, then a must be a multiple of b within n.

So, for b = 1: a =1 to10, 10 pairs.

b=2: a=2,4,6,8,10, 5 pairs.

b=3: a=3,6,9, but n=10, so a=3,6,9, but 9 is beyond n=10? Wait, n=10, so a=3,6,9, but 9 is <=10, so 3 pairs.

b=4: a=4,8, 2 pairs.

b=5: a=5,10, 2 pairs.

b=6: a=6,12, but 12>10, so only a=6, 1 pair.

b=7: a=7,14, but 14>10, so only a=7, but 7 is <=10, so 1 pair.

b=8: a=8,16, but 16>10, so only a=8, 1 pair.

Total: 10 + 5 + 3 + 2 + 2 +1 +1 +1 = 25, which is not matching the sample output of 14. So, my assumption must be wrong.

Wait, perhaps the condition is not simply b divides a.

Let me go back to the initial condition: a + b is a multiple of b * GCD(a,b).

Earlier, I thought it simplifies to b divides a, but that doesn't match the sample.

So, perhaps I made a mistake in the simplification.

Let me try to find another way.

Let me consider that b * GCD(a,b) divides a + b.

Let me denote d = GCD(a, b), so a = d * a1 and b = d * b1, with GCD(a1, b1) =1.

Then, a + b = d * a1 + d * b1 = d * (a1 + b1).

And b * GCD(a,b) = d * b1 * d = d^2 * b1.

So, d^2 * b1 divides d * (a1 + b1), which simplifies to d * b1 divides a1 + b1.

But a1 and b1 are coprime, so GCD(a1, b1) =1.

Therefore, since b1 divides a1 + b1 and GCD(a1, b1) =1, then b1 must be 1.

Thus, b1 =1, which implies that b = d *1 = d, so b = d = GCD(a,b).

Therefore, b divides a.

But in the sample input, when n=10 and m=8, the output is 14, but according to my earlier counting, it should be 25, which doesn't match.

So, perhaps not all b up to m are considered, or there is an error in the counting.

Wait, perhaps in the sample explanation, only certain pairs are listed: (1,1),(2,1),(2,2),(3,1),(4,1),(5,1),(6,1),(6,2),(6,3),(7,1),(8,1),(9,1),(10,1),(10,2), totaling 14 pairs.

So, according to this, not all pairs where b divides a are considered.

Wait, in my earlier count, for b=3, a=3,6,9, but in the sample explanation, only (3,1),(6,1),(6,2),(6,3),(9,1) are included, but according to the condition, for b=3, a can be 3,6,9, but only (6,3) and (9,3) should be considered if b divides a.

Wait, I'm getting confused.

Let me think again.

If b divides a, then a is a multiple of b.

So, for each b, the number of a that are multiples of b up to n.

This is floor(n / b).

So, the total number of pairs should be the sum over b from 1 to m of floor(n / b).

But according to the sample input, when n=10 and m=8, the output is 14, which is equal to floor(10/1) + floor(10/2) + ... + floor(10/8).

Let's calculate that:

floor(10/1) = 10

floor(10/2) = 5

floor(10/3) = 3

floor(10/4) = 2

floor(10/5) = 2

floor(10/6) = 1

floor(10/7) = 1

floor(10/8) = 1

Total: 10 + 5 + 3 + 2 + 2 + 1 +1 +1 = 25, but the sample output is 14. So, there's a discrepancy.

This suggests that my assumption that the condition is equivalent to b divides a is incorrect.

So, perhaps I made a mistake in the earlier derivation.

Let me revisit the condition: a + b is a multiple of b * GCD(a,b).

Using d = GCD(a, b), a = d * a1, b = d * b1, with GCD(a1, b1) =1.

Then, a + b = d * (a1 + b1)

b * GCD(a,b) = d * b1 * d = d^2 * b1

So, d^2 * b1 divides d * (a1 + b1), which simplifies to d * b1 divides a1 + b1.

Since a1 and b1 are coprime, and b1 divides a1 + b1, then b1 divides a1.

But a1 and b1 are coprime, so b1 must be 1.

Therefore, b1 =1, which implies that b = d *1 = d, so b = d = GCD(a,b).

Thus, b divides a.

But according to the sample, not all pairs where b divides a are counted.

Wait, perhaps the condition is stronger than just b divides a.

Wait, perhaps I need to consider that a + b is a multiple of b * GCD(a,b), which is stronger than just b divides a.

Let me check the sample again.

In the sample, for n=10 and m=8, the output is 14, but according to the sum of floor(n/b) for b from 1 to m, it's 25, which doesn't match.

So, perhaps not all pairs where b divides a satisfy the original condition.

Let me check a specific pair.

Take b=2, a=4.

Then, a + b =6, b * GCD(a,b) =2 *2=4.

Does 4 divide 6? No, 6/4 is 1.5, which is not an integer. So, (4,2) does not satisfy the condition, even though b divides a.

But according to the earlier sum, floor(10/2)=5, but in the sample explanation, only (2,2) and (6,2) and (10,2) are included, which is 3 pairs, not 5.

Wait, in the sample explanation, it's not clear which pairs are included.

Wait, in the sample explanation for n=10 and m=8, the pairs are:

(1,1),(2,1),(2,2),(3,1),(4,1),(5,1),(6,1),(6,2),(6,3),(7,1),(8,1),(9,1),(10,1),(10,2)

That's 14 pairs.

Let me see:

- For b=1: a=1 to10, that's 10 pairs.

- For b=2: a=2,6,10, that's 3 pairs.

- For b=3: a=3,6,9, but only (6,3) and (9,3) are included, but in the sample, (6,3) is not listed, only (6,1),(6,2),(6,3) are considered, but in the explanation, only (6,1),(6,2),(6,3) are listed, but in the output, only (6,1),(6,2),(6,3) are counted, but in the explanation, only (6,1),(6,2),(6,3) are listed, but in the output, only (6,1),(6,2),(6,3) are counted.

Wait, I'm getting confused again.

Perhaps the condition is not just b divides a, but there's an additional constraint.

Let me think differently.

Let me consider the condition: a + b is a multiple of b * GCD(a,b).

Let me rearrange it:

a + b ≡ 0 mod (b * GCD(a,b))

Which means a ≡ -b mod (b * GCD(a,b))

Since a ≡ -b mod (b * GCD(a,b)), and b divides a, let's set a = k * b.

Then, k * b + b = b*(k +1) ≡ 0 mod (b * GCD(k * b, b)) = b * GCD(k,1) = b *1 = b.

So, b*(k +1) ≡ 0 mod b.

This simplifies to b*(k +1) is divisible by b, which is always true, since b divides b.

But this seems to suggest that for any a that is a multiple of b, the condition holds, but according to the sample, that's not the case.

Wait, but earlier counterexample: a=4, b=2.

a + b =6, b * GCD(a,b) =4.

6 is not divisible by 4, so the condition doesn't hold, even though b divides a.

So, my earlier assumption is incorrect.

Therefore, the condition is not simply b divides a.

So, perhaps I need to find a stronger condition.

Let me see.

Given that a = k * b, then a + b = b*(k +1).

The condition is that b*(k +1) is divisible by b * GCD(k * b, b) = b * GCD(k,1) = b *1 = b.

So, b*(k +1) is divisible by b, which is always true.

But in the counterexample, a=4, b=2, k=2, a + b =6, b * GCD(a,b)=4, and 6 is not divisible by 4.

So, my earlier logic must be flawed.

Let me try to see where I went wrong.

I set a = k * b, then a + b = b*(k +1).

GCD(a,b) = GCD(k*b, b) = b * GCD(k,1) = b*1 = b.

So, b * GCD(a,b) = b * b = b^2.

So, the condition is that b^2 divides b*(k +1), which simplifies to b divides (k +1).

Therefore, the condition is that b divides (k +1).

Since a = k * b, then k = a / b.

So, the condition is that b divides (a / b +1).

Wait, that seems messy.

Let me rearrange.

From a = k * b, and b divides (k +1), meaning that k +1 is a multiple of b, so k ≡ -1 mod b.

Therefore, a / b ≡ -1 mod b, which implies a ≡ -b mod b^2.

This seems complicated.

Let me think differently.

Let me consider that a + b is a multiple of b * GCD(a,b).

Given that a = k * b, then a + b = b*(k +1).

And b * GCD(a,b) = b * GCD(k*b, b) = b * GCD(k,1)*b = b * b, since GCD(k,1)=1.

Wait, no, GCD(k*b, b) = b * GCD(k,1) = b *1 = b.

So, b * GCD(a,b) = b * b is incorrect.

Wait, GCD(a,b) = GCD(k*b, b) = b * GCD(k,1) = b*1 = b.

Therefore, b * GCD(a,b) = b * b = b^2.

And a + b = b*(k +1).

So, the condition is that b^2 divides b*(k +1), which simplifies to b divides (k +1).

Since k = a / b, then k is an integer.

So, b divides (a / b +1).

Multiply both sides by b: b^2 divides (a + b), which is the original condition.

So, this seems circular.

Perhaps I need to approach this differently.

Let me consider that a + b is a multiple of b * GCD(a,b), and since a is a multiple of b, a = k * b, then a + b = b*(k +1).

So, b^2 divides b*(k +1), which implies b divides (k +1).

Therefore, k ≡ -1 mod b.

So, k = m*b -1 for some integer m.

Therefore, a = k * b = (m*b -1)*b = m*b^2 - b.

So, a = m*b^2 - b.

Now, since a must be positive and <=n, we have 1 <= m*b^2 - b <=n.

This seems complicated, and I'm not sure if this is leading me in the right direction.

Perhaps I need to consider that the condition is equivalent to b * GCD(a,b) divides a + b.

Let me consider the ratio (a + b)/(b * GCD(a,b)) must be an integer.

Given that GCD(a,b) divides both a and b, and b divides b * GCD(a,b), I'm not sure.

Maybe I should look for a different approach.

Let me consider small values and see if I can find a pattern.

Take n=1, m=1.

Only pair is (1,1).

a + b =2, b * GCD(a,b) =1*1=1, which divides 2, so it's valid.

Output should be 1, which matches the sample.

Next, n=2, m=3.

Possible pairs:

(1,1): 1+1=2, 1*1=1 divides 2.

(1,2): 1+2=3, 2*1=2 divides 3? 3/2=1.5, no.

(1,3):1+3=4,3*1=3 divides 4? 4/3≈1.333, no.

(2,1):2+1=3,1*1=1 divides 3.

(2,2):2+2=4,2*2=4 divides 4.

(2,3):2+3=5,3*1=3 divides 5? 5/3≈1.666, no.

So, valid pairs are (1,1),(2,1),(2,2), totaling 3, which matches the sample.

Another sample: n=3, m=5.

Valid pairs:

(1,1):1+1=2,1*1=1 divides 2.

(1,2):1+2=3,2*1=2 divides 3? No.

(1,3):1+3=4,3*1=3 divides 4? No.

(1,4):1+4=5,4*1=4 divides 5? No.

(1,5):1+5=6,5*1=5 divides 6? No.

(2,1):2+1=3,1*1=1 divides 3.

(2,2):2+2=4,2*2=4 divides 4.

(2,3):2+3=5,3*1=3 divides 5? No.

(2,4):2+4=6,4*2=8 divides 6? No.

(2,5):2+5=7,5*1=5 divides 7? No.

(3,1):3+1=4,1*1=1 divides 4.

(3,2):3+2=5,2*1=2 divides 5? No.

(3,3):3+3=6,3*3=9 divides 6? No.

(3,4):3+4=7,4*1=4 divides 7? No.

(3,5):3+5=8,5*1=5 divides 8? No.

Total valid pairs: (1,1),(2,1),(2,2),(3,1), totaling 4, which matches the sample.

So, from these small cases, it seems that only pairs where b divides a +1 are valid.

Wait, let's check:

From the first sample, n=10, m=8, output=14.

If I consider pairs where b divides a +1, let's see:

For b=1: a+1 divisible by 1, which is always true, so a=1 to10, 10 pairs.

b=2: a+1 divisible by 2, so a odd, a=1,3,5,7,9, but n=10, so a=1,3,5,7,9, 5 pairs.

b=3: a+1 divisible by 3, so a=2,5,8, but n=10, so a=2,5,8, 3 pairs.

b=4: a+1 divisible by 4, so a=3,7, but n=10, so a=3,7, 2 pairs.

b=5: a+1 divisible by 5, so a=4,9, but n=10, so a=4,9, 2 pairs.

b=6: a+1 divisible by 6, so a=5,11, but n=10, so only a=5,1 pair.

b=7: a+1 divisible by 7, so a=6,13, but n=10, so only a=6,1 pair.

b=8: a+1 divisible by 8, so a=7,15, but n=10, so only a=7,1 pair.

Total: 10 +5 +3 +2 +2 +1 +1 +1 =24, which is still not matching the sample output of 14.

Wait, this is not matching either.

So, perhaps my assumption is wrong again.

Let me check the sample explanation again.

In the sample input where n=10 and m=8, the output is 14, and the explanation lists:

(1,1),(2,1),(2,2),(3,1),(4,1),(5,1),(6,1),(6,2),(6,3),(7,1),(8,1),(9,1),(10,1),(10,2)

That's 14 pairs.

Looking at these pairs, I can see that for each b, a is such that a is a multiple of b or something else.

Wait, perhaps the condition is that b divides a.

Wait, in the pair (6,3), b=3 divides a=6.

Similarly, (6,2), b=2 divides a=6.

But in the earlier counterexample, (4,2), b=2 divides a=4, but according to the condition, 4 +2=6 is not divisible by 2*2=4, so it's invalid.

But in the sample explanation, (6,2):6+2=8, which is divisible by 2*2=4.

Wait, 8 is divisible by 4, yes, so it's valid.

Similarly, (6,3):6+3=9, which is divisible by 3*3=9, yes.

So, in this case, b divides a, and a + b is divisible by b * GCD(a,b).

Wait, in this case, since b divides a, GCD(a,b)=b, so b * GCD(a,b)=b*b.

So, a + b must be divisible by b*b.

Given that a is a multiple of b, a = k * b.

So, a + b = b*(k +1).

This needs to be divisible by b*b, which simplifies to k +1 being divisible by b.

So, k +1 ≡0 mod b, which means k ≡ -1 mod b.

Therefore, k = m*b -1 for some integer m.

Therefore, a = k * b = (m*b -1)*b = m*b^2 - b.

So, a must be of the form m*b^2 - b.

Given that a >=1 and <=n, we can find m such that 1 <= m*b^2 - b <=n.

This seems like a way to calculate the number of valid a for each b.

Let me see.

For each b from 1 to m:

Calculate the number of integers m such that 1 <= m*b^2 - b <=n.

Let me solve for m:

1 <= m*b^2 - b <=n

Add b to all parts:

1 + b <= m*b^2 <=n + b

Then, (1 + b)/(b^2) <= m <= (n + b)/(b^2)

But m must be an integer, so m starts from ceil((1 + b)/(b^2)) and goes up to floor((n + b)/(b^2)).

But b^2 is b squared, and for b >=2, b^2 is larger than b, so m*b^2 - b can be larger than n quickly.

This seems complicated, and I'm not sure if this is the best approach.

Perhaps there is a better way to count the number of valid pairs.

Let me consider that for each b, the number of a such that a + b is divisible by b * GCD(a,b).

Given that GCD(a,b) divides both a and b, and b divides b * GCD(a,b), I can try to find a relationship between a and b.

Alternatively, perhaps inclusion-exclusion or some number-theoretic function can be used here.

Given the constraints on n and m (up to 2*10^6 per test case, and sum of n and m across all test cases up to 2*10^6), I need an efficient solution, probably O(T * sqrt(N)) or better.

Looking at the provided program, it seems to be attempting to count the number of valid pairs for each test case efficiently.

Let me analyze the provided program to understand its logic.

The program reads the number of test cases t, and for each test case, it reads n and m, then initializes ans to n, and then loops over b from 2 to min(n, m), adding floor((n + b)/(b*b)) to ans for each b.

Finally, it prints ans.

So, it seems to be starting with ans = n, which likely corresponds to b=1.

Then, for b from 2 to min(n, m), it adds floor((n + b)/(b*b)) to ans.

I need to verify if this is the correct way to count the number of valid pairs.

From earlier analysis, for each b, the number of valid a is equal to the number of m such that a = m*b^2 - b <=n and a >=1.

So, a = m*b^2 - b >=1 and <=n.

Rearranged, m*b^2 >= b +1 and m*b^2 <=n + b.

Therefore, m >= ceil((b +1)/b^2) and m <= floor((n + b)/b^2).

Since m must be an integer, the number of valid m is floor((n + b)/b^2) - ceil((b +1)/b^2) +1.

But for b >=2, (b +1)/b^2 is less than 1, since b^2 > b +1 for b >=2.

Therefore, ceil((b +1)/b^2) =1.

And floor((n + b)/b^2) is floor((n + b)/b^2).

Therefore, the number of valid m is floor((n + b)/b^2) -1 +1 = floor((n + b)/b^2).

So, for each b from 2 to m, the number of valid a is floor((n + b)/b^2).

Adding this to ans, which is initially set to n, which corresponds to b=1.

This matches the provided program's logic.

Therefore, the program seems correct based on this analysis.

Let me verify with the sample input.

Sample input:

6

1 1

2 3

3 5

10 8

100 1233

1000000 1145141

Sample output:

1

3

4

14

153

1643498

Let me check for n=10, m=8.

According to the program:

ans =10

For b=2 to min(10,8)=8:

b=2: floor((10 +2)/(2*2))= floor(12/4)=3

b=3: floor((10 +3)/(3*3))= floor(13/9)=1

b=4: floor((10 +4)/(4*4))= floor(14/16)=0

b=5: floor((10 +5)/(5*5))= floor(15/25)=0

b=6: floor((10 +6)/(6*6))= floor(16/36)=0

b=7: floor((10 +7)/(7*7))= floor(17/49)=0

b=8: floor((10 +8)/(8*8))= floor(18/64)=0

So, ans=10 +3 +1 +0 +0 +0 +0 +0=14, which matches the sample output.

Another sample: n=3, m=5.

ans=3

b=2: floor((3+2)/4)= floor(5/4)=1

b=3: floor((3+3)/9)= floor(6/9)=0

b=4: floor((3+4)/16)= floor(7/16)=0

b=5: floor((3+5)/25)= floor(8/25)=0

Total ans=3 +1 +0 +0 +0=4, which matches the sample.

So, the program seems to be correctly implementing the logic we derived.

Therefore, I conclude that the given program is correct.

**Final Answer**

\[ \boxed{\text{True}} \]