Reasoning:
The original assessment contains a logical error in the interpretation of the problem statement and the function's behavior. Let's break down the issue:

1. **Problem Statement Revisited**:
   - The problem requires finding the difference between the sum of cubes of the first `n` natural numbers and the sum of the first `n` natural numbers.
   - The sum of the first `n` natural numbers is correctly calculated as:
     \[ \text{sum\_n} = \frac{n \times (n + 1)}{2} \]
   - The sum of the cubes of the first `n` natural numbers is:
     \[ \text{sum\_cubes\_n} = \left( \frac{n \times (n + 1)}{2} \right)^2 \]

2. **Function Behavior**:
   - The function `func_1` calculates `sum_n` and `sum_cubes_n` correctly.
   - However, the function returns the difference between `sum_cubes_n` and `sum_n`, which is:
     \[ \text{result} = \left( \frac{n \times (n + 1)}{2} \right)^2 - \frac{n \times (n + 1)}{2} \]

3. **Mathematical Simplification**:
   - Let \( S = \frac{n \times (n + 1)}{2} \).
   - The function computes:
     \[ \text{result} = S^2 - S \]
   - This can be factored as:
     \[ \text{result} = S(S - 1) \]
   - Substituting back \( S = \frac{n \times (n + 1)}{2} \):
     \[ \text{result} = \left( \frac{n \times (n + 1)}{2} \right) \left( \frac{n \times (n + 1)}{2} - 1 \right) \]

4. **Test Cases Verification**:
   - For \( n = 3 \):
     \[ \text{sum\_n} = 6 \]
     \[ \text{sum\_cubes\_n} = 36 \]
     \[ \text{result} = 36 - 6 = 30 \]
   - For \( n = 5 \):
     \[ \text{sum\_n} = 15 \]
     \[ \text{sum\_cubes\_n} = 225 \]
     \[ \text{result} = 225 - 15 = 210 \]
   - For \( n = 2 \):
     \[ \text{sum\_n} = 3 \]
     \[ \text{sum\_cubes\_n} = 9 \]
     \[ \text{result} = 9 - 3 = 6 \]

The function `func_1` is indeed computing the correct difference as specified in the problem statement. The original assessment's conclusion that the function always returns 0 is incorrect.

Final: **True**