The code updates the value of `dp[j]` by adding `dp[j - 1]` to it. Given the initial conditions:

- \( n \) is an integer such that \( 2 \leq n \leq 10^6 \)
- \( f_{\text{max}_n} \) is a positive integer
- \( \text{MOD} = 10 \)
- \( \text{dp} \) is a list of length \( f_{\text{max}_n} + 1 \) where \( \text{dp}[0] = 1 \) and for every \( j \) from 1 to \( f_{\text{max}_n} \), \( \text{dp}[j] = (2 \times \text{dp}[j - 1] + \text{dp}[j - 2] + \ldots + \text{dp}[0]) \% 10 \)
- \( i = n + 1 \)
- \( j = f_{\text{max}_n} - 2 \)

The initial value of \( \text{dp}[j] \) is given by the formula \( \text{dp}[j] = (2 \times \text{dp}[j - 1] + \text{dp}[j - 2] + \ldots + \text{dp}[0]) \% 10 \). After executing the line `dp[j] += dp[j - 1]`, the new value of \( \text{dp}[j] \) becomes \( \text{dp}[j] + \text{dp}[j - 1] \) modulo 10.

Therefore, the output state is:

Output State: **\( n \) is an integer such that \( 2 \leq n \leq 10^6 \); \( f_{\text{max}_n} \) is a positive integer; \( \text{MOD} = 10 \); \( \text{dp} \) is a list of length \( f_{\text{max}_n} + 1 \) where \( \text{dp}[0] = 1 \) and for every \( j \) from 1 to \( f_{\text{max}_n} \), \( \text{dp}[j] = (2 \times \text{dp}[j - 1] + \text{dp}[j - 2] + \ldots + \text{dp}[0]) \% 10 \); \( i = n + 1 \); \( j = f_{\text{max}_n} - 2 \); \( \text{dp}[j] \) is updated to \( (\text{dp}[j] + \text{dp}[j - 1]) \% 10 \)**