Let's break down the initial state and the calculation step by step:

1. **Initial Values:**
   - `i` is 1.
   - `l` is 1.
   - `ql` is not explicitly defined, but it will be used in the calculation of `m`.

2. **Expression for `m`:**
   - `m` is defined as `b[s - 1] + (bd[s] * (ql - a[s - 1]) / ad[s])`.
   - Here, `b`, `bd`, `a`, and `ad` are lists or arrays, and `s` is an index.
   - Since `s` is not defined, we cannot determine its exact value, but we know that `s` must be such that `s-1` is a valid index for the lists `b`, `bd`, `a`, and `ad`.

3. **Expression for `ql`:**
   - `ql` is updated as `ql - a[s - 1]`.
   - This means `ql` is reduced by the value of `a[s - 1]`.

Given these details, let's assume a specific scenario to illustrate the calculation. For simplicity, let's assume:
- `b = [10, 20, 30]`
- `bd = [2, 3, 4]`
- `a = [5, 6, 7]`
- `ad = [1, 2, 3]`
- `s = 2` (this is just an example; the actual value of `s` is not specified)

With these assumptions:
- `b[s - 1] = b[1] = 20`
- `bd[s] = bd[2] = 4`
- `a[s - 1] = a[1] = 6`
- `ad[s] = ad[2] = 3`

Now, calculate `m`:
\[ m = b[s - 1] + \left( \frac{bd[s] \times (ql - a[s - 1])}{ad[s]} \right) \]
\[ m = 20 + \left( \frac{4 \times (ql - 6)}{3} \right) \]

Since `ql` is not explicitly defined, let's assume `ql` is initially set to some value, say `ql = 10` (for illustration purposes).

Then:
\[ m = 20 + \left( \frac{4 \times (10 - 6)}{3} \right) \]
\[ m = 20 + \left( \frac{4 \times 4}{3} \right) \]
\[ m = 20 + \left( \frac{16}{3} \right) \]
\[ m = 20 + 5.3333 \]
\[ m = 25.3333 \]

Since the `print` statement converts `m` to an integer, we get:
\[ m = 25 \]

Therefore, the output will be:
Output: **25**