Given the initial state:

- `s` is a positive integer such that 3 ≤ `s` ≤ 10^12.
- `x` is a non-negative integer such that 0 ≤ `x` ≤ 10^12.
- `count` is set to 2.
- `a` is `s - 1`.

Now evaluating the code:

```
b = s - a
```

Now we calculate the value of `b`:

Since `a` is defined as `s - 1`, we can substitute that into the equation for `b`.

Thus:

```
b = s - (s - 1) = s - s + 1 = 1
```

The values of `s`, `x`, and `count` remain unchanged, while `b` is assigned the value of 1.

So the output state is:

Output State: **`s` is a positive integer such that 3 ≤ `s` ≤ 10^12, `x` is a non-negative integer such that 0 ≤ `x` ≤ 10^12, `count` is set to 2, `a` is `s - 1`, `b` is 1.**