The code snippet `a[l] -= a[r]` subtracts the value of `a[r]` from `a[l]`. Given the initial state, `a[r]` is less than `a[l]`, so after the operation, `a[l]` will be reduced by `a[r]`, but it will still be greater than `a[r]` (or equal if `a[l]` was exactly twice `a[r]`).

The updated value of `k` is `k - 2 * a[r]`, which is already given in the initial state and is not affected by the operation `a[l] -= a[r]`.

Output State: **`t` is an integer such that 1 <= t <= 10^4; for each test case, `n` and `k` are integers such that 1 <= n <= 2 * 10^5 and 1 <= k <= 10^15; `a` is a list of `n` integers where each integer `a_i` satisfies 1 <= a_i <= 10^9; the sum of `n` across all test cases does not exceed 2 * 10^5. The current value of `a[r]` is less than the current value of `a[l]`. If `l` is not equal to `r`, `l` is not necessarily equal to `r`. Additionally, `k` is greater than or equal to twice the value of `a[r]`. The updated value of `k` is `k - 2 * a[r]`. The updated value of `a[l]` is `a[l] - a[r]`.**