Based on the initial state provided:

- `i` is equal to `leftOnes`.
- `aOnes` is equal to `leftOnes` if `aOnes` was initially 0 and `aOnes` was always less than or equal to `bOnes` throughout the loop. Otherwise, `bOnes` is equal to `leftOnes`.
- The condition `(aOnes == newk and bOnes == newk)` is true.

Given this information, we need to determine the values of `aOnes` and `bOnes`.

Since `(aOnes == newk and bOnes == newk)` is true, it means both `aOnes` and `bOnes` have the same value, which is `newk`.

From the condition, if `aOnes` was initially 0 and remained less than or equal to `bOnes`, then `aOnes` would be `leftOnes`. If not, `bOnes` would be `leftOnes`. But since both `aOnes` and `bOnes` are equal to `newk`, it implies that `newk` must be equal to `leftOnes`.

Therefore, `aOnes` and `bOnes` are both equal to `newk`, which is also equal to `leftOnes`.

The `print` statement simply outputs the string `'yes'`.

Output: **yes**