The code `ans = f - s` assigns the value of `f - s` to `ans`. Since `f` is the maximum of `original_s - 1` and `original_f - 1`, and `s` is the minimum of `original_s - 1` and `original_f - 1`, the value of `ans` will be the difference between these two values. The states of the other variables are not affected.

To determine the exact value of `ans`, we need to know the values of `original_s` and `original_f`, which are not provided. However, we can express `ans` in terms of `original_s` and `original_f`.

If `original_s <= original_f`:
- `s = original_s - 1`
- `f = original_f - 1`
- `ans = (original_f - 1) - (original_s - 1) = original_f - original_s`

If `original_s > original_f`:
- `s = original_f - 1`
- `f = original_s - 1`
- `ans = (original_s - 1) - (original_f - 1) = original_s - original_f`

Therefore, the Output State is:
Output State: **`i` is `n`, `n` is a positive integer, `s` is the minimum of `original_s - 1` and `original_f - 1`, `f` is the maximum of `original_s - 1` and `original_f - 1`, `a` and `b` remain in their initial states, `cnt` remains as `[1] + [0]*(n-1)`, `ans` is `original_f - original_s` if `original_s <= original_f` and `ans` is `original_s - original_f` if `original_s > original_f`.**