`sequence.append(sequence[-1] + y)` appends the value of `sequence[-1] + y` to the list `sequence`. The previous value of `sequence[-1]` is `current_sum`, so the new value appended to `sequence` is `current_sum + y`. The variables `n`, `current_sum`, `y`, and `s` are not directly affected by this line of code. 

Therefore, the updated information is:
- `sequence` now includes `current_sum + y`.
- The conditions `n > 1`, `current_sum + y <= s`, and `(s - current_sum - y) % y == 0` are still valid.

Output State: **`n` > 1, `current_sum` + `y` <= `s`, (`s` - `current_sum` - `y`) % `y` == 0, `sequence` includes `current_sum + y`**