The code `current_sum += y` increments the value of `current_sum` by `y`. Given the initial conditions:

- `n > 1`
- `current_sum + y <= s`
- `(s - current_sum - y) % y == 0`
- `sequence` includes `current_sum + y`

After executing the code, `current_sum` is updated to `current_sum + y`. The other conditions and the inclusion in the sequence remain valid.

Output State: **`n` > 1; `current_sum` + `y`; `current_sum + y` <= `s`; (`s` - `current_sum` - `y`) % `y` == 0; `sequence` includes `current_sum + y`**