Correctness: False

Explanation: The code does not correctly implement the problem description. Specifically, the code returns the `substring` itself along with its `start` and `end` indices, but according to the problem description, it should only return the `start` and `end` indices if the substring is found, not the substring itself. Additionally, the `end` index should be inclusive, so it should be `end = start + len(substring)` instead of `end = start + len(substring) - 1`.

Here is a corrected version of the function:

```python
def func_1(string, substring):
    start = string.find(substring)
    if start == -1:
        return None
    end = start + len(substring)
    return (start, end)
```

This corrected function would return `(start, end)` only if the substring is found, and `None` otherwise, which aligns with the problem description.