The code snippet `ans[i + 1] += ans[i]` modifies the value of `ans[i + 1]` by adding `ans[i]` to it. Given the initial state, `ans[i + 1]` is initially `arr[i] + ans[i]`. After the operation, `ans[i + 1]` becomes `(arr[i] + ans[i]) + ans[i]`, which simplifies to `arr[i] + 2 * ans[i]`.

Here's the output state in the required format:

Output State: **`arr` is a list of integers where each integer \( x_i \) satisfies \( 1 \leq x_i \leq 500 \); `n` is an integer such that \( 3 \leq n \leq 500 \); `ans` is a list of integers where `ans[i + 1]` is now `arr[i] + 2 * ans[i]`, `i` is `k + 1`, `ans[k + 1]` is 0, and `arr[k + 2]` is at least `arr[k + 1]`.**