Postcondition: ***`t` is an integer such that \(1 \leq t \leq 10^4\) and `t` is now `t - 1`; `n` is the first integer input; `a` is the second integer input; `b` is the third integer input; `c` is `a * n`; `d` is `b + (n - 2) * a`; `e` is the minimum of `a` and `c` and `d`***

Explanation: 
- If `n == 1`, then `e` is set to `a`.
- If `n != 1`, then `e` is set to the minimum of `c` (which is `a * n`) and `d` (which is `b + (n - 2) * a`).

Thus, in both cases, `e` ends up being the minimum of `a`, `c`, and `d`.