To determine what will be printed by the given `print` statement, we need to analyze the initial state and the conditions provided:

### Initial State and Conditions:
1. `n` and `k` are integers read from the input.
2. `t` is a positive integer (though `t` is not used in the print statement, it is provided in the precondition).
3. If `n` is equal to `k`, then `n` equals `k` (this is a tautology and doesn't change the value of `n` or `k`).
4. If `n` is not equal to `k`, then there are two conditions:
   - If `n + 2 > k * 2`, then `n` satisfies this condition.
   - Otherwise, `n + 2` is less than or equal to `k * 2`.

### Analysis:
- The print statement `print(n - k + 1, end=' ')` will output the value of `n - k + 1` followed by a space.
- The value of `n - k + 1` depends on the values of `n` and `k`.

### Cases Based on Conditions:
1. **Case 1: `n == k`**
   - If `n` is equal to `k`, then `n - k + 1` simplifies to `0 + 1`, which is `1`.
   - Output: **1**

2. **Case 2: `n > k` and `n + 2 > k * 2`**
   - This condition implies `n` is sufficiently larger than `k` such that `n - k + 1` will be a positive integer greater than 1.
   - Example: If `n = 6` and `k = 2`, then `n + 2 = 8` and `k * 2 = 4`, so `n + 2 > k * 2` is true.
   - The output will be `6 - 2 + 1 = 5`.
   - Output: **5**

3. **Case 3: `n > k` and `n + 2 <= k * 2`**
   - This condition implies `n` is not much larger than `k` such that `n - k + 1` will still be a positive integer, but it will be less than or equal to `k - 1 + 1 = k`.
   - Example: If `n = 5` and `k = 3`, then `n + 2 = 7` and `k * 2 = 6`, so `n + 2 > k * 2` is false.
   - The output will be `5 - 3 + 1 = 3`.
   - Output: **3**

4. **Case 4: `n < k`**
   - If `n` is less than `k`, then `n - k + 1` will be a positive integer less than 1, specifically `n - k + 1`.
   - Example: If `n = 2` and `k = 5`, then `n - k + 1 = 2 - 5 + 1 = -2`.
   - Output: **-2**

### Conclusion:
The output of `n - k + 1` depends on the specific values of `n` and `k`. We can describe the output in terms of `n` and `k`:

Output: **n - k + 1**