To determine what will be printed by the `print(suma - 1)` statement, let's break down the initial state and the logic step by step:

### Initial State:
- `n` and `m` are positive integers such that \(1 \leq n, m \leq 2 \times 10^6\).
- `T` is greater than 0.
- `t` is 0.
- `info` is a list of strings obtained from the input.
- `a` is the integer value of `info[0]`.
- `b` is the integer value of `info[1]` and must be at least 1.
- `suma` is the sum of all valid `x` values calculated during the loop, where each `x` is \((a - i \times (i - 1)) // i^2 + 1\) for \(i\) from 1 to `b` if \(a - i \times (i - 1) > 0\), otherwise `x` is 0.

### Calculation of `suma`:
1. For each \(i\) from 1 to `b`:
   - Calculate \(a - i \times (i - 1)\).
   - If \(a - i \times (i - 1) > 0\):
     - Calculate \(x = (a - i \times (i - 1)) // i^2 + 1\).
     - Add `x` to `suma`.
   - Otherwise, set `x` to 0 and add 0 to `suma`.

### Example Calculation:
Let's assume `info` is `["10", "3"]`, so `a = 10` and `b = 3`.

- For \(i = 1\):
  - \(a - i \times (i - 1) = 10 - 1 \times 0 = 10\)
  - \(x = (10 // 1^2) + 1 = 10 + 1 = 11\)
  - `suma += 11`

- For \(i = 2\):
  - \(a - i \times (i - 1) = 10 - 2 \times 1 = 8\)
  - \(x = (8 // 2^2) + 1 = 8 // 4 + 1 = 2 + 1 = 3\)
  - `suma += 3`

- For \(i = 3\):
  - \(a - i \times (i - 1) = 10 - 3 \times 2 = 4\)
  - \(x = (4 // 3^2) + 1 = 4 // 9 + 1 = 0 + 1 = 1\)
  - `suma += 1`

So, `suma = 11 + 3 + 1 = 15`.

### Final Output:
The `print(suma - 1)` statement will print the value of `suma` minus 1.

Output: **14 (where suma is the sum of all valid x values calculated during the loop, and x is (a - i * (i - 1)) // i^2 + 1 for i from 1 to b if a - i * (i - 1) > 0, otherwise x is 0)**