To determine the final output state after all iterations of the loop, we need to understand how the loop modifies the list `a` based on the list `x`.

Here's the loop code again for reference:
```python
for i in range(1, n):
    a[i] = a[i - 1] + x[i - 1]
```
This loop starts with `i=1` and goes up to `i=n-1`. For each iteration, it sets `a[i]` to the value of `a[i-1]` plus `x[i-1]`.

Let's break down the process:

1. Initially, `a` is `[1000, 0, 0, ..., 0]` (with `n` elements).
2. After the first iteration (`i=1`), `a[1]` becomes `a[0] + x[0]`, which is `1000 + x[0]`.
3. After the second iteration (`i=2`), `a[2]` becomes `a[1] + x[1]`, which is `(1000 + x[0]) + x[1]`.
4. This pattern continues until the last iteration (`i=n-1`), where `a[n-1]` becomes `a[n-2] + x[n-2]`.

So, after all iterations, the list `a` will be:
- `a[0] = 1000`
- `a[1] = 1000 + x[0]`
- `a[2] = 1000 + x[0] + x[1]`
- ...
- `a[n-1] = 1000 + x[0] + x[1] + ... + x[n-2]`

The variable `i` will be `n-1` after the loop finishes.

Therefore, the final output state is:
Output State: **`t` is an integer such that 1 <= t <= 10^4, `n` is the new input integer, `x` is a list of `n` integers obtained from the new input, `a` is a list of `n` integers where `a[0] = 1000`, `a[1] = 1000 + x[0]`, `a[2] = 1000 + x[0] + x[1]`, ..., `a[n-1] = 1000 + x[0] + x[1] + ... + x[n-2]`, and `i` is `n-1`.**

In simpler terms, the list `a` will have its first element as `1000`, and each subsequent element will be the sum of `1000` and the cumulative sum of the corresponding elements in `x` up to that point. The variable `i` will be equal to `n-1` after the loop completes.