The code snippet `be = md + 1` updates the value of `be` to `md + 1`. All other variables remain unchanged. Let's list the updated state:

- `A` and `B` are positive integers such that 1 ≤ A, B ≤ 10^6.
- `n` is a positive integer such that 1 ≤ n ≤ 10^5.
- `l`, `t`, and `m` are positive integers such that 1 ≤ l, t, m ≤ 10^6.
- `be` is now `md + 1`.
- `en` is 10^7.
- `ans` is -1.
- `md` is (l + 10^7) // 2.
- `all` is A * (md - l + 1) + B * (sum_n(md - 1) - sum_n(max(l - 2, 0))).
- `val` is max(ceil1(all, m), a + (md - 1) * b).
- The current value of `val` is less than or equal to `t`.

Output State: **`A` and `B` are positive integers such that 1 ≤ A, B ≤ 10^6, `n` is a positive integer such that 1 ≤ n ≤ 10^5, `l`, `t`, and `m` are positive integers such that 1 ≤ l, t, m ≤ 10^6, `be` is (l + 10^7) // 2 + 1, `en` is 10^7, `ans` is -1, `md` is (l + 10^7) // 2, `all` is A * (md - l + 1) + B * (sum_n(md - 1) - sum_n(max(l - 2, 0))), `val` is max(ceil1(all, m), a + (md - 1) * b), the current value of `val` is less than or equal to `t`.**