Let's analyze the code step by step:

1. The initial state is:
   - `h` is a positive integer such that \(h \geq 1\) and \(h < \text{original } h\)
   - `w` is a positive integer such that \(1 \leq w \leq 300\)
   - `j` is assigned the value \(w-1\), so \(j = w-1\)
   
2. The code snippet is:
   ```python
   print('#' if (i + j) % 2 == 0 else '.')
   ```
   Here, the code prints either `'#'` or `'.'` based on the condition `(i + j) % 2 == 0`.

   - Since `i` is not defined in the initial state, let's consider it as a variable that is not affecting our current conditions (as it is not assigned any value here).
   - `j` is already defined as \(j = w - 1\).

3. Evaluating the condition `(i + j) % 2 == 0`:
   - If \((i + j)\) is even, the output will be `'#'`.
   - If \((i + j)\) is odd, the output will be `'.'`.

Since `i` is not defined and does not affect the condition directly from the initial state, the condition \((i + j) % 2 == 0\) depends on whether \(w - 1\) is even or odd. However, since `i` is not specified and can be any integer, we cannot determine the exact outcome without knowing `i`. But given the initial conditions of `j = w - 1`, we know:

- If `w` is even, then `j = w - 1` is odd.
- If `w` is odd, then `j = w - 1` is even.

Thus, the output will depend on whether `i` makes the sum `i + j` even or odd. Since we don't have the exact value of `i`, we can only express the output in terms of the parity of `i + j`.

Output State: **`h` is a positive integer such that \(h \geq 1\) and \(h < \text{original } h\), `w` is a positive integer such that \(1 \leq w \leq 300\), `j` is \(w-1\), and the output is either `'#'` if `i + (w-1)` is even, or `'.'` if `i + (w-1)` is odd.**