The code prints `'#'` if `(i + j) % 2 == 0` and `'.'` if `(i + j) % 2 != 0`. Given the initial conditions, `i` is equal to `w` and `j` is also equal to `w`. So the expression simplifies to checking if `(w + w) % 2 == 0` or `(2 * w) % 2 == 0`.

Since `2 * w` is always even, `(2 * w) % 2` will always be 0, which means the condition `(i + j) % 2 == 0` is always true. Therefore, the output is `'#'`.

The variables `h`, `w`, and `j` remain unchanged, and `i` is now equal to `w`.

Output State: **`h` is a positive integer such that \(h \geq 1\) and \(h < \text{original } h\) and \(h - 1\), `w` is a positive integer such that \(1 \leq w \leq 300\), `j` is `w`, `i` is `w`, and the output is `'#'`.**