To determine the output state, let's analyze the given code and initial state step by step.

The initial state is: `n` = input_n, `m` = input_m, `k` = input_k, `x` = input_x - 1, `y` = input_y - 1.

The code provided is:
```python
full_cycle_length = (2 * n - 2) * m if n > 1 else m
```

This code calculates the value of `full_cycle_length` based on the values of `n` and `m`. 

- If `n` is greater than 1, then `full_cycle_length` is calculated as `(2 * n - 2) * m`.
- If `n` is not greater than 1 (i.e., `n` is 1 or less), then `full_cycle_length` is simply `m`.

Given that `n` equals input_n, we have two scenarios for `full_cycle_length`:
1. If input_n > 1, then `full_cycle_length` = `(2 * input_n - 2) * input_m`.
2. If input_n is not greater than 1, then `full_cycle_length` = `input_m`.

The values of `k`, `x`, and `y` are not changed by this code, so they remain as initially stated: `k` = input_k, `x` = input_x - 1, `y` = input_y - 1.

Therefore, the Output State is: `n` = input_n, `m` = input_m, `k` = input_k, `x` = input_x - 1, `y` = input_y - 1, and `full_cycle_length` equals `(2 * input_n - 2) * input_m` if input_n > 1, otherwise `full_cycle_length` equals `input_m`.

Output State: **`n` = input_n, `m` = input_m, `k` = input_k, `x` = input_x - 1, `y` = input_y - 1, `full_cycle_length` = `(2 * input_n - 2) * input_m` if input_n > 1, otherwise `full_cycle_length` = `input_m`**