`x` is updated by adding `bx ** i * a` to its current value. Given that `i` is `n-2`, and knowing the values of `n`, `m`, `bx`, `by`, `xi`, `yi`, `s`, `x`, and `a`, we can proceed with the calculation.

Since `n` is greater than 1, let's denote `n-2` as `i`. We also know that `bx` is the integer value of `s[1]` and `2 ≤ bx ≤ 40`. The exact value of `bx` isn't specified, but it doesn't affect the structure of the solution. `a` is the integer value of `xs[1]`, and since `2 ≤ bx ≤ 40` and `2 ≤ by ≤ 40`, `a` is also within this range.

The updated value of `x` will be the original value of `x` plus `bx ** (n-2) * a`.

Output State: **`n` is greater than 1, `m` is a positive integer such that 1 ≤ `m` ≤ 10, `bx` is the integer value of `s[1]`, and 2 ≤ `bx` ≤ 40, `by` is an integer such that 2 ≤ `by` ≤ 40, `xi` and `yi` are integers such that 0 ≤ `xi` < `bx` and 0 ≤ `yi` < `by` for all i, `s` is a list of strings obtained from the input, `x` is the sum of `a * bx` plus `bx ** (n-2) * a`, `i` is `n-2`, `a` is the integer value of `xs[1]`.**