Correctness: **True**

Explanation: The annotated program correctly implements the logic required by the problem description. The function `func_1` takes a positive integer `n` as input and returns \(2^{(n-1)}\). This value is indeed the sum of the even-indexed binomial coefficients of the expansion \((1 + 1)^n = 2^n\). The sum of all binomial coefficients for a given \(n\) is \(2^n\), and the sum of the even-indexed coefficients can be derived from this by noting that the sum of the even-indexed coefficients is equal to the sum of the odd-indexed coefficients, which together make up \(2^n\). Therefore, the sum of the even-indexed coefficients is \(2^{(n-1)}\).

The provided test cases (`assert func_1(4) == 8`, `assert func_1(6) == 32`, `assert func_1(2) == 2`) also validate this logic for specific values of `n`.

Since the program meets the problem description for all valid positive integers, the correctness is **True**.