Let's break down the problem step by step:

1. **Identify the loop condition**: The loop condition is `r > l and a[r] == a[r - 1]`.
2. **Current state at the end of the previous iteration**:
   - `ans` is `max(0, le - (st + end + 1))`
   - `le` is the length of list `a`
   - `t` is a positive integer such that \(1 \leq t \leq 10^4\)
   - `n` must be greater than 4
   - `a[0]` must be equal to `a[r - 1]`
   - `l` is equal to `r - 2`
   - `r` is equal to `n - 5`
   - `st` is equal to `2 * (r - l - 1)`
   - `end` is increased by 1

3. **Determine which states need to be adjusted**:
   - The loop condition involves `r` and `l`. Therefore, we need to adjust these two variables.
   - We also need to ensure that `a[r] == a[r - 1]` remains true for the loop to continue.

4. **Adjusting the states**:
   - Since `l` is defined as `r - 2`, we need to decrease `l` by 1 to make `r > l` true.
   - We need to ensure that `a[r] == a[r - 1]` remains true. This means `a[r]` should be equal to `a[r - 1]`.

Given the above analysis, we need to adjust `l` and ensure `a[r] == a[r - 1]` remains true.

**State:**
- `ans` is `max(0, le - (st + end + 1))`
- `le` is the length of list `a`
- `t` is a positive integer such that \(1 \leq t \leq 10^4\)
- `n` must be greater than 4
- `a[0]` must be equal to `a[r - 1]`
- `l` must be decreased by 1 (so `l = r - 3`)
- `r` is equal to `n - 5`
- `st` is equal to `2 * (r - l - 1)`
- `end` is increased by 1

Thus, the final state is:

State: **`ans` is `max(0, le - (st + end + 1))`, `le` is the length of list `a`, `t` is a positive integer such that \(1 \leq t \leq 10^4\), `n` must be greater than 4, `a[0]` must be equal to `a[r - 1]`, `l` must be decreased by 1 (so `l = r - 3`), `r` is equal to `n - 5`, `st` is equal to `2 * (r - l - 1)`, `end` is increased by 1**