Based on the problem description, the provided code, and the output hints, the original assessment appears to be incorrect. The problem description asks to remove the first and last occurrence of a given character from the string, but the output hints indicate that the function actually removes the first and last occurrences of the character and the substring between them if the character appears more than once.

Upon re-examining the code, it's clear that the line `return s[:first_index] + s[first_index + 1:last_index] + s[last_index + 1:]` is the culprit. This line not only removes the first and last occurrences of the character but also removes the substring between them.

The correct implementation should be `return s[:first_index] + s[first_index + 1:]` if there's only one occurrence of the character, and `return s[:first_index] + s[first_index + 1:last_index] + s[last_index + 1:]` is close but not entirely correct if there are multiple occurrences of the character. The correct implementation should be `return s[:first_index] + s[first_index + 1:last_index] + s[last_index + 1:]` if the intention is to remove everything between the first and last occurrence of the character, including those characters themselves.

However, according to the problem description, the intention is to remove only the first and last occurrence of the character, not the substring between them. Therefore, the correct implementation should be `return s[:first_index] + s[first_index + 1:last_index] + s[last_index + 1:]` should be modified to exclude the substring between the first and last occurrence of the character from being removed.

The correct code should be:
```python
def func_1(s: str, ch: str) -> str:
    first_index = s.find(ch)
    last_index = s.rfind(ch)
    if first_index == -1 or last_index == -1 or first_index == last_index:
        return s
    return s[:first_index] + s[first_index + 1:last_index] + s[last_index + 1:]
```
Should be modified to:
```python
def func_1(s: str, ch: str) -> str:
    first_index = s.find(ch)
    last_index = s.rfind(ch)
    if first_index == -1 or last_index == -1 or first_index == last_index:
        return s
    return s[:first_index] + s[first_index + 1:last_index] + s[last_index:]
```
Or even simpler:
```python
def func_1(s: str, ch: str) -> str:
    first_index = s.find(ch)
    last_index = s.rfind(ch)
    if first_index == -1 or last_index == -1 or first_index == last_index:
        return s
    return s.replace(ch, '', 1).replace(ch, '', 1)
```
However, the above solution may not work correctly for all edge cases.

Therefore, the final assessment is:
Final: **False**