Let's analyze the code step by step:

1. The initial state is defined as follows:
   - `n` is an integer between 1 and 100.
   - `s` is a string of `n` lowercase Latin letters.
   - `dp` is a list of length `n + 1`.
   - `i` is `n + 1`.
   - `j` is `n - 1`.
   - `dp[i]` is updated to `min(dp[i], dp[j])` if `s[j:i]` is a substring of `s[:j]`; otherwise, `dp[i]` remains unchanged.

2. The given code snippet updates `dp[i]` based on the following condition:
   ```python
   dp[i] = min(dp[i], dp[j] + (i - j) // (i - j - j) + 1)
   ```

3. First, let's simplify the expression `(i - j) // (i - j - j) + 1`:
   - Since `i = n + 1` and `j = n - 1`, we have `i - j = (n + 1) - (n - 1) = 2`.
   - Substituting these into the expression gives: `(2) // (2 - (n - 1)) + 1 = 2 // (3 - n) + 1`.

4. Now, let's evaluate the division and addition:
   - The term `(2 // (3 - n))` depends on the value of `n`. However, since `n` is between 1 and 100, `(3 - n)` will always be a negative number because `3 - 100 = -97` and `3 - 1 = 2`, but the minimum value is `-97`.
   - In Python, dividing a positive number by a negative number results in a negative quotient. So, `2 // (3 - n)` will always be `-1` (since the quotient of a positive number divided by a negative number is negative and the floor division rounds towards negative infinity).

5. Therefore, the expression simplifies to:
   ```python
   2 // (3 - n) + 1 = -1 + 1 = 0
   ```

6. The updated code now looks like:
   ```python
   dp[i] = min(dp[i], dp[j] + 0) = min(dp[i], dp[j])
   ```

7. This means that `dp[i]` is updated to `min(dp[i], dp[j])` based on the condition that `s[j:i]` is a substring of `s[:j]`.

8. Given the initial conditions and the fact that `i = n + 1` and `j = n - 1`, the only change is to `dp[i]`.

Output State: **`n` is an integer between 1 and 100; `s` is a string of `n` lowercase Latin letters; `dp` is a list of length `n + 1`; `i` is `n + 1`; `j` is `n - 1`; `dp[i]` is updated to `min(dp[i], dp[j])`.**