To determine the output state after the loop has finished executing, we need to carefully follow the loop's logic and see how the variables `A`, `idx_A`, `B`, and `idx_B` change with each iteration. The loop iterates `n` times, and the provided code snippet does not specify the value of `n` or the string `s`. Since the initial state does not involve `s` or `n`, and the final state needs to be derived based on the loop's operations, we need to assume `n` and `s` such that the loop's operations are meaningful.

For simplicity, let's assume `n` is 5 and `s` is a string of length 5 that contains the character '<' in a way that triggers the operations in the loop. Let's assume `s = '<<><<'`.

Here's the step-by-step execution:

1. **Initial State:**
   - `A` is [0, 2, 4]
   - `idx_A` is [1, 3, 4]
   - `B` is []
   - `idx_B` is []

2. **Loop Iteration:**

   - **First Iteration (j = 0, i = 4):**
     - `s[4]` is '<'
     - Since `idx_B` is empty, `B` is updated to `[0]`
     - `idx_B` is updated to `[4]`
     - Current State: `A` is [0, 2, 4]; `idx_A` is [1, 3, 4]; `B` is [0]; `idx_B` is [4]

   - **Second Iteration (j = 1, i = 3):**
     - `s[3]` is '>'
     - No changes to `B` or `idx_B`
     - Current State: `A` is [0, 2, 4]; `idx_A` is [1, 3, 4]; `B` is [0]; `idx_B` is [4]

   - **Third Iteration (j = 2, i = 2):**
     - `s[2]` is '<'
     - `x = B[len(B) - 1] + (idx_B[len(B) - 1] - i) * len(idx_B)`
     - `x = 0 + (4 - 2) * 1 = 2`
     - `B` is updated to `[0, 2]`
     - `idx_B` is updated to `[4, 2]`
     - Current State: `A` is [0, 2, 4]; `idx_A` is [1, 3, 4]; `B` is [0, 2]; `idx_B` is [4, 2]

   - **Fourth Iteration (j = 3, i = 1):**
     - `s[1]` is '<'
     - `x = B[len(B) - 1] + (idx_B[len(B) - 1] - i) * len(idx_B)`
     - `x = 2 + (2 - 1) * 2 = 4`
     - `B` is updated to `[0, 2, 4]`
     - `idx_B` is updated to `[4, 2, 1]`
     - Current State: `A` is [0, 2, 4]; `idx_A` is [1, 3, 4]; `B` is [0, 2, 4]; `idx_B` is [4, 2, 1]

   - **Fifth Iteration (j = 4, i = 0):**
     - `s[0]` is '<'
     - `x = B[len(B) - 1] + (idx_B[len(B) - 1] - i) * len(idx_B)`
     - `x = 4 + (1 - 0) * 3 = 7`
     - `B` is updated to `[0, 2, 4, 7]`
     - `idx_B` is updated to `[4, 2, 1, 0]`
     - Current State: `A` is [0, 2, 4]; `idx_A` is [1, 3, 4]; `B` is [0, 2, 4, 7]; `idx_B` is [4, 2, 1, 0]

The final state after all iterations is:

Output State: **A is [0, 2, 4]; idx_A is [1, 3, 4]; B is [0, 2, 4, 7]; idx_B is [4, 2, 1, 0].**