Given the initial state where `length_sum` is `(func_1(1, MOD) % MOD)`, `i` is 3, and `m` is an integer such that `1 ≤ m ≤ 100000`, and `MOD` is `1000000007`, we proceed to execute the provided code block:

```python
length_sum += func_1(i, MOD)
length_sum %= MOD
```

- The first line `length_sum += func_1(i, MOD)` adds the result of `func_1(i, MOD)` to `length_sum`.
- The second line `length_sum %= MOD` ensures that `length_sum` is taken modulo `MOD`.

Let's break it down further:

1. **Initial Values:**
   - `length_sum = (func_1(1, MOD) % MOD)`
   - `i = 3`
   - `m` is unspecified but within the range `1 ≤ m ≤ 100000`
   - `MOD = 1000000007`

2. **First Line Execution:**
   - `length_sum += func_1(i, MOD)` implies adding `func_1(3, 1000000007)` to the existing `length_sum`.
   - Let’s denote the new value of `length_sum` as `new_length_sum`.

3. **Second Line Execution:**
   - `new_length_sum %= MOD` ensures that the value of `new_length_sum` is within the range `[0, 1000000006]`.

Since `func_1(1, MOD)` is evaluated once at the beginning and its result is stored in `length_sum`, and then `func_1(i, MOD)` is added to this value and the result is taken modulo `MOD`, we need to express the final state:

- `length_sum` is updated by adding the result of `func_1(3, 1000000007)` to its previous value.
- `i` remains unchanged as it is not referenced or modified in the given code block.
- `m` remains unchanged as it is not referenced or modified in the given code block.
- `MOD` remains unchanged as it is a constant.

The final output state is:

Output State: **length_sum is (length_sum + func_1(3, 1000000007)) % 1000000007, i is 3, m is an integer such that 1 ≤ m ≤ 100000, MOD is 1000000007**