Output State: **`sum` is 7, `j` is `n+1`, `i` is 2, `n` must be greater than or equal to 2**

Explanation: 
- Initially, `sum` is 1.
- The code updates `sum` by adding the value `(i * i - (i - 1) * (i - 1)) * i` to it.
- Given `i` is 2, the expression evaluates to `(2 * 2 - (2 - 1) * (2 - 1)) * 2 = (4 - 1) * 2 = 3 * 2 = 6`.
- So, `sum` becomes `1 + 6 = 7`.
- The values of `j`, `i`, and `n` remain unchanged from their initial states. `j` is `n+1`, which means `j` is `n+1`, and `n` must be greater than or equal to 2.