To determine the output of the `print` statement, let's break down the given initial state and the code snippet step by step:

### Initial State Breakdown

1. **Variables and their relationships:**
   - `u` is defined as `c_new - 3`, where `c_new > 2`.
   - `c` and `d` are the values returned by `r()`, which are `c_new` and `d_new` respectively.
   - `t` is set to `False`.
   - `a` is a tuple `(-1000000000.0, c_new, d_new, 2000000000.0)`.
   - `b` is a list `[0, 0, 1, 1]`.

2. **List `b`:**
   - `b` is explicitly given as `[0, 0, 1, 1]`.

3. **Indices used in the print statement:**
   - The print statement uses indices `c * 2 - 1` and `d * 2 - 1` to access elements in the list `b`.

### Calculation of Indices

- Since `c` and `d` are `c_new` and `d_new` respectively, we need to determine the values of `c_new` and `d_new` to calculate the indices.
- The indices are calculated as follows:
  - `index1 = c * 2 - 1`
  - `index2 = d * 2 - 1`

### Accessing Elements in List `b`

- Using the indices `index1` and `index2`, we access elements from the list `b`.
- The list `b` is `[0, 0, 1, 1]`.

### Example Calculation

Let's assume hypothetical values for `c_new` and `d_new` to illustrate the calculation:
- Suppose `c_new = 2` and `d_new = 3` (these values satisfy `c_new > 2`).

Then,
- `c = 2` and `d = 3`
- `index1 = c * 2 - 1 = 2 * 2 - 1 = 3`
- `index2 = d * 2 - 1 = 3 * 2 - 1 = 5`

However, since `b` only has indices up to 3, `index2` being 5 would be out of bounds. Therefore, we need to ensure `c_new` and `d_new` result in valid indices within the bounds of `b`.

Let's consider another valid example:
- Suppose `c_new = 1` and `d_new = 2` (these values do not satisfy `c_new > 2`, so they are invalid).

Let's consider another valid example:
- Suppose `c_new = 2` and `d_new = 2` (these values satisfy `c_new > 2`).

Then,
- `c = 2` and `d = 2`
- `index1 = c * 2 - 1 = 2 * 2 - 1 = 3`
- `index2 = d * 2 - 1 = 2 * 2 - 1 = 3`

Thus,
- `b[index1] = b[3] = 1`
- `b[index2] = b[3] = 1`

### Final Calculation

The expression inside the `print` statement is:
```python
print(b[c * 2 - 1] - b[d * 2 - 1])
```
Substituting the values:
```python
print(b[3] - b[3])  # which is 1 - 1
```

### Output

Therefore, the output of the print statement is:
Output: **0**