To determine what will be printed, let's break down the expression inside the `print` statement:

The expression is `n if n - k <= 1 else 1`.

Given the initial state:
- `t` is a positive integer such that \(1 \leq t \leq 10^3\).
- `n` is an input integer.
- `k` is an input integer.

We need to evaluate the condition `n - k <= 1`:
- If `n - k <= 1` is true, then the expression evaluates to `n`.
- If `n - k <= 1` is false, then the expression evaluates to `1`.

Let's consider both cases:

1. **Case 1: `n - k <= 1` is true**
   - This means \(n - k \leq 1\), so `n` is either equal to `k` or `n` is one more than `k`.
   - In this case, the expression evaluates to `n`.

2. **Case 2: `n - k <= 1` is false**
   - This means \(n - k > 1\), so `n` is greater than `k` by more than 1.
   - In this case, the expression evaluates to `1`.

Based on the above analysis, the output will depend on the relationship between `n` and `k`:
- If \(n - k \leq 1\), the output will be `n`.
- If \(n - k > 1\), the output will be `1`.

Therefore, the output will be either `n` or `1` depending on the values of `n` and `k`.

Output: **n if n - k <= 1 else 1**