Alright, I've got this problem to solve. Let's see what it's asking for. So, there's a ribbon divided into n cells, numbered from 1 to n from left to right. Each cell either has a chip or is free. I can perform operations where I choose a chip and move it to the closest free cell to the left. I can do this any number of times, even zero. My goal is to move the chips so that they form a single block with no free cells between them. And I need to find the minimum number of operations required to achieve this.

First, I need to understand what a "block" means in this context. It means that all the chips are consecutive with no gaps between them. So, if I have chips at positions 1, 3, 4, and 6, I need to move them so that they are, say, at positions 1, 2, 3, and 4, or maybe 2, 3, 4, and 5, as long as there are no gaps between them.

Okay, so the problem is to make the chips contiguous with the minimum number of moves. Each move consists of taking a chip and moving it to the closest free cell to the left.

Let me think about how to approach this.

First, I need to identify the current positions of the chips. Let's say I have an array a of size n, where a[i] is 1 if there's a chip at position i, and 0 if it's free.

I need to rearrange the chips so that they form a contiguous block with no free cells between them, using the minimum number of operations.

An operation is defined as moving a chip to the closest free cell to the left.

Wait, but in the operation, it's not just moving to any free cell to the left, but to the closest free cell to the left.

So, in each operation, I choose a chip that has at least one free cell to its left, and move it to the nearest free cell to the left.

I need to repeat this operation until all chips form a contiguous block.

I need to find the minimum number of such operations.

Let me consider an example to understand better.

Take the first example from the problem:

n = 8

a = [0, 1, 1, 1, 0, 1, 1, 0]

So, positions 2,3,4,6,7 have chips.

I need to make these chips contiguous.

One way is to move the chip from position 7 to position 5, so now a = [0,1,1,1,1,1,0,0]

Now, all chips are contiguous from position 2 to position 6.

That took one operation, which matches the example's output.

Another example:

n = 6

a = [0,1,0,0,0,0]

Here, chips are already contiguous (just one chip), so no operations needed.

n = 6

a = [1,1,1,1,1,1]

All chips are already contiguous, so no operations needed.

n = 5

a = [1,0,1,0,1]

Need to make them contiguous.

Option 1: Move the chip from position 5 to position 2, resulting in [1,1,1,0,0]

Then move the chip from position 3 to position 4, resulting in [1,1,0,1,0]

Wait, that doesn't seem right.

Wait, no, in the first move, I can only move to the closest free cell to the left.

In the initial configuration [1,0,1,0,1], the closest free cell to the left for position 5 is position 4.

So, moving position 5 to position 4: [1,0,1,1,0]

Now, [1,0,1,1,0]

Next, the chip at position 3 can be moved to position 2: [1,1,0,1,0]

Now, [1,1,0,1,0]

Finally, move the chip at position 4 to position 3: [1,1,1,0,0]

So, that took two operations, which matches the example's output.

Another example:

n = 9

a = [0,1,1,0,0,0,1,1,0]

Move the chip at position 7 to position 5: [0,1,1,0,1,0,1,1,0]

Then move the chip at position 8 to position 6: [0,1,1,0,1,1,1,0,0]

Then move the chip at position 4 to position 3: [0,1,1,1,1,1,0,0,0]

So, that took three operations, matching the example.

From these examples, it seems that the number of operations required is equal to the number of gaps between the leftmost and rightmost chips.

Wait, in the first example, there was one operation for n=8, and there was one gap between positions 4 and 6.

In the second example, n=5, two operations, and there were two gaps between positions 1,3,5.

Wait, positions 1,3,5 have chips, so gaps between 1 and 3, and between 3 and 5.

Similarly, in n=9, three operations for three gaps between the chips.

Wait, but in n=5, after first move, [1,1,1,0,0], which has no gaps.

Wait, perhaps the number of operations is equal to the number of chips that are not already in the final positions.

Wait, perhaps it's the number of chips that are not in the leftmost block.

Wait, maybe it's the number of chips that need to be moved to fill the gaps.

Wait, perhaps it's the number of free cells between the leftmost and rightmost chips.

Wait, in the first example, n=8, a=[0,1,1,1,0,1,1,0]

Leftmost chip at position 2, rightmost at position 7.

Between 2 and 7, there are 6 positions: 2,3,4,5,6,7.

Chips are at 2,3,4,6,7, so missing at position 5.

So, one gap, which matches the one operation.

In n=5, a=[1,0,1,0,1]

Leftmost at 1, rightmost at 5.

Positions 1,2,3,4,5.

Chips at 1,3,5, missing at 2 and 4, so two gaps, which matches the two operations.

In n=9, a=[0,1,1,0,0,0,1,1,0]

Leftmost at 2, rightmost at 8.

Positions 2 to 8: 2,3,4,5,6,7,8.

Chips at 2,3,7,8, missing at 4,5,6, so three gaps, matching the three operations.

So, it seems that the number of operations required is equal to the number of free cells between the leftmost and rightmost chips.

So, to generalize, for each test case:

- Find the leftmost chip's position.

- Find the rightmost chip's position.

- Consider the substring from leftmost to rightmost.

- Count the number of free cells (0's) in this substring.

- That count is the number of operations needed.

Wait, in the first example, leftmost at 2, rightmost at 7, substring is positions 2 to 7: [1,1,1,0,1,1], which has one 0, which matches the one operation.

In n=5, positions 1 to 5: [1,0,1,0,1], has two 0's, matching two operations.

In n=9, positions 2 to 8: [1,1,0,0,0,1,1], has three 0's, matching three operations.

Yes, this seems consistent.

So, the strategy is:

- Find the leftmost chip's position.

- Find the rightmost chip's position.

- Look at the substring from leftmost to rightmost.

- Count the number of 0's in this substring.

- That's the number of operations needed.

This seems efficient and straightforward.

Now, let's look at the provided program and see if it implements this logic correctly.

The program is:

def func():

t = int(input(''))

for _ in range(t):

n = int(input(''))

arr = str(input(''))

x = arr.find('1')

y = arr[::-1].find('1')

z = arr[x:n - y]

print(z.count('0'))

So, let's analyze this step by step.

- Read the number of test cases, t.

- For each test case:

- Read n, the number of cells.

- Read arr, which is a string of n integers (0 or 1).

- Find the position of the first '1' from the left, which is the leftmost chip's position. This is stored in x.

- Find the position of the first '1' from the right, which is the rightmost chip's position. This is stored in y.

- Then, z is set to arr[x: n - y].

- Finally, print the count of '0's in z.

Wait, I need to make sure I understand what z represents.

arr is a string of 0's and 1's, representing the cells.

x is the index of the first '1' from the left.

y is the index of the first '1' from the right, but since arr is reversed, y is the position from the end.

So, arr[::-1].find('1') gives the position from the end where the first '1' is found.

Then, n - y would be the starting position from the left for the rightmost chip.

Wait, I need to be careful here.

Let's take an example to see.

Take n=8, arr='0 1 1 1 0 1 1 0'

First, arr.find('1') would give x=1 (since indexing starts at 0, and the first '1' is at position 1).

arr[::-1] is '0 1 1 0 1 1 1 0', and arr[::-1].find('1') would give y=0 (since the first '1' is at position 0 from the end).

Then, z = arr[1 : 8 - 0] = arr[1:8], which is '1 1 1 0 1 1 0'

Then, z.count('0') = 2, but in the example, the answer is 1.

Wait, that doesn't match.

Wait, in the example, the answer is 1, but according to this code, it would output 2.

But according to our earlier reasoning, it should be the number of '0's between the leftmost and rightmost chips, which in this case is one '0' between positions 4 and 5.

Wait, but according to the code, it's counting two '0's in '1 1 1 0 1 1 0'

Wait, positions 2 to 8: [1,1,1,0,1,1,0], which has one '0' at position 5.

But the string '1 1 1 0 1 1 0' has two '0's if spaces are considered.

Wait, perhaps there's an issue with how the input string is being processed.

Assuming arr is read as a string with spaces, like '0 1 1 1 0 1 1 0'

Then, arr.find('1') would return the index of the first '1', which is position 2 (since '0 1' has the '1' at index 2).

Wait, no, in Python, string indices start at 0.

Given arr = '0 1 1 1 0 1 1 0'

Then arr[0] = '0', arr[1] = ' ', arr[2] = '1', etc.

So, arr.find('1') would return 2, since '1' is at position 2.

arr[::-1] is '0 1 1 0 1 1 1 0' [reversed with spaces]

arr[::-1].find('1') would return 0, since the first '1' is at position 0.

Then, z = arr[2 : 8 - 0] = arr[2:8] = '1 1 1 0 1 1 0'

Then, z.count('0') would count the number of '0's in this substring.

But in the example, the correct answer is 1, but according to this, it's counting two '0's (at positions 5 and 8).

Wait, but in the problem, the cells are numbered from 1 to n, and arr is a sequence of 0's and 1's separated by spaces.

So, for n=8, arr='0 1 1 1 0 1 1 0'

The positions are:

Position 1: '0'

Position 2: '1'

Position 3: '1'

Position 4: '1'

Position 5: '0'

Position 6: '1'

Position 7: '1'

Position 8: '0'

Leftmost chip at position 2, rightmost at position 7.

So, substring from position 2 to 7: '1 1 1 0 1 1'

In this substring, there is one '0' at position 5.

But in the string '1 1 1 0 1 1', there are two '0's if spaces are considered.

Wait, no, the spaces are part of the string, so '1 1 1 0 1 1' has '0' only once.

Wait, no, actually, in Python, arr = '0 1 1 1 0 1 1 0'

Then arr[2:8] is '1 1 1 0 1 1'

In this substring, '1 1 1 0 1 1', there is one '0'.

So, z.count('0') should correctly return 1, which matches the example.

Wait, perhaps I miscalculated earlier.

Yes, in arr[2:8], which is '1 1 1 0 1 1', there is only one '0', so z.count('0') is 1, which matches the example.

Okay, so in this case, it works.

Let's check another example.

Take n=5, arr='1 0 1 0 1'

x = arr.find('1') = 0 (since '1' is at position 0)

y = arr[::-1].find('1') = '1 0 1 0 1'[::-1] = '1 0 1 0 1', so arr[::-1].find('1')=0

z = arr[0 : 5 - 0] = arr[0:5] = '1 0 1 0 1'

z.count('0') = 2, which matches the example's output of 2 operations.

Another example: n=6, arr='0 1 0 0 0 0'

x = arr.find('1') = 2

y = arr[::-1].find('1') = '0 0 0 0 1 0'[::-1] = '0 1 0 0 0 0', so arr[::-1].find('1')=1 (position 1 from the end)

Then, z = arr[2 : 6 - 1] = arr[2:5] = '1 0 0'

z.count('0') = 2, but according to the problem, the answer should be 0.

Wait, but in the problem, for n=6, arr='0 1 0 0 0 0', the output is 0.

But according to this code, it would output 2, which is incorrect.

Wait, there's a discrepancy here.

So, in this case, the code is giving the wrong answer.

Wait, perhaps I'm misunderstanding how y is calculated.

Let's look again.

y = arr[::-1].find('1')

For arr='0 1 0 0 0 0', arr[::-1] is '0 0 0 0 1 0'

Then, arr[::-1].find('1') = 4 (since '1' is at position 4 from the start in the reversed string)

Then, n - y = 6 - 4 = 2

So, z = arr[2:2], which is an empty string.

Then, z.count('0') = 0, which matches the example's output.

Wait, but earlier I thought arr[::-1].find('1') would be 1, but actually, in Python, string[::-1].find('1') returns the position in the reversed string, which is from the start, not from the end.

Wait, no, in Python, s[::-1].find('1') returns the index in the reversed string, which corresponds to the position from the end.

Wait, no, in Python, s[::-1] is the reversed string, and find('1') returns the index in that reversed string.

But we need to map it back to the original string.

Wait, perhaps I'm getting confused.

Let's check with n=6, arr='0 1 0 0 0 0'

arr[::-1] is '0 0 0 0 1 0'

arr[::-1].find('1') is 4, because the '1' is at position 4 in the reversed string.

So, y = 4

Then, z = arr[x: n - y] = arr[1 : 6 - 4] = arr[1:2] = '1'

Then, z.count('0') = 0, which matches the example's output of 0.

Wait, but earlier I thought n - y is 2, so arr[1:2] is '1', which has zero '0's.

Yes, that matches.

Wait, but earlier I thought arr.find('1') is 1, but in this arr='0 1 0 0 0 0', arr.find('1') is 2.

Wait, no, let's check:

arr = '0 1 0 0 0 0'

arr.find('1') is position 2 (since '0 '[space]'1'... space is position 1, '1' is position 2)

arr[::-1] is '0 0 0 0 1 0'

arr[::-1].find('1') is position 4.

n - y = 6 - 4 = 2

So, z = arr[2:2], which is an empty string.

Then, z.count('0') = 0, which matches the example.

Wait, but in the earlier miscalculation, I thought z = arr[2:6-1] = arr[2:5], but that's incorrect.

Actually, n - y = 6 - 4 = 2, so z = arr[2:2], which is empty.

Hence, z.count('0') = 0.

So, it works correctly for this case.

Another example: n=6, arr='1 1 1 1 1 1'

x = arr.find('1') = 0

y = arr[::-1].find('1') = 0

z = arr[0:6-0] = arr[0:6] = '1 1 1 1 1 1'

z.count('0') = 0, which matches the example's output.

Another example: n=5, arr='1 0 1 0 1'

x = arr.find('1') = 0

y = arr[::-1].find('1') = 1 (since arr[::-1] = '1 0 1 0 1', first '1' at position 1)

n - y = 5 - 1 = 4

z = arr[0:4] = '1 0 1 0'

z.count('0') = 2, which matches the example's output.

Wait, but according to our earlier manual calculation, it should be two operations.

Wait, but in the problem's example, it's two operations, so this matches.

Wait, but earlier I thought there was a discrepancy, but actually, it's correct.

Wait, perhaps I was mistaken earlier.

Let me check again.

For n=6, arr='0 1 0 0 0 0'

x = arr.find('1') = 2

y = arr[::-1].find('1') = 4

z = arr[2:6-4] = arr[2:2] = '', z.count('0') = 0

Which matches the example's output of 0.

For n=8, arr='0 1 1 1 0 1 1 0'

x = 1 (position of first '1')

Wait, no, arr='0 1 1 1 0 1 1 0', arr.find('1')=1

arr[::-1].find('1')=0

z = arr[1:8-0]=arr[1:8]='1 1 1 0 1 1 0'

z.count('0')=1, which matches the example.

For n=5, arr='1 0 1 0 1'

x=0, y=1, z=arr[0:5-1]=arr[0:4]='1 0 1 0', z.count('0')=2, matches the example.

For n=9, arr='0 1 1 0 0 0 1 1 0'

x=1, y=3 (since arr[::-1].find('1')=3)

z=arr[1:9-3]=arr[1:6]='1 1 0 0 0'

z.count('0')=3, matches the example's output of 3.

So, in all examples, this code produces the correct output.

Therefore, it seems that this code correctly implements the logic we discussed earlier.

Hence, the given program is correct.

**Final Answer**

\[ \boxed{\text{True}} \]