Alright, I have this problem to solve. Let's see what it's about. There's a one-dimensional grid of length n, and each cell contains either a '<' or a '>'. When a pinball is placed on one of these cells, it moves according to the character in that cell: '<' means move left, '>' means move right. After moving, the character in the cell from which it moved inverts (so '<' becomes '>', and '>' becomes '<'). The pinball stops when it goes off the grid, either to the left or to the right.

I need to answer n queries, each corresponding to placing the pinball on the i-th cell and determining how many seconds it takes for the pinball to leave the grid.

First, I need to understand the behavior of the pinball. Let's consider a simple example to see how it works.

Suppose n=3 and s="><<".

- Place pinball on cell 1: '>', so it moves right to cell 2. Now, cell 1 becomes '<'.

  - Cell 2 is '<', so it moves left to cell 1. Cell 2 becomes '>'.

  - Cell 1 is now '<', so it moves left and leaves the grid. Total steps: 2.

Wait, but according to the example in the problem, for n=3 and s="><<", the answers are 3, 6, 5. So my initial thought is wrong. Maybe I miscalculated.

Let me try again.

For i=1:

- Pinball on cell 1: '>', moves to cell 2. s becomes "<< <"

- Pinball on cell 2: '<', moves to cell 1. s becomes "< >"

- Pinball on cell 1: '<', moves left and leaves the grid.

Total steps: 2, but the example says 3. Hmm, maybe I missed something.

Wait, the problem says "the character s_i is inverted after the pinball has moved". So, when the pinball moves from cell i to cell j, s_i is inverted.

In the first step:

- Pinball on cell 1: '>', moves to cell 2. s[1] becomes '<'. So s is now "< <".

- Pinball on cell 2: '<', moves to cell 1. s[2] becomes '>'. s is now "< >".

- Pinball on cell 1: '<', moves left and leaves the grid.

Total steps: 3. Okay, that matches the example.

I see, so the inversion happens after the move, not before.

Alright, now I need to generalize this for any n and any string s.

Constraints are large: n up to 5*10^5, and t test cases with sum of n over all test cases up to 5*10^5. So, I need an efficient solution, O(n) per test case ideally.

Let me think about how to approach this.

One way is to simulate the process for each starting position, but that would be O(n^2), which is too slow.

I need a smarter way.

Let's think about the movement of the pinball.

Each time it moves, it changes direction based on the current character, and then that character inverts.

So, the state of the grid changes over time.

This seems complicated to track directly.

Maybe I can model this in a different way.

Let's consider that each cell has a direction, and the pinball moves accordingly, but the direction changes after each move.

This is similar to a kind of automaton where the state changes with each move.

I need to find a way to calculate the number of steps for each starting position without simulating each step.

Perhaps I can think in terms of cycles or something.

Wait, another idea: since the grid is one-dimensional and the pinball can only move left or right, depending on the current character, and the characters change after each move, maybe I can model the path the pinball takes and find a pattern.

Let me try to think about what happens when the pinball moves.

Suppose the pinball is at position i.

- If s[i] is '>', it moves to i+1, then s[i] becomes '<'.

- If s[i] is '<', it moves to i-1, then s[i] becomes '>'.

So, the grid evolves with each move.

This seems tricky to handle directly.

Is there a way to precompute some values that can help me calculate the number of steps for each starting position efficiently?

Let me consider the possible paths the pinball can take from each starting position until it leaves the grid.

I need to find the number of steps until it exits, for each starting position.

Given the constraints, I need an O(n) or O(n log n) solution.

Another thought: perhaps I can process the grid from left to right and from right to left, keeping track of some cumulative values that help me determine the number of steps.

Let me look at the example again to see if I can find a pattern.

First test case:

n=3

s="><<"

Answers: 3 6 5

Let's see:

- Starting at position 1: '>' -> move right to position 2, s[1] becomes '<'

  - Position 2: '<' -> move left to position 1, s[2] becomes '>'

  - Position 1: '<' -> move left and exit. Total steps: 3.

- Starting at position 2: '<' -> move left to position 1, s[2] becomes '>'

  - Position 1: '<' -> move left and exit. Total steps: 2.

Wait, but according to the example, it's 6. So maybe my simulation is wrong again.

Wait, perhaps the inversion affects future moves.

Let me try again.

Starting at position 2: '<'

- Move left to position 1, s[2] becomes '>'

  - Now s = "< >"

  - Position 1: '<' -> move left and exit. Total steps: 2.

But the example says 6. So clearly, my simulation is incomplete.

Wait, perhaps the inversion affects the path in a way that causes more steps.

Let me try to follow the example's explanation.

In the first test case, for i=1, it takes 3 steps.

For i=2, it takes 6 steps.

Wait, perhaps the pinball can oscillate between cells multiple times before exiting.

I need to find a general way to calculate this without simulating each step.

Maybe I can model this using some kind of graph where each node represents a cell state, but that seems too complicated given the constraints.

Let me look at the code provided and try to understand what it's doing.

The code defines a function func_1(s) that seems to process the string s and print the answers for each position.

It first processes the string to build two arrays A and B.

A seems to be built for positions with '>', and B for positions with '<'.

It uses idx_A and idx_B to keep track of positions where s[i] == '>' and s[i] == '<', respectively.

Then, it iterates through each position i from 0 to n-1, determines whether s[i] is '>' or '<', and based on that, computes the number of steps using values from A and B, along with some indices.

This seems quite optimized, likely O(n) per test case, given the constraints.

But to verify if it's correct, I need to understand the logic behind it.

Let me try to understand the logic for computing the number of steps.

First, it builds A for positions with '>', keeping some cumulative sum.

Similarly, B for positions with '<'.

Then, for each position i, depending on whether s[i] is '>' or '<', it uses the precomputed values in A and B to calculate the number of steps.

Given the complexity of the code and the time constraints, it's challenging to verify its correctness without a clear understanding of the underlying logic.

Perhaps I can test the code with the sample input and see if it produces the correct output.

Sample Input:

3

3

><<

4

<<<<

6

<><<<>

Sample Output:

3 6 5

1 2 3 4

1 4 7 10 8 1

Let me run the code with this input and see if it matches.

Assuming the code is correct and produces the expected output, then it's likely correct.

But since I need to determine if the given program is correct, I should verify it with some test cases.

Let's take the first test case:

n=3

s= ><<

Expected output: 3 6 5

Let me see what the code does.

It first calls func_1(s).

n = 3

s = "><<"

Building A for positions with '>':

- i=0: s[0] == '>', so A=[0], idx_A=[0]

- i=1: s[1] == '<', skip

- i=2: s[2] == '<', skip

So A = [0], idx_A = [0]

Building B for positions with '<':

- i=0: s[0] == '>', skip

- i=1: s[1] == '<', B=[0], idx_B=[1]

- i=2: s[2] == '<', B=[0, (1 - 2)*1 = -1], idx_B=[1,2]

Wait, no, likely it's B.append(B[-1] + (idx_B[-1] - i)*len(idx_B))

Wait, in code:

for j in range(0, n):

    i = n - 1 - j

    if s[i] == '<':

        if len(idx_B) == 0:

            B.append(0)

        else:

            x = B[len(B) - 1] + (idx_B[len(idx_B) - 1] - i) * len(idx_B)

            B.append(x)

        idx_B.append(i)

So for n=3, s= ><<

- j=0, i=2: s[2]=='<'

    - len(idx_B)=0, B.append(0), idx_B=[2]

- j=1, i=1: s[1]=='<'

    - len(idx_B)=1, B.append(B[0] + (idx_B[0] - 1)*1 = 0 + (2-1)*1 = 1)

    - B=[0,1], idx_B=[2,1]

- j=2, i=0: s[0]=='>', skip

So A=[0], idx_A=[0]

B=[0,1], idx_B=[2,1]

Then, it iterates through each position i from 0 to 2:

For i=0:

s[0]=='>'

l=0, r=2

if l < r: # 0 < 2

    a = A[l] = 0

    x = r - (l + 2) = 2 - 2 = 0

    b = B[r - 1] = B[1]=1

    if x >=0: # 0 >=0

        b = b - B[x] = 1 - B[0]=1-0=1

        b = b - (idx_B[x] - idx_B[r - 1]) * (x + 1) = 1 - (2 - 1)*1 = 1 -1=0

    b = b + (idx_B[r - 1] - i)* (l + 1) = 0 + (1 - 0)*1 = 1

    print(a*2 + b*2 + i +1 = 0*2 +1*2 +0 +1 = 0+2+0+1=3)

    l +=1 -> l=1

For i=1:

s[1]=='<'

r -=1 -> r=1

if l <= r: #1 <=1

    if l ==0: # No, l=1

    a = A[l -1] = A[0]=0

    a = a + (i - idx_A[l -1])*l = 0 + (1 - 0)*1 =1

    b = B[r] = B[1]=1

    if r - l >=0: #1 -1 >=0 => 0 >=0

        b = b - B[r - l] =1 - B[0]=1-0=1

        b = b - (idx_B[r - l] - i)*(r - l) =1 - (idx_B[0] -1)*0 =1 - (2-1)*0=1-0=1

    b = b + (idx_B[r] - i)*l =1 + (1 -1)*1=1+0=1

    print(a*2 + b*2 +i +1=1*2 +1*2 +1 +1=2+2+1+1=6)

For i=2:

s[2]=='<'

r -=1 -> r=0

if l <= r: #1 <=0 -> False

elif r ==0:

print(n -i + (i - idx_A[l -1])*2 =3 -2 + (2 -0)*2=1 +4=5)

So, it prints 3 6 5, which matches the sample output.

Another test case:

n=4

s=<<<<

Expected output:1 2 3 4

Let's see:

Build A for '>':

- No '>', so A=[], idx_A=[]

Build B for '<':

- j=0, i=3: s[3]=='<', B=[0], idx_B=[3]

- j=1, i=2: s[2]=='<', B.append(B[0] + (3-2)*1=0+1*1=1), idx_B=[3,2]

- j=2, i=1: s[1]=='<', B.append(1 + (2-1)*2=1+1*2=3), idx_B=[3,2,1]

- j=3, i=0: s[0]=='<', B.append(3 + (1-0)*3=3+1*3=6), idx_B=[3,2,1,0]

So A=[], idx_A=[]

B=[0,1,3,6], idx_B=[3,2,1,0]

Then, for each i from 0 to 3:

i=0:

s[0]=='<'

r=4, l=0

if l <=r: #0 <=4

    if l ==0:

        print(i +1=0+1=1)

    else:

        ...

But l==0, so print 1

i=1:

r=3

if l <=r: #0 <=3

    if l ==0:

        print(i +1=1+1=2)

    else:

        ...

But l==0, so print 2

i=2:

r=2

if l <=r: #0 <=2

    if l ==0:

        print(i +1=2+1=3)

    else:

        ...

l==0, so print 3

i=3:

r=1

if l <=r: #0 <=1

    if l ==0:

        print(i +1=3+1=4)

    else:

        ...

l==0, so print 4

So, it prints 1 2 3 4, matching the sample output.

Another test case:

n=6

s=<><<<>

Build A for '>':

- i=0: s[0]=='<', skip

- i=1: s[1]=='>', A=[0], idx_A=[1]

- i=2: s[2]=='<', skip

- i=3: s[3]=='<', skip

- i=4: s[4]=='<', skip

- i=5: s[5]=='>', A=[0, (1 -5)*1 = -4], idx_A=[1,5]

So A=[0, -4], idx_A=[1,5]

Build B for '<':

- j=0, i=5: s[5]=='>', skip

- j=1, i=4: s[4]=='<', B=[0], idx_B=[4]

- j=2, i=3: s[3]=='<', B.append(B[0] + (4-3)*1=0+1=1), idx_B=[4,3]

- j=3, i=2: s[2]=='<', B.append(1 + (3-2)*2=1+1*2=3), idx_B=[4,3,2]

- j=4, i=1: s[1]=='>', skip

- j=5, i=0: s[0]=='<', B.append(3 + (2-0)*3=3+2*3=9), idx_B=[4,3,2,0]

So B=[0,1,3,9], idx_B=[4,3,2,0]

Then, for each i from 0 to 5:

i=0:

s[0]=='<'

r=4, l=0

if l <=r: #0 <=4

    if l ==0:

        print(i +1=0+1=1)

    else:

        ...

l==0, so print 1

i=1:

s[1]=='>'

l=0, r=3

if l < r: #0 <3

    a = A[l]=0

    x = r - (l +2)=3 -2=1

    b = B[r -1]=B[3-1]=B[2]=3

    if x >=0: #1 >=0

        b = b - B[x]=3 - B[1]=3-1=2

        b = b - (idx_B[x] - idx_B[r -1])* (x +1)=2 - (3 -4)*2=2 - (-1)*2=2 - (-2)=2+2=4

    b = b + (idx_B[r -1] -i)* (l +1)=4 + (4 -1)*1=4 +3=7

    print(a*2 + b*2 +i +1=0*2 +7*2 +1 +1=0+14+1+1=16)

Wait, but the sample output is 1 4 7 10 8 1

So, it's not matching. Wait, perhaps I made a mistake in calculating.

Let me check again.

For i=1:

s[1]=='>'

l=0, r=3

a = A[l]=0

x = r - (l +2)=3 -2=1

b = B[r -1]=B[2]=3

if x >=0:

    b = b - B[x]=3 -1=2

    b = b - (idx_B[x] - idx_B[r -1])*(x +1)=2 - (3 -4)*2=2 - (-1)*2=2 - (-2)=4

b = b + (idx_B[r -1] -i)*(l +1)=4 + (4 -1)*1=4 +3=7

print(0*2 +7*2 +1 +1=0+14+1+1=16)

But sample output is 4, not 16. So perhaps the code is wrong.

Wait, maybe I misread the code.

Looking back at the code:

if s[i] == '>':

    if l < r:

        a = A[l]

        x = r - (l + 2)

        b = B[r - 1]

        if x >= 0:

            b = b - B[x]

            b = b - (idx_B[x] - idx_B[r - 1]) * (x + 1)

        b = b + (idx_B[r - 1] - i) * (l + 1)

        print(a * 2 + b * 2 + i + 1, end=' ')

    elif r == 0:

        print(n - i, end=' ')

    else:

        a = B[r - 1] + (idx_B[r - 1] - i) * r

        b = A[l - 1]

        if l - r > 0:

            b = b - A[l - r - 1]

            b = b - (idx_A[l - 1] - idx_A[l - r - 1]) * (l - r)

        b = b + (i - idx_A[l - 1]) * r

        print(a * 2 + b * 2 + (n - i), end=' ')

    l += 1

else:

    r -= 1

    if l <= r:

        if l == 0:

            print(i + 1, end=' ')

        else:

            a = A[l - 1] + (i - idx_A[l - 1]) * l

            b = B[r]

            if r - l >= 0:

                b = b - B[r - l]

                b = b - (idx_B[r - l] - i) * (r - l)

            b = b + (idx_B[r] - i) * l

            print(a * 2 + b * 2 + i + 1, end=' ')

    elif r == 0:

        print(n - i + (i - idx_A[l - 1]) * 2, end=' ')

    else:

        a = B[r]

        b = A[l - 1]

        if l - r - 1 > 0:

            b = b - A[l - r - 2]

            b = b - (idx_A[l - 1] - idx_A[l - r - 2]) * (l - r - 1)

        b = b + (i - idx_A[l - 1]) * (r + 1)

        print(a * 2 + b * 2 + (n - i), end=' ')

So, in the case above, for i=1, s[1]=='>', l=0, r=3, l < r, so:

a = A[0]=0

x = r - (l + 2)=3 -2=1

b = B[2]=3

since x >=0:

b = b