The code snippet `k -= n - 1` modifies the value of `k` by subtracting `n - 1` from it. Given the initial state where `n` is an even integer within the range 2 to 10^9 and `k` is a non-negative integer that is at least `n - 1` and less than `n·m`, we can reason about the output state as follows:

1. The value of `k` is decreased by `n - 1`, meaning the new value of `k` will still remain non-negative since the minimum value of `k` initially is `n - 1`.
2. The values of `n` and `m` do not change.

Since `k` is reduced by `n - 1`, we can express the new value of `k` as `k' = k - (n - 1)`.

Therefore, the Output State is: **`n` is an even integer such that 2 ≤ n ≤ 10^9; `m` is an integer such that 2 ≤ m ≤ 10^9; `k` is a non-negative integer such that 0 ≤ k < n·m and now `k` is equal to the previous value of `k` minus `n - 1`.**