The variable `remaining_steps` is assigned the value of `k % (m - 1)`. The value of `k` has been updated to the previous value of `k` minus `n - 1`, which can be represented as `k' = k - (n - 1)`. Therefore, `remaining_steps` becomes `(k - (n - 1)) % (m - 1)`. All other variables remain unchanged.

Output State: **`n` is an even integer such that 2 ≤ n ≤ 10^9; `m` is an integer such that 2 ≤ m ≤ 10^9; `k` is equal to `k - (n - 1)`; `full_rows` is equal to `(k - (n - 1)) // (m - 1); `remaining_steps` is equal to `(k - (n - 1)) % (m - 1)`**.