The given code is `b = a ^ x`. Since `a` is equal to `b ^ x`, we can substitute `a` with `b ^ x` in the given code. Therefore, `b = (b ^ x) ^ x`.

We know that `(b ^ x) ^ x` is equal to `b`. This is because the XOR operation (`^`) is its own inverse, meaning that `(b ^ x) ^ x` will result in `b`.

So, `b` is assigned the value of `b`. The states of the other variables are not affected. 

Output State: **`s` is an integer such that 2 <= `s` <= 10^12, `x` is an integer such that 0 <= `x` <= 10^12, `a` is equal to `b` ^ `x`, and `b` remains unchanged**