Let's break down the initial state and the print statement step by step:

### Initial State:
- `i` is `n-2`
- `n` is an integer greater than 1
- `k` is 0
- `r` is the value of `a[n-2] + k // (n-1)` if the condition `(n-2 + 1) * (a[n-1] - a[n-2]) > k` was met at the last iteration, otherwise `r` is `a[n-1]`
- `rem` is `k % (n-1)` if the condition was met, otherwise `rem` is 0
- `y` is 1 if the condition was met, otherwise `y` is 0
- `k` is 0

### Analysis:
1. **Condition Check**:
   - The condition `(n-2 + 1) * (a[n-1] - a[n-2]) > k` simplifies to `(n-1) * (a[n-1] - a[n-2]) > 0`.
   - Since `k` is 0, the condition simplifies further to `(n-1) * (a[n-1] - a[n-2]) > 0`.
   - Given that `n` is an integer greater than 1, `(n-1)` is positive.
   - Therefore, the condition depends on whether `a[n-1] - a[n-2]` is positive.
   - If `a[n-1] > a[n-2]`, the condition is true.
   - If `a[n-1] <= a[n-2]`, the condition is false.

2. **Values of Variables**:
   - If the condition is true:
     - `r = a[n-2] + k // (n-1) = a[n-2] + 0 = a[n-2]`
     - `rem = k % (n-1) = 0 % (n-1) = 0`
     - `y = 1`
   - If the condition is false:
     - `r = a[n-1]`
     - `rem = 0`
     - `y = 0`

3. **Expression to Print**:
   - The expression to print is `(r - 1) * n + 1 + rem + y`.

### Case 1: Condition is True
- `r = a[n-2]`
- `rem = 0`
- `y = 1`
- Expression: `(a[n-2] - 1) * n + 1 + 0 + 1 = (a[n-2] - 1) * n + 2`

### Case 2: Condition is False
- `r = a[n-1]`
- `rem = 0`
- `y = 0`
- Expression: `(a[n-1] - 1) * n + 1 + 0 + 0 = (a[n-1] - 1) * n + 1`

### Final Output:
- If the condition `(n-1) * (a[n-1] - a[n-2]) > 0` is true:
  - Output: **(a[n-2] - 1) * n + 2**
- If the condition `(n-1) * (a[n-1] - a[n-2]) > 0` is false:
  - Output: **(a[n-1] - 1) * n + 1**

Since the exact values of `a[n-1]` and `a[n-2]` are not provided, we cannot determine the exact numerical output. However, based on the given conditions, the output will be one of the two expressions above.

Output: **(a[n-2] - 1) * n + 2 if the condition (n-1) * (a[n-1] - a[n-2]) > 0 is true, otherwise (a[n-1] - 1) * n + 1**