Let's break down the problem step by step based on the initial state and the given conditions.

### Initial State and Conditions:
1. **p1, p2, and p3 are integers read from the input.**
2. **The sum of p1, p2, and p3 is odd.**
3. **p3 is less than the sum of p1 and p2.**
4. **low is the minimum of p3 - p1 and p3 - p2.**
5. **high must be at least cur + 1.**
6. **cur is either low or low + 1 depending on the condition p1 - cur <= p2 - (p3 - cur).**
7. **If the condition is not met, cur is incremented by 1.**

### Calculations and Conditions:
1. **low = min(p3 - p1, p3 - p2):**
   - This determines the smaller difference between p3 and either p1 or p2.
   
2. **cur determination:**
   - If `p1 - cur <= p2 - (p3 - cur)`, then `cur = low`.
   - Otherwise, `cur = low + 1`.

3. **high:**
   - high is at least `cur + 1`, but its exact value isn't needed for the print statement.

### Print Statement:
The print statement is:
```python
print(p1 - cur + p3)
```

### Analysis:
Let's analyze the expression `p1 - cur + p3` under the given conditions.

1. **cur = low if p1 - cur <= p2 - (p3 - cur) else cur = low + 1:**
   - This condition influences the value of `cur`.

2. **Expression `p1 - cur + p3`:**
   - We need to determine the value of `cur` first to compute the expression.

### Case Analysis:
- **Case 1: cur = low**
  - `p1 - low + p3`
  
- **Case 2: cur = low + 1**
  - `p1 - (low + 1) + p3 = p1 - low - 1 + p3`

Since `low = min(p3 - p1, p3 - p2)`, we need to consider the implications of this minimum value on the expression.

### Simplification:
Given the condition `p3 < p1 + p2` and the sum `p1 + p2 + p3` being odd, let's consider the possible scenarios for `low` and `cur`:

- If `low = p3 - p1`, then `cur` will be `p3 - p1` if the condition `p1 - (p3 - p1) <= p2 - (p3 - (p3 - p1))` is met, otherwise `cur` will be `p3 - p1 + 1`.
- If `low = p3 - p2`, then `cur` will be `p3 - p2` if the condition `p1 - (p3 - p2) <= p2 - (p3 - (p3 - p2))` is met, otherwise `cur` will be `p3 - p2 + 1`.

### Final Expression:
Regardless of whether `cur` is `low` or `low + 1`, the expression `p1 - cur + p3` will simplify to:

- If `cur = low`, then `p1 - low + p3` simplifies to `p1 - min(p3 - p1, p3 - p2) + p3`.
- If `cur = low + 1`, then `p1 - (low + 1) + p3` simplifies to `p1 - min(p3 - p1, p3 - p2) - 1 + p3`.

### Conclusion:
The exact value of `cur` depends on the condition `p1 - cur <= p2 - (p3 - cur)`, but the output will be either `p1 - min(p3 - p1, p3 - p2) + p3` or `p1 - min(p3 - p1, p3 - p2) - 1 + p3`.

### Final Output:
Output: **p1 - min(p3 - p1, p3 - p2) + p3 - x (where x is 0 or 1 depending on the condition p1 - cur <= p2 - (p3 - cur))**