To determine what will be printed by the `print` statement, we need to carefully analyze the given initial state and the relationships between the variables.

Given:
- `p1`, `p2`, and `p3` are integers.
- The sum of `p1`, `p2`, and `p3` is odd.
- `low` is the minimum of `p3 - p1` and `p3 - p2`.
- `high` is the maximum of `p3 - p1` and `p3 - p2`.
- `cur` is equal to `low`.
- `p1 - cur` is less than or equal to `p2 - (p3 - cur)`.

We need to understand the expression `p1 - cur + p3`:
- `cur` is set to `low`, which is the minimum of `p3 - p1` and `p3 - p2`.
- To find `p1 - cur + p3`, we need to consider the possible values of `cur`.

Let's break down the conditions and the calculations:
1. `low` is `min(p3 - p1, p3 - p2)`.
2. `high` is `max(p3 - p1, p3 - p2)`.
3. `cur` is `low`, so it can be either `p3 - p1` or `p3 - p2`, whichever is smaller.
4. The condition `p1 - cur` is less than or equal to `p2 - (p3 - cur)` must hold true.

Let's consider the implications of `cur` being `p3 - p1` or `p3 - p2`:

**Case 1: `cur = p3 - p1`**
- `p1 - (p3 - p1) <= p2 - (p3 - (p3 - p1))`
- `p1 - p3 + p1 <= p2 - p1`
- `2p1 - p3 <= p2 - p1`
- `3p1 - p3 <= p2`
- `3p1 <= p2 + p3`

**Case 2: `cur = p3 - p2`**
- `p1 - (p3 - p2) <= p2 - (p3 - (p3 - p2))`
- `p1 - p3 + p2 <= p2 - p2`
- `p1 - p3 + p2 <= 0`
- `p1 + p2 <= p3`

Since `cur` is the minimum of `p3 - p1` and `p3 - p2`, and it must satisfy the given condition, let's consider the implications for `p1 - cur + p3`:

- If `cur = p3 - p1`, then `p1 - (p3 - p1) + p3 = p1 - p3 + p1 + p3 = 2p1`.
- If `cur = p3 - p2`, then `p1 - (p3 - p2) + p3 = p1 - p3 + p2 + p3 = p1 + p2`.

Given the condition `p1 + p2 <= p3` from Case 2, the expression `p1 + p2` is valid. However, since `cur` is the minimum difference, and we need to satisfy `p1 - cur + p3`, the expression simplifies to `p1 + p2` when `cur = p3 - p2`.

Thus, the expression `p1 - cur + p3` simplifies to `p1 + p2` under the given conditions.

Output: **p1 + p2**