Let's break down the initial state and the print statement step by step:

1. **Initial State:**
   - `t` must be greater than 0.
   - `n` must be greater than or equal to 2.
   - `sum` is defined as \(1 + \sum_{k=2}^{n} (k^2 - (k-1)^2) \cdot k\).
   - `i` is \(n + 1\).
   - `j` is \(\text{previous\_n}\).

2. **Understanding the `sum` formula:**
   - The formula for `sum` is \(1 + \sum_{k=2}^{n} (k^2 - (k-1)^2) \cdot k\).
   - Simplify the term inside the summation: \(k^2 - (k-1)^2 = k^2 - (k^2 - 2k + 1) = 2k - 1\).
   - Therefore, the formula becomes: \(1 + \sum_{k=2}^{n} (2k - 1) \cdot k\).
   - Further simplifying: \(1 + \sum_{k=2}^{n} (2k^2 - k)\).
   - This can be split into two separate sums: \(1 + 2 \sum_{k=2}^{n} k^2 - \sum_{k=2}^{n} k\).

3. **Summation calculations:**
   - The sum of squares from 2 to n: \(\sum_{k=2}^{n} k^2 = \sum_{k=1}^{n} k^2 - 1^2 = \frac{n(n+1)(2n+1)}{6} - 1\).
   - The sum of integers from 2 to n: \(\sum_{k=2}^{n} k = \sum_{k=1}^{n} k - 1 = \frac{n(n+1)}{2} - 1\).

4. **Substitute the summation results:**
   - \(1 + 2 \left( \frac{n(n+1)(2n+1)}{6} - 1 \right) - \left( \frac{n(n+1)}{2} - 1 \right)\).
   - Simplify inside the parentheses: \(1 + 2 \left( \frac{n(n+1)(2n+1) - 6}{6} \right) - \left( \frac{n(n+1) - 2}{2} \right)\).
   - Further simplification: \(1 + \frac{n(n+1)(2n+1) - 6}{3} - \frac{n(n+1) - 2}{2}\).
   - Combine the fractions: \(1 + \frac{2(n(n+1)(2n+1) - 6) - 3(n(n+1) - 2)}{6}\).
   - Simplify the numerator: \(1 + \frac{2n(n+1)(2n+1) - 12 - 3n(n+1) + 6}{6}\).
   - Combine like terms: \(1 + \frac{2n(n+1)(2n+1) - 3n(n+1) - 6}{6}\).
   - Factor out \(n(n+1)\): \(1 + \frac{n(n+1)(4n + 2 - 3) - 6}{6}\).
   - Simplify inside the parentheses: \(1 + \frac{n(n+1)(4n - 1) - 6}{6}\).
   - Simplify the entire expression: \(1 + \frac{n(n+1)(4n - 1) - 6}{6}\).

5. **Final expression for `sum`:**
   - \(1 + \frac{n(n+1)(4n - 1) - 6}{6}\).

6. **Print statement:**
   - `print(sum, n + n)` will print the value of `sum` and the value of `n + n`.

7. **Output:**
   - The value of `sum` is \(1 + \frac{n(n+1)(4n - 1) - 6}{6}\).
   - The value of `n + n` is \(2n\).

Output: **1 + \(\frac{n(n+1)(4n - 1) - 6}{6}\), 2n (where n is the value of n)**