The code snippet provided increments the value of `end` by 1. All other variables remain unchanged.

Given the initial state:
- `t` is an integer such that \(1 \leq t \leq 10^4\)
- `n` is an integer such that `n <= le`
- `a` is a list of integers derived from the input
- `le` is the length of the list `a`
- `l` is `n - 1`
- `r` is `n - 1`
- `st` is `n`
- `end` is `1`
- `a[n]` equals `a[n - 1]`
- If `a[0] == a[-1]`, then `ans` is `max(0, le - (st + end))`
- Otherwise, `ans` is `le - max(st, end)`

After executing `end += 1`, the value of `end` changes from `1` to `2`.

Output State: **`t` is an integer such that \(1 \leq t \leq 10^4\); `n` is an integer such that `n <= le`; `a` is a list of integers derived from the input; `le` is the length of the list `a`; `l` is `n - 1`; `r` is `n - 1`; `st` is `n`; `end` is `2`; `a[n]` equals `a[n - 1]`; if `a[0] == a[-1]`, then `ans` is `max(0, le - (st + end))`; otherwise, `ans` is `le - max(st, end)`**