The code snippet `end += 1` increments the value of the variable `end` by 1. The initial value of `end` is given as `2`. Therefore, after the execution of the code, the value of `end` becomes `3`.

All other variables remain unchanged as per the given initial state.

Output State: **`t` is an integer such that \(1 \leq t \leq 10^4\); `n` is the length of the list `a`; `a` is the list of integers where `a[n - 1] == a[n - 2]`; `le` is the length of the list `a`; `l` is `n - 3`; `r` is `n - 3`; `st` is `n - 1`; `end` is `3`; `ans` is `0` if `a[0]` is equal to `a[-1]`, otherwise `ans` is `1`.**