Let's break down the problem step by step:

1. **Initial Values:**
   - `m = 16`
   - `_ = 2`
   - `n = 0`
   - `k > 1`
   - `s = 0`

2. **Loop Execution:**
   - The loop continues as long as `s < k`.
   - In each iteration, `m` doubles (`m *= 2`).
   - `n` is halved (`n //= 2`).
   - `s` increases by the value of `n` (`s += n`).

3. **First Iteration:**
   - `m` becomes `16 * 2 = 32`
   - `n` becomes `0 // 2 = 0`
   - `s` remains `0` because `n` is `0`.

4. **Second Iteration:**
   - `m` becomes `32 * 2 = 64`
   - `n` becomes `0 // 2 = 0`
   - `s` remains `0` because `n` is `0`.

5. **Third Iteration:**
   - `m` becomes `64 * 2 = 128`
   - `n` becomes `0 // 2 = 0`
   - `s` remains `0` because `n` is `0`.

6. **Subsequent Iterations:**
   - Since `n` is `0` and `s` remains `0`, the loop will continue to run, but `s` will never become greater than `k` (since `k > 1` and `s` is always `0`).

7. **Final Values Before Print Statement:**
   - `m = 128`
   - `n = 0`
   - `s = 0`
   - `k > 1`

8. **Print Statement:**
   - The expression inside the print statement is `(2 * (k - (s - n)) - 1) * m`.
   - Substituting the known values:
     - `s - n = 0 - 0 = 0`
     - `k - (s - n) = k - 0 = k`
     - `2 * (k - (s - n)) - 1 = 2 * k - 1`
     - `(2 * k - 1) * m = (2 * k - 1) * 128`

Since `k > 1`, let's assume the smallest possible value for `k` which is `2` (as `k` must be greater than `1`):

- If `k = 2`, then `2 * k - 1 = 2 * 2 - 1 = 3`.
- Therefore, `(2 * k - 1) * m = 3 * 128 = 384`.

Given this reasoning, the output will be:

Output: **384**