Correctness: **False**

The program does not correctly handle the case when `k` is equal to `n * m - 1`. In this case, Lara should end up in cell `(1, 2)`, but the program calculates the row and column incorrectly.

To see why, let's analyze the program's logic. When `k >= n - 1`, the program subtracts `n - 1` from `k` and then calculates the number of full rows and remaining steps. However, when `k` is equal to `n * m - 1`, the program calculates `k -= n - 1` as `k = n * m - n`, and then `full_rows = (n * m - n) // (m - 1)` and `remaining_steps = (n * m - n) % (m - 1)`.

Since `n` is even and `m` is at least 2, `n * m - n` is always a multiple of `m - 1`, so `remaining_steps` is always 0. As a result, when `full_rows % 2 == 0`, the program calculates `row = n - full_rows` as `row = 1` and `col = 2 + remaining_steps` as `col = 2`, which is correct. However, when `full_rows % 2 == 1`, the program calculates `row = n - full_rows` as `row = 1` and `col = m - remaining_steps` as `col = m`, which is incorrect because Lara should end up in cell `(1, 2)`, not `(1, m)`.

To fix this bug, the program should handle the case when `k` is equal to `n * m - 1` separately. Here's an example of how to do it:
```python
import sys

input = sys.stdin.read
data = input().strip().split()
(n, m, k) = (int(data[0]), int(data[1]), int(data[2]))

def func_1(n, m, k):
    if k == n * m - 1:
        print(1, 2)
    elif k < n - 1:
        print(k + 1, 1)
    else:
        k -= n - 1
        full_rows = k // (m - 1)
        remaining_steps = k % (m - 1)
        if full_rows % 2 == 0:
            row = n - full_rows
            col = 2 + remaining_steps
        else:
            row = n - full_rows
            col = m - remaining_steps
        print(row, col)

func_1(n, m, k)
```