The code `ans += l - pos` impacts the value of `ans`. The previous value of `ans` is 0, and since it is stated that `pos` is less than `l`, the expression `l - pos` yields a positive value. The exact outcome for `ans` is determined by the difference between `l` and `pos`. 

Thus, if `l` is any integer greater than `pos`, then `ans` becomes `l - pos`, which is a positive integer. The states of the other variables (`n`, `pos`, `l`, `r`) remain unchanged.

Output State: **`n` is an integer such that 1 ≤ n ≤ 100, `pos` is an integer such that 1 ≤ pos < l ≤ n, `l` is an integer such that 1 ≤ l ≤ r ≤ n, `r` is an integer such that 1 ≤ l ≤ r ≤ n; `ans` is equal to `l - pos`.**