The variable `dx` is assigned the value of `x - final_x`. The value of `final_x` is already defined as `x + (count_R - count_L)`, so substituting this in gives us:

```
dx = x - (x + (count_R - count_L))
dx = x - x - (count_R - count_L)
dx = - (count_R - count_L)
```

The states of the other variables remain unchanged. Therefore, the Output State is: `final_x` is equal to `x + (count_R - count_L)`, `final_y` is equal to `y + (count_U - count_D)`, `operations` is a string of length `n`, `x` is an integer in the range -10^9 <= `x` <= 10^9, `y` is an integer in the range -10^9 <= `y` <= 10^9, and `dx` is equal to `-(count_R - count_L)`.

Output State: **`final_x` is equal to `x + (count_R - count_L)`, `final_y` is equal to `y + (count_U - count_D)`, `operations` is a string of length `n`, `x` is an integer in the range -10^9 <= `x` <= 10^9, `y` is an integer in the range -10^9 <= `y` <= 10^9, `dx` is equal to `-(count_R - count_L)`**.