To determine the final output state after all iterations of the loop are complete, we need to understand the behavior of the loop and how the variables `cnt`, `x`, and `y` evolve with each iteration.

The loop runs for `i` from 1 to `m-1` (since the range is `range(1, m)`). For each iteration:
- `x` is calculated as `n - (i * i - i)`.
- `y` is calculated as `i * i`.
- `cnt` is updated by adding `x // y + (i > 1)` to it.

Let's break down the logic:
- `x // y` computes the integer division of `x` by `y`.
- `(i > 1)` evaluates to 1 if `i` is greater than 1, and 0 if `i` is 1.

For `i = 1`:
- `x = n - (1 * 1 - 1) = n`
- `y = 1 * 1 = 1`
- `cnt = cnt + (n // 1) + (1 > 1) = cnt + n + 0 = cnt + n`

For `i = 2`:
- `x = n - (2 * 2 - 2) = n - 2`
- `y = 2 * 2 = 4`
- `cnt = cnt + ((n - 2) // 4) + (2 > 1) = cnt + (n - 2) // 4 + 1`

For `i = 3`:
- `x = n - (3 * 3 - 3) = n - 6`
- `y = 3 * 3 = 9`
- `cnt = cnt + ((n - 6) // 9) + (3 > 1) = cnt + (n - 6) // 9 + 1`

Following this pattern, the loop will continue until `i` reaches `m-1`.

The final state of `cnt` after all iterations can be described by summing up the contributions from each iteration:

\[ \text{cnt} = n + \sum_{i=2}^{m-1} \left( \left\lfloor \frac{n - (i^2 - i)}{i^2} \right\rfloor + 1 \right) \]

This sum can be simplified as:

\[ \text{cnt} = n + \sum_{i=2}^{m-1} \left\lfloor \frac{n - i(i-1)}{i^2} \right\rfloor + (m-2) \]

In simpler terms, `cnt` will be the initial `n` plus the sum of integer divisions for each `i` from 2 to `m-1`, plus `m-2` to account for the `(i > 1)` term.

Given the initial state and the loop behavior, the final output state is:

Output State: **`cnt` is `n + sum((n - i*(i-1)) // (i*i) for i in range(2, m)) + (m - 2)`**

In natural language: The final value of `cnt` is the initial value of `n` plus the sum of integer divisions of `(n - i*(i-1))` by `i*i` for `i` from 2 to `m-1`, plus `m-2`. The values of `n` and `m` remain the same, and `i` is no longer in the scope after the loop ends.