Let's break down the given initial state and the print statement step by step:

1. **Initial State:**
   - `t` is an integer such that \(1 \leq t \leq 500\).
   - `n` is an input integer such that \(1 \leq n \leq 500\).
   - `mat` is a list of `n` lists, each containing integers from 1 to `n` inclusive.
   - `res` is the sum of \((i + 1) \times (2 \times i + 1)\) for \(i\) from 0 to \(n-1\).
   - `i` is \(n-1\).

2. **Understanding the Variables:**
   - `n` is an integer between 1 and 500.
   - `res` is calculated as the sum of \((i + 1) \times (2 \times i + 1)\) for \(i\) from 0 to \(n-1\).
   - `n << 1` is a bitwise left shift operation, which is equivalent to multiplying `n` by 2.

3. **Calculating `res`:**
   - The formula for `res` is \(\sum_{i=0}^{n-1} (i + 1) \times (2 \times i + 1)\).
   - Let's expand this formula:
     \[
     \sum_{i=0}^{n-1} (i + 1) \times (2 \times i + 1) = \sum_{i=0}^{n-1} (2i^2 + 3i + 1)
     \]
   - This can be simplified to:
     \[
     \sum_{i=0}^{n-1} 2i^2 + \sum_{i=0}^{n-1} 3i + \sum_{i=0}^{n-1} 1
     \]
   - The sums can be calculated as:
     \[
     \sum_{i=0}^{n-1} 2i^2 = 2 \sum_{i=0}^{n-1} i^2 = 2 \left( \frac{(n-1)n(2n-1)}{6} \right)
     \]
     \[
     \sum_{i=0}^{n-1} 3i = 3 \sum_{i=0}^{n-1} i = 3 \left( \frac{(n-1)n}{2} \right)
     \]
     \[
     \sum_{i=0}^{n-1} 1 = n
     \]
   - Combining these, we get:
     \[
     res = 2 \left( \frac{(n-1)n(2n-1)}{6} \right) + 3 \left( \frac{(n-1)n}{2} \right) + n
     \]

4. **Calculating `n << 1`:**
   - `n << 1` is equivalent to \(2 \times n\).

5. **Final Output:**
   - The print statement will output the value of `res` and the value of `n << 1`.

Output: **res, 2 * n (where res is the sum of (i + 1) * (2 * i + 1) for i from 0 to n-1, and n is an integer between 1 and 500)**