To determine what will be printed by the `print(ans)` statement, let's break down the initial state and the expression for `ans` step by step:

1. **Initial State:**
   - `n` is an integer.
   - `m` is an integer.
   - `b` is defined as `min(n, m) + 1`.
   - `t` is greater than 2 (though this variable is not used in the calculation of `ans`).
   - `T` is 2 (though this variable is not used in the calculation of `ans`).

2. **Expression for `ans`:**
   - `ans` is defined as `n + sum((n + b) // (b * b) for b in range(2, min(n, m) + 1))`.

Let's break down the expression for `ans`:

- **Step 1:** Calculate `min(n, m) + 1` and assign it to `b`.
  - This gives us the upper limit for the range in the sum.

- **Step 2:** Compute the sum part of the expression:
  - The sum is over the range from 2 to `min(n, m) + 1` (inclusive).
  - For each `b` in this range, compute `(n + b) // (b * b)`.

- **Step 3:** Add `n` to the result of the sum.

Let's go through an example to illustrate the calculation:

### Example Calculation:
Suppose `n = 5` and `m = 7`.

1. **Calculate `b`:**
   - `b = min(5, 7) + 1 = 5 + 1 = 6`.

2. **Compute the sum:**
   - The range is from 2 to 6.
   - For each `b` in this range, compute `(n + b) // (b * b)`:
     - For `b = 2`: `(5 + 2) // (2 * 2) = 7 // 4 = 1`
     - For `b = 3`: `(5 + 3) // (3 * 3) = 8 // 9 = 0`
     - For `b = 4`: `(5 + 4) // (4 * 4) = 9 // 16 = 0`
     - For `b = 5`: `(5 + 5) // (5 * 5) = 10 // 25 = 0`
     - For `b = 6`: `(5 + 6) // (6 * 6) = 11 // 36 = 0`

   - Sum of these values: `1 + 0 + 0 + 0 + 0 = 1`.

3. **Compute `ans`:**
   - `ans = n + sum = 5 + 1 = 6`.

### General Case:
For any integers `n` and `m`, the value of `ans` will be:
- `n` plus the sum of `(n + b) // (b * b)` for `b` in the range from 2 to `min(n, m) + 1`.

### Final Output:
Output: **ans (where ans is n + sum((n + b) // (b * b) for b in range(2, min(n, m) + 1)))**