Let's break down the initial state and the code snippet step by step:

1. **Initial State:**
   - `i` is 2.
   - `n_cases` is greater than or equal to \(2^{(n-1)}\).
   - `n` is \(\log_2(n_{\text{cases}})\).
   - `power` is \(n - 1\).

2. **Understanding the Variables:**
   - `n_cases` is a number such that \(n_{\text{cases}} \geq 2^{(n-1)}\).
   - `n` is the base-2 logarithm of `n_cases`, i.e., \(n = \log_2(n_{\text{cases}})\).
   - `power` is \(n - 1\).

3. **Calculating `power`:**
   - Since \(n = \log_2(n_{\text{cases}})\), we have \(2^n = n_{\text{cases}}\).
   - Therefore, \(power = n - 1 = \log_2(n_{\text{cases}}) - 1\).

4. **Evaluating the Print Statement:**
   - The print statement is `print(2 ** power)`.
   - Substituting `power` with \(\log_2(n_{\text{cases}}) - 1\), we get:
     \[
     2 ** (\log_2(n_{\text{cases}}) - 1)
     \]
   - Using the property of exponents and logarithms, \(2^{\log_2(x)} = x\), we can simplify:
     \[
     2 ** (\log_2(n_{\text{cases}}) - 1) = 2^{\log_2(n_{\text{cases}})} / 2^1 = n_{\text{cases}} / 2
     \]

Therefore, the print statement will output \(n_{\text{cases}} / 2\).

Output: **n_cases / 2 (where n_cases is the value of n_cases)**