`b` is assigned the value `n - x`. According to the initial state, `n` is the first element of `L`, and `x` is the second element of `L`. So, `b` is calculated as the subtraction of `x` from `n`. The other variables remain unchanged.

Output State: **`N` is an integer such that \(2 \leq N \leq 10^{12}\); `X` is an integer such that \(1 \leq X \leq N-1\); `L` is a list of integers; `n` is the first element of `L`; `x` is the second element of `L`; `res` is equal to `n`; `a` is the second element of `L` (`x`); `b` is `n - x`.**