Let's break down the initial state and the print statement step by step:

1. **Initial State Description:**
   - `t` is an integer between 0 and 499 inclusive.
   - `p1`, `p2`, `p3` are integers assigned the values from the input split.
   - `low` is the minimum of `p3 - p1` and `p3 - p2`.
   - `high` is the maximum of `p3 - p1` and `p3 - p2`.
   - `cur` is equal to `low`.
   - The condition `(p1 - cur <= p2 - (p3 - cur))` is true.

2. **Understanding the Variables:**
   - Since `cur` is equal to `low`, and `low` is the minimum of `p3 - p1` and `p3 - p2`, `cur` will be one of these two values.
   - Given the condition `(p1 - cur <= p2 - (p3 - cur))` is true, let's analyze this:
     - If `cur = p3 - p1`, then the condition becomes `(p1 - (p3 - p1) <= p2 - (p3 - (p3 - p1)))` which simplifies to `(2*p1 - p3 <= p2 - p1)`.
     - If `cur = p3 - p2`, then the condition becomes `(p1 - (p3 - p2) <= p2 - (p3 - (p3 - p2)))` which simplifies to `(p1 - p3 + p2 <= p2 - p3 + p2)` or `(p1 - p3 + p2 <= p2 - p3 + p2)` which simplifies to `(p1 - p3 + p2 <= p2 - p3 + p2)` which further simplifies to `(p1 - p3 + p2 <= p2 - p3 + p2)`.

3. **Simplifying the Condition:**
   - For both cases, the condition simplifies to checking if `p1 - cur` is less than or equal to `p2 - (p3 - cur)`. Given the nature of the problem, it suggests that `cur` is chosen such that the condition holds true.

4. **Print Statement Analysis:**
   - The print statement is `print(p1 - cur + p3)`.
   - Since `cur` is either `p3 - p1` or `p3 - p2`, let's consider both cases:
     - If `cur = p3 - p1`, then `p1 - cur + p3 = p1 - (p3 - p1) + p3 = p1 - p3 + p1 + p3 = 2*p1`.
     - If `cur = p3 - p2`, then `p1 - cur + p3 = p1 - (p3 - p2) + p3 = p1 - p3 + p2 + p3 = p1 + p2`.

5. **Conclusion:**
   - Given the condition `(p1 - cur <= p2 - (p3 - cur))` must hold true, and considering the nature of the problem, the expression `p1 - cur + p3` will evaluate to either `2*p1` or `p1 + p2`.

Since the exact values of `p1` and `p2` are not specified, but the condition ensures that the expression evaluates to one of these forms, we can conclude that the print statement will output either `2*p1` or `p1 + p2`.

Output: **2*p1 or p1 + p2**