Alright, I have this problem to solve. Let's see what it's asking for. So, Nikita has some cubes and he wants to build a tower using these cubes. He can either add one cube on top of the tower or remove one cube from the top in each move. The tower starts with no cubes, and we need to figure out if, after a certain number of moves, the tower can have exactly m cubes.

The input consists of multiple test cases, and for each test case, we're given two integers: n, which is the number of moves, and m, which is the desired number of cubes in the tower at the end.

Our task is to determine for each test case whether it's possible to achieve exactly m cubes in the tower after n moves, and output "Yes" or "No" accordingly.

First, I need to understand the operations Nikita can perform:

1. Add one cube to the top of the tower.

2. Remove one cube from the top of the tower.

He can choose either operation in each move, and the sequence of operations matters because he can't remove a cube if the tower is empty.

So, I need to model the sequence of these operations to see if it's possible to end up with exactly m cubes after n moves.

Let me think about this.

Let's consider that each move can either increment or decrement the number of cubes in the tower, but with the constraint that he can't remove a cube if there are none.

This seems like a problem that can be modeled using simple arithmetic, perhaps by considering the number of addition and subtraction operations.

Let's denote:

- x: the number of times he adds a cube.

- y: the number of times he removes a cube.

Then, we have:

- x + y = n (total moves)

- m = initial cubes (which is 0) + x - y

But, we need to make sure that at no point does y exceed the number of cubes in the tower, because he can't remove a cube that isn't there.

So, m = x - y, and x + y = n.

From these, we can solve for x and y.

Let me solve these equations.

From x + y = n,

And m = x - y,

We can add these two equations:

(x + y) + (x - y) = n + m => 2x = n + m => x = (n + m)/2

Similarly, subtract the second equation from the first:

(x + y) - (x - y) = n - m => 2y = n - m => y = (n - m)/2

So, x = (n + m)/2

y = (n - m)/2

Now, for x and y to be valid, they must be non-negative integers because you can't have a fraction of a move, and you can't have negative moves.

Additionally, we need to ensure that at no point does y exceed the number of cubes in the tower.

Given that, let's see what conditions must hold for x and y.

First, x and y must be integers, so (n + m)/2 and (n - m)/2 must be integers. This implies that n + m and n - m must be even, meaning that n and m must be either both even or both odd.

Second, x and y must be non-negative, so:

x = (n + m)/2 >= 0

y = (n - m)/2 >= 0

Since m >= 0 and n >= m (because y cannot be negative), we have that n >= m.

Also, the sequence of moves must be such that at no point does y exceed the number of cubes in the tower.

This is a bit tricky. We need to ensure that in the sequence of x additions and y removals, the tower never goes negative.

This sounds similar to problems involving balancing parentheses or maintaining a non-negative sum in a sequence.

I think that if x >= y, then it's always possible to arrange the sequence so that the tower never goes negative.

Wait, but that might not always be the case. Let me think of an example.

Suppose n = 3, m = 2.

Then, x = (3 + 2)/2 = 2.5, which is not an integer, so it's invalid. So, in this case, it's impossible.

Another example: n = 3, m = 1.

x = (3 + 1)/2 = 2

y = (3 - 1)/2 = 1

So, x = 2, y = 1.

We need to arrange the sequence of moves: add, add, remove.

This would result in tower heights: 1, 2, 1.

Which ends with m = 1.

So, it's possible.

Another example: n = 2, m = 4.

x = (2 + 4)/2 = 3

y = (2 - 4)/2 = -1

This is invalid because y is negative, so it's impossible.

Another example: n = 5, m = 3.

x = (5 + 3)/2 = 4

y = (5 - 3)/2 = 1

So, x = 4, y = 1.

We need to arrange the sequence: add, add, add, add, remove.

Tower heights: 1, 2, 3, 4, 3.

Which ends with m = 3.

So, it's possible.

Wait, but is there a way where n < m?

Let's see.

If n < m, then y would be negative, which is invalid.

So, n must be >= m.

Also, since x = (n + m)/2, and y = (n - m)/2, both must be integers.

So, the conditions are:

1. n >= m

2. (n + m) is even

3. (n - m) is even

Actually, since (n + m) and (n - m) are both even only if n and m are both even or both odd.

So, another way to say it is that n and m must have the same parity (both even or both odd).

And n >= m.

So, in the code, we need to check if n >= m and n and m have the same parity.

If both conditions are satisfied, then it's possible; otherwise, it's not.

Let me verify this.

Take n = 3, m = 3.

x = (3 + 3)/2 = 3

y = (3 - 3)/2 = 0

So, x = 3, y = 0.

Sequence: add, add, add.

Tower heights: 1, 2, 3.

Which is valid.

n = 4, m = 2.

x = (4 + 2)/2 = 3

y = (4 - 2)/2 = 1

Sequence: add, add, add, remove.

Tower heights: 1, 2, 3, 2.

Valid.

n = 4, m = 4.

x = (4 + 4)/2 = 4

y = (4 - 4)/2 = 0

Sequence: add, add, add, add.

Tower heights: 1, 2, 3, 4.

Valid.

n = 4, m = 0.

x = (4 + 0)/2 = 2

y = (4 - 0)/2 = 2

Sequence: add, remove, add, remove.

Tower heights: 1, 0, 1, 0.

Valid.

n = 4, m = 1.

x = (4 + 1)/2 = 2.5

Invalid.

So, it's impossible.

n = 5, m = 1.

x = (5 + 1)/2 = 3

y = (5 - 1)/2 = 2

Sequence: add, add, add, remove, remove.

Tower heights: 1, 2, 3, 2, 1.

Valid.

n = 5, m = 3.

x = (5 + 3)/2 = 4

y = (5 - 3)/2 = 1

Sequence: add, add, add, add, remove.

Tower heights: 1, 2, 3, 4, 3.

Valid.

n = 5, m = 5.

x = (5 + 5)/2 = 5

y = (5 - 5)/2 = 0

Sequence: add, add, add, add, add.

Tower heights: 1, 2, 3, 4, 5.

Valid.

n = 5, m = 2.

x = (5 + 2)/2 = 3.5

Invalid.

So, seems consistent.

Hence, the conditions are:

- n >= m

- n and m have the same parity (both even or both odd)

If these two conditions are met, then it's possible; otherwise, it's not.

Now, looking at the provided program:

def func():

a = int(input())

for i in range(a):

(b, c) = map(int, input().split())

q = (b, c)

if b == c:

print('YES')

elif b < c:

print('NO')

elif a % 2 == b % 2:

print('Yes')

else:

print('No')

Hmm, there are a few issues here.

First, the variable names are b and c instead of n and m, but that's just naming.

More importantly, the conditions in the if statements don't seem to correctly implement the logic we derived.

Let's go through the code step by step.

1. Read the number of test cases, a.

2. For each test case:

- Read b and c (which are n and m).

- Store them in tuple q.

- If b == c, print 'YES'.

- Else if b < c, print 'NO'.

- Else if a % 2 == b % 2, print 'Yes'.

- Else, print 'No'.

Problems I see:

- The condition 'if b == c' is handled separately, but according to our logic, we need to check if b >= c and if b and c have the same parity.

- The condition 'elif b < c' is correct in that if b < c, it's impossible, so 'NO' should be printed.

- The next condition 'elif a % 2 == b % 2' doesn't make sense because a is the number of test cases, not related to the current test case's n and m.

- It should be checking if b and c have the same parity, i.e., b % 2 == c % 2.

- Also, the spelling of 'Yes' and 'No' is inconsistent; sometimes all caps, sometimes not.

- Additionally, the problem allows for any case in the output, but it's better to be consistent.

So, the correct implementation should be:

For each test case:

- Read n and m.

- If n < m:

- Print 'No'

- Else if n >= m and n and m have the same parity:

- Print 'Yes'

- Else:

- Print 'No'

Or, more concisely:

- If n >= m and n % 2 == m % 2:

- Print 'Yes'

- Else:

- Print 'No'

We can handle the case when n == m separately, but it's already covered in the general condition.

Let me check the sample input and output to verify.

Sample Input:

3

3 3

2 4

5 3

Sample Output:

Yes

No

Yes

According to our logic:

First test case: n=3, m=3

n >= m and both odd, same parity -> Yes

Second test case: n=2, m=4

n < m -> No

Third test case: n=5, m=3

n >= m and both odd, same parity -> Yes

Which matches the sample output.

Another test case:

n=4, m=2

n >= m and both even -> Yes

n=4, m=1

n >= m but 4 even, 1 odd -> No

n=1, m=1

n >= m and both odd -> Yes

n=1, m=0

n >= m but 1 odd, 0 even -> No

n=2, m=0

n >= m and both even -> Yes

Seems consistent.

Therefore, the correct implementation should be:

For each test case:

- Read n and m.

- If n >= m and n % 2 == m % 2:

- Print 'Yes'

- Else:

- Print 'No'

Now, looking back at the provided code:

def func():

a = int(input())

for i in range(a):

(b, c) = map(int, input().split())

q = (b, c)

if b == c:

print('YES')

elif b < c:

print('NO')

elif a % 2 == b % 2:

print('Yes')

else:

print('No')

Issues:

1. The variable 'a' is the number of test cases, but in the condition 'elif a % 2 == b % 2:', it's comparing the number of test cases' parity with b's parity, which is incorrect. It should be comparing b and c's parity.

2. The output sometimes uses 'YES' and 'Yes', which is inconsistent.

3. The condition 'if b == c:' is redundant because it's already covered in the general condition.

A corrected version would be:

def func():

t = int(input())

for _ in range(t):

n, m = map(int, input().split())

if n >= m and n % 2 == m % 2:

print('Yes')

else:

print('No')

This is simpler and correctly implements the logic.

Therefore, the given program is incorrect due to the reasons mentioned.

**Final Answer**

\[\boxed{\text{False}}\]

