Let's break down the initial state and the calculation step-by-step:

1. **Initial Values:**
   - `i` is set to `k-1`.
   - `k` is greater than `k-1`, but since `k` does not change within the loop, this condition is always true.
   - `t` is calculated as \(2^{k-1} \mod \text{MOD}\).
   - `ans` is the cumulative sum of terms \(t\) from \(2^0 \mod \text{MOD}\) to \(2^{k-1} \mod \text{MOD}\) modulo `MOD`.

2. **Loop Execution:**
   - The loop starts with \(t = 2^0 \mod \text{MOD}\).
   - In each iteration, `t` doubles, i.e., \(t = t \times 2 \mod \text{MOD}\).
   - This continues until `i` reaches `k-1`.

3. **Value of `t`:**
   - Initially, \(t = 2^0 \mod \text{MOD} = 1\).
   - After the first iteration, \(t = 2^1 \mod \text{MOD} = 2\).
   - After the second iteration, \(t = 2^2 \mod \text{MOD} = 4\).
   - And so on, until \(t = 2^{k-1} \mod \text{MOD}\).

4. **Cumulative Sum Calculation:**
   - The sum of \(t\) values from \(2^0 \mod \text{MOD}\) to \(2^{k-1} \mod \text{MOD}\) is:
     \[
     \text{ans} = (1 + 2 + 4 + \ldots + 2^{k-1}) \mod \text{MOD}
     \]
   - This is a geometric series with the sum:
     \[
     \text{ans} = (2^k - 1) \mod \text{MOD}
     \]

Given the above, the final value of `ans` is \((2^k - 1) \mod \text{MOD}\).

Output: **(2^k - 1) % MOD**