Reasoning:
The provided program attempts to solve the problem by iterating over the test cases and for each test case, it calculates \( y \) as \( x - 1 \). It then prints \( y \).

Let's analyze the logic:
1. The problem requires finding an integer \( y \) such that \( 1 \leq y < x \) and the expression \( \gcd(x, y) + y \) is maximized.
2. The proposed solution sets \( y = x - 1 \).
3. Let's check the value of \( \gcd(x, y) + y \) when \( y = x - 1 \):
   \[
   \gcd(x, x-1) + (x-1)
   \]
   Since \( x \) and \( x-1 \) are consecutive integers, their greatest common divisor is always 1 (\(\gcd(x, x-1) = 1\)). Therefore:
   \[
   \gcd(x, x-1) + (x-1) = 1 + (x-1) = x
   \]
4. This value \( x \) is indeed the maximum possible value for \( \gcd(x, y) + y \) because for any other \( y \) in the range \( 1 \leq y < x \), \( \gcd(x, y) \leq y \), and thus \( \gcd(x, y) + y \leq y + y = 2y < x \).

Since the logic correctly identifies the maximum value for \( \gcd(x, y) + y \) by setting \( y = x - 1 \), the program is correct.

Correctness: **True**