Let's break down the initial state and the print statement step by step:

1. **Initial State Analysis:**
   - `i` is `i + 1` if `i` was not 0. This means `i` is now 1 (assuming `i` was 0 initially).
   - `n` must be greater than 0. Let's assume `n = 5` for this example.
   - `r` is decreased by 1. If `r` was initially 3, then `r` is now 2.
   - `a` is either \( B[r - 1] + (idx_B[r - 1] - i) \times r \) or \( B[r - 1] + (idx_B[r - 1] - i) \times r - (idx_A[l - 1] - idx_A[l - r - 1]) \times (l - r) \). Since no specific values for `B`, `idx_B`, `A`, `idx_A`, `l` are given, let's assume some values for simplicity:
     - Assume `B = [10, 20, 30]`, `idx_B = [1, 2, 3]`, `A = [5, 10, 15, 20]`, `idx_A = [1, 3, 5, 7]`, and `l = 4`.
     - For `r = 2`, `B[r - 1] = B[1] = 20`, `idx_B[r - 1] = idx_B[1] = 2`, and `i = 1`.
     - Therefore, `a` becomes \( 20 + (2 - 1) \times 2 = 20 + 2 = 22 \).

2. **Calculation of `b`:**
   - `b` is \( A[l - 1] - A[l - r - 1] - (idx_A[l - 1] - idx_A[l - r - 1]) \times (l - r) + (i - idx_A[l - 1]) \times r \).
   - For `r = 2`, `l = 4`, `A[l - 1] = A[3] = 20`, `A[l - r - 1] = A[1] = 10`, `idx_A[l - 1] = idx_A[3] = 7`, `idx_A[l - r - 1] = idx_A[1] = 3`, and `i = 1`.
   - Therefore, `b` becomes \( 20 - 10 - (7 - 3) \times (4 - 2) + (1 - 7) \times 2 = 20 - 10 - 4 \times 2 - 6 \times 2 = 20 - 10 - 8 - 12 = -10 \).

3. **Print Statement Calculation:**
   - The print statement is `print(a * 2 + b * 2 + (n - i), end=' ')`.
   - Substituting the values: `a = 22`, `b = -10`, `n = 5`, and `i = 1`.
   - Therefore, `a * 2 + b * 2 + (n - i) = 22 * 2 + (-10) * 2 + (5 - 1) = 44 - 20 + 4 = 28`.

Output: **28**