The code `x += int(c) * n ** i` impacts the following:
- `x` is updated by adding `int(c) * n ** i` to its current value.
- `c` is the first character of the reversed string `k`, so `int(c)` converts this character (which is a digit since `k` is a non-empty string) to an integer.
- `i` is 0, so `n ** i` is `n ** 0`, which equals 1.

Therefore, the expression simplifies to `x += int(c) * 1`, or simply `x += int(c)`.

Given the initial state where `n` is an integer such that \(2 \leq n \leq 10^9\), `k` is a non-empty string, `x` is 0, `i` is 0, and `c` is the first character of the reversed string `k`, after executing the code, `x` will be updated by the integer value of the first character of the reversed string `k`.

Output State: **`n` is an integer such that \(2 \leq n \leq 10^9\), `k` is a non-empty string, `x` is int(c), `i` is 0, and `c` is the first character of the reversed string `k`.**