`sum_k` is assigned the value of `k * (k + 1) // 2`. Given that `k` is `a + b - 1`, and substituting this into the equation, we get `sum_k = (a + b - 1) * (a + b) // 2`. The values of the other variables remain unchanged.

Output State: **`m` is a non-negative integer such that \(1 \leq m \leq 10^9\), `a` is a positive integer such that \(1 \leq a \leq 10^5\), `b` is a positive integer such that \(1 \leq b \leq 10^5\), `g` is 1, `k` is a positive integer equal to `a + b - 1`, `sum_k` is `(a + b - 1) * (a + b) // 2`.**