`sum_m` is assigned the value of `m * (m + 1) // 2 - k * (k - 1) // 2`. Given the initial state, we know:

- `m` is a non-negative integer such that \(1 \leq m \leq 10^9\)
- `a` is a positive integer such that \(1 \leq a \leq 10^5\)
- `b` is a positive integer such that \(1 \leq b \leq 10^5\)
- `g` is 1
- `k` is a positive integer equal to `a + b - 1`
- `sum_k` is \((a + b - 1) * (a + b) // 2\)

First, let's express `k` in terms of `a` and `b`:
\[ k = a + b - 1 \]

Next, substitute `k` into the expression for `sum_m`:
\[ sum_m = m * (m + 1) // 2 - (a + b - 1) * (a + b - 2) // 2 \]

Therefore, the Output State is:
Output State: **`m` is a non-negative integer such that \(1 \leq m \leq 10^9\); `a` is a positive integer such that \(1 \leq a \leq 10^5\); `b` is a positive integer such that \(1 \leq b \leq 10^5\); `g` is 1; `k` is a positive integer equal to `a + b - 1`; `sum_k` is \((a + b - 1) * (a + b) // 2; `sum_m` is `m * (m + 1) // 2 - (a + b - 1) * (a + b - 2) // 2**.