Let's analyze the loop to determine the final state of the variable `cnt`.

The loop iterates from `i = 1` to `i = m-1`. For each iteration `i`, the following operations are performed:

1. `x = n - (i * i - i)`
2. `y = i * i`
3. `cnt = cnt + x // y + (i > 1)`

Let's break down the expressions inside the loop:

- `x = n - i * i + i` simplifies to `x = n + i - i * i`.
- `y = i * i` is simply the square of `i`.
- `x // y` is the integer division of `x` by `y`.
- `(i > 1)` evaluates to 1 if `i` is greater than 1, and 0 otherwise.

Now, let's consider the value of `x // y`:

- For `i = 1`, `x = n + 1 - 1 = n` and `y = 1`. So, `x // y = n // 1 = n`.
- For `i > 1`, `x = n + i - i * i` and `y = i * i`. So, `x // y = (n + i - i * i) // (i * i)`. This expression will be less than or equal to `n // (i * i)` because `i - i * i` is negative for `i > 1`.

The loop increments `cnt` by `x // y + (i > 1)` for each iteration.

Let's summarize the contributions to `cnt`:

- For `i = 1`, `cnt` is incremented by `n + 0 = n`.
- For `i > 1`, `cnt` is incremented by `(n + i - i * i) // (i * i) + 1`.

The final value of `cnt` can be written as the sum of these increments:

\[ \text{cnt} = n + \sum_{i=2}^{m-1} \left( \frac{n + i - i^2}{i^2} + 1 \right) \]

This can be simplified to:

\[ \text{cnt} = n + \sum_{i=2}^{m-1} \left( \frac{n}{i^2} + \frac{i - i^2}{i^2} + 1 \right) \]
\[ \text{cnt} = n + \sum_{i=2}^{m-1} \left( \frac{n}{i^2} + \frac{1}{i} - 1 + 1 \right) \]
\[ \text{cnt} = n + \sum_{i=2}^{m-1} \left( \frac{n}{i^2} + \frac{1}{i} \right) \]
\[ \text{cnt} = n + \sum_{i=2}^{m-1} \frac{n}{i^2} + \sum_{i=2}^{m-1} \frac{1}{i} \]

The final expression for `cnt` involves summing up the terms for each `i` from 2 to `m-1`.

Output State: **cnt is the sum of n and the series \(\sum_{i=2}^{m-1} \left( \frac{n}{i^2} + \frac{1}{i} \right)\).**