To determine what will be printed, let's break down the problem step-by-step based on the given initial state and the Python code snippet.

### Initial State Breakdown:

1. **Variable `u`:**
   - `u` is defined as a non-zero value minus 2. However, `u` is not used in the provided code snippet, so we can ignore it for this particular print statement.

2. **List `b`:**
   - The list `b` is defined as `[0, 0, y - x, y - x, y - x + v, y - x + v, y - x + v]`.

3. **Variables `c` and `d`:**
   - `c` and `d` are the values returned by the function `r()`.
   - There is a condition that if `c` is less than `d`, then `c` is less than `d`. Otherwise, `c` is greater than or equal to `d`. This condition doesn't change the values of `c` and `d`; it just provides a comparison between them.

### Code Analysis:

The code snippet provided is:
```python
print(b[(d - 1) * 2] - b[(c - 1) * 2])
```

Let's analyze the indices used in the list `b`:

- The index `(d - 1) * 2` will access an element in the list `b` at position `2 * (d - 1)`.
- The index `(c - 1) * 2` will access an element in the list `b` at position `2 * (c - 1)`.

Given the structure of the list `b = [0, 0, y - x, y - x, y - x + v, y - x + v, y - x + v]`, we can see that the even-indexed elements (0, 2, 4, 6) are:
- `b[0] = 0`
- `b[2] = y - x`
- `b[4] = y - x + v`
- `b[6] = y - x + v`

The odd-indexed elements (1, 3, 5) are:
- `b[1] = 0`
- `b[3] = y - x`
- `b[5] = y - x + v`

Since `c` and `d` are returned by `r()` and their relationship is either `c < d` or `c >= d`, the exact values of `c` and `d` are not specified. However, we know they will be integers, and we need to consider the valid indices for the list `b`.

### Possible Values for Indices:

- If `c` and `d` are both 1, the indices would be `(1 - 1) * 2 = 0` and `(1 - 1) * 2 = 0`, resulting in `b[0] - b[0] = 0 - 0 = 0`.
- If `c` is 1 and `d` is 2, the indices would be `(2 - 1) * 2 = 2` and `(1 - 1) * 2 = 0`, resulting in `b[2] - b[0] = (y - x) - 0 = y - x`.
- If `c` is 2 and `d` is 1, the indices would be `(1 - 1) * 2 = 0` and `(2 - 1) * 2 = 2`, resulting in `b[0] - b[2] = 0 - (y - x) = -(y - x)`.
- If `c` and `d` are both 2, the indices would be `(2 - 1) * 2 = 2` and `(2 - 1) * 2 = 2`, resulting in `b[2] - b[2] = (y - x) - (y - x) = 0`.
- If `c` is 1 and `d` is 3, the indices would be `(3 - 1) * 2 = 4` and `(1 - 1) * 2 = 0`, resulting in `b[4] - b[0] = (y - x + v) - 0 = y - x + v`.
- If `c` is 3 and `d` is 1, the indices would be `(1 - 1) * 2 = 0` and `(3 - 1) * 2 = 4`, resulting in `b[0] - b[4] = 0 - (y - x + v) = -(y - x + v)`.
- If `c` and `d` are both 3, the indices would be `(3 - 1) * 2 = 4` and `(3 - 1) * 2 = 4`, resulting in `b[4] - b[4] = (y - x + v) - (y - x + v) = 0`.

### General Case:

Given the above analysis, the printed value depends on the specific values of `c` and `d`. However, the general form of the output can be described as follows:

- If `c` and `d` are such that `(d - 1) * 2` and `(c - 1) * 2` point to the same index, the result will be `0`.
- If `(d - 1) * 2` points to an index with value `y - x` or `y - x + v` and `(c - 1) * 2` points to index `0`, the result will be `y - x` or `y - x + v`.
- If `(c - 1) * 2` points to an index with value `y - x` or `y - x + v` and `(d - 1) * 2` points to index `0`, the result will be `-(y - x)` or `-(y - x + v)`.

### Conclusion:

Based on the general form and the possible values, the output can be described as:

Output: **b[(d - 1) * 2] - b[(c - 1) * 2] (where b is the list [0, 0, y - x, y - x, y - x + v, y - x + v, y - x + v], and c and d are values returned by r())**