To determine the output state after executing the provided Python code, we start with the initial conditions:

- `m` is a positive integer such that \( 1 \leq m \leq 10^9 \)
- `a` is a positive integer such that \( 1 \leq a \leq 100000 \)
- `b` is a positive integer such that \( 1 \leq b \leq 100000 \)
- `g` is equal to 1
- `k` is equal to \( a + b - 1 \)
- \( m \geq k \)
- `sum_k` is equal to \( k \times (k + 1) // 2 \)

Now, we analyze the code:

```
sum_m = m * (m + 1) // 2 - k * (k - 1) // 2
```

This line calculates `sum_m`, which is the sum of the first `m` natural numbers minus the sum of the first `k-1` natural numbers.

Calculating `sum_m`:

1. The expression \( m \times (m + 1) // 2 \) computes the sum of the first `m` numbers.
2. The expression \( k \times (k - 1) // 2 \) computes the sum of the first `k-1` numbers.
3. The difference of these two expressions gives us `sum_m`.

Since `sum_m` is derived from the calculations involving `m` and `k`, we update the output state to reflect the new value of `sum_m`.

The values of `m`, `a`, `b`, `g`, `k`, and `sum_k` remain unchanged after the execution of the code snippet. The only new information is the calculated value of `sum_m`.

Therefore, the output state is:

Output State: **`m` is a positive integer such that 1 <= `m` <= 10^9; `a` is a positive integer such that 1 <= `a` <= 100000; `b` is a positive integer such that 1 <= `b` <= 100000; `g` is equal to 1; `k` is equal to `a + b - 1`; `m` is greater than or equal to `k`; `sum_k` is equal to `k * (k + 1) // 2; `sum_m` is equal to `m * (m + 1) // 2 - k * (k - 1) // 2`.**