The expression `print(n * n - 1) / 2, (n * n + 1) / 2` involves two calculations based on the value of `n`. 

1. The first part calculates `(n * n - 1) / 2`.
2. The second part calculates `(n * n + 1) / 2`.

Since `n` is a positive odd integer larger than 2, we can denote `n` as some odd integer, for example, let's say `n = 3` (the smallest possible value which satisfies the conditions). 

Now, we can calculate:
- For `n = 3`: 
  - `n * n = 3 * 3 = 9`
  - `(n * n - 1) / 2 = (9 - 1) / 2 = 8 / 2 = 4`
  - `(n * n + 1) / 2 = (9 + 1) / 2 = 10 / 2 = 5`

Therefore, the output state based on our calculations is:
Output State: **`n` is an odd integer larger than 2; the results are 4 and 5.**