`f` is assigned the value of `factorial(n - k)`. Given that `k` is 2, we substitute this into the expression, resulting in `f = factorial(n - 2)`. The value of `n` is a positive integer such that 1 ≤ `n` ≤ 50, so `n - 2` will be a non-negative integer as long as `n` is greater than or equal to 2. Therefore, `f` will hold the factorial of `n - 2`. The states of the other variables are not affected. 

Output State: **`n` is a positive integer such that 1 ≤ `n` ≤ 50; `k` is 2; `f` is factorial(n - 2)**