The code snippet modifies the value of `bm` by adding the maximum of `bm` and `a[b] * k + bp` to it. Given that `k` is 0 if the condition `k == 0` is true, we can simplify the expression `a[b] * k + bp` to just `bp` since `a[b] * 0` is 0.

So, `bm` becomes `bm + max(bm, bp)`. Since `bm` is initially `a[b] * (k + 1)`, and `k` is 0, `bm` is initially `a[b]`. Therefore, the expression becomes `bm + max(bm, bp)`, which simplifies to `bm + max(a[b], bp)`.

Thus, the new value of `bm` is `a[b] + max(a[b], bp)`.

Output State: **`t` is a positive integer such that 1 <= t <= 10^4, `i` is 0, `n` is greater than or equal to 1, `k` is 0 if the condition `k == 0` is true, `b` is `p[b] - 1`, `s` is `p[s] - 1`, `a` is a new list of integers obtained from the input, `sp` is `a[s]`, `bp` is `a[b] - 1`, `sm` is `a[s] * (k + 1)`, `bm` is `a[b] + max(a[b], bp)`**