The code snippet `ans += 1` increments the value of `ans` by 1. To determine the final value of `ans`, we need to consider the initial conditions:

- `ans` is calculated based on the condition: If the difference between the second element (`arr[1]`) and the first element (`arr[0]`) in the `arr` list is 2, then `ans` is `x - 1 + 1`. Otherwise, `ans` is `x - 2 + 1`.

Let's break down the calculation of `ans`:

1. If `arr[1] - arr[0] == 2`, then `ans = x - 1 + 1 = x`.
2. If `arr[1] - arr[0] != 2`, then `ans = x - 2 + 1 = x - 1`.

After the code snippet `ans += 1` is executed, the value of `ans` will be incremented by 1:

1. If `arr[1] - arr[0] == 2`, then `ans = x + 1`.
2. If `arr[1] - arr[0] != 2`, then `ans = (x - 1) + 1 = x`.

Therefore, the output state is:

Output State: **`t` is an input integer and must be greater than 0 (decremented by 1) - 1, `n` is the new first integer from the input, `x` is the new second integer from the input and must be greater than or equal to 1, `y` is the new third integer from the input, `arr` is now a sorted list of integers containing the first `x` elements from the original `arr` list plus the element `n + arr[0]`, `i` is 3, `ans` is `x + 1` if the difference between the second element (`arr[1]`) and the first element (`arr[0]`) in the `arr` list is 2, otherwise `ans` is `x`.**