The code `l[i][j] *= b[i] * b[r + j]` multiplies the existing value of `l[i][j]` by `b[i] * b[r + j]`. Given the initial state:

- `j` is 1
- `c` must be at least 1
- `i` is within the range `0 <= i < r - 1`
- `l[i][j]` is `b[i] * b[r + j]` for `j = 1`

For `j = 1`, the value of `l[i][j]` is initially `b[i] * b[r + 1]`. After executing the code, the new value of `l[i][j]` will be `(b[i] * b[r + 1]) * (b[i] * b[r + 1])`.

Therefore, the updated value of `l[i][j]` is `(b[i] * b[r + 1])^2`.

The states of the other variables are not affected.

Output State: **`j` is 1; `c` must be at least 1; `i` is within the range 0 <= i < r - 1; `l[i][j]` is (b[i] * b[r + 1])^2**