Based on the initial state and the given conditions:

- `t` is greater than 1.
- `p1`, `p2`, and `p3` are integers obtained from the input, and their sum is odd.
- `low` is updated to the minimum of `p3 - p1` and `p3 - p2`.
- `high` is updated to the maximum of `p3 - p1` and `p3 - p2`.
- `cur` is set to `low`.
- The current value of `p1 - cur` is less than or equal to the current value of `p2 - (p3 - cur)`.

We need to determine the value of `p1 - cur + p3`.

Given that `cur` is set to `low`, and `low` is the minimum of `p3 - p1` and `p3 - p2`, we have two cases to consider for `cur`:

1. If `p3 - p1` is less than or equal to `p3 - p2`, then `cur = p3 - p1`.
2. If `p3 - p2` is less than `p3 - p1`, then `cur = p3 - p2`.

In both cases, `p1 - cur` simplifies to either `p1 - (p3 - p1)` or `p1 - (p3 - p2)`. Given that `p1 - cur` is less than or equal to `p2 - (p3 - cur)`, let's analyze the expression `p1 - cur + p3`:

- If `cur = p3 - p1`, then `p1 - cur + p3 = p1 - (p3 - p1) + p3 = 2 * p1 - p3 + p3 = 2 * p1`.
- If `cur = p3 - p2`, then `p1 - cur + p3 = p1 - (p3 - p2) + p3 = p1 - p3 + p2 + p3 = p1 + p2`.

Since `p1 - cur` is less than or equal to `p2 - (p3 - cur)`, it implies that `p1 - (p3 - p1) <= p2 - (p3 - p2)`, which simplifies to `2 * p1 - p3 <= p2 - p3 + p3 - p2`, leading to `2 * p1 <= p2`, meaning `p1` is less than or equal to `p2 / 2`.

Therefore, the expression `p1 - cur + p3` will evaluate to `2 * p1` if `cur = p3 - p1` and `p1 - (p3 - p1) <= p2 - (p3 - p2)` holds true, otherwise it will evaluate to `p1 + p2`.

However, without specific values for `p1`, `p2`, and `p3`, we cannot determine which case applies. But we know that the expression will be one of these forms.

Output: **2 * p1 (if p3 - p1 is the minimum) or p1 + p2 (if p3 - p2 is the minimum)**