To determine the new value of `dp[i]` based on the given formula, we need to compute:

\[ dp[i] = (dp[i - 1] + 2 \times (i - 1) \times dp[i - 2]) \% 1000000007 \]

Given:
- `dp[1]` is 1
- `dp[2]` is 3
- `i` is 4

First, let's substitute the known values into the formula:

\[ dp[4] = (dp[3] + 2 \times (4 - 1) \times dp[2]) \% 1000000007 \]

We need to find `dp[3]` first:

\[ dp[3] = (dp[2] + 2 \times (3 - 1) \times dp[1]) \% 1000000007 \]
\[ dp[3] = (3 + 2 \times 2 \times 1) \% 1000000007 \]
\[ dp[3] = (3 + 4) \% 1000000007 \]
\[ dp[3] = 7 \]

Now we can compute `dp[4]`:

\[ dp[4] = (dp[3] + 2 \times (4 - 1) \times dp[2]) \% 1000000007 \]
\[ dp[4] = (7 + 2 \times 3 \times 3) \% 1000000007 \]
\[ dp[4] = (7 + 18) \% 1000000007 \]
\[ dp[4] = 25 \]

Therefore, the updated state is:

Output State: **`t` is an integer such that 1 ≤ t ≤ 10^4, `n` is an integer such that 3 ≤ n ≤ 3 · 10^5, `k` is an integer such that 0 ≤ k ≤ n, `dp[1]` is 1, `dp[2]` is 3, `dp[3]` is 7, `dp[4]` is 25, `i` is 4**