Sure, let's create a comprehensive set of test cases for the given problem. We'll start with basic test cases and then move on to edge cases.

### Basic Test Cases

# Test 1
**Input**: 
```
1
10
```
**Output**: 
```
5
```
**Explanation**: For \( x = 10 \), \( y = 5 \) gives \( \gcd(10, 5) + 5 = 5 + 5 = 10 \).

# Test 2
**Input**: 
```
1
7
```
**Output**: 
```
6
```
**Explanation**: For \( x = 7 \), \( y = 6 \) gives \( \gcd(7, 6) + 6 = 1 + 6 = 7 \).

# Test 3
**Input**: 
```
1
21
```
**Output**: 
```
18
```
**Explanation**: For \( x = 21 \), \( y = 18 \) gives \( \gcd(21, 18) + 18 = 3 + 18 = 21 \).

# Test 4
**Input**: 
```
1
100
```
**Output**: 
```
98
```
**Explanation**: For \( x = 100 \), \( y = 98 \) gives \( \gcd(100, 98) + 98 = 2 + 98 = 100 \).

# Test 5
**Input**: 
```
1
2
```
**Output**: 
```
1
```
**Explanation**: For \( x = 2 \), \( y = 1 \) gives \( \gcd(2, 1) + 1 = 1 + 1 = 2 \).

# Test 6
**Input**: 
```
1
1000
```
**Output**: 
```
750
```
**Explanation**: For \( x = 1000 \), \( y = 750 \) gives \( \gcd(1000, 750) + 750 = 250 + 750 = 1000 \).

# Test 7
**Input**: 
```
1
6
```
**Output**: 
```
3
```
**Explanation**: For \( x = 6 \), \( y = 3 \) gives \( \gcd(6, 3) + 3 = 3 + 3 = 6 \).

### Edge Test Cases

# Test 8
**Input**: 
```
1
3
```
**Output**: 
```
2
```
**Explanation**: For \( x = 3 \), \( y = 2 \) gives \( \gcd(3, 2) + 2 = 1 + 2 = 3 \).

# Test 9
**Input**: 
```
1
4
```
**Output**: 
```
3
```
**Explanation**: For \( x = 4 \), \( y = 3 \) gives \( \gcd(4, 3) + 3 = 1 + 3 = 4 \).

# Test 10
**Input**: 
```
1
5
```
**Output**: 
```
4
```
**Explanation**: For \( x = 5 \), \( y = 4 \) gives \( \gcd(5, 4) + 4 = 1 + 4 = 5 \).

# Test 11
**Input**: 
```
1
8
```
**Output**: 
```
7
```
**Explanation**: For \( x = 8 \), \( y = 7 \) gives \( \gcd(8, 7) + 7 = 1 + 7 = 8 \).

# Test 12
**Input**: 
```
1
9
```
**Output**: 
```
8
```
**Explanation**: For \( x = 9 \), \( y = 8 \) gives \( \gcd(9, 8) + 8 = 1 + 8 = 9 \).

# Test 13
**Input**: 
```
1
11
```
**Output**: 
```
10
```
**Explanation**: For \( x = 11 \), \( y = 10 \) gives \( \gcd(11, 10) + 10 = 1 + 10 = 11 \).

# Test 14
**Input**: 
```
1
12
```
**Output**: 
```
11
```
**Explanation**: For \( x = 12 \), \( y = 11 \) gives \( \gcd(12, 11) + 11 = 1 + 11 = 12 \).

# Test 15
**Input**: 
```
1
13
```
**Output**: 
```
12
```
**Explanation**: For \( x = 13 \), \( y = 12 \) gives \( \gcd(13, 12) + 12 = 1 + 12 = 13 \).

# Test 16
**Input**: 
```
1
14
```
**Output**: 
```
13
```
**Explanation**: For \( x = 14 \), \( y = 13 \) gives \( \gcd(14, 13) + 13 = 1 + 13 = 14 \).

# Test 17
**Input**: 
```
1
15
```
**Output**: 
```
14
```
**Explanation**: For \( x = 15 \), \( y = 14 \) gives \( \gcd(15, 14) + 14 = 1 + 14 = 15 \).

# Test 18
**Input**: 
```
1
16
```
**Output**: 
```
15
```
**Explanation**: For \( x = 16 \), \( y = 15 \) gives \( \gcd(16, 15) + 15 = 1 + 15 = 16 \).

# Test 19
**Input**: 
```
1
17
```
**Output**: 
```
16
```
**Explanation**: For \( x = 17 \), \( y = 16 \) gives \( \gcd(17, 16) + 16 = 1 + 16 = 17 \).

# Test 20
**Input**: 
```
1
18
```
**Output**: 
```
17
```
**Explanation**: For \( x = 18 \), \( y = 17 \) gives \( \gcd(18, 17) + 17 = 1 + 17 = 18 \).

# Test 21
**Input**: 
```
1
19
```
**Output**: 
```
18
```
**Explanation**: For \( x = 19 \), \( y = 18 \) gives \( \gcd(19, 18) + 18 = 1 + 18 = 19 \).

# Test 22
**Input**: 
```
1
20
```
**Output**: 
```
19
```
**Explanation**: For \( x = 20 \), \( y = 19 \) gives \( \gcd(20, 19) + 19 = 1 + 19 = 20 \).

# Test 23
**Input**: 
```
1
1001
```
**Output**: 
```
751
```
**Explanation**: For \( x = 1001 \), \( y = 751 \) gives \( \gcd(1001, 751) + 751 = 1 + 751 = 752 \).

# Test 24
**Input**: 
```
1
999
```
**Output**: 
```
750
```
**Explanation**: For \( x = 999 \), \( y = 750 \) gives \( \gcd(999, 750) + 750 = 3 + 750 = 753 \).

# Test 25
**Input**: 
```
1
1000
```
**Output**: 
```
750
```
**Explanation**: For \( x = 1000 \), \( y = 750 \) gives \( \gcd(1000, 750) + 750 = 250 + 750 = 1000 \).

# Test 26
**Input**: 
```
1
2
```
**Output**: 
```
1
```
**Explanation**: For \( x = 2 \), \( y = 1 \) gives \( \gcd(2, 1) + 1 = 1 +