`a[0]` is updated to `a[0] + (n - x)`. Given that `x` is defined as `a[0] % n`, we can substitute this into the equation to get `a[0] += n - (a[0] % n)`. This simplifies to `a[0] += n - a[0] % n`.

Since `n` is an integer between 1 and 100,000, and `x` is `a[0] % n`, the value of `a[0]` after the operation is `a[0] + n - (a[0] % n)`. 

To simplify further, let's denote `a[0] % n` as `x`. Thus, `a[0]` becomes `a[0] + n - x`. Given that `x = a[0] % n`, the expression simplifies to `a[0] + n - a[0] % n`.

Therefore, the Output State is: `n` is an integer such that \(1 \leq n \leq 100,000\); `a` is the return value of `func_2()`, `x` is `a[0] % n`, and `a[0]` is `a[0] + n - x`.

Output State: **`n` is an integer such that \(1 \leq n \leq 100,000\); `a` is the return value of `func_2()`, `x` is `a[0] % n`, and `a[0]` is `a[0] + n - x`**.