Let's go through the code step-by-step:

1. The initial state is given as follows:
   - `b` is a list of length `n` where each element `b[i] = a[i] % n * (n - 1)`.
   - `a[0]` is updated to `a[0] + n - (a[0] % n)`.
   - Each `a[i]` for `1 <= i < n` is updated to `a[i] + b[i-1]`.
   - `n` is a positive integer within the range \(1 \leq n \leq 100,000\).

2. The code snippet to execute is:
   ```python
   print(*b)
   ```

3. The `print(*b)` statement simply prints the elements of the list `b`. It does not modify the list `b` in any way.

4. Since the list `b` is not modified by the `print` statement, the values of `b` remain as they were in the initial state. Therefore, the values of `b` are still defined by the expressions given in the initial state.

Output State: **`b` is a list of length `n` where each element `b[i] = a[i] % n * (n - 1)`, `a[0]` is updated to `a[0] + n - (a[0] % n)`, each `a[i]` for `1 <= i < n` is updated to `a[i] + b[i-1]`, `n` is a positive integer within the range \(1 \leq n \leq 100,000\)**