The code snippet assigns the value of `-a[i]` to `a[i]`. Given that `i` is 1, this means `a[1]` is being updated to `-a[1]`.

From the initial state:
- `n` is an integer within the range \(1 \leq n \leq 100,000\).
- `i` is 1.
- `a[0]` is \(-a[0]\), which implies `a[0]` is 0 because \(-a[0] = a[0]\) only if `a[0] = 0`.

After the code execution:
- `a[1]` is now \(-a[1]\).
- The values of `n` and `i` remain unchanged.

Output State: **`n` is an integer within the range \(1 \leq n \leq 100,000\); `i` is 1; `a[0]` is 0; `a[1]` is \(-a[1]\).**