The code `count += 1` increments the value of `count` by 1. Since the initial state tells us that `count` is the number of times the condition \((a + b) \% (b * func_1(a, b)) == 0\) was satisfied during the loop's execution, and the condition itself is true, the value of `count` will be incremented by 1. The values of `a`, `b`, `m`, and `n` remain unchanged as they are not affected by this line of code.

Output State: **`a` is 3, `b` is a value within the range [1, m], `m` is a non-negative integer, `n` is a non-negative integer, `count` is the number of times the condition \((a + b) \% (b * func_1(a, b)) == 0\) was satisfied during the loop's execution plus 1 (unchanged), and the condition \((a + b) \% (b * func_1(a, b)) == 0\) is true**