The code snippet `a[l] -= a[r]` modifies the element at index `l` in the list `a` by subtracting the value of the element at index `r` from it.

Given the initial state, the only variable that changes is `a[l]`. All other variables (`t`, `n`, `k`, `l`, `r`, `sunks`) remain unchanged unless they were previously modified, which they were not according to the given initial state.

Therefore, the updated value of `a[l]` is `a[l] - a[r]`.

Output State: **`t` is an integer such that 1 ≤ t ≤ 10^4; for each test case, `n` is an integer such that 1 ≤ n ≤ 2 · 10^5, `a` is a list of `n` integers where `a[l]` is now `a[l] - a[r]` and each integer `a_i` (for i ≠ l) satisfies 1 ≤ a_i ≤ 10^9, and the sum of `n` across all test cases does not exceed 2 · 10^5; `k` is now `k - a[r] * 2`; `l` and `r` remain unchanged unless previously adjusted; `sunks` remains unchanged unless previously incremented.**