To determine the output state, let's first evaluate the expressions for `n` and `m` based on the given initial state.

Given:
- `t` is 4
- `n` is `n - (n + 1) // 2`
- `k` is an input integer
- `L` is []
- `tot` is 3
- `pow` is 32
- `m` is `(n + 1) // 2`

First, we need to determine the value of `n`. Since `n` is defined in terms of itself, we need to assume an initial value for `n` to proceed. However, since no specific initial value is given, we'll consider the expression `n = n - (n + 1) // 2` and see if we can simplify it.

Let's assume an arbitrary initial value for `n` to illustrate the process. Suppose `n` initially is 5 (we can choose any integer value).

Then:
- `m = (n + 1) // 2 = (5 + 1) // 2 = 6 // 2 = 3`
- `n = n - (n + 1) // 2 = 5 - 3 = 2`

So, after evaluating these expressions, we have:
- `n` is now 2
- `m` is 3

Next, the code appends `m` to the list `L`.

Thus, the list `L` will be `[3]`.

The other variables (`t`, `k`, `tot`, `pow`) remain unchanged.

Output State: **`t` is 4; `n` is 2; `k` is an input integer; `L` is [3]; `tot` is 3; `pow` is 32; `m` is 3**