Alright, I've got this problem to solve. Let's see what it's asking for. So, there's this concept of a "good" array, and I need to determine whether certain subarrays are good based on some conditions.

First, let's understand what makes an array "good." According to the problem, an array \( a \) of length \( m \) is considered good if there exists another integer array \( b \) of the same length such that three conditions hold:

1. The sum of elements in \( a \) is equal to the sum of elements in \( b \): \( \sum_{i=1}^{m} a_i = \sum_{i=1}^{m} b_i \).

2. For every index \( i \), \( a_i \) is not equal to \( b_i \): \( a_i \neq b_i \).

3. Every element in \( b \) is positive: \( b_i > 0 \).

So, for a given subarray of \( c \), I need to check if it's possible to create such an array \( b \) that satisfies these three conditions.

Let me try to rephrase this in simpler terms. Essentially, for each subarray from \( l_i \) to \( r_i \), I need to see if I can adjust each element to a different positive integer such that the total sum remains the same.

Hmm, that sounds a bit tricky. Let's think about what constraints this imposes.

First, since \( b_i > 0 \) and \( a_i \neq b_i \), for each \( a_i \), \( b_i \) can be either \( a_i + k \) for some positive integer \( k \), or \( b_i \) can be less than \( a_i \) but still positive.

Wait, no. Since \( b_i \) has to be positive and different from \( a_i \), if \( a_i \) is already greater than 1, \( b_i \) can be \( a_i - 1 \), for example, or \( a_i + 1 \), depending on what keeps it positive.

But I need to ensure that the sum remains the same.

Wait, perhaps I should look at it differently. Suppose I have the sum of the subarray \( s = \sum_{i=l}^{r} a_i \). I need to find another array \( b \) with the same sum, where each \( b_i \) is positive and different from \( a_i \).

One way to approach this is to think about the minimal possible sum for \( b \). Since each \( b_i \) must be positive and different from \( a_i \), the smallest \( b_i \) can be is either \( a_i - 1 \) (if \( a_i > 1 \)) or \( a_i + 1 \) (if \( a_i = 1 \)).

Wait, no. If \( a_i = 1 \), then \( b_i \) cannot be 1, so the smallest \( b_i \) can be is 2. If \( a_i > 1 \), then \( b_i \) can be either \( a_i - 1 \) or something larger, as long as it's not \( a_i \) and positive.

But to minimize the sum of \( b \), I would choose \( b_i \) as close as possible to \( a_i \), but different. So, if \( a_i > 1 \), set \( b_i = a_i - 1 \); if \( a_i = 1 \), set \( b_i = 2 \).

Then, the minimal possible sum for \( b \) would be the sum where each \( b_i \) is set to the smallest possible value as described. If this minimal sum is less than or equal to the original sum \( s \), and the difference between the original sum and this minimal sum is such that it can be distributed among the elements to make up the total sum, then it's possible.

Wait, actually, since the sum of \( b \) must be equal to the sum of \( a \), and I'm trying to minimize the sum of \( b \), if the minimal sum of \( b \) is less than or equal to \( s \), and I can adjust the \( b_i \)'s to match \( s \) while keeping them positive and different from \( a_i \), then the subarray is good.

But perhaps there's a simpler way to look at it.

Let me consider the minimal sum of \( b \):

- For each \( a_i \), if \( a_i > 1 \), then \( b_i \) can be \( a_i - 1 \).

- If \( a_i = 1 \), then \( b_i \) must be at least 2.

So, the minimal possible \( b_i \) is:

- \( a_i - 1 \) if \( a_i > 1 \)

- 2 if \( a_i = 1 \)

Let's denote this minimal \( b_i \) as \( m_i \).

Then, the total minimal sum of \( b \) is \( \sum m_i \).

For the subarray to be good, \( \sum m_i \leq s \), where \( s = \sum a_i \), because I need to be able to adjust the \( b_i \)'s up from \( m_i \) to match the sum \( s \), while keeping \( b_i > 0 \) and \( b_i \neq a_i \).

Wait, but since \( b_i \) must be different from \( a_i \), and I've already set \( m_i \) to the smallest possible value that is different from \( a_i \), then as long as \( \sum m_i \leq s \), I can adjust the \( b_i \)'s to make the sum equal to \( s \).

But, there's a catch. If all \( a_i > 1 \), then \( m_i = a_i - 1 \), so \( \sum m_i = s - k \), where \( k \) is the number of elements in the subarray. In this case, since \( s - k \leq s \), it's always possible to adjust \( b_i \)'s to make the sum equal to \( s \), by increasing some \( b_i \)'s.

Wait, but I need to ensure that \( b_i \) remains positive and different from \( a_i \).

Wait, actually, if \( a_i > 1 \), then \( m_i = a_i - 1 \), which is positive since \( a_i > 1 \). If \( a_i = 1 \), then \( m_i = 2 \), which is also positive.

So, in all cases, \( m_i \) is positive and different from \( a_i \).

Then, the minimal sum \( \sum m_i \) is less than or equal to \( s \), because \( m_i \leq a_i - 1 \) when \( a_i > 1 \), and \( m_i = 2 \) when \( a_i = 1 \).

Wait, but if \( a_i = 1 \), \( m_i = 2 \), which is greater than \( a_i \), so in that case, \( m_i > a_i \).

Wait, no, \( m_i = 2 \) when \( a_i = 1 \), so \( m_i = 2 > 1 = a_i \). For \( a_i > 1 \), \( m_i = a_i - 1 < a_i \).

So, the total \( \sum m_i \) could be less than, equal to, or greater than \( s \), depending on the number of \( a_i = 1 \) in the subarray.

Wait, no. Let's think about it.

Suppose all \( a_i > 1 \), then \( m_i = a_i - 1 \), so \( \sum m_i = s - k \), where \( k \) is the number of elements in the subarray.

If there are some \( a_i = 1 \), then for those, \( m_i = 2 \), so the total \( \sum m_i = s - k + n \times 1 \), where \( n \) is the number of \( a_i = 1 \), and \( k \) is the total number of elements.

Wait, no. Wait, let's calculate it properly.

Let me denote:

- Let \( n \) be the number of elements in the subarray.

- Let \( k \) be the number of elements where \( a_i = 1 \).

Then, for those \( k \) elements, \( m_i = 2 \), and for the remaining \( n - k \) elements, \( m_i = a_i - 1 \).

So, \( \sum m_i = k \times 2 + \sum_{a_i > 1} (a_i - 1) \)

But \( s = \sum a_i \), so \( \sum_{a_i > 1} a_i = s - k \)

Therefore, \( \sum m_i = 2k + (s - k - (n - k)) = 2k + s - k - n + k = s + 2k - n \)

Wait, that seems off.

Wait, no:

Wait, \( \sum m_i = k \times 2 + \sum_{a_i > 1} (a_i - 1) \)

And \( \sum_{a_i > 1} a_i = s - k \), since the sum of all \( a_i \) is \( s \), and \( k \) of them are 1.

Also, \( \sum_{a_i > 1} 1 = n - k \)

Therefore, \( \sum m_i = 2k + (s - k) - (n - k) = 2k + s - k - n + k = s + 2k - n \)

Wait, so \( \sum m_i = s + 2k - n \)

Now, for the subarray to be good, we need to be able to set \( b_i \) to \( m_i \), and have \( \sum b_i = s \). But \( \sum m_i = s + 2k - n \), which may not equal \( s \).

So, if \( \sum m_i \leq s \), then I can adjust the \( b_i \)'s upwards to make the sum equal to \( s \), as long as I don't make \( b_i \) equal to \( a_i \).

But in this case, \( \sum m_i = s + 2k - n \), which may be greater than or less than \( s \).

Wait, so I need \( s + 2k - n \leq s \), which simplifies to \( 2k - n \leq 0 \), or \( 2k \leq n \).

So, if \( 2k \leq n \), then \( \sum m_i \leq s \), and I can adjust the \( b_i \)'s to make the sum equal to \( s \).

But wait, that doesn't sound right. Because if \( \sum m_i > s \), I can't make the sum equal to \( s \) by increasing some \( b_i \)'s, since they are already above \( s \).

Wait, no, if \( \sum m_i > s \), then I can't make the sum equal to \( s \), because \( b_i \) can't be less than \( m_i \).

Wait, but in this case, \( \sum m_i = s + 2k - n \), so if \( 2k - n > 0 \), i.e., \( 2k > n \), then \( \sum m_i > s \), which would make it impossible to have \( \sum b_i = s \).

Wait, but in the earlier step, I thought that if \( \sum m_i \leq s \), then I can adjust \( b_i \)'s upwards to make the sum equal to \( s \). But in reality, \( b_i \) can only be greater than or equal to \( m_i \), and different from \( a_i \).

Wait, but in the minimal case, \( b_i = m_i \), and \( \sum m_i = s + 2k - n \). If \( \sum m_i > s \), then it's impossible to have \( \sum b_i = s \), because the minimal sum is already greater than \( s \).

On the other hand, if \( \sum m_i \leq s \), then I can adjust the \( b_i \)'s upwards to make the sum equal to \( s \), as long as I don't make \( b_i = a_i \).

But is that always possible?

Let me consider a simple example.

Suppose \( n = 1 \), \( a = [1] \), subarray is \( [1] \).

Then, \( m_i = 2 \), which is greater than \( s = 1 \). So, \( \sum m_i = 2 > 1 \), which means it's impossible to have \( b_i = 1 \), because \( b_i \) must be different from \( a_i \) and positive. So, \( b_i \) must be at least 2, but then the sum is 2, which is greater than 1. So, it's impossible, hence NOT good.

Another example: \( n = 2 \), \( a = [1, 2] \), subarray is \( [1, 2] \).

Then, \( m_i \) for \( a_i = 1 \) is 2, and for \( a_i = 2 \) is 1.

So, \( \sum m_i = 2 + 1 = 3 \), and \( s = 1 + 2 = 3 \). So, \( \sum m_i = s \), which means I can set \( b = [2, 1] \), which satisfies all conditions. So, it's good.

Another example: \( n = 3 \), \( a = [1, 1, 2] \), subarray is \( [1, 1, 2] \).

Then, \( m_i \) for \( a_i = 1 \) is 2, and for \( a_i = 2 \) is 1.

So, \( \sum m_i = 2 + 2 + 1 = 5 \), and \( s = 1 + 1 + 2 = 4 \). So, \( \sum m_i = 5 > 4 \), which means it's impossible to have \( \sum b_i = 4 \), because the minimal sum is 5. Hence, NOT good.

Wait, but according to the earlier condition, \( 2k - n = 2 \times 2 - 3 = 1 > 0 \), which matches that \( \sum m_i > s \).

Another example: \( n = 3 \), \( a = [2, 2, 2] \), subarray is \( [2, 2, 2] \).

Then, \( m_i = 1 \) for each, so \( \sum m_i = 3 \), and \( s = 6 \). Since \( \sum m_i = 3 < 6 \), it's possible to adjust \( b_i \)'s to make the sum 6. For example, set \( b = [1, 1, 4] \), which sums to 6, and all \( b_i \) are different from \( a_i \) and positive.

So, in this case, it's good.

Wait, but according to the earlier condition, \( k = 0 \) (since no \( a_i = 1 \)), so \( 2k - n = 0 - 3 = -3 < 0 \), which matches \( \sum m_i < s \).

So, it seems that the condition \( 2k - n \leq 0 \), or \( 2k \leq n \), determines whether it's possible.

But in the earlier example where \( n = 3 \), \( a = [1, 1, 2] \), \( k = 2 \), \( 2k = 4 > 3 = n \), which matches \( \sum m_i > s \), making it impossible.

In the previous example where \( n = 2 \), \( a = [1, 2] \), \( k = 1 \), \( 2k = 2 = n \), which matches \( \sum m_i = s \), making it possible.

In the case where \( n = 1 \), \( a = [1] \), \( k = 1 \), \( 2k = 2 > 1 = n \), which makes it impossible.

Another case: \( n = 1 \), \( a = [2] \), \( k = 0 \), \( 2k = 0 < 1 = n \), which should be possible.

Indeed, \( m_i = 1 \), and \( s = 2 \), so \( \sum m_i = 1 < 2 \), which allows me to set \( b_i = 1 \), but wait, \( b_i \) must be different from \( a_i \), which is 2, so \( b_i = 1 \) is acceptable, and the sum is 1, which is less than 2. So, can I adjust it to make the sum 2? Well, I can set \( b_i = 1 + 1 = 2 \), but then \( b_i = 2 = a_i \), which is not allowed.

Wait, so in this case, it's impossible to have \( b_i \neq a_i \) and \( b_i > 0 \) while having \( \sum b_i = s \).

So, for \( n = 1 \), \( a = [2] \), it's impossible.

Wait, but according to the earlier condition, \( k = 0 \), \( 2k - n = 0 - 1 = -1 < 0 \), which suggests it should be possible, but in reality, it's not.

Hmm, so there's a flaw in this reasoning.

Let me think again.

Perhaps the condition is not just \( 2k \leq n \), but also considering other constraints.

In the case where \( n = 1 \), \( a = [2] \), \( k = 0 \), \( \sum m_i = 1 < s = 2 \), but it's impossible to adjust \( b_i \) to make \( \sum b_i = s \) while keeping \( b_i \neq a_i \).

Wait, why is that? Because \( b_i \) must be different from \( a_i \), which is 2, so \( b_i \) can be 1 or greater than 2, but in this case, setting \( b_i = 1 \) gives sum 1, which is less than 2, and setting \( b_i = 3 \) gives sum 3, which is greater than 2. There's no way to make it exactly 2 without setting \( b_i = 2 \), which is equal to \( a_i \).

So, in this case, even though \( \sum m_i < s \), it's impossible to adjust \( b_i \) to make \( \sum b_i = s \).

So, perhaps the condition is not just \( \sum m_i \leq s \), but also that \( \sum m_i \) can be adjusted to \( s \) without setting any \( b_i = a_i \).

This seems more complicated than I initially thought.

Maybe I need to look for a different approach.

Let me consider the problem differently. For the subarray to be good, I need to find an array \( b \) such that:

1. \( \sum b_i = s \)

2. \( b_i \neq a_i \) for all \( i \)

3. \( b_i > 0 \) for all \( i \)

Perhaps I can think in terms of the differences between \( b_i \) and \( a_i \). Let \( d_i = b_i - a_i \). Then, \( b_i = a_i + d_i \).

Given that \( b_i \neq a_i \), \( d_i \neq 0 \).

Also, \( b_i > 0 \), so \( a_i + d_i > 0 \), which implies \( d_i > -a_i \) (since \( a_i \) is positive, \( d_i \) can be negative but not less than \( -a_i + 1 \)).

Wait, \( a_i + d_i > 0 \), so \( d_i > -a_i \).

Also, \( d_i \neq 0 \).

So, \( d_i \) can be any integer except 0, and \( d_i \geq -a_i + 1 \).

Then, the sum \( \sum (a_i + d_i) = s + \sum d_i = s \), which implies \( \sum d_i = 0 \).

Therefore, I need to find a set of integers \( d_i \) for each \( i \), such that:

- \( d_i \neq 0 \)

- \( d_i \geq -a_i + 1 \)

- \( \sum d_i = 0 \)

This seems like a more general problem of finding integer adjustments that sum to zero, with constraints on each adjustment.

This sounds similar to the problem of distributing a total adjustment of zero across the elements, with each adjustment being non-zero and bounded below by \( -a_i + 1 \).

But this seems a bit too general. Maybe there's a simpler way to look at it.

Let me consider that for each \( a_i \), \( b_i \) can be any positive integer except \( a_i \). So, for each \( a_i \), the possible \( b_i \) values are \( \