To determine which states need to be adjusted for the loop to execute one more time, we need to focus on the conditions in the loop head:

The loop condition is:
\[
(x + y) \cdot x \leq n \quad \text{and} \quad (x + y) \cdot y \leq m
\]

Given the current state at the end of the previous iteration:
- \( x = 1 \)
- \( n \) must be at least 2
- \( m \) must be at least 2
- \( y = 2 \)
- \( cnt = 1 \)

Let's evaluate the loop condition with these values:
\[
(x + y) \cdot x = (1 + 2) \cdot 1 = 3 \cdot 1 = 3
\]
Since \( n \) must be at least 2, \( 3 \leq n \) is true.

Next:
\[
(x + y) \cdot y = (1 + 2) \cdot 2 = 3 \cdot 2 = 6
\]
Since \( m \) must be at least 2, \( 6 \leq m \) is true.

Both conditions are satisfied, so the loop can execute again. However, we need to ensure that the loop can continue executing, which means the conditions must still hold true after the next iteration.

For the loop to continue executing, both conditions must remain true:
1. \((x + y) \cdot x \leq n\)
2. \((x + y) \cdot y \leq m\)

Given the values:
- \( x + y = 3 \)
- Therefore, \((x + y) \cdot x = 3x\) and \((x + y) \cdot y = 3y\)

We need to ensure:
- \( 3x \leq n \)
- \( 3y \leq m \)

Since \( y = 2 \), we need:
- \( 3 \cdot 1 \leq n \) (which is already satisfied as \( n \geq 2 \))
- \( 3 \cdot 2 \leq m \) (which is already satisfied as \( m \geq 2 \))

However, since \( x \) and \( y \) might change within the loop, we need to ensure that the conditions hold for the next iteration. The only way to guarantee this is to ensure that \( n \) and \( m \) are large enough to accommodate the potential increase in \( x \) and \( y \).

Thus, the states that need to be adjusted are:
- \( n \) must be at least 3 (to account for the possibility of \( x \) increasing)
- \( m \) must be at least 6 (to account for the possibility of \( y \) increasing)

State: **`x` is 1, `n` must be at least 3, `m` must be at least 6, `y` is 2, and `cnt` is 1**