Let's break down the problem step by step.

### Step 1: Identify the Loop Condition
The loop condition is given by:
\[ (x + y) \times x \leq n \]
\[ (x + y) \times y \leq m \]

### Step 2: Determine the Current Values
At the end of the previous iteration:
- \( x = 1 \)
- \( n \geq 3 \)
- \( m \geq 6 \)
- \( y = 3 \)
- \( cnt = 2 \)

### Step 3: Evaluate the Loop Condition with Current Values
Substitute the current values into the loop conditions:
1. \( (x + y) \times x = (1 + 3) \times 1 = 4 \leq n \)
2. \( (x + y) \times y = (1 + 3) \times 3 = 12 \leq m \)

Since both conditions are satisfied, the loop will continue to execute.

### Step 4: Determine the Variables in the Loop Head
The loop head involves the variables \( x \), \( y \), \( n \), and \( m \).

### Step 5: Ensure the Loop Can Execute Again
For the loop to execute one more time, the conditions must still be true after the next iteration. The conditions are:
1. \( (x + y) \times x \leq n \)
2. \( (x + y) \times y \leq m \)

Given the current values:
- \( x + y = 4 \)
- Therefore, the conditions simplify to:
  1. \( 4 \times x \leq n \)
  2. \( 4 \times y \leq m \)

Since \( y = 3 \):
- \( 4 \times 3 = 12 \leq m \)

Thus, \( m \geq 12 \).

### Step 6: Adjust the States
To ensure the loop can execute one more time, we need to ensure that:
- \( n \geq 4 \times x \)
- \( m \geq 4 \times y \)

Given \( x = 1 \) and \( y = 3 \):
- \( n \geq 4 \times 1 = 4 \)
- \( m \geq 4 \times 3 = 12 \)

Since \( n \geq 3 \) and \( m \geq 6 \) initially, we need to ensure that \( n \) is at least 4 and \( m \) is at least 12.

### Final Answer
State: **`x` is 1, `n` must be at least 4, `m` must be at least 12, `y` is 3**