Alright, I have this problem to solve. Let's see what it's about. So, there's this physical education lesson in a school, and students are lining up and getting assigned numbers based on their positions and a parameter k. The goal is to find out how many natural numbers k (greater than 1) satisfy the condition that for a given position n and a number x, the settling process assigns x to that position n.

First, I need to understand how the settling process works. It says that the first k people get numbers 1 through k, and then the next k-2 people get numbers k-1 down to 2, and this pattern repeats every 2k-2 positions.

So, for example, if k=3, the sequence would be:

Position: 1 2 3 4 5 6 7 8 9 10...

Numbers: 1 2 3 2 1 2 3 2 1 2...

And the pattern repeats every 4 positions (since 2k-2=4 when k=3).

My task is, given n and x, to find how many k >1 satisfy this condition.

Let me think about how to approach this.

First, I need to find a way to express x in terms of k and n.

Looking at the pattern:

- For positions 1 to k: numbers 1 to k

- Positions k+1 to 2k-2: numbers k-1 to 2

- Then it repeats.

So, the period is 2k-2.

Given a position n, I can find out which segment of the pattern it falls into.

Wait, maybe I should think in terms of modulo operations, considering the periodicity.

But perhaps there's a better mathematical way to model this.

Let me consider that the pattern repeats every 2k-2 positions.

So, the sequence has a cycle of length 2k-2.

Given that, I can find the position within the current cycle.

Let’s denote m = 2k - 2.

So, m is the cycle length.

Then, the position n modulo m will give me the position within the current cycle.

But I need to be careful with how the numbering works within each cycle.

Let me try to find a formula for x in terms of n and k.

First, express n in terms of m:

n = q*m + r, where q is the number of complete cycles before n, and r is the position within the current cycle.

So, r = n mod m.

Now, within each cycle:

- Positions 1 to k: numbers 1 to k

- Positions k+1 to m: numbers k-1 down to 2

So, if r <= k, then x = r

Else, x = m - r + 2

Wait, let's see:

For r > k, x = k - (r - k)

Wait, no.

Let me think again.

In the second part of the cycle (positions k+1 to m):

- Position k+1: k-1

- Position k+2: k-2

- ...

- Position m: 2

So, in general, for r > k, x = k - (r - k)

Wait, let's check with k=3:

m = 4

Positions:

1:1, 2:2, 3:3, 4:2

So, for r=4, x=2

According to the formula x = k - (r - k) = 3 - (4 - 3) = 3 -1 =2, which matches.

Similarly, for r=3, x=3 (since r <=k)

So, the formula seems correct.

Therefore, in general:

if r <=k, x=r

else, x= k - (r -k)

So, x= k - (r -k) = 2k - r

Wait, but in the example above, for r=4, x=2, and 2k - r =6 -4=2, which matches.

Similarly, for r=3, x=3, but 2k - r=6-3=3, which also matches.

Wait, but for r=1, x=1, 2k -r=5, which doesn't match.

Wait, so the formula needs to be:

if r <=k, x=r

else, x=2k - r

Okay, got it.

So, given n, x, and k, I can compute r = n mod m, where m=2k-2

Then, if r <=k, x=r

else, x=2k -r

And I need to find all k >1 such that this holds.

Given that, I can set up an equation based on the above.

First, m=2k-2

r = n mod m

Then, if r <=k, x=r

else, x=2k -r

So, two cases:

1. r <=k => x=r

2. r >k => x=2k -r

In both cases, I can express r in terms of x and k.

Case 1: r <=k, x=r => r=x

Case 2: r >k, x=2k -r => r=2k -x

Now, since r = n mod m, and m=2k-2, r can be from 1 to m (since n >=1)

So, r = n - q*m, where q is such that n - q*m >0 and <=m

Now, I have two expressions for r:

1. r=x (when r <=k)

2. r=2k -x (when r >k)

So, for each case, I can set r equal to x or 2k -x, and solve for k.

But I need to ensure that k >1, and that r is within 1 to m.

Wait, m=2k-2, and k>1.

Also, r = n mod m, so r can be from 1 to m.

Now, let's consider both cases.

Case 1: r=x <=k

So, x <=k

And r=x

But r = n mod m = n mod (2k-2)

So, x = n mod (2k-2)

Therefore, n mod (2k-2) =x

Which implies that n -x is divisible by (2k-2)

So, n -x = q*(2k -2) for some integer q >=0

But since r = n mod m <=k, and m=2k-2, and k >=2, m >=2

So, n -x is divisible by (2k-2)

Similarly, in case 2:

r=2k -x >k

So, 2k -x >k => k >x

And r=2k -x = n mod m = n mod (2k-2)

So, n mod (2k-2) =2k -x

Which implies n - (2k -x) is divisible by (2k-2)

So, n -2k +x = q*(2k-2)

Now, I need to solve these equations for k in both cases.

Let me consider case 1 first:

n -x = q*(2k -2)

So, 2k -2 divides n -x

Similarly, in case 2:

n -2k +x is divisible by (2k -2)

So, 2k -2 divides n -2k +x

Wait, but n -2k +x = - (2k -x -n)

So, 2k -2 divides n -2k +x

But perhaps it's easier to work with the first form.

Now, I need to find all k >1 such that either:

1. x <=k and (2k -2) divides (n -x)

2. k >x and (2k -2) divides (n -2k +x)

Now, I need to find all integers k >1 that satisfy one of these two conditions.

This seems a bit tricky, but perhaps I can iterate over possible k and check these conditions.

But since k can be up to n <=1e9, and t<=100, I need an efficient way to compute this.

Let me think about how to find k that satisfy these conditions.

First, let's consider that m=2k-2

So, m is even, since 2k -2 =2(k-1), which is even.

So, m is even, and m >=2 since k >=2.

Now, in case 1:

m divides (n -x)

In case 2:

m divides (n -2k +x)

But in case 2, k >x, since r=2k -x >k implies k >x.

Wait, but x >=1, since it's a number assigned.

Also, n >=x, since position n is at least x.

Wait, no, n can be less than x, but according to the constraints, 1 <=x <n <=1e9.

Wait, in the problem statement, it says 1 <=x <n <=1e9.

Wait, no, it says 1 <=x <n <=1e9.

Wait, checking the problem statement again:

"the number he received during the settling."

So, x is the number Vasya received, and n is his position.

So, x is between 1 and k, or in the decreasing part, up to k-1.

But in the problem constraints, it's 1 <=x <n <=1e9.

Wait, but in the example, x can be up to n-1, but in some cases, x can be up to k, which can be up to n.

Wait, but in the problem, it's 1 <=x <n <=1e9.

Wait, but in the settling process, x can be up to k, which can be up to n.

But in the problem, it's specified that x <n.

Wait, but in the example, x can be up to n-1.

Wait, in the first test case, n=10, x=2; k can be 2,3,5,6.

For k=2: sequence is 1,2,1,2,1,2,1,2,1,2; so position 10 is 2.

For k=3: 1,2,3,2,1,2,3,2,1,2; position 10 is 2.

For k=5:1,2,3,4,5,4,3,2,1,2; position 10 is 2.

For k=6:1,2,3,4,5,6,5,4,3,2; position 10 is 2.

So, in all these cases, x=2 at position 10.

Similarly, in the second test case, n=3, x=1; only k=2 works.

So, in general, I need to find all k >1 such that, at position n, the number assigned is x.

Given that, I need to find k such that:

- If r <=k, then x=r

- If r >k, then x=2k -r

Where r = n mod m, and m=2k-2.

Now, from above, we have two cases:

1. r <=k implies x=r

2. r >k implies x=2k -r

So, in both cases, we can express r in terms of x and k.

From case 1: r=x <=k

From case 2: r=2k -x >k, which implies k >x

So, combining both cases:

- If r=x <=k

- Or r=2k -x >k (which implies k >x)

Now, r = n mod m, where m=2k-2

So, r can be from 1 to m.

Now, for a given n and x, I need to find k >1 such that either:

- x <=k and n mod m =x

- Or k >x and n mod m =2k -x

Now, m=2k-2

So, n mod m =x for the first case

And n mod m =2k -x for the second case.

Now, n mod m can be expressed as n - floor(n/m)*m

But since m=2k-2, and k is variable, it's a bit tricky.

Perhaps a better approach is to consider that n mod m =x or 2k -x, and m=2k-2.

So, n mod (2k-2) =x or 2k -x

Which implies:

n -x is divisible by (2k-2), or n - (2k -x) is divisible by (2k-2)

So, n -x ≡0 mod (2k-2), or n -2k +x ≡0 mod (2k-2)

Now, let's see if I can solve for k in these equations.

First, consider n -x ≡0 mod (2k-2)

Which means 2k -2 divides n -x

Similarly, n -2k +x ≡0 mod (2k-2)

Which means 2k -2 divides n -2k +x

Now, in the first case, 2k -2 divides n -x

In the second case, 2k -2 divides n -2k +x

Now, in the second case, k >x, since r=2k -x >k implies k >x

So, in the first case, x <=k, and in the second case, k >x

Now, I need to find all k >1 that satisfy either:

- x <=k and (2k -2) divides (n -x)

- k >x and (2k -2) divides (n -2k +x)

Now, I need to find k such that (2k -2) divides (n -x) or (n -2k +x)

But (2k -2) is even, since 2(k-1), and k >=2

So, (2k -2) is at least 2, and even.

Now, perhaps I can set d=2k -2, then k=(d +2)/2

And d divides (n -x) or (n -2k +x)

But substituting k in the second expression:

n -2k +x =n -2*(d +2)/2 +x =n -d -2 +x =n -d -2 +x

So, d divides (n -d -2 +x)

Which is equivalent to d divides (n +x -2 -d)

But this seems a bit messy.

Maybe there's a better way to approach this.

Let me think differently.

Let’s consider that m=2k-2

Then, in the first part of the cycle (positions 1 to k), x=r

In the second part (k+1 to 2k-2), x=2k -r

Now, r = n mod m

So, for x to be equal to r (when r <=k), we have r=x

Or for x to be equal to 2k -r (when r >k), we have r=2k -x

So, in both cases, r is either x or 2k -x

Given that r = n mod m, and m=2k-2

So, n mod m is either x or 2k -x

Which means:

n ≡x mod m, or n ≡2k -x mod m

Now, m=2k-2

So, n -x is divisible by m, or n - (2k -x) is divisible by m

So, m divides (n -x), or m divides (n -2k +x)

Now, m=2k-2

So, 2k -2 divides (n -x), or 2k -2 divides (n -2k +x)

Now, in the first case, 2k -2 divides n -x

Which implies that (2k -2) is a divisor of (n -x)

Similarly, in the second case, 2k -2 divides (n -2k +x)

But in the second case, we also have k >x, since r=2k -x >k implies k >x

So, in the first case: x <=k, and 2k -2 divides n -x

In the second case: k >x, and 2k -2 divides n -2k +x

Now, I need to find all k >1 that satisfy either of these conditions.

Now, to find all k, I can consider the divisors of (n -x) and (n -2k +x)

But since k is involved in both expressions, it's a bit tricky.

Perhaps I can express k in terms of d, where d=2k -2

So, k=(d +2)/2

Then, for the first case, d divides (n -x)

And for the second case, d divides (n -2k +x) =n - (d +2) +x =n -d -2 +x

So, in the second case, d divides (n -d -2 +x)

But d=2k -2, and k >x in this case.

Wait, perhaps this substitution is making it more complicated.

Let me try to think differently.

Let me consider that m=2k-2

And that m divides either (n -x) or (n -2k +x)

So, for each possible m that divides (n -x) or (n -2k +x), I can solve for k.

But k is related to m by m=2k-2, so k=(m +2)/2

So, for each divisor d of (n -x), I can set m=d, then k=(d +2)/2

Similarly, for each divisor d of (n -2k +x), I can set m=d, then k=(d +2)/2

But in the second case, k >x

Wait, perhaps I need to consider all possible m that divide (n -x) or (n -2k +x), and then find k from m.

This seems a bit tangled.

Maybe I need to find a better way to parameterize k.

Let me consider that m=2k-2

So, m is even, and m >=2

Let me set m=2t, where t >=1

Then, k=t +1

So, k >=2, which satisfies the condition k >1

Now, r = n mod m = n mod (2t)

In the first t positions (r <=t), x=r

In the next t-1 positions (r >t), x=2t -r +2

Wait, let's see:

With m=2t, k=t+1

So, positions 1 to t+1: numbers 1 to t+1

Wait, no, k=t+1, so positions 1 to t+1: 1 to t+1

Positions t+2 to 2t: t to 2

So, in terms of r:

If r <=t+1, x=r

Else, x=2t -r +2

Wait, for r=t+1, x=t+1

For r=t+2, x=2t - (t+2) +2=2t -t -2 +2=t

For r=2t, x=2t -2t +2=2

So, it seems correct.

Now, given that, I can set:

If r <=t+1, x=r

Else, x=2t -r +2

Now, I can set r = n mod (2t)

Then, for x=r when r <=t+1

Or x=2t -r +2 when r >t+1

Now, I need to find t such that either:

1. r <=t+1 and x=r

2. r >t+1 and x=2t -r +2

With m=2t, and k=t+1

Now, t >=1, since k >=2

Now, I can express r in terms of t:

r = n mod (2t)

Then, in case 1: r=x <=t+1

In case 2: r=2t -x +2 >t+1, and x=2t -r +2

Wait, in case 2, r=2t -x +2 >t+1

So, 2t -x +2 >t+1 => t -x +2 >1 => t >x -1

Since t >=1 and x >=1, this implies t >=x

Wait, but k=t+1, so k >=x

Wait, no, in the second case, k >x, since r=2t -x +2 >t+1 implies t >x -1, which for t >=1, means t >=x

So, k=t+1 >=x +1 >x

So, in the second case, k >x

Now, in the first case, x <=t+1

In the second case, k >x

Now, I need to find t such that:

- Either x <=t+1 and 2t divides (n -x)

- Or t >=x and 2t divides (n -2(t+1) +x)

Wait, in the second case, m=2t, and n -2k +x =n -2(t+1) +x

So, 2t divides (n -2(t+1) +x)

Simplify: n -2t -2 +x

So, 2t divides (n +x -2t -2)

Now, this seems a bit messy.

Perhaps I can consider both cases separately.

First, for the first case:

x <=t+1 and 2t divides (n -x)

Then, t >=x -1

But t >=1, so t >=max(1, x -1)

And t <= floor((n -x)/2)

Because 2t divides (n -x), so 2t <=n -x

Wait, no, 2t divides n -x, so n -x >=0 and 2t divides n -x

Similarly, in the second case:

t >=x

And 2t divides (n +x -2t -2)

Which can be written as 2t divides (n +x -2 -2t)

Which implies that 2t divides (n +x -2 -2t)

Which can be rearranged to 2t divides (n +x -2) -2t

Which is 2t divides (n +x -2) modulo 2t

Wait, this seems circular.

Perhaps I need to think differently.

Let me consider that in both cases, 2t divides either (n -x) or (n -2(t+1) +x)

So, for each possible t, I can check if 2t divides (n -x) or (n -2(t+1) +x)

But t can be from 1 to floor((n -x)/2), since m=2t must be <=n -x for the first case.

Wait, no, m can be any even number >=2, but it's constrained by the divisibility.

This seems a bit tricky.

Let me consider that for the first case, 2t divides (n -x), and x <=t+1

Similarly, for the second case, 2t divides (n -2(t+1) +x), and t >=x

Now, perhaps I can iterate over possible t, compute k=t+1, and check if either condition holds.

But since t can be up to n, which is up to 1e9, and t<=floor((n -x)/2), it's still manageable.

But I need a smarter way to compute this efficiently for t<=100 test cases.

Wait, t is the number of test cases, up to 100, but n can be up to 1e9.

So, for each test case, I need an efficient way to compute the number of possible k.

Let me think about the first case:

x <=t+1 and 2t divides (n -x)

So, t >=x -1, and t <=floor((n -x)/2)

Similarly, in the second case:

t >=x, and 2t divides (n -2(t+1) +x)

Wait, perhaps I can consider that in the first case, 2t divides (n -x), and t >=x -1

Then, the number of such t is the number of divisors of (n -x)/2 that are >=ceil((x -1)/2)

Wait, perhaps that's too convoluted.

Let me think about it differently.

Let me consider y = n +x

As in the code provided.

Wait, the code provided is:

import math

t = int(input())

for _ in range(t):

L = list(map(int, input().split()))

n = L[0]

x = L[1]

ans = 0

y = n + x

if y % 2 !=0:

print(0)

continue

else:

L1 = func_1((y -2)//2, x)

if n >=3*x -2:

L1 += func_1((n -x)//2, x)

L1 = list(set(L1))

print(len(L1))

continue

def func_1(q, x):

M = []

w = math.sqrt(q)

if w == w//1 and w >=x -1:

M += [w]

i =1

while i <w:

if q %i ==0:

if i >=x -1:

M += [i]

if q//i >=x -1:

M += [q//i]

i +=1

return M

So, the code defines a function func_1 that takes q and x, and finds all integers i such that i >=x -1 and i is a divisor of q, and also q//i >=x -1.

Then, it computes y =n +x

If y is odd, it prints 0

Else, it computes q=(y -2)//2

And calls func_1(q, x)

Then, if n >=3*x -2, it adds the result of func_1((n -x)//2, x)

Finally, it takes the set of all results and prints the length.

Now, I need to understand why this works.

First, y =n +x

If y is odd, then y -2 is odd, and (y -2)//2 is floor((y -2)/2)

Similarly, (n -x)//2 is floor((n -x)/2)

Now, in func_1(q, x), it finds all i such that i >=x -1 and i is a divisor of q, and also q//i >=x -1

Then, it seems that it's finding divisors i of q such that i >=x -1 and q//i >=x -1

Wait, q//i is also a divisor of q, so it's adding both i and q//i to the list M, but only if they are >=x -1

Then, it returns the list M

Then, the main function calls func_1 with q=(y -2)//2 and x, and if n >=3*x -2, it adds the results of func_1((n -x)//2, x)

Then, it takes the set of all these k and prints the number of unique k.

Now, I need to see how this relates to the original problem.

Let me try to relate y =n +x

Given that y =n +x

Then y -2 =n +x -2

And (y -2)//2 = (n +x -2)//2

Similarly, (n -x)//2 = floor((n -x)/2)

Now, perhaps there's a relationship between these expressions and the earlier conditions.

Let me recall that in the first case, 2t divides (n -x)

And in the second case, 2t divides (n -2(t+1) +x)

Now, let's see if I can relate these to y =n +x

In the second case, 2t divides (n -2(t+1) +x) =n -2t -2 +x

Which is (n +x -2) -2t

So, 2t divides (n +x -2) -2t

Which implies that 2t divides (n +x -2)

Because 2t divides (n +x -2) -2t, and 2t divides 2t, hence 2t divides (n +x -2)

Wait, that's interesting.

So, in the second case, 2t divides (n +x -2)

Similarly, in the first case, 2t divides (n -x)

Now, in the code, it computes q=(y -2)//2=(n +x -2)//2

Then, it calls func_1(q, x), which finds divisors i of q such that i >=x -1 and q//i >=x -1, then sets k=i

Similarly, if n >=3*x -2, it calls func_1((n -x)//2, x)

Now, perhaps in the first call to func_1, it's handling the second case where 2t divides (n +x -2), and t=i

Then, in the second call, it's handling the first case where 2t divides (n -x), with t=i

Wait, but in the first call, q=(n +x -2)//2, and func_1 finds divisors i of q such that i >=x -1 and q//i >=x -1

Then, k=i

Similarly, in the second call, q=(n -x)//2, and finds divisors i of q with similar conditions.

Now, I need to see how this relates to the earlier conditions.

Wait, perhaps t=i in the first case, and t=i in the second case.

Then, in the first case, 2t divides (n +x -2), which corresponds to the second settling case.

And in the second case, 2t divides (n -x), which corresponds to the first settling case.

Now, in the code, it takes the union of these two lists and removes duplicates by using a set.

Then, it prints the number of unique k.

Now, I need to verify if this approach is correct.

Let me check with the first test case:

n=10, x=2

y=12

y -2=10

(y -2)//2=5

So, q=5

Then, func_1(5,2)

Find divisors i of 5 such that i >=1 (since x-1=1) and 5//i >=1

Divisors of 5:1,5

i=1: 1>=1 and 5>=1 => include 1

i=5:5>=1 and 1>=1 => include 5

So, M=[1,5]

Then, check if n >=3*x -2 =>10 >=4, which is true

So, call func_1((10 -2)//2,2)=func_1(4,2)

q=4

Divisors of 4:1,2,4

i=1:1>=1 and 4>=1 =>include 1

i=2:2>=1 and 2>=1 =>include 2

i=4:4>=1 and 1>=1 =>include 4

So, M=[1,5,1,2,4]

Then, take set: {1,2,4,5}

So, length is 4, which matches the first test case output.

Similarly, second test case:

n=3,x=1

y=4

y -2=2

(q=1)

func_1(1,1)

Divisors of 1:1

i=1:1>=0 and 1>=0 =>include 1

Then, n >=3*1 -2 =>3>=1, which is true

Call func_1((3-1)//2,1)=func_1(1,1)

Which is again [1]

Then, M=[1,1], set is [1], length=1, which matches the second test case.

Third test case:

n=76,x=4

y=80

y -2=78

q=39

func_1(39,4)

Divisors of 39:1,3,13,39

i=1:1>=3? No

i=3:3>=3 and 13>=3 =>include 3

i=13:13>=3 and 3>=3 =>include 13

i=39:39>=3 and 1>=3? No

So, M=[3,13]

Then, n >=3*4 -2 =>76 >=10, which is true

Call func_1((76-4)//2,4)=func_1(36,4)

Divisors of 36:1,2,3,4,6,9,12,18,36

i=1:1>=3? No

i=2:2>=3? No

i=3:3>=3 and 12>=3 =>include 3

i=4:4>=3 and 9>=3 =>include 4

i=6:6>=3 and 6>=3 =>include 6

i=9:9>=3 and 4>=3 =>include 9

i=12:12>=3 and 3>=3 =>include 12

i=18:18>=3 and 2>=3? No

i=36:36>=3 and 1>=3? No

So, M=[3,13,3,4,6,9,12]

Set is [3,4,6,9,12,13], length=6

But the third test case output is 9, which doesn't match.

Wait, perhaps I made a mistake.

Wait, in the example output, third test case is 9, but according to this, it's 6.

Wait, perhaps I missed some divisors.

Wait, in func_1(39,4):

q=39, x=4

Divisors of 39:1,3,13,39

i=3:3>=3 and 13>=3 =>include 3

i=13:13>=3 and 3>=3 =>include 13

So, M=[3,13]

Then, func_1(36,4):

q=36, x=4

Divisors of 36:1,2,3,4,6,9,12,18,36

i=3:3>=3 and 12>=3 =>include 3

i=4:4>=3 and 9>=3 =>include 4

i=6:6>=3 and 6>=3 =>include 6

i=9:9>=3 and 4>=3 =>include 9

i=12:12>=3 and 3>=3 =>include 12

So, M=[3,13,3,4,6,9,12]

Set is [3,4,6,9,12,13], which is 6 elements.

But the third test case output is 9.

So, perhaps there's a mistake in the code or in my understanding.

Wait, perhaps I need to consider that k=t+1, where t=i

So, k=i +1

So, in the first call to func_1, k=i +1

Similarly, in the second call, k=i +1

So, the actual k values are i +1

So, in the first test case, M=[1,5], so k=2,6

From the second call, M=[1,2,4], so k=2,3,5

Then, the union is [2,3,5,6], which is 4 elements, which matches the first test case.

In the third test case, M=[3,13,3,4,6,9,12], which corresponds to k=4,14,4,5,7,10,13

Set is [4,5,7,10,13,14]

Which is 6 elements, but the output is 9.

Wait, perhaps I missed some divisors.

Wait, in the code, it's func_1((y -2)//2, x)

With y=n +x

So, q=(n +x -2)//2

And in the second call, func_1((n -x)//2, x)

So, q=(n -x)//2

Then, in func_1, it finds i such that i >=x -1 and q//i >=x -1

Then, k=i +1

So, in the third test case, n=76, x=4

y=80, y -2=78, q=39

func_1(39,4):

Divisors of 39:1,3,13,39

i=3:3>=3 and 13>=3 =>include 3

i=13:13>=3 and 3>=3 =>include 13

So, k=4,14

Then, (n -x)//2=36

func_1(36,4):

Divisors of 36:1,2,3,4,6,9,12,18,36

i=3:3>=3 and 12>=3 =>include 3

i=4:4>=3 and 9>=3 =>include 4

i=6:6>=3 and 6>=3 =>include 6

i=9:9>=3 and 4>=3 =>include 9

i=12:12>=3 and 3>=3 =>include 12

So, k=4,5,7,10,13

Then, the union is k=4,5,7,10,13,14

Which is 6 elements, but the output is 9.

Wait, perhaps I missed some divisors.

Wait, in the code, it's checking if w = math.sqrt(q), and if w == w//1 and w >=x -1, then include w

Then, it iterates i from 1 to w, and includes i and q//i if they are >=x -1

Wait, in func_1(q, x):

M = []

w = math.sqrt(q)

if w == w//1 and w >=x -1:

M += [w]

i =1

while i <w:

if q %i ==0:

if i >=x -1:

M += [i]

if q//i >=x -1:

M += [q//i]

i +=1

return M

So, in func_1(39,4):

q=39, x=4

w=sqrt(39)=6.244998, w//1=6.0, which is not equal to w, so skip

Then, i from 1 to 6:

i=1: q%1==0, 1>=3? No

i=2: q%2 !=0, skip

i=3: q%3==0, 3>=3 =>include 3

q//3=13>=3 =>include 13

i=4: q%4 !=0, skip

i=5: q%5 !=0, skip

i=6: q%6 !=0, skip

So, M=[3,13]

Then, k=4,14

Similarly, func_1(36,4):

q=36, x=4

w=sqrt(36)=6.0, which equals w//1=6.0, and 6 >=3 =>include 6

Then, i from 1 to 6:

i=1: q%1==0, 1>=3? No

i=2: q%2==0, 2>=3? No

i=3: q%3==0, 3>=3 =>include 3

q//3=12>=3 =>include 12

i=4: q%4==0, 4>=3 =>include 4

q//4=9>=3 =>include 9

i=5: q%5 !=0, skip

i=6: q%6==0, 6>=3 =>include 6

q//6=6>=3 =>include 6

So, M=[6,3,12,4,9,6]

Then, k=7,14,13,5,10,7

Set is [7,14,13,5,10], since k=i +1

Wait, no, in the code, k=i

Wait, hold on.

In the code, k=i

Wait, but earlier I thought k=i +1, but actually, in the code, k=i

Wait, no, in the code, it's defining t=i, then k=t +1

Wait, no, in the code, it's not explicitly defining k, but in the function func_1, it's collecting i's that satisfy the conditions, and then in the main function, it's considering these i's as k's.

Wait, perhaps I misread the code.

Looking back at the code:

def func_1(q, x):

M = []

w = math.sqrt(q)

if w == w//1 and w >=x -1:

M += [w]

i =1

while i <w:

if q %i ==0:

if i >=x -1:

M += [i]

if q//i >=x -1:

M += [q//i]

i +=1

return M

Then, in the main function, it calls L1 = func_1((y -2)//2, x)

Then, if n >=3*x -2, L1 += func_1((n -x)//2, x)

Then, L1 = list(set(L1))

print(len(L1))

So, it's collecting the values of i from func_1 as possible k's.

But in my earlier reasoning, I set t=i, then k=t +1

But in the code, it's directly using i as k.

This seems inconsistent with my earlier reasoning.

Wait, perhaps in the code, k=i, not t=i

Wait, in my earlier reasoning, t=i, then k=t +1

But in the code, it's using k=i

So, perhaps the code is incorrect in this aspect.

Wait, but according to the first test case, it outputs 4, which matches the expected output.

Wait, in the first test case, k=2,3,5,6 are suitable.

But according to my earlier calculation, with t=i, k=t +1, which would be k=2,4,14, etc., which doesn't match.

Wait, perhaps I need to re-examine this.

Wait, perhaps in the code, k=i, where i=t, and t=k -1

Wait, no, t=i, m=2t, k=t +1

So, k=i +1

But in the code, it's using i as k, which seems incorrect.

Wait, no, in the code, it's using i as t, and then k=t +1

Wait, but in the code, it's collecting i's and then considering them as k's.

Wait, perhaps there's confusion in variable names.

Looking back, in my earlier reasoning, I set t=i, then k=t +1

But in the code, it's collecting i's and treating them as k's.

This suggests that in the code, k=i,