The value of `high` is updated to be equal to `mid`. Since `mid` = `(low + high) // 2`, the new value of `high` is `(low + high) // 2`. The states of the other variables are not affected. We know that `high` ≥ `low` + 1, but since `high` is now equal to `(low + high) // 2`, we can infer that `(low + high) // 2` ≥ `low` + 1. However, this information does not change the fact that `low` < `high`. 

Given `high` = `(low + high) // 2`, we can simplify this to `high` = `mid`, and we know `mid` = `(low + high) // 2`, so `high` = `(low + high) // 2`. Multiplying both sides by 2 gives us `2 * high` = `low + high`, and subtracting `high` from both sides gives us `high` = `low`. However, this would contradict the given condition that `low` < `high`. 

To resolve this, let's analyze the equation `high` = `(low + high) // 2` again. This implies that `2 * high` = `low + high`, which simplifies to `high` = `low`. However, since we know that `high` ≥ `low` + 1 initially, setting `high` to `(low + high) // 2` effectively reduces the gap between `high` and `low`, but it doesn't necessarily make `high` equal to `low`. 

Instead, the correct interpretation is that `high` is now equal to `mid`, which is a value between `low` and the original `high`. This means `low` < `high` still holds, and `high` ≥ `low` + 1 might not hold after the update, depending on the original values of `low` and `high`. 

Given the condition 2 ≤ `n` ≤ `a` + `b` and the constraints on `a` and `b`, these conditions remain unchanged as the code snippet only updates the value of `high`.

Output State: **`n`, `a`, and `b` are integers such that 1 ≤ `a`, `b` ≤ 100 and 2 ≤ `n` ≤ `a` + `b`, `low` < `high`, and `high` = `(low + high) // 2`, which simplifies to `high` = `mid`**