The code snippet updates the `diff` variable by adding to it the product of `(a[i] - 1)` and `m[a[i] - 1]`. Here's the detailed step-by-step impact:

- `diff` is updated to `diff + (a[i] - 1) * m[a[i] - 1]`.
- `i` is currently set to `n - 1`, so the last element of the list `a` is considered.
- `m[a[i] - 1]` is the value in the dictionary `m` corresponding to the key `a[i] - 1`. If this key does not exist in `m`, it is treated as 0.

Therefore, the Output State is: `n` is an input integer where 1 ≤ n ≤ 200000, `a` is a list of `n` integers where 1 ≤ ai ≤ 10^9, `sm` is 0, `m` is an empty dictionary, `ans` is 0, `i` is `n - 1`, `cnt` is incremented by `m[a[n - 1] - 1]`, `diff` is `diff + (a[n - 1] - 1) * m[a[n - 1] - 1]`.

Output State: **`n` is an input integer where 1 ≤ n ≤ 200000, `a` is a list of `n` integers where 1 ≤ ai ≤ 10^9, `sm` is 0, `m` is an empty dictionary, `ans` is 0, `i` is `n - 1`, `cnt` is incremented by `m[a[n - 1] - 1]`, `diff` is `diff + (a[n - 1] - 1) * m[a[n - 1] - 1]`**