The code snippet `diff += a[i] * m[a[i]]` updates the value of `diff` by adding the product of `a[i]` and `m[a[i]]` to the current value of `diff`.

Given the initial state:
- `n` is an input integer where 1 ≤ n ≤ 200000.
- `a` is a list of `n` integers where 1 ≤ ai ≤ 10^9.
- `sm` is `a[n - 2]`.
- `m` is a dictionary.
- `ans` is updated to `ans + -diff - a[n - 2] * (1 - cnt)`.
- `i` is `n - 2`.
- `cnt` is `m[sm]`.
- `diff` is 0.

Let's analyze the impact of the code:

1. **Value of `a[i]`**: Since `i` is `n - 2`, `a[i]` is `a[n - 2]`, which is also `sm`.
2. **Value of `m[a[i]]`**: Since `a[i]` is `sm`, `m[a[i]]` is `m[sm]`, which is `cnt`.
3. **Update of `diff`**: `diff` is updated by adding the product of `a[i]` and `m[a[i]]` to its current value. Since `a[i]` is `sm` and `m[a[i]]` is `cnt`, `diff` becomes `0 + sm * cnt` which simplifies to `diff = sm * cnt`.

Therefore, the output state is:
- `n` is an input integer where 1 ≤ n ≤ 200000.
- `a` is a list of `n` integers where 1 ≤ ai ≤ 10^9.
- `sm` is `a[n - 2]`.
- `m` is a dictionary.
- `ans` is updated to `ans + -diff - a[n - 2] * (1 - cnt)`.
- `i` is `n - 2`.
- `cnt` is `m[sm]`.
- `diff` is `sm * cnt`.

Output State: **`n` is an input integer where 1 ≤ n ≤ 200000, `a` is a list of `n` integers where 1 ≤ ai ≤ 10^9, `sm` is `a[n - 2]`, `m` is a dictionary, `ans` is updated to `ans + -diff - a[n - 2] * (1 - cnt)`, `i` is `n - 2`, `cnt` is `m[sm]`, `diff` is `sm * cnt`.**