The given code snippet updates the value of `ans` based on the current values of `sm`, `diff`, `a[i]`, `n`, `i`, and `cnt`.

### Step-by-Step Analysis:

1. **Initial Values:**
   - `n` is an input integer where \( 1 \leq n \leq 200000 \).
   - `a` is a list of `n` integers where \( 1 \leq a_i \leq 10^9 \).
   - `sm` is \( a[n - 2] \).
   - `m` is a dictionary.
   - `i` is \( n - 2 \).
   - `cnt` is updated based on the presence of `a[i] - 1` in `m`.
   - `diff` is updated based on the presence of `a[i] - 1` in `m`.
   - `ans` is updated based on the presence of `a[i] - 1` in `m` and `a[i] + 1` in `m`.

2. **Code Execution:**
   ```python
   ans += sm - diff - a[i] * (n - i - 1 - cnt)
   ```

3. **Impact on Variables:**
   - `ans` is updated by adding the value of `sm - diff - a[i] * (n - i - 1 - cnt)` to its current value.

### Calculation:

- **Current Values:**
  - `sm = a[n - 2]`
  - `i = n - 2`
  - `a[i] = a[n - 2]` (since `i = n - 2`)
  - `n - i - 1 = n - (n - 2) - 1 = 1`

- **Expression for `ans` Update:**
  - `ans += sm - diff - a[i] * (n - i - 1 - cnt)`
  - Substituting the values:
    - `ans += a[n - 2] - diff - a[n - 2] * (1 - cnt)`
    - Simplifying:
      - `ans += a[n - 2] - diff - a[n - 2] + a[n - 2] * cnt`
      - `ans += -diff + a[n - 2] * cnt`

### Final Output State:

- `n` is an input integer where \( 1 \leq n \leq 200000 \).
- `a` is a list of `n` integers where \( 1 \leq a_i \leq 10^9 \).
- `sm` is \( a[n - 2] \).
- `m` is a dictionary.
- `i` is \( n - 2 \).
- `cnt` is the same as before.
- `diff` is the same as before.
- `ans` is updated to `ans + -diff + a[n - 2] * cnt`.

Output State: **`n` is an input integer where \( 1 \leq n \leq 200000 \), `a` is a list of `n` integers where \( 1 \leq a_i \leq 10^9 \), `sm` is \( a[n - 2] \), `m` is a dictionary, `i` is \( n - 2 \), `cnt` is the same as before, `diff` is the same as before, `ans` is updated to `ans + -diff + a[n - 2] * cnt`.**