The code snippet updates the value of `diff` by adding the product of `a[i]` and `m[a[i]]` to it.

- `i` is currently set to `n - 3`.
- `a[i]` is the value of the element in the list `a` at index `i`.
- `m[a[i]]` is the value in the dictionary `m` corresponding to the key `a[i]`.

Given the initial state:
- `n` is an input integer where \( 1 \leq n \leq 200000 \).
- `a` is a list of `n` integers where \( 1 \leq a_i \leq 10^9 \).
- `sm` is \( a[n - 3] + a[n - 3] \).
- `i` is \( n - 3 \).
- `cnt` is `m[a[n - 3]]`.
- `diff` is 0.
- `ans` is updated to `ans + -diff + a[n - 3] * cnt`.
- `m` is the same as before.

After executing the code:
- `diff` is updated to `a[i] * m[a[i]]`.

Since `i` is `n - 3`, the new value of `diff` is `a[n - 3] * m[a[n - 3]]`.

Therefore, the output state is:
Output State: **`n` is an input integer where \( 1 \leq n \leq 200000 \), `a` is a list of `n` integers where \( 1 \leq a_i \leq 10^9 \), `sm` is \( a[n - 3] + a[n - 3] \), `i` is \( n - 3 \), `cnt` is `m[a[n - 3]]`, `diff` is `a[n - 3] * m[a[n - 3]]`, `ans` is `ans + -0 + a[n - 3] * cnt`, and `m` is the same as before.**