Let's analyze the provided code snippet step by step:

### Initial State:
- `n` is an input integer where \( 1 \leq n \leq 200000 \)
- `a` is a list of `n` integers where \( 1 \leq a_i \leq 10^9 \)
- `sm` is \( a[n - 3] + a[n - 3] \)
- `i` is \( n - 3 \)
- `cnt` is initially 0
- `diff` is initially 0
- `ans` is updated to `ans + -0 + a[n - 3] * cnt`

### Code Snippet:
```python
ans += sm - diff - a[i] * (n - i - 1 - cnt)
```

### Step-by-Step Analysis:
1. **Initial Values:**
   - `sm` = \( a[n - 3] + a[n - 3] \) = \( 2 \times a[n - 3] \)
   - `i` = \( n - 3 \)
   - `cnt` = 0
   - `diff` = 0
   - `ans` = `ans + -0 + a[n - 3] * cnt` = `ans + 0` = `ans`

2. **Expression Breakdown:**
   - `sm - diff` = \( 2 \times a[n - 3] - 0 \) = \( 2 \times a[n - 3] \)
   - `a[i]` = \( a[n - 3] \)
   - `n - i - 1` = \( n - (n - 3) - 1 \) = 3 - 1 = 2
   - `a[i] * (n - i - 1 - cnt)` = \( a[n - 3] \times (2 - 0) \) = \( 2 \times a[n - 3] \)

3. **Final Calculation:**
   - `ans += sm - diff - a[i] * (n - i - 1 - cnt)`
   - `ans += 2 \times a[n - 3] - 2 \times a[n - 3]`
   - `ans += 0`

### Updated State:
- `ans` remains unchanged because the expression `sm - diff - a[i] * (n - i - 1 - cnt)` evaluates to 0.

### Output State:
**`n` is an input integer where \( 1 \leq n \leq 200000 \), `a` is a list of `n` integers where \( 1 \leq a_i \leq 10^9 \), `sm` is \( 2 \times a[n - 3] \), `i` is \( n - 3 \), `cnt` is 0, `diff` is 0, `ans` remains unchanged.**