To evaluate the impact of the code, we analyze the expression `sum_m` which computes a value based on the initial state of the variables.

The initial values are:
- `m` is a positive integer such that \( 1 \leq m \leq 10^9 \)
- `a` is a positive integer such that \( 1 \leq a \leq 10^5 \)
- `b` is a positive integer such that \( 1 \leq b \leq 10^5 \)
- `g` is equal to 1
- `k` is equal to \( a + b - 1 \)
- `m` is greater than or equal to `k`
- `sum_k` is equal to \( (a + b - 1) * (a + b) // 2 \)

The computation for `sum_m` involves subtracting the sum of the first `k-1` integers from the sum of the first `m` integers.

The expression for `sum_m` becomes:
\[
sum\_m = \frac{m \times (m + 1)}{2} - \frac{k \times (k - 1)}{2}
\]

This does not change any precondition but results in a new value for `sum_m`.

Output State: **`m` is a positive integer such that 1 <= m <= 10^9, `a` is a positive integer such that 1 <= a <= 10^5, `b` is a positive integer such that 1 <= b <= 10^5, `g` is equal to 1, `k` is equal to `a + b - 1`, `m` is greater than or equal to `k`, `sum_k` is equal to `(a + b - 1) * (a + b) // 2`, `sum_m` is equal to `m * (m + 1) // 2 - k * (k - 1) // 2`.**