Let's break down the initial state and the calculation step by step:

1. **Initial State**:
   - `t` is an integer such that \(1 \leq t \leq 10^4\).
   - `x` is a list of integers obtained by splitting a string on spaces and converting each element to an integer.
   - `n` is the first element of the list `x`.
   - `a` is the second element of the list `x`.
   - `b` is the third element of the list `x`.
   - `profit` is defined as \( n \cdot a + (b - a) \cdot ( \min(n - 1, b - a) + 1 ) - \frac{ \min(n - 1, b - a) \cdot ( \min(n - 1, b - a) + 1 ) }{2} \).
   - `k` is defined as \( \min(n - 1, b - a) \).
   - `a` is less than `b`.

2. **Expression for `profit`**:
   - Let's denote \( k = \min(n - 1, b - a) \).
   - The profit expression simplifies to:
     \[
     \text{profit} = n \cdot a + (b - a) \cdot (k + 1) - \frac{k \cdot (k + 1)}{2}
     \]

3. **Simplifying the Expression**:
   - Since `a < b`, `k` will be either \( n - 1 \) or \( b - a \), whichever is smaller.
   - If \( n - 1 \leq b - a \), then \( k = n - 1 \).
   - If \( n - 1 > b - a \), then \( k = b - a \).

4. **Final Simplified Form**:
   - For simplicity, let's assume \( n - 1 \leq b - a \) (the more general case):
     \[
     \text{profit} = n \cdot a + (b - a) \cdot (n - 1 + 1) - \frac{(n - 1) \cdot n}{2}
     \]
     \[
     \text{profit} = n \cdot a + (b - a) \cdot n - \frac{n \cdot (n - 1)}{2}
     \]
     \[
     \text{profit} = n \cdot a + n \cdot (b - a) - \frac{n \cdot (n - 1)}{2}
     \]
     \[
     \text{profit} = n \cdot a + n \cdot b - n \cdot a - \frac{n \cdot (n - 1)}{2}
     \]
     \[
     \text{profit} = n \cdot b - \frac{n \cdot (n - 1)}{2}
     \]

5. **Output**:
   - The `print(int(profit))` statement will print the integer value of the simplified profit expression.

Output: **int(n * b - n * (n - 1) / 2)**