To determine what will be printed when the `print(ans)` statement executes, let's break down the initial state and the operations involved:

1. **Initial State:**
   - `t` is an integer such that \(1 \leq t \leq 10^4\).
   - `n` is an integer such that \(1 \leq n \leq 2 \cdot 10^5\).
   - `a` is a list of `n` integers where \(0 \leq a_i < n\).
   - `int(input())` must be greater than 0.
   - `i` is 0.
   - `l` is an input integer greater than 0.
   - `s` is a list of `l` integers where each `s[j]` is equal to the number of times `j` appears in `array`.
   - `array` has `m` elements (where `m` is the length of `array`), each element in `array` is greater than 0.
   - `j` is the last element in `array`.
   - `ans` is a string containing characters corresponding to the cumulative sum of `s[j]` at each position in `array`, starting from 97 (ASCII value of 'a').

2. **Understanding the Variables:**
   - `array` is a list of positive integers.
   - `s` is a frequency list where `s[j]` represents how many times the integer `j` appears in `array`.
   - `j` is the last element of `array`.
   - `ans` is constructed by converting the cumulative sum of `s[j]` for each element in `array` to a character using the ASCII value starting from 97 ('a').

3. **Constructing `ans`:**
   - For each element `j` in `array`, we look up `s[j]` which gives the frequency of `j` in `array`.
   - We then calculate the cumulative sum of these frequencies.
   - Each cumulative sum is converted to a character using the ASCII value starting from 97 ('a').

4. **Example Calculation:**
   - Suppose `array = [1, 2, 1, 3, 2]`.
   - The frequency list `s` would be:
     - `s[1] = 2` (1 appears twice)
     - `s[2] = 2` (2 appears twice)
     - `s[3] = 1` (3 appears once)
   - The cumulative sum of frequencies for each element in `array` would be:
     - For `1`: `s[1] = 2`
     - For `2`: `s[1] + s[2] = 2 + 2 = 4`
     - For `1`: `s[1] + s[2] + s[1] = 2 + 2 + 2 = 6`
     - For `3`: `s[1] + s[2] + s[1] + s[3] = 2 + 2 + 2 + 1 = 7`
     - For `2`: `s[1] + s[2] + s[1] + s[3] + s[2] = 2 + 2 + 2 + 1 + 2 = 9`
   - Converting these cumulative sums to characters starting from 97 ('a'):
     - `2 -> chr(97 + 2 - 1) = chr(98) = 'b'`
     - `4 -> chr(97 + 4 - 1) = chr(100) = 'd'`
     - `6 -> chr(97 + 6 - 1) = chr(102) = 'f'`
     - `7 -> chr(97 + 7 - 1) = chr(103) = 'g'`
     - `9 -> chr(97 + 9 - 1) = chr(105) = 'i'`
   - Therefore, `ans = 'bdfig'`.

5. **General Output:**
   - The `print(ans)` statement will print a string where each character corresponds to the cumulative sum of the frequencies of the elements in `array`, converted to a character starting from 'a'.

Output: **ans (where ans is a string containing characters corresponding to the cumulative sum of the frequencies of the elements in `array`, starting from 'a')**