Let's break down the initial state and the code snippet step by step:

1. **Initial State:**
   - `m` is defined as `m` (which was `0 + b[s - 1]`) plus `(bd[s] * (ql - a[s - 1])) / ad[s]`.
     - Since `m` is initially `0 + b[s - 1]`, let's denote this as `m = b[s - 1]`.
     - We need to know the values of `b`, `bd`, `ad`, `s`, `ql`, and `a` to proceed further.
   - `i` is 1.
   - `s` is the index where `ql` would be inserted to keep the list `a` sorted using `bisect_left`.
   - `l` is 3.
   - `ql` is an input integer minus `a[s - 1]`.

2. **Code Snippet:**
   ```python
   print(int(m), end=' ')
   ```

Given the initial state, we need to determine the value of `m` before it is printed. Let's assume the following for the sake of calculation (since specific values are not provided):

- Assume `b` is a list, and `s - 1` is an index within the list `b`.
- Assume `bd` is a list, and `s` is an index within the list `bd`.
- Assume `ad` is a list, and `s` is an index within the list `ad`.
- Assume `a` is a sorted list, and `s` is the correct index to insert `ql` to keep `a` sorted.
- Assume `ql` is an integer.

For simplicity, let's assume:
- `b = [2]`, so `b[s - 1] = 2`.
- `bd = [4]`, so `bd[s] = 4`.
- `ad = [2]`, so `ad[s] = 2`.
- `a = [1, 2, 3]`, so `a[s - 1] = 1` and `a[s] = 3`.
- `ql = 2`, so `ql - a[s - 1] = 2 - 1 = 1`.

Now, substituting these values into the formula for `m`:
\[ m = b[s - 1] + \frac{bd[s] \times (ql - a[s - 1])}{ad[s]} \]
\[ m = 2 + \frac{4 \times 1}{2} \]
\[ m = 2 + 2 \]
\[ m = 4 \]

Therefore, the `print(int(m), end=' ')` statement will print the integer value of `m`, which is 4.

Output: **4**