To determine the output of the given `print` statement, let's break down the initial state and the expression inside the `print` function.

### Initial State Recap:
- `a` is a list with elements `[first_value_from_r, second_value_from_r, ..., last_value_from_r, 2000000000.0]`.
- `u` is a non-zero value returned by `r()` minus 1.
- `t` is set to `False`.
- `b` is a list `[0, 0, accumulated_values_based_on_conditions]`.
- `c` is `return_value_1`.
- `d` is `return_value_2`.
- It is given that `c < d`.

### Expression Inside Print Statement:
The expression inside the `print` statement is:
```python
b[(d - 1) * 2] - b[(c - 1) * 2]
```

### Analysis:
1. **List `b`**: The list `b` is described as `[0, 0, accumulated_values_based_on_conditions]`. This means it has at least three elements, and the third element is some accumulated value based on certain conditions.
   
2. **Indices Calculation**:
   - `(d - 1) * 2`: Since `d` is an integer greater than `c` and `c` is at least 1 (as it's an index), `(d - 1) * 2` will be an even number. Given the structure of `b`, this index will point to either the first, second, or third element of `b` depending on the value of `d`.
   - `(c - 1) * 2`: Similarly, `(c - 1) * 2` will also be an even number and will point to one of the first, second, or third elements of `b` depending on the value of `c`.

3. **Possible Values of Indices**:
   - If `c = 1` and `d = 2`, then:
     - `(d - 1) * 2 = (2 - 1) * 2 = 2`
     - `(c - 1) * 2 = (1 - 1) * 2 = 0`
     - Therefore, the expression becomes `b[2] - b[0] = accumulated_values_based_on_conditions - 0 = accumulated_values_based_on_conditions`.
   - If `c = 1` and `d = 3`, then:
     - `(d - 1) * 2 = (3 - 1) * 2 = 4`
     - `(c - 1) * 2 = (1 - 1) * 2 = 0`
     - However, since `b` only has three elements, `b[4]` would be out of bounds. Thus, `d` cannot be 3 if `c` is 1 and `b` has only three elements.
   - If `c = 2` and `d = 3`, then:
     - `(d - 1) * 2 = (3 - 1) * 2 = 4`
     - `(c - 1) * 2 = (2 - 1) * 2 = 2`
     - Again, `b[4]` would be out of bounds, so this scenario is not valid either.

Given the constraints and the structure of `b`, the only valid scenario where both indices are within bounds is when `c = 1` and `d = 2`.

### Conclusion:
The expression `b[(d - 1) * 2] - b[(c - 1) * 2]` simplifies to `b[2] - b[0]` when `c = 1` and `d = 2`. Since `b[0]` is `0` and `b[2]` is `accumulated_values_based_on_conditions`, the result of the expression is `accumulated_values_based_on_conditions`.

Output: **accumulated_values_based_on_conditions (where accumulated_values_based_on_conditions is the third element of the list b)**