To determine the postcondition, we need to consider the negation of the if condition. The if condition checks whether `(a - b) % 2 > 0` or `(a - b) % 2 < 0`. The negation of this condition means that `(a - b) % 2` is not greater than 0 and not less than 0, which implies that `(a - b) % 2 == 0`.

Given the precondition, the postcondition should reflect that `t` is still an integer within the range \(1 \leq t \leq 10^4\), `a` and `b` are integers read from the input, at least one of `a` or `b` is odd, neither `2a == b` nor `2b == a`, and `(a - b) % 2 == 0`.

Postcondition: **`t` is an integer such that \(1 \leq t \leq 10^4\); `a` and `b` are integers read from the input; at least one of `a` or `b` is odd; neither `2a == b` nor `2b == a`; and `(a - b)` is even**