The code snippet `b[i] = b[i - 1] + x` updates the value of `b[i]` based on the previous value of `b[i - 1]` and the value of `x`. Given the initial state, `b[1]` is `x` and `b[2]` is `2 * x`. The value of `i` is 3, so `b[3]` will be updated to `b[2] + x`.

Since `b[2]` is `2 * x`, the new value of `b[3]` will be `2 * x + x = 3 * x`.

The values of `t`, `n`, `q`, `c`, `a`, `x`, and `i` remain unchanged.

Output State: **`t` is an integer such that 1 <= t <= 10^4; `n` is an integer such that 1 <= n <= 3 * 10^5; `q` is an integer such that 1 <= q <= 3 * 10^5; `c` is a list of `n` integers where each element is greater than 0 (1 <= c_i <= 10^9); `a` is a list of `n + 1` integers where the first element is 0 and the remaining `n` elements are the integers read from the input; `b` is a list of `n + 1` integers, with `b[1]` equal to `x`, `b[2]` equal to `2 * x`, and `b[3]` equal to `3 * x`; `i` is 3; `x` is 1 if `a[3] > 1` else 2.**