The value of `r` is assigned the value of `m`. According to the initial state, `m` is either `(r - 1) // 2` if `l = -1` or `(n - 1) // 2` if `l = (n - 1) // 2`. Since `r` is now equal to `m`, the condition for `m` remains unchanged. All other variables retain their initial states.

Output State: **`ans` is `f - s`, `f` is unknown, `s` is unknown, `l` is either `-1` or `(n - 1) // 2`, `n` is greater than 0, `m` is `(n - 1) // 2`, `r` is either `(r - 1) // 2` if `l = -1` or `(n - 1) // 2` if `l = (n - 1) // 2`, `r` is equal to `m`**