`b` is assigned the value `z // i * x`. Let's break down the steps:

1. From the initial state, we know:
   - \( z \% (i + 1) == 0 \)
   - \( a = i \times x \)
   - \( b = a / (i + 1) \)
   - Both \( a \) and \( b \) satisfy \( l \leq a \leq r \) and \( l \leq b \leq r \)
   - \( \mathit{math.gcd}(a, b) == x \)
   - \( a \times b // \mathit{math.gcd}(a, b) == y \)
   - The count is updated based on the comparison between \( a \) and \( b \)

2. After executing the line `b = z // i * x`, the new value of `b` is calculated using the formula provided.

Given the initial conditions, the updated value of `b` is `z // i * x`.

Output State: **`z` is at least 1; \( z \% (i + 1) == 0 \); \( a = i \times x \); \( b = z // i * x \); both \( a \) and \( b \) satisfy \( l \leq a \leq r \) and \( l \leq b \leq r \); \( \mathit{math.gcd}(a, b) == x \); \( a \times b // \mathit{math.gcd}(a, b) == y \); the count is updated based on the comparison between \( a \) and \( b \)**