Let's analyze the initial state and the conditions provided:

- `i` is 1.
- `a` and `b` are integers.
- If both `a` and `b` are even, then `a % 2 == 0 and b % 2 == 0` holds.
- Otherwise, at least one of `a` or `b` is odd.
- If `(a - b == -a, a)` or `(b - a == -b, b)` is true, then the respective condition holds.
- Otherwise, neither `(a - b == -a, a)` nor `(b - a == -b, b)` is true, and the difference `(a - b)` is either odd (not divisible by 2) or even (divisible by 2).

Given these conditions, the `print` statement is simply:

```python
print('yes')
```

This statement does not depend on any of the variables or conditions described in the initial state. It simply prints the string `'yes'`.

Therefore, the output is:

Output: **yes**