To determine the new state after executing the given code snippet, let's focus on the impact of the line:

```python
dp[i] = (dp[i - 1] + (i - 1) * dp[i - 2] * 2) % (10 ** 9 + 7)
```

Given the initial state, we know:
- `i` is 3
- `dp` is a list of length `m + 1` with all elements initialized to 0 except `dp[1]` which is 1 and `dp[2]` which is 3.

We need to compute `dp[3]` using the formula provided. Substituting `i = 3` into the formula:

```python
dp[3] = (dp[2] + (3 - 1) * dp[1] * 2) % (10 ** 9 + 7)
```

We know:
- `dp[2]` is 3
- `dp[1]` is 1

Substituting these values:

```python
dp[3] = (3 + (2) * 1 * 2) % (10 ** 9 + 7)
dp[3] = (3 + 4) % (10 ** 9 + 7)
dp[3] = 7 % (10 ** 9 + 7)
dp[3] = 7
```

Thus, `dp[3]` is updated to 7. All other variables remain unchanged.

Output State: **`t` is an integer such that 0 ≤ t ≤ 10^4; `n` is the first integer read from the input (1 ≤ n ≤ 3 · 10^5); `k` is the second integer read from the input (0 ≤ k ≤ n); each of the next k lines contains two integers r_i and c_i, denoting the i-th move you made, where 1 ≤ r_i, c_i ≤ n; the sum of n over all test cases does not exceed 3 · 10^5; `num` is the sum of 1 for each iteration where `c == r` and 2 for each iteration where `c != r`; `i` is 3; `m` is at least 3; `m` is not equal to 1; `dp` is a list of length `m + 1` with all elements initialized to 0 except `dp[1]` which is 1, `dp[2]` which is 3, and `dp[3]` which is 7.**