The code snippet `r -= 1` decrements the value of `r` by 1. Given the initial state, `r` is initially `n - 2`. After the decrement, `r` becomes `n - 3`.

The other variables remain unchanged. Therefore, the output state is:

Output State: **`t` is an integer such that \(1 \leq t \leq 10^4\); `n` is the length of the list `a`; `a` is the list of integers where `a[n - 1] == a[n - 2]`; `le` is the length of the list `a`; `l` is `n - 3`; `r` is `n - 3`; `st` is `n - 1`; `end` is `2`; `ans` is `0` if `a[0]` is equal to `a[-1]`, otherwise `ans` is `1`.**