Postcondition: **`info` is a new list of substrings based on the user's input, `b` is at least 1, `T` is greater than 0, `a` is the integer value of `info[0]`, `i` is `b + 1`, `suma` is \(\left(\frac{a - b^2 - b}{b^2 + 2b + 1}\right) + 1\), `x` is \(\left(\frac{a - b^2 - b}{b^2 + 2b + 1}\right) + 1\). Additionally, \((a - i * (i - 1)) % i ** 2 == 0\) and \(i * (i - 1) % i ** 2 == 0\)**

This postcondition retains all the conditions of the precondition and includes the additional constraints imposed by the if condition.