Let's break down the initial state and the code snippet step by step to determine what will be printed.

### Initial State:
1. `i` is incremented by the length of `array`.
2. `l` is an input integer.
3. `s` is a list of length `l` with elements at the indices specified by `array` incremented by the number of times each index appears in `array`, and all other elements still initialized to 0.
4. `array` is a list of integers provided by the user.
5. `ans` is a string containing the characters corresponding to the ASCII values of the elements in `s` at the indices specified by `array` plus 97, concatenated in the order the indices appear in `array`.

### Step-by-Step Analysis:
1. **Incrementing `i`**:
   - `i` is incremented by the length of `array`. However, `i` is not used in the `print` statement, so it does not affect the output.

2. **Creating the list `s`**:
   - `s` is a list of length `l` initialized to all zeros.
   - For each index `j` in `array`, the element at `s[j]` is incremented by the number of times `j` appears in `array`.

3. **Generating the string `ans`**:
   - For each index `j` in `array`, the corresponding element in `s` is used to generate an ASCII value.
   - The ASCII value is `s[j] + 97`.
   - The character corresponding to this ASCII value is added to the string `ans`.
   - This process is repeated for each index in `array`, and the characters are concatenated in the order the indices appear in `array`.

### Example to Illustrate:
Let's assume:
- `array = [0, 1, 0, 2]`
- `l = 3`

1. **Initialize `s`**:
   - `s = [0, 0, 0]`

2. **Increment elements in `s`**:
   - `array[0] = 0` -> `s[0] += 1` -> `s = [1, 0, 0]`
   - `array[1] = 1` -> `s[1] += 1` -> `s = [1, 1, 0]`
   - `array[2] = 0` -> `s[0] += 1` -> `s = [2, 1, 0]`
   - `array[3] = 2` -> `s[2] += 1` -> `s = [2, 1, 1]`

3. **Generate `ans`**:
   - `array[0] = 0` -> `s[0] = 2` -> ASCII value = 2 + 97 = 99 -> character = 'c'
   - `array[1] = 1` -> `s[1] = 1` -> ASCII value = 1 + 97 = 98 -> character = 'b'
   - `array[2] = 0` -> `s[0] = 2` -> ASCII value = 2 + 97 = 99 -> character = 'c'
   - `array[3] = 2` -> `s[2] = 1` -> ASCII value = 1 + 97 = 98 -> character = 'b'

   - `ans = 'c' + 'b' + 'c' + 'b' = 'cbcb'`

### General Case:
- The string `ans` will be constructed by taking the elements of `s` at the indices specified by `array`, adding 97 to each of these elements to get the corresponding ASCII value, and then converting these ASCII values to characters.
- The characters are concatenated in the order the indices appear in `array`.

### Final Output:
Output: **ans (where ans is a string containing the characters corresponding to the ASCII values of the elements in `s` at the indices specified by `array` plus 97, concatenated in the order the indices appear in `array`)**