Let's break down the initial state and the calculation step by step:

1. **Initial Values:**
   - `i` is 3.
   - `n` is greater than 0 (though its exact value is not specified, it doesn't affect the calculation directly).
   - `l` is 2.
   - `r` is 2.
   - `a` is defined as `B[1] + (idx_B[1] - 3) * 2`.
     - Since `idx_B[1]` is not explicitly defined, let's assume it is a value such that the expression evaluates correctly. For simplicity, let's assume `idx_B[1] = 3` (since `B[1]` is used, and indices are usually zero-based, this makes sense).
     - Therefore, `a = B[1] + (3 - 3) * 2 = B[1] + 0 = B[1]`.
   - `b` is defined as `A[1] - A[-2] + (3 - idx_A[1]) * 2`.
     - Similarly, since `idx_A[1]` is not explicitly defined, let's assume it is a value such that the expression evaluates correctly. For simplicity, let's assume `idx_A[1] = 1` (since `A[1]` is used, and indices are usually zero-based, this makes sense).
     - Therefore, `b = A[1] - A[-2] + (3 - 1) * 2 = A[1] - A[-2] + 4`.

2. **Expression Calculation:**
   - The expression to be printed is `a * 2 + b * 2 + (n - i)`.
   - Substituting the values we have:
     - `a = B[1]`
     - `b = A[1] - A[-2] + 4`
     - `n - i = n - 3`

3. **Final Expression:**
   - The expression becomes `2 * B[1] + 2 * (A[1] - A[-2] + 4) + (n - 3)`.
   - Simplifying further: `2 * B[1] + 2 * A[1] - 2 * A[-2] + 8 + n - 3 = 2 * B[1] + 2 * A[1] - 2 * A[-2] + n + 5`.

Given the initial state and the assumptions made, the final output is:

Output: **2 * B[1] + 2 * A[1] - 2 * A[-2] + n + 5**