
Given a Python loop, an initial execution state, and the output states after the first 3 iterations of the loop, determine the output state after all the executions of the loop have finished. 

You must adhere to the text format: Output State: **output state.**

Initial State: `i` is equal to `n-1`, `j` is 4, `l` is 0, `n` must be greater than 0, `A` is a list of integers, `idx_A` is a list of all indices in `s` where the character is '>', in the order they appear, `B` is a list of integers, `idx_B` is a list of all indices in `s` where the character is '<', in the order they appear, and `idx_B` contains all the indices `i` where `s[i] == '<', `r` is the length of list `B`
Code of the loop:
for i in range(0, n):
    if s[i] == '>':
        if l < r:
            a = A[l]
            x = r - (l + 2)
            b = B[r - 1]
            if x >= 0:
                b = b - B[x]
                b = b - (idx_B[x] - idx_B[r - 1]) * (x + 1)
            b = (idx_B[r - 1] - i) * (l + 1)
            print(a * 2 + b * 2 + i + 1, end=' ')
        elif r == 0:
            print(n - i, end=' ')
        else:
            a = B[r - 1] + (idx_B[r - 1] - i) * r
            b = A[l - 1]
            if l - r > 0:
                b = b - A[l - r - 1]
                b = b - (idx_A[l - 1] - idx_A[l - r - 1]) * (l - r)
            b = b + (i - idx_A[l - 1]) * r
            print(a * 2 + b * 2 + (n - i), end=' ')
        l += 1
    else:
        r -= 1
        if l <= r:
            if l == 0:
                print(i + 1, end=' ')
            else:
                a = A[l - 1]
                a = a + (i - idx_A[l - 1]) * l
                b = B[r]
                if r - l >= 0:
                    b = b - B[r - l]
                    b = b - (idx_B[r - l] - i) * (r - l)
                b = b + (idx_B[r] - i) * l
                print(a * 2 + b * 2 + i + 1, end=' ')
        elif r == 0:
            print(n - i + (i - idx_A[l - 1]) * 2, end=' ')
        else:
            a = B[r]
            b = A[l - 1]
            if l - r - 1 > 0:
                b = b - A[l - r - 2]
                b = b - (idx_A[l - 1] - idx_A[l - r - 2]) * (l - r - 1)
            b = b + (i - idx_A[l - 1]) * (r + 1)
            print(a * 2 + b * 2 + (n - i), end=' ')


The output state after the loop executes the first 3 of times includes what needed to be true for the loop to execute at least that number of times:

Output State after the loop executes 1 time: Postcondition: `i` is less than `n`, `n` is greater than 0, and the character at index `i` in string `s` is either '>' or not '>'. If the character is '>', `l` is increased by 1, `a` is updated to `A[l]` if `l < r`, and `x` is greater than or equal to 0. Additionally, `b` is updated according to the following rules: if `l < r`, `b` is set to `(idx_B[r - 1] - i) * (l + 1)`, and if `l - r > 0` and `r` is not 0, `b` is further updated to `b + (i - idx_A[l - 1]) * r`. If the character is not '>', and `l` is 0, `a` and `b` remain unchanged. Otherwise, `a` is updated to `ord(a) + (i - idx_A[l - 1]) * l` and `b` is updated to `b + (idx_B[r] - i) * l` if `r - l` is non-negative. If `l - r - 1 > 0`, `a` is updated to `B[r]` and `b` is updated to `b + (i - idx_A[l - 1]) * (r + 1)`. If `l - r - 1 <= 0`, the values of `a` and `b` remain unchanged.

**Output State after the loop executes 2 times**: Postcondition: `i` is incremented by 1, `n` is greater than 0. If `s[i]` equals '>', then `l` is incremented by 1, and depending on the value of `l` relative to `r`:
- If `l < r`, then `a` is the value of `A[l]`, `x` is `r - (l + 2)`, and `b` is the value of `(idx_B[r - 1] - i) * (l + 1)` if `x >= 0`. If `r` is 0, no additional variables are changed. If `r` is not 0, then `a` is set to `B[r - 1] + (idx_B[r - 1] - i) * r`, and `b` is set to `A[l - r - 1] - (idx_A[l - 1] - idx_A[l - r - 1]) * (l - r) + (i - idx_A[l - 1]) * r`.
- If `s[i]` does not equal '>', then `r` is decremented by 1. If `l` is 0, the postcondition remains as `i` is incremented by 1, `n` is greater than 0, and `r` is decremented by 1. Otherwise, `a` is the value of `A[l - 1] + (i - idx_A[l - 1]) * l`, and `b` is the value of `B[r - l] - (idx_B[r - l] - i) * (r - l) + (idx_B[r] - i) * l`. If `l - r - 1 > 0`, then `b` is updated to `b + (i - idx_A[l - 1]) * (r + 1)`, otherwise `b` remains unchanged.

**Output State after the loop executes 3 times**: Postcondition: `i` is 3, `n` is greater than 0, `l` is either 2 or 3, `r` is either 1 or 2, `a` is either 8 or 1 depending on whether `l` is not 0, and `b` is either -12 or -15 if `l` is not 0, otherwise `b` is -1.




What is the ouput state after the loop executes all the iterations? Change the values of only the variables in the loop head and body.The state of the other variables in the precondition that are not affected by the loop head and body must remain unchanged.
In your response strictly use the format: Output State: **the output state you calculate.**, and describe this output state in Natural language easily understandable by humans.

