The code snippet `y2 -= d2` updates the value of `y2` by subtracting `d2` from it. Let's analyze the impact:

1. **Initial Values:**
   - `y1 = y1max - d1`
   - `y2 = y2max`
   - `d1` is 1 if `y1 < y2`, otherwise 0.
   - `d2` is 0 if `y1 < y2`, otherwise 1.

2. **Impact of the Code:**
   - If `y1 < y2`, then `d2` is 0, so `y2 -= d2` does not change `y2`.
   - If `y1 >= y2`, then `d2` is 1, so `y2 -= d2` decreases `y2` by 1.

3. **Final Values:**
   - If `y1 < y2`, then `y2` remains `y2max`.
   - If `y1 >= y2`, then `y2` becomes `y2max - 1`.

4. **Unchanged Variables:**
   - `t1, t2, y1max, t0, dt1, dt2, calc1max, calc2max, y1, y1out, y2out, errMin` remain unchanged.

Therefore, the output state is:
Output State: **`t1, t2, y1max, t0, dt1, dt2, calc1max, calc2max, y1, y1out, y2out, errMin` remain unchanged; if `y1 < y2`, then `y2` is `y2max`; otherwise, `y2` is `y2max - 1`.**