Let's analyze the given code snippet and determine the new state of the variables after its execution.

The code snippet is:
```python
t = t + t2 // 15
```

From the initial state, we know:
- `t` is either `b // 2` or `b // 2 + 1` depending on whether `b % 2 == 0` or not.
- `t2` is `a - t1`.

We need to compute the new value of `t` after executing the given line of code.

Given:
- `t1` is `(b // 2) * 15 - b * 4` if `b % 2 == 0`
- `t1` is `((b // 2) + 1) * 15 - b * 4` if `b % 2 != 0`
- `t2` is `a - t1`
- `t` is updated to `t + t2 // 15`

Let's consider both cases for `t`:

### Case 1: `b % 2 == 0`
- `t = b // 2`
- `t1 = (b // 2) * 15 - b * 4`
- `t2 = a - ((b // 2) * 15 - b * 4)`
- `t = t + t2 // 15 = (b // 2) + (a - ((b // 2) * 15 - b * 4)) // 15`

### Case 2: `b % 2 != 0`
- `t = b // 2 + 1`
- `t1 = ((b // 2) + 1) * 15 - b * 4`
- `t2 = a - (((b // 2) + 1) * 15 - b * 4)`
- `t = t + t2 // 15 = (b // 2 + 1) + (a - (((b // 2) + 1) * 15 - b * 4)) // 15`

Since the exact values of `a` and `b` are not specified, we cannot simplify further without specific values. However, we can express the new value of `t` in terms of `a` and `b`.

### Final Output State:
The value of `t` is updated based on the above expressions. All other variables remain unchanged.

Output State: **`a` is an integer; `b` is an integer representing the second input value; `x` and `y` are integers such that 0 ≤ x, y ≤ 99; `n` is greater than 0; `i` is `i_end + 2`; If `b % 2 == 0`, then `t` is `(b // 2) + (a - ((b // 2) * 15 - b * 4)) // 15` and `t1` is `(b // 2) * 15 - b * 4`; Otherwise, `t` is `(b // 2 + 1) + (a - (((b // 2) + 1) * 15 - b * 4)) // 15` and `t1` is `((b // 2) + 1) * 15 - b * 4`; `t2` is `a - t1`.**