To determine what will be printed, let's break down the initial state and the code step by step:

### Initial State:
1. `s` is the second element of the list created from the second line onward of the standard input.
2. `a` is an integer obtained from splitting and converting the string `s`.
3. `b` is now equal to the original value of `b` plus the value of `c` before the assignment, plus the current value of `c`.
4. `c` is an integer obtained from splitting and converting the string `s`.

### Code Snippet:
```python
print((a - -b // 3, -1)[c < b % 3])
```

### Step-by-Step Analysis:
1. **Determine the value of `s`:**
   - `s` is the second element of the list created from the second line onward of the standard input. For example, if the input is:
     ```
     line1
     line2
     line3
     ```
     Then `s` would be "line2".

2. **Determine the values of `a` and `c`:**
   - `a` and `c` are integers obtained from splitting and converting the string `s`.
   - For example, if `s = "10 20"`, then `a = 10` and `c = 20`.

3. **Determine the value of `b`:**
   - `b` is now equal to the original value of `b` plus the value of `c` before the assignment, plus the current value of `c`.
   - Let's assume the original value of `b` is `b_original`.
   - Before the assignment, `c` is some value, say `c_before`.
   - After the assignment, `c` is the new value, say `c_new`.
   - Therefore, `b = b_original + c_before + c_new`.

4. **Evaluate the expression `(a - -b // 3, -1)[c < b % 3]`:**
   - First, compute `b % 3`:
     - `b % 3` is the remainder when `b` is divided by 3.
   - Next, evaluate the condition `c < b % 3`:
     - If `c < b % 3`, the expression evaluates to `-1`.
     - Otherwise, it evaluates to `a - -b // 3`.

5. **Compute `a - -b // 3`:**
   - `a - -b // 3` simplifies to `a + b // 3` because `--b` is equivalent to `b`.

### Example Calculation:
Let's assume the input is:
```
line1
10 20
line3
```
- `s = "10 20"`
- `a = 10`
- `c = 20`
- Assume `b_original = 5` and `c_before = 15` (for illustration purposes).

Then:
- `b = 5 + 15 + 20 = 40`
- `b % 3 = 40 % 3 = 1`
- `c < b % 3` becomes `20 < 1`, which is `False`.

So, the expression `(a - -b // 3, -1)[c < b % 3]` evaluates to `a + b // 3`:
- `b // 3 = 40 // 3 = 13`
- `a + b // 3 = 10 + 13 = 23`

### Final Output:
Output: **23**