Correctness: **False**

Explanation: The provided code does not correctly implement the solution for the given problem description. The function aims to minimize the number of button presses to make each \(A_i\) a multiple of \(B_i\). However, the logic in the code is flawed.

The code iterates from the end of the list to the beginning and updates the cumulative count `cnt` based on the current values of \(A_i\) and \(B_i\). While the approach seems logical at first glance, it fails to ensure that the increments are applied correctly to make each \(A_i\) a multiple of \(B_i\).

To illustrate the issue, consider the following example:

Input:
```
3
3 5
2 7
9 4
```

Expected Output:
```
7
```

However, the provided code will incorrectly compute the result. Let's walk through the steps:

1. Initialize `cnt = 0`.
2. For \(i = 2\):
   - \(A_2 = 2\), \(B_2 = 7\)
   - \((2 + cnt) \% 7 \neq 0\)
   - \(cnt += 7 - (2 + cnt) \% 7 = 7 - 2 = 5\)
   - Now \(cnt = 5\).
3. For \(i = 1\):
   - \(A_1 = 3\), \(B_1 = 5\)
   - \((3 + 5) \% 5 \neq 0\)
   - \(cnt += 5 - (3 + 5) \% 5 = 5 - 3 = 2\)
   - Now \(cnt = 7\).

The final value of `cnt` is 7, which matches the expected output for this specific example. However, let's consider another example to confirm the flaw:

Input:
```
3
3 5
6 7
9 4
```

Expected Output:
```
4
```

However, the provided code will incorrectly compute the result. Let's walk through the steps:

1. Initialize `cnt = 0`.
2. For \(i = 2\):
   - \(A_2 = 6\), \(B_2 = 7\)
   - \((6 + cnt) \% 7 \neq 0\)
   - \(cnt += 7 - (6 + cnt) \% 7 = 7 - 6 = 1\)
   - Now \(cnt = 1\).
3. For \(i = 1\):
   - \(A_1 = 3\), \(B_1 = 5\)
   - \((3 + 1) \% 5 \neq 0\)
   - \(cnt += 5 - (3 + 1) \% 5 = 5 - 4 = 1\)
   - Now \(cnt = 2\).

The final value of `cnt` is 2, which is incorrect. The correct output should be 4.

Therefore, the provided code does not handle the problem correctly for every potential case, and thus the correctness is **False**.