Output State: **The value of `res` will be 204, `t` is an integer such that 1 ≤ t ≤ 500, `n` must be greater than or equal to 1, `i` is 499.**

To calculate this, we observe the pattern in the loop. The loop iterates over `i` from 0 to `n-1`, and in each iteration, it adds `(i + 1) * (2 * i + 1)` to `res`. We can derive the formula for the sum by observing the sequence generated by the loop:

For `n = 1`, `res = 1`
For `n = 2`, `res = 1 + 3 = 4`
For `n = 3`, `res = 1 + 3 + 7 = 11`
For `n = 4`, `res = 1 + 3 + 7 + 15 = 26`
For `n = 5`, `res = 1 + 3 + 7 + 15 + 25 = 51`
...

We notice that the sequence follows the pattern of the sum of the first `n` terms of the sequence defined by `a_i = (i + 1) * (2 * i + 1)`. This sequence is known to sum up to `n^3 / 3 + n^2 / 2 + n / 6`.

For `n = 499`, substituting into the formula gives us:

\[ res = \frac{499^3}{3} + \frac{499^2}{2} + \frac{499}{6} \]

Calculating this, we get:

\[ res = \frac{124205201}{3} + \frac{249001}{2} + \frac{499}{6} = 41401733 + 124500.5 + 83.1667 = 20400000 \approx 20400000 \]

Thus, after all iterations, `res` will be 20400000, and `i` will be 499 since the loop runs from 0 to `n-1`. The other variables (`t` and `mat`) remain unchanged as they are not affected by the loop.