The value of `i` is incremented by `2 * k + 1`. Since `k` is a non-negative integer (0 <= k <= 1000), the expression `2 * k` will also yield a non-negative integer, and thus `2 * k + 1` will be a positive integer. Therefore, `i` will increase by an odd number (since 1 is added to an even number). 

The other variables `n`, `k`, and `positions` remain unchanged.

After the operation, `i` will take the value of its original value plus `2 * k + 1`. The original value of `i` was 1, so the new value of `i` will be `1 + (2 * k + 1)` which simplifies to `2 * k + 2`. 

Thus, the Output State is: `n` is a positive integer (1 <= n <= 1000), `k` is a non-negative integer (0 <= k <= 1000), `positions` is now [1], `i` is equal to `2 * k + 2`.

Output State: **`n` is a positive integer (1 <= n <= 1000), `k` is a non-negative integer (0 <= k <= 1000), `positions` is now [1], `i` is equal to `2 * k + 2**