The code assigns a value to `sum_k`, which is calculated using the formula `k * (k + 1) // 2`. The value of `k` is equal to `a + b - 1`. Given the constraints that `a` and `b` are both positive integers, `k` will also be a positive integer (since it is the sum of two positive integers minus one). The calculation of `sum_k` does not change the values of `a`, `b`, `g`, or `m`, but it determines the value of `sum_k` based on `k`.

Since we don't have specific values for `a` and `b`, we can express `sum_k` in terms of these variables.

Therefore, the Output State is: `m` is a positive integer such that 1 <= m <= 10^9; `a` is a positive integer such that 1 <= a <= 10^5; `b` is a positive integer such that 1 <= b <= 10^5; `g` is equal to 1; `k` is equal to `a + b - 1`; `m` is greater than or equal to `k`; `sum_k` is equal to `k * (k + 1) // 2`.

Output State: **`m` is a positive integer such that 1 <= m <= 10^9; `a` is a positive integer such that 1 <= a <= 10^5; `b` is a positive integer such that 1 <= b <= 10^5; `g` is equal to 1; `k` is equal to `a + b - 1`; `m` is greater than or equal to `k`; `sum_k` is equal to `(a + b - 1) * (a + b) // 2`.**