Correctness: **False**

The provided program does not correctly implement the required functionality. Specifically, there are a few issues with the logic inside the `func_1` function:

1. The initial value of `ans[0]` is set to `arr[0] + 1`, which is incorrect because `a_1` can be any value between 1 and \(10^9\), and it doesn't have to be related to `x_2` (which is `arr[0]`).

2. The loop that calculates the values of `ans` from `ans[1]` to `ans[n-2]` is flawed. The condition `if ans[i + 1] < arr[i + 1]:` is unnecessary and the loop `while ans[i + 1] <= arr[i + 1]:` can lead to incorrect results because it doesn't guarantee that `ans[i + 1] % ans[i]` will equal `arr[i + 1]`.

3. The final element `ans[-1]` is calculated as `ans[-2] + arr[-1]`, which is not necessarily correct. It should be such that `ans[-1] % ans[-2] == arr[-1]`.

Here is a corrected version of the `func_1` function:

```python
def func_1(arr, n):
    ans = [0] * n
    ans[0] = arr[0] + 1  # a_1 can be any value greater than x_2, here we choose x_2 + 1
    for i in range(1, n - 1):
        ans[i] = ans[i - 1] + arr[i]  # a_i should be such that a_i % a_(i-1) == x_i
    ans[-1] = ans[-2] + arr[-1]  # a_n should be such that a_n % a_(n-1) == x_n
    return ans
```

However, a more robust solution would be:

```python
def func_1(arr, n):
    ans = [0] * n
    ans[0] = 1 + max(arr)  # a_1 can be any value greater than the maximum x_i
    for i in range(1, n):
        ans[i] = ans[i - 1] + arr[i - 1]  # a_i should be such that a_i % a_(i-1) == x_i
    return ans
```

This ensures that `a_1` is large enough and that each subsequent `a_i` satisfies the required modulo condition.