The value of `numerator` is multiplied by `total_days - i`. Given that `total_days` is `2^n` and `i` is `1`, we can calculate:

- `total_days - i = 2^n - 1`
- Therefore, `numerator` becomes `numerator * (2^n - 1)`.

Since `numerator` is initially `2^n`, the new value of `numerator` will be:

- `numerator = 2^n * (2^n - 1) = 2^(2n) - 2^n`.

The values of the other variables (`total_days`, `denominator`, and `i`) remain unchanged.

Output State: **`n` is an integer such that 1 ≤ n ≤ 10^18, `k` is an integer such that 2 ≤ k ≤ 10^18, `total_days` is 2^n, `numerator` is 2^(2n) - 2^n, `denominator` is 2^n, `i` is 1**