The code `b = n - x` assigns the value of `n - x` to `b`. Based on the initial state, `n` is the first element of the list `L`, `x` is the second element of the list `L`, and no changes are made to `n`, `x`, `res`, or `a`. Therefore, `b` is now equal to `n - x`.

Output State: **`N` is an integer such that \(2 \leq N \leq 10^{12}\); `X` is an integer such that \(1 \leq X \leq N-1\); `n` is equal to the first element of the list `L`; `x` is equal to the second element of the list `L`; `res` is equal to `n`; `a` is equal to `x`; `b` is equal to `n - x`**