Step-by-step analysis:

1. The initial state includes:
   - `N` is an integer such that \(2 \leq N \leq 10^{12}\)
   - `X` is an integer such that \(1 \leq X \leq N-1\)
   - `n` is equal to the first element of the list `L`
   - `x` is equal to the second element of the list `L`
   - `res` is equal to `n`
   - `a` is equal to `x`
   - `b` is equal to `n - x`
   - `flag` is `True`
   - `q` is equal to `(n - x) // x`

2. The code snippet `b -= q * a` updates the value of `b` by subtracting `q * a` from its current value.

3. From the initial state, we know:
   - `b` is equal to `n - x`
   - `a` is equal to `x`
   - `q` is equal to `(n - x) // x`

4. Substituting these values into the operation `b -= q * a`:
   - `b -= (n - x) // x * x`
   - Since `(n - x) // x * x` is equivalent to `n - x` (assuming `n - x` is exactly divisible by `x` or considering integer division behavior),
   - This simplifies to `b -= (n - x)`.

5. After the operation, `b` will be updated to `b - (n - x)`.

6. Therefore, the new value of `b` will be `b - (n - x)`.

Output State: **`N` is an integer such that \(2 \leq N \leq 10^{12}\), `X` is an integer such that \(1 \leq X \leq N-1\), `n` is equal to the first element of the list `L`, `x` is equal to the second element of the list `L`, `res` is equal to `n`, `a` is equal to `x`, `b` is equal to `b - (n - x)`, `flag` is `True`, `q` is equal to `(n - x) // x`**.