To determine the output state after the loop executes all the iterations, we need to understand the behavior of the loop given the initial state and the loop code. However, the variable `n` and the string `s` are not provided in the initial state, so we need to make some assumptions to proceed with the analysis.

Let's assume `n` is the length of the string `s` and `s` is a string of `>` and `<` characters. For the sake of this example, let's assume `s` is `">>>>"` and `n` is 4.

Given:
- `A` is [0, 1, 3, 12]
- `idx_A` is [1, 2, 3, 6]
- `B` is [0, 1, 3, 6]
- `idx_B` is [3, 2, 1, 0]
- `l` is 0
- `r` is 4
- `s` is `">>>>"` (assumption)
- `n` is 4 (assumption)

We will now walk through the loop iterations:

### Iteration 1 (i = 0):
- `s[0]` is `>`
- `l` is 0, `r` is 4
- `a = A[0] = 0`
- `x = 4 - (0 + 2) = 2`
- `b = B[3] = 6`
- `b = 6 - B[2] = 6 - 3 = 3`
- `b = 3 - (idx_B[2] - idx_B[3]) * (2 + 1) = 3 - (1 - 0) * 3 = 0`
- `b = (idx_B[3] - 0) * (0 + 1) = 3 * 1 = 3`
- Print `0 * 2 + 3 * 2 + 0 + 1 = 7`
- `l` is incremented to 1

### Iteration 2 (i = 1):
- `s[1]` is `>`
- `l` is 1, `r` is 4
- `a = A[1] = 1`
- `x = 4 - (1 + 2) = 1`
- `b = B[3] = 6`
- `b = 6 - B[1] = 6 - 1 = 5`
- `b = 5 - (idx_B[1] - idx_B[3]) * (1 + 1) = 5 - (2 - 0) * 2 = 1`
- `b = (idx_B[3] - 1) * (1 + 1) = 3 * 2 = 6`
- Print `1 * 2 + 6 * 2 + 1 + 1 = 16`
- `l` is incremented to 2

### Iteration 3 (i = 2):
- `s[2]` is `>`
- `l` is 2, `r` is 4
- `a = A[2] = 3`
- `x = 4 - (2 + 2) = 0`
- `b = B[3] = 6`
- `b = 6 - B[0] = 6 - 0 = 6`
- `b = 6 - (idx_B[0] - idx_B[3]) * (0 + 1) = 6 - (3 - 0) * 1 = 3`
- `b = (idx_B[3] - 2) * (2 + 1) = 3 * 3 = 9`
- Print `3 * 2 + 9 * 2 + 2 + 1 = 28`
- `l` is incremented to 3

### Iteration 4 (i = 3):
- `s[3]` is `>`
- `l` is 3, `r` is 4
- `a = A[3] = 12`
- `x = 4 - (3 + 2) = -1` (x is not used in calculations as it's not >= 0)
- `b = B[3] = 6`
- `b = (idx_B[3] - 3) * (3 + 1) = 3 * 4 = 12`
- Print `12 * 2 + 12 * 2 + 3 + 1 = 55`
- `l` is incremented to 4

After all iterations, the values of `A`, `idx_A`, `B`, `idx_B` remain unchanged, and `l` is now 4, `r` is 4.

Output State: **A is [0, 1, 3, 12], idx_A is [1, 2, 3, 6], B is [0, 1, 3, 6], idx_B is [3, 2, 1, 0], l is 4, r is 4.**