The value of `k` is calculated as \((m ** 2 - n ** 2) ** 0.5\). Given that `m` is `n + 1`, we can substitute `m` in the equation:

\[ k = ((n + 1)^2 - n^2) ** 0.5 \]

Expanding the square:

\[ k = (n^2 + 2n + 1 - n^2) ** 0.5 \]

Simplifying the expression inside the square root:

\[ k = (2n + 1) ** 0.5 \]

Since `n` is an integer, \(2n + 1\) is also an integer, and taking the square root of an integer will result in a floating-point number unless \(2n + 1\) is a perfect square. However, the exact value of `k` is not specified further, but it is computed from the given formula.

Therefore, the Output State is: `n` is an input integer such that \(1 \leq n \leq 10^9\) and `n` is not equal to 1, `m` is `n + 1`, `k` is \((2n + 1) ** 0.5\).

Output State: **`n` is an input integer such that \(1 \leq n \leq 10^9\) and `n` is not equal to 1, `m` is `n + 1`, `k` is \((2n + 1) ** 0.5\)**.