The value of `k` is updated to the square root of the difference between `m` squared and `n` squared. Given that `m` is `n + 2` and `k` was initially `2n + 1`, the new value of `k` is calculated as follows:

\[ k = ((n + 2)^2 - n^2)^{0.5} \]
\[ k = ((n^2 + 4n + 4) - n^2)^{0.5} \]
\[ k = (4n + 4)^{0.5} \]
\[ k = (4(n + 1))^{0.5} \]
\[ k = 2\sqrt{n + 1} \]

Therefore, the new value of `k` is \(2\sqrt{n + 1}\).

Output State: **`n` is an input integer such that \(1 \leq n \leq 10^9\) and `n` is not equal to 1, `m` is `n + 2`, `k` is \(2\sqrt{n + 1}\)**