To solve this, we need to analyze the given loop and its behavior based on the provided initial state and the output states after a few iterations. Let's break it down step by step.

### Step 1: Analyze the Code and Initial State
- **Initial State**: `n` is an input integer such that \(1 \leq n \leq 10^9\) and `n` is not equal to 1.
- **Loop**: The loop iterates over `m` starting from `n` up to \(10^{18} + 1\).
- **Inside the Loop**:
  - Calculate \( k = \sqrt{m^2 - n^2} \).
  - Check if `k` is an integer.
  - If `k` is an integer, print `(m, int(k) + n)` and break out of the loop.
  - If the loop completes without finding an integer `k`, print `-1`.

### Step 2: Track Variable Changes
- **Invariant Variables**:
  - `n` remains constant throughout the loop.
- **Variables that Change**:
  - `m` starts at `n` and increments by 1 each iteration.
  - `k` is calculated as \( \sqrt{m^2 - n^2} \).

### Step 3: Summarize the Loop Behavior
- The loop will continue until it finds an `m` such that \( k = \sqrt{m^2 - n^2} \) is an integer.
- If no such `m` is found within the range, the loop will complete and print `-1`.

### Step 4: Verify Relationships
- **First Iteration**:
  - `m = n`
  - \( k = \sqrt{n^2 - n^2} = 0 \)
  - Since `k` is an integer, the loop prints `(n, n)` and breaks.
- **Second Iteration**:
  - `m = n + 1`
  - \( k = \sqrt{(n + 1)^2 - n^2} = \sqrt{n^2 + 2n + 1 - n^2} = \sqrt{2n + 1} \)
  - For `k` to be an integer, \( 2n + 1 \) must be a perfect square.
- **Third Iteration**:
  - `m = n + 2`
  - \( k = \sqrt{(n + 2)^2 - n^2} = \sqrt{n^2 + 4n + 4 - n^2} = \sqrt{4n + 4} = 2\sqrt{n + 1} \)
  - For `k` to be an integer, \( 4n + 4 \) must be a perfect square, i.e., \( n + 1 \) must be a perfect square.

### Final Output State
- **Conditions for Execution**:
  - The loop will find an `m` such that \( k = \sqrt{m^2 - n^2} \) is an integer and print `(m, int(k) + n)`.
  - If no such `m` is found within the range, the loop will print `-1`.

- **Final Values of Variables**:
  - `n` remains unchanged.
  - `m` will be the value where \( k = \sqrt{m^2 - n^2} \) is an integer.
  - `k` will be an integer when the condition is met.

### Conclusion
Output State: **If an integer `k` is found, the loop prints `(m, int(k) + n)` and breaks. If no such `m` is found within the range, the loop prints `-1`.**