### Reasoning:

Let's carefully analyze the problem and the provided program step-by-step.

#### Problem Recap:
The goal is to maximize the sum of all elements in an \( n \times n \) matrix using the following operations:
1. **Type 1 Operation**: Choose a row \( i \) and a permutation \( p_1, p_2, \ldots, p_n \) of integers from 1 to \( n \). Assign \( a_{i, j} := p_j \) for all \( 1 \leq j \leq n \).
2. **Type 2 Operation**: Choose a column \( i \) and a permutation \( p_1, p_2, \ldots, p_n \) of integers from 1 to \( n \). Assign \( a_{j, i} := p_j \) for all \( 1 \leq j \leq n \).

The constraints are:
- No more than \( 2n \) operations.
- Each test case contains a single integer \( n \) (1 ≤ \( n \) ≤ 500).
- The sum of \( n^2 \) over all test cases does not exceed \( 5 \cdot 10^5 \).

#### Program Analysis:
The provided program calculates the sum and prints the operations as follows:

```python
def func():
    t = int(input())
    for _ in range(t):
        n = int(input())
        sum = 1
        for i in range(2, n + 1):
            sum += (i * i - (i - 1) * (i - 1)) * i
        print(sum, n + n)
        for j in range(1, n + 1):
            print(1, n - j + 1, *range(1, n + 1))
            print(2, n - j + 1, *range(1, n + 1))
```

#### Detailed Breakdown:
1. **Sum Calculation**:
   - The sum is calculated as \( 1 + \sum_{i=2}^{n} (i^2 - (i-1)^2) \cdot i \).
   - Simplifying the term inside the summation: \( i^2 - (i-1)^2 = i^2 - (i^2 - 2i + 1) = 2i - 1 \).
   - Thus, the sum becomes \( 1 + \sum_{i=2}^{n} (2i - 1) \cdot i = 1 + \sum_{i=2}^{n} (2i^2 - i) \).
   - This simplifies to \( 1 + 2\sum_{i=2}^{n} i^2 - \sum_{i=2}^{n} i \).
   - Using the formulas \( \sum_{i=1}^{n} i^2 = \frac{n(n+1)(2n+1)}{6} \) and \( \sum_{i=1}^{n} i = \frac{n(n+1)}{2} \), the correct sum should be:
     \[
     1 + 2 \left( \frac{n(n+1)(2n+1)}{6} - 1 \right) - \left( \frac{n(n+1)}{2} - 1 \right)
     \]
     Simplifying this, we get:
     \[
     1 + \frac{n(n+1)(2n+1) - 3n(n+1) + 6}{3} = 1 + \frac{n(n+1)(2n - 2) + 6}{3} = 1 + \frac{2n(n+1)(n-1) + 6}{3} = 1 + \frac{2n^3 - 2n + 6}{3} = \frac{2n^3 + 3n^2 + n + 3}{3}
     \]
     However, the program calculates the sum as:
     \[
     1 + \sum_{i=2}^{n} (2i^2 - i)
     \]
     This is not the correct formula for the maximum sum of the matrix. The program's sum calculation is incorrect.

2. **Operations**:
   - The program performs a Type 1 and Type 2 operation for each row and column with the permutation \( [1, 2, \ldots, n] \).
   - This means each row and each column is filled with the sequence \( [1, 2, \ldots, n] \), which is a valid permutation.
   - However, the sum calculation is incorrect, so the operations do not maximize the sum.

#### Verification:
- The sum calculated by the program is incorrect.
- The operations performed ensure that each row and each column is filled with the sequence \( [1, 2, \ldots, n] \), but this does not maximize the sum.

#### Edge Cases:
- **\( n = 1 \)**: The matrix is \( 1 \times 1 \). The sum should be 1, and the program outputs 1 with 1 operation. This is correct.
- **\( n = 2 \)**: The matrix is \( 2 \times 2 \). The sum should be 7, and the program outputs 7 with 4 operations. This is correct.
- **\( n = 3 \)**: The matrix is \( 3 \times 3 \). The sum should be 24, and the program outputs 24 with 6 operations. This is correct.

However, the general sum calculation is incorrect, and the program does not handle the general case correctly.

### Conclusion:
The program does not correctly calculate the maximum sum for the general case, even though it works for small values of \( n \) due to coincidental values.

**Final: False**