To calculate the output state, let's analyze the given code and initial state.

The initial state is:
- `n` is greater than 1
- `m` = `input_m`
- `k` = `input_k`
- `x` = `input_x` - 1
- `y` = `input_y` - 1
- `full_cycles` equals `input_k // ((2 * input_n - 2) * input_m)`
- `remaining_questions` equals `k % ((2 * n - 2) * m)`
- `min_questions` equals `input_k // ((2 * input_n - 2) * input_m) // (2 * n - 2)`
- `max_questions` equals `full_cycles`

The code updates the value of `max_questions` as follows:
```python
max_questions = (full_cycles + n - 1) // (2 * n - 2)
```

Given that `full_cycles` equals `input_k // ((2 * input_n - 2) * input_m)`, the new value of `max_questions` can be expressed in terms of the initial state variables.

After the code execution, `max_questions` becomes `(input_k // ((2 * input_n - 2) * input_m) + n - 1) // (2 * n - 2)`. 

The other variables (`n`, `m`, `k`, `x`, `y`, `full_cycles`, `remaining_questions`, `min_questions`) do not change.

Therefore, the Output State is: 
`n` is greater than 1, 
`m` = `input_m`, 
`k` = `input_k`, 
`x` = `input_x` - 1, 
`y` = `input_y` - 1, 
`full_cycles` equals `input_k // ((2 * input_n - 2) * input_m)`, 
`remaining_questions` equals `k % ((2 * n - 2) * m)`, 
`min_questions` equals `input_k // ((2 * input_n - 2) * input_m) // (2 * n - 2)`, 
`max_questions` equals `(input_k // ((2 * input_n - 2) * input_m) + n - 1) // (2 * n - 2)`.

Output State: **`n` is greater than 1, `m` = `input_m`, `k` = `input_k`, `x` = `input_x` - 1, `y` = `input_y` - 1, `full_cycles` equals `input_k // ((2 * input_n - 2) * input_m)`, `remaining_questions` equals `k % ((2 * n - 2) * m)`, `min_questions` equals `input_k // ((2 * input_n - 2) * input_m) // (2 * n - 2)`, `max_questions` equals `(input_k // ((2 * input_n - 2) * input_m) + n - 1) // (2 * n - 2)`**