To determine what will be printed by the `print(d2[y] - d2[x])` statement, let's break down the initial state and the relevant parts of the code:

### Initial State:
- `t` is an integer where 1 ≤ t ≤ 10^4.
- `i` is 1.
- `n` is a new input integer (greater than or equal to 3).
- `l` is a new list of integers from the latest user input.
- `d1` is a defaultdict initialized with a default value of 0.
- `d1[2]` is 1.
- `d1[i + 2]` is updated based on conditions inside the loop for each iteration.
- `d2` is a defaultdict initialized with a default value of 0.
- `d2[n - 1]` is 1.
- `m` must be greater than 1.
- `j` is 1.
- `x` and `y` are integers provided by the current user input.
- If `y` > `x`, then `y` is greater than `x`.
- If `y` ≤ `x`, then `y` is less than or equal to `x`.

### Analysis:
1. **Defaultdict `d2` Initialization**:
   - `d2` is initialized with a default value of 0.
   - `d2[n - 1]` is set to 1, where `n` is a new input integer (≥ 3).

2. **User Input `x` and `y`**:
   - `x` and `y` are integers provided by the current user input.
   - The relationship between `x` and `y` is either `y > x` or `y ≤ x`.

3. **Expression `d2[y] - d2[x]`**:
   - `d2[y]` will be 1 if `y == n - 1` and 0 otherwise.
   - `d2[x]` will be 1 if `x == n - 1` and 0 otherwise.
   - The result of `d2[y] - d2[x]` depends on the values of `y` and `x` relative to `n - 1`.

### Possible Outcomes:
- If `y == n - 1` and `x != n - 1`, then `d2[y] = 1` and `d2[x] = 0`, so `d2[y] - d2[x] = 1 - 0 = 1`.
- If `y != n - 1` and `x == n - 1`, then `d2[y] = 0` and `d2[x] = 1`, so `d2[y] - d2[x] = 0 - 1 = -1`.
- If both `y` and `x` are not equal to `n - 1`, then `d2[y] = 0` and `d2[x] = 0`, so `d2[y] - d2[x] = 0 - 0 = 0`.
- If both `y` and `x` are equal to `n - 1`, then `d2[y] = 1` and `d2[x] = 1`, so `d2[y] - d2[x] = 1 - 1 = 0`.

### Conclusion:
Given the initial state and the conditions, the output of the `print(d2[y] - d2[x])` statement will be one of the following:
- **1** if `y == n - 1` and `x != n - 1`.
- **-1** if `y != n - 1` and `x == n - 1`.
- **0** if both `y` and `x` are not equal to `n - 1` or both are equal to `n - 1`.

Since the exact values of `x` and `y` are not provided, we can only describe the possible outcomes based on the given conditions.

Output: **d2[y] - d2[x] (where d2[y] is 1 if y == n - 1 and 0 otherwise, and d2[x] is 1 if x == n - 1 and 0 otherwise)**