### Reasoning:

Let's re-evaluate the problem and the provided solution step-by-step, using the annotations and the original assessment to ensure accuracy.

#### Problem Analysis:
The goal is to maximize the sum of all numbers in an \( n \times n \) matrix using no more than \( 2n \) operations. We can perform two types of operations:
1. Assign a row with a permutation of numbers from 1 to \( n \).
2. Assign a column with a permutation of numbers from 1 to \( n \).

The optimal strategy to maximize the sum involves filling the matrix with the highest possible values. The highest sum can be achieved by filling the matrix with numbers from 1 to \( n \) in a way that maximizes the sum of all elements.

#### Theoretical Maximum Sum:
For an \( n \times n \) matrix, the maximum sum is achieved by filling the matrix with the numbers from 1 to \( n \) in a way that maximizes the sum of all elements. The sum of the first \( n \) natural numbers is given by the formula:
\[ \text{Sum of first } n \text{ natural numbers} = \frac{n(n + 1)}{2} \]

Since each row and column can be filled with a permutation of these numbers, the maximum sum of the matrix is:
\[ \text{Maximum sum} = n \times \left(\frac{n(n + 1)}{2}\right) = \frac{n^2(n + 1)}{2} \]

#### Program Analysis:
The provided program calculates the sum differently:
\[ \text{Sum} = 1 + \sum_{i=2}^{n} (i^2 - (i-1)^2) \times i \]

Let's simplify this expression:
\[ \text{Sum} = 1 + \sum_{i=2}^{n} (i^2 - (i^2 - 2i + 1)) \times i \]
\[ \text{Sum} = 1 + \sum_{i=2}^{n} (2i - 1) \times i \]
\[ \text{Sum} = 1 + \sum_{i=2}^{n} (2i^2 - i) \]
\[ \text{Sum} = 1 + 2\sum_{i=2}^{n} i^2 - \sum_{i=2}^{n} i \]

Using the formulas for the sum of squares and the sum of the first \( n \) natural numbers:
\[ \sum_{i=1}^{n} i^2 = \frac{n(n + 1)(2n + 1)}{6} \]
\[ \sum_{i=1}^{n} i = \frac{n(n + 1)}{2} \]

We can rewrite the sums starting from \( i=2 \):
\[ \sum_{i=2}^{n} i^2 = \sum_{i=1}^{n} i^2 - 1 = \frac{n(n + 1)(2n + 1)}{6} - 1 \]
\[ \sum_{i=2}^{n} i = \sum_{i=1}^{n} i - 1 = \frac{n(n + 1)}{2} - 1 \]

Substituting these into the expression for the sum:
\[ \text{Sum} = 1 + 2\left(\frac{n(n + 1)(2n + 1)}{6} - 1\right) - \left(\frac{n(n + 1)}{2} - 1\right) \]
\[ \text{Sum} = 1 + \frac{2n(n + 1)(2n + 1)}{6} - 2 - \frac{n(n + 1)}{2} + 1 \]
\[ \text{Sum} = \frac{2n(n + 1)(2n + 1)}{6} - \frac{3n(n + 1)}{6} \]
\[ \text{Sum} = \frac{2n(n + 1)(2n + 1) - 3n(n + 1)}{6} \]
\[ \text{Sum} = \frac{n(n + 1)(4n + 2 - 3)}{6} \]
\[ \text{Sum} = \frac{n(n + 1)(4n - 1)}{6} \]

This expression does not match the theoretical maximum sum of \(\frac{n^2(n + 1)}{2}\).

However, let's verify the operations performed by the program:
- The program performs \( 2n \) operations, which is within the allowed limit.
- Each operation fills a row and a column with a permutation of numbers from 1 to \( n \).

Let's verify the operations in the annotated code:
- For each \( j \) from 1 to \( n \), the program performs:
  - Type 1 operation on row \( n - j + 1 \) with permutation \( [1, 2, \ldots, n] \).
  - Type 2 operation on column \( n - j + 1 \) with permutation \( [1, 2, \ldots, n] \).

This strategy ensures that each row and column is filled with the numbers from 1 to \( n \) in a way that maximizes the sum of the matrix. However, the calculated sum does not match the theoretical maximum sum.

#### Conclusion:
The program does not correctly calculate the maximum sum of the matrix. The operations are correct in terms of filling the matrix, but the sum calculation is incorrect.

### Final Evaluation
Final: **False**