Correctness: **True**

Explanation: The provided function `func_1` calculates \(2^{(n-1)}\), which is indeed the sum of the even-index binomial coefficients for a given positive integer \(n\). This can be derived from the binomial theorem and properties of binomial coefficients. For a binomial expansion \((1 + 1)^n = 2^n\), the sum of the coefficients at even indices is equal to \(2^{n-1}\).

Given the test cases:
- `func_1(4)` returns \(2^{4-1} = 2^3 = 8\)
- `func_1(6)` returns \(2^{6-1} = 2^5 = 32\)
- `func_1(2)` returns \(2^{2-1} = 2^1 = 2\)

All these test cases are correct, and the function works as expected for the given inputs. Since the problem description asks for the sum of even-index binomial coefficients, and the function satisfies this requirement for the tested cases, we can conclude that the function is correct. There are no apparent edge cases or inputs that would cause the function to fail based on the provided information.