The expression `dp[n, k] += 9 * 10 ** (i - 1) * (10 ** (k - i) - 10 ** (i - 1))` updates the value of `dp[n, k]`. 

Here, `i` is 1, so we substitute that into the equation:
```
dp[n, k] += 9 * 10 ** (1 - 1) * (10 ** (k - 1) - 10 ** (1 - 1))
```
This simplifies to:
```
dp[n, k] += 9 * 10 ** 0 * (10 ** (k - 1) - 10 ** 0)
dp[n, k] += 9 * (10 ** (k - 1) - 1)
```
The overall value added to `dp[n, k]` depends on the specific values of `k` (which is between 2 and 10) and `n` (which is greater than or equal to 10). 

Now, we include the preconditions that remain valid:
- `l` is an integer such that 1 ≤ `l` ≤ `r` < 10^18
- `r` is an integer such that 1 ≤ `l` ≤ `r` < 10^18
- `k` is an integer such that 2 ≤ `k` ≤ 10
- `n` is greater than or equal to 10
- `i` is now 1

Output State: **`l` is an integer such that 1 ≤ `l` ≤ `r` < 10^18, `r` is an integer such that 1 ≤ `l` ≤ `r` < 10^18, `k` is an integer such that 2 ≤ `k` ≤ 10, `n` is greater than or equal to 10, `i` is 1, `dp[n, k]` is updated by adding `9 * (10 ** (k - 1) - 1)` to its previous value.**