Postcondition: **`i` is `i + 1`, `b` remains the same, `x` is `(a - (i + 1) * i) // (i + 1)`. If `(a - i * (i - 1)) % i ** 2 == 0 and i * (i - 1) % i ** 2 == 0`, then `suma` is `suma + (a - (i + 1) * i) // (i + 1) + 1`. Otherwise, `suma` is `suma + (a - (i + 1) * i) // (i + 1)`.**

However, given that the second condition in the if statement `i * (i - 1) % i ** 2 == 0` is always true (since `i * (i - 1)` is always divisible by `i ** 2`), the overall postcondition simplifies to:

Postcondition: **`i` is `i + 1`, `b` remains the same, `x` is `(a - (i + 1) * i) // (i + 1)`. If `(a - i * (i - 1)) % i ** 2 == 0`, then `suma` is `suma + (a - (i + 1) * i) // (i + 1) + 1`. Otherwise, `suma` is `suma + (a - (i + 1) * i) // (i + 1)`.**