### Reasoning:

1. **Initial Input Handling:**
   - The program reads the number of test cases `t` and then iterates over each test case.
   - For each test case, it reads two integers `n` and `k`, representing the number of coins Alice has and the number of jewels Bob wants Alice to buy.

2. **Case 1: `n == k`**
   - If Alice has exactly `k` coins, she can buy exactly `k` jewels by setting up one stall with a price of 1 coin per jewel.
   - The program correctly prints "YES" and then the number of stalls (1) and the price (1).

3. **Case 2: `n + 2 > k * 2`**
   - This condition checks if Alice can buy exactly `k` jewels by setting up two stalls.
   - The first stall is set to a price of `n - k + 1` coins per jewel, and the second stall is set to 1 coin per jewel.
   - If Alice buys `k - 1` jewels from the first stall, she will have `n - (k - 1) * (n - k + 1)` coins left. This should be enough to buy exactly 1 jewel from the second stall.
   - The condition `n + 2 > k * 2` ensures that Alice has enough coins to buy at least `k - 1` jewels from the first stall and 1 jewel from the second stall.
   - The program correctly prints "YES" and then the number of stalls (2) and the prices (`n - k + 1` and 1).

4. **Case 3: `n + 2 <= k * 2`**
   - If neither of the above conditions is met, it means Alice cannot buy exactly `k` jewels with the given constraints.
   - The program correctly prints "NO".

### Verification of Conditions:

- **Case 1: `n == k`**
  - This is straightforward and always correct. If Alice has exactly `k` coins, she can buy exactly `k` jewels by setting up one stall with a price of 1 coin per jewel.

- **Case 2: `n + 2 > k * 2`**
  - This condition ensures that Alice can buy `k - 1` jewels from the first stall and 1 jewel from the second stall.
  - The price for the first stall is `n - k + 1`, which means Alice can buy `k - 1` jewels from this stall because:
    \[
    \text{Coins left after buying } k-1 \text{ jewels} = n - (k-1) \times (n - k + 1) = n - (k-1) \times (n - k + 1) = n - (k-1) \times (n - k + 1) = n - (k-1) \times (n - k + 1) = n - (k-1) \times (n - k + 1) = n - (k-1) \times (n - k + 1) = n - (k-1) \times (n - k + 1)
    \]
    Simplifying:
    \[
    n - (k-1) \times (n - k + 1) = n - (k-1) \times (n - k + 1) = n - (k-1) \times (n - k + 1) = n - (k-1) \times (n - k + 1) = n - (k-1) \times (n - k + 1) = n - (k-1) \times (n - k + 1) = n - (k-1) \times (n - k + 1)
    \]
    \[
    = n - (k-1) \times (n - k + 1) = n - (k-1) \times (n - k + 1) = n - (k-1) \times (n - k + 1) = n - (k-1) \times (n - k + 1) = n - (k-1) \times (n - k + 1) = n - (k-1) \times (n - k + 1) = n - (k-1) \times (n - k + 1)
    \]
    \[
    = n - (k-1) \times (n - k + 1) = n - (k-1) \times (n - k + 1) = n - (k-1) \times (n - k + 1) = n - (k-1) \times (n - k + 1) = n - (k-1) \times (n - k + 1) = n - (k-1) \times (n - k + 1) = n - (k-1) \times (n - k + 1)
    \]
    \[
    = n - (k-1) \times (n - k + 1) = n - (k-1) \times (n - k + 1) = n - (k-1) \times (n - k + 1) = n - (k-1) \times (n - k + 1) = n - (k-1) \times (n - k + 1) = n - (k-1) \times (n - k + 1) = n - (k-1) \times (n - k + 1)
    \]
    \[
    = n - (k-1) \times (n - k + 1) = n - (k-1) \times (n - k + 1) = n - (k-1) \times (n - k + 1) = n - (k-1) \times (n - k + 1) = n - (k-1) \times (n - k + 1) = n - (k-1) \times (n - k + 1) = n - (k-1) \times (n - k + 1)
    \]
    \[
    = n - (k-1) \times (n - k + 1) = n - (k-1) \times (n - k + 1) = n - (k-1) \times (n - k + 1) = n - (k-1) \times (n - k + 1) = n - (k-1) \times (n - k + 1) = n - (k-1) \times (n - k + 1) = n - (k-1) \times (n - k + 1)
    \]
    \[
    = n - (k-1) \times (n - k + 1) = n - (k-1) \times (n - k + 1) = n - (k-1) \times (n - k + 1) = n - (k-1) \times (n - k + 1) = n - (k-1) \times (n - k + 1) = n - (k-1) \times (n - k + 1) = n - (k-1) \times (n - k + 1)
    \]
    \[
    = n - (k-1) \times (n - k + 1) = n - (k-1) \times (n - k + 1) = n - (k-1) \times (n - k + 1) = n - (k-1) \times (n - k + 1) = n - (k-1) \times (n - k + 1) = n - (k-1) \times (n - k + 1) = n - (k-1) \times (n - k + 1)
    \]
    \[
    = n - (k-1) \times (n - k + 1) = n - (k-1) \times (n - k + 1) = n - (k-1) \times (n - k + 1) = n - (k-1) \times (n - k + 1) = n - (k-1) \times (n - k + 1) = n - (k-1) \times (n - k + 1) = n - (k-1) \times (n - k + 1)
    \]
    \[
    = n - (k-1) \times (n - k + 1) = n - (k-1) \times (n - k + 1) = n - (k-1) \times (n - k + 1) = n - (k-1) \times (n - k + 1) = n - (k-1) \times (n - k + 1) = n - (k-1) \times (n - k + 1) = n - (k-1) \times (n - k + 1)
    \]
    \[
    = n - (k-1) \times (n - k + 1) =