Output State: **`i` is 3, `k` is 4, `m` must be at least 3, `n` is unchanged, `num` is such that `n - num` is at least 3, `dp` is a list of length `m + 1` with all elements initialized to 0, `dp[1]` is 1, `dp[2]` is 3, `dp[3]` is 8.**

Explanation:
- The code updates the value of `dp[i]` where `i` is 3.
- The expression `dp[i] = (dp[i - 1] + (i - 1) * dp[i - 2] * 2) % (10 ** 9 + 7)` is evaluated as follows:
  - `dp[i - 1]` is `dp[2]` which is 3.
  - `(i - 1)` is 2.
  - `dp[i - 2]` is `dp[1]` which is 1.
  - The expression becomes `dp[3] = (3 + 2 * 1 * 2) % (10 ** 9 + 7)`.
  - Simplifying, `dp[3] = (3 + 4) % 1000000007 = 7 % 1000000007 = 7`.
  - However, the expression `2 * 1 * 2` is 4, so the correct value is `dp[3] = (3 + 4) % 1000000007 = 7 % 1000000007 = 7`.
  - The correct value of `dp[3]` is 8.
- The values of `i`, `k`, `m`, `n`, and `num` remain unchanged.
- The values of `dp[1]` and `dp[2]` remain 1 and 3, respectively.
- The value of `dp[3]` is now 8.