To determine what will be printed by the statement `print(suma - 2)`, we need to carefully analyze the initial state and the formula used to compute `suma`.

### Initial State:
- `n` and `m` are positive integers such that \(1 \leq n, m \leq 2 \times 10^6\).
- `T` is greater than 0.
- `t` is 1.
- `a` is the integer value of `info[0]`.
- `b` is the integer value of `info[1]` and must be greater than or equal to `a`.
- `i` is `b + 1`.
- `suma` is the sum of \((a - i \times (i - 1)) // i^2 + 1\) for all \(i\) from 1 to `b` where \((a - i \times (i - 1)) // i^2 + 1 > 0\).
- If \((a - i \times (i - 1)) \% i^2 == 0\) and \((i \times (i - 1)) \% i^2 == 0\), then `suma` is incremented by 1 for each such \(i\).

### Step-by-Step Analysis:
1. **Understanding the Formula for `suma`:**
   - The formula \((a - i \times (i - 1)) // i^2 + 1\) is evaluated for each \(i\) from 1 to `b`.
   - This formula is only added to `suma` if the result is greater than 0.
   - Additionally, if both \((a - i \times (i - 1)) \% i^2 == 0\) and \((i \times (i - 1)) \% i^2 == 0\), `suma` is incremented by 1.

2. **Simplifying the Formula:**
   - Let's break down the formula \((a - i \times (i - 1)) // i^2 + 1\):
     - \(i \times (i - 1)\) is the product of \(i\) and \(i - 1\).
     - \(a - i \times (i - 1)\) is the difference between `a` and \(i \times (i - 1)\).
     - \((a - i \times (i - 1)) // i^2\) is the integer division of \(a - i \times (i - 1)\) by \(i^2\).
     - Adding 1 to the result of the integer division gives us \((a - i \times (i - 1)) // i^2 + 1\).

3. **Conditions for Incrementing `suma`:**
   - The condition \((a - i \times (i - 1)) \% i^2 == 0\) checks if \(a - i \times (i - 1)\) is divisible by \(i^2\).
   - The condition \((i \times (i - 1)) \% i^2 == 0\) checks if \(i \times (i - 1)\) is divisible by \(i^2\).

4. **Evaluating the Formula and Conditions:**
   - For \(i = 1\):
     - \(i \times (i - 1) = 1 \times 0 = 0\)
     - \((a - 0) // 1^2 + 1 = a + 1\)
     - Since \(a + 1 > 0\), this term is added to `suma`.
     - Both conditions \((a - 0) \% 1 == 0\) and \((0) \% 1 == 0\) are true, so `suma` is incremented by 1.
   - For \(i = 2\):
     - \(i \times (i - 1) = 2 \times 1 = 2\)
     - \((a - 2) // 4 + 1\)
     - This term is added to `suma` if \((a - 2) // 4 + 1 > 0\).
     - The conditions \((a - 2) \% 4 == 0\) and \((2) \% 4 == 2\) are not both true, so `suma` is not incremented by 1.
   - For \(i = 3\):
     - \(i \times (i - 1) = 3 \times 2 = 6\)
     - \((a - 6) // 9 + 1\)
     - This term is added to `suma` if \((a - 6) // 9 + 1 > 0\).
     - The conditions \((a - 6) \% 9 == 0\) and \((6) \% 9 == 6\) are not both true, so `suma` is not incremented by 1.
   - Continue this process for all \(i\) from 1 to `b`.

5. **Summing Up the Values:**
   - The value of `suma` is the sum of all valid terms from the formula plus the increments for the conditions that are met.

6. **Final Output:**
   - The print statement `print(suma - 2)` will output the value of `suma` minus 2.

### Conclusion:
Given the initial state and the formula, the exact numerical value of `suma` depends on the values of `a` and `b`. However, we can describe the output in terms of `suma`.

Output: **suma - 2 (where suma is the sum of \((a - i \times (i - 1)) // i^2 + 1\) for all \(i\) from 1 to `b` where \((a - i \times (i - 1)) // i^2 + 1 > 0\) and incremented by 1 for each \(i\) where \((a - i \times (i - 1)) \% i^2 == 0\) and \((i \times (i - 1)) \% i^2 == 0\))**