The code snippet `n -= m` subtracts the value of `m` from `n`. Given that `m` is calculated as `(n + 1) // 2`, the new value of `n` will be `n - (n + 1) // 2`.

Let's break down the transformation:
- Initially, `m` is `(n + 1) // 2`.
- After the operation `n -= m`, the new value of `n` becomes `n - (n + 1) // 2`.

The values of `t`, `k`, `L`, and `m` remain unchanged.

Output State: **`t` is an integer such that \(1 \leq t \leq 5 \cdot 10^4\); `n` is `n - (n + 1) // 2`; `k` is the second integer read from the input; `L` is `[m, m]`; `m` is `(n + 1) // 2`**.