The value of `r` is updated to the current value of `mid`. The initial value of `mid` is calculated as `(-1 + n) / 2`. Since `(mid * c - (n - mid) * d) >= 0` holds true, the value of `mid` is valid for the condition given. The values of `n`, `c`, `d`, and `l` remain unchanged.

Output State: **`n` is an integer such that 3 ≤ n ≤ 500000, `c` and `d` are integers such that 0 ≤ c ≤ d ≤ 10^9, `l = -1`, `r = (-1 + n) / 2`, `mid = (-1 + n) / 2`. The current value of `mid` is such that `(mid * c - (n - mid) * d) >= 0`.**