The code snippet updates the value of `mid` to be the average of `l` and `r`. To determine the new value of `mid`, we need to consider the conditions given in the initial state that affect the values of `l` and `r`.

### Initial State:
- `n` is an integer such that 3 ≤ n ≤ 500000.
- `c` and `d` are integers such that 0 ≤ c ≤ d ≤ 10^9.
- `mid = (-1 + n) / 2`.
- If `(mid * c - (n - mid) * d) >= 0`, then `l = -1` and `r = (-1 + n) / 2`.
- Otherwise, `l = (-1 + n) // 2` and `r = n`.

### Code Execution:
The code snippet `mid = (l + r) / 2` calculates the new value of `mid` as the average of `l` and `r`.

### Calculation:
1. **Case 1: `(mid * c - (n - mid) * d) >= 0`**
   - `l = -1`
   - `r = (-1 + n) / 2`
   - New `mid` is calculated as:
     \[
     \text{new\_mid} = \frac{l + r}{2} = \frac{-1 + \left(\frac{-1 + n}{2}\right)}{2} = \frac{-1 + \frac{n - 1}{2}}{2} = \frac{\frac{-2 + n - 1}{2}}{2} = \frac{\frac{n - 3}{2}}{2} = \frac{n - 3}{4}
     \]

2. **Case 2: `(mid * c - (n - mid) * d) < 0`**
   - `l = (-1 + n) // 2`
   - `r = n`
   - New `mid` is calculated as:
     \[
     \text{new\_mid} = \frac{l + r}{2} = \frac{\left(\frac{-1 + n}{2}\right) + n}{2} = \frac{\frac{n - 1}{2} + n}{2} = \frac{\frac{n - 1 + 2n}{2}}{2} = \frac{\frac{3n - 1}{2}}{2} = \frac{3n - 1}{4}
     \]

### Output State:
- `n` is an integer such that 3 ≤ n ≤ 500000.
- `c` and `d` are integers such that 0 ≤ c ≤ d ≤ 10^9.
- If `(mid * c - (n - mid) * d) >= 0`, then `l = -1`, `r = (-1 + n) / 2`, and `mid = (n - 3) / 4`.
- Otherwise, `l = (-1 + n) // 2`, `r = n`, and `mid = (3n - 1) / 4`.

Output State: **`n` is an integer such that 3 ≤ n ≤ 500000, `c` and `d` are integers such that 0 ≤ c ≤ d ≤ 10^9, if `(mid * c - (n - mid) * d) >= 0` then `l = -1`, `r = (-1 + n) / 2`, and `mid = (n - 3) / 4`, otherwise `l = (-1 + n) // 2`, `r = n`, and `mid = (3n - 1) / 4`.**