The code snippet `r = mid` updates the value of `r` to be equal to `mid`. We need to consider the two possible conditions from the initial state to determine the final value of `r`.

1. If `(mid * c - (n - mid) * d) >= 0`:
   - `l = -1`
   - `r = (-1 + n) / 2`
   - `mid = (n - 3) / 4`

   In this case, `r` is updated to `mid`, which is `(n - 3) / 4`.

2. Otherwise:
   - `l = (-1 + n) // 2`
   - `r = n`
   - `mid = (3 * n - 1) / 4`

   In this case, `r` is updated to `mid`, which is `(3 * n - 1) / 4`.

Therefore, the output state will depend on the condition evaluated in the initial state.

Output State: **`n` is an integer such that 3 ≤ n ≤ 500000, `c` and `d` are integers such that 0 ≤ c ≤ d ≤ 10^9, if `(mid * c - (n - mid) * d) >= 0` then `l = -1`, `r = (n - 3) / 4`, and `mid = (n - 3) / 4`, otherwise `l = (-1 + n) // 2`, `r = (3 * n - 1) / 4`, and `mid = (3 * n - 1) / 4`.**