To determine which states need to be adjusted for the loop to execute one more time, let's analyze the given conditions and the `while` loop statement:

### Given State:
- `n` is an integer such that 3 ≤ n ≤ 500000.
- `c` and `d` are integers such that 0 ≤ c ≤ d ≤ 10^9.
- If `(mid * c - (n - mid) * d) >= 0`, then:
  - `l = -1`
  - `r = (n - 3) / 4`
  - `mid = (n - 3) / 4`
- Otherwise:
  - `l = (-1 + n) // 2`
  - `r = n`
  - `mid = (3 * n - 1) / 4`

### `while` Loop Condition:
```
while l + 1 < r:
```

### Analysis:
The loop will continue as long as `l + 1 < r`. Therefore, we need to ensure that this condition holds true for the next iteration.

#### Case 1: `(mid * c - (n - mid) * d) >= 0`
- `l = -1`
- `r = (n - 3) / 4`
- `mid = (n - 3) / 4`

For the loop to execute again:
- `l + 1 < r` must be true.
- Substituting the values: `-1 + 1 < (n - 3) / 4`
- Simplifying: `0 < (n - 3) / 4`
- Multiplying both sides by 4: `0 < n - 3`
- Adding 3 to both sides: `3 < n`

Since `n` is already given to be in the range 3 ≤ n ≤ 500000, the condition `3 < n` is satisfied for all valid `n` except when `n = 3`.

#### Case 2: `(mid * c - (n - mid) * d) < 0`
- `l = (-1 + n) // 2`
- `r = n`
- `mid = (3 * n - 1) / 4`

For the loop to execute again:
- `l + 1 < r` must be true.
- Substituting the values: `((-1 + n) // 2) + 1 < n`
- Simplifying: `((n - 1) // 2) + 1 < n`
- Simplifying further: `(n - 1) // 2 < n - 1`
- Since `(n - 1) // 2` is the integer division, it is always less than `n - 1` for all positive `n`.

Thus, the condition `l + 1 < r` is always true for all valid `n` in this case.

### Conclusion:
- For the first case, the loop will execute again as long as `n > 3`.
- For the second case, the loop will always execute again for all valid `n`.

Since the given state includes `3 ≤ n ≤ 500000`, and the loop condition is satisfied in both cases, no adjustments are needed for the loop to execute one more time.

### Final State:
State: **`n` is an integer such that 3 ≤ n ≤ 500000, `c` and `d` are integers such that 0 ≤ c ≤ d ≤ 10^9. If `(mid * c - (n - mid) * d) >= 0`, then `l = -1`, `r = (n - 3) / 4`, and `mid = (n - 3) / 4`. Otherwise, `l = (-1 + n) // 2`, `r = n`, and `mid = (3 * n - 1) / 4`.**