The code `mid = (l + r) / 2` updates the value of `mid` to be the average of `l` and `r`. To determine the new value of `mid`, we need to consider the two cases based on the condition `(mid * c - (n - mid) * d) >= 0`.

### Case 1: `(mid * c - (n - mid) * d) >= 0`
- `l = -1`
- `r = (n - 3) / 4`
- `mid = (n - 3) / 4`

In this case, the new value of `mid` is:
\[ \text{mid} = \frac{l + r}{2} = \frac{-1 + \frac{n - 3}{4}}{2} = \frac{-1 + \frac{n - 3}{4}}{2} = \frac{-1 + \frac{n - 3}{4}}{2} = \frac{-4 + n - 3}{8} = \frac{n - 7}{8} \]

### Case 2: `(mid * c - (n - mid) * d) < 0`
- `l = (-1 + n) // 2`
- `r = n`
- `mid = (3 * n - 1) / 4`

In this case, the new value of `mid` is:
\[ \text{mid} = \frac{l + r}{2} = \frac{\left(\frac{-1 + n}{2}\right) + n}{2} = \frac{\frac{-1 + n + 2n}{2}}{2} = \frac{\frac{3n - 1}{2}}{2} = \frac{3n - 1}{4} \]

Therefore, the output state depends on which case was true:

### Case 1:
If `(mid * c - (n - mid) * d) >= 0`:
- `l = -1`
- `r = (n - 3) / 4`
- `mid = (n - 7) / 8`

### Case 2:
If `(mid * c - (n - mid) * d) < 0`:
- `l = (-1 + n) // 2`
- `r = n`
- `mid = (3 * n - 1) / 4`

Output State: **`n` is an integer such that 3 ≤ n ≤ 500000, `c` and `d` are integers such that 0 ≤ c ≤ d ≤ 10^9. If `(mid * c - (n - mid) * d) >= 0`, then `l = -1`, `r = (n - 3) / 4`, and `mid = (n - 7) / 8`. Otherwise, `l = (-1 + n) // 2`, `r = n`, and `mid = (3 * n - 1) / 4`.**