Reasoning:  
The problem statement asks for the difference between the sum of cubes of the first n natural numbers and the sum of the first n natural numbers. The provided function calculates the sum of the first n natural numbers (`sum_n`), then squares this sum to get `sum_cubes_n`, and finally returns the difference `sum_cubes_n - sum_n`.

However, the comment in the code suggests that the function returns `(n * (n + 1) // 2) - (n * (n + 1) // 2)`, which simplifies to 0. This is incorrect because the formula for the sum of cubes of the first n natural numbers is \((\frac{n(n+1)}{2})^2\), and the function should be calculating the difference between this value and the sum of the first n natural numbers, not just subtracting the same value from itself.

Let's verify the test cases:
- For `n = 3`:
  - Sum of cubes: \(1^3 + 2^3 + 3^3 = 36\)
  - Sum of first 3 natural numbers: \(1 + 2 + 3 = 6\)
  - Difference: \(36 - 6 = 30\) (which matches the test case)

- For `n = 5`:
  - Sum of cubes: \(1^3 + 2^3 + 3^3 + 4^3 + 5^3 = 225\)
  - Sum of first 5 natural numbers: \(1 + 2 + 3 + 4 + 5 = 15\)
  - Difference: \(225 - 15 = 210\) (which matches the test case)

- For `n = 2`:
  - Sum of cubes: \(1^3 + 2^3 = 9\)
  - Sum of first 2 natural numbers: \(1 + 2 = 3\)
  - Difference: \(9 - 3 = 6\) (which matches the test case)

The test cases provided are correct, but the comment in the code is misleading and incorrect. The function is correctly implemented to solve the problem as described.

Correctness: **True**