The value of `i` is 1, so the code calculates `odd += abs(i * 2 + 1 - p[i])`. This means `odd` is updated by adding the absolute difference between `i * 2 + 1` (which is `1 * 2 + 1 = 3`) and `p[1]`. The previous value of `odd` is not specified, but it is updated based on this calculation. The values of `n`, `p`, and `i` remain unchanged.

Therefore, the Output State is: `n` is an even integer such that 2 ≤ `n` ≤ 100; `p` is a list of integers with each element decreased by 1; `even` is updated to `even + abs(2 - p[1])`; `odd` is updated to `odd + abs(3 - p[1])`; `i` is 1.

Output State: **`n` is an even integer such that 2 ≤ `n` ≤ 100; `p` is a list of integers with each element decreased by 1; `even` is updated to `even + abs(2 - p[1])`; `odd` is updated to `odd + abs(3 - p[1])`; `i` is 1.**