Let's break down the problem step by step.

### Step-by-Step Analysis:

1. **Identify the Loop Condition:**
   The loop condition is given by:
   \[
   (x + y) * x \leq n \quad \text{and} \quad (x + y) * y \leq m
   \]

2. **Current State Before the Loop:**
   - \( y = 1 \)
   - \( x \) and \( n \) and \( m \) are unknown but assumed to be valid integers.

3. **Determine the Variables in the Loop Head:**
   The loop head involves the variables \( x \), \( y \), \( n \), and \( m \).

4. **Evaluate the Loop Condition with Given \( y \):**
   Since \( y = 1 \), the loop condition becomes:
   \[
   (x + 1) * x \leq n \quad \text{and} \quad (x + 1) * 1 \leq m
   \]
   Simplifying further:
   \[
   (x + 1) * x \leq n \quad \text{and} \quad x + 1 \leq m
   \]

5. **Ensure the First Iteration Can Execute:**
   - For the first iteration, \( x \) must satisfy both conditions:
     - \( (x + 1) * x \leq n \)
     - \( x + 1 \leq m \)

6. **Adjust the State:**
   - To ensure the first iteration can execute, \( x \) must be such that both conditions hold true.
   - Specifically, \( x \) must be less than or equal to \( \min(n / (x + 1), m - 1) \).

Since the exact value of \( x \) is not specified, we need to ensure that there exists at least one valid \( x \) that satisfies both conditions. Therefore, we need to adjust the state to ensure that \( x \) is within a range that allows the loop to execute.

### Final Answer:
State: **`y` is 1, `x` must be such that (x + 1) * x <= n and x + 1 <= m**