To determine the final state of the variables after the loop has completed all its iterations, let's carefully analyze the loop and the given states.

The loop iterates from `i = 2` to `i = n` (inclusive) and updates the `sum` variable in each iteration using the formula:
\[ \text{sum} += (i * i - (i - 1) * (i - 1)) * i \]

Breaking down the formula:
\[ i * i - (i - 1) * (i - 1) = i^2 - (i - 1)^2 = i^2 - (i^2 - 2i + 1) = 2i - 1 \]
Thus, the update formula simplifies to:
\[ \text{sum} += (2i - 1) * i \]
\[ \text{sum} += 2i^2 - i \]

Given the initial state:
- `sum` is 1
- `n` is an input integer
- `j` is 6
- `t` is 1

Using the provided output states after the first 3 iterations:
1. After the first iteration (`i = 2`):
   \[ \text{sum} = 1 + (2 * 2 - 1) * 2 = 1 + 3 * 2 = 1 + 6 = 7 \]
2. After the second iteration (`i = 3`):
   \[ \text{sum} = 7 + (3 * 3 - 2 * 2) * 3 = 7 + 5 * 3 = 7 + 15 = 22 \]
3. After the third iteration (`i = 4`):
   \[ \text{sum} = 22 + (4 * 4 - 3 * 3) * 4 = 22 + 7 * 4 = 22 + 28 = 50 \]

Continuing this pattern, we can generalize the sum calculation. Let's compute the sum for all iterations until `i = n`:

\[ \text{sum} = 1 + \sum_{i=2}^{n} (2i^2 - i) \]

To find the final sum after all iterations, we need to compute the summation from `i = 2` to `i = n` of the expression `(2i^2 - i)` and add it to the initial value of `sum` (which is 1).

Let's compute this step-by-step for a general `n`. For simplicity, let's assume `n` is 5 (as per the given output states).

\[ \text{sum} = 1 + \sum_{i=2}^{5} (2i^2 - i) \]
\[ \text{sum} = 1 + [(2*2^2 - 2) + (2*3^2 - 3) + (2*4^2 - 4) + (2*5^2 - 5)] \]
\[ \text{sum} = 1 + [(8 - 2) + (18 - 3) + (32 - 4) + (50 - 5)] \]
\[ \text{sum} = 1 + [6 + 15 + 28 + 45] \]
\[ \text{sum} = 1 + 94 \]
\[ \text{sum} = 95 \]

Given the pattern and the general formula, we can compute the final sum for any `n`. However, based on the provided states and the calculations, the final sum after all iterations when `n` is 5 is 95.

Output State: **sum is 95, n is an input integer, j is 6, t is 1.**

In natural language, after the loop has completed all its iterations with `n` being 5, the value of `sum` is 95, while `j` remains 6 and `t` remains 1.