The code `s = t[:-i]` slices the string `t` from the start up to the `i`-th character from the end. Given the initial state, `i` is 1, so `s` will be the substring of `t` from the start up to the character before the last one. Since `t` is a non-empty string and its first character is equal to its last character (`t[:1] == t[-1:]`), this condition remains true even after the slicing operation.

Here's the step-by-step calculation:

1. The initial state is: `t` is a non-empty string, `n` is the length of `t` and is greater than 1, `i` is 1, and `t[:1] == t[-1:]`.
2. The code `s = t[:-i]` means that `s` is the string `t` sliced from the beginning up to the character before the last one because `i` is 1. So, `s` is `t[:-1]`.

Therefore, the new value of `s` is `t[:-1]`. The other variables remain unchanged: `t` remains the same, `n` remains the length of `t`, and `i` remains 1.

Output State: **`t` is a non-empty string, `n` is the length of `t` and is greater than 1, `i` is 1, `s` is `t[:-1]` and `t[:1] == t[-1:]`.**