Example Answer:
The value of `x` is updated by subtracting the value of `i` from it. Given that `i` is 9, the updated value of `x` would be x - 9. The initial value of `x` was x - 6 + (i + k), which means the new value of `x` after the operation is (x - 6 + (i + k)) - 9. Therefore, the updated expression for `x` is x - 6 + (i + k) - 9. The Output State is: n is an integer such that 1 ≤ n ≤ 10^4, x is (x - 6 + (i + k)) - 9, i is 9, k is 4, c is 2.
Output State: **n is an integer such that 1 ≤ n ≤ 10^4, x is (x - 6 + (i + k)) - 9, i is 9, k is 4, c is 2**