The code snippet `q = 2 ** (p - 1)` updates the value of `q` based on the value of `p`. Given `p` is 2, the expression `2 ** (p - 1)` evaluates to `2 ** (2 - 1)` which is `2 ** 1` and equals `2`. Therefore, `q` remains `2`.

The other variables remain unchanged. The Output State is:

Output State: **`t` is an integer such that 1 <= t <= 10^4, `x` and `y` are distinct non-negative integers such that 0 <= x, y <= 10^9, `n` is 5, `m` is 0, `k` is 5, `i` is incremented by 1, `l` is '11', `p` is 2, `q` is 2, `f` is 3**