The code snippet `a[i] = a[i - 1] + x[i - 1]` updates the value of `a[i]` based on the values of `a[i - 1]` and `x[i - 1]`.

Given the initial state:
- `t` is an integer such that 1 ≤ t ≤ 10^4
- `n` is an input integer such that 2 ≤ n ≤ 500
- `x` is a list of integers read from the input
- `a` is a list of length `n` initialized with zeros except `a[0]` which is 1000
- `i` is 1
- `n` must be greater than 1

The code updates `a[1]` to be the sum of `a[0]` and `x[0]`. Since `a[0]` is 1000 and `x[0]` is the first element of the list `x`, the new value of `a[1]` will be `1000 + x[0]`.

Therefore, the output state is:
Output State: **`t` is an integer such that 1 ≤ t ≤ 10^4, `n` is an input integer such that 2 ≤ n ≤ 500, `x` is a list of integers read from the input, `a` is a list of length `n` initialized with zeros except `a[0]` which is 1000 and `a[1]` which is 1000 + `x[0]`, `i` is 1, `n` must be greater than 1**