To determine the new value of `cnt` after executing the given line of code, we need to evaluate the expression `min(n // ((x + y) * x), m // ((x + y) * y))` with the given initial state.

Given:
- `x` is 3
- `y` is 1
- `gcd(3, 1) == 1` (which is true)
- `n` must be at least 12
- `cnt` is initially calculated as the sum of `min(n // ((3 + y) * 3), m // ((3 + y) * y))` for all `y` from 2 to the original `y` where `gcd(3, y) == 1`.

First, let's evaluate the new term added to `cnt`:
- `x + y = 3 + 1 = 4`
- `(x + y) * x = 4 * 3 = 12`
- `(x + y) * y = 4 * 1 = 4`
- The expression becomes `min(n // 12, m // 4)`.

Since `n` must be at least 12, `n // 12` will be at least 1. The value of `m // 4` depends on the value of `m`, but we don't have a specific value for `m`. However, we know that the minimum of these two values will be added to `cnt`.

Thus, the new value of `cnt` is the old value of `cnt` plus `min(n // 12, m // 4)`.

Output State: **`x` is 3, `y` is 1, `cnt` is the initial `cnt` plus `min(n // 12, m // 4)`, `n` must be at least 12, and the greatest common divisor of `x` and `y` is 1.**