Let's break down the problem step by step:

1. **Initial States:**
   - `m` must be greater than 0.
   - `count` is 1.
   - `a` is 1.
   - The value of `b` satisfies the condition `(a + b) % (b * func_1(a, b)) == 0`.

2. **Loop Condition:**
   - The loop runs for values of `b` in the range from 1 to `m + 1`.

3. **End of Previous Iteration:**
   - We know that `count` is 1, which means the condition `(a + b) % (b * func_1(a, b)) == 0` was satisfied for some value of `b` in the range from 1 to `m`.

4. **Next Iteration:**
   - For the loop to execute one more time, `b` must be incremented by 1, and it must still satisfy the condition `(a + b) % (b * func_1(a, b)) == 0`.
   - Since `a` is fixed at 1, the condition becomes `(1 + b) % (b * func_1(1, b)) == 0`.

5. **State Adjustment:**
   - `m` must still be greater than 0.
   - `count` must be reset to 1 because we are entering a new iteration.
   - `a` remains 1.
   - `b` must now be the value of `b` from the previous iteration plus 1, and this new value of `b` must satisfy the condition `(1 + b) % (b * func_1(1, b)) == 0`.

Given these points, the state at the start of the next iteration should be:

**State: `m` must be greater than 0, `count` is 1, `a` is 1, and the value of `b` satisfies the condition `(1 + b) % (b * func_1(1, b)) == 0`.**