Output State: `i` is equal to `x`, `x` is greater than `k - 1` and at least 2, `z` is 2^x + 1.

Explanation: The loop runs from `i = 0` to `i = x`, incrementing `i` by 1 each time. After each iteration, `z` is updated by adding `z // (k - 1) + 1` to its current value. Given the pattern observed from the first three iterations, we can deduce that after `x` iterations, `z` will be `2^x + 1`. This is because each iteration roughly doubles the value of `z` plus one, starting from `z = 1` when `i = 0`.