Let's break down the initial state and the print statement step by step:

1. **Initial State:**
   - `p1`, `p2`, and `p3` are integers where \(0 \leq p1 \leq p2 \leq p3 \leq 30\).
   - `t` is greater than 0.
   - `_` is 0.
   - `y` is equal to `p3 - 1`.
   - `x` is 1.
   - `p3` is greater than or equal to 2.

2. **Print Statement:**
   ```python
   print(p1 - x + p3)
   ```

3. **Variable Values:**
   - `p1` is an integer where \(0 \leq p1 \leq p3\).
   - `x` is 1.
   - `p3` is an integer where \(2 \leq p3 \leq 30\).

4. **Expression Calculation:**
   - The expression inside the print statement is `p1 - x + p3`.
   - Substituting the value of `x` (which is 1), the expression becomes `p1 - 1 + p3`.
   - Simplifying the expression, we get `p1 + p3 - 1`.

5. **Range of the Expression:**
   - Since \(0 \leq p1 \leq p3\) and \(2 \leq p3 \leq 30\), the minimum value of `p1 + p3 - 1` is when `p1` is 0 and `p3` is 2:
     \[
     0 + 2 - 1 = 1
     \]
   - The maximum value of `p1 + p3 - 1` is when `p1` is 30 and `p3` is 30:
     \[
     30 + 30 - 1 = 59
     \]

6. **Conclusion:**
   - The print statement will output a value that is the result of the expression `p1 + p3 - 1`, which ranges from 1 to 59.

Output: **p1 + p3 - 1 (where p1 is an integer such that 0 ≤ p1 ≤ p3, and p3 is an integer such that 2 ≤ p3 ≤ 30)**