Let's break down the initial state and the code snippet step by step:

1. **Initial State:**
   - `p1`, `p2`, and `p3` are integers where \(0 \leq p1 \leq p2 \leq p3 \leq 30\).
   - `t` is greater than 0.
   - `_` is 0.
   - `p3` must be greater than or equal to 4.
   - `y` is set to `p3 - 2`.
   - `x` is set to 2.

2. **Code Snippet:**
   ```python
   print(p1 - x + p3)
   ```

3. **Step-by-Step Calculation:**
   - `x` is explicitly set to 2.
   - The expression inside the `print` statement is `p1 - x + p3`.
   - Substituting the value of `x`, the expression becomes `p1 - 2 + p3`.
   - Since `p1` and `p3` are integers and \(0 \leq p1 \leq p3 \leq 30\), and `p3` is at least 4, the value of `p1 - 2 + p3` can be calculated as:
     - `p1 - 2` is an integer that is at least \(-2\) (if `p1` is 0) and at most \(28\) (if `p1` is 30).
     - Adding `p3` to `p1 - 2` results in an integer that is at least \(2\) (if `p1` is 0 and `p3` is 4) and at most \(58\) (if `p1` is 30 and `p3` is 30).

4. **Final Output:**
   - The `print` statement will output the value of `p1 - 2 + p3`.
   - Given the constraints, the exact value of `p1 - 2 + p3` depends on the specific values of `p1` and `p3`, but it will always be an integer between 2 and 58.

Output: **p1 - 2 + p3 (where p1 and p3 are integers such that 0 ≤ p1 ≤ p2 ≤ p3 ≤ 30 and p3 ≥ 4, resulting in an integer between 2 and 58)**