Output State: **`p1`, `p2`, and `p3` are integers where 0 ≤ `p1` ≤ `p2` ≤ `p3` ≤ 30, `t` is greater than 0, `_` is 0, and `y` is set to `p3 - (p3 - p1)`. If `p1 - (p3 - p1)` is less than or equal to `p2 - (p3 - (p3 - p1))`, the function prints `p1 - (p3 - p1) + p3` and breaks out of the loop. Otherwise, the loop continues until `y` is less than `x`, and the function prints `p3`.**

In simpler terms, after the loop has executed all its iterations:
- The variables `p1`, `p2`, and `p3` remain within their initial bounds (0 ≤ `p1` ≤ `p2` ≤ `p3` ≤ 30).
- The variable `t` remains greater than 0.
- The variable `_` remains 0.
- The variable `x` will be incremented by 1 for each iteration until the condition `p1 - x <= p2 - y` is met or `y` becomes less than `x`.
- The variable `y` will be decremented by 1 for each iteration until the condition `p1 - x <= p2 - y` is met or `y` becomes less than `x`.
- If the condition `p1 - x <= p2 - y` is met, the loop prints `p1 - x + p3` and exits.
- If the condition `p1 - x <= p2 - y` is never met, the loop will continue until `y` is less than `x`, and then it will print `p3`.