The code snippet `ans1 -= a[i] * 2` decrements the value of `ans1` by twice the value of the element at index `i` in the list `a`. Given that `i` is initially 0, this means `a[i]` is `a[0]`, the first element of the list `a`.

Therefore, the new value of `ans1` is the previous value of `ans1` minus `2 * a[0]`.

Output State: **`t` is an integer such that 0 ≤ t-2 ≤ 10^4, `n`, `k`, `x` are integers read from the input where 1 ≤ n ≤ 2 · 10^5, 1 ≤ k ≤ n, and `x` must be greater than 0; `a` is a list of `n` integers sorted in descending order as read from the input; `i` is 0; `ans1` is `sum(a) - 2 * a[k + x - 1] - 2 * a[0]`; `ans2` is `sum(a) - 2 * (a[k-1] + a[k] + ... + a[k + x - 2])`; `ans` is the maximum of `ans1` and `ans2` observed during the loop.**