To determine the output state, we need to analyze the provided initial state and the code snippet.

From the initial state:
- `n` is a positive integer such that \( 1 \leq n \leq 10^{10} \)
- `k` is a positive integer such that \( 1 \leq k \leq 10^{10} \)
- `min_sum` is calculated as \( \text{min\_sum} = k \times (k + 1) // 2 \)

The code snippet:
```
d = n // min_sum
```

Let's break down the impact of this code:
1. **Calculation of `min_sum`:** Before executing the code, we need to ensure `min_sum` is calculated based on the values of `k`. If `min_sum` is greater than `n`, the function would have returned -1, but we assume it hasn't, meaning `min_sum` is less than or equal to `n`.
2. **Assignment to `d`:** The variable `d` is assigned the integer division of `n` by `min_sum`. Since both `n` and `min_sum` are known and positive, `d` will be a non-negative integer.

Since the exact values of `n` and `k` have not been specified, we can summarize the output state based on the relationship established between `n`, `k`, and `min_sum`.

Therefore, the output state is:
Output State: **`n` is a positive integer such that 1 ≤ `n` ≤ 10^10, `k` is a positive integer such that 1 ≤ `k` ≤ 10^10; `min_sum` is calculated as `k * (k + 1) // 2`, and `d` is assigned the value `n // min_sum`.**