The code snippet assigns the value of `x2 - x1` to the variable `b`. Given that `x2` is greater than `x1` and `(x2 - x1)` is even, the value of `b` will be an even positive integer.

Here are the variables and their states after the code execution:
- `t` remains a positive integer such that 1 ≤ t ≤ 10^4.
- `r` remains a list containing six integers [h, w, x_a, y_a, x_b, y_b] where 1 ≤ x_a, x_b ≤ h ≤ 10^6 and 1 ≤ y_a, y_b ≤ w ≤ 10^9.
- `n` remains equal to `r[0]`.
- `m` remains equal to `r[1]`.
- `x1` remains equal to `r[2]`.
- `y1` remains equal to `r[3]`.
- `x2` remains equal to `r[4]`.
- `y2` remains equal to `r[5]`.
- `a` remains equal to `y1 - 1` if `y2` is greater than or equal to `y1`, otherwise `a` remains equal to `m - y1`.
- `b` is now equal to `x2 - x1`.

Output State: **`t` is a positive integer such that 1 ≤ t ≤ 10^4; `r` is a list containing six integers [h, w, x_a, y_a, x_b, y_b] where 1 ≤ x_a, x_b ≤ h ≤ 10^6 and 1 ≤ y_a, y_b ≤ w ≤ 10^9; `n` is equal to `r[0]`; `m` is equal to `r[1]`; `x1` is equal to `r[2]`; `y1` is equal to `r[3]`; `x2` is equal to `r[4]`; `y2` is equal to `r[5]`; `a` is equal to `y1 - 1` if `y2` is greater than or equal to `y1`, otherwise `a` is equal to `m - y1`; `b` is equal to `x2 - x1`.**