The value of `x1` is incremented by `a`. Given the initial conditions, `a` is calculated as `y1 - 1` if `y2` is greater than or equal to `y1`, otherwise `a` is `m - y1`. Therefore, the new value of `x1` will be `x1 + a`.

Other variables remain unchanged.

Output State: **`t` is `abs(y2 - y1)`, `r` is a list containing six integers [h, w, x_a, y_a, x_b, y_b] where 1 ≤ x_a, x_b ≤ h ≤ 10^6 and 1 ≤ y_a, y_b ≤ w ≤ 10^9; `n` is equal to `r[0]`; `m` is equal to `r[1]`; `x1` is equal to `r[2] + a`; `y1` is equal to `r[3]`; `x2` is equal to `r[4]`; `y2` is equal to `r[5]`; `a` is equal to `y1 - 1` if `y2` is greater than or equal to `y1`, otherwise `a` is equal to `m - y1`; `b` is equal to `x2 - x1`.**