The given Python code snippet reverses the list `a`. 

Given the initial state, `a` is a list defined as:
\[ a = [1000, 1000 - T[0], (1000 - T[0]) - T[1], \ldots, 1000 - (T[0] + T[1] + \ldots + T[n-2])] \]

After executing the line `a = a[::-1]`, the list `a` is reversed. This means the first element becomes the last, the second element becomes the second-to-last, and so on.

Therefore, the new `a` will be:
\[ a = [1000 - (T[0] + T[1] + \ldots + T[n-2]), \ldots, (1000 - T[0]) - T[1], 1000 - T[0], 1000] \]

The other variables (`t`, `n`, `x`, `T`) remain unchanged.

Output State: **`t` is an integer such that 0 ≤ t ≤ 10^4 - 1, `n` must be greater than 0, `x` is a list of n-1 integers where each element x_i satisfies 1 ≤ x_i ≤ 500, `T` is a list of integers derived from splitting and converting the string `line`, `a` is `[1000 - (T[0] + T[1] + ... + T[n-2]), ..., (1000 - T[0]) - T[1], 1000 - T[0], 1000]`**.