Given the initial state, `n -= m` reduces the value of `n` by `m`. Since `m` is defined as `(n + 1) // 2`, the new value of `n` can be calculated as follows:

- Initially, `m` is `(n + 1) // 2`.
- After executing `n -= m`, the new value of `n` is `n - (n + 1) // 2`.

Since `n` must be at least 2, let's consider the minimum case where `n` is 2:
- `m` would be `(2 + 1) // 2 = 1`.
- After `n -= m`, `n` becomes `2 - 1 = 1`.

However, since `n` must be at least 2, the smallest valid `n` is 2, and the calculation above shows that `n` would become 1, which violates the precondition. Therefore, `n` must be greater than 2 to satisfy the condition `n >= 2` after the operation.

Let's consider a general case where `n` is greater than 2:
- If `n` is an even number, say `n = 4`, then `m` would be `(4 + 1) // 2 = 2`, and `n` becomes `4 - 2 = 2`.
- If `n` is an odd number, say `n = 5`, then `m` would be `(5 + 1) // 2 = 3`, and `n` becomes `5 - 3 = 2`.

In both cases, after the operation, `n` becomes 2, which is the smallest valid value for `n` according to the precondition.

Therefore, the output state is:
Output State: **`t` is 3; `n` is 2; `k` is the second integer from the input; `L` is `[(n + 1) // 2, (n + 1) // 2]`; `tot` is 5; `pow` is 8; `m` is `(n + 1) // 2`**

In natural language: The value of `n` is now 2, while all other variables remain unchanged except that `m` is recalculated based on the new value of `n`.