To determine what will be printed, let's break down the expression inside the `print` statement step-by-step using the given initial state:

1. **Identify the variables and their values:**
   - `t = 3` (though `t` is not used in the print statement)
   - `n = 0` (though `n` is not used in the print statement)
   - `k` is the second integer from the input (its exact value is not provided, so we'll keep it as `k`)
   - `L = [1, 1, 1, 1, 1]` (though `L` is not used in the print statement)
   - `pow = 2`
   - `m = 1` (though `m` is not used in the print statement)
   - `tot` is initially not specified but is increased by `a` (which is 1). Since `a` is 1, `tot` becomes 1.
   - `a = 1`

2. **Evaluate the expression inside the print statement:**
   - The expression is `pow * (2 * (k - tot) - 1)`
   - Substitute the known values into the expression:
     - `pow = 2`
     - `tot = 1`
     - `k` remains as `k` (unknown value)

3. **Simplify the expression:**
   - `pow * (2 * (k - tot) - 1)`
   - `= 2 * (2 * (k - 1) - 1)`
   - `= 2 * (2k - 2 - 1)`
   - `= 2 * (2k - 3)`
   - `= 4k - 6`

Thus, the output of the print statement depends on the value of `k`. Without the specific value of `k`, we can only express the output in terms of `k`.

Output: **4k - 6 (where k is the second integer from the input)**