To determine what will be printed, let's break down the expression step by step:

1. **Expression Breakdown:**
   \[
   (k // 2 + k \% 2) \times (k < 4 \times n - 3) + 2 \times n \times (k \geq 4 \times n - 3) + (k == 4 \times n - 2)
   \]

2. **Understanding Variables:**
   - `n`: First integer from the input split by spaces.
   - `k`: Second integer from the input split by spaces.
   - `s`: First line of input (not used in the expression).

3. **Expression Analysis:**
   - `(k // 2 + k % 2)`: This part evaluates to `k` because `k // 2` gives the integer division of `k` by 2, and `k % 2` gives the remainder when `k` is divided by 2. Adding these two results gives `k`.
   - `(k < 4 * n - 3)`: This is a boolean expression that evaluates to `True` if `k` is less than `4 * n - 3`, and `False` otherwise.
   - `(k >= 4 * n - 3)`: This is a boolean expression that evaluates to `True` if `k` is greater than or equal to `4 * n - 3`, and `False` otherwise.
   - `(k == 4 * n - 2)`: This is a boolean expression that evaluates to `True` if `k` is exactly `4 * n - 2`, and `False` otherwise.

4. **Combining the Expressions:**
   - If `k < 4 * n - 3`, then the expression simplifies to `k`.
   - If `k >= 4 * n - 3` and `k != 4 * n - 2`, then the expression simplifies to `2 * n`.
   - If `k == 4 * n - 2`, then the expression simplifies to `1`.

Given this breakdown, the output depends on the relationship between `k` and `4 * n - 3`:

- If `k < 4 * n - 3`, the output is `k`.
- If `k >= 4 * n - 3` and `k != 4 * n - 2`, the output is `2 * n`.
- If `k == 4 * n - 2`, the output is `1`.

Therefore, the output will be one of the following based on the values of `k` and `n`:
- If `k < 4 * n - 3`, the output is `k`.
- If `k >= 4 * n - 3` and `k != 4 * n - 2`, the output is `2 * n`.
- If `k == 4 * n - 2`, the output is `1`.

Output: **k (if k < 4 * n - 3), 2 * n (if k >= 4 * n - 3 and k != 4 * n - 2), or 1 (if k == 4 * n - 2)**