Let's break down the problem step by step:

1. **Identify the loop condition**: The loop condition is given by the expression `(x + y) * x <= n and (x + y) * y <= m`.

2. **Identify the variables in the loop head**: The variables involved in the loop condition are `x`, `y`, `n`, and `m`.

3. **Current state before the loop**:
   - `x` is 2
   - `y` is 1
   - `n` is at least 5
   - `m` is at least 20

4. **Evaluate the loop condition with the current state**:
   - Calculate `(x + y) * x`: 
     \[
     (2 + 1) * 2 = 3 * 2 = 6
     \]
   - Check if `6 <= n`: Since `n` is at least 5, this part of the condition is satisfied.
   - Calculate `(x + y) * y`:
     \[
     (2 + 1) * 1 = 3 * 1 = 3
     \]
   - Check if `3 <= m`: Since `m` is at least 20, this part of the condition is also satisfied.

Since both parts of the condition are already satisfied with the current values, no adjustments are necessary for the loop to execute the first time.

**Final Answer**:
State: **`x` is 2, `y` is 1, `n` is at least 5, `m` is at least 20**