Let's break down the initial state and the logic step by step:

1. **Initial State:**
   - `n` is at least 5.
   - `j` is `n // 2 - 2`.
   - `k` is `n - (n // 2 - 2)`.

2. **Conditions:**
   - If `s[k]` is '?' or `s[k + j]` is '?' or `s[k]` is equal to `s[k + j]`, then `count` is 1.
   - Otherwise, `count` is 0.
   - Additionally, `count` is equal to `j`.

3. **Analyzing the Conditions:**
   - Since `count` is equal to `j`, we need to determine the value of `j`.
   - Given `n` is at least 5, let's calculate `j`:
     - `j = n // 2 - 2`
     - For example, if `n = 5`, then `j = 5 // 2 - 2 = 2 - 2 = 0`.
     - If `n = 6`, then `j = 6 // 2 - 2 = 3 - 2 = 1`.
     - If `n = 7`, then `j = 7 // 2 - 2 = 3 - 2 = 1`.
     - If `n = 8`, then `j = 8 // 2 - 2 = 4 - 2 = 2`.
     - And so on...

4. **Determining `k`:**
   - `k = n - (n // 2 - 2)`
   - For example, if `n = 5`, then `k = 5 - (5 // 2 - 2) = 5 - (2 - 2) = 5 - 0 = 5`.
   - If `n = 6`, then `k = 6 - (6 // 2 - 2) = 6 - (3 - 2) = 6 - 1 = 5`.
   - If `n = 7`, then `k = 7 - (7 // 2 - 2) = 7 - (3 - 2) = 7 - 1 = 6`.
   - If `n = 8`, then `k = 8 - (8 // 2 - 2) = 8 - (4 - 2) = 8 - 2 = 6`.

5. **Evaluating the Condition:**
   - The condition states that if `s[k]` is '?' or `s[k + j]` is '?' or `s[k]` is equal to `s[k + j]`, then `count` is 1. Otherwise, `count` is 0.
   - However, it also states that `count` is equal to `j`.
   - This means that `count` must be equal to `j`, which implies that the condition `s[k]` is '?' or `s[k + j]` is '?' or `s[k]` is equal to `s[k + j]` must always be true, because otherwise `count` would be 0, which contradicts `count` being equal to `j`.

6. **Final Calculation:**
   - Since `count` is equal to `j`, and `j` is `n // 2 - 2`, the value of `count` is `n // 2 - 2`.
   - The print statement is `print(count * 2)`.
   - Therefore, the output will be `(n // 2 - 2) * 2`.

Given the above analysis, the output will be:

Output: **(n // 2 - 2) * 2**