Let's break down the initial state and the print statement step by step:

1. **Initial State:**
   - `p1`, `p2`, and `p3` are integers provided by the user such that \(0 \leq p1 \leq p2 \leq p3 \leq 30\).
   - `t` is greater than 2 (though it is not used in the print statement).
   - `_` is 2 (though it is not used in the print statement).
   - `low` is the minimum of `p3 - p1` and `p3 - p2`.
   - `high` is the maximum of `p3 - p1` and `p3 - p2`.
   - `cur` is equal to `low`.
   - The current value of `p1 - cur` is less than or equal to `p2 - (p3 - cur)`.

2. **Determine `low` and `high`:**
   - Since \(p1 \leq p2 \leq p3\), `p3 - p1` will always be greater than or equal to `p3 - p2`.
   - Therefore, `low` is `p3 - p2` and `high` is `p3 - p1`.

3. **Determine `cur`:**
   - `cur` is equal to `low`, which is `p3 - p2`.

4. **Evaluate the condition `p1 - cur <= p2 - (p3 - cur)`:**
   - Substitute `cur` with `p3 - p2`:
     \[
     p1 - (p3 - p2) \leq p2 - (p3 - (p3 - p2))
     \]
   - Simplify the right side:
     \[
     p1 - (p3 - p2) \leq p2 - p2
     \]
     \[
     p1 - (p3 - p2) \leq 0
     \]
   - Simplify the left side:
     \[
     p1 - p3 + p2 \leq 0
     \]
   - Rearrange the inequality:
     \[
     p1 + p2 \leq p3
     \]
   - This condition is always true because \(p1 \leq p2 \leq p3\).

5. **Calculate the value of the print statement:**
   - The print statement is:
     \[
     print(p1 - cur + p3)
     \]
   - Substitute `cur` with `p3 - p2`:
     \[
     print(p1 - (p3 - p2) + p3)
     \]
   - Simplify the expression:
     \[
     print(p1 - p3 + p2 + p3)
     \]
     \[
     print(p1 + p2)
     \]

Given the initial state and the steps above, the value printed by the print statement is the sum of `p1` and `p2`.

Output: **p1 + p2 (where p1 and p2 are integers provided by the user such that 0 <= p1 <= p2 <= p3 <= 30)**