Let's break down the initial state and the Python code snippet to determine what will be printed:

### Initial State:
- `n` and `m` are integers converted from their original string values.
- `b` is `min(n, m) + 1`.
- `t` is greater than or equal to 1.
- `T` is 1.
- `ans` is calculated as `n + sum((n + b) // (b * b) for b in range(2, min(n, m) + 1))`.

### Step-by-Step Calculation:
1. **Determine `b`**:
   - `b` is defined as `min(n, m) + 1`.
   - This means `b` is one more than the smaller of `n` and `m`.

2. **Calculate `ans`**:
   - `ans` is defined as `n + sum((n + b) // (b * b) for b in range(2, min(n, m) + 1))`.
   - Let's break this down further:
     - The range `range(2, min(n, m) + 1)` generates numbers from 2 up to and including `min(n, m)`.
     - For each value of `b` in this range, the expression `(n + b) // (b * b)` is evaluated.
     - The results of these evaluations are summed up.
     - Finally, `n` is added to this sum to get `ans`.

### Example Calculation:
Let's assume `n = 5` and `m = 7` for a concrete example:
- `min(n, m) = 5`.
- `b = min(n, m) + 1 = 5 + 1 = 6`.

Now, calculate `ans`:
- The range is `range(2, 6)`, which gives us the values 2, 3, 4, and 5.
- For each `b` in this range:
  - When `b = 2`: \((5 + 2) // (2 * 2) = 7 // 4 = 1\).
  - When `b = 3`: \((5 + 3) // (3 * 3) = 8 // 9 = 0\).
  - When `b = 4`: \((5 + 4) // (4 * 4) = 9 // 16 = 0\).
  - When `b = 5`: \((5 + 5) // (5 * 5) = 10 // 25 = 0\).

Summing these results: \(1 + 0 + 0 + 0 = 1\).

Finally, `ans` is:
\[ ans = n + sum = 5 + 1 = 6 \]

### General Case:
For any given `n` and `m`:
- `b` is `min(n, m) + 1`.
- The sum is calculated over the range from 2 to `min(n, m)`.
- Each term in the sum is \((n + b) // (b * b)\), where `b` is the current value in the range.
- The final `ans` is `n` plus this sum.

### Final Output:
The `print(ans)` statement will print the value of `ans` as calculated above.

Output: **ans (where ans is n + sum((n + b) // (b * b) for b in range(2, min(n, m) + 1)))**