Alright, I have this problem to solve. Let's read it carefully.

So, there are n possible outcomes in a game, and for each outcome, there's a multiplier k_i. I need to bet some integer amount x_i on each outcome. The condition is that no matter which outcome wins, the total return should be more than the total amount I bet.

More formally, if I bet x_1, x_2, ..., x_n on outcomes 1 to n, and the total bet is S = x_1 + x_2 + ... + x_n, then for each i, the return if outcome i wins is k_i * x_i, and this should be greater than S.

So, for each i, k_i * x_i > S.

But S is the sum of all x's, including x_i.

This seems a bit tricky. I need to find such x_i's that satisfy this condition for every i.

Let me think about a simple case. Suppose n=1. Then, S = x_1, and k_1 * x_1 > S, which is k_1 * x_1 > x_1. Since k_1 >= 2, this is always true for any x_1 >=1. So, for n=1, it's always possible.

Now, for n=2, let's say k_1 and k_2. S = x_1 + x_2.

The conditions are:

k_1 * x_1 > x_1 + x_2

k_2 * x_2 > x_1 + x_2

From the first inequality: k_1 * x_1 > S => k_1 * x_1 > x_1 + x_2 => (k_1 - 1) * x_1 > x_2

Similarly, from the second inequality: (k_2 - 1) * x_2 > x_1

So, we have:

x_2 < (k_1 - 1) * x_1

and

x_1 < (k_2 - 1) * x_2

This seems like a system of inequalities that I need to solve for x_1 and x_2.

Let me try to express one variable in terms of the other.

From the second inequality: x_1 < (k_2 - 1) * x_2

Plug this into the first inequality:

x_2 < (k_1 - 1) * x_1 < (k_1 - 1)*(k_2 - 1)*x_2

So, x_2 < (k_1 - 1)*(k_2 - 1)*x_2

For this to hold, (k_1 - 1)*(k_2 - 1) > 1

Because x_2 is positive.

So, if (k_1 - 1)*(k_2 - 1) > 1, then there exists x_1 and x_2 satisfying the conditions.

Similarly, for n=3, I would have to have:

(k_1 - 1)*(k_2 - 1)*(k_3 - 1) > 1, and so on.

Wait, is that the general condition?

Let me check for n=2 again.

If k_1=2 and k_2=2, then (2-1)*(2-1)=1, which is not greater than 1, so no solution exists?

But wait, if k_1=2 and k_2=2, let's see:

The inequalities are:

x_2 < x_1

and

x_1 < x_2

Which implies x_1 < x_2 < x_1, which is impossible. So, no solution exists, which matches the condition.

So, for n=2, solution exists only if (k_1 - 1)*(k_2 - 1) > 1.

Similarly, for n=3, it should be (k_1 - 1)*(k_2 - 1)*(k_3 - 1) > 1.

Wait, but in the problem, n can be up to 50, and k_i >=2, so for n>=2, product can be large.

But in the example, one of the test cases has n=3 with k=[3,2,7], and it has a solution.

Let's check the product: (3-1)*(2-1)*(7-1)=2*1*6=12 >1, so solution exists.

Another test case: n=3, k=[6,3,2], product is (5)*(2)*(1)=10 >1, but output is -1, which seems contradictory.

Wait, no, in the example, for n=3, k=[6,3,2], output is -1, but according to my earlier logic, product is 5*2*1=10 >1, so solution should exist, but output is -1. So, maybe my assumption is wrong.

Hmm, perhaps I need to think differently.

Let me look at the problem again.

I need to find x_i >=1 integers such that for each i, k_i * x_i > S, where S = sum of all x_j.

Let me rearrange the inequality: k_i * x_i > S = x_1 + x_2 + ... + x_n.

Since S includes x_i, I can write: k_i * x_i > x_i + x_2 + ... + x_n.

Which implies (k_i -1) * x_i > x_1 + x_2 + ... + x_n - x_i.

Which is (k_i -1) * x_i > S - x_i.

But S - x_i is the sum of all other x_j's.

So, (k_i -1) * x_i > sum of other x_j's.

Similarly, for each i, (k_i -1) * x_i > sum of other x_j's.

This seems similar to the marriage theorem or some kind of feasibility condition.

Maybe I can think in terms of proportions.

Let me assume that x_i = c * y_i, where y_i are positive integers and c is a positive real number to be determined.

Then, S = c * sum(y_i).

And the condition is k_i * c * y_i > c * sum(y_i), which simplifies to k_i * y_i > sum(y_i).

Wait, this seems promising.

So, for each i, k_i * y_i > sum(y_i).

Let me denote sum(y_i) = Y.

Then, k_i * y_i > Y for each i.

Which can be written as y_i / Y > 1 / k_i.

But sum(y_i) = Y, so sum(y_i / Y) = 1.

So, sum(1 / k_i) < 1 is a necessary condition for the existence of such y_i's.

Wait, let's see.

If sum(1 / k_i) >1, then it's impossible to have y_i / Y > 1 / k_i for all i, because sum(y_i / Y) =1.

But if sum(1 / k_i) <1, then it's possible to choose y_i such that y_i / Y > 1 / k_i for all i.

So, the condition for the existence of a solution is sum(1 / k_i) <1.

Let me check this with the example.

In the first test case, n=3, k=[3,2,7].

Sum of 1/k_i = 1/3 + 1/2 + 1/7 = (14 + 21 + 6)/42 = 41/42 <1, so solution exists, which matches the example.

In the third test case, n=5, k=[5,5,5,5,5].

Sum of 1/k_i = 5*(1/5) =1, which is not less than 1, so no solution, output -1, which matches the example.

In the fifth test case, n=3, k=[6,3,2].

Sum of 1/k_i = 1/6 + 1/3 + 1/2 = 1/6 + 2/6 + 3/6 = 6/6 =1, which is not less than 1, so no solution, output -1, which matches.

In the second test case, n=2, k=[3,3].

Sum of 1/k_i =1/3 +1/3=2/3 <1, so solution exists, which matches the example.

In the fourth test case, n=6, k=[7,9,3,17,9,13].

Sum of 1/k_i =1/7 +1/9 +1/3 +1/17 +1/9 +1/13.

Let's calculate this:

1/7 ≈0.1429

1/9 ≈0.1111

1/3 ≈0.3333

1/17≈0.0588

1/9≈0.1111

1/13≈0.0769

Sum ≈0.1429+0.1111+0.3333+0.0588+0.1111+0.0769≈0.8341 <1, so solution exists, which matches the example.

In the sixth test case, n=5, k=[9,4,6,8,3].

Sum of 1/k_i =1/9 +1/4 +1/6 +1/8 +1/3 = (8+18+12+9+24)/72 = 71/72 <1, so solution exists, which matches.

So, the condition is sum(1/k_i) <1.

Now, assuming this condition holds, how to find such x_i's?

One way is to set x_i proportional to 1/(k_i -1).

Because from earlier, we have (k_i -1)*x_i > S.

If I set x_i = c / (k_i -1), then S = c * sum(1/(k_i -1)).

Then, (k_i -1)*x_i = (k_i -1)*(c/(k_i -1)) = c.

So, c > c * sum(1/(k_i -1)).

Which simplifies to 1 > sum(1/(k_i -1)).

But this is not directly helpful.

Wait, perhaps I need to adjust the constants.

Let me try to set x_i = y_i, where y_i are positive integers, and find c such that S = c * sum(y_i).

Then, (k_i -1)*x_i > S => (k_i -1)*y_i > c*sum(y_i).

Then, c < (k_i -1)*y_i / sum(y_i).

We need this to hold for all i.

So, c < min_over_i { (k_i -1)*y_i / sum(y_i) }.

To maximize c, we need to choose y_i such that this min is as large as possible.

This seems tricky.

Alternatively, I can use the condition that sum(1/k_i) <1, and set x_i proportional to 1/k_i.

But I need integer x_i.

Wait, perhaps I can set x_i = floor(c / k_i) for some c.

But this seems messy.

Let me look for a different approach.

I recall that in some optimization problems, using the least common multiple (LCM) can help in finding integer solutions.

Let me think about it.

Suppose I set x_i = (LCM of all k_j's) / k_i.

Then, k_i * x_i = LCM.

And S = sum over i of (LCM / k_i).

If LCM > S, then k_i * x_i > S for all i.

Wait, let's see.

Let L = LCM of all k_i.

Set x_i = L / k_i.

Then, S = sum over i of (L / k_i).

We need L > S, which is L > sum over i of (L / k_i), which simplifies to 1 > sum over i of (1 / k_i).

But we already have the condition that sum over i of (1 / k_i) <1, so this should hold.

Therefore, this is a valid way to set x_i.

Moreover, since L is a multiple of k_i, x_i is an integer.

Also, x_i >=1 because L >= k_i (since L is LCM of all k_j's, and k_i divides L).

So, this seems like a correct way to set x_i.

Let me check with the first test case.

n=3, k=[3,2,7].

LCM of 3,2,7 is 42.

Then, x_1 =42/3=14, x_2=42/2=21, x_3=42/7=6.

Sum S=14+21+6=41.

Then, for each i:

k_1 * x_1 =3*14=42 >41

k_2 * x_2 =2*21=42 >41

k_3 * x_3 =7*6=42 >41

So, this works.

But in the example, the output is 27 41 12, which sums to 80, and:

3*27=81 >80

2*41=82 >80

7*12=84 >80

So, their solution is different, but both are valid.

So, my approach of setting x_i = L / k_i is correct, but not unique.

Now, let's see for n=2, k=[3,3].

LCM=3.

x_1=3/3=1, x_2=3/3=1.

Sum S=1+1=2.

Check:

3*1=3 >2

3*1=3 >2

So, it works, matches the example.

For n=6, k=[7,9,3,17,9,13].

LCM of 7,9,3,17,9,13.

First, LCM of 7 and 9 is 63.

LCM of 63 and 3 is 63.

LCM of 63 and 17 is 63*17=1071.

LCM of 1071 and 9 is still 1071.

LCM of 1071 and 13 is 1071*13=13923.

So, L=13923.

Then, x_i = L / k_i.

x1=13923/7=1989

x2=13923/9=1547

x3=13923/3=4641

x4=13923/17=819

x5=13923/9=1547

x6=13923/13=1071

Sum S=1989+1547+4641+819+1547+1071=11614

Check:

7*1989=13923 >11614

9*1547=13923 >11614

3*4641=13923 >11614

17*819=13923 >11614

9*1547=13923 >11614

13*1071=13923 >11614

So, it works.

In the example, the output is 1989 1547 4641 819 1547 1071, which matches this.

Now, for n=5, k=[5,5,5,5,5].

LCM=5.

x_i=5/5=1 for all i.

Sum S=5.

Check:

5*1=5 not >5

So, no solution exists, which matches the example.

For n=3, k=[6,3,2].

LCM=6.

x1=6/6=1, x2=6/3=2, x3=6/2=3.

Sum S=1+2+3=6.

Check:

6*1=6 not >6

3*2=6 not >6

2*3=6 not >6

So, no solution exists, which matches the example.

For n=5, k=[9,4,6,8,3].

LCM of 9,4,6,8,3 is LCM of 9 and 4 is 36, LCM of 36 and 6 is 36, LCM of 36 and 8 is 72, LCM of 72 and 3 is 72.

So, L=72.

x1=72/9=8, x2=72/4=18, x3=72/6=12, x4=72/8=9, x5=72/3=24.

Sum S=8+18+12+9+24=71.

Check:

9*8=72 >71

4*18=72 >71

6*12=72 >71

8*9=72 >71

3*24=72 >71

So, it works, matches the example.

Therefore, this approach seems correct.

Now, in the code, they are doing exactly this.

They are computing the LCM of all k_i, then setting x_i = L / k_i, where L is the LCM.

Then, checking if sum(x_i) < L.

If yes, output the x_i's; else, output -1.

This matches my reasoning.

Hence, the program is correct.

**Final Answer**

\[ \boxed{\text{See Solution}} \]