Alright, I've got this problem to solve. Let's see what it's asking for. So, there are n possible outcomes in a game, and for each outcome, there's a multiplier k_i. I need to bet some integer amount x_i on each outcome. The goal is to set these bets such that no matter which outcome wins, the amount I get back is more than the total amount I bet.

More formally, if outcome i wins, I get back k_i * x_i coins, and this should be greater than the total sum of all bets, which is sum(x_j for all j from 1 to n). This needs to hold for every possible winning outcome.

First, I need to understand the constraints:

- There are t test cases, up to 10^4 of them.

- For each test case, n can be up to 50.

- Each k_i is between 2 and 20.

- The sum of n over all test cases is up to 2*10^5, which is manageable.

So, for each test case, I need to either find a set of bets x_i (each at least 1 and up to 10^9) that satisfy the condition for all outcomes, or determine that no such set exists.

Let me try to think about how to approach this.

First, the condition is that for every i from 1 to n:

k_i * x_i > sum(x_j for all j from 1 to n)

This needs to hold for all i simultaneously.

This seems a bit tricky. Let's see if I can manipulate this inequality to find a relationship between the x_i's and the k_i's.

Let me denote s = sum(x_j for all j from 1 to n).

Then, for each i:

k_i * x_i > s

But s = sum(x_j for all j from 1 to n) = x_i + sum(x_j for j != i)

So, k_i * x_i > x_i + sum(x_j for j != i)

Subtract x_i from both sides:

(k_i - 1) * x_i > sum(x_j for j != i)

This seems a bit better.

Now, sum(x_j for j != i) = s - x_i

So, (k_i - 1) * x_i > s - x_i

Add x_i to both sides:

k_i * x_i > s

Wait, that's back to the original inequality. Maybe I need a different approach.

Let me consider that s < min(k_i * x_i for all i)

Because s must be less than each k_i * x_i.

But s = sum(x_j for all j)

So, s < k_i * x_i for all i.

I need to find x_i's such that sum(x_j) < k_i * x_i for all i.

This seems tricky. Maybe I can use the concept of least common multiples or something similar.

Let me look at an example to get some intuition.

Take the first example from the input:

n=3

k=[3,2,7]

One possible solution is x=[27,41,12]

Let's check:

s = 27 + 41 + 12 = 80

For outcome 1: 3*27 = 81 > 80

For outcome 2: 2*41 = 82 > 80

For outcome 3: 7*12 = 84 > 80

Okay, this works.

Another test case:

n=2

k=[3,3]

Solution: x=[1,1]

s=2

3*1=3 >2 for both outcomes.

Good.

Another test case:

n=5

k=[5,5,5,5,5]

Output: -1

Hmm, why is that?

Let's see:

If all k_i are equal, say k=5, then we need s < 5*x_i for all i.

Since s = sum(x_j), and x_j >=1, let's see what's the minimal s.

If x_i =1 for all i, then s=5

But 5*x_i =5, which is not greater than s=5.

So, s must be less than 5*x_i for all i.

But if x_i=1, s=5, which is not less than 5*1=5.

If x_i=2, s=10, which is not less than 5*2=10.

Wait, it needs to be strictly less.

So, s < 5*x_i for all i.

But s = sum(x_j), so minimal s is n*min_x, where min_x is the smallest x_i.

In this case, if all x_i are equal, say x, then s=5*x

Then, 5*x < 5*x for all i, which is impossible since 5*x cannot be less than 5*x.

Hence, no solution exists when all k_i are equal.

Makes sense why output is -1.

Another test case:

n=6

k=[7,9,3,17,9,13]

Solution: x=[1989,1547,4641,819,1547,1071]

Let's check:

s = 1989 + 1547 + 4641 + 819 + 1547 + 1071 = 11614

Then:

7*1989=13923 >11614

9*1547=13923 >11614

3*4641=13923 >11614

17*819=13923 >11614

9*1547=13923 >11614

13*1071=13923 >11614

All conditions are satisfied.

Interesting.

Now, how to generalize this.

I need a method to find x_i such that for each i, k_i*x_i > sum(x_j for all j)

Let me try to express x_i in terms of the other variables.

Let me denote s = sum(x_j for all j)

Then, for each i, k_i*x_i > s

But s = sum(x_j for j != i) + x_i

So, k_i*x_i > sum(x_j for j != i) + x_i

Which implies (k_i - 1)*x_i > sum(x_j for j != i)

This seems useful.

Now, if I can find a way to express sum(x_j for j != i) in terms of x_i, but that seems tricky.

Alternatively, maybe I can assign x_i proportional to some function of k_i.

Let me consider that.

Suppose I set x_i = c / (k_i - 1) for some constant c.

Then, s = sum(c / (k_i -1) for all i)

And for each i, k_i * x_i = k_i * (c / (k_i -1)) = (k_i / (k_i -1)) * c

I need this to be greater than s.

So, (k_i / (k_i -1)) * c > s

But s = sum(c / (k_j -1) for all j)

So, (k_i / (k_i -1)) * c > sum(c / (k_j -1) for all j)

Divide both sides by c (assuming c>0):

k_i / (k_i -1) > sum(1 / (k_j -1) for all j)

This needs to hold for all i.

But this seems like a condition that must be satisfied for a solution to exist.

In other words, for a solution to exist, the following must hold for all i:

k_i / (k_i -1) > sum(1 / (k_j -1) for all j)

This seems like a necessary condition.

Is it also sufficient?

Let me check with the earlier examples.

First example:

n=3

k=[3,2,7]

Compute sum(1/(k_j -1)) = 1/(3-1) + 1/(2-1) + 1/(7-1) = 1/2 + 1 + 1/6 = (3/6 + 6/6 + 1/6) = 10/6 = 5/3

Now, for each i:

k_i / (k_i -1) > 5/3

For i=1: 3/(3-1) = 3/2 > 5/3 ? 3/2 = 1.5, 5/3 ≈1.666, so 1.5 > 1.666? No.

Wait, but in the example, a solution exists. So, my condition seems incorrect.

Hmm, maybe I messed up somewhere.

Let me re-examine my earlier steps.

I set x_i = c / (k_i -1)

Then s = sum(c / (k_j -1) for all j)

And for each i, k_i * x_i = (k_i / (k_i -1)) * c > s = sum(c / (k_j -1) for all j)

Divide both sides by c (assuming c>0):

k_i / (k_i -1) > sum(1 / (k_j -1) for all j)

But in the first example, sum(1 / (k_j -1)) = 1/2 + 1 + 1/6 = 10/6 = 5/3

For i=1: 3/(3-1) = 3/2 = 1.5 > 5/3 ≈1.666? No, 1.5 < 1.666

But a solution exists (x=[27,41,12]), so my condition is not holding.

Hence, perhaps my approach is incorrect.

Let me try another approach.

Let me consider that s < k_i * x_i for all i.

This implies that x_i > s / k_i for all i.

But s = sum(x_j for all j), so x_i > (sum(x_j for all j)) / k_i

This seems tricky to handle directly.

Maybe I can use the method of setting x_i proportional to 1 / k_i.

Let me set x_i = c / k_i for some constant c.

Then s = sum(c / k_j for all j)

And for each i, k_i * x_i = k_i * (c / k_i) = c > s

So, c > sum(c / k_j for all j)

Divide both sides by c: 1 > sum(1 / k_j for all j)

Which implies that sum(1 / k_j for all j) < 1

But in the first example, sum(1/k_j) = 1/3 + 1/2 + 1/7 ≈ 0.333 + 0.5 + 0.142 ≈ 0.975 <1

And a solution exists.

In the second example, n=2, k=[3,3], sum(1/3 + 1/3) = 2/3 <1, and solution exists (x=[1,1])

In the third example, n=5, k=[5,5,5,5,5], sum(1/5 for 5 times) =1, and output is -1.

So, when sum(1/k_j) <1, solution exists; when sum(1/k_j)=1, no solution.

Wait, but in the third example, sum(1/k_j)=1, no solution.

So, perhaps the condition is sum(1/k_j) <1 for a solution to exist.

But in the first example, sum(1/k_j)=0.975<1, solution exists.

In the second example, sum=2/3<1, solution exists.

In the third example, sum=1, no solution.

Another test case:

n=6, k=[7,9,3,17,9,13], sum(1/7 + 1/9 + 1/3 + 1/17 + 1/9 + 1/13)

Calculate:

1/7 ≈0.1428

1/9≈0.1111

1/3≈0.3333

1/17≈0.0588

1/9≈0.1111

1/13≈0.0769

Sum≈0.1428+0.1111+0.3333+0.0588+0.1111+0.0769≈0.834

Which is less than 1, and a solution exists.

Another test case:

n=3, k=[6,3,2], sum(1/6 + 1/3 + 1/2)=0.1667 + 0.3333 + 0.5=1, output -1

Indeed, sum=1, no solution.

Another test case:

n=5, k=[9,4,6,8,3], sum(1/9 + 1/4 + 1/6 + 1/8 + 1/3)=0.1111 + 0.25 + 0.1667 + 0.125 + 0.3333≈0.9861<1, solution exists.

So, it seems that if sum(1/k_j) <1, then a solution exists; otherwise, no solution.

This seems to be a valid condition.

Now, assuming sum(1/k_j) <1, how to find such x_i's?

Let me consider setting x_i = c / k_i for some constant c.

Then s = sum(c / k_j for all j)

We need c > s = sum(c / k_j for all j)

Which simplifies to c > c * sum(1 / k_j)

Divide both sides by c: 1 > sum(1 / k_j)

Which is exactly our condition for the solution to exist.

So, if sum(1 / k_j) <1, then any c >0 will satisfy this inequality.

But we need x_i to be integers, and at least 1.

So, I need to choose c such that c / k_i >=1 for all i, i.e., c >= k_i for all i.

Wait, c / k_i should be at least 1, so c >= k_i for all i.

But to make sure that c > sum(c / k_j), which is equivalent to c * (1 - sum(1 / k_j)) >0, which is already satisfied since sum(1 / k_j) <1.

So, choosing c to be at least the maximum k_i would ensure that x_i >=1 for all i.

But let's see if this works.

Take the first example:

n=3, k=[3,2,7]

sum(1/k)=1/3 + 1/2 + 1/7 ≈0.975<1

Choose c >= max(k_i)=7, say c=7.

Then x_i = c / k_i = 7/3=2.333, but x_i need to be integers, so maybe take ceiling?

But better to choose c such that c is divisible by all k_i, i.e., c is a multiple of the LCM of the k_i's.

Wait, but x_i need to be integers, so c should be divisible by k_i for all i.

So, let's set c to be a multiple of LCM of k_i's.

Let me denote L = LCM(k_1, k_2, ..., k_n)

Then, set c = L.

Then, x_i = L / k_i.

This ensures that x_i are integers.

Now, s = sum(L / k_j for all j)

We need to check if L > s, i.e., L > sum(L / k_j), which simplifies to 1 > sum(1 / k_j), which is our condition for solution existence.

So, this seems to work.

In the first example:

L = LCM(3,2,7)=42

x_i = 42/3=14, 42/2=21, 42/7=6

s=14+21+6=41

Check:

3*14=42>41

2*21=42>41

7*6=42>41

Good.

But in the sample solution, x=[27,41,12], which sums to 80, and 3*27=81>80, 2*41=82>80, 7*12=84>80.

This is also valid, but my approach gives x=[14,21,6], s=41, which is also valid.

So, multiple solutions exist.

In the second example:

n=2, k=[3,3]

L=3

x_i=1,1

s=2

3*1=3>2

Good.

In the third example:

n=5, k=[5,5,5,5,5]

sum(1/5)=1, which is not less than 1, so no solution exists.

Hence, output is -1.

In the fourth example:

n=6, k=[7,9,3,17,9,13]

L=LCM(7,9,3,17,9,13)=LCM(7,9,3,17,13)

Wait, LCM of these numbers.

7 is prime, 9=3^2, 3 is already covered, 17 is prime, 13 is prime.

So, L=LCM(7,9,17,13)=7*9*17*13=7*9=63, 63*17=1071, 1071*13=13923

Wait, but in the sample solution, x=[1989,1547,4641,819,1547,1071], s=11614

But according to my approach, x_i = L / k_i

So, x1=13923/7=1989

x2=13923/9=1547

x3=13923/3=4641

x4=13923/17=819

x5=13923/9=1547

x6=13923/13=1071

Which matches the sample solution.

So, my approach works.

Hence, the general solution is:

- Compute sum(1/k_j) for all j.

- If sum(1/k_j) >=1, output -1.

- Else, compute L = LCM of all k_j.

- Set x_i = L / k_i for all i.

- Output the x_i's.

This should always work, as per the earlier reasoning.

Now, let's look at the provided program and see if it implements this correctly.

Looking at the code:

def func():

t = int(input())

for T in range(t):

def lcm(l):

g = 1

for i in range(len(l)):

g = g * l[i] // gcd(g, l[i])

return g

bets = int(input())

a = [int(x) for x in input().split()]

prod = lcm(a)

sumo = 0

for i in range(bets):

a[i] = prod // a[i]

sumo += int(a[i])

if sumo >= prod:

print(-1)

else:

ans = ''

for i in range(bets):

ans += str(a[i]) + ' '

print(ans)

So, it reads t, the number of test cases.

For each test case:

- Reads n, the number of outcomes.

- Reads the list of k_i's.

- Computes the LCM of the k_i's, denoted as prod.

- Computes x_i = prod // k_i for each i.

- Computes sumo = sum of all x_i's.

- If sumo >= prod, prints -1.

- Else, prints the x_i's.

Wait, but according to my earlier reasoning, sumo should always be less than prod if sum(1/k_j) <1.

But in the code, it checks if sumo >= prod, then prints -1.

But according to my earlier examples, in the third test case, sum(1/k_j)=1, which should output -1, and indeed, sumo would be equal to prod in that case.

Because if sum(1/k_j)=1, then sum(x_i)=prod, since sum(x_i)=sum(prod/k_j)=prod*sum(1/k_j)=prod*1=prod.

Hence, sumo >= prod implies sumo >= prod, which corresponds to sum(1/k_j) >=1, in which case no solution exists.

Hence, the condition is correct.

Therefore, the program seems to implement the correct approach.

It computes the LCM, sets x_i = LCM / k_i, computes the sum of x_i's, and checks if sum(x_i) < LCM.

If yes, outputs the x_i's; else, outputs -1.

This aligns with my earlier reasoning.

Hence, the program is correct.

**Final Answer**

\[ \boxed{\text{True}} \]