Let's break down the initial state and the conditions step by step:

1. **Initial State:**
   - `l` is `n - 2`
   - `r` is 0
   - `st` is `n - 3`
   - `end` is increased by 3 (let's denote this new value as `end_new`)
   - If the first element of `a` is equal to the last element of `a`, then `ans` is `-1`.
   - Otherwise, if `st == 0` and `end == 0` and `a[0] != a[-1]`, then `ans` remains unchanged.
   - Otherwise, `ans` is `- (n - 2)`.

2. **Conditions for `ans`:**
   - If `a[0] == a[-1]`, then `ans = -1`.
   - If `st == 0` and `end == 0` and `a[0] != a[-1]`, then `ans` remains unchanged.
   - Otherwise, `ans = -(n - 2)`.

3. **Values of Variables:**
   - `l = n - 2`
   - `r = 0`
   - `st = n - 3`
   - `end_new = end + 3`

4. **Determining `ans`:**
   - Since `st = n - 3` and `end_new = end + 3`, it is clear that `st` cannot be `0` unless `n - 3 = 0`, which implies `n = 3`. 
   - For `end_new` to be `0`, `end` must be `-3`, but since `end` is a count of elements and cannot be negative, this scenario is not possible.
   - Therefore, the only condition that matters here is `a[0] == a[-1]`.

5. **Final Value of `ans`:**
   - If `a[0] == a[-1]`, then `ans = -1`.
   - Otherwise, `ans = -(n - 2)`.

Given that the problem does not specify the actual values of `a[0]` and `a[-1]`, we need to consider both scenarios:
- If `a[0] == a[-1]`, then `ans = -1`.
- Otherwise, `ans = -(n - 2)`.

Since the problem does not give us the specific values of `a[0]` and `a[-1]`, we assume the general case where `a[0] != a[-1]` (as the other case would make `ans = -1` and the max(0, -1) would still be 0).

Therefore, `ans = -(n - 2)`.

6. **Final Print Statement:**
   - The print statement is `print(max(0, ans))`.
   - Given `ans = -(n - 2)`, `max(0, -(n - 2))` will be `0` because `-(n - 2)` is always negative for any positive `n`.

Output: **0**