Alright, I've got this problem to solve. Let's see what it's asking for. So, there are n signs of the apocalypse, and each sign appears every a_i years. The signs have to occur sequentially, meaning that after the first sign appears, we start waiting for the second sign in the next year, and so on, until the nth sign appears.

First, I need to understand how the signs occur. Each sign i occurs in years that are multiples of a_i, like a_i, 2*a_i, 3*a_i, and so on. But the tribe waits for each sign to occur strictly after the previous one. So, if the first sign occurs in year x, they start waiting for the second sign in year x+1, and so forth.

My goal is to find out in which year the nth sign will occur, given that all signs must have occurred in this sequential manner.

Let me look at the example provided to get a better understanding.

In the first test case:

n = 6

a = [3, 2, 4, 5, 9, 18]

And the output is 36.

Let's see how this works:

- The first sign occurs every 3 years: 3, 6, 9, 12, 15, 18, 21, 24, 27, 30, 33, 36,...

- The second sign occurs every 2 years: 2, 4, 6, 8, 10, 12, 14, 16, 18, 20, 22, 24, 26, 28, 30, 32, 34, 36,...

- And so on for the other signs.

But according to the problem, after the first sign occurs, say in year 3, then we start waiting for the second sign in year 4 and onwards.

So, in year 3, the first sign occurs.

Then, starting from year 4, we wait for the second sign. The second sign occurs in years 2, 4, 6, 8, etc. So, the earliest occurrence after year 3 is year 4.

So, the second sign occurs in year 4.

Now, starting from year 5, we wait for the third sign, which occurs every 4 years: 4, 8, 12, 16, 20, 24, 28, 32, 36,...

The earliest occurrence after year 4 is year 8.

So, the third sign occurs in year 8.

Next, starting from year 9, we wait for the fourth sign, which occurs every 5 years: 5, 10, 15, 20, 25, 30, 35, 40,...

The earliest occurrence after year 8 is year 10.

So, the fourth sign occurs in year 10.

Then, starting from year 11, we wait for the fifth sign, which occurs every 9 years: 9, 18, 27, 36,...

The earliest occurrence after year 10 is year 18.

So, the fifth sign occurs in year 18.

Finally, starting from year 19, we wait for the sixth sign, which occurs every 18 years: 18, 36, 54,...

The earliest occurrence after year 18 is year 36.

So, the sixth sign occurs in year 36, which matches the example output.

Okay, so the approach seems to be that for each sign, we find the smallest year where that sign occurs after the previous sign's year.

In other words, for each sign i from 1 to n:

- Find the smallest year y such that y is greater than the year the previous sign occurred (y > year_{i-1}) and y is a multiple of a_i.

- Set year_i = y.

And the final answer is year_n.

Now, how can I implement this efficiently, especially since n can be up to 100 and a_i can be up to 10^6, and t can be up to 1000, so I need an efficient solution.

Let me think about how to compute the year for each sign efficiently.

One way is to keep track of the current year, and for each sign, find the smallest year that is greater than the current year and is a multiple of a_i.

This can be done by finding the smallest multiple of a_i that is greater than the current year.

Mathematically, this is ceil(current_year / a_i + 1) * a_i.

Alternatively, it can be calculated as current_year + a_i - (current_year % a_i) if current_year % a_i != 0, else current_year + a_i.

Wait, actually, in code, it's easier to write it as:

if current_year % a_i == 0:

next_year = current_year + a_i

else:

next_year = current_year - (current_year % a_i) + a_i

But in Python, we can use the modulo operation to simplify this.

Wait, actually, in Python, we can use:

next_year = current_year + (a_i - current_year % a_i) % a_i

This works because if current_year % a_i == 0, then (a_i - 0) % a_i = 0, so next_year = current_year + 0 = current_year, but we need to add a_i in this case to get the next multiple.

Wait, no, if current_year % a_i == 0, then (a_i - 0) % a_i = 0, so next_year = current_year + 0 = current_year, but we need to get the next multiple, which is current_year + a_i.

So, to fix this, I can write:

next_year = current_year + ((a_i - current_year % a_i) % a_i)

But if current_year % a_i == 0, then next_year = current_year + (a_i - 0) % a_i = current_year + 0, which is current_year, but I need current_year + a_i.

So, perhaps a better way is:

if current_year % a_i == 0:

next_year = current_year + a_i

else:

next_year = current_year + a_i - (current_year % a_i)

But this seems a bit cumbersome. Is there a better way?

Wait, I recall that in programming, a common way to find the smallest multiple of a_i greater than or equal to current_year is:

next_year = ((current_year + a_i - 1) // a_i) * a_i

This works because ((current_year + a_i - 1) // a_i) is the ceiling of current_year / a_i, and multiplying it back by a_i gives the smallest multiple of a_i that is >= current_year.

And in code, this is efficient.

So, for each sign, we can compute the next_year as:

next_year = ((current_year + a_i - 1) // a_i) * a_i

And set current_year = next_year.

Starting from current_year = 0.

Wait, but in the example, they start from year 0, and the first sign occurs in year 3, then 4, then 8, etc.

Let me verify with the first test case:

n = 6

a = [3, 2, 4, 5, 9, 18]

Start with current_year = 0.

For i=1:

next_year = ((0 + 3 - 1) // 3) * 3 = (2 // 3) * 3 = 0 * 3 = 0, but this is not correct because the first sign occurs in year 3.

Wait, there's an error here.

Wait, (0 + 3 - 1) = 2, 2 // 3 = 0, 0 * 3 = 0.

But we need it to be 3.

Hmm, perhaps I need to adjust the formula.

Wait, maybe it's better to write:

if current_year % a_i == 0:

next_year = current_year

else:

next_year = current_year + (a_i - current_year % a_i)

But in the example, we need to make sure that the next_year is strictly greater than the current_year.

Wait, in the problem, it says "strictly after the previous sign", so next_year must be greater than current_year.

So, if current_year is a multiple of a_i, then next_year should be current_year + a_i.

Else, next_year should be the smallest multiple of a_i greater than current_year.

So, in code:

if current_year % a_i == 0:

next_year = current_year + a_i

else:

next_year = current_year + (a_i - current_year % a_i)

This should work.

Let's test it with the first test case:

Start with current_year = 0.

For i=1, a_i=3:

0 % 3 == 0, so next_year = 0 + 3 = 3

Set current_year = 3

For i=2, a_i=2:

3 % 2 == 1, so next_year = 3 + (2 - 1) = 4

Set current_year = 4

For i=3, a_i=4:

4 % 4 == 0, so next_year = 4 + 4 = 8

Set current_year = 8

For i=4, a_i=5:

8 % 5 == 3, so next_year = 8 + (5 - 3) = 10

Set current_year = 10

For i=5, a_i=9:

10 % 9 == 1, so next_year = 10 + (9 - 1) = 18

Set current_year = 18

For i=6, a_i=18:

18 % 18 == 0, so next_year = 18 + 18 = 36

Set current_year = 36

Which matches the example.

Great, this seems correct.

So, in code, I can implement this logic.

But looking at the given program:

def func():

t = int(input())

for _ in range(t):

n = int(input())

a = list(map(int, input().split()))

year = 0

for ai in a:

year += year % ai or ai

print(year)

Wait, this looks different from what I thought.

Let's see what this code does.

It initializes year=0.

Then, for each ai in a:

year += year % ai or ai

So, year %= ai or ai

Wait, no, it's year += year % ai or ai

Wait, in Python, "or" returns the first truthy value.

So, year % ai or ai means:

if year % ai is truthy (i.e., not zero), then year % ai, else ai

So, year += year % ai if year % ai else ai

Which is equivalent to:

if year % ai != 0:

year += year % ai

else:

year += ai

Wait, but in my earlier logic, when year % ai == 0, I should add ai to year.

Here, it's doing the opposite: if year % ai != 0, add year % ai, else add ai.

But in my earlier logic, when year % ai != 0, I should add (ai - year % ai), not year % ai.

Wait, in my earlier correct logic:

if year % ai == 0:

next_year = year + ai

else:

next_year = year + (ai - year % ai)

But in the given code, it's:

if year % ai != 0:

year += year % ai

else:

year += ai

Which is different from what I have.

Let me check with the first test case.

Start with year=0.

For i=1, ai=3:

0 % 3 == 0, so year += 3 → year=3

For i=2, ai=2:

3 % 2 == 1 != 0, so year += 1 → year=4

For i=3, ai=4:

4 % 4 == 0, so year += 4 → year=8

For i=4, ai=5:

8 % 5 == 3 != 0, so year += 3 → year=11

Wait, but in the correct sequence, the third sign should occur in year 8, then wait for the fourth sign starting from year 9, and the fourth sign occurs in year 10, not year 11.

Wait, there's a discrepancy here.

In the correct sequence, for ai=5, current_year=8, 8 % 5 == 3, so next_year = 8 + (5 - 3) = 10

But in the given code, it adds 3, making year=11, which is incorrect.

So, the given code is incorrect.

Wait, but in the example, it's supposed to output 36, and according to the correct sequence, it should be 36.

But in the step above, for ai=5, it should be year=10, but according to the code, it's year=11.

Wait, perhaps in the next step, it corrects itself.

Let's continue:

For i=5, ai=9:

11 % 9 == 2 !=0, so year +=2 → year=13

For i=6, ai=18:

13 %18 ==13 !=0, so year +=13 → year=26

Which is not matching the expected output of 36.

Hmm, so there's something wrong here.

Wait, perhaps I misread the code.

Looking again:

year += year % ai or ai

Which means:

year += (year % ai) if (year % ai) else ai

So, it's adding year % ai when it's not zero, else ai.

But in my earlier logic, when year % ai !=0, I should add (ai - year % ai).

So, the given code is adding year % ai, which is incorrect.

It should be adding (ai - year % ai).

Let me check with the first few steps:

Start with year=0.

For ai=3:

0 %3 ==0, so year +=3 → year=3

Correct.

For ai=2:

3%2 ==1 !=0, so year +=1 → year=4

But according to correct logic, should add (2 -1)=1, so year=4

Ok, same.

For ai=4:

4%4==0, so year +=4 → year=8

Correct.

For ai=5:

8%5==3 !=0, so year +=3 → year=11

But according to correct logic, should add (5-3)=2, so year=10

But here it's adding 3, making year=11.

So, it's incorrect.

But in the example, it's giving 36, which matches the correct output.

Wait, perhaps in subsequent steps, it corrects the error.

Let's see:

For ai=9:

11%9==2 !=0, so year +=2 → year=13

According to correct logic, should add (9-2)=7, so year=18

But here it's year=13

For ai=18:

13%18==13 !=0, so year +=13 → year=26

According to correct logic, should add (18-13)=5, so year=18

Wait, but according to the example, it's supposed to be 36.

But according to this, it's adding 13 to 13, making 26, which is not matching.

Wait, perhaps I made a mistake in calculating the steps.

Let me try recalculating.

Starting with year=0.

ai=3:

0%3==0 → year +=3 → year=3

ai=2:

3%2==1 !=0 → year +=1 → year=4

ai=4:

4%4==0 → year +=4 → year=8

ai=5:

8%5==3 !=0 → year +=3 → year=11

ai=9:

11%9==2 !=0 → year +=2 → year=13

ai=18:

13%18==13 !=0 → year +=13 → year=26

So, according to this, the output would be 26, but the example shows 36.

Wait, maybe I misread the example.

Looking back at the example:

Input:

4

6

3 2 4 5 9 18

5

1 2 3 4 5

5

1 1 1 1 1

6

50 30 711 200 503 1006

Output:

36

5

5

2012

Wait, but according to the given program, for the first test case, it would output 26, not 36.

So, there's inconsistency here.

Wait, perhaps I miscalculated.

Let's try running the given program with the first test case.

n=6

a=[3,2,4,5,9,18]

year=0

For ai=3:

0%3==0 → year +=3 → year=3

For ai=2:

3%2==1 !=0 → year +=1 → year=4

For ai=4:

4%4==0 → year +=4 → year=8

For ai=5:

8%5==3 !=0 → year +=3 → year=11

For ai=9:

11%9==2 !=0 → year +=2 → year=13

For ai=18:

13%18==13 !=0 → year +=13 → year=26

So, according to this, the output should be 26, but the example shows 36.

Therefore, the given program is incorrect.

But the problem says "the given program is correct based on the provided problem description."

Wait, perhaps I'm misunderstanding something.

Wait, maybe the "or" operator in Python returns the second operand if the first is False.

So, year % ai or ai

So, if year % ai is 0, which is False, then it returns ai.

Else, it returns year % ai.

So, year += ai if year % ai ==0 else year % ai

Which matches what I wrote earlier.

But according to the correct logic, it should be:

if year % ai ==0:

year += ai

else:

year += ai - (year % ai)

Which is different from what the given code does.

So, the given code is incorrect.

But in the example, it's supposed to output 36, but according to my calculation, it outputs 26.

Wait, maybe I made a mistake in the calculation.

Let me simulate it again.

Start with year=0.

ai=3:

0%3==0 → year +=3 → year=3

ai=2:

3%2==1 !=0 → year +=1 → year=4

ai=4:

4%4==0 → year +=4 → year=8

ai=5:

8%5==3 !=0 → year +=3 → year=11

ai=9:

11%9==2 !=0 → year +=2 → year=13

ai=18:

13%18==13 !=0 → year +=13 → year=26

So, according to this, it's 26, but the example shows 36.

Therefore, the given program is incorrect.

Wait, perhaps there's a misunderstanding in the problem statement.

Wait, in the problem statement, it says:

"the tribe starts waiting for the occurrence of the (i+1)-th sign, starting from the year x+1."

So, strictly after the previous sign.

So, for each sign i, the waiting starts from the year immediately after the previous sign occurred.

And the (i+1)-th sign must occur in a year greater than x.

So, for ai, find the smallest year y > x where y is a multiple of ai.

Given that, for ai, the smallest y = ceil((x+1)/ai) * ai

Which is equal to:

if (x+1) % ai ==0:

y = x+1

else:

y = x + (ai - (x+1) % ai)

Wait, in code:

if (x+1) % ai ==0:

y = x+1

else:

y = x + (ai - (x+1) % ai)

But in the given code, it's:

if x % ai ==0:

y = x + ai

else:

y = x + (x % ai)

Which is different.

Wait, perhaps I need to adjust the logic.

Let me think differently.

For each sign i, find the smallest y > x where y is a multiple of ai.

Given x, to find y:

y = ceil((x+1)/ai) * ai

Which is the same as:

y = ((x+1 + ai -1) // ai) * ai

In code, it's:

y = ((x+1 + ai -1) // ai) * ai

But in the given code, it's:

if x % ai ==0:

y = x + ai

else:

y = x + (x % ai)

Which is not matching.

So, the given code is incorrect.

Let me implement the correct logic.

I can write a function to compute the next occurrence of ai after x.

def next_occurrence(x, ai):

if (x +1) % ai ==0:

return x+1

else:

return x + (ai - (x+1) % ai)

But perhaps there's a better way.

Wait, in the given code, it's:

year += year % ai or ai

Which is equivalent to:

if year % ai ==0:

year += ai

else:

year += year % ai

But according to the correct logic, it should be:

if (year +1) % ai ==0:

year +=1

else:

year += (ai - (year+1) % ai)

So, the given code is incorrect.

Therefore, Correctness: False

But according to the example, it's supposed to output 36, but according to the given code, it outputs 26.

Wait, perhaps I miscalculated.

Let me check again.

n=6

a=[3,2,4,5,9,18]

year=0

For ai=3:

0%3==0 → year +=3 → year=3

For ai=2:

3%2==1 !=0 → year +=1 → year=4

For ai=4:

4%4==0 → year +=4 → year=8

For ai=5:

8%5==3 !=0 → year +=3 → year=11

For ai=9:

11%9==2 !=0 → year +=2 → year=13

For ai=18:

13%18==13 !=0 → year +=13 → year=26

But according to the correct sequence, it should be:

year=0

For ai=3: year=3

For ai=2: year=4

For ai=4: year=8

For ai=5: year=10

For ai=9: year=18

For ai=18: year=36

So, the given code is indeed incorrect.

Therefore, Correctness: False

**Final Solution**

To solve this problem, we need to determine the year in which the nth sign occurs, given that each sign occurs periodically and sequentially.

## Approach

1. **Understanding the Problem**:
   - Each sign occurs at multiples of a given period.
   - Signs must occur sequentially, meaning each subsequent sign must occur in a year strictly after the previous sign.

2. **Logic**:
   - Start from year 0.
   - For each sign, calculate the smallest year greater than the current year that is a multiple of the sign's period.
   - Update the current year to this new year for the next sign.

3. **Efficient Calculation**:
   - Use modulo operations to find the next occurrence of each sign.
   - If the current year is a multiple of the sign's period, add the period to get the next occurrence.
   - Otherwise, add the difference needed to reach the next multiple.

## Solution Code

```python
def find_apocalypse_year():
    import sys
    input = sys.stdin.read
    data = input().split()
    
    t = int(data[0])
    index = 1
    for _ in range(t):
        n = int(data[index])
        a = list(map(int, data[index+1:index+1+n]))
        year = 0
        for ai in a:
            if year % ai == 0:
                year += ai
            else:
                year += (ai - year % ai)
        print(year)
        index += 1 + n

find_apocalypse_year()
```

## Explanation

- **Initialization**:
  - Read the input values.
  - For each test case, read the number of signs `n` and their periods `a`.

- **Year Calculation**:
  - Start with `year = 0`.
  - For each sign period `ai` in `a`:
    - If `year` is a multiple of `ai`, add `ai` to `year`.
    - Otherwise, add the difference to reach the next multiple of `ai`.

- **Output**:
  - Print the final year for each test case.

This approach ensures that we correctly compute the year when all signs have occurred sequentially, adhering to their periodicities.