The code `m = (r + l) // 2` calculates the midpoint between `r` and `l` and assigns it to `m`. Given the initial conditions:
- `l` is either `-1` or `(n - 1) // 2`.
- `r` is either `(n - 1) // 2` or `n`.

Let's consider the two cases for `l` and `r`:

1. **Case 1: `l = -1` and `r = n`**
   - `m = (-1 + n) // 2`

2. **Case 2: `l = (n - 1) // 2` and `r = n`**
   - `m = ((n - 1) // 2 + n) // 2`

Now let's calculate the exact values for each case:
- For Case 1: `m = (-1 + n) // 2 = (n - 1) // 2`
- For Case 2: `m = ((n - 1) // 2 + n) // 2 = ((2 * (n - 1) + 2 * n) // 4) = ((2n - 2 + 2n) // 4) = (4n - 2) // 4 = (n - 1) // 2`

In both cases, `m` is calculated as `(n - 1) // 2`.

Output State: **`l` is `-1` or `(n - 1) // 2`; `r` is `n`; `m` is `(n - 1) // 2`**