Reasoning:

The program aims to reconstruct a permutation `p` from an array `a` based on the relationship \(a_i = \text{MEX}(p_1, p_2, \ldots, p_i) - p_i\). The key steps in the program are:

1. **Initialization**: The program initializes `p` as a list of `-1` values, which will be filled with the permutation elements. It also initializes `mex` to `n`, which is the maximum possible value for the MEX in the initial state.

2. **Backward Construction**: The program constructs the permutation `p` in reverse order (from `n-1` to `0`). For each index `i`, it calculates `p[i]` as `mex - a[i]`. This step is based on the given relationship:
   \[
   a_i = \text{MEX}(p_1, p_2, \ldots, p_i) - p_i \implies p_i = \text{MEX}(p_1, p_2, \ldots, p_i) - a_i
   \]
   Since `mex` is the current MEX of the array `p` from `i` to `n-1`, this calculation is correct.

3. **Update MEX**: After calculating `p[i]`, the program updates `mex` to be the minimum of the current `mex` and `p[i]`. This ensures that `mex` is always the smallest non-negative integer that has not yet been used in the permutation.

4. **Output**: Finally, the program prints the constructed permutation `p` for each test case.

Let's verify the correctness with the provided example:

- **Test Case 1**:
  - `n = 5`
  - `a = [1, 1, -2, 1, 2]`
  - Initialize `p = [-1, -1, -1, -1, -1]` and `mex = 5`.

  - For `i = 4`:
    \[
    p[4] = 5 - 2 = 3 \quad \text{(since } a[4] = 2\text{)}
    \]
    \[
    \text{mex} = \min(5, 3) = 3
    \]
    - `p = [-1, -1, -1, -1, 3]`

  - For `i = 3`:
    \[
    p[3] = 3 - 1 = 2 \quad \text{(since } a[3] = 1\text{)}
    \]
    \[
    \text{mex} = \min(3, 2) = 2
    \]
    - `p = [-1, -1, -1, 2, 3]`

  - For `i = 2`:
    \[
    p[2] = 2 - (-2) = 4 \quad \text{(since } a[2] = -2\text{)}
    \]
    \[
    \text{mex} = \min(2, 4) = 2
    \]
    - `p = [-1, -1, 4, 2, 3]`

  - For `i = 1`:
    \[
    p[1] = 2 - 1 = 1 \quad \text{(since } a[1] = 1\text{)}
    \]
    \[
    \text{mex} = \min(2, 1) = 1
    \]
    - `p = [-1, 1, 4, 2, 3]`

  - For `i = 0`:
    \[
    p[0] = 1 - 1 = 0 \quad \text{(since } a[0] = 1\text{)}
    \]
    \[
    \text{mex} = \min(1, 0) = 0
    \]
    - `p = [0, 1, 4, 2, 3]`

  - The final `p` is `[0, 1, 4, 2, 3]`, which matches the example output.

- **Test Case 2**:
  - `n = 5`
  - `a = [1, 1, 1, 1, 1]`
  - Initialize `p = [-1, -1, -1, -1, -1]` and `mex = 5`.

  - For `i = 4`:
    \[
    p[4] = 5 - 1 = 4 \quad \text{(since } a[4] = 1\text{)}
    \]
    \[
    \text{mex} = \min(5, 4) = 4
    \]
    - `p = [-1, -1, -1, -1, 4]`

  - For `i = 3`:
    \[
    p[3] = 4 - 1 = 3 \quad \text{(since } a[3] = 1\text{)}
    \]
    \[
    \text{mex} = \min(4, 3) = 3
    \]
    - `p = [-1, -1, -1, 3, 4]`

  - For `i = 2`:
    \[
    p[2] = 3 - 1 = 2 \quad \text{(since } a[2] = 1\text{)}
    \]
    \[
    \text{mex} = \min(3, 2) = 2
    \]
    - `p = [-1, -1, 2, 3, 4]`

  - For `i = 1`:
    \[
    p[1] = 2 - 1 = 1 \quad \text{(since } a[1] = 1\text{)}
    \]
    \[
    \text{mex} = \min(2, 1) = 1
    \]
    - `p = [-1, 1, 2, 3, 4]`

  - For `i = 0`:
    \[
    p[0] = 1 - 1 = 0 \quad \text{(since } a[0] = 1\text{)}
    \]
    \[
    \text{mex} = \min(1, 0) = 0
    \]
    - `p = [0, 1, 2, 3, 4]`

  - The final `p` is `[0, 1, 2, 3, 4]`, which matches the example output.

- **Test Case 3**:
  - `n = 3`
  - `a = [-2, 1, 2]`
  - Initialize `p = [-1, -1, -1]` and `mex = 3`.

  - For `i = 2`:
    \[
    p[2] = 3 - 2 = 1 \quad \text{(since } a[2] = 2\text{)}
    \]
    \[
    \text{mex} = \min(3, 1) = 1
    \]
    - `p = [-1, -1, 1]`

  - For `i = 1`:
    \[
    p[1] = 1 - 1 = 0 \quad \text{(since } a[1] = 1\text{)}
    \]
    \[
    \text{mex} = \min(1, 0) = 0
    \]
    - `p = [-1, 0, 1]`

  - For `i = 0`:
    \[
    p[0] = 0 - (-2) = 2 \quad \text{(since } a[0] = -2\text{)}
    \]
    \[
    \text{mex} = \min(0, 2) = 0
    \]
    - `p = [2, 0, 1]`

  - The final `p` is `[2, 0, 1]`, which matches the example output.

The program correctly reconstructs the permutation `p` for each test case based on the given array `a` and the relationship \(a_i = \text{MEX}(p_1, p_2, \ldots, p_i) - p_i\).

Correctness: **True**