The initial state is:
- `n` is a positive integer such that \(1 \leq n \leq 2 \times 10^9\) and \(n \geq 6\)
- `count` is 0
- `a` is `a + 1`
- `b` is 1
- `rem` is `n - 4`

The code snippet is:
```
b = a
```

This line of code assigns the current value of `a` to `b`. Therefore, `b` now holds the value of `a`.

The updated values are:
- `n` remains a positive integer such that \(1 \leq n \leq 2 \times 10^9\) and \(n \geq 6\)
- `count` remains 0
- `a` remains `a + 1`
- `b` is now `a`
- `rem` remains `n - 4`

Thus, the output state is:
Output State: **`n` is a positive integer such that \(1 \leq n \leq 2 \times 10^9\) and \(n \geq 6\), `count` is 0, `a` is `a + 1`, `b` is `a`, `rem` is `n - 4`**