Let's carefully analyze the problem and the provided solution to ensure its correctness.

### Problem Recap

The goal is to maximize the sum of an \( n \times n \) matrix using type 1 and type 2 operations, where:
- Type 1 operation: Assign a row to a permutation of numbers from 1 to \( n \).
- Type 2 operation: Assign a column to a permutation of numbers from 1 to \( n \).

The maximum sum can be achieved by ensuring each row and column contains unique numbers from 1 to \( n \).

### Solution Analysis

The provided solution consists of the following steps:
1. **Matrix Initialization**: The matrix is initialized with rows filled with permutations from 1 to \( n \). However, this initialization is not used later in the code.
2. **Sum Calculation**: The sum of the matrix elements is calculated using the formula:
   \[
   \text{res} = \sum_{i=0}^{n-1} (i + 1) \times (2 \times i + 1)
   \]
3. **Output the Sum and Number of Operations**: The calculated sum and the number of operations (which is \( 2n \)) are printed.
4. **Operations Description**: The operations are described in reverse order (from \( n \) to 1), setting each row and column to the permutation [1, 2, ..., \( n \)].

### Verification

Let's verify if the solution is correct:

1. **Sum Calculation**:
   - The formula used to calculate the sum is:
     \[
     \text{res} = \sum_{i=0}^{n-1} (i + 1) \times (2 \times i + 1)
     \]
   - Simplifying the formula:
     \[
     \text{res} = \sum_{i=1}^{n} i \times (2i - 1) = \sum_{i=1}^{n} (2i^2 - i)
     \]
     \[
     \text{res} = 2 \sum_{i=1}^{n} i^2 - \sum_{i=1}^{n} i
     \]
     Using the formulas for the sum of squares and the sum of the first \( n \) natural numbers:
     \[
     \sum_{i=1}^{n} i^2 = \frac{n(n+1)(2n+1)}{6}
     \]
     \[
     \sum_{i=1}^{n} i = \frac{n(n+1)}{2}
     \]
     Substituting these into the formula:
     \[
     \text{res} = 2 \times \frac{n(n+1)(2n+1)}{6} - \frac{n(n+1)}{2}
     \]
     \[
     \text{res} = \frac{n(n+1)(2n+1)}{3} - \frac{n(n+1)}{2}
     \]
     \[
     \text{res} = \frac{2n(n+1)(2n+1) - 3n(n+1)}{6}
     \]
     \[
     \text{res} = \frac{n(n+1)(4n+2 - 3)}{6}
     \]
     \[
     \text{res} = \frac{n(n+1)(4n-1)}{6}
     \]
   - This formula is correct and results in the maximum sum.

2. **Number of Operations**:
   - The solution uses exactly \( 2n \) operations, which is within the allowed limit.

3. **Operations Description**:
   - The operations described ensure that each row and column is set to a permutation of numbers from 1 to \( n \), achieving the maximum sum.

### Conclusion

The provided solution correctly calculates the maximum sum and describes the operations to achieve this sum within the allowed limit of \( 2n \) operations.

### Final Evaluation

Final: **True**