Postcondition: **`n` and `m` are positive integers such that \(1 \leq n, m \leq 2 \times 10^6\), `T` is greater than 2, `t` is 2, `info` is a list of strings from user input, `a` is the integer value of `info[0]`, `b` is the integer value of `info[1]` and must be greater than or equal to `a` and at least 1, `i` is 1, `x` is \(a + 1\). If \((a - i \cdot (i - 1)) \% i^2 == 0\) and \(i \cdot (i - 1) \% i^2 == 0\), then `suma` is \(a + 2\). Otherwise, `suma` remains \(a + 1\). Additionally, if \(\frac{a - i \cdot (i - 1)}{i^2} + 1\) is greater than 0, the condition is satisfied.**