To determine what will be printed by the `print(int(ans))` statement, let's break down the initial state and the formula used to compute `ans`.

### Initial State:
- `n` and `m` are integers provided by user input.
- `t` must be greater than 1.
- `i` is 1.
- `count` is `m + 1`.
- `ans` is computed as `n + sum(int((int(n / k) - (k - 1)) / k) + 1 for k in range(2, m + 1))`.
- `m` must be greater than or equal to the number of iterations the loop executed.
- `countmins` is `m`.
- `g` is `int(n / (m + 1)) - m`.
- If `g` is less than `countmins`, the loop breaks before reaching `count = m + 1`.

### Step-by-Step Calculation:
1. **Understanding `ans`**:
   - `ans` is defined as `n + sum(int((int(n / k) - (k - 1)) / k) + 1 for k in range(2, m + 1))`.
   - This formula involves a summation over a range from 2 to `m + 1`.

2. **Breaking Down the Summation**:
   - For each `k` in the range from 2 to `m + 1`, the term inside the summation is `int((int(n / k) - (k - 1)) / k) + 1`.
   - This term calculates a value based on `n` and `k`.

3. **Summing the Terms**:
   - The summation `sum(int((int(n / k) - (k - 1)) / k) + 1 for k in range(2, m + 1))` adds up these terms for all `k` from 2 to `m + 1`.

4. **Adding `n`**:
   - The final value of `ans` is `n` plus the result of the summation.

5. **Converting to Integer**:
   - The `print(int(ans))` statement converts `ans` to an integer before printing it.

### Example Calculation:
Let's assume `n = 10` and `m = 3` for a concrete example:

- `ans = 10 + sum(int((int(10 / k) - (k - 1)) / k) + 1 for k in range(2, 4))`
- For `k = 2`:
  - `int(10 / 2) = 5`
  - `5 - 1 = 4`
  - `int(4 / 2) = 2`
  - `2 + 1 = 3`
- For `k = 3`:
  - `int(10 / 3) = 3`
  - `3 - 2 = 1`
  - `int(1 / 3) = 0`
  - `0 + 1 = 1`
- Summation: `3 + 1 = 4`
- `ans = 10 + 4 = 14`

### Final Output:
Given the initial state and the formula, the `print(int(ans))` statement will print the integer value of `ans`.

Output: **14 (where ans is the value of n plus the sum of the terms calculated for each k in the range from 2 to m + 1)**