The code `b = a ^ x` updates the value of `b` to be the result of `a` raised to the power of `x`. Given the initial state where `a` is the result of `b ^ x`, we can substitute this into the equation to get:

1. Initially, `a = b ^ x`.
2. After executing `b = a ^ x`, we substitute `a` with `b ^ x`, resulting in `b = (b ^ x) ^ x`.

Using the properties of exponents, we know that `(b ^ x) ^ x` simplifies to `b ^ (x * x)` or `b ^ (x ** 2)`. Thus, `b` is now updated to `b ^ (x ** 2)`.

The values of `s` and `x` remain unchanged. Therefore, the output state is:

Output State: **`s` is a non-negative integer such that 2 ≤ s ≤ 10^12, `x` is a non-negative integer such that 0 ≤ x ≤ 10^12, `b` is `b ^ (x ** 2)`**