`pl` is updated to `pl + (2 * (dl / vd) + f) * vp`. Given the initial conditions, let's break down the calculation:

- `pl` is updated by adding `(2 * (dl / vd) + f) * vp` to its current value.
- Since `dl` was set to equal `pl` previously (`dl = pl`), `dl / vd` simplifies to `pl / vd`.
- So, the expression becomes `pl + (2 * (pl / vd) + f) * vp`.

Since the initial state is that `vp` is an integer obtained from `int(raw_input())` and satisfies `0 <= vp <= c`, `pl + c <= c`, and `dl` is increased by `vd` and equals `pl`, we can directly use these conditions.

The updated `pl` is:

\[ \text{new\_pl} = \text{pl} + (2 \times (\text{pl} / \text{vd}) + f) \times \text{vp} \]

Given `pl + c <= c`, it implies `pl <= c - 1` (since `c` is an upper bound and `pl` is less than `c`).

Therefore, the Output State is: 
`vp` is an integer obtained from `int(raw_input())` and satisfies `0 <= vp <= c`; `pl` is updated to `pl + (2 * (pl / vd) + f) * vp`; `pl + c <= c`; `dl` is increased by `vd` and equals `pl`; `count` is incremented by 1.

Output State: **`vp` is an integer obtained from `int(raw_input())` and satisfies `0 <= vp <= c`; `pl` is updated to `pl + (2 * (pl / vd) + f) * vp`; `pl + c <= c`; `dl` is increased by `vd` and equals `pl`; `count` is incremented by 1**