Let's evaluate the given code snippet:

```
y = 2 ** (i - 1) * (2 * f - 1)
```

Given the initial state:
- `t` is an integer such that 1 ≤ t ≤ 5 · 10^4
- `n` is 8
- `k` is 7
- `s` is 8
- `i` is 4
- `d` is 0
- `p` is 5
- `g` is 8
- `h` is 0
- `y` is 2
- `f` is -1

Substitute the known values into the equation:
- `i` is 4
- `f` is -1

So,
```
y = 2 ** (4 - 1) * (2 * (-1) - 1)
y = 2 ** 3 * (-2 - 1)
y = 8 * (-3)
y = -24
```

The only variable that changes is `y`. All other variables retain their original values.

Output State: **`t` is an integer such that 1 ≤ t ≤ 5 · 10^4; `n` is 8; `k` is 7; `s` is 8; `i` is 4; `d` is 0; `p` is 5; `g` is 8; `h` is 0; `y` is -24; `f` is -1.**