Let's break down the problem step by step:

1. **Identify the loop condition**: The loop condition is `i <= m and i * i <= n + i`.

2. **Current state before the loop**:
   - `i` is 1.
   - `n` is a positive integer.
   - `m` is a positive integer.
   - `ans` is 0 (this variable is not part of the loop condition).

3. **Analyze the loop condition**:
   - For the loop to execute the first time, both parts of the condition must be true:
     - `i <= m`: Since `i` is currently 1 and `m` is a positive integer, this part of the condition will always be true as long as `m` is at least 1.
     - `i * i <= n + i`: Substituting `i = 1`, this becomes `1 * 1 <= n + 1` or `1 <= n + 1`. This simplifies to `1 <= n + 1`, which is always true for any positive integer `n`.

4. **Conclusion**:
   - Both parts of the loop condition are already satisfied given the current state (`i = 1`, `n` is a positive integer, `m` is a positive integer). Therefore, no adjustments are needed.

**Final Answer**:
State: **`i` is 1, `n` is a positive integer, `m` is a positive integer**