The code snippet updates the value of `t1` using the formula `t * 15 - b * 4`. We need to determine the new value of `t1` based on the given conditions.

- `a` is an integer (converted from its original string value).
- `b` is an integer (converted from its original string value).
- `x` and `y` are integers where 0 ≤ x, y ≤ 99.
- `n` is greater than 2.
- `i` is 2.
- `t1` is initially equal to `b * 15 - b * 4`.
- `t` is initially equal to `b`.
- If `t` is even, `t` is updated to `b // 2`.
- If `t` is odd, `t` is updated to `b // 2 + 1`.

Given these conditions, let's calculate the new value of `t1`:

1. **Initial Value of `t1`:**
   - `t1 = b * 15 - b * 4`
   - Simplifying, `t1 = b * (15 - 4) = b * 11`

2. **Update `t` based on its parity:**
   - If `t` (which is `b`) is even, `t` becomes `b // 2`.
   - If `t` (which is `b`) is odd, `t` becomes `b // 2 + 1`.

3. **New Value of `t1`:**
   - `t1 = t * 15 - b * 4`
   - If `b` is even, `t = b // 2`, so `t1 = (b // 2) * 15 - b * 4`.
   - If `b` is odd, `t = b // 2 + 1`, so `t1 = (b // 2 + 1) * 15 - b * 4`.

Let's summarize the output state:

- If `b` is even:
  - `t1 = (b // 2) * 15 - b * 4`
  - Simplifying, `t1 = (b * 15) / 2 - b * 4 = (15b / 2) - 4b = (15b - 8b) / 2 = 7b / 2`

- If `b` is odd:
  - `t1 = (b // 2 + 1) * 15 - b * 4`
  - Simplifying, `t1 = ((b // 2) * 15 + 15) - b * 4 = (15b / 2 + 15) - 4b = (15b - 8b) / 2 + 15 = 7b / 2 + 15`

Therefore, the output state is:

Output State: **`a` is an integer, `b` is an integer, `x` and `y` are integers where 0 ≤ x, y ≤ 99, `n` is greater than 2, `i` is 2, `t1` is `(7b / 2)` if `b` is even, or `(7b / 2 + 15)` if `b` is odd.**