Alright, I've got this problem to solve. Let's see what it's asking for. So, I have an array of integers, and I need to perform exactly K operations on it. In each operation, I can select any contiguous subarray (which could even be empty) and insert the sum of that subarray anywhere in the array. My goal is to maximize the sum of the array after K operations, and since the sum can be very large, I need to output it modulo 10^9 + 7.

First, I need to understand what exactly an operation does. When I select a subarray and insert its sum into the array, where can I insert it? Can I insert it at any position, including the beginning or the end? Yes, the problem says "insert the sum anywhere in the array." So, I can choose to add this sum at any index in the array, effectively splitting the array at that point and inserting the new element.

My aim is to maximize the sum of the array after K operations. Since I can choose which subarray to sum and where to insert it, I need to find a strategy that allows me to increase the total sum as much as possible.

Let me consider the initial sum of the array, which is just the sum of all its elements. Each operation allows me to insert a sum of a subarray into the array, which effectively adds that sum to the total sum, because I'm inserting a new element equal to the sum of some subarray.

Wait a minute, but when I insert the sum of a subarray, I'm adding a new element to the array, but I'm not removing anything. So, the total sum increases by the value of the sum I'm inserting.

Therefore, each operation can increase the sum of the array by the sum of the subarray I choose.

My goal is to maximize the sum after K operations, so I should choose the subarray with the maximum possible sum each time and insert it into the array.

But, there's a catch. Because in each operation, I can choose any contiguous subarray, including empty subarrays, which have a sum of zero. So, if I choose an empty subarray, I'm inserting zero into the array, which doesn't change the sum.

But, if I choose a subarray with a positive sum, I can increase the total sum.

Wait, but the array can contain negative numbers as well, since the constraints say that array elements can be from -10^9 to 10^9.

So, I need to be careful about choosing subarrays with positive sums.

Let me think about this step by step.

First, I need to find the subarray with the maximum sum in the current array.

Then, in each operation, I can insert this maximum subarray sum into the array, thereby increasing the total sum by that amount.

But, after inserting this sum, the array changes, and potentially, the new maximum subarray sum could be different.

Wait, but in reality, since I'm inserting a new element equal to the sum of some subarray, the new array will have one more element than before.

But, perhaps there's a smarter way to approach this.

Let me consider the initial sum of the array, S.

After the first operation, I can insert the sum of some subarray, say M, into the array, so the new sum is S + M.

Then, in the second operation, I can insert another sum of some subarray into the new array, which now has n+1 elements.

But, what's the best choice for M each time?

Wait, maybe I can find the maximum possible sum that can be achieved after K operations.

Let me consider that in each operation, I can add the sum of any subarray to the array.

So, in terms of increasing the total sum, each operation allows me to add the sum of some subarray to the total sum.

Therefore, to maximize the sum after K operations, I need to choose, in each operation, the subarray with the maximum possible sum to add.

But, the problem is that after each operation, the array changes, so the maximum subarray sum might change.

This seems complicated.

Is there a better way to look at this?

Let me consider that in each operation, I can choose any contiguous subarray, compute its sum, and insert that sum into the array.

Importantly, the sum of the entire array increases by that subarray sum because I'm adding a new element equal to that sum.

So, if I can choose the subarray with the maximum sum in each operation, and insert it, then the total sum would increase by that maximum subarray sum in each operation.

But, as the array grows with each operation, finding the maximum subarray sum each time might not be straightforward.

Wait, but perhaps there's a pattern here.

Suppose I have the initial array with sum S.

In the first operation, I choose the maximum subarray sum, say M, and insert it into the array. Now, the total sum becomes S + M.

In the second operation, I can again choose the maximum subarray sum from the new array, which might be M again, and insert it, making the total sum S + M + M = S + 2M.

Continuing this way, it seems that in each operation, I can add M to the total sum.

Therefore, after K operations, the total sum would be S + K*M.

But, is this always the case?

Wait, maybe not, because as I insert M into the array, the new array has an additional element M, which could potentially affect the maximum subarray sum.

But, if M is the maximum sum of any subarray in the original array, then in the new array, the maximum subarray sum could be M or possibly larger if combining M with some existing elements.

Wait, let's think carefully.

Suppose I have an array [A, B, C], with sum S = A + B + C.

The maximum subarray sum is M, say M = A + B.

After inserting M, the array becomes [A, B, C, M].

Now, the new maximum subarray sum could be M or A + B + M, which is A + B + M = M + M = 2M, if M = A + B.

Wait, but M is A + B, and adding M to the array makes the array [A, B, C, M].

The new maximum subarray could be A + B + M = M + M = 2M.

But, is that possible?

Wait, A + B + M = A + B + (A + B) = 2*(A + B) = 2M.

Similarly, if I have M as the maximum subarray sum, then in the new array, I can have subarrays that include M and previous elements, potentially summing up to 2M.

But, is 2M always achievable?

Wait, in the first operation, I can choose any contiguous subarray, including the one that sums to M, and insert M anywhere.

Then, in the second operation, I can choose the subarray that includes the newly inserted M and some previous elements to sum up to 2M.

But, is there a better way?

Wait, perhaps in the second operation, I can choose the subarray that includes the newly inserted M and the subarray that led to M, effectively summing to 2M.

But, to confirm, let's take an example.

Suppose initial array is [1, 2, 3], sum S = 6.

The maximum subarray sum M = 6.

After inserting M, the array becomes [1, 2, 3, 6].

Now, in the second operation, the maximum subarray sum could be 6 (the last element), or 1 + 2 + 3 + 6 = 12.

Wait, but 12 is larger than 2M (which is 12), so in this case, it's possible to have a subarray sum of 12.

Wait, but M was 6, and 12 is 2M.

So, in this case, it's equal to 2M.

But, in general, it might be possible to have subarrays summing to more than 2M.

Wait, in this example, with [1,2,3,6], the maximum subarray sum is indeed 12, which is 2M.

But, if I have a different array, say [1, -1, 2], sum S = 2.

The maximum subarray sum M = 2 (the subarray [2]).

After inserting M, the array becomes [1, -1, 2, 2].

The new maximum subarray sum could be 2 (the last element), or 2 + 2 = 4.

So, in this case, it's 4, which is 2M.

Again, 2M.

So, perhaps in general, after the first insertion, the maximum subarray sum is 2M.

Then, in the third operation, if I insert 2M, the array becomes [original elements, M, 2M], and the new maximum subarray sum could be M + 2M = 3M.

Wait, but in reality, it could be higher because I can choose larger subarrays.

Wait, in the second operation, I can choose the subarray that includes the first M and the new 2M, summing to M + 2M = 3M.

Wait, but in the example above, with [1,2,3,6], inserting 6 again would make it [1,2,3,6,6], and the maximum subarray sum could be 6 + 6 = 12, which is 2M, or 1 + 2 + 3 + 6 + 6 = 18, which is 3M.

Wait, but 18 is 3M, which is higher than 2M.

So, perhaps in each operation, I can add M to the previous maximum subarray sum.

Wait, perhaps the maximum subarray sum after K operations is (K+1)*M.

Wait, in the first operation, I insert M, sum becomes S + M.

In the second operation, I can insert M again, sum becomes S + 2M.

Wait, but in the example above, after inserting M twice, the sum is S + M + 2M = S + 3M.

Wait, perhaps I'm getting confused.

Let me try to formalize this.

Let S be the initial sum of the array.

Let M be the maximum subarray sum.

After the first operation, I insert M, sum becomes S + M.

After the second operation, I can insert M again, sum becomes S + 2M.

After K operations, sum is S + K*M.

But, in the example above, with [1,2,3], M=6, after two operations, sum is S + M + 2M = S + 3M = 6 + 3*6 = 24, but the array after two operations is [1,2,3,6,12], sum is 1 + 2 + 3 + 6 + 12 = 24, which matches.

Another example: [1, -1, 2], M=2, after two operations, sum is S + M + 2M = 2 + 2*2 = 6, and the array could be [1, -1, 2, 2, 4], sum=1 -1 +2 +2 +4=8, which is S + 3M = 2 + 6 = 8.

Wait, there's inconsistency here.

Wait, perhaps I need to think differently.

Let me consider that in each operation, I can insert any subarray sum, and I want to maximize the sum.

So, in each operation, I should insert the maximum possible value.

But, the maximum subarray sum is M, so inserting M each time would give me S + K*M.

But, in reality, as I insert M, the new array can have larger subarrays that sum to more than M.

So, perhaps S + K*M is a lower bound, but the actual sum can be higher.

In the example above, with [1,-1,2], M=2, after one operation: insert 2, array becomes [1,-1,2,2], sum=1-1+2+2=4=S+M=2+2=4.

After second operation: insert M=2 again, array becomes [1,-1,2,2,2], sum=1-1+2+2+2=6=S+2M=2+4=6.

But, in reality, the maximum subarray sum in the new array is 2+2+2=6, which is 3M.

So, if I insert 3M in the second operation, sum becomes S + M + 3M = S + 4M =2+8=10.

But, is that allowed?

Wait, no. Because in each operation, I can insert the sum of any subarray.

After the first operation, the array is [1,-1,2,2], maximum subarray sum is 2+2=4.

So, M=4.

Then, inserting 4, the array becomes [1,-1,2,2,4], sum=1-1+2+2+4=8=S+M=2+6=8.

Wait, S + M =2 +6=8, but M=4.

Wait, perhaps I'm miscalculating.

Wait, initial S=1-1+2=2, M=2.

After first operation: insert M=2, array becomes [1,-1,2,2], sum=1-1+2+2=4=S+M=2+2=4.

Then, in second operation: maximum subarray sum is 2+2=4, insert 4, array becomes [1,-1,2,2,4], sum=1-1+2+2+4=8=S+M=2+6=8.

Wait, but M=4, so S + M =2 +6=8.

Wait, perhaps I need to consider that M changes after each insertion.

Wait, in the first operation, M is the maximum subarray sum of the original array.

After inserting M, the new array has a new maximum subarray sum, which could be larger than M.

Then, in the next operation, M is updated to this new maximum subarray sum.

So, perhaps I need to iteratively compute the new M after each insertion.

But, this seems computationally expensive, especially since K can be up to 2e5.

I need a better approach.

Let me consider that in each operation, I can insert any sum of a subarray, and I want to maximize the sum.

So, the best choice is to insert the maximum possible sum each time.

But, the maximum sum of a subarray can be computed using Kadane's algorithm.

Wait, but after each insertion, the array changes, and I have to compute the new maximum subarray sum.

This seems too slow for the constraints.

I need a smarter way.

Let me consider that each insertion of M increases the sum by M, and potentially increases the maximum subarray sum.

But, perhaps there's a pattern or a formula that can be used to compute the final sum after K operations.

Let me consider that after each operation, I can insert the current maximum subarray sum, and that this insertion allows the next maximum subarray sum to be larger.

But, I need to find a general formula.

Let me consider that after the first operation, I insert M, sum becomes S + M.

After the second operation, I can insert the new maximum subarray sum, which is M + M = 2M, so sum becomes S + M + 2M = S + 3M.

After the third operation, I can insert 3M, sum becomes S + 3M + 3M = S + 6M.

After the fourth operation, insert 6M, sum becomes S + 6M + 6M = S + 12M.

I see a pattern here: the coefficient of M doubles each time after the first operation.

Wait, let's see:

Operation 0: sum = S

Operation 1: sum = S + M

Operation 2: sum = S + M + 2M = S + 3M

Operation 3: sum = S + 3M + 4M = S + 7M

Operation 4: sum = S + 7M + 8M = S + 15M

Wait, the coefficients are 1, 3, 7, 15, which are 2^k -1.

Wait, for k=1: 2^1 -1 =1

k=2: 2^2 -1=3

k=3:2^3 -1=7

k=4:2^4 -1=15

So, after K operations, the sum would be S + (2^K -1)*M.

But, in the earlier example, with [1,-1,2], S=2, M=2, after 2 operations, sum should be 2 + (4-1)*2 =2 +6=8, which matches the earlier calculation.

Another example: [1,2,3], S=6, M=6, after 2 operations, sum=6 + (4-1)*6=6 +18=24, which matches the earlier calculation.

Wait, but in the seventh test case in the example input, with all elements being -10^9, the sum should decrease, but according to this formula, M would be 0 (since the maximum subarray sum is 0, choosing an empty subarray), and the sum would be S + (2^K -1)*0 = S, which is correct only if S is non-negative.

But, in the seventh test case, S is negative, and according to the formula, sum would be S + (2^K -1)*0 = S, but in the example output, it's 42, which is S modulo 10^9 +7.

Wait, but in the note, it says that for negative sums, we need to handle them properly with modulo.

Wait, in the seventh test case, S = -6*10^9, and M=0, so sum should be S + (2^K -1)*0 = S = -6*10^9.

But, modulo 10^9 +7, -6*10^9 modulo 10^9 +7 is calculated as (-6*10^9) % (10^9 +7).

But, to compute negative modulo correctly, we can add MOD to make it positive.

So, (-6*10^9) % (10^9 +7) = (-6*10^9 + 7*(10^9 +7)) % (10^9 +7)

Wait, but in the code, it's done as ((s + t) % MOD + MOD) % MOD, which ensures non-negative result.

But, in this case, S is negative, and M=0, so sum is S, which should be computed modulo 10^9 +7.

In the seventh test case, the output is 42, which matches the explanation in the note.

So, perhaps the formula holds: sum = S + (2^K -1)*M, where M is the maximum subarray sum.

But, I need to confirm if M is correctly computed.

Wait, in the seventh test case, all elements are -10^9, so the maximum subarray sum M is 0, from choosing an empty subarray.

Yes, that makes sense.

Therefore, the general formula seems to be sum = S + (2^K -1)*M.

But, why does this formula hold?

Let's see:

After operation 1: sum = S + M

After operation 2: sum = S + M + 2M = S + 3M

After operation 3: sum = S + 3M + 4M = S + 7M

After operation 4: sum = S + 7M + 8M = S + 15M

...

After operation K: sum = S + (2^K -1)*M

This seems to fit the pattern.

Therefore, the final sum after K operations is S + (2^K -1)*M.

But, I need to make sure that M is correctly computed as the maximum subarray sum.

Also, since K can be up to 2e5, and T is up to 1e4, but the total sum of N and K over all test cases is up to 2e5, it's feasible.

Now, in the code provided, let's see what it does.

It reads T, the number of test cases.

For each test case:

- Reads N and K.

- Reads the array A.

- Computes S, the sum of A.

- Computes T, which is the maximum subarray sum using Kadane's algorithm.

- Then, computes the answer as (S + T) % MOD + (2^(K-1) -1)*T % MOD, but it seems different.

Wait, looking at the code:

ans = ((s + t) % MOD + MOD) % MOD

Then, for i in range(K-1):

t *= 2

t %= MOD

ans += t

ans %= MOD

Wait, this seems to be adding T doubled in each of the remaining K-1 operations.

Wait, but according to my earlier formula, it should be S + (2^K -1)*M.

But, in the code, it's computing ans = (S + T) % MOD + for each of the remaining K-1 operations, add T doubled each time.

Wait, no, in the code, it's:

ans = (S + T) % MOD

Then, for K-1 times:

t = (t * 2) % MOD

ans = (ans + t) % MOD

So, it's ans = S + T + 2*T + 4*T + ... + 2^(K-1)*T

Which is S + T*(1 + 2 + 4 + ... + 2^(K-1)) = S + T*(2^K -1)

Which matches my earlier formula: S + (2^K -1)*M.

Therefore, the code is correct.

But, I need to make sure that T is correctly computed as the maximum subarray sum.

In the code, T is computed using Kadane's algorithm:

t, tmp = 0, 0

for x in A:

tmp += x

if tmp < 0:

tmp = 0

t = max(tmp, t)

This is a standard implementation of Kadane's algorithm to find the maximum subarray sum.

Finally, the answer is computed as (S + (2^K -1)*T) % MOD.

But, in the code, it's computed as (S + T) % MOD + (2 + 4 + ... + 2^(K-1))*T % MOD.

Wait, but 2 + 4 + ... + 2^(K-1) = 2*(2^{K-1} -1)/(2-1) = 2^k -2.

So, ans = (S + T) % MOD + (2^k -2)*T % MOD

Which is S + T + (2^k -2)*T = S + (2^k -1)*T, which matches the earlier formula.

Therefore, the code is correct.

Hence, Correctness: **True**

**Final Answer**

\boxed{\text{True}}