Let's break down the task step by step:

1. **Initial State:**
   - `t` is an integer such that \(1 \leq t \leq 500\).
   - `n` is an input integer such that \(1 \leq n \leq 500\) and `n` must be greater than 0.
   - `mat` is a list of `n` lists, each containing integers from 1 to `n` inclusive.
   - `res` is the sum of \((i + 1) * (2 * i + 1)\) for \(i\) from 0 to \(n-1\).
   - `i` is \(n-1\).

2. **Understanding the Variables:**
   - `n` is a positive integer between 1 and 500.
   - `res` is calculated as follows:
     \[
     \text{res} = \sum_{i=0}^{n-1} (i + 1) * (2 * i + 1)
     \]
   - `i` is \(n-1\).

3. **Calculating `res`:**
   - The formula \((i + 1) * (2 * i + 1)\) can be expanded to:
     \[
     (i + 1) * (2 * i + 1) = 2i^2 + 3i + 1
     \]
   - Therefore, `res` is the sum of \(2i^2 + 3i + 1\) for \(i\) from 0 to \(n-1\):
     \[
     \text{res} = \sum_{i=0}^{n-1} (2i^2 + 3i + 1)
     \]
   - This can be further broken down into:
     \[
     \text{res} = 2 \sum_{i=0}^{n-1} i^2 + 3 \sum_{i=0}^{n-1} i + \sum_{i=0}^{n-1} 1
     \]
   - Using the formulas for the sum of squares and the sum of integers:
     \[
     \sum_{i=0}^{n-1} i^2 = \frac{(n-1)n(2n-1)}{6}
     \]
     \[
     \sum_{i=0}^{n-1} i = \frac{(n-1)n}{2}
     \]
     \[
     \sum_{i=0}^{n-1} 1 = n
     \]
   - Substituting these into the equation for `res`:
     \[
     \text{res} = 2 \left( \frac{(n-1)n(2n-1)}{6} \right) + 3 \left( \frac{(n-1)n}{2} \right) + n
     \]
     \[
     \text{res} = \frac{(n-1)n(2n-1)}{3} + \frac{3(n-1)n}{2} + n
     \]
     \[
     \text{res} = \frac{2(n-1)n(2n-1) + 9(n-1)n + 6n}{6}
     \]
     \[
     \text{res} = \frac{2(n-1)n(2n-1) + 9(n-1)n + 6n}{6}
     \]
     \[
     \text{res} = \frac{2(n-1)n(2n-1) + 9(n-1)n + 6n}{6}
     \]
     \[
     \text{res} = \frac{2(n-1)n(2n-1) + 9(n-1)n + 6n}{6}
     \]
     \[
     \text{res} = \frac{2(n-1)n(2n-1) + 9(n-1)n + 6n}{6}
     \]
     \[
     \text{res} = \frac{2(n-1)n(2n-1) + 9(n-1)n + 6n}{6}
     \]

4. **Calculating `n << 1`:**
   - The bitwise left shift operator `<<` shifts the bits of `n` to the left by 1 position, which is equivalent to multiplying `n` by 2.
   - Therefore, `n << 1` is \(2n\).

5. **Final Output:**
   - The `print` statement will output the value of `res` and the value of `n << 1`.
   - Since `res` is a sum of a formula and `n << 1` is \(2n\), the output will be:
     \[
     \text{res} = \frac{2(n-1)n(2n-1) + 9(n-1)n + 6n}{6}
     \]
     \[
     \text{n << 1} = 2n
     \]

Output: **res, 2n (where res is the sum of (i + 1) * (2 * i + 1) for i from 0 to n-1, and 2n is twice the value of n)**