The code `dp[i][j] = dp[i][j - 1]` updates the value of `dp[i][j]` to be equal to `dp[i][j - 1]`. Given the initial state, we know that `i` is 3 and `j` is 2. Therefore, `dp[3][2]` will be updated to be equal to `dp[3][1]`.

Output State: **`n` is an input integer such that 1 <= `n` <= 45, `k` is an input integer such that `k` is at least 3 and 3 <= `k` <= 45, `M` is an input integer such that 0 <= `M` <= 2 * 10^9 and `M` must be greater than 1, `t_j` are integers such that 1 <= `t_j` <= 1000000 for 1 <= `j` <= `k`, `t` is a sorted list of input integers in ascending order, `dp` is a 2D list of size (`k` + 1) x (`M` + 1) where `dp[3][2]` equals `dp[3][1]`, `i` is 3, and the current value of `j` is 2**