Let's break down the initial state and the code snippet step by step:

1. **Initial State:**
   - `n = 0`
   - `h = (n - k + 1) // (n - k + 1) + (n - k + 1) // 1`
   - `costs = [n - k + 1, 1]`
   - `h` is greater than or equal to `k`

2. **Calculate `h`:**
   - `n - k + 1` is a common term in the expression for `h`.
   - Since `n = 0`, the term `n - k + 1` simplifies to `1 - k`.
   - The expression for `h` becomes:
     \[
     h = (1 - k) // (1 - k) + (1 - k) // 1
     \]
   - The first term `(1 - k) // (1 - k)`:
     - If `k = 1`, then `1 - k = 0`, and `0 // 0` is undefined (division by zero).
     - If `k ≠ 1`, then `1 - k` is a non-zero integer, and `(1 - k) // (1 - k)` is always 1.
   - The second term `(1 - k) // 1`:
     - This is simply `1 - k`.

   Therefore, if `k ≠ 1`:
   \[
   h = 1 + (1 - k)
   \]
   Simplifying:
   \[
   h = 2 - k
   \]

3. **Check the condition `h` is greater than or equal to `k`:**
   - For `h` to be greater than or equal to `k`, we need:
     \[
     2 - k \geq k
     \]
   - Solving for `k`:
     \[
     2 \geq 2k
     \]
     \[
     1 \geq k
     \]
   - This means `k` must be 0 or 1.

4. **Evaluate `h` for valid `k` values:**
   - If `k = 0`:
     \[
     h = 2 - 0 = 2
     \]
   - If `k = 1`:
     \[
     h = 2 - 1 = 1
     \]
   - However, if `k = 1`, the first term `(1 - k) // (1 - k)` would be `0 // 0`, which is undefined. Therefore, `k` must be 0.

5. **Final values:**
   - `n = 0`
   - `k = 0`
   - `h = 2`
   - `costs = [1, 1]`

6. **Code snippet:**
   ```
   print(2)
   ```

The code snippet `print(2)` will print the integer 2.

Output: **2**