To determine what will be printed by the `print(b, 'B')` statement, let's break down the initial state and the construction of the list `b`.

### Initial State:
- `a` is a list with at least 4 elements.
- `c` and `d` are the new values returned by the function `r()`, but they are not used in the `print` statement.
- `b` is updated to a specific list based on the elements of `a`.

### Construction of `b`:
- `b` is initialized as `[0, 0, v1, v1 if v1 > x1 - w1 else 1, 2*v1 if v1 > z1 - y1 else v1 + 1, v2 if v2 > x2 - w2 else 1, v2 + (v2 if v2 > z2 - y2 else 1), ..., vn if vn > xn - wn else 1, vn + (vn if vn > zn - yn else 1)]`.

Let's break down the construction of `b`:

1. **First two elements**: `b` starts with `[0, 0]`.
2. **Subsequent elements**:
   - For each element in `a`, the differences `v1, v2, ..., vn` are calculated as `y - x` for each iteration.
   - The next elements in `b` are constructed based on the conditions:
     - `v1 if v1 > x1 - w1 else 1`
     - `2*v1 if v1 > z1 - y1 else v1 + 1`
     - `v2 if v2 > x2 - w2 else 1`
     - `v2 + (v2 if v2 > z2 - y2 else 1)`
     - And so on for each subsequent element in `a`.

### Example Calculation:
Assume `a = [1, 2, 3, 4, 5, 6]` for simplicity.

1. **First two elements**: `b = [0, 0]`.
2. **For the first element**:
   - `v1 = 2 - 1 = 1`
   - `v1 if v1 > 1 - 1 else 1` -> `1 if 1 > 0 else 1` -> `1`
   - `2*v1 if v1 > 3 - 2 else v1 + 1` -> `2*1 if 1 > 1 else 1 + 1` -> `2`
   - So, `b = [0, 0, 1, 2]`.

3. **For the second element**:
   - `v2 = 3 - 2 = 1`
   - `v2 if v2 > 2 - 1 else 1` -> `1 if 1 > 1 else 1` -> `1`
   - `v2 + (v2 if v2 > 4 - 3 else 1)` -> `1 + (1 if 1 > 1 else 1)` -> `1 + 1` -> `2`
   - So, `b = [0, 0, 1, 2, 1, 2]`.

4. **For the third element**:
   - `v3 = 4 - 3 = 1`
   - `v3 if v3 > 3 - 2 else 1` -> `1 if 1 > 1 else 1` -> `1`
   - `v3 + (v3 if v3 > 5 - 4 else 1)` -> `1 + (1 if 1 > 1 else 1)` -> `1 + 1` -> `2`
   - So, `b = [0, 0, 1, 2, 1, 2, 1, 2]`.

5. **For the fourth element**:
   - `v4 = 5 - 4 = 1`
   - `v4 if v4 > 4 - 3 else 1` -> `1 if 1 > 1 else 1` -> `1`
   - `v4 + (v4 if v4 > 6 - 5 else 1)` -> `1 + (1 if 1 > 1 else 1)` -> `1 + 1` -> `2`
   - So, `b = [0, 0, 1, 2, 1, 2, 1, 2, 1, 2]`.

### Final Output:
The `print(b, 'B')` statement will print the list `b` followed by the string 'B'. Given the construction of `b` based on the elements of `a`, the output will be:

Output: **[0, 0, 1, 2, 1, 2, 1, 2, 1, 2] B** (where the exact values depend on the specific elements of `a`).