To evaluate the code snippet, let's first analyze the statement:

```
dp[n, k] += 9 * 10 ** (i - 1) * (10 ** (k - i) - 10 ** (i - 1))
```

Given the initial state:
- `dp[n, k]` is -720
- `k` is 2
- `i` is 1

Now, we can substitute these values into the expression:

1. Calculate `10 ** (i - 1)`:
   - \(i - 1 = 1 - 1 = 0\)
   - \(10 ** 0 = 1\)

2. Calculate `10 ** (k - i)`:
   - \(k - i = 2 - 1 = 1\)
   - \(10 ** 1 = 10\)

3. Now substitute these values into the expression:
   - Calculate \(10 ** (k - i) - 10 ** (i - 1)\):
     - \(10 - 1 = 9\)

4. Now, compute the entire multiplication:
   - \(9 * 10 ** (i - 1) * (10 ** (k - i) - 10 ** (i - 1))\):
   - \(9 * 1 * 9 = 81\)

5. Finally, update `dp[n, k]`:
   - \(dp[n, k] = -720 + 81 = -639\)

The new value for `dp[n, k]` is -639. The other variables remain unchanged.

Therefore, the output state is:
Output State: **`l` is an integer such that 1 <= `l` <= `r` < 10^18, `r` is an integer such that 1 <= `l` <= `r` < 10^18, `k` is 2, `dp[n, k]` is -639, `i` is 1**