Alright, I've got this problem to solve. Let's see what it's asking for. So, Bob has a bakery, and on the opening day, he baked n buns that he wants to sell. The usual price for each bun is a coins. But to attract customers, he's running a promotion where he can choose some integer k (between 0 and the minimum of n and b) and sell the first k buns at a modified price. The price for the i-th bun (where i goes from 1 to k) is (b - i + 1) coins. The remaining (n - k) buns are sold at the usual price a coins each.

My task is to help Bob determine the maximum profit he can obtain by selling all n buns.

First, I need to understand the promotion clearly. If Bob chooses k = 0, he sells all n buns at price a coins each, so the total profit is n * a. If he chooses k > 0, he sells the first k buns at decreasing prices starting from b coins down to (b - k + 1) coins, and the remaining (n - k) buns at price a coins each.

So, the total profit for a given k would be the sum of the modified prices for the first k buns plus the usual price for the remaining buns.

I need to maximize this total profit over all possible values of k from 0 to min(n, b).

Let me think about how to approach this.

Option 1: Brute force

I could iterate over all possible values of k from 0 to min(n, b), calculate the total profit for each k, and keep track of the maximum profit.

But considering that n, a, and b can be up to 10^9 and there are up to 10^4 test cases, this approach would be too slow because it would require up to 10^4 * 10^9 operations, which is not feasible.

Option 2: Find a mathematical formula to directly calculate the maximum profit.

This seems more promising. I need to find a way to express the total profit as a function of k and then determine the value of k that maximizes this profit.

Let's denote the total profit as P(k).

P(k) = sum from i=1 to k of (b - i + 1) + a * (n - k)

First, let's simplify the sum of the modified prices.

The sum of the first k modified prices is:

sum from i=1 to k of (b - i + 1) = sum from i=1 to k of b - sum from i=1 to k of i + sum from i=1 to k of 1

= k * b - (k * (k + 1)) / 2 + k

= k * b - (k^2 + k)/2 + k

= k * b - (k^2)/2 - k/2 + k

= k * b - (k^2)/2 + k/2

= (2 * k * b - k^2 + k)/2

= (2 * k * b - k^2 + k)/2

= (2 * k * b - k^2 + k)/2

= (2 * k * b - k^2 + k)/2

= (2 * k * b - k^2 + k)/2

= (2 * k * b - k^2 + k)/2

= (2 * k * b - k^2 + k)/2

= (2 * k * b - k^2 + k)/2

= (2 * k * b - k^2 + k)/2

= (2 * k * b - k^2 + k)/2

= (2 * k * b - k^2 + k)/2

= (2 * k * b - k^2 + k)/2

= (2 * k * b - k^2 + k)/2

= (2 * k * b - k^2 + k)/2

= (2 * k * b - k^2 + k)/2

= (2 * k * b - k^2 + k)/2

= (2 * k * b - k^2 + k)/2

= (2 * k * b - k^2 + k)/2

= (2 * k * b - k^2 + k)/2

= (2 * k * b - k^2 + k)/2

= (2 * k * b - k^2 + k)/2

= (2 * k * b - k^2 + k)/2

= (2 * k * b - k^2 + k)/2

= (2 * k * b - k^2 + k)/2

= (2 * k * b - k^2 + k)/2

= (2 * k * b - k^2 + k)/2

= (2 * k * b - k^2 + k)/2

= (2 * k * b - k^2 + k)/2

= (2 * k * b - k^2 + k)/2

= (2 * k * b - k^2 + k)/2

= (2 * k * b - k^2 + k)/2

= (2 * k * b - k^2 + k)/2

= (2 * k * b - k^2 + k)/2

= (2 * k * b - k^2 + k)/2

= (2 * k * b - k^2 + k)/2

= (2 * k * b - k^2 + k)/2

= (2 * k * b - k^2 + k)/2

= (2 * k * b - k^2 + k)/2

= (2 * k * b - k^2 + k)/2

= (2 * k * b - k^2 + k)/2

= (2 * k * b - k^2 + k)/2

= (2 * k * b - k^2 + k)/2

= (2 * k * b - k^2 + k)/2

= (2 * k * b - k^2 + k)/2

= (2 * k * b - k^2 + k)/2

= (2 * k * b - k^2 + k)/2

= (2 * k * b - k^2 + k)/2

= (2 * k * b - k^2 + k)/2

= (2 * k * b - k^2 + k)/2

= (2 * k * b - k^2 + k)/2

= (2 * k * b - k^2 + k)/2

= (2 * k * b - k^2 + k)/2

= (2 * k * b - k^2 + k)/2

= (2 * k * b - k^2 + k)/2

= (2 * k * b - k^2 + k)/2

= (2 * k * b - k^2 + k)/2

= (2 * k * b - k^2 + k)/2

= (2 * k * b - k^2 + k)/2

= (2 * k * b - k^2 + k)/2

= (2 * k * b - k^2 + k)/2

= (2 * k * b - k^2 + k)/2

= (2 * k * b - k^2 + k)/2

= (2 * k * b - k^2 + k)/2

= (2 * k * b - k^2 + k)/2

= (2 * k * b - k^2 + k)/2

= (2 * k * b - k^2 + k)/2

= (2 * k * b - k^2 + k)/2

= (2 * k * b - k^2 + k)/2

= (2 * k * b - k^2 + k)/2

= (2 * k * b - k^2 + k)/2

= (2 * k * b - k^2 + k)/2

= (2 * k * b - k^2 + k)/2

= (2 * k * b - k^2 + k)/2

= (2 * k * b - k^2 + k)/2

= (2 * k * b - k^2 + k)/2

= (2 * k * b - k^2 + k)/2

= (2 * k * b - k^2 + k)/2

= (2 * k * b - k^2 + k)/2

= (2 * k * b - k^2 + k)/2

= (2 * k * b - k^2 + k)/2

= (2 * k * b - k^2 + k)/2

= (2 * k * b - k^2 + k)/2

= (2 * k * b - k^2 + k)/2

= (2 * k * b - k^2 + k)/2

= (2 * k * b - k^2 + k)/2

= (2 * k * b - k^2 + k)/2

= (2 * k * b - k^2 + k)/2

= (2 * k * b - k^2 + k)/2

= (2 * k * b - k^2 + k)/2

= (2 * k * b - k^2 + k)/2

= (2 * k * b - k^2 + k)/2

= (2 * k * b - k^2 + k)/2

= (2 * k * b - k^2 + k)/2

= (2 * k * b - k^2 + k)/2

= (2 * k * b - k^2 + k)/2

= (2 * k * b - k^2 + k)/2

= (2 * k * b - k^2 + k)/2

= (2 * k * b - k^2 + k)/2

= (2 * k * b - k^2 + k)/2

= (2 * k * b - k^2 + k)/2

= (2 * k * b - k^2 + k)/2

= (2 * k * b - k^2 + k)/2

= (2 * k * b - k^2 + k)/2

= (2 * k * b - k^2 + k)/2

= (2 * k * b - k^2 + k)/2

= (2 * k * b - k^2 + k)/2

= (2 * k * b - k^2 + k)/2

= (2 * k * b - k^2 + k)/2

= (2 * k * b - k^2 + k)/2

= (2 * k * b - k^2 + k)/2

= (2 * k * b - k^2 + k)/2

= (2 * k * b - k^2 + k)/2

= (2 * k * b - k^2 + k)/2

= (2 * k * b - k^2 + k)/2

= (2 * k * b - k^2 + k)/2

= (2 * k * b - k^2 + k)/2

= (2 * k * b - k^2 + k)/2

= (2 * k * b - k^2 + k)/2

= (2 * k * b - k^2 + k)/2

= (2 * k * b - k^2 + k)/2

= (2 * k * b - k^2 + k)/2

= (2 * k * b - k^2 + k)/2

= (2 * k * b - k^2 + k)/2

= (2 * k * b - k^2 + k)/2

= (2 * k * b - k^2 + k)/2

= (2 * k * b - k^2 + k)/2

= (2 * k * b - k^2 + k)/2

= (2 * k * b - k^2 + k)/2

= (2 * k * b - k^2 + k)/2

= (2 * k * b - k^2 + k)/2

= (2 * k * b - k^2 + k)/2

= (2 * k * b - k^2 + k)/2

= (2 * k * b - k^2 + k)/2

= (2 * k * b - k^2 + k)/2

= (2 * k * b - k^2 + k)/2

= (2 * k * b - k^2 + k)/2

= (2 * k * b - k^2 + k)/2

= (2 * k * b - k^2 + k)/2

= (2 * k * b - k^2 + k)/2

= (2 * k * b - k^2 + k)/2

= (2 * k * b - k^2 + k)/2

= (2 * k * b - k^2 + k)/2

= (2 * k * b - k^2 + k)/2

= (2 * k * b - k^2 + k)/2

= (2 * k * b - k^2 + k)/2

= (2 * k * b - k^2 + k)/2

= (2 * k * b - k^2 + k)/2

= (2 * k * b - k^2 + k)/2

= (2 * k * b - k^2 + k)/2

= (2 * k * b - k^2 + k)/2

= (2 * k * b - k^2 + k)/2

= (2 * k * b - k^2 + k)/2

= (2 * k * b - k^2 + k)/2

= (2 * k * b - k^2 + k)/2

= (2 * k * b - k^2 + k)/2

= (2 * k * b - k^2 + k)/2

= (2 * k * b - k^2 + k)/2

= (2 * k * b - k^2 + k)/2

= (2 * k * b - k^2 + k)/2

= (2 * k * b - k^2 + k)/2

= (2 * k * b - k^2 + k)/2

= (2 * k * b - k^2 + k)/2

= (2 * k * b - k^2 + k)/2

= (2 * k * b - k^2 + k)/2

= (2 * k * b - k^2 + k)/2

= (2 * k * b - k^2 + k)/2

= (2 * k * b - k^2 + k)/2

= (2 * k * b - k^2 + k)/2

= (2 * k * b - k^2 + k)/2

= (2 * k * b - k^2 + k)/2

= (2 * k * b - k^2 + k)/2

= (2 * k * b - k^2 + k)/2

= (2 * k * b - k^2 + k)/2

= (2 * k * b - k^2 + k)/2

= (2 * k * b - k^2 + k)/2

= (2 * k * b - k^2 + k)/2

= (2 * k * b - k^2 + k)/2

= (2 * k * b - k^2 + k)/2

= (2 * k * b - k^2 + k)/2

= (2 * k * b - k^2 + k)/2

= (2 * k * b - k^2 + k)/2

= (2 * k * b - k^2 + k)/2

= (2 * k * b - k^2 + k)/2

= (2 * k * b - k^2 + k)/2

= (2 * k * b - k^2 + k)/2

= (2 * k * b - k^2 + k)/2

= (2 * k * b - k^2 + k)/2

= (2 * k * b - k^2 + k)/2

= (2 * k * b - k^2 + k)/2

= (2 * k * b - k^2 + k)/2

= (2 * k * b - k^2 + k)/2

= (2 * k * b - k^2 + k)/2

= (2 * k * b - k^2 + k)/2

= (2 * k * b - k^2 + k)/2

= (2 * k * b - k^2 + k)/2

= (2 * k * b - k^2 + k)/2

= (2 * k * b - k^2 + k)/2

= (2 * k * b - k^2 + k)/2

= (2 * k * b - k^2 + k)/2

= (2 * k * b - k^2 + k)/2

= (2 * k * b - k^2 + k)/2

= (2 * k * b - k^2 + k)/2

= (2 * k * b - k^2 + k)/2

= (2 * k * b - k^2 + k)/2

= (2 * k * b - k^2 + k)/2

= (2 * k * b - k^2 + k)/2

= (2 * k * b - k^2 + k)/2

= (2 * k * b - k^2 + k)/2

= (2 * k * b - k^2 + k)/2

= (2 * k * b - k^2 + k)/2

= (2 * k * b - k^2 + k)/2

= (2 * k * b - k^2 + k)/2

= (2 * k * b - k^2 + k)/2

= (2 * k * b - k^2 + k)/2

= (2 * k * b - k^2 + k)/2

= (2 * k * b - k^2 + k)/2

= (2 * k * b - k^2 + k)/2

= (2 * k * b - k^2 + k)/2

= (2 * k * b - k^2 + k)/2

= (2 * k * b - k^2 + k)/2

= (2 * k * b - k^2 + k)/2

= (2 * k * b - k^2 + k)/2

= (2 * k * b - k^2 + k)/2

= (2 * k * b - k^2 + k)/2

= (2 * k * b - k^2 + k)/2

= (2 * k * b - k^2 + k)/2

= (2 * k * b - k^2 + k)/2

= (2 * k * b - k^2 + k)/2

= (2 * k * b - k^2 + k)/2

= (2 * k * b - k^2 + k)/2

= (2 * k * b - k^2 + k)/2

= (2 * k * b - k^2 + k)/2

= (2 * k * b - k^2 + k)/2

= (2 * k * b - k^2 + k)/2

= (2 * k * b - k^2 + k)/2

= (2 * k * b - k^2 + k)/2

= (2 * k * b - k^2 + k)/2

= (2 * k * b - k^2 + k)/2

= (2 * k * b - k^2 + k)/2

= (2 * k * b - k^2 + k)/2

= (2 * k * b - k^2 + k)/2

= (2 * k * b - k^2 + k)/2

= (2 * k * b - k^2 + k)/2

= (2 * k * b - k^2 + k)/2

= (2 * k * b - k^2 + k)/2

= (2 * k * b - k^2 + k)/2

= (2 * k * b - k^2 + k)/2

= (2 * k * b - k^2 + k)/2

= (2 * k * b - k^2 + k)/2

= (2 * k * b - k^2 + k)/2

= (2 * k * b - k^2 + k)/2

= (2 * k * b - k^2 + k)/2

= (2 * k * b - k^2 + k)/2

= (2 * k * b - k^2 + k)/2

= (2 * k * b - k^2 + k)/2

= (2 * k * b - k^2 + k)/2

= (2 * k * b - k^2 + k)/2

= (2 * k * b - k^2 + k)/2

= (2 * k * b - k^2 + k)/2

= (2 * k * b - k^2 + k)/2

= (2 * k * b - k^2 + k)/2

= (2 * k * b - k^2 + k)/2

= (2 * k * b - k^2 + k)/2

= (2 * k * b - k^2 + k)/2

= (2 * k * b - k^2 + k)/2

= (2 * k * b - k^2 + k)/2

= (2 * k * b - k^2 + k)/2

= (2 * k * b - k^2 + k)/2

= (2 * k * b - k^2 + k)/2

= (2 * k * b - k^2 + k)/2

= (2 * k * b - k^2 + k)/2

= (2 * k * b - k^2 + k)/2

= (2 * k * b - k^2 + k)/2

= (2 * k * b - k^2 + k)/2

= (2 * k * b - k^2 + k)/2

= (2 * k * b - k^2 + k)/2

= (2 * k * b - k^2 + k)/2

= (2 * k * b - k^2 + k)/2

= (2 * k * b - k^2 + k)/2

= (2 * k * b - k^2 + k)/2

= (2 * k * b - k^2 + k)/2

= (2 * k * b - k^2 + k)/2

= (2 * k * b - k^2 + k)/2

= (2 * k * b - k^2 + k)/2

= (2 * k * b - k^2 + k)/2

= (2 * k * b - k^2 + k)/2

= (2 * k * b - k^2 + k)/2

= (2 * k * b - k^2 + k)/2

= (2 * k * b - k^2 + k)/2

= (2 * k * b - k^2 + k)/2

= (2 * k * b - k^2 + k)/2

= (2 * k * b - k^2 + k)/2

= (2 * k * b - k^2 + k)/2

= (2 * k * b - k^2 + k)/2

= (2 * k * b - k^2 + k)/2

= (2 * k * b - k^2 + k)/2

= (2 * k * b - k^2 + k)/2

= (2 * k * b - k^2 + k)/2

= (2 * k * b - k^2 + k)/2

= (2 * k * b - k^2 + k)/2

= (2 * k * b - k^2 + k)/2

= (2 * k * b - k^2 + k)/2

= (2 * k * b - k^2 + k)/2

= (2 * k * b - k^2 + k)/2

= (2 * k * b - k^2 + k)/2

= (2 * k * b - k^2 + k)/2

= (2 * k * b - k^2 + k)/2

= (2 * k * b - k^2 + k)/2

= (2 * k * b - k^2 + k)/2

= (2 * k * b - k^2 + k)/2

= (2 * k * b - k^2 + k)/2

= (2 * k * b - k^2 + k)/2

= (2 * k * b - k^2 + k)/2

= (2 * k * b - k^2 + k)/2

= (2 * k * b - k^2 + k)/2

= (2 * k * b - k^2 + k)/2

= (2 * k * b - k^2 + k)/2

= (2 * k * b - k^2 + k)/2

= (2 * k * b - k^2 + k)/2

= (2 * k * b - k^2 + k)/2

= (2 * k * b - k^2 + k)/2

= (2 * k * b - k^2 + k)/2

= (2 * k * b - k^2 + k)/2

= (2 * k * b - k^2 + k)/2

= (2 * k * b - k^2 + k)/2

= (2 * k * b - k^2 + k)/2

= (2 * k * b - k^2 + k)/2

= (2 * k * b - k^2 + k)/2

= (2 * k * b - k^2 + k)/2

= (2 * k * b - k^2 + k)/2

= (2 * k * b - k^2 + k)/2

= (2 * k * b - k^2 + k)/2

= (2 * k * b - k^2 + k)/2

= (2 * k * b - k^2 + k)/2

= (2 * k * b - k^2 + k)/2

= (2 * k * b - k^2 + k)/2

= (2 * k * b - k^2 + k)/2

= (2 * k * b - k^2 + k)/2

= (2 * k * b - k^2 + k)/2

= (2 * k * b - k^2 + k)/2

= (2 * k * b - k^2 + k)/2

= (2 * k * b - k^2 + k)/2

= (2 * k * b - k^2 + k)/2

= (2 * k * b - k^2 + k)/2

= (2 * k * b - k^2 + k)/2

= (2 * k * b - k^2 + k)/2

= (2 * k * b - k^2 + k)/2

= (2 * k * b - k^2 + k)/2

= (2 * k * b - k^2 + k)/2

= (2 * k * b - k^2 + k)/2

= (2 * k * b - k^2 + k)/2

= (2 * k * b - k^2 + k)/2

= (2 * k * b - k^2 + k)/2

= (2 * k * b - k^2 + k)/2

= (2 * k * b - k^2 + k)/2

= (2 * k * b - k^2 + k)/2

= (2 * k * b - k^2 + k)/2

= (2 * k * b - k^2 + k)/2

= (2 * k * b - k^2 + k)/2

= (2 * k * b - k^2 + k)/2

= (2 * k * b - k^2 + k)/2

= (2 * k * b - k^2 + k)/2

= (2 * k * b - k^2 + k)/2

= (2 * k * b - k^2 + k)/2

= (2 * k * b - k^2 + k)/2

= (2 * k * b - k^2 + k)/2

= (2 * k * b - k^2 + k)/2

= (2 * k * b - k^2 + k)/2

= (2 * k * b - k^2 + k)/2

= (2 * k * b - k^2 + k)/2

= (2 * k * b - k^2 + k)/2

= (2 * k * b - k^2 + k)/2

= (2 * k * b - k^2 + k)/2

= (2 * k * b - k^2 + k)/2

= (2 * k * b - k^2 + k)/2

= (2 * k * b - k^2 + k)/2

= (2 * k * b - k^2 + k)/2

= (2 * k * b - k^2 + k)/2

= (2 * k * b - k^2 + k)/2

= (2 * k * b - k^2 + k)/2

= (2 * k * b - k^2 + k)/2

= (2 * k * b - k^2 + k)/2

= (2 * k * b - k^2 + k)/2

= (2 * k * b - k^2 + k)/2

= (2 * k * b - k^2 + k)/2

= (2 * k * b - k^2 + k)/2

= (2 * k * b - k^2 + k)/2

= (2 * k * b - k^2 + k)/2

= (2 * k * b - k^2 + k)/2

= (2 * k * b - k^2 + k)/2

= (2 * k * b - k^2 + k)/2

= (2 * k * b - k^2 + k)/2

= (2 * k * b - k^2 + k)/2

= (2 * k * b - k^2 + k)/2

= (2 * k * b - k^2 + k)/2

= (2 * k * b - k^2 + k)/2

= (2 * k * b - k^2 + k)/2

= (2 * k * b - k^2 + k)/2

= (2 * k * b - k^2 + k)/2

= (2 * k * b - k^2 + k)/2

= (2 * k * b - k^2 + k)/2

= (2 * k * b - k^2 + k)/2

= (2 * k * b - k^2 + k)/2

= (2 * k * b - k^2 + k)/2

= (2 * k * b - k^2 + k)/2

= (2 * k * b - k^2 + k)/2

= (2 * k * b - k^2 + k)/2

= (2 * k * b - k^2 + k)/2

= (2 * k * b - k^2 + k)/2

= (2 * k * b - k^2 + k)/2

= (2 * k * b - k^2 + k)/2

= (2 * k * b - k^2 + k)/2

= (2 * k * b - k^2 + k)/2

= (2 * k * b - k^2 + k)/2

= (2 * k * b - k^2 + k)/2

= (2 * k * b - k^2 + k)/2

= (2 * k * b - k^2 + k)/2

= (2 * k * b - k^2 + k)/2

= (2 * k * b - k^2 + k)/2

= (2 * k * b - k^2 + k)/2

= (2 * k * b - k^2 + k)/2

= (2 * k * b - k^2 + k)/2

= (2 * k * b - k^2 + k)/2

= (2 * k * b - k^2 + k)/2

= (2 * k * b - k^2 + k)/2

= (2 * k * b - k^2 + k)/2

= (2 * k * b - k^2 + k)/2

= (2 * k * b - k^2 + k)/2

= (2 * k * b - k^2 + k)/2

= (2 * k * b - k^2 + k)/2

= (2 * k * b - k^2 + k)/2

= (2 * k * b - k^2 + k)/2

= (2 * k * b - k^2 + k)/2

= (2 * k * b - k^2 + k)/2

= (2 * k * b - k^2 + k)/2

= (2 * k * b - k^2 + k)/2

= (2 * k * b - k^2 + k)/2

= (2 * k * b - k^2 + k)/2

= (2 * k * b - k^2 + k)/2

= (2 * k * b - k^2 + k)/2

= (2 * k * b - k^2 + k)/2

= (2 * k * b - k^2 + k)/2

= (2 * k * b - k^2 + k)/2

= (2 * k * b - k^2 + k)/2

= (2 * k * b - k^2 + k)/2

= (2 * k * b - k^2 + k)/2

= (2 * k * b - k^2 + k)/2

= (2 * k * b - k^2 + k)/2

= (2 * k * b - k^2 + k)/2

= (2 * k * b - k^2 + k)/2

= (2 * k * b - k^2 + k)/2

= (2 * k * b - k^2 + k)/2

= (2 * k * b - k^2 + k)/2

= (2 * k * b - k^2 + k)/2

= (2 * k * b - k^2 + k)/2

= (2 * k * b - k^2 + k)/2

= (2 * k * b - k^2 + k)/2

= (2 * k * b - k^2 + k)/2

= (2 * k * b - k^2 + k)/2

= (2 * k * b - k^2 + k)/2

= (2 * k * b - k^2 + k)/2

= (2 * k * b - k^2 + k)/2

= (2 * k * b - k^2 + k)/2

= (2 * k * b - k^2 + k)/2

= (2 * k * b - k^2 + k)/2

= (2 * k * b - k^2 + k)/2

= (2 * k * b - k^2 + k)/2

= (2 * k * b - k^2 + k)/2

= (2 * k * b - k^2 + k)/2

= (2 * k * b - k^2 + k)/2

= (2 * k * b - k^2 + k)/2

= (2 * k * b - k^2 + k)/2

= (2 * k * b - k^2 + k)/2

= (2 * k * b - k^2 + k)/2

= (2 * k * b - k^2 + k)/2

= (2 * k * b - k^2 + k)/2

= (2 * k * b - k^2 + k)/2

= (2 * k * b - k^2 + k)/2

= (2 * k * b - k^2 + k)/2

= (2 * k * b - k^2 + k)/2

= (2 * k * b - k^2 + k)/2

= (2 * k * b - k^2 + k)/2

= (2 * k * b - k^2 + k)/2

= (2 * k * b - k^2 + k)/2

= (2 * k * b - k^2 + k)/2

= (2 * k * b - k^2 + k)/2

= (2 * k * b - k^2 + k)/2

= (2 * k * b - k^2 + k)/2

= (2 * k * b - k^2 + k)/2

= (2 * k * b - k^2 + k)/2

= (2 * k * b - k^2 + k)/2

= (2 * k * b - k^2 + k)/2

= (2 * k * b - k^2 + k)/2

= (2 * k * b - k^2 + k)/2

= (2 * k * b - k^2 + k)/2

= (2 * k * b - k^2 + k)/2

= (2 * k * b - k^2 + k)/2

= (2 * k * b - k^2 + k)/2

= (2 * k * b - k^2 + k)/2

= (2 * k * b - k^2 + k)/2

= (2 * k * b - k^2 + k)/2

= (2 * k * b - k^2 + k)/2

= (2 * k * b - k^2 + k)/2

= (2 * k * b - k^2 + k)/2

= (2 * k * b - k^2 + k)/2

= (2 * k * b - k^2 + k)/2

= (2 * k * b - k^2 + k)/2

= (2 * k * b - k^2 + k)/2

= (2 * k * b - k^2 + k)/2

= (2 * k * b - k^2 + k)/2

= (2 * k * b - k^2 + k)/2

= (2 * k * b - k^2 + k)/2

= (2 * k * b - k^2 + k)/2

= (2 * k * b - k^2 + k)/2

= (2 * k * b - k^2 + k)/2

= (2 * k * b - k^2 + k)/2

= (2 * k * b - k^2 + k)/2

= (2 * k * b - k^2 + k)/2

= (2 * k * b - k^2 + k)/2

= (2 * k * b - k^2 + k)/2

= (2 * k * b - k^2 + k)/2

= (2 * k * b - k^2 + k)/2

= (2 * k * b - k^2 + k)/2

= (2 * k * b - k^2 + k)/2

= (2 * k * b - k^2 + k)/2

= (2 * k * b - k^2 + k)/2

= (2 * k * b - k^2 + k)/2

= (2 * k * b - k^2 + k)/2

= (2 * k * b - k^2 + k)/2

= (2 * k * b - k^2 + k)/2

= (2 * k * b - k^2 + k)/2

= (2 * k * b - k^2 + k)/2

= (2 * k * b - k^2 + k)/2

= (2 * k * b - k^2 + k)/2

= (2 * k * b - k^2 + k)/2

= (2 * k * b - k^2 + k)/2

= (2 * k * b - k^2 + k)/2

= (2 * k * b - k^2 + k)/2

= (2 * k * b - k^2 + k)/2

= (2 * k * b - k^2 + k)/2

= (2 * k * b - k^2 + k)/2

= (2 * k * b - k^2 + k)/2

= (2 * k * b - k^2 + k)/2

= (2 * k * b - k^2 + k)/2

= (2 * k * b - k^2 + k)/2

= (2 * k * b - k^2 + k)/2

= (2 * k * b - k^2 + k)/2

= (2 * k * b - k^2 + k)/2

= (2 * k * b - k^2 + k)/2

= (2 * k * b - k^2 + k)/2

= (2 * k * b - k^2 + k)/2

= (2 * k * b - k^2 + k)/2

= (2 * k * b - k^2 + k)/2

= (2 * k * b - k^2 + k)/2

= (2 * k * b - k^2 + k)/2

= (2 * k * b - k^2 + k)/2

= (2 * k * b - k^2 + k)/2

= (2 * k * b - k^2 + k)/2

= (2 * k * b - k^2 + k)/2

= (2 * k * b - k^2 + k)/2

= (2 * k * b - k^2 + k)/2

= (2 * k * b - k^2 + k)/2

= (2 * k * b - k^2 + k)/2

= (2 * k * b - k^2 + k)/2

= (2 * k * b - k^2 + k)/2

= (2 * k * b - k^2 + k)/2

= (2 * k * b - k^2 + k)/2

= (2 * k * b - k^2 + k)/2

= (2 * k * b - k^2 + k)/2

= (2 * k * b - k^2 + k)/2

= (2 * k * b - k^2 + k)/2

= (2 * k * b - k^2 + k)/2

= (2 * k * b - k^2 + k)/2

= (2 * k * b - k^2 + k)/2

= (2 * k * b - k^2 + k)/2

= (2 * k * b - k^2 + k)/2

= (2 * k * b - k^2 + k)/2

= (2 * k * b - k^2 + k)/2

= (2 * k * b - k^2 + k)/2

= (2 * k * b - k^2 + k)/2