To thoroughly evaluate the correctness of the given program, let's re-examine the problem description, the provided code, and the annotations, and compare them with the original assessment.

### Problem Recap:
We need to calculate the expected value of the sum of friendship values of all `k` pairs chosen for excursions, expressed as a fraction \(\frac{p}{q}\), where \(p\) and \(q\) are coprime integers. The final output should be \(p \cdot q^{-1} \bmod (10^9+7)\).

### Mathematical Derivation:
The expected value for a single friend pair with initial friendship value \(f\) over `k` excursions is:
\[ E = f \cdot \left(1 + \frac{k-1}{C(n,2)} + \frac{(k-1)(k-2)}{C(n,2)^2} + \ldots \right) \]
This simplifies to:
\[ E = f \cdot \left(1 + \frac{k-1}{C(n,2)-1}\right) \]

Summing over all friend pairs, the expected value \(E_{total}\) is:
\[ E_{total} = \sum_{i=1}^{m} f_i \cdot \left(1 + \frac{k-1}{C(n,2)-1}\right) \]
\[ E_{total} = \left(\sum_{i=1}^{m} f_i\right) + \left(\sum_{i=1}^{m} f_i\right) \cdot \frac{k-1}{C(n,2)-1} \]
\[ E_{total} = \text{sum\_f} + \text{sum\_f} \cdot \frac{k-1}{C(n,2)-1} \]
\[ E_{total} = \text{sum\_f} \cdot \left(1 + \frac{k-1}{C(n,2)-1}\right) \]

Expressing \(E_{total}\) as a fraction \(\frac{p}{q}\):
\[ E_{total} = \frac{\text{sum\_f} \cdot (C(n,2) - 1 + k - 1)}{C(n,2) - 1} \]
\[ E_{total} = \frac{\text{sum\_f} \cdot (C(n,2) + k - 2)}{C(n,2) - 1} \]

Where \(C(n,2) = \frac{n(n-1)}{2}\).

### Code Analysis:
The provided code calculates `p` and `q` as follows:
\[ p = 2 \cdot k \cdot C(n,2) \cdot \text{sum\_f} + m \cdot k \cdot (k - 1) \]
\[ q = 2 \cdot C(n,2)^2 \]

However, these formulas do not match the derived expected value formula. Let's derive the correct formulas:

\[ p = \text{sum\_f} \cdot (C(n,2) + k - 2) \]
\[ q = C(n,2) - 1 \]

### Correct Implementation:
The correct implementation should be:
```python
import math

def func():
    t = int(input())
    M = 10 ** 9 + 7
    for i in range(t):
        n, m, k = map(int, input().split())
        sum_f = 0
        for j in range(m):
            a, b, f = map(int, input().split())
            sum_f += f
        cn2 = n * (n - 1) // 2
        p = sum_f * (cn2 + k - 2)
        q = cn2 - 1
        gcd = math.gcd(p, q)
        p = p // gcd
        q = q // gcd
        print(int(p * pow(q, -1, M) % M))

func()
```

### Conclusion:
The original code does not correctly implement the derived formula for the expected value. The correct formulas for `p` and `q` should be:
\[ p = \text{sum\_f} \cdot (C(n,2) + k - 2) \]
\[ q = C(n,2) - 1 \]

Thus, the original assessment is inaccurate.

Final: **False**