To determine the output state, let's analyze the given loop and how it modifies the variables `arr`, `ans`, and `tem`.

### Initial State:
- `arr`: A list of integers
- `ans`: An empty list
- `tem`: 1

### Loop Analysis:
The loop iterates over the list `arr` in reverse order (from the last element to the first element). For each element in the list, it multiplies the current value of `tem` by the element and appends the result to the list `ans`.

### Step-by-Step Execution:
1. **Initialization**: `tem = 1`, `ans = []`
2. **First Iteration (i = len(arr) - 1)**:
   - `tem *= arr[len(arr) - 1]` → `tem = 1 * arr[len(arr) - 1]`
   - `ans.append(tem)` → `ans = [arr[len(arr) - 1]]`
3. **Second Iteration (i = len(arr) - 2)**:
   - `tem *= arr[len(arr) - 2]` → `tem = arr[len(arr) - 1] * arr[len(arr) - 2]`
   - `ans.append(tem)` → `ans = [arr[len(arr) - 1], arr[len(arr) - 1] * arr[len(arr) - 2]]`
4. **Continuing this pattern**:
   - For each iteration `i`, `tem` becomes the product of all elements from `arr[i]` to `arr[len(arr) - 1]`.
   - `ans` appends the current value of `tem` after each iteration.

### Final Output State:
- `arr`: Remains unchanged as the loop does not modify `arr`.
- `ans`: A list where each element is the cumulative product of the elements in `arr` from the end up to the current element.
- `tem`: The product of all elements in `arr`.

### Example:
If `arr = [2, 3, 4]`:
- Iteration 1 (i = 2): `tem = 1 * 4`, `ans = [4]`
- Iteration 2 (i = 1): `tem = 4 * 3`, `ans = [4, 12]`
- Iteration 3 (i = 0): `tem = 12 * 2`, `ans = [4, 12, 24]`

### Final Output State:
- `arr`: `[2, 3, 4]`
- `ans`: `[4, 12, 24]`
- `tem`: `24`

**Output State: arr is a list of integers; ans is a list of cumulative products of arr elements in reverse order; tem is the product of all elements in arr.**