Given the initial state:
- \( n \) is an integer such that \( 1 \leq n \leq 10^{18} \)
- \( n = n - \text{min}(k, \text{candies}) \)
- \( k = 1 \)
- \( \text{candies} = \text{candies} - \text{min}(k, \text{candies}) - \text{petya\_eaten} \)
- \( \text{vasya\_eaten} = \text{min}(k, \text{candies}) \)
- \( \text{petya\_eaten} = \text{candies} // 10 \)
- \( \text{candies} > 0 \)

The code block to execute is:
```
vasya_eaten += min(k, candies)
candies -= min(k, candies)
petya_eaten = candies // 10
candies -= petya_eaten
```

Let's analyze each line:

1. `vasya_eaten += min(k, candies)`
   - From the initial state, we know that `vasya_eaten = min(k, candies)`.
   - After this line, `vasya_eaten` becomes `2 \times \text{min}(k, \text{candies})`.

2. `candies -= min(k, candies)`
   - This line subtracts `min(k, candies)` from `candies`.
   - So, `candies` becomes `candies - \text{min}(k, \text{candies})`.

3. `petya_eaten = candies // 10`
   - This line updates `petya_eaten` to be the integer division of `candies` by 10.

4. `candies -= petya_eaten`
   - This line subtracts `petya_eaten` (which is `candies // 10`) from `candies`.
   - So, `candies` becomes `candies - \text{candies} // 10`.

Now, let's summarize the effects:
- Initially, `vasya_eaten = \text{min}(k, \text{candies})` and `k = 1`.
- After the first line, `vasya_eaten` becomes `2 \times \text{min}(k, \text{candies})`.
- After the second line, `candies` becomes `candies - \text{min}(k, \text{candies})`.
- After the third line, `petya_eaten` is set to `candies // 10`.
- After the fourth line, `candies` becomes `candies - \text{candies} // 10`.

Since `k = 1`, `min(k, candies)` simplifies to `1` if `candies >= 1` (which it must be since `candies > 0`). Therefore, the final state can be simplified as follows:
- `vasya_eaten = 2 \times 1 = 2`
- `candies = \text{candies} - 1`
- `petya_eaten = (\text{candies} - 1) // 10`
- `candies = (\text{candies} - 1) - ((\text{candies} - 1) // 10)`

Thus, the final output state is:
Output State: **vasya\_eaten is 2, candies is candies - 1, petya\_eaten is (\text{candies} - 1) // 10, n is n - 1**