Let's analyze the loop step by step to determine the final state of the variables after all iterations.

### Initial State
- \( i = 2 \)
- \( n \geq 2 \)
- \( \text{cur} = 2 \)

### Loop Condition
The loop continues as long as \( i \times \text{cur} \leq n \).

### Loop Body
- \( \text{ans} += 4 \times \text{cur} \)
- \( \text{cur} += 1 \)

### Iteration Analysis
#### First Iteration
- \( i = 2 \)
- \( \text{cur} = 2 \)
- \( i \times \text{cur} = 2 \times 2 = 4 \leq n \) (since \( n \geq 4 \))
- \( \text{ans} += 4 \times 2 = 8 \)
- \( \text{cur} += 1 = 3 \)

Output State after 1 iteration:
- \( i = 2 \)
- \( n \geq 4 \)
- \( \text{cur} = 3 \)
- \( \text{ans} = 8 \)

#### Second Iteration
- \( i = 2 \)
- \( \text{cur} = 3 \)
- \( i \times \text{cur} = 2 \times 3 = 6 \leq n \) (since \( n \geq 6 \))
- \( \text{ans} += 4 \times 3 = 12 \)
- \( \text{cur} += 1 = 4 \)

Output State after 2 iterations:
- \( i = 2 \)
- \( n \geq 6 \)
- \( \text{cur} = 4 \)
- \( \text{ans} = 8 + 12 = 20 \)

#### Third Iteration
- \( i = 2 \)
- \( \text{cur} = 4 \)
- \( i \times \text{cur} = 2 \times 4 = 8 \leq n \) (since \( n \geq 8 \))
- \( \text{ans} += 4 \times 4 = 16 \)
- \( \text{cur} += 1 = 5 \)

Output State after 3 iterations:
- \( i = 2 \)
- \( n \geq 8 \)
- \( \text{cur} = 5 \)
- \( \text{ans} = 20 + 16 = 36 \)

### Generalization
From the above iterations, we can generalize that each iteration increments \(\text{cur}\) by 1 and adds \(4 \times \text{cur}\) to \(\text{ans}\). The loop will continue until \( i \times \text{cur} > n \).

Let's denote the number of iterations as \( k \). After \( k \) iterations:
- \( \text{cur} = 2 + k \)
- \( i \times \text{cur} \leq n \Rightarrow 2 \times (2 + k) \leq n \Rightarrow 4 + 2k \leq n \Rightarrow n \geq 4 + 2k \)
- \( \text{ans} = 4 \times 2 + 4 \times 3 + 4 \times 4 + \ldots + 4 \times (2 + k) \)
- \( \text{ans} = 4(2 + 3 + 4 + \ldots + (2 + k)) \)
- Sum of an arithmetic series: \( 2 + 3 + 4 + \ldots + (2 + k) = \frac{k(k + 3)}{2} \)
- Therefore, \( \text{ans} = 4 \times \frac{k(k + 3)}{2} = 2k(k + 3) \)

When the loop ends, \( \text{cur} = 2 + k \) and \( i \times \text{cur} > n \), so \( 4 + 2k < n \).

### Final Output State
After all iterations, the loop terminates when \( i \times \text{cur} > n \):
- \( \text{cur} = 2 + k \) where \( k \) is the number of iterations such that \( 4 + 2k < n \)
- \( \text{ans} = 2k(k + 3) \)

Output State: **'i' is 2, 'cur' is \( 2 + k \) where \( k \) is the number of iterations such that \( 4 + 2k < n \), 'n' must satisfy \( 4 + 2k < n \), 'ans' is \( 2k(k + 3) \)**