The code snippet `x -= 2 ** i - 1` modifies the value of `x` by subtracting `2 ** i - 1` from it. Given the initial state, `i` is 58, so `2 ** i - 1` equals `2 ** 58 - 1`. Therefore, `x` is decreased by this value.

Let's calculate the new value of `x`:
- Initial value of `x` is at least `2^59 - 1`.
- Subtract `2 ** 58 - 1` from `x`.

The new value of `x` is:
\[ x_{\text{new}} = x_{\text{initial}} - (2^{58} - 1) \]

Since `x_{\text{initial}}` is at least `2^{59} - 1`, the minimum new value of `x` is:
\[ x_{\text{new}} = (2^{59} - 1) - (2^{58} - 1) = 2^{59} - 2^{58} = 2^{58}(2 - 1) = 2^{58} \]

So, `x` will be at least `2^{58}` after the operation. The other variables remain unchanged.

Output State: **`t` is an integer such that 1 <= `t` <= 1000, and for each of the `t` test cases, `X` is an integer such that 2 <= `X` <= 10^18; `x` is at least 2^58; `subseq_lens` is [58]; `mx` is 0 or 59; `i` is 58 and not equal to 0.**