The variable `full_rows` is assigned the value of `k // (m - 1)`. In this case, `k` has already been updated to `k - (n - 1)` in the previous step. Since `m` is an integer such that `2 ≤ m ≤ 10^9`, the value of `m - 1` is at least `1`. 

Now let's express the new value of `full_rows`:

1. The value of `k` is now `k' = k - (n - 1)`.
2. Since `k'` is non-negative and less than `n·m`, we can calculate `full_rows` as `full_rows = (k - (n - 1)) // (m - 1)`.

Thus, the Output State will incorporate the updated value of `k` and the calculated value of `full_rows`.

Output State: **`n` is an even integer such that 2 ≤ n ≤ 10^9; `m` is an integer such that 2 ≤ m ≤ 10^9; `k` is a non-negative integer such that 0 ≤ k < n·m and now `k` is equal to the previous value of `k` minus `n - 1; `full_rows` is equal to `(previous k - (n - 1)) // (m - 1)`**.