The code snippet `ans += ss` appends the character `ss` to the string `ans`. Given that `ans` was initially an empty string, after this operation, `ans` will be equal to `ss`.

Here's the updated output state:

Output State: **`t` is an integer such that 1 ≤ t ≤ 10^5, `n`, `k`, `m` are integers read from the input, `s` is a non-empty string, `ss` is the next character in the string `s`, `cur_ss` is `ord(ss) - ord('a')`. If `cur & (1 << cur_ss) == 0`, then `cur` is updated to `cur + (1 << cur_ss)`. If after the update, `cur` equals `(1 << k) - 1`, then `cnt` becomes 1 and `ans` becomes the string `s`; otherwise, `cnt` remains 0 and `ans` remains an empty string. `cnt` is now 1; `cur` is 0; `ans` is `ss`.**