To determine the final output state after all iterations of the loop, we need to understand how the loop evolves with each iteration based on the given initial state and the provided intermediate output states.

### Initial State:
- `a` is `[0, 0, d_1, d_1, d_1 + d_2, d_1 + d_2, ..., sum(d_1, ..., d_{n-2}), sum(d_1, ..., d_{n-2}) + d_{n-1}]`
- `u` is `0`
- `t` is `0`
- `a` is `-1000000000.0`
- `b` is `[0, 0]`

### Loop Code:
```python
for w, x, y, z in zip(a, a[1:], a[2:], a[3:]):
    v = y - x
    b += b[-2] + v ** (v > x - w), b[-1] + v ** (v > z - y)
```

### Observations from Intermediate States:
1. **After 1st Iteration:**
   - `a` remains `[0, 1, 2, 3]`
   - `b` becomes `[0, 0, v]` where `v = y - x = 2 - 1 = 1`
   
2. **After 2nd Iteration:**
   - `a` remains `[0, 1, 2, 3]`
   - `b` becomes `[0, 0, 1, v]` where `v = y - x = 3 - 2 = 1`
   
3. **After 3rd Iteration:**
   - `a` remains `[0, 1, 2, 3]`
   - `b` becomes `[0, 0, 1, 1, (1) + (1)]` which simplifies to `[0, 0, 1, 1, 2]`

### Analysis:
- The loop iterates over the elements of `a` in groups of four (`w, x, y, z`).
- For each iteration, it calculates `v = y - x`.
- It then appends two new elements to `b`:
  - `b[-2] + v ** (v > x - w)`
  - `b[-1] + v ** (v > z - y)`

### Given `a` is `[0, 1, 2, 3]`:
- The loop can only run once because there are only 4 elements in `a`, and `zip(a, a[1:], a[2:], a[3:])` will only produce one tuple `(0, 1, 2, 3)`.

### Final Calculation:
- `v = y - x = 2 - 1 = 1`
- `b[-2]` is `0` and `b[-1]` is `0` initially.
- After the first iteration:
  - `b[-2] + v ** (v > x - w) = 0 + 1 ** (1 > 1 - 0) = 0 + 1 = 1`
  - `b[-1] + v ** (v > z - y) = 0 + 1 ** (1 > 3 - 2) = 0 + 1 = 1`
- Thus, `b` becomes `[0, 0, 1, 1]`.

### Conclusion:
Since the loop can only run once with the given `a`, the final output state is:

Output State: **[0, 0, 1, 1]**.

In natural language, this means that after the loop has executed all possible iterations (which is just one in this case), the list `b` contains the initial two zeros followed by two ones.