To determine the output of the `print(dp[m])` statement, let's analyze the given initial state and the formula used to populate the `dp` array.

### Initial State and Formula:
- The `dp` array is populated from `dp[1]` to `dp[m]` using the formula:
  \[
  dp[i] = (dp[i - 1] + (i - 1) \cdot dp[i - 2] \cdot 2) \mod (10^9 + 7)
  \]
- The values of `t`, `n`, `k`, `num`, and `m` remain unchanged, but they are not directly used in the formula for `dp[i]`.

### Calculation Steps:
1. **Initialization**: Typically, `dp[0]` and `dp[1]` are initialized to some base values. Since the problem does not specify these base values, we will assume common initializations:
   - `dp[0] = 0`
   - `dp[1] = 1`
   
2. **Recursive Calculation**:
   - For `i = 2` to `m`, the value of `dp[i]` is calculated using the given formula.

### Example Calculation:
Let's walk through the calculation for a small value of `m` to understand the pattern.

- **Base Cases**:
  - `dp[0] = 0`
  - `dp[1] = 1`

- **For `i = 2`**:
  \[
  dp[2] = (dp[1] + (2 - 1) \cdot dp[0] \cdot 2) \mod (10^9 + 7)
  \]
  \[
  dp[2] = (1 + 1 \cdot 0 \cdot 2) \mod (10^9 + 7) = 1 \mod (10^9 + 7) = 1
  \]

- **For `i = 3`**:
  \[
  dp[3] = (dp[2] + (3 - 1) \cdot dp[1] \cdot 2) \mod (10^9 + 7)
  \]
  \[
  dp[3] = (1 + 2 \cdot 1 \cdot 2) \mod (10^9 + 7) = (1 + 4) \mod (10^9 + 7) = 5 \mod (10^9 + 7) = 5
  \]

- **For `i = 4`**:
  \[
  dp[4] = (dp[3] + (4 - 1) \cdot dp[2] \cdot 2) \mod (10^9 + 7)
  \]
  \[
  dp[4] = (5 + 3 \cdot 1 \cdot 2) \mod (10^9 + 7) = (5 + 6) \mod (10^9 + 7) = 11 \mod (10^9 + 7) = 11
  \]

### General Description:
The value of `dp[m]` is the result of the recursive formula applied from `dp[2]` to `dp[m]` with the base cases `dp[0] = 0` and `dp[1] = 1`. Since the exact value of `m` is not provided, we can't compute the exact numerical value of `dp[m]`. However, based on the structure of the problem, the print statement will output the calculated value of `dp[m]`.

### Final Output:
Output: **dp[m] (where dp[m] is calculated using the recursive formula starting from dp[0] = 0 and dp[1] = 1)**