The code snippet `ans += y` increments the value of `ans` by the value of `y`. Here's the detailed impact:

- `ans` is incremented by the value of `y`.
- All other variables (`t`, `n`, `x`, `y`, `tt`, `ii`, `i`, `a`, `tmp`) remain unchanged.

Given the initial state:
- `t` is a positive integer where 1 ≤ t ≤ 10^4.
- `n` is an input integer where 4 ≤ n ≤ 10^9.
- `x` is an input integer where 2 ≤ x ≤ min(n, 2 · 10^5).
- `y` is an input integer.
- `tt` is greater than 2.
- `ii` is 2.
- `i` is `len(a) - 1`.
- `a` is a sorted list of integers in ascending order.
- `tmp` is a list of integers.
- `ans` is the final computed value based on the loop's operations.

After executing `ans += y`:
- `ans` is now `ans + y`.

Therefore, the Output State is:
**`t` is a positive integer where 1 ≤ t ≤ 10^4, `n` is an input integer where 4 ≤ n ≤ 10^9, `x` is an input integer where 2 ≤ x ≤ min(n, 2 · 10^5), `y` is an input integer, `tt` is greater than 2, `ii` is 2, `i` is `len(a) - 1`, `a` is a sorted list of integers in ascending order, `tmp` is a list of integers, and `ans` is `ans + y`.**