The code snippet `cnt -= 1` decrements the value of `cnt` by 1. Given that the initial value of `cnt` is `k - 2`, after the decrement, `cnt` will be `k - 3`.

The other variables (`n`, `k`, `v`, `l`, and `i`) remain unchanged.

Therefore, the Output State is:
Output State: **`n` is a positive integer such that `n >= 3 * k`, `k` is an integer such that `3 <= k <= n`, `v` is the value returned by `func_2()` during the last iteration (`i = 1`) and `v < n`, `cnt` is `k - 3`, `l` is `func_2() + 1`, `i` is `3`.**