The statement `P[i] = P[i - 1] + 1` assigns the value of `P[i - 1] + 1` to `P[i]`. Since the value of `i` is equal to `N`, `P[N]` will be updated. The value of `P[N - 1]` is used for this assignment, but the previous state of `P[0]` remains unchanged because `i` was not equal to 0. 

Therefore, the output state is: `S` is a string of length `N`, `N` is an integer such that 2 <= N <= 100000, `Q` is an integer such that 1 <= Q <= 100000, `P[0]` remains unchanged, and `P[N]` is updated to `P[N - 1] + 1`.

Output State: **`S` is a string of length `N`, `N` is an integer such that 2 <= N <= 100000, `Q` is an integer such that 1 <= Q <= 100000, `P[0]` remains unchanged, and `P[N]` is updated to `P[N - 1] + 1**