The code appends the result of `k0 - sum(ans)` to the list `ans`. Given the initial state, `k0` is 1 and `ans` is `[2, -1, 2]`. The sum of `ans` is `2 + (-1) + 2 = 3`. Therefore, the value to be appended is `1 - 3 = -2`.

Thus, the updated `ans` list becomes `[2, -1, 2, -2]`.

Output State: **`t` is an integer such that 1 ≤ `t` ≤ 10^4, `l1` is a list of substrings obtained by splitting the input line on whitespace, `n` is the integer value of the first element of `l1`, `k` is 0, `k0` is 1, `arr` is [0, 1], `i` is 1, `c` is `c + 1`, `ans` is [2, -1, 2, -2]**