Postcondition: ***`n` and `m` are positive integers such that \(1 \leq n, m \leq 2 \times 10^6\), `T` is greater than 2, `t` is 2, `info` is a list of strings from user input, `a` is the integer value of `info[0]`, `b` is the integer value of `info[1]` and must be greater than or equal to `a` and at least 1, `i` is 2, `x` is \(\frac{a - 2}{4} + 1\). If \((a - i \cdot (i - 1)) \% i^2 == 0\) and \(i \cdot (i - 1) \% i^2 == 0\) are both satisfied, `suma` is \(a + 3 + \frac{a - 2}{4}\). Otherwise, `suma` is \(a + 1 + \frac{a - 2}{4} + 1\).***