To determine what will be printed, let's break down the initial state and the code snippet step by step.

1. **Initial State Analysis:**
   - `j` is explicitly given as 3.
   - `n + r + 1` is derived from the condition where \( r \) is the largest integer such that \( r \times n < \frac{n \times (n + 1)}{2} \).

2. **Finding \( r \):**
   - We need to find the largest integer \( r \) such that \( r \times n < \frac{n \times (n + 1)}{2} \).
   - This inequality can be rewritten as \( r < \frac{n + 1}{2} \).
   - Therefore, \( r \) is the floor value of \( \frac{n + 1}{2} - 1 \), i.e., \( r = \left\lfloor \frac{n + 1}{2} - 1 \right\rfloor \).

3. **Determining \( n \):**
   - Since \( n + r + 1 \) is given, we can express \( r \) in terms of \( n \).
   - From the formula \( r = \left\lfloor \frac{n + 1}{2} - 1 \right\rfloor \), we substitute \( r \) into \( n + r + 1 \):
     \[
     n + \left\lfloor \frac{n + 1}{2} - 1 \right\rfloor + 1 = k \quad \text{(for some integer } k \text{)}
     \]
   - Simplifying, we get:
     \[
     n + \left\lfloor \frac{n + 1}{2} - 1 \right\rfloor + 1 = k \implies n + \left\lfloor \frac{n + 1}{2} \right\rfloor - 1 + 1 = k \implies n + \left\lfloor \frac{n + 1}{2} \right\rfloor = k
     \]

4. **Solving for \( n \):**
   - To find \( n \), we need to test values that satisfy the equation.
   - Let's assume \( n = 3 \):
     \[
     r = \left\lfloor \frac{3 + 1}{2} - 1 \right\rfloor = \left\lfloor 2 - 1 \right\rfloor = 1
     \]
     \[
     n + r + 1 = 3 + 1 + 1 = 5
     \]
   - This satisfies the condition since \( r = 1 \) and \( 1 \times 3 < \frac{3 \times 4}{2} = 6 \).

5. **Code Execution:**
   - Given \( n = 3 \), the code snippet is:
     ```
     print(*range(1, n + 1))
     ```
   - This will print the range from 1 to \( n + 1 \), which is 1 to 4.

Output: **1 2 3 4**