Let's analyze the annotated code and the return postconditions step by step to determine the functionality of the function.

### Step-by-Step Analysis

1. **Initial State**:
   - The function `func_1` accepts a parameter `n`, which is a positive integer.

2. **First Condition Check**:
   - If `n` is either 0 or 1, the function immediately returns 1.
     ```python
     if (n == 0 or n == 1) :
         return 1
     ```
   - In this case, the function returns 1.

3. **Sequence Calculation**:
   - If `n` is neither 0 nor 1, the function initializes two variables `S0` and `S1` to 1.
     ```python
     S0, S1 = 1, 1
     ```
   - It then enters a loop that iterates from 2 to `n` (inclusive).
     ```python
     for i in range(2, n + 1):
         S_next = 2 * S1 + S0
         S0, S1 = S1, S_next
     ```
   - In each iteration of the loop:
     - `S_next` is calculated using the formula \(S_{next} = 2S_1 + S_0\).
     - The values of `S0` and `S1` are updated such that `S0` becomes `S1` and `S1` becomes `S_next`.

4. **Final Return**:
   - After the loop completes, the function returns `S1`.
     ```python
     return S1
     ```

### Edge Cases and Missing Logic

- **Edge Case: `n` is 0 or 1**:
  - If `n` is 0 or 1, the function correctly returns 1 as per the code.

- **General Case**:
  - For any other positive integer `n > 1`, the function correctly computes the (n+1)th term in the sequence defined by \(S_0 = 1\), \(S_1 = 1\), and \(S_i = 2S_{i-1} + S_{i-2}\) for \(i \geq 2\).

- **No Missing Logic**:
  - The code correctly implements the logic described in the annotations without any missing steps or conditions.

### Summary

The function `func_1` accepts a positive integer `n` and returns:
- **1** if `n` is either 0 or 1.
- The (n+1)th term in the sequence defined by \(S_0 = 1\), \(S_1 = 1\), and \(S_i = 2S_{i-1} + S_{i-2}\) for \(i \geq 2\) if `n` is greater than 1.

### Functionality:
**The function `func_1` accepts a positive integer `n` and returns 1 if `n` is either 0 or 1, or the (n+1)th term in the sequence defined by \(S_0 = 1\), \(S_1 = 1\), and \(S_i = 2S_{i-1} + S_{i-2}\) for \(i \geq 2\) if `n` is greater than 1.**