Let's break down the problem step by step:

1. **Identify the loop head variables**: The loop head variables are `i` and `a`.

2. **Determine the conditions for the loop to continue**:
   - The loop starts from `i = 1` and goes up to `len(a) - 1`.
   - For the loop to continue, `i` must be less than `len(a)`.

3. **Current state at the end of the previous iteration**:
   - `i` is 2.
   - `a` is a list of integers with at least 2 elements.
   - `ans` is either increased by 1 if `a[2] - a[1] == 2`, or set to `(a[2] - a[1]) // 2` and `tmp` is a list containing the element `(a[2] - a[1]) // 2`.
   - `y` is updated to `y - ((a[2] - a[1]) // 2 - 1)` if `(a[2] - a[1]) % 2 == 0` and `y > (a[2] - a[1]) // 2 - 1`. If the condition `a[2] - a[1] == 2` is not met, the values of `ans`, `tmp`, and `y` remain unchanged.

4. **Adjust the states for the next iteration**:
   - Since `i` is currently 2, the next value of `i` will be 3.
   - We need to check if `i < len(a)` to determine if the loop should continue. Given that `i` is 2 and assuming `a` has more than 3 elements, the loop will continue.

5. **Update the states**:
   - `i` will be incremented to 3.
   - The other variables (`a`, `ans`, `tmp`, and `y`) will retain their current values unless the loop body changes them.

Therefore, the state at the start of the next iteration of the loop is:

State: **`i` is 3, `a` is a list of integers with at least 2 elements, `ans` is either increased by 1 if `a[3] - a[2] == 2`, or set to `(a[3] - a[2]) // 2` and `tmp` is a list containing the element `(a[3] - a[2]) // 2`, `y` is updated to `y - ((a[3] - a[2]) // 2 - 1)` if `(a[3] - a[2]) % 2 == 0` and `y > (a[3] - a[2]) // 2 - 1`. If the condition `a[3] - a[2] == 2` is not met, the values of `ans`, `tmp`, and `y` remain unchanged.**