The code `y_max_sq = r_plus_1_squared - x_squared - 1` calculates the value of `y_max_sq`. Given the initial state, we know:
- `r_squared` is \(r \times r\)
- `r_plus_1_squared` is \((r + 1) \times (r + 1)\)
- `x_squared` is \(x * x\)

Substituting these into the equation, we get:
\[ y_max_sq = (r + 1)^2 - x^2 - 1 \]

Expanding \((r + 1)^2\) gives:
\[ (r + 1)^2 = r^2 + 2r + 1 \]

So:
\[ y_max_sq = r^2 + 2r + 1 - x^2 - 1 \]
\[ y_max_sq = r^2 + 2r - x^2 \]

Since `r_squared` is \(r \times r\), we can substitute \(r^2\) with `r_squared`:
\[ y_max_sq = r_squared + 2r - x_squared \]

Therefore, the Output State is:
Output State: **`r` is an integer such that \(1 \leq r \leq 10^5\), `count` is adjusted according to the condition, `r_squared` is \(r \times r\), `r_plus_1_squared` is \((r + 1) \times (r + 1)\), `x_squared` is \(x * x\), `y_min_sq` is \(r_squared - x_squared\), `y_max_sq` is \(r_squared + 2r - x_squared\)**