To determine the postcondition, we need to ensure that the negation of the if condition is included while retaining all the conditions stated in the precondition. Let's break down the if condition and its negation:

The if condition is:
```
if ((a - b == -a, a) or (b - a == -b, b)):
```

This condition seems to be checking two separate conditions:
1. `(a - b == -a, a)`
2. `(b - a == -b, b)`

However, the syntax `(a - b == -a, a)` and `(b - a == -b, b)` suggests a tuple rather than a logical operation. Assuming this is a typo and the intended condition is:
```
if ((a - b == -a) or (b - a == -b)):
```

Let's simplify these conditions:
1. `a - b == -a` simplifies to `2a == b`
2. `b - a == -b` simplifies to `2b == a`

So, the if condition is essentially:
```
if (2a == b) or (2b == a):
```

The negation of this condition would be:
```
not ((2a == b) or (2b == a))
```

Using De Morgan's laws, this becomes:
```
(2a != b) and (2b != a)
```

Now, let's formulate the postcondition including the negation of the if condition and retaining the precondition:

Precondition: `t` is an integer such that \(1 \leq t \leq 10^4\); `a` and `b` are integers read from the input. At least one of `a` or `b` is odd.

Negation of the if condition: `2a != b` and `2b != a`.

Combining these, the postcondition is:

Postcondition: **`t` is an integer such that \(1 \leq t \leq 10^4\); `a` and `b` are integers read from the input. At least one of `a` or `b` is odd. Additionally, `2a` is not equal to `b` and `2b` is not equal to `a`.**