Let's break down the initial state and the code snippet step by step to determine what will be printed when the `print(ans)` statement executes.

### Initial State:
1. **`n`**: At least 1.
2. **`k`**: An input integer (not used in the calculation of `ans`).
3. **`m`**: A positive integer such that \(1 \leq m \leq 2 \times 10^6\) (not used in the calculation of `ans`).
4. **`ans`**: Equal to \( n + \sum_{i=2}^{\text{root}} \left( \frac{n + i}{i^2} \right) \).
5. **`root`**: Equal to the integer part of the square root of `n` plus 1.
6. **`i`**: Equal to `root` + 1.
7. **`cnt`**: Equal to \((\text{root} + 1) \times (\text{root} + 1)\).

### Step-by-Step Calculation:
1. **Calculate `root`**:
   - `root` is the integer part of the square root of `n` plus 1.
   - Mathematically, \( \text{root} = \lfloor \sqrt{n} \rfloor + 1 \).

2. **Calculate the sum \(\sum_{i=2}^{\text{root}} \left( \frac{n + i}{i^2} \right)\)**:
   - This sum is calculated from \(i = 2\) to \(i = \text{root}\).
   - For each \(i\), the term \(\frac{n + i}{i^2}\) is added to the sum.

3. **Calculate `ans`**:
   - `ans` is the sum of `n` and the sum calculated in step 2.
   - Mathematically, \( \text{ans} = n + \sum_{i=2}^{\text{root}} \left( \frac{n + i}{i^2} \right) \).

### Example Calculation:
Let's assume \( n = 10 \) for a concrete example:
1. **Calculate `root`**:
   - \( \sqrt{10} \approx 3.162 \)
   - \( \lfloor 3.162 \rfloor = 3 \)
   - \( \text{root} = 3 + 1 = 4 \)

2. **Calculate the sum \(\sum_{i=2}^{4} \left( \frac{10 + i}{i^2} \right)\)**:
   - For \( i = 2 \): \( \frac{10 + 2}{2^2} = \frac{12}{4} = 3 \)
   - For \( i = 3 \): \( \frac{10 + 3}{3^2} = \frac{13}{9} \approx 1.444 \)
   - For \( i = 4 \): \( \frac{10 + 4}{4^2} = \frac{14}{16} = 0.875 \)
   - Sum: \( 3 + 1.444 + 0.875 \approx 5.319 \)

3. **Calculate `ans`**:
   - \( \text{ans} = 10 + 5.319 = 15.319 \)

### General Output:
Since the exact value of `n` is not provided, we can describe the output in terms of `n` and the formula used to calculate `ans`.

Output: **ans (where ans is \( n + \sum_{i=2}^{\text{root}} \left( \frac{n + i}{i^2} \right) \) and root is the integer part of the square root of n plus 1)**