Postcondition: **`n`, `l`, and `y` remain unchanged. `x` is `y + 2`. If `l[y + 2] > a` and `l[y + 2] > b`, then `a` is set to `l[y + 2]` if `l[y + 2] - a >= l[y + 2] - b`; otherwise, `b` is set to `l[y + 2]`. `c` is incremented by 1. If `l[y + 2] <= a` or `l[y + 2] <= b`, then `a` is set to `l[y + 2]` if `a - l[y + 2] <= b - l[y + 2]` and `l[y + 2] < a` and `l[y + 2] < b`; otherwise, `b` is set to `l[y + 2]`. If `l[y + 2] >= a` or `l[y + 2] >= b`, then `a` is set to `l[y + 2]` if `a >= l[y + 2]`; otherwise, `b` is set to `l[y + 2]`.**