`ans` is updated by adding `(3 - a % 3 + b % 3) % 3` to its current value. Given that `ans` is initially `ans * 3`, let's denote the initial value of `ans` as `3k` where `k` is an integer. 

1. Calculate `a % 3`: Since `a` must be greater than 0, `a % 3` can be 0, 1, or 2.
2. Calculate `b % 3`: Similarly, `b % 3` can be 0, 1, or 2.
3. Compute `(3 - a % 3 + b % 3) % 3`: This expression depends on the values of `a % 3` and `b % 3`.

Let's consider all possible cases:

- If `a % 3 = 0` and `b % 3 = 0`, then `(3 - 0 + 0) % 3 = 3 % 3 = 0`.
- If `a % 3 = 0` and `b % 3 = 1`, then `(3 - 0 + 1) % 3 = 4 % 3 = 1`.
- If `a % 3 = 0` and `b % 3 = 2`, then `(3 - 0 + 2) % 3 = 5 % 3 = 2`.
- If `a % 3 = 1` and `b % 3 = 0`, then `(3 - 1 + 0) % 3 = 2 % 3 = 2`.
- If `a % 3 = 1` and `b % 3 = 1`, then `(3 - 1 + 1) % 3 = 3 % 3 = 0`.
- If `a % 3 = 1` and `b % 3 = 2`, then `(3 - 1 + 2) % 3 = 4 % 3 = 1`.
- If `a % 3 = 2` and `b % 3 = 0`, then `(3 - 2 + 0) % 3 = 1 % 3 = 1`.
- If `a % 3 = 2` and `b % 3 = 1`, then `(3 - 2 + 1) % 3 = 2 % 3 = 2`.
- If `a % 3 = 2` and `b % 3 = 2`, then `(3 - 2 + 2) % 3 = 3 % 3 = 0`.

Given these cases, `ans` is updated by adding either 0, 1, or 2 to `3k`. Therefore, `ans` will be `3k`, `3k+1`, or `3k+2`.

Output State: **`a` must be greater than 0, `b` must be greater than 0, `ans` is `3k`, `3k+1`, or `3k+2`**, where `k` is an integer.