Let's break down the initial state and the operations step by step:

1. **Initial Values:**
   - `t` is a positive integer such that \(1 \leq t \leq 10^4\).
   - `i` is 0.
   - `n` is equal to `t`.
   - `m` is 0.
   - `k` is `t`.
   - `l` is the binary string representation of `k` without the '0b' prefix.
   - `p` is the length of `l`.
   - `q` is \(2^{(\text{length of binary representation of } k - 1)}\).

2. **Calculating `l`:**
   - `l` is the binary string representation of `k` without the '0b' prefix. For example, if `k` is 5, then `l` would be "101".

3. **Calculating `p`:**
   - `p` is the length of `l`. If `l` is "101", then `p` would be 3.

4. **Calculating `q`:**
   - `q` is \(2^{(\text{length of binary representation of } k - 1)}\). This means `q` is \(2^{(p - 1)}\). Using the previous example where `p` is 3, `q` would be \(2^{(3 - 1)} = 2^2 = 4\).

5. **Final Expression:**
   - The expression to be evaluated is `k - q`.

Given the above steps, let's denote `t` as `k` and assume a specific value for `t` to illustrate the calculation. Let's take `t = 5` for simplicity:

- `k = 5`
- `l = "101"` (binary representation of 5)
- `p = 3` (length of "101")
- `q = 4` (since \(2^{(3 - 1)} = 4\))

So, `k - q` would be `5 - 4 = 1`.

Therefore, the output of the print statement will be:

Output: **1**