Alright, I've got this problem to solve. Let's see what it's asking for. So, I have an array of integers, and I can perform exactly k operations on it. In each operation, I select a contiguous subarray (which could even be empty), calculate its sum, and insert that sum anywhere in the array. I need to maximize the sum of the array after k such operations, and since the result can be very large, I have to output it modulo 10^9 + 7.

First, I need to understand what exactly an operation entails. I can choose any contiguous subarray, compute its sum, and insert that sum into the array at any position. The key here is that I'm inserting the sum into the array, which increases the array's length by one each time.

My goal is to maximize the sum of the array after k operations. So, I should aim to insert the largest possible sums into the array in each operation.

Let me think about how to approach this.

Option 1: Always select the entire array and insert its sum.

If I always select the entire array and insert its sum, then in each operation, I'm adding the current sum of the array to itself, effectively doubling the sum each time.

Wait, no. Actually, if I have an array with sum S, and I insert S into it, the new sum becomes S + S = 2S. Then, if I insert 2S into the array, the new sum becomes 2S + 2S = 4S, and so on. So after k operations, the sum would be S * 2^k.

But is this the optimal strategy? Maybe not, because there might be a way to get a larger sum by selecting different subarrays.

Option 2: Select the subarray with the maximum sum and insert it.

Instead of always selecting the entire array, maybe I should select the subarray that has the maximum possible sum and insert that sum into the array.

For example, if I have an array [1, -2, 3], the maximum subarray sum is 3 (the subarray [3]), so I can insert 3 into the array, making it [1, -2, 3, 3]. Then, the sum is 1 -2 +3 +3 = 5.

If I had just selected the entire array each time, the sum would be:

Initial sum: 1 -2 +3 = 2

After first operation: insert 2, array becomes [1, -2, 3, 2], sum=5

After second operation: insert 5, array becomes [1, -2, 3, 2, 5], sum=9

And so on, doubling each time.

Wait, but in the second operation, inserting 5 gives me a larger sum than inserting the maximum subarray sum of 5 again.

Wait, no. In the second operation, the maximum subarray sum is now 5, so inserting 5 would give me the same result as inserting the total sum.

Wait, maybe they are equivalent in some cases.

Let me think more generally.

Suppose I have an array with sum S, and the maximum subarray sum is M.

If I insert S into the array, the new sum is S + S = 2S.

If I insert M into the array, the new sum is S + M.

So, inserting S gives 2S, while inserting M gives S + M.

Which one is larger?

Well, 2S vs S + M. That depends on whether S > M or not.

If S > M, then 2S > S + M.

If S == M, then 2S == S + M.

If S < M, then 2S < S + M.

Wait, but S can be less than M only if there are negative elements in the array.

Wait, actually, no. The maximum subarray sum M is the largest sum of any contiguous subarray, which could be larger than S if some parts of the array are negative.

Wait, for example, array [1, -1, 2], sum S = 2, maximum subarray is [2], M=2, so S + M = 4, 2S = 4, same.

Another example: [1, -2, 3], S=2, M=3, so S + M =5, 2S=4, so S + M > 2S.

So in this case, inserting M is better than inserting S.

Wait, but in the first operation, if I insert M=3, array becomes [1,-2,3,3], sum=5.

Then in the second operation, S=5, M=3 (since [3] is the maximum subarray), so S + M =8, vs 2S=10.

Wait, but inserting S=5 would make the array [1,-2,3,3,5], sum=10, which is better.

So, in this case, inserting S is better than inserting M.

Wait, but in the first operation, inserting M=3 gave me sum=5, and inserting S=2 gave me sum=4, but in the second operation, inserting S=5 gives sum=10, while inserting M=3 gives sum=8.

So, in this case, inserting S is better.

But in the first operation, inserting M was better than inserting S.

Wait, maybe it's not straightforward.

Perhaps, in general, inserting S in each operation leads to sum S * 2^k, while inserting M in each operation leads to sum S + M * (2^k -1).

Wait, let's see.

If I insert S each time:

After operation 1: sum = S + S = 2S

After operation 2: sum = 2S + 2S = 4S

After operation 3: sum = 4S + 4S = 8S

...

After operation k: sum = S * 2^k

If I insert M each time:

After operation 1: sum = S + M

After operation 2: sum = S + M + M = S + 2M

After operation 3: sum = S + 2M + M = S + 3M

...

After operation k: sum = S + kM

So, inserting S leads to S * 2^k, while inserting M leads to S + kM.

Comparing S * 2^k vs S + kM.

Well, for large k, S * 2^k grows much faster, but for small k, it depends.

But in the problem, k can be up to 2*10^5, which is large, so S * 2^k would dominate.

But, there might be cases where S is negative or zero, or M is very large.

Wait, S can be negative if the array has negative numbers.

Wait, but in that case, inserting S would make the sum worse, since S is negative.

So, perhaps, the optimal strategy is:

- If S >= 0, then insert S in each operation, getting S * 2^k.

- If S < 0, then insert M in each operation, getting S + kM.

But, wait, in the example above, where a=[1,-2,3], S=2, M=3, inserting S leads to S*2^k, which is 2*(2^k), and inserting M leads to S + k*M = 2 + 3k.

For k=1: 2*2 =4 vs 2+3=5, so inserting M is better.

For k=2: 2*4=8 vs 2+6=8, same.

For k=3: 2*8=16 vs 2+9=11, inserting S is better.

So, for k=1, inserting M is better, for k=2, both same, for k>=3, inserting S is better.

So, it's not straightforward to choose one strategy over the other for all k.

Perhaps, the optimal strategy is to insert S if S >= M, else insert M.

Wait, but in the above example, S=2, M=3, S < M, so insert M until S >= M.

But in that case, after inserting M once, S becomes 5, which is greater than M=3, so then insert S in the remaining operations.

So, for k=1: insert M=3, sum=5

k=2: insert S=5, sum=10

k=3: insert S=10, sum=20

and so on.

So, in this case, for k>=2, it's better to insert S after the first operation.

Wait, but in the earlier calculation, for k=2, inserting S twice gives sum=8, inserting M twice gives sum=8, same.

Wait, no, for k=2:

- Insert S twice: sum=4 (first insertion), then 8 (second insertion)

- Insert M twice: sum=5 (first insertion), then 8 (second insertion)

Wait, no, in my earlier calculation, for k=2:

- Insert S twice: sum=4 (first insertion), then 8 (second insertion)

- Insert M twice: sum=5 (first insertion), then 8 (second insertion)

So, same as above.

But in reality, for k=2, inserting M first and then S gives sum=10, which is better.

Wait, let's clarify:

Start with a=[1,-2,3], S=2, M=3.

Operation 1: insert M=3, array becomes [1,-2,3,3], S=5.

Operation 2: insert S=5, array becomes [1,-2,3,3,5], S=10.

Alternatively, operation 1: insert S=2, array becomes [1,-2,3,2], S=4.

Operation 2: insert S=4, array becomes [1,-2,3,2,4], S=8.

So, inserting M in the first operation and then S gives a better sum than inserting S in both operations.

Wait, but in this case, inserting M only in the first operation and then S gives a better sum.

So, perhaps the optimal strategy is to insert M once, and then insert S in the remaining k-1 operations.

Then, the total sum would be S + M * 2^{k-1}.

Wait, no.

Wait, let's see:

After inserting M once, S becomes S + M.

Then, in the next k-1 operations, inserting S each time would multiply S by 2^{k-1}.

Wait, no.

Wait, after inserting M once, S becomes S + M.

Then, inserting S in the next operation makes S = (S + M) * 2.

Wait, no, inserting S adds S to the array, so S_new = S + S = 2S.

Wait, no, wait: if I have S, and I insert S, then the new S is S + S = 2S.

Wait, but in the earlier example, starting with S=2, insert M=3, S becomes 5.

Then, insert S=5, S becomes 10.

Then, insert S=10, S becomes 20, and so on.

So, after inserting M once, then inserting S in the remaining k-1 operations, the sum becomes S + M * 2^{k-1}.

Wait, no, in the example:

k=1: insert M, S=5

k=2: insert S, S=10

k=3: insert S, S=20

Which is S + M * 2^{k-1} = 2 + 3 * 2^{2} = 2 + 12 =14, which doesn't match the actual sum of 20.

Wait, perhaps it's S + M * (2^{k-1} -1).

Wait, S + M * (2^{k-1} -1) = 2 + 3*(4-1)=2 + 9=11, which is still not 20.

Hmm, perhaps my formula is wrong.

Wait, perhaps it's better to think recursively.

Let me denote sum after k operations as f(k).

Then, f(0) = S.

If I insert M in operation 1, then f(1) = S + M.

Then, if I insert S in operation 2, f(2) = f(1) + f(1) = 2*f(1) = 2*(S + M).

Similarly, f(3) = 2*f(2) = 4*(S + M).

So, in general, if I insert M once and then insert S in the remaining k-1 operations, f(k) = (S + M) * 2^{k-1}.

In the example, k=3: f(3)= (2 + 3)*2^{2}=5*4=20, which matches the earlier calculation.

Wait, but for k=2: f(2)=(2+3)*2=10, which also matches.

For k=1: f(1)=5, which matches.

So, the formula seems correct: f(k) = (S + M) * 2^{k-1}.

But, is this better than inserting S in all operations, which gives f(k)=S * 2^k.

Comparing (S + M)*2^{k-1} vs S*2^k.

Simplify: (S + M)*2^{k-1} vs S*2^k.

Multiply both sides by 2: (S + M)*2^k vs 2*S*2^k.

Wait, that doesn't help.

Wait, no, let's compute the ratio:

(S + M)*2^{k-1} / (S * 2^k) = (S + M)/(2S)

So, when (S + M)/(2S) >1, then (S + M)*2^{k-1} > S*2^k.

That is, when S + M > 2S, i.e., M > S.

So, if M > S, then inserting M once and then inserting S in the remaining operations gives a better sum than inserting S in all operations.

Similarly, if M <= S, then inserting S in all operations is better.

So, in the example, M=3 > S=2, so inserting M once and then S gives a better sum for k>=1.

Wait, but for k=1, inserting M gives sum=5, and inserting S gives sum=4, which matches.

For k=2, inserting M then S gives sum=10, while inserting S twice gives sum=8, which is better.

Wait, but according to the formula, (S + M)*2^{k-1} = (2 + 3)*2^{1}=10, while S*2^k=2*4=8, which matches.

So, in this case, inserting M once and then S is better.

But, for k=1, inserting M is better.

For k=2, inserting M then S is better.

For k=3, (S + M)*2^{k-1} =5*4=20, while S*2^k=2*8=16, still better.

Wait, but in the earlier calculation, for k=3, inserting M once and then S in the remaining operations gives sum=20, while inserting S in all operations gives sum=16.

So, indeed, inserting M once and then S is better.

But is there a better strategy?

Wait, maybe inserting M multiple times.

For example, insert M twice:

k=1: insert M, sum=5

k=2: insert M=3, sum=8

Which is less than inserting M once and then S=5, which gives sum=10.

So, inserting M twice is worse than inserting M once and then S.

Similarly, inserting M three times: sum=11, which is less than inserting M once and then S twice: 20.

So, inserting M once and then S in the remaining operations is better than inserting M multiple times.

What if I insert M more than once?

For example, insert M once, then S once, then M once.

Wait, but in general, it seems that inserting M only once at the beginning and then S in the remaining operations gives the best sum.

Is there a scenario where inserting M more than once is better?

Probably not, based on the above observation.

So, in general, the strategy is:

- If M > S, insert M once, then insert S in the remaining k-1 operations.

- Else, insert S in all k operations.

Wait, but in the first operation, inserting M gives sum=S + M, then inserting S in the remaining operations gives sum=(S + M) * 2^{k-1}.

While inserting S in all operations gives sum=S * 2^k.

So, if M > S, then (S + M)*2^{k-1} > S*2^k.

As we saw earlier.

So, the condition is: if M > S, use the first strategy, else use the second.

Wait, but in the formula, (S + M)*2^{k-1} vs S*2^k.

Let's see for M > S:

(S + M)*2^{k-1} > S*2^k

Because S + M > 2S implies M > S.

So, yes, if M > S, then inserting M once and then S in the remaining operations is better.

Similarly, if M <= S, then inserting S in all operations is better.

So, in code, I can check if M > S, then compute (S + M)*2^{k-1}, else compute S*2^k.

Wait, but in the earlier example, M=3 > S=2, so use (S + M)*2^{k-1}=5*2^{k-1}.

For k=1: 5*1=5

For k=2:5*2=10

For k=3:5*4=20

Which matches the manual calculation.

While inserting S in all operations:2*2^k.

For k=1:4

For k=2:8

For k=3:16

So, indeed, better to insert M once and then S.

But, is there a case where inserting M more than once is better?

Let's try another example.

Take a=[-1, -2], S=-3, M=-1.

Here, M > S (-1 > -3), so according to the strategy, insert M once and then S in remaining operations.

So, k=1: insert M, sum=S + M=-3 + (-1)=-4

Then, insert S: sum=-4 + (-4)=-8

While inserting S in all operations: k=1: insert S, sum=S + S=-6

k=2: insert S, sum=-6 + (-6)=-12

So, in this case, inserting M once and then S gives -8, which is better than inserting S twice giving -12.

But both are negative sums, so in this case, inserting M once and then S is better than inserting S in all operations.

But, in this case, M > S (-1 > -3), so the strategy holds.

Another example: a=[0,0,0], S=0, M=0.

Inserting M once and then S: sum remains 0.

Inserting S in all operations: sum remains 0.

Same result.

Another example: a=[1,2,3], S=6, M=6.

Here, M == S, so inserting M once and then S gives (6 + 6)*2^{k-1}=12*2^{k-1}

Inserting S in all operations gives 6*2^k=6*2^k=12*2^{k-1}

So, both strategies give the same result when M == S.

Hence, the general strategy is:

- If M > S, then use (S + M)*2^{k-1}

- Else, use S*2^k

Now, I need to implement this in code.

But, there is a catch.

The problem mentions that the sum can be very large, so I need to compute the answer modulo 10^9 + 7.

Also, the array can have negative numbers, so M can be negative if all elements are negative.

I need to handle that.

Also, k can be up to 2*10^5, and t (number of test cases) can be up to 10^4, with the sum of n and k across all test cases being up to 2*10^5.

So, I need an efficient solution.

First, for each test case, I need to compute S and M.

S is just the sum of the array.

M is the maximum subarray sum.

I need to compute M efficiently.

I recall that the maximum subarray sum can be computed in O(n) time using Kadane's algorithm.

So, for each test case, I can compute S and M.

Then, depending on whether M > S, I choose the formula accordingly.

Wait, but in the code provided, there's a function func_2(arr) which seems to compute M.

Let me look at the code.

Given code:

from math import *

t = int(input())

for _ in range(t):

(n, k) = map(int, input().split())

a = list(map(int, input().split()))

max_segment = func_2(a)

if max_segment[0] == -1:

max_segment[0] = 0

answer = max_segment[0] * 2 ** k + sum(a) - max_segment[0]

print(func_1(answer))

def func_1(number):

return number % 1000000007

def func_2(arr):

new_segment = []

max_segment = [0, 0]

segments_variants = []

max_sum = -1

for i in range(len(arr)):

if new_segment:

if arr[i] < 0:

if max_segment[0] > new_segment[0]:

segments_variants.append(max_segment + [i - 1])

else:

segments_variants.append(new_segment + [i - 1])

max_segment = new_segment

new_segment = []

max_segment[0] += arr[i]

else:

max_segment[0] += arr[i]

new_segment[0] += arr[i]

else:

if arr[i] >= 0:

new_segment = [arr[i], i]

max_segment[0] += arr[i]

segments_variants.append(max_segment + [len(arr) - 1])

segments_variants.append(new_segment + [len(arr) - 1])

total_max_segment = [-1]

for segment in segments_variants:

if total_max_segment[0] < segment[0]:

total_max_segment = segment

if len(total_max_segment) == 1:

total_max_segment = [-1]

return total_max_segment

def func_3(number, quantity):

answer = 0

In the code, func_2(arr) seems to be attempting to find the maximum subarray sum.

But it looks overly complicated, and I'm not entirely sure what it's doing.

I think it's better to implement Kadane's algorithm for finding M.

But for now, let's assume that func_2(arr) correctly returns the maximum subarray sum.

Then, in the main code:

max_segment = func_2(a)

if max_segment[0] == -1:

max_segment[0] = 0

answer = max_segment[0] * 2 ** k + sum(a) - max_segment[0]

print(func_1(answer))

Wait, according to my earlier reasoning, if M > S, then use (S + M)*2^{k-1}, else use S*2^k.

But in the code, it's computing answer = M * 2^k + S - M.

Wait, let's see:

If M > S, according to my strategy, use (S + M)*2^{k-1}.

Else, use S*2^k.

But in the code, it's computing M*2^k + S - M.

Let me see if these are equivalent.

Let's compare:

My formula:

If M > S: (S + M)*2^{k-1}

Else: S*2^k

Code's formula:

M*2^