Let's analyze the given code snippet step by step:

1. **Initial State**: 
   - `A[i][m - 1] = 1`
   - `A[i + 1][m - 1] = 1`
   - `A[i][m] = undefined`
   - `A[i + 1][m] = undefined`
   - If the condition `A[i][j] == 1 and A[i + 1][j] == 1 and (A[i][j + 1] == 1) and (A[i + 1][j + 1] == 1)` is true, `ops` contains the element \((i + 1, m)\). If the condition is false, the values of `A[i][m]` and `A[i + 1][m]` remain undefined and `ops` does not change.

2. **Code Snippet**:
   ```python
   ops.append((i + 1, j + 1))
   ```

3. **Impact of the Code**:
   - The line `ops.append((i + 1, j + 1))` appends the tuple `(i + 1, j + 1)` to the list `ops`.
   - This means `ops` now includes this new element.
   - However, since the condition in the initial state was not specified to be checked again, we assume that the condition is true based on the provided initial state and that `ops` already contains \((i + 1, m)\).

4. **Output State**:
   - The values of `A[i][m - 1]`, `A[i + 1][m - 1]`, `A[i][m]`, and `A[i + 1][m]` remain as they are.
   - The list `ops` now contains both \((i + 1, m)\) and \((i + 1, j + 1)\).

Therefore, the updated state of the variables and list is:

Output State: **`A[i][m - 1] = 1`, `A[i + 1][m - 1] = 1`, `A[i][m] = undefined`, `A[i + 1][m] = undefined`, `ops` contains \((i + 1, m)\) and \((i + 1, j + 1)\)**.