Given the initial state and the code snippet, we need to determine the new state of the variables after the code execution.

Initial State:
- `t` is `t + 1`
- `k` is an input integer
- `x` is an input integer and must be greater than or equal to 0
- `a` is an input integer
- `z` is `2 + 1 // (k - 1)`
- `i` is `i + 1`

Code:
```python
z += z // (k - 1) + 1
```

The code modifies the value of `z` by adding `z // (k - 1) + 1` to its current value.

Let's break down the calculation:

1. The initial value of `z` is `2 + 1 // (k - 1)`.
2. The expression `z // (k - 1) + 1` is added to `z`.

Let's denote the initial value of `z` as `z_initial = 2 + 1 // (k - 1)`.

The new value of `z` after the code execution will be:
\[ z_{\text{new}} = z_{\text{initial}} + \left(\frac{z_{\text{initial}}}{k - 1}\right) + 1 \]

Given that `z_initial = 2 + 1 // (k - 1)`, we substitute this into the equation:
\[ z_{\text{new}} = \left(2 + \frac{1}{k - 1}\right) + \left(\frac{2 + \frac{1}{k - 1}}{k - 1}\right) + 1 \]

Simplifying further:
\[ z_{\text{new}} = 2 + \frac{1}{k - 1} + \frac{2}{k - 1} + \frac{1}{(k - 1)^2} + 1 \]
\[ z_{\text{new}} = 3 + \frac{3}{k - 1} + \frac{1}{(k - 1)^2} \]

Since `1 // (k - 1)` will be `0` for `k >= 2` and `1` for `k = 1`, we need to consider both cases:

- If `k = 1`, then `z_initial = 2 + 1 // 0` which is undefined. However, typically, we assume `k != 1` in such contexts to avoid division by zero.
- For `k >= 2`, `z_initial = 2 + 0 = 2`.

Thus, for `k >= 2`:
\[ z_{\text{new}} = 3 + \frac{3}{k - 1} + \frac{1}{(k - 1)^2} \]

The other variables `t`, `k`, `x`, `a`, and `i` remain unchanged.

Output State: **`t` is `t + 1`, `k` is an input integer, `x` is an input integer and must be greater than or equal to 0, `a` is an input integer, `z` is `3 + 3 // (k - 1) + 1 // (k - 1)^2`, `i` is `i + 1`**

Note: The expression `3 + 3 // (k - 1) + 1 // (k - 1)^2` is the new value of `z` for `k >= 2`. For `k = 1`, the initial state would be undefined due to division by zero, so we assume `k >= 2` for practical purposes.