Let's break down the initial state and the code snippet to determine what will be printed:

### Initial State:
- `n` and `m` are integers such that `min(n, m) >= 1`.
- `b` is `min(n, m) + 1`.
- `t` is a positive integer greater than 1.
- `T` is 2.
- `ans` is calculated as `sum(n // i + 1 for i in range(1, min(n, m) + 1))`.

### Code Snippet:
```python
print(ans)
```

### Step-by-Step Analysis:
1. **Determine `min(n, m)`**:
   - Since `min(n, m) >= 1`, let's denote `k = min(n, m)`. Therefore, `k` is a positive integer.

2. **Calculate `b`**:
   - `b = k + 1`.

3. **Calculate `ans`**:
   - `ans` is the sum of `n // i + 1` for each `i` in the range from 1 to `k + 1`.
   - This means we need to evaluate the expression `n // i + 1` for each `i` from 1 to `k`.

4. **Expression Breakdown**:
   - For each `i` in the range from 1 to `k`, `n // i` gives the integer division of `n` by `i`.
   - Adding 1 to each result gives us `n // i + 1`.

5. **Summing Up**:
   - The final value of `ans` is the sum of all these values.

### Example Calculation:
Let's assume `n = 5` and `m = 3` for concreteness:
- `k = min(5, 3) = 3`.
- `b = 3 + 1 = 4`.
- `ans = sum(5 // i + 1 for i in range(1, 4))`.

Calculating each term:
- For `i = 1`: `5 // 1 + 1 = 5 + 1 = 6`.
- For `i = 2`: `5 // 2 + 1 = 2 + 1 = 3`.
- For `i = 3`: `5 // 3 + 1 = 1 + 1 = 2`.

Summing these up:
- `ans = 6 + 3 + 2 = 11`.

### General Case:
For any `n` and `m` where `min(n, m) = k`:
- `ans = sum(n // i + 1 for i in range(1, k + 1))`.

### Final Output:
The `print(ans)` statement will print the sum of `n // i + 1` for each `i` from 1 to `min(n, m)`.

Output: **ans (where ans is the sum of n // i + 1 for each i from 1 to min(n, m))**