To determine the output state, we need to evaluate the expression `ans <= n * max(a, b)` given the initial state.

Given:
- `k` is an integer such that 0 <= k <= min(n, b).
- `a` and `b` are integers such that 1 <= a, b <= 10^9.
- `n` is an integer such that 1 <= n <= 10^9.
- `ans` is calculated as `k * b + (n - k) * a`.

We need to determine if `ans <= n * max(a, b)`.

First, let's express `ans`:
- `ans = k * b + (n - k) * a`

Now, let's compare `ans` with `n * max(a, b)`:
- `n * max(a, b)` will be either `n * a` if `a >= b` or `n * b` if `b >= a`.

Let's consider two cases:
1. **Case 1:** `a >= b`
   - `n * max(a, b) = n * a`
   - We need to check if `k * b + (n - k) * a <= n * a`
   - Simplifying, `k * b + (n - k) * a <= n * a` becomes `k * b <= k * a` since `(n - k) * a` cancels out on both sides.
   - Since `b <= a` (because `a >= b`), `k * b <= k * a` is always true for any `k` in the range 0 <= k <= min(n, b).

2. **Case 2:** `b >= a`
   - `n * max(a, b) = n * b`
   - We need to check if `k * b + (n - k) * a <= n * b`
   - Simplifying, `k * b + (n - k) * a <= n * b` becomes `(n - k) * a <= (n - k) * b` since `k * b` cancels out on both sides.
   - Since `a <= b` (because `b >= a`), `(n - k) * a <= (n - k) * b` is always true for any `k` in the range 0 <= k <= min(n, b).

In both cases, the inequality `ans <= n * max(a, b)` holds true.

Output State: **The program returns True**