The code snippet `ans[i + 1] += ans[i]` updates the value of `ans[1]` by adding `ans[0]` to it. Given the initial state, `i` is 0, `ans[0]` is `arr[0] + 1`, and `ans[1]` is `arr[0] + (arr[0] + 1)`. After the code executes, `ans[1]` will be `arr[0] + (arr[0] + 1) + (arr[0] + 1)`, which simplifies to `3 * arr[0] + 2`. The other parts of the initial state remain unchanged.

Output State: **`arr` is a list of integers such that \(1 \leq \text{arr}[i] \leq 500\) for all \(1 \leq i < n\), `n` is an integer such that \(3 \leq n \leq 500\), `ans` is a list of `n` integers where `ans[0]` is `arr[0] + 1` and `ans[1]` is `3 * arr[0] + 2`, the rest of the elements in `ans` are zeros, `i` is 0, and `ans[1]` is less than `arr[1]`**.