Alright, I've got this problem to solve. Let's see what it's asking for. So, I'm given two positive integers, n and m, and I need to find the number of ordered pairs (a, b) where 1 ≤ a ≤ n and 1 ≤ b ≤ m, with the condition that a + b is a multiple of b multiplied by the greatest common divisor (GCD) of a and b. That condition sounds a bit tricky, so I need to break it down.

First, let's understand the condition: a + b should be a multiple of b * GCD(a, b). In mathematical terms, that means there exists some integer k such that a + b = k * b * GCD(a, b).

I need to find all pairs (a, b) that satisfy this equation within the given constraints.

Given the constraints, n and m can be up to 2 million, and there can be up to 10,000 test cases, with the sum of n and m across all test cases not exceeding 2 million. That means I need an efficient solution, probably O(n log n) or better, to handle the large input sizes.

Let's think about how to approach this.

First, I know that GCD(a, b) is a divisor of both a and b. But in this problem, the GCD is taken between a and b, and b is multiplied by this GCD in the denominator.

Wait, actually, the condition is a + b is a multiple of b * GCD(a, b). So, a + b ≡ 0 mod (b * GCD(a, b)).

Let's denote d = GCD(a, b). Then, a = d * a', and b = d * b', where GCD(a', b') = 1.

Substituting into the condition:

d * a' + d * b' ≡ 0 mod (d * b' * d)

Wait, that seems off. Let's recast this.

Given d = GCD(a, b), then a = d * a', b = d * b', with GCD(a', b') = 1.

Then, a + b = d * a' + d * b' = d * (a' + b').

The condition is that d * (a' + b') is a multiple of b * d = d * (d * b') = d^2 * b'.

Wait, that doesn't seem right. Let's double-check.

Wait, b = d * b', so b * d = d * (d * b') = d^2 * b'.

So, the condition is d * (a' + b') is a multiple of d^2 * b'.

Simplify by dividing both sides by d (since d ≠ 0):

a' + b' is a multiple of d * b'.

But GCD(a', b') = 1, so a' and b' are coprime.

This seems like a key point.

Let me think differently. Maybe I can express the condition in terms of a' and b'.

Given that a = d * a' and b = d * b', with GCD(a', b') = 1.

Then, a + b = d * (a' + b').

The condition is that a + b is a multiple of b * d = d^2 * b'.

So, d * (a' + b') is a multiple of d^2 * b'.

Dividing both sides by d (since d ≠ 0), we get:

a' + b' is a multiple of d * b'.

Since a' and b' are coprime, and b' divides a' + b', then b' divides a'.

But GCD(a', b') = 1, so b' = 1.

Wait, does that make sense? If b' divides a', and GCD(a', b') = 1, then b' must be 1.

So, b' = 1.

Then, b = d * b' = d * 1 = d.

So, b = d.

Also, since b' = 1, then a' and 1 are coprime, which is always true.

So, a' can be any integer greater than or equal to 1.

Wait, but a' = a / d, and a = d * a', so a can be any multiple of d.

Given that b = d, and a is a multiple of d, let's see what this implies for the condition.

So, a is a multiple of b, since a is a multiple of d and b = d.

Wait, b = d, and a is a multiple of d, so a is a multiple of b.

Let me see if that's always the case.

Wait, but in general, a can be any multiple of d, and b = d.

So, a is a multiple of b.

But is that always true? Or is there more to it?

Wait, perhaps I need to consider the condition more carefully.

Let me try plugging in some small values to see if I can find a pattern.

Take the first example in the problem:

n = 1, m = 1.

Possible pair: (1,1).

Check if 1 + 1 is a multiple of 1 * GCD(1,1) = 1 * 1 = 1.

Yes, 2 is a multiple of 1.

So, only one valid pair, which matches the sample output.

Second sample:

n = 2, m = 3.

Possible pairs: (1,1), (1,2), (1,3), (2,1), (2,2), (2,3).

Let's check each:

(1,1): 1+1=2 is a multiple of 1*1=1. Yes.

(1,2): 1+2=3 is a multiple of 2*1=2. 3 is not a multiple of 2. No.

(1,3): 1+3=4 is a multiple of 3*1=3. 4 is not a multiple of 3. No.

(2,1): 2+1=3 is a multiple of 1*GCD(2,1)=1*1=1. Yes.

(2,2): 2+2=4 is a multiple of 2*GCD(2,2)=2*2=4. Yes.

(2,3): 2+3=5 is a multiple of 3*GCD(2,3)=3*1=3. 5 is not a multiple of 3. No.

So, valid pairs are (1,1), (2,1), (2,2). Total 3, which matches the sample output.

Third sample:

n=3, m=5.

Possible pairs: (1,1), (1,2), (1,3), (1,4), (1,5), (2,1), (2,2), (2,3), (2,4), (2,5), (3,1), (3,2), (3,3), (3,4), (3,5).

From the second sample, we know (1,1) is valid, (2,1), (2,2) are valid.

Check additional pairs:

(3,1): 3+1=4 is a multiple of 1*GCD(3,1)=1*1=1. Yes.

(3,2): 3+2=5 is a multiple of 2*GCD(3,2)=2*1=2. 5 is not a multiple of 2. No.

(3,3): 3+3=6 is a multiple of 3*GCD(3,3)=3*3=9. 6 is not a multiple of 9. No.

(3,4): 3+4=7 is a multiple of 4*GCD(3,4)=4*1=4. 7 is not a multiple of 4. No.

(3,5): 3+5=8 is a multiple of 5*GCD(3,5)=5*1=5. 8 is not a multiple of 5. No.

So, valid pairs are (1,1), (2,1), (2,2), (3,1). Total 4, matching the sample output.

From these examples, it seems that pairs where b divides a are often valid, but there might be more to it.

Wait, in the first sample, (1,1) is valid.

In the second sample, (2,1), (2,2) are valid.

In the third sample, (3,1) is valid.

It seems like when b divides a, the condition holds.

Wait, but in the second sample, (2,1) and (2,2) are valid, and in the third sample, (3,1) is valid.

Wait, (2,1): a=2, b=1, 2 is a multiple of 1.

(2,2): a=2, b=2, 2 is a multiple of 2.

(3,1): a=3, b=1, 3 is a multiple of 1.

So, in these cases, a is a multiple of b.

Is this a general pattern?

Let me check another example.

Take n=10, m=8.

From the sample, there are 14 valid pairs.

If I consider all pairs where a is a multiple of b, how many are there?

For b=1, a can be 1 to 10, all are multiples of 1.

For b=2, a can be 2,4,6,8,10.

For b=3, a can be 3,6,9.

For b=4, a can be 4,8.

For b=5, a can be 5,10.

For b=6, a can be 6.

For b=7, a can be 7.

For b=8, a can be 8.

Total: for b=1:10, b=2:5, b=3:3, b=4:2, b=5:2, b=6:1, b=7:1, b=8:1.

Sum: 10+5+3+2+2+1+1+1=25.

But according to the sample, there are only 14 valid pairs.

So, my assumption that a is a multiple of b is too broad; there are more constraints.

Wait, perhaps not all multiples are valid.

Looking back at the condition: a + b is a multiple of b * GCD(a,b).

In the case where a is a multiple of b, let's see.

If a is a multiple of b, then a = k * b for some integer k ≥ 1.

Then, GCD(a, b) = GCD(k * b, b) = b.

So, b * GCD(a, b) = b * b = b².

Then, a + b = k * b + b = b * (k + 1).

So, the condition is that b * (k + 1) is a multiple of b².

Simplify by dividing both sides by b (assuming b ≠ 0):

k + 1 is a multiple of b.

So, k + 1 ≡ 0 mod b.

Which means k ≡ -1 mod b.

So, k = m * b - 1 for some integer m ≥ 1.

Therefore, a = k * b = (m * b - 1) * b = m * b² - b.

So, a = m * b² - b.

Given that a must be ≥1 and ≤n.

Wait, this seems like a way to express a in terms of b and m.

But it's getting complicated.

Maybe there's a better way to approach this.

Let me consider fixing b and finding the possible a's that satisfy the condition for each b.

So, for each b from 1 to m, find the number of a in 1 to n such that a + b is a multiple of b * GCD(a, b).

Given that GCD(a, b) divides a and b, let's denote d = GCD(a, b).

Then, a = d * a', b = d * b', with GCD(a', b') = 1.

Then, a + b = d * a' + d * b' = d * (a' + b').

The condition is that d * (a' + b') is a multiple of b * d = d * (d * b') = d² * b'.

Simplify by dividing both sides by d (assuming d ≠ 0):

a' + b' is a multiple of d * b'.

But a' and b' are coprime.

So, b' divides a' + b'.

Since b' divides a' + b' and GCD(a', b') = 1, then b' divides a'.

But since GCD(a', b') = 1, the only way b' divides a' is if b' = 1.

Therefore, b' = 1.

So, b = d * 1 = d.

And a = d * a', where a' is any positive integer.

So, a is any multiple of d.

But since b = d, a is any multiple of b.

Wait, but earlier when I considered a is a multiple of b, it didn't match the sample output.

Maybe I need to consider the condition more carefully.

Let me see.

From above, we have that b' = 1, so b = d.

And a = d * a', where a' is any positive integer.

But a must be ≤ n.

So, for each b, which is equal to d, a can be any multiple of b up to n.

Wait, but in the sample input where n=2, m=3, the valid pairs are (1,1), (2,1), (2,2).

But according to this, for b=1, a can be 1,2 (multiples of 1 up to 2), for b=2, a can be 2 (multiple of 2 up to 2), and for b=3, a can be 3 (but 3 > 2, so none).

Total valid pairs: (1,1), (2,1), (2,2), which matches the sample output of 3.

Wait, but earlier when n=10, m=8, according to this, for b=1, a=1 to 10; b=2, a=2,4,6,8,10; b=3, a=3,6,9; b=4, a=4,8; b=5, a=5,10; b=6, a=6; b=7, a=7; b=8, a=8.

Total: 10 + 5 + 3 + 2 + 2 + 1 + 1 + 1 = 25, but the sample output is 14.

So, there must be some overcounting or misinterpretation.

Wait, perhaps not all pairs where a is a multiple of b satisfy the original condition.

Maybe there are additional constraints.

Let me check the condition again.

Given a + b is a multiple of b * GCD(a,b).

From above, if a is a multiple of b, then GCD(a,b) = b, and the condition becomes a + b is a multiple of b * b = b².

Given that a is a multiple of b, a = k * b, so a + b = k * b + b = b * (k + 1).

So, b * (k + 1) must be a multiple of b², which implies that k + 1 is a multiple of b.

So, k + 1 ≡ 0 mod b, meaning k ≡ -1 mod b.

Thus, k = m * b - 1 for some integer m ≥ 1.

Therefore, a = k * b = (m * b - 1) * b = m * b² - b.

So, a must be of the form m * b² - b, for some m ≥ 1, and 1 ≤ a ≤ n.

Wait, but in the second sample, n=2, m=3.

For b=1:

a = m * 1² - 1 = m - 1.

a must be ≥1 and ≤2.

So, m - 1 ≥1 ⇒ m ≥2.

m -1 ≤2 ⇒ m ≤3.

So, m can be 2,3.

Thus, a=1,2.

So, pairs (1,1),(2,1).

For b=2:

a = m * 4 - 2.

a must be ≥1 and ≤2.

So, m=1: a=4-2=2 (valid).

m=2: a=8-2=6 (>2, invalid).

So, only a=2.

Pair (2,2).

For b=3:

a = m * 9 - 3.

a must be ≥1 and ≤2.

m=1: 9-3=6 (>2, invalid).

So, no valid a.

Total valid pairs: (1,1),(2,1),(2,2), which matches the sample output of 3.

Similarly, for n=10, m=8.

Let's compute the number of valid a for each b.

For b=1:

a = m * 1 -1 = m -1.

1 ≤ m-1 ≤10 ⇒ m=2 to m=11.

So, a=1 to 10, total 10 pairs.

For b=2:

a = m *4 -2.

1 ≤ 4m -2 ≤10.

Solve 4m -2 ≥1 ⇒ m ≥ 0.75 ⇒ m ≥1.

4m -2 ≤10 ⇒ 4m ≤12 ⇒ m ≤3.

So, m=1,2,3.

a=2,6,10. So, pairs (2,2),(6,2),(10,2).

But wait, in the earlier count, for b=2, a can be 2,4,6,8,10, but according to this, only a=2,6,10 are valid.

So, (4,2) and (8,2) are invalid.

Wait, let's check (4,2):

a=4, b=2.

a+b=6.

b * GCD(4,2)=2*2=4.

Is 6 a multiple of 4? No.

So, (4,2) is invalid.

Similarly, (8,2): a+b=10, which is not a multiple of 4.

Only (2,2), (6,2), (10,2) are valid.

For b=3:

a = m*9 -3.

1 ≤9m -3 ≤10.

9m -3 ≥1 ⇒ m ≥ 4/9 ⇒ m ≥1.

9m -3 ≤10 ⇒ 9m ≤13 ⇒ m ≤1.44 ⇒ m=1.

a=6.

But 6 > n=10? Wait, n=10, so a=6 is valid.

Wait, but earlier I thought a=6 is valid.

Wait, but in the initial count, for b=3, a can be 3,6,9.

But according to this formula, only a=6 is valid.

Wait, let's check a=3, b=3.

a+b=6.

b * GCD(3,3)=3*3=9.

Is 6 a multiple of 9? No.

So, (3,3) is invalid.

a=6, b=3.

a+b=9.

b * GCD(6,3)=3*3=9.

9 is a multiple of 9. So, (6,3) is valid.

a=9, b=3.

a+b=12.

b * GCD(9,3)=3*3=9.

12 is not a multiple of 9. So, (9,3) is invalid.

Thus, only (6,3) is valid.

Similarly, for b=4:

a = m*16 -4.

1 ≤16m -4 ≤10.

16m -4 ≥1 ⇒ m ≥ 5/16 ⇒ m ≥1.

16m -4 ≤10 ⇒16m ≤14 ⇒ m ≤0.875.

So, no integer m satisfies this.

Thus, no valid a for b=4.

For b=5:

a = m*25 -5.

1 ≤25m -5 ≤10.

25m -5 ≥1 ⇒ m ≥ 6/25 ⇒ m ≥1.

25m -5 ≤10 ⇒25m ≤15 ⇒ m ≤0.6.

No integer m satisfies this.

So, no valid a for b=5.

For b=6:

a = m*36 -6.

1 ≤36m -6 ≤10.

36m -6 ≥1 ⇒ m ≥7/36 ⇒ m ≥1.

36m -6 ≤10 ⇒36m ≤16 ⇒ m ≤0.444.

No integer m satisfies this.

So, no valid a for b=6.

For b=7:

a = m*49 -7.

1 ≤49m -7 ≤10.

49m -7 ≥1 ⇒ m ≥8/49 ⇒ m ≥1.

49m -7 ≤10 ⇒49m ≤17 ⇒ m ≤0.347.

No integer m satisfies this.

So, no valid a for b=7.

For b=8:

a = m*64 -8.

1 ≤64m -8 ≤10.

64m -8 ≥1 ⇒ m ≥9/64 ⇒ m ≥1.

64m -8 ≤10 ⇒64m ≤18 ⇒ m ≤0.281.

No integer m satisfies this.

So, no valid a for b=8.

Total valid pairs:

From b=1: a=1,2,3,4,5,6,7,8,9,10.

Wait, but according to the formula, only a= m-1 for m=2 to m=11, which is a=1 to 10.

But earlier, for b=1, a can be any multiple of b, which is any a, but according to the condition, it's only a=m-1.

Wait, no, for b=1, GCD(a,1)=1, so the condition is a+1 is a multiple of 1*1=1, which is always true.

Wait, but earlier in the general case, we derived that a must be of the form m*b² - b.

For b=1, a = m*1 -1 = m-1.

So, a can be any integer ≥1, since m can be from 2 to n+1.

Wait, but in this specific case, since b=1, GCD(a,1)=1, so a+1 must be a multiple of 1*1=1, which is always true.

So, all a from 1 to n are valid when b=1.

But in the general case for other b, a must be of the form m*b² - b, and only specific a's are valid.

So, perhaps for b=1, all a are valid, and for b>1, only specific a's are valid.

Let's verify this.

From the earlier examples:

In n=2, m=3:

For b=1: all a=1,2 are valid.

For b=2: only a=2,6,10, but a=6 and 10 are out of range.

So, only a=2 is valid.

For b=3: only a=6 is valid, but a=6 > n=2, so no valid a.

Total valid pairs: (1,1),(2,1),(2,2), which is 3, matching the sample.

In n=3, m=5:

For b=1: a=1,2,3.

For b=2: a=2,6,10, but a=6 and 10 > n=3, so only a=2.

For b=3: a=6 > n=3, so no valid a.

For b=4: no valid a.

For b=5: no valid a.

Total valid pairs: (1,1),(2,1),(2,2),(3,1), which is 4, matching the sample.

In n=10, m=8:

For b=1: a=1 to 10.

For b=2: a=2,6,10.

For b=3: a=6.

For b=4: no valid a.

For b=5: no valid a.

For b=6: no valid a.

For b=7: no valid a.

For b=8: no valid a.

Total valid pairs: for b=1:10, b=2:3, b=3:1. Total 14, matching the sample.

So, the general approach is:

- For b=1, all a from 1 to n are valid.

- For b>1, a must be of the form m*b² - b, for m ≥1, and 1 ≤ a ≤n.

So, for each b from 1 to m:

- If b=1, add n to the count.

- If b>1, find the number of integers a of the form m*b² - b that lie between 1 and n, inclusive.

To find the number of such a's for each b>1:

Given a = m*b² - b.

We need 1 ≤ m*b² - b ≤ n.

Solve for m:

1 ≤ m*b² - b ⇒ m ≥ ceil( (1 + b)/b² )

And m*b² - b ≤ n ⇒ m ≤ floor( (n + b)/b² )

So, m can range from ceil( (1 + b)/b² ) to floor( (n + b)/b² ), inclusive.

The number of valid m's is floor( (n + b)/b² ) - ceil( (1 + b)/b² ) + 1, if floor() >= ceil(), else 0.

Therefore, for each b from 1 to m:

- If b=1, add n to the count.

- If b>1, compute floor( (n + b)/b² ) - ceil( (1 + b)/b² ) + 1, and add to the count if positive.

This seems efficient, as for each b, the computation is O(1), and b ranges up to m, which is up to 2e6, and with t up to 1e4, but with the sum of m and n across all test cases up to 2e6, it should be manageable.

However, since t can be up to 1e4, and for each test case, m can be up to 2e6, but with the sum of m across all test cases up to 2e6, it's better to handle the test cases independently but efficiently.

So, in code, I can iterate over each test case, and for each b from 1 to m, compute the number of valid a's as described.

But to optimize, perhaps I can find a way to compute the sum over b from 1 to m of the number of valid a's for each b.

Looking back at the formula:

For b=1: n

For b>1: floor( (n + b)/b² ) - ceil( (1 + b)/b² ) + 1, if >=0 else 0.

I can precompute floor( (n + b)/b² ) and ceil( (1 + b)/b² ) for each b from 1 to m.

But perhaps there's a better mathematical approach.

Alternatively, I can iterate b from 1 to m, and for each b, compute the number of a's that satisfy the condition.

Given that sum of m across all test cases is up to 2e6, and t is up to 1e4, but sum of m across all test cases is 2e6, it should be fine.

Let me consider implementing this approach.

But looking at the given code:

def func():

T = int(input())

for t in range(T):

info = input().split()

(a, b) = (int(info[0]), int(info[1]))

suma = 0

for i in range(1, b + 1):

x = (a - i * (i - 1)) // i ** 2 + 1

if (a - i * (i - 1)) // i ** 2 + 1 > 0:

suma += x

if (a - i * (i - 1)) % i ** 2 == 0 and i * (i - 1) % i ** 2 == 0:

suma += 1

print(suma - 2)

Wait, this seems different from what I derived.

Let's see what this code is doing.

It's iterating i from 1 to b (inclusive), and for each i, computing x = floor( (a - i*(i-1)) / i² ) + 1.

Then, if x > 0, add x to suma.

Additionally, if (a - i*(i-1)) % i² == 0 and i*(i-1) % i² == 0, then add 1 more to suma.

Finally, print suma - 2.

This seems like an attempt to count the number of a's for each i (which corresponds to b in my earlier notation).

But I need to understand how this relates to my earlier derivation.

Let me compare.

In my earlier approach, for each b, the number of a's is:

- If b=1: n

- If b>1: floor( (n + b)/b² ) - ceil( (1 + b)/b² ) + 1

But in the code, it's iterating i from 1 to b, and computing x = floor( (a - i*(i-1)) / i² ) + 1.

Wait, a corresponds to n, and b corresponds to m in my notation.

So, for each i (which is b in my notation), it's computing floor( (n - i*(i-1)) / i² ) + 1.

I need to see if this is equivalent to my formula.

Wait, in my formula for b>1, it's floor( (n + b)/b² ) - ceil( (1 + b)/b² ) + 1.

This seems different from floor( (n - i*(i-1)) / i² ) + 1.

So, perhaps there's another way to look at this.

Let me consider that i*(i-1) is being subtracted from n, and then divided by i².

Wait, in my earlier derivation, for b=i, a = m*i² - i.

So, a ranges from i²*m - i, for m from 1 to floor( (n + i)/i² ).

Wait, perhaps there's a connection.

Let me think differently.

Suppose I solve for m in a = m*b² - b.

Given a, b, m = (a + b)/b², provided that (a + b) is divisible by b².

So, for each b, the number of m's such that m = ceil( (1 + b)/b² ) to floor( (n + b)/b² ).

But in the code, it's computing floor( (n - i*(i-1)) / i² ) + 1.

Wait, perhaps it's a different way of counting the same thing.

Let me try to see.

For b=i, a = m*i² - i.

We need 1 ≤ m*i² - i ≤ n.

So, m*i² - i ≥1 ⇒ m ≥ ceil( (1 + i)/i² )

And m*i² - i ≤n ⇒ m ≤ floor( (n + i)/i² )

So, number of m's is floor( (n + i)/i² ) - ceil( (1 + i)/i² ) + 1.

But in the code, it's computing floor( (n - i*(i-1)) / i² ) + 1.

Wait, i*(i-1) = i² - i.

So, n - i*(i-1) = n - i² + i.

So, floor( (n - i² + i)/i² ) +1 = floor( (n + i)/i² - 1 ) +1 = floor( (n + i)/i² )

Which matches floor( (n + i)/i² ), which is the upper bound for m.

Similarly, the lower bound is ceil( (1 + i)/i² ).

So, the difference is floor( (n + i)/i² ) - ceil( (1 + i)/i² ) + 1.

But in the code, it's just floor( (n - i*(i-1))/i² ) +1, which is floor( (n + i)/i² ).

So, it seems like the code is only considering floor( (n + i)/i² ), but according to my earlier formula, it should be floor( (n + i)/i² ) - ceil( (1 + i)/i² ) + 1.

So, there's a discrepancy here.

Perhaps the code is handling b=1 separately.

Wait, in the code, for i=1:

i*(i-1) = 0.

So, floor( (n - 0)/1 ) +1 = n +1.

But for b=1, according to my earlier approach, the number of a's is n.

So, it's overcounting by 1 for b=1.

Wait, but in the code, it's suma - 2 at the end.

So, perhaps it's compensating for overcounting.

Wait, let's see.

For b=1:

x = floor( (n - 0)/1 ) +1 = n +1.

But actually, for b=1, the number of a's should be n.

So, it's overcounting by 1.

For b>1:

x = floor( (n - i*(i-1))/i² ) +1 = floor( (n + i)/i² ).

But according to my formula, it should be floor( (n + i)/i² ) - ceil( (1 + i)/i² ) + 1.

So, it seems like the code is not subtracting ceil( (1 + i)/i² ) -1.

Wait, but in the code, there's an additional condition:

if (a - i*(i-1)) // i² +1 >0 and (a - i*(i-1)) % i² ==0 and i*(i-1) % i² ==0:

suma +=1

This seems like an attempt to handle the ceiling part.

Wait, perhaps it's trying to adjust for the ceil( (1 + i)/i² ).

But it's getting complicated.

Let me try to see with an example.

Take n=2, m=3.

For i=1:

x = floor( (2 - 0)/1 ) +1 = 2 +1 =3.

But for b=1, the number of a's should be 2.

So, it's overcounting by 1.

For i=2:

x = floor( (2 - 2*1)/4 ) +1 = floor( (2 - 2)/4 ) +1 = floor(0/4) +1 =0 +1=1.

Check if (2 - 2*1) %4 ==0 and 2*1 %4 ==0:

(0)%4==0 and 2%4==0 → true, so suma +=1.

So, for i=2, suma +=1 +1 =2.

For i=3:

x = floor( (2 - 3*2)/9 ) +1 = floor( (2 - 6)/9 ) +1 = floor(-4/9) +1 = floor(-0.444) +1 = -1 +1 =0.

Since x >0 is not true, no addition.

So, total suma =3 (from i=1) +2 (from i=2) +0 (from i=3) =5.

Then, print suma -2 =3, which matches the sample.

Wait, but according to my earlier manual count, for n=2, m=3, there should be 3 valid pairs.

So, it's working.

Let me check for n=3, m=5.

For i=1:

x = floor( (3 -0)/1 ) +1 =3 +1=4.

For i=2:

x = floor( (3 -2)/4 ) +1 = floor(1/4) +1=0 +1=1.

Check if (3-2)%4==0 and 2%4==0 →1%4==0 (false), so no additional +1.

For i=3:

x = floor( (3 -6)/9 ) +1 = floor(-3/9) +1 = floor(-0.333) +1=-1 +1=0.

No addition.

So, suma=4+1+0=5.

Then, print suma -2=3, but according to the sample, it should be 4.

Wait, discrepancy here.

Wait, in the sample, for n=3, m=5, output is 4.

But according to this code, suma=5-2=3.

But earlier manual count showed 4 valid pairs: (1,1),(2,1),(2,2),(3,1).

So, the code is giving 3, but should be 4.

Hmm, seems like the code is incorrect.

Wait, perhaps I made a mistake in calculating suma.

Let's recalculate for n=3, m=5.

For i=1:

x = floor( (3 -0)/1 ) +1=3+1=4.

For i=2:

x = floor( (3 -2)/4 ) +1= floor(1/4)+1=0+1=1.

Check if (3-2)%4==0 and 2%4==0 →1%4≠0 → no addition.

For i=3:

x = floor( (3-6)/9 ) +1= floor(-3/9)+1=-1+1=0.

No addition.

So, suma=4+1+0=5.

Then, print suma -2=3.

But according to manual count, there are 4 valid pairs.

So, perhaps the code is incorrect.

Wait, perhaps the "-2" at the end is not general.

In the first sample, for n=2, m=3, manual count is 3, code gives 5-2=3, matches.

For n=3, m=5, manual count is 4, code gives 5-2=3, doesn't match.

So, perhaps the "-2" is not correct.

Alternatively, perhaps the code is partially correct but missing some adjustments.

This suggests that the given code might be incorrect.

Wait, but the problem says it's a correct program.

Wait, no, the problem presents two versions, and says you can make hacks only if both versions are solved.

But in the instructions, it says "the given program is correct", but perhaps that's for version 2.

Wait, looking back, it says "the two versions are different problems. You may want to read both versions. You can make hacks only if both versions are solved."

So, perhaps version 1 and version 2 are different problems, and I need to consider both.

But in the instructions for each version, it says "the given program is correct", but perhaps that's not the case.

Given the discrepancy I found, it seems like the code might be incorrect.

Alternatively, perhaps I made a mistake in my manual count.

Let me double-check for n=3, m=5.

Possible pairs:

(1,1): valid.

(2,1): valid.

(3,1): valid.

(2,2): a+b=4, b*GCD(2,2)=4. 4 is a multiple of 4. Valid.

(3,3): a+b=6, b*GCD(3,3)=9. 6 is not a multiple of 9. Invalid.

(1,2): a+b=3, b*GCD(1,2)=2. 3 is not a multiple of 2. Invalid.

(1,3): a+b=4, b*GCD(1,3)=3. 4 is not a multiple of 3. Invalid.

(1,4): a+b=5, b*GCD(1,4)=4. 5 is not a multiple of 4. Invalid.

(1,5): a+b=6, b*GCD