The code `ans += l - pos` updates the variable `ans` by adding the value of `l - pos` to its current value. Given the initial conditions:

- `pos` is less than `l`
- Therefore, `l - pos` is a positive integer.

Since `ans` is initially 0, the new value of `ans` will be `l - pos`. The values of `n`, `pos`, `l`, and `r` remain unchanged.

Output State: **`n` is an integer such that 1 ≤ n ≤ 100; `pos` is an integer such that 1 ≤ pos ≤ n; `l` is an integer such that 1 ≤ l ≤ n; `r` is an integer such that 1 ≤ l ≤ r ≤ n; `ans` is `l - pos`.**