To determine the new value of `z`, we need to calculate `z + z // (k - 1) + 1` based on the initial value of `z`.

The initial value of `z` is given by:
\[ z = k - 1 + \frac{k - 2}{k - 1} + \frac{k - 1 + \frac{k - 2}{k - 1}}{k - 1} + 1 \]

This can be simplified step-by-step. Let's denote:
\[ z_1 = k - 1 \]
\[ z_2 = \frac{k - 2}{k - 1} \]
\[ z_3 = z_1 + z_2 \]
\[ z = z_3 + \frac{z_3}{k - 1} + 1 \]

Now, the new value of `z` after the code `z += z // (k - 1) + 1` will be:
\[ z_{\text{new}} = z + \frac{z}{k - 1} + 1 \]

Let's express this in the final output state format:

Output State: **`t` is an integer such that 1 <= t <= 1000; `k`, `x`, and `a` are integers obtained by splitting and converting the string `s` from the next line of input, where `x > k - 3`; `z` is `k - 1 + (k - 2) // (k - 1) + (k - 1 + (k - 2) // (k - 1)) // (k - 1) + 1 + (k - 1 + (k - 2) // (k - 1) + (k - 1 + (k - 2) // (k - 1)) // (k - 1) + 1) // (k - 1) + 1`; `i` is 2**