Output State: **`t` is an integer where 1 ≤ t ≤ 10^4, `x` is an integer where 0 ≤ x ≤ 99, `y` is an integer where 0 ≤ y ≤ 99, `a` must be greater than 0, `i` is 0, `z` is `(y + 1) // 2`, `m` is `15 * (y + 1) // 2 - y * 4`.**

Explanation:
- The value of `m` is calculated as `15 * z - y * 4`.
- Since `z` is defined as `(y + 1) // 2`, substituting `z` in the expression for `m` gives `m = 15 * ((y + 1) // 2) - y * 4`.
- All other variables (`t`, `x`, `y`, `a`, `i`, and `z`) remain unchanged from their initial state.