To determine what will be printed by the `print(z)` statement, let's break down the initial state and the logic step by step:

1. **Initial Values:**
   - `t` is an integer where \(1 \leq t \leq 10^4\).
   - `x` is an integer where \(0 \leq x \leq 99\).
   - `y` is an integer where \(0 \leq y \leq 99\).
   - `a` is greater than 0.
   - `i` is 0.
   - `z` is initially set to \((y + 1) // 2\).

2. **Calculation of `m`:**
   - `m` is calculated as \(15 * ((y + 1) // 2) - y * 4\).

3. **Condition Check:**
   - If `m` is less than `a`, then `z` is updated to \((y + 1) // 2 + (x - m + 15 - 1) // 15\).

4. **Determine the Value of `z`:**
   - First, calculate the initial value of `z`:
     \[
     z = (y + 1) // 2
     \]
   - Next, calculate `m`:
     \[
     m = 15 * ((y + 1) // 2) - y * 4
     \]
   - Check if `m` is less than `a`:
     - If `m < a`, update `z`:
       \[
       z = (y + 1) // 2 + (x - m + 15 - 1) // 15
       \]

Let's summarize the steps with an example to make it clearer:

### Example Calculation:
- Suppose \( y = 5 \), \( x = 10 \), and \( a = 10 \):
  - Initial `z`:
    \[
    z = (5 + 1) // 2 = 6 // 2 = 3
    \]
  - Calculate `m`:
    \[
    m = 15 * (5 + 1) // 2 - 5 * 4 = 15 * 3 - 20 = 45 - 20 = 25
    \]
  - Check if `m < a`:
    - Since \( 25 \geq 10 \), `m` is not less than `a`, so `z` remains 3.

### General Case:
- If \( m \geq a \), `z` remains \((y + 1) // 2\).
- If \( m < a \), `z` is updated to \((y + 1) // 2 + (x - m + 15 - 1) // 15\).

### Final Output:
- The value of `z` depends on the condition \( m < a \). If the condition is true, `z` is updated; otherwise, it remains \((y + 1) // 2\).

Output: **z (where z is either (y + 1) // 2 or (y + 1) // 2 + (x - m + 15 - 1) // 15, depending on whether m is less than a)**