To determine what will be printed, let's analyze the given initial state and the print statement step by step.

### Initial State:
1. `t` is at least 0 (though `t` is not used in the print statement, we can ignore it for this task).
2. `p1`, `p2`, and `p3` are integers such that \(0 \leq p1 \leq p2 \leq p3 \leq 30\).
3. The sum of `p1`, `p2`, and `p3` is odd.
4. If `p3` is greater than or equal to the sum of `p1` and `p2`, `p3` retains its original value. Otherwise, `p3` retains its original value (this condition seems redundant as `p3` always retains its original value based on the given condition).
5. `x` is 0.
6. `y` is equal to `p3`.
7. `p1 - x` is less than or equal to `p2 - y`.

### Print Statement:
```python
print(p1 - x + p3)
```

### Analysis:
- Given that `x` is 0, the expression `p1 - x` simplifies to `p1`.
- Therefore, the print statement simplifies to `print(p1 + p3)`.

### Constraints:
- Since `0 \leq p1 \leq p2 \leq p3 \leq 30` and the sum `p1 + p2 + p3` is odd, we know that `p1`, `p2`, and `p3` are integers within this range, and their sum is odd.
- The condition `p1 - x <= p2 - y` simplifies to `p1 <= p2 - p3` given `x = 0` and `y = p3`. However, since `p1 <= p2` and `p2 <= p3`, this condition is inherently satisfied and does not provide additional constraints.

### Output:
The print statement `print(p1 + p3)` will output the sum of `p1` and `p3`.

Output: **p1 + p3 (where p1 and p3 are integers such that 0 ≤ p1 ≤ p2 ≤ p3 ≤ 30 and p1 + p2 + p3 is odd)**