The code `ans += 4 * cur` updates the value of `ans` by adding `4 * cur` to its current value. From the initial state, we know that `ans` is updated according to the formula `ans + 4 * (cur + 1)` and `cur` is increased by 1. This means before the current line of code, `ans` had the value of `ans + 4 * (cur + 1)` and `cur` was increased by 1.

After running `ans += 4 * cur`, the new value of `ans` will be:

\[ \text{new } ans = (\text{original } ans + 4 \times (cur + 1)) + 4 \times cur \]
\[ \text{new } ans = \text{original } ans + 4 \times (cur + 1) + 4 \times cur \]
\[ \text{new } ans = \text{original } ans + 4 \times cur + 4 + 4 \times cur \]
\[ \text{new } ans = \text{original } ans + 8 \times cur + 4 \]

Since the original `ans` was already updated to `ans + 4 * (cur + 1)` and `cur` was increased by 1, we can substitute these into the equation:

\[ \text{new } ans = (ans + 4 \times (cur + 1)) + 8 \times cur + 4 \]
\[ \text{new } ans = ans + 4 \times cur + 4 + 8 \times cur + 4 \]
\[ \text{new } ans = ans + 12 \times cur + 8 \]

Given the initial conditions and the code execution, the output state is:

Output State: **`n` is at least 4, `ans` is equal to the original `ans` plus 12 times `cur` plus 8, `cur` is increased by 1.**