Let's analyze the loop step by step to determine the final state of the variables after the loop has executed.

### Initial State
- `n` must be greater than or equal to 2
- `i` is 2
- `cur` is 2

### Loop Condition
The loop continues as long as `i * cur <= n`.

### Loop Body
- `ans += 4 * cur`
- `cur += 1`

### Iteration Analysis
1. **First Iteration:**
   - `i = 2`, `cur = 2`
   - Check condition: `2 * 2 <= n` -> `4 <= n` (must be true)
   - `ans += 4 * 2` -> `ans += 8`
   - `cur += 1` -> `cur = 3`

2. **Second Iteration:**
   - `i = 2`, `cur = 3`
   - Check condition: `2 * 3 <= n` -> `6 <= n` (must be true)
   - `ans += 4 * 3` -> `ans += 12`
   - `cur += 1` -> `cur = 4`

3. **Third Iteration:**
   - `i = 2`, `cur = 4`
   - Check condition: `2 * 4 <= n` -> `8 <= n` (must be true)
   - `ans += 4 * 4` -> `ans += 16`
   - `cur += 1` -> `cur = 5`

### General Pattern
From the first few iterations, we observe that each iteration increases `cur` by 1 and adds `4 * cur` to `ans`. Therefore, after `k` iterations:
- `cur` will be `2 + k`
- `ans` will be the sum of `4 * (2 + 1 + 2 + ... + (2 + k - 1))`

The sum of the sequence `2 + 3 + 4 + ... + (2 + k - 1)` is the sum of an arithmetic series with the first term `2` and the last term `(2 + k - 1)` and `k` terms. The sum of this series is:
\[ \text{Sum} = \frac{k}{2} \times [2 + (2 + k - 1)] = \frac{k}{2} \times (k + 1) = \frac{k(k + 1)}{2} \]

Thus, after `k` iterations:
- `cur = 2 + k`
- `ans = 4 \times \frac{k(k + 1)}{2} = 2k(k + 1)`

### Final Output State
- `i` remains 2 after the loop since the loop does not modify it
- `cur` will be `2 + k` where `k` is the number of iterations
- `ans` will be `2k(k + 1)` where `k` is the number of iterations

Given that the loop runs as long as `i * cur <= n`, the final state depends on the value of `n` and the number of iterations `k` such that `2k(k + 1) <= n`.

### Output State
Output State: **`i` is 2, `cur` is 2 + k, `ans` is 2k(k + 1), `n` must be at least 2k(k + 1)**