The code snippet updates the `dp` table based on the formula `dp[i][j] = max(dp[i][j], dp[i - 1][j - t[i - 1]] + 1)`. Here's a step-by-step breakdown:

1. **Initial Values**: 
   - `t` is `[n, k, M]`
   - `dp` is a 2D list with dimensions `(k + 1) x (M + 1)` where each element is 0 except `dp[1][j]` which is 1 for `j >= t[0]`
   - `k` is greater than or equal to 1
   - `M` is greater than 0
   - `j` is 3

2. **Updating the DP Table**:
   - The first row of `dp` (`dp[1]`) is already initialized such that `dp[1][j] = 1` for `j >= t[0]`.
   - For subsequent rows (`i > 1`), the value `dp[i][j]` is updated based on the maximum of its current value and the value from the previous row at `dp[i-1][j - t[i-1]] + 1` if `j >= t[i-1]`.

Given that `j` is 3, we only need to consider the updates for `dp[2]` since `t[1] = k` and we start from `i = 2`.

Let's update `dp[2][3]`:
- For `dp[2][3]`: We need to check if `3 >= t[1]` (i.e., `3 >= k`). Since `k` is at least 1, this condition holds true.
- So, `dp[2][3] = max(dp[2][3], dp[1][3 - k] + 1)`

Since `dp[1][j] = 1` for `j >= t[0]` and `t[0] = n`, we need to know the value of `n` and `k` to determine the exact value of `dp[1][3 - k]`.

Assuming `n` is at least 3 (since `j` is 3 and we are considering `dp[1][3 - k]`), `dp[1][3 - k]` would be 1 because `3 - k` is non-negative.

Thus, `dp[2][3] = max(dp[2][3], 1 + 1) = max(dp[2][3], 2)`.

Since `dp[2][3]` was initially 0, the new value of `dp[2][3]` will be 2.

All other elements in the `dp` table remain unchanged.

Output State: **`t` is `[n, k, M]`, `dp` is a 2D list with dimensions `(k + 1) x (M + 1)` where each element is 0 except `dp[1][j]` which is 1 for `j >= n`, `dp[2][3]` is 2, and all other elements remain 0, `k` is greater than or equal to 1, `M` is greater than 0, and `j` is 3**.