The code snippet provided is `x2 -= a`. This means the value of `x2` is decreased by the value of `a`.

Initial State: 
- `t` is `abs(y2 - y1)`
- `h` and `w` are positive integers such that 1 <= h <= 10^6 and 1 <= w <= 10^9
- `x_a`, `y_a`, `x_b`, and `y_b` are positive integers such that 1 <= x_a, x_b <= h and 1 <= y_a, y_b <= w
- `r` is a list of integers read from input
- `n` is `r[0]`
- `m` is `r[1]`
- `x1` is `r[2] + 1 + a`
- `x2` is `r[4]`
- `(x2 - x1) % 2 != 0`
- `y1` is still not equal to `y2`
- `b` is `x2 - x1`

After the execution of `x2 -= a`, the value of `x2` will be `x2 - a`.

Output State: **`t` is `abs(y2 - y1)`, `h` and `w` are positive integers such that 1 <= h <= 10^6 and 1 <= w <= 10^9; `x_a`, `y_a`, `x_b`, and `y_b` are positive integers such that 1 <= x_a, x_b <= h and 1 <= y_a, y_b <= w; `r` is a list of integers read from input; `n` is `r[0]`; `m` is `r[1]`; `x1` is `r[2] + 1 + a`; `x2` is `r[4] - a`; `(x2 - x1) % 2 != 0`; `y1` is still not equal to `y2`; `b` is `x2 - x1`.**

In natural language: The value of `x2` has been decreased by `a`, so `x2` is now `r[4] - a`. All other variables remain unchanged.