The code snippet `y1 += a` increments the value of `y1` by `a`. Given the initial state, `y1` is initially not equal to `y2`, and `y2` is `m`. After the increment, `y1` will be `y1 + a`.

Here is the updated output state:

Output State: **`t` is `abs(y2 - y1)`, `h` and `w` are positive integers such that 1 <= h <= 10^6 and 1 <= w <= 10^9; `x_a`, `y_a`, `x_b`, and `y_b` are positive integers such that 1 <= x_a, x_b <= h and 1 <= y_a, y_b <= w; `r` is a list of integers read from input; `n` is `r[0]`; `m` is `r[1]`; `x1` is `r[2] + 1 + a`; `x2` is `r[4] - a`; `(x2 - x1) % 2 != 0`; `y1` is `y1 + a`; `y2` is `m`; `b` is `x2 - x1`; `x2` is greater than `x1`, `x1` is greater than or equal to 1, and `x2` is less than or equal to `n`; `y2` is not equal to `y1` unless `a` was such that `y1 + a` equals `m`.**

In simpler terms, the value of `y1` has been increased by `a`, and `y2` remains `m`. All other variables retain their initial values.