The code snippet `ans += m` increments the value of `ans` by `m`. Given the initial state, `ans` is initially set to `m` if `i` ('C') is not a key in `hmp`; otherwise, `ans` is 0. Since the operation `ans += m` is performed, `ans` will be `ans + m`.

If `i` ('C') was not a key in `hmp`, `ans` was initially `m`, and after the operation, `ans` becomes `m + m`, which is `2 * m`.
If `i` ('C') was a key in `hmp`, `ans` was initially `0`, and after the operation, `ans` becomes `0 + m`, which is `m`.

Therefore, the new value of `ans` is either `m` or `2 * m` depending on whether 'C' was a key in `hmp` or not.

Output State: **`t` is an integer input by the user such that 1 ≤ `t` ≤ 1000; `n` and `m` are integers input by the user such that 1 ≤ `n` ≤ 50 and 1 ≤ `m` ≤ 5; `a` is a string of length `n` consisting of characters from 'A' to 'G'; `s` is a string input by the user; `p` is 'ABCDEF'; `hmp` is a Counter object representing the frequency of each character in `s`; `i` is 'C'; `ans` is either `m` or `2 * m` depending on whether 'C' was a key in `hmp` or not.**