Based on the initial state provided:

- `t` must be greater than 0 (though this does not affect the print statement).
- `steps` is 2.
- `a` and `b` are input integers.
- `c` and `d` are the first and second integers entered, respectively.
- `e` and `f` are the first and second integers from input split and converted to integers, which means `c = e` and `d = f`.
- `g` and `h` are the first and second integers from input split and converted to integers, but since no new integers are entered here, they should be the same as `c` and `d`, i.e., `g = c` and `h = d`.

The expression for `x` is:
\[ x = (c - g) \times (c - g) + (d - h) \times (d - h) \]

Given that `c = e`, `d = f`, `g = c`, and `h = d`, we can simplify the expression for `x`:
\[ x = (c - c) \times (c - c) + (d - d) \times (d - d) = 0 + 0 = 0 \]

Therefore, the print statement will output the value of `x`, which is 0.

Output: **0**