Based on the initial state provided:

- `t` is a positive integer such that 1 ≤ t ≤ 500.
- `_` is 1.
- `p1`, `p2`, and `p3` are integers entered by the user.
- The sum of `p1`, `p2`, and `p3` is odd.
- `p3` is less than `p1 + p2`.
- `x` is either 0 or 1.
- `y` must be `p3`.

Given these conditions, we need to determine the value of `p1 - x + p3` that will be printed.

Since `x` is either 0 or 1, and `p3` is a specific integer entered by the user, let's break it down:

- If `x = 0`, then `p1 - x + p3` simplifies to `p1 + p3`.
- If `x = 1`, then `p1 - x + p3` simplifies to `p1 - 1 + p3`.

However, without knowing the exact value of `x`, we cannot definitively state the exact numerical result. But we know the expression `p1 - x + p3` will evaluate to either `p1 + p3` or `p1 - 1 + p3`.

Output: **p1 + p3 if x = 0, or p1 - 1 + p3 if x = 1**