Let's break down the given initial state and variables to determine what will be printed by the `print` statement.

### Initial State Recap:
- `t` is an integer read from the input and is greater than or equal to 1.
- `n` is a non-negative integer.
- `r` is the largest integer `i` such that `n * (n + 1) // 2 > i * n` holds true, and it ensures that `n + r + 1` is at least 2.
- `sum` is a cumulative sum (though it is not used in the print statement).
- `j` is `n + r`.

### Determining the Value of `r`:
The condition for `r` is `n * (n + 1) // 2 > i * n`. We need to find the largest `i` that satisfies this inequality.

Let's rewrite the inequality:
\[ n * (n + 1) // 2 > i * n \]

Dividing both sides by `n` (assuming `n > 0`):
\[ (n + 1) // 2 > i \]

So, `i` must be less than `(n + 1) // 2`. The largest integer `i` that satisfies this is:
\[ r = (n + 1) // 2 - 1 \]

However, we also need to ensure that `n + r + 1` is at least 2:
\[ n + r + 1 \geq 2 \]
\[ n + ((n + 1) // 2 - 1) + 1 \geq 2 \]
\[ n + (n + 1) // 2 \geq 2 \]

This condition is always satisfied for `n >= 0`.

### Determining the Value of `j`:
\[ j = n + r \]
\[ j = n + ((n + 1) // 2 - 1) \]
\[ j = n + (n + 1) // 2 - 1 \]

### Final Calculation:
- If `n` is even, say `n = 2k`, then `(n + 1) // 2 = k + 1`, so `r = k`, and `j = 2k + k = 3k`.
- If `n` is odd, say `n = 2k + 1`, then `(n + 1) // 2 = k + 1`, so `r = k`, and `j = 2k + 1 + k = 3k + 1`.

In both cases, `j` is effectively `n + (n + 1) // 2 - 1`.

### Output:
The `print` statement will output `1`, followed by the value of `j`, and the `end=' '` will ensure there's a space after the output.

Output: **1, j (where j = n + (n + 1) // 2 - 1)**