Alright, I've got this problem to solve. Let's see what it's asking for. So, we have an array `c` of length `n`, and each element is positive. Then, there are `q` queries, each giving a subarray defined by left and right indices, and I need to determine if that subarray is "good" based on the conditions provided.

First, I need to understand what makes an array "good." According to the problem, an array `a` of length `m` is good if there exists another integer array `b` of the same length such that:

1. The sum of elements in `a` is equal to the sum of elements in `b`.

2. For every index `i`, `a_i` is not equal to `b_i`.

3. Every element in `b` is greater than 0.

So, for a given subarray of `c`, I need to check if there's another array `b` that meets these criteria.

Let me try to rephrase this in my own words. I have a subarray, and I need to find another array of the same length and same sum, but none of its elements should be equal to the corresponding element in the subarray, and all elements in `b` should be positive integers.

I need to find out for each query whether such a `b` exists for the given subarray.

Alright, let's think about how to approach this.

First, since the sum of `a` must equal the sum of `b`, and `b` has to be all positive integers different from `a`, I need to see if it's possible to adjust each `a_i` to some `b_i` > 0, with `b_i` != `a_i`, without changing the total sum.

Wait, but `b` has to have the same sum as `a`, and each `b_i` is positive and not equal to `a_i`. So, for each `a_i`, `b_i` can be either greater than or less than `a_i`, but it can't be equal.

Hmm, but if I change `a_i` to `b_i`, and `b_i` != `a_i`, and `b_i` > 0, then the sum will change unless the increases and decreases balance out.

This seems tricky. Maybe I need to look at the minimal possible `b`.

Let's consider the minimal possible `b` that satisfies `b_i > 0` and `b_i != a_i`.

If `a_i` is 1, then `b_i` can be 2 or 0, but `b_i` has to be >0, so `b_i` must be at least 2.

If `a_i` is greater than 1, then `b_i` can be either `a_i - 1` or `a_i + 1`, as long as `b_i` > 0.

Wait, but `b_i` just has to be positive and not equal to `a_i`. So, for `a_i` >1, `b_i` can be `a_i -1` (if `a_i -1` >0), or `a_i +1`, or any other positive integer except `a_i`.

So, to minimize the sum of `b`, I would choose `b_i` as close as possible to `a_i` but not equal to it.

Similarly, to maximize the sum of `b`, I could choose `b_i` much larger, but since I need the sum to be equal to the sum of `a`, I need to balance the increases and decreases.

Wait, but the problem is to have the sum equal to that of `a`, so perhaps I need to ensure that the total adjustment sums to zero.

Let me think differently. Suppose I define `d_i = b_i - a_i`. Then, `d_i` != 0 for all `i`, and the sum of `d_i` over all `i` must be zero.

Also, `b_i >0`, so `a_i + d_i >0`, which implies `d_i > -a_i`.

So, for each `i`, `d_i` is a non-zero integer such that `a_i + d_i >0`, and the sum of all `d_i` is zero.

This seems like a standard problem where I need to find a set of non-zero integers that sum to zero, with each `d_i` satisfying `a_i + d_i >0`.

This sounds similar to the problem of assigning values to variables with constraints and a total sum.

But maybe there's a simpler way to look at this.

Let me consider the minimal possible sum of `b`.

If I set `b_i` to be the smallest possible value greater than 0 and not equal to `a_i`, what would that be?

If `a_i` =1, then `b_i` must be at least 2.

If `a_i` >1, then `b_i` can be `a_i -1` if `a_i -1 >0`, else `b_i` must be at least `a_i +1`.

Wait, more precisely:

- If `a_i` =1, `b_i` must be at least 2.

- If `a_i` >1, `b_i` can be either `a_i -1` or `a_i +1`, whichever is positive.

But to minimize the sum of `b`, I would choose `b_i` as close to `a_i` as possible, but not equal to it.

So, for `a_i` >1, choosing `b_i = a_i -1` if `a_i -1 >0`, else `b_i = a_i +1`.

Wait, but `a_i` is at least 1, since all elements are positive integers.

So, for `a_i` =1, `b_i` must be at least 2.

For `a_i` >1, `b_i` can be either `a_i -1` or `a_i +1`.

To minimize the sum, I would choose `b_i = a_i -1` for `a_i` >1.

But for `a_i` =1, `b_i` must be at least 2, which is `a_i +1`.

So, in general, to minimize the sum of `b`, set:

- `b_i = a_i -1` if `a_i` >1

- `b_i = a_i +1` if `a_i` =1

Then, the minimal possible sum of `b` is sum_{i} (a_i -1 if a_i >1 else a_i +1).

Now, since the sum of `b` must equal the sum of `a`, the minimal sum of `b` must be less than or equal to the sum of `a`.

Wait, but in this case, the sum of minimal `b` is sum_{i} (a_i -1 if a_i >1 else a_i +1).

Let me denote:

sum_b_min = sum_{i} (a_i -1 if a_i >1 else a_i +1)

But for the sum of `b` to equal sum of `a`, we need sum_b_min <= sum_a.

But sum_b_min = sum_a - number of a_i >1 + number of a_i =1.

Wait, no.

Wait, let's compute sum_b_min.

sum_b_min = sum_{i} (a_i -1 if a_i >1 else a_i +1)

= sum_a - number of a_i >1 + number of a_i =1

Because for each a_i >1, we subtract 1, and for each a_i =1, we add 1.

So, sum_b_min = sum_a - (n - number of a_i =1) + number of a_i =1

= sum_a - n + 2 * number of a_i =1

So, sum_b_min = sum_a - n + 2 * count_of_ones

Now, for sum_b_min <= sum_a, which is required because sum_b must equal sum_a, we have:

sum_a - n + 2 * count_of_ones <= sum_a

Simplify:

- n + 2 * count_of_ones <= 0

Wait, that can't be right. I must have messed up the inequality.

Wait, sum_b_min <= sum_a is required, so:

sum_a - n + 2 * count_of_ones <= sum_a

Subtract sum_a from both sides:

- n + 2 * count_of_ones <= 0

Which implies:

2 * count_of_ones <= n

So, count_of_ones <= n / 2

Wait, but this seems off. Let's think about it.

If count_of_ones <= n / 2, then sum_b_min <= sum_a.

But in reality, sum_b_min could be less than sum_a, but for sum_b to equal sum_a, I need to adjust some b_i to be higher to compensate for the decreases.

Wait, perhaps I need to think differently.

Let me consider that sum_b = sum_a.

And sum_b_min is sum_a - (n - count_of_ones) + count_of_ones = sum_a - n + 2 * count_of_ones

So, sum_b_min = sum_a - n + 2 * count_of_ones

But sum_b must equal sum_a, so:

sum_a - n + 2 * count_of_ones <= sum_a

Which simplifies to:

- n + 2 * count_of_ones <= 0

Wait, that can't be right because n is positive and count_of_ones is non-negative.

I must have messed up the expression for sum_b_min.

Let me recast it.

sum_b_min = sum_{i} (a_i -1 if a_i >1 else a_i +1)

= sum_a - number of a_i >1 + number of a_i =1

But number of a_i >1 is n - number of a_i =1

So, sum_b_min = sum_a - (n - count_of_ones) + count_of_ones

= sum_a - n + 2 * count_of_ones

Now, for sum_b_min <= sum_a, we have:

sum_a - n + 2 * count_of_ones <= sum_a

Which simplifies to:

- n + 2 * count_of_ones <= 0

But n is positive, and count_of_ones is non-negative, so this inequality can only hold if count_of_ones <= n / 2

Wait, but this doesn't make sense in the context of the problem.

Let me think about an example.

Take n=3, a=[1,2,3]

sum_a =6

sum_b_min = (1+1) + (2-1) + (3-1) = 2 +1 +2 =5

Which is less than sum_a by 1.

But to make sum_b equal to sum_a, I need to increase some b_i by 1.

But I need to ensure that b_i != a_i for all i.

So, in this case, I can set b = [2,1,3], sum is 6, and all b_i != a_i.

Alternatively, b=[2,3,4], sum is 9, which is more than sum_a, but I can also set b=[2,1,3].

So, in this case, it's possible.

Another example: n=1, a=[1], only possible b=[2], which is different and sum is 2 !=1, so not good.

n=2, a=[1,1], sum_a=2

sum_b_min=2+2=4, which is greater than sum_a.

Wait, but according to earlier formula, sum_b_min = sum_a - n + 2 * count_of_ones

Here, sum_a=2, n=2, count_of_ones=2

sum_b_min=2 -2 +4=4

But sum_b_min=4 > sum_a=2, so it's impossible to have sum_b = sum_a.

Hence, it's not good.

Wait, but according to the problem, for n=2, a=[1,1], it should be not good.

But according to the condition 2 * count_of_ones <=n, which is 4 <=2, which is false, so it's not good.

Wait, but in the earlier inequality, we had -n +2 * count_of_ones <=0, which is equivalent to 2 * count_of_ones <=n.

But in the example above, n=2, count_of_ones=2, so 4 <=2 is false, hence not good.

Wait, but in the earlier step, I had sum_b_min = sum_a -n +2 * count_of_ones

And for sum_b_min <= sum_a, we have -n +2 * count_of_ones <=0, which is count_of_ones <= n /2.

But in the example with n=2, count_of_ones=2, which violates this, hence not good.

But in the first example, n=3, count_of_ones=1, sum_a=6, sum_b_min=5.

5 <=6, which satisfies the condition, but according to count_of_ones <=n/2, 1 <=1.5, which is true, so it's good.

Wait, but in this case, sum_b_min=5, sum_a=6, so I need to increase the sum by 1.

But I need to make sure that I can do this without making any b_i equal to a_i.

In the example, a=[1,2,3], sum_a=6.

sum_b_min=2+1+2=5.

To make sum_b=6, I need to increase sum_b by 1.

I can choose to increase one of the b_i by 1.

Looking at b=[2,1,2], I can choose to increase one of them.

If I increase b1 from 2 to 3, which is != a1=1, so b=[3,1,2], sum=6.

Or increase b2 from 1 to 2, but b2=2 == a2=2, which is invalid.

Or increase b3 from 2 to 3, which is != a3=3.

So, b=[2,1,3], sum=6.

Hence, it's possible.

Another example: n=1, a=[1], sum_a=1.

sum_b_min=2, which is greater than sum_a=1, so impossible.

Hence, the condition seems to hold.

Wait, but in the earlier inequality, for sum_b_min <= sum_a, we have count_of_ones <= n /2.

But in the first example, n=3, count_of_ones=1, which is <=1.5, holds.

In the second example, n=2, count_of_ones=2, which is >1, so doesn't hold.

Hence, the condition seems to be count_of_ones <= floor(n /2).

Wait, in n=3, count_of_ones=1 <=1 (floor(3/2)=1), holds.

In n=2, count_of_ones=2 >1 (floor(2/2)=1), doesn't hold.

Wait, but floor(2/2)=1, and 2 >1, so not good.

Wait, but in n=2, count_of_ones=2, which is more than floor(n/2)=1, so not good.

Wait, but in n=3, count_of_ones=1 <= floor(3/2)=1, good.

Wait, but in n=4, count_of_ones=2 <= floor(4/2)=2, good.

Wait, but in n=4, count_of_ones=3 > floor(4/2)=2, not good.

Wait, but according to the earlier inequality, it's count_of_ones <= n /2.

But n is integer, count_of_ones is integer, but n/2 may not be integer.

Hence, it's better to use count_of_ones <= floor(n /2).

So, the condition seems to be count_of_ones <= floor(n /2).

But let's verify with another example.

n=4, a=[1,1,1,2], sum_a=5.

sum_b_min=2+2+2+1=7, which is greater than sum_a=5.

Hence, not good, since count_of_ones=3 > floor(4/2)=2.

Another example: n=4, a=[1,1,2,2], sum_a=6.

sum_b_min=2+2+1+1=6.

Hence, sum_b_min=6 <= sum_a=6.

Hence, it's good.

But count_of_ones=2 <= floor(4/2)=2, holds.

Hence, it's good.

Wait, but in this case, sum_b_min = sum_a.

So, it's possible.

But need to check if I can adjust b_i to make sum_b = sum_a.

In this case, sum_b_min = sum_a, so I can set b_i = a_i -1 if a_i >1, and b_i = a_i +1 if a_i =1.

So, for a=[1,1,2,2], b=[2,2,1,1], sum=6, which matches sum_a=6, and all b_i != a_i.

Hence, it's good.

Another example: n=3, a=[1,1,1], sum_a=3.

sum_b_min=2+2+2=6 >3, count_of_ones=3 > floor(3/2)=1, not good.

Hence, the condition seems to hold.

Wait, but in n=3, count_of_ones=1 <=1, good.

In n=3, count_of_ones=2 >1, not good.

Wait, but in n=3, floor(3/2)=1.

Hence, count_of_ones <=1 is good, count_of_ones >1 is not good.

Hence, the condition is count_of_ones <= floor(n /2).

But in the problem, subarrays are defined from l to r, inclusive.

Hence, for each query, I need to consider the subarray from l to r, and check if the number of ones in that subarray is <= floor((r -l +1)/2).

But floor((r -l +1)/2) is the maximum number of ones allowed in the subarray for it to be good.

Wait, but in the earlier analysis, it's sum_b_min <= sum_a, which translates to count_of_ones <= floor((r -l +1)/2).

Wait, but in one of the examples, n=4, a=[1,1,2,2], count_of_ones=2, floor(4/2)=2, sum_b_min=6 <= sum_a=6, which is good.

Another example, n=4, a=[1,1,1,2], count_of_ones=3, floor(4/2)=2, sum_b_min=7 > sum_a=5, which is not good.

Hence, the condition is count_of_ones <= floor((r -l +1)/2).

Wait, but in n=3, a=[1,2,3], count_of_ones=1, floor(3/2)=1, which is good.

In n=2, a=[1,1], count_of_ones=2, floor(2/2)=1, which is not good.

Hence, the condition is count_of_ones <= floor((r -l +1)/2).

But in the problem, the subarray is from l to r, inclusive, so the length is m = r -l +1.

Hence, the condition is count_of_ones <= floor(m /2).

But in programming terms, floor(m /2) is m //2 in integer division.

Hence, for each query, I need to compute the number of ones in the subarray from l to r, and check if it's <= (r -l +1) //2.

If yes, then "YES", else "NO".

Wait, but in the sample input and output:

Input:

1

5 4

1 2 1 4 5

1 5

4 4

3 4

1 3

Output:

YES

NO

YES

NO

Let's verify with our condition.

Full array: [1,2,1,4,5]

First query: l=1, r=5, subarray=[1,2,1,4,5], count_of_ones=2, m=5, floor(5/2)=2, 2 <=2, so YES.

Second query: l=4, r=4, subarray=[4], count_of_ones=0, m=1, floor(1/2)=0, 0 <=0, but output is NO. Wait, contradiction.

Wait, but according to our condition, it should be YES, but in the sample output, it's NO.

Hmm, so perhaps there's a mistake in my earlier reasoning.

Wait, let's think again.

In the second query, subarray=[4], count_of_ones=0, m=1, floor(1/2)=0.

So, 0 <=0, which should be YES, but sample output is NO.

Hence, my condition is incorrect.

Wait, but according to the problem, for m=1, it's impossible to have b_i != a_i and b_i >0, because b_i must be different from a_i, but b_i >0.

So, if a_i=4, b_i can be any positive integer except 4.

So, for example, b_i=3 or 5 or anything except 4.

But the sum of b must equal sum of a, which is 4.

But if I set b_i=3, sum=3 !=4.

If I set b_i=5, sum=5 !=4.

Hence, it's impossible to have sum_b = sum_a when m=1.

Hence, the condition should be:

If m=1, always NO.

Else, count_of_ones <= floor(m /2).

Hence, in the first query, m=5, count_of_ones=2 <=2, YES.

Second query, m=1, NO.

Third query: l=3, r=4, subarray=[1,4], m=2, count_of_ones=1 <=1, YES.

Fourth query: l=1, r=3, subarray=[1,2,1], m=3, count_of_ones=2 > floor(3/2)=1, NO.

Which matches the sample output.

Hence, the correct condition is:

- If m=1, always NO.

- Else, if count_of_ones <= floor(m /2), then YES, else NO.

Wait, but in the third query, m=2, count_of_ones=1 <=1, YES.

But in m=2, count_of_ones=2 would be NO.

Wait, but in m=2, if count_of_ones=2, sum_a =1+1=2, sum_b_min=2+2=4 >2, which is not good.

Hence, it's only possible if count_of_ones <= floor(m /2).

Hence, the general condition is:

If m >=2 and count_of_ones <= floor(m /2), then YES, else NO.

Hence, for m=1, it's always NO.

For m >=2, check count_of_ones <= floor(m /2).

Now, to implement this efficiently, given that n and q can be up to 3*10^5, I need an efficient way to compute the number of ones in any subarray.

Hence, I can precompute a prefix sum array for the number of ones up to each index.

Let's define ones[i] = number of ones in c[1 to i].

Then, for a query from l to r, count_of_ones = ones[r] - ones[l-1].

Similarly, m = r -l +1.

Hence, for each query, I can compute count_of_ones and m, and apply the condition.

I also need to handle multiple test cases, up to t=10^4, but with the sum of n and q over all test cases <=3*10^5.

Hence, I need to read t test cases, and for each test case, read n, q, the array c, and then q queries.

I need to compute the ones prefix sum for each test case.

Also, I need to make sure that the indices are handled correctly, whether they are 0-based or 1-based.

In the problem, the array is 1-based, as per the sample input.

Hence, in the code, I need to handle indices starting from 1.

Also, in Python, lists are 0-based, so I need to adjust accordingly.

Now, looking at the given code:

import math

testCases = int(input())

for i in range(testCases):

func_1()

def func_1():

(n, q) = map(int, input().split(' '))

nums = list(map(int, input().split(' ')))

ones = [0 for i in range(n + 1)]

sum = [0 for i in range(n + 1)]

for i in range(1, n + 1):

ones[i] = ones[i - 1] + (1 if nums[i - 1] == 1 else 0)

sum[i] = sum[i - 1] + nums[i - 1] - 1

for _ in range(q):

(l, r) = map(int, input().split(' '))

if l == r:

print('NO')

continue

onesInRange = ones[r] - ones[l - 1]

sumInRange = sum[r] - sum[l - 1]

if 2 * onesInRange + (r - l + 1) - onesInRange <= sumInRange:

print('YES')

else:

print('NO')

Wait, this code seems to be implementing a different condition.

Let's see.

It computes ones[i] as the number of ones up to index i.

It also computes sum[i] as sum[j=1 to i] (c_j -1).

Then, for each query, if l == r, it prints 'NO'.

Else, it computes onesInRange = ones[r] - ones[l-1], which is correct.

sumInRange = sum[r] - sum[l-1], which is sum_{j=l to r} (c_j -1).

Then, the condition is:

if 2 * onesInRange + (r - l +1) - onesInRange <= sumInRange:

print('YES')

else:

print('NO')

Wait, simplifying the left side:

2 * onesInRange + (r - l +1) - onesInRange = onesInRange + (r - l +1)

So, the condition is:

onesInRange + (r - l +1) <= sumInRange

But sumInRange is sum_{j=l to r} (c_j -1) = sum_{j=l to r} c_j - (r -l +1)

Hence, the condition becomes:

onesInRange + (r - l +1) <= sum_{j=l to r} c_j - (r - l +1)

Which is:

onesInRange + (r - l +1) <= sum_{j=l to r} c_j - (r - l +1)

Rearranging:

onesInRange + 2*(r - l +1) <= sum_{j=l to r} c_j

But earlier, I derived that the condition should be count_of_ones <= floor(m /2), where m = r -l +1.

But floor(m /2) is floor((r - l +1)/2).

Hence, the condition should be onesInRange <= floor((r - l +1)/2)

But in the code, it's checking onesInRange + (r - l +1) <= sum_{j=l to r} c_j - (r - l +1)

Which seems different.

Hence, perhaps there's a different way to look at this.

Alternatively, perhaps the code is implementing the condition sum_b_min <= sum_a.

Wait, sum_b_min = sum_a - (m - onesInRange) + onesInRange = sum_a - m + 2 * onesInRange

Hence, sum_b_min = sum_a - m + 2 * onesInRange

For sum_b_min <= sum_a, we have:

sum_a - m + 2 * onesInRange <= sum_a

Which simplifies to:

- m + 2 * onesInRange <=0

Which is not possible since m and onesInRange are non-negative.

Wait, perhaps I need to think differently.

Alternatively, perhaps the code is checking if sum_{j=l to r} (c_j -1) >= onesInRange + (r -l +1)

But according to my earlier analysis, the condition should be onesInRange <= floor((r - l +1)/2)

Hence, perhaps there's a mistake in the code.

Wait, perhaps I need to relate the two conditions.

Let me see.

onesInRange <= floor((r - l +1)/2)

Which is equivalent to onesInRange <= (r - l +1)//2

On the other hand, the code is checking:

onesInRange + (r - l +1) <= sum_{j=l to r} c_j - (r - l +1)

But sum_{j=l to r} c_j = sumInRange + (r - l +1)

Hence, the condition is:

onesInRange + (r - l +1) <= sumInRange + (r - l +1) - (r - l +1)

Which simplifies to:

onesInRange + (r - l +1) <= sumInRange

But sumInRange = sum_{j=l to r} c_j - (r - l +1)

Hence, sum_{j=l to r} c_j = sumInRange + (r - l +1)

So, the condition is:

onesInRange + (r - l +1) <= sum_{j=l to r} c_j - (r - l +1)

Which is:

onesInRange + 2*(r - l +1) <= sum_{j=l to r} c_j

But according to my earlier analysis, the condition should be onesInRange <= floor((r - l +1)/2)

Hence, these seem different.

Wait, perhaps there's a relationship between sum_{j=l to r} c_j and onesInRange.

Alternatively, perhaps I need to consider that for the array to be good, not only the sum condition but also the possibility to adjust b_i such that sum_b = sum_a.

Wait, perhaps I need to consider that in addition to the count_of_ones <= floor(m /2), there should be enough "room" in the other elements to adjust the sum.

Wait, but in the earlier examples, it seemed that count_of_ones <= floor(m /2) was sufficient.

But perhaps there are cases where this is not enough.

Looking back at the sample input:

n=5, q=4

a=[1,2,1,4,5]

Queries:

1. l=1, r=5, m=5, count_of_ones=2, floor(5/2)=2, 2<=2, YES

2. l=4, r=4, m=1, count_of_ones=0, m=1, always NO

3. l=3, r=4, m=2, count_of_ones=1, 1<=1, YES

4. l=1, r=3, m=3, count_of_ones=2, 2>1, NO

Which matches the sample output.

Hence, perhaps the condition is sufficient.

But in the code, it's checking onesInRange + (r - l +1) <= sum_{j=l to r} c_j - (r - l +1)

Which seems more restrictive.

Wait, perhaps I need to see if sum_{j=l to r} c_j >= onesInRange + 2*(r - l +1)

Because sum_{j=l to r} c_j - (r - l +1) >= onesInRange + (r - l +1)

Which is sum_{j=l to r} c_j >= onesInRange + 2*(r - l +1)

But I'm not sure why this would be necessary.

Perhaps there's a different way to approach this.

Alternatively, maybe I need to consider that for each one in the subarray, I need to increase it by at least 1, and for others, I can decrease them by at most 1.

Hence, the total sum increase needed is count_of_ones * 1, and the total sum decrease possible is (m - count_of_ones) *1.

Hence, to make sum_b = sum_a, I need sum_a + increase - decrease = sum_a

Which implies increase = decrease.

But increase is at least count_of_ones *1, and decrease is at most (m - count_of_ones)*1.

Hence, count_of_ones <= m - count_of_ones

Which simplifies to 2 * count_of_ones <= m

Which is count_of_ones <= floor(m /2)

Hence, this confirms my earlier condition.

Therefore, the condition is count_of_ones <= floor(m /2)

Hence, the code should be implementing this condition.

But in the given code, it's checking onesInRange + (r - l +1) <= sumInRange

Where sumInRange = sum_{j=l to r} c_j - (r - l +1)

Hence, the condition in the code is:

onesInRange + (r - l +1) <= sum_{j=l to r} c_j - (r - l +1)

Which is sum_{j=l to r} c_j >= onesInRange + 2*(r - l +1)

But according to my analysis, it should be onesInRange <= floor((r - l +1)/2)

Hence, the code seems to be implementing a different condition.

Wait, perhaps these two conditions are equivalent under certain circumstances.

Let me see.

If onesInRange <= floor(m /2), then sum_{j=l to r} c_j >= sum_{j=l to r} 1 + 2*(m - floor(m /2))

Wait, that seems convoluted.

Alternatively, perhaps the code is incorrect.

Wait, in the sample input, for the first query, sum_{1 to 5} c_j =1+2+1+4+5=13

sumInRange =13 -5=8

onesInRange=2

m=5

Check: 2 +5 <=8, which is 7 <=8, which is true, so YES.

Second query: m=1, skip.

Third query: sum_{3 to4} c_j=1+4=5, sumInRange=5-2=3

onesInRange=1

Check:1 +4 <=3, which is 5 <=3, false, so NO.

But according to my earlier analysis, it should be YES.

Wait, but m=2, floor(2/2)=1, onesInRange=1 <=1, should be YES, but according to the code, it's NO.

Hence, the code is incorrect.

Hence, the given code is incorrect.

Hence, Correctness: False

**Final Solution**

To solve this problem, we need to determine if a given subarray is "good" based on specific conditions. An array is considered good if there exists another array `b` with certain properties related to the original array `a`.

### Approach

1. **Understanding the Problem:**
   - We need to check if the subarray `c[l..r]` is good.
   - For the subarray to be good:
     - The sum of elements in `a` should equal the sum of elements in `b`.
     - Each element in `b` should be different from the corresponding element in `a`.
     - All elements in `b` should be positive integers.

2. **Key Insight:**
   - To minimize the sum of `b`, set `b_i = a_i - 1` if `a_i > 1`, otherwise `b_i = a_i + 1`.
   - Calculate the minimal possible sum of `b` and check if it is less than or equal to the sum of `a`.

3. **Efficient Calculation:**
   - Precompute prefix sums for the count of ones and the sum of elements adjusted by -1.
   - For each query, compute the count of ones and the adjusted sum in the subarray.
   - Check if the count of ones is less than or equal to half the length of the subarray (floor division).

4. **Edge Cases:**
   - Subarrays of length 1 are always "NO" because `b_i` cannot equal `a_i`.

### Solution Code

```python
def main():
    import sys
    input = sys.stdin.read
    data = input().split()
    
    idx = 0
    t = int(data[idx])
    idx += 1
    for _ in range(t):
        n = int(data[idx])
        q = int(data[idx + 1])
        idx += 2
        c = list(map(int, data[idx:idx + n]))
        idx += n
        ones = [0] * (n + 1)
        sum_adj = [0] * (n + 1)
        for i in range(1, n + 1):
            ones[i] = ones[i - 1] + (1 if c[i - 1] == 1 else 0)
            sum_adj[i] = sum_adj[i - 1] + (c[i - 1] - 