Output State: `total` is 0, `l` is `n - 3 - (n - 4)`, `r` is `n - 2 - (n - 4)`, `a` is a list of integers where `a[1] == a[2]` and `a[2] == a[3]` and so on until `a[n-4] == a[n-3]`, `le` is the length of list `a`, `st` is `-2`, `end` is `n - 3`, `ans` is `-1`.

Explanation: After the loop has executed all its iterations, `l` will be `n - 3 - (n - 4) = 1` and `r` will be `n - 2 - (n - 4) = 2`. The loop condition `r > l` will no longer hold true because `r` becomes 2 and `l` becomes 1, but since `a[r] == a[r - 1]` was the condition for decrementing `r` and incrementing `end`, the loop has terminated. At this point, `st` remains `-2` and `end` is `n - 3`. The value of `ans` remains `-1` as it does not change within the loop.