The code `s += s // (k - 1) + 1` updates the value of `s` based on its current value and the value of `k`.

1. **Initial Values:**
   - `t` is an integer such that 1 ≤ t ≤ 1000
   - `k` is an integer
   - `x` must be greater than 1
   - `a` is an integer
   - `s` is 2
   - `i` is 1

2. **Code Execution:**
   - `s` is initially 2.
   - The expression `s // (k - 1)` performs integer division of `s` by `(k - 1)`.
   - The result of `s // (k - 1)` is added to 1.
   - This sum is then added to the current value of `s`.

3. **Calculation:**
   - Let's denote the new value of `s` as `s_new`.
   - `s_new = s + (s // (k - 1)) + 1`
   - Substituting the initial value of `s` (which is 2):
     - `s_new = 2 + (2 // (k - 1)) + 1`
   - Simplifying further:
     - `s_new = 3 + (2 // (k - 1))`

4. **Impact on Variables:**
   - `s` is updated to `3 + (2 // (k - 1))`.
   - All other variables (`t`, `k`, `x`, `a`, `i`) remain unchanged.

5. **Output State:**
   - `t` is an integer such that 1 ≤ t ≤ 1000
   - `k` is an integer
   - `x` must be greater than 1
   - `a` is an integer
   - `s` is `3 + (2 // (k - 1))`
   - `i` is 1

Output State: **`t` is an integer such that 1 ≤ t ≤ 1000, `k` is an integer, `x` must be greater than 1, `a` is an integer, `s` is `3 + (2 // (k - 1))`, `i` is 1**