To determine what will be printed by the given `print` statement, let's break down the initial state and the logic step by step:

### Initial State:
- `t` is an integer such that \(1 \leq t \leq 1000\).
- `k` is an integer.
- `x` is an integer.
- `a` is an integer.
- `s` is the result of the expression: 
  \[
  s = 1 + \sum_{i=0}^{x-1} \left( \frac{s}{k-1} + 1 \right)
  \]
- `i` is `x - 1`.

### Step-by-Step Analysis:
1. **Expression for `s`:**
   - The expression for `s` is:
     \[
     s = 1 + \sum_{i=0}^{x-1} \left( \frac{s}{k-1} + 1 \right)
     \]
   - This is a recursive formula where `s` depends on itself. To simplify, let's consider the sum part:
     \[
     \sum_{i=0}^{x-1} \left( \frac{s}{k-1} + 1 \right)
     \]
   - Each term in the sum is \(\frac{s}{k-1} + 1\), and there are `x` such terms:
     \[
     \sum_{i=0}^{x-1} \left( \frac{s}{k-1} + 1 \right) = x \left( \frac{s}{k-1} + 1 \right)
     \]
   - Substituting this back into the expression for `s`:
     \[
     s = 1 + x \left( \frac{s}{k-1} + 1 \right)
     \]
   - Simplifying further:
     \[
     s = 1 + x \cdot \frac{s}{k-1} + x
     \]
     \[
     s = 1 + x + x \cdot \frac{s}{k-1}
     \]
     \[
     s = 1 + x + \frac{x \cdot s}{k-1}
     \]
   - Rearranging to solve for `s`:
     \[
     s - \frac{x \cdot s}{k-1} = 1 + x
     \]
     \[
     s \left( 1 - \frac{x}{k-1} \right) = 1 + x
     \]
     \[
     s = \frac{1 + x}{1 - \frac{x}{k-1}}
     \]
     \[
     s = \frac{(1 + x)(k-1)}{k-1 - x}
     \]

2. **Condition in the `print` Statement:**
   - The `print` statement checks if `a` is greater than or equal to `s`:
     \[
     \text{print('YES' if } a \geq s \text{ else 'NO')}
     \]
   - We need to compare `a` with the value of `s` calculated above.

### Final Output:
- The output will be either 'YES' or 'NO' depending on whether `a` is greater than or equal to the calculated value of `s`.
- Since the exact values of `a`, `k`, and `x` are not provided, we cannot compute the exact numerical value of `s`. However, the output will be determined by the comparison of `a` with the value of `s` derived from the formula.

Output: **'YES' if \( a \geq \frac{(1 + x)(k-1)}{k-1 - x} \) else 'NO' (where \( s = \frac{(1 + x)(k-1)}{k-1 - x} \))**