Alright, I have this problem to solve. Let's read it carefully.

So, there are n items in a shop, each with two parameters: a_i and b_i. Alice wants to choose a subset of these items to buy, and then Bob will take some of them for free or pay for them based on certain conditions.

Let me try to understand the rules:

1. Alice selects a subset of items to buy.

2. Bob then does one of two things:

   a. If Alice bought less than k items, Bob takes all of them for free.

   b. If Alice bought k or more items, Bob takes k items for free that Alice bought, and pays for the rest.

3. Alice's profit is the amount Bob pays her minus the amount she spent buying the items.

Alice wants to maximize her profit, and Bob wants to minimize Alice's profit. I need to find Alice's profit when both act optimally.

First, I need to model this situation mathematically.

Let's denote:

- S: the set of items Alice buys.

- T: the set of items Bob buys from Alice (pays for).

Given the rules:

- If |S| < k, Bob takes all of S for free, so T = empty set.

- If |S| >= k, Bob takes k items for free and pays for the remaining |S| - k items.

So, Alice's profit is:

Profit = sum_{i in T} b_i - sum_{j in S} a_j

Bob wants to minimize this profit, so he will choose which k items to take for free to minimize what he has to pay.

Alice needs to choose S to maximize the profit, considering that Bob will act to minimize it.

This seems like a minimax problem.

Let me think about this step by step.

Case 1: |S| < k

- Bob takes all items for free.

- T = empty set.

- Profit = 0 - sum_{j in S} a_j = -sum_{j in S} a_j

Since a_j >= 1, this profit is negative or zero.

Case 2: |S| >= k

- Bob takes k items for free and pays for |S| - k items.

- Bob will choose which k items to take for free to minimize what he has to pay.

- Specifically, Bob will choose the k items with the smallest b_i to take for free, leaving Alice with the items having the largest b_i to sell.

So, in this case, the items in T are the |S| - k items with the largest b_i.

Therefore, Alice's profit is:

sum of the largest (|S| - k) b_i's - sum of all a_j for j in S.

Alice needs to choose S to maximize this expression.

This seems complex because the profit depends on both a_j and b_i in a coupled way.

Let me try to reformulate this.

Let me consider the combined gain for each item: b_i - a_i.

If Alice buys an item, she spends a_i and may gain b_i from Bob.

But Bob gets to choose which k items to take for free, so he will choose the items with the smallest b_i to minimize what he has to pay.

Wait, perhaps I need to think differently.

Let me consider that for items Alice includes in S:

- She pays a_i.

- If Bob doesn't take it for free, he pays b_i.

So, Alice's profit for each item in S is:

- If Bob takes it for free: -a_i

- If Bob pays for it: b_i - a_i

Bob will choose which k items to take for free to minimize Alice's profit.

So, for a given S, Bob will select the k items with the smallest b_i to take for free.

Then, Alice's profit is:

sum_{i in S} (b_i - a_i) - 2 * sum_{i in T} a_i

Wait, that might not be accurate.

Let me think again.

For each item in S:

- Alice pays a_i.

- If Bob takes it for free, Alice gets nothing back.

- If Bob pays for it, Alice gets b_i.

So, Alice's profit is:

sum_{i in T} b_i - sum_{j in S} a_j

Where T is the set of items Bob pays for.

Given that T = S - the k items Bob takes for free.

So, T = S - K, where K is the set of k items Bob takes for free.

Bob will choose K to minimize Alice's profit, meaning he will choose the k items with the smallest b_i in S.

Therefore, T consists of the items in S with the largest b_i, excluding the k smallest b_i.

Wait, more precisely:

- Bob takes the k items with the smallest b_i in S for free.

- Alice sells the remaining |S| - k items with the largest b_i in S.

So, Alice's profit is:

sum_{i in S - K} b_i - sum_{j in S} a_j

Where K is the set of k items in S with the smallest b_i.

Bob chooses K to minimize this profit.

Alice chooses S to maximize the profit given that Bob chooses K optimally.

This is equivalent to:

Alice chooses S to maximize [sum_{i in S} (b_i - a_i) - sum_{k smallest b_i in S} (-a_i)]

Wait, perhaps I need to approach this differently.

Let me consider the following:

Define c_i = b_i - a_i

Then, Alice's profit can be written as:

sum_{i in T} c_i + sum_{i in T} a_i - sum_{j in S} a_j

Wait, that seems off.

Wait, let's directly write:

Profit = sum_{i in T} b_i - sum_{j in S} a_j

Where T = S - K, and K is the set of k items in S with the smallest b_i.

So, T consists of the items in S without the k items having the smallest b_i.

Thus, Profit = sum_{i in S} b_i - sum_{i in K} b_i - sum_{j in S} a_j

Simplify:

Profit = sum_{i in S} (b_i - a_i) - sum_{i in K} b_i

Bob chooses K to minimize this profit, i.e., to minimize sum_{i in K} b_i

Since K is the set of k smallest b_i in S, sum_{i in K} b_i is the sum of the k smallest b_i in S.

Therefore, Profit = sum_{i in S} (b_i - a_i) - sum_{i in K} b_i

Alice wants to maximize this profit by choosing S.

Wait, perhaps I can rearrange this.

Let me denote:

sum_{i in S} (b_i - a_i) - sum_{i in K} b_i = sum_{i in S} (-a_i) + sum_{i in S} b_i - sum_{i in K} b_i

Wait, that seems messy.

Let me think differently.

Let me consider that for each item in S, Alice pays a_i and gets b_i if Bob pays for it.

But Bob will take the k items with the smallest b_i for free.

So, the items in S with the smallest b_i are taken for free by Bob, and the remaining items are paid by Bob.

Therefore, Alice's profit is:

sum_{i in S - K} b_i - sum_{j in S} a_j

Where K is the set of k items in S with the smallest b_i.

So, to maximize this, Alice needs to choose S such that the sum of b_i for the items not in K minus the sum of a_j for all items in S is maximized.

This seems tricky.

Perhaps I can sort the items based on b_i and try to select the best items for Alice.

Wait, maybe I should consider the difference b_i - a_i and sort accordingly.

Wait, perhaps I need to consider the items in decreasing order of b_i - a_i.

Wait, perhaps dynamic programming is needed, but n can be up to 2e5, so DP might not be efficient.

Wait, maybe I can greedily select items based on some criteria.

Let me consider that Alice wants to maximize profit, which is sum of b_i for the items Bob pays for minus sum of a_i for all items she buys.

Bob, in turn, wants to minimize this profit by choosing which k items to take for free.

So, for a given S, Bob will choose the k items with the smallest b_i to take for free, leaving Alice with the items having the largest b_i.

Therefore, for a given S, Alice's profit is sum of the (|S| - k) largest b_i in S minus sum of a_i for all items in S.

Alice needs to choose S to maximize this expression.

This seems complex, but perhaps there is a way to optimize this selection.

Let me consider sorting the items based on b_i in descending order.

If Alice selects the top |S| items with the largest b_i, then the (|S| - k) largest b_i would be the first (|S| - k) items in this sorted list.

Wait, perhaps I can iterate over possible sizes of S starting from k up to n and compute the profit for each possible size.

Wait, but n can be up to 2e5, so this needs to be efficient.

Let me think about the following approach:

- Sort the items in decreasing order of b_i.

- Then, for a given size m = |S|, the (m - k) largest b_i are the first (m - k) items in the sorted list.

- The sum of b_i for T would be sum of the first (m - k) b_i.

- The sum of a_j for S would be sum of a_j for the first m items.

- So, profit for a given m is sum_{i=1 to m - k} b_i - sum_{j=1 to m} a_j

- Alice needs to choose m to maximize this profit.

Wait, but this might not be entirely correct because the sets S can be any subset of items, not necessarily the top m items.

However, since Bob will take the k smallest b_i in S for free, by choosing the top m items, the k smallest b_i would be the m - k to m items in the sorted list.

Wait, perhaps I need to adjust this.

Let me try to formalize this.

Suppose I sort the items in decreasing order of b_i.

Let's index them from 1 to n, where item 1 has the largest b_i, item 2 has the next largest, and so on.

For a given m, if Alice chooses the top m items, then the k smallest b_i in S would be the m - k to m items.

Wait, more precisely, the k smallest b_i in the top m items are the m - k +1 to m items.

Therefore, the sum of b_i for T would be sum of the first m - k items.

The sum of a_j for S would be sum of a_j for the first m items.

Therefore, profit = sum_{i=1 to m - k} b_i - sum_{j=1 to m} a_j

Alice needs to choose m to maximize this profit.

But, she can also choose any other subset of m items, not necessarily the top m.

However, intuitively, choosing the top m items seems optimal because we want the largest possible b_i in T.

Wait, but need to confirm this.

Assume that Alice chooses any other subset of m items, but since Bob will take the k smallest b_i in S for free, choosing the top m items seems still optimal.

Because, in any other subset, the (m - k) largest b_i might be smaller than those in the top m.

Wait, perhaps it's not straightforward.

Let me consider a small example.

Take the first test case:

n=2, k=0

a=[2,1]

b=[1,2]

If Alice chooses both items:

Bob takes 0 items for free (since k=0), so he pays for both items.

Profit = 2 + 1 - (2 + 1) = 0

If Alice chooses only the second item:

Bob takes 0 items for free, pays for the second item.

Profit = 2 - 1 = 1

If Alice chooses only the first item:

Bob takes 0 items for free, pays for the first item.

Profit = 1 - 2 = -1

So, the maximum profit is 1.

Which matches the sample output.

In this case, choosing the single item with the highest b_i - a_i = 2 -1 =1 is better than choosing both items.

Wait, b_i - a_i for item 1: 1 - 2 = -1

For item 2: 2 -1 =1

So, choosing the item with positive b_i - a_i is better.

Wait, but in this case, k=0, so Bob takes no items for free.

So, profit = sum_{i in S} (b_i - a_i)

Alice should choose the items where b_i - a_i >0.

Wait, perhaps in the case where k=0, it's straightforward: choose the items where b_i - a_i >0, and maximize the sum of (b_i - a_i).

But in general, when k >0, it's more complicated.

Wait, perhaps I can generalize this.

Let me consider that when k=0, Alice should choose the items where b_i - a_i >0, and maximize the sum of (b_i - a_i).

When k >=1, it's different because Bob takes k items for free, choosing the ones with smallest b_i.

Wait, perhaps I can consider that Alice should choose items where b_i - a_i >0, and ensure that the k smallest b_i in S are as large as possible.

Wait, I'm getting confused.

Let me consider another approach.

Let me consider that Alice's profit is:

sum_{i in T} b_i - sum_{j in S} a_j

Where T = S - K, and K is the set of k items in S with the smallest b_i.

So, profit = sum_{i in S} b_i - sum_{i in K} b_i - sum_{j in S} a_j

Rearranged:

profit = sum_{i in S} (b_i - a_i) - sum_{i in K} b_i

Alice wants to maximize this profit.

Bob chooses K to minimize this profit.

Wait, perhaps I can consider that for a given S, Bob chooses K to minimize sum_{i in K} b_i, which is equivalent to choosing the k smallest b_i in S.

Therefore, for a given S, profit = sum_{i in S} (b_i - a_i) - sum_{i in K} b_i

Alice wants to maximize this over all possible S.

Wait, perhaps I can rearrange this expression.

Let me see:

profit = sum_{i in S} (b_i - a_i) - sum_{i in K} b_i

= sum_{i in S - K} b_i - sum_{j in S} a_j

Wait, same as before.

Alternatively, perhaps I can consider:

profit = sum_{i in S} (b_i - a_i) - sum_{i in K} b_i

= sum_{i in S} (-a_i) + sum_{i in S} b_i - sum_{i in K} b_i

= sum_{i in S} (-a_i) + sum_{i in S - K} b_i

Which is the same as the original profit formula.

This seems too circular.

Let me try to think differently.

Suppose Alice chooses a set S of size m >=k.

Bob will take the k items with the smallest b_i in S for free.

Therefore, the profit is sum of (b_i - a_i) for the items in S except the k items with the smallest b_i.

Wait, more precisely:

sum_{i in S} (b_i - a_i) - sum_{i in K} b_i

Where K is the set of k items in S with the smallest b_i.

So, profit = sum_{i in S} (b_i - a_i) - sum_{i in K} b_i

= sum_{i in S - K} b_i - sum_{j in S} a_j

Wait, same as before.

Let me try to find a way to compute this efficiently.

Perhaps I can sort the items in decreasing order of b_i.

Then, for a given m >=k, the sum of the (m -k) largest b_i is sum of the first (m -k) b_i in the sorted list.

The sum of a_j for S is sum of the first m a_j in the sorted list.

Therefore, profit for this S is sum_{i=1 to m -k} b_i - sum_{j=1 to m} a_j

Alice needs to choose m to maximize this profit.

But, perhaps she can also choose subsets that are not the top m items, but some other combination.

However, intuitively, choosing the top m items seems optimal.

Let me verify this with the second test case.

Second test case:

n=4, k=1

a=[1,2,1,4]

b=[3,3,2,3]

Sort items by b_i descending: items with b=3,3,3,2

Indices: 1,2,4,3

Sum of first (m -k) b_i: for m=1, m -k=0, sum=0; m=2, m -k=1, sum=3; m=3, m -k=2, sum=3+3=6; m=4, m -k=3, sum=3+3+3=9

Sum of first m a_j: m=1, sum=1; m=2, sum=1+2=3; m=3, sum=1+2+1=4; m=4, sum=1+2+1+4=8

Profit: m=1: 0 -1 = -1

m=2:3 -3=0

m=3:6 -4=2

m=4:9 -8=1

So, maximum profit is 2.

But according to the sample output, it's 1.

Wait, perhaps I'm missing something.

Wait, in the sample explanation, it says Alice buys items 1,2,3 and Bob takes item 1 for free, paying for items 2 and 3.

Profit = 3 + 2 - (1 + 2 +1) = 5 - 4 =1

Alternatively, if Alice buys items 1,2,3,4, Bob can take item 3 for free (b=2 is smallest), and pay for items 1,2,4.

Profit = 3 +3 +3 - (1 +2 +1 +4) =9 - 8=1

So, in both cases, profit is 1.

But according to my earlier calculation, choosing m=3 should give profit=2, but sample output is 1.

So, perhaps my approach is incorrect.

Wait, maybe I need to consider that when m >=k, Bob chooses which k items to take for free, and he will choose the items with the smallest b_i to minimize Alice's profit.

Therefore, in the case where m=3, Alice chooses items 1,2,3.

Bob will take the item with the smallest b_i among them, which is item 3 (b=2), for free.

Therefore, Alice's profit is (b1 + b2) - (a1 + a2 + a3) = (3 +3) - (1 +2 +1) =6 -4=2

But according to the sample explanation, profit is 1.

Wait, perhaps I'm misunderstanding something.

Wait, in the sample explanation, it says Alice buys items 1,2,3, and Bob takes item 1 for free, paying for items 2 and 3.

Wait, but according to the rules, Bob should take the k items with the smallest b_i for free.

Wait, no, Bob chooses which k items to take for free to minimize Alice's profit.

So, in this case, if Alice chooses items 1,2,3:

Bob can choose to take item 3 for free (smallest b_i=2), and pay for items 1 and 2.

Profit = b1 + b2 - (a1 + a2 + a3) =3 +3 - (1 +2 +1)=5 -4=1

Alternatively, Bob could choose to take item 2 for free (b=3), and pay for items 1 and 3.

Profit = b1 + b3 - (a1 + a2 + a3)=3 +2 - (1 +2 +1)=5 -4=1

Or take item 1 for free (b=3), pay for items 2 and 3.

Profit = b2 + b3 - (a1 + a2 + a3)=3 +2 - (1 +2 +1)=5 -4=1

So, in all cases, profit is 1.

But earlier, I thought that profit could be 2, but that was incorrect because I assumed Bob would take the smallest b_i, but actually, Bob can choose which k items to take for free to minimize Alice's profit.

Wait, but in this case, taking any item for free results in the same profit.

Wait, but in the earlier calculation, if Alice chooses items 1,2,3, and Bob takes item 3 for free, profit is 1.

If Alice chooses items 1,2,3,4, and Bob takes item 3 for free, profit is 1.

If Alice chooses only items 2 and 4:

Bob takes the smallest b_i, which is b=3 for item 2 or 4.

Wait, both have b=3.

So, Bob takes one of them for free, say item 2.

Then, Alice's profit is b4 - (a2 + a4)=3 - (2 +4)=3 -6=-3

Alternatively, if Bob takes item 4 for free, profit is b2 - (a2 + a4)=3 -6=-3

Worse for Alice.

So, indeed, choosing items 1,2,3 gives profit 1, which matches the sample.

Therefore, my earlier approach was incorrect.

So, perhaps I need to reconsider.

Let me think differently.

Let me consider that Alice's profit is:

sum_{i in S - K} b_i - sum_{j in S} a_j

Where K is the set of k items in S with the smallest b_i.

I need to maximize this over all possible S.

This seems tricky.

Perhaps I can consider the following approach:

- Sort the items in decreasing order of b_i.

- Then, for m from k to n, compute profit as sum of the first (m -k) b_i minus sum of the first m a_j.

- Choose the maximum among these profits.

Wait, in the second test case, for m=3:

sum of first (3-1)=2 b_i: b1 + b2=3+3=6

sum of first 3 a_j: a1 + a2 + a3=1 +2 +1=4

profit=6 -4=2

But according to the sample, it's 1.

So, perhaps this approach is incorrect.

Wait, perhaps I need to adjust for the fact that Bob can choose which k items to take for free, not necessarily the k smallest b_i in S.

Wait, no, the problem says Bob chooses which k items to take for free to minimize Alice's profit.

So, he will choose the k items with the smallest b_i in S.

Therefore, in the earlier calculation, for m=3, sum of (m -k)=2 largest b_i is 3+3=6, sum of first m a_j is 1+2+1=4, profit=2.

But according to the sample, it's 1.

So, perhaps there is a mistake in assuming that Bob takes the k smallest b_i.

Wait, no, in the sample, even though m=3, sum of (m -k)=2 largest b_i is 3+3=6, sum of a_j for m=3 is 1+2+1=4, profit=2.

But in reality, profit is 1.

So, perhaps this approach is incorrect.

Wait, perhaps I need to consider that when m >=k, profit is sum_{i in S} (b_i - a_i) - sum_{i in K} b_i

Where K is the set of k items in S with the smallest b_i.

So, profit = sum_{i in S} (b_i - a_i) - sum_{i in K} b_i

= sum_{i in S - K} b_i - sum_{j in S} a_j

In the sample, for S={1,2,3}, sum_{i in S} (b_i - a_i)= (3-1) + (3-2) + (2-1)=2 +1 +1=4

sum_{i in K} b_i=2 (the smallest b