Based on the initial state provided:

- `t` is an integer such that \(1 \leq t \leq 676\). This value is not relevant to the print statement.
- `i` is 0.
- `n` is the first integer input by the user.
- `k` is the second integer input by the user and `k` is not equal to 1.
- `s` is the string 'aaaaaaaaa'.
- `j` is 105.

The print statement is:
```python
print((2 - (n == 1)) * s)
```

Let's break it down step by step:

1. The expression `(n == 1)` checks if `n` is equal to 1. If `n` is 1, this expression evaluates to `True`, which is equivalent to `1` in Python. If `n` is not 1, it evaluates to `False`, which is equivalent to `0`.

2. The expression `2 - (n == 1)` subtracts the result of `(n == 1)` from 2. If `n` is 1, then `2 - (n == 1)` becomes `2 - 1 = 1`. If `n` is not 1, then `2 - (n == 1)` becomes `2 - 0 = 2`.

3. The result of `2 - (n == 1)` is then multiplied by the string `s` ('aaaaaaaaa'). If `n` is 1, the result is `1 * 'aaaaaaaaa' = 'aaaaaaaaa'`. If `n` is not 1, the result is `2 * 'aaaaaaaaa' = 'aaaaaaaaa'aaaaaaa`.

Therefore, regardless of the value of `n` (as long as it is not 1), the string `s` will be repeated either once or twice.

Output: **'aaaaaaaaa'aaaaaaa**