In the given initial state, we have the following variables:

- `n` is an input positive integer (1 ≤ n ≤ 100).
- `pos` is an input integer (1 ≤ pos ≤ n).
- `l` is an input positive integer (1 ≤ l ≤ r ≤ n).
- `r` is an input positive integer (1 ≤ r ≤ n).
- `ans` is initialized to 0.
- The current value of `pos` is greater than `r`.

The code `ans += pos - r` modifies the variable `ans`. 

Calculating the new value of `ans`:
- Since `ans` was initially 0, the new value of `ans` will be `0 + (pos - r)`, which simplifies to `ans = pos - r`.

Output State: **`n` is an input positive integer (1 ≤ n ≤ 100), `pos` is an input integer (1 ≤ pos ≤ n), `l` is an input positive integer (1 ≤ l ≤ r ≤ n), `r` is an input positive integer (1 ≤ r ≤ n), `ans` is equal to `pos - r` and the current value of `pos` is greater than `r`.**