The code updates the value of `dp[n, k]` by adding `9 * 10 ** (i - 1) * (10 ** (k - i) - 10 ** (i - 1))`. Here, `i` is 1 and `k` is a positive integer such that `1 <= k <= 10`. The value of `n` must be greater than or equal to \(10^k\).

Let's substitute the known values into the expression:

1. Since `i` is 1, `10 ** (i - 1)` becomes `10 ** 0` which is 1.
2. The expression simplifies to `9 * 1 * (10 ** (k - 1) - 10 ** 0) = 9 * (10 ** (k - 1) - 1)`.

So, `dp[n, k]` is updated by adding `9 * (10 ** (k - 1) - 1)` to its current value.

The output state is: `i` is 1, `k` is a positive integer such that `1 <= k <= 10`, `n` must be greater than or equal to \(10^k\), and `dp[n, k]` is increased by `9 * (10 ** (k - 1) - 1)`.
Output State: **`i` is 1, `k` is a positive integer such that `1 <= k <= 10`, `n` must be greater than or equal to \(10^k\), `dp[n, k]` is increased by `9 * (10 ** (k - 1) - 1)`**.