Let's analyze the given code and the initial state step by step.

### Initial State:
- `n` is an integer such that \( n \geq 10^k \)
- `k` is a positive integer such that \( 1 \leq k \leq 10 \)
- `dp` is a dictionary used for memoization
- The key `(n, k)` exists in the dictionary `dp` with the value 9

### Code of the Loop:
```python
for i in range(1, k):
    dp[n, k] += 9 * 10 ** (i - 1) * (10 ** (k - i) - 10 ** (i - 1))
```

### Step-by-Step Analysis:

1. **Analyze the Loop**:
   - The loop runs from `i = 1` to `i = k-1`.
   - In each iteration, the value of `dp[n, k]` is updated by adding `9 * 10 ** (i - 1) * (10 ** (k - i) - 10 ** (i - 1))`.

2. **Track Variable Changes**:
   - `n` remains unchanged because it is only used as the key in the dictionary `dp`.
   - `k` remains unchanged because it is the upper limit of the loop and is not modified within the loop.
   - `dp[n, k]` is updated in each iteration based on the formula `9 * 10 ** (i - 1) * (10 ** (k - i) - 10 ** (i - 1))`.

3. **Summarize the Loop Behavior**:
   - The loop updates `dp[n, k]` by summing up the contributions from each iteration.
   - Each contribution is calculated as `9 * 10 ** (i - 1) * (10 ** (k - i) - 10 ** (i - 1))`.
   - For example:
     - When `i = 1`, the contribution is `9 * 10 ** 0 * (10 ** (k - 1) - 10 ** 0) = 9 * (10 ** (k - 1) - 1)`.
     - When `i = 2`, the contribution is `9 * 10 ** 1 * (10 ** (k - 2) - 10 ** 1) = 90 * (10 ** (k - 2) - 10)`.
     - And so on.

4. **Verify Relationships**:
   - After `k-1` iterations, the final value of `dp[n, k]` will be the sum of all contributions from `i = 1` to `i = k-1`.
   - The final value of `dp[n, k]` can be expressed as:
     \[
     dp[n, k] = 9 \sum_{i=1}^{k-1} 10^{i-1} \cdot (10^{k-i} - 10^{i-1})
     \]
   - Simplifying the summation:
     \[
     dp[n, k] = 9 \sum_{i=1}^{k-1} (10^{k-1} - 10^{2(i-1)})
     \]
     \[
     dp[n, k] = 9 \left[ (k-1) \cdot 10^{k-1} - \sum_{i=1}^{k-1} 10^{2(i-1)} \right]
     \]
     \[
     dp[n, k] = 9 \left[ (k-1) \cdot 10^{k-1} - \frac{10^2 - 10^{2(k-1)}}{10^2 - 1} \right]
     \]
     \[
     dp[n, k] = 9 \left[ (k-1) \cdot 10^{k-1} - \frac{10^2 - 10^{2(k-1)}}{99} \right]
     \]

### Final Output State:
After the loop has executed all `k-1` iterations, the values of `n` and `k` remain unchanged, and the value of `dp[n, k]` is updated according to the derived formula.

Output State: **`n` is an integer such that \( n \geq 10^k \), `k` is a positive integer such that \( 1 \leq k \leq 10 \), and `dp[n, k]` is updated to \( 9 \left[ (k-1) \cdot 10^{k-1} - \frac{10^2 - 10^{2(k-1)}}{99} \right]`.**