To determine the output state, let's analyze the given code and its impact on the variables:

### Initial State:
- `n` and `m` are positive integers such that \(1 \leq n, m \leq 2 \times 10^6\) and \(n \geq 6\) and \(m \geq 3\).
- `x` is 2.
- `y` is 1.
- `cnt` is the sum of `min(n / ((x + y) * x), m // ((x + y) * y))` for all pairs of `x` and `y` where `math.gcd(x, y) == 1` and the conditions \((x + y) * x <= n\) and \((x + y) * y <= m\) are satisfied. Additionally, the greatest common divisor of `x` and `y` is 1.

### Code Execution:
```
cnt += min(n / ((x + y) * x), m // ((x + y) * y))
```

### Step-by-Step Analysis:
1. **Calculate \(x + y\):**
   - \(x = 2\)
   - \(y = 1\)
   - \(x + y = 2 + 1 = 3\)

2. **Calculate \((x + y) * x\):**
   - \((x + y) * x = 3 * 2 = 6\)

3. **Calculate \((x + y) * y\):**
   - \((x + y) * y = 3 * 1 = 3\)

4. **Check the conditions:**
   - \((x + y) * x \leq n\): \(6 \leq n\) (since \(n \geq 6\), this condition is satisfied).
   - \((x + y) * y \leq m\): \(3 \leq m\) (since \(m \geq 3\), this condition is satisfied).

5. **Calculate the minimum value:**
   - \(n / ((x + y) * x) = n / 6\)
   - \(m // ((x + y) * y) = m // 3\)
   - `min(n / 6, m // 3)`

6. **Update `cnt`:**
   - `cnt` is initially the sum of `min(n / ((x + y) * x), m // ((x + y) * y))` for all valid pairs of `x` and `y`.
   - After executing the code, `cnt` is incremented by `min(n / 6, m // 3)`.

### Output State:
- `n` and `m` remain positive integers such that \(1 \leq n, m \leq 2 \times 10^6\) and \(n \geq 6\) and \(m \geq 3\).
- `x` is 2.
- `y` is 1.
- `cnt` is now the initial value of `cnt` plus `min(n / 6, m // 3)`.

Output State: **`n` and `m` remain positive integers such that \(1 \leq n, m \leq 2 \times 10^6\) and \(n \geq 6\) and \(m \geq 3\), `x` is 2, `y` is 1, and `cnt` is the initial value of `cnt` plus `min(n / 6, m // 3)`.**