The code snippet updates the value of `cnt` by adding the minimum of two expressions: `n / ((x + y) * x)` and `m // ((x + y) * y)`. Let's break down the calculation:

1. **Initial Values:**
   - `n` is a positive integer such that \(12 \leq n \leq 2 \times 10^6\)
   - `m` is a positive integer such that \(4 \leq m \leq 2 \times 10^6\)
   - `x` is 3
   - `y` is 2
   - `cnt` remains unchanged (let's denote its initial value as `cnt_initial`)

2. **Expression Calculation:**
   - First, calculate `(x + y) * x`:
     \[
     (x + y) * x = (3 + 2) * 3 = 5 * 3 = 15
     \]
   - Second, calculate `(x + y) * y`:
     \[
     (x + y) * y = (3 + 2) * 2 = 5 * 2 = 10
     \]

3. **Evaluate the Two Expressions:**
   - First expression: `n / 15`
   - Second expression: `m // 10`

4. **Determine the Minimum:**
   - The value added to `cnt` will be the minimum of `n / 15` and `m // 10`.

5. **Update `cnt`:**
   - `cnt` is updated to `cnt_initial + min(n / 15, m // 10)`

Therefore, the output state is:
Output State: **`n` is a positive integer such that \(12 \leq n \leq 2 \times 10^6\), `m` is a positive integer such that \(4 \leq m \leq 2 \times 10^6\), `x` is 3, `y` is 2, `cnt` is `cnt_initial + min(n / 15, m // 10)`**.