Alright, I have this problem to solve. Let's see what it's about. So, Nikita had a word consisting of exactly 3 lowercase Latin letters. Each letter has a position in the alphabet from 1 to 26, where 'a' is 1, 'b' is 2, up to 'z' is 26. He encoded the word by summing up the positions of its letters. For example, "cat" is 3 + 1 + 20 = 24.

But, the problem is that this encoding can be ambiguous because different words can have the same sum. For example, "ava" also sums to 24. So, given the sum, I need to find the lexicographically smallest word that could have produced that sum.

First, I need to understand what "lexicographically smallest" means. It means that among all possible words that could have the same sum, I need to find the one that would come first in a dictionary. So, for example, "aav" would be smaller than "ava" because 'a' is smaller than 'v' at the second position.

Okay, so the input is a number n (3 ≤ n ≤ 78), which is the sum of the positions of the three letters. I need to output a string of three lowercase letters that sums to n and is the smallest possible in lexicographical order.

Let me think about how to approach this.

I know that to make the word lexicographically smallest, I should make the first letter as small as possible, then the second, and so on.

So, starting with the first letter, I should choose the smallest possible letter ('a', which is 1), and then try to make the remaining two letters sum to n - 1.

But I need to ensure that the remaining two letters are also as small as possible.

Wait, but if I make the first letter 'a', then the next two letters should be as small as possible to make the word smallest.

But, depending on the value of n, I might need to adjust the letters accordingly.

Let me consider the minimum and maximum possible sums.

The minimum sum is 3, which is 'aaa' (1+1+1=3), and the maximum sum is 78, which is 'zzz' (26+26+26=78).

So, for n=3, the only possible word is 'aaa'.

For n=4, it's 'aab' or 'aba' or 'baa', but the smallest is 'aab'.

Wait, but 'aab' is smaller than 'aba' and 'baa' because 'a' is smaller than 'b' in the first position where they differ.

Wait, no, 'aab' and 'aba' differ at the second position, where 'a' is smaller than 'b', so 'aab' is smaller than 'aba'. And 'aab' is smaller than 'baa' because 'a' is smaller than 'b' in the first position.

So, to make the word smallest, I should maximize the number of 'a's from left to right.

So, the general strategy is to set the first letter to 'a' if possible, then the second to 'a' if possible, and so on.

But, depending on the sum, I might need to increase some letters.

Let me think about how to implement this.

One way is to set the first letter to 'a', then try to make the second letter 'a', and set the third letter to n - 2.

But, n - 2 could be larger than 26, which is not allowed.

So, I need to handle cases where n - 2 > 26, which means the third letter would have to be 'z', and I need to adjust the second letter accordingly.

Wait, perhaps it's better to consider the possible ranges for n and handle them separately.

Let's see:

- For n from 3 to 28:

In this range, it's possible to have the first two letters as 'a' and the third letter ranging from 'a' to 'z'.

Because 'aaz' sums to 1+1+26=28.

- For n from 29 to 53:

In this range, the first letter can be 'a', and the second letter ranges from 'b' to 'z', and the third letter adjusted accordingly.

Wait, 'a' + 'b' + 'z' is 1 + 2 + 26 = 29.

'a' + 'z' + 'z' is 1 + 26 + 26 = 53.

- For n from 54 to 78:

In this range, the first letter has to be at least 'b', because 'aaa' is 3 and 'aab' is 4, up to 'aaz' is 28, 'abz' is 29, up to 'azz' is 53, 'baa' is 54, up to 'zzz' is 78.

Wait, but I need to find the smallest possible word for each n.

Let me try to find a pattern or formula to directly compute the word based on n.

I recall that in problems involving minimizing or maximizing lexicographical order, it's often similar to converting a number into a base corresponding to the number of possible characters, but here it's a bit different because the sum is involved, not a direct positional system.

Alternatively, perhaps I can iterate from 'aaa' to 'zzz', calculate their sums, and find the one with the smallest lexicographical order that matches the given sum.

But since n can be up to 100 test cases, and for each test case, n is up to 78, I need an efficient way to compute this without iterating through all possible combinations.

Let me see if I can find a pattern.

Let's consider that the letters are a, b, c, ..., z, with a=1 to z=26.

I need to find three letters a, b, c such that a + b + c = n, and among all possible combinations where a + b + c = n, I need the one with the smallest lexicographical order.

To minimize the word lexicographically, I should minimize the first letter, then the second, and so on.

So, I should set the first letter to the smallest possible value, then the second to the smallest possible value, given the first, and so on.

So, starting with the first letter:

- Set the first letter to 'a' (1) if possible.

- Then, set the second letter to 'a' (1) if possible.

- Set the third letter to n - 2.

- If n - 2 > 26, then set the third letter to 'z' (26), and adjust the second letter accordingly.

Wait, perhaps I can generalize this.

Let me consider that I have three letters: l1, l2, l3, where l1 <= l2 <= l3 to make it smallest lexicographically.

Wait, no, to make it smallest lexicographically, it's not necessarily that l1 <= l2 <= l3, but rather that l1 is as small as possible, then l2 is as small as possible given l1, and so on.

So, perhaps it's better to iterate from left to right, assigning the smallest possible letter at each position, given the remaining sum.

This is similar to how you would perform subtraction in base 26, but with a twist because the letters start from 1, not 0.

Let me try to formalize this.

Let's denote the three letters as l1, l2, l3, each ranging from 1 to 26.

I need to have l1 + l2 + l3 = n.

To make the word smallest, I should minimize l1 first, then l2, then l3.

So, set l1 to the smallest possible value, which is 1 ( 'a' ), if n - 2 >= 2 (since l2 and l3 must be at least 1 each).

Wait, n - 2 >=1, because l2 and l3 must be at least 1.

Wait, no, l2 and l3 must be at least 1, so n - l1 >= 2.

But, to minimize l1, set l1 = max(1, n - 52), because l2 + l3 can be at most 52 (26 + 26).

Wait, more precisely, to make l1 as small as possible, set l1 = max(1, n - 52), because l2 + l3 can be at most 52.

Similarly, for l2, set it to max(1, n - l1 - 26), and l3 = n - l1 - l2.

Wait, perhaps I need to think recursively.

But maybe there's a better way.

I recall that in standard algorithms, to get the smallest lexicographical combination with a given sum, you assign the smallest possible value to the first position, then recursively do the same for the remaining positions.

In this case, for three positions, it's manageable.

So, here's a plan:

1. Set l1 to the smallest possible value, which is 1 ( 'a' ), if n - 2 >=1, i.e., n >=3.

   - Which it always is, since n >=3.

2. Then, set l2 to the smallest possible value, which is 1, if n - l1 -1 >=1, i.e., n - l1 >=2.

3. Set l3 to n - l1 - l2.

4. However, ensure that l3 <=26.

If l3 >26, then I need to increase l2 to make l3 <=26.

So, let's formalize this.

Set l1 =1.

Set l2 = max(1, n - l1 -26).

Set l3 = n - l1 - l2.

Ensure that l2 <=26 and l3 >=1.

Wait, l2 can be up to 26, but l3 must be at least 1.

So, perhaps it's better to set l3 to min(26, n - l1 -1), and set l2 = n - l1 - l3.

Wait, perhaps.

Let me try to think differently.

Let me consider that l1 is as small as possible, then l2 is as small as possible given l1, and l3 is determined by n - l1 - l2.

To make l3 as small as possible, but l3 cannot be smaller than 1.

So, for a given l1 and l2, l3 = n - l1 - l2, and l3 must be between 1 and 26.

Therefore, for l3 to be >=1, n - l1 - l2 >=1, which implies l2 <= n - l1 -1.

Similarly, l2 >=1 and l2 <=26.

So, l2 can be from max(1, n - l1 -26) to min(26, n - l1 -1).

Wait, no.

Wait, l3 = n - l1 - l2, and l3 must be between 1 and 26.

So, n - l1 - l2 >=1 and n - l1 - l2 <=26.

Therefore, l2 <= n - l1 -1 and l2 >= n - l1 -26.

Wait, n - l1 - l2 >=1 => l2 <= n - l1 -1.

And n - l1 - l2 <=26 => l2 >= n - l1 -26.

Also, l2 >=1 and l2 <=26.

So, combining these, l2 should be in the range [max(1, n - l1 -26), min(26, n - l1 -1)].

Our goal is to set l1 as small as possible, then l2 as small as possible within that range, and l3 is determined.

So, to minimize the word, set l1 =1, then set l2 to the smallest possible value in its range, which is max(1, n -1 -26) = max(1, n -27).

But n can be up to 78, so n -27 can be up to 51, but l2 cannot exceed 26.

Wait, n -1 -26 = n -27.

If n -27 >1, then l2 = n -27, else l2 =1.

But l2 cannot be more than 26.

Wait, perhaps I'm overcomplicating this.

Let me consider specific examples to see the pattern.

Take n=24.

Possible words:

- 'aav': 1 +1 +22 =24

- 'ava':1 +22 +1=24

- 'cat':3 +1 +20=24

- 'tac':20 +1 +3=24

Among these, 'aav' is the smallest lexicographically.

So, to get 'aav', it seems like setting l1='a', l2='a', l3='v'.

Similarly, for n=70, the output is 'rzz': 'r' is 18, 'z' is 26, so 18+26+26=70.

For n=3, it's 'aaa':1+1+1=3.

For n=55, it's 'czz':3+26+26=55.

For n=48, it's 'auz':1+21+26=48.

So, looking at these examples, it seems like the program provided does the following:

- If n >52, set l1 to the letter corresponding to n -53, and l2 and l3 to 'z'.

- If n >27, set l1='a', l2 to the letter corresponding to n -28, and l3='z'.

- If n ==27, set it to 'aay'.

- Else, set l1 and l2 to 'a', and l3 to the letter corresponding to n -3.

Wait, but in the example for n=24, it's 'aav', which follows the second condition: n >27, set l1='a', l2='a', l3='v' (n -28 =24 -28=-4, which doesn't make sense.

Wait, perhaps there's a mistake in interpreting the conditions.

Wait, in the program:

if n >52:

word += alphabet[n -53] + 'zz'

elif n >27:

word += 'a' + alphabet[n -28] + 'z'

elif n ==27:

word = 'aay'

else:

word += 'aa' + alphabet[n -3]

So, for n=24, which is >27, it would set word='a' + alphabet[24-28] + 'z' = 'a' + alphabet[-4] + 'z'.

Wait, that doesn't make sense because alphabet[-4] would be an invalid index.

Wait, alphabet is string.ascii_lowercase, which is 'abcdefghijklmnopqrstuvwxyz', indexed from 0 to 25.

So, alphabet[-4] is 'w', but this seems incorrect.

Wait, perhaps I'm misunderstanding the indexing.

Wait, in Python, string indices start at 0.

So, alphabet[0] = 'a', alphabet[1] = 'b', ..., alphabet[25] = 'z'.

So, for n=24 >27 is False, so it goes to the else clause: 'aa' + alphabet[n-3] = 'aa' + alphabet[21] = 'aa' + 'v' = 'aav', which matches the example.

For n=70 >52, so alphabet[70-53] = alphabet[17] = 'r', so 'rzz', which matches the example.

For n=27 ==27, so 'aay', which matches the example.

For n=55 >52, so alphabet[55-53] = alphabet[2] = 'c', so 'czz', which matches the example.

For n=48 >52 is False, so >27 is True, so 'a' + alphabet[48-28] + 'z' = 'a' + alphabet[20] + 'z' = 'a' + 'u' + 'z' = 'auz', which matches the example.

So, the program seems to handle the cases correctly based on the examples.

But, is this logic general? Let's see.

First, understand the conditions:

- If n >52, set the first letter to the letter corresponding to n -53, and the next two letters to 'z'.

- If n >27, set the first letter to 'a', the second to n -28, and the third to 'z'.

- If n ==27, set it to 'aay'.

- Else, set the first two letters to 'a', and the third to n -3.

Let's verify these conditions.

First, n >52:

The maximum sum for 'aaz' is 1 +1 +26=28.

Wait, but 52 corresponds to 'azz':1 +26 +26=53.

Wait, no, 'azz' is 1 +26 +26=53.

Wait, n >52 means n >=53, which corresponds to 'azz' and above.

So, for n >=53, the first letter should be at least 'a' +1='b', because 'aaa' is 3, 'aab' is 4, ..., 'aaz' is 28, 'abz' is 29, ..., 'azz' is 53, 'baa' is 54, and so on.

Wait, but in the program, for n >52, it sets the first letter to alphabet[n -53] and the next two to 'z'.

For n=53, alphabet[53-53]=alphabet[0]='a', so 'azz', which is correct.

For n=54, alphabet[1]='b', so 'bzz', which is correct.

Similarly, up to n=78, which is alphabet[25]='z' + 'zz' = 'zzz'.

So, this seems correct.

Next, for n >27 and n <=52.

n=28: 'aaz' =1 +1 +26=28.

n=29: 'abz' =1 +2 +26=29.

...

n=53: 'azz' =1 +26 +26=53.

Wait, but in the program, for n >27, it sets word='a' + alphabet[n -28] + 'z'.

For n=28, alphabet[28-28]=alphabet[0]='a', so 'aaz'.

For n=29, alphabet[1]='b', so 'abz'.

...

For n=53, alphabet[25]='z', so 'azz'.

This seems correct.

Then, for n==27, it sets word='aay'.

Which is 1 +1 +25=27.

But, why is there a special case for n==27?

Because if n==27, according to the else clause, it would be 'aa' + alphabet[24]='aaX', where X is the 24th letter, which is 'x', but 'aax' sums to 1+1+24=26, which is less than 27.

Wait, alphabet[24] is 'y', since indexing starts at 0.

Wait, no, alphabet[24] is 'y', because 'a' is 0, 'b' is 1, ..., 'y' is 24, 'z' is 25.

Wait, no, 'a' is 0, 'b' is 1, ..., 'y' is 24, 'z' is 25.

So, for n=27, 'aa' + alphabet[24] = 'aay' =1 +1 +25=27, which is correct.

So, why is there a special case for n==27?

Because if we use the else clause for n=27, it would be 'aa' + alphabet[24]='aay', which is correct.

But in the program, there is a separate condition for n==27, setting word='aay'.

Perhaps to handle it explicitly.

But, in reality, it's redundant because the else clause would handle it correctly.

Wait, let's check.

For n=27, which is not greater than 27, so it goes to the else clause: 'aa' + alphabet[27-3]='aa' + alphabet[24]='aay', which is correct.

So, the special case for n==27 is unnecessary.

Perhaps it's there to override or correct something.

Wait, maybe to ensure that it's 'aay' and not something else.

But, seems like it's covered by the else clause.

Moving on.

Finally, for n <=27, it sets 'aa' + alphabet[n-3].

For n=3, 'aa' + 'a' = 'aaa', which is correct.

For n=4, 'aa' + 'b' = 'aab', which is correct.

...

For n=27, as above, 'aay'.

This seems correct.

So, overall, the program handles the cases correctly based on the examples and the logic seems sound.

Therefore, I would say that the given program is correct.

**Final Answer**

\[ \boxed{\text{True}} \]