The code `ans[i + 1] += ans[i]` updates the value of `ans[1]` by adding the value of `ans[0]` to it.

Initial State:
- `arr` is a list of integers where 1 <= len(arr) <= 500, each element `x_i` in `arr` satisfies 1 <= `x_i` <= 500.
- `n` is an integer such that 3 <= `n` <= 500.
- `ans` is a list of `n` zeros with `ans[0]` now equal to `arr[0] + 1`.
- `ans[1]` is now equal to `arr[0] + (arr[0] + 1) + (arr[0] + 1)`.
- `i` is 0.
- The current value of `ans[1]` is less than `arr[1]`.

Step-by-step impact:
1. `ans[i + 1]` refers to `ans[1]`.
2. `ans[i]` refers to `ans[0]`, which is `arr[0] + 1`.
3. The value of `ans[1]` is updated by adding `ans[0]` to it.

Calculations:
- `ans[0] = arr[0] + 1`
- `ans[1] = arr[0] + (arr[0] + 1) + (arr[0] + 1)`
- `ans[1] += ans[0]`
- `ans[1] = arr[0] + (arr[0] + 1) + (arr[0] + 1) + (arr[0] + 1)`
- Simplifying, `ans[1] = arr[0] + arr[0] + 1 + arr[0] + 1 + arr[0] + 1`
- `ans[1] = 4 * arr[0] + 3`

Output State: **`arr` is a list of integers where 1 <= len(arr) <= 500, each element `x_i` in `arr` satisfies 1 <= `x_i` <= 500, `n` is an integer such that 3 <= `n` <= 500, `ans` is a list of `n` zeros with `ans[0]` now equal to `arr[0] + 1`, `ans[1]` now equal to `4 * arr[0] + 3`, `i` is 0, and the current value of `ans[1]` is less than `arr[1]`.**