To determine the output state, let's evaluate the given Python code snippet step by step:

### Initial State:
- `n` and `m` are positive integers such that \(1 \leq n, m \leq 2 \times 10^6\)
- `T` is greater than 1
- `t` is 2
- `info` is a list of strings obtained from splitting the new input
- `a` is the integer value of `info[0]`
- `b` is the integer value of `info[1]` and must be at least 1
- `i` is 1
- `suma` is 0

### Code Snippet:
```python
x = (a - i * (i - 1)) // i ** 2 + 1
```

### Step-by-Step Calculation:
1. **Evaluate `i * (i - 1)`**:
   - Since `i` is 1, `i * (i - 1) = 1 * (1 - 1) = 1 * 0 = 0`.

2. **Evaluate `a - i * (i - 1)`**:
   - This simplifies to `a - 0 = a`.

3. **Evaluate `i ** 2`**:
   - Since `i` is 1, `i ** 2 = 1 ** 2 = 1`.

4. **Evaluate `(a - i * (i - 1)) // i ** 2`**:
   - This simplifies to `a // 1 = a`.

5. **Evaluate `(a - i * (i - 1)) // i ** 2 + 1`**:
   - This simplifies to `a + 1`.

### Final Value of `x`:
- `x` is assigned the value `a + 1`.

### Output State:
- `n` and `m` are positive integers such that \(1 \leq n, m \leq 2 \times 10^6\)
- `T` is greater than 1
- `t` is 2
- `info` is a list of strings obtained from splitting the new input
- `a` is the integer value of `info[0]`
- `b` is the integer value of `info[1]` and must be at least 1
- `i` is 1
- `suma` is 0
- `x` is `a + 1`

Output State: **`n` and `m` are positive integers such that \(1 \leq n, m \leq 2 \times 10^6\), `T` is greater than 1, `t` is 2, `info` is a list of strings obtained from splitting the new input, `a` is the integer value of `info[0]`, `b` is the integer value of `info[1]` and must be at least 1, `i` is 1, `suma` is 0, `x` is `a + 1`.**