Reasoning:

The original assessment is correct. The program provided does not correctly implement the logic to count the number of ordered pairs \((a, b)\) such that \(1 \le a \le n\), \(1 \le b \le m\), and \(a + b\) is a multiple of \(b \cdot \gcd(a, b)\).

Let's break down the issues with the provided program:

1. **Function `func_1`**:
   - This function correctly computes the greatest common divisor (GCD) of two numbers \(a\) and \(b\). It uses the Euclidean algorithm, which is a well-known and correct method for finding the GCD.

2. **Function `func_2`**:
   - The function `func_2` is supposed to count the number of valid pairs \((a, b)\) that satisfy the given conditions.
   - However, the logic inside `func_2` is flawed and does not align with the problem requirements.
   - The loop iterates over \(i\) from 1 to \(m-1\), but it does not correctly handle the pairs \((a, b)\) where \(1 \le a \le n\) and \(1 \le b \le m\).
   - The calculation of `x` and `y`:
     - `x = n - (i * i - i)`
     - `y = i * i`
   - The increment of `cnt`:
     - `cnt = cnt + x // y + (i > 1)`
   - This logic does not correctly check if \(a + b\) is a multiple of \(b \cdot \gcd(a, b)\). Instead, it seems to be performing some unrelated arithmetic operations and counting based on those results.

3. **Example Analysis**:
   - For the input \(n = 2\) and \(m = 3\), the correct output should be 3, as the valid pairs are \((1, 1)\), \((2, 1)\), and \((2, 2)\).
   - Let's trace the execution of `func_2(2, 3)`:
     - For \(i = 1\):
       - `x = 2 - (1 * 1 - 1) = 2 - 0 = 2`
       - `y = 1 * 1 = 1`
       - `cnt = cnt + 2 // 1 + (1 > 1) = 0 + 2 + 0 = 2`
     - For \(i = 2\):
       - `x = 2 - (2 * 2 - 2) = 2 - 2 = 0`
       - `y = 2 * 2 = 4`
       - `cnt = cnt + 0 // 4 + (2 > 1) = 2 + 0 + 1 = 3`
     - The function returns 3, which is incorrect because it should return 3 for the valid pairs \((1, 1)\), \((2, 1)\), and \((2, 2)\).

4. **Correct Approach**:
   - To correctly solve the problem, we need to iterate over all possible pairs \((a, b)\) and check if \(a + b\) is a multiple of \(b \cdot \gcd(a, b)\).
   - The correct implementation would involve a nested loop over \(a\) and \(b\) and a check for the condition \(a + b \mod (b \cdot \gcd(a, b)) == 0\).

Given the above analysis, the original assessment is accurate. The provided program does not correctly solve the problem as described.

Final: **False**