The code snippet appends the value of `(a[i] - a[i - 1]) // 2` to the list `tmp`. Given the initial state:

- `i` is 3.
- `a` is a sorted list of integers in ascending order with at least 3 elements.

Let's calculate the new value to be appended:

1. `a[i]` refers to the element at index 3 (since `i` is 3).
2. `a[i - 1]` refers to the element at index 2 (since `i - 1` is 2).
3. The expression `(a[i] - a[i - 1]) // 2` calculates the integer division of the difference between these two elements by 2.

Let's denote the elements of `a` as follows:
- `a[2]` is the third element in the list.
- `a[3]` is the fourth element in the list.

The value to be appended to `tmp` is `(a[3] - a[2]) // 2`.

After appending this value to `tmp`, the updated state is:

- `t` is a positive integer where 1 ≤ t ≤ 10^4.
- `n` is an input integer where 4 ≤ n ≤ 10^9.
- `x` is an input integer where 2 ≤ x ≤ min(n, 2 · 10^5).
- `y` is an input integer.
- `tt` is greater than 2.
- `ii` is 2.
- `i` is 3.
- `a` is a sorted list of integers in ascending order with at least 3 elements.
- `tmp` is now a list containing one element: `(a[3] - a[2]) // 2`.
- `ans` is initially `x + y - 2`.

Output State: **`t` is a positive integer where 1 ≤ t ≤ 10^4, `n` is an input integer where 4 ≤ n ≤ 10^9, `x` is an input integer where 2 ≤ x ≤ min(n, 2 · 10^5), `y` is an input integer, `tt` is greater than 2, `ii` is 2, `i` is 3, `a` is a sorted list of integers in ascending order with at least 3 elements, `tmp` is a list containing one element: `(a[3] - a[2]) // 2`, `ans` is initially `x + y - 2`.**