The code `S0, S1 = S1, S_next` updates the values of `S0` and `S1`. According to the initial state, `S1` is `2 * S1 + S0` and `S_next` is `4 * S1 + 2 * S0`. 

1. Calculate the initial value of `S1`:
   \[
   S1 = 2 * S1 + S0 = 2 * (4 * S1 + 2 * S0) + S0 = 8 * S1 + 4 * S0 + S0 = 8 * S1 + 5 * S0
   \]
   This simplifies to:
   \[
   S1 = -\frac{5}{7} * S0
   \]

2. The value of `S_next` is:
   \[
   S_next = 4 * S1 + 2 * S0 = 4 * (-\frac{5}{7} * S0) + 2 * S0 = -\frac{20}{7} * S0 + 2 * S0 = -\frac{20}{7} * S0 + \frac{14}{7} * S0 = -\frac{6}{7} * S0
   \]

3. After executing `S0, S1 = S1, S_next`, the new values are:
   \[
   S0 = S_next = -\frac{6}{7} * S0
   \]
   \[
   S1 = -\frac{5}{7} * S0
   \]

Therefore, the updated values are:
- `n` is greater than 2
- `i` is 3
- `S0` is `-6/7 * S0`
- `S1` is `-5/7 * S0`

Output State: **`n` is greater than 2, `i` is 3, `S0` is `-6/7 * S0`, `S1` is `-5/7 * S0`**