Output State: **`n` is a positive integer and neither 0 nor 1; `S0` is 1; `S1` is 1; `i` is `n`; `S0` is \((-2^n - 1) / (-7)\) * `S0`; `S1` is \((-2^n + 1) / (-7)\) * `S0`**.

### Step-by-Step Reasoning:

1. **Initial State**: 
   - `n` is a positive integer and neither 0 nor 1.
   - `S0` is 1.
   - `S1` is 1.

2. **Loop Code Analysis**:
   - The loop iterates from `i = 2` to `i = n`.
   - For each iteration, `S_next = 2 * S1 + S0`.
   - After calculating `S_next`, `S0` and `S1` are updated: `S0 = S1` and `S1 = S_next`.

3. **First Iteration (i = 2)**:
   - `S_next = 2 * S1 + S0 = 2 * 1 + 1 = 3`.
   - Update: `S0 = 1`, `S1 = 3`.

4. **Second Iteration (i = 3)**:
   - `S_next = 2 * S1 + S0 = 2 * 3 + 1 = 7`.
   - Update: `S0 = 3`, `S1 = 7`.

5. **General Iteration (i = k)**:
   - Assume after `k-1` iterations, `S0` and `S1` are known.
   - `S_next = 2 * S1 + S0`.
   - Update: `S0 = S1`, `S1 = S_next`.

6. **Final Iteration (i = n)**:
   - After `n-1` iterations, `S0` and `S1` will be calculated as per the above pattern.
   - The general form after `n-1` iterations can be derived by observing the pattern:
     - For `n = 2`: `S0 = 1`, `S1 = 3`.
     - For `n = 3`: `S0 = 3`, `S1 = 7`.
     - For `n = 4`: `S0 = 7`, `S1 = 15`.

   - The pattern suggests that `S0` and `S1` follow the recurrence relation \(S_{next} = 2S1 + S0\).

7. **Solving the Recurrence Relation**:
   - Let's solve the recurrence relation \(S_n = 2S_{n-1} + S_{n-2}\).
   - The characteristic equation is \(x^2 - 2x - 1 = 0\), which has roots \(x = 1 + \sqrt{2}\) and \(x = 1 - \sqrt{2}\).
   - The general solution is \(S_n = A(1 + \sqrt{2})^n + B(1 - \sqrt{2})^n\).
   - Using initial conditions \(S_0 = 1\) and \(S_1 = 1\), we get:
     - \(1 = A + B\)
     - \(1 = A(1 + \sqrt{2}) + B(1 - \sqrt{2})\)

   - Solving these equations gives \(A = \frac{1}{2\sqrt{2}}\) and \(B = \frac{-1}{2\sqrt{2}}\).

8. **Final Values**:
   - For large \(n\), the dominant term is \(A(1 + \sqrt{2})^n\).
   - Simplifying, we get:
     - \(S0 = \frac{(1 + \sqrt{2})^{n-1} - (1 - \sqrt{2})^{n-1}}{\sqrt{2}}\)
     - \(S1 = 2S0 + S0 = 3S0\)

   - Simplifying further, we get:
     - \(S0 = \frac{(-2^n - 1)}{-7} \times S0\)
     - \(S1 = \frac{(-2^n + 1)}{-7} \times S0\)

9. **Conclusion**:
   - After `n` iterations, `i` will be `n`.
   - `S0` and `S1` will be as derived above.

Thus, the final output state is:
**`n` is a positive integer and neither 0 nor 1; `S0` is 1; `S1` is 1; `i` is `n`; `S0` is \((-2^n - 1) / (-7)\) * `S0`; `S1` is \((-2^n + 1) / (-7)\) * `S0`.**