To determine the output state after the loop completes, we need to understand the behavior of the loop and how the variables `A`, `idx_A`, `B`, `idx_B`, `l`, and `r` evolve during each iteration. However, the given loop code depends on an external list `s` which is not provided in the initial state. For the sake of this exercise, let's assume `s` is a list of `>` and `<` characters that dictate the flow of the loop. Without the specific `s`, we can only provide a generic explanation of how the loop might affect the state.

Given the loop's structure, it modifies `l` and `r` based on the characters in `s`. Let's consider a hypothetical `s` to illustrate the loop's behavior.

Assume `s = ['>', '>', '<', '<']` and `n = 4`. Here's how the loop might behave:

1. **Iteration 1 (i=0, s[0]='>')**:
   - Since `s[0] == '>'`, the code executes the first `if` block.
   - `l < r` is true (0 < 4).
   - `a = A[l] = A[0] = 0`
   - `x = r - (l + 2) = 4 - (0 + 2) = 2`
   - `b = B[r - 1] = B[3] = 7`
   - `x >= 0` is true, so:
     - `b = b - B[x] = 7 - B[2] = 7 - 4 = 3`
     - `b = b - (idx_B[x] - idx_B[r - 1]) * (x + 1) = 3 - (1 - 0) * 3 = 3 - 3 = 0`
     - `b = (idx_B[r - 1] - i) * (l + 1) = (0 - 0) * 1 = 0`
   - `print(a * 2 + b * 2 + i + 1, end=' ')` prints `1`.
   - `l += 1` makes `l = 1`.

2. **Iteration 2 (i=1, s[1]='>')**:
   - Since `s[1] == '>'`, the code executes the first `if` block.
   - `l < r` is true (1 < 4).
   - `a = A[l] = A[1] = 2`
   - `x = r - (l + 2) = 4 - (1 + 2) = 1`
   - `b = B[r - 1] = B[3] = 7`
   - `x >= 0` is true, so:
     - `b = b - B[x] = 7 - B[1] = 7 - 2 = 5`
     - `b = b - (idx_B[x] - idx_B[r - 1]) * (x + 1) = 5 - (3 - 0) * 2 = 5 - 6 = -1`
     - `b = (idx_B[r - 1] - i) * (l + 1) = (0 - 1) * 2 = -2`
   - `print(a * 2 + b * 2 + i + 1, end=' ')` prints `0`.
   - `l += 1` makes `l = 2`.

3. **Iteration 3 (i=2, s[2]='<')**:
   - Since `s[2] == '<'`, the code executes the `else` block.
   - `r -= 1` makes `r = 3`.
   - `l <= r` is true (2 <= 3).
   - `a = A[l - 1] = A[1] = 2`
   - `a = a + (i - idx_A[l - 1]) * l = 2 + (2 - 3) * 2 = 2 - 2 = 0`
   - `b = B[r] = B[3] = 7`
   - `r - l >= 0` is true (3 - 2 >= 0), so:
     - `b = b - B[r - l] = 7 - B[1] = 7 - 2 = 5`
     - `b = b - (idx_B[r - l] - i) * (r - l) = 5 - (3 - 2) * 1 = 5 - 1 = 4`
     - `b = b + (idx_B[r] - i) * l = 4 + (0 - 2) * 2 = 4 - 4 = 0`
   - `print(a * 2 + b * 2 + i + 1, end=' ')` prints `3`.
   - No change to `l`.

4. **Iteration 4 (i=3, s[3]='<')**:
   - Since `s[3] == '<'`, the code executes the `else` block.
   - `r -= 1` makes `r = 2`.
   - `l <= r` is true (2 <= 2).
   - `a = A[l - 1] = A[1] = 2`
   - `a = a + (i - idx_A[l - 1]) * l = 2 + (3 - 3) * 2 = 2 + 0 = 2`
   - `b = B[r] = B[2] = 4`
   - `r - l >= 0` is false (2 - 2 == 0), so:
     - `b = b + (idx_B[r] - i) * l = 4 + (1 - 3) * 2 = 4 - 4 = 0`
   - `print(a * 2 + b * 2 + i + 1, end=' ')` prints `7`.
   - No change to `l`.

After the loop completes, the output printed would be `1 0 3 7`.

The state of the variables `A`, `idx_A`, `B`, `idx_B` remains unchanged as they are not modified in the loop. The variables `l` and `r` are modified to `l = 2` and `r = 2`.

Output State: **A is [0, 2, 4]; idx_A is [1, 3, 4]; B is [0, 2, 4, 7]; idx_B is [4, 2, 1, 0]; l is 2; r is 2**.