Let's break down the problem step by step:

1. **Identify the loop head variables**: The loop head variables are `i` and `b` (since the loop iterates over a range defined by these two values).

2. **Determine the current state after the previous iteration**:
   - `n` is greater than `b`
   - `k` is an integer such that \(2 \leq k < n \leq 100\)
   - `b` is an integer such that \(1 \leq b \leq n\)
   - `i` is `b - k`
   - `remaining_tabs[b - k]` is `0`

3. **Understand the loop range**: The loop runs from `b` down to `-1` in steps of `-k`.

4. **Determine the condition for the next iteration**:
   - For the loop to continue, `i` must be greater than or equal to `-1`.
   - The new value of `i` will be `i + (-k)`.

5. **Calculate the new state**:
   - The initial value of `i` is `b - k`.
   - After the first iteration, `i` becomes `(b - k) - k = b - 2k`.
   - For the loop to continue, `b - 2k` must be greater than or equal to `-1`.

6. **Adjust the states**:
   - `i` will be updated to `b - 2k` if it satisfies the condition `b - 2k >= -1`.
   - `b` remains unchanged because it is not modified within the loop.

7. **Formulate the new state**:
   - `i` will be `b - 2k` if `b - 2k >= -1`.
   - If `b - 2k < -1`, the loop would have stopped, so the condition `b - 2k >= -1` must hold true.

Given this reasoning, the new state is:

**`n` is greater than `b`, `k` is an integer such that \(2 \leq k < n \leq 100\), `b` is an integer such that \(1 \leq b \leq n\), `i` is \(b - 2k\) where \(b - 2k \geq -1\)**

State: **`n` is greater than `b`, `k` is an integer such that \(2 \leq k < n \leq 100\), `b` is an integer such that \(1 \leq b \leq n\), `i` is \(b - 2k\) where \(b - 2k \geq -1\)**