Alright, I've got this problem to solve. Let's see what it's about. There are three friends playing chess together. In each game, two of them play against each other. The winner gets 2 points, the loser gets 0, and in case of a draw, both get 1 point each. After all the games, their scores are p1, p2, and p3, with p1 ≤ p2 ≤ p3. I need to find the maximum number of draws that could have happened, or determine if the scores are invalid.

First, I need to understand the scoring system. Each game can result in either a win or a draw. If it's a win, the winner gets 2 points, and the loser gets 0. If it's a draw, both players get 1 point each. So, in every game, the total points awarded are either 2 (in case of a win) or 2 (in case of a draw). Wait, that's interesting. So, regardless of whether it's a win or a draw, the total points added after each game is always 2.

Let me verify that. In a win, one player gets 2 and the other gets 0, so total points added are 2. In a draw, both get 1, so total is still 2. Okay, so the total points after all games will always be twice the number of games played.

Let's denote the number of games played as 'm'. Then, total points = 2m.

Given p1 + p2 + p3 = total points = 2m.

So, the sum of p1, p2, p3 must be even, because it's equal to 2m. If the sum is odd, it's impossible, and we should return -1.

Looking back at the sample input, in the first case, p1=0, p2=0, p3=0. Sum is 0, which is even, so m=0. No games were played, so no draws, which matches the output of 0.

Second case: p1=0, p2=1, p3=1. Sum is 2, so m=1. Only one game was played. If it was a draw, both players get 1 point each. So, if two players drew, their scores would be 1 and 1, and the third player has 0. That matches the input, and the output is 1 draw.

Third case: p1=0, p2=2, p3=3. Sum is 5, which is odd. So, it's impossible, but in the sample input, it's p1=0, p2=2, p3=3, but in the given program, it's p1=0, p2=1, p3=10, which is different. Wait, no, checking the program, it's p1=0, p2=2, p3=3 in one of the test cases. But in the explanation, it's different. I need to make sure I'm looking at the right thing.

Wait, the problem description has 7 test cases:

1. 0 0 0 → 0

2. 0 1 1 → 1

3. 1 1 1 → -1

4. 1 1 2 → 2

5. 3 3 3 → -1

6. 3 4 5 → 6

7. 1 1 10 → 2

But in the program, it's:

cas_de_test = [(0, 0, 0), (0, 1, 1), (0, 2, 3), (3, 3, 3), (3, 4, 5), (1, 1, 10), (0, 0, 6)]

Wait, the third test case in the program is (0,2,3), but in the problem description, it's (1,1,1). Hmm, maybe they changed it or something. I need to focus on the program's logic rather than the specific test cases.

So, back to the logic.

We have p1 ≤ p2 ≤ p3, and p1 + p2 + p3 = 2m.

First, check if p1 + p2 + p3 is even. If not, return -1.

Then, m = (p1 + p2 + p3) / 2.

Now, I need to maximize the number of draws. Each draw contributes 2 points to the total (1 for each player), while each win contributes 2 points to the winner.

To maximize draws, I should minimize wins.

But I need to satisfy the individual scores p1, p2, p3.

Let me think about how to distribute the points.

Let me consider the number of draws.

In a draw, two players each get 1 point, so total points from draws is 2 per draw.

In a win, one player gets 2 points, and the other gets 0, so total points from wins is also 2 per win.

But in terms of individual scores, draws affect two players, while wins affect only one.

I need to maximize the number of draws, which means minimizing the number of wins.

But wins affect one player's score by +2, while draws affect two players' scores by +1 each.

Given that, I need to see how many draws can occur while still achieving the given p1, p2, p3.

Let me try to model this.

Let’s denote:

- d: number of draws

- w: number of wins

Then, total games: m = d + w.

Total points: 2m = 2d + 2w.

But we also have the individual scores.

Let’s think about how the draws and wins affect the individual scores.

Each draw involves two players, and each draw increases each of their scores by 1.

Each win involves one player winning and getting +2, and the other getting 0.

So, for each win, one player's score increases by 2.

Now, to maximize draws, I need to maximize d, which means minimizing w.

But I need to ensure that the individual scores can be achieved with some combination of draws and wins.

This seems a bit tricky.

Maybe I can look at the differences between the scores.

Since p1 ≤ p2 ≤ p3, p3 is the highest score.

Let me consider that the maximum score p3 could be achieved only through wins, since draws would spread points to two players.

But p3 could have come from a combination of wins and draws.

Wait, perhaps I should consider the minimal number of wins required to achieve p3, and then see how the rest can be draws.

Let’s think about p3.

p3 must have gained all its points from wins and draws.

Each win gives +2, and each draw gives +1.

But in a win, p3 is the winner, and in a draw, p3 is one of the drawing players.

Wait, but in draws, two players draw and both get +1.

So, p3's score comes from wins (2 points per win) and draws (1 point per draw).

Similarly, p2 and p1 get points from draws they participate in and wins they win.

This seems a bit complicated.

Maybe I can model this with equations.

Let’s define:

- Let d_ab be the number of draws between player a and player b.

- Similarly, d_ac and d_bc.

- Let w_a be the number of wins for player a.

Similarly, w_b and w_c.

Then, the total points for each player can be expressed as:

p_a = d_ab + d_ac + 2 * w_a

p_b = d_ab + d_bc + 2 * w_b

p_c = d_ac + d_bc + 2 * w_c

And the total number of games is:

m = d_ab + d_ac + d_bc + w_a + w_b + w_c

But this seems too many variables.

Maybe there's a smarter way.

Let’s think about the sum of p1, p2, p3.

p1 + p2 + p3 = 2m

And we have p1 ≤ p2 ≤ p3.

I need to maximize the number of draws.

Wait, perhaps I can think in terms of the minimal number of wins.

Each win increases one player's score by 2, while each draw increases two players' scores by 1 each.

To maximize draws, I need to minimize wins.

So, what's the minimal number of wins required to achieve the given scores?

Let’s think about p3.

p3 must have achieved p3 points, which can be a combination of wins and draws.

But it's getting complicated.

Let me look at the sample inputs.

First sample: 0 0 0

No games were played, so no draws. That makes sense.

Second sample: 0 1 1

Sum is 2, so m=1.

If they played one game, and it was a draw between the second and third players, which matches the scores. So, one draw.

Third sample: 1 1 1

Sum is 3, which is odd. So, impossible. Output -1.

Fourth sample: 1 1 2

Sum is 4, so m=2.

How can this be achieved?

Option 1: Two draws between different pairs.

For example, first and second draw in one game, and first and third draw in another game.

Then, p1 = 1 (from each draw) → total 2

p2 = 1 (from first draw)

p3 = 1 (from second draw)

But that gives p1=2, p2=1, p3=1, which doesn't match the input of 1,1,2.

Wait, so that's not working.

Option 2: One draw between second and third, and one win for the third.

So, in the draw, p2 and p3 get 1 each.

In the win for p3, p3 gets 2, and one of the others gets 0.

If p3 plays against p1 in the win, then p3 gets 2, p1 gets 0.

So, total:

p1: 0 (from win) + 1 (from draw) = 1

p2: 1 (from draw)

p3: 1 (from draw) + 2 (from win) = 3

But p3 should be 2, not 3. So, that doesn't work.

Wait, maybe I miscalculated.

Wait, if p3 has a draw with p2, then p2 and p3 get 1 each.

Then, p3 has a win against p1, so p3 gets 2 more, and p1 gets 0.

So, p1: 0 + 1 (from draw) = 1

p2: 1 (from draw)

p3: 1 (from draw) + 2 (from win) = 3

But p3 should be 2, not 3. So, that doesn't work.

Alternatively, maybe p3 has a draw with p2, and then p3 has a loss to p1.

But loss means p3 gets 0, and p1 gets 2.

But that would make p3: 1 (from draw) + 0 (from loss) = 1, which doesn't match p3=2.

Hmm.

Alternatively, maybe p3 has one win against p1, and one draw with p2.

So, p1: 0 (from loss) + 1 (from draw) = 1

p2: 1 (from draw)

p3: 2 (from win) + 1 (from draw) = 3

Again, p3=3, but should be 2.

Wait, that doesn't work.

Alternatively, p3 has one win and one loss.

But that would give p3: 2 (from win) + 0 (from loss) = 2

But then, who did p3 draw with?

Wait, maybe p3 has one win against p1 and one loss to p2.

So, p1: 0 (from loss) + 1 (from draw with p2?) Wait, but p2 didn't win against p3.

Wait, p2 won against p3 in the loss.

Wait, I'm getting confused.

Let me try to think differently.

Let’s consider that in m games, there are d draws and w wins, with m = d + w.

Total points: 2m = 2d + 2w.

But also, p1 + p2 + p3 = 2m.

Each draw affects two players by +1 each, and each win affects one player by +2.

So, the total points can be expressed as:

p1 + p2 + p3 = sum of points from draws and wins.

But I need to find a way to maximize d.

Maybe I can think in terms of the minimal number of wins required.

Each win increases one player's score by 2, while each draw increases two players' scores by 1 each.

So, to maximize draws, I need to minimize wins.

Let’s consider the highest score, p3.

p3 can gain points from wins and draws.

Each win gives p3 +2, and each draw gives p3 +1.

Similarly, p2 and p1 gain points from draws they participate in.

Let’s try to satisfy p3's score with as few wins as possible.

So, let’s see how many wins p3 must have to achieve p3 points.

Since each win gives +2, and each draw gives +1, the minimal number of wins for p3 is ceil(p3 / 2).

Wait, no. If p3 has w wins and d_d draws, then p3 = 2*w + d_d.

So, w = (p3 - d_d) / 2.

Since w must be integer, and p3 - d_d must be even.

But this is getting complicated.

Let me try to express d in terms of known quantities.

Let’s denote d as the total number of draws.

Each draw involves two players, and increases each of their scores by 1.

So, the total points from draws is 2*d.

The remaining points must come from wins.

Total points from wins is 2*w.

So, 2*m = 2*d + 2*w ⇒ m = d + w.

Also, p1 + p2 + p3 = 2*m = 2*(d + w).

Now, let’s consider the individual scores.

p1 = points from draws p1 is involved in + points from wins p1 wins.

Similarly for p2 and p3.

Let’s denote:

- d_ab: number of draws between a and b.

- d_ac: number of draws between a and c.

- d_bc: number of draws between b and c.

- w_a: number of wins for a.

- w_b: number of wins for b.

- w_c: number of wins for c.

Then:

p1 = d_ab + d_ac + 2*w1

p2 = d_ab + d_bc + 2*w2

p3 = d_ac + d_bc + 2*w3

And total draws: d = d_ab + d_ac + d_bc

Total wins: w = w1 + w2 + w3

Total games: m = d + w

Total points: 2*m = p1 + p2 + p3

Now, to maximize d, we need to minimize w.

So, we need to minimize w1 + w2 + w3.

Given that p1, p2, p3 are fixed, we can try to minimize the number of wins.

But this seems too abstract.

Maybe I can look for upper and lower bounds on d.

Let’s consider that in order to maximize d, we need to maximize the number of draws, which means that as many points as possible should come from draws.

But each draw contributes +1 to two players' scores.

So, for p1, p2, p3, the sum of their scores is 2*m.

Now, to maximize d, we need to maximize 2*d, which is the points coming from draws.

Therefore, the remaining points, 2*w = p1 + p2 + p3 - 2*d, must be distributed through wins.

But p1, p2, p3 are fixed, so 2*w = p1 + p2 + p3 - 2*d.

But w must be an integer greater than or equal to 0.

So, p1 + p2 + p3 - 2*d >= 0 and must be even, since 2*w is even.

Also, w >= 0 ⇒ p1 + p2 + p3 - 2*d >= 0 ⇒ d <= (p1 + p2 + p3)/2.

But we need to ensure that the individual scores can be achieved with the chosen d and w.

This is getting too vague.

Let me look at the program provided.

In the program, for each test case (p1, p2, p3):

- Check if p1 + p2 + p3 is even. If not, return -1.

- Then, m = (p1 + p2 + p3) / 2.

- If m > 3 or p3 > m, return -1.

- Then, egalites = p1 + p2 + p3 - 2*(p3 - p2) - 2*(p3 - p1)

- If egalites < 0, return -1.

- Else, return egalites // 2.

Wait, in the program, it's egalites = total_points - 2 * (p3 - p2) - 2 * (p3 - p1)

Let me see what that equals.

Total points = p1 + p2 + p3.

So, egalites = p1 + p2 + p3 - 2*(p3 - p2) - 2*(p3 - p1)

Let’s simplify that:

= p1 + p2 + p3 - 2*p3 + 4*p2 - 2*p3 + 4*p1

Wait, no, that's not right.

Wait, let's compute it step by step.

First, p1 + p2 + p3 - 2*(p3 - p2) - 2*(p3 - p1)

= p1 + p2 + p3 - 2*p3 + 2*p2 - 2*p3 + 2*p1

= (p1 + 2*p1) + (p2 + 2*p2) + (p3 - 2*p3 - 2*p3)

= 3*p1 + 3*p2 - 3*p3

= 3*(p1 + p2 - p3)

So, egalites = 3*(p1 + p2 - p3)

Then, egalites // 2 = floor(3*(p1 + p2 - p3)/2)

But in the program, it's egalites // 2.

But in the fourth sample input: p1=1, p2=1, p3=2

So, p1 + p2 - p3 = 1 + 1 - 2 = 0

So, egalites = 0

Then, egalites // 2 = 0, but the sample output is 2.

Wait, that doesn't match.

Wait, in the fourth sample input, p1=1, p2=1, p3=2

Sum is 4, which is even, m=2.

p3=2 <= m=2, so it's okay.

Then, egalites = p1 + p2 + p3 - 2*(p3 - p2) - 2*(p3 - p1) = 4 - 2*(2-1) - 2*(2-1) = 4 - 2*1 - 2*1 = 4 - 2 - 2 = 0

Then, egalites // 2 = 0, but the sample output is 2.

Wait, that doesn't match.

Wait, perhaps I misread the sample input.

Looking back, the sample input is:

7

0 0 0

0 1 1

1 1 1

1 1 2

3 3 3

3 4 5

1 1 10

And the output is:

0

1

-1

2

-1

6

2

But in the program, it's:

cas_de_test = [(0, 0, 0), (0, 1, 1), (0, 2, 3), (3, 3, 3), (3, 4, 5), (1, 1, 10), (0, 0, 6)]

Wait, the third test case in the program is (0,2,3), but in the sample input, it's (1,1,1). So, perhaps they are different.

Wait, maybe there's a mismatch between the sample input and the program's test cases.

Alternatively, perhaps the program has a mistake.

Wait, in the program, it's cas_de_test = [(0,0,0), (0,1,1), (0,2,3), (3,3,3), (3,4,5), (1,1,10), (0,0,6)]

But in the problem description, the test cases are:

1. 0 0 0 → 0

2. 0 1 1 → 1

3. 1 1 1 → -1

4. 1 1 2 → 2

5. 3 3 3 → -1

6. 3 4 5 → 6

7. 1 1 10 → 2

So, perhaps the program has different test cases.

Wait, but in the problem description, the third test case is p1=1, p2=1, p3=1, which is impossible because the sum is odd, so output -1.

But in the program, it's (0,2,3), which is different.

Wait, perhaps it's a typo in the problem description or the program.

Anyway, I need to focus on the logic of the program.

So, in the program:

- Check if p1 + p2 + p3 is even. If not, return -1.

- m = (p1 + p2 + p3) / 2

- If m > 3 or p3 > m, return -1

- egalites = p1 + p2 + p3 - 2*(p3 - p2) - 2*(p3 - p1)

- If egalites < 0, return -1

- Else, return egalites // 2

Wait, but as I calculated earlier, egalites = 3*(p1 + p2 - p3)

Is that correct?

Let’s check with sample input 4: p1=1, p2=1, p3=2

Sum = 4, m=2

egalites = 1 + 1 + 2 - 2*(2-1) - 2*(2-1) = 4 - 2 - 2 = 0

But according to the sample output, it should be 2.

So, the program would return 0, but the sample output is 2.

This suggests that the program is incorrect.

Wait, but maybe I'm misunderstanding something.

Let me check another sample input.

Sample input 6: p1=3, p2=4, p3=5

Sum=12, m=6

egalites =