`_acc` is initially calculated as \( A + (A + B) \% \text{MOD} \), `_max` is B, and `MOD` remains unchanged. The value of `i` is `k`. The code `_acc += (_acc + _max) \% \text{MOD}` increments `_acc` by the value of `(_acc + _max) \% \text{MOD}`.

First, let's calculate the initial value of `_acc`:
\[
\text{_acc} = A + (A + B) \% \text{MOD}
\]

Next, we need to calculate the value added to `_acc`:
\[
(\text{_acc} + \text{_max}) \% \text{MOD} = (A + (A + B) \% \text{MOD} + B) \% \text{MOD}
\]
Simplify the expression inside the modulo operation:
\[
A + (A + B) \% \text{MOD} + B = A + A + B + B \% \text{MOD} = 2A + 2B + (B \% \text{MOD})
\]
Thus, the updated `_acc` becomes:
\[
\text{_acc} = (A + (A + B) \% \text{MOD}) + (2A + 2B + (B \% \text{MOD})) \% \text{MOD}
\]
Since adding multiples of `MOD` does not affect the modulo result, we simplify further:
\[
\text{_acc} = (A + (A + B) \% \text{MOD} + 2A + 2B + B \% \text{MOD}) \% \text{MOD} = (3A + 3B + (A + B) \% \text{MOD} + B \% \text{MOD}) \% \text{MOD}
\]
This simplifies to:
\[
\text{_acc} = (3A + 3B + ((A + B) + B) \% \text{MOD}) \% \text{MOD} = (3A + 3B + (A + 2B) \% \text{MOD}) \% \text{MOD}
\]

So, the final value of `_acc` is:
\[
\text{_acc} = (3A + 3B + (A + 2B) \% \text{MOD}) \% \text{MOD}
\]

The states of the other variables remain unchanged.

Output State: **\_acc is \((3A + 3B + (A + 2B) \% \text{MOD}) \% \text{MOD}\), \_max is B, MOD is unchanged, i is k**