To determine the output of the `print` statement, let's break down the given initial state and the variables involved:

1. **Variables and Constraints:**
   - `t` is an integer such that \(1 \leq t \leq 500\). (This variable `t` is not used in the print statement, so we can ignore it for this task.)
   - `p_1`, `p_2`, and `p_3` are integers such that \(0 \leq p_1 \leq p_2 \leq p_3 \leq 30\).
   - `p1`, `p2`, and `p3` are the integers read from the input, and they satisfy the same constraints as `p_1`, `p_2`, and `p_3`.
   - The sum of `p1`, `p2`, and `p3` is odd.
   - `p3` is less than `p1 + p2`.
   - `low` is defined as `p3 - p1`.
   - `high` is at least `p3 - p2 + 1`.
   - `cur` is defined as `p3 - p2`.

2. **Expression to Evaluate:**
   - The print statement is `print(p1 - cur + p3)`.

3. **Substitute `cur`:**
   - Since `cur` is defined as `p3 - p2`, we can substitute `cur` in the expression:
     \[
     p1 - cur + p3 = p1 - (p3 - p2) + p3 = p1 - p3 + p2 + p3 = p1 + p2
     \]

4. **Final Expression:**
   - The expression simplifies to `p1 + p2`.

5. **Constraints on `p1` and `p2`:**
   - We know that \(0 \leq p_1 \leq p_2 \leq p_3 \leq 30\).
   - The sum \(p1 + p2 + p3\) is odd.
   - `p3` is less than `p1 + p2`, so \(p1 + p2 > p3\).

Given these constraints, the output of the print statement is the sum of `p1` and `p2`.

Output: **p1 + p2**