Let's break down the problem step-by-step based on the given initial state and the print statement.

### Initial State Recap:
- `t` is an integer such that 0 <= t <= 499.
- `p_1`, `p_2`, and `p_3` are integers such that 0 <= p_1 <= p_2 <= p_3 <= 30.
- The sum of `p1`, `p2`, and `p3` is odd.
- If `p3` is greater than or equal to the sum of `p1` and `p2`, then `p3 >= p1 + p2` holds. Otherwise, `p3` is less than the sum of `p1` and `p2`.
- `low` is the minimum of `p3 - p1` and `p3 - p2`.
- `high` is the maximum of `p3 - p1` and `p3 - p2`.
- `cur` is equal to `low`.
- `p1 - cur` is less than or equal to `p2 - (p3 - cur)`.

### Analysis:
1. **`p3 - p1` and `p3 - p2`**:
   - Since `p1 <= p2 <= p3`, `p3 - p1` and `p3 - p2` are non-negative integers.
   - `low` is the smaller of `p3 - p1` and `p3 - p2`.
   - `high` is the larger of `p3 - p1` and `p3 - p2`.

2. **`cur`**:
   - `cur` is set to `low`, which means `cur` is the smaller difference between `p3` and `p1` or `p3` and `p2`.

3. **Condition `p1 - cur <= p2 - (p3 - cur)`**:
   - This condition ensures that the value of `cur` is chosen such that the difference between `p1` and `cur` is not greater than the difference between `p2` and the remaining part of `p3` after subtracting `cur`.

4. **Print Statement**:
   - The print statement is `print(p1 - cur + p3)`.
   - We need to determine the value of `p1 - cur + p3`.

### Breaking Down the Expression `p1 - cur + p3`:
- `cur` is the minimum of `p3 - p1` and `p3 - p2`.
- If `cur = p3 - p1`, then `p1 - cur = p1 - (p3 - p1) = 2*p1 - p3`.
- If `cur = p3 - p2`, then `p1 - cur = p1 - (p3 - p2) = p1 - p3 + p2`.
- In either case, the expression `p1 - cur + p3` simplifies as follows:
  - If `cur = p3 - p1`: `p1 - cur + p3 = p1 - (p3 - p1) + p3 = 2*p1 - p3 + p3 = 2*p1`.
  - If `cur = p3 - p2`: `p1 - cur + p3 = p1 - (p3 - p2) + p3 = p1 - p3 + p2 + p3 = p1 + p2`.

However, given the condition `p1 - cur <= p2 - (p3 - cur)`, we can infer that `cur` is chosen to satisfy this inequality. This condition leans towards `cur` being `p3 - p2` when `p1` and `p2` are closer to each other compared to `p1` and `p3`.

### Conclusion:
Given the conditions and the nature of the problem, the expression `p1 - cur + p3` simplifies to `p1 + p2` when `cur = p3 - p2`.

### Output:
Output: **p1 + p2**