To determine the output of the `print(p1 - cur + p3)` statement, let's break down the given initial state and the relationships between the variables:

1. **Variables and Conditions:**
   - `t` is an integer such that 0 <= t <= 499 (This variable is not used in the `print` statement, so we can ignore it for this task).
   - `p_1`, `p_2`, and `p_3` are integers such that 0 <= p_1 <= p_2 <= p_3 <= 30.
   - `p1`, `p2`, and `p3` are the integers read from the input, and they satisfy the same constraints as `p_1`, `p_2`, and `p_3`.
   - The sum of `p1`, `p2`, and `p3` is odd.
   - If `p3` is greater than or equal to the sum of `p1` and `p2`, then the condition `p3 >= p1 + p2` holds. Otherwise, `p3` is less than the sum of `p1` and `p2`.
   - `low` is the minimum of `p3 - p1` and `p3 - p2`.
   - `high` is the maximum of `p3 - p1` and `p3 - p2`.
   - `cur` is such that `cur` is either `low` or `low + 1` and `low + 1 <= high`.

2. **Deriving the Output:**
   - We need to compute `p1 - cur + p3`.
   - `cur` can either be `low` or `low + 1`.

Let's analyze the possible values of `cur` and how they affect the output:

- **Case 1: `cur = low`**
  - `low` is the minimum of `p3 - p1` and `p3 - p2`.
  - If `cur = low`, then `p1 - cur + p3` becomes `p1 - (min(p3 - p1, p3 - p2)) + p3`.

- **Case 2: `cur = low + 1`**
  - If `cur = low + 1`, then `p1 - cur + p3` becomes `p1 - (min(p3 - p1, p3 - p2) + 1) + p3`.

To provide a more precise description, let's consider the constraints and the conditions:

- Since `p1 + p2 + p3` is odd, and `p1 <= p2 <= p3`, `p3` cannot be equal to `p1 + p2` (because `p3 >= p1 + p2` would make the sum even).
- Therefore, `p3` must be greater than `p1 + p2`.
- This implies `p3 - p1` and `p3 - p2` are both positive and `p3 - p2 < p3 - p1` (since `p1 <= p2`).

Given this, we have:
- `low = p3 - p2`
- `high = p3 - p1`
- `cur` can be `p3 - p2` or `p3 - p2 + 1`.

Let's calculate the output for both cases:
- If `cur = p3 - p2`, then `p1 - cur + p3 = p1 - (p3 - p2) + p3 = p1 - p3 + p2 + p3 = p1 + p2`.
- If `cur = p3 - p2 + 1`, then `p1 - cur + p3 = p1 - (p3 - p2 + 1) + p3 = p1 - p3 + p2 + p3 - 1 = p1 + p2 - 1`.

Since `cur` is either `low` or `low + 1`, and `low + 1 <= high`, the output can be either `p1 + p2` or `p1 + p2 - 1`.

Output: **p1 + p2 or p1 + p2 - 1 (depending on whether cur is p3 - p2 or p3 - p2 + 1)**