To determine what will be printed by the `print(p1 - cur + p3)` statement, let's break down the initial state and the variables involved step-by-step:

1. **Initial State and Conditions:**
   - `t` is an integer such that \(0 \leq t \leq 499\).
   - `p_1`, `p_2`, and `p_3` are integers such that \(0 \leq p_1 \leq p_2 \leq p_3 \leq 30\).
   - `p1`, `p2`, and `p3` are integers read from the input.
   - The sum of `p1`, `p2`, and `p3` is odd.
   - If `p3` is greater than or equal to the sum of `p1` and `p2`, then `p3 >= p1 + p2` holds. Otherwise, `p3` is less than the sum of `p1` and `p2`.
   - `low` is the minimum of `p3 - p1` and `p3 - p2`.
   - `high` is at least `low + 2`.
   - `cur` is either `low` or `low + 1` if `p1 - cur <= p2 - (p3 - cur)`, otherwise `cur` is either `low + 1` or `low + 2` and `low + 1 <= high`.

2. **Deriving `low` and `high`:**
   - `low = min(p3 - p1, p3 - p2)`
   - `high` is at least `low + 2`.

3. **Determining `cur`:**
   - `cur` is chosen based on the condition `p1 - cur <= p2 - (p3 - cur)`.
   - If the condition is true, `cur` can be either `low` or `low + 1`.
   - If the condition is false, `cur` can be either `low + 1` or `low + 2`, and `low + 1 <= high`.

4. **Expression to Print:**
   - The `print` statement outputs `p1 - cur + p3`.

To understand the output, let's consider the expression `p1 - cur + p3`:
- `p1` and `p3` are given input values.
- `cur` is determined based on the conditions mentioned above.

Since `cur` can be `low`, `low + 1`, or `low + 2`, the value of `p1 - cur + p3` will depend on the specific values of `p1`, `p2`, `p3`, and the condition `p1 - cur <= p2 - (p3 - cur)`.

Let's analyze the expression:
- `low = min(p3 - p1, p3 - p2)`
- If `cur = low`, then `p1 - cur + p3 = p1 - low + p3`.
- If `cur = low + 1`, then `p1 - cur + p3 = p1 - (low + 1) + p3`.
- If `cur = low + 2`, then `p1 - cur + p3 = p1 - (low + 2) + p3`.

Given the constraints and the conditions, the exact value of `cur` depends on the relationship between `p1`, `p2`, and `p3`. However, we can describe the output in terms of these variables.

Since `low` is the minimum of `p3 - p1` and `p3 - p2`, and `cur` is either `low`, `low + 1`, or `low + 2`, the output will be one of the following:
- `p1 - low + p3`
- `p1 - (low + 1) + p3`
- `p1 - (low + 2) + p3`

Given the conditions, the most precise description of the output is:

Output: **p1 - cur + p3 (where cur is either low, low + 1, or low + 2 based on the conditions provided)**