To determine the output of the given print statement, we need to carefully analyze the initial state and the relationships between the variables.

### Initial State Recap:
- `t` is an integer such that 1 <= t <= 499 (though `t` is not used in the print statement).
- `p1`, `p2`, and `p3` are integers such that 0 <= p1 <= p2 <= p3 <= 30.
- The sum of `p1`, `p2`, and `p3` is odd.
- If `p3` is greater than or equal to the sum of `p1` and `p2`, then the condition `p3 >= p1 + p2` holds.
- `low` is the minimum of `p3 - p1` and `p3 - p2`.
- `high` is the maximum of `p3 - p1` and `p3 - p2`.
- `cur` is equal to `low`.
- The current value of `cur` satisfies the condition `p1 - cur <= p2 - (p3 - cur)`.

### Analysis of the Print Statement:
The statement to be printed is:
```python
print(p1 - cur + p3)
```

Let's break down the expression `p1 - cur + p3`:

1. **Understanding `cur`**:
   - `cur` is set to `low`, which is the minimum of `p3 - p1` and `p3 - p2`.
   - Given `0 <= p1 <= p2 <= p3`, `p3 - p1` and `p3 - p2` are non-negative.
   - Since `p1 <= p2`, `p3 - p1 >= p3 - p2`. Thus, `low = p3 - p2`.

2. **Expression Simplification**:
   - Now, `cur = p3 - p2`.
   - Substitute `cur` in the expression: `p1 - cur + p3 = p1 - (p3 - p2) + p3`.
   - Simplify: `p1 - p3 + p2 + p3 = p1 + p2`.

### Conclusion:
The expression `p1 - cur + p3` simplifies to `p1 + p2`.

### Output:
Output: **p1 + p2**