Postcondition: ***`n` is a positive integer (1 <= n <= 10^5), `x` is an integer (-10^9 <= x <= 10^9), `cnt0` is the count of '0' in `s`, `cnt1` is the count of '1' in `s`, and `balance` is assigned the value `cnt0 - cnt1`. If `cnt0 - cnt1` is not equal to 0 and `(x - balance) % (cnt0 - cnt1) == 0`, the function prints -1. Otherwise, the function prints the result of `(x - balance) // (cnt0 - cnt1) + 1`, which is defined when `cnt0 - cnt1` is not zero. If `cnt0 - cnt1` is zero, the behavior is undefined, and special handling may be required for that case.***