Let's break down the initial state and the code snippet to determine what will be printed:

### Initial State:
- `n` and `m` are positive integers such that \(1 \leq n, m \leq 2 \times 10^6\).
- `T` is greater than 0.
- `t` is 0.
- `info` is a list of strings obtained from splitting the input.
- `a` is the integer value of `info[0]`.
- `b` is the integer value of `info[1]` and must be greater than or equal to its initial value.
- `i` is `b`.
- `suma` is the sum of \((a - i * (i - 1)) // i^2 + 1\) for all \(i\) from 1 to `b` where \(a - i * (i - 1) > 0\).

### Code Snippet:
```python
print(suma - 1)
```

### Step-by-Step Analysis:
1. **Understanding `info` and `a`, `b`:**
   - `info` is a list of strings obtained from splitting the input.
   - `a` is the integer value of `info[0]`.
   - `b` is the integer value of `info[1]`.

2. **Calculating `suma`:**
   - `suma` is the sum of \((a - i * (i - 1)) // i^2 + 1\) for all \(i\) from 1 to `b` where \(a - i * (i - 1) > 0\).
   - This means we need to iterate over \(i\) from 1 to `b` and add the value \((a - i * (i - 1)) // i^2 + 1\) to `suma` if \(a - i * (i - 1) > 0\).

3. **Evaluating the Expression:**
   - For each \(i\) from 1 to `b`, we check if \(a - i * (i - 1) > 0\).
   - If true, we compute \((a - i * (i - 1)) // i^2 + 1\) and add it to `suma`.

4. **Final Calculation:**
   - The code snippet `print(suma - 1)` will print the value of `suma` minus 1.

### Example Calculation:
Let's assume `a = 10` and `b = 3` for simplicity:
- For \(i = 1\):
  - \(a - i * (i - 1) = 10 - 1 * 0 = 10 > 0\)
  - \((10 - 1 * 0) // 1^2 + 1 = 10 // 1 + 1 = 11\)
- For \(i = 2\):
  - \(a - i * (i - 1) = 10 - 2 * 1 = 8 > 0\)
  - \((10 - 2 * 1) // 2^2 + 1 = 8 // 4 + 1 = 2 + 1 = 3\)
- For \(i = 3\):
  - \(a - i * (i - 1) = 10 - 3 * 2 = 4 > 0\)
  - \((10 - 3 * 2) // 3^2 + 1 = 4 // 9 + 1 = 0 + 1 = 1\)

So, `suma = 11 + 3 + 1 = 15`.

Finally, `print(suma - 1)` will print `15 - 1 = 14`.

### General Output:
Since the exact values of `a` and `b` are not provided, we can only describe the output in terms of the given formula and conditions.

Output: **suma - 1 (where suma is the sum of \((a - i * (i - 1)) // i^2 + 1\) for all \(i\) from 1 to `b` where \(a - i * (i - 1) > 0\))**