To analyze the code, we first need to evaluate the assignment taking into account the initial state of the variables.

Given:
- `left` is 1,
- `right` is `2^steps - 1`.

The code line provided is:
```
left = right = (right + left) / 2 + 1
```

1. Calculate the value of `(right + left) / 2 + 1`:
   - `right + left` = `(2^steps - 1) + 1` = `2^steps`.
   - Therefore, `(right + left) / 2` = `2^steps / 2` = `2^(steps - 1)`.
   - Adding 1 gives `2^(steps - 1) + 1`.

2. Now both `left` and `right` are assigned the value `2^(steps - 1) + 1`.

Since `left` and `right` are both set to `2^(steps - 1) + 1`, we conclude that the value of `left` becomes equal to `right`.

In the output state:
- The values of `left` and `right` are both `2^(steps - 1) + 1`.

Therefore, the Output State is: 
Output State: **`n` is an integer such that 1 ≤ `n` ≤ 50, `k` is an integer such that 1 ≤ `k` ≤ 2^`n` - 1, `steps` is now decremented by 1, `index` is an even integer not equal to `2^{steps - 1}`, `left` is `2^(steps - 1) + 1`, `right` is `2^(steps - 1) + 1`.**