The expression `right = (right + left) / 2 - 1` modifies the value of `right`. The previous values of `right` and `left` were not specified, so we cannot determine the exact new value of `right`. However, the operation combines the current values of `right` and `left`, averages them, and then subtracts 1. The variable `steps` is not affected by this operation.

Therefore, the Output State is: `n` is an integer such that 1 ≤ `n` ≤ 50; `k` is an integer such that 1 ≤ `k` ≤ 2^`n` - 1; `steps` is decremented by 1; `right` is modified based on its previous value and `left`.

Output State: **`n` is an integer such that 1 ≤ `n` ≤ 50; `k` is an integer such that 1 ≤ `k` ≤ 2^`n` - 1; `steps` is decremented by 1; `right` is modified based on its previous value and `left.**