The code snippet uses string formatting to concatenate parts of the strings `tem`, `ext4`, and `ext7`. Let's break down the steps:

1. **Concatenation Components:**
   - `tem[0]`: The first character of `tem`.
   - `ext4`: A string of `'4'` characters repeated `a[0] - four` times.
   - `tem[1:-1]`: All characters of `tem` except the first and last.
   - `ext7`: A string of `'7'` characters repeated `a[1] - seven` times.
   - `tem[-1]`: The last character of `tem`.

2. **String Formatting:**
   - The formatted string combines these components in the order specified.

Given the conditions:
- \((four \leq a[0] \land seven \leq a[1]) \lor (four2 \leq a[0] \land seven2 \leq a[1])\) still holds.
- `tem[-1]` is not equal to `'7'`.

Since `tem[-1]` is not `'7'`, `ext7` will be constructed using `a[1] - seven` characters. 

Let's denote:
- \( len\_tem = \text{length of } tem \)
- \( len\_ext4 = a[0] - four \)
- \( len\_ext7 = a[1] - seven \)

The resulting string will be:
- `tem[0]`: First character of `tem`.
- Followed by `len\_ext4` number of `'4'` characters.
- Followed by all characters of `tem` except the first and last.
- Followed by `len\_ext7` number of `'7'` characters.
- Ending with `tem[-1]`: Last character of `tem`.

Thus, the final output string will be constructed as follows:

Output State: **`tem[0] + '4' * (a[0] - four) + tem[1:len(tem)-1] + '7' * (a[1] - seven) + tem[-1]`**