Alright, I've got this problem to solve. Let's see what it's asking for. So, I'm given an array x_2, x_3, ..., x_n, and I need to find an array a_1, a_2, ..., a_n such that each a_i is between 1 and 10^9, and for each i from 2 to n, x_i equals a_i modulo a_{i-1}. The modulo operation gives the remainder when a_i is divided by a_{i-1}.

First, I need to understand what this means. Modulo operation has some properties that I should keep in mind. For any two integers a and b, where b is non-zero, a mod b is the remainder of the division of a by b. It's always non-negative and less than b. So, x_i = a_i mod a_{i-1} implies that x_i < a_{i-1}, because the remainder is always less than the divisor.

Given that, I need to find a sequence a_1, a_2, ..., a_n that satisfies these conditions. The problem allows me to choose any a that meets these criteria, so I don't need to find all possible solutions, just one that works.

Let me consider the constraints:

- 1 ≤ a_i ≤ 10^9 for all 1 ≤ i ≤ n.

- x_i = a_i mod a_{i-1} for all 2 ≤ i ≤ n.

- The input consists of multiple test cases, with t test cases, each having its own n and x array.

- The sum of n over all test cases doesn't exceed 2*10^5, which is manageable.

Given that n can be up to 500 per test case and t up to 10^4, but the total sum of n is limited to 2*10^5, I need an efficient solution.

Let's think about how to approach this. Starting from a_1, I need to determine a_2 such that a_2 mod a_1 = x_2. Similarly, a_3 mod a_2 = x_3, and so on.

One way to think about this is to choose a_1 first, and then choose each subsequent a_i based on the previous one and x_i.

But the given solution seems to be taking a different approach. It's setting ans = [10^9] * n, meaning initializing all a_i to 10^9, and then starting from the end and setting ans[i] = ans[i+1] - x[i].

Wait, that seems suspicious. If I set a_i = a_{i+1} - x_i, then a_i might become negative if a_{i+1} < x_i, which isn't allowed since a_i >=1. Also, I need to ensure that a_i mod a_{i-1} = x_i, which might not hold with this approach.

Let me verify this with the first example:

Input:

5

4

2 4 1

Output:

3 5 4 9

Let's see:

a1 = 3

a2 = 5

a3 = 4

a4 = 9

Check:

a2 mod a1 = 5 mod 3 = 2 = x2

a3 mod a2 = 4 mod 5 = 4 = x3

a4 mod a3 = 9 mod 4 = 1 = x4

This seems correct.

Now, according to the given program, it initializes ans = [10^9, 10^9, 10^9, 10^9]

Then, for i from n-2 down to 0:

ans[i] = ans[i+1] - x[i]

So, for i=2:

ans[2] = ans[3] - x[2] = 10^9 - 1 = 999999999

Then for i=1:

ans[1] = ans[2] - x[1] = 999999999 - 4 = 999999995

Then for i=0:

ans[0] = ans[1] - x[0] = 999999995 - 2 = 999999993

So, ans = [999999993, 999999995, 999999999, 1000000000]

Now, check:

a2 mod a1 = 999999995 mod 999999993 = 2 = x2

a3 mod a2 = 999999999 mod 999999995 = 4 = x3

a4 mod a3 = 1000000000 mod 999999999 = 1 = x4

So, this also satisfies the conditions. Therefore, the given program is correct for this test case.

Wait, but in the sample output, they have a different solution: 3,5,4,9. So, multiple solutions are possible, which is fine, as long as one is found.

Let me see another test case:

Input:

3

1 1

Output:

2 5 11

Check:

a1=2

a2=5

a3=11

x2=1, x3=1

Check:

5 mod 2 = 1 (correct)

11 mod 5 = 1 (correct)

Now, according to the program:

Initialize ans = [10^9, 10^9, 10^9]

Set ans[1] = ans[2] - x[1] = 10^9 -1 = 999999999

ans[0] = ans[1] - x[0] = 999999999 -1 = 999999998

So, ans = [999999998, 999999999, 1000000000]

Check:

a2 mod a1 = 999999999 mod 999999998 = 1 (correct)

a3 mod a2 = 1000000000 mod 999999999 = 1 (correct)

Again, it works.

Another test case:

Input:

2

500

Output:

501 500

Check:

a1=501

a2=500

x2=500

Check:

500 mod 501 = 500 (correct)

According to the program:

ans = [10^9, 10^9]

ans[0] = ans[1] - x[0] = 10^9 -500 = 999999500

So, ans = [999999500, 1000000000]

Check:

a2 mod a1 = 1000000000 mod 999999500 = 500 (correct)

So, again, it works.

Wait, but in the sample output, they have [501,500], which also works.

So, seems like the program is correct.

But I need to think if there are cases where this approach fails.

Consider that a_i must be greater than x_i, because a_i mod a_{i-1} = x_i, which implies that a_i >= x_i.

Also, a_i can be equal to x_i + k*a_{i-1} for some integer k >=0, but since we are dealing with modulo, a_i can be x_i + m*a_{i-1}, where m is an integer.

But in the program's approach, it sets a_i = a_{i+1} - x_i.

Wait, but a_{i+1} can be very large, up to 10^9, so a_i could be up to 10^9 -1, which is still within the limit.

But is this always correct?

Wait, no. If a_{i+1} < x_i, then a_i = a_{i+1} - x_i would be negative, which is invalid.

But according to the problem, x_i <=500, and a_{i+1} >=1, but a_{i+1} could be up to 10^9, so a_{i+1} - x_i could be as low as 1 -500 = -499, which is negative, which is invalid.

Wait, but in the program, all a_i are initialized to 10^9, which is much larger than x_i, so a_{i+1} - x_i would be 10^9 - x_i, which is still positive, since x_i <=500.

Wait, but in the last element, a_n is set to 10^9, and a_{n-1} = 10^9 - x_{n-1}, which is 10^9 - x_{n-1}, which is positive since x_{n-1} <=500.

Similarly, a_{n-2} = a_{n-1} - x_{n-2} = (10^9 - x_{n-1}) - x_{n-2}, which could be potentially less than 1 if x_{n-1} + x_{n-2} >=10^9.

Wait, but in the constraints, n can be up to 500, and x_i up to 500, so the sum of x_i could be up to 500*500=250,000, which is less than 10^9.

Wait, no, n-1 up to 499, x_i up to 500, so sum up to 499*500=249,500, which is still less than 10^9.

Therefore, a_1 = a_2 - x_1 = (a_3 - x_2) - x_1 = ... = 10^9 - sum(x_{n-1} to x_1), which is at least 10^9 - 249,500 >1, so a_1 is always positive.

Hence, no issue there.

Now, does this always satisfy a_i mod a_{i-1} = x_i?

Let's see.

Given a_i = a_{i+1} - x_i.

We need to check if a_{i+1} mod a_i = x_{i+1}.

Wait, no, we need to check if a_i mod a_{i-1} = x_i.

Wait, in the program's approach, a_i = a_{i+1} - x_i.

Then, a_i mod a_{i-1} = (a_{i+1} - x_i) mod a_{i-1}.

But I need this to be equal to x_i.

Wait, that doesn't seem right.

Wait, perhaps there's a different way to look at it.

Let me consider the relationship.

I need a_i mod a_{i-1} = x_i.

Which means a_i = k*a_{i-1} + x_i, for some integer k >=0.

So, a_i = k*a_{i-1} + x_i.

The program sets a_i = a_{i+1} - x_i.

But in this approach, it's not directly related to a_{i-1}.

Wait, maybe there's a different way to see this.

Let me consider building the array from the end.

Suppose I set a_n to some value, say 10^9.

Then, a_{n-1} should satisfy a_n mod a_{n-1} = x_n.

Wait, no, x_n = a_n mod a_{n-1}.

But according to the problem, x_i = a_i mod a_{i-1}.

Wait, in the program, it's setting a_i = a_{i+1} - x_i.

But according to the problem, x_{i+1} = a_{i+1} mod a_i.

Wait, I think there's confusion in indexing.

Wait, in the problem, x_i = a_i mod a_{i-1}.

But in the program, it's setting ans[i] = ans[i+1] - x[i].

Wait, perhaps it's better to think of it differently.

Suppose I set a_n to some value, say 10^9.

Then, for a_{n-1}, I need a_{n-1} such that a_n mod a_{n-1} = x_n.

Which means a_n = k*a_{n-1} + x_n for some integer k.

So, a_{n-1} = (a_n - x_n)/k, for some integer k.

But this seems complicated.

Alternatively, to make it simpler, I can choose a_{n-1} such that a_n = m*a_{n-1} + x_n, for some integer m.

To simplify, I can choose a_{n-1} such that a_n - x_n is divisible by a_{n-1}.

But this seems tricky.

Alternatively, I can choose a_{n-1} to be greater than x_n, and set a_n = a_{n-1} + x_n.

Then, a_n mod a_{n-1} = x_n, because (a_{n-1} + x_n) mod a_{n-1} = x_n.

This seems to work.

Similarly, for a_{n-2}, I can set a_{n-2} = a_{n-1} + x_{n-1}, and so on.

Wait, but in the program, it's setting a_i = a_{i+1} - x_i.

Which is different from a_i = a_{i+1} + x_i.

So, perhaps there's a different logic.

Wait, maybe I need to think recursively.

Let me consider the last element.

Set a_n = some value, say 10^9.

Then, set a_{n-1} = a_n - x_n.

Then, check if a_n mod a_{n-1} = x_n.

Let's see: a_n mod (a_n - x_n) should equal x_n.

Is that true?

Let's compute a_n mod (a_n - x_n).

We have a_n = (a_n - x_n) + x_n.

So, a_n mod (a_n - x_n) = x_n.

Yes, that's correct.

Because a_n = (a_n - x_n) + x_n, so the remainder when dividing a_n by (a_n - x_n) is x_n.

Hence, this satisfies the condition.

Similarly, for a_{n-2}, set a_{n-2} = a_{n-1} - x_{n-1}.

Then, a_{n-1} mod a_{n-2} should equal x_{n-1}.

Let's check: a_{n-1} = a_{n-2} + x_{n-1}.

Wait, no: a_{n-2} = a_{n-1} - x_{n-1}.

So, a_{n-1} = a_{n-2} + x_{n-1}.

Then, a_{n-1} mod a_{n-2} = (a_{n-2} + x_{n-1}) mod a_{n-2} = x_{n-1}.

Which is correct.

So, this approach works.

Therefore, the given program is correct.

Hence, Correctness: **True**

**Final Solution**

To solve this problem, we need to find an array \( a_1, a_2, \dots, a_n \) such that each element satisfies the condition \( x_i = a_i \bmod a_{i-1} \) for \( 2 \leq i \leq n \), given the constraints \( 1 \leq a_i \leq 10^9 \).

## Approach
1. **Initialization**: Start by initializing all elements of the array \( a \) to a large value, specifically \( 10^9 \).
2. **Backward Calculation**: Traverse the array from the second last element to the first element.
   - For each element \( a_i \), set \( a_i = a_{i+1} - x_i \).
3. **Validation**: Ensure that all \( a_i \) values are positive, which is guaranteed given the constraints on \( n \) and \( x_i \).

This approach leverages the properties of the modulo operation. By setting \( a_i = a_{i+1} - x_i \), we ensure that \( a_{i+1} \bmod a_i = x_i \), provided \( a_{i+1} > x_i \), which holds true due to the initial large value assignment.

## Solution Code
```python
t = int(input())
while t:
    n = int(input())
    arr = [int(x) for x in input().split(' ')]
    ans = func_1(arr, n)
    for i in ans:
        print(i, end=' ')
    print()
    t -= 1

def func_1(arr, n):
    ans = [10**9] * n
    i = n - 2
    while i >= 0:
        ans[i] = ans[i + 1] - arr[i]
        i -= 1
    return ans
```

## Explanation
- **Initialization**: We initialize the array `ans` with \( 10^9 \) for all elements.
- **Backward Calculation**: Starting from the second last element (index \( n-2 \)) down to the first element (index 0), we set each \( a_i \) to \( a_{i+1} - x_i \).
- **Output**: For each test case, we print the resulting array `ans`.

This method ensures that each \( a_i \) is calculated such that \( a_{i+1} \bmod a_i = x_i \), fulfilling the problem's requirements efficiently.