`ans` is updated by adding the difference between `l` and `pos`. Since the current value of `pos` is less than `l`, the expression `l - pos` will yield a positive value. Therefore, `ans` will now be equal to `l - pos`. The states of the other variables remain unchanged.

Output State: **`n` is an input positive integer (1 ≤ n ≤ 100), `pos` is an input integer (1 ≤ pos ≤ n), `l` is an input positive integer (1 ≤ l ≤ r ≤ n), `r` is an input positive integer (1 ≤ r ≤ n), `ans` is equal to `l - pos`.**