The code snippet `ans[i + 1] += ans[i]` updates the value of `ans[1]` by adding `ans[0]` to it. Given the initial state, let's break down the impact:

- `ans[0]` is `arr[0] + 1`.
- `ans[1]` is initially `3 * arr[0] + 2 + arr[0] + 1`, which simplifies to `4 * arr[0] + 3`.
- The code adds `ans[0]` (which is `arr[0] + 1`) to `ans[1]` (which is `4 * arr[0] + 3`).

So, the new value of `ans[1]` is:
\[ \text{ans[1]} = 4 * \text{arr[0]} + 3 + \text{arr[0]} + 1 = 5 * \text{arr[0]} + 4 \]

The rest of the variables and conditions remain unchanged. Therefore, the output state is:

Output State: **`arr` is a list of integers such that \(1 \leq \text{arr}[i] \leq 500\) for all \(1 \leq i < n\), `n` is an integer such that \(3 \leq n \leq 500\), `ans` is a list of `n` integers where `ans[0]` is `arr[0] + 1`, `ans[1]` is `5 * arr[0] + 4`, and the rest of the elements in `ans` are zeros, `i` is 0, and `ans[1]` is less than `arr[1]`**.