The initial state includes:
- `vp` is an integer entered by the user and satisfies `vp <= c`
- `vd` must be such that `vp * (3 + f * (vp / vd)) + vp <= c`
- `t` is 2
- `f` is an integer entered by the user
- `c` is the integer input from `raw_input()`
- `t_read` is an integer entered by the user through `raw_input()`
- `pl` is `vp * (2 + f * (vp / vd)) + vp`
- `dl` is equal to `pl`
- `count` is 1

The code snippet modifies `pl` by the following calculation:
```python
pl += (2 * (dl / vd) + f) * vp
```

Given `dl` is equal to `pl`, we substitute `dl` with `pl` in the code snippet:
```python
pl += (2 * (pl / vd) + f) * vp
```

Since `pl = vp * (2 + f * (vp / vd)) + vp`, let's substitute this into the equation:
```python
pl += (2 * ((vp * (2 + f * (vp / vd)) + vp) / vd) + f) * vp
```

Simplifying the expression:
```python
pl += (2 * (vp * (2 + f * (vp / vd)) / vd + vp / vd) + f) * vp
pl += (2 * (vp * (2 / vd + f * (vp / (vd * vd))) + vp / vd) + f) * vp
pl += (2 * (vp * (2 / vd + f * (vp / (vd * vd))) + vp / vd) + f) * vp
pl += (2 * (vp * (2 / vd + f * (vp / (vd * vd))) + vp / vd) + f) * vp
pl += (2 * (vp * (2 / vd + f * (vp / (vd * vd))) + vp / vd) + f) * vp
pl += (2 * (vp * (2 / vd + f * (vp / (vd * vd))) + vp / vd) + f) * vp
```

After simplifying:
```python
pl += (2 * (vp * (2 / vd + f * (vp / (vd * vd))) + vp / vd) + f) * vp
```

This results in updating `pl` by adding `(2 * (vp * (2 / vd + f * (vp / (vd * vd))) + vp / vd) + f) * vp` to its current value.

Output State: **`vp` is an integer entered by the user and satisfies `vp <= c`; `vd` must be such that `vp * (3 + f * (vp / vd)) + vp <= c`; `t` is 2; `f` is an integer entered by the user; `c` is the integer input from `raw_input()`; `t_read` is an integer entered by the user through `raw_input()`; `pl` is updated to `pl + (2 * (vp * (2 / vd + f * (vp / (vd * vd))) + vp / vd) + f) * vp`; `dl` is equal to `pl`; `count` is 1.**