To determine what will be printed by the `print(ans)` statement, let's break down the initial state and the code snippet step by step.

### Initial State:
- `n` remains unchanged.
- `k` remains unchanged.
- `ans` is updated to `n` plus the sum of `(n + i) // (i * i)` for all `i` from 2 to `root` inclusive.
- `root` remains unchanged.

### Variables and Objects:
- `n`: An integer value that remains unchanged.
- `k`: An integer value that remains unchanged.
- `ans`: Initially, `ans` is some value, but it is updated to `n` plus the sum of the expression `(n + i) // (i * i)` for all `i` from 2 to `root` inclusive.
- `root`: An integer value that remains unchanged.

### Calculation:
The value of `ans` is calculated as follows:
1. Start with the initial value of `ans` (which we don't know explicitly).
2. Add `n` to the initial value of `ans`.
3. For each `i` from 2 to `root` inclusive, compute the value of `(n + i) // (i * i)`.
4. Sum all these computed values.
5. Add this sum to `n`.

### Example Calculation:
Let's assume some values to understand the calculation better:
- Suppose `n = 10` and `root = 5`.

The calculation for `ans` would be:
- `ans` is updated to `10` plus the sum of `(10 + i) // (i * i)` for `i` from 2 to 5.

Let's compute each term:
- For `i = 2`: `(10 + 2) // (2 * 2) = 12 // 4 = 3`
- For `i = 3`: `(10 + 3) // (3 * 3) = 13 // 9 = 1`
- For `i = 4`: `(10 + 4) // (4 * 4) = 14 // 16 = 0`
- For `i = 5`: `(10 + 5) // (5 * 5) = 15 // 25 = 0`

Sum of these terms: `3 + 1 + 0 + 0 = 4`

So, `ans` is updated to `10 + 4 = 14`.

### General Description:
The value of `ans` is the sum of `n` and the sum of the expression `(n + i) // (i * i)` for all `i` from 2 to `root` inclusive.

### Final Output:
The `print(ans)` statement will print the value of `ans` which is `n` plus the sum of `(n + i) // (i * i)` for all `i` from 2 to `root` inclusive.

Output: **ans (where ans is the value of n plus the sum of (n + i) // (i * i) for all i from 2 to root inclusive)**