### Reasoning:

1. **Understanding the Problem:**
   - The goal is to maximize the sum of all elements in an \( n \times n \) matrix.
   - We can perform two types of operations: Type 1 (assign a permutation to a row) and Type 2 (assign a permutation to a column).
   - The maximum possible sum is \( n \times \frac{n(n+1)}{2} \), which is the sum of all integers from 1 to \( n \) repeated \( n \) times.

2. **Analyzing the Provided Program:**
   - The program starts by reading the number of test cases \( t \).
   - For each test case, it reads the size of the matrix \( n \).
   - It calculates the sum using the formula \( \text{sum} = 1 + \sum_{i=2}^{n} (i^2 - (i-1)^2) \times i \).
   - It prints the calculated sum and \( 2n \) (the number of operations).
   - It then performs \( n \) Type 1 operations and \( n \) Type 2 operations, each using the permutation \( [1, 2, \ldots, n] \).

3. **Sum Calculation:**
   - The sum calculation in the program is:
     \[
     \text{sum} = 1 + \sum_{i=2}^{n} (i^2 - (i-1)^2) \times i
     \]
   - Simplifying the term inside the sum:
     \[
     i^2 - (i-1)^2 = i^2 - (i^2 - 2i + 1) = 2i - 1
     \]
   - Therefore, the sum becomes:
     \[
     \text{sum} = 1 + \sum_{i=2}^{n} (2i - 1) \times i
     \]
   - Expanding the sum:
     \[
     \text{sum} = 1 + \sum_{i=2}^{n} (2i^2 - i)
     \]
   - This can be further simplified:
     \[
     \text{sum} = 1 + 2 \sum_{i=2}^{n} i^2 - \sum_{i=2}^{n} i
     \]
   - The sum of squares from 2 to \( n \) is:
     \[
     \sum_{i=2}^{n} i^2 = \sum_{i=1}^{n} i^2 - 1^2 = \frac{n(n+1)(2n+1)}{6} - 1
     \]
   - The sum of integers from 2 to \( n \) is:
     \[
     \sum_{i=2}^{n} i = \sum_{i=1}^{n} i - 1 = \frac{n(n+1)}{2} - 1
     \]
   - Substituting these back:
     \[
     \text{sum} = 1 + 2 \left( \frac{n(n+1)(2n+1)}{6} - 1 \right) - \left( \frac{n(n+1)}{2} - 1 \right)
     \]
     \[
     \text{sum} = 1 + \frac{n(n+1)(2n+1)}{3} - 2 - \frac{n(n+1)}{2} + 1
     \]
     \[
     \text{sum} = \frac{n(n+1)(2n+1)}{3} - \frac{n(n+1)}{2}
     \]
     \[
     \text{sum} = \frac{2n(n+1)(2n+1) - 3n(n+1)}{6}
     \]
     \[
     \text{sum} = \frac{n(n+1)(4n + 2 - 3)}{6}
     \]
     \[
     \text{sum} = \frac{n(n+1)(4n - 1)}{6}
     \]
   - This is not the correct formula for the maximum sum, which should be:
     \[
     \text{sum} = n \times \frac{n(n+1)}{2}
     \]

4. **Operations:**
   - The program performs \( n \) Type 1 operations and \( n \) Type 2 operations, each using the permutation \( [1, 2, \ldots, n] \).
   - This ensures that each row and each column will contain the permutation \( [1, 2, \ldots, n] \), which is the correct approach to maximize the sum of the matrix.

5. **Conclusion:**
   - The sum calculation in the program is incorrect.
   - However, the operations performed are correct and will indeed maximize the sum of the matrix.

### Final Evaluation:
The original assessment is correct. The program is incorrect because the sum calculation is wrong. The correct sum should be \( n \times \frac{n(n+1)}{2} \), not the sum calculated by the provided formula. Despite this, the operations performed are correct and will maximize the sum of the matrix.

Final: **False**