`D` is assigned the value of `L - M`. From the initial state, we know:
- \( G = \text{func\_1}(a, b) \)
- \( L = \text{func\_2}(a, b) \)
- \( M = \left( \frac{L}{b} - 1 \right) \times G \)

Substituting \( M \) into the equation for \( D \):
\[ D = L - \left( \left( \frac{L}{b} - 1 \right) \times G \right) \]
\[ D = L - \left( \frac{L}{b} \times G - G \right) \]
\[ D = L - \frac{L \times G}{b} + G \]
\[ D = L + G - \frac{L \times G}{b} \]

The states of the other variables are not affected. Therefore, the Output State is:
**`a` is a positive integer, `b` is a positive integer with `a â‰  b`, `G` is the result of `func_1(a, b)`, `L` is the result of `func_2(a, b)`, `M` is \(\left(\frac{L}{b} - 1\right) \times G\), `D` is \(L + G - \frac{L \times G}{b}\)**