Let's break down the initial state and the expression to be printed step by step:

1. **Initial State:**
   - `t` is `k-1`
   - `p1` is an input integer
   - `p2` is an input integer
   - `p3` is an input integer
   - `low` is `min(p3 - p1, p3 - p2)`
   - `high` is `max(p3 - p1, p3 - p2)`
   - `cur` is `low`
   - `(p1 - cur <= p2 - (p3 - cur))`

2. **Expression to be printed:**
   ```python
   print(p1 - cur + p3)
   ```

3. **Determine the value of `cur`:**
   - Since `cur` is defined as `low`, we need to find the value of `low`.
   - `low` is `min(p3 - p1, p3 - p2)`, which means `low` is the smaller of the two values `p3 - p1` and `p3 - p2`.

4. **Substitute `cur` with `low` in the expression:**
   - The expression becomes `p1 - low + p3`.

5. **Simplify the expression:**
   - We know that `low` is either `p3 - p1` or `p3 - p2`, so let's consider both cases:
     - If `low = p3 - p1`, then the expression becomes `p1 - (p3 - p1) + p3 = p1 - p3 + p1 + p3 = 2 * p1`.
     - If `low = p3 - p2`, then the expression becomes `p1 - (p3 - p2) + p3 = p1 - p3 + p2 + p3 = p1 + p2`.

6. **Check the condition `(p1 - cur <= p2 - (p3 - cur))`:**
   - This condition must hold true for the expression to be evaluated correctly.
   - Substituting `cur` with `low`:
     - If `low = p3 - p1`, the condition becomes `p1 - (p3 - p1) <= p2 - (p3 - (p3 - p1))` which simplifies to `2 * p1 - p3 <= p2 + p1 - p3` or `p1 <= p2`.
     - If `low = p3 - p2`, the condition becomes `p1 - (p3 - p2) <= p2 - (p3 - (p3 - p2))` which simplifies to `p1 + p2 - p3 <= p2` or `p1 <= p3`.

7. **Conclusion:**
   - Given the condition `(p1 - cur <= p2 - (p3 - cur))` must hold, we can determine that the correct value of `low` is `p3 - p1` if `p1 <= p2`, and `p3 - p2` if `p1 > p2`.
   - Therefore, the expression `p1 - cur + p3` will evaluate to either `2 * p1` or `p1 + p2` depending on the relationship between `p1` and `p2`.

Since the exact values of `p1` and `p2` are not specified, we can only describe the result in terms of these variables.

Output: **2 * p1 (if p1 <= p2) or p1 + p2 (if p1 > p2)**