To determine the output of the `print(suma - 1)` statement, we need to carefully analyze the given initial state and the provided code snippet.

### Initial State Breakdown:
1. **T**: An integer greater than 0.
2. **info**: A list of substrings from the new input.
3. **n and m**: These are mentioned but not explicitly defined in the initial state. However, they are not directly used in the provided code snippet.
4. **t**: Initialized to 1.
5. **a**: The integer value of `info[0]`.
6. **b**: The integer value of `info[1]`.
7. **i**: Initially set to `b + 1` after the loop ends.
8. **suma**: The sum of all `x` values calculated for each `i` from 1 to `b` where `a - i * (i - 1) > 0`.

### Calculation of `suma`:
- `suma` is the sum of `x` values where `x` is calculated as `a - i * (i - 1)` for each `i` from 1 to `b`.
- The loop runs for `i` from 1 to `b` and only adds `x` to `suma` if `a - i * (i - 1) > 0`.

### Final Calculation:
- The `print(suma - 1)` statement will print the value of `suma` minus 1.

### Step-by-Step Calculation:
1. **Initialization**: `suma` is initialized to 0.
2. **Loop Execution**:
   - For each `i` from 1 to `b`, compute `x = a - i * (i - 1)`.
   - If `x > 0`, add `x` to `suma`.
3. **Final Output**:
   - After the loop, `suma` will hold the sum of all valid `x` values.
   - The final printed value will be `suma - 1`.

### Example Calculation:
Let's assume `a = 10` and `b = 4` for concreteness.

- For `i = 1`: `x = 10 - 1 * 0 = 10` (add to `suma`), `suma = 10`.
- For `i = 2`: `x = 10 - 2 * 1 = 8` (add to `suma`), `suma = 18`.
- For `i = 3`: `x = 10 - 3 * 2 = 4` (add to `suma`), `suma = 22`.
- For `i = 4`: `x = 10 - 4 * 3 = -2` (do not add to `suma`), `suma = 22`.

Thus, `suma = 22`, and the printed value will be `22 - 1 = 21`.

### Generalized Output:
Based on the provided initial state and the logic of the code, the final printed value will be `suma - 1`.

Output: **suma - 1 (where suma is the sum of all x values calculated for each i from 1 to b where a - i * (i - 1) > 0)**