Let's break down the problem step by step:

1. **Initial State:**
   - `t` is an integer between 1 and \(10^4\), inclusive, and greater than 0.
   - `r` is the minimum of `w` and `b + x`.
   - `w`, `b`, `a`, `c`, `d`, `x`, and `l` retain their original values.
   - `l` is the maximum of 1 and `b - x`.

2. **Expression Analysis:**
   - We need to evaluate the expression `abs(l - d) <= x and abs(r - d) <= x`.

3. **Evaluate `r`:**
   - Since `r` is the minimum of `w` and `b + x`, we have:
     \[
     r = \min(w, b + x)
     \]

4. **Evaluate `l`:**
   - Since `l` is the maximum of 1 and `b - x`, we have:
     \[
     l = \max(1, b - x)
     \]

5. **Evaluate `abs(l - d) <= x`:**
   - This checks if the absolute difference between `l` and `d` is less than or equal to `x`.

6. **Evaluate `abs(r - d) <= x`:**
   - This checks if the absolute difference between `r` and `d` is less than or equal to `x`.

7. **Final Expression:**
   - The expression `abs(l - d) <= x and abs(r - d) <= x` will be true if both conditions are satisfied.

8. **Print Statement:**
   - The print statement uses a conditional expression:
     \[
     \text{print}\left(*\left(['Draw'], ['Bob']\right)[\text{abs}(l - d) \leq x \text{ and } \text{abs}(r - d) \leq x]\right)
     \]
   - If the condition is true, it will print `['Draw']`, otherwise it will print `['Bob']`.

Given the initial state and the conditions, let's assume specific values for `w`, `b`, `x`, and `d` to illustrate the logic. For simplicity, let's assume:
- `w = 10`
- `b = 5`
- `x = 2`
- `d = 3`

Then:
- `r = \min(10, 5 + 2) = \min(10, 7) = 7`
- `l = \max(1, 5 - 2) = \max(1, 3) = 3`

Now, evaluating the conditions:
- `abs(l - d) = abs(3 - 3) = 0`, which is <= x (since x = 2).
- `abs(r - d) = abs(7 - 3) = 4`, which is not <= x (since x = 2).

Since the condition `abs(l - d) <= x and abs(r - d) <= x` is false, the print statement will output `['Bob']`.

Output: **['Bob']**