`b` is assigned the value of `(n + a - 1) // a`. Given that `a` is 1, this simplifies to `b = (n + 1 - 1) // 1`, which further simplifies to `b = n // 1`. Since `b` is the result of dividing a positive integer `n` by 1, `b` will be equal to `n`. The states of the other variables remain unaffected. Therefore, the Output State is: `n` is a positive integer such that 1 <= n <= 10^9, `a` is 1, and `b` is equal to `n`.

Output State: **`n` is a positive integer such that 1 <= n <= 10^9, `a` is 1, `b` is equal to `n`.**