Output State: The value of `size` will be the highest integer such that \(2^{(size + 1)} - 1 \leq number\).

To understand this, let's break down the loop condition:

The expression `(1 << size + 1) - 1` is equivalent to \(2^{(size + 1)} - 1\). This means the loop continues as long as \(2^{(size + 1)} - 1\) is less than or equal to `number`. 

For example, if `number` is 15:
- When `size` is 0, \(2^{(0 + 1)} - 1 = 1\), which is less than 15, so the loop runs.
- When `size` is 1, \(2^{(1 + 1)} - 1 = 3\), which is still less than 15, so the loop runs again.
- When `size` is 2, \(2^{(2 + 1)} - 1 = 7\), which is still less than 15, so the loop runs again.
- When `size` is 3, \(2^{(3 + 1)} - 1 = 15\), which is equal to 15, so the loop runs one last time.
- When `size` is 4, \(2^{(4 + 1)} - 1 = 31\), which is greater than 15, so the loop stops.

Thus, for `number` = 15, the final value of `size` will be 3.

In general, the value of `size` will be the largest integer such that \(2^{(size + 1)} - 1 \leq number\).