Postcondition: **`n` and `m` are positive integers such that \(1 \leq n, m \leq 2 \times 10^6\), `T` is greater than 0, `t` is 1, `info` is a list of strings from the input, `a` is the integer value of the first string in `info`, `b` is the integer value of the second string in `info` and must be greater than or equal to 2, `x` is \((a - 2) // 4 + 1\), `i` is 2. If \((a - i * (i - 1)) % i ** 2 == 0\) and \(i * (i - 1) % i ** 2 == 0\), then `suma` is increased by \((a - 2) // 4 + 2\). Otherwise, `suma` is increased by \((a - 2) // 4 + 1\).**