To determine the output state, let's analyze the given code and initial conditions step by step.

1. `n` equals the first input integer.
2. `pos` equals the second input integer.
3. `l` equals the third input integer.
4. `r` equals the fourth input integer.
5. `1 <= n <= 100`.
6. `1 <= pos <= n`.
7. `1 <= l <= r <= n`.
8. `l` is not equal to 1.
9. `r` is not equal to `n`.
10. `move_to_l` equals `abs(pos - l)`.
11. `move_to_r` equals `abs(pos - r)`.

The code calculates `close_both_sides` as the minimum between `move_to_l + (r - l + 2)` and `move_to_r + (r - l + 2)`.

Given that `move_to_l = abs(pos - l)` and `move_to_r = abs(pos - r)`, the expressions for `close_both_sides` can be written in terms of the initial variables as follows:

- `move_to_l + (r - l + 2) = abs(pos - l) + (r - l + 2)`
- `move_to_r + (r - l + 2) = abs(pos - r) + (r - l + 2)`

Since `close_both_sides` is the minimum of these two expressions, its value depends on which of `move_to_l` or `move_to_r` is smaller, considering the additional constant `(r - l + 2)` is the same for both.

The initial conditions regarding the ranges of `n`, `pos`, `l`, and `r`, as well as the conditions that `l` is not equal to 1 and `r` is not equal to `n`, remain unchanged as they are not affected by the calculation of `close_both_sides`.

Thus, the output state includes all the initial conditions plus the new variable `close_both_sides`, which is equal to the minimum of `abs(pos - l) + (r - l + 2)` and `abs(pos - r) + (r - l + 2)`.

Output State: **`n` equals the first input integer, `pos` equals the second input integer, `l` equals the third input integer, `r` equals the fourth input integer, `1 <= n <= 100`, `1 <= pos <= n`, `1 <= l <= r <= n`, `l` is not equal to 1, `r` is not equal to `n`, `move_to_l` equals `abs(pos - l)`, `move_to_r` equals `abs(pos - r)`, and `close_both_sides` equals `min(abs(pos - l) + (r - l + 2), abs(pos - r) + (r - l + 2))`.**