The code updates the value of `k` to be the sum of `a` and `b` minus 1. Since `a` and `b` are positive integers, the value of `k` will be `a + b - 1`. The other variables remain unchanged. Therefore, the Output State is: `m` is a non-negative integer such that \(1 \leq m \leq 10^9\), `a` is a positive integer such that \(1 \leq a \leq 10^5\), `b` is a positive integer such that \(1 \leq b \leq 10^5\), `g` is equal to 1, and `k` is `a + b - 1`.

Output State: **`m` is a non-negative integer such that \(1 \leq m \leq 10^9\), `a` is a positive integer such that \(1 \leq a \leq 10^5\), `b` is a positive integer such that \(1 \leq b \leq 10^5\), `g` is equal to 1, and `k` is `a + b - 1`**