The code calculates `sum_m` based on the formula `m * (m + 1) // 2 - k * (k - 1) // 2`. Here, `k` is already defined as `a + b - 1`. Let's break down the calculation step-by-step:

1. The value of `k` is `a + b - 1`.
2. The value of `sum_k` is given as `k * (k + 1) // 2`, which is a constant.
3. The new value of `sum_m` is calculated as `m * (m + 1) // 2 - k * (k - 1) // 2`.

Since `k` is `a + b - 1`, we substitute this into the formula for `sum_m`:
\[ sum_m = m * (m + 1) // 2 - (a + b - 1) * (a + b - 1 - 1) // 2 \]
\[ sum_m = m * (m + 1) // 2 - (a + b - 1) * (a + b - 2) // 2 \]

The other variables remain unchanged. Therefore, the output state is:
Output State: **`m` is a non-negative integer such that \(1 \leq m \leq 10^9\), `a` is a positive integer such that \(1 \leq a \leq 10^5\), `b` is a positive integer such that \(1 \leq b \leq 10^5\), `g` is equal to 1, `k` is `a + b - 1`, `sum_k` is \(k * (k + 1) // 2\), `sum_m` is `m * (m + 1) // 2 - k * (k - 1) // 2**