The code snippet `x1 += a` modifies the value of `x1` by adding `a` to it. Given the initial state, we know that `a` is either `y2 - 1` or `m - y2` depending on the initial relationship between `y1` and `y2`. The other variables remain unchanged.

Output State: **`t` is `abs(y2 - y1)`, `h` and `w` are positive integers such that 1 <= h <= 10^6 and 1 <= w <= 10^9; `x_a`, `y_a`, `x_b`, and `y_b` are positive integers such that 1 <= x_a, x_b <= h and 1 <= y_a, y_b <= w; it is guaranteed that x_a != x_b or y_a != y_b; the sum of h over all test cases does not exceed 10^6; `r` is a list of integers read from input; `n` is `r[0]`, `m` is `r[1]`, `x1` is `r[2] + 1 + a`, `x2` is `r[4]`, and `(x2 - x1) % 2 != 0`. `y1` is still not equal to `y2`. `b` is `x2 - x1`.**