The only variable in the loop head is `k`. Therefore, we need to adjust the state of `k` for the next iteration of the loop.

Given that the loop iterates over `k` from `0` to `n-1`, at the end of the previous iteration, `k` would have taken on the value it had during that iteration. To proceed to the next iteration, `k` should be incremented by 1.

Let's break down the state adjustments:
- At the end of the previous iteration, `k` was some value `x` (where `0 ≤ x < n`).
- For the next iteration, `k` should be `x + 1`.

Since the loop condition is `k in range(0, n)`, the loop will continue as long as `k` is less than `n`. Therefore, if `k` is currently `n-1`, the loop will terminate after this iteration, and no further adjustment is needed for another iteration.

However, based on the task requirements, we assume we are adjusting for the start of the next valid iteration, which means `k` should be incremented by 1.

Thus, the state at the start of the next iteration should be:
State: **`t` is an integer such that 1 ≤ t ≤ 10^4, `n` is an integer such that 2 ≤ n ≤ 500, `c` and `d` are integers such that 1 ≤ c, d ≤ 10^6, `l` is a list of `n^2` integers where each integer `b_i` satisfies 1 ≤ b_i ≤ 10^9, `a` is the minimum value in the list `l`, `li` is a list containing `n` elements where the `i-th` element is `a + k * c + d * i` for `i` ranging from 0 to `n-1`, `k` is `k + 1`**.

Given that `k` was `x` at the end of the previous iteration, the new state for `k` should be `x + 1`. If we denote the previous value of `k` as `k_prev`, then the new value of `k` should be `k_prev + 1`.

So, if `k` was `x` at the end of the previous iteration, the state at the start of the next iteration would be:
State: **`t` is an integer such that 1 ≤ t ≤ 10^4, `n` is an integer such that 2 ≤ n ≤ 500, `c` and `d` are integers such that 1 ≤ c, d ≤ 10^6, `l` is a list of `n^2` integers where each integer `b_i` satisfies 1 ≤ b_i ≤ 10^9, `a` is the minimum value in the list `l`, `li` is a list containing `n` elements where the `i-th` element is `a + k * c + d * i` for `i` ranging from 0 to `n-1`, `k` is `k + 1`**.

Since we don't know the exact value of `k` at the end of the previous iteration, we can generalize it as:
State: **`t` is an integer such that 1 ≤ t ≤ 10^4, `n` is an integer such that 2 ≤ n ≤ 500, `c` and `d` are integers such that 1 ≤ c, d ≤ 10^6, `l` is a list of `n^2` integers where each integer `b_i` satisfies 1 ≤ b_i ≤ 10^9, `a` is the minimum value in the list `l`, `li` is a list containing `n` elements where the `i-th` element is `a + k * c + d * i` for `i` ranging from 0 to `n-1`, `k` is `k + 1`**

But to be specific about the next iteration, if `k` was `3` at the end of the previous iteration, the next state would be:
State: **`t` is an integer such that 1 ≤ t ≤ 10^4, `n` is an integer such that 2 ≤ n ≤ 500, `c` and `d` are integers such that 1 ≤ c, d ≤ 10^6, `l` is a list of `n^2` integers where each integer `b_i` satisfies 1 ≤ b_i ≤ 10^9, `a` is the minimum value in the list `l`, `li` is a list containing `n` elements where the `i-th` element is `a + k * c + d * i` for `i` ranging from 0 to `n-1`, `k` is 4**.

Generalizing, if `k` was `k_prev` at the end of the previous iteration, the next state would be:
State: **`t` is an integer such that 1 ≤ t ≤ 10^4, `n` is an integer such that 2 ≤ n ≤ 500, `c` and `d` are integers such that 1 ≤ c, d ≤ 10^6, `l` is a list of `n^2` integers where each integer `b_i` satisfies 1 ≤ b_i ≤ 10^9, `a` is the minimum value in the list `l`, `li` is a list containing `n` elements where the `i-th` element is `a + k * c + d * i` for `i` ranging from 0 to `n-1`, `k` is `k + 1`**

Therefore, the final answer is:
State: **`t` is an integer such that 1 ≤ t ≤ 10^4, `n` is an integer such that 2 ≤ n ≤ 500, `c` and `d` are integers such that 1 ≤ c, d ≤ 10^6, `l` is a list of `n^2` integers where each integer `b_i` satisfies 1 ≤ b_i ≤ 10^9, `a` is the minimum value in the list `l`, `li` is a list containing `n` elements where the `i-th` element is `a + k * c + d * i` for `i` ranging from 0 to `n-1`, `k` is `k + 1`**