Let's break down the initial state and the code step by step:

1. **Initial State**:
   - `t` is an integer between 1 and 500 inclusive.
   - `p1`, `p2`, `p3` are integers assigned the values from the input split by spaces.
   - `low` is the minimum of `p3 - p1` and `p3 - p2`.
   - `high` is the maximum of `p3 - p1` and `p3 - p2`.
   - `cur` is equal to `low`.
   - `(p1 - cur <= p2 - (p3 - cur))` is true.

2. **Code Snippet**:
   ```python
   print(p1 - cur + p3)
   ```

3. **Analysis**:
   - Since `cur` is equal to `low`, we need to determine the value of `low`.
   - `low` is defined as the minimum of `p3 - p1` and `p3 - p2`.
   - Given that `(p1 - cur <= p2 - (p3 - cur))` is true, substituting `cur` with `low` gives us:
     \[
     p1 - low \leq p2 - (p3 - low)
     \]
     Simplifying this inequality:
     \[
     p1 - low \leq p2 - p3 + low
     \]
     Rearranging terms:
     \[
     p1 + p3 \leq p2 + 2 \cdot low
     \]
     This implies that `low` must be such that the above inequality holds true.

4. **Determine `low`**:
   - Since `low` is the minimum of `p3 - p1` and `p3 - p2`, let's denote `p3 - p1 = a` and `p3 - p2 = b`.
   - Therefore, `low = min(a, b)`.
   - Given the inequality `p1 + p3 â‰¤ p2 + 2 \cdot low`, we substitute back:
     \[
     p1 + p3 \leq p2 + 2 \cdot \min(p3 - p1, p3 - p2)
     \]

5. **Final Calculation**:
   - The expression to print is `p1 - cur + p3`.
   - Since `cur = low`, we have:
     \[
     p1 - low + p3
     \]
   - Using the definition of `low`, we get:
     \[
     p1 - \min(p3 - p1, p3 - p2) + p3
     \]

6. **Simplification**:
   - If `p3 - p1` is smaller, then `low = p3 - p1` and the expression becomes:
     \[
     p1 - (p3 - p1) + p3 = p1 - p3 + p1 + p3 = 2 \cdot p1
     \]
   - If `p3 - p2` is smaller, then `low = p3 - p2` and the expression becomes:
     \[
     p1 - (p3 - p2) + p3 = p1 - p3 + p2 + p3 = p1 + p2
     \]

Given the conditions, the exact value depends on the relative sizes of `p3 - p1` and `p3 - p2`, but the expression simplifies to either `2 * p1` or `p1 + p2`.

Since the exact values of `p1`, `p2`, and `p3` are not specified, we can only express the result in terms of these variables.

Output: **p1 + p2**