First, let's evaluate the initial state of `res`:
\[ res = (0 + (0 + 1) * (2 * 0 + 1)) = (0 + 1 * 1) = 1 \]

Given the code snippet:
```python
res += (i + 1) * (2 * i + 1)
```
We know from the initial state that `i` is 1. So, we substitute `i` with 1 in the expression:
\[ (i + 1) * (2 * i + 1) = (1 + 1) * (2 * 1 + 1) = 2 * 3 = 6 \]

Therefore, the value of `res` is updated by adding 6 to its current value:
\[ res = 1 + 6 = 7 \]

The value of `t`, `n`, and `i` remains unchanged.

Output State: **`res` is 7, `t` is an integer such that \(1 \leq t \leq 500\), `n` must be greater than 0, `i` is 1**