Alright, I have this problem to solve. Let's understand what's being asked here. So, Polycarp has a string `s` consisting of lowercase Latin letters, and he encodes it using a specific algorithm. My task is to write a program that decodes the encoded string back to the original string `s`.

First, I need to understand the encoding algorithm clearly. The algorithm has two main steps:

1. **Construct the auxiliary string `r`**: This string consists of all distinct letters from `s`, sorted in alphabetical order.

2. **Encoding the string `s`**: Each character in `s` is replaced by its symmetric character from the string `r`. For example, the first character of `r` is replaced by the last character of `r`, the second by the second last, and so on.

Given an encoded string `b`, I need to decode it back to the original string `s`.

Let me look at the example provided to understand this better.

**Example:**

- Original string `s`: "codeforces"

- Construct `r`: "cdefors" (all distinct letters in sorted order)

- Encoding:

  - 'c' -> 's'

  - 'o' -> 'e'

  - 'd' -> 'r'

  - 'f' -> 'o'

  - 'e' -> 'f'

  - 'c' -> 's'

  - 'o' -> 'e'

  - 'r' -> 'd'

  - 'c' -> 's'

  - 'e' -> 'f'

- Encoded string `b`: "serofedsoc"

Now, given `b` = "serofedsoc", I need to decode it back to "codeforces".

To decode, I need to reverse the encoding process. That means, for each character in `b`, I need to find out which character in `s` was replaced by it, based on the symmetric mapping defined by `r`.

So, in the decoding process, I need to:

1. Determine the string `r` from the encoded string `b`. Since `r` consists of unique sorted characters from `s`, and `s` is decoded from `b`, I can construct `r` from the unique sorted characters of `b`, because `b` is just a rearrangement of `s`.

2. Create a mapping from the encoded characters back to the original characters based on the symmetric relationship in `r`.

Wait a minute, in the encoding process, `r` is constructed from `s`, but in decoding, I don't have `s`. However, since `r` consists of unique sorted characters from `s`, and `b` is encoded from `s` using `r`, the unique sorted characters in `b` should be the same as in `s`, because the encoding is a bijection based on `r`.

Therefore, I can construct `r` from the unique sorted characters of `b`.

Then, I need to create a mapping where each character in `r` is mapped back to its symmetric character in `r`.

For example, in the earlier case:

`r` = "cdefors"

Symmetric mapping would be:

- 'c' -> 's'

- 'd' -> 'r'

- 'e' -> 'o'

- 'f' -> 'f'

- 'o' -> 'e'

- 'r' -> 'd'

- 's' -> 'c'

For decoding, I need to reverse this mapping:

- 's' -> 'c'

- 'r' -> 'd'

- 'o' -> 'e'

- 'f' -> 'f'

- 'e' -> 'o'

- 'd' -> 'r'

- 'c' -> 's'

So, for each character in `b`, I replace it with the corresponding character in the reversed mapping.

Given that, I can implement the decoding function.

Now, looking at the provided program:

```python
import sys

input = sys.stdin.read
data = input().split()
index = 0
t = int(data[index])
index += 1
results = []
for _ in range(t):
    n = int(data[index])
    index += 1
    b = data[index]
    index += 1
    results.append(func_1(b))
print('\n'.join(results))

def func_1(encoded):
    r = ''.join(sorted(set(encoded)))
    mapping = {r[i]: r[-(i + 1)] for i in range(len(r))}
    return ''.join((mapping[char] for char in encoded))
```

Let's analyze this program step by step.

1. **Reading input:**

   - `input = sys.stdin.read` reads all input at once.

   - `data = input().split()` splits the input into words.

   - `index = 0` initializes an index to track the current position in `data`.

2. **Processing each test case:**

   - `t = int(data[index])` reads the number of test cases.

   - For each test case:

     - `n = int(data[index])` reads the length of the encoded string.

     - `b = data[index]` reads the encoded string.

     - `results.append(func_1(b))` decodes the string using `func_1`.

   - Finally, `print('\n'.join(results))` prints all decoded strings.

3. **Decoding function `func_1`:**

   - `r = ''.join(sorted(set(encoded)))` constructs the string `r` from the unique sorted characters of the encoded string.

   - `mapping = {r[i]: r[-(i + 1)] for i in range(len(r))}` creates a mapping where each character in `r` is mapped to its symmetric character in `r`.

   - `return ''.join((mapping[char] for char in encoded))` replaces each character in the encoded string with its corresponding character from the mapping.

Wait a second, in the decoding process, should I be using the symmetric mapping directly, or should I be using the reverse of this mapping?

In the earlier example, for decoding "serofedsoc" back to "codeforces", I need to map 's' back to 'c', 'e' back to 'o', etc., which is the reverse of the encoding mapping.

But in the program, `mapping` is defined as `r[i]` to `r[-(i + 1)]`, which seems to be the same as the encoding mapping, not the reverse.

Let me verify this.

Given `r` = "cdefors"

Encoding mapping:

- 'c' -> 's'

- 'd' -> 'r'

- 'e' -> 'o'

- 'f' -> 'f'

- 'o' -> 'e'

- 'r' -> 'd'

- 's' -> 'c'

Decoding mapping should be:

- 's' -> 'c'

- 'r' -> 'd'

- 'o' -> 'e'

- 'f' -> 'f'

- 'e' -> 'o'

- 'd' -> 'r'

- 'c' -> 's'

So, the decoding mapping is essentially the reverse of the encoding mapping.

In the program, the mapping is defined as `r[i]` to `r[-(i + 1)]`, which matches the encoding mapping, not the decoding mapping.

Therefore, the program seems to be incorrect because it's applying the encoding mapping again, instead of the decoding mapping.

Wait, but if I look closely, perhaps I'm misunderstanding something.

Let's think differently. Since the mapping is symmetric, applying the same mapping twice should bring back the original string.

Let's test this with the example.

Given `r` = "cdefors"

Mapping:

- 'c' -> 's'

- 'd' -> 'r'

- 'e' -> 'o'

- 'f' -> 'f'

- 'o' -> 'e'

- 'r' -> 'd'

- 's' -> 'c'

If I apply this mapping twice:

- 'c' -> 's' -> 'c'

- 'd' -> 'r' -> 'd'

- 'e' -> 'o' -> 'e'

- 'f' -> 'f' -> 'f'

- 'o' -> 'e' -> 'o'

- 'r' -> 'd' -> 'r'

- 's' -> 'c' -> 's'

So, applying the same mapping twice returns to the original character.

Therefore, applying the encoding mapping again effectively decodes the string.

Ah, that makes sense. So, in this case, since the mapping is an involution (applying it twice returns the original), using the same mapping for decoding is correct.

Let me verify this with the example.

Given encoded string `b` = "serofedsoc"

Applying the mapping:

- 's' -> 'c'

- 'e' -> 'o'

- 'r' -> 'd'

- 'o' -> 'e'

- 'f' -> 'f'

- 'e' -> 'o'

- 'd' -> 'd'

- 's' -> 'c'

- 'o' -> 'o'

- 'c' -> 's'

Which gives "codeforces", which matches the original string.

So, in this case, applying the same mapping again decodes the string correctly.

Therefore, the program is correct.

Wait, but is this always true?

Let me consider another example.

Take `s` = "fft"

Unique sorted `r` = "ft"

Mapping:

- 'f' -> 't'

- 't' -> 'f'

Encoding:

- 'f' -> 't'

- 'f' -> 't'

- 't' -> 'f'

So, encoded `b` = "ttf"

Decoding using the same mapping:

- 't' -> 'f'

- 't' -> 'f'

- 'f' -> 't'

Which gives "fft", matching the original string.

Another example:

`s` = "algorithm"

Unique sorted `r` = "agilmort"

Mapping:

- 'a' -> 't'

- 'g' -> 'r'

- 'i' -> 'o'

- 'l' -> 'm'

- 'm' -> 'l'

- 'o' -> 'i'

- 'r' -> 'g'

- 't' -> 'a'

Encoding:

- 'a' -> 't'

- 'l' -> 'm'

- 'g' -> 'r'

- 'o' -> 'i'

- 'r' -> 'g'

- 'i' -> 'o'

- 't' -> 'a'

- 'h' -> ? Wait, 'h' is not in `r`, but since `r` is "agilmort", and 'h' is not present, but in the example, it's present in the output.

Wait, in the example, one of the test cases is:

Input:

9

tlrhgmaoi

Output:

algorithm

Wait, but in this case, `b` = "tlrhgmaoi"

Let's see:

Unique sorted `r` = "agilmort"

Mapping:

- 'a' -> 't'

- 'g' -> 'r'

- 'i' -> 'o'

- 'l' -> 'm'

- 'm' -> 'l'

- 'o' -> 'i'

- 'r' -> 'g'

- 't' -> 'a'

Decoding `b` = "tlrhgmaoi":

- 't' -> 'a'

- 'l' -> 'm'

- 'r' -> 'g'

- 'h' -> ? Wait, 'h' is not in `r`, but in the mapping.

Wait, perhaps I need to consider that `r` is constructed from the unique sorted characters of `b`, which should be the same as from `s`.

In this case, `b` = "tlrhgmaoi", unique sorted `r` = "aghilmort"

Wait, but in the mapping above, it's "agilmort". Anyway, assuming 'h' is not present in `r`, but in the encoded string, which should not happen because `r` contains all unique characters from `s`, and `b` is encoded from `s` using `r`.

Wait, perhaps I need to make sure that all characters in `b` are present in `r`.

But in the example, it's given as correct.

Wait, maybe I need to consider that 'h' is present in `s`, but not in `r`, but that can't be, because `r` contains all unique characters from `s`.

Wait, no, `r` contains all unique characters from `s`, sorted.

So, if 'h' is in `s`, it should be in `r`.

Wait, in the example, `s` = "algorithm", `r` = "agilmort", which includes 'h'.

Wait, no, "algorithm" consists of letters a, l, g, o, r, i, t, h, m. So `r` = "aghimort".

Wait, but in the example, output is "algorithm", and `b` = "tlrhgmaoi".

Let's map it back:

- 't' -> 'a'

- 'l' -> 'm'

- 'r' -> 'g'

- 'h' -> 'h' (assuming 'h' maps to itself if it's in the middle)

- 'g' -> 'r'

- 'm' -> 'l'

- 'a' -> 't'

- 'o' -> 'i'

- 'i' -> 'o'

Which gives "algorithm".

So, in this case, it works.

Therefore, the program seems correct.

Another test case:

Input:

1

1

w

Output:

w

Here, `b` = "w", unique sorted `r` = "w", mapping {'w': 'w'}, so decoding "w" -> "w", which is correct.

Last test case:

Input:

15

hnndledmnhlttin

Output:

meetinthemiddle

Let's see:

Unique sorted `r` from `b` = "hnndledmnhlttin" -> unique sorted is "dehilmnnt"

Mapping:

- 'd' -> 't'

- 'e' -> 'n'

- 'h' -> 'n'

- 'i' -> 'l'

- 'l' -> 'i'

- 'm' -> 'h'

- 'n' -> 'e'

- 't' -> 'd'

Decoding "hnndledmnhlttin":

- 'h' -> 'n'

- 'n' -> 'e'

- 'n' -> 'e'

- 'd' -> 't'

- 'l' -> 'i'

- 'e' -> 'n'

- 'd' -> 't'

- 'm' -> 'h'

- 'n' -> 'e'

- 'h' -> 'n'

- 'l' -> 'i'

- 't' -> 'd'

- 't' -> 'd'

- 'i' -> 'l'

- 'n' -> 'e'

Which gives "neetinhtneniddele" -> Wait, that doesn't match "meetinthemiddle". Did I make a mistake?

Wait, perhaps I misordered `r`. Let's sort "dehilmnnt" correctly: "dehilmnt"

Mapping:

- 'd' -> 't'

- 'e' -> 'n'

- 'h' -> 'l'

- 'i' -> 'm'

- 'l' -> 'h'

- 'm' -> 'i'

- 'n' -> 'e'

- 't' -> 'd'

Decoding "hnndledmnhlttin":

- 'h' -> 'l'

- 'n' -> 'e'

- 'n' -> 'e'

- 'd' -> 't'

- 'l' -> 'h'

- 'e' -> 'n'

- 'd' -> 't'

- 'm' -> 'i'

- 'n' -> 'e'

- 'h' -> 'l'

- 'l' -> 'h'

- 't' -> 'd'

- 't' -> 'd'

- 'i' -> 'm'

- 'n' -> 'e'

Which gives "leetehntileddme", which is not "meetinthemiddle". So, perhaps I messed up the mapping.

Wait, maybe I need to consider the correct order of `r`.

Let's list the unique characters in "hnndledmnhlttin":

- h, n, d, l, e, m, t, i

Sorted: d,e,h,i,l,m,n,t

So, `r` = "dehilmnt"

Mapping:

- 'd' -> 't'

- 'e' -> 'n'

- 'h' -> 'm'

- 'i' -> 'l'

- 'l' -> 'i'

- 'm' -> 'h'

- 'n' -> 'e'

- 't' -> 'd'

Decoding "hnndledmnhlttin":

- 'h' -> 'm'

- 'n' -> 'e'

- 'n' -> 'e'

- 'd' -> 't'

- 'l' -> 'i'

- 'e' -> 'n'

- 'd' -> 't'

- 'm' -> 'h'

- 'n' -> 'e'

- 'h' -> 'm'

- 'l' -> 'i'

- 't' -> 'd'

- 't' -> 'd'

- 'i' -> 'l'

- 'n' -> 'e'

Which gives "meetinthemiddle", matching the expected output.

Therefore, the program seems to be correct.

I think I made a mistake earlier in the mapping, but upon correct mapping, it works.

Hence, the program is correct.

**Final Answer**

\[ \boxed{\text{The given program is correct.}} \]