Alright, I've got this problem to solve. Let's see what it's about. So, Polycarp has a string made of lowercase Latin letters, and he encodes it using a specific algorithm. First, he creates an auxiliary string 'r' which consists of all the distinct letters from the original string 's', sorted in alphabetical order. Then, he replaces each character in 's' with its symmetric counterpart from 'r'. For example, the first character in 'r' is replaced by the last in 'r', the second by the second last, and so on.

Given the encoded string, I need to write a program that decodes it back to the original string 's'. The input consists of multiple test cases, each with a string 'b' that is the encoded version of some original string 's'. My task is to find 's' from 'b'.

First, I need to understand the encoding process thoroughly to reverse it correctly. Let's break it down.

1. **Constructing 'r':** 'r' is made by taking all unique characters from 's' and sorting them alphabetically. So, for "codeforces", 'r' is "cdefors".

2. **Encoding 's' to 'b':** Each character in 's' is replaced by its symmetric counterpart in 'r'. For example:
   - 'c' (first in 'r') is replaced by 's' (last in 'r').
   - 'o' (second in 'r') is replaced by 'e' (second last in 'r').
   - 'd' (third in 'r') is replaced by 'r' (third last in 'r').
   - And so on.

So, to decode 'b' back to 's', I need to reverse this process. Given 'b', I need to find 'r' and then map each character in 'b' back to its original character in 's' using the same symmetry in 'r'.

Wait a minute, but in the encoding process, 'r' is derived from 's', which is what we're trying to find. So, how can I find 'r' if I don't have 's'?

Hmm, that's tricky. Let's think differently. Since 'r' is made up of unique sorted characters from 's', and the encoding is done based on 'r', perhaps 'r' can be derived from 'b' in a similar way, because 'b' is derived from 's' using 'r'.

Let's consider that 'b' is encoded from 's' using 'r', and 'r' is the sorted unique characters of 's'. Since 's' and 'b' are related through 'r', and 'r' is deterministic from 's', maybe there's a way to reconstruct 'r' from 'b'.

Wait, 'b' is derived from 's' using 'r', but 'r' is derived from 's'. However, since the mapping is symmetric, perhaps I can find a way to map characters back using the same symmetry.

Let me try to reverse the process.

Given 'b', I need to find 's'. To do that, I need to know 'r', which is the sorted unique characters of 's'. But I don't have 's', so I can't directly get 'r'. However, since 'b' is encoded from 's' using 'r', there might be a way to deduce 'r' from 'b'.

Let's consider that in the encoding process, each character in 's' is replaced by its symmetric counterpart in 'r'. So, in 'b', each character corresponds to a character in 's' via this symmetry in 'r'.

If I can find 'r', then I can create a mapping from 'b' back to 's' by reversing the symmetry.

Wait, perhaps I can assume that 'r' for 'b' is the same as 'r' for 's', since 'r' is based on the unique sorted characters of 's', and 'b' is just a rearrangement based on 'r'.

So, if I can find 'r' from 'b', I can use it to decode 'b' back to 's'.

Let me try that.

Given 'b', I can find 'r' as the sorted unique characters of 'b', because 'b' should have the same unique characters as 's', just rearranged.

Wait, is that correct? Let's see.

In the encoding process, each character in 's' is replaced by another character in 'r', but all characters are from the same set. So, the unique characters in 'b' should be the same as those in 's', just possibly in a different order.

Therefore, 'r' for 's' should be the same as 'r' for 'b', since they have the same unique characters, just sorted.

So, I can derive 'r' from 'b' by taking its unique characters and sorting them.

Once I have 'r', I can create a mapping from 'b' back to 's' by reversing the symmetry.

In other words, in 'r', the first character maps to the last, the second to the second last, and so on. So, to decode, I need to map each character in 'b' to its corresponding character in 's' using the reverse of this symmetry.

Let me illustrate with the example provided:

Encoded 'b': "serofedsoc"

'r' for 'b' is "cdefors" (sorted unique characters of 'b').

Now, the symmetry in 'r' is:

c -> s

d -> r

e -> o

f -> f

o -> d

r -> d

s -> c

But wait, 'r' has duplicate characters like 'd' and 'o', which might cause issues.

Wait, no, 'r' is supposed to have unique sorted characters, so duplicates should be removed.

Wait, in the problem statement, 'r' is made of distinct letters from 's', sorted alphabetically. So, 'r' should have unique characters only.

In the example, 'r' is "cdefors", which has no duplicates.

So, in this case, the mapping is:

c -> s

d -> r

e -> o

f -> f

o -> e

r -> d

s -> c

So, to decode 'b' back to 's', I need to map each character in 'b' to its corresponding character in 's' based on this mapping.

For instance, the first character in 'b' is 's', which maps back to 'c'.

Second character is 'e', which maps back to 'o'.

Third is 'r', which maps back to 'd'.

And so on, resulting in "codeforces".

So, it seems that if I can derive 'r' from 'b' and create this mapping, I can decode 'b' to 's'.

Now, I need to implement this in code.

Given that there are multiple test cases, and the input is large, I need an efficient way to handle this.

Let's outline the steps for each test case:

1. Read the encoded string 'b'.

2. Determine 'r' as the sorted unique characters of 'b'.

3. Create a mapping from each character in 'r' to its symmetric counterpart in 'r'.

4. Use this mapping to decode 'b' back to 's'.

5. Output 's'.

I need to make sure that the mapping is correctly established. Specifically, for each character in 'r', its position i (0-based) should map to position len(r) - 1 - i.

For example, if 'r' is "cdefors", which has 7 characters:

Indices: 0 1 2 3 4 5 6

Characters: c d e f o r s

So, mapping is:

c (0) -> s (6)

d (1) -> r (5)

e (2) -> o (4)

f (3) -> f (3)

s (6) -> c (0)

r (5) -> d (1)

o (4) -> e (2)

So, in the decoding, each character in 'b' is replaced by its corresponding character in 's' based on this mapping.

Now, in code, I can create a dictionary that maps each character in 'r' to its symmetric counterpart.

Then, for each character in 'b', I look up this dictionary to get the original character in 's'.

Let me try to write a small example to verify this.

Take 'b' = "serofedsoc"

'r' = "cdefors"

Mapping:

c -> s

d -> r

e -> o

f -> f

o -> e

r -> d

s -> c

So, decoding "serofedsoc":

s -> c

e -> o

r -> d

o -> e

f -> f

e -> o

d -> r

s -> c

o -> e

c -> s

Which gives "codeforces", which matches the original 's'.

Great, so this approach seems correct.

Now, I need to implement this efficiently, especially considering the constraints:

- Up to 10^4 test cases.

- Each test case has up to 2*10^5 characters in 'b'.

- Total sum of n over all test cases doesn't exceed 2*10^5.

Given these constraints, I need to make sure that my code is efficient and doesn't have unnecessary overhead.

I should read all input at once and process it accordingly to avoid slow I/O.

In Python, reading all input at once using sys.stdin.read() and splitting it into tokens is efficient.

Then, I can iterate through the test cases accordingly.

Also, for each test case, constructing 'r' by sorting the unique characters of 'b' should be straightforward.

Creating the mapping dictionary should also be straightforward.

Then, decoding 'b' by mapping each character using the dictionary and joining them back into a string.

Finally, collecting all results and printing them at once.

Let me think about potential edge cases:

1. Single character: If 'b' is a single character, 'r' will have one character. The mapping should map that character to itself.

2. All characters in 'b' are the same: For example, 'b' = "aaa". 'r' will be "a", mapping 'a' to itself.

3. 'b' has all unique characters: In this case, 'r' is the same as 'b' sorted.

4. 'b' has duplicates: For example, 'b' = "aabbcc", 'r' will be "abc".

5. 'b' contains only one unique character: Same as case 2.

6. 'b' is empty: But according to constraints, n >=1, so no need to handle empty strings.

7. 'b' has the minimum length, n=1: Already covered in case 1.

I need to make sure that my code handles these cases correctly.

Also, I need to ensure that the mapping is correctly established, especially when the number of characters is even or odd.

For example, if 'r' has an even number of characters:

'r' = "abcd"

Mapping:

a -> d

b -> c

c -> b

d -> a

If 'r' has an odd number of characters:

'r' = "abc"

Mapping:

a -> c

b -> b

c -> a

So, the middle character maps to itself.

In code, this can be handled by mapping r[i] to r[len(r)-1-i] for each i from 0 to len(r)//2.

Now, let's look at the provided program and see if it implements this correctly.

The program is:

import sys

input = sys.stdin.read

data = input().split()

index = 0

t = int(data[index])

index += 1

results = []

for _ in range(t):

n = int(data[index])

index += 1

b = data[index]

index += 1

results.append(func_1(b))

print('\n'.join(results))

def func_1(encoded):

r = ''.join(sorted(set(encoded)))

mapping = {r[i]: r[-(i + 1)] for i in range(len(r))}

return ''.join((mapping[char] for char in encoded))

So, let's analyze this step by step.

1. It reads all input at once using sys.stdin.read() and splits it into tokens stored in 'data'.

2. It initializes 'index' to 0.

3. It reads the number of test cases 't' from data[index] and increments index.

4. It initializes an empty list 'results' to store the decoded strings.

5. For each test case:

a. Reads 'n' from data[index] and increments index.

b. Reads 'b' from data[index] and increments index.

c. Calls func_1(b) to decode 'b' and appends the result to 'results'.

6. After processing all test cases, it prints all results joined by newline.

Now, looking at func_1:

def func_1(encoded):

r = ''.join(sorted(set(encoded)))

mapping = {r[i]: r[-(i + 1)] for i in range(len(r))}

return ''.join((mapping[char] for char in encoded))

1. It creates 'r' by converting 'encoded' to a set (to get unique characters), sorting them, and joining them into a string.

2. It creates a mapping dictionary where each character in 'r' is mapped to its symmetric counterpart in 'r'.

3. It decodes 'encoded' by replacing each character using the mapping dictionary and joins them back into a string.

This seems to align with the approach I outlined earlier.

Let's verify with the example:

Encoded 'b': "serofedsoc"

'r' = "cdefors"

mapping:

c -> s

d -> r

e -> o

f -> f

o -> e

r -> d

s -> c

Decoding "serofedsoc" using this mapping gives "codeforces", which matches the expected output.

Another test case:

Encoded 'b': "ttfhgmaoi"

Assuming this is a typo, and it should be "tlrhgmaoi" based on the output "algorithm".

Let's verify:

'b' = "tlrhgmaoi"

Unique sorted characters 'r' = "agilmort"

Mapping:

t -> a

r -> o

o -> r

m -> m

a -> t

g -> g

l -> l

i -> i

So, decoding "tlrhgmaoi" would be:

t -> a

l -> l

r -> o

h -> g

g -> g

m -> m

a -> t

o -> r

i -> i

Which gives "allgmtri", but the expected output is "algorithm". Hmm, that doesn't match.

Wait, perhaps I miscounted the mapping.

'r' = "agilmort"

Indices:

0:a 7-0=7:t

1:g 7-1=6:m

2:i 7-2=5:o

3:l 7-3=4:r

4:m 7-4=3:l

5:o 7-5=2:i

6:m 7-6=1:g

7:t 7-7=0:a

Wait, but 'm' appears twice in 'r', but 'r' should have unique characters. Wait, in 'tlrhgmaoi', the unique sorted characters are "agilmort", which are all unique.

So, mapping:

a -> t

g -> m

i -> i

l -> r

m -> o

o -> o

r -> l

t -> a

So, decoding "tlrhgmaoi":

t -> a

l -> r

r -> l

h -> (not in mapping, but 'h' should be in mapping)

Wait, 'h' is in 'b', but not in 'r'. Wait, in the example, 'b' is "tlrhgmaoi", and 'r' is "agilmort". But 'h' is in 'b', but not in 'r'. Wait, no, 'r' includes all unique characters from 'b', which are "aghlmiort".

Wait, perhaps I made a mistake in identifying 'r'.

Let's list the unique characters in "tlrhgmaoi":

t, l, r, h, g, m, a, o, i

Sorted: a, g, h, i, l, m, o, r, t

So, 'r' = "aghilmort"

Mapping:

a -> t

g -> r

h -> o

i -> i

l -> m

m -> l

o -> h

r -> g

t -> a

So, decoding "tlrhgmaoi":

t -> a

l -> m

r -> g

h -> o

g -> r

m -> l

a -> t

o -> h

i -> i

Which gives "amgolorlthi", which doesn't match "algorithm". Something's wrong here.

Wait, perhaps I miscounted the mapping.

'r' = "aghilmort"

Indices:

0:a 8-0-1=7:t

1:g 8-1-1=6:r

2:h 8-2-1=5:o

3:i 8-3-1=4:m

4:l 8-4-1=3:i

5:m 8-5-1=2:l

6:o 8-6-1=1:g

7:r 8-7-1=0:a

8:t 8-8-1=7:r

Wait, that can't be right. len(r) = 8, indices from 0 to 7.

So, mapping:

r[0] -> r[7]

r[1] -> r[6]

r[2] -> r[5]

r[3] -> r[4]

r[4] -> r[3]

r[5] -> r[2]

r[6] -> r[1]

r[7] -> r[0]

So, for 'r' = "aghilmort":

a -> r

g -> o

h -> l

i -> m

l -> i

m -> h

o -> g

r -> a

t -> t

So, decoding "tlrhgmaoi":

t -> t

l -> i

r -> a

h -> h

g -> o

m -> h

a -> r

o -> g

i -> m

Which gives "tiaho hrgm", which doesn't match "algorithm". There must be a mistake in my understanding.

Wait, perhaps I misidentified 'r'. Let's look back at the example.

In the example, for 'b' = "tlrhgmaoi", the expected output is "algorithm".

So, 's' = "algorithm"

'r' should be the sorted unique characters of 's', which are "a-g-h-i-l-m-o-r-t" = "aghilmort"

Encoding:

a -> r

g -> o

h -> l

i -> m

l -> i

m -> h

o -> g

r -> a

t -> t

So, encoding "algorithm" would be:

a -> r

l -> i

g -> o

o -> g

r -> a

i -> m

t -> t

h -> l

m -> h

Which gives "rio g a m t l h"

But the encoded 'b' is "tlrhgmaoi", which seems different. Maybe I messed up the order.

Wait, in "algorithm":

Indices:

0:a -> r

1:l -> i

2:g -> o

3:o -> g

4:r -> a

5:i -> m

6:t -> t

7:h -> l

8:m -> h

So, encoded 'b' should be "rilgotaml", but the example has "tlrhgmaoi". There's a discrepancy here.

Wait, perhaps the example is incorrect, or I'm misunderstanding something.

Alternatively, maybe the mapping is based on the position in 'r', not the character itself.

Wait, perhaps I need to map based on the position in 'r', not the character.

Let me try again.

'r' = "aghilmort"

Mapping:

a (pos 0) -> t (pos 7)

g (pos 1) -> r (pos 7-1=6)

h (pos 2) -> o (pos 5)

i (pos 3) -> m (pos 4)

l (pos 4) -> i (pos 3)

m (pos 5) -> l (pos 2)

o (pos 6) -> g (pos 1)

r (pos 7) -> a (pos 0)

t (pos 7) -> a (pos 0)

Wait, pos 7 is 't', so t -> a

So, decoding "tlrhgmaoi":

t (pos 7) -> a

l (pos 4) -> i

r (pos 7) -> a

h (pos 2) -> l

g (pos 1) -> o

m (pos 5) -> l

a (pos 0) -> t

o (pos 6) -> g

i (pos 3) -> m

Which gives "ailol ltgm", which is still not "algorithm". I must be making a mistake.

Wait, perhaps 'r' has unique characters, but in the mapping, positions are based on the sorted unique characters.

Wait, in the example, 'b' is "tlrhgmaoi", which should decode to "algorithm".

Let's see:

Mapping:

t -> a

l -> l

r -> g

h -> o

g -> r

m -> m

a -> t

o -> h

i -> i

So, decoding "tlrhgmaoi" would be "allgmtri", which is not "algorithm". There's inconsistency here.

Wait, maybe the mapping is based on the symmetric positions, considering 'r' has unique characters.

Wait, perhaps I need to pair the characters in 'r' symmetrically and map accordingly.

For 'r' = "aghilmort":

Positions:

0:a -7:t

1:g -6:o

2:h -5:m

3:i -4:l

4:l -3:i

5:m -2:h

6:o -1:g

7:r -0:a

So, mapping:

a -> t

g -> o

h -> m

i -> l

l -> i

m -> h

o -> g

r -> a

t -> t

So, decoding "tlrhgmaoi":

t (t -> a)

l (l -> i)

r (r -> a)

h (h -> m)

g (g -> o)

m (m -> h)

a (a -> t)

o (o -> g)

i (i -> l)

Which gives "aiamothgtl", which is not "algorithm". Clearly, I'm doing something wrong.

Wait, perhaps the mapping should be based on the index in 'r', where the first character maps to the last, second to the second last, and so on.

For 'r' = "aghilmort" (positions 0 to 7):

Mapping:

0:a -> 7:r

1:g -> 6:o

2:h -> 5:m

3:i -> 4:l

4:l -> 3:i

5:m -> 2:h

6:o -> 1:g

7:r -> 0:a

So, decoding "tlrhgmaoi":

t (t is at pos 7 in 'r' -> a)

l (l is at pos 4 in 'r' -> i)

r (r is at pos 7 in 'r' -> a)

h (h is at pos 2 in 'r' -> m)

g (g is at pos 1 in 'r' -> o)

m (m is at pos 5 in 'r' -> h)

a (a is at pos 0 in 'r' -> r)

o (o is at pos 6 in 'r' -> g)

i (i is at pos 3 in 'r' -> l)

Which gives "a m a o h r g l", which is "amaiohrgl", still not "algorithm". There's clearly a mistake in my approach.

Wait, perhaps I need to consider that 'r' is "aghilmort", and the mapping is:

a -> r

g -> o

h -> m

i -> l

l -> i

m -> h

o -> g

r -> a

t -> t

So, decoding "tlrhgmaoi":

t -> t

l -> i

r -> a

h -> m

g -> o

m -> h

a -> r

o -> g

i -> l

Which gives "timorghl", which is still not "algorithm". I must be missing something.

Wait, perhaps the mapping is incorrect. Maybe I need to map based on the symmetric positions correctly.

Let's try to create a mapping where for each character in 'r', it's mapped to its symmetric counterpart.

For 'r' = "aghilmort":

Positions:

0:a - 7:r

1:g - 6:o

2:h - 5:m

3:i - 4:l

So, mapping:

a ->